<?xml version="1.0"?>


<!DOCTYPE rdf:RDF [
    <!ENTITY owl "http://www.w3.org/2002/07/owl#" >
    <!ENTITY dc "http://purl.org/dc/elements/1.1/" >
    <!ENTITY xsd "http://www.w3.org/2001/XMLSchema#" >
    <!ENTITY rdfs "http://www.w3.org/2000/01/rdf-schema#" >
    <!ENTITY rdf "http://www.w3.org/1999/02/22-rdf-syntax-ns#" >
]>


<rdf:RDF xmlns="http://cbml.googlecode.com/svn/trunk/upperC2Ont.owl#"
     xml:base="http://cbml.googlecode.com/svn/trunk/upperC2Ont.owl"
     xmlns:dc="http://purl.org/dc/elements/1.1/"
     xmlns:rdfs="http://www.w3.org/2000/01/rdf-schema#"
     xmlns:owl="http://www.w3.org/2002/07/owl#"
     xmlns:xsd="http://www.w3.org/2001/XMLSchema#"
     xmlns:rdf="http://www.w3.org/1999/02/22-rdf-syntax-ns#">
    <owl:Ontology rdf:about="http://cbml.googlecode.com/svn/trunk/upperC2Ont.owl">
        <rdfs:label>Upper C2 Ontology</rdfs:label>
    </owl:Ontology>
    


    <!-- 
    ///////////////////////////////////////////////////////////////////////////////////////
    //
    // Annotation properties
    //
    ///////////////////////////////////////////////////////////////////////////////////////
     -->

    <owl:AnnotationProperty rdf:about="&rdfs;isDefinedBy"/>
    


    <!-- 
    ///////////////////////////////////////////////////////////////////////////////////////
    //
    // Datatypes
    //
    ///////////////////////////////////////////////////////////////////////////////////////
     -->

    


    <!-- http://www.w3.org/1999/02/22-rdf-syntax-ns#PlainLiteral -->

    <rdfs:Datatype rdf:about="&rdf;PlainLiteral"/>
    


    <!-- http://www.w3.org/2001/XMLSchema#string -->

    <rdfs:Datatype rdf:about="&xsd;string"/>
    


    <!-- 
    ///////////////////////////////////////////////////////////////////////////////////////
    //
    // Object Properties
    //
    ///////////////////////////////////////////////////////////////////////////////////////
     -->

    


    <!-- http://www.w3.org/2002/07/owl#topObjectProperty -->

    <owl:ObjectProperty rdf:about="&owl;topObjectProperty"/>
    


    <!-- 
    ///////////////////////////////////////////////////////////////////////////////////////
    //
    // Classes
    //
    ///////////////////////////////////////////////////////////////////////////////////////
     -->

    


    <!-- http://cbml.googlecode.com/svn/trunk/upperC2Ont.owl#Action -->

    <owl:Class rdf:about="http://cbml.googlecode.com/svn/trunk/upperC2Ont.owl#Action">
        <rdfs:subClassOf rdf:resource="http://cbml.googlecode.com/svn/trunk/upperC2Ont.owl#Event"/>
        <rdfs:comment>&#39;Something that is done.&#39;
&lt;http://www.oed.com/viewdictionaryentry/Entry/1938&gt;</rdfs:comment>
    </owl:Class>
    


    <!-- http://cbml.googlecode.com/svn/trunk/upperC2Ont.owl#Animal -->

    <owl:Class rdf:about="http://cbml.googlecode.com/svn/trunk/upperC2Ont.owl#Animal">
        <rdfs:subClassOf rdf:resource="http://cbml.googlecode.com/svn/trunk/upperC2Ont.owl#LivingThing"/>
        <rdfs:comment>&#39;A living organism which feeds on organic matter, typically having specialized sense organs and a nervous system and able to respond rapidly to stimuli; any living creature, including man.&#39;
&lt;http://www.oed.com/viewdictionaryentry/Entry/273779&gt;</rdfs:comment>
    </owl:Class>
    


    <!-- http://cbml.googlecode.com/svn/trunk/upperC2Ont.owl#Capability -->

    <owl:Class rdf:about="http://cbml.googlecode.com/svn/trunk/upperC2Ont.owl#Capability">
        <rdfs:subClassOf rdf:resource="http://cbml.googlecode.com/svn/trunk/upperC2Ont.owl#Property"/>
        <rdfs:comment>&#39;Power or ability in general, whether physical or mental; capacity.&#39;
&lt;http://www.oed.com/viewdictionaryentry/Entry/27353&gt;</rdfs:comment>
    </owl:Class>
    


    <!-- http://cbml.googlecode.com/svn/trunk/upperC2Ont.owl#CommunicationAct -->

    <owl:Class rdf:about="http://cbml.googlecode.com/svn/trunk/upperC2Ont.owl#CommunicationAct">
        <rdfs:subClassOf rdf:resource="http://cbml.googlecode.com/svn/trunk/upperC2Ont.owl#Action"/>
        <rdfs:comment>&#39;The transmission or exchange of information, knowledge, or ideas, by means of speech, writing, mechanical or electronic media&#39;
&lt;http://www.oed.com/viewdictionaryentry/Entry/37309&gt;</rdfs:comment>
    </owl:Class>
    


    <!-- http://cbml.googlecode.com/svn/trunk/upperC2Ont.owl#Entity -->

    <owl:Class rdf:about="http://cbml.googlecode.com/svn/trunk/upperC2Ont.owl#Entity">
        <rdfs:subClassOf rdf:resource="&owl;Thing"/>
        <owl:disjointWith rdf:resource="http://cbml.googlecode.com/svn/trunk/upperC2Ont.owl#Event"/>
        <rdfs:comment>&#39;Being, existence, as opposed to non-existence; the existence, as distinguished from the qualities or relations, of anything.&#39;
&lt;http://www.oed.com/viewdictionaryentry/Entry/62904&gt;</rdfs:comment>
    </owl:Class>
    


    <!-- http://cbml.googlecode.com/svn/trunk/upperC2Ont.owl#Equipment -->

    <owl:Class rdf:about="http://cbml.googlecode.com/svn/trunk/upperC2Ont.owl#Equipment">
        <rdfs:subClassOf rdf:resource="http://cbml.googlecode.com/svn/trunk/upperC2Ont.owl#Materiel"/>
        <rdfs:comment>&#39;All nonexpendable items needed to outfit or equip an individual
or organization&#39;
&lt;http://www.dtic.mil/doctrine/new_pubs/jp1_02.pdf&gt;comment
</rdfs:comment>
    </owl:Class>
    


    <!-- http://cbml.googlecode.com/svn/trunk/upperC2Ont.owl#Event -->

    <owl:Class rdf:about="http://cbml.googlecode.com/svn/trunk/upperC2Ont.owl#Event">
        <rdfs:subClassOf rdf:resource="&owl;Thing"/>
        <rdfs:comment>&#39;Anything that happens, or is contemplated as happening; an incident, occurrence&#39;
&lt;http://www.oed.com/viewdictionaryentry/Entry/65287&gt;</rdfs:comment>
    </owl:Class>
    


    <!-- http://cbml.googlecode.com/svn/trunk/upperC2Ont.owl#Facility -->

    <owl:Class rdf:about="http://cbml.googlecode.com/svn/trunk/upperC2Ont.owl#Facility">
        <rdfs:subClassOf rdf:resource="http://cbml.googlecode.com/svn/trunk/upperC2Ont.owl#Entity"/>
        <rdfs:comment>&#39;A real property entity consisting of one or more of the following: a building, a
structure, a utility system, pavement, and underlying land&#39;
&lt;http://www.dtic.mil/doctrine/new_pubs/jp1_02.pdf&gt;</rdfs:comment>
    </owl:Class>
    


    <!-- http://cbml.googlecode.com/svn/trunk/upperC2Ont.owl#GeospatialBoundary -->

    <owl:Class rdf:about="http://cbml.googlecode.com/svn/trunk/upperC2Ont.owl#GeospatialBoundary">
        <rdfs:subClassOf rdf:resource="http://cbml.googlecode.com/svn/trunk/upperC2Ont.owl#GeospatialRegion"/>
        <rdfs:comment>&#39;Boundary of a GeospatialRegion&#39;
&lt;http://C2-Core-Taxonomy-OWL-DL#GeospatialBoundary&gt;</rdfs:comment>
    </owl:Class>
    


    <!-- http://cbml.googlecode.com/svn/trunk/upperC2Ont.owl#GeospatialFeature -->

    <owl:Class rdf:about="http://cbml.googlecode.com/svn/trunk/upperC2Ont.owl#GeospatialFeature">
        <rdfs:subClassOf rdf:resource="http://cbml.googlecode.com/svn/trunk/upperC2Ont.owl#Entity"/>
        <rdfs:comment>&#39;A PhysicalEntity whose (relatively) stable location in some GeospatialRegion can be described by location-specific data.&#39;
&lt;http://UCore-SL-Taxonomy-OWL-DL#GeographicFeature&gt;</rdfs:comment>
    </owl:Class>
    


    <!-- http://cbml.googlecode.com/svn/trunk/upperC2Ont.owl#GeospatialLocation -->

    <owl:Class rdf:about="http://cbml.googlecode.com/svn/trunk/upperC2Ont.owl#GeospatialLocation">
        <rdfs:subClassOf rdf:resource="http://cbml.googlecode.com/svn/trunk/upperC2Ont.owl#GeospatialRegion"/>
        <rdfs:comment>&#39;A GeospatialRegion at which a Entity or Event is located&#39;
&lt;http://C2-Core-Taxonomy-OWL-DL#GeospatialLocation&gt;</rdfs:comment>
    </owl:Class>
    


    <!-- http://cbml.googlecode.com/svn/trunk/upperC2Ont.owl#GeospatialRegion -->

    <owl:Class rdf:about="http://cbml.googlecode.com/svn/trunk/upperC2Ont.owl#GeospatialRegion">
        <rdfs:subClassOf rdf:resource="http://cbml.googlecode.com/svn/trunk/upperC2Ont.owl#SpatialRegion"/>
        <rdfs:comment>&#39;Spatial region at or near the surface of the Earth&#39;
&lt;http://C2-Core-Taxonomy-OWL-DL#GeospatialRegion&gt;</rdfs:comment>
    </owl:Class>
    


    <!-- http://cbml.googlecode.com/svn/trunk/upperC2Ont.owl#GroupOfThings -->

    <owl:Class rdf:about="http://cbml.googlecode.com/svn/trunk/upperC2Ont.owl#GroupOfThings">
        <rdfs:subClassOf rdf:resource="http://cbml.googlecode.com/svn/trunk/upperC2Ont.owl#Entity"/>
        <rdfs:comment>&#39;An assemblage of things&#39;
&lt;http://www.oed.com/viewdictionaryentry/Entry/81855&gt;</rdfs:comment>
    </owl:Class>
    


    <!-- http://cbml.googlecode.com/svn/trunk/upperC2Ont.owl#LivingThing -->

    <owl:Class rdf:about="http://cbml.googlecode.com/svn/trunk/upperC2Ont.owl#LivingThing">
        <rdfs:subClassOf rdf:resource="http://cbml.googlecode.com/svn/trunk/upperC2Ont.owl#Entity"/>
        <rdfs:comment>&#39;A living organism; an animal or plant.&#39;
&lt;http://www.oed.com/viewdictionaryentry/Entry/200786&gt;</rdfs:comment>
    </owl:Class>
    


    <!-- http://cbml.googlecode.com/svn/trunk/upperC2Ont.owl#Materiel -->

    <owl:Class rdf:about="http://cbml.googlecode.com/svn/trunk/upperC2Ont.owl#Materiel">
        <rdfs:subClassOf rdf:resource="http://cbml.googlecode.com/svn/trunk/upperC2Ont.owl#Entity"/>
        <rdfs:comment>&#39;The equipment, supplies, etc., used by an army, navy, or other organization, as distinguished from the personnel or body of people employed.&#39;
&lt;http://www.oed.com/viewdictionaryentry/Entry/114943&gt;</rdfs:comment>
    </owl:Class>
    


    <!-- http://cbml.googlecode.com/svn/trunk/upperC2Ont.owl#Organization -->

    <owl:Class rdf:about="http://cbml.googlecode.com/svn/trunk/upperC2Ont.owl#Organization">
        <rdfs:subClassOf rdf:resource="http://cbml.googlecode.com/svn/trunk/upperC2Ont.owl#Entity"/>
        <rdfs:comment>&#39;An organized body of people with a particular purpose, as a business, government department, charity, etc.&#39;
&lt;http://www.oed.com/viewdictionaryentry/Entry/132452&gt;</rdfs:comment>
    </owl:Class>
    


    <!-- http://cbml.googlecode.com/svn/trunk/upperC2Ont.owl#Person -->

    <owl:Class rdf:about="http://cbml.googlecode.com/svn/trunk/upperC2Ont.owl#Person">
        <rdfs:subClassOf rdf:resource="http://cbml.googlecode.com/svn/trunk/upperC2Ont.owl#Animal"/>
        <rdfs:comment>&#39;The self, being, or individual personality of a man or woman, esp. as distinct from his or her occupation, works, etc. &#39;
&lt;http://www.oed.com/viewdictionaryentry/Entry/141476&gt;</rdfs:comment>
    </owl:Class>
    


    <!-- http://cbml.googlecode.com/svn/trunk/upperC2Ont.owl#PhysicalProperty -->

    <owl:Class rdf:about="http://cbml.googlecode.com/svn/trunk/upperC2Ont.owl#PhysicalProperty">
        <rdfs:subClassOf rdf:resource="http://cbml.googlecode.com/svn/trunk/upperC2Ont.owl#Property"/>
        <rdfs:comment>&#39;A Property that inheres_in some PhysicalEntity&#39;
&lt;http://C2-Core-Taxonomy-OWL-DL#PhysicalProperty&gt;</rdfs:comment>
    </owl:Class>
    


    <!-- http://cbml.googlecode.com/svn/trunk/upperC2Ont.owl#Property -->

    <owl:Class rdf:about="http://cbml.googlecode.com/svn/trunk/upperC2Ont.owl#Property">
        <rdfs:subClassOf rdf:resource="&owl;Thing"/>
        <rdfs:comment>&#39;An attribute, characteristic, or quality of a thing.&#39;
&lt;http://www.oed.com/viewdictionaryentry/Entry/152674&gt;</rdfs:comment>
    </owl:Class>
    


    <!-- http://cbml.googlecode.com/svn/trunk/upperC2Ont.owl#Role -->

    <owl:Class rdf:about="http://cbml.googlecode.com/svn/trunk/upperC2Ont.owl#Role">
        <rdfs:subClassOf rdf:resource="http://cbml.googlecode.com/svn/trunk/upperC2Ont.owl#Property"/>
        <rdfs:comment>&#39;The function performed by someone or something in a particular situation or process.&#39; &lt;http://www.oed.com/viewdictionaryentry/Entry/166971&gt;</rdfs:comment>
    </owl:Class>
    


    <!-- http://cbml.googlecode.com/svn/trunk/upperC2Ont.owl#SpatialRegion -->

    <owl:Class rdf:about="http://cbml.googlecode.com/svn/trunk/upperC2Ont.owl#SpatialRegion">
        <owl:disjointWith rdf:resource="http://cbml.googlecode.com/svn/trunk/upperC2Ont.owl#TemporalRegion"/>
        <rdfs:isDefinedBy rdf:resource="http://www.ifomis.org/bfo/1.1/snap#SpatialRegion"/>
    </owl:Class>
    


    <!-- http://cbml.googlecode.com/svn/trunk/upperC2Ont.owl#TemporalBoundary -->

    <owl:Class rdf:about="http://cbml.googlecode.com/svn/trunk/upperC2Ont.owl#TemporalBoundary">
        <rdfs:label>Temporal Boundary</rdfs:label>
        <rdfs:subClassOf rdf:resource="http://cbml.googlecode.com/svn/trunk/upperC2Ont.owl#TemporalRegion"/>
        <rdfs:comment>Boundary of a TemporalRegion</rdfs:comment>
    </owl:Class>
    


    <!-- http://cbml.googlecode.com/svn/trunk/upperC2Ont.owl#TemporalInstant -->

    <owl:Class rdf:about="http://cbml.googlecode.com/svn/trunk/upperC2Ont.owl#TemporalInstant">
        <rdfs:label>Temporal Instant</rdfs:label>
        <rdfs:subClassOf rdf:resource="http://cbml.googlecode.com/svn/trunk/upperC2Ont.owl#TemporalRegion"/>
        <rdfs:isDefinedBy rdf:resource="http://www.ifomis.org/bfo/1.1/span#TemporalInstant"/>
    </owl:Class>
    


    <!-- http://cbml.googlecode.com/svn/trunk/upperC2Ont.owl#TemporalRegion -->

    <owl:Class rdf:about="http://cbml.googlecode.com/svn/trunk/upperC2Ont.owl#TemporalRegion">
        <rdfs:label>Temporal Region</rdfs:label>
        <rdfs:isDefinedBy rdf:resource="http://www.ifomis.org/bfo/1.1/span#TemporalRegion"/>
    </owl:Class>
    


    <!-- http://cbml.googlecode.com/svn/trunk/upperC2Ont.owl#TemportalInterval -->

    <owl:Class rdf:about="http://cbml.googlecode.com/svn/trunk/upperC2Ont.owl#TemportalInterval">
        <rdfs:label>Temporal Interval</rdfs:label>
        <rdfs:subClassOf rdf:resource="http://cbml.googlecode.com/svn/trunk/upperC2Ont.owl#TemporalRegion"/>
        <rdfs:isDefinedBy rdf:resource="http://www.ifomis.org/bfo/1.1/span#TemporalInterval"/>
    </owl:Class>
    


    <!-- http://www.w3.org/2002/07/owl#Thing -->

    <owl:Class rdf:about="&owl;Thing">
        <rdfs:comment>&#39;That which exists individually (in the most general sense, in fact or in idea); that which is or may be in any way an object of perception, knowledge, or thought; an entity, a being. (Including persons, in contexts where personality is not significant.)&#39;
&lt;http://www.oed.com/viewdictionaryentry/Entry/200786&gt;</rdfs:comment>
    </owl:Class>
</rdf:RDF>



<!-- Generated by the OWL API (version 3.2.3.22702) http://owlapi.sourceforge.net -->

