<rdf:RDF
    xmlns="http://cbml.googlecode.com/svn/trunk/jc3iedmOnt/jc3iedmSubExtOnt.owl#"
    xmlns:rdf="http://www.w3.org/1999/02/22-rdf-syntax-ns#"
    xmlns:owl="http://www.w3.org/2002/07/owl#"
    xmlns:xsd="http://www.w3.org/2001/XMLSchema#"
    xmlns:rdfs="http://www.w3.org/2000/01/rdf-schema#"
  xml:base="http://cbml.googlecode.com/svn/trunk/jc3iedmOnt/jc3iedmSubExtOnt.owl#">
  <owl:Ontology rdf:about="#">
    <owl:imports rdf:resource="jc3iedmSubOnt.owl#"/>
    <owl:imports rdf:resource="jc3iedmBase.owl#"/>
  </owl:Ontology>
  <owl:Class rdf:ID="UN_Dangerous_Goods_NUM_2485">
    <rdfs:subClassOf>
      <owl:Restriction>
        <owl:hasValue xml:lang="en">2485</owl:hasValue>
        <owl:onProperty rdf:resource="jc3iedmBase.owl#consumable-materiel-type-united-nations-number-code"/>
      </owl:Restriction>
    </rdfs:subClassOf>
    <rdfs:label xml:lang="en">UN Dangerous Goods # 2485</rdfs:label>
    <rdfs:comment xml:lang="en">N-butyl isocyanate. Includes the agent(s): n-butyl isocyanate.</rdfs:comment>
    <rdfs:subClassOf>
      <owl:Restriction>
        <owl:hasValue xml:lang="en">2485</owl:hasValue>
        <owl:onProperty rdf:resource="jc3iedmBase.owl#consumable-materiel-type-united-nations-number-code"/>
      </owl:Restriction>
    </rdfs:subClassOf>
  </owl:Class>
  <owl:Class rdf:ID="Centreline_drogue_and_wingtip_drogue">
    <rdfs:subClassOf rdf:resource="jc3iedmSubOnt.owl#MISCELLANEOUS-EQUIPMENT-TYPE-Aircraft_refuelling"/>
    <rdfs:subClassOf>
      <owl:Restriction>
        <owl:hasValue xml:lang="en">CDWD</owl:hasValue>
        <owl:onProperty rdf:resource="jc3iedmBase.owl#miscellaneous-equipment-type-subcategory-code"/>
      </owl:Restriction>
    </rdfs:subClassOf>
    <rdfs:label xml:lang="en">Centreline drogue and wingtip drogue</rdfs:label>
    <rdfs:comment xml:lang="en">Two components of a refuelling system by which centreline drogue and wingtip drogue devices can provide fuel on a receiver aircraft.</rdfs:comment>
  </owl:Class>
  <owl:Class rdf:ID="Gun">
    <rdfs:subClassOf rdf:resource="jc3iedmSubOnt.owl#WEAPON-TYPE-Field_artillery"/>
    <rdfs:subClassOf rdf:resource="jc3iedmSubOnt.owl#WEAPON-TYPE-Cannon"/>
    <rdfs:subClassOf>
      <owl:Restriction>
        <owl:hasValue xml:lang="en">GUN</owl:hasValue>
        <owl:onProperty rdf:resource="jc3iedmBase.owl#weapon-type-subcategory-code"/>
      </owl:Restriction>
    </rdfs:subClassOf>
    <rdfs:label xml:lang="en">Gun</rdfs:label>
    <rdfs:comment xml:lang="en">A cannon with a relatively long barrel, operating with a relatively low angle of fire, and having a high muzzle velocity.</rdfs:comment>
    <rdfs:subClassOf>
      <owl:Restriction>
        <owl:hasValue xml:lang="en">GUN</owl:hasValue>
        <owl:onProperty rdf:resource="jc3iedmBase.owl#weapon-type-subcategory-code"/>
      </owl:Restriction>
    </rdfs:subClassOf>
  </owl:Class>
  <owl:Class rdf:ID="Low_frequency_active_system">
    <rdfs:subClassOf rdf:resource="jc3iedmSubOnt.owl#ELECTRONIC-EQUIPMENT-TYPE-Communication"/>
    <rdfs:subClassOf>
      <owl:Restriction>
        <owl:hasValue xml:lang="en">LFRACS</owl:hasValue>
        <owl:onProperty rdf:resource="jc3iedmBase.owl#electronic-equipment-type-subcategory-code"/>
      </owl:Restriction>
    </rdfs:subClassOf>
    <rdfs:label xml:lang="en">Low frequency active system</rdfs:label>
    <rdfs:comment xml:lang="en">Large shipboard sonar that uses intense sound for long-range surveillance and detecting submarines.</rdfs:comment>
  </owl:Class>
  <owl:Class rdf:ID="Reconnaissance_tank">
    <rdfs:subClassOf rdf:resource="jc3iedmSubOnt.owl#WEAPON-TYPE-Tank"/>
    <rdfs:subClassOf>
      <owl:Restriction>
        <owl:hasValue xml:lang="en">RECTNK</owl:hasValue>
        <owl:onProperty rdf:resource="jc3iedmBase.owl#weapon-type-subcategory-code"/>
      </owl:Restriction>
    </rdfs:subClassOf>
    <rdfs:label xml:lang="en">Reconnaissance tank</rdfs:label>
    <rdfs:comment xml:lang="en">A mobile armoured vehicle providing firepower and crew protection for reconnaissance activities.</rdfs:comment>
  </owl:Class>
  <owl:Class rdf:ID="Marsh">
    <rdfs:subClassOf rdf:resource="jc3iedmSubOnt.owl#GEOGRAPHIC-FEATURE-Solid_surface"/>
    <rdfs:subClassOf rdf:resource="jc3iedmSubOnt.owl#GEOGRAPHIC-FEATURE-TYPE-Wetland"/>
    <rdfs:subClassOf rdf:resource="jc3iedmSubOnt.owl#GEOGRAPHIC-FEATURE-Liquid_surface"/>
    <rdfs:subClassOf>
      <owl:Restriction>
        <owl:hasValue xml:lang="en">MARSH</owl:hasValue>
        <owl:onProperty rdf:resource="jc3iedmBase.owl#geographic-feature-type-subcategory-code"/>
      </owl:Restriction>
    </rdfs:subClassOf>
    <rdfs:label xml:lang="en">Marsh</rdfs:label>
    <rdfs:comment xml:lang="en">An area of wet, often spongy ground that is subject to frequent or tidal inundations, but not considered to be continually under water.</rdfs:comment>
    <rdfs:subClassOf>
      <owl:Restriction>
        <owl:hasValue xml:lang="en">MARSH</owl:hasValue>
        <owl:onProperty rdf:resource="jc3iedmBase.owl#geographic-feature-type-subcategory-code"/>
      </owl:Restriction>
    </rdfs:subClassOf>
    <rdfs:subClassOf>
      <owl:Restriction>
        <owl:hasValue xml:lang="en">MARSH</owl:hasValue>
        <owl:onProperty rdf:resource="jc3iedmBase.owl#geographic-feature-type-subcategory-code"/>
      </owl:Restriction>
    </rdfs:subClassOf>
  </owl:Class>
  <owl:Class rdf:ID="UN_Dangerous_Goods_NUM_2029">
    <rdfs:subClassOf>
      <owl:Restriction>
        <owl:hasValue xml:lang="en">2029</owl:hasValue>
        <owl:onProperty rdf:resource="jc3iedmBase.owl#consumable-materiel-type-united-nations-number-code"/>
      </owl:Restriction>
    </rdfs:subClassOf>
    <rdfs:label xml:lang="en">UN Dangerous Goods # 2029</rdfs:label>
    <rdfs:comment xml:lang="en">Hydrazine, anhydrous. Includes the agent(s): hydrazine.</rdfs:comment>
    <rdfs:subClassOf>
      <owl:Restriction>
        <owl:hasValue xml:lang="en">2029</owl:hasValue>
        <owl:onProperty rdf:resource="jc3iedmBase.owl#consumable-materiel-type-united-nations-number-code"/>
      </owl:Restriction>
    </rdfs:subClassOf>
  </owl:Class>
  <owl:Class rdf:about="#Cutter,_static">
    <rdfs:subClassOf rdf:resource="jc3iedmSubOnt.owl#MARITIME-EQUIPMENT-TYPE-Cutter"/>
    <rdfs:subClassOf>
      <owl:Restriction>
        <owl:hasValue xml:lang="en">CUTTST</owl:hasValue>
        <owl:onProperty rdf:resource="jc3iedmBase.owl#maritime-equipment-type-subcategory-code"/>
      </owl:Restriction>
    </rdfs:subClassOf>
    <rdfs:label xml:lang="en">Cutter, static</rdfs:label>
    <rdfs:comment xml:lang="en">A device that is static and cuts the cable by use of mechanical forces.</rdfs:comment>
  </owl:Class>
  <owl:Class rdf:about="#Identification_friend/foe">
    <rdfs:subClassOf rdf:resource="jc3iedmSubOnt.owl#ELECTRONIC-EQUIPMENT-TYPE-Sensor"/>
    <rdfs:subClassOf>
      <owl:Restriction>
        <owl:hasValue xml:lang="en">IDNTFF</owl:hasValue>
        <owl:onProperty rdf:resource="jc3iedmBase.owl#electronic-equipment-type-subcategory-code"/>
      </owl:Restriction>
    </rdfs:subClassOf>
    <rdfs:label xml:lang="en">Identification friend/foe</rdfs:label>
    <rdfs:comment xml:lang="en">A system using electromagnetic transmissions to which equipment carried by friendly forces automatically responds.</rdfs:comment>
  </owl:Class>
  <owl:Class rdf:ID="Fit">
    <rdfs:subClassOf>
      <owl:Restriction>
        <owl:hasValue xml:lang="en">FT</owl:hasValue>
        <owl:onProperty rdf:resource="jc3iedmBase.owl#person-status-physical-status-code"/>
      </owl:Restriction>
    </rdfs:subClassOf>
    <rdfs:label xml:lang="en">Fit</rdfs:label>
    <rdfs:subClassOf>
      <owl:Restriction>
        <owl:hasValue xml:lang="en">FT</owl:hasValue>
        <owl:onProperty rdf:resource="jc3iedmBase.owl#person-status-physical-status-code"/>
      </owl:Restriction>
    </rdfs:subClassOf>
    <rdfs:subClassOf>
      <owl:Restriction>
        <owl:hasValue xml:lang="en">FT</owl:hasValue>
        <owl:onProperty rdf:resource="jc3iedmBase.owl#person-status-physical-status-code"/>
      </owl:Restriction>
    </rdfs:subClassOf>
    <rdfs:subClassOf>
      <owl:Restriction>
        <owl:hasValue xml:lang="en">FT</owl:hasValue>
        <owl:onProperty rdf:resource="jc3iedmBase.owl#person-status-physical-status-code"/>
      </owl:Restriction>
    </rdfs:subClassOf>
    <rdfs:subClassOf>
      <owl:Restriction>
        <owl:hasValue xml:lang="en">FT</owl:hasValue>
        <owl:onProperty rdf:resource="jc3iedmBase.owl#person-status-physical-status-code"/>
      </owl:Restriction>
    </rdfs:subClassOf>
    <rdfs:subClassOf>
      <owl:Restriction>
        <owl:hasValue xml:lang="en">FT</owl:hasValue>
        <owl:onProperty rdf:resource="jc3iedmBase.owl#person-status-physical-status-code"/>
      </owl:Restriction>
    </rdfs:subClassOf>
    <rdfs:comment xml:lang="en">A status indicating that a PERSON is considered as having normal physical capabilities.</rdfs:comment>
    <rdfs:subClassOf>
      <owl:Restriction>
        <owl:hasValue xml:lang="en">FT</owl:hasValue>
        <owl:onProperty rdf:resource="jc3iedmBase.owl#person-status-physical-status-code"/>
      </owl:Restriction>
    </rdfs:subClassOf>
  </owl:Class>
  <owl:Class rdf:about="#Rifle,_assault">
    <rdfs:subClassOf rdf:resource="jc3iedmSubOnt.owl#WEAPON-TYPE-Small_arms"/>
    <rdfs:subClassOf>
      <owl:Restriction>
        <owl:hasValue xml:lang="en">RFLASS</owl:hasValue>
        <owl:onProperty rdf:resource="jc3iedmBase.owl#weapon-type-subcategory-code"/>
      </owl:Restriction>
    </rdfs:subClassOf>
    <rdfs:label xml:lang="en">Rifle, assault</rdfs:label>
    <rdfs:comment xml:lang="en">A firearm used in an assault role, that has a rifled bore designed to be fired from the shoulder.</rdfs:comment>
  </owl:Class>
  <owl:Class rdf:ID="Night_observation_device">
    <rdfs:subClassOf rdf:resource="jc3iedmSubOnt.owl#ELECTRONIC-EQUIPMENT-TYPE-Sensor"/>
    <rdfs:subClassOf>
      <owl:Restriction>
        <owl:hasValue xml:lang="en">NGOBDV</owl:hasValue>
        <owl:onProperty rdf:resource="jc3iedmBase.owl#electronic-equipment-type-subcategory-code"/>
      </owl:Restriction>
    </rdfs:subClassOf>
    <rdfs:label xml:lang="en">Night observation device</rdfs:label>
    <rdfs:comment xml:lang="en">A scope, goggles, camera or other device that uses either ambient light amplification or thermal imaging using the infrared spectrum enabling vision during periods of low light.</rdfs:comment>
  </owl:Class>
  <owl:Class rdf:ID="Khat">
    <rdfs:subClassOf rdf:resource="jc3iedmSubOnt.owl#CONSUMABLE-MATERIEL-TYPE-Drug"/>
    <rdfs:subClassOf>
      <owl:Restriction>
        <owl:hasValue xml:lang="en">KHAT</owl:hasValue>
        <owl:onProperty rdf:resource="jc3iedmBase.owl#consumable-materiel-type-subcategory-code"/>
      </owl:Restriction>
    </rdfs:subClassOf>
    <rdfs:label xml:lang="en">Khat</rdfs:label>
    <rdfs:comment xml:lang="en">The leaves of this shrub, chewed or infused as a stimulant.</rdfs:comment>
  </owl:Class>
  <owl:Class rdf:about="#Wagon,_warflat">
    <rdfs:subClassOf rdf:resource="jc3iedmSubOnt.owl#RAILCAR-TYPE-Rolling_stock"/>
    <rdfs:subClassOf>
      <owl:Restriction>
        <owl:hasValue xml:lang="en">WGNWFL</owl:hasValue>
        <owl:onProperty rdf:resource="jc3iedmBase.owl#railcar-type-subcategory-code"/>
      </owl:Restriction>
    </rdfs:subClassOf>
    <rdfs:label xml:lang="en">Wagon, warflat</rdfs:label>
    <rdfs:comment xml:lang="en">Rolling stock used to move specific military loads, for example AIFVs (UK Warrior).</rdfs:comment>
  </owl:Class>
  <owl:Class rdf:about="#Ballistic_missile_launcher,_short_range">
    <rdfs:subClassOf rdf:resource="jc3iedmSubOnt.owl#WEAPON-TYPE-Missile_system"/>
    <rdfs:subClassOf>
      <owl:Restriction>
        <owl:hasValue xml:lang="en">BMLSR</owl:hasValue>
        <owl:onProperty rdf:resource="jc3iedmBase.owl#weapon-type-subcategory-code"/>
      </owl:Restriction>
    </rdfs:subClassOf>
    <rdfs:label xml:lang="en">Ballistic missile launcher, short range</rdfs:label>
    <rdfs:comment xml:lang="en">A structural device designed to support and hold a short range ballistic missile in position for firing.</rdfs:comment>
  </owl:Class>
  <owl:Class rdf:ID="UN_Dangerous_Goods_NUM_1838">
    <rdfs:subClassOf>
      <owl:Restriction>
        <owl:hasValue xml:lang="en">1838</owl:hasValue>
        <owl:onProperty rdf:resource="jc3iedmBase.owl#consumable-materiel-type-united-nations-number-code"/>
      </owl:Restriction>
    </rdfs:subClassOf>
    <rdfs:label xml:lang="en">UN Dangerous Goods # 1838</rdfs:label>
    <rdfs:comment xml:lang="en">Titanium tetrachloride. Includes the agent(s): titanium tetrachloride.</rdfs:comment>
    <rdfs:subClassOf>
      <owl:Restriction>
        <owl:hasValue xml:lang="en">1838</owl:hasValue>
        <owl:onProperty rdf:resource="jc3iedmBase.owl#consumable-materiel-type-united-nations-number-code"/>
      </owl:Restriction>
    </rdfs:subClassOf>
  </owl:Class>
  <owl:Class rdf:ID="UN_Dangerous_Goods_NUM_1184">
    <rdfs:subClassOf>
      <owl:Restriction>
        <owl:hasValue xml:lang="en">1184</owl:hasValue>
        <owl:onProperty rdf:resource="jc3iedmBase.owl#consumable-materiel-type-united-nations-number-code"/>
      </owl:Restriction>
    </rdfs:subClassOf>
    <rdfs:label xml:lang="en">UN Dangerous Goods # 1184</rdfs:label>
    <rdfs:comment xml:lang="en">Ethylene dichloride. Includes the agent(s): 1,2 dichloroethane.</rdfs:comment>
    <rdfs:subClassOf>
      <owl:Restriction>
        <owl:hasValue xml:lang="en">1184</owl:hasValue>
        <owl:onProperty rdf:resource="jc3iedmBase.owl#consumable-materiel-type-united-nations-number-code"/>
      </owl:Restriction>
    </rdfs:subClassOf>
  </owl:Class>
  <owl:Class rdf:ID="UN_Dangerous_Goods_NUM_1810">
    <rdfs:subClassOf>
      <owl:Restriction>
        <owl:hasValue xml:lang="en">1810</owl:hasValue>
        <owl:onProperty rdf:resource="jc3iedmBase.owl#consumable-materiel-type-united-nations-number-code"/>
      </owl:Restriction>
    </rdfs:subClassOf>
    <rdfs:label xml:lang="en">UN Dangerous Goods # 1810</rdfs:label>
    <rdfs:comment xml:lang="en">Phosphorus oxychloride. Includes the agent(s): phosphorus oxychloride.</rdfs:comment>
    <rdfs:subClassOf>
      <owl:Restriction>
        <owl:hasValue xml:lang="en">1810</owl:hasValue>
        <owl:onProperty rdf:resource="jc3iedmBase.owl#consumable-materiel-type-united-nations-number-code"/>
      </owl:Restriction>
    </rdfs:subClassOf>
  </owl:Class>
  <owl:Class rdf:ID="Tank_destroyer">
    <rdfs:subClassOf rdf:resource="jc3iedmSubOnt.owl#WEAPON-TYPE-Anti-tank"/>
    <rdfs:subClassOf>
      <owl:Restriction>
        <owl:hasValue xml:lang="en">TKDTRY</owl:hasValue>
        <owl:onProperty rdf:resource="jc3iedmBase.owl#weapon-type-subcategory-code"/>
      </owl:Restriction>
    </rdfs:subClassOf>
    <rdfs:label xml:lang="en">Tank destroyer</rdfs:label>
    <rdfs:comment xml:lang="en">A tracked vehicle that relies on speed and firepower and has minimum armoured protection, usually armed with either anti-tank guided missile launcher, 80-90 MM gun or a recoilless rifle.</rdfs:comment>
  </owl:Class>
  <owl:Class rdf:ID="Glacier">
    <rdfs:subClassOf rdf:resource="jc3iedmSubOnt.owl#GEOGRAPHIC-FEATURE-TYPE-Snow/ice"/>
    <rdfs:subClassOf rdf:resource="jc3iedmSubOnt.owl#GEOGRAPHIC-FEATURE-Solid_surface"/>
    <rdfs:subClassOf>
      <owl:Restriction>
        <owl:hasValue xml:lang="en">GLACER</owl:hasValue>
        <owl:onProperty rdf:resource="jc3iedmBase.owl#geographic-feature-type-subcategory-code"/>
      </owl:Restriction>
    </rdfs:subClassOf>
    <rdfs:label xml:lang="en">Glacier</rdfs:label>
    <rdfs:comment xml:lang="en">A large mass of snow and ice moving slowly down a slope or valley from above the snowline.</rdfs:comment>
    <rdfs:subClassOf>
      <owl:Restriction>
        <owl:hasValue xml:lang="en">GLACER</owl:hasValue>
        <owl:onProperty rdf:resource="jc3iedmBase.owl#geographic-feature-type-subcategory-code"/>
      </owl:Restriction>
    </rdfs:subClassOf>
  </owl:Class>
  <owl:Class rdf:about="#Link_16,_voice">
    <rdfs:subClassOf rdf:resource="jc3iedmSubOnt.owl#NETWORK-SERVICE-Tactical_data_link"/>
    <rdfs:subClassOf>
      <owl:Restriction>
        <owl:hasValue xml:lang="en">LNK16V</owl:hasValue>
        <owl:onProperty rdf:resource="jc3iedmBase.owl#network-service-subcategory-code"/>
      </owl:Restriction>
    </rdfs:subClassOf>
    <rdfs:label xml:lang="en">Link 16, voice</rdfs:label>
    <rdfs:comment xml:lang="en">A service that provides the basic elements for the transmission of voice of Link 16.</rdfs:comment>
  </owl:Class>
  <owl:Class rdf:about="#Anti-tank_missile_launcher,_heavy">
    <rdfs:subClassOf rdf:resource="jc3iedmSubOnt.owl#WEAPON-TYPE-Missile_system"/>
    <rdfs:subClassOf rdf:resource="jc3iedmSubOnt.owl#WEAPON-TYPE-Anti-tank"/>
    <rdfs:subClassOf>
      <owl:Restriction>
        <owl:hasValue xml:lang="en">ATMLHV</owl:hasValue>
        <owl:onProperty rdf:resource="jc3iedmBase.owl#weapon-type-subcategory-code"/>
      </owl:Restriction>
    </rdfs:subClassOf>
    <rdfs:label xml:lang="en">Anti-tank missile launcher, heavy</rdfs:label>
    <rdfs:comment xml:lang="en">A heavy structural device designed to support and hold an anti-tank missile in position for firing.</rdfs:comment>
    <rdfs:subClassOf>
      <owl:Restriction>
        <owl:hasValue xml:lang="en">ATMLHV</owl:hasValue>
        <owl:onProperty rdf:resource="jc3iedmBase.owl#weapon-type-subcategory-code"/>
      </owl:Restriction>
    </rdfs:subClassOf>
  </owl:Class>
  <owl:Class rdf:ID="Electrooptical">
    <rdfs:subClassOf rdf:resource="jc3iedmSubOnt.owl#ELECTRONIC-EQUIPMENT-TYPE-Communication"/>
    <rdfs:subClassOf>
      <owl:Restriction>
        <owl:hasValue xml:lang="en">ELTOPT</owl:hasValue>
        <owl:onProperty rdf:resource="jc3iedmBase.owl#electronic-equipment-type-subcategory-code"/>
      </owl:Restriction>
    </rdfs:subClassOf>
    <rdfs:label xml:lang="en">Electrooptical</rdfs:label>
    <rdfs:comment xml:lang="en">Equipment that deals with the translation of electromagnetic radiation in the visible and infrared portion of the spectrum into a format suitable for electronic application and vice versa.</rdfs:comment>
  </owl:Class>
  <owl:Class rdf:about="#Tank_gun,_heavy">
    <rdfs:subClassOf rdf:resource="jc3iedmSubOnt.owl#WEAPON-TYPE-Anti-tank"/>
    <rdfs:subClassOf>
      <owl:Restriction>
        <owl:hasValue xml:lang="en">TKGUNH</owl:hasValue>
        <owl:onProperty rdf:resource="jc3iedmBase.owl#weapon-type-subcategory-code"/>
      </owl:Restriction>
    </rdfs:subClassOf>
    <rdfs:label xml:lang="en">Tank gun, heavy</rdfs:label>
    <rdfs:comment xml:lang="en">Heavy, turret mounted, tank gun, calibre over 120 MM, for use in the field against tanks.</rdfs:comment>
  </owl:Class>
  <owl:Class rdf:ID="Fighter">
    <rdfs:subClassOf rdf:resource="jc3iedmSubOnt.owl#AIRCRAFT-TYPE-Fixed_wing"/>
    <rdfs:subClassOf>
      <owl:Restriction>
        <owl:hasValue xml:lang="en">FIGHTR</owl:hasValue>
        <owl:onProperty rdf:resource="jc3iedmBase.owl#aircraft-type-airframe-design-code"/>
      </owl:Restriction>
    </rdfs:subClassOf>
    <rdfs:label xml:lang="en">Fighter</rdfs:label>
    <rdfs:comment xml:lang="en">A generic term to describe a type of fast and manoeuvrable fixed wing aircraft capable of tactical air operations against air and/or surface targets.</rdfs:comment>
  </owl:Class>
  <owl:Class rdf:ID="NBC_kit">
    <rdfs:subClassOf rdf:resource="jc3iedmSubOnt.owl#CONSUMABLE-MATERIEL-TYPE-Personal_equipment"/>
    <rdfs:subClassOf>
      <owl:Restriction>
        <owl:hasValue xml:lang="en">NBCKIT</owl:hasValue>
        <owl:onProperty rdf:resource="jc3iedmBase.owl#consumable-materiel-type-subcategory-code"/>
      </owl:Restriction>
    </rdfs:subClassOf>
    <rdfs:label xml:lang="en">NBC kit</rdfs:label>
    <rdfs:comment xml:lang="en">The personal equipment and or medical supplies issued to a person for protection against chemical, biological, radiological, or nuclear materiel contamination or exposure.</rdfs:comment>
  </owl:Class>
  <owl:Class rdf:about="#Radar,_ground_surveillance">
    <rdfs:subClassOf rdf:resource="jc3iedmSubOnt.owl#ELECTRONIC-EQUIPMENT-TYPE-Radar"/>
    <rdfs:subClassOf rdf:resource="jc3iedmSubOnt.owl#ELECTRONIC-EQUIPMENT-TYPE-Sensor"/>
    <rdfs:subClassOf>
      <owl:Restriction>
        <owl:hasValue xml:lang="en">RDRGRS</owl:hasValue>
        <owl:onProperty rdf:resource="jc3iedmBase.owl#electronic-equipment-type-subcategory-code"/>
      </owl:Restriction>
    </rdfs:subClassOf>
    <rdfs:label xml:lang="en">Radar, ground surveillance</rdfs:label>
    <rdfs:comment xml:lang="en">Radar with the normal function of maintaining continuous watch over an area.</rdfs:comment>
    <rdfs:subClassOf>
      <owl:Restriction>
        <owl:hasValue xml:lang="en">RDRGRS</owl:hasValue>
        <owl:onProperty rdf:resource="jc3iedmBase.owl#electronic-equipment-type-subcategory-code"/>
      </owl:Restriction>
    </rdfs:subClassOf>
  </owl:Class>
  <owl:Class rdf:about="#Gun/howitzer">
    <rdfs:subClassOf rdf:resource="jc3iedmSubOnt.owl#WEAPON-TYPE-Field_artillery"/>
    <rdfs:subClassOf rdf:resource="jc3iedmSubOnt.owl#WEAPON-TYPE-Cannon"/>
    <rdfs:subClassOf>
      <owl:Restriction>
        <owl:hasValue xml:lang="en">GUNHOW</owl:hasValue>
        <owl:onProperty rdf:resource="jc3iedmBase.owl#weapon-type-subcategory-code"/>
      </owl:Restriction>
    </rdfs:subClassOf>
    <rdfs:label xml:lang="en">Gun/howitzer</rdfs:label>
    <rdfs:comment xml:lang="en">A cannon that has the capability of both low-angle and high-angles of fire.</rdfs:comment>
    <rdfs:subClassOf>
      <owl:Restriction>
        <owl:hasValue xml:lang="en">GUNHOW</owl:hasValue>
        <owl:onProperty rdf:resource="jc3iedmBase.owl#weapon-type-subcategory-code"/>
      </owl:Restriction>
    </rdfs:subClassOf>
  </owl:Class>
  <owl:Class rdf:about="#Radar,_counter-battery_ranging">
    <rdfs:subClassOf rdf:resource="jc3iedmSubOnt.owl#ELECTRONIC-EQUIPMENT-TYPE-Radar"/>
    <rdfs:subClassOf rdf:resource="jc3iedmSubOnt.owl#ELECTRONIC-EQUIPMENT-TYPE-Fire_control"/>
    <rdfs:subClassOf>
      <owl:Restriction>
        <owl:hasValue xml:lang="en">RDRCBR</owl:hasValue>
        <owl:onProperty rdf:resource="jc3iedmBase.owl#electronic-equipment-type-subcategory-code"/>
      </owl:Restriction>
    </rdfs:subClassOf>
    <rdfs:label xml:lang="en">Radar, counter-battery ranging</rdfs:label>
    <rdfs:comment xml:lang="en">Weapon locating radar capable of locating guns, mortars and rockets.</rdfs:comment>
    <rdfs:subClassOf>
      <owl:Restriction>
        <owl:hasValue xml:lang="en">RDRCBR</owl:hasValue>
        <owl:onProperty rdf:resource="jc3iedmBase.owl#electronic-equipment-type-subcategory-code"/>
      </owl:Restriction>
    </rdfs:subClassOf>
  </owl:Class>
  <owl:Class rdf:ID="UN_Dangerous_Goods_NUM_1569">
    <rdfs:subClassOf>
      <owl:Restriction>
        <owl:hasValue xml:lang="en">1569</owl:hasValue>
        <owl:onProperty rdf:resource="jc3iedmBase.owl#consumable-materiel-type-united-nations-number-code"/>
      </owl:Restriction>
    </rdfs:subClassOf>
    <rdfs:label xml:lang="en">UN Dangerous Goods # 1569</rdfs:label>
    <rdfs:comment xml:lang="en">Bromoacetone. Includes the agent(s): bromoacetone.</rdfs:comment>
    <rdfs:subClassOf>
      <owl:Restriction>
        <owl:hasValue xml:lang="en">1569</owl:hasValue>
        <owl:onProperty rdf:resource="jc3iedmBase.owl#consumable-materiel-type-united-nations-number-code"/>
      </owl:Restriction>
    </rdfs:subClassOf>
  </owl:Class>
  <owl:Class rdf:about="#Wagon,_refrigerated">
    <rdfs:subClassOf rdf:resource="jc3iedmSubOnt.owl#RAILCAR-TYPE-Rolling_stock"/>
    <rdfs:subClassOf>
      <owl:Restriction>
        <owl:hasValue xml:lang="en">WGNRFG</owl:hasValue>
        <owl:onProperty rdf:resource="jc3iedmBase.owl#railcar-type-subcategory-code"/>
      </owl:Restriction>
    </rdfs:subClassOf>
    <rdfs:label xml:lang="en">Wagon, refrigerated</rdfs:label>
    <rdfs:comment xml:lang="en">Rolling stock used to move refrigerated cargoes by rail.</rdfs:comment>
  </owl:Class>
  <owl:Class rdf:ID="Ecstasy_-_MDMA">
    <rdfs:subClassOf rdf:resource="jc3iedmSubOnt.owl#CONSUMABLE-MATERIEL-TYPE-Drug"/>
    <rdfs:subClassOf>
      <owl:Restriction>
        <owl:hasValue xml:lang="en">ECSMDM</owl:hasValue>
        <owl:onProperty rdf:resource="jc3iedmBase.owl#consumable-materiel-type-subcategory-code"/>
      </owl:Restriction>
    </rdfs:subClassOf>
    <rdfs:label xml:lang="en">Ecstasy - MDMA</rdfs:label>
    <rdfs:comment xml:lang="en">Methylenedioxymethamphetamine, an amphetamine-based drug that causes euphoric and hallucinatory effects, originally produced as an appetite suppressant.</rdfs:comment>
  </owl:Class>
  <owl:Class rdf:about="#Sweep,_magnetic_solenoid">
    <rdfs:subClassOf rdf:resource="jc3iedmSubOnt.owl#MARITIME-EQUIPMENT-TYPE-Sweep"/>
    <rdfs:subClassOf>
      <owl:Restriction>
        <owl:hasValue xml:lang="en">SWPMGS</owl:hasValue>
        <owl:onProperty rdf:resource="jc3iedmBase.owl#maritime-equipment-type-subcategory-code"/>
      </owl:Restriction>
    </rdfs:subClassOf>
    <rdfs:label xml:lang="en">Sweep, magnetic solenoid</rdfs:label>
    <rdfs:comment xml:lang="en">Equipment designed to locate mines by use of large number of horizontal coils through which a small current is passed.</rdfs:comment>
  </owl:Class>
  <owl:Class rdf:about="#Sweep,_hovercraft_acoustic">
    <rdfs:subClassOf rdf:resource="jc3iedmSubOnt.owl#MARITIME-EQUIPMENT-TYPE-Sweep"/>
    <rdfs:subClassOf>
      <owl:Restriction>
        <owl:hasValue xml:lang="en">SWPHVA</owl:hasValue>
        <owl:onProperty rdf:resource="jc3iedmBase.owl#maritime-equipment-type-subcategory-code"/>
      </owl:Restriction>
    </rdfs:subClassOf>
    <rdfs:label xml:lang="en">Sweep, hovercraft acoustic</rdfs:label>
    <rdfs:comment xml:lang="en">Equipment mounted on a hovercraft designed to be used in minesweeping operations, utilising the acoustic firing mechanisms of the target mines.</rdfs:comment>
  </owl:Class>
  <owl:Class rdf:ID="Communication_antenna">
    <rdfs:subClassOf rdf:resource="jc3iedmSubOnt.owl#ELECTRONIC-EQUIPMENT-TYPE-Communication"/>
    <rdfs:subClassOf>
      <owl:Restriction>
        <owl:hasValue xml:lang="en">COMANT</owl:hasValue>
        <owl:onProperty rdf:resource="jc3iedmBase.owl#electronic-equipment-type-subcategory-code"/>
      </owl:Restriction>
    </rdfs:subClassOf>
    <rdfs:label xml:lang="en">Communication antenna</rdfs:label>
    <rdfs:comment xml:lang="en">An equipment for sending or receiving electromagnetic waves.</rdfs:comment>
  </owl:Class>
  <owl:Class rdf:about="#Large_isolated_rock,_boulder,_or_rocky_formation">
    <rdfs:subClassOf rdf:resource="jc3iedmSubOnt.owl#GEOGRAPHIC-FEATURE-Solid_surface"/>
    <rdfs:subClassOf rdf:resource="jc3iedmSubOnt.owl#GEOGRAPHIC-FEATURE-TYPE-Landform"/>
    <rdfs:subClassOf>
      <owl:Restriction>
        <owl:hasValue xml:lang="en">LRGRCK</owl:hasValue>
        <owl:onProperty rdf:resource="jc3iedmBase.owl#geographic-feature-type-subcategory-code"/>
      </owl:Restriction>
    </rdfs:subClassOf>
    <rdfs:label xml:lang="en">Large isolated rock, boulder, or rocky formation</rdfs:label>
    <rdfs:comment xml:lang="en">A conspicuous isolated rocky formation or single large stone existing in its entirety above the high water mark. From offshore it would appear to a mariner as a single point on land and would be appropriate for use in navigation.</rdfs:comment>
    <rdfs:subClassOf>
      <owl:Restriction>
        <owl:hasValue xml:lang="en">LRGRCK</owl:hasValue>
        <owl:onProperty rdf:resource="jc3iedmBase.owl#geographic-feature-type-subcategory-code"/>
      </owl:Restriction>
    </rdfs:subClassOf>
  </owl:Class>
  <owl:Class rdf:about="#Surface-to-surface_missile_launcher,_long_range">
    <rdfs:subClassOf rdf:resource="jc3iedmSubOnt.owl#WEAPON-TYPE-Missile_system"/>
    <rdfs:subClassOf>
      <owl:Restriction>
        <owl:hasValue xml:lang="en">SSMLLR</owl:hasValue>
        <owl:onProperty rdf:resource="jc3iedmBase.owl#weapon-type-subcategory-code"/>
      </owl:Restriction>
    </rdfs:subClassOf>
    <rdfs:label xml:lang="en">Surface-to-surface missile launcher, long range</rdfs:label>
    <rdfs:comment xml:lang="en">A structural device designed to support and hold a long range surface to surface missile in position for firing.</rdfs:comment>
  </owl:Class>
  <owl:Class rdf:ID="Leaflet">
    <rdfs:subClassOf rdf:resource="jc3iedmSubOnt.owl#CONSUMABLE-MATERIEL-TYPE-General_supplies"/>
    <rdfs:subClassOf>
      <owl:Restriction>
        <owl:hasValue xml:lang="en">LEAFLT</owl:hasValue>
        <owl:onProperty rdf:resource="jc3iedmBase.owl#consumable-materiel-type-subcategory-code"/>
      </owl:Restriction>
    </rdfs:subClassOf>
    <rdfs:label xml:lang="en">Leaflet</rdfs:label>
    <rdfs:comment xml:lang="en">A small sized leaf of paper containing printed matter, chiefly for gratuitous distribution.</rdfs:comment>
  </owl:Class>
  <owl:Class rdf:ID="Contact">
    <rdfs:subClassOf rdf:resource="jc3iedmSubOnt.owl#AMMUNITION-TYPE-Seabed_mine"/>
    <rdfs:subClassOf rdf:resource="jc3iedmSubOnt.owl#AMMUNITION-TYPE-Sea_mine"/>
    <rdfs:subClassOf rdf:resource="jc3iedmSubOnt.owl#AMMUNITION-TYPE-Mine,_not_otherwise_specified"/>
    <rdfs:subClassOf rdf:resource="jc3iedmSubOnt.owl#AMMUNITION-TYPE-Mine,_maritime,_moving"/>
    <rdfs:subClassOf rdf:resource="jc3iedmSubOnt.owl#AMMUNITION-TYPE-Mine,_deep_moored"/>
    <rdfs:subClassOf rdf:resource="jc3iedmSubOnt.owl#AMMUNITION-TYPE-Mine,_shallow_moored"/>
    <rdfs:label xml:lang="en">Contact</rdfs:label>
    <rdfs:subClassOf rdf:resource="jc3iedmSubOnt.owl#AMMUNITION-TYPE-Moving_mine,_sea"/>
    <rdfs:subClassOf>
      <owl:Restriction>
        <owl:hasValue xml:lang="en">CONTCT</owl:hasValue>
        <owl:onProperty rdf:resource="jc3iedmBase.owl#ammunition-type-mine-maritime-firing-code"/>
      </owl:Restriction>
    </rdfs:subClassOf>
    <rdfs:subClassOf rdf:resource="jc3iedmSubOnt.owl#AMMUNITION-TYPE-Mine,_moored"/>
    <rdfs:subClassOf rdf:resource="jc3iedmSubOnt.owl#AMMUNITION-TYPE-Mine,_not_known"/>
    <rdfs:comment xml:lang="en">A (maritime) mine firing mechanism that is designed to fire by physical contact between the target mine or its appendages.</rdfs:comment>
  </owl:Class>
  <owl:Class rdf:ID="MCI_Mode_1">
    <rdfs:subClassOf rdf:resource="jc3iedmSubOnt.owl#NETWORK-SERVICE-MCI"/>
    <rdfs:subClassOf>
      <owl:Restriction>
        <owl:hasValue xml:lang="en">MCIMD1</owl:hasValue>
        <owl:onProperty rdf:resource="jc3iedmBase.owl#network-service-subcategory-code"/>
      </owl:Restriction>
    </rdfs:subClassOf>
    <rdfs:label xml:lang="en">MCI Mode 1</rdfs:label>
    <rdfs:comment xml:lang="en">MCI gateway service proving DEM and MEM facilities.</rdfs:comment>
  </owl:Class>
  <owl:Class rdf:about="#Sweep,_helicopter_magnetic">
    <rdfs:subClassOf rdf:resource="jc3iedmSubOnt.owl#MARITIME-EQUIPMENT-TYPE-Sweep"/>
    <rdfs:subClassOf>
      <owl:Restriction>
        <owl:hasValue xml:lang="en">SWPHMA</owl:hasValue>
        <owl:onProperty rdf:resource="jc3iedmBase.owl#maritime-equipment-type-subcategory-code"/>
      </owl:Restriction>
    </rdfs:subClassOf>
    <rdfs:label xml:lang="en">Sweep, helicopter magnetic</rdfs:label>
    <rdfs:comment xml:lang="en">Equipment mounted on a helicopter designed to locate mines by use of a conducting cable through which is passed a high current, towed behind a minesweeper helicopter.</rdfs:comment>
  </owl:Class>
  <owl:Class rdf:ID="UN_Dangerous_Goods_NUM_1541">
    <rdfs:subClassOf>
      <owl:Restriction>
        <owl:hasValue xml:lang="en">1541</owl:hasValue>
        <owl:onProperty rdf:resource="jc3iedmBase.owl#consumable-materiel-type-united-nations-number-code"/>
      </owl:Restriction>
    </rdfs:subClassOf>
    <rdfs:label xml:lang="en">UN Dangerous Goods # 1541</rdfs:label>
    <rdfs:comment xml:lang="en">Acetone cyanohydrin, stabilized. Includes the agent(s): acetone cyanohydrin.</rdfs:comment>
    <rdfs:subClassOf>
      <owl:Restriction>
        <owl:hasValue xml:lang="en">1541</owl:hasValue>
        <owl:onProperty rdf:resource="jc3iedmBase.owl#consumable-materiel-type-united-nations-number-code"/>
      </owl:Restriction>
    </rdfs:subClassOf>
  </owl:Class>
  <owl:Class rdf:ID="Pack_ice">
    <rdfs:subClassOf rdf:resource="jc3iedmSubOnt.owl#GEOGRAPHIC-FEATURE-TYPE-Snow/ice"/>
    <rdfs:subClassOf rdf:resource="jc3iedmSubOnt.owl#GEOGRAPHIC-FEATURE-Solid_surface"/>
    <rdfs:subClassOf>
      <owl:Restriction>
        <owl:hasValue xml:lang="en">PCKICE</owl:hasValue>
        <owl:onProperty rdf:resource="jc3iedmBase.owl#geographic-feature-type-subcategory-code"/>
      </owl:Restriction>
    </rdfs:subClassOf>
    <rdfs:label xml:lang="en">Pack ice</rdfs:label>
    <rdfs:comment xml:lang="en">An area of ice formed by the drifting and crushing together of floating pieces of ice.</rdfs:comment>
    <rdfs:subClassOf>
      <owl:Restriction>
        <owl:hasValue xml:lang="en">PCKICE</owl:hasValue>
        <owl:onProperty rdf:resource="jc3iedmBase.owl#geographic-feature-type-subcategory-code"/>
      </owl:Restriction>
    </rdfs:subClassOf>
  </owl:Class>
  <owl:Class rdf:about="#Buoy,_navigation">
    <rdfs:subClassOf rdf:resource="jc3iedmSubOnt.owl#MARITIME-EQUIPMENT-TYPE-Buoy"/>
    <rdfs:subClassOf>
      <owl:Restriction>
        <owl:hasValue xml:lang="en">BUOYNV</owl:hasValue>
        <owl:onProperty rdf:resource="jc3iedmBase.owl#maritime-equipment-type-subcategory-code"/>
      </owl:Restriction>
    </rdfs:subClassOf>
    <rdfs:label xml:lang="en">Buoy, navigation</rdfs:label>
    <rdfs:comment xml:lang="en">A floating object fastened in a particular place to point out the position of a specific hazard or obstacle for navigation purposes.</rdfs:comment>
  </owl:Class>
  <owl:Class rdf:ID="Immobilised">
    <rdfs:subClassOf>
      <owl:Restriction>
        <owl:hasValue xml:lang="en">IMMBLS</owl:hasValue>
        <owl:onProperty rdf:resource="jc3iedmBase.owl#materiel-status-operational-status-qualifier-code"/>
      </owl:Restriction>
    </rdfs:subClassOf>
    <rdfs:label xml:lang="en">Immobilised</rdfs:label>
    <rdfs:comment xml:lang="en">Subjectively judged by the reporting organisation that a specific materiel or its component is incapable of movement in its current condition.</rdfs:comment>
    <rdfs:subClassOf>
      <owl:Restriction>
        <owl:hasValue xml:lang="en">IMMBLS</owl:hasValue>
        <owl:onProperty rdf:resource="jc3iedmBase.owl#materiel-status-operational-status-qualifier-code"/>
      </owl:Restriction>
    </rdfs:subClassOf>
    <rdfs:subClassOf>
      <owl:Restriction>
        <owl:hasValue xml:lang="en">IMMBLS</owl:hasValue>
        <owl:onProperty rdf:resource="jc3iedmBase.owl#materiel-status-operational-status-qualifier-code"/>
      </owl:Restriction>
    </rdfs:subClassOf>
  </owl:Class>
  <owl:Class rdf:ID="Breached">
    <rdfs:subClassOf>
      <owl:Restriction>
        <owl:hasValue xml:lang="en">BRCHED</owl:hasValue>
        <owl:onProperty rdf:resource="jc3iedmBase.owl#facility-status-operational-status-qualifier-code"/>
      </owl:Restriction>
    </rdfs:subClassOf>
    <rdfs:label xml:lang="en">Breached</rdfs:label>
    <rdfs:comment xml:lang="en">Subjectively judged by the reporting organisation that a FACILITY has been penetrated.</rdfs:comment>
  </owl:Class>
  <owl:Class rdf:about="#Wagon,_cargo_(enclosed)">
    <rdfs:subClassOf rdf:resource="jc3iedmSubOnt.owl#RAILCAR-TYPE-Rolling_stock"/>
    <rdfs:subClassOf>
      <owl:Restriction>
        <owl:hasValue xml:lang="en">WGNCRG</owl:hasValue>
        <owl:onProperty rdf:resource="jc3iedmBase.owl#railcar-type-subcategory-code"/>
      </owl:Restriction>
    </rdfs:subClassOf>
    <rdfs:label xml:lang="en">Wagon, cargo (enclosed)</rdfs:label>
    <rdfs:comment xml:lang="en">Rolling stock used to move boxed or palletised equipment/stores and closed by means of fixed doors either sliding or hinged.</rdfs:comment>
  </owl:Class>
  <owl:Class rdf:ID="Photographic">
    <rdfs:subClassOf rdf:resource="jc3iedmSubOnt.owl#ELECTRONIC-EQUIPMENT-TYPE-Sensor"/>
    <rdfs:subClassOf>
      <owl:Restriction>
        <owl:hasValue xml:lang="en">PHOTOG</owl:hasValue>
        <owl:onProperty rdf:resource="jc3iedmBase.owl#electronic-equipment-type-subcategory-code"/>
      </owl:Restriction>
    </rdfs:subClassOf>
    <rdfs:label xml:lang="en">Photographic</rdfs:label>
    <rdfs:comment xml:lang="en">No definition provided in ADatP-3 Baseline 13.1 FFIRN/FUD 1434/1.</rdfs:comment>
  </owl:Class>
  <owl:Class rdf:about="#Sonar,_variable_depth,_passive">
    <rdfs:subClassOf rdf:resource="jc3iedmSubOnt.owl#MARITIME-EQUIPMENT-TYPE-Sonar,_maritime"/>
    <rdfs:subClassOf>
      <owl:Restriction>
        <owl:hasValue xml:lang="en">SONRVP</owl:hasValue>
        <owl:onProperty rdf:resource="jc3iedmBase.owl#maritime-equipment-type-subcategory-code"/>
      </owl:Restriction>
    </rdfs:subClassOf>
    <rdfs:label xml:lang="en">Sonar, variable depth, passive</rdfs:label>
    <rdfs:comment xml:lang="en">No definition provided in ADatP-3 Baseline 13.1 FFIRN/FUD 1434/1.</rdfs:comment>
  </owl:Class>
  <owl:Class rdf:about="#Sonar,_ship">
    <rdfs:subClassOf rdf:resource="jc3iedmSubOnt.owl#MARITIME-EQUIPMENT-TYPE-Sonar,_maritime"/>
    <rdfs:subClassOf>
      <owl:Restriction>
        <owl:hasValue xml:lang="en">SONRSH</owl:hasValue>
        <owl:onProperty rdf:resource="jc3iedmBase.owl#maritime-equipment-type-subcategory-code"/>
      </owl:Restriction>
    </rdfs:subClassOf>
    <rdfs:label xml:lang="en">Sonar, ship</rdfs:label>
    <rdfs:comment xml:lang="en">Equipment mounted on a ship that uses acoustic or SOund Navigation And Ranging (SONAR) technology.</rdfs:comment>
  </owl:Class>
  <owl:Class rdf:ID="File_transfer_protocol">
    <rdfs:subClassOf rdf:resource="jc3iedmSubOnt.owl#NETWORK-SERVICE-Data_transfer"/>
    <rdfs:subClassOf>
      <owl:Restriction>
        <owl:hasValue xml:lang="en">FTP</owl:hasValue>
        <owl:onProperty rdf:resource="jc3iedmBase.owl#network-service-subcategory-code"/>
      </owl:Restriction>
    </rdfs:subClassOf>
    <rdfs:label xml:lang="en">File transfer protocol</rdfs:label>
    <rdfs:comment xml:lang="en">A service that provides the basic elements of file sharing between hosts.</rdfs:comment>
  </owl:Class>
  <owl:Class rdf:ID="Mescaline">
    <rdfs:subClassOf rdf:resource="jc3iedmSubOnt.owl#CONSUMABLE-MATERIEL-TYPE-Drug"/>
    <rdfs:subClassOf>
      <owl:Restriction>
        <owl:hasValue xml:lang="en">MSCLNE</owl:hasValue>
        <owl:onProperty rdf:resource="jc3iedmBase.owl#consumable-materiel-type-subcategory-code"/>
      </owl:Restriction>
    </rdfs:subClassOf>
    <rdfs:label xml:lang="en">Mescaline</rdfs:label>
    <rdfs:comment xml:lang="en">A hallucinogenic alkaloid present in mescal buttons.</rdfs:comment>
  </owl:Class>
  <owl:Class rdf:ID="LORAN-C">
    <rdfs:subClassOf rdf:resource="jc3iedmSubOnt.owl#ELECTRONIC-EQUIPMENT-TYPE-Navigational_aid"/>
    <rdfs:subClassOf>
      <owl:Restriction>
        <owl:hasValue xml:lang="en">LORANC</owl:hasValue>
        <owl:onProperty rdf:resource="jc3iedmBase.owl#electronic-equipment-type-subcategory-code"/>
      </owl:Restriction>
    </rdfs:subClassOf>
    <rdfs:label xml:lang="en">LORAN-C</rdfs:label>
    <rdfs:comment xml:lang="en">No definition provided in ADatP-3 Baseline 13.1 FFIRN/FUD 1200/1.</rdfs:comment>
  </owl:Class>
  <owl:Class rdf:about="#Armoured_infantry_fighting/combat_vehicle">
    <rdfs:subClassOf>
      <owl:Restriction>
        <owl:hasValue xml:lang="en">AIFV</owl:hasValue>
        <owl:onProperty rdf:resource="jc3iedmBase.owl#weapon-type-subcategory-code"/>
      </owl:Restriction>
    </rdfs:subClassOf>
    <rdfs:label xml:lang="en">Armoured infantry fighting/combat vehicle</rdfs:label>
    <rdfs:comment xml:lang="en">An armoured vehicle used for transporting an infantry team and able to support it by the use of weapons.</rdfs:comment>
  </owl:Class>
  <owl:Class rdf:about="#Rations,_combat">
    <rdfs:subClassOf rdf:resource="jc3iedmSubOnt.owl#CONSUMABLE-MATERIEL-TYPE-Food"/>
    <rdfs:subClassOf>
      <owl:Restriction>
        <owl:hasValue xml:lang="en">RATCO</owl:hasValue>
        <owl:onProperty rdf:resource="jc3iedmBase.owl#consumable-materiel-type-subcategory-code"/>
      </owl:Restriction>
    </rdfs:subClassOf>
    <rdfs:label xml:lang="en">Rations, combat</rdfs:label>
    <rdfs:comment xml:lang="en">A package of fixed portions of food allotted for persons.</rdfs:comment>
  </owl:Class>
  <owl:Class rdf:ID="Scrapped">
    <rdfs:subClassOf>
      <owl:Restriction>
        <owl:hasValue xml:lang="en">SCRPPD</owl:hasValue>
        <owl:onProperty rdf:resource="jc3iedmBase.owl#materiel-status-operational-status-qualifier-code"/>
      </owl:Restriction>
    </rdfs:subClassOf>
    <rdfs:label xml:lang="en">Scrapped</rdfs:label>
    <rdfs:comment xml:lang="en">Subjectively judged by the reporting organisation that a specific materiel is dismantled or taken apart into pieces to store or destroy.</rdfs:comment>
  </owl:Class>
  <owl:Class rdf:about="#Sweep,_pressure">
    <rdfs:subClassOf rdf:resource="jc3iedmSubOnt.owl#MARITIME-EQUIPMENT-TYPE-Sweep"/>
    <rdfs:subClassOf>
      <owl:Restriction>
        <owl:hasValue xml:lang="en">SWPPRS</owl:hasValue>
        <owl:onProperty rdf:resource="jc3iedmBase.owl#maritime-equipment-type-subcategory-code"/>
      </owl:Restriction>
    </rdfs:subClassOf>
    <rdfs:label xml:lang="en">Sweep, pressure</rdfs:label>
    <rdfs:comment xml:lang="en">Equipment designed to locate mine by use of pressure differentials.</rdfs:comment>
  </owl:Class>
  <owl:Class rdf:ID="Centreline_drogue">
    <rdfs:subClassOf rdf:resource="jc3iedmSubOnt.owl#MISCELLANEOUS-EQUIPMENT-TYPE-Aircraft_refuelling"/>
    <rdfs:subClassOf>
      <owl:Restriction>
        <owl:hasValue xml:lang="en">CD</owl:hasValue>
        <owl:onProperty rdf:resource="jc3iedmBase.owl#miscellaneous-equipment-type-subcategory-code"/>
      </owl:Restriction>
    </rdfs:subClassOf>
    <rdfs:label xml:lang="en">Centreline drogue</rdfs:label>
    <rdfs:comment xml:lang="en">A component of a refuelling system by which a centreline drogue device can provide fuel on a receiver aircraft.</rdfs:comment>
  </owl:Class>
  <owl:Class rdf:about="#Bathythermograph,_expendable">
    <rdfs:subClassOf rdf:resource="jc3iedmSubOnt.owl#ELECTRONIC-EQUIPMENT-TYPE-Sensor"/>
    <rdfs:subClassOf>
      <owl:Restriction>
        <owl:hasValue xml:lang="en">BTHTGE</owl:hasValue>
        <owl:onProperty rdf:resource="jc3iedmBase.owl#electronic-equipment-type-subcategory-code"/>
      </owl:Restriction>
    </rdfs:subClassOf>
    <rdfs:label xml:lang="en">Bathythermograph, expendable</rdfs:label>
    <rdfs:comment xml:lang="en">An expendable device that records the ocean temperature at various depths. Used to assist in the determination of characteristics of sound propagation and sonar detection.</rdfs:comment>
  </owl:Class>
  <owl:Class rdf:about="#GPS_receiver,_military">
    <rdfs:subClassOf rdf:resource="jc3iedmSubOnt.owl#ELECTRONIC-EQUIPMENT-TYPE-Navigational_aid"/>
    <rdfs:subClassOf>
      <owl:Restriction>
        <owl:hasValue xml:lang="en">GPSMIL</owl:hasValue>
        <owl:onProperty rdf:resource="jc3iedmBase.owl#electronic-equipment-type-subcategory-code"/>
      </owl:Restriction>
    </rdfs:subClassOf>
    <rdfs:label xml:lang="en">GPS receiver, military</rdfs:label>
    <rdfs:comment xml:lang="en">A military electronic system that receives and translates signals from global positioning system satellites.</rdfs:comment>
  </owl:Class>
  <owl:Class rdf:about="#River/stream">
    <rdfs:subClassOf rdf:resource="jc3iedmSubOnt.owl#GEOGRAPHIC-FEATURE-TYPE-Inland_water"/>
    <rdfs:subClassOf rdf:resource="jc3iedmSubOnt.owl#GEOGRAPHIC-FEATURE-Liquid_surface"/>
    <rdfs:subClassOf>
      <owl:Restriction>
        <owl:hasValue xml:lang="en">RVRSTR</owl:hasValue>
        <owl:onProperty rdf:resource="jc3iedmBase.owl#geographic-feature-type-subcategory-code"/>
      </owl:Restriction>
    </rdfs:subClassOf>
    <rdfs:label xml:lang="en">River/stream</rdfs:label>
    <rdfs:comment xml:lang="en">A natural flowing watercourse.</rdfs:comment>
    <rdfs:subClassOf>
      <owl:Restriction>
        <owl:hasValue xml:lang="en">RVRSTR</owl:hasValue>
        <owl:onProperty rdf:resource="jc3iedmBase.owl#geographic-feature-type-subcategory-code"/>
      </owl:Restriction>
    </rdfs:subClassOf>
  </owl:Class>
  <owl:Class rdf:ID="Influence">
    <rdfs:subClassOf>
      <owl:Restriction>
        <owl:hasValue xml:lang="en">INFLUN</owl:hasValue>
        <owl:onProperty rdf:resource="jc3iedmBase.owl#ammunition-type-mine-maritime-firing-code"/>
      </owl:Restriction>
    </rdfs:subClassOf>
    <rdfs:subClassOf rdf:resource="jc3iedmSubOnt.owl#AMMUNITION-TYPE-Mine,_moored"/>
    <rdfs:subClassOf rdf:resource="jc3iedmSubOnt.owl#AMMUNITION-TYPE-Moving_mine,_sea"/>
    <rdfs:subClassOf rdf:resource="jc3iedmSubOnt.owl#AMMUNITION-TYPE-Mine,_shallow_moored"/>
    <rdfs:label xml:lang="en">Influence</rdfs:label>
    <rdfs:subClassOf rdf:resource="jc3iedmSubOnt.owl#AMMUNITION-TYPE-Mine,_deep_moored"/>
    <rdfs:subClassOf rdf:resource="jc3iedmSubOnt.owl#AMMUNITION-TYPE-Sea_mine"/>
    <rdfs:comment xml:lang="en">A (maritime) mine firing mechanism actuated by the effect of a target on some physical condition in the vicinity of the mine or on radiations emanating from the mine.</rdfs:comment>
    <rdfs:subClassOf rdf:resource="jc3iedmSubOnt.owl#AMMUNITION-TYPE-Mine,_seabed_-_explosive_charge_500kg_or_greater"/>
    <rdfs:subClassOf rdf:resource="jc3iedmSubOnt.owl#AMMUNITION-TYPE-Mine,_maritime,_moving"/>
    <rdfs:subClassOf rdf:resource="jc3iedmSubOnt.owl#AMMUNITION-TYPE-Mine,_not_otherwise_specified"/>
    <rdfs:subClassOf rdf:resource="jc3iedmSubOnt.owl#AMMUNITION-TYPE-Mine,_seabed_-_explosive_charge_less_than_500kg"/>
    <rdfs:subClassOf>
      <owl:Restriction>
        <owl:hasValue xml:lang="en">INFLUN</owl:hasValue>
        <owl:onProperty rdf:resource="jc3iedmBase.owl#ammunition-type-mine-maritime-firing-code"/>
      </owl:Restriction>
    </rdfs:subClassOf>
    <rdfs:subClassOf rdf:resource="jc3iedmSubOnt.owl#AMMUNITION-TYPE-Seabed_mine"/>
    <rdfs:subClassOf rdf:resource="jc3iedmSubOnt.owl#AMMUNITION-TYPE-Mine,_not_known"/>
  </owl:Class>
  <owl:Class rdf:ID="Classic_wizard">
    <rdfs:subClassOf>
      <owl:Restriction>
        <owl:hasValue xml:lang="en">CLSWZD</owl:hasValue>
        <owl:onProperty rdf:resource="jc3iedmBase.owl#electronic-equipment-type-subcategory-code"/>
      </owl:Restriction>
    </rdfs:subClassOf>
    <rdfs:label xml:lang="en">Classic wizard</rdfs:label>
    <rdfs:comment xml:lang="en">A High Frequency Direction Finding ocean surveillance system.</rdfs:comment>
  </owl:Class>
  <owl:Class rdf:about="#Staff/stave">
    <rdfs:subClassOf>
      <owl:Restriction>
        <owl:hasValue xml:lang="en">STAFF</owl:hasValue>
        <owl:onProperty rdf:resource="jc3iedmBase.owl#maritime-equipment-type-subcategory-code"/>
      </owl:Restriction>
    </rdfs:subClassOf>
    <rdfs:label xml:lang="en">Staff/stave</rdfs:label>
    <rdfs:comment xml:lang="en">A part of the buoy equipment.</rdfs:comment>
  </owl:Class>
  <owl:Class rdf:ID="Peat">
    <rdfs:subClassOf rdf:resource="jc3iedmSubOnt.owl#CONSUMABLE-MATERIEL-TYPE-Fuel"/>
    <rdfs:subClassOf>
      <owl:Restriction>
        <owl:hasValue xml:lang="en">PEAT</owl:hasValue>
        <owl:onProperty rdf:resource="jc3iedmBase.owl#consumable-materiel-type-subcategory-code"/>
      </owl:Restriction>
    </rdfs:subClassOf>
    <rdfs:label xml:lang="en">Peat</rdfs:label>
    <rdfs:comment xml:lang="en">Dried bog or swamp matter used for fuel.</rdfs:comment>
  </owl:Class>
  <owl:Class rdf:about="#Sonar,_critical_angle_towed_array">
    <rdfs:subClassOf rdf:resource="jc3iedmSubOnt.owl#MARITIME-EQUIPMENT-TYPE-Sonar,_maritime"/>
    <rdfs:subClassOf>
      <owl:Restriction>
        <owl:hasValue xml:lang="en">SONRCR</owl:hasValue>
        <owl:onProperty rdf:resource="jc3iedmBase.owl#maritime-equipment-type-subcategory-code"/>
      </owl:Restriction>
    </rdfs:subClassOf>
    <rdfs:label xml:lang="en">Sonar, critical angle towed array</rdfs:label>
    <rdfs:comment xml:lang="en">No definition provided in ADatP-3 Baseline 13.1 FFIRN/FUD 1434/1.</rdfs:comment>
  </owl:Class>
  <owl:Class rdf:about="#Rations,_fresh">
    <rdfs:subClassOf rdf:resource="jc3iedmSubOnt.owl#CONSUMABLE-MATERIEL-TYPE-Food"/>
    <rdfs:subClassOf>
      <owl:Restriction>
        <owl:hasValue xml:lang="en">RATFR</owl:hasValue>
        <owl:onProperty rdf:resource="jc3iedmBase.owl#consumable-materiel-type-subcategory-code"/>
      </owl:Restriction>
    </rdfs:subClassOf>
    <rdfs:label xml:lang="en">Rations, fresh</rdfs:label>
    <rdfs:comment xml:lang="en">Fresh food allotted for persons.</rdfs:comment>
  </owl:Class>
  <owl:Class rdf:about="#Anti-tank_grenade_launcher,_medium">
    <rdfs:subClassOf rdf:resource="jc3iedmSubOnt.owl#WEAPON-TYPE-Anti-tank"/>
    <rdfs:subClassOf>
      <owl:Restriction>
        <owl:hasValue xml:lang="en">ATGRLM</owl:hasValue>
        <owl:onProperty rdf:resource="jc3iedmBase.owl#weapon-type-subcategory-code"/>
      </owl:Restriction>
    </rdfs:subClassOf>
    <rdfs:label xml:lang="en">Anti-tank grenade launcher, medium</rdfs:label>
    <rdfs:comment xml:lang="en">A medium structural device designed to support and hold an anti-tank grenade in position for firing.</rdfs:comment>
  </owl:Class>
  <owl:Class rdf:ID="Soman">
    <rdfs:subClassOf rdf:resource="jc3iedmSubOnt.owl#CHEMICAL-MATERIEL-TYPE-G-agent"/>
    <rdfs:subClassOf rdf:resource="jc3iedmSubOnt.owl#CHEMICAL-MATERIEL-TYPE-Nerve_agent"/>
    <rdfs:subClassOf>
      <owl:Restriction>
        <owl:hasValue xml:lang="en">SOMAN</owl:hasValue>
        <owl:onProperty rdf:resource="jc3iedmBase.owl#chemical-materiel-type-subcategory-code"/>
      </owl:Restriction>
    </rdfs:subClassOf>
    <rdfs:label xml:lang="en">Soman</rdfs:label>
    <rdfs:comment xml:lang="en">A colourless liquid use as a nerve gas. Chemically, is fluoromethylpinacolyloxyphosphine oxide.</rdfs:comment>
    <rdfs:subClassOf>
      <owl:Restriction>
        <owl:hasValue xml:lang="en">SOMAN</owl:hasValue>
        <owl:onProperty rdf:resource="jc3iedmBase.owl#chemical-materiel-type-subcategory-code"/>
      </owl:Restriction>
    </rdfs:subClassOf>
  </owl:Class>
  <owl:Class rdf:about="#Air-defence_missile_launcher,_short_range">
    <rdfs:subClassOf rdf:resource="jc3iedmSubOnt.owl#WEAPON-TYPE-Air-defence"/>
    <rdfs:subClassOf rdf:resource="jc3iedmSubOnt.owl#WEAPON-TYPE-Missile_system"/>
    <rdfs:subClassOf>
      <owl:Restriction>
        <owl:hasValue xml:lang="en">ADMLSR</owl:hasValue>
        <owl:onProperty rdf:resource="jc3iedmBase.owl#weapon-type-subcategory-code"/>
      </owl:Restriction>
    </rdfs:subClassOf>
    <rdfs:label xml:lang="en">Air-defence missile launcher, short range</rdfs:label>
    <rdfs:comment xml:lang="en">A structural device designed to support and hold a short range air defence missile in position for firing.</rdfs:comment>
    <rdfs:subClassOf>
      <owl:Restriction>
        <owl:hasValue xml:lang="en">ADMLSR</owl:hasValue>
        <owl:onProperty rdf:resource="jc3iedmBase.owl#weapon-type-subcategory-code"/>
      </owl:Restriction>
    </rdfs:subClassOf>
  </owl:Class>
  <owl:Class rdf:about="#Lake/pond">
    <rdfs:subClassOf rdf:resource="jc3iedmSubOnt.owl#GEOGRAPHIC-FEATURE-TYPE-Inland_water"/>
    <rdfs:subClassOf rdf:resource="jc3iedmSubOnt.owl#GEOGRAPHIC-FEATURE-Liquid_surface"/>
    <rdfs:subClassOf>
      <owl:Restriction>
        <owl:hasValue xml:lang="en">LKEPND</owl:hasValue>
        <owl:onProperty rdf:resource="jc3iedmBase.owl#geographic-feature-type-subcategory-code"/>
      </owl:Restriction>
    </rdfs:subClassOf>
    <rdfs:label xml:lang="en">Lake/pond</rdfs:label>
    <rdfs:comment xml:lang="en">A body of water surrounded by land.</rdfs:comment>
    <rdfs:subClassOf>
      <owl:Restriction>
        <owl:hasValue xml:lang="en">LKEPND</owl:hasValue>
        <owl:onProperty rdf:resource="jc3iedmBase.owl#geographic-feature-type-subcategory-code"/>
      </owl:Restriction>
    </rdfs:subClassOf>
  </owl:Class>
  <owl:Class rdf:about="#Radar,_air-surveillance">
    <rdfs:subClassOf rdf:resource="jc3iedmSubOnt.owl#ELECTRONIC-EQUIPMENT-TYPE-Radar"/>
    <rdfs:subClassOf>
      <owl:Restriction>
        <owl:hasValue xml:lang="en">RDRARS</owl:hasValue>
        <owl:onProperty rdf:resource="jc3iedmBase.owl#electronic-equipment-type-subcategory-code"/>
      </owl:Restriction>
    </rdfs:subClassOf>
    <rdfs:label xml:lang="en">Radar, air-surveillance</rdfs:label>
    <rdfs:comment xml:lang="en">The radar used for systematic observation of air space by electronic or other means, primarily for the purpose of identifying and determining the movements of aircraft and missiles, friendly and enemy, in the air space under observation.</rdfs:comment>
  </owl:Class>
  <owl:Class rdf:ID="Autogyro">
    <rdfs:subClassOf rdf:resource="jc3iedmSubOnt.owl#AIRCRAFT-TYPE-Rotary_wing"/>
    <rdfs:subClassOf>
      <owl:Restriction>
        <owl:hasValue xml:lang="en">AUTOGY</owl:hasValue>
        <owl:onProperty rdf:resource="jc3iedmBase.owl#aircraft-type-airframe-design-code"/>
      </owl:Restriction>
    </rdfs:subClassOf>
    <rdfs:label xml:lang="en">Autogyro</rdfs:label>
    <rdfs:comment xml:lang="en">An aircraft powered by a conventional propeller and a freewheeling, horizontal rotor.</rdfs:comment>
  </owl:Class>
  <owl:Class rdf:about="#Air-defence_missile_launcher,_theatre">
    <rdfs:subClassOf rdf:resource="jc3iedmSubOnt.owl#WEAPON-TYPE-Air-defence"/>
    <rdfs:subClassOf rdf:resource="jc3iedmSubOnt.owl#WEAPON-TYPE-Missile_system"/>
    <rdfs:subClassOf>
      <owl:Restriction>
        <owl:hasValue xml:lang="en">ADMLT</owl:hasValue>
        <owl:onProperty rdf:resource="jc3iedmBase.owl#weapon-type-subcategory-code"/>
      </owl:Restriction>
    </rdfs:subClassOf>
    <rdfs:label xml:lang="en">Air-defence missile launcher, theatre</rdfs:label>
    <rdfs:comment xml:lang="en">A structural device designed to support and hold a theatre air defence missile in position for firing.</rdfs:comment>
    <rdfs:subClassOf>
      <owl:Restriction>
        <owl:hasValue xml:lang="en">ADMLT</owl:hasValue>
        <owl:onProperty rdf:resource="jc3iedmBase.owl#weapon-type-subcategory-code"/>
      </owl:Restriction>
    </rdfs:subClassOf>
  </owl:Class>
  <owl:Class rdf:ID="UN_Dangerous_Goods_NUM_1790">
    <rdfs:subClassOf>
      <owl:Restriction>
        <owl:hasValue xml:lang="en">1790</owl:hasValue>
        <owl:onProperty rdf:resource="jc3iedmBase.owl#consumable-materiel-type-united-nations-number-code"/>
      </owl:Restriction>
    </rdfs:subClassOf>
    <rdfs:label xml:lang="en">UN Dangerous Goods # 1790</rdfs:label>
    <rdfs:comment xml:lang="en">Hydrofluoric acid. Includes the agent(s): hydrogen fluoride.</rdfs:comment>
    <rdfs:subClassOf>
      <owl:Restriction>
        <owl:hasValue xml:lang="en">1790</owl:hasValue>
        <owl:onProperty rdf:resource="jc3iedmBase.owl#consumable-materiel-type-united-nations-number-code"/>
      </owl:Restriction>
    </rdfs:subClassOf>
  </owl:Class>
  <owl:Class rdf:about="#Wagon,_cargo,_sliding_sides">
    <rdfs:subClassOf rdf:resource="jc3iedmSubOnt.owl#RAILCAR-TYPE-Rolling_stock"/>
    <rdfs:subClassOf>
      <owl:Restriction>
        <owl:hasValue xml:lang="en">WGNCSS</owl:hasValue>
        <owl:onProperty rdf:resource="jc3iedmBase.owl#railcar-type-subcategory-code"/>
      </owl:Restriction>
    </rdfs:subClassOf>
    <rdfs:label xml:lang="en">Wagon, cargo, sliding sides</rdfs:label>
    <rdfs:comment xml:lang="en">Rolling stock used to move boxed or palletised equipment/stores and closed by means of sliding curtained side panels.</rdfs:comment>
  </owl:Class>
  <owl:Class rdf:ID="Grassland">
    <rdfs:label xml:lang="en">Grassland</rdfs:label>
    <rdfs:comment xml:lang="en">An area composed of uncultured plants which have little or no woody tissue.</rdfs:comment>
  </owl:Class>
  <owl:Class rdf:ID="Low_frequency_analysis_and_recording_system">
    <rdfs:subClassOf rdf:resource="jc3iedmSubOnt.owl#ELECTRONIC-EQUIPMENT-TYPE-Electronic_warfare"/>
    <rdfs:subClassOf>
      <owl:Restriction>
        <owl:hasValue xml:lang="en">LFRARC</owl:hasValue>
        <owl:onProperty rdf:resource="jc3iedmBase.owl#electronic-equipment-type-subcategory-code"/>
      </owl:Restriction>
    </rdfs:subClassOf>
    <rdfs:label xml:lang="en">Low frequency analysis and recording system</rdfs:label>
    <rdfs:comment xml:lang="en">System that detects sounds emitted by submarines using a hydrophone lowered from a passive omnidirectional sonobuoy. Also known as LOFAR system.</rdfs:comment>
  </owl:Class>
  <owl:Class rdf:ID="Prepared_for_execution">
    <rdfs:subClassOf>
      <owl:Restriction>
        <owl:hasValue xml:lang="en">PRPEXE</owl:hasValue>
        <owl:onProperty rdf:resource="jc3iedmBase.owl#facility-status-operational-status-qualifier-code"/>
      </owl:Restriction>
    </rdfs:subClassOf>
    <rdfs:label xml:lang="en">Prepared for execution</rdfs:label>
    <rdfs:comment xml:lang="en">Subjectively judged by the reporting organisation that a FACILITY has been made ready to assume a particular role.</rdfs:comment>
  </owl:Class>
  <owl:Class rdf:about="#Battery,_dry/wet_cell">
    <rdfs:subClassOf rdf:resource="jc3iedmSubOnt.owl#CONSUMABLE-MATERIEL-TYPE-General_supplies"/>
    <rdfs:subClassOf>
      <owl:Restriction>
        <owl:hasValue xml:lang="en">BATDWC</owl:hasValue>
        <owl:onProperty rdf:resource="jc3iedmBase.owl#consumable-materiel-type-subcategory-code"/>
      </owl:Restriction>
    </rdfs:subClassOf>
    <rdfs:label xml:lang="en">Battery, dry/wet cell</rdfs:label>
    <rdfs:comment xml:lang="en">A portable container of a wet/dry cell or cells carrying an electric charge, as a source of current.</rdfs:comment>
  </owl:Class>
  <owl:Class rdf:ID="NATO_standard_fuel_code_F18">
    <rdfs:subClassOf rdf:resource="jc3iedmSubOnt.owl#CONSUMABLE-MATERIEL-TYPE-Fuel"/>
    <rdfs:subClassOf>
      <owl:Restriction>
        <owl:hasValue xml:lang="en">NASF18</owl:hasValue>
        <owl:onProperty rdf:resource="jc3iedmBase.owl#consumable-materiel-type-subcategory-code"/>
      </owl:Restriction>
    </rdfs:subClassOf>
    <rdfs:label xml:lang="en">NATO standard fuel code F18</rdfs:label>
    <rdfs:comment xml:lang="en">Gasoline, Aviation, Grade 100/130.</rdfs:comment>
  </owl:Class>
  <owl:Class rdf:ID="Phosgene">
    <rdfs:subClassOf rdf:resource="jc3iedmSubOnt.owl#CHEMICAL-MATERIEL-TYPE-Blood_agent"/>
    <rdfs:subClassOf>
      <owl:Restriction>
        <owl:hasValue xml:lang="en">PHOSGN</owl:hasValue>
        <owl:onProperty rdf:resource="jc3iedmBase.owl#chemical-materiel-type-subcategory-code"/>
      </owl:Restriction>
    </rdfs:subClassOf>
    <rdfs:label xml:lang="en">Phosgene</rdfs:label>
    <rdfs:comment xml:lang="en">A poisonous gas formerly used in warfare. [COCl2.]</rdfs:comment>
  </owl:Class>
  <owl:Class rdf:ID="Arsine">
    <rdfs:subClassOf rdf:resource="jc3iedmSubOnt.owl#CHEMICAL-MATERIEL-TYPE-Blood_agent"/>
    <rdfs:subClassOf>
      <owl:Restriction>
        <owl:hasValue xml:lang="en">ARSINE</owl:hasValue>
        <owl:onProperty rdf:resource="jc3iedmBase.owl#chemical-materiel-type-subcategory-code"/>
      </owl:Restriction>
    </rdfs:subClassOf>
    <rdfs:label xml:lang="en">Arsine</rdfs:label>
    <rdfs:comment xml:lang="en">A poisonous gas made by the reaction of some arsenic compounds with acids. [AsH3.]</rdfs:comment>
  </owl:Class>
  <owl:Class rdf:ID="Link_11B">
    <rdfs:subClassOf rdf:resource="jc3iedmSubOnt.owl#NETWORK-SERVICE-Tactical_data_link"/>
    <rdfs:subClassOf>
      <owl:Restriction>
        <owl:hasValue xml:lang="en">LNK11B</owl:hasValue>
        <owl:onProperty rdf:resource="jc3iedmBase.owl#network-service-subcategory-code"/>
      </owl:Restriction>
    </rdfs:subClassOf>
    <rdfs:label xml:lang="en">Link 11B</rdfs:label>
    <rdfs:comment xml:lang="en">A service that provides the basic elements for the transmission of specific message of Link 11B.</rdfs:comment>
  </owl:Class>
  <owl:Class rdf:ID="Toran">
    <rdfs:subClassOf rdf:resource="jc3iedmSubOnt.owl#ELECTRONIC-EQUIPMENT-TYPE-Navigational_aid"/>
    <rdfs:subClassOf>
      <owl:Restriction>
        <owl:hasValue xml:lang="en">TORAN</owl:hasValue>
        <owl:onProperty rdf:resource="jc3iedmBase.owl#electronic-equipment-type-subcategory-code"/>
      </owl:Restriction>
    </rdfs:subClassOf>
    <rdfs:label xml:lang="en">Toran</rdfs:label>
    <rdfs:comment xml:lang="en">A hyperbolic radio navigation system offering coverage in the Bay of Biscay and the Western Approaches.</rdfs:comment>
  </owl:Class>
  <owl:Class rdf:ID="Panoramic_view">
    <rdfs:subClassOf rdf:resource="jc3iedmSubOnt.owl#ELECTRONIC-EQUIPMENT-TYPE-Sensor"/>
    <rdfs:subClassOf>
      <owl:Restriction>
        <owl:hasValue xml:lang="en">PANOVW</owl:hasValue>
        <owl:onProperty rdf:resource="jc3iedmBase.owl#electronic-equipment-type-subcategory-code"/>
      </owl:Restriction>
    </rdfs:subClassOf>
    <rdfs:label xml:lang="en">Panoramic view</rdfs:label>
    <rdfs:comment xml:lang="en">No definition provided in ADatP-3 Baseline 13.1 FFIRN/FUD 1677/7.</rdfs:comment>
  </owl:Class>
  <owl:Class rdf:about="#Radar,_counter-mortar_ranging">
    <rdfs:subClassOf rdf:resource="jc3iedmSubOnt.owl#ELECTRONIC-EQUIPMENT-TYPE-Radar"/>
    <rdfs:subClassOf rdf:resource="jc3iedmSubOnt.owl#ELECTRONIC-EQUIPMENT-TYPE-Fire_control"/>
    <rdfs:subClassOf>
      <owl:Restriction>
        <owl:hasValue xml:lang="en">RDRCMR</owl:hasValue>
        <owl:onProperty rdf:resource="jc3iedmBase.owl#electronic-equipment-type-subcategory-code"/>
      </owl:Restriction>
    </rdfs:subClassOf>
    <rdfs:label xml:lang="en">Radar, counter-mortar ranging</rdfs:label>
    <rdfs:comment xml:lang="en">Mortar locating radar capable of locating mortars.</rdfs:comment>
    <rdfs:subClassOf>
      <owl:Restriction>
        <owl:hasValue xml:lang="en">RDRCMR</owl:hasValue>
        <owl:onProperty rdf:resource="jc3iedmBase.owl#electronic-equipment-type-subcategory-code"/>
      </owl:Restriction>
    </rdfs:subClassOf>
  </owl:Class>
  <owl:Class rdf:ID="Multiple_rocket_launcher">
    <rdfs:subClassOf rdf:resource="jc3iedmSubOnt.owl#WEAPON-TYPE-Rocket_artillery"/>
    <rdfs:subClassOf>
      <owl:Restriction>
        <owl:hasValue xml:lang="en">MLRS</owl:hasValue>
        <owl:onProperty rdf:resource="jc3iedmBase.owl#weapon-type-subcategory-code"/>
      </owl:Restriction>
    </rdfs:subClassOf>
    <rdfs:label xml:lang="en">Multiple rocket launcher</rdfs:label>
    <rdfs:comment xml:lang="en">A structural device designed to support and hold multiple rockets in position for firing.</rdfs:comment>
  </owl:Class>
  <owl:Class rdf:ID="River_bank">
    <rdfs:subClassOf rdf:resource="jc3iedmSubOnt.owl#GEOGRAPHIC-FEATURE-TYPE-Inland_water"/>
    <rdfs:subClassOf rdf:resource="jc3iedmSubOnt.owl#GEOGRAPHIC-FEATURE-Solid_surface"/>
    <rdfs:subClassOf>
      <owl:Restriction>
        <owl:hasValue xml:lang="en">RVRBNK</owl:hasValue>
        <owl:onProperty rdf:resource="jc3iedmBase.owl#geographic-feature-type-subcategory-code"/>
      </owl:Restriction>
    </rdfs:subClassOf>
    <rdfs:label xml:lang="en">River bank</rdfs:label>
    <rdfs:comment xml:lang="en">The limit line between the water area of a river and the area of land.</rdfs:comment>
    <rdfs:subClassOf>
      <owl:Restriction>
        <owl:hasValue xml:lang="en">RVRBNK</owl:hasValue>
        <owl:onProperty rdf:resource="jc3iedmBase.owl#geographic-feature-type-subcategory-code"/>
      </owl:Restriction>
    </rdfs:subClassOf>
  </owl:Class>
  <owl:Class rdf:ID="Transit_receiver">
    <rdfs:subClassOf rdf:resource="jc3iedmSubOnt.owl#ELECTRONIC-EQUIPMENT-TYPE-Communication"/>
    <rdfs:subClassOf>
      <owl:Restriction>
        <owl:hasValue xml:lang="en">TRNRCV</owl:hasValue>
        <owl:onProperty rdf:resource="jc3iedmBase.owl#electronic-equipment-type-subcategory-code"/>
      </owl:Restriction>
    </rdfs:subClassOf>
    <rdfs:label xml:lang="en">Transit receiver</rdfs:label>
    <rdfs:comment xml:lang="en">A satellite based navigation system.</rdfs:comment>
  </owl:Class>
  <owl:Class rdf:ID="Undermined_land">
    <rdfs:subClassOf rdf:resource="jc3iedmSubOnt.owl#GEOGRAPHIC-FEATURE-Solid_surface"/>
    <rdfs:subClassOf rdf:resource="jc3iedmSubOnt.owl#GEOGRAPHIC-FEATURE-TYPE-Landform"/>
    <rdfs:subClassOf>
      <owl:Restriction>
        <owl:hasValue xml:lang="en">UNDRML</owl:hasValue>
        <owl:onProperty rdf:resource="jc3iedmBase.owl#geographic-feature-type-subcategory-code"/>
      </owl:Restriction>
    </rdfs:subClassOf>
    <rdfs:label xml:lang="en">Undermined land</rdfs:label>
    <rdfs:comment xml:lang="en">Area undermined through mining activities that has already partly subsided or that is in the process of subsiding.</rdfs:comment>
    <rdfs:subClassOf>
      <owl:Restriction>
        <owl:hasValue xml:lang="en">UNDRML</owl:hasValue>
        <owl:onProperty rdf:resource="jc3iedmBase.owl#geographic-feature-type-subcategory-code"/>
      </owl:Restriction>
    </rdfs:subClassOf>
  </owl:Class>
  <owl:Class rdf:ID="IFF_mode_C">
    <rdfs:subClassOf rdf:resource="jc3iedmSubOnt.owl#NETWORK-SERVICE-Identification_friend_or_foe"/>
    <rdfs:subClassOf>
      <owl:Restriction>
        <owl:hasValue xml:lang="en">IFFMC</owl:hasValue>
        <owl:onProperty rdf:resource="jc3iedmBase.owl#network-service-subcategory-code"/>
      </owl:Restriction>
    </rdfs:subClassOf>
    <rdfs:label xml:lang="en">IFF mode C</rdfs:label>
    <rdfs:comment xml:lang="en">A service that provides the data for IFF mode C.</rdfs:comment>
  </owl:Class>
  <owl:Class rdf:ID="Air-defence_automatic_cannon">
    <rdfs:subClassOf rdf:resource="jc3iedmSubOnt.owl#WEAPON-TYPE-Air-defence"/>
    <rdfs:subClassOf>
      <owl:Restriction>
        <owl:hasValue xml:lang="en">ADCAN</owl:hasValue>
        <owl:onProperty rdf:resource="jc3iedmBase.owl#weapon-type-subcategory-code"/>
      </owl:Restriction>
    </rdfs:subClassOf>
    <rdfs:label xml:lang="en">Air-defence automatic cannon</rdfs:label>
    <rdfs:comment xml:lang="en">An automatic cannon, usually linked to remote sensors, used primarily in the role of air defence.</rdfs:comment>
  </owl:Class>
  <owl:Class rdf:ID="UN_Dangerous_Goods_NUM_1834">
    <rdfs:subClassOf>
      <owl:Restriction>
        <owl:hasValue xml:lang="en">1834</owl:hasValue>
        <owl:onProperty rdf:resource="jc3iedmBase.owl#consumable-materiel-type-united-nations-number-code"/>
      </owl:Restriction>
    </rdfs:subClassOf>
    <rdfs:label xml:lang="en">UN Dangerous Goods # 1834</rdfs:label>
    <rdfs:comment xml:lang="en">Sulphuryl chloride. Includes the agent(s): sulphuryl chloride.</rdfs:comment>
    <rdfs:subClassOf>
      <owl:Restriction>
        <owl:hasValue xml:lang="en">1834</owl:hasValue>
        <owl:onProperty rdf:resource="jc3iedmBase.owl#consumable-materiel-type-united-nations-number-code"/>
      </owl:Restriction>
    </rdfs:subClassOf>
  </owl:Class>
  <owl:Class rdf:about="#Data_link,_optical">
    <rdfs:subClassOf rdf:resource="jc3iedmSubOnt.owl#ELECTRONIC-EQUIPMENT-TYPE-Communication"/>
    <rdfs:subClassOf>
      <owl:Restriction>
        <owl:hasValue xml:lang="en">DTLOPT</owl:hasValue>
        <owl:onProperty rdf:resource="jc3iedmBase.owl#electronic-equipment-type-subcategory-code"/>
      </owl:Restriction>
    </rdfs:subClassOf>
    <rdfs:label xml:lang="en">Data link, optical</rdfs:label>
    <rdfs:comment xml:lang="en">Those parts of two data terminal equipments that are controlled by a protocol along with the interconnecting optical data circuit, that together enable data transfer.</rdfs:comment>
  </owl:Class>
  <owl:Class rdf:about="#Anti-tank_rocket_launcher,_light">
    <rdfs:subClassOf rdf:resource="jc3iedmSubOnt.owl#WEAPON-TYPE-Anti-tank"/>
    <rdfs:subClassOf>
      <owl:Restriction>
        <owl:hasValue xml:lang="en">ATRLLT</owl:hasValue>
        <owl:onProperty rdf:resource="jc3iedmBase.owl#weapon-type-subcategory-code"/>
      </owl:Restriction>
    </rdfs:subClassOf>
    <rdfs:label xml:lang="en">Anti-tank rocket launcher, light</rdfs:label>
    <rdfs:comment xml:lang="en">A light structural device designed to support and hold an anti-tank rocket in position for firing.</rdfs:comment>
  </owl:Class>
  <owl:Class rdf:ID="Heroin">
    <rdfs:subClassOf rdf:resource="jc3iedmSubOnt.owl#CONSUMABLE-MATERIEL-TYPE-Drug"/>
    <rdfs:subClassOf>
      <owl:Restriction>
        <owl:hasValue xml:lang="en">HEROIN</owl:hasValue>
        <owl:onProperty rdf:resource="jc3iedmBase.owl#consumable-materiel-type-subcategory-code"/>
      </owl:Restriction>
    </rdfs:subClassOf>
    <rdfs:label xml:lang="en">Heroin</rdfs:label>
    <rdfs:comment xml:lang="en">A highly addictive crystalline analgesic drug derived from morphine, often used as a narcotic.</rdfs:comment>
  </owl:Class>
  <owl:Class rdf:ID="IFF_mode_2">
    <rdfs:subClassOf rdf:resource="jc3iedmSubOnt.owl#NETWORK-SERVICE-Identification_friend_or_foe"/>
    <rdfs:subClassOf>
      <owl:Restriction>
        <owl:hasValue xml:lang="en">IFFM2</owl:hasValue>
        <owl:onProperty rdf:resource="jc3iedmBase.owl#network-service-subcategory-code"/>
      </owl:Restriction>
    </rdfs:subClassOf>
    <rdfs:label xml:lang="en">IFF mode 2</rdfs:label>
    <rdfs:comment xml:lang="en">A service that provides the data for IFF mode 2.</rdfs:comment>
  </owl:Class>
  <owl:Class rdf:ID="Moraine">
    <rdfs:subClassOf rdf:resource="jc3iedmSubOnt.owl#GEOGRAPHIC-FEATURE-Solid_surface"/>
    <rdfs:subClassOf rdf:resource="jc3iedmSubOnt.owl#GEOGRAPHIC-FEATURE-TYPE-Landform"/>
    <rdfs:subClassOf>
      <owl:Restriction>
        <owl:hasValue xml:lang="en">MORANE</owl:hasValue>
        <owl:onProperty rdf:resource="jc3iedmBase.owl#geographic-feature-type-subcategory-code"/>
      </owl:Restriction>
    </rdfs:subClassOf>
    <rdfs:label xml:lang="en">Moraine</rdfs:label>
    <rdfs:comment xml:lang="en">An accumulation of soil and stone debris deposited by a glacier.</rdfs:comment>
    <rdfs:subClassOf>
      <owl:Restriction>
        <owl:hasValue xml:lang="en">MORANE</owl:hasValue>
        <owl:onProperty rdf:resource="jc3iedmBase.owl#geographic-feature-type-subcategory-code"/>
      </owl:Restriction>
    </rdfs:subClassOf>
  </owl:Class>
  <owl:Class rdf:ID="Inland_shoreline">
    <rdfs:subClassOf rdf:resource="jc3iedmSubOnt.owl#GEOGRAPHIC-FEATURE-TYPE-Inland_water"/>
    <rdfs:subClassOf rdf:resource="jc3iedmSubOnt.owl#GEOGRAPHIC-FEATURE-Solid_surface"/>
    <rdfs:subClassOf>
      <owl:Restriction>
        <owl:hasValue xml:lang="en">INLNDS</owl:hasValue>
        <owl:onProperty rdf:resource="jc3iedmBase.owl#geographic-feature-type-subcategory-code"/>
      </owl:Restriction>
    </rdfs:subClassOf>
    <rdfs:label xml:lang="en">Inland shoreline</rdfs:label>
    <rdfs:comment xml:lang="en">The land-water boundary for all inland hydrographic features having shorelines, Lake /Pond, or Island.</rdfs:comment>
    <rdfs:subClassOf>
      <owl:Restriction>
        <owl:hasValue xml:lang="en">INLNDS</owl:hasValue>
        <owl:onProperty rdf:resource="jc3iedmBase.owl#geographic-feature-type-subcategory-code"/>
      </owl:Restriction>
    </rdfs:subClassOf>
  </owl:Class>
  <owl:Class rdf:ID="Tabun">
    <rdfs:subClassOf rdf:resource="jc3iedmSubOnt.owl#CHEMICAL-MATERIEL-TYPE-G-agent"/>
    <rdfs:subClassOf rdf:resource="jc3iedmSubOnt.owl#CHEMICAL-MATERIEL-TYPE-Nerve_agent"/>
    <rdfs:subClassOf>
      <owl:Restriction>
        <owl:hasValue xml:lang="en">TABUN</owl:hasValue>
        <owl:onProperty rdf:resource="jc3iedmBase.owl#chemical-materiel-type-subcategory-code"/>
      </owl:Restriction>
    </rdfs:subClassOf>
    <rdfs:label xml:lang="en">Tabun</rdfs:label>
    <rdfs:comment xml:lang="en">An organophosphorus nerve gas.</rdfs:comment>
    <rdfs:subClassOf>
      <owl:Restriction>
        <owl:hasValue xml:lang="en">TABUN</owl:hasValue>
        <owl:onProperty rdf:resource="jc3iedmBase.owl#chemical-materiel-type-subcategory-code"/>
      </owl:Restriction>
    </rdfs:subClassOf>
  </owl:Class>
  <owl:Class rdf:ID="UN_Dangerous_Goods_NUM_1897">
    <rdfs:subClassOf>
      <owl:Restriction>
        <owl:hasValue xml:lang="en">1897</owl:hasValue>
        <owl:onProperty rdf:resource="jc3iedmBase.owl#consumable-materiel-type-united-nations-number-code"/>
      </owl:Restriction>
    </rdfs:subClassOf>
    <rdfs:label xml:lang="en">UN Dangerous Goods # 1897</rdfs:label>
    <rdfs:comment xml:lang="en">Tetrachloroethylene. Includes the agent(s): tetrachloroethylene.</rdfs:comment>
    <rdfs:subClassOf>
      <owl:Restriction>
        <owl:hasValue xml:lang="en">1897</owl:hasValue>
        <owl:onProperty rdf:resource="jc3iedmBase.owl#consumable-materiel-type-united-nations-number-code"/>
      </owl:Restriction>
    </rdfs:subClassOf>
  </owl:Class>
  <owl:Class rdf:ID="UN_Dangerous_Goods_NUM_1556">
    <rdfs:subClassOf>
      <owl:Restriction>
        <owl:hasValue xml:lang="en">1556</owl:hasValue>
        <owl:onProperty rdf:resource="jc3iedmBase.owl#consumable-materiel-type-united-nations-number-code"/>
      </owl:Restriction>
    </rdfs:subClassOf>
    <rdfs:label xml:lang="en">UN Dangerous Goods # 1556</rdfs:label>
    <rdfs:comment xml:lang="en">Arsenic compound, liquid, N.O.S., inorganic, including: Arsenates, N.O.S., Arsenites, N.O.S.; and Arsenic sulphides, N.O.S. Includes the agent(s): Phenyldichloroarsine; Methyldichloroarsine.</rdfs:comment>
    <rdfs:subClassOf>
      <owl:Restriction>
        <owl:hasValue xml:lang="en">1556</owl:hasValue>
        <owl:onProperty rdf:resource="jc3iedmBase.owl#consumable-materiel-type-united-nations-number-code"/>
      </owl:Restriction>
    </rdfs:subClassOf>
  </owl:Class>
  <owl:Class rdf:about="#Marker,_middle">
    <rdfs:subClassOf rdf:resource="jc3iedmSubOnt.owl#ELECTRONIC-EQUIPMENT-TYPE-Navigational_aid"/>
    <rdfs:subClassOf>
      <owl:Restriction>
        <owl:hasValue xml:lang="en">MRKRMD</owl:hasValue>
        <owl:onProperty rdf:resource="jc3iedmBase.owl#electronic-equipment-type-subcategory-code"/>
      </owl:Restriction>
    </rdfs:subClassOf>
    <rdfs:label xml:lang="en">Marker, middle</rdfs:label>
    <rdfs:comment xml:lang="en">A marker beacon that defines a point along the glide path of an Instrument Landing System (ILS) normally located at or near the point of decision height (ILS Category I).</rdfs:comment>
  </owl:Class>
  <owl:Class rdf:about="#Buoy,_position_number">
    <rdfs:subClassOf rdf:resource="jc3iedmSubOnt.owl#MARITIME-EQUIPMENT-TYPE-Buoy"/>
    <rdfs:subClassOf>
      <owl:Restriction>
        <owl:hasValue xml:lang="en">BUOYPS</owl:hasValue>
        <owl:onProperty rdf:resource="jc3iedmBase.owl#maritime-equipment-type-subcategory-code"/>
      </owl:Restriction>
    </rdfs:subClassOf>
    <rdfs:label xml:lang="en">Buoy, position number</rdfs:label>
    <rdfs:comment xml:lang="en">A marked floating object fastened in a particular place to point out the position of a specific hazard or obstacle or act as a marker for some specific reason.</rdfs:comment>
  </owl:Class>
  <owl:Class rdf:ID="UN_Dangerous_Goods_NUM_1693">
    <rdfs:subClassOf>
      <owl:Restriction>
        <owl:hasValue xml:lang="en">1693</owl:hasValue>
        <owl:onProperty rdf:resource="jc3iedmBase.owl#consumable-materiel-type-united-nations-number-code"/>
      </owl:Restriction>
    </rdfs:subClassOf>
    <rdfs:label xml:lang="en">UN Dangerous Goods # 1693</rdfs:label>
    <rdfs:comment xml:lang="en">Tear gas substance, liquid or solid, N.O.S. Includes the agent(s): 2-Chlorobenzalmalononitrile (CS) (listed as 2810 in ERG).</rdfs:comment>
    <rdfs:subClassOf>
      <owl:Restriction>
        <owl:hasValue xml:lang="en">1693</owl:hasValue>
        <owl:onProperty rdf:resource="jc3iedmBase.owl#consumable-materiel-type-united-nations-number-code"/>
      </owl:Restriction>
    </rdfs:subClassOf>
  </owl:Class>
  <owl:Class rdf:ID="Crack">
    <rdfs:subClassOf rdf:resource="jc3iedmSubOnt.owl#CONSUMABLE-MATERIEL-TYPE-Drug"/>
    <rdfs:subClassOf>
      <owl:Restriction>
        <owl:hasValue xml:lang="en">CRACK</owl:hasValue>
        <owl:onProperty rdf:resource="jc3iedmBase.owl#consumable-materiel-type-subcategory-code"/>
      </owl:Restriction>
    </rdfs:subClassOf>
    <rdfs:label xml:lang="en">Crack</rdfs:label>
    <rdfs:comment xml:lang="en">A potent hard crystalline form of cocaine broken into small pieces and inhaled or smoked for its stimulating effect.</rdfs:comment>
  </owl:Class>
  <owl:Class rdf:ID="Mountain_pass">
    <rdfs:subClassOf rdf:resource="jc3iedmSubOnt.owl#GEOGRAPHIC-FEATURE-Solid_surface"/>
    <rdfs:subClassOf rdf:resource="jc3iedmSubOnt.owl#GEOGRAPHIC-FEATURE-TYPE-Landform"/>
    <rdfs:subClassOf>
      <owl:Restriction>
        <owl:hasValue xml:lang="en">MNTPSS</owl:hasValue>
        <owl:onProperty rdf:resource="jc3iedmBase.owl#geographic-feature-type-subcategory-code"/>
      </owl:Restriction>
    </rdfs:subClassOf>
    <rdfs:label xml:lang="en">Mountain pass</rdfs:label>
    <rdfs:comment xml:lang="en">A natural route through a low place in a mountain range.</rdfs:comment>
    <rdfs:subClassOf>
      <owl:Restriction>
        <owl:hasValue xml:lang="en">MNTPSS</owl:hasValue>
        <owl:onProperty rdf:resource="jc3iedmBase.owl#geographic-feature-type-subcategory-code"/>
      </owl:Restriction>
    </rdfs:subClassOf>
  </owl:Class>
  <owl:Class rdf:ID="Hashish_oil">
    <rdfs:subClassOf rdf:resource="jc3iedmSubOnt.owl#CONSUMABLE-MATERIEL-TYPE-Drug"/>
    <rdfs:subClassOf>
      <owl:Restriction>
        <owl:hasValue xml:lang="en">HASOIL</owl:hasValue>
        <owl:onProperty rdf:resource="jc3iedmBase.owl#consumable-materiel-type-subcategory-code"/>
      </owl:Restriction>
    </rdfs:subClassOf>
    <rdfs:label xml:lang="en">Hashish oil</rdfs:label>
    <rdfs:comment xml:lang="en">A dark brown to black oily substance possessing a THC content averaging 20 percent.</rdfs:comment>
  </owl:Class>
  <owl:Class rdf:ID="Psilocybin">
    <rdfs:subClassOf rdf:resource="jc3iedmSubOnt.owl#CONSUMABLE-MATERIEL-TYPE-Drug"/>
    <rdfs:subClassOf>
      <owl:Restriction>
        <owl:hasValue xml:lang="en">PSLCYB</owl:hasValue>
        <owl:onProperty rdf:resource="jc3iedmBase.owl#consumable-materiel-type-subcategory-code"/>
      </owl:Restriction>
    </rdfs:subClassOf>
    <rdfs:label xml:lang="en">Psilocybin</rdfs:label>
    <rdfs:comment xml:lang="en">A hallucinogenic alkaloid found in toadstools of the genus Psilocybe.</rdfs:comment>
  </owl:Class>
  <owl:Class rdf:ID="Anti-tank_grenade_launcher">
    <rdfs:subClassOf rdf:resource="jc3iedmSubOnt.owl#WEAPON-TYPE-Anti-tank"/>
    <rdfs:subClassOf>
      <owl:Restriction>
        <owl:hasValue xml:lang="en">ATGRLC</owl:hasValue>
        <owl:onProperty rdf:resource="jc3iedmBase.owl#weapon-type-subcategory-code"/>
      </owl:Restriction>
    </rdfs:subClassOf>
    <rdfs:label xml:lang="en">Anti-tank grenade launcher</rdfs:label>
    <rdfs:comment xml:lang="en">A structural device designed to support and hold an anti-tank grenade in position for firing.</rdfs:comment>
  </owl:Class>
  <owl:Class rdf:ID="Telegraph">
    <rdfs:subClassOf rdf:resource="jc3iedmSubOnt.owl#ELECTRONIC-EQUIPMENT-TYPE-Communication"/>
    <rdfs:subClassOf>
      <owl:Restriction>
        <owl:hasValue xml:lang="en">TELGPH</owl:hasValue>
        <owl:onProperty rdf:resource="jc3iedmBase.owl#electronic-equipment-type-subcategory-code"/>
      </owl:Restriction>
    </rdfs:subClassOf>
    <rdfs:label xml:lang="en">Telegraph</rdfs:label>
    <rdfs:comment xml:lang="en">Pertaining to or designating equipments connected to the end of a subscribers line or telegraph circuit, which can either establish or receive calls, or store and retransmit signals, and which can be uniquely identified.</rdfs:comment>
  </owl:Class>
  <owl:Class rdf:ID="Flame-thrower">
    <rdfs:subClassOf rdf:resource="jc3iedmSubOnt.owl#WEAPON-TYPE-Small_arms"/>
    <rdfs:subClassOf>
      <owl:Restriction>
        <owl:hasValue xml:lang="en">FLAMET</owl:hasValue>
        <owl:onProperty rdf:resource="jc3iedmBase.owl#weapon-type-subcategory-code"/>
      </owl:Restriction>
    </rdfs:subClassOf>
    <rdfs:label xml:lang="en">Flame-thrower</rdfs:label>
    <rdfs:comment xml:lang="en">A weapon that projects incendiary fuel and has provision for ignition of this fuel.</rdfs:comment>
  </owl:Class>
  <owl:Class rdf:ID="Satellite">
    <rdfs:subClassOf rdf:resource="jc3iedmSubOnt.owl#AIRCRAFT-TYPE-Space_vehicle"/>
    <rdfs:subClassOf>
      <owl:Restriction>
        <owl:hasValue xml:lang="en">SATEL</owl:hasValue>
        <owl:onProperty rdf:resource="jc3iedmBase.owl#aircraft-type-airframe-design-code"/>
      </owl:Restriction>
    </rdfs:subClassOf>
    <rdfs:label xml:lang="en">Satellite</rdfs:label>
    <rdfs:comment xml:lang="en">A space vehicle that orbits the earth.</rdfs:comment>
  </owl:Class>
  <owl:Class rdf:about="#Sonar,_depressed_angle_towed_array">
    <rdfs:subClassOf rdf:resource="jc3iedmSubOnt.owl#MARITIME-EQUIPMENT-TYPE-Sonar,_maritime"/>
    <rdfs:subClassOf>
      <owl:Restriction>
        <owl:hasValue xml:lang="en">SONRDT</owl:hasValue>
        <owl:onProperty rdf:resource="jc3iedmBase.owl#maritime-equipment-type-subcategory-code"/>
      </owl:Restriction>
    </rdfs:subClassOf>
    <rdfs:label xml:lang="en">Sonar, depressed angle towed array</rdfs:label>
    <rdfs:comment xml:lang="en">No definition provided in ADatP-3 Baseline 13.1 FFIRN/FUD 1434/1.</rdfs:comment>
  </owl:Class>
  <owl:Class rdf:ID="UN_Dangerous_Goods_NUM_2480">
    <rdfs:subClassOf>
      <owl:Restriction>
        <owl:hasValue xml:lang="en">2480</owl:hasValue>
        <owl:onProperty rdf:resource="jc3iedmBase.owl#consumable-materiel-type-united-nations-number-code"/>
      </owl:Restriction>
    </rdfs:subClassOf>
    <rdfs:label xml:lang="en">UN Dangerous Goods # 2480</rdfs:label>
    <rdfs:comment xml:lang="en">Methyl isocyanate. Includes the agent(s): methyl isocyanate.</rdfs:comment>
    <rdfs:subClassOf>
      <owl:Restriction>
        <owl:hasValue xml:lang="en">2480</owl:hasValue>
        <owl:onProperty rdf:resource="jc3iedmBase.owl#consumable-materiel-type-united-nations-number-code"/>
      </owl:Restriction>
    </rdfs:subClassOf>
  </owl:Class>
  <owl:Class rdf:ID="Volcano_dike">
    <rdfs:subClassOf rdf:resource="jc3iedmSubOnt.owl#GEOGRAPHIC-FEATURE-Solid_surface"/>
    <rdfs:subClassOf rdf:resource="jc3iedmSubOnt.owl#GEOGRAPHIC-FEATURE-TYPE-Landform"/>
    <rdfs:subClassOf>
      <owl:Restriction>
        <owl:hasValue xml:lang="en">VLCNOD</owl:hasValue>
        <owl:onProperty rdf:resource="jc3iedmBase.owl#geographic-feature-type-subcategory-code"/>
      </owl:Restriction>
    </rdfs:subClassOf>
    <rdfs:label xml:lang="en">Volcano dike</rdfs:label>
    <rdfs:comment xml:lang="en">A steep ridge of igneous rock.</rdfs:comment>
    <rdfs:subClassOf>
      <owl:Restriction>
        <owl:hasValue xml:lang="en">VLCNOD</owl:hasValue>
        <owl:onProperty rdf:resource="jc3iedmBase.owl#geographic-feature-type-subcategory-code"/>
      </owl:Restriction>
    </rdfs:subClassOf>
  </owl:Class>
  <owl:Class rdf:ID="Beacon">
    <rdfs:subClassOf rdf:resource="jc3iedmSubOnt.owl#ELECTRONIC-EQUIPMENT-TYPE-Navigational_aid"/>
    <rdfs:subClassOf>
      <owl:Restriction>
        <owl:hasValue xml:lang="en">BEACON</owl:hasValue>
        <owl:onProperty rdf:resource="jc3iedmBase.owl#electronic-equipment-type-subcategory-code"/>
      </owl:Restriction>
    </rdfs:subClassOf>
    <rdfs:label xml:lang="en">Beacon</rdfs:label>
    <rdfs:comment xml:lang="en">An electronic source that emits a distinctive or characteristic signal used for the determination of bearings, courses, or locations.</rdfs:comment>
  </owl:Class>
  <owl:Class rdf:ID="UN_Dangerous_Goods_NUM_2329">
    <rdfs:subClassOf>
      <owl:Restriction>
        <owl:hasValue xml:lang="en">2329</owl:hasValue>
        <owl:onProperty rdf:resource="jc3iedmBase.owl#consumable-materiel-type-united-nations-number-code"/>
      </owl:Restriction>
    </rdfs:subClassOf>
    <rdfs:label xml:lang="en">UN Dangerous Goods # 2329</rdfs:label>
    <rdfs:comment xml:lang="en">Trimethyl phosphate. Includes the agent(s): trimethyl phosphite.</rdfs:comment>
    <rdfs:subClassOf>
      <owl:Restriction>
        <owl:hasValue xml:lang="en">2329</owl:hasValue>
        <owl:onProperty rdf:resource="jc3iedmBase.owl#consumable-materiel-type-united-nations-number-code"/>
      </owl:Restriction>
    </rdfs:subClassOf>
  </owl:Class>
  <owl:Class rdf:about="#Mortar,_very_heavy">
    <rdfs:subClassOf rdf:resource="jc3iedmSubOnt.owl#WEAPON-TYPE-Mortar"/>
    <rdfs:subClassOf>
      <owl:Restriction>
        <owl:hasValue xml:lang="en">MRTVHV</owl:hasValue>
        <owl:onProperty rdf:resource="jc3iedmBase.owl#weapon-type-subcategory-code"/>
      </owl:Restriction>
    </rdfs:subClassOf>
    <rdfs:label xml:lang="en">Mortar, very heavy</rdfs:label>
    <rdfs:comment xml:lang="en">An indirect fire weapon, usually with a shorter range than a howitzer, employs a higher angle of fire, and its calibre is 151mm or larger.</rdfs:comment>
  </owl:Class>
  <owl:Class rdf:ID="IFF_mode_1">
    <rdfs:subClassOf rdf:resource="jc3iedmSubOnt.owl#NETWORK-SERVICE-Identification_friend_or_foe"/>
    <rdfs:subClassOf>
      <owl:Restriction>
        <owl:hasValue xml:lang="en">IFFM1</owl:hasValue>
        <owl:onProperty rdf:resource="jc3iedmBase.owl#network-service-subcategory-code"/>
      </owl:Restriction>
    </rdfs:subClassOf>
    <rdfs:label xml:lang="en">IFF mode 1</rdfs:label>
    <rdfs:comment xml:lang="en">A service that provides the data for IFF mode 1.</rdfs:comment>
  </owl:Class>
  <owl:Class rdf:about="#Sweep,_mechanical_snagline">
    <rdfs:subClassOf rdf:resource="jc3iedmSubOnt.owl#MARITIME-EQUIPMENT-TYPE-Sweep"/>
    <rdfs:subClassOf>
      <owl:Restriction>
        <owl:hasValue xml:lang="en">SWPMCS</owl:hasValue>
        <owl:onProperty rdf:resource="jc3iedmBase.owl#maritime-equipment-type-subcategory-code"/>
      </owl:Restriction>
    </rdfs:subClassOf>
    <rdfs:label xml:lang="en">Sweep, mechanical snagline</rdfs:label>
    <rdfs:comment xml:lang="en">Equipment designed to locate mines by use of a wire to catch the snagline of a moored mine.</rdfs:comment>
  </owl:Class>
  <owl:Class rdf:ID="Coastline">
    <rdfs:subClassOf rdf:resource="jc3iedmSubOnt.owl#GEOGRAPHIC-FEATURE-Solid_surface"/>
    <rdfs:subClassOf rdf:resource="jc3iedmSubOnt.owl#GEOGRAPHIC-FEATURE-TYPE-Coastal_hydrography"/>
    <rdfs:subClassOf>
      <owl:Restriction>
        <owl:hasValue xml:lang="en">CSTLNE</owl:hasValue>
        <owl:onProperty rdf:resource="jc3iedmBase.owl#geographic-feature-type-subcategory-code"/>
      </owl:Restriction>
    </rdfs:subClassOf>
    <rdfs:label xml:lang="en">Coastline</rdfs:label>
    <rdfs:comment xml:lang="en">A line generally following the contact between a land mass and a body of water, based on the low water line, and used as a reference for measuring international boundaries such as Territorial Limits or Exclusive Economic Zone (EEZ).</rdfs:comment>
    <rdfs:subClassOf>
      <owl:Restriction>
        <owl:hasValue xml:lang="en">CSTLNE</owl:hasValue>
        <owl:onProperty rdf:resource="jc3iedmBase.owl#geographic-feature-type-subcategory-code"/>
      </owl:Restriction>
    </rdfs:subClassOf>
  </owl:Class>
  <owl:Class rdf:ID="Oasis">
    <rdfs:label xml:lang="en">Oasis</rdfs:label>
    <rdfs:comment xml:lang="en">A small, isolated, fertile or green area in a desert region usually having a spring or well.</rdfs:comment>
  </owl:Class>
  <owl:Class rdf:ID="Optical">
    <rdfs:subClassOf rdf:resource="jc3iedmSubOnt.owl#ELECTRONIC-EQUIPMENT-TYPE-Sensor"/>
    <rdfs:subClassOf>
      <owl:Restriction>
        <owl:hasValue xml:lang="en">OPTICL</owl:hasValue>
        <owl:onProperty rdf:resource="jc3iedmBase.owl#electronic-equipment-type-subcategory-code"/>
      </owl:Restriction>
    </rdfs:subClassOf>
    <rdfs:label xml:lang="en">Optical</rdfs:label>
    <rdfs:comment xml:lang="en">No definition provided in ADatP-3 Baseline 13.1 FFIRN/FUD 1677/7.</rdfs:comment>
  </owl:Class>
  <owl:Class rdf:about="#GPS_receiver,_commercial">
    <rdfs:subClassOf rdf:resource="jc3iedmSubOnt.owl#ELECTRONIC-EQUIPMENT-TYPE-Navigational_aid"/>
    <rdfs:subClassOf>
      <owl:Restriction>
        <owl:hasValue xml:lang="en">GPSCOM</owl:hasValue>
        <owl:onProperty rdf:resource="jc3iedmBase.owl#electronic-equipment-type-subcategory-code"/>
      </owl:Restriction>
    </rdfs:subClassOf>
    <rdfs:label xml:lang="en">GPS receiver, commercial</rdfs:label>
    <rdfs:comment xml:lang="en">A commercial electronic system that receives and translates signals from global positioning system satellites.</rdfs:comment>
  </owl:Class>
  <owl:Class rdf:about="#Rangefinder,_laser">
    <rdfs:subClassOf rdf:resource="jc3iedmSubOnt.owl#ELECTRONIC-EQUIPMENT-TYPE-Sensor"/>
    <rdfs:subClassOf>
      <owl:Restriction>
        <owl:hasValue xml:lang="en">RNGLAS</owl:hasValue>
        <owl:onProperty rdf:resource="jc3iedmBase.owl#electronic-equipment-type-subcategory-code"/>
      </owl:Restriction>
    </rdfs:subClassOf>
    <rdfs:label xml:lang="en">Rangefinder, laser</rdfs:label>
    <rdfs:comment xml:lang="en">A device that uses laser energy for determining the distance from the device to a place or object.</rdfs:comment>
  </owl:Class>
  <owl:Class rdf:about="#Buoy,_master_reference">
    <rdfs:subClassOf rdf:resource="jc3iedmSubOnt.owl#MARITIME-EQUIPMENT-TYPE-Buoy"/>
    <rdfs:subClassOf>
      <owl:Restriction>
        <owl:hasValue xml:lang="en">BUOYMS</owl:hasValue>
        <owl:onProperty rdf:resource="jc3iedmBase.owl#maritime-equipment-type-subcategory-code"/>
      </owl:Restriction>
    </rdfs:subClassOf>
    <rdfs:label xml:lang="en">Buoy, master reference</rdfs:label>
    <rdfs:comment xml:lang="en">A floating object fastened in a particular place to point out the position acting as a reference marker for MCM operations.</rdfs:comment>
  </owl:Class>
  <owl:Class rdf:about="#Anti-tank_missile_launcher,_medium">
    <rdfs:subClassOf rdf:resource="jc3iedmSubOnt.owl#WEAPON-TYPE-Missile_system"/>
    <rdfs:subClassOf rdf:resource="jc3iedmSubOnt.owl#WEAPON-TYPE-Anti-tank"/>
    <rdfs:subClassOf>
      <owl:Restriction>
        <owl:hasValue xml:lang="en">ATMLMD</owl:hasValue>
        <owl:onProperty rdf:resource="jc3iedmBase.owl#weapon-type-subcategory-code"/>
      </owl:Restriction>
    </rdfs:subClassOf>
    <rdfs:label xml:lang="en">Anti-tank missile launcher, medium</rdfs:label>
    <rdfs:comment xml:lang="en">A medium structural device designed to support and hold an anti-tank missile in position for firing.</rdfs:comment>
    <rdfs:subClassOf>
      <owl:Restriction>
        <owl:hasValue xml:lang="en">ATMLMD</owl:hasValue>
        <owl:onProperty rdf:resource="jc3iedmBase.owl#weapon-type-subcategory-code"/>
      </owl:Restriction>
    </rdfs:subClassOf>
  </owl:Class>
  <owl:Class rdf:about="#Howitzer,_light">
    <rdfs:subClassOf rdf:resource="jc3iedmSubOnt.owl#WEAPON-TYPE-Field_artillery"/>
    <rdfs:subClassOf rdf:resource="jc3iedmSubOnt.owl#WEAPON-TYPE-Cannon"/>
    <rdfs:subClassOf>
      <owl:Restriction>
        <owl:hasValue xml:lang="en">HOWTLT</owl:hasValue>
        <owl:onProperty rdf:resource="jc3iedmBase.owl#weapon-type-subcategory-code"/>
      </owl:Restriction>
    </rdfs:subClassOf>
    <rdfs:label xml:lang="en">Howitzer, light</rdfs:label>
    <rdfs:comment xml:lang="en">A light cannon that combines certain characteristics of guns and mortars. Normally a cannon with a tube length of 20 to 30 calibres; however, the tube length can exceed 30 calibres and still be considered a howitzer when the high angle firing zoning solution permits range overlap between charges.</rdfs:comment>
    <rdfs:subClassOf>
      <owl:Restriction>
        <owl:hasValue xml:lang="en">HOWTLT</owl:hasValue>
        <owl:onProperty rdf:resource="jc3iedmBase.owl#weapon-type-subcategory-code"/>
      </owl:Restriction>
    </rdfs:subClassOf>
  </owl:Class>
  <owl:Class rdf:ID="Telnet">
    <rdfs:subClassOf rdf:resource="jc3iedmSubOnt.owl#NETWORK-SERVICE-Data_transfer"/>
    <rdfs:subClassOf>
      <owl:Restriction>
        <owl:hasValue xml:lang="en">TELNET</owl:hasValue>
        <owl:onProperty rdf:resource="jc3iedmBase.owl#network-service-subcategory-code"/>
      </owl:Restriction>
    </rdfs:subClassOf>
    <rdfs:label xml:lang="en">Telnet</rdfs:label>
    <rdfs:comment xml:lang="en">A service using the terminal emulation protocol of TCP/IP. Options give TELNET the ability to transfer binary data, support byte macros, emulate graphics terminals, and convey information to support centralised terminal management.</rdfs:comment>
  </owl:Class>
  <owl:Class rdf:about="#Radio,_guidance">
    <rdfs:subClassOf rdf:resource="jc3iedmSubOnt.owl#ELECTRONIC-EQUIPMENT-TYPE-Communication"/>
    <rdfs:subClassOf>
      <owl:Restriction>
        <owl:hasValue xml:lang="en">RADGDN</owl:hasValue>
        <owl:onProperty rdf:resource="jc3iedmBase.owl#electronic-equipment-type-subcategory-code"/>
      </owl:Restriction>
    </rdfs:subClassOf>
    <rdfs:label xml:lang="en">Radio, guidance</rdfs:label>
    <rdfs:comment xml:lang="en">Remote control of the motion of a craft or vehicle by means of radio waves.</rdfs:comment>
  </owl:Class>
  <owl:Class rdf:ID="Bathythermograph">
    <rdfs:subClassOf rdf:resource="jc3iedmSubOnt.owl#ELECTRONIC-EQUIPMENT-TYPE-Sensor"/>
    <rdfs:subClassOf>
      <owl:Restriction>
        <owl:hasValue xml:lang="en">BTHTGH</owl:hasValue>
        <owl:onProperty rdf:resource="jc3iedmBase.owl#electronic-equipment-type-subcategory-code"/>
      </owl:Restriction>
    </rdfs:subClassOf>
    <rdfs:label xml:lang="en">Bathythermograph</rdfs:label>
    <rdfs:comment xml:lang="en">A device that records the ocean temperature at various depths. Used to assist in the determination of characteristics of sound propagation and sonar detection.</rdfs:comment>
  </owl:Class>
  <owl:Class rdf:ID="Electronic_mail">
    <rdfs:subClassOf rdf:resource="jc3iedmSubOnt.owl#NETWORK-SERVICE-Message_handling_service"/>
    <rdfs:subClassOf>
      <owl:Restriction>
        <owl:hasValue xml:lang="en">EMAIL</owl:hasValue>
        <owl:onProperty rdf:resource="jc3iedmBase.owl#network-service-subcategory-code"/>
      </owl:Restriction>
    </rdfs:subClassOf>
    <rdfs:label xml:lang="en">Electronic mail</rdfs:label>
    <rdfs:comment xml:lang="en">A communications service that provides correspondence in the form of messages transmitted between user terminals over a network.</rdfs:comment>
  </owl:Class>
  <owl:Class rdf:about="#Buoy,_short_scope">
    <rdfs:subClassOf rdf:resource="jc3iedmSubOnt.owl#MARITIME-EQUIPMENT-TYPE-Buoy"/>
    <rdfs:subClassOf>
      <owl:Restriction>
        <owl:hasValue xml:lang="en">BUOYSS</owl:hasValue>
        <owl:onProperty rdf:resource="jc3iedmBase.owl#maritime-equipment-type-subcategory-code"/>
      </owl:Restriction>
    </rdfs:subClassOf>
    <rdfs:label xml:lang="en">Buoy, short scope</rdfs:label>
    <rdfs:comment xml:lang="en">A buoy used as a navigational reference that remains nearly vertical over its sinker.</rdfs:comment>
  </owl:Class>
  <owl:Class rdf:ID="VINSON">
    <rdfs:subClassOf rdf:resource="jc3iedmSubOnt.owl#ELECTRONIC-EQUIPMENT-TYPE-Communication"/>
    <rdfs:subClassOf>
      <owl:Restriction>
        <owl:hasValue xml:lang="en">VINSON</owl:hasValue>
        <owl:onProperty rdf:resource="jc3iedmBase.owl#electronic-equipment-type-subcategory-code"/>
      </owl:Restriction>
    </rdfs:subClassOf>
    <rdfs:label xml:lang="en">VINSON</rdfs:label>
    <rdfs:comment xml:lang="en">A secure device for voice and FM communications.</rdfs:comment>
  </owl:Class>
  <owl:Class rdf:about="#Lagoon/reef_pool">
    <rdfs:subClassOf rdf:resource="jc3iedmSubOnt.owl#GEOGRAPHIC-FEATURE-TYPE-Inland_water"/>
    <rdfs:subClassOf rdf:resource="jc3iedmSubOnt.owl#GEOGRAPHIC-FEATURE-Liquid_surface"/>
    <rdfs:subClassOf>
      <owl:Restriction>
        <owl:hasValue xml:lang="en">LAGOON</owl:hasValue>
        <owl:onProperty rdf:resource="jc3iedmBase.owl#geographic-feature-type-subcategory-code"/>
      </owl:Restriction>
    </rdfs:subClassOf>
    <rdfs:label xml:lang="en">Lagoon/reef pool</rdfs:label>
    <rdfs:comment xml:lang="en">Open body of water separated from the sea by a sand bank or coral reef.</rdfs:comment>
    <rdfs:subClassOf>
      <owl:Restriction>
        <owl:hasValue xml:lang="en">LAGOON</owl:hasValue>
        <owl:onProperty rdf:resource="jc3iedmBase.owl#geographic-feature-type-subcategory-code"/>
      </owl:Restriction>
    </rdfs:subClassOf>
  </owl:Class>
  <owl:Class rdf:ID="Partly_dismantled">
    <rdfs:subClassOf>
      <owl:Restriction>
        <owl:hasValue xml:lang="en">PRTDSM</owl:hasValue>
        <owl:onProperty rdf:resource="jc3iedmBase.owl#facility-status-operational-status-qualifier-code"/>
      </owl:Restriction>
    </rdfs:subClassOf>
    <rdfs:label xml:lang="en">Partly dismantled</rdfs:label>
    <rdfs:comment xml:lang="en">Subjectively judged by the reporting organisation that a FACILITY is taken apart to some extent.</rdfs:comment>
    <rdfs:subClassOf>
      <owl:Restriction>
        <owl:hasValue xml:lang="en">PRTDSM</owl:hasValue>
        <owl:onProperty rdf:resource="jc3iedmBase.owl#facility-status-operational-status-qualifier-code"/>
      </owl:Restriction>
    </rdfs:subClassOf>
    <rdfs:subClassOf>
      <owl:Restriction>
        <owl:hasValue xml:lang="en">PRTDSM</owl:hasValue>
        <owl:onProperty rdf:resource="jc3iedmBase.owl#facility-status-operational-status-qualifier-code"/>
      </owl:Restriction>
    </rdfs:subClassOf>
  </owl:Class>
  <owl:Class rdf:about="#Locomotive,_steam">
    <rdfs:subClassOf rdf:resource="jc3iedmSubOnt.owl#RAILCAR-TYPE-Locomotive"/>
    <rdfs:subClassOf>
      <owl:Restriction>
        <owl:hasValue xml:lang="en">LCMSTM</owl:hasValue>
        <owl:onProperty rdf:resource="jc3iedmBase.owl#railcar-type-subcategory-code"/>
      </owl:Restriction>
    </rdfs:subClassOf>
    <rdfs:label xml:lang="en">Locomotive, steam</rdfs:label>
    <rdfs:comment xml:lang="en">A locomotive that uses the principle of heating water above its boiling point to produce steam, the expansion in a sealed vessel the pressure becomes the engine(s) source of tractive power.</rdfs:comment>
  </owl:Class>
  <owl:Class rdf:ID="Intact_but_unrecoverable">
    <rdfs:subClassOf>
      <owl:Restriction>
        <owl:hasValue xml:lang="en">INTREC</owl:hasValue>
        <owl:onProperty rdf:resource="jc3iedmBase.owl#materiel-status-operational-status-qualifier-code"/>
      </owl:Restriction>
    </rdfs:subClassOf>
    <rdfs:label xml:lang="en">Intact but unrecoverable</rdfs:label>
    <rdfs:comment xml:lang="en">Subjectively judged by the reporting organisation to be in an area unsuitable for recovery due to political, military, or geographic/environmental considerations.</rdfs:comment>
    <rdfs:subClassOf>
      <owl:Restriction>
        <owl:hasValue xml:lang="en">INTREC</owl:hasValue>
        <owl:onProperty rdf:resource="jc3iedmBase.owl#materiel-status-operational-status-qualifier-code"/>
      </owl:Restriction>
    </rdfs:subClassOf>
  </owl:Class>
  <owl:Class rdf:about="#Gully/gorge">
    <rdfs:subClassOf rdf:resource="jc3iedmSubOnt.owl#GEOGRAPHIC-FEATURE-Solid_surface"/>
    <rdfs:subClassOf rdf:resource="jc3iedmSubOnt.owl#GEOGRAPHIC-FEATURE-TYPE-Landform"/>
    <rdfs:subClassOf>
      <owl:Restriction>
        <owl:hasValue xml:lang="en">GULLY</owl:hasValue>
        <owl:onProperty rdf:resource="jc3iedmBase.owl#geographic-feature-type-subcategory-code"/>
      </owl:Restriction>
    </rdfs:subClassOf>
    <rdfs:label xml:lang="en">Gully/gorge</rdfs:label>
    <rdfs:comment xml:lang="en">A long, narrow, deep erosion with steep banks.</rdfs:comment>
    <rdfs:subClassOf>
      <owl:Restriction>
        <owl:hasValue xml:lang="en">GULLY</owl:hasValue>
        <owl:onProperty rdf:resource="jc3iedmBase.owl#geographic-feature-type-subcategory-code"/>
      </owl:Restriction>
    </rdfs:subClassOf>
  </owl:Class>
  <owl:Class rdf:ID="UN_Dangerous_Goods_NUM_1695">
    <rdfs:subClassOf>
      <owl:Restriction>
        <owl:hasValue xml:lang="en">1695</owl:hasValue>
        <owl:onProperty rdf:resource="jc3iedmBase.owl#consumable-materiel-type-united-nations-number-code"/>
      </owl:Restriction>
    </rdfs:subClassOf>
    <rdfs:label xml:lang="en">UN Dangerous Goods # 1695</rdfs:label>
    <rdfs:comment xml:lang="en">Chloroacetone, stabilized. Includes the agent(s): chloroacetone.</rdfs:comment>
    <rdfs:subClassOf>
      <owl:Restriction>
        <owl:hasValue xml:lang="en">1695</owl:hasValue>
        <owl:onProperty rdf:resource="jc3iedmBase.owl#consumable-materiel-type-united-nations-number-code"/>
      </owl:Restriction>
    </rdfs:subClassOf>
  </owl:Class>
  <owl:Class rdf:about="#Grenade_launcher,_heavy">
    <rdfs:subClassOf rdf:resource="jc3iedmSubOnt.owl#WEAPON-TYPE-Small_arms"/>
    <rdfs:subClassOf rdf:resource="jc3iedmSubOnt.owl#WEAPON-TYPE-Anti-tank"/>
    <rdfs:subClassOf>
      <owl:Restriction>
        <owl:hasValue xml:lang="en">GRLNHV</owl:hasValue>
        <owl:onProperty rdf:resource="jc3iedmBase.owl#weapon-type-subcategory-code"/>
      </owl:Restriction>
    </rdfs:subClassOf>
    <rdfs:label xml:lang="en">Grenade launcher, heavy</rdfs:label>
    <rdfs:comment xml:lang="en">A heavy structural device designed to support and hold a grenade in position for firing.</rdfs:comment>
    <rdfs:subClassOf>
      <owl:Restriction>
        <owl:hasValue xml:lang="en">GRLNHV</owl:hasValue>
        <owl:onProperty rdf:resource="jc3iedmBase.owl#weapon-type-subcategory-code"/>
      </owl:Restriction>
    </rdfs:subClassOf>
  </owl:Class>
  <owl:Class rdf:ID="UN_Dangerous_Goods_NUM_1836">
    <rdfs:subClassOf>
      <owl:Restriction>
        <owl:hasValue xml:lang="en">1836</owl:hasValue>
        <owl:onProperty rdf:resource="jc3iedmBase.owl#consumable-materiel-type-united-nations-number-code"/>
      </owl:Restriction>
    </rdfs:subClassOf>
    <rdfs:label xml:lang="en">UN Dangerous Goods # 1836</rdfs:label>
    <rdfs:comment xml:lang="en">Thionyl chloride. Includes the agent(s): thionyl chloride.</rdfs:comment>
    <rdfs:subClassOf>
      <owl:Restriction>
        <owl:hasValue xml:lang="en">1836</owl:hasValue>
        <owl:onProperty rdf:resource="jc3iedmBase.owl#consumable-materiel-type-united-nations-number-code"/>
      </owl:Restriction>
    </rdfs:subClassOf>
  </owl:Class>
  <owl:Class rdf:about="#Wagon,_articulated_vehicle_transporter">
    <rdfs:subClassOf rdf:resource="jc3iedmSubOnt.owl#RAILCAR-TYPE-Rolling_stock"/>
    <rdfs:subClassOf>
      <owl:Restriction>
        <owl:hasValue xml:lang="en">WGNART</owl:hasValue>
        <owl:onProperty rdf:resource="jc3iedmBase.owl#railcar-type-subcategory-code"/>
      </owl:Restriction>
    </rdfs:subClassOf>
    <rdfs:label xml:lang="en">Wagon, articulated vehicle transporter</rdfs:label>
    <rdfs:comment xml:lang="en">Rolling stock specifically designed to carry an articulated truck by rail (for example EUROSTAR).</rdfs:comment>
  </owl:Class>
  <owl:Class rdf:about="#Radar,_height-finding">
    <rdfs:subClassOf rdf:resource="jc3iedmSubOnt.owl#ELECTRONIC-EQUIPMENT-TYPE-Radar"/>
    <rdfs:subClassOf rdf:resource="jc3iedmSubOnt.owl#ELECTRONIC-EQUIPMENT-TYPE-Navigational_aid"/>
    <rdfs:subClassOf>
      <owl:Restriction>
        <owl:hasValue xml:lang="en">RDRHFD</owl:hasValue>
        <owl:onProperty rdf:resource="jc3iedmBase.owl#electronic-equipment-type-subcategory-code"/>
      </owl:Restriction>
    </rdfs:subClassOf>
    <rdfs:label xml:lang="en">Radar, height-finding</rdfs:label>
    <rdfs:comment xml:lang="en">A radar used to display the distance between an aircraft datum and the surface vertically below as determined by a reflecting radar transmission.</rdfs:comment>
    <rdfs:subClassOf>
      <owl:Restriction>
        <owl:hasValue xml:lang="en">RDRHFD</owl:hasValue>
        <owl:onProperty rdf:resource="jc3iedmBase.owl#electronic-equipment-type-subcategory-code"/>
      </owl:Restriction>
    </rdfs:subClassOf>
  </owl:Class>
  <owl:Class rdf:ID="UN_Dangerous_Goods_NUM_2202">
    <rdfs:subClassOf>
      <owl:Restriction>
        <owl:hasValue xml:lang="en">2202</owl:hasValue>
        <owl:onProperty rdf:resource="jc3iedmBase.owl#consumable-materiel-type-united-nations-number-code"/>
      </owl:Restriction>
    </rdfs:subClassOf>
    <rdfs:label xml:lang="en">UN Dangerous Goods # 2202</rdfs:label>
    <rdfs:comment xml:lang="en">Hydrogen selenide, anhydrous. Includes the agent(s): hydrogen selenide.</rdfs:comment>
    <rdfs:subClassOf>
      <owl:Restriction>
        <owl:hasValue xml:lang="en">2202</owl:hasValue>
        <owl:onProperty rdf:resource="jc3iedmBase.owl#consumable-materiel-type-united-nations-number-code"/>
      </owl:Restriction>
    </rdfs:subClassOf>
  </owl:Class>
  <owl:Class rdf:ID="MCI_Mode_2">
    <rdfs:subClassOf rdf:resource="jc3iedmSubOnt.owl#NETWORK-SERVICE-MCI"/>
    <rdfs:subClassOf>
      <owl:Restriction>
        <owl:hasValue xml:lang="en">MCIMD2</owl:hasValue>
        <owl:onProperty rdf:resource="jc3iedmBase.owl#network-service-subcategory-code"/>
      </owl:Restriction>
    </rdfs:subClassOf>
    <rdfs:label xml:lang="en">MCI Mode 2</rdfs:label>
    <rdfs:comment xml:lang="en">MCI gateway service proving MEM facilities.</rdfs:comment>
  </owl:Class>
  <owl:Class rdf:ID="Phencyclidine">
    <rdfs:subClassOf rdf:resource="jc3iedmSubOnt.owl#CONSUMABLE-MATERIEL-TYPE-Drug"/>
    <rdfs:subClassOf>
      <owl:Restriction>
        <owl:hasValue xml:lang="en">PCP</owl:hasValue>
        <owl:onProperty rdf:resource="jc3iedmBase.owl#consumable-materiel-type-subcategory-code"/>
      </owl:Restriction>
    </rdfs:subClassOf>
    <rdfs:label xml:lang="en">Phencyclidine</rdfs:label>
    <rdfs:comment xml:lang="en">A piperidine derivative used as a veterinary anaesthetic and a hallucinogenic drug.</rdfs:comment>
  </owl:Class>
  <owl:Class rdf:ID="UN_Dangerous_Goods_NUM_3333">
    <rdfs:subClassOf>
      <owl:Restriction>
        <owl:hasValue xml:lang="en">3333</owl:hasValue>
        <owl:onProperty rdf:resource="jc3iedmBase.owl#consumable-materiel-type-united-nations-number-code"/>
      </owl:Restriction>
    </rdfs:subClassOf>
    <rdfs:label xml:lang="en">UN Dangerous Goods # 3333</rdfs:label>
    <rdfs:comment xml:lang="en">Radioactive material, type A package, special form, fissile.</rdfs:comment>
  </owl:Class>
  <owl:Class rdf:ID="UN_Dangerous_Goods_NUM_1589">
    <rdfs:subClassOf>
      <owl:Restriction>
        <owl:hasValue xml:lang="en">1589</owl:hasValue>
        <owl:onProperty rdf:resource="jc3iedmBase.owl#consumable-materiel-type-united-nations-number-code"/>
      </owl:Restriction>
    </rdfs:subClassOf>
    <rdfs:label xml:lang="en">UN Dangerous Goods # 1589</rdfs:label>
    <rdfs:comment xml:lang="en">Cyanogen chloride, stabilized. Includes the agent(s): cyanogen chloride.</rdfs:comment>
    <rdfs:subClassOf>
      <owl:Restriction>
        <owl:hasValue xml:lang="en">1589</owl:hasValue>
        <owl:onProperty rdf:resource="jc3iedmBase.owl#consumable-materiel-type-united-nations-number-code"/>
      </owl:Restriction>
    </rdfs:subClassOf>
  </owl:Class>
  <owl:Class rdf:ID="Visual">
    <rdfs:subClassOf rdf:resource="jc3iedmSubOnt.owl#ELECTRONIC-EQUIPMENT-TYPE-Sensor"/>
    <rdfs:subClassOf>
      <owl:Restriction>
        <owl:hasValue xml:lang="en">VISUAL</owl:hasValue>
        <owl:onProperty rdf:resource="jc3iedmBase.owl#electronic-equipment-type-subcategory-code"/>
      </owl:Restriction>
    </rdfs:subClassOf>
    <rdfs:label xml:lang="en">Visual</rdfs:label>
    <rdfs:comment xml:lang="en">Equipment that uses the visual portion of the electromagnetic spectrum.</rdfs:comment>
  </owl:Class>
  <owl:Class rdf:ID="UN_Dangerous_Goods_NUM_1238">
    <rdfs:subClassOf>
      <owl:Restriction>
        <owl:hasValue xml:lang="en">1238</owl:hasValue>
        <owl:onProperty rdf:resource="jc3iedmBase.owl#consumable-materiel-type-united-nations-number-code"/>
      </owl:Restriction>
    </rdfs:subClassOf>
    <rdfs:label xml:lang="en">UN Dangerous Goods # 1238</rdfs:label>
    <rdfs:comment xml:lang="en">Methyl chloroformate. Includes the agent(s): methyl chloroformate.</rdfs:comment>
    <rdfs:subClassOf>
      <owl:Restriction>
        <owl:hasValue xml:lang="en">1238</owl:hasValue>
        <owl:onProperty rdf:resource="jc3iedmBase.owl#consumable-materiel-type-united-nations-number-code"/>
      </owl:Restriction>
    </rdfs:subClassOf>
  </owl:Class>
  <owl:Class rdf:about="#Rations,_tin">
    <rdfs:subClassOf rdf:resource="jc3iedmSubOnt.owl#CONSUMABLE-MATERIEL-TYPE-Food"/>
    <rdfs:subClassOf>
      <owl:Restriction>
        <owl:hasValue xml:lang="en">RATTI</owl:hasValue>
        <owl:onProperty rdf:resource="jc3iedmBase.owl#consumable-materiel-type-subcategory-code"/>
      </owl:Restriction>
    </rdfs:subClassOf>
    <rdfs:label xml:lang="en">Rations, tin</rdfs:label>
    <rdfs:comment xml:lang="en">Food preserved in a container allotted for persons.</rdfs:comment>
  </owl:Class>
  <owl:Class rdf:about="#Artillery,_very_heavy">
    <rdfs:subClassOf rdf:resource="jc3iedmSubOnt.owl#WEAPON-TYPE-Field_artillery"/>
    <rdfs:subClassOf>
      <owl:Restriction>
        <owl:hasValue xml:lang="en">ARTVHV</owl:hasValue>
        <owl:onProperty rdf:resource="jc3iedmBase.owl#weapon-type-subcategory-code"/>
      </owl:Restriction>
    </rdfs:subClassOf>
    <rdfs:label xml:lang="en">Artillery, very heavy</rdfs:label>
    <rdfs:comment xml:lang="en">Heavy artillery, calibre of 211 MM or larger, for use in the field in support of manoeuvre forces.</rdfs:comment>
  </owl:Class>
  <owl:Class rdf:about="#Locomotive,_electric">
    <rdfs:subClassOf rdf:resource="jc3iedmSubOnt.owl#RAILCAR-TYPE-Locomotive"/>
    <rdfs:subClassOf>
      <owl:Restriction>
        <owl:hasValue xml:lang="en">LCMELC</owl:hasValue>
        <owl:onProperty rdf:resource="jc3iedmBase.owl#railcar-type-subcategory-code"/>
      </owl:Restriction>
    </rdfs:subClassOf>
    <rdfs:label xml:lang="en">Locomotive, electric</rdfs:label>
    <rdfs:comment xml:lang="en">A locomotive that uses electric engine(s) as its source of tractive power, the electricity being supplied from an external source, typically via a pantograph (overhead electrical cable).</rdfs:comment>
  </owl:Class>
  <owl:Class rdf:about="#Radio,_teletype">
    <rdfs:subClassOf rdf:resource="jc3iedmSubOnt.owl#ELECTRONIC-EQUIPMENT-TYPE-Communication"/>
    <rdfs:subClassOf>
      <owl:Restriction>
        <owl:hasValue xml:lang="en">RADTLT</owl:hasValue>
        <owl:onProperty rdf:resource="jc3iedmBase.owl#electronic-equipment-type-subcategory-code"/>
      </owl:Restriction>
    </rdfs:subClassOf>
    <rdfs:label xml:lang="en">Radio, teletype</rdfs:label>
    <rdfs:comment xml:lang="en">The system for communication by teleprinter over radio circuits (RATT).</rdfs:comment>
  </owl:Class>
  <owl:Class rdf:ID="Telex">
    <rdfs:subClassOf rdf:resource="jc3iedmSubOnt.owl#NETWORK-SERVICE-Message_handling_service"/>
    <rdfs:subClassOf>
      <owl:Restriction>
        <owl:hasValue xml:lang="en">TELEX</owl:hasValue>
        <owl:onProperty rdf:resource="jc3iedmBase.owl#network-service-subcategory-code"/>
      </owl:Restriction>
    </rdfs:subClassOf>
    <rdfs:label xml:lang="en">Telex</rdfs:label>
    <rdfs:comment xml:lang="en">A communications service using a system consisting of teletypewriters connected to a telephonic network to send and receive signals.</rdfs:comment>
  </owl:Class>
  <owl:Class rdf:ID="MCI_Mode_3">
    <rdfs:subClassOf rdf:resource="jc3iedmSubOnt.owl#NETWORK-SERVICE-MCI"/>
    <rdfs:subClassOf>
      <owl:Restriction>
        <owl:hasValue xml:lang="en">MCIMD3</owl:hasValue>
        <owl:onProperty rdf:resource="jc3iedmBase.owl#network-service-subcategory-code"/>
      </owl:Restriction>
    </rdfs:subClassOf>
    <rdfs:label xml:lang="en">MCI Mode 3</rdfs:label>
    <rdfs:comment xml:lang="en">MCI gateway service proving DEM facilities.</rdfs:comment>
  </owl:Class>
  <owl:Class rdf:ID="Rail">
    <rdfs:label xml:lang="en">Rail</rdfs:label>
    <rdfs:comment xml:lang="en">Represents the general mode of transportation used in surface movement by rail.</rdfs:comment>
  </owl:Class>
  <owl:Class rdf:about="#Magnetic_V,_vertical_component">
    <rdfs:comment xml:lang="en">A (maritime) mine firing mechanism with a magnetic influence circuit which responds to the vertical component of the magnetic field of a ship.</rdfs:comment>
    <rdfs:subClassOf rdf:resource="jc3iedmSubOnt.owl#AMMUNITION-TYPE-Seabed_mine"/>
    <rdfs:subClassOf>
      <owl:Restriction>
        <owl:hasValue xml:lang="en">MAGNVV</owl:hasValue>
        <owl:onProperty rdf:resource="jc3iedmBase.owl#ammunition-type-mine-maritime-firing-code"/>
      </owl:Restriction>
    </rdfs:subClassOf>
    <rdfs:subClassOf rdf:resource="jc3iedmSubOnt.owl#AMMUNITION-TYPE-Mine,_shallow_moored"/>
    <rdfs:subClassOf rdf:resource="jc3iedmSubOnt.owl#AMMUNITION-TYPE-Mine,_not_known"/>
    <rdfs:subClassOf rdf:resource="jc3iedmSubOnt.owl#AMMUNITION-TYPE-Mine,_deep_moored"/>
    <rdfs:subClassOf rdf:resource="jc3iedmSubOnt.owl#AMMUNITION-TYPE-Sea_mine"/>
    <rdfs:subClassOf rdf:resource="jc3iedmSubOnt.owl#AMMUNITION-TYPE-Mine,_maritime,_moving"/>
    <rdfs:subClassOf rdf:resource="jc3iedmSubOnt.owl#AMMUNITION-TYPE-Mine,_seabed_-_explosive_charge_500kg_or_greater"/>
    <rdfs:subClassOf rdf:resource="jc3iedmSubOnt.owl#AMMUNITION-TYPE-Moving_mine,_sea"/>
    <rdfs:subClassOf>
      <owl:Restriction>
        <owl:hasValue xml:lang="en">MAGNVV</owl:hasValue>
        <owl:onProperty rdf:resource="jc3iedmBase.owl#ammunition-type-mine-maritime-firing-code"/>
      </owl:Restriction>
    </rdfs:subClassOf>
    <rdfs:label xml:lang="en">Magnetic V, vertical component</rdfs:label>
    <rdfs:subClassOf rdf:resource="jc3iedmSubOnt.owl#AMMUNITION-TYPE-Mine,_seabed_-_explosive_charge_less_than_500kg"/>
    <rdfs:subClassOf rdf:resource="jc3iedmSubOnt.owl#AMMUNITION-TYPE-Mine,_moored"/>
    <rdfs:subClassOf rdf:resource="jc3iedmSubOnt.owl#AMMUNITION-TYPE-Mine,_not_otherwise_specified"/>
  </owl:Class>
  <owl:Class rdf:ID="Communication_system">
    <rdfs:subClassOf rdf:resource="jc3iedmSubOnt.owl#ELECTRONIC-EQUIPMENT-TYPE-Communication"/>
    <rdfs:subClassOf>
      <owl:Restriction>
        <owl:hasValue xml:lang="en">COMSYS</owl:hasValue>
        <owl:onProperty rdf:resource="jc3iedmBase.owl#electronic-equipment-type-subcategory-code"/>
      </owl:Restriction>
    </rdfs:subClassOf>
    <rdfs:label xml:lang="en">Communication system</rdfs:label>
    <rdfs:comment xml:lang="en">A set of equipment designed for communications purposes.</rdfs:comment>
  </owl:Class>
  <owl:Class rdf:ID="Waterfall">
    <rdfs:subClassOf rdf:resource="jc3iedmSubOnt.owl#GEOGRAPHIC-FEATURE-TYPE-Inland_water"/>
    <rdfs:subClassOf rdf:resource="jc3iedmSubOnt.owl#GEOGRAPHIC-FEATURE-Liquid_surface"/>
    <rdfs:subClassOf>
      <owl:Restriction>
        <owl:hasValue xml:lang="en">WATRFL</owl:hasValue>
        <owl:onProperty rdf:resource="jc3iedmBase.owl#geographic-feature-type-subcategory-code"/>
      </owl:Restriction>
    </rdfs:subClassOf>
    <rdfs:label xml:lang="en">Waterfall</rdfs:label>
    <rdfs:comment xml:lang="en">A vertical or nearly vertical descent of water.</rdfs:comment>
    <rdfs:subClassOf>
      <owl:Restriction>
        <owl:hasValue xml:lang="en">WATRFL</owl:hasValue>
        <owl:onProperty rdf:resource="jc3iedmBase.owl#geographic-feature-type-subcategory-code"/>
      </owl:Restriction>
    </rdfs:subClassOf>
  </owl:Class>
  <owl:Class rdf:ID="MBR_position">
    <rdfs:subClassOf rdf:resource="jc3iedmSubOnt.owl#ELECTRONIC-EQUIPMENT-TYPE-Navigational_aid"/>
    <rdfs:subClassOf>
      <owl:Restriction>
        <owl:hasValue xml:lang="en">MBRPOS</owl:hasValue>
        <owl:onProperty rdf:resource="jc3iedmBase.owl#electronic-equipment-type-subcategory-code"/>
      </owl:Restriction>
    </rdfs:subClassOf>
    <rdfs:label xml:lang="en">MBR position</rdfs:label>
    <rdfs:comment xml:lang="en">No definition provided in ADatP-3 Baseline 13.1 FFIRN/FUD 1200/1.</rdfs:comment>
  </owl:Class>
  <owl:Class rdf:about="#Mortar,_light">
    <rdfs:subClassOf rdf:resource="jc3iedmSubOnt.owl#WEAPON-TYPE-Mortar"/>
    <rdfs:subClassOf>
      <owl:Restriction>
        <owl:hasValue xml:lang="en">MRTLGT</owl:hasValue>
        <owl:onProperty rdf:resource="jc3iedmBase.owl#weapon-type-subcategory-code"/>
      </owl:Restriction>
    </rdfs:subClassOf>
    <rdfs:label xml:lang="en">Mortar, light</rdfs:label>
    <rdfs:comment xml:lang="en">A man-portable, muzzle-loading, indirect fire weapon with either a rifled or smooth bore. It usually has a shorter range than a howitzer, employs a higher angle of fire, and its calibre is usually 60mm or smaller.</rdfs:comment>
  </owl:Class>
  <owl:Class rdf:ID="Under_construction">
    <rdfs:subClassOf>
      <owl:Restriction>
        <owl:hasValue xml:lang="en">UNCNST</owl:hasValue>
        <owl:onProperty rdf:resource="jc3iedmBase.owl#facility-status-operational-status-qualifier-code"/>
      </owl:Restriction>
    </rdfs:subClassOf>
    <rdfs:label xml:lang="en">Under construction</rdfs:label>
    <rdfs:comment xml:lang="en">Subjectively judged by the reporting organisation that a FACILITY is being built.</rdfs:comment>
    <rdfs:subClassOf>
      <owl:Restriction>
        <owl:hasValue xml:lang="en">UNCNST</owl:hasValue>
        <owl:onProperty rdf:resource="jc3iedmBase.owl#facility-status-operational-status-qualifier-code"/>
      </owl:Restriction>
    </rdfs:subClassOf>
    <rdfs:subClassOf>
      <owl:Restriction>
        <owl:hasValue xml:lang="en">UNCNST</owl:hasValue>
        <owl:onProperty rdf:resource="jc3iedmBase.owl#facility-status-operational-status-qualifier-code"/>
      </owl:Restriction>
    </rdfs:subClassOf>
    <rdfs:subClassOf>
      <owl:Restriction>
        <owl:hasValue xml:lang="en">UNCNST</owl:hasValue>
        <owl:onProperty rdf:resource="jc3iedmBase.owl#facility-status-operational-status-qualifier-code"/>
      </owl:Restriction>
    </rdfs:subClassOf>
  </owl:Class>
  <owl:Class rdf:ID="UN_Dangerous_Goods_NUM_1557">
    <rdfs:subClassOf>
      <owl:Restriction>
        <owl:hasValue xml:lang="en">1557</owl:hasValue>
        <owl:onProperty rdf:resource="jc3iedmBase.owl#consumable-materiel-type-united-nations-number-code"/>
      </owl:Restriction>
    </rdfs:subClassOf>
    <rdfs:label xml:lang="en">UN Dangerous Goods # 1557</rdfs:label>
    <rdfs:comment xml:lang="en">Arsenic compound, solid, N.O.S., inorganic, including: Arsenates, N.O.S.; Arsenites, N.O.S.; and Arsenic sulphides, N.O.S. Includes the agent(s): Lewisite.</rdfs:comment>
    <rdfs:subClassOf>
      <owl:Restriction>
        <owl:hasValue xml:lang="en">1557</owl:hasValue>
        <owl:onProperty rdf:resource="jc3iedmBase.owl#consumable-materiel-type-united-nations-number-code"/>
      </owl:Restriction>
    </rdfs:subClassOf>
  </owl:Class>
  <owl:Class rdf:ID="Valley">
    <rdfs:subClassOf rdf:resource="jc3iedmSubOnt.owl#GEOGRAPHIC-FEATURE-Solid_surface"/>
    <rdfs:subClassOf rdf:resource="jc3iedmSubOnt.owl#GEOGRAPHIC-FEATURE-TYPE-Landform"/>
    <rdfs:subClassOf>
      <owl:Restriction>
        <owl:hasValue xml:lang="en">VALLEY</owl:hasValue>
        <owl:onProperty rdf:resource="jc3iedmBase.owl#geographic-feature-type-subcategory-code"/>
      </owl:Restriction>
    </rdfs:subClassOf>
    <rdfs:label xml:lang="en">Valley</rdfs:label>
    <rdfs:comment xml:lang="en">A stretched-out groove in the land, usually formed by streams or rivers. A valley begins with high ground on three sides, and usually has a course of running water through it.</rdfs:comment>
    <rdfs:subClassOf>
      <owl:Restriction>
        <owl:hasValue xml:lang="en">VALLEY</owl:hasValue>
        <owl:onProperty rdf:resource="jc3iedmBase.owl#geographic-feature-type-subcategory-code"/>
      </owl:Restriction>
    </rdfs:subClassOf>
  </owl:Class>
  <owl:Class rdf:ID="Shoreline">
    <rdfs:subClassOf rdf:resource="jc3iedmSubOnt.owl#GEOGRAPHIC-FEATURE-Solid_surface"/>
    <rdfs:subClassOf rdf:resource="jc3iedmSubOnt.owl#GEOGRAPHIC-FEATURE-TYPE-Coastal_hydrography"/>
    <rdfs:subClassOf>
      <owl:Restriction>
        <owl:hasValue xml:lang="en">SHRLNE</owl:hasValue>
        <owl:onProperty rdf:resource="jc3iedmBase.owl#geographic-feature-type-subcategory-code"/>
      </owl:Restriction>
    </rdfs:subClassOf>
    <rdfs:label xml:lang="en">Shoreline</rdfs:label>
    <rdfs:comment xml:lang="en">A line drawn along the normal limit of wave action above either Mean High Water Springs (MHWS) or Mean High High Water (MHHW) as defined by the National Authority.</rdfs:comment>
    <rdfs:subClassOf>
      <owl:Restriction>
        <owl:hasValue xml:lang="en">SHRLNE</owl:hasValue>
        <owl:onProperty rdf:resource="jc3iedmBase.owl#geographic-feature-type-subcategory-code"/>
      </owl:Restriction>
    </rdfs:subClassOf>
  </owl:Class>
  <owl:Class rdf:ID="Low_light_level_television">
    <rdfs:subClassOf rdf:resource="jc3iedmSubOnt.owl#ELECTRONIC-EQUIPMENT-TYPE-Sensor"/>
    <rdfs:subClassOf>
      <owl:Restriction>
        <owl:hasValue xml:lang="en">LGLVTV</owl:hasValue>
        <owl:onProperty rdf:resource="jc3iedmBase.owl#electronic-equipment-type-subcategory-code"/>
      </owl:Restriction>
    </rdfs:subClassOf>
    <rdfs:label xml:lang="en">Low light level television</rdfs:label>
    <rdfs:comment xml:lang="en">Television-type system that uses ambient light to reduce the value of the ratio of brightness between target and background and the brightness of the background that is used for day/night surveillance, target acquisition, fire control, fire adjustment, target identification, and target tracking; the LLLTV cannot see in complete darkness, it needs some ambient light from the atmosphere, moon, stars etc.</rdfs:comment>
  </owl:Class>
  <owl:Class rdf:ID="Volcano">
    <rdfs:subClassOf rdf:resource="jc3iedmSubOnt.owl#GEOGRAPHIC-FEATURE-Solid_surface"/>
    <rdfs:subClassOf rdf:resource="jc3iedmSubOnt.owl#GEOGRAPHIC-FEATURE-TYPE-Landform"/>
    <rdfs:subClassOf>
      <owl:Restriction>
        <owl:hasValue xml:lang="en">VOLCNO</owl:hasValue>
        <owl:onProperty rdf:resource="jc3iedmBase.owl#geographic-feature-type-subcategory-code"/>
      </owl:Restriction>
    </rdfs:subClassOf>
    <rdfs:label xml:lang="en">Volcano</rdfs:label>
    <rdfs:comment xml:lang="en">A mountain or hill, often conical, formed around a vent in the earth's crust through which molten rock, ash, or gases are or have been expelled.</rdfs:comment>
    <rdfs:subClassOf>
      <owl:Restriction>
        <owl:hasValue xml:lang="en">VOLCNO</owl:hasValue>
        <owl:onProperty rdf:resource="jc3iedmBase.owl#geographic-feature-type-subcategory-code"/>
      </owl:Restriction>
    </rdfs:subClassOf>
  </owl:Class>
  <owl:Class rdf:ID="Sea">
    <rdfs:label xml:lang="en">Sea</rdfs:label>
    <rdfs:comment xml:lang="en">Represents the general mode of transportation used in movement by sea.</rdfs:comment>
  </owl:Class>
  <owl:Class rdf:ID="Direct_fire_gun">
    <rdfs:subClassOf rdf:resource="jc3iedmSubOnt.owl#WEAPON-TYPE-Small_arms"/>
    <rdfs:subClassOf>
      <owl:Restriction>
        <owl:hasValue xml:lang="en">DFGN</owl:hasValue>
        <owl:onProperty rdf:resource="jc3iedmBase.owl#weapon-type-subcategory-code"/>
      </owl:Restriction>
    </rdfs:subClassOf>
    <rdfs:label xml:lang="en">Direct fire gun</rdfs:label>
    <rdfs:comment xml:lang="en">A cannon with a relatively low angle of fire, having a high muzzle velocity with a tube length of 30 calibres or more that delivers fire on a target using the target itself as a point of aim for either the weapon or the director.</rdfs:comment>
  </owl:Class>
  <owl:Class rdf:about="#Sonar,_dipping,_active">
    <rdfs:subClassOf rdf:resource="jc3iedmSubOnt.owl#MARITIME-EQUIPMENT-TYPE-Sonar,_maritime"/>
    <rdfs:subClassOf>
      <owl:Restriction>
        <owl:hasValue xml:lang="en">SONRDA</owl:hasValue>
        <owl:onProperty rdf:resource="jc3iedmBase.owl#maritime-equipment-type-subcategory-code"/>
      </owl:Restriction>
    </rdfs:subClassOf>
    <rdfs:label xml:lang="en">Sonar, dipping, active</rdfs:label>
    <rdfs:comment xml:lang="en">No definition provided in ADatP-3 Baseline 13.1 FFIRN/FUD 1434/1.</rdfs:comment>
  </owl:Class>
  <owl:Class rdf:about="#Radar,_inverse_synthetic_aperture">
    <rdfs:subClassOf rdf:resource="jc3iedmSubOnt.owl#ELECTRONIC-EQUIPMENT-TYPE-Radar"/>
    <rdfs:subClassOf>
      <owl:Restriction>
        <owl:hasValue xml:lang="en">RDISAR</owl:hasValue>
        <owl:onProperty rdf:resource="jc3iedmBase.owl#electronic-equipment-type-subcategory-code"/>
      </owl:Restriction>
    </rdfs:subClassOf>
    <rdfs:label xml:lang="en">Radar, inverse synthetic aperture</rdfs:label>
    <rdfs:comment xml:lang="en">A high-resolution radar that tracks a moving object by using a stationary single radiating antenna element that transmits when the moving object is at sequential positions on its line of movement. Used in maritime surveillance.</rdfs:comment>
  </owl:Class>
  <owl:Class rdf:ID="UN_Dangerous_Goods_NUM_1859">
    <rdfs:subClassOf>
      <owl:Restriction>
        <owl:hasValue xml:lang="en">1859</owl:hasValue>
        <owl:onProperty rdf:resource="jc3iedmBase.owl#consumable-materiel-type-united-nations-number-code"/>
      </owl:Restriction>
    </rdfs:subClassOf>
    <rdfs:label xml:lang="en">UN Dangerous Goods # 1859</rdfs:label>
    <rdfs:comment xml:lang="en">Silicon tetrafluoride. Includes the agent(s): silicon tetrafluoride.</rdfs:comment>
    <rdfs:subClassOf>
      <owl:Restriction>
        <owl:hasValue xml:lang="en">1859</owl:hasValue>
        <owl:onProperty rdf:resource="jc3iedmBase.owl#consumable-materiel-type-united-nations-number-code"/>
      </owl:Restriction>
    </rdfs:subClassOf>
  </owl:Class>
  <owl:Class rdf:ID="Morphine">
    <rdfs:subClassOf rdf:resource="jc3iedmSubOnt.owl#CONSUMABLE-MATERIEL-TYPE-Drug"/>
    <rdfs:subClassOf>
      <owl:Restriction>
        <owl:hasValue xml:lang="en">MORFIN</owl:hasValue>
        <owl:onProperty rdf:resource="jc3iedmBase.owl#consumable-materiel-type-subcategory-code"/>
      </owl:Restriction>
    </rdfs:subClassOf>
    <rdfs:label xml:lang="en">Morphine</rdfs:label>
    <rdfs:comment xml:lang="en">An analgesic and narcotic drug obtained from opium and used medicinally to relieve pain.</rdfs:comment>
  </owl:Class>
  <owl:Class rdf:about="#Sweep,_OROPESA">
    <rdfs:subClassOf rdf:resource="jc3iedmSubOnt.owl#MARITIME-EQUIPMENT-TYPE-Sweep"/>
    <rdfs:subClassOf>
      <owl:Restriction>
        <owl:hasValue xml:lang="en">SWPORO</owl:hasValue>
        <owl:onProperty rdf:resource="jc3iedmBase.owl#maritime-equipment-type-subcategory-code"/>
      </owl:Restriction>
    </rdfs:subClassOf>
    <rdfs:label xml:lang="en">Sweep, OROPESA</rdfs:label>
    <rdfs:comment xml:lang="en">Equipment designed to locate mines using a length of sweep wire that is towed by a single ship, lateral displacement being caused by an Otter and depth being controlled at the ship end by a Kite at the Otter end by a float and float wire.</rdfs:comment>
  </owl:Class>
  <owl:Class rdf:ID="Coal">
    <rdfs:subClassOf rdf:resource="jc3iedmSubOnt.owl#CONSUMABLE-MATERIEL-TYPE-Fuel"/>
    <rdfs:subClassOf>
      <owl:Restriction>
        <owl:hasValue xml:lang="en">COAL</owl:hasValue>
        <owl:onProperty rdf:resource="jc3iedmBase.owl#consumable-materiel-type-subcategory-code"/>
      </owl:Restriction>
    </rdfs:subClassOf>
    <rdfs:label xml:lang="en">Coal</rdfs:label>
    <rdfs:comment xml:lang="en">Fuel made from carbon, cinder or ember.</rdfs:comment>
  </owl:Class>
  <owl:Class rdf:ID="Sequence">
    <rdfs:subClassOf rdf:resource="jc3iedmSubOnt.owl#AMMUNITION-TYPE-Mine,_seabed_-_explosive_charge_less_than_500kg"/>
    <rdfs:subClassOf>
      <owl:Restriction>
        <owl:hasValue xml:lang="en">SEQUEN</owl:hasValue>
        <owl:onProperty rdf:resource="jc3iedmBase.owl#ammunition-type-mine-maritime-firing-code"/>
      </owl:Restriction>
    </rdfs:subClassOf>
    <rdfs:label xml:lang="en">Sequence</rdfs:label>
    <rdfs:subClassOf rdf:resource="jc3iedmSubOnt.owl#AMMUNITION-TYPE-Mine,_not_otherwise_specified"/>
    <rdfs:subClassOf rdf:resource="jc3iedmSubOnt.owl#AMMUNITION-TYPE-Mine,_seabed_-_explosive_charge_500kg_or_greater"/>
    <rdfs:subClassOf rdf:resource="jc3iedmSubOnt.owl#AMMUNITION-TYPE-Mine,_moored"/>
    <rdfs:subClassOf rdf:resource="jc3iedmSubOnt.owl#AMMUNITION-TYPE-Mine,_shallow_moored"/>
    <rdfs:subClassOf rdf:resource="jc3iedmSubOnt.owl#AMMUNITION-TYPE-Mine,_not_known"/>
    <rdfs:subClassOf rdf:resource="jc3iedmSubOnt.owl#AMMUNITION-TYPE-Moving_mine,_sea"/>
    <rdfs:subClassOf rdf:resource="jc3iedmSubOnt.owl#AMMUNITION-TYPE-Mine,_deep_moored"/>
    <rdfs:subClassOf>
      <owl:Restriction>
        <owl:hasValue xml:lang="en">SEQUEN</owl:hasValue>
        <owl:onProperty rdf:resource="jc3iedmBase.owl#ammunition-type-mine-maritime-firing-code"/>
      </owl:Restriction>
    </rdfs:subClassOf>
    <rdfs:comment xml:lang="en">A (maritime) mine firing mechanism that has a firing circuit which requires actuation by a predetermined sequence of influences of predetermined magnitude.</rdfs:comment>
    <rdfs:subClassOf rdf:resource="jc3iedmSubOnt.owl#AMMUNITION-TYPE-Sea_mine"/>
    <rdfs:subClassOf rdf:resource="jc3iedmSubOnt.owl#AMMUNITION-TYPE-Seabed_mine"/>
    <rdfs:subClassOf rdf:resource="jc3iedmSubOnt.owl#AMMUNITION-TYPE-Mine,_maritime,_moving"/>
  </owl:Class>
  <owl:Class rdf:ID="Fixed_and_prefabricated">
    <rdfs:subClassOf rdf:resource="jc3iedmSubOnt.owl#MILITARY-OBSTACLE-TYPE-Anti-tank_obstacle"/>
    <rdfs:subClassOf rdf:resource="jc3iedmSubOnt.owl#MILITARY-OBSTACLE-TYPE-Tetrahedron"/>
    <rdfs:subClassOf rdf:resource="jc3iedmSubOnt.owl#MILITARY-OBSTACLE-TYPE-Dragon_teeth"/>
    <rdfs:subClassOf>
      <owl:Restriction>
        <owl:hasValue xml:lang="en">FXAMOV</owl:hasValue>
        <owl:onProperty rdf:resource="jc3iedmBase.owl#military-obstacle-type-subcategory-code"/>
      </owl:Restriction>
    </rdfs:subClassOf>
    <rdfs:label xml:lang="en">Fixed and prefabricated</rdfs:label>
    <rdfs:comment xml:lang="en">The obstacle is prefabricated and can not be moved.</rdfs:comment>
    <rdfs:subClassOf>
      <owl:Restriction>
        <owl:hasValue xml:lang="en">FXAMOV</owl:hasValue>
        <owl:onProperty rdf:resource="jc3iedmBase.owl#military-obstacle-type-subcategory-code"/>
      </owl:Restriction>
    </rdfs:subClassOf>
    <rdfs:subClassOf>
      <owl:Restriction>
        <owl:hasValue xml:lang="en">FXAMOV</owl:hasValue>
        <owl:onProperty rdf:resource="jc3iedmBase.owl#military-obstacle-type-subcategory-code"/>
      </owl:Restriction>
    </rdfs:subClassOf>
  </owl:Class>
  <owl:Class rdf:ID="Pressure">
    <rdfs:subClassOf rdf:resource="jc3iedmSubOnt.owl#AMMUNITION-TYPE-Moving_mine,_sea"/>
    <rdfs:subClassOf rdf:resource="jc3iedmSubOnt.owl#AMMUNITION-TYPE-Mine,_deep_moored"/>
    <rdfs:subClassOf rdf:resource="jc3iedmSubOnt.owl#AMMUNITION-TYPE-Mine,_not_known"/>
    <rdfs:subClassOf rdf:resource="jc3iedmSubOnt.owl#AMMUNITION-TYPE-Mine,_maritime,_moving"/>
    <rdfs:label xml:lang="en">Pressure</rdfs:label>
    <rdfs:subClassOf rdf:resource="jc3iedmSubOnt.owl#AMMUNITION-TYPE-Seabed_mine"/>
    <rdfs:subClassOf rdf:resource="jc3iedmSubOnt.owl#AMMUNITION-TYPE-Mine,_shallow_moored"/>
    <rdfs:subClassOf rdf:resource="jc3iedmSubOnt.owl#AMMUNITION-TYPE-Mine,_seabed_-_explosive_charge_500kg_or_greater"/>
    <rdfs:comment xml:lang="en">A (maritime) mine firing mechanism with a pressure sensitive circuit which responds to the pressure variation as a result of a ship or sweep.</rdfs:comment>
    <rdfs:subClassOf rdf:resource="jc3iedmSubOnt.owl#AMMUNITION-TYPE-Mine,_moored"/>
    <rdfs:subClassOf rdf:resource="jc3iedmSubOnt.owl#AMMUNITION-TYPE-Sea_mine"/>
    <rdfs:subClassOf>
      <owl:Restriction>
        <owl:hasValue xml:lang="en">PRESUR</owl:hasValue>
        <owl:onProperty rdf:resource="jc3iedmBase.owl#ammunition-type-mine-maritime-firing-code"/>
      </owl:Restriction>
    </rdfs:subClassOf>
    <rdfs:subClassOf rdf:resource="jc3iedmSubOnt.owl#AMMUNITION-TYPE-Mine,_seabed_-_explosive_charge_less_than_500kg"/>
    <rdfs:subClassOf rdf:resource="jc3iedmSubOnt.owl#AMMUNITION-TYPE-Mine,_not_otherwise_specified"/>
    <rdfs:subClassOf>
      <owl:Restriction>
        <owl:hasValue xml:lang="en">PRESUR</owl:hasValue>
        <owl:onProperty rdf:resource="jc3iedmBase.owl#ammunition-type-mine-maritime-firing-code"/>
      </owl:Restriction>
    </rdfs:subClassOf>
  </owl:Class>
  <owl:Class rdf:ID="Phosgene_oxime">
    <rdfs:subClassOf rdf:resource="jc3iedmSubOnt.owl#CHEMICAL-MATERIEL-TYPE-Blood_agent"/>
    <rdfs:subClassOf>
      <owl:Restriction>
        <owl:hasValue xml:lang="en">PHSGNO</owl:hasValue>
        <owl:onProperty rdf:resource="jc3iedmBase.owl#chemical-materiel-type-subcategory-code"/>
      </owl:Restriction>
    </rdfs:subClassOf>
    <rdfs:label xml:lang="en">Phosgene oxime</rdfs:label>
    <rdfs:comment xml:lang="en">A poisonous gas formerly used in warfare derived from phosgene used to block the oxygenation of aemoglobin. [COCl2.] (Blood agent)</rdfs:comment>
  </owl:Class>
  <owl:Class rdf:ID="Machine_gun">
    <rdfs:subClassOf rdf:resource="jc3iedmSubOnt.owl#WEAPON-TYPE-Small_arms"/>
    <rdfs:subClassOf>
      <owl:Restriction>
        <owl:hasValue xml:lang="en">MACGUN</owl:hasValue>
        <owl:onProperty rdf:resource="jc3iedmBase.owl#weapon-type-subcategory-code"/>
      </owl:Restriction>
    </rdfs:subClassOf>
    <rdfs:label xml:lang="en">Machine gun</rdfs:label>
    <rdfs:comment xml:lang="en">An automatic gun giving continuous fire.</rdfs:comment>
  </owl:Class>
  <owl:Class rdf:about="#Radar,_earth_satellite/space_tracking">
    <rdfs:subClassOf rdf:resource="jc3iedmSubOnt.owl#ELECTRONIC-EQUIPMENT-TYPE-Radar"/>
    <rdfs:subClassOf rdf:resource="jc3iedmSubOnt.owl#ELECTRONIC-EQUIPMENT-TYPE-Navigational_aid"/>
    <rdfs:subClassOf>
      <owl:Restriction>
        <owl:hasValue xml:lang="en">RDREST</owl:hasValue>
        <owl:onProperty rdf:resource="jc3iedmBase.owl#electronic-equipment-type-subcategory-code"/>
      </owl:Restriction>
    </rdfs:subClassOf>
    <rdfs:label xml:lang="en">Radar, earth satellite/space tracking</rdfs:label>
    <rdfs:comment xml:lang="en">A radar used for tracking satellite or other objects in space.</rdfs:comment>
    <rdfs:subClassOf>
      <owl:Restriction>
        <owl:hasValue xml:lang="en">RDREST</owl:hasValue>
        <owl:onProperty rdf:resource="jc3iedmBase.owl#electronic-equipment-type-subcategory-code"/>
      </owl:Restriction>
    </rdfs:subClassOf>
  </owl:Class>
  <owl:Class rdf:ID="UN_Dangerous_Goods_NUM_2692">
    <rdfs:subClassOf>
      <owl:Restriction>
        <owl:hasValue xml:lang="en">2692</owl:hasValue>
        <owl:onProperty rdf:resource="jc3iedmBase.owl#consumable-materiel-type-united-nations-number-code"/>
      </owl:Restriction>
    </rdfs:subClassOf>
    <rdfs:label xml:lang="en">UN Dangerous Goods # 2692</rdfs:label>
    <rdfs:comment xml:lang="en">Boron tribromide. Includes the agent(s): boron tribromide.</rdfs:comment>
    <rdfs:subClassOf>
      <owl:Restriction>
        <owl:hasValue xml:lang="en">2692</owl:hasValue>
        <owl:onProperty rdf:resource="jc3iedmBase.owl#consumable-materiel-type-united-nations-number-code"/>
      </owl:Restriction>
    </rdfs:subClassOf>
  </owl:Class>
  <owl:Class rdf:ID="UN_Dangerous_Goods_NUM_3332">
    <rdfs:subClassOf>
      <owl:Restriction>
        <owl:hasValue xml:lang="en">3332</owl:hasValue>
        <owl:onProperty rdf:resource="jc3iedmBase.owl#consumable-materiel-type-united-nations-number-code"/>
      </owl:Restriction>
    </rdfs:subClassOf>
    <rdfs:label xml:lang="en">UN Dangerous Goods # 3332</rdfs:label>
    <rdfs:comment xml:lang="en">Radioactive material, type A package, special form, non fissile or fissile-excepted.</rdfs:comment>
  </owl:Class>
  <owl:Class rdf:ID="UN_Dangerous_Goods_NUM_2382">
    <rdfs:subClassOf>
      <owl:Restriction>
        <owl:hasValue xml:lang="en">2382</owl:hasValue>
        <owl:onProperty rdf:resource="jc3iedmBase.owl#consumable-materiel-type-united-nations-number-code"/>
      </owl:Restriction>
    </rdfs:subClassOf>
    <rdfs:label xml:lang="en">UN Dangerous Goods # 2382</rdfs:label>
    <rdfs:comment xml:lang="en">Dimethylhydrazine, symmetrical. Includes the agent(s): 1,1-dimethylhydrazine.</rdfs:comment>
    <rdfs:subClassOf>
      <owl:Restriction>
        <owl:hasValue xml:lang="en">2382</owl:hasValue>
        <owl:onProperty rdf:resource="jc3iedmBase.owl#consumable-materiel-type-united-nations-number-code"/>
      </owl:Restriction>
    </rdfs:subClassOf>
  </owl:Class>
  <owl:Class rdf:ID="Revetting_material">
    <rdfs:subClassOf rdf:resource="jc3iedmSubOnt.owl#CONSUMABLE-MATERIEL-TYPE-Construction_materials"/>
    <rdfs:subClassOf>
      <owl:Restriction>
        <owl:hasValue xml:lang="en">REVET</owl:hasValue>
        <owl:onProperty rdf:resource="jc3iedmBase.owl#consumable-materiel-type-subcategory-code"/>
      </owl:Restriction>
    </rdfs:subClassOf>
    <rdfs:label xml:lang="en">Revetting material</rdfs:label>
    <rdfs:comment xml:lang="en">Steel or other supporting material used in constructing a wall of earth.</rdfs:comment>
  </owl:Class>
  <owl:Class rdf:ID="Depression">
    <rdfs:subClassOf rdf:resource="jc3iedmSubOnt.owl#GEOGRAPHIC-FEATURE-Solid_surface"/>
    <rdfs:subClassOf rdf:resource="jc3iedmSubOnt.owl#GEOGRAPHIC-FEATURE-TYPE-Landform"/>
    <rdfs:subClassOf>
      <owl:Restriction>
        <owl:hasValue xml:lang="en">DPRSSN</owl:hasValue>
        <owl:onProperty rdf:resource="jc3iedmBase.owl#geographic-feature-type-subcategory-code"/>
      </owl:Restriction>
    </rdfs:subClassOf>
    <rdfs:label xml:lang="en">Depression</rdfs:label>
    <rdfs:comment xml:lang="en">A low area surrounded by higher ground.</rdfs:comment>
    <rdfs:subClassOf>
      <owl:Restriction>
        <owl:hasValue xml:lang="en">DPRSSN</owl:hasValue>
        <owl:onProperty rdf:resource="jc3iedmBase.owl#geographic-feature-type-subcategory-code"/>
      </owl:Restriction>
    </rdfs:subClassOf>
  </owl:Class>
  <owl:Class rdf:ID="Natural_gas">
    <rdfs:subClassOf rdf:resource="jc3iedmSubOnt.owl#CONSUMABLE-MATERIEL-TYPE-Fuel"/>
    <rdfs:subClassOf>
      <owl:Restriction>
        <owl:hasValue xml:lang="en">NATGAS</owl:hasValue>
        <owl:onProperty rdf:resource="jc3iedmBase.owl#consumable-materiel-type-subcategory-code"/>
      </owl:Restriction>
    </rdfs:subClassOf>
    <rdfs:label xml:lang="en">Natural gas</rdfs:label>
    <rdfs:comment xml:lang="en">A flammable gas, consisting largely of methane and other hydrocarbons, occurring naturally underground and used as fuel.</rdfs:comment>
  </owl:Class>
  <owl:Class rdf:about="#Anti-tank_gun,_light">
    <rdfs:subClassOf rdf:resource="jc3iedmSubOnt.owl#WEAPON-TYPE-Anti-tank"/>
    <rdfs:subClassOf>
      <owl:Restriction>
        <owl:hasValue xml:lang="en">ATGNLT</owl:hasValue>
        <owl:onProperty rdf:resource="jc3iedmBase.owl#weapon-type-subcategory-code"/>
      </owl:Restriction>
    </rdfs:subClassOf>
    <rdfs:label xml:lang="en">Anti-tank gun, light</rdfs:label>
    <rdfs:comment xml:lang="en">A light gun designed to destroy tanks.</rdfs:comment>
  </owl:Class>
  <owl:Class rdf:ID="Botanical_garden">
    <rdfs:label xml:lang="en">Botanical garden</rdfs:label>
    <rdfs:comment xml:lang="en">A cultural area where plants and/or trees are displayed.</rdfs:comment>
  </owl:Class>
  <owl:Class rdf:ID="UN_Dangerous_Goods_NUM_3321">
    <rdfs:subClassOf>
      <owl:Restriction>
        <owl:hasValue xml:lang="en">3321</owl:hasValue>
        <owl:onProperty rdf:resource="jc3iedmBase.owl#consumable-materiel-type-united-nations-number-code"/>
      </owl:Restriction>
    </rdfs:subClassOf>
    <rdfs:label xml:lang="en">UN Dangerous Goods # 3321</rdfs:label>
    <rdfs:comment xml:lang="en">Radioactive material, low specific activity (LSA-II), non fissile or fissile-excepted.</rdfs:comment>
  </owl:Class>
  <owl:Class rdf:about="#Sweep,_acoustic_combined">
    <rdfs:subClassOf rdf:resource="jc3iedmSubOnt.owl#MARITIME-EQUIPMENT-TYPE-Sweep"/>
    <rdfs:subClassOf>
      <owl:Restriction>
        <owl:hasValue xml:lang="en">SWPACC</owl:hasValue>
        <owl:onProperty rdf:resource="jc3iedmBase.owl#maritime-equipment-type-subcategory-code"/>
      </owl:Restriction>
    </rdfs:subClassOf>
    <rdfs:label xml:lang="en">Sweep, acoustic combined</rdfs:label>
    <rdfs:comment xml:lang="en">Equipment designed to locate mines by use of a sweep designed to operate the acoustic firing system of a mine, MF and LF frequency 30 to 15000HZ.</rdfs:comment>
  </owl:Class>
  <owl:Class rdf:ID="Ice_shelf">
    <rdfs:subClassOf rdf:resource="jc3iedmSubOnt.owl#GEOGRAPHIC-FEATURE-TYPE-Snow/ice"/>
    <rdfs:subClassOf rdf:resource="jc3iedmSubOnt.owl#GEOGRAPHIC-FEATURE-Solid_surface"/>
    <rdfs:subClassOf>
      <owl:Restriction>
        <owl:hasValue xml:lang="en">ICESHL</owl:hasValue>
        <owl:onProperty rdf:resource="jc3iedmBase.owl#geographic-feature-type-subcategory-code"/>
      </owl:Restriction>
    </rdfs:subClassOf>
    <rdfs:label xml:lang="en">Ice shelf</rdfs:label>
    <rdfs:comment xml:lang="en">A sheet of thick ice, with level or undulating surface, attached to the land but mostly afloat which is bounded on the seaward side by an Ice Cliff.</rdfs:comment>
    <rdfs:subClassOf>
      <owl:Restriction>
        <owl:hasValue xml:lang="en">ICESHL</owl:hasValue>
        <owl:onProperty rdf:resource="jc3iedmBase.owl#geographic-feature-type-subcategory-code"/>
      </owl:Restriction>
    </rdfs:subClassOf>
  </owl:Class>
  <owl:Class rdf:about="#Snags/submerged_stumps">
    <rdfs:subClassOf rdf:resource="jc3iedmSubOnt.owl#GEOGRAPHIC-FEATURE-Solid_surface"/>
    <rdfs:subClassOf rdf:resource="jc3iedmSubOnt.owl#GEOGRAPHIC-FEATURE-TYPE-Landform"/>
    <rdfs:subClassOf>
      <owl:Restriction>
        <owl:hasValue xml:lang="en">SNGSSS</owl:hasValue>
        <owl:onProperty rdf:resource="jc3iedmBase.owl#geographic-feature-type-subcategory-code"/>
      </owl:Restriction>
    </rdfs:subClassOf>
    <rdfs:label xml:lang="en">Snags/submerged stumps</rdfs:label>
    <rdfs:comment xml:lang="en">A stem or a trunk of a tree below the surface of water.</rdfs:comment>
    <rdfs:subClassOf>
      <owl:Restriction>
        <owl:hasValue xml:lang="en">SNGSSS</owl:hasValue>
        <owl:onProperty rdf:resource="jc3iedmBase.owl#geographic-feature-type-subcategory-code"/>
      </owl:Restriction>
    </rdfs:subClassOf>
  </owl:Class>
  <owl:Class rdf:ID="UN_Dangerous_Goods_NUM_1092">
    <rdfs:subClassOf>
      <owl:Restriction>
        <owl:hasValue xml:lang="en">1092</owl:hasValue>
        <owl:onProperty rdf:resource="jc3iedmBase.owl#consumable-materiel-type-united-nations-number-code"/>
      </owl:Restriction>
    </rdfs:subClassOf>
    <rdfs:label xml:lang="en">UN Dangerous Goods # 1092</rdfs:label>
    <rdfs:comment xml:lang="en">Acrolein, stabilized. Includes the agent(s): acrolein.</rdfs:comment>
    <rdfs:subClassOf>
      <owl:Restriction>
        <owl:hasValue xml:lang="en">1092</owl:hasValue>
        <owl:onProperty rdf:resource="jc3iedmBase.owl#consumable-materiel-type-united-nations-number-code"/>
      </owl:Restriction>
    </rdfs:subClassOf>
  </owl:Class>
  <owl:Class rdf:ID="Lubricant">
    <rdfs:subClassOf rdf:resource="jc3iedmSubOnt.owl#CONSUMABLE-MATERIEL-TYPE-POL"/>
    <rdfs:subClassOf>
      <owl:Restriction>
        <owl:hasValue xml:lang="en">LUBRIC</owl:hasValue>
        <owl:onProperty rdf:resource="jc3iedmBase.owl#consumable-materiel-type-subcategory-code"/>
      </owl:Restriction>
    </rdfs:subClassOf>
    <rdfs:label xml:lang="en">Lubricant</rdfs:label>
    <rdfs:comment xml:lang="en">A material, usually an oil, used to lubricate machinery.</rdfs:comment>
  </owl:Class>
  <owl:Class rdf:ID="Wingtip_drogue">
    <rdfs:subClassOf rdf:resource="jc3iedmSubOnt.owl#MISCELLANEOUS-EQUIPMENT-TYPE-Aircraft_refuelling"/>
    <rdfs:subClassOf>
      <owl:Restriction>
        <owl:hasValue xml:lang="en">WD</owl:hasValue>
        <owl:onProperty rdf:resource="jc3iedmBase.owl#miscellaneous-equipment-type-subcategory-code"/>
      </owl:Restriction>
    </rdfs:subClassOf>
    <rdfs:label xml:lang="en">Wingtip drogue</rdfs:label>
    <rdfs:comment xml:lang="en">A component of a refuelling system by which a wingtip drogue device can provide fuel on a receiver aircraft.</rdfs:comment>
  </owl:Class>
  <owl:Class rdf:about="#Wagon,_ISO_container(s)">
    <rdfs:subClassOf rdf:resource="jc3iedmSubOnt.owl#RAILCAR-TYPE-Rolling_stock"/>
    <rdfs:subClassOf>
      <owl:Restriction>
        <owl:hasValue xml:lang="en">WGNISO</owl:hasValue>
        <owl:onProperty rdf:resource="jc3iedmBase.owl#railcar-type-subcategory-code"/>
      </owl:Restriction>
    </rdfs:subClassOf>
    <rdfs:label xml:lang="en">Wagon, ISO container(s)</rdfs:label>
    <rdfs:comment xml:lang="en">Rolling stock used to move standard ISO containers, either single or multiple containers.</rdfs:comment>
  </owl:Class>
  <owl:Class rdf:ID="Machine_pistol">
    <rdfs:subClassOf rdf:resource="jc3iedmSubOnt.owl#WEAPON-TYPE-Small_arms"/>
    <rdfs:subClassOf>
      <owl:Restriction>
        <owl:hasValue xml:lang="en">MCHPTL</owl:hasValue>
        <owl:onProperty rdf:resource="jc3iedmBase.owl#weapon-type-subcategory-code"/>
      </owl:Restriction>
    </rdfs:subClassOf>
    <rdfs:label xml:lang="en">Machine pistol</rdfs:label>
    <rdfs:comment xml:lang="en">A small hand-held firearm capable of giving continuous fire.</rdfs:comment>
  </owl:Class>
  <owl:Class rdf:about="#Sweep,_hovercraft_mechanical">
    <rdfs:subClassOf rdf:resource="jc3iedmSubOnt.owl#MARITIME-EQUIPMENT-TYPE-Sweep"/>
    <rdfs:subClassOf>
      <owl:Restriction>
        <owl:hasValue xml:lang="en">SWPHVE</owl:hasValue>
        <owl:onProperty rdf:resource="jc3iedmBase.owl#maritime-equipment-type-subcategory-code"/>
      </owl:Restriction>
    </rdfs:subClassOf>
    <rdfs:label xml:lang="en">Sweep, hovercraft mechanical</rdfs:label>
    <rdfs:comment xml:lang="en">Equipment mounted on a hovercraft designed to locate mines in the lane swept by mechanical means.</rdfs:comment>
  </owl:Class>
  <owl:Class rdf:ID="Anti-tank_missile_launcher">
    <rdfs:subClassOf rdf:resource="jc3iedmSubOnt.owl#WEAPON-TYPE-Missile_system"/>
    <rdfs:subClassOf rdf:resource="jc3iedmSubOnt.owl#WEAPON-TYPE-Anti-tank"/>
    <rdfs:subClassOf>
      <owl:Restriction>
        <owl:hasValue xml:lang="en">ATMIS</owl:hasValue>
        <owl:onProperty rdf:resource="jc3iedmBase.owl#weapon-type-subcategory-code"/>
      </owl:Restriction>
    </rdfs:subClassOf>
    <rdfs:label xml:lang="en">Anti-tank missile launcher</rdfs:label>
    <rdfs:comment xml:lang="en">A structural device designed to support and hold an anti-tank missile in position for firing.</rdfs:comment>
    <rdfs:subClassOf>
      <owl:Restriction>
        <owl:hasValue xml:lang="en">ATMIS</owl:hasValue>
        <owl:onProperty rdf:resource="jc3iedmBase.owl#weapon-type-subcategory-code"/>
      </owl:Restriction>
    </rdfs:subClassOf>
  </owl:Class>
  <owl:Class rdf:about="#Artillery,_heavy">
    <rdfs:subClassOf rdf:resource="jc3iedmSubOnt.owl#WEAPON-TYPE-Field_artillery"/>
    <rdfs:subClassOf>
      <owl:Restriction>
        <owl:hasValue xml:lang="en">ARTHEV</owl:hasValue>
        <owl:onProperty rdf:resource="jc3iedmBase.owl#weapon-type-subcategory-code"/>
      </owl:Restriction>
    </rdfs:subClassOf>
    <rdfs:label xml:lang="en">Artillery, heavy</rdfs:label>
    <rdfs:comment xml:lang="en">Field artillery cannon with a calibre normally between 161mm and 210mm.</rdfs:comment>
  </owl:Class>
  <owl:Class rdf:ID="Directory">
    <rdfs:subClassOf rdf:resource="jc3iedmSubOnt.owl#NETWORK-SERVICE-Message_handling_service"/>
    <rdfs:subClassOf>
      <owl:Restriction>
        <owl:hasValue xml:lang="en">DRCTRY</owl:hasValue>
        <owl:onProperty rdf:resource="jc3iedmBase.owl#network-service-subcategory-code"/>
      </owl:Restriction>
    </rdfs:subClassOf>
    <rdfs:label xml:lang="en">Directory</rdfs:label>
    <rdfs:comment xml:lang="en">A service provided through capabilities used by OSI applications, OSI management processes, other OSI layer entities, and telecommunication services, providing a dynamic "name-to-address mapping".</rdfs:comment>
  </owl:Class>
  <owl:Class rdf:about="#Wagon,_car_transporter">
    <rdfs:subClassOf rdf:resource="jc3iedmSubOnt.owl#RAILCAR-TYPE-Rolling_stock"/>
    <rdfs:subClassOf>
      <owl:Restriction>
        <owl:hasValue xml:lang="en">WGNCAR</owl:hasValue>
        <owl:onProperty rdf:resource="jc3iedmBase.owl#railcar-type-subcategory-code"/>
      </owl:Restriction>
    </rdfs:subClassOf>
    <rdfs:label xml:lang="en">Wagon, car transporter</rdfs:label>
    <rdfs:comment xml:lang="en">Rolling stock specifically designed to carry civilian or military cars by rail (for example EURORAIL).</rdfs:comment>
  </owl:Class>
  <owl:Class rdf:ID="Intercept_receiver">
    <rdfs:subClassOf rdf:resource="jc3iedmSubOnt.owl#ELECTRONIC-EQUIPMENT-TYPE-Electronic_warfare"/>
    <rdfs:subClassOf>
      <owl:Restriction>
        <owl:hasValue xml:lang="en">INTERC</owl:hasValue>
        <owl:onProperty rdf:resource="jc3iedmBase.owl#electronic-equipment-type-subcategory-code"/>
      </owl:Restriction>
    </rdfs:subClassOf>
    <rdfs:label xml:lang="en">Intercept receiver</rdfs:label>
    <rdfs:comment xml:lang="en">A receiver utilising the electromagnetic spectrum for the interception of speech and data information.</rdfs:comment>
  </owl:Class>
  <owl:Class rdf:about="#Jungle,_coastal/estuary">
    <rdfs:label xml:lang="en">Jungle, coastal/estuary</rdfs:label>
    <rdfs:comment xml:lang="en">An area of jungle on generally swampy ground where movement is slow and difficult.</rdfs:comment>
  </owl:Class>
  <owl:Class rdf:ID="Chloropicrin">
    <rdfs:subClassOf rdf:resource="jc3iedmSubOnt.owl#CHEMICAL-MATERIEL-TYPE-Incapacitating_agent"/>
    <rdfs:subClassOf>
      <owl:Restriction>
        <owl:hasValue xml:lang="en">CHLRPC</owl:hasValue>
        <owl:onProperty rdf:resource="jc3iedmBase.owl#chemical-materiel-type-subcategory-code"/>
      </owl:Restriction>
    </rdfs:subClassOf>
    <rdfs:label xml:lang="en">Chloropicrin</rdfs:label>
    <rdfs:comment xml:lang="en">A poisonous gas made by the reaction of some chloro compounds with nitrated phenol.</rdfs:comment>
  </owl:Class>
  <owl:Class rdf:ID="UN_Dangerous_Goods_NUM_3331">
    <rdfs:subClassOf>
      <owl:Restriction>
        <owl:hasValue xml:lang="en">3331</owl:hasValue>
        <owl:onProperty rdf:resource="jc3iedmBase.owl#consumable-materiel-type-united-nations-number-code"/>
      </owl:Restriction>
    </rdfs:subClassOf>
    <rdfs:label xml:lang="en">UN Dangerous Goods # 3331</rdfs:label>
    <rdfs:comment xml:lang="en">Radioactive material, transported under special arrangement, fissile.</rdfs:comment>
  </owl:Class>
  <owl:Class rdf:ID="UN_Dangerous_Goods_NUM_3322">
    <rdfs:subClassOf>
      <owl:Restriction>
        <owl:hasValue xml:lang="en">3322</owl:hasValue>
        <owl:onProperty rdf:resource="jc3iedmBase.owl#consumable-materiel-type-united-nations-number-code"/>
      </owl:Restriction>
    </rdfs:subClassOf>
    <rdfs:label xml:lang="en">UN Dangerous Goods # 3322</rdfs:label>
    <rdfs:comment xml:lang="en">Radioactive material, low specific activity (LSA-III), non fissile or fissile-excepted.</rdfs:comment>
  </owl:Class>
  <owl:Class rdf:ID="Sonar">
    <rdfs:subClassOf rdf:resource="jc3iedmSubOnt.owl#ELECTRONIC-EQUIPMENT-TYPE-Sensor"/>
    <rdfs:subClassOf>
      <owl:Restriction>
        <owl:hasValue xml:lang="en">SONAR</owl:hasValue>
        <owl:onProperty rdf:resource="jc3iedmBase.owl#electronic-equipment-type-subcategory-code"/>
      </owl:Restriction>
    </rdfs:subClassOf>
    <rdfs:label xml:lang="en">Sonar</rdfs:label>
    <rdfs:comment xml:lang="en">SOund NAvigation Ranging. A sonic device used primarily for the detection and location of underwater objects.</rdfs:comment>
  </owl:Class>
  <owl:Class rdf:about="#Very_sensitive,_anti_sweeper">
    <rdfs:subClassOf rdf:resource="jc3iedmSubOnt.owl#AMMUNITION-TYPE-Sea_mine"/>
    <rdfs:subClassOf rdf:resource="jc3iedmSubOnt.owl#AMMUNITION-TYPE-Mine,_shallow_moored"/>
    <rdfs:subClassOf rdf:resource="jc3iedmSubOnt.owl#AMMUNITION-TYPE-Mine,_moored"/>
    <rdfs:subClassOf>
      <owl:Restriction>
        <owl:hasValue xml:lang="en">VERSEN</owl:hasValue>
        <owl:onProperty rdf:resource="jc3iedmBase.owl#ammunition-type-mine-maritime-firing-code"/>
      </owl:Restriction>
    </rdfs:subClassOf>
    <rdfs:subClassOf rdf:resource="jc3iedmSubOnt.owl#AMMUNITION-TYPE-Mine,_maritime,_moving"/>
    <rdfs:subClassOf rdf:resource="jc3iedmSubOnt.owl#AMMUNITION-TYPE-Mine,_seabed_-_explosive_charge_less_than_500kg"/>
    <rdfs:subClassOf rdf:resource="jc3iedmSubOnt.owl#AMMUNITION-TYPE-Moving_mine,_sea"/>
    <rdfs:subClassOf>
      <owl:Restriction>
        <owl:hasValue xml:lang="en">VERSEN</owl:hasValue>
        <owl:onProperty rdf:resource="jc3iedmBase.owl#ammunition-type-mine-maritime-firing-code"/>
      </owl:Restriction>
    </rdfs:subClassOf>
    <rdfs:subClassOf rdf:resource="jc3iedmSubOnt.owl#AMMUNITION-TYPE-Mine,_seabed_-_explosive_charge_500kg_or_greater"/>
    <rdfs:subClassOf rdf:resource="jc3iedmSubOnt.owl#AMMUNITION-TYPE-Mine,_not_otherwise_specified"/>
    <rdfs:subClassOf rdf:resource="jc3iedmSubOnt.owl#AMMUNITION-TYPE-Mine,_not_known"/>
    <rdfs:subClassOf rdf:resource="jc3iedmSubOnt.owl#AMMUNITION-TYPE-Mine,_deep_moored"/>
    <rdfs:subClassOf rdf:resource="jc3iedmSubOnt.owl#AMMUNITION-TYPE-Seabed_mine"/>
    <rdfs:label xml:lang="en">Very sensitive, anti sweeper</rdfs:label>
    <rdfs:comment xml:lang="en">A (maritime) mine firing mechanism that is fitted with a sensitive firing mechanism that react to a small influences of pressure, acoustic or magnetic (for magnetic values of less than 200 nanotesla are sufficient.)</rdfs:comment>
  </owl:Class>
  <owl:Class rdf:ID="Shipboard_emitter_locator">
    <rdfs:subClassOf rdf:resource="jc3iedmSubOnt.owl#ELECTRONIC-EQUIPMENT-TYPE-Navigational_aid"/>
    <rdfs:subClassOf>
      <owl:Restriction>
        <owl:hasValue xml:lang="en">SHETLC</owl:hasValue>
        <owl:onProperty rdf:resource="jc3iedmBase.owl#electronic-equipment-type-subcategory-code"/>
      </owl:Restriction>
    </rdfs:subClassOf>
    <rdfs:label xml:lang="en">Shipboard emitter locator</rdfs:label>
    <rdfs:comment xml:lang="en">No definition provided in ADatP-3 Baseline 13.1 FFIRN/FUD 1434/1.</rdfs:comment>
  </owl:Class>
  <owl:Class rdf:about="#Battle-tank,_medium">
    <rdfs:subClassOf rdf:resource="jc3iedmSubOnt.owl#WEAPON-TYPE-Tank"/>
    <rdfs:subClassOf>
      <owl:Restriction>
        <owl:hasValue xml:lang="en">BTNKME</owl:hasValue>
        <owl:onProperty rdf:resource="jc3iedmBase.owl#weapon-type-subcategory-code"/>
      </owl:Restriction>
    </rdfs:subClassOf>
    <rdfs:label xml:lang="en">Battle-tank, medium</rdfs:label>
    <rdfs:comment xml:lang="en">An armoured fighting vehicle of more than 20 and less than 50 metric tons which, as its primary function, is designed to close with the enemy and engage their armour and infantry with direct fire.</rdfs:comment>
  </owl:Class>
  <owl:Class rdf:about="#Sweep,_mechanical_team">
    <rdfs:subClassOf rdf:resource="jc3iedmSubOnt.owl#MARITIME-EQUIPMENT-TYPE-Sweep"/>
    <rdfs:subClassOf>
      <owl:Restriction>
        <owl:hasValue xml:lang="en">SWPMCT</owl:hasValue>
        <owl:onProperty rdf:resource="jc3iedmBase.owl#maritime-equipment-type-subcategory-code"/>
      </owl:Restriction>
    </rdfs:subClassOf>
    <rdfs:label xml:lang="en">Sweep, mechanical team</rdfs:label>
    <rdfs:comment xml:lang="en">Equipment designed to locate mines by towing either a mechanical or influence gear through the liquid with the intention of cutting or destruction of mines. Sweep wire towed between two or more ships using only kites to keep the sweep down.</rdfs:comment>
  </owl:Class>
  <owl:Class rdf:ID="UN_Dangerous_Goods_NUM_2910">
    <rdfs:subClassOf>
      <owl:Restriction>
        <owl:hasValue xml:lang="en">2910</owl:hasValue>
        <owl:onProperty rdf:resource="jc3iedmBase.owl#consumable-materiel-type-united-nations-number-code"/>
      </owl:Restriction>
    </rdfs:subClassOf>
    <rdfs:label xml:lang="en">UN Dangerous Goods # 2910</rdfs:label>
    <rdfs:comment xml:lang="en">Radioactive material, excepted package - limited quantity of material.</rdfs:comment>
  </owl:Class>
  <owl:Class rdf:about="#Surface-to-surface_missile_launcher,_medium_range">
    <rdfs:subClassOf rdf:resource="jc3iedmSubOnt.owl#WEAPON-TYPE-Missile_system"/>
    <rdfs:subClassOf>
      <owl:Restriction>
        <owl:hasValue xml:lang="en">SSMLMR</owl:hasValue>
        <owl:onProperty rdf:resource="jc3iedmBase.owl#weapon-type-subcategory-code"/>
      </owl:Restriction>
    </rdfs:subClassOf>
    <rdfs:label xml:lang="en">Surface-to-surface missile launcher, medium range</rdfs:label>
    <rdfs:comment xml:lang="en">A structural device designed to support and hold a medium range surface to surface missile in position for firing.</rdfs:comment>
  </owl:Class>
  <owl:Class rdf:about="#Battle-tank,_heavy">
    <rdfs:subClassOf rdf:resource="jc3iedmSubOnt.owl#WEAPON-TYPE-Tank"/>
    <rdfs:subClassOf>
      <owl:Restriction>
        <owl:hasValue xml:lang="en">BTNKHE</owl:hasValue>
        <owl:onProperty rdf:resource="jc3iedmBase.owl#weapon-type-subcategory-code"/>
      </owl:Restriction>
    </rdfs:subClassOf>
    <rdfs:label xml:lang="en">Battle-tank, heavy</rdfs:label>
    <rdfs:comment xml:lang="en">An armoured fighting vehicle of more than 50 metric tons which, as its primary function, is designed to close with the enemy and engage their armour and infantry with direct fire.</rdfs:comment>
  </owl:Class>
  <owl:Class rdf:ID="UN_Dangerous_Goods_NUM_2810">
    <rdfs:subClassOf>
      <owl:Restriction>
        <owl:hasValue xml:lang="en">2810</owl:hasValue>
        <owl:onProperty rdf:resource="jc3iedmBase.owl#consumable-materiel-type-united-nations-number-code"/>
      </owl:Restriction>
    </rdfs:subClassOf>
    <rdfs:label xml:lang="en">UN Dangerous Goods # 2810</rdfs:label>
    <rdfs:comment xml:lang="en">Toxic liquid, organic, N.O.S. Includes the agent(s): Tabun, Sarin, Soman, Cyclosarin, Mustard (Bis(2-chloroethyl)sulphide), Nitrogen Mustard (HN-1), Nitrogen Mustard (HN-2), Nitrogen Mustard (HN-3), thickened tabun, Thickened Soman, Thickened Cyclosarin, Thickened S+D23ulphur Mustard, Thickened VX, VX, Sulphur Mustard-T mixture, Levinstein mustard, Vx.</rdfs:comment>
    <rdfs:subClassOf>
      <owl:Restriction>
        <owl:hasValue xml:lang="en">2810</owl:hasValue>
        <owl:onProperty rdf:resource="jc3iedmBase.owl#consumable-materiel-type-united-nations-number-code"/>
      </owl:Restriction>
    </rdfs:subClassOf>
  </owl:Class>
  <owl:Class rdf:about="#Underground_water/phreatic_water">
    <rdfs:subClassOf rdf:resource="jc3iedmSubOnt.owl#GEOGRAPHIC-FEATURE-TYPE-Inland_water"/>
    <rdfs:subClassOf rdf:resource="jc3iedmSubOnt.owl#GEOGRAPHIC-FEATURE-Liquid_surface"/>
    <rdfs:subClassOf>
      <owl:Restriction>
        <owl:hasValue xml:lang="en">UNDRGW</owl:hasValue>
        <owl:onProperty rdf:resource="jc3iedmBase.owl#geographic-feature-type-subcategory-code"/>
      </owl:Restriction>
    </rdfs:subClassOf>
    <rdfs:label xml:lang="en">Underground water/phreatic water</rdfs:label>
    <rdfs:comment xml:lang="en">Water situated underground but reachable by wells.</rdfs:comment>
    <rdfs:subClassOf>
      <owl:Restriction>
        <owl:hasValue xml:lang="en">UNDRGW</owl:hasValue>
        <owl:onProperty rdf:resource="jc3iedmBase.owl#geographic-feature-type-subcategory-code"/>
      </owl:Restriction>
    </rdfs:subClassOf>
  </owl:Class>
  <owl:Class rdf:ID="Dry_gap">
    <rdfs:subClassOf rdf:resource="jc3iedmSubOnt.owl#GEOGRAPHIC-FEATURE-Solid_surface"/>
    <rdfs:subClassOf rdf:resource="jc3iedmSubOnt.owl#GEOGRAPHIC-FEATURE-TYPE-Landform"/>
    <rdfs:subClassOf>
      <owl:Restriction>
        <owl:hasValue xml:lang="en">DRYGAP</owl:hasValue>
        <owl:onProperty rdf:resource="jc3iedmBase.owl#geographic-feature-type-subcategory-code"/>
      </owl:Restriction>
    </rdfs:subClassOf>
    <rdfs:label xml:lang="en">Dry gap</rdfs:label>
    <rdfs:comment xml:lang="en">A waterless ravine or mountain pass.</rdfs:comment>
    <rdfs:subClassOf>
      <owl:Restriction>
        <owl:hasValue xml:lang="en">DRYGAP</owl:hasValue>
        <owl:onProperty rdf:resource="jc3iedmBase.owl#geographic-feature-type-subcategory-code"/>
      </owl:Restriction>
    </rdfs:subClassOf>
  </owl:Class>
  <owl:Class rdf:ID="Nearshore">
    <rdfs:subClassOf rdf:resource="jc3iedmSubOnt.owl#GEOGRAPHIC-FEATURE-Solid_surface"/>
    <rdfs:subClassOf rdf:resource="jc3iedmSubOnt.owl#GEOGRAPHIC-FEATURE-TYPE-Coastal_hydrography"/>
    <rdfs:subClassOf>
      <owl:Restriction>
        <owl:hasValue xml:lang="en">NRSHRE</owl:hasValue>
        <owl:onProperty rdf:resource="jc3iedmBase.owl#geographic-feature-type-subcategory-code"/>
      </owl:Restriction>
    </rdfs:subClassOf>
    <rdfs:label xml:lang="en">Nearshore</rdfs:label>
    <rdfs:comment xml:lang="en">Area between the 10 meter depth curve and the low water line defined by either Mean Low Water Springs (MLWS) or Mean Low Low Water (MLLW) as defined by the National Authority and the International Hydrographic Organisation.</rdfs:comment>
    <rdfs:subClassOf>
      <owl:Restriction>
        <owl:hasValue xml:lang="en">NRSHRE</owl:hasValue>
        <owl:onProperty rdf:resource="jc3iedmBase.owl#geographic-feature-type-subcategory-code"/>
      </owl:Restriction>
    </rdfs:subClassOf>
  </owl:Class>
  <owl:Class rdf:about="#Radar,_high_resolution">
    <rdfs:subClassOf rdf:resource="jc3iedmSubOnt.owl#ELECTRONIC-EQUIPMENT-TYPE-Radar"/>
    <rdfs:subClassOf rdf:resource="jc3iedmSubOnt.owl#ELECTRONIC-EQUIPMENT-TYPE-Navigational_aid"/>
    <rdfs:subClassOf>
      <owl:Restriction>
        <owl:hasValue xml:lang="en">RDRHRL</owl:hasValue>
        <owl:onProperty rdf:resource="jc3iedmBase.owl#electronic-equipment-type-subcategory-code"/>
      </owl:Restriction>
    </rdfs:subClassOf>
    <rdfs:label xml:lang="en">Radar, high resolution</rdfs:label>
    <rdfs:comment xml:lang="en">A radar that provides detailed information on the size and shape of a target and surface imaging.</rdfs:comment>
    <rdfs:subClassOf>
      <owl:Restriction>
        <owl:hasValue xml:lang="en">RDRHRL</owl:hasValue>
        <owl:onProperty rdf:resource="jc3iedmBase.owl#electronic-equipment-type-subcategory-code"/>
      </owl:Restriction>
    </rdfs:subClassOf>
  </owl:Class>
  <owl:Class rdf:ID="Burned_out">
    <rdfs:subClassOf>
      <owl:Restriction>
        <owl:hasValue xml:lang="en">BRNOUT</owl:hasValue>
        <owl:onProperty rdf:resource="jc3iedmBase.owl#facility-status-operational-status-qualifier-code"/>
      </owl:Restriction>
    </rdfs:subClassOf>
    <rdfs:label xml:lang="en">Burned out</rdfs:label>
    <rdfs:comment xml:lang="en">Subjectively judged by the reporting organisation that a FACILITY has been set on fire and is destroyed.</rdfs:comment>
  </owl:Class>
  <owl:Class rdf:ID="Paint">
    <rdfs:subClassOf rdf:resource="jc3iedmSubOnt.owl#CONSUMABLE-MATERIEL-TYPE-General_supplies"/>
    <rdfs:subClassOf>
      <owl:Restriction>
        <owl:hasValue xml:lang="en">PAINT</owl:hasValue>
        <owl:onProperty rdf:resource="jc3iedmBase.owl#consumable-materiel-type-subcategory-code"/>
      </owl:Restriction>
    </rdfs:subClassOf>
    <rdfs:label xml:lang="en">Paint</rdfs:label>
    <rdfs:comment xml:lang="en">A substance consisting of a solid colouring matter dissolved in a liquid vehicle, as water or oil, used to impart a colour by being spread over a surface.</rdfs:comment>
  </owl:Class>
  <owl:Class rdf:about="#Sonar,_passive">
    <rdfs:subClassOf rdf:resource="jc3iedmSubOnt.owl#MARITIME-EQUIPMENT-TYPE-Sonar,_maritime"/>
    <rdfs:subClassOf>
      <owl:Restriction>
        <owl:hasValue xml:lang="en">SONRPS</owl:hasValue>
        <owl:onProperty rdf:resource="jc3iedmBase.owl#maritime-equipment-type-subcategory-code"/>
      </owl:Restriction>
    </rdfs:subClassOf>
    <rdfs:label xml:lang="en">Sonar, passive</rdfs:label>
    <rdfs:comment xml:lang="en">A system that detects acoustic radiation from another vessel or object.</rdfs:comment>
  </owl:Class>
  <owl:Class rdf:ID="Dirigible">
    <rdfs:subClassOf rdf:resource="jc3iedmSubOnt.owl#AIRCRAFT-TYPE-Lighter_than_air"/>
    <rdfs:subClassOf>
      <owl:Restriction>
        <owl:hasValue xml:lang="en">DIRIG</owl:hasValue>
        <owl:onProperty rdf:resource="jc3iedmBase.owl#aircraft-type-airframe-design-code"/>
      </owl:Restriction>
    </rdfs:subClassOf>
    <rdfs:label xml:lang="en">Dirigible</rdfs:label>
    <rdfs:comment xml:lang="en">A powered lighter than air aircraft.</rdfs:comment>
  </owl:Class>
  <owl:Class rdf:ID="Pager">
    <rdfs:subClassOf rdf:resource="jc3iedmSubOnt.owl#NETWORK-SERVICE-Message_handling_service"/>
    <rdfs:subClassOf>
      <owl:Restriction>
        <owl:hasValue xml:lang="en">PAGER</owl:hasValue>
        <owl:onProperty rdf:resource="jc3iedmBase.owl#network-service-subcategory-code"/>
      </owl:Restriction>
    </rdfs:subClassOf>
    <rdfs:label xml:lang="en">Pager</rdfs:label>
    <rdfs:comment xml:lang="en">A communications service making use of a small radio device which bleeps or vibrates to inform the wearer that someone wishes to contact them or that it has received a short text message.</rdfs:comment>
  </owl:Class>
  <owl:Class rdf:ID="Boom_and_wingtip_drogue">
    <rdfs:subClassOf rdf:resource="jc3iedmSubOnt.owl#MISCELLANEOUS-EQUIPMENT-TYPE-Aircraft_refuelling"/>
    <rdfs:subClassOf>
      <owl:Restriction>
        <owl:hasValue xml:lang="en">BWD</owl:hasValue>
        <owl:onProperty rdf:resource="jc3iedmBase.owl#miscellaneous-equipment-type-subcategory-code"/>
      </owl:Restriction>
    </rdfs:subClassOf>
    <rdfs:label xml:lang="en">Boom and wingtip drogue</rdfs:label>
    <rdfs:comment xml:lang="en">Two components of a refuelling system by which a boom and a wingtip drogue devices provide fuel on a receiver aircraft.</rdfs:comment>
  </owl:Class>
  <owl:Class rdf:ID="UN_Dangerous_Goods_NUM_3323">
    <rdfs:subClassOf>
      <owl:Restriction>
        <owl:hasValue xml:lang="en">3323</owl:hasValue>
        <owl:onProperty rdf:resource="jc3iedmBase.owl#consumable-materiel-type-united-nations-number-code"/>
      </owl:Restriction>
    </rdfs:subClassOf>
    <rdfs:label xml:lang="en">UN Dangerous Goods # 3323</rdfs:label>
    <rdfs:comment xml:lang="en">Radioactive material, type C package, non fissile or fissile-excepted.</rdfs:comment>
  </owl:Class>
  <owl:Class rdf:ID="UN_Dangerous_Goods_NUM_2188">
    <rdfs:subClassOf>
      <owl:Restriction>
        <owl:hasValue xml:lang="en">2188</owl:hasValue>
        <owl:onProperty rdf:resource="jc3iedmBase.owl#consumable-materiel-type-united-nations-number-code"/>
      </owl:Restriction>
    </rdfs:subClassOf>
    <rdfs:label xml:lang="en">UN Dangerous Goods # 2188</rdfs:label>
    <rdfs:comment xml:lang="en">Arsine. Includes the agent(s): arsine.</rdfs:comment>
    <rdfs:subClassOf>
      <owl:Restriction>
        <owl:hasValue xml:lang="en">2188</owl:hasValue>
        <owl:onProperty rdf:resource="jc3iedmBase.owl#consumable-materiel-type-united-nations-number-code"/>
      </owl:Restriction>
    </rdfs:subClassOf>
  </owl:Class>
  <owl:Class rdf:about="#Water_(except_inland)">
    <rdfs:subClassOf rdf:resource="jc3iedmSubOnt.owl#GEOGRAPHIC-FEATURE-TYPE-Coastal_hydrography"/>
    <rdfs:subClassOf rdf:resource="jc3iedmSubOnt.owl#GEOGRAPHIC-FEATURE-Liquid_surface"/>
    <rdfs:subClassOf>
      <owl:Restriction>
        <owl:hasValue xml:lang="en">WATER</owl:hasValue>
        <owl:onProperty rdf:resource="jc3iedmBase.owl#geographic-feature-type-subcategory-code"/>
      </owl:Restriction>
    </rdfs:subClassOf>
    <rdfs:label xml:lang="en">Water (except inland)</rdfs:label>
    <rdfs:comment xml:lang="en">An area of water that normally has tidal fluctuations.</rdfs:comment>
    <rdfs:subClassOf>
      <owl:Restriction>
        <owl:hasValue xml:lang="en">WATER</owl:hasValue>
        <owl:onProperty rdf:resource="jc3iedmBase.owl#geographic-feature-type-subcategory-code"/>
      </owl:Restriction>
    </rdfs:subClassOf>
  </owl:Class>
  <owl:Class rdf:ID="UN_Dangerous_Goods_NUM_3330">
    <rdfs:subClassOf>
      <owl:Restriction>
        <owl:hasValue xml:lang="en">3330</owl:hasValue>
        <owl:onProperty rdf:resource="jc3iedmBase.owl#consumable-materiel-type-united-nations-number-code"/>
      </owl:Restriction>
    </rdfs:subClassOf>
    <rdfs:label xml:lang="en">UN Dangerous Goods # 3330</rdfs:label>
    <rdfs:comment xml:lang="en">Radioactive material, type C package, fissile.</rdfs:comment>
  </owl:Class>
  <owl:Class rdf:about="#Sonar,_hand_held">
    <rdfs:subClassOf rdf:resource="jc3iedmSubOnt.owl#MARITIME-EQUIPMENT-TYPE-Sonar,_maritime"/>
    <rdfs:subClassOf>
      <owl:Restriction>
        <owl:hasValue xml:lang="en">SONRHH</owl:hasValue>
        <owl:onProperty rdf:resource="jc3iedmBase.owl#maritime-equipment-type-subcategory-code"/>
      </owl:Restriction>
    </rdfs:subClassOf>
    <rdfs:label xml:lang="en">Sonar, hand held</rdfs:label>
    <rdfs:comment xml:lang="en">A hand held acoustic device used primarily for the detection and location of underwater objects.</rdfs:comment>
  </owl:Class>
  <owl:Class rdf:ID="Pins">
    <rdfs:subClassOf rdf:resource="jc3iedmSubOnt.owl#ELECTRONIC-EQUIPMENT-TYPE-Navigational_aid"/>
    <rdfs:subClassOf>
      <owl:Restriction>
        <owl:hasValue xml:lang="en">PINS</owl:hasValue>
        <owl:onProperty rdf:resource="jc3iedmBase.owl#electronic-equipment-type-subcategory-code"/>
      </owl:Restriction>
    </rdfs:subClassOf>
    <rdfs:label xml:lang="en">Pins</rdfs:label>
    <rdfs:comment xml:lang="en">No definition provided in ADatP-3 Baseline 13.1 FFIRN/FUD 1200/1.</rdfs:comment>
  </owl:Class>
  <owl:Class rdf:ID="UN_Dangerous_Goods_NUM_1381">
    <rdfs:subClassOf>
      <owl:Restriction>
        <owl:hasValue xml:lang="en">1381</owl:hasValue>
        <owl:onProperty rdf:resource="jc3iedmBase.owl#consumable-materiel-type-united-nations-number-code"/>
      </owl:Restriction>
    </rdfs:subClassOf>
    <rdfs:label xml:lang="en">UN Dangerous Goods # 1381</rdfs:label>
    <rdfs:comment xml:lang="en">Phosphorus, white or yellow, dry or under water or in solution. Includes the agent(s): white phosphorous.</rdfs:comment>
    <rdfs:subClassOf>
      <owl:Restriction>
        <owl:hasValue xml:lang="en">1381</owl:hasValue>
        <owl:onProperty rdf:resource="jc3iedmBase.owl#consumable-materiel-type-united-nations-number-code"/>
      </owl:Restriction>
    </rdfs:subClassOf>
  </owl:Class>
  <owl:Class rdf:ID="UN_Dangerous_Goods_NUM_2811">
    <rdfs:subClassOf>
      <owl:Restriction>
        <owl:hasValue xml:lang="en">2811</owl:hasValue>
        <owl:onProperty rdf:resource="jc3iedmBase.owl#consumable-materiel-type-united-nations-number-code"/>
      </owl:Restriction>
    </rdfs:subClassOf>
    <rdfs:label xml:lang="en">UN Dangerous Goods # 2811</rdfs:label>
    <rdfs:comment xml:lang="en">Toxic solid, organic, N.O.S. Includes the agent(s) referred to as: Phosgene Oxime; 3-Quinuclidinyl benzilate; Capsaicin.</rdfs:comment>
    <rdfs:subClassOf>
      <owl:Restriction>
        <owl:hasValue xml:lang="en">2811</owl:hasValue>
        <owl:onProperty rdf:resource="jc3iedmBase.owl#consumable-materiel-type-united-nations-number-code"/>
      </owl:Restriction>
    </rdfs:subClassOf>
  </owl:Class>
  <owl:Class rdf:ID="Wire">
    <rdfs:subClassOf rdf:resource="jc3iedmSubOnt.owl#CONSUMABLE-MATERIEL-TYPE-Construction_materials"/>
    <rdfs:subClassOf>
      <owl:Restriction>
        <owl:hasValue xml:lang="en">WIRE</owl:hasValue>
        <owl:onProperty rdf:resource="jc3iedmBase.owl#consumable-materiel-type-subcategory-code"/>
      </owl:Restriction>
    </rdfs:subClassOf>
    <rdfs:label xml:lang="en">Wire</rdfs:label>
    <rdfs:comment xml:lang="en">A pliable metallic strand or rod made in many lengths and diameters.</rdfs:comment>
  </owl:Class>
  <owl:Class rdf:ID="Matting">
    <rdfs:subClassOf rdf:resource="jc3iedmSubOnt.owl#CONSUMABLE-MATERIEL-TYPE-Construction_materials"/>
    <rdfs:subClassOf>
      <owl:Restriction>
        <owl:hasValue xml:lang="en">MATING</owl:hasValue>
        <owl:onProperty rdf:resource="jc3iedmBase.owl#consumable-materiel-type-subcategory-code"/>
      </owl:Restriction>
    </rdfs:subClassOf>
    <rdfs:label xml:lang="en">Matting</rdfs:label>
    <rdfs:comment xml:lang="en">Steel or other material used to construct a supporting surface over ground.</rdfs:comment>
  </owl:Class>
  <owl:Class rdf:ID="Diesel_fuel">
    <rdfs:subClassOf rdf:resource="jc3iedmSubOnt.owl#CONSUMABLE-MATERIEL-TYPE-POL"/>
    <rdfs:subClassOf>
      <owl:Restriction>
        <owl:hasValue xml:lang="en">DIESEL</owl:hasValue>
        <owl:onProperty rdf:resource="jc3iedmBase.owl#consumable-materiel-type-subcategory-code"/>
      </owl:Restriction>
    </rdfs:subClassOf>
    <rdfs:label xml:lang="en">Diesel fuel</rdfs:label>
    <rdfs:comment xml:lang="en">A petroleum fraction intended to be used as fuel in diesel engines.</rdfs:comment>
  </owl:Class>
  <owl:Class rdf:ID="Uniform">
    <rdfs:subClassOf rdf:resource="jc3iedmSubOnt.owl#CONSUMABLE-MATERIEL-TYPE-Personal_equipment"/>
    <rdfs:subClassOf>
      <owl:Restriction>
        <owl:hasValue xml:lang="en">UNIFRM</owl:hasValue>
        <owl:onProperty rdf:resource="jc3iedmBase.owl#consumable-materiel-type-subcategory-code"/>
      </owl:Restriction>
    </rdfs:subClassOf>
    <rdfs:label xml:lang="en">Uniform</rdfs:label>
    <rdfs:comment xml:lang="en">A distinctive dress of uniform cut, materials, and colour worn by all the members of a particular naval, military, or other force to which it is recognised as properly belonging and peculiar.</rdfs:comment>
  </owl:Class>
  <owl:Class rdf:ID="IFF_mode_S">
    <rdfs:subClassOf rdf:resource="jc3iedmSubOnt.owl#NETWORK-SERVICE-Identification_friend_or_foe"/>
    <rdfs:subClassOf>
      <owl:Restriction>
        <owl:hasValue xml:lang="en">IFFMS</owl:hasValue>
        <owl:onProperty rdf:resource="jc3iedmBase.owl#network-service-subcategory-code"/>
      </owl:Restriction>
    </rdfs:subClassOf>
    <rdfs:label xml:lang="en">IFF mode S</rdfs:label>
    <rdfs:comment xml:lang="en">A service that provides the data for IFF mode S.</rdfs:comment>
  </owl:Class>
  <owl:Class rdf:ID="In_maintenance">
    <rdfs:subClassOf>
      <owl:Restriction>
        <owl:hasValue xml:lang="en">INMNT</owl:hasValue>
        <owl:onProperty rdf:resource="jc3iedmBase.owl#materiel-status-operational-status-qualifier-code"/>
      </owl:Restriction>
    </rdfs:subClassOf>
    <rdfs:label xml:lang="en">In maintenance</rdfs:label>
    <rdfs:comment xml:lang="en">Subjectively judged by the reporting organisation that a specific materiel is under some kind of service.</rdfs:comment>
    <rdfs:subClassOf>
      <owl:Restriction>
        <owl:hasValue xml:lang="en">INMNT</owl:hasValue>
        <owl:onProperty rdf:resource="jc3iedmBase.owl#facility-status-operational-status-qualifier-code"/>
      </owl:Restriction>
    </rdfs:subClassOf>
    <rdfs:subClassOf>
      <owl:Restriction>
        <owl:hasValue xml:lang="en">INMNT</owl:hasValue>
        <owl:onProperty rdf:resource="jc3iedmBase.owl#facility-status-operational-status-qualifier-code"/>
      </owl:Restriction>
    </rdfs:subClassOf>
    <rdfs:subClassOf>
      <owl:Restriction>
        <owl:hasValue xml:lang="en">INMNT</owl:hasValue>
        <owl:onProperty rdf:resource="jc3iedmBase.owl#facility-status-operational-status-qualifier-code"/>
      </owl:Restriction>
    </rdfs:subClassOf>
  </owl:Class>
  <owl:Class rdf:about="#Spring/water_hole">
    <rdfs:subClassOf rdf:resource="jc3iedmSubOnt.owl#GEOGRAPHIC-FEATURE-TYPE-Inland_water"/>
    <rdfs:subClassOf rdf:resource="jc3iedmSubOnt.owl#GEOGRAPHIC-FEATURE-Liquid_surface"/>
    <rdfs:subClassOf>
      <owl:Restriction>
        <owl:hasValue xml:lang="en">SPRING</owl:hasValue>
        <owl:onProperty rdf:resource="jc3iedmBase.owl#geographic-feature-type-subcategory-code"/>
      </owl:Restriction>
    </rdfs:subClassOf>
    <rdfs:label xml:lang="en">Spring/water hole</rdfs:label>
    <rdfs:comment xml:lang="en">A natural outflow of water from below the ground surface.</rdfs:comment>
    <rdfs:subClassOf>
      <owl:Restriction>
        <owl:hasValue xml:lang="en">SPRING</owl:hasValue>
        <owl:onProperty rdf:resource="jc3iedmBase.owl#geographic-feature-type-subcategory-code"/>
      </owl:Restriction>
    </rdfs:subClassOf>
  </owl:Class>
  <owl:Class rdf:ID="UN_Dangerous_Goods_NUM_1080">
    <rdfs:subClassOf>
      <owl:Restriction>
        <owl:hasValue xml:lang="en">1080</owl:hasValue>
        <owl:onProperty rdf:resource="jc3iedmBase.owl#consumable-materiel-type-united-nations-number-code"/>
      </owl:Restriction>
    </rdfs:subClassOf>
    <rdfs:label xml:lang="en">UN Dangerous Goods # 1080</rdfs:label>
    <rdfs:comment xml:lang="en">Sulphur hexafluoride. Includes the agent(s): sulphur hexafluoride.</rdfs:comment>
    <rdfs:subClassOf>
      <owl:Restriction>
        <owl:hasValue xml:lang="en">1080</owl:hasValue>
        <owl:onProperty rdf:resource="jc3iedmBase.owl#consumable-materiel-type-united-nations-number-code"/>
      </owl:Restriction>
    </rdfs:subClassOf>
  </owl:Class>
  <owl:Class rdf:about="#Sweep,_mechanical">
    <rdfs:subClassOf rdf:resource="jc3iedmSubOnt.owl#MARITIME-EQUIPMENT-TYPE-Sweep"/>
    <rdfs:subClassOf>
      <owl:Restriction>
        <owl:hasValue xml:lang="en">SWPMEC</owl:hasValue>
        <owl:onProperty rdf:resource="jc3iedmBase.owl#maritime-equipment-type-subcategory-code"/>
      </owl:Restriction>
    </rdfs:subClassOf>
    <rdfs:label xml:lang="en">Sweep, mechanical</rdfs:label>
    <rdfs:comment xml:lang="en">Equipment designed to locate mines in the lane swept by mechanical means.</rdfs:comment>
  </owl:Class>
  <owl:Class rdf:about="#Howitzer,_medium">
    <rdfs:subClassOf rdf:resource="jc3iedmSubOnt.owl#WEAPON-TYPE-Field_artillery"/>
    <rdfs:subClassOf rdf:resource="jc3iedmSubOnt.owl#WEAPON-TYPE-Cannon"/>
    <rdfs:subClassOf>
      <owl:Restriction>
        <owl:hasValue xml:lang="en">HOWTMD</owl:hasValue>
        <owl:onProperty rdf:resource="jc3iedmBase.owl#weapon-type-subcategory-code"/>
      </owl:Restriction>
    </rdfs:subClassOf>
    <rdfs:label xml:lang="en">Howitzer, medium</rdfs:label>
    <rdfs:comment xml:lang="en">A medium cannon that combines certain characteristics of guns and mortars. Normally a cannon with a tube length of 20 to 30 calibres; however, the tube length can exceed 30 calibres and still be considered a howitzer when the high angle firing zoning solution permits range overlap between charges.</rdfs:comment>
    <rdfs:subClassOf>
      <owl:Restriction>
        <owl:hasValue xml:lang="en">HOWTMD</owl:hasValue>
        <owl:onProperty rdf:resource="jc3iedmBase.owl#weapon-type-subcategory-code"/>
      </owl:Restriction>
    </rdfs:subClassOf>
  </owl:Class>
  <owl:Class rdf:ID="Lost">
    <rdfs:subClassOf>
      <owl:Restriction>
        <owl:hasValue xml:lang="en">LST</owl:hasValue>
        <owl:onProperty rdf:resource="jc3iedmBase.owl#organisation-status-operational-status-qualifier-code"/>
      </owl:Restriction>
    </rdfs:subClassOf>
    <rdfs:label xml:lang="en">Lost</rdfs:label>
    <rdfs:comment xml:lang="en">Subjectively judged by the reporting organisation that a specific organisation is missing under unknown circumstances.</rdfs:comment>
    <rdfs:subClassOf>
      <owl:Restriction>
        <owl:hasValue xml:lang="en">LST</owl:hasValue>
        <owl:onProperty rdf:resource="jc3iedmBase.owl#facility-status-operational-status-qualifier-code"/>
      </owl:Restriction>
    </rdfs:subClassOf>
    <rdfs:subClassOf>
      <owl:Restriction>
        <owl:hasValue xml:lang="en">LST</owl:hasValue>
        <owl:onProperty rdf:resource="jc3iedmBase.owl#materiel-status-operational-status-qualifier-code"/>
      </owl:Restriction>
    </rdfs:subClassOf>
  </owl:Class>
  <owl:Class rdf:ID="Close_in_weapon_system">
    <rdfs:subClassOf rdf:resource="jc3iedmSubOnt.owl#WEAPON-TYPE-Air-defence"/>
    <rdfs:subClassOf>
      <owl:Restriction>
        <owl:hasValue xml:lang="en">CINWPS</owl:hasValue>
        <owl:onProperty rdf:resource="jc3iedmBase.owl#weapon-type-subcategory-code"/>
      </owl:Restriction>
    </rdfs:subClassOf>
    <rdfs:label xml:lang="en">Close in weapon system</rdfs:label>
    <rdfs:comment xml:lang="en">An anti-aircraft weapon system employed, as a last resort, in the air defence role.</rdfs:comment>
  </owl:Class>
  <owl:Class rdf:ID="UN_Dangerous_Goods_NUM_2032">
    <rdfs:subClassOf>
      <owl:Restriction>
        <owl:hasValue xml:lang="en">2032</owl:hasValue>
        <owl:onProperty rdf:resource="jc3iedmBase.owl#consumable-materiel-type-united-nations-number-code"/>
      </owl:Restriction>
    </rdfs:subClassOf>
    <rdfs:label xml:lang="en">UN Dangerous Goods # 2032</rdfs:label>
    <rdfs:comment xml:lang="en">Nitric acid, red fuming. Includes the agent(s): fuming nitric acid.</rdfs:comment>
    <rdfs:subClassOf>
      <owl:Restriction>
        <owl:hasValue xml:lang="en">2032</owl:hasValue>
        <owl:onProperty rdf:resource="jc3iedmBase.owl#consumable-materiel-type-united-nations-number-code"/>
      </owl:Restriction>
    </rdfs:subClassOf>
  </owl:Class>
  <owl:Class rdf:about="#Radar,_direction_finding">
    <rdfs:subClassOf rdf:resource="jc3iedmSubOnt.owl#ELECTRONIC-EQUIPMENT-TYPE-Radar"/>
    <rdfs:subClassOf rdf:resource="jc3iedmSubOnt.owl#ELECTRONIC-EQUIPMENT-TYPE-Navigational_aid"/>
    <rdfs:subClassOf>
      <owl:Restriction>
        <owl:hasValue xml:lang="en">RDRDFD</owl:hasValue>
        <owl:onProperty rdf:resource="jc3iedmBase.owl#electronic-equipment-type-subcategory-code"/>
      </owl:Restriction>
    </rdfs:subClassOf>
    <rdfs:label xml:lang="en">Radar, direction finding</rdfs:label>
    <rdfs:comment xml:lang="en">The radar used for determining the bearing of an electromagnetic emission.</rdfs:comment>
    <rdfs:subClassOf>
      <owl:Restriction>
        <owl:hasValue xml:lang="en">RDRDFD</owl:hasValue>
        <owl:onProperty rdf:resource="jc3iedmBase.owl#electronic-equipment-type-subcategory-code"/>
      </owl:Restriction>
    </rdfs:subClassOf>
  </owl:Class>
  <owl:Class rdf:about="#Anti-tank_grenade_launcher,_heavy">
    <rdfs:subClassOf rdf:resource="jc3iedmSubOnt.owl#WEAPON-TYPE-Anti-tank"/>
    <rdfs:subClassOf>
      <owl:Restriction>
        <owl:hasValue xml:lang="en">ATGRLH</owl:hasValue>
        <owl:onProperty rdf:resource="jc3iedmBase.owl#weapon-type-subcategory-code"/>
      </owl:Restriction>
    </rdfs:subClassOf>
    <rdfs:label xml:lang="en">Anti-tank grenade launcher, heavy</rdfs:label>
    <rdfs:comment xml:lang="en">A heavy structural device designed to support and hold an anti-tank grenade in position for firing.</rdfs:comment>
  </owl:Class>
  <owl:Class rdf:ID="Tear_gas">
    <rdfs:subClassOf rdf:resource="jc3iedmSubOnt.owl#CHEMICAL-MATERIEL-TYPE-Irritant"/>
    <rdfs:subClassOf>
      <owl:Restriction>
        <owl:hasValue xml:lang="en">TRGAS</owl:hasValue>
        <owl:onProperty rdf:resource="jc3iedmBase.owl#chemical-materiel-type-subcategory-code"/>
      </owl:Restriction>
    </rdfs:subClassOf>
    <rdfs:label xml:lang="en">Tear gas</rdfs:label>
    <rdfs:comment xml:lang="en">A type of chemical compound used in riot control agents.</rdfs:comment>
  </owl:Class>
  <owl:Class rdf:ID="UN_Dangerous_Goods_NUM_3324">
    <rdfs:subClassOf>
      <owl:Restriction>
        <owl:hasValue xml:lang="en">3324</owl:hasValue>
        <owl:onProperty rdf:resource="jc3iedmBase.owl#consumable-materiel-type-united-nations-number-code"/>
      </owl:Restriction>
    </rdfs:subClassOf>
    <rdfs:label xml:lang="en">UN Dangerous Goods # 3324</rdfs:label>
    <rdfs:comment xml:lang="en">Radioactive material, low specific activity (LSA-II), fissile.</rdfs:comment>
  </owl:Class>
  <owl:Class rdf:ID="Electronic_support_measure">
    <rdfs:subClassOf rdf:resource="jc3iedmSubOnt.owl#ELECTRONIC-EQUIPMENT-TYPE-Electronic_warfare"/>
    <rdfs:subClassOf>
      <owl:Restriction>
        <owl:hasValue xml:lang="en">ELSPSM</owl:hasValue>
        <owl:onProperty rdf:resource="jc3iedmBase.owl#electronic-equipment-type-subcategory-code"/>
      </owl:Restriction>
    </rdfs:subClassOf>
    <rdfs:label xml:lang="en">Electronic support measure</rdfs:label>
    <rdfs:comment xml:lang="en">Equipment that provides detection, identification, and direction-finding for radar and communication signals emanating from ships, aircraft, submarines, and other emitters.</rdfs:comment>
  </owl:Class>
  <owl:Class rdf:about="#Radar,_early_warning/acquisition">
    <rdfs:subClassOf rdf:resource="jc3iedmSubOnt.owl#ELECTRONIC-EQUIPMENT-TYPE-Radar"/>
    <rdfs:subClassOf rdf:resource="jc3iedmSubOnt.owl#ELECTRONIC-EQUIPMENT-TYPE-Fire_control"/>
    <rdfs:subClassOf>
      <owl:Restriction>
        <owl:hasValue xml:lang="en">RDREWA</owl:hasValue>
        <owl:onProperty rdf:resource="jc3iedmBase.owl#electronic-equipment-type-subcategory-code"/>
      </owl:Restriction>
    </rdfs:subClassOf>
    <rdfs:label xml:lang="en">Radar, early warning/acquisition</rdfs:label>
    <rdfs:comment xml:lang="en">A radar used for early notification of the launch or approach of unknown weapons or weapon carriers.</rdfs:comment>
    <rdfs:subClassOf>
      <owl:Restriction>
        <owl:hasValue xml:lang="en">RDREWA</owl:hasValue>
        <owl:onProperty rdf:resource="jc3iedmBase.owl#electronic-equipment-type-subcategory-code"/>
      </owl:Restriction>
    </rdfs:subClassOf>
  </owl:Class>
  <owl:Class rdf:ID="Hops">
    <rdfs:label xml:lang="en">Hops</rdfs:label>
    <rdfs:comment xml:lang="en">An area covered by the systematic planting of hop vines.</rdfs:comment>
  </owl:Class>
  <owl:Class rdf:about="#Sonar,_variable_depth,_active">
    <rdfs:subClassOf rdf:resource="jc3iedmSubOnt.owl#MARITIME-EQUIPMENT-TYPE-Sonar,_maritime"/>
    <rdfs:subClassOf>
      <owl:Restriction>
        <owl:hasValue xml:lang="en">SONRVA</owl:hasValue>
        <owl:onProperty rdf:resource="jc3iedmBase.owl#maritime-equipment-type-subcategory-code"/>
      </owl:Restriction>
    </rdfs:subClassOf>
    <rdfs:label xml:lang="en">Sonar, variable depth, active</rdfs:label>
    <rdfs:comment xml:lang="en">No definition provided in ADatP-3 Baseline 13.1 FFIRN/FUD 1434/1.</rdfs:comment>
  </owl:Class>
  <owl:Class rdf:ID="Vineyard">
    <rdfs:label xml:lang="en">Vineyard</rdfs:label>
    <rdfs:comment xml:lang="en">An area covered by the systematic planting of grape vines.</rdfs:comment>
  </owl:Class>
  <owl:Class rdf:ID="JP-8_fuel">
    <rdfs:subClassOf rdf:resource="jc3iedmSubOnt.owl#CONSUMABLE-MATERIEL-TYPE-Fuel"/>
    <rdfs:subClassOf>
      <owl:Restriction>
        <owl:hasValue xml:lang="en">JP8F</owl:hasValue>
        <owl:onProperty rdf:resource="jc3iedmBase.owl#consumable-materiel-type-subcategory-code"/>
      </owl:Restriction>
    </rdfs:subClassOf>
    <rdfs:label xml:lang="en">JP-8 fuel</rdfs:label>
    <rdfs:comment xml:lang="en">Aviation kerosene, Specification MIL-T-83133 (F-34), interchangeable with AVTUR/FSII, NATO F-34.</rdfs:comment>
  </owl:Class>
  <owl:Class rdf:ID="Booby_trap">
    <rdfs:subClassOf rdf:resource="jc3iedmSubOnt.owl#CONSUMABLE-MATERIEL-TYPE-Improvised_explosive_device"/>
    <rdfs:subClassOf>
      <owl:Restriction>
        <owl:hasValue xml:lang="en">BBYTRP</owl:hasValue>
        <owl:onProperty rdf:resource="jc3iedmBase.owl#consumable-materiel-type-subcategory-code"/>
      </owl:Restriction>
    </rdfs:subClassOf>
    <rdfs:label xml:lang="en">Booby trap</rdfs:label>
    <rdfs:comment xml:lang="en">An explosive or non-explosive device or other material deliberately placed to cause casualties when an apparently harmless object is disturbed or a normally safe act is performed.</rdfs:comment>
  </owl:Class>
  <owl:Class rdf:ID="Shotgun">
    <rdfs:subClassOf rdf:resource="jc3iedmSubOnt.owl#WEAPON-TYPE-Small_arms"/>
    <rdfs:subClassOf>
      <owl:Restriction>
        <owl:hasValue xml:lang="en">SHOTGU</owl:hasValue>
        <owl:onProperty rdf:resource="jc3iedmBase.owl#weapon-type-subcategory-code"/>
      </owl:Restriction>
    </rdfs:subClassOf>
    <rdfs:label xml:lang="en">Shotgun</rdfs:label>
    <rdfs:comment xml:lang="en">A smooth-bore gun for firing small pellets at short range.</rdfs:comment>
  </owl:Class>
  <owl:Class rdf:ID="Ecstasy_-_MDA">
    <rdfs:subClassOf rdf:resource="jc3iedmSubOnt.owl#CONSUMABLE-MATERIEL-TYPE-Drug"/>
    <rdfs:subClassOf>
      <owl:Restriction>
        <owl:hasValue xml:lang="en">ECSMDA</owl:hasValue>
        <owl:onProperty rdf:resource="jc3iedmBase.owl#consumable-materiel-type-subcategory-code"/>
      </owl:Restriction>
    </rdfs:subClassOf>
    <rdfs:label xml:lang="en">Ecstasy - MDA</rdfs:label>
    <rdfs:comment xml:lang="en">Methylenedioxyamphetamine, an amphetamine-based drug that causes euphoric and hallucinatory effects, originally produced as an appetite suppressant.</rdfs:comment>
  </owl:Class>
  <owl:Class rdf:ID="Remote_access">
    <rdfs:subClassOf rdf:resource="jc3iedmSubOnt.owl#NETWORK-SERVICE-Data_transfer"/>
    <rdfs:subClassOf>
      <owl:Restriction>
        <owl:hasValue xml:lang="en">RMTACC</owl:hasValue>
        <owl:onProperty rdf:resource="jc3iedmBase.owl#network-service-subcategory-code"/>
      </owl:Restriction>
    </rdfs:subClassOf>
    <rdfs:label xml:lang="en">Remote access</rdfs:label>
    <rdfs:comment xml:lang="en">A service that enable the operation of a remote node from a local node.</rdfs:comment>
  </owl:Class>
  <owl:Class rdf:ID="Passable">
    <rdfs:subClassOf>
      <owl:Restriction>
        <owl:hasValue xml:lang="en">PASABL</owl:hasValue>
        <owl:onProperty rdf:resource="jc3iedmBase.owl#facility-status-operational-status-qualifier-code"/>
      </owl:Restriction>
    </rdfs:subClassOf>
    <rdfs:label xml:lang="en">Passable</rdfs:label>
    <rdfs:comment xml:lang="en">Subjectively judged by the reporting organisation that a FACILITY can be crossed.</rdfs:comment>
  </owl:Class>
  <owl:Class rdf:ID="Instrument_landing_system_localiser">
    <rdfs:subClassOf rdf:resource="jc3iedmSubOnt.owl#ELECTRONIC-EQUIPMENT-TYPE-Instrument_landing_system"/>
    <rdfs:subClassOf>
      <owl:Restriction>
        <owl:hasValue xml:lang="en">ILSLOC</owl:hasValue>
        <owl:onProperty rdf:resource="jc3iedmBase.owl#electronic-equipment-type-subcategory-code"/>
      </owl:Restriction>
    </rdfs:subClassOf>
    <rdfs:label xml:lang="en">Instrument landing system localiser</rdfs:label>
    <rdfs:comment xml:lang="en">A system of horizontal guidance embodied in the instrument landing system which indicates the horizontal deviation of the aircraft from its optimum path of descent along the axis of the runway.</rdfs:comment>
  </owl:Class>
  <owl:Class rdf:ID="UN_Dangerous_Goods_NUM_1741">
    <rdfs:subClassOf>
      <owl:Restriction>
        <owl:hasValue xml:lang="en">1741</owl:hasValue>
        <owl:onProperty rdf:resource="jc3iedmBase.owl#consumable-materiel-type-united-nations-number-code"/>
      </owl:Restriction>
    </rdfs:subClassOf>
    <rdfs:label xml:lang="en">UN Dangerous Goods # 1741</rdfs:label>
    <rdfs:comment xml:lang="en">Boron trichloride. Includes the agent(s): boron trichloride.</rdfs:comment>
    <rdfs:subClassOf>
      <owl:Restriction>
        <owl:hasValue xml:lang="en">1741</owl:hasValue>
        <owl:onProperty rdf:resource="jc3iedmBase.owl#consumable-materiel-type-united-nations-number-code"/>
      </owl:Restriction>
    </rdfs:subClassOf>
  </owl:Class>
  <owl:Class rdf:ID="Acoustic_high_frequency">
    <rdfs:subClassOf rdf:resource="jc3iedmSubOnt.owl#AMMUNITION-TYPE-Mine,_maritime,_moving"/>
    <rdfs:subClassOf rdf:resource="jc3iedmSubOnt.owl#AMMUNITION-TYPE-Mine,_moored"/>
    <rdfs:comment xml:lang="en">A (maritime) mine firing mechanism with an acoustic high frequency circuit, 20 to 50 Hz, which responds to the acoustic field of a ship or sweep.</rdfs:comment>
    <rdfs:subClassOf rdf:resource="jc3iedmSubOnt.owl#AMMUNITION-TYPE-Seabed_mine"/>
    <rdfs:subClassOf rdf:resource="jc3iedmSubOnt.owl#AMMUNITION-TYPE-Mine,_deep_moored"/>
    <rdfs:subClassOf>
      <owl:Restriction>
        <owl:hasValue xml:lang="en">ACOUHF</owl:hasValue>
        <owl:onProperty rdf:resource="jc3iedmBase.owl#ammunition-type-mine-maritime-firing-code"/>
      </owl:Restriction>
    </rdfs:subClassOf>
    <rdfs:subClassOf rdf:resource="jc3iedmSubOnt.owl#AMMUNITION-TYPE-Mine,_not_otherwise_specified"/>
    <rdfs:subClassOf rdf:resource="jc3iedmSubOnt.owl#AMMUNITION-TYPE-Moving_mine,_sea"/>
    <rdfs:subClassOf rdf:resource="jc3iedmSubOnt.owl#AMMUNITION-TYPE-Mine,_shallow_moored"/>
    <rdfs:subClassOf rdf:resource="jc3iedmSubOnt.owl#AMMUNITION-TYPE-Mine,_seabed_-_explosive_charge_less_than_500kg"/>
    <rdfs:subClassOf rdf:resource="jc3iedmSubOnt.owl#AMMUNITION-TYPE-Sea_mine"/>
    <rdfs:subClassOf rdf:resource="jc3iedmSubOnt.owl#AMMUNITION-TYPE-Mine,_seabed_-_explosive_charge_500kg_or_greater"/>
    <rdfs:subClassOf>
      <owl:Restriction>
        <owl:hasValue xml:lang="en">ACOUHF</owl:hasValue>
        <owl:onProperty rdf:resource="jc3iedmBase.owl#ammunition-type-mine-maritime-firing-code"/>
      </owl:Restriction>
    </rdfs:subClassOf>
    <rdfs:subClassOf rdf:resource="jc3iedmSubOnt.owl#AMMUNITION-TYPE-Mine,_not_known"/>
    <rdfs:label xml:lang="en">Acoustic high frequency</rdfs:label>
  </owl:Class>
  <owl:Class rdf:ID="Ketamine">
    <rdfs:subClassOf rdf:resource="jc3iedmSubOnt.owl#CONSUMABLE-MATERIEL-TYPE-Drug"/>
    <rdfs:subClassOf>
      <owl:Restriction>
        <owl:hasValue xml:lang="en">KTMINE</owl:hasValue>
        <owl:onProperty rdf:resource="jc3iedmBase.owl#consumable-materiel-type-subcategory-code"/>
      </owl:Restriction>
    </rdfs:subClassOf>
    <rdfs:label xml:lang="en">Ketamine</rdfs:label>
    <rdfs:comment xml:lang="en">An anaesthetic and pain-killing drug, also used (illicitly) as a hallucinogen.</rdfs:comment>
  </owl:Class>
  <owl:Class rdf:ID="Radar_scope">
    <rdfs:subClassOf rdf:resource="jc3iedmSubOnt.owl#ELECTRONIC-EQUIPMENT-TYPE-Radar"/>
    <rdfs:subClassOf rdf:resource="jc3iedmSubOnt.owl#ELECTRONIC-EQUIPMENT-TYPE-Navigational_aid"/>
    <rdfs:subClassOf>
      <owl:Restriction>
        <owl:hasValue xml:lang="en">RDRSCP</owl:hasValue>
        <owl:onProperty rdf:resource="jc3iedmBase.owl#electronic-equipment-type-subcategory-code"/>
      </owl:Restriction>
    </rdfs:subClassOf>
    <rdfs:label xml:lang="en">Radar scope</rdfs:label>
    <rdfs:comment xml:lang="en">A cathode ray oscilloscope on the screen of which radar echoes are represented for observation.</rdfs:comment>
    <rdfs:subClassOf>
      <owl:Restriction>
        <owl:hasValue xml:lang="en">RDRSCP</owl:hasValue>
        <owl:onProperty rdf:resource="jc3iedmBase.owl#electronic-equipment-type-subcategory-code"/>
      </owl:Restriction>
    </rdfs:subClassOf>
  </owl:Class>
  <owl:Class rdf:ID="UN_Dangerous_Goods_NUM_1158">
    <rdfs:subClassOf>
      <owl:Restriction>
        <owl:hasValue xml:lang="en">1158</owl:hasValue>
        <owl:onProperty rdf:resource="jc3iedmBase.owl#consumable-materiel-type-united-nations-number-code"/>
      </owl:Restriction>
    </rdfs:subClassOf>
    <rdfs:label xml:lang="en">UN Dangerous Goods # 1158</rdfs:label>
    <rdfs:comment xml:lang="en">Diisopropylamine. Includes the agent(s): diisopropylamine.</rdfs:comment>
    <rdfs:subClassOf>
      <owl:Restriction>
        <owl:hasValue xml:lang="en">1158</owl:hasValue>
        <owl:onProperty rdf:resource="jc3iedmBase.owl#consumable-materiel-type-united-nations-number-code"/>
      </owl:Restriction>
    </rdfs:subClassOf>
  </owl:Class>
  <owl:Class rdf:ID="Mothballed">
    <rdfs:subClassOf>
      <owl:Restriction>
        <owl:hasValue xml:lang="en">MTHBLD</owl:hasValue>
        <owl:onProperty rdf:resource="jc3iedmBase.owl#materiel-status-operational-status-qualifier-code"/>
      </owl:Restriction>
    </rdfs:subClassOf>
    <rdfs:label xml:lang="en">Mothballed</rdfs:label>
    <rdfs:comment xml:lang="en">Subjectively judged by the reporting organisation that a specific materiel has been preserved to some degree.</rdfs:comment>
  </owl:Class>
  <owl:Class rdf:about="#Locomotive,_diesel/electric">
    <rdfs:subClassOf rdf:resource="jc3iedmSubOnt.owl#RAILCAR-TYPE-Locomotive"/>
    <rdfs:subClassOf>
      <owl:Restriction>
        <owl:hasValue xml:lang="en">LCMDSE</owl:hasValue>
        <owl:onProperty rdf:resource="jc3iedmBase.owl#railcar-type-subcategory-code"/>
      </owl:Restriction>
    </rdfs:subClassOf>
    <rdfs:label xml:lang="en">Locomotive, diesel/electric</rdfs:label>
    <rdfs:comment xml:lang="en">A locomotive that uses diesel engine(s) to produce electricity for electric engine(s) that provide the engine with its source of tractive power.</rdfs:comment>
  </owl:Class>
  <owl:Class rdf:about="#Tank_gun,_medium">
    <rdfs:subClassOf rdf:resource="jc3iedmSubOnt.owl#WEAPON-TYPE-Anti-tank"/>
    <rdfs:subClassOf>
      <owl:Restriction>
        <owl:hasValue xml:lang="en">TKGUNM</owl:hasValue>
        <owl:onProperty rdf:resource="jc3iedmBase.owl#weapon-type-subcategory-code"/>
      </owl:Restriction>
    </rdfs:subClassOf>
    <rdfs:label xml:lang="en">Tank gun, medium</rdfs:label>
    <rdfs:comment xml:lang="en">Medium, turret mounted, tank gun, calibre between 90 and 120 MM, for use in the field against tanks.</rdfs:comment>
  </owl:Class>
  <owl:Class rdf:ID="UN_Dangerous_Goods_NUM_1005">
    <rdfs:subClassOf>
      <owl:Restriction>
        <owl:hasValue xml:lang="en">1005</owl:hasValue>
        <owl:onProperty rdf:resource="jc3iedmBase.owl#consumable-materiel-type-united-nations-number-code"/>
      </owl:Restriction>
    </rdfs:subClassOf>
    <rdfs:label xml:lang="en">UN Dangerous Goods # 1005</rdfs:label>
    <rdfs:comment xml:lang="en">Ammonia, anhydrous. Includes the agent(s): ammonia.</rdfs:comment>
    <rdfs:subClassOf>
      <owl:Restriction>
        <owl:hasValue xml:lang="en">1005</owl:hasValue>
        <owl:onProperty rdf:resource="jc3iedmBase.owl#consumable-materiel-type-united-nations-number-code"/>
      </owl:Restriction>
    </rdfs:subClassOf>
  </owl:Class>
  <owl:Class rdf:ID="UN_Dangerous_Goods_NUM_3325">
    <rdfs:subClassOf>
      <owl:Restriction>
        <owl:hasValue xml:lang="en">3325</owl:hasValue>
        <owl:onProperty rdf:resource="jc3iedmBase.owl#consumable-materiel-type-united-nations-number-code"/>
      </owl:Restriction>
    </rdfs:subClassOf>
    <rdfs:label xml:lang="en">UN Dangerous Goods # 3325</rdfs:label>
    <rdfs:comment xml:lang="en">Radioactive material, low specific activity (LSA-III), fissile.</rdfs:comment>
  </owl:Class>
  <owl:Class rdf:ID="Multi-look_mines">
    <rdfs:label xml:lang="en">Multi-look mines</rdfs:label>
    <rdfs:subClassOf rdf:resource="jc3iedmSubOnt.owl#AMMUNITION-TYPE-Mine,_deep_moored"/>
    <rdfs:subClassOf>
      <owl:Restriction>
        <owl:hasValue xml:lang="en">MULTLM</owl:hasValue>
        <owl:onProperty rdf:resource="jc3iedmBase.owl#ammunition-type-mine-maritime-firing-code"/>
      </owl:Restriction>
    </rdfs:subClassOf>
    <rdfs:subClassOf rdf:resource="jc3iedmSubOnt.owl#AMMUNITION-TYPE-Mine,_shallow_moored"/>
    <rdfs:subClassOf rdf:resource="jc3iedmSubOnt.owl#AMMUNITION-TYPE-Mine,_not_known"/>
    <rdfs:subClassOf>
      <owl:Restriction>
        <owl:hasValue xml:lang="en">MULTLM</owl:hasValue>
        <owl:onProperty rdf:resource="jc3iedmBase.owl#ammunition-type-mine-maritime-firing-code"/>
      </owl:Restriction>
    </rdfs:subClassOf>
    <rdfs:comment xml:lang="en">A type of maritime mine actuation.</rdfs:comment>
    <rdfs:subClassOf rdf:resource="jc3iedmSubOnt.owl#AMMUNITION-TYPE-Mine,_not_otherwise_specified"/>
    <rdfs:subClassOf rdf:resource="jc3iedmSubOnt.owl#AMMUNITION-TYPE-Seabed_mine"/>
    <rdfs:subClassOf rdf:resource="jc3iedmSubOnt.owl#AMMUNITION-TYPE-Sea_mine"/>
    <rdfs:subClassOf rdf:resource="jc3iedmSubOnt.owl#AMMUNITION-TYPE-Mine,_maritime,_moving"/>
    <rdfs:subClassOf rdf:resource="jc3iedmSubOnt.owl#AMMUNITION-TYPE-Moving_mine,_sea"/>
    <rdfs:subClassOf rdf:resource="jc3iedmSubOnt.owl#AMMUNITION-TYPE-Mine,_seabed_-_explosive_charge_500kg_or_greater"/>
    <rdfs:subClassOf rdf:resource="jc3iedmSubOnt.owl#AMMUNITION-TYPE-Mine,_moored"/>
    <rdfs:subClassOf rdf:resource="jc3iedmSubOnt.owl#AMMUNITION-TYPE-Mine,_seabed_-_explosive_charge_less_than_500kg"/>
  </owl:Class>
  <owl:Class rdf:about="#Sonar,_dipping,_passive">
    <rdfs:subClassOf rdf:resource="jc3iedmSubOnt.owl#MARITIME-EQUIPMENT-TYPE-Sonar,_maritime"/>
    <rdfs:subClassOf>
      <owl:Restriction>
        <owl:hasValue xml:lang="en">SONRDP</owl:hasValue>
        <owl:onProperty rdf:resource="jc3iedmBase.owl#maritime-equipment-type-subcategory-code"/>
      </owl:Restriction>
    </rdfs:subClassOf>
    <rdfs:label xml:lang="en">Sonar, dipping, passive</rdfs:label>
    <rdfs:comment xml:lang="en">No definition provided in ADatP-3 Baseline 13.1 FFIRN/FUD 1434/1.</rdfs:comment>
  </owl:Class>
  <owl:Class rdf:about="#Artillery,_light">
    <rdfs:subClassOf rdf:resource="jc3iedmSubOnt.owl#WEAPON-TYPE-Field_artillery"/>
    <rdfs:subClassOf>
      <owl:Restriction>
        <owl:hasValue xml:lang="en">ARTLGT</owl:hasValue>
        <owl:onProperty rdf:resource="jc3iedmBase.owl#weapon-type-subcategory-code"/>
      </owl:Restriction>
    </rdfs:subClassOf>
    <rdfs:label xml:lang="en">Artillery, light</rdfs:label>
    <rdfs:comment xml:lang="en">Field artillery cannon with a calibre of 120mm and less.</rdfs:comment>
  </owl:Class>
  <owl:Class rdf:ID="Oil">
    <rdfs:subClassOf rdf:resource="jc3iedmSubOnt.owl#CONSUMABLE-MATERIEL-TYPE-POL"/>
    <rdfs:subClassOf>
      <owl:Restriction>
        <owl:hasValue xml:lang="en">OIL</owl:hasValue>
        <owl:onProperty rdf:resource="jc3iedmBase.owl#consumable-materiel-type-subcategory-code"/>
      </owl:Restriction>
    </rdfs:subClassOf>
    <rdfs:label xml:lang="en">Oil</rdfs:label>
    <rdfs:comment xml:lang="en">A substance having the following characters (or most of them): viz. those of being liquid at ordinary temperatures, of a viscid consistence and characteristic smooth and sticky (unctuous) feel, lighter than water and insoluble in it, soluble in alcohol and ether, inflammable, chemically neutral.</rdfs:comment>
  </owl:Class>
  <owl:Class rdf:ID="UN_Dangerous_Goods_NUM_2199">
    <rdfs:subClassOf>
      <owl:Restriction>
        <owl:hasValue xml:lang="en">2199</owl:hasValue>
        <owl:onProperty rdf:resource="jc3iedmBase.owl#consumable-materiel-type-united-nations-number-code"/>
      </owl:Restriction>
    </rdfs:subClassOf>
    <rdfs:label xml:lang="en">UN Dangerous Goods # 2199</rdfs:label>
    <rdfs:comment xml:lang="en">Phosphine. Includes the agent(s): phosphine.</rdfs:comment>
    <rdfs:subClassOf>
      <owl:Restriction>
        <owl:hasValue xml:lang="en">2199</owl:hasValue>
        <owl:onProperty rdf:resource="jc3iedmBase.owl#consumable-materiel-type-united-nations-number-code"/>
      </owl:Restriction>
    </rdfs:subClassOf>
  </owl:Class>
  <owl:Class rdf:about="#Surface-to-surface_missile_launcher,_short_range">
    <rdfs:subClassOf rdf:resource="jc3iedmSubOnt.owl#WEAPON-TYPE-Missile_system"/>
    <rdfs:subClassOf>
      <owl:Restriction>
        <owl:hasValue xml:lang="en">SSMLSR</owl:hasValue>
        <owl:onProperty rdf:resource="jc3iedmBase.owl#weapon-type-subcategory-code"/>
      </owl:Restriction>
    </rdfs:subClassOf>
    <rdfs:label xml:lang="en">Surface-to-surface missile launcher, short range</rdfs:label>
    <rdfs:comment xml:lang="en">A structural device designed to support and hold a short range surface to surface missile in position for firing.</rdfs:comment>
  </owl:Class>
  <owl:Class rdf:ID="UN_Dangerous_Goods_NUM_1282">
    <rdfs:subClassOf>
      <owl:Restriction>
        <owl:hasValue xml:lang="en">1282</owl:hasValue>
        <owl:onProperty rdf:resource="jc3iedmBase.owl#consumable-materiel-type-united-nations-number-code"/>
      </owl:Restriction>
    </rdfs:subClassOf>
    <rdfs:label xml:lang="en">UN Dangerous Goods # 1282</rdfs:label>
    <rdfs:comment xml:lang="en">Pyridine. Includes the agent(s): pyridine.</rdfs:comment>
    <rdfs:subClassOf>
      <owl:Restriction>
        <owl:hasValue xml:lang="en">1282</owl:hasValue>
        <owl:onProperty rdf:resource="jc3iedmBase.owl#consumable-materiel-type-united-nations-number-code"/>
      </owl:Restriction>
    </rdfs:subClassOf>
  </owl:Class>
  <owl:Class rdf:ID="Radio_broadcast_device">
    <rdfs:subClassOf rdf:resource="jc3iedmSubOnt.owl#ELECTRONIC-EQUIPMENT-TYPE-Public_address_system"/>
    <rdfs:subClassOf rdf:resource="jc3iedmSubOnt.owl#ELECTRONIC-EQUIPMENT-TYPE-Communication"/>
    <rdfs:subClassOf>
      <owl:Restriction>
        <owl:hasValue xml:lang="en">RADBRD</owl:hasValue>
        <owl:onProperty rdf:resource="jc3iedmBase.owl#electronic-equipment-type-subcategory-code"/>
      </owl:Restriction>
    </rdfs:subClassOf>
    <rdfs:label xml:lang="en">Radio broadcast device</rdfs:label>
    <rdfs:comment xml:lang="en">Organised wireless broadcasting in sound as a medium of communication or as an art form.</rdfs:comment>
    <rdfs:subClassOf>
      <owl:Restriction>
        <owl:hasValue xml:lang="en">RADBRD</owl:hasValue>
        <owl:onProperty rdf:resource="jc3iedmBase.owl#electronic-equipment-type-subcategory-code"/>
      </owl:Restriction>
    </rdfs:subClassOf>
  </owl:Class>
  <owl:Class rdf:ID="Inland_waterway">
    <rdfs:label xml:lang="en">Inland waterway</rdfs:label>
    <rdfs:comment xml:lang="en">Represents the general mode of transportation used in movement by inland waterways.</rdfs:comment>
  </owl:Class>
  <owl:Class rdf:ID="Remote_intrusion_detection_device">
    <rdfs:subClassOf rdf:resource="jc3iedmSubOnt.owl#ELECTRONIC-EQUIPMENT-TYPE-Sensor"/>
    <rdfs:subClassOf>
      <owl:Restriction>
        <owl:hasValue xml:lang="en">RTINDD</owl:hasValue>
        <owl:onProperty rdf:resource="jc3iedmBase.owl#electronic-equipment-type-subcategory-code"/>
      </owl:Restriction>
    </rdfs:subClassOf>
    <rdfs:label xml:lang="en">Remote intrusion detection device</rdfs:label>
    <rdfs:comment xml:lang="en">An equipment used to detect objects moving into or within an area of interest.</rdfs:comment>
  </owl:Class>
  <owl:Class rdf:ID="Brahms">
    <rdfs:subClassOf rdf:resource="jc3iedmSubOnt.owl#ELECTRONIC-EQUIPMENT-TYPE-Communication"/>
    <rdfs:subClassOf>
      <owl:Restriction>
        <owl:hasValue xml:lang="en">BRAHMS</owl:hasValue>
        <owl:onProperty rdf:resource="jc3iedmBase.owl#electronic-equipment-type-subcategory-code"/>
      </owl:Restriction>
    </rdfs:subClassOf>
    <rdfs:label xml:lang="en">Brahms</rdfs:label>
    <rdfs:comment xml:lang="en">A voice encryption Terminal that provides secure speech over a civil or military phone system.</rdfs:comment>
  </owl:Class>
  <owl:Class rdf:about="#Radio,_direction_finding">
    <rdfs:subClassOf rdf:resource="jc3iedmSubOnt.owl#ELECTRONIC-EQUIPMENT-TYPE-Communication"/>
    <rdfs:subClassOf>
      <owl:Restriction>
        <owl:hasValue xml:lang="en">RADDFD</owl:hasValue>
        <owl:onProperty rdf:resource="jc3iedmBase.owl#electronic-equipment-type-subcategory-code"/>
      </owl:Restriction>
    </rdfs:subClassOf>
    <rdfs:label xml:lang="en">Radio, direction finding</rdfs:label>
    <rdfs:comment xml:lang="en">Equipment that uses radio signal intercepts and their azimuths to determine a location of a transmitter.</rdfs:comment>
  </owl:Class>
  <owl:Class rdf:ID="Hill">
    <rdfs:subClassOf rdf:resource="jc3iedmSubOnt.owl#GEOGRAPHIC-FEATURE-Solid_surface"/>
    <rdfs:subClassOf rdf:resource="jc3iedmSubOnt.owl#GEOGRAPHIC-FEATURE-TYPE-Landform"/>
    <rdfs:subClassOf>
      <owl:Restriction>
        <owl:hasValue xml:lang="en">HILL</owl:hasValue>
        <owl:onProperty rdf:resource="jc3iedmBase.owl#geographic-feature-type-subcategory-code"/>
      </owl:Restriction>
    </rdfs:subClassOf>
    <rdfs:label xml:lang="en">Hill</rdfs:label>
    <rdfs:comment xml:lang="en">A small, isolated elevation, smaller than a mountain.</rdfs:comment>
    <rdfs:subClassOf>
      <owl:Restriction>
        <owl:hasValue xml:lang="en">HILL</owl:hasValue>
        <owl:onProperty rdf:resource="jc3iedmBase.owl#geographic-feature-type-subcategory-code"/>
      </owl:Restriction>
    </rdfs:subClassOf>
  </owl:Class>
  <owl:Class rdf:ID="UN_Dangerous_Goods_NUM_1198">
    <rdfs:subClassOf>
      <owl:Restriction>
        <owl:hasValue xml:lang="en">1198</owl:hasValue>
        <owl:onProperty rdf:resource="jc3iedmBase.owl#consumable-materiel-type-united-nations-number-code"/>
      </owl:Restriction>
    </rdfs:subClassOf>
    <rdfs:label xml:lang="en">UN Dangerous Goods # 1198</rdfs:label>
    <rdfs:comment xml:lang="en">Formaldehyde solution, flammable. Includes the agent(s): formaldehyde.</rdfs:comment>
    <rdfs:subClassOf>
      <owl:Restriction>
        <owl:hasValue xml:lang="en">1198</owl:hasValue>
        <owl:onProperty rdf:resource="jc3iedmBase.owl#consumable-materiel-type-united-nations-number-code"/>
      </owl:Restriction>
    </rdfs:subClassOf>
  </owl:Class>
  <owl:Class rdf:about="#Air-defence_missile_launcher,_long_range">
    <rdfs:subClassOf rdf:resource="jc3iedmSubOnt.owl#WEAPON-TYPE-Air-defence"/>
    <rdfs:subClassOf rdf:resource="jc3iedmSubOnt.owl#WEAPON-TYPE-Missile_system"/>
    <rdfs:subClassOf>
      <owl:Restriction>
        <owl:hasValue xml:lang="en">ADMLLR</owl:hasValue>
        <owl:onProperty rdf:resource="jc3iedmBase.owl#weapon-type-subcategory-code"/>
      </owl:Restriction>
    </rdfs:subClassOf>
    <rdfs:label xml:lang="en">Air-defence missile launcher, long range</rdfs:label>
    <rdfs:comment xml:lang="en">A structural device designed to support and hold a long range air defence missile in position for firing.</rdfs:comment>
    <rdfs:subClassOf>
      <owl:Restriction>
        <owl:hasValue xml:lang="en">ADMLLR</owl:hasValue>
        <owl:onProperty rdf:resource="jc3iedmBase.owl#weapon-type-subcategory-code"/>
      </owl:Restriction>
    </rdfs:subClassOf>
  </owl:Class>
  <owl:Class rdf:ID="UN_Dangerous_Goods_NUM_1722">
    <rdfs:subClassOf>
      <owl:Restriction>
        <owl:hasValue xml:lang="en">1722</owl:hasValue>
        <owl:onProperty rdf:resource="jc3iedmBase.owl#consumable-materiel-type-united-nations-number-code"/>
      </owl:Restriction>
    </rdfs:subClassOf>
    <rdfs:label xml:lang="en">UN Dangerous Goods # 1722</rdfs:label>
    <rdfs:comment xml:lang="en">Allyl chloroformate. Includes the agent(s): allyl chloroformate.</rdfs:comment>
    <rdfs:subClassOf>
      <owl:Restriction>
        <owl:hasValue xml:lang="en">1722</owl:hasValue>
        <owl:onProperty rdf:resource="jc3iedmBase.owl#consumable-materiel-type-united-nations-number-code"/>
      </owl:Restriction>
    </rdfs:subClassOf>
  </owl:Class>
  <owl:Class rdf:ID="Fixed_fortification_artillery">
    <rdfs:subClassOf rdf:resource="jc3iedmSubOnt.owl#WEAPON-TYPE-Cannon"/>
    <rdfs:subClassOf>
      <owl:Restriction>
        <owl:hasValue xml:lang="en">FFART</owl:hasValue>
        <owl:onProperty rdf:resource="jc3iedmBase.owl#weapon-type-subcategory-code"/>
      </owl:Restriction>
    </rdfs:subClassOf>
    <rdfs:label xml:lang="en">Fixed fortification artillery</rdfs:label>
    <rdfs:comment xml:lang="en">Guns inside a fortress.</rdfs:comment>
  </owl:Class>
  <owl:Class rdf:ID="Aviation_fuel">
    <rdfs:subClassOf rdf:resource="jc3iedmSubOnt.owl#CONSUMABLE-MATERIEL-TYPE-POL"/>
    <rdfs:subClassOf>
      <owl:Restriction>
        <owl:hasValue xml:lang="en">AVNFU</owl:hasValue>
        <owl:onProperty rdf:resource="jc3iedmBase.owl#consumable-materiel-type-subcategory-code"/>
      </owl:Restriction>
    </rdfs:subClassOf>
    <rdfs:label xml:lang="en">Aviation fuel</rdfs:label>
    <rdfs:comment xml:lang="en">A petroleum fraction used as fuel in aeroplane engines.</rdfs:comment>
  </owl:Class>
  <owl:Class rdf:about="#Sonar,_active">
    <rdfs:subClassOf rdf:resource="jc3iedmSubOnt.owl#MARITIME-EQUIPMENT-TYPE-Sonar,_maritime"/>
    <rdfs:subClassOf>
      <owl:Restriction>
        <owl:hasValue xml:lang="en">SONRAC</owl:hasValue>
        <owl:onProperty rdf:resource="jc3iedmBase.owl#maritime-equipment-type-subcategory-code"/>
      </owl:Restriction>
    </rdfs:subClassOf>
    <rdfs:label xml:lang="en">Sonar, active</rdfs:label>
    <rdfs:comment xml:lang="en">A system that projects acoustic energy into the water and measures the speed of its return from a reflective surface as an echo to detect an underwater object and determine its range and bearing.</rdfs:comment>
  </owl:Class>
  <owl:Class rdf:ID="Cay">
    <rdfs:subClassOf rdf:resource="jc3iedmSubOnt.owl#GEOGRAPHIC-FEATURE-Solid_surface"/>
    <rdfs:subClassOf rdf:resource="jc3iedmSubOnt.owl#GEOGRAPHIC-FEATURE-TYPE-Landform"/>
    <rdfs:subClassOf>
      <owl:Restriction>
        <owl:hasValue xml:lang="en">CAY</owl:hasValue>
        <owl:onProperty rdf:resource="jc3iedmBase.owl#geographic-feature-type-subcategory-code"/>
      </owl:Restriction>
    </rdfs:subClassOf>
    <rdfs:label xml:lang="en">Cay</rdfs:label>
    <rdfs:comment xml:lang="en">A small insular feature, which may contain scant vegetation; usually composed of sand or coral. Often applied to smaller coral shoals.</rdfs:comment>
    <rdfs:subClassOf>
      <owl:Restriction>
        <owl:hasValue xml:lang="en">CAY</owl:hasValue>
        <owl:onProperty rdf:resource="jc3iedmBase.owl#geographic-feature-type-subcategory-code"/>
      </owl:Restriction>
    </rdfs:subClassOf>
  </owl:Class>
  <owl:Class rdf:ID="Channel">
    <rdfs:subClassOf rdf:resource="jc3iedmSubOnt.owl#GEOGRAPHIC-FEATURE-TYPE-Inland_water"/>
    <rdfs:subClassOf rdf:resource="jc3iedmSubOnt.owl#GEOGRAPHIC-FEATURE-Liquid_surface"/>
    <rdfs:subClassOf>
      <owl:Restriction>
        <owl:hasValue xml:lang="en">CHANEL</owl:hasValue>
        <owl:onProperty rdf:resource="jc3iedmBase.owl#geographic-feature-type-subcategory-code"/>
      </owl:Restriction>
    </rdfs:subClassOf>
    <rdfs:label xml:lang="en">Channel</rdfs:label>
    <rdfs:comment xml:lang="en">That part of a body of water, sometimes dredged, deep enough for navigation through an area otherwise not navigable. It is usually marked by a single or double line of navigational aids.</rdfs:comment>
    <rdfs:subClassOf>
      <owl:Restriction>
        <owl:hasValue xml:lang="en">CHANEL</owl:hasValue>
        <owl:onProperty rdf:resource="jc3iedmBase.owl#geographic-feature-type-subcategory-code"/>
      </owl:Restriction>
    </rdfs:subClassOf>
  </owl:Class>
  <owl:Class rdf:ID="Pipeline">
    <rdfs:label xml:lang="en">Pipeline</rdfs:label>
    <rdfs:comment xml:lang="en">Represents the mode of transportation of materiel by pipeline.</rdfs:comment>
  </owl:Class>
  <owl:Class rdf:ID="Clothing">
    <rdfs:subClassOf rdf:resource="jc3iedmSubOnt.owl#CONSUMABLE-MATERIEL-TYPE-Personal_equipment"/>
    <rdfs:subClassOf>
      <owl:Restriction>
        <owl:hasValue xml:lang="en">CLTHNG</owl:hasValue>
        <owl:onProperty rdf:resource="jc3iedmBase.owl#consumable-materiel-type-subcategory-code"/>
      </owl:Restriction>
    </rdfs:subClassOf>
    <rdfs:label xml:lang="en">Clothing</rdfs:label>
    <rdfs:comment xml:lang="en">Articles of dress or attire worn by individuals.</rdfs:comment>
  </owl:Class>
  <owl:Class rdf:about="#Wagon,_bulk_fuel">
    <rdfs:subClassOf rdf:resource="jc3iedmSubOnt.owl#RAILCAR-TYPE-Rolling_stock"/>
    <rdfs:subClassOf>
      <owl:Restriction>
        <owl:hasValue xml:lang="en">WGNFUL</owl:hasValue>
        <owl:onProperty rdf:resource="jc3iedmBase.owl#railcar-type-subcategory-code"/>
      </owl:Restriction>
    </rdfs:subClassOf>
    <rdfs:label xml:lang="en">Wagon, bulk fuel</rdfs:label>
    <rdfs:comment xml:lang="en">Rolling stock used to move bulk fuel by rail. [Also often known as tank wagons.]</rdfs:comment>
  </owl:Class>
  <owl:Class rdf:ID="UN_Dangerous_Goods_NUM_3326">
    <rdfs:subClassOf>
      <owl:Restriction>
        <owl:hasValue xml:lang="en">3326</owl:hasValue>
        <owl:onProperty rdf:resource="jc3iedmBase.owl#consumable-materiel-type-united-nations-number-code"/>
      </owl:Restriction>
    </rdfs:subClassOf>
    <rdfs:label xml:lang="en">UN Dangerous Goods # 3326</rdfs:label>
    <rdfs:comment xml:lang="en">Radioactive material, surface contaminated objects (SCO-I or SCO-II), fissile.</rdfs:comment>
  </owl:Class>
  <owl:Class rdf:about="#Crevice/crevasse">
    <rdfs:subClassOf rdf:resource="jc3iedmSubOnt.owl#GEOGRAPHIC-FEATURE-Solid_surface"/>
    <rdfs:subClassOf rdf:resource="jc3iedmSubOnt.owl#GEOGRAPHIC-FEATURE-TYPE-Landform"/>
    <rdfs:subClassOf>
      <owl:Restriction>
        <owl:hasValue xml:lang="en">CRVCEC</owl:hasValue>
        <owl:onProperty rdf:resource="jc3iedmBase.owl#geographic-feature-type-subcategory-code"/>
      </owl:Restriction>
    </rdfs:subClassOf>
    <rdfs:label xml:lang="en">Crevice/crevasse</rdfs:label>
    <rdfs:comment xml:lang="en">A narrow fissure, crack, or rift in the Earths surface, snow or ice.</rdfs:comment>
    <rdfs:subClassOf>
      <owl:Restriction>
        <owl:hasValue xml:lang="en">CRVCEC</owl:hasValue>
        <owl:onProperty rdf:resource="jc3iedmBase.owl#geographic-feature-type-subcategory-code"/>
      </owl:Restriction>
    </rdfs:subClassOf>
  </owl:Class>
  <owl:Class rdf:about="#Anti-tank_rocket_launcher,_heavy">
    <rdfs:subClassOf rdf:resource="jc3iedmSubOnt.owl#WEAPON-TYPE-Anti-tank"/>
    <rdfs:subClassOf>
      <owl:Restriction>
        <owl:hasValue xml:lang="en">ATRLHV</owl:hasValue>
        <owl:onProperty rdf:resource="jc3iedmBase.owl#weapon-type-subcategory-code"/>
      </owl:Restriction>
    </rdfs:subClassOf>
    <rdfs:label xml:lang="en">Anti-tank rocket launcher, heavy</rdfs:label>
    <rdfs:comment xml:lang="en">A heavy structural device designed to support and hold an anti-tank rocket in position for firing.</rdfs:comment>
  </owl:Class>
  <owl:Class rdf:about="#Machine_gun,_heavy">
    <rdfs:subClassOf rdf:resource="jc3iedmSubOnt.owl#WEAPON-TYPE-Small_arms"/>
    <rdfs:subClassOf>
      <owl:Restriction>
        <owl:hasValue xml:lang="en">MACGHV</owl:hasValue>
        <owl:onProperty rdf:resource="jc3iedmBase.owl#weapon-type-subcategory-code"/>
      </owl:Restriction>
    </rdfs:subClassOf>
    <rdfs:label xml:lang="en">Machine gun, heavy</rdfs:label>
    <rdfs:comment xml:lang="en">A heavy automatic gun giving continuous fire.</rdfs:comment>
  </owl:Class>
  <owl:Class rdf:ID="Thermal_infrared">
    <rdfs:subClassOf rdf:resource="jc3iedmSubOnt.owl#ELECTRONIC-EQUIPMENT-TYPE-Sensor"/>
    <rdfs:subClassOf>
      <owl:Restriction>
        <owl:hasValue xml:lang="en">THEINF</owl:hasValue>
        <owl:onProperty rdf:resource="jc3iedmBase.owl#electronic-equipment-type-subcategory-code"/>
      </owl:Restriction>
    </rdfs:subClassOf>
    <rdfs:label xml:lang="en">Thermal infrared</rdfs:label>
    <rdfs:comment xml:lang="en">A device that detects emitted infrared energy from both target and background, converts the infrared wavelengths to the visual spectrum.</rdfs:comment>
  </owl:Class>
  <owl:Class rdf:ID="Opium">
    <rdfs:subClassOf rdf:resource="jc3iedmSubOnt.owl#CONSUMABLE-MATERIEL-TYPE-Drug"/>
    <rdfs:subClassOf>
      <owl:Restriction>
        <owl:hasValue xml:lang="en">OPIUM</owl:hasValue>
        <owl:onProperty rdf:resource="jc3iedmBase.owl#consumable-materiel-type-subcategory-code"/>
      </owl:Restriction>
    </rdfs:subClassOf>
    <rdfs:label xml:lang="en">Opium</rdfs:label>
    <rdfs:comment xml:lang="en">A reddish-brown heavy-scented addictive drug prepared from the juice of the opium poppy, used in medicine as an analgesic and narcotic.</rdfs:comment>
  </owl:Class>
  <owl:Class rdf:ID="Underwater_sand_ridge">
    <rdfs:subClassOf rdf:resource="jc3iedmSubOnt.owl#GEOGRAPHIC-FEATURE-Solid_surface"/>
    <rdfs:subClassOf rdf:resource="jc3iedmSubOnt.owl#GEOGRAPHIC-FEATURE-TYPE-Landform"/>
    <rdfs:subClassOf>
      <owl:Restriction>
        <owl:hasValue xml:lang="en">UNDRSR</owl:hasValue>
        <owl:onProperty rdf:resource="jc3iedmBase.owl#geographic-feature-type-subcategory-code"/>
      </owl:Restriction>
    </rdfs:subClassOf>
    <rdfs:label xml:lang="en">Underwater sand ridge</rdfs:label>
    <rdfs:comment xml:lang="en">Sand on the sea floor having steeper sides and less regular topography than a rise.</rdfs:comment>
    <rdfs:subClassOf>
      <owl:Restriction>
        <owl:hasValue xml:lang="en">UNDRSR</owl:hasValue>
        <owl:onProperty rdf:resource="jc3iedmBase.owl#geographic-feature-type-subcategory-code"/>
      </owl:Restriction>
    </rdfs:subClassOf>
  </owl:Class>
  <owl:Class rdf:ID="UN_Dangerous_Goods_NUM_3246">
    <rdfs:subClassOf>
      <owl:Restriction>
        <owl:hasValue xml:lang="en">3246</owl:hasValue>
        <owl:onProperty rdf:resource="jc3iedmBase.owl#consumable-materiel-type-united-nations-number-code"/>
      </owl:Restriction>
    </rdfs:subClassOf>
    <rdfs:label xml:lang="en">UN Dangerous Goods # 3246</rdfs:label>
    <rdfs:comment xml:lang="en">Methanesulphonyl chloride. Includes the agent(s): methanesulfonyl chloride.</rdfs:comment>
    <rdfs:subClassOf>
      <owl:Restriction>
        <owl:hasValue xml:lang="en">3246</owl:hasValue>
        <owl:onProperty rdf:resource="jc3iedmBase.owl#consumable-materiel-type-united-nations-number-code"/>
      </owl:Restriction>
    </rdfs:subClassOf>
  </owl:Class>
  <owl:Class rdf:ID="Submachine_gun">
    <rdfs:subClassOf rdf:resource="jc3iedmSubOnt.owl#WEAPON-TYPE-Small_arms"/>
    <rdfs:subClassOf>
      <owl:Restriction>
        <owl:hasValue xml:lang="en">SUBMAC</owl:hasValue>
        <owl:onProperty rdf:resource="jc3iedmBase.owl#weapon-type-subcategory-code"/>
      </owl:Restriction>
    </rdfs:subClassOf>
    <rdfs:label xml:lang="en">Submachine gun</rdfs:label>
    <rdfs:comment xml:lang="en">A lightweight automatic or semiautomatic gun.</rdfs:comment>
  </owl:Class>
  <owl:Class rdf:about="#Howitzer,_heavy">
    <rdfs:subClassOf rdf:resource="jc3iedmSubOnt.owl#WEAPON-TYPE-Field_artillery"/>
    <rdfs:subClassOf rdf:resource="jc3iedmSubOnt.owl#WEAPON-TYPE-Cannon"/>
    <rdfs:subClassOf>
      <owl:Restriction>
        <owl:hasValue xml:lang="en">HOWTHV</owl:hasValue>
        <owl:onProperty rdf:resource="jc3iedmBase.owl#weapon-type-subcategory-code"/>
      </owl:Restriction>
    </rdfs:subClassOf>
    <rdfs:label xml:lang="en">Howitzer, heavy</rdfs:label>
    <rdfs:comment xml:lang="en">A heavy cannon that combines certain characteristics of guns and mortars. Normally a cannon with a tube length of 20 to 30 calibres; however, the tube length can exceed 30 calibres and still be considered a howitzer when the high angle firing zoning solution permits range overlap between charges.</rdfs:comment>
    <rdfs:subClassOf>
      <owl:Restriction>
        <owl:hasValue xml:lang="en">HOWTHV</owl:hasValue>
        <owl:onProperty rdf:resource="jc3iedmBase.owl#weapon-type-subcategory-code"/>
      </owl:Restriction>
    </rdfs:subClassOf>
  </owl:Class>
  <owl:Class rdf:ID="UN_Dangerous_Goods_NUM_1093">
    <rdfs:subClassOf>
      <owl:Restriction>
        <owl:hasValue xml:lang="en">1093</owl:hasValue>
        <owl:onProperty rdf:resource="jc3iedmBase.owl#consumable-materiel-type-united-nations-number-code"/>
      </owl:Restriction>
    </rdfs:subClassOf>
    <rdfs:label xml:lang="en">UN Dangerous Goods # 1093</rdfs:label>
    <rdfs:comment xml:lang="en">Acrylonitrile, stabilized. Includes the agent(s): acrylonitrile.</rdfs:comment>
    <rdfs:subClassOf>
      <owl:Restriction>
        <owl:hasValue xml:lang="en">1093</owl:hasValue>
        <owl:onProperty rdf:resource="jc3iedmBase.owl#consumable-materiel-type-united-nations-number-code"/>
      </owl:Restriction>
    </rdfs:subClassOf>
  </owl:Class>
  <owl:Class rdf:about="#Ice_peak/nunatak">
    <rdfs:subClassOf rdf:resource="jc3iedmSubOnt.owl#GEOGRAPHIC-FEATURE-TYPE-Snow/ice"/>
    <rdfs:subClassOf rdf:resource="jc3iedmSubOnt.owl#GEOGRAPHIC-FEATURE-Solid_surface"/>
    <rdfs:subClassOf>
      <owl:Restriction>
        <owl:hasValue xml:lang="en">ICEPKN</owl:hasValue>
        <owl:onProperty rdf:resource="jc3iedmBase.owl#geographic-feature-type-subcategory-code"/>
      </owl:Restriction>
    </rdfs:subClassOf>
    <rdfs:label xml:lang="en">Ice peak/nunatak</rdfs:label>
    <rdfs:comment xml:lang="en">A rocky peak projecting above a surrounding ice field that may be perpetually covered with ice.</rdfs:comment>
    <rdfs:subClassOf>
      <owl:Restriction>
        <owl:hasValue xml:lang="en">ICEPKN</owl:hasValue>
        <owl:onProperty rdf:resource="jc3iedmBase.owl#geographic-feature-type-subcategory-code"/>
      </owl:Restriction>
    </rdfs:subClassOf>
  </owl:Class>
  <owl:Class rdf:ID="Raydist_non-director">
    <rdfs:subClassOf rdf:resource="jc3iedmSubOnt.owl#ELECTRONIC-EQUIPMENT-TYPE-Navigational_aid"/>
    <rdfs:subClassOf>
      <owl:Restriction>
        <owl:hasValue xml:lang="en">RYDSTN</owl:hasValue>
        <owl:onProperty rdf:resource="jc3iedmBase.owl#electronic-equipment-type-subcategory-code"/>
      </owl:Restriction>
    </rdfs:subClassOf>
    <rdfs:label xml:lang="en">Raydist non-director</rdfs:label>
    <rdfs:comment xml:lang="en">No definition provided in ADatP-3 Baseline 13.1 FFIRN/FUD 1200/1.</rdfs:comment>
  </owl:Class>
  <owl:Class rdf:about="#Harbour,_natural">
    <rdfs:subClassOf rdf:resource="jc3iedmSubOnt.owl#GEOGRAPHIC-FEATURE-TYPE-Coastal_hydrography"/>
    <rdfs:subClassOf rdf:resource="jc3iedmSubOnt.owl#GEOGRAPHIC-FEATURE-Liquid_surface"/>
    <rdfs:subClassOf>
      <owl:Restriction>
        <owl:hasValue xml:lang="en">HRBRNT</owl:hasValue>
        <owl:onProperty rdf:resource="jc3iedmBase.owl#geographic-feature-type-subcategory-code"/>
      </owl:Restriction>
    </rdfs:subClassOf>
    <rdfs:label xml:lang="en">Harbour, natural</rdfs:label>
    <rdfs:comment xml:lang="en">A place of shelter for ships; where they may lie close to and sheltered by the shore or by works extended from it.</rdfs:comment>
    <rdfs:subClassOf>
      <owl:Restriction>
        <owl:hasValue xml:lang="en">HRBRNT</owl:hasValue>
        <owl:onProperty rdf:resource="jc3iedmBase.owl#geographic-feature-type-subcategory-code"/>
      </owl:Restriction>
    </rdfs:subClassOf>
  </owl:Class>
  <owl:Class rdf:ID="JP-4_fuel">
    <rdfs:subClassOf rdf:resource="jc3iedmSubOnt.owl#CONSUMABLE-MATERIEL-TYPE-Fuel"/>
    <rdfs:subClassOf>
      <owl:Restriction>
        <owl:hasValue xml:lang="en">JP4F</owl:hasValue>
        <owl:onProperty rdf:resource="jc3iedmBase.owl#consumable-materiel-type-subcategory-code"/>
      </owl:Restriction>
    </rdfs:subClassOf>
    <rdfs:label xml:lang="en">JP-4 fuel</rdfs:label>
    <rdfs:comment xml:lang="en">A wide cut gasoline type fuel. Specification MIL-T-5624, interchangeable with AVTAG/FSII, NATO F-40.</rdfs:comment>
  </owl:Class>
  <owl:Class rdf:about="#Wagon,_mineral">
    <rdfs:subClassOf rdf:resource="jc3iedmSubOnt.owl#RAILCAR-TYPE-Rolling_stock"/>
    <rdfs:subClassOf>
      <owl:Restriction>
        <owl:hasValue xml:lang="en">WGNMNR</owl:hasValue>
        <owl:onProperty rdf:resource="jc3iedmBase.owl#railcar-type-subcategory-code"/>
      </owl:Restriction>
    </rdfs:subClassOf>
    <rdfs:label xml:lang="en">Wagon, mineral</rdfs:label>
    <rdfs:comment xml:lang="en">Rolling stock used to move bulk mineral by rail with unloading facilities from either side.</rdfs:comment>
  </owl:Class>
  <owl:Class rdf:ID="Transport">
    <rdfs:subClassOf rdf:resource="jc3iedmSubOnt.owl#AIRCRAFT-TYPE-Fixed_wing"/>
    <rdfs:subClassOf rdf:resource="jc3iedmSubOnt.owl#AIRCRAFT-TYPE-Rotary_wing"/>
    <rdfs:subClassOf>
      <owl:Restriction>
        <owl:hasValue xml:lang="en">CARGO</owl:hasValue>
        <owl:onProperty rdf:resource="jc3iedmBase.owl#aircraft-type-airframe-design-code"/>
      </owl:Restriction>
    </rdfs:subClassOf>
    <rdfs:label xml:lang="en">Transport</rdfs:label>
    <rdfs:comment xml:lang="en">An aircraft designed primarily for the carriage of personnel and/or cargo, and/or fuel.</rdfs:comment>
    <rdfs:subClassOf>
      <owl:Restriction>
        <owl:hasValue xml:lang="en">CARGO</owl:hasValue>
        <owl:onProperty rdf:resource="jc3iedmBase.owl#aircraft-type-airframe-design-code"/>
      </owl:Restriction>
    </rdfs:subClassOf>
  </owl:Class>
  <owl:Class rdf:about="#Wagon,_special_purpose">
    <rdfs:subClassOf rdf:resource="jc3iedmSubOnt.owl#RAILCAR-TYPE-Rolling_stock"/>
    <rdfs:subClassOf>
      <owl:Restriction>
        <owl:hasValue xml:lang="en">WGNSPP</owl:hasValue>
        <owl:onProperty rdf:resource="jc3iedmBase.owl#railcar-type-subcategory-code"/>
      </owl:Restriction>
    </rdfs:subClassOf>
    <rdfs:label xml:lang="en">Wagon, special purpose</rdfs:label>
    <rdfs:comment xml:lang="en">Rolling stock used to move specialised or outsized loads by rail, for example MBTs, other outsized loads.</rdfs:comment>
  </owl:Class>
  <owl:Class rdf:ID="Slightly_incapacitated">
    <rdfs:subClassOf>
      <owl:Restriction>
        <owl:hasValue xml:lang="en">SI</owl:hasValue>
        <owl:onProperty rdf:resource="jc3iedmBase.owl#person-status-physical-status-code"/>
      </owl:Restriction>
    </rdfs:subClassOf>
    <rdfs:subClassOf>
      <owl:Restriction>
        <owl:hasValue xml:lang="en">SI</owl:hasValue>
        <owl:onProperty rdf:resource="jc3iedmBase.owl#person-status-physical-status-code"/>
      </owl:Restriction>
    </rdfs:subClassOf>
    <rdfs:subClassOf>
      <owl:Restriction>
        <owl:hasValue xml:lang="en">SI</owl:hasValue>
        <owl:onProperty rdf:resource="jc3iedmBase.owl#person-status-physical-status-code"/>
      </owl:Restriction>
    </rdfs:subClassOf>
    <rdfs:label xml:lang="en">Slightly incapacitated</rdfs:label>
    <rdfs:comment xml:lang="en">A status indicating that a PERSON is incapacitated, but without any major reduction of normal physical capabilities.</rdfs:comment>
    <rdfs:subClassOf>
      <owl:Restriction>
        <owl:hasValue xml:lang="en">SI</owl:hasValue>
        <owl:onProperty rdf:resource="jc3iedmBase.owl#person-status-physical-status-code"/>
      </owl:Restriction>
    </rdfs:subClassOf>
    <rdfs:subClassOf>
      <owl:Restriction>
        <owl:hasValue xml:lang="en">SI</owl:hasValue>
        <owl:onProperty rdf:resource="jc3iedmBase.owl#person-status-physical-status-code"/>
      </owl:Restriction>
    </rdfs:subClassOf>
    <rdfs:subClassOf>
      <owl:Restriction>
        <owl:hasValue xml:lang="en">SI</owl:hasValue>
        <owl:onProperty rdf:resource="jc3iedmBase.owl#person-status-physical-status-code"/>
      </owl:Restriction>
    </rdfs:subClassOf>
    <rdfs:subClassOf>
      <owl:Restriction>
        <owl:hasValue xml:lang="en">SI</owl:hasValue>
        <owl:onProperty rdf:resource="jc3iedmBase.owl#person-status-physical-status-code"/>
      </owl:Restriction>
    </rdfs:subClassOf>
    <rdfs:subClassOf>
      <owl:Restriction>
        <owl:hasValue xml:lang="en">SI</owl:hasValue>
        <owl:onProperty rdf:resource="jc3iedmBase.owl#person-status-physical-status-code"/>
      </owl:Restriction>
    </rdfs:subClassOf>
  </owl:Class>
  <owl:Class rdf:ID="UN_Dangerous_Goods_NUM_1017">
    <rdfs:subClassOf>
      <owl:Restriction>
        <owl:hasValue xml:lang="en">1017</owl:hasValue>
        <owl:onProperty rdf:resource="jc3iedmBase.owl#consumable-materiel-type-united-nations-number-code"/>
      </owl:Restriction>
    </rdfs:subClassOf>
    <rdfs:label xml:lang="en">UN Dangerous Goods # 1017</rdfs:label>
    <rdfs:comment xml:lang="en">Chlorine. Includes the agent(s): chlorine.</rdfs:comment>
    <rdfs:subClassOf>
      <owl:Restriction>
        <owl:hasValue xml:lang="en">1017</owl:hasValue>
        <owl:onProperty rdf:resource="jc3iedmBase.owl#consumable-materiel-type-united-nations-number-code"/>
      </owl:Restriction>
    </rdfs:subClassOf>
  </owl:Class>
  <owl:Class rdf:ID="JP-7_fuel">
    <rdfs:subClassOf rdf:resource="jc3iedmSubOnt.owl#CONSUMABLE-MATERIEL-TYPE-Fuel"/>
    <rdfs:subClassOf>
      <owl:Restriction>
        <owl:hasValue xml:lang="en">JP7F</owl:hasValue>
        <owl:onProperty rdf:resource="jc3iedmBase.owl#consumable-materiel-type-subcategory-code"/>
      </owl:Restriction>
    </rdfs:subClassOf>
    <rdfs:label xml:lang="en">JP-7 fuel</rdfs:label>
    <rdfs:comment xml:lang="en">A kerosene type fuel of low volatility and high thermal stability. Specification MIL-T-38219.</rdfs:comment>
  </owl:Class>
  <owl:Class rdf:ID="UN_Dangerous_Goods_NUM_3327">
    <rdfs:subClassOf>
      <owl:Restriction>
        <owl:hasValue xml:lang="en">3327</owl:hasValue>
        <owl:onProperty rdf:resource="jc3iedmBase.owl#consumable-materiel-type-united-nations-number-code"/>
      </owl:Restriction>
    </rdfs:subClassOf>
    <rdfs:label xml:lang="en">UN Dangerous Goods # 3327</rdfs:label>
    <rdfs:comment xml:lang="en">Radioactive material, type A package, fissile, non-special form.</rdfs:comment>
  </owl:Class>
  <owl:Class rdf:ID="Grenade_launcher">
    <rdfs:subClassOf rdf:resource="jc3iedmSubOnt.owl#WEAPON-TYPE-Small_arms"/>
    <rdfs:subClassOf rdf:resource="jc3iedmSubOnt.owl#WEAPON-TYPE-Anti-tank"/>
    <rdfs:subClassOf>
      <owl:Restriction>
        <owl:hasValue xml:lang="en">GRENLN</owl:hasValue>
        <owl:onProperty rdf:resource="jc3iedmBase.owl#weapon-type-subcategory-code"/>
      </owl:Restriction>
    </rdfs:subClassOf>
    <rdfs:label xml:lang="en">Grenade launcher</rdfs:label>
    <rdfs:comment xml:lang="en">A structural device designed to support and hold a grenade in position for firing.</rdfs:comment>
    <rdfs:subClassOf>
      <owl:Restriction>
        <owl:hasValue xml:lang="en">GRENLN</owl:hasValue>
        <owl:onProperty rdf:resource="jc3iedmBase.owl#weapon-type-subcategory-code"/>
      </owl:Restriction>
    </rdfs:subClassOf>
  </owl:Class>
  <owl:Class rdf:ID="Combat_direction_finding">
    <rdfs:subClassOf rdf:resource="jc3iedmSubOnt.owl#ELECTRONIC-EQUIPMENT-TYPE-Electronic_warfare"/>
    <rdfs:subClassOf>
      <owl:Restriction>
        <owl:hasValue xml:lang="en">CBDCFD</owl:hasValue>
        <owl:onProperty rdf:resource="jc3iedmBase.owl#electronic-equipment-type-subcategory-code"/>
      </owl:Restriction>
    </rdfs:subClassOf>
    <rdfs:label xml:lang="en">Combat direction finding</rdfs:label>
    <rdfs:comment xml:lang="en">A system that may be hardened or ruggedized for use in combat employed for determining the bearing of an electromagnetic emission.</rdfs:comment>
  </owl:Class>
  <owl:Class rdf:ID="Flooded_area">
    <rdfs:subClassOf rdf:resource="jc3iedmSubOnt.owl#GEOGRAPHIC-FEATURE-TYPE-Inland_water"/>
    <rdfs:subClassOf rdf:resource="jc3iedmSubOnt.owl#GEOGRAPHIC-FEATURE-Liquid_surface"/>
    <rdfs:subClassOf>
      <owl:Restriction>
        <owl:hasValue xml:lang="en">FLDDAR</owl:hasValue>
        <owl:onProperty rdf:resource="jc3iedmBase.owl#geographic-feature-type-subcategory-code"/>
      </owl:Restriction>
    </rdfs:subClassOf>
    <rdfs:label xml:lang="en">Flooded area</rdfs:label>
    <rdfs:comment xml:lang="en">Land subject to controlled inundation (i.e. flooded by the regulation of the level of water impounded by a dam or beaver dam), and is normally associated with permanently flooded areas in which trees are still standing. Also known as inundated land.</rdfs:comment>
    <rdfs:subClassOf>
      <owl:Restriction>
        <owl:hasValue xml:lang="en">FLDDAR</owl:hasValue>
        <owl:onProperty rdf:resource="jc3iedmBase.owl#geographic-feature-type-subcategory-code"/>
      </owl:Restriction>
    </rdfs:subClassOf>
  </owl:Class>
  <owl:Class rdf:ID="UN_Dangerous_Goods_NUM_1754">
    <rdfs:subClassOf>
      <owl:Restriction>
        <owl:hasValue xml:lang="en">1754</owl:hasValue>
        <owl:onProperty rdf:resource="jc3iedmBase.owl#consumable-materiel-type-united-nations-number-code"/>
      </owl:Restriction>
    </rdfs:subClassOf>
    <rdfs:label xml:lang="en">UN Dangerous Goods # 1754</rdfs:label>
    <rdfs:comment xml:lang="en">Chlorosulphonic acid (with or without sulphur trioxide). Includes the agent(s): chlorosulphonic acid.</rdfs:comment>
    <rdfs:subClassOf>
      <owl:Restriction>
        <owl:hasValue xml:lang="en">1754</owl:hasValue>
        <owl:onProperty rdf:resource="jc3iedmBase.owl#consumable-materiel-type-united-nations-number-code"/>
      </owl:Restriction>
    </rdfs:subClassOf>
  </owl:Class>
  <owl:Class rdf:ID="Poster">
    <rdfs:subClassOf rdf:resource="jc3iedmSubOnt.owl#CONSUMABLE-MATERIEL-TYPE-General_supplies"/>
    <rdfs:subClassOf>
      <owl:Restriction>
        <owl:hasValue xml:lang="en">POSTER</owl:hasValue>
        <owl:onProperty rdf:resource="jc3iedmBase.owl#consumable-materiel-type-subcategory-code"/>
      </owl:Restriction>
    </rdfs:subClassOf>
    <rdfs:label xml:lang="en">Poster</rdfs:label>
    <rdfs:comment xml:lang="en">A placard posted or displayed in a public place as an announcement or advertisement.</rdfs:comment>
  </owl:Class>
  <owl:Class rdf:ID="Paint_brush">
    <rdfs:subClassOf rdf:resource="jc3iedmSubOnt.owl#CONSUMABLE-MATERIEL-TYPE-General_supplies"/>
    <rdfs:subClassOf>
      <owl:Restriction>
        <owl:hasValue xml:lang="en">PNTBRS</owl:hasValue>
        <owl:onProperty rdf:resource="jc3iedmBase.owl#consumable-materiel-type-subcategory-code"/>
      </owl:Restriction>
    </rdfs:subClassOf>
    <rdfs:label xml:lang="en">Paint brush</rdfs:label>
    <rdfs:comment xml:lang="en">A device designed to apply paint.</rdfs:comment>
  </owl:Class>
  <owl:Class rdf:ID="UN_Dangerous_Goods_NUM_1294">
    <rdfs:subClassOf>
      <owl:Restriction>
        <owl:hasValue xml:lang="en">1294</owl:hasValue>
        <owl:onProperty rdf:resource="jc3iedmBase.owl#consumable-materiel-type-united-nations-number-code"/>
      </owl:Restriction>
    </rdfs:subClassOf>
    <rdfs:label xml:lang="en">UN Dangerous Goods # 1294</rdfs:label>
    <rdfs:comment xml:lang="en">Toluene. Includes the agent(s): toluene.</rdfs:comment>
    <rdfs:subClassOf>
      <owl:Restriction>
        <owl:hasValue xml:lang="en">1294</owl:hasValue>
        <owl:onProperty rdf:resource="jc3iedmBase.owl#consumable-materiel-type-united-nations-number-code"/>
      </owl:Restriction>
    </rdfs:subClassOf>
  </owl:Class>
  <owl:Class rdf:ID="Geothermal_feature">
    <rdfs:subClassOf rdf:resource="jc3iedmSubOnt.owl#GEOGRAPHIC-FEATURE-Solid_surface"/>
    <rdfs:subClassOf rdf:resource="jc3iedmSubOnt.owl#GEOGRAPHIC-FEATURE-TYPE-Landform"/>
    <rdfs:subClassOf>
      <owl:Restriction>
        <owl:hasValue xml:lang="en">GEOTHR</owl:hasValue>
        <owl:onProperty rdf:resource="jc3iedmBase.owl#geographic-feature-type-subcategory-code"/>
      </owl:Restriction>
    </rdfs:subClassOf>
    <rdfs:label xml:lang="en">Geothermal feature</rdfs:label>
    <rdfs:comment xml:lang="en">A terrain surface feature controlled by or derived from the heat of the Earths interior.</rdfs:comment>
    <rdfs:subClassOf>
      <owl:Restriction>
        <owl:hasValue xml:lang="en">GEOTHR</owl:hasValue>
        <owl:onProperty rdf:resource="jc3iedmBase.owl#geographic-feature-type-subcategory-code"/>
      </owl:Restriction>
    </rdfs:subClassOf>
  </owl:Class>
  <owl:Class rdf:ID="Hashish">
    <rdfs:subClassOf rdf:resource="jc3iedmSubOnt.owl#CONSUMABLE-MATERIEL-TYPE-Drug"/>
    <rdfs:subClassOf>
      <owl:Restriction>
        <owl:hasValue xml:lang="en">HASHSH</owl:hasValue>
        <owl:onProperty rdf:resource="jc3iedmBase.owl#consumable-materiel-type-subcategory-code"/>
      </owl:Restriction>
    </rdfs:subClassOf>
    <rdfs:label xml:lang="en">Hashish</rdfs:label>
    <rdfs:comment xml:lang="en">A resinous product of the top leaves and tender parts of hemp, smoked or chewed for its narcotic effects.</rdfs:comment>
  </owl:Class>
  <owl:Class rdf:about="#Direct_fire_gun,_medium">
    <rdfs:subClassOf rdf:resource="jc3iedmSubOnt.owl#WEAPON-TYPE-Small_arms"/>
    <rdfs:subClassOf>
      <owl:Restriction>
        <owl:hasValue xml:lang="en">DFGNMD</owl:hasValue>
        <owl:onProperty rdf:resource="jc3iedmBase.owl#weapon-type-subcategory-code"/>
      </owl:Restriction>
    </rdfs:subClassOf>
    <rdfs:label xml:lang="en">Direct fire gun, medium</rdfs:label>
    <rdfs:comment xml:lang="en">No definition provided in APP-6A.</rdfs:comment>
  </owl:Class>
  <owl:Class rdf:ID="Magnetic">
    <rdfs:subClassOf rdf:resource="jc3iedmSubOnt.owl#AMMUNITION-TYPE-Mine,_deep_moored"/>
    <rdfs:subClassOf rdf:resource="jc3iedmSubOnt.owl#AMMUNITION-TYPE-Mine,_seabed_-_explosive_charge_less_than_500kg"/>
    <rdfs:subClassOf rdf:resource="jc3iedmSubOnt.owl#AMMUNITION-TYPE-Mine,_maritime,_moving"/>
    <rdfs:subClassOf>
      <owl:Restriction>
        <owl:hasValue xml:lang="en">MAGNET</owl:hasValue>
        <owl:onProperty rdf:resource="jc3iedmBase.owl#ammunition-type-mine-maritime-firing-code"/>
      </owl:Restriction>
    </rdfs:subClassOf>
    <rdfs:subClassOf rdf:resource="jc3iedmSubOnt.owl#AMMUNITION-TYPE-Mine,_moored"/>
    <rdfs:label xml:lang="en">Magnetic</rdfs:label>
    <rdfs:subClassOf rdf:resource="jc3iedmSubOnt.owl#AMMUNITION-TYPE-Mine,_shallow_moored"/>
    <rdfs:subClassOf rdf:resource="jc3iedmSubOnt.owl#AMMUNITION-TYPE-Moving_mine,_sea"/>
    <rdfs:subClassOf rdf:resource="jc3iedmSubOnt.owl#AMMUNITION-TYPE-Mine,_not_known"/>
    <rdfs:comment xml:lang="en">A (maritime) mine firing mechanism with a magnetic influence circuit that responds to the magnetic field of a ship.</rdfs:comment>
    <rdfs:subClassOf rdf:resource="jc3iedmSubOnt.owl#AMMUNITION-TYPE-Sea_mine"/>
    <rdfs:subClassOf rdf:resource="jc3iedmSubOnt.owl#AMMUNITION-TYPE-Seabed_mine"/>
    <rdfs:subClassOf rdf:resource="jc3iedmSubOnt.owl#AMMUNITION-TYPE-Mine,_not_otherwise_specified"/>
    <rdfs:subClassOf>
      <owl:Restriction>
        <owl:hasValue xml:lang="en">MAGNET</owl:hasValue>
        <owl:onProperty rdf:resource="jc3iedmBase.owl#ammunition-type-mine-maritime-firing-code"/>
      </owl:Restriction>
    </rdfs:subClassOf>
    <rdfs:subClassOf rdf:resource="jc3iedmSubOnt.owl#AMMUNITION-TYPE-Mine,_seabed_-_explosive_charge_500kg_or_greater"/>
  </owl:Class>
  <owl:Class rdf:about="#Sweep,_hovercraft_magnetic">
    <rdfs:subClassOf rdf:resource="jc3iedmSubOnt.owl#MARITIME-EQUIPMENT-TYPE-Sweep"/>
    <rdfs:subClassOf>
      <owl:Restriction>
        <owl:hasValue xml:lang="en">SWPHVM</owl:hasValue>
        <owl:onProperty rdf:resource="jc3iedmBase.owl#maritime-equipment-type-subcategory-code"/>
      </owl:Restriction>
    </rdfs:subClassOf>
    <rdfs:label xml:lang="en">Sweep, hovercraft magnetic</rdfs:label>
    <rdfs:comment xml:lang="en">Equipment mounted on a hovercraft designed to locate mines by use of a conducting cable through which is passed a high current, towed behind a minesweeper hovercraft.</rdfs:comment>
  </owl:Class>
  <owl:Class rdf:ID="Tactical_air_reconnaissance_photo_system">
    <rdfs:subClassOf rdf:resource="jc3iedmSubOnt.owl#ELECTRONIC-EQUIPMENT-TYPE-Sensor"/>
    <rdfs:subClassOf>
      <owl:Restriction>
        <owl:hasValue xml:lang="en">TARPHS</owl:hasValue>
        <owl:onProperty rdf:resource="jc3iedmBase.owl#electronic-equipment-type-subcategory-code"/>
      </owl:Restriction>
    </rdfs:subClassOf>
    <rdfs:label xml:lang="en">Tactical air reconnaissance photo system</rdfs:label>
    <rdfs:comment xml:lang="en">Photographic sensor that obtains photographic information from the air that is installed on a tactical air vehicle.</rdfs:comment>
  </owl:Class>
  <owl:Class rdf:about="#Sweep,_magnetic_antenna">
    <rdfs:subClassOf rdf:resource="jc3iedmSubOnt.owl#MARITIME-EQUIPMENT-TYPE-Sweep"/>
    <rdfs:subClassOf>
      <owl:Restriction>
        <owl:hasValue xml:lang="en">SWPMGA</owl:hasValue>
        <owl:onProperty rdf:resource="jc3iedmBase.owl#maritime-equipment-type-subcategory-code"/>
      </owl:Restriction>
    </rdfs:subClassOf>
    <rdfs:label xml:lang="en">Sweep, magnetic antenna</rdfs:label>
    <rdfs:comment xml:lang="en">Equipment designed to locate mines in the lane swept with either a single or multiple ship rig and is designed to ensure that the sweep wire is not brought into contact with the mines antenna until the mine is a safe distance astern.</rdfs:comment>
  </owl:Class>
  <owl:Class rdf:ID="Hypertext_transfer_protocol">
    <rdfs:subClassOf rdf:resource="jc3iedmSubOnt.owl#NETWORK-SERVICE-Data_transfer"/>
    <rdfs:subClassOf>
      <owl:Restriction>
        <owl:hasValue xml:lang="en">HTTP</owl:hasValue>
        <owl:onProperty rdf:resource="jc3iedmBase.owl#network-service-subcategory-code"/>
      </owl:Restriction>
    </rdfs:subClassOf>
    <rdfs:label xml:lang="en">Hypertext transfer protocol</rdfs:label>
    <rdfs:comment xml:lang="en">A service provided through Hypertext Transfer Protocol (HTTP) that is an application-level protocol with the lightness and speed necessary for distributed, collaborative, hypermedia information systems.</rdfs:comment>
  </owl:Class>
  <owl:Class rdf:about="#Sweep,_magnetic_open_loop">
    <rdfs:subClassOf rdf:resource="jc3iedmSubOnt.owl#MARITIME-EQUIPMENT-TYPE-Sweep"/>
    <rdfs:subClassOf>
      <owl:Restriction>
        <owl:hasValue xml:lang="en">SWPMGO</owl:hasValue>
        <owl:onProperty rdf:resource="jc3iedmBase.owl#maritime-equipment-type-subcategory-code"/>
      </owl:Restriction>
    </rdfs:subClassOf>
    <rdfs:label xml:lang="en">Sweep, magnetic open loop</rdfs:label>
    <rdfs:comment xml:lang="en">Equipment designed to locate mines by use of a conducting cable, open loop shaped through which is passed a high current, towed behind a minesweeper.</rdfs:comment>
  </owl:Class>
  <owl:Class rdf:ID="Quinuclidinyl_benzilate">
    <rdfs:subClassOf rdf:resource="jc3iedmSubOnt.owl#CHEMICAL-MATERIEL-TYPE-Vomiting_agent"/>
    <rdfs:subClassOf rdf:resource="jc3iedmSubOnt.owl#CHEMICAL-MATERIEL-TYPE-Incapacitating_agent"/>
    <rdfs:subClassOf>
      <owl:Restriction>
        <owl:hasValue xml:lang="en">QNCLDN</owl:hasValue>
        <owl:onProperty rdf:resource="jc3iedmBase.owl#chemical-materiel-type-subcategory-code"/>
      </owl:Restriction>
    </rdfs:subClassOf>
    <rdfs:label xml:lang="en">Quinuclidinyl benzilate</rdfs:label>
    <rdfs:comment xml:lang="en">A poisonous gas formerly used in warfare.</rdfs:comment>
    <rdfs:subClassOf>
      <owl:Restriction>
        <owl:hasValue xml:lang="en">QNCLDN</owl:hasValue>
        <owl:onProperty rdf:resource="jc3iedmBase.owl#chemical-materiel-type-subcategory-code"/>
      </owl:Restriction>
    </rdfs:subClassOf>
  </owl:Class>
  <owl:Class rdf:ID="UN_Dangerous_Goods_NUM_3328">
    <rdfs:subClassOf>
      <owl:Restriction>
        <owl:hasValue xml:lang="en">3328</owl:hasValue>
        <owl:onProperty rdf:resource="jc3iedmBase.owl#consumable-materiel-type-united-nations-number-code"/>
      </owl:Restriction>
    </rdfs:subClassOf>
    <rdfs:label xml:lang="en">UN Dangerous Goods # 3328</rdfs:label>
    <rdfs:comment xml:lang="en">Radioactive material, type B(U) package, fissile.</rdfs:comment>
  </owl:Class>
  <owl:Class rdf:about="#Combination,_overlap">
    <rdfs:subClassOf rdf:resource="jc3iedmSubOnt.owl#AMMUNITION-TYPE-Mine,_moored"/>
    <rdfs:subClassOf>
      <owl:Restriction>
        <owl:hasValue xml:lang="en">COMBIN</owl:hasValue>
        <owl:onProperty rdf:resource="jc3iedmBase.owl#ammunition-type-mine-maritime-firing-code"/>
      </owl:Restriction>
    </rdfs:subClassOf>
    <rdfs:subClassOf rdf:resource="jc3iedmSubOnt.owl#AMMUNITION-TYPE-Moving_mine,_sea"/>
    <rdfs:label xml:lang="en">Combination, overlap</rdfs:label>
    <rdfs:subClassOf rdf:resource="jc3iedmSubOnt.owl#AMMUNITION-TYPE-Mine,_seabed_-_explosive_charge_less_than_500kg"/>
    <rdfs:subClassOf rdf:resource="jc3iedmSubOnt.owl#AMMUNITION-TYPE-Mine,_deep_moored"/>
    <rdfs:comment xml:lang="en">A (maritime) mine firing mechanism that fires depending upon the previous simultaneous or subsequent reception of signals resulting from other influences, such as acoustic and pressure.</rdfs:comment>
    <rdfs:subClassOf rdf:resource="jc3iedmSubOnt.owl#AMMUNITION-TYPE-Sea_mine"/>
    <rdfs:subClassOf rdf:resource="jc3iedmSubOnt.owl#AMMUNITION-TYPE-Mine,_not_known"/>
    <rdfs:subClassOf rdf:resource="jc3iedmSubOnt.owl#AMMUNITION-TYPE-Mine,_not_otherwise_specified"/>
    <rdfs:subClassOf rdf:resource="jc3iedmSubOnt.owl#AMMUNITION-TYPE-Seabed_mine"/>
    <rdfs:subClassOf rdf:resource="jc3iedmSubOnt.owl#AMMUNITION-TYPE-Mine,_maritime,_moving"/>
    <rdfs:subClassOf rdf:resource="jc3iedmSubOnt.owl#AMMUNITION-TYPE-Mine,_shallow_moored"/>
    <rdfs:subClassOf rdf:resource="jc3iedmSubOnt.owl#AMMUNITION-TYPE-Mine,_seabed_-_explosive_charge_500kg_or_greater"/>
    <rdfs:subClassOf>
      <owl:Restriction>
        <owl:hasValue xml:lang="en">COMBIN</owl:hasValue>
        <owl:onProperty rdf:resource="jc3iedmBase.owl#ammunition-type-mine-maritime-firing-code"/>
      </owl:Restriction>
    </rdfs:subClassOf>
  </owl:Class>
  <owl:Class rdf:ID="UN_Dangerous_Goods_NUM_1016">
    <rdfs:subClassOf>
      <owl:Restriction>
        <owl:hasValue xml:lang="en">1016</owl:hasValue>
        <owl:onProperty rdf:resource="jc3iedmBase.owl#consumable-materiel-type-united-nations-number-code"/>
      </owl:Restriction>
    </rdfs:subClassOf>
    <rdfs:label xml:lang="en">UN Dangerous Goods # 1016</rdfs:label>
    <rdfs:comment xml:lang="en">Carbon monoxide, compressed. Includes the agent(s): carbon monoxide.</rdfs:comment>
    <rdfs:subClassOf>
      <owl:Restriction>
        <owl:hasValue xml:lang="en">1016</owl:hasValue>
        <owl:onProperty rdf:resource="jc3iedmBase.owl#consumable-materiel-type-united-nations-number-code"/>
      </owl:Restriction>
    </rdfs:subClassOf>
  </owl:Class>
  <owl:Class rdf:about="#Wagon,_flatbed">
    <rdfs:subClassOf rdf:resource="jc3iedmSubOnt.owl#RAILCAR-TYPE-Rolling_stock"/>
    <rdfs:subClassOf>
      <owl:Restriction>
        <owl:hasValue xml:lang="en">WGNFLB</owl:hasValue>
        <owl:onProperty rdf:resource="jc3iedmBase.owl#railcar-type-subcategory-code"/>
      </owl:Restriction>
    </rdfs:subClassOf>
    <rdfs:label xml:lang="en">Wagon, flatbed</rdfs:label>
    <rdfs:comment xml:lang="en">Rolling stock used to move either large bulky cargoes, for example B vehicles, or large linear cargoes, for example logs/cut timber, replacement sections of track.</rdfs:comment>
  </owl:Class>
  <owl:Class rdf:about="#Jungle,_secondary">
    <rdfs:label xml:lang="en">Jungle, secondary</rdfs:label>
    <rdfs:comment xml:lang="en">An area that has thick undergrowth created through rapid growth after an area of primary jungle has been cleared, movement will be slow and noisy, heat increased due to a lack of canopy and visibility will be reduced to around 20m.</rdfs:comment>
  </owl:Class>
  <owl:Class rdf:ID="Cave">
    <rdfs:subClassOf rdf:resource="jc3iedmSubOnt.owl#GEOGRAPHIC-FEATURE-Solid_surface"/>
    <rdfs:subClassOf rdf:resource="jc3iedmSubOnt.owl#GEOGRAPHIC-FEATURE-TYPE-Landform"/>
    <rdfs:subClassOf>
      <owl:Restriction>
        <owl:hasValue xml:lang="en">CAVE</owl:hasValue>
        <owl:onProperty rdf:resource="jc3iedmBase.owl#geographic-feature-type-subcategory-code"/>
      </owl:Restriction>
    </rdfs:subClassOf>
    <rdfs:label xml:lang="en">Cave</rdfs:label>
    <rdfs:comment xml:lang="en">A natural subterranean chamber or series of chambers open to the Earths surface.</rdfs:comment>
    <rdfs:subClassOf>
      <owl:Restriction>
        <owl:hasValue xml:lang="en">CAVE</owl:hasValue>
        <owl:onProperty rdf:resource="jc3iedmBase.owl#geographic-feature-type-subcategory-code"/>
      </owl:Restriction>
    </rdfs:subClassOf>
  </owl:Class>
  <owl:Class rdf:ID="Link_14">
    <rdfs:subClassOf rdf:resource="jc3iedmSubOnt.owl#NETWORK-SERVICE-Tactical_data_link"/>
    <rdfs:subClassOf>
      <owl:Restriction>
        <owl:hasValue xml:lang="en">LNK14</owl:hasValue>
        <owl:onProperty rdf:resource="jc3iedmBase.owl#network-service-subcategory-code"/>
      </owl:Restriction>
    </rdfs:subClassOf>
    <rdfs:label xml:lang="en">Link 14</rdfs:label>
    <rdfs:comment xml:lang="en">A service that provides the basic elements for the transmission of specific message of Link 14.</rdfs:comment>
  </owl:Class>
  <owl:Class rdf:ID="Trimeric_mustard">
    <rdfs:subClassOf rdf:resource="jc3iedmSubOnt.owl#CHEMICAL-MATERIEL-TYPE-Blood_agent"/>
    <rdfs:subClassOf>
      <owl:Restriction>
        <owl:hasValue xml:lang="en">TRMRCM</owl:hasValue>
        <owl:onProperty rdf:resource="jc3iedmBase.owl#chemical-materiel-type-subcategory-code"/>
      </owl:Restriction>
    </rdfs:subClassOf>
    <rdfs:label xml:lang="en">Trimeric mustard</rdfs:label>
    <rdfs:comment xml:lang="en">A thickened colourless oily liquid, whose vapour is a powerful irritant and vesicant, used in chemical weapons.</rdfs:comment>
  </owl:Class>
  <owl:Class rdf:ID="UN_Dangerous_Goods_NUM_1131">
    <rdfs:subClassOf>
      <owl:Restriction>
        <owl:hasValue xml:lang="en">1131</owl:hasValue>
        <owl:onProperty rdf:resource="jc3iedmBase.owl#consumable-materiel-type-united-nations-number-code"/>
      </owl:Restriction>
    </rdfs:subClassOf>
    <rdfs:label xml:lang="en">UN Dangerous Goods # 1131</rdfs:label>
    <rdfs:comment xml:lang="en">Carbon disulphide. Includes the agent(s): carbon disulphide.</rdfs:comment>
    <rdfs:subClassOf>
      <owl:Restriction>
        <owl:hasValue xml:lang="en">1131</owl:hasValue>
        <owl:onProperty rdf:resource="jc3iedmBase.owl#consumable-materiel-type-united-nations-number-code"/>
      </owl:Restriction>
    </rdfs:subClassOf>
  </owl:Class>
  <owl:Class rdf:about="#Anti-tank_gun,_medium">
    <rdfs:subClassOf rdf:resource="jc3iedmSubOnt.owl#WEAPON-TYPE-Anti-tank"/>
    <rdfs:subClassOf>
      <owl:Restriction>
        <owl:hasValue xml:lang="en">ATGNMD</owl:hasValue>
        <owl:onProperty rdf:resource="jc3iedmBase.owl#weapon-type-subcategory-code"/>
      </owl:Restriction>
    </rdfs:subClassOf>
    <rdfs:label xml:lang="en">Anti-tank gun, medium</rdfs:label>
    <rdfs:comment xml:lang="en">A medium gun designed to destroy tanks.</rdfs:comment>
  </owl:Class>
  <owl:Class rdf:ID="UN_Dangerous_Goods_NUM_2915">
    <rdfs:subClassOf>
      <owl:Restriction>
        <owl:hasValue xml:lang="en">2915</owl:hasValue>
        <owl:onProperty rdf:resource="jc3iedmBase.owl#consumable-materiel-type-united-nations-number-code"/>
      </owl:Restriction>
    </rdfs:subClassOf>
    <rdfs:label xml:lang="en">UN Dangerous Goods # 2915</rdfs:label>
    <rdfs:comment xml:lang="en">Radioactive material, type A package, non-special form, non fissile or fissile-excepted.</rdfs:comment>
  </owl:Class>
  <owl:Class rdf:ID="Moderately_damaged">
    <rdfs:subClassOf>
      <owl:Restriction>
        <owl:hasValue xml:lang="en">MODDAM</owl:hasValue>
        <owl:onProperty rdf:resource="jc3iedmBase.owl#materiel-status-operational-status-qualifier-code"/>
      </owl:Restriction>
    </rdfs:subClassOf>
    <rdfs:comment xml:lang="en">Subjectively judged by the reporting organisation to be moderately damaged.</rdfs:comment>
    <rdfs:subClassOf>
      <owl:Restriction>
        <owl:hasValue xml:lang="en">MODDAM</owl:hasValue>
        <owl:onProperty rdf:resource="jc3iedmBase.owl#facility-status-operational-status-qualifier-code"/>
      </owl:Restriction>
    </rdfs:subClassOf>
    <rdfs:subClassOf>
      <owl:Restriction>
        <owl:hasValue xml:lang="en">MODDAM</owl:hasValue>
        <owl:onProperty rdf:resource="jc3iedmBase.owl#materiel-status-operational-status-qualifier-code"/>
      </owl:Restriction>
    </rdfs:subClassOf>
    <rdfs:subClassOf>
      <owl:Restriction>
        <owl:hasValue xml:lang="en">MODDAM</owl:hasValue>
        <owl:onProperty rdf:resource="jc3iedmBase.owl#facility-status-operational-status-qualifier-code"/>
      </owl:Restriction>
    </rdfs:subClassOf>
    <rdfs:label xml:lang="en">Moderately damaged</rdfs:label>
    <rdfs:subClassOf>
      <owl:Restriction>
        <owl:hasValue xml:lang="en">MODDAM</owl:hasValue>
        <owl:onProperty rdf:resource="jc3iedmBase.owl#organisation-status-operational-status-qualifier-code"/>
      </owl:Restriction>
    </rdfs:subClassOf>
    <rdfs:subClassOf>
      <owl:Restriction>
        <owl:hasValue xml:lang="en">MODDAM</owl:hasValue>
        <owl:onProperty rdf:resource="jc3iedmBase.owl#organisation-status-operational-status-qualifier-code"/>
      </owl:Restriction>
    </rdfs:subClassOf>
    <rdfs:subClassOf>
      <owl:Restriction>
        <owl:hasValue xml:lang="en">MODDAM</owl:hasValue>
        <owl:onProperty rdf:resource="jc3iedmBase.owl#materiel-status-operational-status-qualifier-code"/>
      </owl:Restriction>
    </rdfs:subClassOf>
    <rdfs:subClassOf>
      <owl:Restriction>
        <owl:hasValue xml:lang="en">MODDAM</owl:hasValue>
        <owl:onProperty rdf:resource="jc3iedmBase.owl#facility-status-operational-status-qualifier-code"/>
      </owl:Restriction>
    </rdfs:subClassOf>
    <rdfs:subClassOf>
      <owl:Restriction>
        <owl:hasValue xml:lang="en">MODDAM</owl:hasValue>
        <owl:onProperty rdf:resource="jc3iedmBase.owl#organisation-status-operational-status-qualifier-code"/>
      </owl:Restriction>
    </rdfs:subClassOf>
  </owl:Class>
  <owl:Class rdf:about="#Wagon,_hopper">
    <rdfs:subClassOf rdf:resource="jc3iedmSubOnt.owl#RAILCAR-TYPE-Rolling_stock"/>
    <rdfs:subClassOf>
      <owl:Restriction>
        <owl:hasValue xml:lang="en">WGNHPR</owl:hasValue>
        <owl:onProperty rdf:resource="jc3iedmBase.owl#railcar-type-subcategory-code"/>
      </owl:Restriction>
    </rdfs:subClassOf>
    <rdfs:label xml:lang="en">Wagon, hopper</rdfs:label>
    <rdfs:comment xml:lang="en">Rolling stock used to move bulk loose material by rail and unloaded by gravity through bottom doors. [Mineral or foodstuffs e.g. grain are typical cargoes.]</rdfs:comment>
  </owl:Class>
  <owl:Class rdf:ID="Pingo">
    <rdfs:subClassOf rdf:resource="jc3iedmSubOnt.owl#GEOGRAPHIC-FEATURE-TYPE-Snow/ice"/>
    <rdfs:subClassOf rdf:resource="jc3iedmSubOnt.owl#GEOGRAPHIC-FEATURE-Solid_surface"/>
    <rdfs:subClassOf>
      <owl:Restriction>
        <owl:hasValue xml:lang="en">PINGO</owl:hasValue>
        <owl:onProperty rdf:resource="jc3iedmBase.owl#geographic-feature-type-subcategory-code"/>
      </owl:Restriction>
    </rdfs:subClassOf>
    <rdfs:label xml:lang="en">Pingo</rdfs:label>
    <rdfs:comment xml:lang="en">A cone or dome shaped mound or hill of peat or soil, usually with a core of ice. It is found in tundra regions and is produced by the pressure of water or ice accumulating underground and pushing upward.</rdfs:comment>
    <rdfs:subClassOf>
      <owl:Restriction>
        <owl:hasValue xml:lang="en">PINGO</owl:hasValue>
        <owl:onProperty rdf:resource="jc3iedmBase.owl#geographic-feature-type-subcategory-code"/>
      </owl:Restriction>
    </rdfs:subClassOf>
  </owl:Class>
  <owl:Class rdf:ID="UN_Dangerous_Goods_NUM_2442">
    <rdfs:subClassOf>
      <owl:Restriction>
        <owl:hasValue xml:lang="en">2442</owl:hasValue>
        <owl:onProperty rdf:resource="jc3iedmBase.owl#consumable-materiel-type-united-nations-number-code"/>
      </owl:Restriction>
    </rdfs:subClassOf>
    <rdfs:label xml:lang="en">UN Dangerous Goods # 2442</rdfs:label>
    <rdfs:comment xml:lang="en">Trichloroacetyl chloride. Includes the agent(s): trichloroacetyl chloride.</rdfs:comment>
    <rdfs:subClassOf>
      <owl:Restriction>
        <owl:hasValue xml:lang="en">2442</owl:hasValue>
        <owl:onProperty rdf:resource="jc3iedmBase.owl#consumable-materiel-type-united-nations-number-code"/>
      </owl:Restriction>
    </rdfs:subClassOf>
  </owl:Class>
  <owl:Class rdf:ID="UN_Dangerous_Goods_NUM_2195">
    <rdfs:subClassOf>
      <owl:Restriction>
        <owl:hasValue xml:lang="en">2195</owl:hasValue>
        <owl:onProperty rdf:resource="jc3iedmBase.owl#consumable-materiel-type-united-nations-number-code"/>
      </owl:Restriction>
    </rdfs:subClassOf>
    <rdfs:label xml:lang="en">UN Dangerous Goods # 2195</rdfs:label>
    <rdfs:comment xml:lang="en">Tellurium hexafluoride. Includes the agent(s): tellurium hexafluoride.</rdfs:comment>
    <rdfs:subClassOf>
      <owl:Restriction>
        <owl:hasValue xml:lang="en">2195</owl:hasValue>
        <owl:onProperty rdf:resource="jc3iedmBase.owl#consumable-materiel-type-united-nations-number-code"/>
      </owl:Restriction>
    </rdfs:subClassOf>
  </owl:Class>
  <owl:Class rdf:ID="Vertical_line_array_difar">
    <rdfs:subClassOf rdf:resource="jc3iedmSubOnt.owl#ELECTRONIC-EQUIPMENT-TYPE-Sensor"/>
    <rdfs:subClassOf>
      <owl:Restriction>
        <owl:hasValue xml:lang="en">VLAD</owl:hasValue>
        <owl:onProperty rdf:resource="jc3iedmBase.owl#electronic-equipment-type-subcategory-code"/>
      </owl:Restriction>
    </rdfs:subClassOf>
    <rdfs:label xml:lang="en">Vertical line array difar</rdfs:label>
    <rdfs:comment xml:lang="en">An expendable, non-repairable sonobuoy known as VLAD (DIFAR is short for Directional Frequency Analysis and Recording System) designed to increase the detection of signals of interest in an environment where there is an ever-increasing amount of ambient noise.</rdfs:comment>
  </owl:Class>
  <owl:Class rdf:ID="UN_Dangerous_Goods_NUM_2831">
    <rdfs:subClassOf>
      <owl:Restriction>
        <owl:hasValue xml:lang="en">2831</owl:hasValue>
        <owl:onProperty rdf:resource="jc3iedmBase.owl#consumable-materiel-type-united-nations-number-code"/>
      </owl:Restriction>
    </rdfs:subClassOf>
    <rdfs:label xml:lang="en">UN Dangerous Goods # 2831</rdfs:label>
    <rdfs:comment xml:lang="en">1,1,1-trichloroethane. Includes the agent(s): 1,1,1-trichloroethane.</rdfs:comment>
    <rdfs:subClassOf>
      <owl:Restriction>
        <owl:hasValue xml:lang="en">2831</owl:hasValue>
        <owl:onProperty rdf:resource="jc3iedmBase.owl#consumable-materiel-type-united-nations-number-code"/>
      </owl:Restriction>
    </rdfs:subClassOf>
  </owl:Class>
  <owl:Class rdf:ID="UN_Dangerous_Goods_NUM_1067">
    <rdfs:subClassOf>
      <owl:Restriction>
        <owl:hasValue xml:lang="en">1067</owl:hasValue>
        <owl:onProperty rdf:resource="jc3iedmBase.owl#consumable-materiel-type-united-nations-number-code"/>
      </owl:Restriction>
    </rdfs:subClassOf>
    <rdfs:label xml:lang="en">UN Dangerous Goods # 1067</rdfs:label>
    <rdfs:comment xml:lang="en">Dinitrogen tetroxide (nitrogen dioxide). Includes the agent(s): nitrogen dioxide.</rdfs:comment>
    <rdfs:subClassOf>
      <owl:Restriction>
        <owl:hasValue xml:lang="en">1067</owl:hasValue>
        <owl:onProperty rdf:resource="jc3iedmBase.owl#consumable-materiel-type-united-nations-number-code"/>
      </owl:Restriction>
    </rdfs:subClassOf>
  </owl:Class>
  <owl:Class rdf:ID="UN_Dangerous_Goods_NUM_1978">
    <rdfs:subClassOf>
      <owl:Restriction>
        <owl:hasValue xml:lang="en">1978</owl:hasValue>
        <owl:onProperty rdf:resource="jc3iedmBase.owl#consumable-materiel-type-united-nations-number-code"/>
      </owl:Restriction>
    </rdfs:subClassOf>
    <rdfs:label xml:lang="en">UN Dangerous Goods # 1978</rdfs:label>
    <rdfs:comment xml:lang="en">Propane. Includes the agent(s): propane.</rdfs:comment>
    <rdfs:subClassOf>
      <owl:Restriction>
        <owl:hasValue xml:lang="en">1978</owl:hasValue>
        <owl:onProperty rdf:resource="jc3iedmBase.owl#consumable-materiel-type-united-nations-number-code"/>
      </owl:Restriction>
    </rdfs:subClassOf>
  </owl:Class>
  <owl:Class rdf:ID="Flume">
    <rdfs:subClassOf rdf:resource="jc3iedmSubOnt.owl#GEOGRAPHIC-FEATURE-TYPE-Inland_water"/>
    <rdfs:subClassOf rdf:resource="jc3iedmSubOnt.owl#GEOGRAPHIC-FEATURE-Liquid_surface"/>
    <rdfs:subClassOf>
      <owl:Restriction>
        <owl:hasValue xml:lang="en">FLUME</owl:hasValue>
        <owl:onProperty rdf:resource="jc3iedmBase.owl#geographic-feature-type-subcategory-code"/>
      </owl:Restriction>
    </rdfs:subClassOf>
    <rdfs:label xml:lang="en">Flume</rdfs:label>
    <rdfs:comment xml:lang="en">An open, inclined channel which carries water for use in such operations as mining or logging.</rdfs:comment>
    <rdfs:subClassOf>
      <owl:Restriction>
        <owl:hasValue xml:lang="en">FLUME</owl:hasValue>
        <owl:onProperty rdf:resource="jc3iedmBase.owl#geographic-feature-type-subcategory-code"/>
      </owl:Restriction>
    </rdfs:subClassOf>
  </owl:Class>
  <owl:Class rdf:ID="Cocaine">
    <rdfs:subClassOf rdf:resource="jc3iedmSubOnt.owl#CONSUMABLE-MATERIEL-TYPE-Drug"/>
    <rdfs:subClassOf>
      <owl:Restriction>
        <owl:hasValue xml:lang="en">COCANE</owl:hasValue>
        <owl:onProperty rdf:resource="jc3iedmBase.owl#consumable-materiel-type-subcategory-code"/>
      </owl:Restriction>
    </rdfs:subClassOf>
    <rdfs:label xml:lang="en">Cocaine</rdfs:label>
    <rdfs:comment xml:lang="en">A drug derived from coca or prepared synthetically, used as a local anaesthetic and as a stimulant.</rdfs:comment>
  </owl:Class>
  <owl:Class rdf:ID="Land_subject_to_inundation">
    <rdfs:subClassOf rdf:resource="jc3iedmSubOnt.owl#GEOGRAPHIC-FEATURE-TYPE-Inland_water"/>
    <rdfs:subClassOf rdf:resource="jc3iedmSubOnt.owl#GEOGRAPHIC-FEATURE-Solid_surface"/>
    <rdfs:subClassOf rdf:resource="jc3iedmSubOnt.owl#GEOGRAPHIC-FEATURE-Liquid_surface"/>
    <rdfs:subClassOf>
      <owl:Restriction>
        <owl:hasValue xml:lang="en">LNDSBJ</owl:hasValue>
        <owl:onProperty rdf:resource="jc3iedmBase.owl#geographic-feature-type-subcategory-code"/>
      </owl:Restriction>
    </rdfs:subClassOf>
    <rdfs:label xml:lang="en">Land subject to inundation</rdfs:label>
    <rdfs:comment xml:lang="en">An area periodically covered by flood water, excluding tidal waters.</rdfs:comment>
    <rdfs:subClassOf>
      <owl:Restriction>
        <owl:hasValue xml:lang="en">LNDSBJ</owl:hasValue>
        <owl:onProperty rdf:resource="jc3iedmBase.owl#geographic-feature-type-subcategory-code"/>
      </owl:Restriction>
    </rdfs:subClassOf>
    <rdfs:subClassOf>
      <owl:Restriction>
        <owl:hasValue xml:lang="en">LNDSBJ</owl:hasValue>
        <owl:onProperty rdf:resource="jc3iedmBase.owl#geographic-feature-type-subcategory-code"/>
      </owl:Restriction>
    </rdfs:subClassOf>
  </owl:Class>
  <owl:Class rdf:ID="Cyclo-Sarin">
    <rdfs:subClassOf rdf:resource="jc3iedmSubOnt.owl#CHEMICAL-MATERIEL-TYPE-G-agent"/>
    <rdfs:subClassOf rdf:resource="jc3iedmSubOnt.owl#CHEMICAL-MATERIEL-TYPE-Nerve_agent"/>
    <rdfs:subClassOf>
      <owl:Restriction>
        <owl:hasValue xml:lang="en">CYCLSR</owl:hasValue>
        <owl:onProperty rdf:resource="jc3iedmBase.owl#chemical-materiel-type-subcategory-code"/>
      </owl:Restriction>
    </rdfs:subClassOf>
    <rdfs:label xml:lang="en">Cyclo-Sarin</rdfs:label>
    <rdfs:comment xml:lang="en">An organophosphorus nerve gas evolved from Sarin.</rdfs:comment>
    <rdfs:subClassOf>
      <owl:Restriction>
        <owl:hasValue xml:lang="en">CYCLSR</owl:hasValue>
        <owl:onProperty rdf:resource="jc3iedmBase.owl#chemical-materiel-type-subcategory-code"/>
      </owl:Restriction>
    </rdfs:subClassOf>
  </owl:Class>
  <owl:Class rdf:ID="Petrol">
    <rdfs:subClassOf rdf:resource="jc3iedmSubOnt.owl#CONSUMABLE-MATERIEL-TYPE-POL"/>
    <rdfs:subClassOf>
      <owl:Restriction>
        <owl:hasValue xml:lang="en">PETROL</owl:hasValue>
        <owl:onProperty rdf:resource="jc3iedmBase.owl#consumable-materiel-type-subcategory-code"/>
      </owl:Restriction>
    </rdfs:subClassOf>
    <rdfs:label xml:lang="en">Petrol</rdfs:label>
    <rdfs:comment xml:lang="en">A refined petroleum product intended to be used as fuel in gasoline engines.</rdfs:comment>
  </owl:Class>
  <owl:Class rdf:ID="Air">
    <rdfs:label xml:lang="en">Air</rdfs:label>
    <rdfs:comment xml:lang="en">Represents the general mode of transportation used in movement by air.</rdfs:comment>
  </owl:Class>
  <owl:Class rdf:ID="Liquefied_petroleum_gas">
    <rdfs:subClassOf rdf:resource="jc3iedmSubOnt.owl#CONSUMABLE-MATERIEL-TYPE-Fuel"/>
    <rdfs:subClassOf>
      <owl:Restriction>
        <owl:hasValue xml:lang="en">LPG</owl:hasValue>
        <owl:onProperty rdf:resource="jc3iedmBase.owl#consumable-materiel-type-subcategory-code"/>
      </owl:Restriction>
    </rdfs:subClassOf>
    <rdfs:label xml:lang="en">Liquefied petroleum gas</rdfs:label>
    <rdfs:comment xml:lang="en">Liquefied petroleum gas.</rdfs:comment>
  </owl:Class>
  <owl:Class rdf:ID="UN_Dangerous_Goods_NUM_2916">
    <rdfs:subClassOf>
      <owl:Restriction>
        <owl:hasValue xml:lang="en">2916</owl:hasValue>
        <owl:onProperty rdf:resource="jc3iedmBase.owl#consumable-materiel-type-united-nations-number-code"/>
      </owl:Restriction>
    </rdfs:subClassOf>
    <rdfs:label xml:lang="en">UN Dangerous Goods # 2916</rdfs:label>
    <rdfs:comment xml:lang="en">Radioactive material, type B(U) package, non fissile or fissile-excepted.</rdfs:comment>
  </owl:Class>
  <owl:Class rdf:ID="Rapids">
    <rdfs:subClassOf rdf:resource="jc3iedmSubOnt.owl#GEOGRAPHIC-FEATURE-TYPE-Inland_water"/>
    <rdfs:subClassOf rdf:resource="jc3iedmSubOnt.owl#GEOGRAPHIC-FEATURE-Liquid_surface"/>
    <rdfs:subClassOf>
      <owl:Restriction>
        <owl:hasValue xml:lang="en">RAPIDS</owl:hasValue>
        <owl:onProperty rdf:resource="jc3iedmBase.owl#geographic-feature-type-subcategory-code"/>
      </owl:Restriction>
    </rdfs:subClassOf>
    <rdfs:label xml:lang="en">Rapids</rdfs:label>
    <rdfs:comment xml:lang="en">A place in a stream or river where the current is swift and the surface is usually broken by boulders and rocks.</rdfs:comment>
    <rdfs:subClassOf>
      <owl:Restriction>
        <owl:hasValue xml:lang="en">RAPIDS</owl:hasValue>
        <owl:onProperty rdf:resource="jc3iedmBase.owl#geographic-feature-type-subcategory-code"/>
      </owl:Restriction>
    </rdfs:subClassOf>
  </owl:Class>
  <owl:Class rdf:ID="Passive">
    <rdfs:subClassOf>
      <owl:Restriction>
        <owl:hasValue xml:lang="en">PASIVE</owl:hasValue>
        <owl:onProperty rdf:resource="jc3iedmBase.owl#ammunition-type-mine-maritime-firing-code"/>
      </owl:Restriction>
    </rdfs:subClassOf>
    <rdfs:subClassOf rdf:resource="jc3iedmSubOnt.owl#AMMUNITION-TYPE-Mine,_deep_moored"/>
    <rdfs:subClassOf rdf:resource="jc3iedmSubOnt.owl#AMMUNITION-TYPE-Mine,_not_otherwise_specified"/>
    <rdfs:subClassOf rdf:resource="jc3iedmSubOnt.owl#AMMUNITION-TYPE-Sea_mine"/>
    <rdfs:subClassOf rdf:resource="jc3iedmSubOnt.owl#AMMUNITION-TYPE-Mine,_moored"/>
    <rdfs:subClassOf rdf:resource="jc3iedmSubOnt.owl#AMMUNITION-TYPE-Mine,_shallow_moored"/>
    <rdfs:subClassOf rdf:resource="jc3iedmSubOnt.owl#AMMUNITION-TYPE-Moving_mine,_sea"/>
    <rdfs:label xml:lang="en">Passive</rdfs:label>
    <rdfs:subClassOf rdf:resource="jc3iedmSubOnt.owl#AMMUNITION-TYPE-Mine,_seabed_-_explosive_charge_less_than_500kg"/>
    <rdfs:subClassOf rdf:resource="jc3iedmSubOnt.owl#AMMUNITION-TYPE-Seabed_mine"/>
    <rdfs:subClassOf rdf:resource="jc3iedmSubOnt.owl#AMMUNITION-TYPE-Mine,_not_known"/>
    <rdfs:subClassOf rdf:resource="jc3iedmSubOnt.owl#AMMUNITION-TYPE-Mine,_seabed_-_explosive_charge_500kg_or_greater"/>
    <rdfs:subClassOf rdf:resource="jc3iedmSubOnt.owl#AMMUNITION-TYPE-Mine,_maritime,_moving"/>
    <rdfs:subClassOf>
      <owl:Restriction>
        <owl:hasValue xml:lang="en">PASIVE</owl:hasValue>
        <owl:onProperty rdf:resource="jc3iedmBase.owl#ammunition-type-mine-maritime-firing-code"/>
      </owl:Restriction>
    </rdfs:subClassOf>
    <rdfs:comment xml:lang="en">A (maritime) mine firing mechanism that does not emit a signal to detect the presence of a target.</rdfs:comment>
  </owl:Class>
  <owl:Class rdf:ID="Glider">
    <rdfs:subClassOf rdf:resource="jc3iedmSubOnt.owl#AIRCRAFT-TYPE-Fixed_wing"/>
    <rdfs:subClassOf>
      <owl:Restriction>
        <owl:hasValue xml:lang="en">GLIDER</owl:hasValue>
        <owl:onProperty rdf:resource="jc3iedmBase.owl#aircraft-type-airframe-design-code"/>
      </owl:Restriction>
    </rdfs:subClassOf>
    <rdfs:label xml:lang="en">Glider</rdfs:label>
    <rdfs:comment xml:lang="en">A fixed wing aircraft that flies without an engine.</rdfs:comment>
  </owl:Class>
  <owl:Class rdf:ID="Ecstasy_-_MDEA">
    <rdfs:subClassOf rdf:resource="jc3iedmSubOnt.owl#CONSUMABLE-MATERIEL-TYPE-Drug"/>
    <rdfs:subClassOf>
      <owl:Restriction>
        <owl:hasValue xml:lang="en">ECSMDE</owl:hasValue>
        <owl:onProperty rdf:resource="jc3iedmBase.owl#consumable-materiel-type-subcategory-code"/>
      </owl:Restriction>
    </rdfs:subClassOf>
    <rdfs:label xml:lang="en">Ecstasy - MDEA</rdfs:label>
    <rdfs:comment xml:lang="en">Methylenedioxy-ethylamphetamine, an amphetamine-based drug that causes euphoric and hallucinatory effects, originally produced as an appetite suppressant.</rdfs:comment>
  </owl:Class>
  <owl:Class rdf:ID="UN_Dangerous_Goods_NUM_2668">
    <rdfs:subClassOf>
      <owl:Restriction>
        <owl:hasValue xml:lang="en">2668</owl:hasValue>
        <owl:onProperty rdf:resource="jc3iedmBase.owl#consumable-materiel-type-united-nations-number-code"/>
      </owl:Restriction>
    </rdfs:subClassOf>
    <rdfs:label xml:lang="en">UN Dangerous Goods # 2668</rdfs:label>
    <rdfs:comment xml:lang="en">Chloroacetonitrile. Includes the agent(s): chloroacetonitrile.</rdfs:comment>
    <rdfs:subClassOf>
      <owl:Restriction>
        <owl:hasValue xml:lang="en">2668</owl:hasValue>
        <owl:onProperty rdf:resource="jc3iedmBase.owl#consumable-materiel-type-united-nations-number-code"/>
      </owl:Restriction>
    </rdfs:subClassOf>
  </owl:Class>
  <owl:Class rdf:about="#Sonar,_reflector_Diablo">
    <rdfs:subClassOf rdf:resource="jc3iedmSubOnt.owl#MARITIME-EQUIPMENT-TYPE-Sonar,_maritime"/>
    <rdfs:subClassOf>
      <owl:Restriction>
        <owl:hasValue xml:lang="en">SONRRD</owl:hasValue>
        <owl:onProperty rdf:resource="jc3iedmBase.owl#maritime-equipment-type-subcategory-code"/>
      </owl:Restriction>
    </rdfs:subClassOf>
    <rdfs:label xml:lang="en">Sonar, reflector Diablo</rdfs:label>
    <rdfs:comment xml:lang="en">A device to make a training mine appear larger or for use during diving conning run ICOS 42+ sides etc.</rdfs:comment>
  </owl:Class>
  <owl:Class rdf:ID="Newspaper">
    <rdfs:subClassOf rdf:resource="jc3iedmSubOnt.owl#CONSUMABLE-MATERIEL-TYPE-General_supplies"/>
    <rdfs:subClassOf>
      <owl:Restriction>
        <owl:hasValue xml:lang="en">NWSPPR</owl:hasValue>
        <owl:onProperty rdf:resource="jc3iedmBase.owl#consumable-materiel-type-subcategory-code"/>
      </owl:Restriction>
    </rdfs:subClassOf>
    <rdfs:label xml:lang="en">Newspaper</rdfs:label>
    <rdfs:comment xml:lang="en">A printed publication containing the news, commonly with the addition of advertisements and other matters of interest.</rdfs:comment>
  </owl:Class>
  <owl:Class rdf:ID="UN_Dangerous_Goods_NUM_2783">
    <rdfs:subClassOf>
      <owl:Restriction>
        <owl:hasValue xml:lang="en">2783</owl:hasValue>
        <owl:onProperty rdf:resource="jc3iedmBase.owl#consumable-materiel-type-united-nations-number-code"/>
      </owl:Restriction>
    </rdfs:subClassOf>
    <rdfs:label xml:lang="en">UN Dangerous Goods # 2783</rdfs:label>
    <rdfs:comment xml:lang="en">Organophosphorus pesticide, solid, toxic. Includes the agent(s): parathion, malathion.</rdfs:comment>
    <rdfs:subClassOf>
      <owl:Restriction>
        <owl:hasValue xml:lang="en">2783</owl:hasValue>
        <owl:onProperty rdf:resource="jc3iedmBase.owl#consumable-materiel-type-united-nations-number-code"/>
      </owl:Restriction>
    </rdfs:subClassOf>
  </owl:Class>
  <owl:Class rdf:ID="UN_Dangerous_Goods_NUM_1911">
    <rdfs:subClassOf>
      <owl:Restriction>
        <owl:hasValue xml:lang="en">1911</owl:hasValue>
        <owl:onProperty rdf:resource="jc3iedmBase.owl#consumable-materiel-type-united-nations-number-code"/>
      </owl:Restriction>
    </rdfs:subClassOf>
    <rdfs:label xml:lang="en">UN Dangerous Goods # 1911</rdfs:label>
    <rdfs:comment xml:lang="en">Diborane. Includes the agent(s): diborane.</rdfs:comment>
    <rdfs:subClassOf>
      <owl:Restriction>
        <owl:hasValue xml:lang="en">1911</owl:hasValue>
        <owl:onProperty rdf:resource="jc3iedmBase.owl#consumable-materiel-type-united-nations-number-code"/>
      </owl:Restriction>
    </rdfs:subClassOf>
  </owl:Class>
  <owl:Class rdf:ID="UN_Dangerous_Goods_NUM_2196">
    <rdfs:subClassOf>
      <owl:Restriction>
        <owl:hasValue xml:lang="en">2196</owl:hasValue>
        <owl:onProperty rdf:resource="jc3iedmBase.owl#consumable-materiel-type-united-nations-number-code"/>
      </owl:Restriction>
    </rdfs:subClassOf>
    <rdfs:label xml:lang="en">UN Dangerous Goods # 2196</rdfs:label>
    <rdfs:comment xml:lang="en">Tungsten hexafluoride. Includes the agent(s): tungsten hexafluoride.</rdfs:comment>
    <rdfs:subClassOf>
      <owl:Restriction>
        <owl:hasValue xml:lang="en">2196</owl:hasValue>
        <owl:onProperty rdf:resource="jc3iedmBase.owl#consumable-materiel-type-united-nations-number-code"/>
      </owl:Restriction>
    </rdfs:subClassOf>
  </owl:Class>
  <owl:Class rdf:ID="Moveable_and_prefabricated">
    <rdfs:subClassOf rdf:resource="jc3iedmSubOnt.owl#MILITARY-OBSTACLE-TYPE-Anti-tank_obstacle"/>
    <rdfs:subClassOf rdf:resource="jc3iedmSubOnt.owl#MILITARY-OBSTACLE-TYPE-Tetrahedron"/>
    <rdfs:subClassOf rdf:resource="jc3iedmSubOnt.owl#MILITARY-OBSTACLE-TYPE-Dragon_teeth"/>
    <rdfs:subClassOf>
      <owl:Restriction>
        <owl:hasValue xml:lang="en">MOVAPR</owl:hasValue>
        <owl:onProperty rdf:resource="jc3iedmBase.owl#military-obstacle-type-subcategory-code"/>
      </owl:Restriction>
    </rdfs:subClassOf>
    <rdfs:label xml:lang="en">Moveable and prefabricated</rdfs:label>
    <rdfs:comment xml:lang="en">The obstacle is prefabricated and can be moved.</rdfs:comment>
    <rdfs:subClassOf>
      <owl:Restriction>
        <owl:hasValue xml:lang="en">MOVAPR</owl:hasValue>
        <owl:onProperty rdf:resource="jc3iedmBase.owl#military-obstacle-type-subcategory-code"/>
      </owl:Restriction>
    </rdfs:subClassOf>
    <rdfs:subClassOf>
      <owl:Restriction>
        <owl:hasValue xml:lang="en">MOVAPR</owl:hasValue>
        <owl:onProperty rdf:resource="jc3iedmBase.owl#military-obstacle-type-subcategory-code"/>
      </owl:Restriction>
    </rdfs:subClassOf>
  </owl:Class>
  <owl:Class rdf:ID="UN_Dangerous_Goods_NUM_1143">
    <rdfs:subClassOf>
      <owl:Restriction>
        <owl:hasValue xml:lang="en">1143</owl:hasValue>
        <owl:onProperty rdf:resource="jc3iedmBase.owl#consumable-materiel-type-united-nations-number-code"/>
      </owl:Restriction>
    </rdfs:subClassOf>
    <rdfs:label xml:lang="en">UN Dangerous Goods # 1143</rdfs:label>
    <rdfs:comment xml:lang="en">Crotonaldehyde, stabilized. Includes the agent(s): crotonaldehyde.</rdfs:comment>
    <rdfs:subClassOf>
      <owl:Restriction>
        <owl:hasValue xml:lang="en">1143</owl:hasValue>
        <owl:onProperty rdf:resource="jc3iedmBase.owl#consumable-materiel-type-united-nations-number-code"/>
      </owl:Restriction>
    </rdfs:subClassOf>
  </owl:Class>
  <owl:Class rdf:ID="Air-defence_gun">
    <rdfs:subClassOf rdf:resource="jc3iedmSubOnt.owl#WEAPON-TYPE-Air-defence"/>
    <rdfs:subClassOf>
      <owl:Restriction>
        <owl:hasValue xml:lang="en">ADGUN</owl:hasValue>
        <owl:onProperty rdf:resource="jc3iedmBase.owl#weapon-type-subcategory-code"/>
      </owl:Restriction>
    </rdfs:subClassOf>
    <rdfs:label xml:lang="en">Air-defence gun</rdfs:label>
    <rdfs:comment xml:lang="en">A gun used primarily in the role of air defence.</rdfs:comment>
  </owl:Class>
  <owl:Class rdf:ID="UN_Dangerous_Goods_NUM_1809">
    <rdfs:subClassOf>
      <owl:Restriction>
        <owl:hasValue xml:lang="en">1809</owl:hasValue>
        <owl:onProperty rdf:resource="jc3iedmBase.owl#consumable-materiel-type-united-nations-number-code"/>
      </owl:Restriction>
    </rdfs:subClassOf>
    <rdfs:label xml:lang="en">UN Dangerous Goods # 1809</rdfs:label>
    <rdfs:comment xml:lang="en">Phosphorus trichloride. Includes the agent(s): phosphorus trichloride.</rdfs:comment>
    <rdfs:subClassOf>
      <owl:Restriction>
        <owl:hasValue xml:lang="en">1809</owl:hasValue>
        <owl:onProperty rdf:resource="jc3iedmBase.owl#consumable-materiel-type-united-nations-number-code"/>
      </owl:Restriction>
    </rdfs:subClassOf>
  </owl:Class>
  <owl:Class rdf:ID="UN_Dangerous_Goods_NUM_1008">
    <rdfs:subClassOf>
      <owl:Restriction>
        <owl:hasValue xml:lang="en">1008</owl:hasValue>
        <owl:onProperty rdf:resource="jc3iedmBase.owl#consumable-materiel-type-united-nations-number-code"/>
      </owl:Restriction>
    </rdfs:subClassOf>
    <rdfs:label xml:lang="en">UN Dangerous Goods # 1008</rdfs:label>
    <rdfs:comment xml:lang="en">Boron trifluoride. Includes the agent(s): boron trifluoride.</rdfs:comment>
    <rdfs:subClassOf>
      <owl:Restriction>
        <owl:hasValue xml:lang="en">1008</owl:hasValue>
        <owl:onProperty rdf:resource="jc3iedmBase.owl#consumable-materiel-type-united-nations-number-code"/>
      </owl:Restriction>
    </rdfs:subClassOf>
  </owl:Class>
  <owl:Class rdf:ID="Megaphone">
    <rdfs:subClassOf rdf:resource="jc3iedmSubOnt.owl#ELECTRONIC-EQUIPMENT-TYPE-Public_address_system"/>
    <rdfs:subClassOf>
      <owl:Restriction>
        <owl:hasValue xml:lang="en">MEGPHN</owl:hasValue>
        <owl:onProperty rdf:resource="jc3iedmBase.owl#electronic-equipment-type-subcategory-code"/>
      </owl:Restriction>
    </rdfs:subClassOf>
    <rdfs:label xml:lang="en">Megaphone</rdfs:label>
    <rdfs:comment xml:lang="en">An electronic instrument for carrying sound a long distance.</rdfs:comment>
  </owl:Class>
  <owl:Class rdf:ID="Video_broadcast_device">
    <rdfs:subClassOf rdf:resource="jc3iedmSubOnt.owl#ELECTRONIC-EQUIPMENT-TYPE-Public_address_system"/>
    <rdfs:subClassOf rdf:resource="jc3iedmSubOnt.owl#ELECTRONIC-EQUIPMENT-TYPE-Communication"/>
    <rdfs:subClassOf>
      <owl:Restriction>
        <owl:hasValue xml:lang="en">VIDBRD</owl:hasValue>
        <owl:onProperty rdf:resource="jc3iedmBase.owl#electronic-equipment-type-subcategory-code"/>
      </owl:Restriction>
    </rdfs:subClassOf>
    <rdfs:label xml:lang="en">Video broadcast device</rdfs:label>
    <rdfs:comment xml:lang="en">A device that stores images to be displayed on a television screen or other cathode-ray tube device.</rdfs:comment>
    <rdfs:subClassOf>
      <owl:Restriction>
        <owl:hasValue xml:lang="en">VIDBRD</owl:hasValue>
        <owl:onProperty rdf:resource="jc3iedmBase.owl#electronic-equipment-type-subcategory-code"/>
      </owl:Restriction>
    </rdfs:subClassOf>
  </owl:Class>
  <owl:Class rdf:ID="UN_Dangerous_Goods_NUM_2917">
    <rdfs:subClassOf>
      <owl:Restriction>
        <owl:hasValue xml:lang="en">2917</owl:hasValue>
        <owl:onProperty rdf:resource="jc3iedmBase.owl#consumable-materiel-type-united-nations-number-code"/>
      </owl:Restriction>
    </rdfs:subClassOf>
    <rdfs:label xml:lang="en">UN Dangerous Goods # 2917</rdfs:label>
    <rdfs:comment xml:lang="en">Radioactive material, type B(M) package, non fissile or fissile-excepted.</rdfs:comment>
  </owl:Class>
  <owl:Class rdf:ID="GHB">
    <rdfs:subClassOf rdf:resource="jc3iedmSubOnt.owl#CONSUMABLE-MATERIEL-TYPE-Drug"/>
    <rdfs:subClassOf>
      <owl:Restriction>
        <owl:hasValue xml:lang="en">GHB</owl:hasValue>
        <owl:onProperty rdf:resource="jc3iedmBase.owl#consumable-materiel-type-subcategory-code"/>
      </owl:Restriction>
    </rdfs:subClassOf>
    <rdfs:label xml:lang="en">GHB</rdfs:label>
    <rdfs:comment xml:lang="en">Gamma hydroxy butyrate, a designer drug with anaesthetic properties, claimed also to be an aphrodisiac.</rdfs:comment>
  </owl:Class>
  <owl:Class rdf:ID="Balloon">
    <rdfs:subClassOf rdf:resource="jc3iedmSubOnt.owl#AIRCRAFT-TYPE-Lighter_than_air"/>
    <rdfs:subClassOf>
      <owl:Restriction>
        <owl:hasValue xml:lang="en">BALOON</owl:hasValue>
        <owl:onProperty rdf:resource="jc3iedmBase.owl#aircraft-type-airframe-design-code"/>
      </owl:Restriction>
    </rdfs:subClassOf>
    <rdfs:label xml:lang="en">Balloon</rdfs:label>
    <rdfs:comment xml:lang="en">An unpowered lighter than air aircraft.</rdfs:comment>
  </owl:Class>
  <owl:Class rdf:about="#Radar,_airborne">
    <rdfs:subClassOf rdf:resource="jc3iedmSubOnt.owl#ELECTRONIC-EQUIPMENT-TYPE-Radar"/>
    <rdfs:subClassOf rdf:resource="jc3iedmSubOnt.owl#ELECTRONIC-EQUIPMENT-TYPE-Navigational_aid"/>
    <rdfs:subClassOf>
      <owl:Restriction>
        <owl:hasValue xml:lang="en">RDRARB</owl:hasValue>
        <owl:onProperty rdf:resource="jc3iedmBase.owl#electronic-equipment-type-subcategory-code"/>
      </owl:Restriction>
    </rdfs:subClassOf>
    <rdfs:label xml:lang="en">Radar, airborne</rdfs:label>
    <rdfs:comment xml:lang="en">A radar carried through the air by an aircraft.</rdfs:comment>
    <rdfs:subClassOf>
      <owl:Restriction>
        <owl:hasValue xml:lang="en">RDRARB</owl:hasValue>
        <owl:onProperty rdf:resource="jc3iedmBase.owl#electronic-equipment-type-subcategory-code"/>
      </owl:Restriction>
    </rdfs:subClassOf>
  </owl:Class>
  <owl:Class rdf:about="#Crew_served_weapon,_unknown_type">
    <rdfs:subClassOf>
      <owl:Restriction>
        <owl:hasValue xml:lang="en">CRWPUN</owl:hasValue>
        <owl:onProperty rdf:resource="jc3iedmBase.owl#weapon-type-subcategory-code"/>
      </owl:Restriction>
    </rdfs:subClassOf>
    <rdfs:label xml:lang="en">Crew served weapon, unknown type</rdfs:label>
    <rdfs:comment xml:lang="en">No definition provided in ADatP-3 Baseline 13.1 FFIRN/FUD 1650/6.</rdfs:comment>
  </owl:Class>
  <owl:Class rdf:ID="Medicine">
    <rdfs:subClassOf rdf:resource="jc3iedmSubOnt.owl#CONSUMABLE-MATERIEL-TYPE-Medical_supply"/>
    <rdfs:subClassOf>
      <owl:Restriction>
        <owl:hasValue xml:lang="en">MEDICN</owl:hasValue>
        <owl:onProperty rdf:resource="jc3iedmBase.owl#consumable-materiel-type-subcategory-code"/>
      </owl:Restriction>
    </rdfs:subClassOf>
    <rdfs:label xml:lang="en">Medicine</rdfs:label>
    <rdfs:comment xml:lang="en">Any substance or preparation used in the treatment of disease.</rdfs:comment>
  </owl:Class>
  <owl:Class rdf:ID="UN_Dangerous_Goods_NUM_1079">
    <rdfs:subClassOf>
      <owl:Restriction>
        <owl:hasValue xml:lang="en">1079</owl:hasValue>
        <owl:onProperty rdf:resource="jc3iedmBase.owl#consumable-materiel-type-united-nations-number-code"/>
      </owl:Restriction>
    </rdfs:subClassOf>
    <rdfs:label xml:lang="en">UN Dangerous Goods # 1079</rdfs:label>
    <rdfs:comment xml:lang="en">Sulphur dioxide. Includes the agent(s) referred to as: sulphur dioxide.</rdfs:comment>
    <rdfs:subClassOf>
      <owl:Restriction>
        <owl:hasValue xml:lang="en">1079</owl:hasValue>
        <owl:onProperty rdf:resource="jc3iedmBase.owl#consumable-materiel-type-united-nations-number-code"/>
      </owl:Restriction>
    </rdfs:subClassOf>
  </owl:Class>
  <owl:Class rdf:ID="High_frequency_direction_finder">
    <rdfs:subClassOf rdf:resource="jc3iedmSubOnt.owl#ELECTRONIC-EQUIPMENT-TYPE-Electronic_warfare"/>
    <rdfs:subClassOf>
      <owl:Restriction>
        <owl:hasValue xml:lang="en">HFRDFD</owl:hasValue>
        <owl:onProperty rdf:resource="jc3iedmBase.owl#electronic-equipment-type-subcategory-code"/>
      </owl:Restriction>
    </rdfs:subClassOf>
    <rdfs:label xml:lang="en">High frequency direction finder</rdfs:label>
    <rdfs:comment xml:lang="en">No definition provided in ADatP-3 Baseline 13.1 FFIRN/FUD 1434/1.</rdfs:comment>
  </owl:Class>
  <owl:Class rdf:ID="Howitzer">
    <rdfs:subClassOf rdf:resource="jc3iedmSubOnt.owl#WEAPON-TYPE-Field_artillery"/>
    <rdfs:subClassOf rdf:resource="jc3iedmSubOnt.owl#WEAPON-TYPE-Cannon"/>
    <rdfs:subClassOf>
      <owl:Restriction>
        <owl:hasValue xml:lang="en">HOWIT</owl:hasValue>
        <owl:onProperty rdf:resource="jc3iedmBase.owl#weapon-type-subcategory-code"/>
      </owl:Restriction>
    </rdfs:subClassOf>
    <rdfs:label xml:lang="en">Howitzer</rdfs:label>
    <rdfs:comment xml:lang="en">A cannon that combines certain characteristics of guns and mortars. Normally a cannon with a tube length of 20 to 30 calibres; however, the tube length can exceed 30 calibres and still be considered a howitzer when the high angle firing zoning solution permits range overlap between charges.</rdfs:comment>
    <rdfs:subClassOf>
      <owl:Restriction>
        <owl:hasValue xml:lang="en">HOWIT</owl:hasValue>
        <owl:onProperty rdf:resource="jc3iedmBase.owl#weapon-type-subcategory-code"/>
      </owl:Restriction>
    </rdfs:subClassOf>
  </owl:Class>
  <owl:Class rdf:about="#Radar,_joint_surveillance_target_attack">
    <rdfs:subClassOf rdf:resource="jc3iedmSubOnt.owl#ELECTRONIC-EQUIPMENT-TYPE-Radar"/>
    <rdfs:subClassOf>
      <owl:Restriction>
        <owl:hasValue xml:lang="en">RDRJST</owl:hasValue>
        <owl:onProperty rdf:resource="jc3iedmBase.owl#electronic-equipment-type-subcategory-code"/>
      </owl:Restriction>
    </rdfs:subClassOf>
    <rdfs:label xml:lang="en">Radar, joint surveillance target attack</rdfs:label>
    <rdfs:comment xml:lang="en">A long-range, air-to-ground surveillance system designed to locate, classify and track ground targets in all weather conditions.</rdfs:comment>
  </owl:Class>
  <owl:Class rdf:ID="DOB">
    <rdfs:subClassOf rdf:resource="jc3iedmSubOnt.owl#CONSUMABLE-MATERIEL-TYPE-Drug"/>
    <rdfs:subClassOf>
      <owl:Restriction>
        <owl:hasValue xml:lang="en">DOB</owl:hasValue>
        <owl:onProperty rdf:resource="jc3iedmBase.owl#consumable-materiel-type-subcategory-code"/>
      </owl:Restriction>
    </rdfs:subClassOf>
    <rdfs:label xml:lang="en">DOB</rdfs:label>
    <rdfs:comment xml:lang="en">A synthetic phenethylamine substance marked by visual hallucinations.</rdfs:comment>
  </owl:Class>
  <owl:Class rdf:ID="Cyanogen_chloride">
    <rdfs:subClassOf rdf:resource="jc3iedmSubOnt.owl#CHEMICAL-MATERIEL-TYPE-Blood_agent"/>
    <rdfs:subClassOf>
      <owl:Restriction>
        <owl:hasValue xml:lang="en">CYNGNC</owl:hasValue>
        <owl:onProperty rdf:resource="jc3iedmBase.owl#chemical-materiel-type-subcategory-code"/>
      </owl:Restriction>
    </rdfs:subClassOf>
    <rdfs:label xml:lang="en">Cyanogen chloride</rdfs:label>
    <rdfs:comment xml:lang="en">A colourless flammable highly poisonous gas made by oxidising hydrogen cyanide. (Blood agent)</rdfs:comment>
  </owl:Class>
  <owl:Class rdf:ID="Amateur_radio_device">
    <rdfs:subClassOf rdf:resource="jc3iedmSubOnt.owl#ELECTRONIC-EQUIPMENT-TYPE-Communication"/>
    <rdfs:subClassOf>
      <owl:Restriction>
        <owl:hasValue xml:lang="en">AMTRAD</owl:hasValue>
        <owl:onProperty rdf:resource="jc3iedmBase.owl#electronic-equipment-type-subcategory-code"/>
      </owl:Restriction>
    </rdfs:subClassOf>
    <rdfs:label xml:lang="en">Amateur radio device</rdfs:label>
    <rdfs:comment xml:lang="en">The transmission and reception of radio-frequency electromagnetic waves as a means of communication usually as a hobby.</rdfs:comment>
  </owl:Class>
  <owl:Class rdf:ID="UN_Dangerous_Goods_NUM_1048">
    <rdfs:subClassOf>
      <owl:Restriction>
        <owl:hasValue xml:lang="en">1048</owl:hasValue>
        <owl:onProperty rdf:resource="jc3iedmBase.owl#consumable-materiel-type-united-nations-number-code"/>
      </owl:Restriction>
    </rdfs:subClassOf>
    <rdfs:label xml:lang="en">UN Dangerous Goods # 1048</rdfs:label>
    <rdfs:comment xml:lang="en">Hydrogen bromide, anhydrous. Includes the agent(s): hydrogen bromide.</rdfs:comment>
    <rdfs:subClassOf>
      <owl:Restriction>
        <owl:hasValue xml:lang="en">1048</owl:hasValue>
        <owl:onProperty rdf:resource="jc3iedmBase.owl#consumable-materiel-type-united-nations-number-code"/>
      </owl:Restriction>
    </rdfs:subClassOf>
  </owl:Class>
  <owl:Class rdf:ID="Forward_looking_infrared">
    <rdfs:subClassOf rdf:resource="jc3iedmSubOnt.owl#ELECTRONIC-EQUIPMENT-TYPE-Sensor"/>
    <rdfs:subClassOf>
      <owl:Restriction>
        <owl:hasValue xml:lang="en">FLIR</owl:hasValue>
        <owl:onProperty rdf:resource="jc3iedmBase.owl#electronic-equipment-type-subcategory-code"/>
      </owl:Restriction>
    </rdfs:subClassOf>
    <rdfs:label xml:lang="en">Forward looking infrared</rdfs:label>
    <rdfs:comment xml:lang="en">An airborne, electro-optical thermal imaging device that detects far-infrared energy, converts the energy into an electronic signal, and provides a visible image for day or night viewing. Also called FLIR.</rdfs:comment>
  </owl:Class>
  <owl:Class rdf:ID="Magnetic_anomaly_detector">
    <rdfs:subClassOf rdf:resource="jc3iedmSubOnt.owl#ELECTRONIC-EQUIPMENT-TYPE-Sensor"/>
    <rdfs:subClassOf>
      <owl:Restriction>
        <owl:hasValue xml:lang="en">MGANDT</owl:hasValue>
        <owl:onProperty rdf:resource="jc3iedmBase.owl#electronic-equipment-type-subcategory-code"/>
      </owl:Restriction>
    </rdfs:subClassOf>
    <rdfs:label xml:lang="en">Magnetic anomaly detector</rdfs:label>
    <rdfs:comment xml:lang="en">A device that detects minute natural or man-made variations in the Earth's magnetic field and is used to detect submarines from aircraft.</rdfs:comment>
  </owl:Class>
  <owl:Class rdf:about="#Buoy,_beacon_dan">
    <rdfs:subClassOf rdf:resource="jc3iedmSubOnt.owl#MARITIME-EQUIPMENT-TYPE-Buoy"/>
    <rdfs:subClassOf>
      <owl:Restriction>
        <owl:hasValue xml:lang="en">BUOYBC</owl:hasValue>
        <owl:onProperty rdf:resource="jc3iedmBase.owl#maritime-equipment-type-subcategory-code"/>
      </owl:Restriction>
    </rdfs:subClassOf>
    <rdfs:label xml:lang="en">Buoy, beacon dan</rdfs:label>
    <rdfs:comment xml:lang="en">A temporary marker active buoy used during minesweeping operations to indicate the boundaries of swept paths, swept areas, known hazards or other locations for some specific reason.</rdfs:comment>
  </owl:Class>
  <owl:Class rdf:about="#Artillery,_medium">
    <rdfs:subClassOf rdf:resource="jc3iedmSubOnt.owl#WEAPON-TYPE-Field_artillery"/>
    <rdfs:subClassOf>
      <owl:Restriction>
        <owl:hasValue xml:lang="en">ARTMED</owl:hasValue>
        <owl:onProperty rdf:resource="jc3iedmBase.owl#weapon-type-subcategory-code"/>
      </owl:Restriction>
    </rdfs:subClassOf>
    <rdfs:label xml:lang="en">Artillery, medium</rdfs:label>
    <rdfs:comment xml:lang="en">Field artillery cannon with a calibre between 121 and 160mm.</rdfs:comment>
  </owl:Class>
  <owl:Class rdf:about="#Rock_strata/rock_formation">
    <rdfs:subClassOf rdf:resource="jc3iedmSubOnt.owl#GEOGRAPHIC-FEATURE-Solid_surface"/>
    <rdfs:subClassOf rdf:resource="jc3iedmSubOnt.owl#GEOGRAPHIC-FEATURE-TYPE-Landform"/>
    <rdfs:subClassOf>
      <owl:Restriction>
        <owl:hasValue xml:lang="en">RCKSTR</owl:hasValue>
        <owl:onProperty rdf:resource="jc3iedmBase.owl#geographic-feature-type-subcategory-code"/>
      </owl:Restriction>
    </rdfs:subClassOf>
    <rdfs:label xml:lang="en">Rock strata/rock formation</rdfs:label>
    <rdfs:comment xml:lang="en">A visual topographic outcrop, layers or beds of rock.</rdfs:comment>
    <rdfs:subClassOf>
      <owl:Restriction>
        <owl:hasValue xml:lang="en">RCKSTR</owl:hasValue>
        <owl:onProperty rdf:resource="jc3iedmBase.owl#geographic-feature-type-subcategory-code"/>
      </owl:Restriction>
    </rdfs:subClassOf>
  </owl:Class>
  <owl:Class rdf:ID="UN_Dangerous_Goods_NUM_2055">
    <rdfs:subClassOf>
      <owl:Restriction>
        <owl:hasValue xml:lang="en">2055</owl:hasValue>
        <owl:onProperty rdf:resource="jc3iedmBase.owl#consumable-materiel-type-united-nations-number-code"/>
      </owl:Restriction>
    </rdfs:subClassOf>
    <rdfs:label xml:lang="en">UN Dangerous Goods # 2055</rdfs:label>
    <rdfs:comment xml:lang="en">Styrene monomer, stabilized. Includes the agent(s): styrene.</rdfs:comment>
    <rdfs:subClassOf>
      <owl:Restriction>
        <owl:hasValue xml:lang="en">2055</owl:hasValue>
        <owl:onProperty rdf:resource="jc3iedmBase.owl#consumable-materiel-type-united-nations-number-code"/>
      </owl:Restriction>
    </rdfs:subClassOf>
  </owl:Class>
  <owl:Class rdf:ID="NATO_standard_fuel_code_F44">
    <rdfs:subClassOf rdf:resource="jc3iedmSubOnt.owl#CONSUMABLE-MATERIEL-TYPE-Fuel"/>
    <rdfs:subClassOf>
      <owl:Restriction>
        <owl:hasValue xml:lang="en">NASF44</owl:hasValue>
        <owl:onProperty rdf:resource="jc3iedmBase.owl#consumable-materiel-type-subcategory-code"/>
      </owl:Restriction>
    </rdfs:subClassOf>
    <rdfs:label xml:lang="en">NATO standard fuel code F44</rdfs:label>
    <rdfs:comment xml:lang="en">Turbine Fuel, Aviation, High Flash Type With S748.</rdfs:comment>
  </owl:Class>
  <owl:Class rdf:ID="UN_Dangerous_Goods_NUM_2676">
    <rdfs:subClassOf>
      <owl:Restriction>
        <owl:hasValue xml:lang="en">2676</owl:hasValue>
        <owl:onProperty rdf:resource="jc3iedmBase.owl#consumable-materiel-type-united-nations-number-code"/>
      </owl:Restriction>
    </rdfs:subClassOf>
    <rdfs:label xml:lang="en">UN Dangerous Goods # 2676</rdfs:label>
    <rdfs:comment xml:lang="en">Stibine. Includes the agent(s): stibine.</rdfs:comment>
    <rdfs:subClassOf>
      <owl:Restriction>
        <owl:hasValue xml:lang="en">2676</owl:hasValue>
        <owl:onProperty rdf:resource="jc3iedmBase.owl#consumable-materiel-type-united-nations-number-code"/>
      </owl:Restriction>
    </rdfs:subClassOf>
  </owl:Class>
  <owl:Class rdf:about="#Incapacitated,_not_walking">
    <rdfs:subClassOf>
      <owl:Restriction>
        <owl:hasValue xml:lang="en">IN</owl:hasValue>
        <owl:onProperty rdf:resource="jc3iedmBase.owl#person-status-physical-status-code"/>
      </owl:Restriction>
    </rdfs:subClassOf>
    <rdfs:subClassOf>
      <owl:Restriction>
        <owl:hasValue xml:lang="en">IN</owl:hasValue>
        <owl:onProperty rdf:resource="jc3iedmBase.owl#person-status-physical-status-code"/>
      </owl:Restriction>
    </rdfs:subClassOf>
    <rdfs:subClassOf>
      <owl:Restriction>
        <owl:hasValue xml:lang="en">IN</owl:hasValue>
        <owl:onProperty rdf:resource="jc3iedmBase.owl#person-status-physical-status-code"/>
      </owl:Restriction>
    </rdfs:subClassOf>
    <rdfs:label xml:lang="en">Incapacitated, not walking</rdfs:label>
    <rdfs:subClassOf>
      <owl:Restriction>
        <owl:hasValue xml:lang="en">IN</owl:hasValue>
        <owl:onProperty rdf:resource="jc3iedmBase.owl#person-status-physical-status-code"/>
      </owl:Restriction>
    </rdfs:subClassOf>
    <rdfs:subClassOf>
      <owl:Restriction>
        <owl:hasValue xml:lang="en">IN</owl:hasValue>
        <owl:onProperty rdf:resource="jc3iedmBase.owl#person-status-physical-status-code"/>
      </owl:Restriction>
    </rdfs:subClassOf>
    <rdfs:subClassOf>
      <owl:Restriction>
        <owl:hasValue xml:lang="en">IN</owl:hasValue>
        <owl:onProperty rdf:resource="jc3iedmBase.owl#person-status-physical-status-code"/>
      </owl:Restriction>
    </rdfs:subClassOf>
    <rdfs:comment xml:lang="en">A status indicating that a PERSON is so seriously incapacitated that the person is not capable of walking and can only be moved by stretcher.</rdfs:comment>
    <rdfs:subClassOf>
      <owl:Restriction>
        <owl:hasValue xml:lang="en">IN</owl:hasValue>
        <owl:onProperty rdf:resource="jc3iedmBase.owl#person-status-physical-status-code"/>
      </owl:Restriction>
    </rdfs:subClassOf>
  </owl:Class>
  <owl:Class rdf:ID="Acoustic_low_frequency">
    <rdfs:label xml:lang="en">Acoustic low frequency</rdfs:label>
    <rdfs:subClassOf rdf:resource="jc3iedmSubOnt.owl#AMMUNITION-TYPE-Mine,_not_known"/>
    <rdfs:subClassOf rdf:resource="jc3iedmSubOnt.owl#AMMUNITION-TYPE-Mine,_maritime,_moving"/>
    <rdfs:subClassOf rdf:resource="jc3iedmSubOnt.owl#AMMUNITION-TYPE-Mine,_seabed_-_explosive_charge_500kg_or_greater"/>
    <rdfs:subClassOf rdf:resource="jc3iedmSubOnt.owl#AMMUNITION-TYPE-Sea_mine"/>
    <rdfs:subClassOf rdf:resource="jc3iedmSubOnt.owl#AMMUNITION-TYPE-Seabed_mine"/>
    <rdfs:comment xml:lang="en">A (maritime) mine firing mechanism with an acoustic low frequency circuit, less than 2 Hz, which responds to the acoustic field of a ship or sweep.</rdfs:comment>
    <rdfs:subClassOf rdf:resource="jc3iedmSubOnt.owl#AMMUNITION-TYPE-Mine,_seabed_-_explosive_charge_less_than_500kg"/>
    <rdfs:subClassOf rdf:resource="jc3iedmSubOnt.owl#AMMUNITION-TYPE-Mine,_shallow_moored"/>
    <rdfs:subClassOf rdf:resource="jc3iedmSubOnt.owl#AMMUNITION-TYPE-Mine,_deep_moored"/>
    <rdfs:subClassOf>
      <owl:Restriction>
        <owl:hasValue xml:lang="en">ACOULF</owl:hasValue>
        <owl:onProperty rdf:resource="jc3iedmBase.owl#ammunition-type-mine-maritime-firing-code"/>
      </owl:Restriction>
    </rdfs:subClassOf>
    <rdfs:subClassOf>
      <owl:Restriction>
        <owl:hasValue xml:lang="en">ACOULF</owl:hasValue>
        <owl:onProperty rdf:resource="jc3iedmBase.owl#ammunition-type-mine-maritime-firing-code"/>
      </owl:Restriction>
    </rdfs:subClassOf>
    <rdfs:subClassOf rdf:resource="jc3iedmSubOnt.owl#AMMUNITION-TYPE-Moving_mine,_sea"/>
    <rdfs:subClassOf rdf:resource="jc3iedmSubOnt.owl#AMMUNITION-TYPE-Mine,_not_otherwise_specified"/>
    <rdfs:subClassOf rdf:resource="jc3iedmSubOnt.owl#AMMUNITION-TYPE-Mine,_moored"/>
  </owl:Class>
  <owl:Class rdf:ID="Moveable">
    <rdfs:subClassOf rdf:resource="jc3iedmSubOnt.owl#MILITARY-OBSTACLE-TYPE-Anti-tank_obstacle"/>
    <rdfs:subClassOf rdf:resource="jc3iedmSubOnt.owl#MILITARY-OBSTACLE-TYPE-Tetrahedron"/>
    <rdfs:subClassOf rdf:resource="jc3iedmSubOnt.owl#MILITARY-OBSTACLE-TYPE-Dragon_teeth"/>
    <rdfs:subClassOf>
      <owl:Restriction>
        <owl:hasValue xml:lang="en">MOVABL</owl:hasValue>
        <owl:onProperty rdf:resource="jc3iedmBase.owl#military-obstacle-type-subcategory-code"/>
      </owl:Restriction>
    </rdfs:subClassOf>
    <rdfs:label xml:lang="en">Moveable</rdfs:label>
    <rdfs:comment xml:lang="en">It is possible to move the obstacle.</rdfs:comment>
    <rdfs:subClassOf>
      <owl:Restriction>
        <owl:hasValue xml:lang="en">MOVABL</owl:hasValue>
        <owl:onProperty rdf:resource="jc3iedmBase.owl#military-obstacle-type-subcategory-code"/>
      </owl:Restriction>
    </rdfs:subClassOf>
    <rdfs:subClassOf>
      <owl:Restriction>
        <owl:hasValue xml:lang="en">MOVABL</owl:hasValue>
        <owl:onProperty rdf:resource="jc3iedmBase.owl#military-obstacle-type-subcategory-code"/>
      </owl:Restriction>
    </rdfs:subClassOf>
  </owl:Class>
  <owl:Class rdf:ID="Antenna">
    <rdfs:subClassOf rdf:resource="jc3iedmSubOnt.owl#AMMUNITION-TYPE-Mine,_maritime,_moving"/>
    <rdfs:label xml:lang="en">Antenna</rdfs:label>
    <rdfs:subClassOf rdf:resource="jc3iedmSubOnt.owl#AMMUNITION-TYPE-Mine,_seabed_-_explosive_charge_less_than_500kg"/>
    <rdfs:subClassOf rdf:resource="jc3iedmSubOnt.owl#AMMUNITION-TYPE-Mine,_deep_moored"/>
    <rdfs:subClassOf>
      <owl:Restriction>
        <owl:hasValue xml:lang="en">ANTENA</owl:hasValue>
        <owl:onProperty rdf:resource="jc3iedmBase.owl#ammunition-type-mine-maritime-firing-code"/>
      </owl:Restriction>
    </rdfs:subClassOf>
    <rdfs:subClassOf>
      <owl:Restriction>
        <owl:hasValue xml:lang="en">ANTENA</owl:hasValue>
        <owl:onProperty rdf:resource="jc3iedmBase.owl#ammunition-type-mine-maritime-firing-code"/>
      </owl:Restriction>
    </rdfs:subClassOf>
    <rdfs:subClassOf rdf:resource="jc3iedmSubOnt.owl#AMMUNITION-TYPE-Mine,_seabed_-_explosive_charge_500kg_or_greater"/>
    <rdfs:subClassOf rdf:resource="jc3iedmSubOnt.owl#AMMUNITION-TYPE-Mine,_moored"/>
    <rdfs:subClassOf rdf:resource="jc3iedmSubOnt.owl#AMMUNITION-TYPE-Moving_mine,_sea"/>
    <rdfs:subClassOf rdf:resource="jc3iedmSubOnt.owl#AMMUNITION-TYPE-Sea_mine"/>
    <rdfs:subClassOf rdf:resource="jc3iedmSubOnt.owl#AMMUNITION-TYPE-Mine,_not_known"/>
    <rdfs:comment xml:lang="en">A contact (maritime) mine firing mechanism which, when touched by a ferrous object, set up galvanic action to fire the mine. The antenna generally takes the form of a special section in the mooring cable, and/or special cable suspended above the mine by a float.</rdfs:comment>
    <rdfs:subClassOf rdf:resource="jc3iedmSubOnt.owl#AMMUNITION-TYPE-Mine,_shallow_moored"/>
    <rdfs:subClassOf rdf:resource="jc3iedmSubOnt.owl#AMMUNITION-TYPE-Mine,_not_otherwise_specified"/>
    <rdfs:subClassOf rdf:resource="jc3iedmSubOnt.owl#AMMUNITION-TYPE-Seabed_mine"/>
  </owl:Class>
  <owl:Class rdf:ID="UN_Dangerous_Goods_NUM_1134">
    <rdfs:subClassOf>
      <owl:Restriction>
        <owl:hasValue xml:lang="en">1134</owl:hasValue>
        <owl:onProperty rdf:resource="jc3iedmBase.owl#consumable-materiel-type-united-nations-number-code"/>
      </owl:Restriction>
    </rdfs:subClassOf>
    <rdfs:label xml:lang="en">UN Dangerous Goods # 1134</rdfs:label>
    <rdfs:comment xml:lang="en">Chlorobenzene. Includes the agent(s): chlorobenzene.</rdfs:comment>
    <rdfs:subClassOf>
      <owl:Restriction>
        <owl:hasValue xml:lang="en">1134</owl:hasValue>
        <owl:onProperty rdf:resource="jc3iedmBase.owl#consumable-materiel-type-united-nations-number-code"/>
      </owl:Restriction>
    </rdfs:subClassOf>
  </owl:Class>
  <owl:Class rdf:ID="Submarine_towed_array">
    <rdfs:subClassOf rdf:resource="jc3iedmSubOnt.owl#MARITIME-EQUIPMENT-TYPE-Towed_array_surveillance_system,_tactical"/>
    <rdfs:subClassOf rdf:resource="jc3iedmSubOnt.owl#MARITIME-EQUIPMENT-TYPE-Towed_array_surveillance_system"/>
    <rdfs:subClassOf>
      <owl:Restriction>
        <owl:hasValue xml:lang="en">SUBTWA</owl:hasValue>
        <owl:onProperty rdf:resource="jc3iedmBase.owl#maritime-equipment-type-subcategory-code"/>
      </owl:Restriction>
    </rdfs:subClassOf>
    <rdfs:label xml:lang="en">Submarine towed array</rdfs:label>
    <rdfs:comment xml:lang="en">No definition provided in ADatP-3 Baseline 13.1 FFIRN/FUD 1434/1.</rdfs:comment>
    <rdfs:subClassOf>
      <owl:Restriction>
        <owl:hasValue xml:lang="en">SUBTWA</owl:hasValue>
        <owl:onProperty rdf:resource="jc3iedmBase.owl#maritime-equipment-type-subcategory-code"/>
      </owl:Restriction>
    </rdfs:subClassOf>
  </owl:Class>
  <owl:Class rdf:about="#Jungle,_primary">
    <rdfs:label xml:lang="en">Jungle, primary</rdfs:label>
    <rdfs:comment xml:lang="en">An area in lowland tropics, which has heavy rainfall. It has a thick 3 tier canopy up to 60m high and a reasonably clear floor that may permit some vehicular movement. Visibility may not exceed 50m.</rdfs:comment>
  </owl:Class>
  <owl:Class rdf:ID="Hummock">
    <rdfs:subClassOf rdf:resource="jc3iedmSubOnt.owl#GEOGRAPHIC-FEATURE-Solid_surface"/>
    <rdfs:subClassOf rdf:resource="jc3iedmSubOnt.owl#GEOGRAPHIC-FEATURE-TYPE-Landform"/>
    <rdfs:subClassOf>
      <owl:Restriction>
        <owl:hasValue xml:lang="en">HUMOCK</owl:hasValue>
        <owl:onProperty rdf:resource="jc3iedmBase.owl#geographic-feature-type-subcategory-code"/>
      </owl:Restriction>
    </rdfs:subClassOf>
    <rdfs:label xml:lang="en">Hummock</rdfs:label>
    <rdfs:comment xml:lang="en">An area of higher elevation within a swamp, bog, or marsh.</rdfs:comment>
    <rdfs:subClassOf>
      <owl:Restriction>
        <owl:hasValue xml:lang="en">HUMOCK</owl:hasValue>
        <owl:onProperty rdf:resource="jc3iedmBase.owl#geographic-feature-type-subcategory-code"/>
      </owl:Restriction>
    </rdfs:subClassOf>
  </owl:Class>
  <owl:Class rdf:ID="UN_Dangerous_Goods_NUM_1098">
    <rdfs:subClassOf>
      <owl:Restriction>
        <owl:hasValue xml:lang="en">1098</owl:hasValue>
        <owl:onProperty rdf:resource="jc3iedmBase.owl#consumable-materiel-type-united-nations-number-code"/>
      </owl:Restriction>
    </rdfs:subClassOf>
    <rdfs:label xml:lang="en">UN Dangerous Goods # 1098</rdfs:label>
    <rdfs:comment xml:lang="en">Allyl alcohol. Includes the agent(s): allyl alcohol.</rdfs:comment>
    <rdfs:subClassOf>
      <owl:Restriction>
        <owl:hasValue xml:lang="en">1098</owl:hasValue>
        <owl:onProperty rdf:resource="jc3iedmBase.owl#consumable-materiel-type-united-nations-number-code"/>
      </owl:Restriction>
    </rdfs:subClassOf>
  </owl:Class>
  <owl:Class rdf:ID="Recoilless_gun">
    <rdfs:subClassOf rdf:resource="jc3iedmSubOnt.owl#WEAPON-TYPE-Anti-tank"/>
    <rdfs:subClassOf>
      <owl:Restriction>
        <owl:hasValue xml:lang="en">RECGUN</owl:hasValue>
        <owl:onProperty rdf:resource="jc3iedmBase.owl#weapon-type-subcategory-code"/>
      </owl:Restriction>
    </rdfs:subClassOf>
    <rdfs:label xml:lang="en">Recoilless gun</rdfs:label>
    <rdfs:comment xml:lang="en">A weapon capable of being fired from either a ground mount or from a vehicle, and capable of destroying tanks.</rdfs:comment>
  </owl:Class>
  <owl:Class rdf:ID="Raydist_director">
    <rdfs:subClassOf rdf:resource="jc3iedmSubOnt.owl#ELECTRONIC-EQUIPMENT-TYPE-Navigational_aid"/>
    <rdfs:subClassOf>
      <owl:Restriction>
        <owl:hasValue xml:lang="en">RYDSTD</owl:hasValue>
        <owl:onProperty rdf:resource="jc3iedmBase.owl#electronic-equipment-type-subcategory-code"/>
      </owl:Restriction>
    </rdfs:subClassOf>
    <rdfs:label xml:lang="en">Raydist director</rdfs:label>
    <rdfs:comment xml:lang="en">No definition provided in ADatP-3 Baseline 13.1 FFIRN/FUD 1200/1.</rdfs:comment>
  </owl:Class>
  <owl:Class rdf:ID="UN_Dangerous_Goods_NUM_1338">
    <rdfs:subClassOf>
      <owl:Restriction>
        <owl:hasValue xml:lang="en">1338</owl:hasValue>
        <owl:onProperty rdf:resource="jc3iedmBase.owl#consumable-materiel-type-united-nations-number-code"/>
      </owl:Restriction>
    </rdfs:subClassOf>
    <rdfs:label xml:lang="en">UN Dangerous Goods # 1338</rdfs:label>
    <rdfs:comment xml:lang="en">Phosphorus, amorphous. Includes the agent(s): red phosphorous.</rdfs:comment>
    <rdfs:subClassOf>
      <owl:Restriction>
        <owl:hasValue xml:lang="en">1338</owl:hasValue>
        <owl:onProperty rdf:resource="jc3iedmBase.owl#consumable-materiel-type-united-nations-number-code"/>
      </owl:Restriction>
    </rdfs:subClassOf>
  </owl:Class>
  <owl:Class rdf:ID="Swamp">
    <rdfs:subClassOf rdf:resource="jc3iedmSubOnt.owl#GEOGRAPHIC-FEATURE-Solid_surface"/>
    <rdfs:subClassOf rdf:resource="jc3iedmSubOnt.owl#GEOGRAPHIC-FEATURE-TYPE-Wetland"/>
    <rdfs:subClassOf rdf:resource="jc3iedmSubOnt.owl#GEOGRAPHIC-FEATURE-Liquid_surface"/>
    <rdfs:subClassOf>
      <owl:Restriction>
        <owl:hasValue xml:lang="en">SWAMP</owl:hasValue>
        <owl:onProperty rdf:resource="jc3iedmBase.owl#geographic-feature-type-subcategory-code"/>
      </owl:Restriction>
    </rdfs:subClassOf>
    <rdfs:label xml:lang="en">Swamp</rdfs:label>
    <rdfs:comment xml:lang="en">A low lying saturated area covered with water all or most of the year, where accumulating dead vegetation does not rapidly decay. It can exist on flat-lying areas created by certain geomorphic environments.</rdfs:comment>
    <rdfs:subClassOf>
      <owl:Restriction>
        <owl:hasValue xml:lang="en">SWAMP</owl:hasValue>
        <owl:onProperty rdf:resource="jc3iedmBase.owl#geographic-feature-type-subcategory-code"/>
      </owl:Restriction>
    </rdfs:subClassOf>
    <rdfs:subClassOf>
      <owl:Restriction>
        <owl:hasValue xml:lang="en">SWAMP</owl:hasValue>
        <owl:onProperty rdf:resource="jc3iedmBase.owl#geographic-feature-type-subcategory-code"/>
      </owl:Restriction>
    </rdfs:subClassOf>
  </owl:Class>
  <owl:Class rdf:ID="Acoustic">
    <rdfs:subClassOf rdf:resource="jc3iedmSubOnt.owl#AMMUNITION-TYPE-Seabed_mine"/>
    <rdfs:subClassOf rdf:resource="jc3iedmSubOnt.owl#AMMUNITION-TYPE-Sea_mine"/>
    <rdfs:comment xml:lang="en">A (maritime) mine firing mechanism with an acoustic circuit which responds to the acoustic field of a ship or sweep.</rdfs:comment>
    <rdfs:subClassOf>
      <owl:Restriction>
        <owl:hasValue xml:lang="en">ACOUST</owl:hasValue>
        <owl:onProperty rdf:resource="jc3iedmBase.owl#ammunition-type-mine-maritime-firing-code"/>
      </owl:Restriction>
    </rdfs:subClassOf>
    <rdfs:subClassOf rdf:resource="jc3iedmSubOnt.owl#AMMUNITION-TYPE-Mine,_seabed_-_explosive_charge_less_than_500kg"/>
    <rdfs:subClassOf>
      <owl:Restriction>
        <owl:hasValue xml:lang="en">ACOUST</owl:hasValue>
        <owl:onProperty rdf:resource="jc3iedmBase.owl#ammunition-type-mine-maritime-firing-code"/>
      </owl:Restriction>
    </rdfs:subClassOf>
    <rdfs:subClassOf rdf:resource="jc3iedmSubOnt.owl#AMMUNITION-TYPE-Mine,_shallow_moored"/>
    <rdfs:subClassOf rdf:resource="jc3iedmSubOnt.owl#AMMUNITION-TYPE-Mine,_maritime,_moving"/>
    <rdfs:subClassOf rdf:resource="jc3iedmSubOnt.owl#AMMUNITION-TYPE-Mine,_not_otherwise_specified"/>
    <rdfs:subClassOf>
      <owl:Restriction>
        <owl:hasValue xml:lang="en">ACOUST</owl:hasValue>
        <owl:onProperty rdf:resource="jc3iedmBase.owl#ammunition-type-mine-maritime-firing-code"/>
      </owl:Restriction>
    </rdfs:subClassOf>
    <rdfs:subClassOf rdf:resource="jc3iedmSubOnt.owl#AMMUNITION-TYPE-Mine,_seabed_-_explosive_charge_500kg_or_greater"/>
    <rdfs:subClassOf rdf:resource="jc3iedmSubOnt.owl#AMMUNITION-TYPE-Mine,_moored"/>
    <rdfs:subClassOf rdf:resource="jc3iedmSubOnt.owl#AMMUNITION-TYPE-Maritime_mine_disposal_charge"/>
    <rdfs:subClassOf rdf:resource="jc3iedmSubOnt.owl#AMMUNITION-TYPE-Moving_mine,_sea"/>
    <rdfs:subClassOf rdf:resource="jc3iedmSubOnt.owl#AMMUNITION-TYPE-Mine,_not_known"/>
    <rdfs:subClassOf rdf:resource="jc3iedmSubOnt.owl#AMMUNITION-TYPE-Mine,_deep_moored"/>
    <rdfs:label xml:lang="en">Acoustic</rdfs:label>
  </owl:Class>
  <owl:Class rdf:ID="UN_Dangerous_Goods_NUM_2198">
    <rdfs:subClassOf>
      <owl:Restriction>
        <owl:hasValue xml:lang="en">2198</owl:hasValue>
        <owl:onProperty rdf:resource="jc3iedmBase.owl#consumable-materiel-type-united-nations-number-code"/>
      </owl:Restriction>
    </rdfs:subClassOf>
    <rdfs:label xml:lang="en">UN Dangerous Goods # 2198</rdfs:label>
    <rdfs:comment xml:lang="en">Phosphorus pentafluoride. Includes the agent(s): phosphorus pentafluoride.</rdfs:comment>
    <rdfs:subClassOf>
      <owl:Restriction>
        <owl:hasValue xml:lang="en">2198</owl:hasValue>
        <owl:onProperty rdf:resource="jc3iedmBase.owl#consumable-materiel-type-united-nations-number-code"/>
      </owl:Restriction>
    </rdfs:subClassOf>
  </owl:Class>
  <owl:Class rdf:about="#Pistol/revolver">
    <rdfs:subClassOf rdf:resource="jc3iedmSubOnt.owl#WEAPON-TYPE-Small_arms"/>
    <rdfs:subClassOf>
      <owl:Restriction>
        <owl:hasValue xml:lang="en">PISTOL</owl:hasValue>
        <owl:onProperty rdf:resource="jc3iedmBase.owl#weapon-type-subcategory-code"/>
      </owl:Restriction>
    </rdfs:subClassOf>
    <rdfs:label xml:lang="en">Pistol/revolver</rdfs:label>
    <rdfs:comment xml:lang="en">A small hand-held firearm.</rdfs:comment>
  </owl:Class>
  <owl:Class rdf:ID="Covered_by_fire">
    <rdfs:subClassOf>
      <owl:Restriction>
        <owl:hasValue xml:lang="en">CVRFIR</owl:hasValue>
        <owl:onProperty rdf:resource="jc3iedmBase.owl#facility-status-operational-status-qualifier-code"/>
      </owl:Restriction>
    </rdfs:subClassOf>
    <rdfs:label xml:lang="en">Covered by fire</rdfs:label>
    <rdfs:comment xml:lang="en">Subjectively judged by the reporting organisation that a FACILITY is being protected by weaponry.</rdfs:comment>
    <rdfs:subClassOf>
      <owl:Restriction>
        <owl:hasValue xml:lang="en">CVRFIR</owl:hasValue>
        <owl:onProperty rdf:resource="jc3iedmBase.owl#facility-status-operational-status-qualifier-code"/>
      </owl:Restriction>
    </rdfs:subClassOf>
    <rdfs:subClassOf>
      <owl:Restriction>
        <owl:hasValue xml:lang="en">CVRFIR</owl:hasValue>
        <owl:onProperty rdf:resource="jc3iedmBase.owl#facility-status-operational-status-qualifier-code"/>
      </owl:Restriction>
    </rdfs:subClassOf>
  </owl:Class>
  <owl:Class rdf:ID="Telephone">
    <rdfs:subClassOf rdf:resource="jc3iedmSubOnt.owl#NETWORK-SERVICE-Voice_service"/>
    <rdfs:subClassOf rdf:resource="jc3iedmSubOnt.owl#ELECTRONIC-EQUIPMENT-TYPE-Communication"/>
    <rdfs:subClassOf>
      <owl:Restriction>
        <owl:hasValue xml:lang="en">TELEPH</owl:hasValue>
        <owl:onProperty rdf:resource="jc3iedmBase.owl#network-service-subcategory-code"/>
      </owl:Restriction>
    </rdfs:subClassOf>
    <rdfs:label xml:lang="en">Telephone</rdfs:label>
    <rdfs:comment xml:lang="en">A service that provides communication services to a fixed device.</rdfs:comment>
    <rdfs:subClassOf>
      <owl:Restriction>
        <owl:hasValue xml:lang="en">TELEPH</owl:hasValue>
        <owl:onProperty rdf:resource="jc3iedmBase.owl#electronic-equipment-type-subcategory-code"/>
      </owl:Restriction>
    </rdfs:subClassOf>
  </owl:Class>
  <owl:Class rdf:ID="Cleared">
    <rdfs:subClassOf>
      <owl:Restriction>
        <owl:hasValue xml:lang="en">CLEARD</owl:hasValue>
        <owl:onProperty rdf:resource="jc3iedmBase.owl#materiel-status-operational-status-qualifier-code"/>
      </owl:Restriction>
    </rdfs:subClassOf>
    <rdfs:label xml:lang="en">Cleared</rdfs:label>
    <rdfs:comment xml:lang="en">The piece of materiel is weapon and explosive free.</rdfs:comment>
    <rdfs:subClassOf>
      <owl:Restriction>
        <owl:hasValue xml:lang="en">CLEARD</owl:hasValue>
        <owl:onProperty rdf:resource="jc3iedmBase.owl#materiel-status-operational-status-qualifier-code"/>
      </owl:Restriction>
    </rdfs:subClassOf>
  </owl:Class>
  <owl:Class rdf:about="#Bamboo/cane">
    <rdfs:label xml:lang="en">Bamboo/cane</rdfs:label>
    <rdfs:comment xml:lang="en">Woody, treelike grass.</rdfs:comment>
  </owl:Class>
  <owl:Class rdf:ID="UN_Dangerous_Goods_NUM_1114">
    <rdfs:subClassOf>
      <owl:Restriction>
        <owl:hasValue xml:lang="en">1114</owl:hasValue>
        <owl:onProperty rdf:resource="jc3iedmBase.owl#consumable-materiel-type-united-nations-number-code"/>
      </owl:Restriction>
    </rdfs:subClassOf>
    <rdfs:label xml:lang="en">UN Dangerous Goods # 1114</rdfs:label>
    <rdfs:comment xml:lang="en">Benzene. Includes the agent(s): benzene.</rdfs:comment>
    <rdfs:subClassOf>
      <owl:Restriction>
        <owl:hasValue xml:lang="en">1114</owl:hasValue>
        <owl:onProperty rdf:resource="jc3iedmBase.owl#consumable-materiel-type-united-nations-number-code"/>
      </owl:Restriction>
    </rdfs:subClassOf>
  </owl:Class>
  <owl:Class rdf:about="#Marker,_outer">
    <rdfs:subClassOf rdf:resource="jc3iedmSubOnt.owl#ELECTRONIC-EQUIPMENT-TYPE-Navigational_aid"/>
    <rdfs:subClassOf>
      <owl:Restriction>
        <owl:hasValue xml:lang="en">MRKROU</owl:hasValue>
        <owl:onProperty rdf:resource="jc3iedmBase.owl#electronic-equipment-type-subcategory-code"/>
      </owl:Restriction>
    </rdfs:subClassOf>
    <rdfs:label xml:lang="en">Marker, outer</rdfs:label>
    <rdfs:comment xml:lang="en">A marker beacon at or near the glide path intercept altitude of an instrument landing system approach.</rdfs:comment>
  </owl:Class>
  <owl:Class rdf:about="#DM-40_(APSS/cubic)">
    <rdfs:subClassOf rdf:resource="jc3iedmSubOnt.owl#ELECTRONIC-EQUIPMENT-TYPE-Navigational_aid"/>
    <rdfs:subClassOf>
      <owl:Restriction>
        <owl:hasValue xml:lang="en">DM40AP</owl:hasValue>
        <owl:onProperty rdf:resource="jc3iedmBase.owl#electronic-equipment-type-subcategory-code"/>
      </owl:Restriction>
    </rdfs:subClassOf>
    <rdfs:label xml:lang="en">DM-40 (APSS/cubic)</rdfs:label>
    <rdfs:comment xml:lang="en">No definition provided in ADatP-3 Baseline 13.1 FFIRN/FUD 1200/1.</rdfs:comment>
  </owl:Class>
  <owl:Class rdf:ID="Surface-to-surface_missile_launcher">
    <rdfs:subClassOf rdf:resource="jc3iedmSubOnt.owl#WEAPON-TYPE-Missile_system"/>
    <rdfs:subClassOf>
      <owl:Restriction>
        <owl:hasValue xml:lang="en">SSMIS</owl:hasValue>
        <owl:onProperty rdf:resource="jc3iedmBase.owl#weapon-type-subcategory-code"/>
      </owl:Restriction>
    </rdfs:subClassOf>
    <rdfs:label xml:lang="en">Surface-to-surface missile launcher</rdfs:label>
    <rdfs:comment xml:lang="en">A structural device designed to support and hold a surface to surface missile in position for firing.</rdfs:comment>
  </owl:Class>
  <owl:Class rdf:about="#Magnetic_T,_total_component">
    <rdfs:subClassOf rdf:resource="jc3iedmSubOnt.owl#AMMUNITION-TYPE-Mine,_shallow_moored"/>
    <rdfs:subClassOf rdf:resource="jc3iedmSubOnt.owl#AMMUNITION-TYPE-Moving_mine,_sea"/>
    <rdfs:subClassOf rdf:resource="jc3iedmSubOnt.owl#AMMUNITION-TYPE-Mine,_seabed_-_explosive_charge_less_than_500kg"/>
    <rdfs:subClassOf rdf:resource="jc3iedmSubOnt.owl#AMMUNITION-TYPE-Mine,_moored"/>
    <rdfs:subClassOf rdf:resource="jc3iedmSubOnt.owl#AMMUNITION-TYPE-Mine,_seabed_-_explosive_charge_500kg_or_greater"/>
    <rdfs:subClassOf rdf:resource="jc3iedmSubOnt.owl#AMMUNITION-TYPE-Sea_mine"/>
    <rdfs:subClassOf rdf:resource="jc3iedmSubOnt.owl#AMMUNITION-TYPE-Mine,_maritime,_moving"/>
    <rdfs:subClassOf rdf:resource="jc3iedmSubOnt.owl#AMMUNITION-TYPE-Mine,_not_otherwise_specified"/>
    <rdfs:subClassOf>
      <owl:Restriction>
        <owl:hasValue xml:lang="en">MAGNTT</owl:hasValue>
        <owl:onProperty rdf:resource="jc3iedmBase.owl#ammunition-type-mine-maritime-firing-code"/>
      </owl:Restriction>
    </rdfs:subClassOf>
    <rdfs:subClassOf rdf:resource="jc3iedmSubOnt.owl#AMMUNITION-TYPE-Seabed_mine"/>
    <rdfs:label xml:lang="en">Magnetic T, total component</rdfs:label>
    <rdfs:subClassOf rdf:resource="jc3iedmSubOnt.owl#AMMUNITION-TYPE-Mine,_not_known"/>
    <rdfs:subClassOf>
      <owl:Restriction>
        <owl:hasValue xml:lang="en">MAGNTT</owl:hasValue>
        <owl:onProperty rdf:resource="jc3iedmBase.owl#ammunition-type-mine-maritime-firing-code"/>
      </owl:Restriction>
    </rdfs:subClassOf>
    <rdfs:subClassOf rdf:resource="jc3iedmSubOnt.owl#AMMUNITION-TYPE-Mine,_deep_moored"/>
    <rdfs:comment xml:lang="en">A (maritime) mine with a magnetic influence circuit that responds to the total component of the magnetic field of a ship.</rdfs:comment>
  </owl:Class>
  <owl:Class rdf:about="#Data_link,_radio">
    <rdfs:subClassOf rdf:resource="jc3iedmSubOnt.owl#ELECTRONIC-EQUIPMENT-TYPE-Communication"/>
    <rdfs:subClassOf>
      <owl:Restriction>
        <owl:hasValue xml:lang="en">DTLRAD</owl:hasValue>
        <owl:onProperty rdf:resource="jc3iedmBase.owl#electronic-equipment-type-subcategory-code"/>
      </owl:Restriction>
    </rdfs:subClassOf>
    <rdfs:label xml:lang="en">Data link, radio</rdfs:label>
    <rdfs:comment xml:lang="en">Those parts of two data terminal equipments that are controlled by a protocol along with the interconnecting radio data circuit, that together enable data transfer.</rdfs:comment>
  </owl:Class>
  <owl:Class rdf:about="#Radar,_meteorological">
    <rdfs:subClassOf rdf:resource="jc3iedmSubOnt.owl#ELECTRONIC-EQUIPMENT-TYPE-Radar"/>
    <rdfs:subClassOf>
      <owl:Restriction>
        <owl:hasValue xml:lang="en">RDRMET</owl:hasValue>
        <owl:onProperty rdf:resource="jc3iedmBase.owl#electronic-equipment-type-subcategory-code"/>
      </owl:Restriction>
    </rdfs:subClassOf>
    <rdfs:label xml:lang="en">Radar, meteorological</rdfs:label>
    <rdfs:comment xml:lang="en">A radar used to observe and measure meteorological conditions.</rdfs:comment>
  </owl:Class>
  <owl:Class rdf:ID="Desert">
    <rdfs:label xml:lang="en">Desert</rdfs:label>
    <rdfs:comment xml:lang="en">A waterless, desolate area of land with little or no vegetation typically covered with sand.</rdfs:comment>
  </owl:Class>
  <owl:Class rdf:ID="Anti-ship_surface_missile_launcher">
    <rdfs:subClassOf rdf:resource="jc3iedmSubOnt.owl#WEAPON-TYPE-Missile_system"/>
    <rdfs:subClassOf>
      <owl:Restriction>
        <owl:hasValue xml:lang="en">ASSML</owl:hasValue>
        <owl:onProperty rdf:resource="jc3iedmBase.owl#weapon-type-subcategory-code"/>
      </owl:Restriction>
    </rdfs:subClassOf>
    <rdfs:label xml:lang="en">Anti-ship surface missile launcher</rdfs:label>
    <rdfs:comment xml:lang="en">A structural device designed to support and hold an anti-ship surface missile in position for firing.</rdfs:comment>
  </owl:Class>
  <owl:Class rdf:ID="UN_Dangerous_Goods_NUM_1135">
    <rdfs:subClassOf>
      <owl:Restriction>
        <owl:hasValue xml:lang="en">1135</owl:hasValue>
        <owl:onProperty rdf:resource="jc3iedmBase.owl#consumable-materiel-type-united-nations-number-code"/>
      </owl:Restriction>
    </rdfs:subClassOf>
    <rdfs:label xml:lang="en">UN Dangerous Goods # 1135</rdfs:label>
    <rdfs:comment xml:lang="en">Ethylene chlorohydrin. Includes the agent(s): chloroethanol.</rdfs:comment>
    <rdfs:subClassOf>
      <owl:Restriction>
        <owl:hasValue xml:lang="en">1135</owl:hasValue>
        <owl:onProperty rdf:resource="jc3iedmBase.owl#consumable-materiel-type-united-nations-number-code"/>
      </owl:Restriction>
    </rdfs:subClassOf>
  </owl:Class>
  <owl:Class rdf:ID="Shipboard_inertial_system">
    <rdfs:subClassOf rdf:resource="jc3iedmSubOnt.owl#ELECTRONIC-EQUIPMENT-TYPE-Navigational_aid"/>
    <rdfs:subClassOf>
      <owl:Restriction>
        <owl:hasValue xml:lang="en">SHINST</owl:hasValue>
        <owl:onProperty rdf:resource="jc3iedmBase.owl#electronic-equipment-type-subcategory-code"/>
      </owl:Restriction>
    </rdfs:subClassOf>
    <rdfs:label xml:lang="en">Shipboard inertial system</rdfs:label>
    <rdfs:comment xml:lang="en">No definition provided in ADatP-3 Baseline 13.1 FFIRN/FUD 1434/1.</rdfs:comment>
  </owl:Class>
  <owl:Class rdf:about="#Sweep,_acoustic_LF">
    <rdfs:subClassOf rdf:resource="jc3iedmSubOnt.owl#MARITIME-EQUIPMENT-TYPE-Sweep"/>
    <rdfs:subClassOf>
      <owl:Restriction>
        <owl:hasValue xml:lang="en">SWPACL</owl:hasValue>
        <owl:onProperty rdf:resource="jc3iedmBase.owl#maritime-equipment-type-subcategory-code"/>
      </owl:Restriction>
    </rdfs:subClassOf>
    <rdfs:label xml:lang="en">Sweep, acoustic LF</rdfs:label>
    <rdfs:comment xml:lang="en">Equipment designed to locate mines by use of a sweep designed to operate the acoustic firing system of a mine, low frequency, up to 30Hz.</rdfs:comment>
  </owl:Class>
  <owl:Class rdf:about="#Buoy,_PM-5">
    <rdfs:subClassOf rdf:resource="jc3iedmSubOnt.owl#MARITIME-EQUIPMENT-TYPE-Buoy"/>
    <rdfs:subClassOf>
      <owl:Restriction>
        <owl:hasValue xml:lang="en">BUOYPM</owl:hasValue>
        <owl:onProperty rdf:resource="jc3iedmBase.owl#maritime-equipment-type-subcategory-code"/>
      </owl:Restriction>
    </rdfs:subClassOf>
    <rdfs:label xml:lang="en">Buoy, PM-5</rdfs:label>
    <rdfs:comment xml:lang="en">No definition provided in ADatP-3 Baseline 13.1 FFIRN/FUD 1196/1.</rdfs:comment>
  </owl:Class>
  <owl:Class rdf:ID="Tundra">
    <rdfs:subClassOf rdf:resource="jc3iedmSubOnt.owl#GEOGRAPHIC-FEATURE-Solid_surface"/>
    <rdfs:subClassOf rdf:resource="jc3iedmSubOnt.owl#GEOGRAPHIC-FEATURE-TYPE-Landform"/>
    <rdfs:subClassOf>
      <owl:Restriction>
        <owl:hasValue xml:lang="en">TUNDRA</owl:hasValue>
        <owl:onProperty rdf:resource="jc3iedmBase.owl#geographic-feature-type-subcategory-code"/>
      </owl:Restriction>
    </rdfs:subClassOf>
    <rdfs:label xml:lang="en">Tundra</rdfs:label>
    <rdfs:comment xml:lang="en">A prairie-like region in the Arctic and Subarctic zones in which the subsoil is permanently frozen.</rdfs:comment>
    <rdfs:subClassOf>
      <owl:Restriction>
        <owl:hasValue xml:lang="en">TUNDRA</owl:hasValue>
        <owl:onProperty rdf:resource="jc3iedmBase.owl#geographic-feature-type-subcategory-code"/>
      </owl:Restriction>
    </rdfs:subClassOf>
  </owl:Class>
  <owl:Class rdf:ID="Esker">
    <rdfs:subClassOf rdf:resource="jc3iedmSubOnt.owl#GEOGRAPHIC-FEATURE-Solid_surface"/>
    <rdfs:subClassOf rdf:resource="jc3iedmSubOnt.owl#GEOGRAPHIC-FEATURE-TYPE-Landform"/>
    <rdfs:subClassOf>
      <owl:Restriction>
        <owl:hasValue xml:lang="en">ESKER</owl:hasValue>
        <owl:onProperty rdf:resource="jc3iedmBase.owl#geographic-feature-type-subcategory-code"/>
      </owl:Restriction>
    </rdfs:subClassOf>
    <rdfs:label xml:lang="en">Esker</rdfs:label>
    <rdfs:comment xml:lang="en">A long, narrow ridge of sand and gravel deposited by a glacial stream.</rdfs:comment>
    <rdfs:subClassOf>
      <owl:Restriction>
        <owl:hasValue xml:lang="en">ESKER</owl:hasValue>
        <owl:onProperty rdf:resource="jc3iedmBase.owl#geographic-feature-type-subcategory-code"/>
      </owl:Restriction>
    </rdfs:subClassOf>
  </owl:Class>
  <owl:Class rdf:about="#Multiple_rocket_launcher,_medium">
    <rdfs:subClassOf rdf:resource="jc3iedmSubOnt.owl#WEAPON-TYPE-Rocket_artillery"/>
    <rdfs:subClassOf>
      <owl:Restriction>
        <owl:hasValue xml:lang="en">MLRSMD</owl:hasValue>
        <owl:onProperty rdf:resource="jc3iedmBase.owl#weapon-type-subcategory-code"/>
      </owl:Restriction>
    </rdfs:subClassOf>
    <rdfs:label xml:lang="en">Multiple rocket launcher, medium</rdfs:label>
    <rdfs:comment xml:lang="en">A medium structural device designed to support and hold multiple rockets in position for firing.</rdfs:comment>
  </owl:Class>
  <owl:Class rdf:about="#Sweep,_mechanical_chain">
    <rdfs:subClassOf rdf:resource="jc3iedmSubOnt.owl#MARITIME-EQUIPMENT-TYPE-Sweep"/>
    <rdfs:subClassOf>
      <owl:Restriction>
        <owl:hasValue xml:lang="en">SWPMCC</owl:hasValue>
        <owl:onProperty rdf:resource="jc3iedmBase.owl#maritime-equipment-type-subcategory-code"/>
      </owl:Restriction>
    </rdfs:subClassOf>
    <rdfs:label xml:lang="en">Sweep, mechanical chain</rdfs:label>
    <rdfs:comment xml:lang="en">Equipment designed to locate mines in the lane swept by mechanical means, chains, normally fixed between two or more minesweeping vessels, dragged across the sea-bed.</rdfs:comment>
  </owl:Class>
  <owl:Class rdf:ID="Di-phosgene">
    <rdfs:subClassOf rdf:resource="jc3iedmSubOnt.owl#CHEMICAL-MATERIEL-TYPE-Blood_agent"/>
    <rdfs:subClassOf>
      <owl:Restriction>
        <owl:hasValue xml:lang="en">DIPSGN</owl:hasValue>
        <owl:onProperty rdf:resource="jc3iedmBase.owl#chemical-materiel-type-subcategory-code"/>
      </owl:Restriction>
    </rdfs:subClassOf>
    <rdfs:label xml:lang="en">Di-phosgene</rdfs:label>
    <rdfs:comment xml:lang="en">A poisonous gas formerly used in warfare derived from phosgene. [COCl2.]</rdfs:comment>
  </owl:Class>
  <owl:Class rdf:ID="Threat_warning_system">
    <rdfs:subClassOf rdf:resource="jc3iedmSubOnt.owl#ELECTRONIC-EQUIPMENT-TYPE-Communication"/>
    <rdfs:subClassOf>
      <owl:Restriction>
        <owl:hasValue xml:lang="en">THRTWS</owl:hasValue>
        <owl:onProperty rdf:resource="jc3iedmBase.owl#electronic-equipment-type-subcategory-code"/>
      </owl:Restriction>
    </rdfs:subClassOf>
    <rdfs:label xml:lang="en">Threat warning system</rdfs:label>
    <rdfs:comment xml:lang="en">A system that provides platform threat warning or targeting support through passive reception of electromagnetic energy.</rdfs:comment>
  </owl:Class>
  <owl:Class rdf:ID="Mustard_distilled">
    <rdfs:subClassOf rdf:resource="jc3iedmSubOnt.owl#CHEMICAL-MATERIEL-TYPE-Blood_agent"/>
    <rdfs:subClassOf>
      <owl:Restriction>
        <owl:hasValue xml:lang="en">MSTRDD</owl:hasValue>
        <owl:onProperty rdf:resource="jc3iedmBase.owl#chemical-materiel-type-subcategory-code"/>
      </owl:Restriction>
    </rdfs:subClassOf>
    <rdfs:label xml:lang="en">Mustard distilled</rdfs:label>
    <rdfs:comment xml:lang="en">A colourless oily liquid, whose vapour is a powerful irritant and vesicant, used in chemical weapons.</rdfs:comment>
  </owl:Class>
  <owl:Class rdf:ID="UN_Dangerous_Goods_NUM_2911">
    <rdfs:subClassOf>
      <owl:Restriction>
        <owl:hasValue xml:lang="en">2911</owl:hasValue>
        <owl:onProperty rdf:resource="jc3iedmBase.owl#consumable-materiel-type-united-nations-number-code"/>
      </owl:Restriction>
    </rdfs:subClassOf>
    <rdfs:label xml:lang="en">UN Dangerous Goods # 2911</rdfs:label>
    <rdfs:comment xml:lang="en">Radioactive material, excepted package - instruments or articles.</rdfs:comment>
  </owl:Class>
  <owl:Class rdf:ID="Boom">
    <rdfs:subClassOf rdf:resource="jc3iedmSubOnt.owl#MISCELLANEOUS-EQUIPMENT-TYPE-Aircraft_refuelling"/>
    <rdfs:subClassOf>
      <owl:Restriction>
        <owl:hasValue xml:lang="en">BOOM</owl:hasValue>
        <owl:onProperty rdf:resource="jc3iedmBase.owl#miscellaneous-equipment-type-subcategory-code"/>
      </owl:Restriction>
    </rdfs:subClassOf>
    <rdfs:label xml:lang="en">Boom</rdfs:label>
    <rdfs:comment xml:lang="en">A component of a refuelling system by which a boom device on an aerial refuelling tanker is inserted into a receptacle on a receiver aircraft.</rdfs:comment>
  </owl:Class>
  <owl:Class rdf:ID="Destroyed">
    <rdfs:subClassOf>
      <owl:Restriction>
        <owl:hasValue xml:lang="en">DSTRYD</owl:hasValue>
        <owl:onProperty rdf:resource="jc3iedmBase.owl#organisation-status-operational-status-qualifier-code"/>
      </owl:Restriction>
    </rdfs:subClassOf>
    <rdfs:label xml:lang="en">Destroyed</rdfs:label>
    <rdfs:comment xml:lang="en">Subjectively judged by the reporting organisation that an ORGANISATION is not, and not expected ever to be, capable of performing the missions or functions for which it is created.</rdfs:comment>
    <rdfs:subClassOf>
      <owl:Restriction>
        <owl:hasValue xml:lang="en">DSTRYD</owl:hasValue>
        <owl:onProperty rdf:resource="jc3iedmBase.owl#facility-status-operational-status-qualifier-code"/>
      </owl:Restriction>
    </rdfs:subClassOf>
    <rdfs:subClassOf>
      <owl:Restriction>
        <owl:hasValue xml:lang="en">DSTRYD</owl:hasValue>
        <owl:onProperty rdf:resource="jc3iedmBase.owl#materiel-status-operational-status-qualifier-code"/>
      </owl:Restriction>
    </rdfs:subClassOf>
  </owl:Class>
  <owl:Class rdf:ID="UN_Dangerous_Goods_NUM_1888">
    <rdfs:subClassOf>
      <owl:Restriction>
        <owl:hasValue xml:lang="en">1888</owl:hasValue>
        <owl:onProperty rdf:resource="jc3iedmBase.owl#consumable-materiel-type-united-nations-number-code"/>
      </owl:Restriction>
    </rdfs:subClassOf>
    <rdfs:label xml:lang="en">UN Dangerous Goods # 1888</rdfs:label>
    <rdfs:comment xml:lang="en">Chloroform. Includes the agent(s): chloroform.</rdfs:comment>
    <rdfs:subClassOf>
      <owl:Restriction>
        <owl:hasValue xml:lang="en">1888</owl:hasValue>
        <owl:onProperty rdf:resource="jc3iedmBase.owl#consumable-materiel-type-united-nations-number-code"/>
      </owl:Restriction>
    </rdfs:subClassOf>
  </owl:Class>
  <owl:Class rdf:ID="LSD">
    <rdfs:subClassOf rdf:resource="jc3iedmSubOnt.owl#CONSUMABLE-MATERIEL-TYPE-Drug"/>
    <rdfs:subClassOf>
      <owl:Restriction>
        <owl:hasValue xml:lang="en">LSD</owl:hasValue>
        <owl:onProperty rdf:resource="jc3iedmBase.owl#consumable-materiel-type-subcategory-code"/>
      </owl:Restriction>
    </rdfs:subClassOf>
    <rdfs:label xml:lang="en">LSD</rdfs:label>
    <rdfs:comment xml:lang="en">Lysergic acid diethylamide.</rdfs:comment>
  </owl:Class>
  <owl:Class rdf:ID="Hydrogen_cyanide">
    <rdfs:subClassOf rdf:resource="jc3iedmSubOnt.owl#CHEMICAL-MATERIEL-TYPE-Blood_agent"/>
    <rdfs:subClassOf>
      <owl:Restriction>
        <owl:hasValue xml:lang="en">HDRNCY</owl:hasValue>
        <owl:onProperty rdf:resource="jc3iedmBase.owl#chemical-materiel-type-subcategory-code"/>
      </owl:Restriction>
    </rdfs:subClassOf>
    <rdfs:label xml:lang="en">Hydrogen cyanide</rdfs:label>
    <rdfs:comment xml:lang="en">A highly poisonous gas or volatile liquid with an odour of bitter almonds, made by the action of acids on cyanides. [HCN.]</rdfs:comment>
  </owl:Class>
  <owl:Class rdf:about="#Sonobuoy,_passive">
    <rdfs:subClassOf rdf:resource="jc3iedmSubOnt.owl#MARITIME-EQUIPMENT-TYPE-Buoy"/>
    <rdfs:subClassOf rdf:resource="jc3iedmSubOnt.owl#MARITIME-EQUIPMENT-TYPE-Sonar,_maritime"/>
    <rdfs:subClassOf>
      <owl:Restriction>
        <owl:hasValue xml:lang="en">SONOPA</owl:hasValue>
        <owl:onProperty rdf:resource="jc3iedmBase.owl#maritime-equipment-type-subcategory-code"/>
      </owl:Restriction>
    </rdfs:subClassOf>
    <rdfs:label xml:lang="en">Sonobuoy, passive</rdfs:label>
    <rdfs:comment xml:lang="en">No definition provided in ADatP-3 Baseline 13.1 FFIRN/FUD 1434/1.</rdfs:comment>
    <rdfs:subClassOf>
      <owl:Restriction>
        <owl:hasValue xml:lang="en">SONOPA</owl:hasValue>
        <owl:onProperty rdf:resource="jc3iedmBase.owl#maritime-equipment-type-subcategory-code"/>
      </owl:Restriction>
    </rdfs:subClassOf>
  </owl:Class>
  <owl:Class rdf:about="#Sweep,_mechanical_net">
    <rdfs:subClassOf rdf:resource="jc3iedmSubOnt.owl#MARITIME-EQUIPMENT-TYPE-Sweep"/>
    <rdfs:subClassOf>
      <owl:Restriction>
        <owl:hasValue xml:lang="en">SWPMCN</owl:hasValue>
        <owl:onProperty rdf:resource="jc3iedmBase.owl#maritime-equipment-type-subcategory-code"/>
      </owl:Restriction>
    </rdfs:subClassOf>
    <rdfs:label xml:lang="en">Sweep, mechanical net</rdfs:label>
    <rdfs:comment xml:lang="en">Equipment designed to locate mines in the lane swept by mechanical means; nets normally fixed between two or more minesweeping vessels.</rdfs:comment>
  </owl:Class>
  <owl:Class rdf:ID="Guided_cruise_missile_launcher">
    <rdfs:subClassOf rdf:resource="jc3iedmSubOnt.owl#WEAPON-TYPE-Missile_system"/>
    <rdfs:subClassOf>
      <owl:Restriction>
        <owl:hasValue xml:lang="en">GCML</owl:hasValue>
        <owl:onProperty rdf:resource="jc3iedmBase.owl#weapon-type-subcategory-code"/>
      </owl:Restriction>
    </rdfs:subClassOf>
    <rdfs:label xml:lang="en">Guided cruise missile launcher</rdfs:label>
    <rdfs:comment xml:lang="en">A structural device designed to support and hold a guided cruise missile in position for firing.</rdfs:comment>
  </owl:Class>
  <owl:Class rdf:ID="Fitted_with_ship_counter">
    <rdfs:subClassOf rdf:resource="jc3iedmSubOnt.owl#AMMUNITION-TYPE-Mine,_deep_moored"/>
    <rdfs:subClassOf rdf:resource="jc3iedmSubOnt.owl#AMMUNITION-TYPE-Sea_mine"/>
    <rdfs:subClassOf rdf:resource="jc3iedmSubOnt.owl#AMMUNITION-TYPE-Moving_mine,_sea"/>
    <rdfs:subClassOf rdf:resource="jc3iedmSubOnt.owl#AMMUNITION-TYPE-Mine,_moored"/>
    <rdfs:label xml:lang="en">Fitted with ship counter</rdfs:label>
    <rdfs:subClassOf>
      <owl:Restriction>
        <owl:hasValue xml:lang="en">FITWSC</owl:hasValue>
        <owl:onProperty rdf:resource="jc3iedmBase.owl#ammunition-type-mine-maritime-firing-code"/>
      </owl:Restriction>
    </rdfs:subClassOf>
    <rdfs:subClassOf rdf:resource="jc3iedmSubOnt.owl#AMMUNITION-TYPE-Mine,_seabed_-_explosive_charge_500kg_or_greater"/>
    <rdfs:subClassOf rdf:resource="jc3iedmSubOnt.owl#AMMUNITION-TYPE-Mine,_not_known"/>
    <rdfs:subClassOf rdf:resource="jc3iedmSubOnt.owl#AMMUNITION-TYPE-Mine,_seabed_-_explosive_charge_less_than_500kg"/>
    <rdfs:subClassOf rdf:resource="jc3iedmSubOnt.owl#AMMUNITION-TYPE-Mine,_shallow_moored"/>
    <rdfs:subClassOf rdf:resource="jc3iedmSubOnt.owl#AMMUNITION-TYPE-Mine,_maritime,_moving"/>
    <rdfs:comment xml:lang="en">A (maritime) mine firing mechanism fitted with a ship counting mechanism, a tactical device.</rdfs:comment>
    <rdfs:subClassOf rdf:resource="jc3iedmSubOnt.owl#AMMUNITION-TYPE-Seabed_mine"/>
    <rdfs:subClassOf rdf:resource="jc3iedmSubOnt.owl#AMMUNITION-TYPE-Mine,_not_otherwise_specified"/>
    <rdfs:subClassOf>
      <owl:Restriction>
        <owl:hasValue xml:lang="en">FITWSC</owl:hasValue>
        <owl:onProperty rdf:resource="jc3iedmBase.owl#ammunition-type-mine-maritime-firing-code"/>
      </owl:Restriction>
    </rdfs:subClassOf>
  </owl:Class>
  <owl:Class rdf:about="#Sweep,_magnetic_electrode">
    <rdfs:subClassOf rdf:resource="jc3iedmSubOnt.owl#MARITIME-EQUIPMENT-TYPE-Sweep"/>
    <rdfs:subClassOf>
      <owl:Restriction>
        <owl:hasValue xml:lang="en">SWPMGE</owl:hasValue>
        <owl:onProperty rdf:resource="jc3iedmBase.owl#maritime-equipment-type-subcategory-code"/>
      </owl:Restriction>
    </rdfs:subClassOf>
    <rdfs:label xml:lang="en">Sweep, magnetic electrode</rdfs:label>
    <rdfs:comment xml:lang="en">Equipment designed to locate mines by use of two buoyant conducting cable an electrode fitted between each leg, the electrical circuit being completed through the seawater.</rdfs:comment>
  </owl:Class>
  <owl:Class rdf:ID="Foreshore">
    <rdfs:subClassOf rdf:resource="jc3iedmSubOnt.owl#GEOGRAPHIC-FEATURE-Solid_surface"/>
    <rdfs:subClassOf rdf:resource="jc3iedmSubOnt.owl#GEOGRAPHIC-FEATURE-TYPE-Coastal_hydrography"/>
    <rdfs:subClassOf>
      <owl:Restriction>
        <owl:hasValue xml:lang="en">FRESHR</owl:hasValue>
        <owl:onProperty rdf:resource="jc3iedmBase.owl#geographic-feature-type-subcategory-code"/>
      </owl:Restriction>
    </rdfs:subClassOf>
    <rdfs:label xml:lang="en">Foreshore</rdfs:label>
    <rdfs:comment xml:lang="en">Area between the low water line defined by Mean Low Water Springs (MLWS) or Mean Low Low Water (MLLW) as appropriate and the normal limit of wave action above Mean High Water Springs (MHWS) or Mean High High Water (MHHW) as appropriate.</rdfs:comment>
    <rdfs:subClassOf>
      <owl:Restriction>
        <owl:hasValue xml:lang="en">FRESHR</owl:hasValue>
        <owl:onProperty rdf:resource="jc3iedmBase.owl#geographic-feature-type-subcategory-code"/>
      </owl:Restriction>
    </rdfs:subClassOf>
  </owl:Class>
  <owl:Class rdf:ID="Communication_vehicle">
    <rdfs:subClassOf rdf:resource="jc3iedmSubOnt.owl#ELECTRONIC-EQUIPMENT-TYPE-Communication"/>
    <rdfs:subClassOf>
      <owl:Restriction>
        <owl:hasValue xml:lang="en">COMVEH</owl:hasValue>
        <owl:onProperty rdf:resource="jc3iedmBase.owl#electronic-equipment-type-subcategory-code"/>
      </owl:Restriction>
    </rdfs:subClassOf>
    <rdfs:label xml:lang="en">Communication vehicle</rdfs:label>
    <rdfs:comment xml:lang="en">A vehicle equipped with communication devices.</rdfs:comment>
  </owl:Class>
  <owl:Class rdf:about="#Anti-tank_missile_launcher,_light">
    <rdfs:subClassOf rdf:resource="jc3iedmSubOnt.owl#WEAPON-TYPE-Missile_system"/>
    <rdfs:subClassOf rdf:resource="jc3iedmSubOnt.owl#WEAPON-TYPE-Anti-tank"/>
    <rdfs:subClassOf>
      <owl:Restriction>
        <owl:hasValue xml:lang="en">ATMLLT</owl:hasValue>
        <owl:onProperty rdf:resource="jc3iedmBase.owl#weapon-type-subcategory-code"/>
      </owl:Restriction>
    </rdfs:subClassOf>
    <rdfs:label xml:lang="en">Anti-tank missile launcher, light</rdfs:label>
    <rdfs:comment xml:lang="en">A light structural device designed to support and hold an anti-tank missile in position for firing.</rdfs:comment>
    <rdfs:subClassOf>
      <owl:Restriction>
        <owl:hasValue xml:lang="en">ATMLLT</owl:hasValue>
        <owl:onProperty rdf:resource="jc3iedmBase.owl#weapon-type-subcategory-code"/>
      </owl:Restriction>
    </rdfs:subClassOf>
  </owl:Class>
  <owl:Class rdf:ID="Link_11">
    <rdfs:subClassOf rdf:resource="jc3iedmSubOnt.owl#NETWORK-SERVICE-Tactical_data_link"/>
    <rdfs:subClassOf>
      <owl:Restriction>
        <owl:hasValue xml:lang="en">LNK11</owl:hasValue>
        <owl:onProperty rdf:resource="jc3iedmBase.owl#network-service-subcategory-code"/>
      </owl:Restriction>
    </rdfs:subClassOf>
    <rdfs:label xml:lang="en">Link 11</rdfs:label>
    <rdfs:comment xml:lang="en">A service that provides the basic elements for the transmission of specific message of Link 11.</rdfs:comment>
  </owl:Class>
  <owl:Class rdf:ID="UN_Dangerous_Goods_NUM_1062">
    <rdfs:subClassOf>
      <owl:Restriction>
        <owl:hasValue xml:lang="en">1062</owl:hasValue>
        <owl:onProperty rdf:resource="jc3iedmBase.owl#consumable-materiel-type-united-nations-number-code"/>
      </owl:Restriction>
    </rdfs:subClassOf>
    <rdfs:label xml:lang="en">UN Dangerous Goods # 1062</rdfs:label>
    <rdfs:comment xml:lang="en">Methyl bromide with not more than 2% chloropicrin. Includes the agent(s): methyl bromide.</rdfs:comment>
    <rdfs:subClassOf>
      <owl:Restriction>
        <owl:hasValue xml:lang="en">1062</owl:hasValue>
        <owl:onProperty rdf:resource="jc3iedmBase.owl#consumable-materiel-type-united-nations-number-code"/>
      </owl:Restriction>
    </rdfs:subClassOf>
  </owl:Class>
  <owl:Class rdf:about="#Wagon,_liquid">
    <rdfs:subClassOf rdf:resource="jc3iedmSubOnt.owl#RAILCAR-TYPE-Rolling_stock"/>
    <rdfs:subClassOf>
      <owl:Restriction>
        <owl:hasValue xml:lang="en">WGNLQD</owl:hasValue>
        <owl:onProperty rdf:resource="jc3iedmBase.owl#railcar-type-subcategory-code"/>
      </owl:Restriction>
    </rdfs:subClassOf>
    <rdfs:label xml:lang="en">Wagon, liquid</rdfs:label>
    <rdfs:comment xml:lang="en">Rolling stock used to move bulk liquids by rail.</rdfs:comment>
  </owl:Class>
  <owl:Class rdf:ID="Backshore">
    <rdfs:subClassOf rdf:resource="jc3iedmSubOnt.owl#GEOGRAPHIC-FEATURE-Solid_surface"/>
    <rdfs:subClassOf rdf:resource="jc3iedmSubOnt.owl#GEOGRAPHIC-FEATURE-TYPE-Coastal_hydrography"/>
    <rdfs:subClassOf>
      <owl:Restriction>
        <owl:hasValue xml:lang="en">BCKSHR</owl:hasValue>
        <owl:onProperty rdf:resource="jc3iedmBase.owl#geographic-feature-type-subcategory-code"/>
      </owl:Restriction>
    </rdfs:subClassOf>
    <rdfs:label xml:lang="en">Backshore</rdfs:label>
    <rdfs:comment xml:lang="en">Area between the normal limit of wave action above either Mean High Water Springs (MHWS) or Mean High High Water (MHHW) as defined by the National Authority and the maximum limit of wave action.</rdfs:comment>
    <rdfs:subClassOf>
      <owl:Restriction>
        <owl:hasValue xml:lang="en">BCKSHR</owl:hasValue>
        <owl:onProperty rdf:resource="jc3iedmBase.owl#geographic-feature-type-subcategory-code"/>
      </owl:Restriction>
    </rdfs:subClassOf>
  </owl:Class>
  <owl:Class rdf:ID="Active">
    <rdfs:subClassOf>
      <owl:Restriction>
        <owl:hasValue xml:lang="en">ACTIVE</owl:hasValue>
        <owl:onProperty rdf:resource="jc3iedmBase.owl#ammunition-type-mine-maritime-firing-code"/>
      </owl:Restriction>
    </rdfs:subClassOf>
    <rdfs:subClassOf rdf:resource="jc3iedmSubOnt.owl#AMMUNITION-TYPE-Mine,_maritime,_moving"/>
    <rdfs:subClassOf rdf:resource="jc3iedmSubOnt.owl#AMMUNITION-TYPE-Mine,_not_otherwise_specified"/>
    <rdfs:subClassOf rdf:resource="jc3iedmSubOnt.owl#AMMUNITION-TYPE-Moving_mine,_sea"/>
    <rdfs:subClassOf rdf:resource="jc3iedmSubOnt.owl#AMMUNITION-TYPE-Mine,_seabed_-_explosive_charge_less_than_500kg"/>
    <rdfs:comment xml:lang="en">A (maritime) mine firing mechanism actuated by the reflection from a target of a signal emitted by the mine.</rdfs:comment>
    <rdfs:subClassOf rdf:resource="jc3iedmSubOnt.owl#AMMUNITION-TYPE-Sea_mine"/>
    <rdfs:subClassOf rdf:resource="jc3iedmSubOnt.owl#AMMUNITION-TYPE-Seabed_mine"/>
    <rdfs:subClassOf rdf:resource="jc3iedmSubOnt.owl#AMMUNITION-TYPE-Mine,_deep_moored"/>
    <rdfs:subClassOf>
      <owl:Restriction>
        <owl:hasValue xml:lang="en">ACTIVE</owl:hasValue>
        <owl:onProperty rdf:resource="jc3iedmBase.owl#ammunition-type-mine-maritime-firing-code"/>
      </owl:Restriction>
    </rdfs:subClassOf>
    <rdfs:subClassOf rdf:resource="jc3iedmSubOnt.owl#AMMUNITION-TYPE-Mine,_moored"/>
    <rdfs:label xml:lang="en">Active</rdfs:label>
    <rdfs:subClassOf rdf:resource="jc3iedmSubOnt.owl#AMMUNITION-TYPE-Mine,_seabed_-_explosive_charge_500kg_or_greater"/>
    <rdfs:subClassOf rdf:resource="jc3iedmSubOnt.owl#AMMUNITION-TYPE-Mine,_shallow_moored"/>
    <rdfs:subClassOf rdf:resource="jc3iedmSubOnt.owl#AMMUNITION-TYPE-Mine,_not_known"/>
  </owl:Class>
  <owl:Class rdf:ID="Heavily_damaged">
    <rdfs:subClassOf>
      <owl:Restriction>
        <owl:hasValue xml:lang="en">HVYDAM</owl:hasValue>
        <owl:onProperty rdf:resource="jc3iedmBase.owl#materiel-status-operational-status-qualifier-code"/>
      </owl:Restriction>
    </rdfs:subClassOf>
    <rdfs:label xml:lang="en">Heavily damaged</rdfs:label>
    <rdfs:comment xml:lang="en">Subjectively judged by the reporting organisation to be heavily damaged.</rdfs:comment>
    <rdfs:subClassOf>
      <owl:Restriction>
        <owl:hasValue xml:lang="en">HVYDAM</owl:hasValue>
        <owl:onProperty rdf:resource="jc3iedmBase.owl#materiel-status-operational-status-qualifier-code"/>
      </owl:Restriction>
    </rdfs:subClassOf>
    <rdfs:subClassOf>
      <owl:Restriction>
        <owl:hasValue xml:lang="en">HVYDAM</owl:hasValue>
        <owl:onProperty rdf:resource="jc3iedmBase.owl#facility-status-operational-status-qualifier-code"/>
      </owl:Restriction>
    </rdfs:subClassOf>
    <rdfs:subClassOf>
      <owl:Restriction>
        <owl:hasValue xml:lang="en">HVYDAM</owl:hasValue>
        <owl:onProperty rdf:resource="jc3iedmBase.owl#organisation-status-operational-status-qualifier-code"/>
      </owl:Restriction>
    </rdfs:subClassOf>
    <rdfs:subClassOf>
      <owl:Restriction>
        <owl:hasValue xml:lang="en">HVYDAM</owl:hasValue>
        <owl:onProperty rdf:resource="jc3iedmBase.owl#facility-status-operational-status-qualifier-code"/>
      </owl:Restriction>
    </rdfs:subClassOf>
    <rdfs:subClassOf>
      <owl:Restriction>
        <owl:hasValue xml:lang="en">HVYDAM</owl:hasValue>
        <owl:onProperty rdf:resource="jc3iedmBase.owl#organisation-status-operational-status-qualifier-code"/>
      </owl:Restriction>
    </rdfs:subClassOf>
  </owl:Class>
  <owl:Class rdf:about="#2C-B">
    <rdfs:subClassOf rdf:resource="jc3iedmSubOnt.owl#CONSUMABLE-MATERIEL-TYPE-Drug"/>
    <rdfs:subClassOf>
      <owl:Restriction>
        <owl:hasValue xml:lang="en">2CB</owl:hasValue>
        <owl:onProperty rdf:resource="jc3iedmBase.owl#consumable-materiel-type-subcategory-code"/>
      </owl:Restriction>
    </rdfs:subClassOf>
    <rdfs:label xml:lang="en">2C-B</rdfs:label>
    <rdfs:comment xml:lang="en">A synthetic hallucinogenic substance marked by visual hallucinations similar to mescaline  a component of the peyote cactus.</rdfs:comment>
  </owl:Class>
  <owl:Class rdf:ID="UN_Dangerous_Goods_NUM_1076">
    <rdfs:subClassOf>
      <owl:Restriction>
        <owl:hasValue xml:lang="en">1076</owl:hasValue>
        <owl:onProperty rdf:resource="jc3iedmBase.owl#consumable-materiel-type-united-nations-number-code"/>
      </owl:Restriction>
    </rdfs:subClassOf>
    <rdfs:label xml:lang="en">UN Dangerous Goods # 1076</rdfs:label>
    <rdfs:comment xml:lang="en">Phosgene. Includes the agent(s): Phosgene; Diphosgene.</rdfs:comment>
    <rdfs:subClassOf>
      <owl:Restriction>
        <owl:hasValue xml:lang="en">1076</owl:hasValue>
        <owl:onProperty rdf:resource="jc3iedmBase.owl#consumable-materiel-type-united-nations-number-code"/>
      </owl:Restriction>
    </rdfs:subClassOf>
  </owl:Class>
  <owl:Class rdf:ID="UN_Dangerous_Goods_NUM_1994">
    <rdfs:subClassOf>
      <owl:Restriction>
        <owl:hasValue xml:lang="en">1994</owl:hasValue>
        <owl:onProperty rdf:resource="jc3iedmBase.owl#consumable-materiel-type-united-nations-number-code"/>
      </owl:Restriction>
    </rdfs:subClassOf>
    <rdfs:label xml:lang="en">UN Dangerous Goods # 1994</rdfs:label>
    <rdfs:comment xml:lang="en">Iron pentacarbonyl. Includes the agent(s): iron pentacarbonyl.</rdfs:comment>
    <rdfs:subClassOf>
      <owl:Restriction>
        <owl:hasValue xml:lang="en">1994</owl:hasValue>
        <owl:onProperty rdf:resource="jc3iedmBase.owl#consumable-materiel-type-united-nations-number-code"/>
      </owl:Restriction>
    </rdfs:subClassOf>
  </owl:Class>
  <owl:Class rdf:ID="Air-defence_missile_launcher">
    <rdfs:subClassOf rdf:resource="jc3iedmSubOnt.owl#WEAPON-TYPE-Air-defence"/>
    <rdfs:subClassOf rdf:resource="jc3iedmSubOnt.owl#WEAPON-TYPE-Missile_system"/>
    <rdfs:subClassOf>
      <owl:Restriction>
        <owl:hasValue xml:lang="en">ADMIS</owl:hasValue>
        <owl:onProperty rdf:resource="jc3iedmBase.owl#weapon-type-subcategory-code"/>
      </owl:Restriction>
    </rdfs:subClassOf>
    <rdfs:label xml:lang="en">Air-defence missile launcher</rdfs:label>
    <rdfs:comment xml:lang="en">A structural device designed to support and hold an air defence missile in position for firing.</rdfs:comment>
    <rdfs:subClassOf>
      <owl:Restriction>
        <owl:hasValue xml:lang="en">ADMIS</owl:hasValue>
        <owl:onProperty rdf:resource="jc3iedmBase.owl#weapon-type-subcategory-code"/>
      </owl:Restriction>
    </rdfs:subClassOf>
  </owl:Class>
  <owl:Class rdf:about="#Wagon,_open_container">
    <rdfs:subClassOf rdf:resource="jc3iedmSubOnt.owl#RAILCAR-TYPE-Rolling_stock"/>
    <rdfs:subClassOf>
      <owl:Restriction>
        <owl:hasValue xml:lang="en">WGNOPC</owl:hasValue>
        <owl:onProperty rdf:resource="jc3iedmBase.owl#railcar-type-subcategory-code"/>
      </owl:Restriction>
    </rdfs:subClassOf>
    <rdfs:label xml:lang="en">Wagon, open container</rdfs:label>
    <rdfs:comment xml:lang="en">Rolling stock used to move bulk loose items by rail.</rdfs:comment>
  </owl:Class>
  <owl:Class rdf:about="#Wagon,_track_repair_and_maintenance">
    <rdfs:subClassOf rdf:resource="jc3iedmSubOnt.owl#RAILCAR-TYPE-Rolling_stock"/>
    <rdfs:subClassOf>
      <owl:Restriction>
        <owl:hasValue xml:lang="en">WGNRPR</owl:hasValue>
        <owl:onProperty rdf:resource="jc3iedmBase.owl#railcar-type-subcategory-code"/>
      </owl:Restriction>
    </rdfs:subClassOf>
    <rdfs:label xml:lang="en">Wagon, track repair and maintenance</rdfs:label>
    <rdfs:comment xml:lang="en">Rolling stock used to repair (replace track) or maintain the railway track and track bed.</rdfs:comment>
  </owl:Class>
  <owl:Class rdf:ID="UN_Dangerous_Goods_NUM_2912">
    <rdfs:subClassOf>
      <owl:Restriction>
        <owl:hasValue xml:lang="en">2912</owl:hasValue>
        <owl:onProperty rdf:resource="jc3iedmBase.owl#consumable-materiel-type-united-nations-number-code"/>
      </owl:Restriction>
    </rdfs:subClassOf>
    <rdfs:label xml:lang="en">UN Dangerous Goods # 2912</rdfs:label>
    <rdfs:comment xml:lang="en">Radioactive material, low specific activity (LSA-I), non fissile or fissile-excepted.</rdfs:comment>
  </owl:Class>
  <owl:Class rdf:ID="UN_Dangerous_Goods_NUM_1889">
    <rdfs:subClassOf>
      <owl:Restriction>
        <owl:hasValue xml:lang="en">1889</owl:hasValue>
        <owl:onProperty rdf:resource="jc3iedmBase.owl#consumable-materiel-type-united-nations-number-code"/>
      </owl:Restriction>
    </rdfs:subClassOf>
    <rdfs:label xml:lang="en">UN Dangerous Goods # 1889</rdfs:label>
    <rdfs:comment xml:lang="en">Cyanogen bromide. Includes the agent(s): cyanogen bromide.</rdfs:comment>
    <rdfs:subClassOf>
      <owl:Restriction>
        <owl:hasValue xml:lang="en">1889</owl:hasValue>
        <owl:onProperty rdf:resource="jc3iedmBase.owl#consumable-materiel-type-united-nations-number-code"/>
      </owl:Restriction>
    </rdfs:subClassOf>
  </owl:Class>
  <owl:Class rdf:about="#Cutter,_end">
    <rdfs:subClassOf rdf:resource="jc3iedmSubOnt.owl#MARITIME-EQUIPMENT-TYPE-Cutter"/>
    <rdfs:subClassOf>
      <owl:Restriction>
        <owl:hasValue xml:lang="en">CUTTEN</owl:hasValue>
        <owl:onProperty rdf:resource="jc3iedmBase.owl#maritime-equipment-type-subcategory-code"/>
      </owl:Restriction>
    </rdfs:subClassOf>
    <rdfs:label xml:lang="en">Cutter, end</rdfs:label>
    <rdfs:comment xml:lang="en">In naval mine warfare a device fitted to the end of a sweep wire to cut or part the mooring of mines or obstructors; it may also be fitted in, or to, the mooring of a mine or obstructors to part a sweep wire.</rdfs:comment>
  </owl:Class>
  <owl:Class rdf:ID="Rock">
    <rdfs:subClassOf rdf:resource="jc3iedmSubOnt.owl#GEOGRAPHIC-FEATURE-Solid_surface"/>
    <rdfs:subClassOf rdf:resource="jc3iedmSubOnt.owl#GEOGRAPHIC-FEATURE-TYPE-Landform"/>
    <rdfs:subClassOf>
      <owl:Restriction>
        <owl:hasValue xml:lang="en">ROCK</owl:hasValue>
        <owl:onProperty rdf:resource="jc3iedmBase.owl#geographic-feature-type-subcategory-code"/>
      </owl:Restriction>
    </rdfs:subClassOf>
    <rdfs:label xml:lang="en">Rock</rdfs:label>
    <rdfs:comment xml:lang="en">An isolated rocky formation or a single large stone above or below the water surface.</rdfs:comment>
    <rdfs:subClassOf>
      <owl:Restriction>
        <owl:hasValue xml:lang="en">ROCK</owl:hasValue>
        <owl:onProperty rdf:resource="jc3iedmBase.owl#geographic-feature-type-subcategory-code"/>
      </owl:Restriction>
    </rdfs:subClassOf>
  </owl:Class>
  <owl:Class rdf:about="#Incapacitated,_walking">
    <rdfs:subClassOf>
      <owl:Restriction>
        <owl:hasValue xml:lang="en">IW</owl:hasValue>
        <owl:onProperty rdf:resource="jc3iedmBase.owl#person-status-physical-status-code"/>
      </owl:Restriction>
    </rdfs:subClassOf>
    <rdfs:subClassOf>
      <owl:Restriction>
        <owl:hasValue xml:lang="en">IW</owl:hasValue>
        <owl:onProperty rdf:resource="jc3iedmBase.owl#person-status-physical-status-code"/>
      </owl:Restriction>
    </rdfs:subClassOf>
    <rdfs:subClassOf>
      <owl:Restriction>
        <owl:hasValue xml:lang="en">IW</owl:hasValue>
        <owl:onProperty rdf:resource="jc3iedmBase.owl#person-status-physical-status-code"/>
      </owl:Restriction>
    </rdfs:subClassOf>
    <rdfs:subClassOf>
      <owl:Restriction>
        <owl:hasValue xml:lang="en">IW</owl:hasValue>
        <owl:onProperty rdf:resource="jc3iedmBase.owl#person-status-physical-status-code"/>
      </owl:Restriction>
    </rdfs:subClassOf>
    <rdfs:subClassOf>
      <owl:Restriction>
        <owl:hasValue xml:lang="en">IW</owl:hasValue>
        <owl:onProperty rdf:resource="jc3iedmBase.owl#person-status-physical-status-code"/>
      </owl:Restriction>
    </rdfs:subClassOf>
    <rdfs:subClassOf>
      <owl:Restriction>
        <owl:hasValue xml:lang="en">IW</owl:hasValue>
        <owl:onProperty rdf:resource="jc3iedmBase.owl#person-status-physical-status-code"/>
      </owl:Restriction>
    </rdfs:subClassOf>
    <rdfs:label xml:lang="en">Incapacitated, walking</rdfs:label>
    <rdfs:comment xml:lang="en">A status indicating that a PERSON is incapacitated, but is capable of walking.</rdfs:comment>
    <rdfs:subClassOf>
      <owl:Restriction>
        <owl:hasValue xml:lang="en">IW</owl:hasValue>
        <owl:onProperty rdf:resource="jc3iedmBase.owl#person-status-physical-status-code"/>
      </owl:Restriction>
    </rdfs:subClassOf>
    <rdfs:subClassOf>
      <owl:Restriction>
        <owl:hasValue xml:lang="en">IW</owl:hasValue>
        <owl:onProperty rdf:resource="jc3iedmBase.owl#person-status-physical-status-code"/>
      </owl:Restriction>
    </rdfs:subClassOf>
  </owl:Class>
  <owl:Class rdf:about="#Snow_field/ice_field">
    <rdfs:subClassOf rdf:resource="jc3iedmSubOnt.owl#GEOGRAPHIC-FEATURE-TYPE-Snow/ice"/>
    <rdfs:subClassOf rdf:resource="jc3iedmSubOnt.owl#GEOGRAPHIC-FEATURE-Solid_surface"/>
    <rdfs:subClassOf>
      <owl:Restriction>
        <owl:hasValue xml:lang="en">SNWICE</owl:hasValue>
        <owl:onProperty rdf:resource="jc3iedmBase.owl#geographic-feature-type-subcategory-code"/>
      </owl:Restriction>
    </rdfs:subClassOf>
    <rdfs:label xml:lang="en">Snow field/ice field</rdfs:label>
    <rdfs:comment xml:lang="en">A large area permanently covered by snow or ice over land or water.</rdfs:comment>
    <rdfs:subClassOf>
      <owl:Restriction>
        <owl:hasValue xml:lang="en">SNWICE</owl:hasValue>
        <owl:onProperty rdf:resource="jc3iedmBase.owl#geographic-feature-type-subcategory-code"/>
      </owl:Restriction>
    </rdfs:subClassOf>
  </owl:Class>
  <owl:Class rdf:about="#Air-defence_gun,_heavy">
    <rdfs:subClassOf rdf:resource="jc3iedmSubOnt.owl#WEAPON-TYPE-Air-defence"/>
    <rdfs:subClassOf>
      <owl:Restriction>
        <owl:hasValue xml:lang="en">ADHEV</owl:hasValue>
        <owl:onProperty rdf:resource="jc3iedmBase.owl#weapon-type-subcategory-code"/>
      </owl:Restriction>
    </rdfs:subClassOf>
    <rdfs:label xml:lang="en">Air-defence gun, heavy</rdfs:label>
    <rdfs:comment xml:lang="en">A heavy gun used primarily in the role of air defence.</rdfs:comment>
  </owl:Class>
  <owl:Class rdf:about="#Sonobuoy,_directional_command_activated_system">
    <rdfs:subClassOf rdf:resource="jc3iedmSubOnt.owl#MARITIME-EQUIPMENT-TYPE-Buoy"/>
    <rdfs:subClassOf rdf:resource="jc3iedmSubOnt.owl#MARITIME-EQUIPMENT-TYPE-Sonar,_maritime"/>
    <rdfs:subClassOf>
      <owl:Restriction>
        <owl:hasValue xml:lang="en">SONODC</owl:hasValue>
        <owl:onProperty rdf:resource="jc3iedmBase.owl#maritime-equipment-type-subcategory-code"/>
      </owl:Restriction>
    </rdfs:subClassOf>
    <rdfs:label xml:lang="en">Sonobuoy, directional command activated system</rdfs:label>
    <rdfs:comment xml:lang="en">No definition provided in ADatP-3 Baseline 13.1 FFIRN/FUD 1434/1.</rdfs:comment>
    <rdfs:subClassOf>
      <owl:Restriction>
        <owl:hasValue xml:lang="en">SONODC</owl:hasValue>
        <owl:onProperty rdf:resource="jc3iedmBase.owl#maritime-equipment-type-subcategory-code"/>
      </owl:Restriction>
    </rdfs:subClassOf>
  </owl:Class>
  <owl:Class rdf:ID="UN_Dangerous_Goods_NUM_1972">
    <rdfs:subClassOf>
      <owl:Restriction>
        <owl:hasValue xml:lang="en">1972</owl:hasValue>
        <owl:onProperty rdf:resource="jc3iedmBase.owl#consumable-materiel-type-united-nations-number-code"/>
      </owl:Restriction>
    </rdfs:subClassOf>
    <rdfs:label xml:lang="en">UN Dangerous Goods # 1972</rdfs:label>
    <rdfs:comment xml:lang="en">Methane, refrigerated liquid or natural gas, refrigerated liquid with high methane content. Includes the agent(s): methane.</rdfs:comment>
    <rdfs:subClassOf>
      <owl:Restriction>
        <owl:hasValue xml:lang="en">1972</owl:hasValue>
        <owl:onProperty rdf:resource="jc3iedmBase.owl#consumable-materiel-type-united-nations-number-code"/>
      </owl:Restriction>
    </rdfs:subClassOf>
  </owl:Class>
  <owl:Class rdf:about="#Marker,_back_course">
    <rdfs:subClassOf rdf:resource="jc3iedmSubOnt.owl#ELECTRONIC-EQUIPMENT-TYPE-Navigational_aid"/>
    <rdfs:subClassOf>
      <owl:Restriction>
        <owl:hasValue xml:lang="en">MRKRBA</owl:hasValue>
        <owl:onProperty rdf:resource="jc3iedmBase.owl#electronic-equipment-type-subcategory-code"/>
      </owl:Restriction>
    </rdfs:subClassOf>
    <rdfs:label xml:lang="en">Marker, back course</rdfs:label>
    <rdfs:comment xml:lang="en">A marker beacon that indicates the final approach fix, where approach descent is commenced.</rdfs:comment>
  </owl:Class>
  <owl:Class rdf:about="#Single_rocket_launcher,_medium">
    <rdfs:subClassOf rdf:resource="jc3iedmSubOnt.owl#WEAPON-TYPE-Rocket_artillery"/>
    <rdfs:subClassOf>
      <owl:Restriction>
        <owl:hasValue xml:lang="en">SRKLMD</owl:hasValue>
        <owl:onProperty rdf:resource="jc3iedmBase.owl#weapon-type-subcategory-code"/>
      </owl:Restriction>
    </rdfs:subClassOf>
    <rdfs:label xml:lang="en">Single rocket launcher, medium</rdfs:label>
    <rdfs:comment xml:lang="en">A medium structural device designed to support and hold a rocket in position for firing.</rdfs:comment>
  </owl:Class>
  <owl:Class rdf:ID="Mobile_phone">
    <rdfs:subClassOf rdf:resource="jc3iedmSubOnt.owl#NETWORK-SERVICE-Voice_service"/>
    <rdfs:subClassOf>
      <owl:Restriction>
        <owl:hasValue xml:lang="en">MOBILE</owl:hasValue>
        <owl:onProperty rdf:resource="jc3iedmBase.owl#network-service-subcategory-code"/>
      </owl:Restriction>
    </rdfs:subClassOf>
    <rdfs:label xml:lang="en">Mobile phone</rdfs:label>
    <rdfs:comment xml:lang="en">A service that provides communication services to a non-fixed device.</rdfs:comment>
  </owl:Class>
  <owl:Class rdf:ID="Audio_storage_device">
    <rdfs:subClassOf rdf:resource="jc3iedmSubOnt.owl#ELECTRONIC-EQUIPMENT-TYPE-Data-processing"/>
    <rdfs:subClassOf rdf:resource="jc3iedmSubOnt.owl#ELECTRONIC-EQUIPMENT-TYPE-Communication"/>
    <rdfs:subClassOf>
      <owl:Restriction>
        <owl:hasValue xml:lang="en">AUDSTD</owl:hasValue>
        <owl:onProperty rdf:resource="jc3iedmBase.owl#electronic-equipment-type-subcategory-code"/>
      </owl:Restriction>
    </rdfs:subClassOf>
    <rdfs:label xml:lang="en">Audio storage device</rdfs:label>
    <rdfs:comment xml:lang="en">A device, usually film, tapes, or Laser Disk used for the storage of sound.</rdfs:comment>
    <rdfs:subClassOf>
      <owl:Restriction>
        <owl:hasValue xml:lang="en">AUDSTD</owl:hasValue>
        <owl:onProperty rdf:resource="jc3iedmBase.owl#electronic-equipment-type-subcategory-code"/>
      </owl:Restriction>
    </rdfs:subClassOf>
  </owl:Class>
  <owl:Class rdf:ID="UN_Dangerous_Goods_NUM_2913">
    <rdfs:subClassOf>
      <owl:Restriction>
        <owl:hasValue xml:lang="en">2913</owl:hasValue>
        <owl:onProperty rdf:resource="jc3iedmBase.owl#consumable-materiel-type-united-nations-number-code"/>
      </owl:Restriction>
    </rdfs:subClassOf>
    <rdfs:label xml:lang="en">UN Dangerous Goods # 2913</rdfs:label>
    <rdfs:comment xml:lang="en">Radioactive material, surface contaminated objects (SCO-I or SCO-II), non fissile or fissile-excepted.</rdfs:comment>
  </owl:Class>
  <owl:Class rdf:ID="Forest">
    <rdfs:label xml:lang="en">Forest</rdfs:label>
    <rdfs:comment xml:lang="en">A dense growth of trees, plants and underbrush covering a large area.</rdfs:comment>
  </owl:Class>
  <owl:Class rdf:ID="UN_Dangerous_Goods_NUM_3172">
    <rdfs:subClassOf>
      <owl:Restriction>
        <owl:hasValue xml:lang="en">3172</owl:hasValue>
        <owl:onProperty rdf:resource="jc3iedmBase.owl#consumable-materiel-type-united-nations-number-code"/>
      </owl:Restriction>
    </rdfs:subClassOf>
    <rdfs:label xml:lang="en">UN Dangerous Goods # 3172</rdfs:label>
    <rdfs:comment xml:lang="en">Toxins, extracted from living sources, N.O.S. Includes the agent(s): Botulinum toxins; Clostidium perfringens toxins; Conotoxin; Ricin; Saxitoxin;Shiga toxin; Staphylococcus aureus toxins; Tetrodotoxin; Verotoxin; Microcystin; Trichothecene mycotoxin.</rdfs:comment>
  </owl:Class>
  <owl:Class rdf:about="#Wagon,_brake">
    <rdfs:subClassOf rdf:resource="jc3iedmSubOnt.owl#RAILCAR-TYPE-Rolling_stock"/>
    <rdfs:subClassOf>
      <owl:Restriction>
        <owl:hasValue xml:lang="en">WGNBRK</owl:hasValue>
        <owl:onProperty rdf:resource="jc3iedmBase.owl#railcar-type-subcategory-code"/>
      </owl:Restriction>
    </rdfs:subClassOf>
    <rdfs:label xml:lang="en">Wagon, brake</rdfs:label>
    <rdfs:comment xml:lang="en">Rolling stock used to assist with the control of a formed train, that when used are manned and contain auxiliary braking apparatus.</rdfs:comment>
  </owl:Class>
  <owl:Class rdf:about="#Locomotive,_tender">
    <rdfs:subClassOf rdf:resource="jc3iedmSubOnt.owl#RAILCAR-TYPE-Locomotive"/>
    <rdfs:subClassOf>
      <owl:Restriction>
        <owl:hasValue xml:lang="en">LCMTND</owl:hasValue>
        <owl:onProperty rdf:resource="jc3iedmBase.owl#railcar-type-subcategory-code"/>
      </owl:Restriction>
    </rdfs:subClassOf>
    <rdfs:label xml:lang="en">Locomotive, tender</rdfs:label>
    <rdfs:comment xml:lang="en">A locomotive tender is used to carry coal and water for a steam locomotive when not integral to the locomotive design.</rdfs:comment>
  </owl:Class>
  <owl:Class rdf:about="#Radar,_navigation">
    <rdfs:subClassOf rdf:resource="jc3iedmSubOnt.owl#ELECTRONIC-EQUIPMENT-TYPE-Radar"/>
    <rdfs:subClassOf rdf:resource="jc3iedmSubOnt.owl#ELECTRONIC-EQUIPMENT-TYPE-Navigational_aid"/>
    <rdfs:subClassOf>
      <owl:Restriction>
        <owl:hasValue xml:lang="en">RDRNAV</owl:hasValue>
        <owl:onProperty rdf:resource="jc3iedmBase.owl#electronic-equipment-type-subcategory-code"/>
      </owl:Restriction>
    </rdfs:subClassOf>
    <rdfs:label xml:lang="en">Radar, navigation</rdfs:label>
    <rdfs:comment xml:lang="en">A navigation radar is a means by which direction and/or position is assessed when moving from one point to another. The radar facilitates navigation by determining position and may also provide vector information for calculating direction and speed.</rdfs:comment>
    <rdfs:subClassOf>
      <owl:Restriction>
        <owl:hasValue xml:lang="en">RDRNAV</owl:hasValue>
        <owl:onProperty rdf:resource="jc3iedmBase.owl#electronic-equipment-type-subcategory-code"/>
      </owl:Restriction>
    </rdfs:subClassOf>
  </owl:Class>
  <owl:Class rdf:about="#Grass/scrub/brush">
    <rdfs:label xml:lang="en">Grass/scrub/brush</rdfs:label>
    <rdfs:comment xml:lang="en">Area composed of uncultured plants which may have some woody tissue.</rdfs:comment>
  </owl:Class>
  <owl:Class rdf:about="#Landslide/scree">
    <rdfs:subClassOf rdf:resource="jc3iedmSubOnt.owl#GEOGRAPHIC-FEATURE-Solid_surface"/>
    <rdfs:subClassOf rdf:resource="jc3iedmSubOnt.owl#GEOGRAPHIC-FEATURE-TYPE-Landform"/>
    <rdfs:subClassOf>
      <owl:Restriction>
        <owl:hasValue xml:lang="en">LNDSLD</owl:hasValue>
        <owl:onProperty rdf:resource="jc3iedmBase.owl#geographic-feature-type-subcategory-code"/>
      </owl:Restriction>
    </rdfs:subClassOf>
    <rdfs:label xml:lang="en">Landslide/scree</rdfs:label>
    <rdfs:comment xml:lang="en">A mass of land, with a high potential of slipping down from a mountain, hill, etc.</rdfs:comment>
    <rdfs:subClassOf>
      <owl:Restriction>
        <owl:hasValue xml:lang="en">LNDSLD</owl:hasValue>
        <owl:onProperty rdf:resource="jc3iedmBase.owl#geographic-feature-type-subcategory-code"/>
      </owl:Restriction>
    </rdfs:subClassOf>
  </owl:Class>
  <owl:Class rdf:about="#Sweep,_acoustic">
    <rdfs:subClassOf rdf:resource="jc3iedmSubOnt.owl#MARITIME-EQUIPMENT-TYPE-Sweep"/>
    <rdfs:subClassOf>
      <owl:Restriction>
        <owl:hasValue xml:lang="en">SWPACO</owl:hasValue>
        <owl:onProperty rdf:resource="jc3iedmBase.owl#maritime-equipment-type-subcategory-code"/>
      </owl:Restriction>
    </rdfs:subClassOf>
    <rdfs:label xml:lang="en">Sweep, acoustic</rdfs:label>
    <rdfs:comment xml:lang="en">Equipment designed to be used in minesweeping operations, utilizing the acoustic firing mechanisms of the target mines.</rdfs:comment>
  </owl:Class>
  <owl:Class rdf:ID="Fitted_with_delayed_arming_or_rising_mechanism">
    <rdfs:subClassOf rdf:resource="jc3iedmSubOnt.owl#AMMUNITION-TYPE-Mine,_deep_moored"/>
    <rdfs:subClassOf rdf:resource="jc3iedmSubOnt.owl#AMMUNITION-TYPE-Sea_mine"/>
    <rdfs:comment xml:lang="en">A (maritime) mine firing mechanism fitted with a timing mechanism that keeps the mine circuits open (off) for a preset time after laying. If fitted with also a rising mechanism the release and rising of the mine can be delayed by means of a device fitted to either the sinker or to the windings of the mooring cable.</rdfs:comment>
    <rdfs:subClassOf rdf:resource="jc3iedmSubOnt.owl#AMMUNITION-TYPE-Mine,_not_otherwise_specified"/>
    <rdfs:subClassOf rdf:resource="jc3iedmSubOnt.owl#AMMUNITION-TYPE-Mine,_not_known"/>
    <rdfs:subClassOf rdf:resource="jc3iedmSubOnt.owl#AMMUNITION-TYPE-Moving_mine,_sea"/>
    <rdfs:subClassOf rdf:resource="jc3iedmSubOnt.owl#AMMUNITION-TYPE-Mine,_moored"/>
    <rdfs:subClassOf rdf:resource="jc3iedmSubOnt.owl#AMMUNITION-TYPE-Seabed_mine"/>
    <rdfs:subClassOf>
      <owl:Restriction>
        <owl:hasValue xml:lang="en">FITWDA</owl:hasValue>
        <owl:onProperty rdf:resource="jc3iedmBase.owl#ammunition-type-mine-maritime-firing-code"/>
      </owl:Restriction>
    </rdfs:subClassOf>
    <rdfs:subClassOf rdf:resource="jc3iedmSubOnt.owl#AMMUNITION-TYPE-Mine,_maritime,_moving"/>
    <rdfs:subClassOf rdf:resource="jc3iedmSubOnt.owl#AMMUNITION-TYPE-Mine,_shallow_moored"/>
    <rdfs:subClassOf rdf:resource="jc3iedmSubOnt.owl#AMMUNITION-TYPE-Mine,_seabed_-_explosive_charge_500kg_or_greater"/>
    <rdfs:subClassOf>
      <owl:Restriction>
        <owl:hasValue xml:lang="en">FITWDA</owl:hasValue>
        <owl:onProperty rdf:resource="jc3iedmBase.owl#ammunition-type-mine-maritime-firing-code"/>
      </owl:Restriction>
    </rdfs:subClassOf>
    <rdfs:subClassOf rdf:resource="jc3iedmSubOnt.owl#AMMUNITION-TYPE-Mine,_seabed_-_explosive_charge_less_than_500kg"/>
    <rdfs:label xml:lang="en">Fitted with delayed arming or rising mechanism</rdfs:label>
  </owl:Class>
  <owl:Class rdf:ID="IFF_mode_3A">
    <rdfs:subClassOf rdf:resource="jc3iedmSubOnt.owl#NETWORK-SERVICE-Identification_friend_or_foe"/>
    <rdfs:subClassOf>
      <owl:Restriction>
        <owl:hasValue xml:lang="en">IFFM3A</owl:hasValue>
        <owl:onProperty rdf:resource="jc3iedmBase.owl#network-service-subcategory-code"/>
      </owl:Restriction>
    </rdfs:subClassOf>
    <rdfs:label xml:lang="en">IFF mode 3A</rdfs:label>
    <rdfs:comment xml:lang="en">A service that provides the data for IFF mode 3A.</rdfs:comment>
  </owl:Class>
  <owl:Class rdf:about="#Air-defence_gun,_light">
    <rdfs:subClassOf rdf:resource="jc3iedmSubOnt.owl#WEAPON-TYPE-Air-defence"/>
    <rdfs:subClassOf>
      <owl:Restriction>
        <owl:hasValue xml:lang="en">ADLGT</owl:hasValue>
        <owl:onProperty rdf:resource="jc3iedmBase.owl#weapon-type-subcategory-code"/>
      </owl:Restriction>
    </rdfs:subClassOf>
    <rdfs:label xml:lang="en">Air-defence gun, light</rdfs:label>
    <rdfs:comment xml:lang="en">A light gun used primarily in the role of air defence.</rdfs:comment>
  </owl:Class>
  <owl:Class rdf:ID="Disassembled">
    <rdfs:subClassOf>
      <owl:Restriction>
        <owl:hasValue xml:lang="en">DISASM</owl:hasValue>
        <owl:onProperty rdf:resource="jc3iedmBase.owl#materiel-status-operational-status-qualifier-code"/>
      </owl:Restriction>
    </rdfs:subClassOf>
    <rdfs:label xml:lang="en">Disassembled</rdfs:label>
    <rdfs:comment xml:lang="en">Subjectively judged by the reporting organisation that the MATERIEL is taken apart in a way that it can be reassembled.</rdfs:comment>
    <rdfs:subClassOf>
      <owl:Restriction>
        <owl:hasValue xml:lang="en">DISASM</owl:hasValue>
        <owl:onProperty rdf:resource="jc3iedmBase.owl#facility-status-operational-status-qualifier-code"/>
      </owl:Restriction>
    </rdfs:subClassOf>
  </owl:Class>
  <owl:Class rdf:ID="Ford">
    <rdfs:subClassOf rdf:resource="jc3iedmSubOnt.owl#GEOGRAPHIC-FEATURE-TYPE-Inland_water"/>
    <rdfs:subClassOf rdf:resource="jc3iedmSubOnt.owl#GEOGRAPHIC-FEATURE-Liquid_surface"/>
    <rdfs:subClassOf>
      <owl:Restriction>
        <owl:hasValue xml:lang="en">FORD</owl:hasValue>
        <owl:onProperty rdf:resource="jc3iedmBase.owl#geographic-feature-type-subcategory-code"/>
      </owl:Restriction>
    </rdfs:subClassOf>
    <rdfs:label xml:lang="en">Ford</rdfs:label>
    <rdfs:comment xml:lang="en">A shallow part of a body of water that can be crossed without bridging, boats, or rafts. A location in a water barrier where the physical characteristics of current, bottom, and approaches permit the passage of personnel and/or vehicles and other equipment that remain in contact with the bottom.</rdfs:comment>
    <rdfs:subClassOf>
      <owl:Restriction>
        <owl:hasValue xml:lang="en">FORD</owl:hasValue>
        <owl:onProperty rdf:resource="jc3iedmBase.owl#geographic-feature-type-subcategory-code"/>
      </owl:Restriction>
    </rdfs:subClassOf>
  </owl:Class>
  <owl:Class rdf:about="#Sweep,_acoustic_explosive">
    <rdfs:subClassOf rdf:resource="jc3iedmSubOnt.owl#MARITIME-EQUIPMENT-TYPE-Sweep"/>
    <rdfs:subClassOf>
      <owl:Restriction>
        <owl:hasValue xml:lang="en">SWPACE</owl:hasValue>
        <owl:onProperty rdf:resource="jc3iedmBase.owl#maritime-equipment-type-subcategory-code"/>
      </owl:Restriction>
    </rdfs:subClassOf>
    <rdfs:label xml:lang="en">Sweep, acoustic explosive</rdfs:label>
    <rdfs:comment xml:lang="en">Equipment designed to locate mines by use of a sweep using the detonation of explosive charges to actuate the acoustic sensors in the mine.</rdfs:comment>
  </owl:Class>
  <owl:Class rdf:about="#Buoy,_calibration">
    <rdfs:subClassOf rdf:resource="jc3iedmSubOnt.owl#ELECTRONIC-EQUIPMENT-TYPE-Navigational_aid"/>
    <rdfs:subClassOf>
      <owl:Restriction>
        <owl:hasValue xml:lang="en">BUOYCL</owl:hasValue>
        <owl:onProperty rdf:resource="jc3iedmBase.owl#electronic-equipment-type-subcategory-code"/>
      </owl:Restriction>
    </rdfs:subClassOf>
    <rdfs:label xml:lang="en">Buoy, calibration</rdfs:label>
    <rdfs:comment xml:lang="en">No definition provided in ADatP-3 Baseline 13.1 FFIRN/FUD 1434/1.</rdfs:comment>
  </owl:Class>
  <owl:Class rdf:ID="Bomber">
    <rdfs:subClassOf rdf:resource="jc3iedmSubOnt.owl#AIRCRAFT-TYPE-Fixed_wing"/>
    <rdfs:subClassOf>
      <owl:Restriction>
        <owl:hasValue xml:lang="en">BOMBER</owl:hasValue>
        <owl:onProperty rdf:resource="jc3iedmBase.owl#aircraft-type-airframe-design-code"/>
      </owl:Restriction>
    </rdfs:subClassOf>
    <rdfs:label xml:lang="en">Bomber</rdfs:label>
    <rdfs:comment xml:lang="en">An aircraft capable of air operations using air to ground ordnance to destroy or neutralize enemy forces or installations.</rdfs:comment>
  </owl:Class>
  <owl:Class rdf:ID="Helicopter">
    <rdfs:subClassOf rdf:resource="jc3iedmSubOnt.owl#AIRCRAFT-TYPE-Rotary_wing"/>
    <rdfs:subClassOf>
      <owl:Restriction>
        <owl:hasValue xml:lang="en">HELO</owl:hasValue>
        <owl:onProperty rdf:resource="jc3iedmBase.owl#aircraft-type-airframe-design-code"/>
      </owl:Restriction>
    </rdfs:subClassOf>
    <rdfs:label xml:lang="en">Helicopter</rdfs:label>
    <rdfs:comment xml:lang="en">A rotary wing aircraft capable of atmospheric flight and dependent on rotating blades for lift.</rdfs:comment>
  </owl:Class>
  <owl:Class rdf:ID="Savannah">
    <rdfs:label xml:lang="en">Savannah</rdfs:label>
    <rdfs:comment xml:lang="en">A grassy plain in tropical and subtropical regions, with few trees.</rdfs:comment>
  </owl:Class>
  <owl:Class rdf:about="#Balloon,_hand_held">
    <rdfs:subClassOf rdf:resource="jc3iedmSubOnt.owl#CONSUMABLE-MATERIEL-TYPE-General_supplies"/>
    <rdfs:subClassOf>
      <owl:Restriction>
        <owl:hasValue xml:lang="en">BALNHH</owl:hasValue>
        <owl:onProperty rdf:resource="jc3iedmBase.owl#consumable-materiel-type-subcategory-code"/>
      </owl:Restriction>
    </rdfs:subClassOf>
    <rdfs:label xml:lang="en">Balloon, hand held</rdfs:label>
    <rdfs:comment xml:lang="en">An airtight envelope of paper, silk or similar material filled with light gas or air designed to be held by hand.</rdfs:comment>
  </owl:Class>
  <owl:Class rdf:about="#River/stream_vanishing_point">
    <rdfs:subClassOf rdf:resource="jc3iedmSubOnt.owl#GEOGRAPHIC-FEATURE-TYPE-Inland_water"/>
    <rdfs:subClassOf rdf:resource="jc3iedmSubOnt.owl#GEOGRAPHIC-FEATURE-Solid_surface"/>
    <rdfs:subClassOf rdf:resource="jc3iedmSubOnt.owl#GEOGRAPHIC-FEATURE-Liquid_surface"/>
    <rdfs:subClassOf>
      <owl:Restriction>
        <owl:hasValue xml:lang="en">RVRSTV</owl:hasValue>
        <owl:onProperty rdf:resource="jc3iedmBase.owl#geographic-feature-type-subcategory-code"/>
      </owl:Restriction>
    </rdfs:subClassOf>
    <rdfs:label xml:lang="en">River/stream vanishing point</rdfs:label>
    <rdfs:comment xml:lang="en">Point at which a river or stream passes into the ground.</rdfs:comment>
    <rdfs:subClassOf>
      <owl:Restriction>
        <owl:hasValue xml:lang="en">RVRSTV</owl:hasValue>
        <owl:onProperty rdf:resource="jc3iedmBase.owl#geographic-feature-type-subcategory-code"/>
      </owl:Restriction>
    </rdfs:subClassOf>
    <rdfs:subClassOf>
      <owl:Restriction>
        <owl:hasValue xml:lang="en">RVRSTV</owl:hasValue>
        <owl:onProperty rdf:resource="jc3iedmBase.owl#geographic-feature-type-subcategory-code"/>
      </owl:Restriction>
    </rdfs:subClassOf>
  </owl:Class>
  <owl:Class rdf:about="#Radar,_counter-artillery">
    <rdfs:subClassOf rdf:resource="jc3iedmSubOnt.owl#ELECTRONIC-EQUIPMENT-TYPE-Radar"/>
    <rdfs:subClassOf rdf:resource="jc3iedmSubOnt.owl#ELECTRONIC-EQUIPMENT-TYPE-Fire_control"/>
    <rdfs:subClassOf>
      <owl:Restriction>
        <owl:hasValue xml:lang="en">RDRCAT</owl:hasValue>
        <owl:onProperty rdf:resource="jc3iedmBase.owl#electronic-equipment-type-subcategory-code"/>
      </owl:Restriction>
    </rdfs:subClassOf>
    <rdfs:label xml:lang="en">Radar, counter-artillery</rdfs:label>
    <rdfs:comment xml:lang="en">A radar used to detect and locate enemy artillery weapon systems.</rdfs:comment>
    <rdfs:subClassOf>
      <owl:Restriction>
        <owl:hasValue xml:lang="en">RDRCAT</owl:hasValue>
        <owl:onProperty rdf:resource="jc3iedmBase.owl#electronic-equipment-type-subcategory-code"/>
      </owl:Restriction>
    </rdfs:subClassOf>
  </owl:Class>
  <owl:Class rdf:about="#Radar,_relocatable_over-the-horizon">
    <rdfs:subClassOf rdf:resource="jc3iedmSubOnt.owl#ELECTRONIC-EQUIPMENT-TYPE-Radar"/>
    <rdfs:subClassOf rdf:resource="jc3iedmSubOnt.owl#ELECTRONIC-EQUIPMENT-TYPE-Navigational_aid"/>
    <rdfs:subClassOf>
      <owl:Restriction>
        <owl:hasValue xml:lang="en">RROTHR</owl:hasValue>
        <owl:onProperty rdf:resource="jc3iedmBase.owl#electronic-equipment-type-subcategory-code"/>
      </owl:Restriction>
    </rdfs:subClassOf>
    <rdfs:label xml:lang="en">Radar, relocatable over-the-horizon</rdfs:label>
    <rdfs:comment xml:lang="en">A relocatable radar system makes use of the atmospheric reflection and refraction phenomena to extend its range of detection beyond line of sight.</rdfs:comment>
    <rdfs:subClassOf>
      <owl:Restriction>
        <owl:hasValue xml:lang="en">RROTHR</owl:hasValue>
        <owl:onProperty rdf:resource="jc3iedmBase.owl#electronic-equipment-type-subcategory-code"/>
      </owl:Restriction>
    </rdfs:subClassOf>
  </owl:Class>
  <owl:Class rdf:ID="Multi_mode">
    <rdfs:label xml:lang="en">Multi mode</rdfs:label>
    <rdfs:comment xml:lang="en">Represents transportation utilizing more than one mode of transportation.</rdfs:comment>
  </owl:Class>
  <owl:Class rdf:about="#Anti-tank_gun,_heavy">
    <rdfs:subClassOf rdf:resource="jc3iedmSubOnt.owl#WEAPON-TYPE-Anti-tank"/>
    <rdfs:subClassOf>
      <owl:Restriction>
        <owl:hasValue xml:lang="en">ATGNHV</owl:hasValue>
        <owl:onProperty rdf:resource="jc3iedmBase.owl#weapon-type-subcategory-code"/>
      </owl:Restriction>
    </rdfs:subClassOf>
    <rdfs:label xml:lang="en">Anti-tank gun, heavy</rdfs:label>
    <rdfs:comment xml:lang="en">A heavy gun designed to destroy tanks.</rdfs:comment>
  </owl:Class>
  <owl:Class rdf:ID="UN_Dangerous_Goods_NUM_2194">
    <rdfs:subClassOf>
      <owl:Restriction>
        <owl:hasValue xml:lang="en">2194</owl:hasValue>
        <owl:onProperty rdf:resource="jc3iedmBase.owl#consumable-materiel-type-united-nations-number-code"/>
      </owl:Restriction>
    </rdfs:subClassOf>
    <rdfs:label xml:lang="en">UN Dangerous Goods # 2194</rdfs:label>
    <rdfs:comment xml:lang="en">Selenium hexafluoride. Includes the agent(s): selenium hexafluoride.</rdfs:comment>
    <rdfs:subClassOf>
      <owl:Restriction>
        <owl:hasValue xml:lang="en">2194</owl:hasValue>
        <owl:onProperty rdf:resource="jc3iedmBase.owl#consumable-materiel-type-united-nations-number-code"/>
      </owl:Restriction>
    </rdfs:subClassOf>
  </owl:Class>
  <owl:Class rdf:ID="UN_Dangerous_Goods_NUM_1064">
    <rdfs:subClassOf>
      <owl:Restriction>
        <owl:hasValue xml:lang="en">1064</owl:hasValue>
        <owl:onProperty rdf:resource="jc3iedmBase.owl#consumable-materiel-type-united-nations-number-code"/>
      </owl:Restriction>
    </rdfs:subClassOf>
    <rdfs:label xml:lang="en">UN Dangerous Goods # 1064</rdfs:label>
    <rdfs:comment xml:lang="en">Methyl mercaptan. Includes the agent(s): methyl mercaptan.</rdfs:comment>
    <rdfs:subClassOf>
      <owl:Restriction>
        <owl:hasValue xml:lang="en">1064</owl:hasValue>
        <owl:onProperty rdf:resource="jc3iedmBase.owl#consumable-materiel-type-united-nations-number-code"/>
      </owl:Restriction>
    </rdfs:subClassOf>
  </owl:Class>
  <owl:Class rdf:about="#Air-defence_missile_launcher,_medium_range">
    <rdfs:subClassOf rdf:resource="jc3iedmSubOnt.owl#WEAPON-TYPE-Air-defence"/>
    <rdfs:subClassOf rdf:resource="jc3iedmSubOnt.owl#WEAPON-TYPE-Missile_system"/>
    <rdfs:subClassOf>
      <owl:Restriction>
        <owl:hasValue xml:lang="en">ADMLMR</owl:hasValue>
        <owl:onProperty rdf:resource="jc3iedmBase.owl#weapon-type-subcategory-code"/>
      </owl:Restriction>
    </rdfs:subClassOf>
    <rdfs:label xml:lang="en">Air-defence missile launcher, medium range</rdfs:label>
    <rdfs:comment xml:lang="en">A structural device designed to support and hold a medium range air defence missile in position for firing.</rdfs:comment>
    <rdfs:subClassOf>
      <owl:Restriction>
        <owl:hasValue xml:lang="en">ADMLMR</owl:hasValue>
        <owl:onProperty rdf:resource="jc3iedmBase.owl#weapon-type-subcategory-code"/>
      </owl:Restriction>
    </rdfs:subClassOf>
  </owl:Class>
  <owl:Class rdf:ID="UN_Dangerous_Goods_NUM_2900">
    <rdfs:subClassOf>
      <owl:Restriction>
        <owl:hasValue xml:lang="en">2900</owl:hasValue>
        <owl:onProperty rdf:resource="jc3iedmBase.owl#consumable-materiel-type-united-nations-number-code"/>
      </owl:Restriction>
    </rdfs:subClassOf>
    <rdfs:label xml:lang="en">UN Dangerous Goods # 2900</rdfs:label>
    <rdfs:comment xml:lang="en">Infectious substance, affecting animals only. Includes the agent(s): African swine fever virus; Highly pathogenic Avian influenza virus (synonym: fowl plague); Bluetongue virus; Foot and mouth disease virus; Goat pox virus; Herpes virus (Aujeszkys disease); Hog cholera virus (synonym: Swine fever virus); Lyssa virus; Newcastle disease virus; Peste des petits ruminants virus; Porcine enterovirus type-9 (synonym: Swine vesicular disease virus); Rinderpest virus (synonym: Cattle plague; Sheep pox virus; Teschen disease virus; Vesicular stomatitis virus; Mycoplasma mycoides; Contagious bovine pleuropneumonia; Contagious Equine Metritis; Heartwater (Cowdria); Screwworm Myiasis (synonym: Blowfly; Cochliomyia hominivorax); Swine vesicular disease.</rdfs:comment>
  </owl:Class>
  <owl:Class rdf:about="#Mortar,_heavy">
    <rdfs:subClassOf rdf:resource="jc3iedmSubOnt.owl#WEAPON-TYPE-Mortar"/>
    <rdfs:subClassOf>
      <owl:Restriction>
        <owl:hasValue xml:lang="en">MRTHEV</owl:hasValue>
        <owl:onProperty rdf:resource="jc3iedmBase.owl#weapon-type-subcategory-code"/>
      </owl:Restriction>
    </rdfs:subClassOf>
    <rdfs:label xml:lang="en">Mortar, heavy</rdfs:label>
    <rdfs:comment xml:lang="en">A towed or vehicle-mounted, indirect fire weapon with either a rifled or smooth bore. It usually has a shorter range than a howitzer, employs a higher angle of fire, and its calibre is usually between 108mm and 150mm.</rdfs:comment>
  </owl:Class>
  <owl:Class rdf:about="#Surveillance_towed_array_(long_range)_system">
    <rdfs:subClassOf rdf:resource="jc3iedmSubOnt.owl#MARITIME-EQUIPMENT-TYPE-Towed_array_surveillance_system,_tactical"/>
    <rdfs:subClassOf rdf:resource="jc3iedmSubOnt.owl#MARITIME-EQUIPMENT-TYPE-Towed_array_surveillance_system"/>
    <rdfs:subClassOf>
      <owl:Restriction>
        <owl:hasValue xml:lang="en">SUBTAS</owl:hasValue>
        <owl:onProperty rdf:resource="jc3iedmBase.owl#maritime-equipment-type-subcategory-code"/>
      </owl:Restriction>
    </rdfs:subClassOf>
    <rdfs:label xml:lang="en">Surveillance towed array (long range) system</rdfs:label>
    <rdfs:comment xml:lang="en">No definition provided in ADatP-3 Baseline 13.1 FFIRN/FUD 1434/1.</rdfs:comment>
    <rdfs:subClassOf>
      <owl:Restriction>
        <owl:hasValue xml:lang="en">SUBTAS</owl:hasValue>
        <owl:onProperty rdf:resource="jc3iedmBase.owl#maritime-equipment-type-subcategory-code"/>
      </owl:Restriction>
    </rdfs:subClassOf>
  </owl:Class>
  <owl:Class rdf:ID="UN_Dangerous_Goods_NUM_2814">
    <rdfs:subClassOf>
      <owl:Restriction>
        <owl:hasValue xml:lang="en">2814</owl:hasValue>
        <owl:onProperty rdf:resource="jc3iedmBase.owl#consumable-materiel-type-united-nations-number-code"/>
      </owl:Restriction>
    </rdfs:subClassOf>
    <rdfs:label xml:lang="en">UN Dangerous Goods # 2814</rdfs:label>
    <rdfs:comment xml:lang="en">Infectious substance, affecting humans. Includes the agent(s): Chikungunya virus; Crimean-Congo hemorrhagic fever virus; Dengue fever virus; Eastern equine encephalitis virus; Ebola virus; Hantaan virus; Junin virus; Lassa virus; Lymphocytic choriomeningitis virus; Machupo virus; Marburg virus; Monkeypox; Rift Valley Fever virus; Tick-borne encephalitis virus; Variola virus; Venezuelan equine encephalitis virus; Western equine encephalitis virus; Yellow fever virus; Japanese encephalitis virus; Coxiella burnetii; Bart quintana; Rickettsia prowasecki; Rickettsia rickettsii; Bacillus anthracis; Brucella abortus; Brucella melitensis; Brucella suis; Chlamydia psittaci; Clostridium botulinum; Francisella tularensis; Burkholderia mallei; Burkholderia pseudomallei; Salmonella typhi; Shigella dysenteriae; Vibrio cholerae; Yersinia pestis.</rdfs:comment>
  </owl:Class>
  <owl:Class rdf:about="#Radar,_ranging">
    <rdfs:subClassOf rdf:resource="jc3iedmSubOnt.owl#ELECTRONIC-EQUIPMENT-TYPE-Radar"/>
    <rdfs:subClassOf>
      <owl:Restriction>
        <owl:hasValue xml:lang="en">RDRRNG</owl:hasValue>
        <owl:onProperty rdf:resource="jc3iedmBase.owl#electronic-equipment-type-subcategory-code"/>
      </owl:Restriction>
    </rdfs:subClassOf>
    <rdfs:label xml:lang="en">Radar, ranging</rdfs:label>
    <rdfs:comment xml:lang="en">A radar used for the process of establishing target distance.</rdfs:comment>
  </owl:Class>
  <owl:Class rdf:about="#Machine_gun,_light">
    <rdfs:subClassOf rdf:resource="jc3iedmSubOnt.owl#WEAPON-TYPE-Small_arms"/>
    <rdfs:subClassOf>
      <owl:Restriction>
        <owl:hasValue xml:lang="en">MACGLT</owl:hasValue>
        <owl:onProperty rdf:resource="jc3iedmBase.owl#weapon-type-subcategory-code"/>
      </owl:Restriction>
    </rdfs:subClassOf>
    <rdfs:label xml:lang="en">Machine gun, light</rdfs:label>
    <rdfs:comment xml:lang="en">A light automatic gun giving continuous fire.</rdfs:comment>
  </owl:Class>
  <owl:Class rdf:ID="Mini-ranger_model">
    <rdfs:subClassOf rdf:resource="jc3iedmSubOnt.owl#ELECTRONIC-EQUIPMENT-TYPE-Navigational_aid"/>
    <rdfs:subClassOf>
      <owl:Restriction>
        <owl:hasValue xml:lang="en">MINIRN</owl:hasValue>
        <owl:onProperty rdf:resource="jc3iedmBase.owl#electronic-equipment-type-subcategory-code"/>
      </owl:Restriction>
    </rdfs:subClassOf>
    <rdfs:label xml:lang="en">Mini-ranger model</rdfs:label>
    <rdfs:comment xml:lang="en">No definition provided in ADatP-3 Baseline 13.1 FFIRN/FUD 1200/1.</rdfs:comment>
  </owl:Class>
  <owl:Class rdf:about="#Sand_dune/sand_hill">
    <rdfs:subClassOf rdf:resource="jc3iedmSubOnt.owl#GEOGRAPHIC-FEATURE-Solid_surface"/>
    <rdfs:subClassOf rdf:resource="jc3iedmSubOnt.owl#GEOGRAPHIC-FEATURE-TYPE-Landform"/>
    <rdfs:subClassOf>
      <owl:Restriction>
        <owl:hasValue xml:lang="en">SNDDUN</owl:hasValue>
        <owl:onProperty rdf:resource="jc3iedmBase.owl#geographic-feature-type-subcategory-code"/>
      </owl:Restriction>
    </rdfs:subClassOf>
    <rdfs:label xml:lang="en">Sand dune/sand hill</rdfs:label>
    <rdfs:comment xml:lang="en">Ridges or hills of sand.</rdfs:comment>
    <rdfs:subClassOf>
      <owl:Restriction>
        <owl:hasValue xml:lang="en">SNDDUN</owl:hasValue>
        <owl:onProperty rdf:resource="jc3iedmBase.owl#geographic-feature-type-subcategory-code"/>
      </owl:Restriction>
    </rdfs:subClassOf>
  </owl:Class>
  <owl:Class rdf:ID="Chlamydia">
    <rdfs:subClassOf rdf:resource="jc3iedmSubOnt.owl#BIOLOGICAL-MATERIEL-TYPE-Bacterial"/>
    <rdfs:subClassOf>
      <owl:Restriction>
        <owl:hasValue xml:lang="en">CHLMYD</owl:hasValue>
        <owl:onProperty rdf:resource="jc3iedmBase.owl#biological-materiel-type-subcategory-code"/>
      </owl:Restriction>
    </rdfs:subClassOf>
    <rdfs:label xml:lang="en">Chlamydia</rdfs:label>
    <rdfs:comment xml:lang="en">A very small parasitic bacterium that, like a virus, requires the biochemical mechanisms of another cell in order to reproduce.</rdfs:comment>
  </owl:Class>
  <owl:Class rdf:ID="IFF_mode_5">
    <rdfs:subClassOf rdf:resource="jc3iedmSubOnt.owl#NETWORK-SERVICE-Identification_friend_or_foe"/>
    <rdfs:subClassOf>
      <owl:Restriction>
        <owl:hasValue xml:lang="en">IFFM5</owl:hasValue>
        <owl:onProperty rdf:resource="jc3iedmBase.owl#network-service-subcategory-code"/>
      </owl:Restriction>
    </rdfs:subClassOf>
    <rdfs:label xml:lang="en">IFF mode 5</rdfs:label>
    <rdfs:comment xml:lang="en">A service that provides the data for IFF mode 5.</rdfs:comment>
  </owl:Class>
  <owl:Class rdf:ID="Cropland">
    <rdfs:label xml:lang="en">Cropland</rdfs:label>
    <rdfs:comment xml:lang="en">An area that has been tilled for the planting of crops.</rdfs:comment>
  </owl:Class>
  <owl:Class rdf:ID="Anti-tank_gun">
    <rdfs:subClassOf rdf:resource="jc3iedmSubOnt.owl#WEAPON-TYPE-Anti-tank"/>
    <rdfs:subClassOf>
      <owl:Restriction>
        <owl:hasValue xml:lang="en">ATGUN</owl:hasValue>
        <owl:onProperty rdf:resource="jc3iedmBase.owl#weapon-type-subcategory-code"/>
      </owl:Restriction>
    </rdfs:subClassOf>
    <rdfs:label xml:lang="en">Anti-tank gun</rdfs:label>
    <rdfs:comment xml:lang="en">A gun designed to destroy tanks.</rdfs:comment>
  </owl:Class>
  <owl:Class rdf:about="#Radar,_air-traffic_control">
    <rdfs:subClassOf rdf:resource="jc3iedmSubOnt.owl#ELECTRONIC-EQUIPMENT-TYPE-Radar"/>
    <rdfs:subClassOf>
      <owl:Restriction>
        <owl:hasValue xml:lang="en">RDRATC</owl:hasValue>
        <owl:onProperty rdf:resource="jc3iedmBase.owl#electronic-equipment-type-subcategory-code"/>
      </owl:Restriction>
    </rdfs:subClassOf>
    <rdfs:label xml:lang="en">Radar, air-traffic control</rdfs:label>
    <rdfs:comment xml:lang="en">A radar used for monitoring air traffic.</rdfs:comment>
  </owl:Class>
  <owl:Class rdf:about="#Buoy,_standard_dan">
    <rdfs:subClassOf rdf:resource="jc3iedmSubOnt.owl#MARITIME-EQUIPMENT-TYPE-Buoy"/>
    <rdfs:subClassOf>
      <owl:Restriction>
        <owl:hasValue xml:lang="en">BUOYSD</owl:hasValue>
        <owl:onProperty rdf:resource="jc3iedmBase.owl#maritime-equipment-type-subcategory-code"/>
      </owl:Restriction>
    </rdfs:subClassOf>
    <rdfs:label xml:lang="en">Buoy, standard dan</rdfs:label>
    <rdfs:comment xml:lang="en">A temporary marker active buoy used during minesweeping operations to indicate the boundaries of swept paths, swept areas, known hazards or other locations for some specific reason.</rdfs:comment>
  </owl:Class>
  <owl:Class rdf:ID="UN_Dangerous_Goods_NUM_1595">
    <rdfs:subClassOf>
      <owl:Restriction>
        <owl:hasValue xml:lang="en">1595</owl:hasValue>
        <owl:onProperty rdf:resource="jc3iedmBase.owl#consumable-materiel-type-united-nations-number-code"/>
      </owl:Restriction>
    </rdfs:subClassOf>
    <rdfs:label xml:lang="en">UN Dangerous Goods # 1595</rdfs:label>
    <rdfs:comment xml:lang="en">Dimethyl sulphate. Includes the agent(s): dimethyl sulfate.</rdfs:comment>
    <rdfs:subClassOf>
      <owl:Restriction>
        <owl:hasValue xml:lang="en">1595</owl:hasValue>
        <owl:onProperty rdf:resource="jc3iedmBase.owl#consumable-materiel-type-united-nations-number-code"/>
      </owl:Restriction>
    </rdfs:subClassOf>
  </owl:Class>
  <owl:Class rdf:ID="Hedgerow">
    <rdfs:label xml:lang="en">Hedgerow</rdfs:label>
    <rdfs:comment xml:lang="en">A continuous growth of shrubbery planted as a fence, a boundary, or a wind break.</rdfs:comment>
  </owl:Class>
  <owl:Class rdf:ID="Road">
    <rdfs:subClassOf rdf:resource="jc3iedmBase.owl#ROAD"/>
    <rdfs:label xml:lang="en">Road</rdfs:label>
    <rdfs:comment xml:lang="en">Represents the general mode of transportation used in surface movement by road.</rdfs:comment>
  </owl:Class>
  <owl:Class rdf:ID="Bog">
    <rdfs:subClassOf rdf:resource="jc3iedmSubOnt.owl#GEOGRAPHIC-FEATURE-Solid_surface"/>
    <rdfs:subClassOf rdf:resource="jc3iedmSubOnt.owl#GEOGRAPHIC-FEATURE-TYPE-Wetland"/>
    <rdfs:subClassOf rdf:resource="jc3iedmSubOnt.owl#GEOGRAPHIC-FEATURE-Liquid_surface"/>
    <rdfs:subClassOf>
      <owl:Restriction>
        <owl:hasValue xml:lang="en">BOG</owl:hasValue>
        <owl:onProperty rdf:resource="jc3iedmBase.owl#geographic-feature-type-subcategory-code"/>
      </owl:Restriction>
    </rdfs:subClassOf>
    <rdfs:label xml:lang="en">Bog</rdfs:label>
    <rdfs:comment xml:lang="en">A poorly drained or periodically flooded area, excluding tidal waters, with soil rich in plant residue.</rdfs:comment>
    <rdfs:subClassOf>
      <owl:Restriction>
        <owl:hasValue xml:lang="en">BOG</owl:hasValue>
        <owl:onProperty rdf:resource="jc3iedmBase.owl#geographic-feature-type-subcategory-code"/>
      </owl:Restriction>
    </rdfs:subClassOf>
    <rdfs:subClassOf>
      <owl:Restriction>
        <owl:hasValue xml:lang="en">BOG</owl:hasValue>
        <owl:onProperty rdf:resource="jc3iedmBase.owl#geographic-feature-type-subcategory-code"/>
      </owl:Restriction>
    </rdfs:subClassOf>
  </owl:Class>
  <owl:Class rdf:ID="Fan">
    <rdfs:subClassOf rdf:resource="jc3iedmSubOnt.owl#GEOGRAPHIC-FEATURE-Solid_surface"/>
    <rdfs:subClassOf rdf:resource="jc3iedmSubOnt.owl#GEOGRAPHIC-FEATURE-TYPE-Landform"/>
    <rdfs:subClassOf>
      <owl:Restriction>
        <owl:hasValue xml:lang="en">FAN</owl:hasValue>
        <owl:onProperty rdf:resource="jc3iedmBase.owl#geographic-feature-type-subcategory-code"/>
      </owl:Restriction>
    </rdfs:subClassOf>
    <rdfs:label xml:lang="en">Fan</rdfs:label>
    <rdfs:comment xml:lang="en">A gently sloping fan shaped feature usually found near the lower termination of a canyon.</rdfs:comment>
    <rdfs:subClassOf>
      <owl:Restriction>
        <owl:hasValue xml:lang="en">FAN</owl:hasValue>
        <owl:onProperty rdf:resource="jc3iedmBase.owl#geographic-feature-type-subcategory-code"/>
      </owl:Restriction>
    </rdfs:subClassOf>
  </owl:Class>
  <owl:Class rdf:ID="SHF">
    <rdfs:subClassOf rdf:resource="jc3iedmSubOnt.owl#MARITIME-EQUIPMENT-TYPE-Buoy"/>
    <rdfs:subClassOf>
      <owl:Restriction>
        <owl:hasValue xml:lang="en">SHF</owl:hasValue>
        <owl:onProperty rdf:resource="jc3iedmBase.owl#maritime-equipment-type-subcategory-code"/>
      </owl:Restriction>
    </rdfs:subClassOf>
    <rdfs:label xml:lang="en">SHF</rdfs:label>
    <rdfs:comment xml:lang="en">A relaying air dropped sonobuoy 4-64 channels.</rdfs:comment>
  </owl:Class>
  <owl:Class rdf:ID="UN_Dangerous_Goods_NUM_1244">
    <rdfs:subClassOf>
      <owl:Restriction>
        <owl:hasValue xml:lang="en">1244</owl:hasValue>
        <owl:onProperty rdf:resource="jc3iedmBase.owl#consumable-materiel-type-united-nations-number-code"/>
      </owl:Restriction>
    </rdfs:subClassOf>
    <rdfs:label xml:lang="en">UN Dangerous Goods # 1244</rdfs:label>
    <rdfs:comment xml:lang="en">Methylhydrazine. Includes the agent(s): methyl hydrazine.</rdfs:comment>
    <rdfs:subClassOf>
      <owl:Restriction>
        <owl:hasValue xml:lang="en">1244</owl:hasValue>
        <owl:onProperty rdf:resource="jc3iedmBase.owl#consumable-materiel-type-united-nations-number-code"/>
      </owl:Restriction>
    </rdfs:subClassOf>
  </owl:Class>
  <owl:Class rdf:about="#Radar,_guidance">
    <rdfs:subClassOf rdf:resource="jc3iedmSubOnt.owl#ELECTRONIC-EQUIPMENT-TYPE-Radar"/>
    <rdfs:subClassOf rdf:resource="jc3iedmSubOnt.owl#ELECTRONIC-EQUIPMENT-TYPE-Navigational_aid"/>
    <rdfs:subClassOf>
      <owl:Restriction>
        <owl:hasValue xml:lang="en">RDRGUD</owl:hasValue>
        <owl:onProperty rdf:resource="jc3iedmBase.owl#electronic-equipment-type-subcategory-code"/>
      </owl:Restriction>
    </rdfs:subClassOf>
    <rdfs:label xml:lang="en">Radar, guidance</rdfs:label>
    <rdfs:comment xml:lang="en">A radar that provides information used to guide an object such as a missile to a target.</rdfs:comment>
    <rdfs:subClassOf>
      <owl:Restriction>
        <owl:hasValue xml:lang="en">RDRGUD</owl:hasValue>
        <owl:onProperty rdf:resource="jc3iedmBase.owl#electronic-equipment-type-subcategory-code"/>
      </owl:Restriction>
    </rdfs:subClassOf>
  </owl:Class>
  <owl:Class rdf:ID="UN_Dangerous_Goods_NUM_2323">
    <rdfs:subClassOf>
      <owl:Restriction>
        <owl:hasValue xml:lang="en">2323</owl:hasValue>
        <owl:onProperty rdf:resource="jc3iedmBase.owl#consumable-materiel-type-united-nations-number-code"/>
      </owl:Restriction>
    </rdfs:subClassOf>
    <rdfs:label xml:lang="en">UN Dangerous Goods # 2323</rdfs:label>
    <rdfs:comment xml:lang="en">Triethyl phosphate. Includes the agent(s): triethyl phosphite.</rdfs:comment>
    <rdfs:subClassOf>
      <owl:Restriction>
        <owl:hasValue xml:lang="en">2323</owl:hasValue>
        <owl:onProperty rdf:resource="jc3iedmBase.owl#consumable-materiel-type-united-nations-number-code"/>
      </owl:Restriction>
    </rdfs:subClassOf>
  </owl:Class>
  <owl:Class rdf:ID="Ice_cliff">
    <rdfs:subClassOf rdf:resource="jc3iedmSubOnt.owl#GEOGRAPHIC-FEATURE-TYPE-Snow/ice"/>
    <rdfs:subClassOf rdf:resource="jc3iedmSubOnt.owl#GEOGRAPHIC-FEATURE-Solid_surface"/>
    <rdfs:subClassOf>
      <owl:Restriction>
        <owl:hasValue xml:lang="en">ICECLF</owl:hasValue>
        <owl:onProperty rdf:resource="jc3iedmBase.owl#geographic-feature-type-subcategory-code"/>
      </owl:Restriction>
    </rdfs:subClassOf>
    <rdfs:label xml:lang="en">Ice cliff</rdfs:label>
    <rdfs:comment xml:lang="en">The vertical face of a glacier or ice shelf.</rdfs:comment>
    <rdfs:subClassOf>
      <owl:Restriction>
        <owl:hasValue xml:lang="en">ICECLF</owl:hasValue>
        <owl:onProperty rdf:resource="jc3iedmBase.owl#geographic-feature-type-subcategory-code"/>
      </owl:Restriction>
    </rdfs:subClassOf>
  </owl:Class>
  <owl:Class rdf:about="#Coarse,_anti-sweep">
    <rdfs:subClassOf rdf:resource="jc3iedmSubOnt.owl#AMMUNITION-TYPE-Mine,_moored"/>
    <rdfs:subClassOf rdf:resource="jc3iedmSubOnt.owl#AMMUNITION-TYPE-Mine,_maritime,_moving"/>
    <rdfs:subClassOf rdf:resource="jc3iedmSubOnt.owl#AMMUNITION-TYPE-Mine,_not_known"/>
    <rdfs:subClassOf rdf:resource="jc3iedmSubOnt.owl#AMMUNITION-TYPE-Moving_mine,_sea"/>
    <rdfs:subClassOf rdf:resource="jc3iedmSubOnt.owl#AMMUNITION-TYPE-Mine,_seabed_-_explosive_charge_500kg_or_greater"/>
    <rdfs:subClassOf rdf:resource="jc3iedmSubOnt.owl#AMMUNITION-TYPE-Seabed_mine"/>
    <rdfs:subClassOf rdf:resource="jc3iedmSubOnt.owl#AMMUNITION-TYPE-Mine,_not_otherwise_specified"/>
    <rdfs:comment xml:lang="en">A (maritime) mine firing mechanism fitted that is regarded as coarse firing.</rdfs:comment>
    <rdfs:subClassOf rdf:resource="jc3iedmSubOnt.owl#AMMUNITION-TYPE-Mine,_deep_moored"/>
    <rdfs:subClassOf rdf:resource="jc3iedmSubOnt.owl#AMMUNITION-TYPE-Sea_mine"/>
    <rdfs:subClassOf rdf:resource="jc3iedmSubOnt.owl#AMMUNITION-TYPE-Mine,_shallow_moored"/>
    <rdfs:subClassOf>
      <owl:Restriction>
        <owl:hasValue xml:lang="en">COARAS</owl:hasValue>
        <owl:onProperty rdf:resource="jc3iedmBase.owl#ammunition-type-mine-maritime-firing-code"/>
      </owl:Restriction>
    </rdfs:subClassOf>
    <rdfs:label xml:lang="en">Coarse, anti-sweep</rdfs:label>
    <rdfs:subClassOf>
      <owl:Restriction>
        <owl:hasValue xml:lang="en">COARAS</owl:hasValue>
        <owl:onProperty rdf:resource="jc3iedmBase.owl#ammunition-type-mine-maritime-firing-code"/>
      </owl:Restriction>
    </rdfs:subClassOf>
    <rdfs:subClassOf rdf:resource="jc3iedmSubOnt.owl#AMMUNITION-TYPE-Mine,_seabed_-_explosive_charge_less_than_500kg"/>
  </owl:Class>
  <owl:Class rdf:ID="Mural">
    <rdfs:subClassOf rdf:resource="jc3iedmSubOnt.owl#CONSUMABLE-MATERIEL-TYPE-General_supplies"/>
    <rdfs:subClassOf>
      <owl:Restriction>
        <owl:hasValue xml:lang="en">MURAL</owl:hasValue>
        <owl:onProperty rdf:resource="jc3iedmBase.owl#consumable-materiel-type-subcategory-code"/>
      </owl:Restriction>
    </rdfs:subClassOf>
    <rdfs:label xml:lang="en">Mural</rdfs:label>
    <rdfs:comment xml:lang="en">A painting executed on a wall or ceiling as part of a scheme or decoration.</rdfs:comment>
  </owl:Class>
  <owl:Class rdf:about="#Radar,_side-looking">
    <rdfs:subClassOf rdf:resource="jc3iedmSubOnt.owl#ELECTRONIC-EQUIPMENT-TYPE-Radar"/>
    <rdfs:subClassOf>
      <owl:Restriction>
        <owl:hasValue xml:lang="en">RDRSLR</owl:hasValue>
        <owl:onProperty rdf:resource="jc3iedmBase.owl#electronic-equipment-type-subcategory-code"/>
      </owl:Restriction>
    </rdfs:subClassOf>
    <rdfs:label xml:lang="en">Radar, side-looking</rdfs:label>
    <rdfs:comment xml:lang="en">A radar, viewing at right angles to the axis of the vehicle, which produces a presentation of terrain or moving targets.</rdfs:comment>
  </owl:Class>
  <owl:Class rdf:about="#Sweep,_acoustic_AF">
    <rdfs:subClassOf rdf:resource="jc3iedmSubOnt.owl#MARITIME-EQUIPMENT-TYPE-Sweep"/>
    <rdfs:subClassOf>
      <owl:Restriction>
        <owl:hasValue xml:lang="en">SWPAAF</owl:hasValue>
        <owl:onProperty rdf:resource="jc3iedmBase.owl#maritime-equipment-type-subcategory-code"/>
      </owl:Restriction>
    </rdfs:subClassOf>
    <rdfs:label xml:lang="en">Sweep, acoustic AF</rdfs:label>
    <rdfs:comment xml:lang="en">Equipment designed to locate mines by use of a sweep designed to operate the acoustic firing system of a mine, audio frequency.</rdfs:comment>
  </owl:Class>
  <owl:Class rdf:ID="Rifle">
    <rdfs:subClassOf rdf:resource="jc3iedmSubOnt.owl#WEAPON-TYPE-Small_arms"/>
    <rdfs:subClassOf>
      <owl:Restriction>
        <owl:hasValue xml:lang="en">RIFLE</owl:hasValue>
        <owl:onProperty rdf:resource="jc3iedmBase.owl#weapon-type-subcategory-code"/>
      </owl:Restriction>
    </rdfs:subClassOf>
    <rdfs:label xml:lang="en">Rifle</rdfs:label>
    <rdfs:comment xml:lang="en">A firearm that has a rifled bore designed to be fired from the shoulder.</rdfs:comment>
  </owl:Class>
  <owl:Class rdf:ID="Surface-to-air_missile_launcher">
    <rdfs:subClassOf rdf:resource="jc3iedmSubOnt.owl#WEAPON-TYPE-Missile_system"/>
    <rdfs:subClassOf>
      <owl:Restriction>
        <owl:hasValue xml:lang="en">SAMISL</owl:hasValue>
        <owl:onProperty rdf:resource="jc3iedmBase.owl#weapon-type-subcategory-code"/>
      </owl:Restriction>
    </rdfs:subClassOf>
    <rdfs:label xml:lang="en">Surface-to-air missile launcher</rdfs:label>
    <rdfs:comment xml:lang="en">A structural device designed to support and hold a surface to air missile in position for firing.</rdfs:comment>
  </owl:Class>
  <owl:Class rdf:ID="Telephone_switch">
    <rdfs:subClassOf rdf:resource="jc3iedmSubOnt.owl#ELECTRONIC-EQUIPMENT-TYPE-Communication"/>
    <rdfs:subClassOf>
      <owl:Restriction>
        <owl:hasValue xml:lang="en">TELSWT</owl:hasValue>
        <owl:onProperty rdf:resource="jc3iedmBase.owl#electronic-equipment-type-subcategory-code"/>
      </owl:Restriction>
    </rdfs:subClassOf>
    <rdfs:label xml:lang="en">Telephone switch</rdfs:label>
    <rdfs:comment xml:lang="en">A device for making and breaking the connections in a telephone system.</rdfs:comment>
  </owl:Class>
  <owl:Class rdf:about="#Jungle,_cultivation">
    <rdfs:label xml:lang="en">Jungle, cultivation</rdfs:label>
    <rdfs:comment xml:lang="en">Areas which include areas such as rice paddies which will tend to be open, flat, dirty and swampy to areas such as rubber plantations which offer similar characteristics to primary jungle except for the fact that the trees will be in straight lines.</rdfs:comment>
  </owl:Class>
  <owl:Class rdf:about="#Grenade_launcher,_medium">
    <rdfs:subClassOf rdf:resource="jc3iedmSubOnt.owl#WEAPON-TYPE-Small_arms"/>
    <rdfs:subClassOf rdf:resource="jc3iedmSubOnt.owl#WEAPON-TYPE-Anti-tank"/>
    <rdfs:subClassOf>
      <owl:Restriction>
        <owl:hasValue xml:lang="en">GRLNMD</owl:hasValue>
        <owl:onProperty rdf:resource="jc3iedmBase.owl#weapon-type-subcategory-code"/>
      </owl:Restriction>
    </rdfs:subClassOf>
    <rdfs:label xml:lang="en">Grenade launcher, medium</rdfs:label>
    <rdfs:comment xml:lang="en">A medium structural device designed to support and hold a grenade in position for firing.</rdfs:comment>
    <rdfs:subClassOf>
      <owl:Restriction>
        <owl:hasValue xml:lang="en">GRLNMD</owl:hasValue>
        <owl:onProperty rdf:resource="jc3iedmBase.owl#weapon-type-subcategory-code"/>
      </owl:Restriction>
    </rdfs:subClassOf>
  </owl:Class>
  <owl:Class rdf:ID="Multi-channel_JEZEBEL_relay">
    <rdfs:subClassOf rdf:resource="jc3iedmSubOnt.owl#MARITIME-EQUIPMENT-TYPE-Buoy"/>
    <rdfs:subClassOf>
      <owl:Restriction>
        <owl:hasValue xml:lang="en">MCJZBR</owl:hasValue>
        <owl:onProperty rdf:resource="jc3iedmBase.owl#maritime-equipment-type-subcategory-code"/>
      </owl:Restriction>
    </rdfs:subClassOf>
    <rdfs:label xml:lang="en">Multi-channel JEZEBEL relay</rdfs:label>
    <rdfs:comment xml:lang="en">A relaying air dropped sonobuoy with 4-64 channels.</rdfs:comment>
  </owl:Class>
  <owl:Class rdf:ID="UN_Dangerous_Goods_NUM_1053">
    <rdfs:subClassOf>
      <owl:Restriction>
        <owl:hasValue xml:lang="en">1053</owl:hasValue>
        <owl:onProperty rdf:resource="jc3iedmBase.owl#consumable-materiel-type-united-nations-number-code"/>
      </owl:Restriction>
    </rdfs:subClassOf>
    <rdfs:label xml:lang="en">UN Dangerous Goods # 1053</rdfs:label>
    <rdfs:comment xml:lang="en">Hydrogen sulphide. Includes the agent(s): hydrogen sulphide.</rdfs:comment>
    <rdfs:subClassOf>
      <owl:Restriction>
        <owl:hasValue xml:lang="en">1053</owl:hasValue>
        <owl:onProperty rdf:resource="jc3iedmBase.owl#consumable-materiel-type-united-nations-number-code"/>
      </owl:Restriction>
    </rdfs:subClassOf>
  </owl:Class>
  <owl:Class rdf:about="#Anti-tank_grenade_launcher,_light">
    <rdfs:subClassOf rdf:resource="jc3iedmSubOnt.owl#WEAPON-TYPE-Anti-tank"/>
    <rdfs:subClassOf>
      <owl:Restriction>
        <owl:hasValue xml:lang="en">ATGRLL</owl:hasValue>
        <owl:onProperty rdf:resource="jc3iedmBase.owl#weapon-type-subcategory-code"/>
      </owl:Restriction>
    </rdfs:subClassOf>
    <rdfs:label xml:lang="en">Anti-tank grenade launcher, light</rdfs:label>
    <rdfs:comment xml:lang="en">A light structural device designed to support and hold an anti-tank grenade in position for firing.</rdfs:comment>
  </owl:Class>
  <owl:Class rdf:ID="NATO_standard_fuel_code_F35">
    <rdfs:subClassOf rdf:resource="jc3iedmSubOnt.owl#CONSUMABLE-MATERIEL-TYPE-Fuel"/>
    <rdfs:subClassOf>
      <owl:Restriction>
        <owl:hasValue xml:lang="en">NASF35</owl:hasValue>
        <owl:onProperty rdf:resource="jc3iedmBase.owl#consumable-materiel-type-subcategory-code"/>
      </owl:Restriction>
    </rdfs:subClassOf>
    <rdfs:label xml:lang="en">NATO standard fuel code F35</rdfs:label>
    <rdfs:comment xml:lang="en">Turbine Fuel, Aviation, Kerosene Type.</rdfs:comment>
  </owl:Class>
  <owl:Class rdf:ID="Reef">
    <rdfs:subClassOf rdf:resource="jc3iedmSubOnt.owl#GEOGRAPHIC-FEATURE-Solid_surface"/>
    <rdfs:subClassOf rdf:resource="jc3iedmSubOnt.owl#GEOGRAPHIC-FEATURE-TYPE-Landform"/>
    <rdfs:subClassOf>
      <owl:Restriction>
        <owl:hasValue xml:lang="en">REEF</owl:hasValue>
        <owl:onProperty rdf:resource="jc3iedmBase.owl#geographic-feature-type-subcategory-code"/>
      </owl:Restriction>
    </rdfs:subClassOf>
    <rdfs:label xml:lang="en">Reef</rdfs:label>
    <rdfs:comment xml:lang="en">A rocky or coral elevation at or near enough to the surface of the sea to be a danger to surface navigation.</rdfs:comment>
    <rdfs:subClassOf>
      <owl:Restriction>
        <owl:hasValue xml:lang="en">REEF</owl:hasValue>
        <owl:onProperty rdf:resource="jc3iedmBase.owl#geographic-feature-type-subcategory-code"/>
      </owl:Restriction>
    </rdfs:subClassOf>
  </owl:Class>
  <owl:Class rdf:ID="Island">
    <rdfs:subClassOf rdf:resource="jc3iedmSubOnt.owl#GEOGRAPHIC-FEATURE-Solid_surface"/>
    <rdfs:subClassOf rdf:resource="jc3iedmSubOnt.owl#GEOGRAPHIC-FEATURE-TYPE-Coastal_hydrography"/>
    <rdfs:subClassOf>
      <owl:Restriction>
        <owl:hasValue xml:lang="en">ISLAND</owl:hasValue>
        <owl:onProperty rdf:resource="jc3iedmBase.owl#geographic-feature-type-subcategory-code"/>
      </owl:Restriction>
    </rdfs:subClassOf>
    <rdfs:label xml:lang="en">Island</rdfs:label>
    <rdfs:comment xml:lang="en">A land mass smaller than a continent and surrounded by water.</rdfs:comment>
    <rdfs:subClassOf>
      <owl:Restriction>
        <owl:hasValue xml:lang="en">ISLAND</owl:hasValue>
        <owl:onProperty rdf:resource="jc3iedmBase.owl#geographic-feature-type-subcategory-code"/>
      </owl:Restriction>
    </rdfs:subClassOf>
  </owl:Class>
  <owl:Class rdf:about="#High_frequency_direction_finder,_Outboard">
    <rdfs:subClassOf rdf:resource="jc3iedmSubOnt.owl#ELECTRONIC-EQUIPMENT-TYPE-Electronic_warfare"/>
    <rdfs:subClassOf>
      <owl:Restriction>
        <owl:hasValue xml:lang="en">HFDFOT</owl:hasValue>
        <owl:onProperty rdf:resource="jc3iedmBase.owl#electronic-equipment-type-subcategory-code"/>
      </owl:Restriction>
    </rdfs:subClassOf>
    <rdfs:label xml:lang="en">High frequency direction finder, Outboard</rdfs:label>
    <rdfs:comment xml:lang="en">A direction finder that can detect, locate, and identify targets at long range. OUTBOARD - Organizational Unit Tactical Baseline Operational Area Radio Detection.</rdfs:comment>
  </owl:Class>
  <owl:Class rdf:ID="UN_Dangerous_Goods_NUM_1245">
    <rdfs:subClassOf>
      <owl:Restriction>
        <owl:hasValue xml:lang="en">1245</owl:hasValue>
        <owl:onProperty rdf:resource="jc3iedmBase.owl#consumable-materiel-type-united-nations-number-code"/>
      </owl:Restriction>
    </rdfs:subClassOf>
    <rdfs:label xml:lang="en">UN Dangerous Goods # 1245</rdfs:label>
    <rdfs:comment xml:lang="en">Methyl isobutyl ketone. Includes the agent(s): methyl isobutyl ketone.</rdfs:comment>
    <rdfs:subClassOf>
      <owl:Restriction>
        <owl:hasValue xml:lang="en">1245</owl:hasValue>
        <owl:onProperty rdf:resource="jc3iedmBase.owl#consumable-materiel-type-united-nations-number-code"/>
      </owl:Restriction>
    </rdfs:subClassOf>
  </owl:Class>
  <owl:Class rdf:ID="Link_4">
    <rdfs:subClassOf rdf:resource="jc3iedmSubOnt.owl#NETWORK-SERVICE-Tactical_data_link"/>
    <rdfs:subClassOf>
      <owl:Restriction>
        <owl:hasValue xml:lang="en">LNK4</owl:hasValue>
        <owl:onProperty rdf:resource="jc3iedmBase.owl#network-service-subcategory-code"/>
      </owl:Restriction>
    </rdfs:subClassOf>
    <rdfs:label xml:lang="en">Link 4</rdfs:label>
    <rdfs:comment xml:lang="en">A service that provides the basic elements for the transmission of specific message of Link 4.</rdfs:comment>
  </owl:Class>
  <owl:Class rdf:ID="Methamphetamine">
    <rdfs:subClassOf rdf:resource="jc3iedmSubOnt.owl#CONSUMABLE-MATERIEL-TYPE-Drug"/>
    <rdfs:subClassOf>
      <owl:Restriction>
        <owl:hasValue xml:lang="en">MTHAMP</owl:hasValue>
        <owl:onProperty rdf:resource="jc3iedmBase.owl#consumable-materiel-type-subcategory-code"/>
      </owl:Restriction>
    </rdfs:subClassOf>
    <rdfs:label xml:lang="en">Methamphetamine</rdfs:label>
    <rdfs:comment xml:lang="en">An amphetamine derivative with quicker and longer action, used as a stimulant.</rdfs:comment>
  </owl:Class>
  <owl:Class rdf:about="#Single_rocket_launcher,_heavy">
    <rdfs:subClassOf rdf:resource="jc3iedmSubOnt.owl#WEAPON-TYPE-Rocket_artillery"/>
    <rdfs:subClassOf>
      <owl:Restriction>
        <owl:hasValue xml:lang="en">SRKLHV</owl:hasValue>
        <owl:onProperty rdf:resource="jc3iedmBase.owl#weapon-type-subcategory-code"/>
      </owl:Restriction>
    </rdfs:subClassOf>
    <rdfs:label xml:lang="en">Single rocket launcher, heavy</rdfs:label>
    <rdfs:comment xml:lang="en">A heavy structural device designed to support and hold a rocket in position for firing.</rdfs:comment>
  </owl:Class>
  <owl:Class rdf:ID="UN_Dangerous_Goods_NUM_1830">
    <rdfs:subClassOf>
      <owl:Restriction>
        <owl:hasValue xml:lang="en">1830</owl:hasValue>
        <owl:onProperty rdf:resource="jc3iedmBase.owl#consumable-materiel-type-united-nations-number-code"/>
      </owl:Restriction>
    </rdfs:subClassOf>
    <rdfs:label xml:lang="en">UN Dangerous Goods # 1830</rdfs:label>
    <rdfs:comment xml:lang="en">Sulphuric acid with more than 51% acid. Includes the agent(s): sulphuric acid.</rdfs:comment>
    <rdfs:subClassOf>
      <owl:Restriction>
        <owl:hasValue xml:lang="en">1830</owl:hasValue>
        <owl:onProperty rdf:resource="jc3iedmBase.owl#consumable-materiel-type-united-nations-number-code"/>
      </owl:Restriction>
    </rdfs:subClassOf>
  </owl:Class>
  <owl:Class rdf:ID="Single_rocket_launcher">
    <rdfs:subClassOf rdf:resource="jc3iedmSubOnt.owl#WEAPON-TYPE-Rocket_artillery"/>
    <rdfs:subClassOf>
      <owl:Restriction>
        <owl:hasValue xml:lang="en">SRCLAU</owl:hasValue>
        <owl:onProperty rdf:resource="jc3iedmBase.owl#weapon-type-subcategory-code"/>
      </owl:Restriction>
    </rdfs:subClassOf>
    <rdfs:label xml:lang="en">Single rocket launcher</rdfs:label>
    <rdfs:comment xml:lang="en">A structural device designed to support and hold a rocket in position for firing.</rdfs:comment>
  </owl:Class>
  <owl:Class rdf:about="#Buoy,_marker">
    <rdfs:subClassOf rdf:resource="jc3iedmSubOnt.owl#MARITIME-EQUIPMENT-TYPE-Buoy"/>
    <rdfs:subClassOf>
      <owl:Restriction>
        <owl:hasValue xml:lang="en">BUOYMR</owl:hasValue>
        <owl:onProperty rdf:resource="jc3iedmBase.owl#maritime-equipment-type-subcategory-code"/>
      </owl:Restriction>
    </rdfs:subClassOf>
    <rdfs:label xml:lang="en">Buoy, marker</rdfs:label>
    <rdfs:comment xml:lang="en">A floating object fastened in a particular place to point out the position of a specific hazard or obstacle or act as a marker for some specific purpose.</rdfs:comment>
  </owl:Class>
  <owl:Class rdf:ID="Denied">
    <rdfs:subClassOf>
      <owl:Restriction>
        <owl:hasValue xml:lang="en">DENIED</owl:hasValue>
        <owl:onProperty rdf:resource="jc3iedmBase.owl#materiel-status-operational-status-qualifier-code"/>
      </owl:Restriction>
    </rdfs:subClassOf>
    <rdfs:label xml:lang="en">Denied</rdfs:label>
    <rdfs:comment xml:lang="en">Subjectively judged by the reporting organisation that a MATERIEL is unavailable through means such as removal, contamination or erection of obstructions.</rdfs:comment>
    <rdfs:subClassOf>
      <owl:Restriction>
        <owl:hasValue xml:lang="en">DENIED</owl:hasValue>
        <owl:onProperty rdf:resource="jc3iedmBase.owl#facility-status-operational-status-qualifier-code"/>
      </owl:Restriction>
    </rdfs:subClassOf>
    <rdfs:subClassOf>
      <owl:Restriction>
        <owl:hasValue xml:lang="en">DENIED</owl:hasValue>
        <owl:onProperty rdf:resource="jc3iedmBase.owl#facility-status-operational-status-qualifier-code"/>
      </owl:Restriction>
    </rdfs:subClassOf>
    <rdfs:subClassOf>
      <owl:Restriction>
        <owl:hasValue xml:lang="en">DENIED</owl:hasValue>
        <owl:onProperty rdf:resource="jc3iedmBase.owl#materiel-status-operational-status-qualifier-code"/>
      </owl:Restriction>
    </rdfs:subClassOf>
  </owl:Class>
  <owl:Class rdf:ID="Sound_surveillance_system">
    <rdfs:subClassOf rdf:resource="jc3iedmSubOnt.owl#ELECTRONIC-EQUIPMENT-TYPE-Sensor"/>
    <rdfs:subClassOf>
      <owl:Restriction>
        <owl:hasValue xml:lang="en">SDSVST</owl:hasValue>
        <owl:onProperty rdf:resource="jc3iedmBase.owl#electronic-equipment-type-subcategory-code"/>
      </owl:Restriction>
    </rdfs:subClassOf>
    <rdfs:label xml:lang="en">Sound surveillance system</rdfs:label>
    <rdfs:comment xml:lang="en">High-gain long fixed arrays in deep ocean basins that provide deep-water long-range detection capability using acoustic signals.</rdfs:comment>
  </owl:Class>
  <owl:Class rdf:ID="Beach">
    <rdfs:subClassOf rdf:resource="jc3iedmSubOnt.owl#GEOGRAPHIC-FEATURE-Solid_surface"/>
    <rdfs:subClassOf rdf:resource="jc3iedmSubOnt.owl#GEOGRAPHIC-FEATURE-TYPE-Coastal_hydrography"/>
    <rdfs:subClassOf>
      <owl:Restriction>
        <owl:hasValue xml:lang="en">BEACH</owl:hasValue>
        <owl:onProperty rdf:resource="jc3iedmBase.owl#geographic-feature-type-subcategory-code"/>
      </owl:Restriction>
    </rdfs:subClassOf>
    <rdfs:label xml:lang="en">Beach</rdfs:label>
    <rdfs:comment xml:lang="en">The shore of the sea or lake, sandy or pebbly, brought up by the waves (including the foreshore area).</rdfs:comment>
    <rdfs:subClassOf>
      <owl:Restriction>
        <owl:hasValue xml:lang="en">BEACH</owl:hasValue>
        <owl:onProperty rdf:resource="jc3iedmBase.owl#geographic-feature-type-subcategory-code"/>
      </owl:Restriction>
    </rdfs:subClassOf>
  </owl:Class>
  <owl:Class rdf:about="#Radar,_synthetic_aperture">
    <rdfs:subClassOf rdf:resource="jc3iedmSubOnt.owl#ELECTRONIC-EQUIPMENT-TYPE-Radar"/>
    <rdfs:subClassOf>
      <owl:Restriction>
        <owl:hasValue xml:lang="en">RDSNRS</owl:hasValue>
        <owl:onProperty rdf:resource="jc3iedmBase.owl#electronic-equipment-type-subcategory-code"/>
      </owl:Restriction>
    </rdfs:subClassOf>
    <rdfs:label xml:lang="en">Radar, synthetic aperture</rdfs:label>
    <rdfs:comment xml:lang="en">A high-resolution radar that simulates a large aperture by using a single radiating antenna element installed on a moving platform and transmitting at sequential positions on a line.</rdfs:comment>
  </owl:Class>
  <owl:Class rdf:about="#Scrub/brush/bush">
    <rdfs:label xml:lang="en">Scrub/brush/bush</rdfs:label>
    <rdfs:comment xml:lang="en">A characterisation of an area with low-growing woody plants.</rdfs:comment>
  </owl:Class>
  <owl:Class rdf:ID="Lightly_damaged">
    <rdfs:label xml:lang="en">Lightly damaged</rdfs:label>
    <rdfs:subClassOf>
      <owl:Restriction>
        <owl:hasValue xml:lang="en">LGTDAM</owl:hasValue>
        <owl:onProperty rdf:resource="jc3iedmBase.owl#organisation-status-operational-status-qualifier-code"/>
      </owl:Restriction>
    </rdfs:subClassOf>
    <rdfs:subClassOf>
      <owl:Restriction>
        <owl:hasValue xml:lang="en">LGTDAM</owl:hasValue>
        <owl:onProperty rdf:resource="jc3iedmBase.owl#facility-status-operational-status-qualifier-code"/>
      </owl:Restriction>
    </rdfs:subClassOf>
    <rdfs:subClassOf>
      <owl:Restriction>
        <owl:hasValue xml:lang="en">LGTDAM</owl:hasValue>
        <owl:onProperty rdf:resource="jc3iedmBase.owl#facility-status-operational-status-qualifier-code"/>
      </owl:Restriction>
    </rdfs:subClassOf>
    <rdfs:subClassOf>
      <owl:Restriction>
        <owl:hasValue xml:lang="en">LGTDAM</owl:hasValue>
        <owl:onProperty rdf:resource="jc3iedmBase.owl#organisation-status-operational-status-qualifier-code"/>
      </owl:Restriction>
    </rdfs:subClassOf>
    <rdfs:subClassOf>
      <owl:Restriction>
        <owl:hasValue xml:lang="en">LGTDAM</owl:hasValue>
        <owl:onProperty rdf:resource="jc3iedmBase.owl#materiel-status-operational-status-qualifier-code"/>
      </owl:Restriction>
    </rdfs:subClassOf>
    <rdfs:comment xml:lang="en">Subjectively judged by the reporting organisation to be only lightly damaged.</rdfs:comment>
    <rdfs:subClassOf>
      <owl:Restriction>
        <owl:hasValue xml:lang="en">LGTDAM</owl:hasValue>
        <owl:onProperty rdf:resource="jc3iedmBase.owl#organisation-status-operational-status-qualifier-code"/>
      </owl:Restriction>
    </rdfs:subClassOf>
    <rdfs:subClassOf>
      <owl:Restriction>
        <owl:hasValue xml:lang="en">LGTDAM</owl:hasValue>
        <owl:onProperty rdf:resource="jc3iedmBase.owl#facility-status-operational-status-qualifier-code"/>
      </owl:Restriction>
    </rdfs:subClassOf>
    <rdfs:subClassOf>
      <owl:Restriction>
        <owl:hasValue xml:lang="en">LGTDAM</owl:hasValue>
        <owl:onProperty rdf:resource="jc3iedmBase.owl#materiel-status-operational-status-qualifier-code"/>
      </owl:Restriction>
    </rdfs:subClassOf>
    <rdfs:subClassOf>
      <owl:Restriction>
        <owl:hasValue xml:lang="en">LGTDAM</owl:hasValue>
        <owl:onProperty rdf:resource="jc3iedmBase.owl#materiel-status-operational-status-qualifier-code"/>
      </owl:Restriction>
    </rdfs:subClassOf>
  </owl:Class>
  <owl:Class rdf:ID="Sound_ranging">
    <rdfs:subClassOf rdf:resource="jc3iedmSubOnt.owl#ELECTRONIC-EQUIPMENT-TYPE-Sensor"/>
    <rdfs:subClassOf>
      <owl:Restriction>
        <owl:hasValue xml:lang="en">SDRANG</owl:hasValue>
        <owl:onProperty rdf:resource="jc3iedmBase.owl#electronic-equipment-type-subcategory-code"/>
      </owl:Restriction>
    </rdfs:subClassOf>
    <rdfs:label xml:lang="en">Sound ranging</rdfs:label>
    <rdfs:comment xml:lang="en">A device used for the process of establishing target distance using sound.</rdfs:comment>
  </owl:Class>
  <owl:Class rdf:about="#Wagon,_cattle">
    <rdfs:subClassOf rdf:resource="jc3iedmSubOnt.owl#RAILCAR-TYPE-Rolling_stock"/>
    <rdfs:subClassOf>
      <owl:Restriction>
        <owl:hasValue xml:lang="en">WGNCTL</owl:hasValue>
        <owl:onProperty rdf:resource="jc3iedmBase.owl#railcar-type-subcategory-code"/>
      </owl:Restriction>
    </rdfs:subClassOf>
    <rdfs:label xml:lang="en">Wagon, cattle</rdfs:label>
    <rdfs:comment xml:lang="en">Rolling stock used to move livestock by rail.</rdfs:comment>
  </owl:Class>
  <owl:Class rdf:ID="UN_Dangerous_Goods_NUM_1040">
    <rdfs:subClassOf>
      <owl:Restriction>
        <owl:hasValue xml:lang="en">1040</owl:hasValue>
        <owl:onProperty rdf:resource="jc3iedmBase.owl#consumable-materiel-type-united-nations-number-code"/>
      </owl:Restriction>
    </rdfs:subClassOf>
    <rdfs:label xml:lang="en">UN Dangerous Goods # 1040</rdfs:label>
    <rdfs:comment xml:lang="en">Ethylene oxide, or Ethylene oxide with nitrogen up to a total pressure of 1 mpa (10 bar) at 50 C. Includes the agent(s): ethylene oxide.</rdfs:comment>
    <rdfs:subClassOf>
      <owl:Restriction>
        <owl:hasValue xml:lang="en">1040</owl:hasValue>
        <owl:onProperty rdf:resource="jc3iedmBase.owl#consumable-materiel-type-united-nations-number-code"/>
      </owl:Restriction>
    </rdfs:subClassOf>
  </owl:Class>
  <owl:Class rdf:about="#Bandages/dressings">
    <rdfs:subClassOf rdf:resource="jc3iedmSubOnt.owl#CONSUMABLE-MATERIEL-TYPE-Medical_supply"/>
    <rdfs:subClassOf>
      <owl:Restriction>
        <owl:hasValue xml:lang="en">BNDDR</owl:hasValue>
        <owl:onProperty rdf:resource="jc3iedmBase.owl#consumable-materiel-type-subcategory-code"/>
      </owl:Restriction>
    </rdfs:subClassOf>
    <rdfs:label xml:lang="en">Bandages/dressings</rdfs:label>
    <rdfs:comment xml:lang="en">Medical material applied to cover and protect an injury.</rdfs:comment>
  </owl:Class>
  <owl:Class rdf:ID="Teletype">
    <rdfs:subClassOf rdf:resource="jc3iedmSubOnt.owl#ELECTRONIC-EQUIPMENT-TYPE-Communication"/>
    <rdfs:subClassOf>
      <owl:Restriction>
        <owl:hasValue xml:lang="en">TELTYP</owl:hasValue>
        <owl:onProperty rdf:resource="jc3iedmBase.owl#electronic-equipment-type-subcategory-code"/>
      </owl:Restriction>
    </rdfs:subClassOf>
    <rdfs:label xml:lang="en">Teletype</rdfs:label>
    <rdfs:comment xml:lang="en">A telegraph instrument for transmitting telegraph messages as they are typed on a keyboard and printing incoming ones.</rdfs:comment>
  </owl:Class>
  <owl:Class rdf:ID="JP-5_fuel">
    <rdfs:subClassOf rdf:resource="jc3iedmSubOnt.owl#CONSUMABLE-MATERIEL-TYPE-Fuel"/>
    <rdfs:subClassOf>
      <owl:Restriction>
        <owl:hasValue xml:lang="en">JP5F</owl:hasValue>
        <owl:onProperty rdf:resource="jc3iedmBase.owl#consumable-materiel-type-subcategory-code"/>
      </owl:Restriction>
    </rdfs:subClassOf>
    <rdfs:label xml:lang="en">JP-5 fuel</rdfs:label>
    <rdfs:comment xml:lang="en">Aviation kerosene, high flash point type, for ship borne aircraft. Specification MIL-T-5624, interchangeable with AVCAT/FSII, NATO F-44.</rdfs:comment>
  </owl:Class>
  <owl:Class rdf:ID="Sarin">
    <rdfs:subClassOf rdf:resource="jc3iedmSubOnt.owl#CHEMICAL-MATERIEL-TYPE-G-agent"/>
    <rdfs:subClassOf rdf:resource="jc3iedmSubOnt.owl#CHEMICAL-MATERIEL-TYPE-Nerve_agent"/>
    <rdfs:subClassOf>
      <owl:Restriction>
        <owl:hasValue xml:lang="en">SARIN</owl:hasValue>
        <owl:onProperty rdf:resource="jc3iedmBase.owl#chemical-materiel-type-subcategory-code"/>
      </owl:Restriction>
    </rdfs:subClassOf>
    <rdfs:label xml:lang="en">Sarin</rdfs:label>
    <rdfs:comment xml:lang="en">An organophosphorus nerve gas.</rdfs:comment>
    <rdfs:subClassOf>
      <owl:Restriction>
        <owl:hasValue xml:lang="en">SARIN</owl:hasValue>
        <owl:onProperty rdf:resource="jc3iedmBase.owl#chemical-materiel-type-subcategory-code"/>
      </owl:Restriction>
    </rdfs:subClassOf>
  </owl:Class>
  <owl:Class rdf:ID="IFF_mode_3">
    <rdfs:subClassOf rdf:resource="jc3iedmSubOnt.owl#NETWORK-SERVICE-Identification_friend_or_foe"/>
    <rdfs:subClassOf>
      <owl:Restriction>
        <owl:hasValue xml:lang="en">IFFM3</owl:hasValue>
        <owl:onProperty rdf:resource="jc3iedmBase.owl#network-service-subcategory-code"/>
      </owl:Restriction>
    </rdfs:subClassOf>
    <rdfs:label xml:lang="en">IFF mode 3</rdfs:label>
    <rdfs:comment xml:lang="en">A service that provides the data for IFF mode 3.</rdfs:comment>
  </owl:Class>
  <owl:Class rdf:ID="Handbill">
    <rdfs:subClassOf rdf:resource="jc3iedmSubOnt.owl#CONSUMABLE-MATERIEL-TYPE-General_supplies"/>
    <rdfs:subClassOf>
      <owl:Restriction>
        <owl:hasValue xml:lang="en">HANDBL</owl:hasValue>
        <owl:onProperty rdf:resource="jc3iedmBase.owl#consumable-materiel-type-subcategory-code"/>
      </owl:Restriction>
    </rdfs:subClassOf>
    <rdfs:label xml:lang="en">Handbill</rdfs:label>
    <rdfs:comment xml:lang="en">A printed notice or advertisement on a single page, intended to be delivered or circulated by hand.</rdfs:comment>
  </owl:Class>
  <owl:Class rdf:ID="Anti-aircraft_artillery">
    <rdfs:subClassOf rdf:resource="jc3iedmSubOnt.owl#WEAPON-TYPE-Air-defence"/>
    <rdfs:subClassOf>
      <owl:Restriction>
        <owl:hasValue xml:lang="en">AAARTR</owl:hasValue>
        <owl:onProperty rdf:resource="jc3iedmBase.owl#weapon-type-subcategory-code"/>
      </owl:Restriction>
    </rdfs:subClassOf>
    <rdfs:label xml:lang="en">Anti-aircraft artillery</rdfs:label>
    <rdfs:comment xml:lang="en">An anti-aircraft weapon employed in the air defence role.</rdfs:comment>
  </owl:Class>
  <owl:Class rdf:about="#Radio,_telephone">
    <rdfs:subClassOf rdf:resource="jc3iedmSubOnt.owl#ELECTRONIC-EQUIPMENT-TYPE-Communication"/>
    <rdfs:subClassOf>
      <owl:Restriction>
        <owl:hasValue xml:lang="en">RADTLP</owl:hasValue>
        <owl:onProperty rdf:resource="jc3iedmBase.owl#electronic-equipment-type-subcategory-code"/>
      </owl:Restriction>
    </rdfs:subClassOf>
    <rdfs:label xml:lang="en">Radio, telephone</rdfs:label>
    <rdfs:comment xml:lang="en">Telephone set that may be carried by a person and that uses a radio link with a telepoint base station or a base station of a mobile radio communication cellular system.</rdfs:comment>
  </owl:Class>
  <owl:Class rdf:ID="UN_Dangerous_Goods_NUM_1050">
    <rdfs:subClassOf>
      <owl:Restriction>
        <owl:hasValue xml:lang="en">1050</owl:hasValue>
        <owl:onProperty rdf:resource="jc3iedmBase.owl#consumable-materiel-type-united-nations-number-code"/>
      </owl:Restriction>
    </rdfs:subClassOf>
    <rdfs:label xml:lang="en">UN Dangerous Goods # 1050</rdfs:label>
    <rdfs:comment xml:lang="en">Hydrogen chloride, anhydrous. Includes the agent(s): hydrogen chloride.</rdfs:comment>
    <rdfs:subClassOf>
      <owl:Restriction>
        <owl:hasValue xml:lang="en">1050</owl:hasValue>
        <owl:onProperty rdf:resource="jc3iedmBase.owl#consumable-materiel-type-united-nations-number-code"/>
      </owl:Restriction>
    </rdfs:subClassOf>
  </owl:Class>
  <owl:Class rdf:about="#Water,_fit_for_human_consumption">
    <rdfs:subClassOf rdf:resource="jc3iedmSubOnt.owl#CONSUMABLE-MATERIEL-TYPE-Water"/>
    <rdfs:subClassOf>
      <owl:Restriction>
        <owl:hasValue xml:lang="en">WTRHUM</owl:hasValue>
        <owl:onProperty rdf:resource="jc3iedmBase.owl#consumable-materiel-type-subcategory-code"/>
      </owl:Restriction>
    </rdfs:subClassOf>
    <rdfs:label xml:lang="en">Water, fit for human consumption</rdfs:label>
    <rdfs:comment xml:lang="en">H2O that has been filtered and processed to remove poisons/toxins harmful to humans.</rdfs:comment>
  </owl:Class>
  <owl:Class rdf:about="#Sonobuoy,_active">
    <rdfs:subClassOf rdf:resource="jc3iedmSubOnt.owl#MARITIME-EQUIPMENT-TYPE-Buoy"/>
    <rdfs:subClassOf rdf:resource="jc3iedmSubOnt.owl#MARITIME-EQUIPMENT-TYPE-Sonar,_maritime"/>
    <rdfs:subClassOf>
      <owl:Restriction>
        <owl:hasValue xml:lang="en">SONOAC</owl:hasValue>
        <owl:onProperty rdf:resource="jc3iedmBase.owl#maritime-equipment-type-subcategory-code"/>
      </owl:Restriction>
    </rdfs:subClassOf>
    <rdfs:label xml:lang="en">Sonobuoy, active</rdfs:label>
    <rdfs:comment xml:lang="en">No definition provided in ADatP-3 Baseline 13.1 FFIRN/FUD 1434/1.</rdfs:comment>
    <rdfs:subClassOf>
      <owl:Restriction>
        <owl:hasValue xml:lang="en">SONOAC</owl:hasValue>
        <owl:onProperty rdf:resource="jc3iedmBase.owl#maritime-equipment-type-subcategory-code"/>
      </owl:Restriction>
    </rdfs:subClassOf>
  </owl:Class>
  <owl:Class rdf:ID="Integrated_underwater_surveillance_system">
    <rdfs:subClassOf rdf:resource="jc3iedmSubOnt.owl#ELECTRONIC-EQUIPMENT-TYPE-Sensor"/>
    <rdfs:subClassOf>
      <owl:Restriction>
        <owl:hasValue xml:lang="en">INUWSS</owl:hasValue>
        <owl:onProperty rdf:resource="jc3iedmBase.owl#electronic-equipment-type-subcategory-code"/>
      </owl:Restriction>
    </rdfs:subClassOf>
    <rdfs:label xml:lang="en">Integrated underwater surveillance system</rdfs:label>
    <rdfs:comment xml:lang="en">Fixed, mobile, and deployable acoustic listening arrays that provide a means for submarine detection.</rdfs:comment>
  </owl:Class>
  <owl:Class rdf:about="#Buoy,_datum_dan">
    <rdfs:subClassOf rdf:resource="jc3iedmSubOnt.owl#MARITIME-EQUIPMENT-TYPE-Buoy"/>
    <rdfs:subClassOf>
      <owl:Restriction>
        <owl:hasValue xml:lang="en">BUOYDT</owl:hasValue>
        <owl:onProperty rdf:resource="jc3iedmBase.owl#maritime-equipment-type-subcategory-code"/>
      </owl:Restriction>
    </rdfs:subClassOf>
    <rdfs:label xml:lang="en">Buoy, datum dan</rdfs:label>
    <rdfs:comment xml:lang="en">A dan buoy intended as a geographical reference or check, which needs to be more visible and more securely moored than a normal dan buoy.</rdfs:comment>
  </owl:Class>
  <owl:Class rdf:ID="Paper">
    <rdfs:subClassOf rdf:resource="jc3iedmSubOnt.owl#CONSUMABLE-MATERIEL-TYPE-General_supplies"/>
    <rdfs:subClassOf>
      <owl:Restriction>
        <owl:hasValue xml:lang="en">PAPER</owl:hasValue>
        <owl:onProperty rdf:resource="jc3iedmBase.owl#consumable-materiel-type-subcategory-code"/>
      </owl:Restriction>
    </rdfs:subClassOf>
    <rdfs:label xml:lang="en">Paper</rdfs:label>
    <rdfs:comment xml:lang="en">A substance composed of fibres interlaced into a compact web.</rdfs:comment>
  </owl:Class>
  <owl:Class rdf:about="#Sonobuoy,_command_activated_system">
    <rdfs:subClassOf rdf:resource="jc3iedmSubOnt.owl#MARITIME-EQUIPMENT-TYPE-Buoy"/>
    <rdfs:subClassOf rdf:resource="jc3iedmSubOnt.owl#MARITIME-EQUIPMENT-TYPE-Sonar,_maritime"/>
    <rdfs:subClassOf>
      <owl:Restriction>
        <owl:hasValue xml:lang="en">SONOCA</owl:hasValue>
        <owl:onProperty rdf:resource="jc3iedmBase.owl#maritime-equipment-type-subcategory-code"/>
      </owl:Restriction>
    </rdfs:subClassOf>
    <rdfs:label xml:lang="en">Sonobuoy, command activated system</rdfs:label>
    <rdfs:comment xml:lang="en">No definition provided in ADatP-3 Baseline 13.1 FFIRN/FUD 1434/1.</rdfs:comment>
    <rdfs:subClassOf>
      <owl:Restriction>
        <owl:hasValue xml:lang="en">SONOCA</owl:hasValue>
        <owl:onProperty rdf:resource="jc3iedmBase.owl#maritime-equipment-type-subcategory-code"/>
      </owl:Restriction>
    </rdfs:subClassOf>
  </owl:Class>
  <owl:Class rdf:ID="UN_Dangerous_Goods_NUM_1605">
    <rdfs:subClassOf>
      <owl:Restriction>
        <owl:hasValue xml:lang="en">1605</owl:hasValue>
        <owl:onProperty rdf:resource="jc3iedmBase.owl#consumable-materiel-type-united-nations-number-code"/>
      </owl:Restriction>
    </rdfs:subClassOf>
    <rdfs:label xml:lang="en">UN Dangerous Goods # 1605</rdfs:label>
    <rdfs:comment xml:lang="en">Ethylene dibromide. Includes the agent(s): ethylene dibromide.</rdfs:comment>
    <rdfs:subClassOf>
      <owl:Restriction>
        <owl:hasValue xml:lang="en">1605</owl:hasValue>
        <owl:onProperty rdf:resource="jc3iedmBase.owl#consumable-materiel-type-united-nations-number-code"/>
      </owl:Restriction>
    </rdfs:subClassOf>
  </owl:Class>
  <owl:Class rdf:about="#Boom_and_centreline_drogue,_and_wingtip_drogue">
    <rdfs:subClassOf rdf:resource="jc3iedmSubOnt.owl#MISCELLANEOUS-EQUIPMENT-TYPE-Aircraft_refuelling"/>
    <rdfs:subClassOf>
      <owl:Restriction>
        <owl:hasValue xml:lang="en">BCDW</owl:hasValue>
        <owl:onProperty rdf:resource="jc3iedmBase.owl#miscellaneous-equipment-type-subcategory-code"/>
      </owl:Restriction>
    </rdfs:subClassOf>
    <rdfs:label xml:lang="en">Boom and centreline drogue, and wingtip drogue</rdfs:label>
    <rdfs:comment xml:lang="en">Three components of a refuelling system by which a boom, centreline drogue and wingtip drogue devices can provide fuel on a receiver aircraft.</rdfs:comment>
  </owl:Class>
  <owl:Class rdf:ID="Television">
    <rdfs:subClassOf rdf:resource="jc3iedmSubOnt.owl#ELECTRONIC-EQUIPMENT-TYPE-Communication"/>
    <rdfs:subClassOf>
      <owl:Restriction>
        <owl:hasValue xml:lang="en">TELEVS</owl:hasValue>
        <owl:onProperty rdf:resource="jc3iedmBase.owl#electronic-equipment-type-subcategory-code"/>
      </owl:Restriction>
    </rdfs:subClassOf>
    <rdfs:label xml:lang="en">Television</rdfs:label>
    <rdfs:comment xml:lang="en">A device for the transmission of signals representing scenes, images of the scenes being reproduced on a screen as they are received.</rdfs:comment>
  </owl:Class>
  <owl:Class rdf:about="#Rifle,_carbine">
    <rdfs:subClassOf rdf:resource="jc3iedmSubOnt.owl#WEAPON-TYPE-Small_arms"/>
    <rdfs:subClassOf>
      <owl:Restriction>
        <owl:hasValue xml:lang="en">RFLCRB</owl:hasValue>
        <owl:onProperty rdf:resource="jc3iedmBase.owl#weapon-type-subcategory-code"/>
      </owl:Restriction>
    </rdfs:subClassOf>
    <rdfs:label xml:lang="en">Rifle, carbine</rdfs:label>
    <rdfs:comment xml:lang="en">A short firearm, usually a rifle that has a rifled bore designed to be fired from the shoulder.</rdfs:comment>
  </owl:Class>
  <owl:Class rdf:about="#Anti-tank_rocket_launcher,_medium">
    <rdfs:subClassOf rdf:resource="jc3iedmSubOnt.owl#WEAPON-TYPE-Anti-tank"/>
    <rdfs:subClassOf>
      <owl:Restriction>
        <owl:hasValue xml:lang="en">ATRLMD</owl:hasValue>
        <owl:onProperty rdf:resource="jc3iedmBase.owl#weapon-type-subcategory-code"/>
      </owl:Restriction>
    </rdfs:subClassOf>
    <rdfs:label xml:lang="en">Anti-tank rocket launcher, medium</rdfs:label>
    <rdfs:comment xml:lang="en">A medium structural device designed to support and hold an anti-tank rocket in position for firing.</rdfs:comment>
  </owl:Class>
  <owl:Class rdf:ID="Magazine">
    <rdfs:subClassOf rdf:resource="jc3iedmSubOnt.owl#CONSUMABLE-MATERIEL-TYPE-General_supplies"/>
    <rdfs:subClassOf>
      <owl:Restriction>
        <owl:hasValue xml:lang="en">MAGZNE</owl:hasValue>
        <owl:onProperty rdf:resource="jc3iedmBase.owl#consumable-materiel-type-subcategory-code"/>
      </owl:Restriction>
    </rdfs:subClassOf>
    <rdfs:label xml:lang="en">Magazine</rdfs:label>
    <rdfs:comment xml:lang="en">A periodical publication containing articles by various writers.</rdfs:comment>
  </owl:Class>
  <owl:Class rdf:ID="Infrared_detection_system">
    <rdfs:subClassOf rdf:resource="jc3iedmSubOnt.owl#ELECTRONIC-EQUIPMENT-TYPE-Sensor"/>
    <rdfs:subClassOf rdf:resource="jc3iedmSubOnt.owl#ELECTRONIC-EQUIPMENT-TYPE-Electronic_warfare"/>
    <rdfs:subClassOf>
      <owl:Restriction>
        <owl:hasValue xml:lang="en">INDETS</owl:hasValue>
        <owl:onProperty rdf:resource="jc3iedmBase.owl#electronic-equipment-type-subcategory-code"/>
      </owl:Restriction>
    </rdfs:subClassOf>
    <rdfs:label xml:lang="en">Infrared detection system</rdfs:label>
    <rdfs:comment xml:lang="en">Equipment used to detect signals that fall within the region of the electromagnetic spectrum between the long wavelength extreme of the visible spectrum (about 0.7 micrometers) and the shortest microwaves (about 1 millimetre).</rdfs:comment>
    <rdfs:subClassOf>
      <owl:Restriction>
        <owl:hasValue xml:lang="en">INDETS</owl:hasValue>
        <owl:onProperty rdf:resource="jc3iedmBase.owl#electronic-equipment-type-subcategory-code"/>
      </owl:Restriction>
    </rdfs:subClassOf>
  </owl:Class>
  <owl:Class rdf:ID="Anti-tank_rocket_launcher">
    <rdfs:subClassOf rdf:resource="jc3iedmSubOnt.owl#WEAPON-TYPE-Anti-tank"/>
    <rdfs:subClassOf>
      <owl:Restriction>
        <owl:hasValue xml:lang="en">ATROC</owl:hasValue>
        <owl:onProperty rdf:resource="jc3iedmBase.owl#weapon-type-subcategory-code"/>
      </owl:Restriction>
    </rdfs:subClassOf>
    <rdfs:label xml:lang="en">Anti-tank rocket launcher</rdfs:label>
    <rdfs:comment xml:lang="en">A structural device designed to support and hold an anti-tank rocket in position for firing.</rdfs:comment>
  </owl:Class>
  <owl:Class rdf:ID="Kerosene">
    <rdfs:subClassOf rdf:resource="jc3iedmSubOnt.owl#CONSUMABLE-MATERIEL-TYPE-POL"/>
    <rdfs:subClassOf>
      <owl:Restriction>
        <owl:hasValue xml:lang="en">KEROS</owl:hasValue>
        <owl:onProperty rdf:resource="jc3iedmBase.owl#consumable-materiel-type-subcategory-code"/>
      </owl:Restriction>
    </rdfs:subClassOf>
    <rdfs:label xml:lang="en">Kerosene</rdfs:label>
    <rdfs:comment xml:lang="en">A mixture of liquid hydrocarbons, a commercial product of the distillation of petroleum intended to be used in kerosene based engines.</rdfs:comment>
  </owl:Class>
  <owl:Class rdf:about="#Direct_fire_gun,_light">
    <rdfs:subClassOf rdf:resource="jc3iedmSubOnt.owl#WEAPON-TYPE-Small_arms"/>
    <rdfs:subClassOf>
      <owl:Restriction>
        <owl:hasValue xml:lang="en">DFGNLT</owl:hasValue>
        <owl:onProperty rdf:resource="jc3iedmBase.owl#weapon-type-subcategory-code"/>
      </owl:Restriction>
    </rdfs:subClassOf>
    <rdfs:label xml:lang="en">Direct fire gun, light</rdfs:label>
    <rdfs:comment xml:lang="en">No definition provided in APP-6A.</rdfs:comment>
  </owl:Class>
  <owl:Class rdf:ID="UN_Dangerous_Goods_NUM_1051">
    <rdfs:subClassOf>
      <owl:Restriction>
        <owl:hasValue xml:lang="en">1051</owl:hasValue>
        <owl:onProperty rdf:resource="jc3iedmBase.owl#consumable-materiel-type-united-nations-number-code"/>
      </owl:Restriction>
    </rdfs:subClassOf>
    <rdfs:label xml:lang="en">UN Dangerous Goods # 1051</rdfs:label>
    <rdfs:comment xml:lang="en">Hydrogen cyanide, stabilized containing less than 3% water. Includes the agent(s): hydrogen cyanide.</rdfs:comment>
    <rdfs:subClassOf>
      <owl:Restriction>
        <owl:hasValue xml:lang="en">1051</owl:hasValue>
        <owl:onProperty rdf:resource="jc3iedmBase.owl#consumable-materiel-type-united-nations-number-code"/>
      </owl:Restriction>
    </rdfs:subClassOf>
  </owl:Class>
  <owl:Class rdf:ID="Link_22">
    <rdfs:subClassOf rdf:resource="jc3iedmSubOnt.owl#NETWORK-SERVICE-Tactical_data_link"/>
    <rdfs:subClassOf>
      <owl:Restriction>
        <owl:hasValue xml:lang="en">LNK22</owl:hasValue>
        <owl:onProperty rdf:resource="jc3iedmBase.owl#network-service-subcategory-code"/>
      </owl:Restriction>
    </rdfs:subClassOf>
    <rdfs:label xml:lang="en">Link 22</rdfs:label>
    <rdfs:comment xml:lang="en">A service that provides the basic elements for the transmission of specific message of Link 22.</rdfs:comment>
  </owl:Class>
  <owl:Class rdf:ID="IFF_mode_4">
    <rdfs:subClassOf rdf:resource="jc3iedmSubOnt.owl#NETWORK-SERVICE-Identification_friend_or_foe"/>
    <rdfs:subClassOf>
      <owl:Restriction>
        <owl:hasValue xml:lang="en">IFFM4</owl:hasValue>
        <owl:onProperty rdf:resource="jc3iedmBase.owl#network-service-subcategory-code"/>
      </owl:Restriction>
    </rdfs:subClassOf>
    <rdfs:label xml:lang="en">IFF mode 4</rdfs:label>
    <rdfs:comment xml:lang="en">A service that provides the data for IFF mode 4.</rdfs:comment>
  </owl:Class>
  <owl:Class rdf:ID="UN_Dangerous_Goods_NUM_2204">
    <rdfs:subClassOf>
      <owl:Restriction>
        <owl:hasValue xml:lang="en">2204</owl:hasValue>
        <owl:onProperty rdf:resource="jc3iedmBase.owl#consumable-materiel-type-united-nations-number-code"/>
      </owl:Restriction>
    </rdfs:subClassOf>
    <rdfs:label xml:lang="en">UN Dangerous Goods # 2204</rdfs:label>
    <rdfs:comment xml:lang="en">Carbonyl sulphide. Includes the agent(s): carbonyl sulphide.</rdfs:comment>
    <rdfs:subClassOf>
      <owl:Restriction>
        <owl:hasValue xml:lang="en">2204</owl:hasValue>
        <owl:onProperty rdf:resource="jc3iedmBase.owl#consumable-materiel-type-united-nations-number-code"/>
      </owl:Restriction>
    </rdfs:subClassOf>
  </owl:Class>
  <owl:Class rdf:about="#Radar,_side-looking_airborne">
    <rdfs:subClassOf rdf:resource="jc3iedmSubOnt.owl#ELECTRONIC-EQUIPMENT-TYPE-Radar"/>
    <rdfs:subClassOf>
      <owl:Restriction>
        <owl:hasValue xml:lang="en">RDSLAR</owl:hasValue>
        <owl:onProperty rdf:resource="jc3iedmBase.owl#electronic-equipment-type-subcategory-code"/>
      </owl:Restriction>
    </rdfs:subClassOf>
    <rdfs:label xml:lang="en">Radar, side-looking airborne</rdfs:label>
    <rdfs:comment xml:lang="en">An airborne radar, viewing at right angles to the axis of the vehicle, which produces a presentation of terrain or moving targets.</rdfs:comment>
  </owl:Class>
  <owl:Class rdf:about="#Battle-tank,_light">
    <rdfs:subClassOf rdf:resource="jc3iedmSubOnt.owl#WEAPON-TYPE-Tank"/>
    <rdfs:subClassOf>
      <owl:Restriction>
        <owl:hasValue xml:lang="en">BTNKLI</owl:hasValue>
        <owl:onProperty rdf:resource="jc3iedmBase.owl#weapon-type-subcategory-code"/>
      </owl:Restriction>
    </rdfs:subClassOf>
    <rdfs:label xml:lang="en">Battle-tank, light</rdfs:label>
    <rdfs:comment xml:lang="en">An armoured fighting vehicle of less than 20 metric tons which, as its primary function, is designed to close with the enemy and engage their armour and infantry with direct fire.</rdfs:comment>
  </owl:Class>
  <owl:Class rdf:about="#Transmitter,_microwave">
    <rdfs:subClassOf rdf:resource="jc3iedmSubOnt.owl#ELECTRONIC-EQUIPMENT-TYPE-Communication"/>
    <rdfs:subClassOf>
      <owl:Restriction>
        <owl:hasValue xml:lang="en">TRTMWV</owl:hasValue>
        <owl:onProperty rdf:resource="jc3iedmBase.owl#electronic-equipment-type-subcategory-code"/>
      </owl:Restriction>
    </rdfs:subClassOf>
    <rdfs:label xml:lang="en">Transmitter, microwave</rdfs:label>
    <rdfs:comment xml:lang="en">An apparatus producing microwave frequency energy intended to be radiated by an antenna, normally for the purpose of radio communication.</rdfs:comment>
  </owl:Class>
  <owl:Class rdf:ID="Minehunting_sonar_decoy">
    <rdfs:subClassOf rdf:resource="jc3iedmSubOnt.owl#AMMUNITION-TYPE-Mine,_moored"/>
    <rdfs:subClassOf rdf:resource="jc3iedmSubOnt.owl#AMMUNITION-TYPE-Mine,_seabed_-_explosive_charge_less_than_500kg"/>
    <rdfs:subClassOf rdf:resource="jc3iedmSubOnt.owl#AMMUNITION-TYPE-Sea_mine"/>
    <rdfs:subClassOf rdf:resource="jc3iedmSubOnt.owl#AMMUNITION-TYPE-Mine,_seabed_-_explosive_charge_500kg_or_greater"/>
    <rdfs:subClassOf rdf:resource="jc3iedmSubOnt.owl#AMMUNITION-TYPE-Mine,_maritime,_moving"/>
    <rdfs:subClassOf rdf:resource="jc3iedmSubOnt.owl#AMMUNITION-TYPE-Mine,_shallow_moored"/>
    <rdfs:subClassOf rdf:resource="jc3iedmSubOnt.owl#AMMUNITION-TYPE-Mine,_deep_moored"/>
    <rdfs:subClassOf>
      <owl:Restriction>
        <owl:hasValue xml:lang="en">MINHSD</owl:hasValue>
        <owl:onProperty rdf:resource="jc3iedmBase.owl#ammunition-type-mine-maritime-firing-code"/>
      </owl:Restriction>
    </rdfs:subClassOf>
    <rdfs:subClassOf rdf:resource="jc3iedmSubOnt.owl#AMMUNITION-TYPE-Seabed_mine"/>
    <rdfs:subClassOf rdf:resource="jc3iedmSubOnt.owl#AMMUNITION-TYPE-Moving_mine,_sea"/>
    <rdfs:label xml:lang="en">Minehunting sonar decoy</rdfs:label>
    <rdfs:subClassOf rdf:resource="jc3iedmSubOnt.owl#AMMUNITION-TYPE-Mine,_not_known"/>
    <rdfs:subClassOf>
      <owl:Restriction>
        <owl:hasValue xml:lang="en">MINHSD</owl:hasValue>
        <owl:onProperty rdf:resource="jc3iedmBase.owl#ammunition-type-mine-maritime-firing-code"/>
      </owl:Restriction>
    </rdfs:subClassOf>
    <rdfs:subClassOf rdf:resource="jc3iedmSubOnt.owl#AMMUNITION-TYPE-Mine,_not_otherwise_specified"/>
    <rdfs:comment xml:lang="en">A small object with a large sonar signal, or inert minelike objects, Non-mine Bottom Objects (NOMBOs).</rdfs:comment>
  </owl:Class>
  <owl:Class rdf:about="#Multiple_rocket_launcher,_heavy">
    <rdfs:subClassOf rdf:resource="jc3iedmSubOnt.owl#WEAPON-TYPE-Rocket_artillery"/>
    <rdfs:subClassOf>
      <owl:Restriction>
        <owl:hasValue xml:lang="en">MLRSHV</owl:hasValue>
        <owl:onProperty rdf:resource="jc3iedmBase.owl#weapon-type-subcategory-code"/>
      </owl:Restriction>
    </rdfs:subClassOf>
    <rdfs:label xml:lang="en">Multiple rocket launcher, heavy</rdfs:label>
    <rdfs:comment xml:lang="en">A heavy structural device designed to support and hold multiple rockets in position for firing.</rdfs:comment>
  </owl:Class>
  <owl:Class rdf:about="#Wagon,_potable_water">
    <rdfs:subClassOf rdf:resource="jc3iedmSubOnt.owl#RAILCAR-TYPE-Rolling_stock"/>
    <rdfs:subClassOf>
      <owl:Restriction>
        <owl:hasValue xml:lang="en">WGNWAT</owl:hasValue>
        <owl:onProperty rdf:resource="jc3iedmBase.owl#railcar-type-subcategory-code"/>
      </owl:Restriction>
    </rdfs:subClassOf>
    <rdfs:label xml:lang="en">Wagon, potable water</rdfs:label>
    <rdfs:comment xml:lang="en">Rolling stock used to move potable water by rail.</rdfs:comment>
  </owl:Class>
  <owl:Class rdf:about="#Spray_(tank)">
    <rdfs:subClassOf rdf:resource="jc3iedmSubOnt.owl#CONSUMABLE-MATERIEL-TYPE-General_supplies"/>
    <rdfs:subClassOf>
      <owl:Restriction>
        <owl:hasValue xml:lang="en">SPRAY</owl:hasValue>
        <owl:onProperty rdf:resource="jc3iedmBase.owl#consumable-materiel-type-subcategory-code"/>
      </owl:Restriction>
    </rdfs:subClassOf>
    <rdfs:label xml:lang="en">Spray (tank)</rdfs:label>
    <rdfs:comment xml:lang="en">A container used to dispense chemical or biological agents.</rdfs:comment>
  </owl:Class>
  <owl:Class rdf:ID="Book">
    <rdfs:subClassOf rdf:resource="jc3iedmSubOnt.owl#CONSUMABLE-MATERIEL-TYPE-General_supplies"/>
    <rdfs:subClassOf>
      <owl:Restriction>
        <owl:hasValue xml:lang="en">BOOK</owl:hasValue>
        <owl:onProperty rdf:resource="jc3iedmBase.owl#consumable-materiel-type-subcategory-code"/>
      </owl:Restriction>
    </rdfs:subClassOf>
    <rdfs:label xml:lang="en">Book</rdfs:label>
    <rdfs:comment xml:lang="en">A literary composition such as would occupy one or more volumes, without regard to the material form or forms in which it actually exists.</rdfs:comment>
  </owl:Class>
  <owl:Class rdf:about="#Radar,_fire-control">
    <rdfs:subClassOf rdf:resource="jc3iedmSubOnt.owl#ELECTRONIC-EQUIPMENT-TYPE-Radar"/>
    <rdfs:subClassOf rdf:resource="jc3iedmSubOnt.owl#ELECTRONIC-EQUIPMENT-TYPE-Fire_control"/>
    <rdfs:subClassOf>
      <owl:Restriction>
        <owl:hasValue xml:lang="en">RDRFC</owl:hasValue>
        <owl:onProperty rdf:resource="jc3iedmBase.owl#electronic-equipment-type-subcategory-code"/>
      </owl:Restriction>
    </rdfs:subClassOf>
    <rdfs:label xml:lang="en">Radar, fire-control</rdfs:label>
    <rdfs:comment xml:lang="en">Radar used to provide target information inputs to a weapon fire control system.</rdfs:comment>
    <rdfs:subClassOf>
      <owl:Restriction>
        <owl:hasValue xml:lang="en">RDRFC</owl:hasValue>
        <owl:onProperty rdf:resource="jc3iedmBase.owl#electronic-equipment-type-subcategory-code"/>
      </owl:Restriction>
    </rdfs:subClassOf>
  </owl:Class>
  <owl:Class rdf:about="#Radar,_over-the-horizon">
    <rdfs:subClassOf rdf:resource="jc3iedmSubOnt.owl#ELECTRONIC-EQUIPMENT-TYPE-Radar"/>
    <rdfs:subClassOf rdf:resource="jc3iedmSubOnt.owl#ELECTRONIC-EQUIPMENT-TYPE-Navigational_aid"/>
    <rdfs:subClassOf>
      <owl:Restriction>
        <owl:hasValue xml:lang="en">RDOTHR</owl:hasValue>
        <owl:onProperty rdf:resource="jc3iedmBase.owl#electronic-equipment-type-subcategory-code"/>
      </owl:Restriction>
    </rdfs:subClassOf>
    <rdfs:label xml:lang="en">Radar, over-the-horizon</rdfs:label>
    <rdfs:comment xml:lang="en">A radar system that makes use of the atmospheric reflection and refraction phenomena to extend its range of detection beyond line of sight.</rdfs:comment>
    <rdfs:subClassOf>
      <owl:Restriction>
        <owl:hasValue xml:lang="en">RDOTHR</owl:hasValue>
        <owl:onProperty rdf:resource="jc3iedmBase.owl#electronic-equipment-type-subcategory-code"/>
      </owl:Restriction>
    </rdfs:subClassOf>
  </owl:Class>
  <owl:Class rdf:about="#Embankment/fill">
    <rdfs:subClassOf rdf:resource="jc3iedmSubOnt.owl#GEOGRAPHIC-FEATURE-Solid_surface"/>
    <rdfs:subClassOf rdf:resource="jc3iedmSubOnt.owl#GEOGRAPHIC-FEATURE-TYPE-Landform"/>
    <rdfs:subClassOf>
      <owl:Restriction>
        <owl:hasValue xml:lang="en">EMBANK</owl:hasValue>
        <owl:onProperty rdf:resource="jc3iedmBase.owl#geographic-feature-type-subcategory-code"/>
      </owl:Restriction>
    </rdfs:subClassOf>
    <rdfs:label xml:lang="en">Embankment/fill</rdfs:label>
    <rdfs:comment xml:lang="en">A raised long mound of earth or other material.</rdfs:comment>
    <rdfs:subClassOf>
      <owl:Restriction>
        <owl:hasValue xml:lang="en">EMBANK</owl:hasValue>
        <owl:onProperty rdf:resource="jc3iedmBase.owl#geographic-feature-type-subcategory-code"/>
      </owl:Restriction>
    </rdfs:subClassOf>
  </owl:Class>
  <owl:Class rdf:ID="Salt_pan">
    <rdfs:subClassOf rdf:resource="jc3iedmSubOnt.owl#GEOGRAPHIC-FEATURE-TYPE-Inland_water"/>
    <rdfs:subClassOf rdf:resource="jc3iedmSubOnt.owl#GEOGRAPHIC-FEATURE-Solid_surface"/>
    <rdfs:subClassOf>
      <owl:Restriction>
        <owl:hasValue xml:lang="en">SLTPAN</owl:hasValue>
        <owl:onProperty rdf:resource="jc3iedmBase.owl#geographic-feature-type-subcategory-code"/>
      </owl:Restriction>
    </rdfs:subClassOf>
    <rdfs:label xml:lang="en">Salt pan</rdfs:label>
    <rdfs:comment xml:lang="en">A flat area of natural surface salt deposits.</rdfs:comment>
    <rdfs:subClassOf>
      <owl:Restriction>
        <owl:hasValue xml:lang="en">SLTPAN</owl:hasValue>
        <owl:onProperty rdf:resource="jc3iedmBase.owl#geographic-feature-type-subcategory-code"/>
      </owl:Restriction>
    </rdfs:subClassOf>
  </owl:Class>
  <owl:Class rdf:ID="Rickettsiae">
    <rdfs:subClassOf rdf:resource="jc3iedmSubOnt.owl#BIOLOGICAL-MATERIEL-TYPE-Bacterial"/>
    <rdfs:subClassOf>
      <owl:Restriction>
        <owl:hasValue xml:lang="en">RCKETS</owl:hasValue>
        <owl:onProperty rdf:resource="jc3iedmBase.owl#biological-materiel-type-subcategory-code"/>
      </owl:Restriction>
    </rdfs:subClassOf>
    <rdfs:label xml:lang="en">Rickettsiae</rdfs:label>
    <rdfs:comment xml:lang="en">Any of a group of very small bacteria that cause typhus and other febrile diseases.</rdfs:comment>
  </owl:Class>
  <owl:Class rdf:ID="UN_Dangerous_Goods_NUM_1268">
    <rdfs:subClassOf>
      <owl:Restriction>
        <owl:hasValue xml:lang="en">1268</owl:hasValue>
        <owl:onProperty rdf:resource="jc3iedmBase.owl#consumable-materiel-type-united-nations-number-code"/>
      </owl:Restriction>
    </rdfs:subClassOf>
    <rdfs:label xml:lang="en">UN Dangerous Goods # 1268</rdfs:label>
    <rdfs:comment xml:lang="en">Petroleum distillates, N.O.S. or Petroleum products, N.O.S.</rdfs:comment>
    <rdfs:subClassOf>
      <owl:Restriction>
        <owl:hasValue xml:lang="en">1268</owl:hasValue>
        <owl:onProperty rdf:resource="jc3iedmBase.owl#consumable-materiel-type-united-nations-number-code"/>
      </owl:Restriction>
    </rdfs:subClassOf>
  </owl:Class>
  <owl:Class rdf:about="#Tank_gun,_light">
    <rdfs:subClassOf rdf:resource="jc3iedmSubOnt.owl#WEAPON-TYPE-Anti-tank"/>
    <rdfs:subClassOf>
      <owl:Restriction>
        <owl:hasValue xml:lang="en">TKGUNL</owl:hasValue>
        <owl:onProperty rdf:resource="jc3iedmBase.owl#weapon-type-subcategory-code"/>
      </owl:Restriction>
    </rdfs:subClassOf>
    <rdfs:label xml:lang="en">Tank gun, light</rdfs:label>
    <rdfs:comment xml:lang="en">Light, turret mounted, tank gun, calibre under 90 MM, for use in the field against tanks.</rdfs:comment>
  </owl:Class>
  <owl:Class rdf:about="#High_frequency_direction_finder,_Bullseye">
    <rdfs:subClassOf rdf:resource="jc3iedmSubOnt.owl#ELECTRONIC-EQUIPMENT-TYPE-Electronic_warfare"/>
    <rdfs:subClassOf>
      <owl:Restriction>
        <owl:hasValue xml:lang="en">HFDFBL</owl:hasValue>
        <owl:onProperty rdf:resource="jc3iedmBase.owl#electronic-equipment-type-subcategory-code"/>
      </owl:Restriction>
    </rdfs:subClassOf>
    <rdfs:label xml:lang="en">High frequency direction finder, Bullseye</rdfs:label>
    <rdfs:comment xml:lang="en">Equipment that uses a circularly-disposed antenna array, looks similar to a bulls-eye, and can detect, locate and identify targets at long range.</rdfs:comment>
  </owl:Class>
  <owl:Class rdf:ID="Mustard-Lewisite">
    <rdfs:subClassOf rdf:resource="jc3iedmSubOnt.owl#CHEMICAL-MATERIEL-TYPE-Blood_agent"/>
    <rdfs:subClassOf>
      <owl:Restriction>
        <owl:hasValue xml:lang="en">MSTRDL</owl:hasValue>
        <owl:onProperty rdf:resource="jc3iedmBase.owl#chemical-materiel-type-subcategory-code"/>
      </owl:Restriction>
    </rdfs:subClassOf>
    <rdfs:label xml:lang="en">Mustard-Lewisite</rdfs:label>
    <rdfs:comment xml:lang="en">A mixture of distilled mustard and Lewisite.</rdfs:comment>
  </owl:Class>
  <owl:Class rdf:ID="Single_side_band">
    <rdfs:subClassOf rdf:resource="jc3iedmSubOnt.owl#ELECTRONIC-EQUIPMENT-TYPE-Communication"/>
    <rdfs:subClassOf>
      <owl:Restriction>
        <owl:hasValue xml:lang="en">SNGSDE</owl:hasValue>
        <owl:onProperty rdf:resource="jc3iedmBase.owl#electronic-equipment-type-subcategory-code"/>
      </owl:Restriction>
    </rdfs:subClassOf>
    <rdfs:label xml:lang="en">Single side band</rdfs:label>
    <rdfs:comment xml:lang="en">A secure voice communications security systems device.</rdfs:comment>
  </owl:Class>
  <owl:Class rdf:ID="Covered_radio_teletype">
    <rdfs:subClassOf rdf:resource="jc3iedmSubOnt.owl#ELECTRONIC-EQUIPMENT-TYPE-Communication"/>
    <rdfs:subClassOf>
      <owl:Restriction>
        <owl:hasValue xml:lang="en">CVRRAD</owl:hasValue>
        <owl:onProperty rdf:resource="jc3iedmBase.owl#electronic-equipment-type-subcategory-code"/>
      </owl:Restriction>
    </rdfs:subClassOf>
    <rdfs:label xml:lang="en">Covered radio teletype</rdfs:label>
    <rdfs:comment xml:lang="en">A tactical format or encipher relay of messages.</rdfs:comment>
  </owl:Class>
  <owl:Class rdf:ID="Nitrogen_mustard">
    <rdfs:subClassOf rdf:resource="jc3iedmSubOnt.owl#CHEMICAL-MATERIEL-TYPE-Blood_agent"/>
    <rdfs:subClassOf>
      <owl:Restriction>
        <owl:hasValue xml:lang="en">NTRGNM</owl:hasValue>
        <owl:onProperty rdf:resource="jc3iedmBase.owl#chemical-materiel-type-subcategory-code"/>
      </owl:Restriction>
    </rdfs:subClassOf>
    <rdfs:label xml:lang="en">Nitrogen mustard</rdfs:label>
    <rdfs:comment xml:lang="en">A nitrated colourless oily liquid, whose vapour is a powerful irritant and vesicant, used in chemical weapons.</rdfs:comment>
  </owl:Class>
  <owl:Class rdf:ID="Armoured_reconnaissance_vehicle">
    <rdfs:subClassOf>
      <owl:Restriction>
        <owl:hasValue xml:lang="en">ARV</owl:hasValue>
        <owl:onProperty rdf:resource="jc3iedmBase.owl#weapon-type-subcategory-code"/>
      </owl:Restriction>
    </rdfs:subClassOf>
    <rdfs:label xml:lang="en">Armoured reconnaissance vehicle</rdfs:label>
    <rdfs:comment xml:lang="en">A lightly armoured, highly mobile vehicle, serving as the main reconnaissance in infantry and airborne operations.</rdfs:comment>
  </owl:Class>
  <owl:Class rdf:ID="Cut">
    <rdfs:subClassOf rdf:resource="jc3iedmSubOnt.owl#GEOGRAPHIC-FEATURE-Solid_surface"/>
    <rdfs:subClassOf rdf:resource="jc3iedmSubOnt.owl#GEOGRAPHIC-FEATURE-TYPE-Landform"/>
    <rdfs:subClassOf>
      <owl:Restriction>
        <owl:hasValue xml:lang="en">CUT</owl:hasValue>
        <owl:onProperty rdf:resource="jc3iedmBase.owl#geographic-feature-type-subcategory-code"/>
      </owl:Restriction>
    </rdfs:subClassOf>
    <rdfs:label xml:lang="en">Cut</rdfs:label>
    <rdfs:comment xml:lang="en">An excavation of the Earths surface to provide passage for a road, railroad, canal, etc.</rdfs:comment>
    <rdfs:subClassOf>
      <owl:Restriction>
        <owl:hasValue xml:lang="en">CUT</owl:hasValue>
        <owl:onProperty rdf:resource="jc3iedmBase.owl#geographic-feature-type-subcategory-code"/>
      </owl:Restriction>
    </rdfs:subClassOf>
  </owl:Class>
  <owl:Class rdf:about="#Marker,_inner">
    <rdfs:subClassOf rdf:resource="jc3iedmSubOnt.owl#ELECTRONIC-EQUIPMENT-TYPE-Navigational_aid"/>
    <rdfs:subClassOf>
      <owl:Restriction>
        <owl:hasValue xml:lang="en">MRKRIN</owl:hasValue>
        <owl:onProperty rdf:resource="jc3iedmBase.owl#electronic-equipment-type-subcategory-code"/>
      </owl:Restriction>
    </rdfs:subClassOf>
    <rdfs:label xml:lang="en">Marker, inner</rdfs:label>
    <rdfs:comment xml:lang="en">A marker beacon used with an Instrument Landing System Category II precision approach located between the middle marker and the end of the ILS runway that indicates that the pilot is at the designated decision height.</rdfs:comment>
  </owl:Class>
  <owl:Class rdf:ID="Switchboard">
    <rdfs:subClassOf rdf:resource="jc3iedmSubOnt.owl#ELECTRONIC-EQUIPMENT-TYPE-Communication"/>
    <rdfs:subClassOf>
      <owl:Restriction>
        <owl:hasValue xml:lang="en">SWCBRD</owl:hasValue>
        <owl:onProperty rdf:resource="jc3iedmBase.owl#electronic-equipment-type-subcategory-code"/>
      </owl:Restriction>
    </rdfs:subClassOf>
    <rdfs:label xml:lang="en">Switchboard</rdfs:label>
    <rdfs:comment xml:lang="en">A board for frame bearing a set of switches for connecting and disconnecting the various circuits of an electrical system, such as a telegraph or telephone.</rdfs:comment>
  </owl:Class>
  <owl:Class rdf:ID="UN_Dangerous_Goods_NUM_1698">
    <rdfs:subClassOf>
      <owl:Restriction>
        <owl:hasValue xml:lang="en">1698</owl:hasValue>
        <owl:onProperty rdf:resource="jc3iedmBase.owl#consumable-materiel-type-united-nations-number-code"/>
      </owl:Restriction>
    </rdfs:subClassOf>
    <rdfs:label xml:lang="en">UN Dangerous Goods # 1698</rdfs:label>
    <rdfs:comment xml:lang="en">Diphenylamine chloroarsine. Includes the agent(s): adamsite.</rdfs:comment>
    <rdfs:subClassOf>
      <owl:Restriction>
        <owl:hasValue xml:lang="en">1698</owl:hasValue>
        <owl:onProperty rdf:resource="jc3iedmBase.owl#consumable-materiel-type-united-nations-number-code"/>
      </owl:Restriction>
    </rdfs:subClassOf>
  </owl:Class>
  <owl:Class rdf:ID="Fault">
    <rdfs:subClassOf rdf:resource="jc3iedmSubOnt.owl#GEOGRAPHIC-FEATURE-Solid_surface"/>
    <rdfs:subClassOf rdf:resource="jc3iedmSubOnt.owl#GEOGRAPHIC-FEATURE-TYPE-Landform"/>
    <rdfs:subClassOf>
      <owl:Restriction>
        <owl:hasValue xml:lang="en">FAULT</owl:hasValue>
        <owl:onProperty rdf:resource="jc3iedmBase.owl#geographic-feature-type-subcategory-code"/>
      </owl:Restriction>
    </rdfs:subClassOf>
    <rdfs:label xml:lang="en">Fault</rdfs:label>
    <rdfs:comment xml:lang="en">A fracture in the Earths crust with displacement on one side of the fracture relative to the other.</rdfs:comment>
    <rdfs:subClassOf>
      <owl:Restriction>
        <owl:hasValue xml:lang="en">FAULT</owl:hasValue>
        <owl:onProperty rdf:resource="jc3iedmBase.owl#geographic-feature-type-subcategory-code"/>
      </owl:Restriction>
    </rdfs:subClassOf>
  </owl:Class>
  <owl:Class rdf:ID="UN_Dangerous_Goods_NUM_2919">
    <rdfs:subClassOf>
      <owl:Restriction>
        <owl:hasValue xml:lang="en">2919</owl:hasValue>
        <owl:onProperty rdf:resource="jc3iedmBase.owl#consumable-materiel-type-united-nations-number-code"/>
      </owl:Restriction>
    </rdfs:subClassOf>
    <rdfs:label xml:lang="en">UN Dangerous Goods # 2919</rdfs:label>
    <rdfs:comment xml:lang="en">Radioactive material, transported under special arrangement, non fissile or fissile-excepted.</rdfs:comment>
  </owl:Class>
  <owl:Class rdf:ID="Marked">
    <rdfs:subClassOf>
      <owl:Restriction>
        <owl:hasValue xml:lang="en">MARKED</owl:hasValue>
        <owl:onProperty rdf:resource="jc3iedmBase.owl#facility-status-operational-status-qualifier-code"/>
      </owl:Restriction>
    </rdfs:subClassOf>
    <rdfs:label xml:lang="en">Marked</rdfs:label>
    <rdfs:comment xml:lang="en">Subjectively judged by the reporting organisation that a FACILITY has been identified.</rdfs:comment>
    <rdfs:subClassOf>
      <owl:Restriction>
        <owl:hasValue xml:lang="en">MARKED</owl:hasValue>
        <owl:onProperty rdf:resource="jc3iedmBase.owl#facility-status-operational-status-qualifier-code"/>
      </owl:Restriction>
    </rdfs:subClassOf>
    <rdfs:subClassOf>
      <owl:Restriction>
        <owl:hasValue xml:lang="en">MARKED</owl:hasValue>
        <owl:onProperty rdf:resource="jc3iedmBase.owl#facility-status-operational-status-qualifier-code"/>
      </owl:Restriction>
    </rdfs:subClassOf>
    <rdfs:subClassOf>
      <owl:Restriction>
        <owl:hasValue xml:lang="en">MARKED</owl:hasValue>
        <owl:onProperty rdf:resource="jc3iedmBase.owl#facility-status-operational-status-qualifier-code"/>
      </owl:Restriction>
    </rdfs:subClassOf>
    <rdfs:subClassOf>
      <owl:Restriction>
        <owl:hasValue xml:lang="en">MARKED</owl:hasValue>
        <owl:onProperty rdf:resource="jc3iedmBase.owl#facility-status-operational-status-qualifier-code"/>
      </owl:Restriction>
    </rdfs:subClassOf>
  </owl:Class>
  <owl:Class rdf:about="#Sweep,_helicopter_mechanical">
    <rdfs:subClassOf rdf:resource="jc3iedmSubOnt.owl#MARITIME-EQUIPMENT-TYPE-Sweep"/>
    <rdfs:subClassOf>
      <owl:Restriction>
        <owl:hasValue xml:lang="en">SWPHME</owl:hasValue>
        <owl:onProperty rdf:resource="jc3iedmBase.owl#maritime-equipment-type-subcategory-code"/>
      </owl:Restriction>
    </rdfs:subClassOf>
    <rdfs:label xml:lang="en">Sweep, helicopter mechanical</rdfs:label>
    <rdfs:comment xml:lang="en">Equipment mounted on a helicopter designed to locate mines in the lane swept by mechanical means.</rdfs:comment>
  </owl:Class>
  <owl:Class rdf:about="#Ballistic_missile_launcher,_long_range">
    <rdfs:subClassOf rdf:resource="jc3iedmSubOnt.owl#WEAPON-TYPE-Missile_system"/>
    <rdfs:subClassOf>
      <owl:Restriction>
        <owl:hasValue xml:lang="en">BMLLR</owl:hasValue>
        <owl:onProperty rdf:resource="jc3iedmBase.owl#weapon-type-subcategory-code"/>
      </owl:Restriction>
    </rdfs:subClassOf>
    <rdfs:label xml:lang="en">Ballistic missile launcher, long range</rdfs:label>
    <rdfs:comment xml:lang="en">A structural device designed to support and hold a long range ballistic missile in position for firing.</rdfs:comment>
  </owl:Class>
  <owl:Class rdf:ID="Link_1">
    <rdfs:subClassOf rdf:resource="jc3iedmSubOnt.owl#NETWORK-SERVICE-Tactical_data_link"/>
    <rdfs:subClassOf>
      <owl:Restriction>
        <owl:hasValue xml:lang="en">LNK1</owl:hasValue>
        <owl:onProperty rdf:resource="jc3iedmBase.owl#network-service-subcategory-code"/>
      </owl:Restriction>
    </rdfs:subClassOf>
    <rdfs:label xml:lang="en">Link 1</rdfs:label>
    <rdfs:comment xml:lang="en">A service that provides the basic elements for the transmission of specific message of Link 1.</rdfs:comment>
  </owl:Class>
  <owl:Class rdf:ID="NESTOR">
    <rdfs:subClassOf rdf:resource="jc3iedmSubOnt.owl#ELECTRONIC-EQUIPMENT-TYPE-Communication"/>
    <rdfs:subClassOf>
      <owl:Restriction>
        <owl:hasValue xml:lang="en">NESTOR</owl:hasValue>
        <owl:onProperty rdf:resource="jc3iedmBase.owl#electronic-equipment-type-subcategory-code"/>
      </owl:Restriction>
    </rdfs:subClassOf>
    <rdfs:label xml:lang="en">NESTOR</rdfs:label>
    <rdfs:comment xml:lang="en">A secure voice communication security systems device.</rdfs:comment>
  </owl:Class>
  <owl:Class rdf:about="#Radar,_air_defence_tracking">
    <rdfs:subClassOf rdf:resource="jc3iedmSubOnt.owl#ELECTRONIC-EQUIPMENT-TYPE-Radar"/>
    <rdfs:subClassOf>
      <owl:Restriction>
        <owl:hasValue xml:lang="en">RDRADT</owl:hasValue>
        <owl:onProperty rdf:resource="jc3iedmBase.owl#electronic-equipment-type-subcategory-code"/>
      </owl:Restriction>
    </rdfs:subClassOf>
    <rdfs:label xml:lang="en">Radar, air defence tracking</rdfs:label>
    <rdfs:comment xml:lang="en">A radar used specifically in an air-defence tracking mode.</rdfs:comment>
  </owl:Class>
  <owl:Class rdf:ID="Acoustic_audio_frequency">
    <rdfs:subClassOf rdf:resource="jc3iedmSubOnt.owl#AMMUNITION-TYPE-Mine,_moored"/>
    <rdfs:subClassOf rdf:resource="jc3iedmSubOnt.owl#AMMUNITION-TYPE-Mine,_seabed_-_explosive_charge_500kg_or_greater"/>
    <rdfs:subClassOf rdf:resource="jc3iedmSubOnt.owl#AMMUNITION-TYPE-Sea_mine"/>
    <rdfs:subClassOf>
      <owl:Restriction>
        <owl:hasValue xml:lang="en">ACOUAF</owl:hasValue>
        <owl:onProperty rdf:resource="jc3iedmBase.owl#ammunition-type-mine-maritime-firing-code"/>
      </owl:Restriction>
    </rdfs:subClassOf>
    <rdfs:label xml:lang="en">Acoustic audio frequency</rdfs:label>
    <rdfs:subClassOf rdf:resource="jc3iedmSubOnt.owl#AMMUNITION-TYPE-Mine,_not_known"/>
    <rdfs:subClassOf>
      <owl:Restriction>
        <owl:hasValue xml:lang="en">ACOUAF</owl:hasValue>
        <owl:onProperty rdf:resource="jc3iedmBase.owl#ammunition-type-mine-maritime-firing-code"/>
      </owl:Restriction>
    </rdfs:subClassOf>
    <rdfs:subClassOf rdf:resource="jc3iedmSubOnt.owl#AMMUNITION-TYPE-Mine,_deep_moored"/>
    <rdfs:subClassOf rdf:resource="jc3iedmSubOnt.owl#AMMUNITION-TYPE-Moving_mine,_sea"/>
    <rdfs:subClassOf rdf:resource="jc3iedmSubOnt.owl#AMMUNITION-TYPE-Mine,_seabed_-_explosive_charge_less_than_500kg"/>
    <rdfs:comment xml:lang="en">A (maritime) mine firing mechanism with an acoustic audio circuit which responds to the acoustic field of a ship or sweep.</rdfs:comment>
    <rdfs:subClassOf rdf:resource="jc3iedmSubOnt.owl#AMMUNITION-TYPE-Seabed_mine"/>
    <rdfs:subClassOf rdf:resource="jc3iedmSubOnt.owl#AMMUNITION-TYPE-Mine,_shallow_moored"/>
    <rdfs:subClassOf rdf:resource="jc3iedmSubOnt.owl#AMMUNITION-TYPE-Mine,_not_otherwise_specified"/>
    <rdfs:subClassOf rdf:resource="jc3iedmSubOnt.owl#AMMUNITION-TYPE-Mine,_maritime,_moving"/>
  </owl:Class>
  <owl:Class rdf:about="#Ballistic_missile_launcher,_medium_range">
    <rdfs:subClassOf rdf:resource="jc3iedmSubOnt.owl#WEAPON-TYPE-Missile_system"/>
    <rdfs:subClassOf>
      <owl:Restriction>
        <owl:hasValue xml:lang="en">BMLMR</owl:hasValue>
        <owl:onProperty rdf:resource="jc3iedmBase.owl#weapon-type-subcategory-code"/>
      </owl:Restriction>
    </rdfs:subClassOf>
    <rdfs:label xml:lang="en">Ballistic missile launcher, medium range</rdfs:label>
    <rdfs:comment xml:lang="en">A structural device designed to support and hold a medium range ballistic missile in position for firing.</rdfs:comment>
  </owl:Class>
  <owl:Class rdf:ID="UN_Dangerous_Goods_NUM_2909">
    <rdfs:subClassOf>
      <owl:Restriction>
        <owl:hasValue xml:lang="en">2909</owl:hasValue>
        <owl:onProperty rdf:resource="jc3iedmBase.owl#consumable-materiel-type-united-nations-number-code"/>
      </owl:Restriction>
    </rdfs:subClassOf>
    <rdfs:label xml:lang="en">UN Dangerous Goods # 2909</rdfs:label>
    <rdfs:comment xml:lang="en">Radioactive material, excepted package - articles manufactured from natural uranium or depleted uranium or natural thorium.</rdfs:comment>
  </owl:Class>
  <owl:Class rdf:ID="VX">
    <rdfs:subClassOf rdf:resource="jc3iedmSubOnt.owl#CHEMICAL-MATERIEL-TYPE-G-agent"/>
    <rdfs:subClassOf rdf:resource="jc3iedmSubOnt.owl#CHEMICAL-MATERIEL-TYPE-Nerve_agent"/>
    <rdfs:subClassOf rdf:resource="jc3iedmSubOnt.owl#CHEMICAL-MATERIEL-TYPE-V-agent"/>
    <rdfs:subClassOf>
      <owl:Restriction>
        <owl:hasValue xml:lang="en">VX</owl:hasValue>
        <owl:onProperty rdf:resource="jc3iedmBase.owl#chemical-materiel-type-subcategory-code"/>
      </owl:Restriction>
    </rdfs:subClassOf>
    <rdfs:label xml:lang="en">VX</rdfs:label>
    <rdfs:comment xml:lang="en">An organophosphorus nerve gas.</rdfs:comment>
    <rdfs:subClassOf>
      <owl:Restriction>
        <owl:hasValue xml:lang="en">VX</owl:hasValue>
        <owl:onProperty rdf:resource="jc3iedmBase.owl#chemical-materiel-type-subcategory-code"/>
      </owl:Restriction>
    </rdfs:subClassOf>
    <rdfs:subClassOf>
      <owl:Restriction>
        <owl:hasValue xml:lang="en">VX</owl:hasValue>
        <owl:onProperty rdf:resource="jc3iedmBase.owl#chemical-materiel-type-subcategory-code"/>
      </owl:Restriction>
    </rdfs:subClassOf>
  </owl:Class>
  <owl:Class rdf:ID="UN_Dangerous_Goods_NUM_2334">
    <rdfs:subClassOf>
      <owl:Restriction>
        <owl:hasValue xml:lang="en">2334</owl:hasValue>
        <owl:onProperty rdf:resource="jc3iedmBase.owl#consumable-materiel-type-united-nations-number-code"/>
      </owl:Restriction>
    </rdfs:subClassOf>
    <rdfs:label xml:lang="en">UN Dangerous Goods # 2334</rdfs:label>
    <rdfs:comment xml:lang="en">Allylamine. Includes the agent(s): allyl amine.</rdfs:comment>
    <rdfs:subClassOf>
      <owl:Restriction>
        <owl:hasValue xml:lang="en">2334</owl:hasValue>
        <owl:onProperty rdf:resource="jc3iedmBase.owl#consumable-materiel-type-united-nations-number-code"/>
      </owl:Restriction>
    </rdfs:subClassOf>
  </owl:Class>
  <owl:Class rdf:about="#Bluff/cliff/escarpment">
    <rdfs:subClassOf rdf:resource="jc3iedmSubOnt.owl#GEOGRAPHIC-FEATURE-Solid_surface"/>
    <rdfs:subClassOf rdf:resource="jc3iedmSubOnt.owl#GEOGRAPHIC-FEATURE-TYPE-Landform"/>
    <rdfs:subClassOf>
      <owl:Restriction>
        <owl:hasValue xml:lang="en">BLUFF</owl:hasValue>
        <owl:onProperty rdf:resource="jc3iedmBase.owl#geographic-feature-type-subcategory-code"/>
      </owl:Restriction>
    </rdfs:subClassOf>
    <rdfs:label xml:lang="en">Bluff/cliff/escarpment</rdfs:label>
    <rdfs:comment xml:lang="en">A steep, vertical, or overhanging face of rock or earth.</rdfs:comment>
    <rdfs:subClassOf>
      <owl:Restriction>
        <owl:hasValue xml:lang="en">BLUFF</owl:hasValue>
        <owl:onProperty rdf:resource="jc3iedmBase.owl#geographic-feature-type-subcategory-code"/>
      </owl:Restriction>
    </rdfs:subClassOf>
  </owl:Class>
  <owl:Class rdf:ID="Pamphlet">
    <rdfs:subClassOf rdf:resource="jc3iedmSubOnt.owl#CONSUMABLE-MATERIEL-TYPE-General_supplies"/>
    <rdfs:subClassOf>
      <owl:Restriction>
        <owl:hasValue xml:lang="en">PMPHLT</owl:hasValue>
        <owl:onProperty rdf:resource="jc3iedmBase.owl#consumable-materiel-type-subcategory-code"/>
      </owl:Restriction>
    </rdfs:subClassOf>
    <rdfs:label xml:lang="en">Pamphlet</rdfs:label>
    <rdfs:comment xml:lang="en">A small treatise occupying fewer pages than would make a book, issued as a separate work; always unbound, with or without paper covers.</rdfs:comment>
  </owl:Class>
  <owl:Class rdf:ID="Cathode_ray_tube">
    <rdfs:subClassOf rdf:resource="jc3iedmSubOnt.owl#ELECTRONIC-EQUIPMENT-TYPE-Data-processing"/>
    <rdfs:subClassOf rdf:resource="jc3iedmSubOnt.owl#ELECTRONIC-EQUIPMENT-TYPE-Communication"/>
    <rdfs:subClassOf rdf:resource="jc3iedmSubOnt.owl#ELECTRONIC-EQUIPMENT-TYPE-Sensor"/>
    <rdfs:subClassOf>
      <owl:Restriction>
        <owl:hasValue xml:lang="en">CTRYTB</owl:hasValue>
        <owl:onProperty rdf:resource="jc3iedmBase.owl#electronic-equipment-type-subcategory-code"/>
      </owl:Restriction>
    </rdfs:subClassOf>
    <rdfs:label xml:lang="en">Cathode ray tube</rdfs:label>
    <rdfs:comment xml:lang="en">A high-vacuum tube in which cathode rays produce a luminous image on a fluorescent screen.</rdfs:comment>
    <rdfs:subClassOf>
      <owl:Restriction>
        <owl:hasValue xml:lang="en">CTRYTB</owl:hasValue>
        <owl:onProperty rdf:resource="jc3iedmBase.owl#electronic-equipment-type-subcategory-code"/>
      </owl:Restriction>
    </rdfs:subClassOf>
    <rdfs:subClassOf>
      <owl:Restriction>
        <owl:hasValue xml:lang="en">CTRYTB</owl:hasValue>
        <owl:onProperty rdf:resource="jc3iedmBase.owl#electronic-equipment-type-subcategory-code"/>
      </owl:Restriction>
    </rdfs:subClassOf>
  </owl:Class>
  <owl:Class rdf:ID="Sonarbuoy">
    <rdfs:subClassOf rdf:resource="jc3iedmSubOnt.owl#MARITIME-EQUIPMENT-TYPE-Buoy"/>
    <rdfs:subClassOf rdf:resource="jc3iedmSubOnt.owl#MARITIME-EQUIPMENT-TYPE-Sonar,_maritime"/>
    <rdfs:subClassOf>
      <owl:Restriction>
        <owl:hasValue xml:lang="en">SONARB</owl:hasValue>
        <owl:onProperty rdf:resource="jc3iedmBase.owl#maritime-equipment-type-subcategory-code"/>
      </owl:Restriction>
    </rdfs:subClassOf>
    <rdfs:label xml:lang="en">Sonarbuoy</rdfs:label>
    <rdfs:comment xml:lang="en">No definition provided in ADatP-3 BL 11.</rdfs:comment>
    <rdfs:subClassOf>
      <owl:Restriction>
        <owl:hasValue xml:lang="en">SONARB</owl:hasValue>
        <owl:onProperty rdf:resource="jc3iedmBase.owl#maritime-equipment-type-subcategory-code"/>
      </owl:Restriction>
    </rdfs:subClassOf>
  </owl:Class>
  <owl:Class rdf:about="#Magnetic_H,_horizontal_component">
    <rdfs:subClassOf>
      <owl:Restriction>
        <owl:hasValue xml:lang="en">MAGNHH</owl:hasValue>
        <owl:onProperty rdf:resource="jc3iedmBase.owl#ammunition-type-mine-maritime-firing-code"/>
      </owl:Restriction>
    </rdfs:subClassOf>
    <rdfs:label xml:lang="en">Magnetic H, horizontal component</rdfs:label>
    <rdfs:subClassOf rdf:resource="jc3iedmSubOnt.owl#AMMUNITION-TYPE-Mine,_moored"/>
    <rdfs:subClassOf rdf:resource="jc3iedmSubOnt.owl#AMMUNITION-TYPE-Moving_mine,_sea"/>
    <rdfs:comment xml:lang="en">A (maritime) mine firing mechanism with a magnetic influence circuit that responds to the horizontal component of the magnetic field of a ship.</rdfs:comment>
    <rdfs:subClassOf rdf:resource="jc3iedmSubOnt.owl#AMMUNITION-TYPE-Mine,_shallow_moored"/>
    <rdfs:subClassOf rdf:resource="jc3iedmSubOnt.owl#AMMUNITION-TYPE-Mine,_seabed_-_explosive_charge_less_than_500kg"/>
    <rdfs:subClassOf rdf:resource="jc3iedmSubOnt.owl#AMMUNITION-TYPE-Mine,_deep_moored"/>
    <rdfs:subClassOf rdf:resource="jc3iedmSubOnt.owl#AMMUNITION-TYPE-Mine,_seabed_-_explosive_charge_500kg_or_greater"/>
    <rdfs:subClassOf rdf:resource="jc3iedmSubOnt.owl#AMMUNITION-TYPE-Mine,_not_known"/>
    <rdfs:subClassOf rdf:resource="jc3iedmSubOnt.owl#AMMUNITION-TYPE-Mine,_not_otherwise_specified"/>
    <rdfs:subClassOf rdf:resource="jc3iedmSubOnt.owl#AMMUNITION-TYPE-Mine,_maritime,_moving"/>
    <rdfs:subClassOf>
      <owl:Restriction>
        <owl:hasValue xml:lang="en">MAGNHH</owl:hasValue>
        <owl:onProperty rdf:resource="jc3iedmBase.owl#ammunition-type-mine-maritime-firing-code"/>
      </owl:Restriction>
    </rdfs:subClassOf>
    <rdfs:subClassOf rdf:resource="jc3iedmSubOnt.owl#AMMUNITION-TYPE-Seabed_mine"/>
    <rdfs:subClassOf rdf:resource="jc3iedmSubOnt.owl#AMMUNITION-TYPE-Sea_mine"/>
  </owl:Class>
  <owl:Class rdf:ID="UN_Dangerous_Goods_NUM_1560">
    <rdfs:subClassOf>
      <owl:Restriction>
        <owl:hasValue xml:lang="en">1560</owl:hasValue>
        <owl:onProperty rdf:resource="jc3iedmBase.owl#consumable-materiel-type-united-nations-number-code"/>
      </owl:Restriction>
    </rdfs:subClassOf>
    <rdfs:label xml:lang="en">UN Dangerous Goods # 1560</rdfs:label>
    <rdfs:comment xml:lang="en">Arsenic trichloride. Includes the agent(s): arsenic trichloride.</rdfs:comment>
    <rdfs:subClassOf>
      <owl:Restriction>
        <owl:hasValue xml:lang="en">1560</owl:hasValue>
        <owl:onProperty rdf:resource="jc3iedmBase.owl#consumable-materiel-type-united-nations-number-code"/>
      </owl:Restriction>
    </rdfs:subClassOf>
  </owl:Class>
  <owl:Class rdf:about="#Visual_BRG/radar_range">
    <rdfs:subClassOf rdf:resource="jc3iedmSubOnt.owl#ELECTRONIC-EQUIPMENT-TYPE-Navigational_aid"/>
    <rdfs:subClassOf>
      <owl:Restriction>
        <owl:hasValue xml:lang="en">VSLBRG</owl:hasValue>
        <owl:onProperty rdf:resource="jc3iedmBase.owl#electronic-equipment-type-subcategory-code"/>
      </owl:Restriction>
    </rdfs:subClassOf>
    <rdfs:label xml:lang="en">Visual BRG/radar range</rdfs:label>
    <rdfs:comment xml:lang="en">No definition provided in ADatP-3 Baseline 13.1 FFIRN/FUD 1200/1.</rdfs:comment>
  </owl:Class>
  <owl:Class rdf:ID="Visual_storage_device">
    <rdfs:subClassOf rdf:resource="jc3iedmSubOnt.owl#ELECTRONIC-EQUIPMENT-TYPE-Data-processing"/>
    <rdfs:subClassOf rdf:resource="jc3iedmSubOnt.owl#ELECTRONIC-EQUIPMENT-TYPE-Communication"/>
    <rdfs:subClassOf>
      <owl:Restriction>
        <owl:hasValue xml:lang="en">VISSTR</owl:hasValue>
        <owl:onProperty rdf:resource="jc3iedmBase.owl#electronic-equipment-type-subcategory-code"/>
      </owl:Restriction>
    </rdfs:subClassOf>
    <rdfs:label xml:lang="en">Visual storage device</rdfs:label>
    <rdfs:comment xml:lang="en">A device, usually film, tape, Digital Video Device (DVD) or Laser Disk used for the storage of pictures.</rdfs:comment>
    <rdfs:subClassOf>
      <owl:Restriction>
        <owl:hasValue xml:lang="en">VISSTR</owl:hasValue>
        <owl:onProperty rdf:resource="jc3iedmBase.owl#electronic-equipment-type-subcategory-code"/>
      </owl:Restriction>
    </rdfs:subClassOf>
  </owl:Class>
  <owl:Class rdf:ID="C2IS">
    <rdfs:subClassOf rdf:resource="jc3iedmSubOnt.owl#ELECTRONIC-EQUIPMENT-TYPE-C3I"/>
    <rdfs:subClassOf>
      <owl:Restriction>
        <owl:hasValue xml:lang="en">C2IS</owl:hasValue>
        <owl:onProperty rdf:resource="jc3iedmBase.owl#electronic-equipment-type-subcategory-code"/>
      </owl:Restriction>
    </rdfs:subClassOf>
    <rdfs:label xml:lang="en">C2IS</rdfs:label>
    <rdfs:comment xml:lang="en">Equipment specifically designed to use as a command and control information system.</rdfs:comment>
  </owl:Class>
  <owl:Class rdf:ID="Lacking_vital_resources">
    <rdfs:subClassOf>
      <owl:Restriction>
        <owl:hasValue xml:lang="en">LVR</owl:hasValue>
        <owl:onProperty rdf:resource="jc3iedmBase.owl#organisation-status-operational-status-qualifier-code"/>
      </owl:Restriction>
    </rdfs:subClassOf>
    <rdfs:subClassOf>
      <owl:Restriction>
        <owl:hasValue xml:lang="en">LVR</owl:hasValue>
        <owl:onProperty rdf:resource="jc3iedmBase.owl#materiel-status-operational-status-qualifier-code"/>
      </owl:Restriction>
    </rdfs:subClassOf>
    <rdfs:comment xml:lang="en">Subjectively judged by the reporting organisation that a MATERIEL is deficient or lacking of some mission-critical resources (e.g., fuel, ammunition).</rdfs:comment>
    <rdfs:subClassOf>
      <owl:Restriction>
        <owl:hasValue xml:lang="en">LVR</owl:hasValue>
        <owl:onProperty rdf:resource="jc3iedmBase.owl#facility-status-operational-status-qualifier-code"/>
      </owl:Restriction>
    </rdfs:subClassOf>
    <rdfs:subClassOf>
      <owl:Restriction>
        <owl:hasValue xml:lang="en">LVR</owl:hasValue>
        <owl:onProperty rdf:resource="jc3iedmBase.owl#materiel-status-operational-status-qualifier-code"/>
      </owl:Restriction>
    </rdfs:subClassOf>
    <rdfs:label xml:lang="en">Lacking vital resources</rdfs:label>
    <rdfs:subClassOf>
      <owl:Restriction>
        <owl:hasValue xml:lang="en">LVR</owl:hasValue>
        <owl:onProperty rdf:resource="jc3iedmBase.owl#organisation-status-operational-status-qualifier-code"/>
      </owl:Restriction>
    </rdfs:subClassOf>
    <rdfs:subClassOf>
      <owl:Restriction>
        <owl:hasValue xml:lang="en">LVR</owl:hasValue>
        <owl:onProperty rdf:resource="jc3iedmBase.owl#facility-status-operational-status-qualifier-code"/>
      </owl:Restriction>
    </rdfs:subClassOf>
    <rdfs:subClassOf>
      <owl:Restriction>
        <owl:hasValue xml:lang="en">LVR</owl:hasValue>
        <owl:onProperty rdf:resource="jc3iedmBase.owl#organisation-status-operational-status-qualifier-code"/>
      </owl:Restriction>
    </rdfs:subClassOf>
    <rdfs:subClassOf>
      <owl:Restriction>
        <owl:hasValue xml:lang="en">LVR</owl:hasValue>
        <owl:onProperty rdf:resource="jc3iedmBase.owl#facility-status-operational-status-qualifier-code"/>
      </owl:Restriction>
    </rdfs:subClassOf>
    <rdfs:subClassOf>
      <owl:Restriction>
        <owl:hasValue xml:lang="en">LVR</owl:hasValue>
        <owl:onProperty rdf:resource="jc3iedmBase.owl#materiel-status-operational-status-qualifier-code"/>
      </owl:Restriction>
    </rdfs:subClassOf>
  </owl:Class>
  <owl:Class rdf:ID="Blood">
    <rdfs:subClassOf rdf:resource="jc3iedmSubOnt.owl#CONSUMABLE-MATERIEL-TYPE-Medical_supply"/>
    <rdfs:subClassOf>
      <owl:Restriction>
        <owl:hasValue xml:lang="en">BLOOD</owl:hasValue>
        <owl:onProperty rdf:resource="jc3iedmBase.owl#consumable-materiel-type-subcategory-code"/>
      </owl:Restriction>
    </rdfs:subClassOf>
    <rdfs:label xml:lang="en">Blood</rdfs:label>
    <rdfs:comment xml:lang="en">The red liquid circulating in the arteries and veins of man and the higher animals, by which the tissues are constantly nourished and renewed.</rdfs:comment>
  </owl:Class>
  <owl:Class rdf:about="#Radar,_primary">
    <rdfs:subClassOf rdf:resource="jc3iedmSubOnt.owl#ELECTRONIC-EQUIPMENT-TYPE-Radar"/>
    <rdfs:subClassOf rdf:resource="jc3iedmSubOnt.owl#ELECTRONIC-EQUIPMENT-TYPE-Navigational_aid"/>
    <rdfs:subClassOf>
      <owl:Restriction>
        <owl:hasValue xml:lang="en">RDRPRI</owl:hasValue>
        <owl:onProperty rdf:resource="jc3iedmBase.owl#electronic-equipment-type-subcategory-code"/>
      </owl:Restriction>
    </rdfs:subClassOf>
    <rdfs:label xml:lang="en">Radar, primary</rdfs:label>
    <rdfs:comment xml:lang="en">A radar that is designated to be the primary in a particular platform.</rdfs:comment>
    <rdfs:subClassOf>
      <owl:Restriction>
        <owl:hasValue xml:lang="en">RDRPRI</owl:hasValue>
        <owl:onProperty rdf:resource="jc3iedmBase.owl#electronic-equipment-type-subcategory-code"/>
      </owl:Restriction>
    </rdfs:subClassOf>
  </owl:Class>
  <owl:Class rdf:ID="Assault_gun">
    <rdfs:subClassOf rdf:resource="jc3iedmSubOnt.owl#WEAPON-TYPE-Cannon"/>
    <rdfs:subClassOf>
      <owl:Restriction>
        <owl:hasValue xml:lang="en">ASSGUN</owl:hasValue>
        <owl:onProperty rdf:resource="jc3iedmBase.owl#weapon-type-subcategory-code"/>
      </owl:Restriction>
    </rdfs:subClassOf>
    <rdfs:label xml:lang="en">Assault gun</rdfs:label>
    <rdfs:comment xml:lang="en">A cannon, with a relatively long barrel, operating with a relatively low angle of fire, and having a high muzzle velocity.</rdfs:comment>
  </owl:Class>
  <owl:Class rdf:about="#Grenade_launcher,_light">
    <rdfs:subClassOf rdf:resource="jc3iedmSubOnt.owl#WEAPON-TYPE-Small_arms"/>
    <rdfs:subClassOf rdf:resource="jc3iedmSubOnt.owl#WEAPON-TYPE-Anti-tank"/>
    <rdfs:subClassOf>
      <owl:Restriction>
        <owl:hasValue xml:lang="en">GRLNLT</owl:hasValue>
        <owl:onProperty rdf:resource="jc3iedmBase.owl#weapon-type-subcategory-code"/>
      </owl:Restriction>
    </rdfs:subClassOf>
    <rdfs:label xml:lang="en">Grenade launcher, light</rdfs:label>
    <rdfs:comment xml:lang="en">A light structural device designed to support and hold a grenade in position for firing.</rdfs:comment>
    <rdfs:subClassOf>
      <owl:Restriction>
        <owl:hasValue xml:lang="en">GRLNLT</owl:hasValue>
        <owl:onProperty rdf:resource="jc3iedmBase.owl#weapon-type-subcategory-code"/>
      </owl:Restriction>
    </rdfs:subClassOf>
  </owl:Class>
  <owl:Class rdf:about="#Multiple_rocket_launcher,_light">
    <rdfs:subClassOf rdf:resource="jc3iedmSubOnt.owl#WEAPON-TYPE-Rocket_artillery"/>
    <rdfs:subClassOf>
      <owl:Restriction>
        <owl:hasValue xml:lang="en">MLRSLT</owl:hasValue>
        <owl:onProperty rdf:resource="jc3iedmBase.owl#weapon-type-subcategory-code"/>
      </owl:Restriction>
    </rdfs:subClassOf>
    <rdfs:label xml:lang="en">Multiple rocket launcher, light</rdfs:label>
    <rdfs:comment xml:lang="en">A light structural device designed to support and hold multiple rockets in position for firing.</rdfs:comment>
  </owl:Class>
  <owl:Class rdf:about="#Water,_fit_for_medical_use">
    <rdfs:subClassOf rdf:resource="jc3iedmSubOnt.owl#CONSUMABLE-MATERIEL-TYPE-Water"/>
    <rdfs:subClassOf>
      <owl:Restriction>
        <owl:hasValue xml:lang="en">WTRMED</owl:hasValue>
        <owl:onProperty rdf:resource="jc3iedmBase.owl#consumable-materiel-type-subcategory-code"/>
      </owl:Restriction>
    </rdfs:subClassOf>
    <rdfs:label xml:lang="en">Water, fit for medical use</rdfs:label>
    <rdfs:comment xml:lang="en">H2O that has been filtered or processed to remove poisons/toxins harmful to humans and that has also been sterilised to enable it to be used for medical purposes.</rdfs:comment>
  </owl:Class>
  <owl:Class rdf:ID="Anti-aircraft_machine_gun">
    <rdfs:subClassOf rdf:resource="jc3iedmSubOnt.owl#WEAPON-TYPE-Air-defence"/>
    <rdfs:subClassOf>
      <owl:Restriction>
        <owl:hasValue xml:lang="en">AAMGUN</owl:hasValue>
        <owl:onProperty rdf:resource="jc3iedmBase.owl#weapon-type-subcategory-code"/>
      </owl:Restriction>
    </rdfs:subClassOf>
    <rdfs:label xml:lang="en">Anti-aircraft machine gun</rdfs:label>
    <rdfs:comment xml:lang="en">An anti-aircraft gun, normally belt fed, employed in the air defence role.</rdfs:comment>
  </owl:Class>
  <owl:Class rdf:about="#Buoy,_deep_dan">
    <rdfs:subClassOf rdf:resource="jc3iedmSubOnt.owl#MARITIME-EQUIPMENT-TYPE-Buoy"/>
    <rdfs:subClassOf>
      <owl:Restriction>
        <owl:hasValue xml:lang="en">BUOYDP</owl:hasValue>
        <owl:onProperty rdf:resource="jc3iedmBase.owl#maritime-equipment-type-subcategory-code"/>
      </owl:Restriction>
    </rdfs:subClassOf>
    <rdfs:label xml:lang="en">Buoy, deep dan</rdfs:label>
    <rdfs:comment xml:lang="en">A temporary marker active buoy used in deep water during minesweeping operations to indicate the boundaries of swept paths, swept areas, known hazards or other locations for some specific reason.</rdfs:comment>
  </owl:Class>
  <owl:Class rdf:ID="Polar_ice">
    <rdfs:subClassOf rdf:resource="jc3iedmSubOnt.owl#GEOGRAPHIC-FEATURE-TYPE-Snow/ice"/>
    <rdfs:subClassOf rdf:resource="jc3iedmSubOnt.owl#GEOGRAPHIC-FEATURE-Solid_surface"/>
    <rdfs:subClassOf>
      <owl:Restriction>
        <owl:hasValue xml:lang="en">PLRICE</owl:hasValue>
        <owl:onProperty rdf:resource="jc3iedmBase.owl#geographic-feature-type-subcategory-code"/>
      </owl:Restriction>
    </rdfs:subClassOf>
    <rdfs:label xml:lang="en">Polar ice</rdfs:label>
    <rdfs:comment xml:lang="en">The heaviest, thickest form of ice over land or water.</rdfs:comment>
    <rdfs:subClassOf>
      <owl:Restriction>
        <owl:hasValue xml:lang="en">PLRICE</owl:hasValue>
        <owl:onProperty rdf:resource="jc3iedmBase.owl#geographic-feature-type-subcategory-code"/>
      </owl:Restriction>
    </rdfs:subClassOf>
  </owl:Class>
  <owl:Class rdf:ID="UN_Dangerous_Goods_NUM_1699">
    <rdfs:subClassOf>
      <owl:Restriction>
        <owl:hasValue xml:lang="en">1699</owl:hasValue>
        <owl:onProperty rdf:resource="jc3iedmBase.owl#consumable-materiel-type-united-nations-number-code"/>
      </owl:Restriction>
    </rdfs:subClassOf>
    <rdfs:label xml:lang="en">UN Dangerous Goods # 1699</rdfs:label>
    <rdfs:comment xml:lang="en">Diphenylchloroarsine, liquid or solid. Includes the agent(s): diphenylchloroarsine.</rdfs:comment>
    <rdfs:subClassOf>
      <owl:Restriction>
        <owl:hasValue xml:lang="en">1699</owl:hasValue>
        <owl:onProperty rdf:resource="jc3iedmBase.owl#consumable-materiel-type-united-nations-number-code"/>
      </owl:Restriction>
    </rdfs:subClassOf>
  </owl:Class>
  <owl:Class rdf:ID="Marijuana">
    <rdfs:subClassOf rdf:resource="jc3iedmSubOnt.owl#CONSUMABLE-MATERIEL-TYPE-Drug"/>
    <rdfs:subClassOf>
      <owl:Restriction>
        <owl:hasValue xml:lang="en">MARJUN</owl:hasValue>
        <owl:onProperty rdf:resource="jc3iedmBase.owl#consumable-materiel-type-subcategory-code"/>
      </owl:Restriction>
    </rdfs:subClassOf>
    <rdfs:label xml:lang="en">Marijuana</rdfs:label>
    <rdfs:comment xml:lang="en">The dried leaves, flowering tops, and stems of the hemp, used as an intoxicating or hallucinogenic drug and usu. smoked in cigarettes; cannabis.</rdfs:comment>
  </owl:Class>
  <owl:Class rdf:about="#Sweep,_protective_combination">
    <rdfs:subClassOf rdf:resource="jc3iedmSubOnt.owl#MARITIME-EQUIPMENT-TYPE-Sweep"/>
    <rdfs:subClassOf>
      <owl:Restriction>
        <owl:hasValue xml:lang="en">SWPPRT</owl:hasValue>
        <owl:onProperty rdf:resource="jc3iedmBase.owl#maritime-equipment-type-subcategory-code"/>
      </owl:Restriction>
    </rdfs:subClassOf>
    <rdfs:label xml:lang="en">Sweep, protective combination</rdfs:label>
    <rdfs:comment xml:lang="en">Equipment designed to locate mines by use of a sweep designed to operate the acoustic firing system of a mine, MF and LF frequency 30 to 15000HZ.</rdfs:comment>
  </owl:Class>
  <owl:Class rdf:about="#Direct_fire_gun,_heavy">
    <rdfs:subClassOf rdf:resource="jc3iedmSubOnt.owl#WEAPON-TYPE-Small_arms"/>
    <rdfs:subClassOf>
      <owl:Restriction>
        <owl:hasValue xml:lang="en">DFGNHV</owl:hasValue>
        <owl:onProperty rdf:resource="jc3iedmBase.owl#weapon-type-subcategory-code"/>
      </owl:Restriction>
    </rdfs:subClassOf>
    <rdfs:label xml:lang="en">Direct fire gun, heavy</rdfs:label>
    <rdfs:comment xml:lang="en">No definition provided in APP-6A.</rdfs:comment>
  </owl:Class>
  <owl:Class rdf:ID="Wood">
    <rdfs:subClassOf rdf:resource="jc3iedmSubOnt.owl#CONSUMABLE-MATERIEL-TYPE-General_supplies"/>
    <rdfs:subClassOf rdf:resource="jc3iedmSubOnt.owl#CONSUMABLE-MATERIEL-TYPE-Fuel"/>
    <rdfs:subClassOf>
      <owl:Restriction>
        <owl:hasValue xml:lang="en">WOOD</owl:hasValue>
        <owl:onProperty rdf:resource="jc3iedmBase.owl#consumable-materiel-type-subcategory-code"/>
      </owl:Restriction>
    </rdfs:subClassOf>
    <rdfs:label xml:lang="en">Wood</rdfs:label>
    <rdfs:comment xml:lang="en">A material used for construction or fuel.</rdfs:comment>
    <rdfs:subClassOf>
      <owl:Restriction>
        <owl:hasValue xml:lang="en">WOOD</owl:hasValue>
        <owl:onProperty rdf:resource="jc3iedmBase.owl#consumable-materiel-type-subcategory-code"/>
      </owl:Restriction>
    </rdfs:subClassOf>
  </owl:Class>
  <owl:Class rdf:ID="UN_Dangerous_Goods_NUM_1580">
    <rdfs:subClassOf>
      <owl:Restriction>
        <owl:hasValue xml:lang="en">1580</owl:hasValue>
        <owl:onProperty rdf:resource="jc3iedmBase.owl#consumable-materiel-type-united-nations-number-code"/>
      </owl:Restriction>
    </rdfs:subClassOf>
    <rdfs:label xml:lang="en">UN Dangerous Goods # 1580</rdfs:label>
    <rdfs:comment xml:lang="en">Chloropicrin. Includes the agent(s): chloropicrin.</rdfs:comment>
    <rdfs:subClassOf>
      <owl:Restriction>
        <owl:hasValue xml:lang="en">1580</owl:hasValue>
        <owl:onProperty rdf:resource="jc3iedmBase.owl#consumable-materiel-type-united-nations-number-code"/>
      </owl:Restriction>
    </rdfs:subClassOf>
  </owl:Class>
  <owl:Class rdf:ID="Sebkha">
    <rdfs:subClassOf rdf:resource="jc3iedmSubOnt.owl#GEOGRAPHIC-FEATURE-TYPE-Inland_water"/>
    <rdfs:subClassOf rdf:resource="jc3iedmSubOnt.owl#GEOGRAPHIC-FEATURE-Solid_surface"/>
    <rdfs:subClassOf>
      <owl:Restriction>
        <owl:hasValue xml:lang="en">SEBKHA</owl:hasValue>
        <owl:onProperty rdf:resource="jc3iedmBase.owl#geographic-feature-type-subcategory-code"/>
      </owl:Restriction>
    </rdfs:subClassOf>
    <rdfs:label xml:lang="en">Sebkha</rdfs:label>
    <rdfs:comment xml:lang="en">A natural depression in arid or semi-arid regions whose bed is covered with salt encrusted clayey soil.</rdfs:comment>
    <rdfs:subClassOf>
      <owl:Restriction>
        <owl:hasValue xml:lang="en">SEBKHA</owl:hasValue>
        <owl:onProperty rdf:resource="jc3iedmBase.owl#geographic-feature-type-subcategory-code"/>
      </owl:Restriction>
    </rdfs:subClassOf>
  </owl:Class>
  <owl:Class rdf:ID="Amphetamine">
    <rdfs:subClassOf rdf:resource="jc3iedmSubOnt.owl#CONSUMABLE-MATERIEL-TYPE-Drug"/>
    <rdfs:subClassOf>
      <owl:Restriction>
        <owl:hasValue xml:lang="en">AMPHTM</owl:hasValue>
        <owl:onProperty rdf:resource="jc3iedmBase.owl#consumable-materiel-type-subcategory-code"/>
      </owl:Restriction>
    </rdfs:subClassOf>
    <rdfs:label xml:lang="en">Amphetamine</rdfs:label>
    <rdfs:comment xml:lang="en">A synthetic drug used esp. as a stimulant.</rdfs:comment>
  </owl:Class>
  <owl:Class rdf:about="#Locomotive,_diesel">
    <rdfs:subClassOf rdf:resource="jc3iedmSubOnt.owl#RAILCAR-TYPE-Locomotive"/>
    <rdfs:subClassOf>
      <owl:Restriction>
        <owl:hasValue xml:lang="en">LCMDSL</owl:hasValue>
        <owl:onProperty rdf:resource="jc3iedmBase.owl#railcar-type-subcategory-code"/>
      </owl:Restriction>
    </rdfs:subClassOf>
    <rdfs:label xml:lang="en">Locomotive, diesel</rdfs:label>
    <rdfs:comment xml:lang="en">A locomotive that uses diesel engine(s) as its source of tractive power.</rdfs:comment>
  </owl:Class>
  <owl:Class rdf:ID="UN_Dangerous_Goods_NUM_2521">
    <rdfs:subClassOf>
      <owl:Restriction>
        <owl:hasValue xml:lang="en">2521</owl:hasValue>
        <owl:onProperty rdf:resource="jc3iedmBase.owl#consumable-materiel-type-united-nations-number-code"/>
      </owl:Restriction>
    </rdfs:subClassOf>
    <rdfs:label xml:lang="en">UN Dangerous Goods # 2521</rdfs:label>
    <rdfs:comment xml:lang="en">Diketene, stabilized. Includes the agent(s): diketene.</rdfs:comment>
    <rdfs:subClassOf>
      <owl:Restriction>
        <owl:hasValue xml:lang="en">2521</owl:hasValue>
        <owl:onProperty rdf:resource="jc3iedmBase.owl#consumable-materiel-type-united-nations-number-code"/>
      </owl:Restriction>
    </rdfs:subClassOf>
  </owl:Class>
  <owl:Class rdf:about="#Sweep,_magnetic_closed_loop">
    <rdfs:subClassOf rdf:resource="jc3iedmSubOnt.owl#MARITIME-EQUIPMENT-TYPE-Sweep"/>
    <rdfs:subClassOf>
      <owl:Restriction>
        <owl:hasValue xml:lang="en">SWPMGC</owl:hasValue>
        <owl:onProperty rdf:resource="jc3iedmBase.owl#maritime-equipment-type-subcategory-code"/>
      </owl:Restriction>
    </rdfs:subClassOf>
    <rdfs:label xml:lang="en">Sweep, magnetic closed loop</rdfs:label>
    <rdfs:comment xml:lang="en">Equipment designed to locate mines by use of a conducting cable, loop shaped through which is passed a high current, towed behind a minesweeper.</rdfs:comment>
  </owl:Class>
  <owl:Class rdf:ID="Mountain">
    <rdfs:subClassOf rdf:resource="jc3iedmSubOnt.owl#GEOGRAPHIC-FEATURE-Solid_surface"/>
    <rdfs:subClassOf rdf:resource="jc3iedmSubOnt.owl#GEOGRAPHIC-FEATURE-TYPE-Landform"/>
    <rdfs:subClassOf>
      <owl:Restriction>
        <owl:hasValue xml:lang="en">MOUNTN</owl:hasValue>
        <owl:onProperty rdf:resource="jc3iedmBase.owl#geographic-feature-type-subcategory-code"/>
      </owl:Restriction>
    </rdfs:subClassOf>
    <rdfs:label xml:lang="en">Mountain</rdfs:label>
    <rdfs:comment xml:lang="en">A natural elevation of the earth's surface rising more or less abruptly from the surrounding level, and attaining an altitude which, relatively to adjacent elevations, is impressive or notable.</rdfs:comment>
    <rdfs:subClassOf>
      <owl:Restriction>
        <owl:hasValue xml:lang="en">MOUNTN</owl:hasValue>
        <owl:onProperty rdf:resource="jc3iedmBase.owl#geographic-feature-type-subcategory-code"/>
      </owl:Restriction>
    </rdfs:subClassOf>
  </owl:Class>
  <owl:Class rdf:about="#Water,_neither_medical_nor_human_use">
    <rdfs:subClassOf rdf:resource="jc3iedmSubOnt.owl#CONSUMABLE-MATERIEL-TYPE-Water"/>
    <rdfs:subClassOf>
      <owl:Restriction>
        <owl:hasValue xml:lang="en">WTROTH</owl:hasValue>
        <owl:onProperty rdf:resource="jc3iedmBase.owl#consumable-materiel-type-subcategory-code"/>
      </owl:Restriction>
    </rdfs:subClassOf>
    <rdfs:label xml:lang="en">Water, neither medical nor human use</rdfs:label>
    <rdfs:comment xml:lang="en">H2O that may have a level of poisons/toxins or bacteria that make it unfit for human consumption or medical usage, but that may be used for other purposes.</rdfs:comment>
  </owl:Class>
  <owl:Class rdf:ID="Loudspeaker">
    <rdfs:subClassOf rdf:resource="jc3iedmSubOnt.owl#ELECTRONIC-EQUIPMENT-TYPE-Public_address_system"/>
    <rdfs:subClassOf rdf:resource="jc3iedmSubOnt.owl#ELECTRONIC-EQUIPMENT-TYPE-Communication"/>
    <rdfs:subClassOf>
      <owl:Restriction>
        <owl:hasValue xml:lang="en">LOUDSP</owl:hasValue>
        <owl:onProperty rdf:resource="jc3iedmBase.owl#electronic-equipment-type-subcategory-code"/>
      </owl:Restriction>
    </rdfs:subClassOf>
    <rdfs:label xml:lang="en">Loudspeaker</rdfs:label>
    <rdfs:comment xml:lang="en">An instrument for converting variations in an applied electrical current or voltage into corresponding sound waves.</rdfs:comment>
    <rdfs:subClassOf>
      <owl:Restriction>
        <owl:hasValue xml:lang="en">LOUDSP</owl:hasValue>
        <owl:onProperty rdf:resource="jc3iedmBase.owl#electronic-equipment-type-subcategory-code"/>
      </owl:Restriction>
    </rdfs:subClassOf>
  </owl:Class>
  <owl:Class rdf:ID="Trees">
    <rdfs:label xml:lang="en">Trees</rdfs:label>
    <rdfs:comment xml:lang="en">Woody-perennial plants, having a self-supporting main stem or trunk.</rdfs:comment>
  </owl:Class>
  <owl:Class rdf:ID="Boom_and_centreline_drogue">
    <rdfs:subClassOf rdf:resource="jc3iedmSubOnt.owl#MISCELLANEOUS-EQUIPMENT-TYPE-Aircraft_refuelling"/>
    <rdfs:subClassOf>
      <owl:Restriction>
        <owl:hasValue xml:lang="en">BCD</owl:hasValue>
        <owl:onProperty rdf:resource="jc3iedmBase.owl#miscellaneous-equipment-type-subcategory-code"/>
      </owl:Restriction>
    </rdfs:subClassOf>
    <rdfs:label xml:lang="en">Boom and centreline drogue</rdfs:label>
    <rdfs:comment xml:lang="en">Two components of a refuelling system by which a boom and a centreline drogue devices can provide fuel on a receiver aircraft.</rdfs:comment>
  </owl:Class>
  <owl:Class rdf:ID="Data_link">
    <rdfs:subClassOf rdf:resource="jc3iedmSubOnt.owl#ELECTRONIC-EQUIPMENT-TYPE-Communication"/>
    <rdfs:subClassOf>
      <owl:Restriction>
        <owl:hasValue xml:lang="en">DATLNK</owl:hasValue>
        <owl:onProperty rdf:resource="jc3iedmBase.owl#electronic-equipment-type-subcategory-code"/>
      </owl:Restriction>
    </rdfs:subClassOf>
    <rdfs:label xml:lang="en">Data link</rdfs:label>
    <rdfs:comment xml:lang="en">The equipment providing the means of transmitting and receiving data.</rdfs:comment>
  </owl:Class>
  <owl:Class rdf:ID="Lewisite">
    <rdfs:subClassOf rdf:resource="jc3iedmSubOnt.owl#CHEMICAL-MATERIEL-TYPE-Blood_agent"/>
    <rdfs:subClassOf>
      <owl:Restriction>
        <owl:hasValue xml:lang="en">LWSITE</owl:hasValue>
        <owl:onProperty rdf:resource="jc3iedmBase.owl#chemical-materiel-type-subcategory-code"/>
      </owl:Restriction>
    </rdfs:subClassOf>
    <rdfs:label xml:lang="en">Lewisite</rdfs:label>
    <rdfs:comment xml:lang="en">A dark oily liquid producing an irritant gas that causes blisters, developed for use in chemical warfare.</rdfs:comment>
  </owl:Class>
  <owl:Class rdf:about="#Radar,_advanced_synthetic_aperture">
    <rdfs:subClassOf rdf:resource="jc3iedmSubOnt.owl#ELECTRONIC-EQUIPMENT-TYPE-Radar"/>
    <rdfs:subClassOf rdf:resource="jc3iedmSubOnt.owl#ELECTRONIC-EQUIPMENT-TYPE-Sensor"/>
    <rdfs:subClassOf>
      <owl:Restriction>
        <owl:hasValue xml:lang="en">RDRASA</owl:hasValue>
        <owl:onProperty rdf:resource="jc3iedmBase.owl#electronic-equipment-type-subcategory-code"/>
      </owl:Restriction>
    </rdfs:subClassOf>
    <rdfs:label xml:lang="en">Radar, advanced synthetic aperture</rdfs:label>
    <rdfs:comment xml:lang="en">A multimode real-time, high-resolution reconnaissance system carried on an aircraft with all-weather, day-night, and long-range mapping capabilities. ASARS detects and accurately locates stationary and moving ground targets.</rdfs:comment>
    <rdfs:subClassOf>
      <owl:Restriction>
        <owl:hasValue xml:lang="en">RDRASA</owl:hasValue>
        <owl:onProperty rdf:resource="jc3iedmBase.owl#electronic-equipment-type-subcategory-code"/>
      </owl:Restriction>
    </rdfs:subClassOf>
  </owl:Class>
  <owl:Class rdf:ID="UN_Dangerous_Goods_NUM_2534">
    <rdfs:subClassOf>
      <owl:Restriction>
        <owl:hasValue xml:lang="en">2534</owl:hasValue>
        <owl:onProperty rdf:resource="jc3iedmBase.owl#consumable-materiel-type-united-nations-number-code"/>
      </owl:Restriction>
    </rdfs:subClassOf>
    <rdfs:label xml:lang="en">UN Dangerous Goods # 2534</rdfs:label>
    <rdfs:comment xml:lang="en">Methylchlorosilane. Includes the agent(s): methyl chlorosilane.</rdfs:comment>
    <rdfs:subClassOf>
      <owl:Restriction>
        <owl:hasValue xml:lang="en">2534</owl:hasValue>
        <owl:onProperty rdf:resource="jc3iedmBase.owl#consumable-materiel-type-united-nations-number-code"/>
      </owl:Restriction>
    </rdfs:subClassOf>
  </owl:Class>
  <owl:Class rdf:about="#Link_16,_data">
    <rdfs:subClassOf rdf:resource="jc3iedmSubOnt.owl#NETWORK-SERVICE-Tactical_data_link"/>
    <rdfs:subClassOf>
      <owl:Restriction>
        <owl:hasValue xml:lang="en">LNK16D</owl:hasValue>
        <owl:onProperty rdf:resource="jc3iedmBase.owl#network-service-subcategory-code"/>
      </owl:Restriction>
    </rdfs:subClassOf>
    <rdfs:label xml:lang="en">Link 16, data</rdfs:label>
    <rdfs:comment xml:lang="en">A service that provides the basic elements for the transmission of data of Link 16.</rdfs:comment>
  </owl:Class>
  <owl:Class rdf:about="#Mortar,_medium">
    <rdfs:subClassOf rdf:resource="jc3iedmSubOnt.owl#WEAPON-TYPE-Mortar"/>
    <rdfs:subClassOf>
      <owl:Restriction>
        <owl:hasValue xml:lang="en">MRTMED</owl:hasValue>
        <owl:onProperty rdf:resource="jc3iedmBase.owl#weapon-type-subcategory-code"/>
      </owl:Restriction>
    </rdfs:subClassOf>
    <rdfs:label xml:lang="en">Mortar, medium</rdfs:label>
    <rdfs:comment xml:lang="en">A man-portable, muzzle-loading, indirect fire weapon with either a rifled or smooth bore. It usually has a shorter range than a howitzer, employs a higher angle of fire, and its calibre is usually between 61mm and 107mm.</rdfs:comment>
  </owl:Class>
  <owl:Class rdf:ID="Sensitive_for_normal_target">
    <rdfs:subClassOf rdf:resource="jc3iedmSubOnt.owl#AMMUNITION-TYPE-Sea_mine"/>
    <rdfs:subClassOf>
      <owl:Restriction>
        <owl:hasValue xml:lang="en">SENFNT</owl:hasValue>
        <owl:onProperty rdf:resource="jc3iedmBase.owl#ammunition-type-mine-maritime-firing-code"/>
      </owl:Restriction>
    </rdfs:subClassOf>
    <rdfs:subClassOf rdf:resource="jc3iedmSubOnt.owl#AMMUNITION-TYPE-Mine,_deep_moored"/>
    <rdfs:label xml:lang="en">Sensitive for normal target</rdfs:label>
    <rdfs:subClassOf rdf:resource="jc3iedmSubOnt.owl#AMMUNITION-TYPE-Mine,_moored"/>
    <rdfs:subClassOf rdf:resource="jc3iedmSubOnt.owl#AMMUNITION-TYPE-Mine,_seabed_-_explosive_charge_500kg_or_greater"/>
    <rdfs:subClassOf rdf:resource="jc3iedmSubOnt.owl#AMMUNITION-TYPE-Mine,_not_known"/>
    <rdfs:subClassOf rdf:resource="jc3iedmSubOnt.owl#AMMUNITION-TYPE-Mine,_shallow_moored"/>
    <rdfs:subClassOf rdf:resource="jc3iedmSubOnt.owl#AMMUNITION-TYPE-Moving_mine,_sea"/>
    <rdfs:subClassOf rdf:resource="jc3iedmSubOnt.owl#AMMUNITION-TYPE-Seabed_mine"/>
    <rdfs:subClassOf rdf:resource="jc3iedmSubOnt.owl#AMMUNITION-TYPE-Mine,_seabed_-_explosive_charge_less_than_500kg"/>
    <rdfs:subClassOf>
      <owl:Restriction>
        <owl:hasValue xml:lang="en">SENFNT</owl:hasValue>
        <owl:onProperty rdf:resource="jc3iedmBase.owl#ammunition-type-mine-maritime-firing-code"/>
      </owl:Restriction>
    </rdfs:subClassOf>
    <rdfs:subClassOf rdf:resource="jc3iedmSubOnt.owl#AMMUNITION-TYPE-Mine,_not_otherwise_specified"/>
    <rdfs:comment xml:lang="en">A (maritime) mine firing mechanism that may actuated by a small change in its influence field.</rdfs:comment>
    <rdfs:subClassOf rdf:resource="jc3iedmSubOnt.owl#AMMUNITION-TYPE-Mine,_maritime,_moving"/>
  </owl:Class>
  <owl:Class rdf:ID="UN_Dangerous_Goods_NUM_3329">
    <rdfs:subClassOf>
      <owl:Restriction>
        <owl:hasValue xml:lang="en">3329</owl:hasValue>
        <owl:onProperty rdf:resource="jc3iedmBase.owl#consumable-materiel-type-united-nations-number-code"/>
      </owl:Restriction>
    </rdfs:subClassOf>
    <rdfs:label xml:lang="en">UN Dangerous Goods # 3329</rdfs:label>
    <rdfs:comment xml:lang="en">Radioactive material, type B(M) package, fissile.</rdfs:comment>
  </owl:Class>
  <owl:Class rdf:about="#Air-defence_gun,_medium">
    <rdfs:subClassOf rdf:resource="jc3iedmSubOnt.owl#WEAPON-TYPE-Air-defence"/>
    <rdfs:subClassOf>
      <owl:Restriction>
        <owl:hasValue xml:lang="en">ADMED</owl:hasValue>
        <owl:onProperty rdf:resource="jc3iedmBase.owl#weapon-type-subcategory-code"/>
      </owl:Restriction>
    </rdfs:subClassOf>
    <rdfs:label xml:lang="en">Air-defence gun, medium</rdfs:label>
    <rdfs:comment xml:lang="en">A medium gun used primarily in the role of air defence.</rdfs:comment>
  </owl:Class>
  <owl:Class rdf:ID="Terrain">
    <rdfs:label xml:lang="en">Terrain</rdfs:label>
    <rdfs:comment xml:lang="en">Represents the general mode of transportation used in surface movement other than road and rail.</rdfs:comment>
  </owl:Class>
  <owl:Class rdf:ID="NATO_standard_fuel_code_F34">
    <rdfs:subClassOf rdf:resource="jc3iedmSubOnt.owl#CONSUMABLE-MATERIEL-TYPE-Fuel"/>
    <rdfs:subClassOf>
      <owl:Restriction>
        <owl:hasValue xml:lang="en">NASF34</owl:hasValue>
        <owl:onProperty rdf:resource="jc3iedmBase.owl#consumable-materiel-type-subcategory-code"/>
      </owl:Restriction>
    </rdfs:subClassOf>
    <rdfs:label xml:lang="en">NATO standard fuel code F34</rdfs:label>
    <rdfs:comment xml:lang="en">Turbine Fuel, Aviation, Kerosene Type With S748.</rdfs:comment>
  </owl:Class>
  <owl:Class rdf:about="#Radar,_bomb_navigation">
    <rdfs:subClassOf rdf:resource="jc3iedmSubOnt.owl#ELECTRONIC-EQUIPMENT-TYPE-Radar"/>
    <rdfs:subClassOf rdf:resource="jc3iedmSubOnt.owl#ELECTRONIC-EQUIPMENT-TYPE-Navigational_aid"/>
    <rdfs:subClassOf>
      <owl:Restriction>
        <owl:hasValue xml:lang="en">RDRBNV</owl:hasValue>
        <owl:onProperty rdf:resource="jc3iedmBase.owl#electronic-equipment-type-subcategory-code"/>
      </owl:Restriction>
    </rdfs:subClassOf>
    <rdfs:label xml:lang="en">Radar, bomb navigation</rdfs:label>
    <rdfs:comment xml:lang="en">A radar used specifically for bomb navigation.</rdfs:comment>
    <rdfs:subClassOf>
      <owl:Restriction>
        <owl:hasValue xml:lang="en">RDRBNV</owl:hasValue>
        <owl:onProperty rdf:resource="jc3iedmBase.owl#electronic-equipment-type-subcategory-code"/>
      </owl:Restriction>
    </rdfs:subClassOf>
  </owl:Class>
  <owl:Class rdf:ID="Submarine_towed_array_surveillance_system">
    <rdfs:subClassOf rdf:resource="jc3iedmSubOnt.owl#MARITIME-EQUIPMENT-TYPE-Towed_array_surveillance_system,_tactical"/>
    <rdfs:subClassOf rdf:resource="jc3iedmSubOnt.owl#MARITIME-EQUIPMENT-TYPE-Towed_array_surveillance_system"/>
    <rdfs:subClassOf>
      <owl:Restriction>
        <owl:hasValue xml:lang="en">SUBTSS</owl:hasValue>
        <owl:onProperty rdf:resource="jc3iedmBase.owl#maritime-equipment-type-subcategory-code"/>
      </owl:Restriction>
    </rdfs:subClassOf>
    <rdfs:label xml:lang="en">Submarine towed array surveillance system</rdfs:label>
    <rdfs:comment xml:lang="en">No definition provided in ADatP-3 Baseline 13.1 FFIRN/FUD 1434/1.</rdfs:comment>
    <rdfs:subClassOf>
      <owl:Restriction>
        <owl:hasValue xml:lang="en">SUBTSS</owl:hasValue>
        <owl:onProperty rdf:resource="jc3iedmBase.owl#maritime-equipment-type-subcategory-code"/>
      </owl:Restriction>
    </rdfs:subClassOf>
  </owl:Class>
  <owl:Class rdf:ID="Multi-channel_DIFAR_relay">
    <rdfs:subClassOf rdf:resource="jc3iedmSubOnt.owl#MARITIME-EQUIPMENT-TYPE-Buoy"/>
    <rdfs:subClassOf>
      <owl:Restriction>
        <owl:hasValue xml:lang="en">MCDFRR</owl:hasValue>
        <owl:onProperty rdf:resource="jc3iedmBase.owl#maritime-equipment-type-subcategory-code"/>
      </owl:Restriction>
    </rdfs:subClassOf>
    <rdfs:label xml:lang="en">Multi-channel DIFAR relay</rdfs:label>
    <rdfs:comment xml:lang="en">A relaying Directional Frequency Ranging sonobuoy with 4-64 Channels.</rdfs:comment>
  </owl:Class>
  <owl:Class rdf:about="#Single_rocket_launcher,_light">
    <rdfs:subClassOf rdf:resource="jc3iedmSubOnt.owl#WEAPON-TYPE-Rocket_artillery"/>
    <rdfs:subClassOf>
      <owl:Restriction>
        <owl:hasValue xml:lang="en">SRKLLG</owl:hasValue>
        <owl:onProperty rdf:resource="jc3iedmBase.owl#weapon-type-subcategory-code"/>
      </owl:Restriction>
    </rdfs:subClassOf>
    <rdfs:label xml:lang="en">Single rocket launcher, light</rdfs:label>
    <rdfs:comment xml:lang="en">A light structural device designed to support and hold a rocket in position for firing.</rdfs:comment>
  </owl:Class>
  <owl:Class rdf:ID="UN_Dangerous_Goods_NUM_1045">
    <rdfs:subClassOf>
      <owl:Restriction>
        <owl:hasValue xml:lang="en">1045</owl:hasValue>
        <owl:onProperty rdf:resource="jc3iedmBase.owl#consumable-materiel-type-united-nations-number-code"/>
      </owl:Restriction>
    </rdfs:subClassOf>
    <rdfs:label xml:lang="en">UN Dangerous Goods # 1045</rdfs:label>
    <rdfs:comment xml:lang="en">Fluorine, compressed. Includes the agent(s): fluorine.</rdfs:comment>
    <rdfs:subClassOf>
      <owl:Restriction>
        <owl:hasValue xml:lang="en">1045</owl:hasValue>
        <owl:onProperty rdf:resource="jc3iedmBase.owl#consumable-materiel-type-united-nations-number-code"/>
      </owl:Restriction>
    </rdfs:subClassOf>
  </owl:Class>
  <owl:Class rdf:ID="Nursery">
    <rdfs:label xml:lang="en">Nursery</rdfs:label>
    <rdfs:comment xml:lang="en">A place where shrubs, flowers, plants and trees are grown for transplanting, seed or grafting.</rdfs:comment>
  </owl:Class>
  <owl:Class rdf:ID="Tactical_air_navigation">
    <rdfs:subClassOf rdf:resource="jc3iedmSubOnt.owl#ELECTRONIC-EQUIPMENT-TYPE-Navigational_aid"/>
    <rdfs:subClassOf>
      <owl:Restriction>
        <owl:hasValue xml:lang="en">TACTAN</owl:hasValue>
        <owl:onProperty rdf:resource="jc3iedmBase.owl#electronic-equipment-type-subcategory-code"/>
      </owl:Restriction>
    </rdfs:subClassOf>
    <rdfs:label xml:lang="en">Tactical air navigation</rdfs:label>
    <rdfs:comment xml:lang="en">An electronic air navigation system operating on an ultra high frequency, able to provide continuous bearing and slant range to a selected station.</rdfs:comment>
  </owl:Class>
  <owl:Class rdf:about="#Wagon,_passenger">
    <rdfs:subClassOf rdf:resource="jc3iedmSubOnt.owl#RAILCAR-TYPE-Rolling_stock"/>
    <rdfs:subClassOf>
      <owl:Restriction>
        <owl:hasValue xml:lang="en">WGNPAS</owl:hasValue>
        <owl:onProperty rdf:resource="jc3iedmBase.owl#railcar-type-subcategory-code"/>
      </owl:Restriction>
    </rdfs:subClassOf>
    <rdfs:label xml:lang="en">Wagon, passenger</rdfs:label>
    <rdfs:comment xml:lang="en">Rolling stock used for the transportation of passengers.</rdfs:comment>
  </owl:Class>
  <owl:Class rdf:about="#Cutter,_explosive">
    <rdfs:subClassOf rdf:resource="jc3iedmSubOnt.owl#MARITIME-EQUIPMENT-TYPE-Cutter"/>
    <rdfs:subClassOf>
      <owl:Restriction>
        <owl:hasValue xml:lang="en">CUTTEX</owl:hasValue>
        <owl:onProperty rdf:resource="jc3iedmBase.owl#maritime-equipment-type-subcategory-code"/>
      </owl:Restriction>
    </rdfs:subClassOf>
    <rdfs:label xml:lang="en">Cutter, explosive</rdfs:label>
    <rdfs:comment xml:lang="en">In naval mine warfare an explosive device fitted to a sweep wire to cut or part the mooring of mines or obstructors; it may also be fitted in, or to, the mooring of a mine or obstructors to part a sweep wire.</rdfs:comment>
  </owl:Class>
  <owl:Class rdf:ID="Letter_bomb">
    <rdfs:subClassOf rdf:resource="jc3iedmSubOnt.owl#CONSUMABLE-MATERIEL-TYPE-Improvised_explosive_device"/>
    <rdfs:subClassOf>
      <owl:Restriction>
        <owl:hasValue xml:lang="en">LTRBMB</owl:hasValue>
        <owl:onProperty rdf:resource="jc3iedmBase.owl#consumable-materiel-type-subcategory-code"/>
      </owl:Restriction>
    </rdfs:subClassOf>
    <rdfs:label xml:lang="en">Letter bomb</rdfs:label>
    <rdfs:comment xml:lang="en">An improvised explosive device deliberately sent by postal or other services, as an apparently harmless letter or parcel, to cause casualties to the addressee.</rdfs:comment>
  </owl:Class>
  <owl:Class rdf:ID="UN_Dangerous_Goods_NUM_1697">
    <rdfs:subClassOf>
      <owl:Restriction>
        <owl:hasValue xml:lang="en">1697</owl:hasValue>
        <owl:onProperty rdf:resource="jc3iedmBase.owl#consumable-materiel-type-united-nations-number-code"/>
      </owl:Restriction>
    </rdfs:subClassOf>
    <rdfs:label xml:lang="en">UN Dangerous Goods # 1697</rdfs:label>
    <rdfs:comment xml:lang="en">Chloroacetophenone. Includes the agent(s): Tear Gas (CN).</rdfs:comment>
    <rdfs:subClassOf>
      <owl:Restriction>
        <owl:hasValue xml:lang="en">1697</owl:hasValue>
        <owl:onProperty rdf:resource="jc3iedmBase.owl#consumable-materiel-type-united-nations-number-code"/>
      </owl:Restriction>
    </rdfs:subClassOf>
  </owl:Class>
  <owl:Class rdf:about="#Orchard/plantation">
    <rdfs:label xml:lang="en">Orchard/plantation</rdfs:label>
    <rdfs:comment xml:lang="en">An area covered by systematic plantings of trees which yield fruits, nuts or other products.</rdfs:comment>
  </owl:Class>
  <owl:Class rdf:about="#Warning_and_control_system,_airborne">
    <rdfs:subClassOf rdf:resource="jc3iedmSubOnt.owl#ELECTRONIC-EQUIPMENT-TYPE-Sensor"/>
    <rdfs:subClassOf>
      <owl:Restriction>
        <owl:hasValue xml:lang="en">WCSAIR</owl:hasValue>
        <owl:onProperty rdf:resource="jc3iedmBase.owl#electronic-equipment-type-subcategory-code"/>
      </owl:Restriction>
    </rdfs:subClassOf>
    <rdfs:label xml:lang="en">Warning and control system, airborne</rdfs:label>
    <rdfs:comment xml:lang="en">Search and height finding radars and communications equipment (AWACS) designed to provide air surveillance and to control airborne weapons systems usually carried by an aircraft.</rdfs:comment>
  </owl:Class>
  <owl:Class rdf:ID="PARKHILL">
    <rdfs:subClassOf rdf:resource="jc3iedmSubOnt.owl#ELECTRONIC-EQUIPMENT-TYPE-Communication"/>
    <rdfs:subClassOf>
      <owl:Restriction>
        <owl:hasValue xml:lang="en">PRKHLL</owl:hasValue>
        <owl:onProperty rdf:resource="jc3iedmBase.owl#electronic-equipment-type-subcategory-code"/>
      </owl:Restriction>
    </rdfs:subClassOf>
    <rdfs:label xml:lang="en">PARKHILL</rdfs:label>
    <rdfs:comment xml:lang="en">A secure voice communications terminal.</rdfs:comment>
  </owl:Class>
  <owl:Class rdf:ID="Ledge">
    <rdfs:subClassOf rdf:resource="jc3iedmSubOnt.owl#GEOGRAPHIC-FEATURE-Solid_surface"/>
    <rdfs:subClassOf rdf:resource="jc3iedmSubOnt.owl#GEOGRAPHIC-FEATURE-TYPE-Landform"/>
    <rdfs:subClassOf>
      <owl:Restriction>
        <owl:hasValue xml:lang="en">LEDGE</owl:hasValue>
        <owl:onProperty rdf:resource="jc3iedmBase.owl#geographic-feature-type-subcategory-code"/>
      </owl:Restriction>
    </rdfs:subClassOf>
    <rdfs:label xml:lang="en">Ledge</rdfs:label>
    <rdfs:comment xml:lang="en">A narrow, flat surface or shelf, especially one that projects, as from a wall of rock.</rdfs:comment>
    <rdfs:subClassOf>
      <owl:Restriction>
        <owl:hasValue xml:lang="en">LEDGE</owl:hasValue>
        <owl:onProperty rdf:resource="jc3iedmBase.owl#geographic-feature-type-subcategory-code"/>
      </owl:Restriction>
    </rdfs:subClassOf>
  </owl:Class>
  <owl:Class rdf:about="#Sweep,_helicopter_acoustic">
    <rdfs:subClassOf rdf:resource="jc3iedmSubOnt.owl#MARITIME-EQUIPMENT-TYPE-Sweep"/>
    <rdfs:subClassOf>
      <owl:Restriction>
        <owl:hasValue xml:lang="en">SWPHAC</owl:hasValue>
        <owl:onProperty rdf:resource="jc3iedmBase.owl#maritime-equipment-type-subcategory-code"/>
      </owl:Restriction>
    </rdfs:subClassOf>
    <rdfs:label xml:lang="en">Sweep, helicopter acoustic</rdfs:label>
    <rdfs:comment xml:lang="en">Equipment mounted on a helicopter designed to be used in minesweeping operations, utilizing the acoustic firing mechanisms of the target mines.</rdfs:comment>
  </owl:Class>
  <owl:Class rdf:ID="UN_Dangerous_Goods_NUM_2908">
    <rdfs:subClassOf>
      <owl:Restriction>
        <owl:hasValue xml:lang="en">2908</owl:hasValue>
        <owl:onProperty rdf:resource="jc3iedmBase.owl#consumable-materiel-type-united-nations-number-code"/>
      </owl:Restriction>
    </rdfs:subClassOf>
    <rdfs:label xml:lang="en">UN Dangerous Goods # 2908</rdfs:label>
    <rdfs:comment xml:lang="en">Radioactive material, expected package - empty packaging.</rdfs:comment>
  </owl:Class>
  <owl:Class rdf:ID="NATO_standard_fuel_code_F40">
    <rdfs:subClassOf rdf:resource="jc3iedmSubOnt.owl#CONSUMABLE-MATERIEL-TYPE-Fuel"/>
    <rdfs:subClassOf>
      <owl:Restriction>
        <owl:hasValue xml:lang="en">NASF40</owl:hasValue>
        <owl:onProperty rdf:resource="jc3iedmBase.owl#consumable-materiel-type-subcategory-code"/>
      </owl:Restriction>
    </rdfs:subClassOf>
    <rdfs:label xml:lang="en">NATO standard fuel code F40</rdfs:label>
    <rdfs:comment xml:lang="en">Turbine Fuel, Aviation, Wide Cut Type, With S748.</rdfs:comment>
  </owl:Class>
  <owl:Class rdf:about="#Buoy,_dan">
    <rdfs:subClassOf rdf:resource="jc3iedmSubOnt.owl#MARITIME-EQUIPMENT-TYPE-Buoy"/>
    <rdfs:subClassOf>
      <owl:Restriction>
        <owl:hasValue xml:lang="en">BUOYDN</owl:hasValue>
        <owl:onProperty rdf:resource="jc3iedmBase.owl#maritime-equipment-type-subcategory-code"/>
      </owl:Restriction>
    </rdfs:subClassOf>
    <rdfs:label xml:lang="en">Buoy, dan</rdfs:label>
    <rdfs:comment xml:lang="en">A temporary marker buoy used during minesweeping operations to indicate the boundaries of swept paths, swept areas, known hazards or other locations of reference points.</rdfs:comment>
  </owl:Class>
</rdf:RDF>
