<rdf:RDF
    xmlns:rdf="http://www.w3.org/1999/02/22-rdf-syntax-ns#"
    xmlns:owl="http://www.w3.org/2002/07/owl#"
    xmlns:xsd="http://www.w3.org/2001/XMLSchema#"
    xmlns="http://cbml.googlecode.com/svn/trunk/jc3iedmOnt/rootClassOnt/jc3iedm_PLAN-ORDERExtended.owl#"
    xmlns:rdfs="http://www.w3.org/2000/01/rdf-schema#"
  xml:base="http://cbml.googlecode.com/svn/trunk/jc3iedmOnt/rootClassOnt/jc3iedm_PLAN-ORDERExtended.owl#" > 
  <rdf:Description rdf:about="#">
    <owl:imports rdf:resource="jc3iedm_PLAN-ORDER.owl#"/>
    <rdf:type rdf:resource="http://www.w3.org/2002/07/owl#Ontology"/>
  </rdf:Description>
  <rdf:Description rdf:about="jc3iedm_PLAN-ORDER.owl#PLAN">
    <rdf:type rdf:resource="http://www.w3.org/2002/07/owl#Class"/>
    <rdfs:label xml:lang="en">plan</rdfs:label>
    <rdfs:comment xml:lang="en">A proposal for putting into effect a command decision or project; it represents the preparation for future or anticipated operations.</rdfs:comment>
    <rdfs:subClassOf rdf:resource="jc3iedm_PLAN-ORDER.owl#PLAN-ORDER"/>
  </rdf:Description>
  <rdf:Description rdf:about="jc3iedm_PLAN-ORDER.owl#ORDER">
    <rdf:type rdf:resource="http://www.w3.org/2002/07/owl#Class"/>
    <rdfs:label xml:lang="en">order</rdfs:label>
    <rdfs:comment xml:lang="en">A communication that conveys instructions from a superior to a subordinate.</rdfs:comment>
    <rdfs:subClassOf rdf:resource="jc3iedm_PLAN-ORDER.owl#PLAN-ORDER"/>
  </rdf:Description>
  <rdf:Description rdf:about="#PLAN_Not_otherwise_specified">
    <rdfs:label xml:lang="en">not otherwise specified</rdfs:label>
    <rdfs:subClassOf rdf:resource="jc3iedm_PLAN-ORDER.owl#PLAN"/>
    <rdfs:comment xml:lang="en">The appropriate value is not in the set of specified values.</rdfs:comment>
    <rdf:type rdf:resource="http://www.w3.org/2002/07/owl#Class"/>
  </rdf:Description>
  <rdf:Description rdf:about="jc3iedm_PLAN-ORDER.owl#plan-order-category-code">
    <rdf:type rdf:resource="http://www.w3.org/2002/07/owl#DatatypeProperty"/>
    <rdfs:domain rdf:resource="jc3iedm_PLAN-ORDER.owl#PLAN-ORDER"/>
    <rdfs:range rdf:resource="http://www.w3.org/2001/XMLSchema#string"/>
  </rdf:Description>
  <rdf:Description rdf:about="#ORDER_Warning_order">
    <rdfs:label xml:lang="en">warning order</rdfs:label>
    <rdfs:subClassOf rdf:resource="jc3iedm_PLAN-ORDER.owl#ORDER"/>
    <rdfs:comment xml:lang="en">An order to assist units and their staffs initiate the preparations for and the execution of their new mission by giving them the maximum warning and essential details of impending operations and information of time available.</rdfs:comment>
    <rdf:type rdf:resource="http://www.w3.org/2002/07/owl#Class"/>
  </rdf:Description>
  <rdf:Description rdf:about="#ORDER_Administrative/Logistics_order">
    <rdfs:label xml:lang="en">administrative/logistics order</rdfs:label>
    <rdfs:subClassOf rdf:resource="jc3iedm_PLAN-ORDER.owl#ORDER"/>
    <rdfs:comment xml:lang="en">An order to give the commanderâ€™s plan for administrative and service support of operations.</rdfs:comment>
    <rdf:type rdf:resource="http://www.w3.org/2002/07/owl#Class"/>
  </rdf:Description>
  <rdf:Description rdf:about="jc3iedm_PLAN-ORDER.owl#PLAN-ORDER">
    <rdf:type rdf:resource="http://www.w3.org/2002/07/owl#Class"/>
    <rdfs:label xml:lang="en">plan order</rdfs:label>
    <rdfs:comment xml:lang="en">A planned or ordered scheme worked out beforehand for the accomplishment of an operational objective.</rdfs:comment>
  </rdf:Description>
  <rdf:Description rdf:about="jc3iedm_PLAN-ORDER.owl#physical_model_only">
    <rdf:type rdf:resource="http://www.w3.org/2002/07/owl#DatatypeProperty"/>
    <rdfs:domain rdf:resource="jc3iedm_PLAN-ORDER.owl#PLAN-ORDER"/>
  </rdf:Description>
  <rdf:Description rdf:about="#ORDER_Operations_order">
    <rdfs:label xml:lang="en">operations order</rdfs:label>
    <rdfs:subClassOf rdf:resource="jc3iedm_PLAN-ORDER.owl#ORDER"/>
    <rdfs:comment xml:lang="en">An order that includes only such detail as is necessary for commanders of subordinate formations/units to issue their own orders and to ensure coordination.</rdfs:comment>
    <rdf:type rdf:resource="http://www.w3.org/2002/07/owl#Class"/>
  </rdf:Description>
  <rdf:Description rdf:about="#PLAN_Operations_plan">
    <rdfs:label xml:lang="en">operations plan</rdfs:label>
    <rdfs:subClassOf rdf:resource="jc3iedm_PLAN-ORDER.owl#PLAN"/>
    <rdfs:comment xml:lang="en">A mechanism which a command uses to plan/prepare to conduct military operations.</rdfs:comment>
    <rdf:type rdf:resource="http://www.w3.org/2002/07/owl#Class"/>
  </rdf:Description>
  <rdf:Description rdf:about="#ORDER_Not_otherwise_specified">
    <rdfs:label xml:lang="en">not otherwise specified</rdfs:label>
    <rdfs:subClassOf rdf:resource="jc3iedm_PLAN-ORDER.owl#ORDER"/>
    <rdfs:comment xml:lang="en">The appropriate value is not in the set of specified values.</rdfs:comment>
    <rdf:type rdf:resource="http://www.w3.org/2002/07/owl#Class"/>
  </rdf:Description>
  <rdf:Description rdf:about="#ORDER_Fragmentary_order_to_existing_operation_order">
    <rdfs:label xml:lang="en">fragmentary order to existing operation order</rdfs:label>
    <rdfs:subClassOf rdf:resource="jc3iedm_PLAN-ORDER.owl#ORDER"/>
    <rdfs:comment xml:lang="en">An abbreviated form of an Operations order.</rdfs:comment>
    <rdf:type rdf:resource="http://www.w3.org/2002/07/owl#Class"/>
  </rdf:Description>
</rdf:RDF>
