<rdf:RDF
    xmlns:rdf="http://www.w3.org/1999/02/22-rdf-syntax-ns#"
    xmlns="http://cbml.googlecode.com/svn/trunk/jc3iedmOnt/rootClassOnt/jc3iedm_CAPABILITYExtended.owl#"
    xmlns:owl="http://www.w3.org/2002/07/owl#"
    xmlns:xsd="http://www.w3.org/2001/XMLSchema#"
    xmlns:rdfs="http://www.w3.org/2000/01/rdf-schema#"
  xml:base="http://cbml.googlecode.com/svn/trunk/jc3iedmOnt/rootClassOnt/jc3iedm_CAPABILITYExtended.owl#" > 
  <rdf:Description rdf:about="#OPERATIONAL-CAPABILITY_Mountain">
    <rdfs:label xml:lang="en">mountain</rdfs:label>
    <rdfs:subClassOf rdf:resource="jc3iedm_CAPABILITY.owl#OPERATIONAL-CAPABILITY"/>
    <rdfs:comment xml:lang="en">The capability to conduct military operations in mountainous areas.</rdfs:comment>
    <rdf:type rdf:resource="http://www.w3.org/2002/07/owl#Class"/>
  </rdf:Description>
  <rdf:Description rdf:about="#ENGINEERING-CAPABILITY_Construction">
    <rdfs:label xml:lang="en">construction</rdfs:label>
    <rdfs:subClassOf rdf:resource="jc3iedm_CAPABILITY.owl#ENGINEERING-CAPABILITY"/>
    <rdfs:comment xml:lang="en">The action or process of constructing.</rdfs:comment>
    <rdf:type rdf:resource="http://www.w3.org/2002/07/owl#Class"/>
  </rdf:Description>
  <rdf:Description rdf:about="#SUPPORT-CAPABILITY_Education">
    <rdfs:label xml:lang="en">education</rdfs:label>
    <rdfs:subClassOf rdf:resource="jc3iedm_CAPABILITY.owl#SUPPORT-CAPABILITY"/>
    <rdfs:comment xml:lang="en">The capability to provide education services.</rdfs:comment>
    <rdf:type rdf:resource="http://www.w3.org/2002/07/owl#Class"/>
  </rdf:Description>
  <rdf:Description rdf:about="jc3iedm_CAPABILITY.owl#OPERATIONAL-CAPABILITY">
    <rdf:type rdf:resource="http://www.w3.org/2002/07/owl#Class"/>
    <rdfs:label xml:lang="en">operational capability</rdfs:label>
    <rdfs:comment xml:lang="en">A CAPABILITY, required for planning, of those objects and types of objects that are deemed as having the ability, the training and the equipment to perform an operation.</rdfs:comment>
    <rdfs:subClassOf rdf:resource="jc3iedm_CAPABILITY.owl#CAPABILITY"/>
  </rdf:Description>
  <rdf:Description rdf:about="#OPERATIONAL-CAPABILITY_Electronic_warfare,_jamming">
    <rdfs:label xml:lang="en">electronic warfare, jamming</rdfs:label>
    <rdfs:subClassOf rdf:resource="jc3iedm_CAPABILITY.owl#OPERATIONAL-CAPABILITY"/>
    <rdfs:comment xml:lang="en">The capability to deliver radiation, re-radiation or reflection of electromagnetic energy with the object of impairing the use of electronic devices, equipment or systems being used by an enemy.</rdfs:comment>
    <rdf:type rdf:resource="http://www.w3.org/2002/07/owl#Class"/>
  </rdf:Description>
  <rdf:Description rdf:about="#OPERATIONAL-CAPABILITY_Signal,_radio_relay">
    <rdfs:label xml:lang="en">signal, radio relay</rdfs:label>
    <rdfs:subClassOf rdf:resource="jc3iedm_CAPABILITY.owl#OPERATIONAL-CAPABILITY"/>
    <rdfs:comment xml:lang="en">The capability in signal services to manage, operate and control a communications radio relay.</rdfs:comment>
    <rdf:type rdf:resource="http://www.w3.org/2002/07/owl#Class"/>
  </rdf:Description>
  <rdf:Description rdf:about="#OPERATIONAL-CAPABILITY_Close_air_support">
    <rdfs:label xml:lang="en">close air support</rdfs:label>
    <rdfs:subClassOf rdf:resource="jc3iedm_CAPABILITY.owl#OPERATIONAL-CAPABILITY"/>
    <rdfs:comment xml:lang="en">The capability to perform an air action against hostile targets which are in close proximity to friendly forces and which require detailed integration of each air mission with the fire and movement of those forces.</rdfs:comment>
    <rdf:type rdf:resource="http://www.w3.org/2002/07/owl#Class"/>
  </rdf:Description>
  <rdf:Description rdf:about="#MAINTENANCE-CAPABILITY_Shipwright">
    <rdfs:label xml:lang="en">shipwright</rdfs:label>
    <rdfs:subClassOf rdf:resource="jc3iedm_CAPABILITY.owl#MAINTENANCE-CAPABILITY"/>
    <rdfs:comment xml:lang="en">Equipment and resources for the construction, fitting and repairing the wooden parts of a docked vessel.</rdfs:comment>
    <rdf:type rdf:resource="http://www.w3.org/2002/07/owl#Class"/>
  </rdf:Description>
  <rdf:Description rdf:about="jc3iedm_CAPABILITY.owl#capability-category-code">
    <rdf:type rdf:resource="http://www.w3.org/2002/07/owl#DatatypeProperty"/>
    <rdfs:domain rdf:resource="jc3iedm_CAPABILITY.owl#CAPABILITY"/>
    <rdfs:range rdf:resource="http://www.w3.org/2001/XMLSchema#string"/>
  </rdf:Description>
  <rdf:Description rdf:about="#SUPPORT-CAPABILITY_Sewage">
    <rdfs:label xml:lang="en">sewage</rdfs:label>
    <rdfs:subClassOf rdf:resource="jc3iedm_CAPABILITY.owl#SUPPORT-CAPABILITY"/>
    <rdfs:comment xml:lang="en">The capability to provide sewage and refuse disposal.</rdfs:comment>
    <rdf:type rdf:resource="http://www.w3.org/2002/07/owl#Class"/>
  </rdf:Description>
  <rdf:Description rdf:about="#SURVEILLANCE-CAPABILITY_Not_known">
    <rdfs:label xml:lang="en">not known</rdfs:label>
    <rdfs:subClassOf rdf:resource="jc3iedm_CAPABILITY.owl#SURVEILLANCE-CAPABILITY"/>
    <rdfs:comment xml:lang="en">It is not possible to determine which value is most applicable.</rdfs:comment>
    <rdf:type rdf:resource="http://www.w3.org/2002/07/owl#Class"/>
  </rdf:Description>
  <rdf:Description rdf:about="#OPERATIONAL-CAPABILITY_Mortuary/graves_registry">
    <rdfs:label xml:lang="en">mortuary/graves registry</rdfs:label>
    <rdfs:subClassOf rdf:resource="jc3iedm_CAPABILITY.owl#OPERATIONAL-CAPABILITY"/>
    <rdfs:comment xml:lang="en">The capability to provide care and disposition of deceased personnel.</rdfs:comment>
    <rdf:type rdf:resource="http://www.w3.org/2002/07/owl#Class"/>
  </rdf:Description>
  <rdf:Description rdf:about="#OPERATIONAL-CAPABILITY_Electronic_warfare,_intercept">
    <rdfs:label xml:lang="en">electronic warfare, intercept</rdfs:label>
    <rdfs:subClassOf rdf:resource="jc3iedm_CAPABILITY.owl#OPERATIONAL-CAPABILITY"/>
    <rdfs:comment xml:lang="en">The capability to intercept intentional or unintentional radiated electromagnetic energy for the purpose of immediate threat recognition.</rdfs:comment>
    <rdf:type rdf:resource="http://www.w3.org/2002/07/owl#Class"/>
  </rdf:Description>
  <rdf:Description rdf:about="#OPERATIONAL-CAPABILITY_Finance">
    <rdfs:label xml:lang="en">finance</rdfs:label>
    <rdfs:subClassOf rdf:resource="jc3iedm_CAPABILITY.owl#OPERATIONAL-CAPABILITY"/>
    <rdfs:comment xml:lang="en">The capability to provide financial advice and guidance, support for the procurement process, providing pay and disbursing support.</rdfs:comment>
    <rdf:type rdf:resource="http://www.w3.org/2002/07/owl#Class"/>
  </rdf:Description>
  <rdf:Description rdf:about="#OPERATIONAL-CAPABILITY_Supply_(water)">
    <rdfs:label xml:lang="en">supply (water)</rdfs:label>
    <rdfs:subClassOf rdf:resource="jc3iedm_CAPABILITY.owl#OPERATIONAL-CAPABILITY"/>
    <rdfs:comment xml:lang="en">The capability to provide drinking water.</rdfs:comment>
    <rdf:type rdf:resource="http://www.w3.org/2002/07/owl#Class"/>
  </rdf:Description>
  <rdf:Description rdf:about="#MOBILITY-CAPABILITY_Water,_subsurface">
    <rdfs:label xml:lang="en">water, subsurface</rdfs:label>
    <rdfs:subClassOf rdf:resource="jc3iedm_CAPABILITY.owl#MOBILITY-CAPABILITY"/>
    <rdfs:comment xml:lang="en">The capability of a device to move on or under the water surface.</rdfs:comment>
    <rdf:type rdf:resource="http://www.w3.org/2002/07/owl#Class"/>
  </rdf:Description>
  <rdf:Description rdf:about="#FIRE-CAPABILITY_Sea_to_air">
    <rdfs:label xml:lang="en">sea to air</rdfs:label>
    <rdfs:subClassOf rdf:resource="jc3iedm_CAPABILITY.owl#FIRE-CAPABILITY"/>
    <rdfs:comment xml:lang="en">The specific value implies that a specific FIRE-CAPABILITY involves firing from a vessel to airborne targets.</rdfs:comment>
    <rdf:type rdf:resource="http://www.w3.org/2002/07/owl#Class"/>
  </rdf:Description>
  <rdf:Description rdf:about="#OPERATIONAL-CAPABILITY_Personnel_services">
    <rdfs:label xml:lang="en">personnel services</rdfs:label>
    <rdfs:subClassOf rdf:resource="jc3iedm_CAPABILITY.owl#OPERATIONAL-CAPABILITY"/>
    <rdfs:comment xml:lang="en">The capability to provide the support services needed by military and civilian personnel.</rdfs:comment>
    <rdf:type rdf:resource="http://www.w3.org/2002/07/owl#Class"/>
  </rdf:Description>
  <rdf:Description rdf:about="#SUPPORT-CAPABILITY_Water">
    <rdfs:label xml:lang="en">water</rdfs:label>
    <rdfs:subClassOf rdf:resource="jc3iedm_CAPABILITY.owl#SUPPORT-CAPABILITY"/>
    <rdfs:comment xml:lang="en">The capability to provide potable water.</rdfs:comment>
    <rdf:type rdf:resource="http://www.w3.org/2002/07/owl#Class"/>
  </rdf:Description>
  <rdf:Description rdf:about="#MOBILITY-CAPABILITY_Arctic">
    <rdfs:label xml:lang="en">arctic</rdfs:label>
    <rdfs:subClassOf rdf:resource="jc3iedm_CAPABILITY.owl#MOBILITY-CAPABILITY"/>
    <rdfs:comment xml:lang="en">The capability to move on or through ice.</rdfs:comment>
    <rdf:type rdf:resource="http://www.w3.org/2002/07/owl#Class"/>
  </rdf:Description>
  <rdf:Description rdf:about="#MOBILITY-CAPABILITY_Land,_railed">
    <rdfs:label xml:lang="en">land, railed</rdfs:label>
    <rdfs:subClassOf rdf:resource="jc3iedm_CAPABILITY.owl#MOBILITY-CAPABILITY"/>
    <rdfs:comment xml:lang="en">The capability of a device to move along rails.</rdfs:comment>
    <rdf:type rdf:resource="http://www.w3.org/2002/07/owl#Class"/>
  </rdf:Description>
  <rdf:Description rdf:about="#OPERATIONAL-CAPABILITY_Transportation,_SPOD/SPOE">
    <rdfs:label xml:lang="en">transportation, spod/spoe</rdfs:label>
    <rdfs:subClassOf rdf:resource="jc3iedm_CAPABILITY.owl#OPERATIONAL-CAPABILITY"/>
    <rdfs:comment xml:lang="en">The capability to provide transportation services at seaports where cargo or personnel arrive or depart.</rdfs:comment>
    <rdf:type rdf:resource="http://www.w3.org/2002/07/owl#Class"/>
  </rdf:Description>
  <rdf:Description rdf:about="#SURVEILLANCE-CAPABILITY_Communication">
    <rdfs:label xml:lang="en">communication</rdfs:label>
    <rdfs:subClassOf rdf:resource="jc3iedm_CAPABILITY.owl#SURVEILLANCE-CAPABILITY"/>
    <rdfs:comment xml:lang="en">The ability to gain information by exploiting communications systems.</rdfs:comment>
    <rdf:type rdf:resource="http://www.w3.org/2002/07/owl#Class"/>
  </rdf:Description>
  <rdf:Description rdf:about="#OPERATIONAL-CAPABILITY_Supply,_laundry/bath">
    <rdfs:label xml:lang="en">supply, laundry/bath</rdfs:label>
    <rdfs:subClassOf rdf:resource="jc3iedm_CAPABILITY.owl#OPERATIONAL-CAPABILITY"/>
    <rdfs:comment xml:lang="en">The capability to provide laundry and/or bath services.</rdfs:comment>
    <rdf:type rdf:resource="http://www.w3.org/2002/07/owl#Class"/>
  </rdf:Description>
  <rdf:Description rdf:about="#OPERATIONAL-CAPABILITY_Attack">
    <rdfs:label xml:lang="en">attack</rdfs:label>
    <rdfs:subClassOf rdf:resource="jc3iedm_CAPABILITY.owl#OPERATIONAL-CAPABILITY"/>
    <rdfs:comment xml:lang="en">The capability to perform an offensive mission.</rdfs:comment>
    <rdf:type rdf:resource="http://www.w3.org/2002/07/owl#Class"/>
  </rdf:Description>
  <rdf:Description rdf:about="#OPERATIONAL-CAPABILITY_Military_intelligence,_tactical_exploitation">
    <rdfs:label xml:lang="en">military intelligence, tactical exploitation</rdfs:label>
    <rdfs:subClassOf rdf:resource="jc3iedm_CAPABILITY.owl#OPERATIONAL-CAPABILITY"/>
    <rdfs:comment xml:lang="en">The capability to use information required for the planning and conducting tactical operations.</rdfs:comment>
    <rdf:type rdf:resource="http://www.w3.org/2002/07/owl#Class"/>
  </rdf:Description>
  <rdf:Description rdf:about="#OPERATIONAL-CAPABILITY_Air_to_ground">
    <rdfs:label xml:lang="en">air to ground</rdfs:label>
    <rdfs:subClassOf rdf:resource="jc3iedm_CAPABILITY.owl#OPERATIONAL-CAPABILITY"/>
    <rdfs:comment xml:lang="en">The capability to perform air to ground operations.</rdfs:comment>
    <rdf:type rdf:resource="http://www.w3.org/2002/07/owl#Class"/>
  </rdf:Description>
  <rdf:Description rdf:about="#MOBILITY-CAPABILITY_Land,_wheeled">
    <rdfs:label xml:lang="en">land, wheeled</rdfs:label>
    <rdfs:subClassOf rdf:resource="jc3iedm_CAPABILITY.owl#MOBILITY-CAPABILITY"/>
    <rdfs:comment xml:lang="en">The capability of a device to move on wheels.</rdfs:comment>
    <rdf:type rdf:resource="http://www.w3.org/2002/07/owl#Class"/>
  </rdf:Description>
  <rdf:Description rdf:about="#OPERATIONAL-CAPABILITY_Railway">
    <rdfs:label xml:lang="en">railway</rdfs:label>
    <rdfs:subClassOf rdf:resource="jc3iedm_CAPABILITY.owl#OPERATIONAL-CAPABILITY"/>
    <rdfs:comment xml:lang="en">The capability to provide rail services.</rdfs:comment>
    <rdf:type rdf:resource="http://www.w3.org/2002/07/owl#Class"/>
  </rdf:Description>
  <rdf:Description rdf:about="#OPERATIONAL-CAPABILITY_Theatre_missile_defence">
    <rdfs:label xml:lang="en">theatre missile defence</rdfs:label>
    <rdfs:subClassOf rdf:resource="jc3iedm_CAPABILITY.owl#OPERATIONAL-CAPABILITY"/>
    <rdfs:comment xml:lang="en">The capability to manage, operate and maintain theatre missile defence assets.</rdfs:comment>
    <rdf:type rdf:resource="http://www.w3.org/2002/07/owl#Class"/>
  </rdf:Description>
  <rdf:Description rdf:about="#SUPPORT-CAPABILITY_Supply_(class_II)">
    <rdfs:label xml:lang="en">supply (class ii)</rdfs:label>
    <rdfs:subClassOf rdf:resource="jc3iedm_CAPABILITY.owl#SUPPORT-CAPABILITY"/>
    <rdfs:comment xml:lang="en">The capability to provide materiel (supplies for which allowances are established by tables of organisation and equipment).</rdfs:comment>
    <rdf:type rdf:resource="http://www.w3.org/2002/07/owl#Class"/>
  </rdf:Description>
  <rdf:Description rdf:about="#SUPPORT-CAPABILITY_Infrastructure_support">
    <rdfs:label xml:lang="en">infrastructure support</rdfs:label>
    <rdfs:subClassOf rdf:resource="jc3iedm_CAPABILITY.owl#SUPPORT-CAPABILITY"/>
    <rdfs:comment xml:lang="en">The capability to provide infrastructure support.</rdfs:comment>
    <rdf:type rdf:resource="http://www.w3.org/2002/07/owl#Class"/>
  </rdf:Description>
  <rdf:Description rdf:about="#OPERATIONAL-CAPABILITY_C2">
    <rdfs:label xml:lang="en">c2</rdfs:label>
    <rdfs:subClassOf rdf:resource="jc3iedm_CAPABILITY.owl#OPERATIONAL-CAPABILITY"/>
    <rdfs:comment xml:lang="en">The capability to exercise the authority, responsibilities and activities of military commanders in direction and co-ordination or military forces and the implementation of orders related to the execution of operations.</rdfs:comment>
    <rdf:type rdf:resource="http://www.w3.org/2002/07/owl#Class"/>
  </rdf:Description>
  <rdf:Description rdf:about="#SUPPORT-CAPABILITY_Compressed_air">
    <rdfs:label xml:lang="en">compressed air</rdfs:label>
    <rdfs:subClassOf rdf:resource="jc3iedm_CAPABILITY.owl#SUPPORT-CAPABILITY"/>
    <rdfs:comment xml:lang="en">The capability to provide air at more than atmospheric pressure - often used to power mechanical devices or to provide a portable supply of oxygen.</rdfs:comment>
    <rdf:type rdf:resource="http://www.w3.org/2002/07/owl#Class"/>
  </rdf:Description>
  <rdf:Description rdf:about="#OPERATIONAL-CAPABILITY_Electronic_warfare">
    <rdfs:label xml:lang="en">electronic warfare</rdfs:label>
    <rdfs:subClassOf rdf:resource="jc3iedm_CAPABILITY.owl#OPERATIONAL-CAPABILITY"/>
    <rdfs:comment xml:lang="en">The capability involving the use of electromagnetic energy to determine, exploit, reduce, or prevent hostile use of the electromagnetic spectrum and action to retain its effective use by friendly forces.</rdfs:comment>
    <rdf:type rdf:resource="http://www.w3.org/2002/07/owl#Class"/>
  </rdf:Description>
  <rdf:Description rdf:about="#OPERATIONAL-CAPABILITY_Electronic_ranging">
    <rdfs:label xml:lang="en">electronic ranging</rdfs:label>
    <rdfs:subClassOf rdf:resource="jc3iedm_CAPABILITY.owl#OPERATIONAL-CAPABILITY"/>
    <rdfs:comment xml:lang="en">The capability to establish target distance electronically.</rdfs:comment>
    <rdf:type rdf:resource="http://www.w3.org/2002/07/owl#Class"/>
  </rdf:Description>
  <rdf:Description rdf:about="#SURVEILLANCE-CAPABILITY_Signal">
    <rdfs:label xml:lang="en">signal</rdfs:label>
    <rdfs:subClassOf rdf:resource="jc3iedm_CAPABILITY.owl#SURVEILLANCE-CAPABILITY"/>
    <rdfs:comment xml:lang="en">The ability to gain information from exploiting EMS (not imagery) systems.</rdfs:comment>
    <rdf:type rdf:resource="http://www.w3.org/2002/07/owl#Class"/>
  </rdf:Description>
  <rdf:Description rdf:about="#OPERATIONAL-CAPABILITY_Counter_intelligence">
    <rdfs:label xml:lang="en">counter intelligence</rdfs:label>
    <rdfs:subClassOf rdf:resource="jc3iedm_CAPABILITY.owl#OPERATIONAL-CAPABILITY"/>
    <rdfs:comment xml:lang="en">The capability to conduct activities that are concerned with identifying and counteracting the threat to security posed by hostile intelligence services or organisations, or by individuals engaged in espionage, sabotage, subversion or terrorism.</rdfs:comment>
    <rdf:type rdf:resource="http://www.w3.org/2002/07/owl#Class"/>
  </rdf:Description>
  <rdf:Description rdf:about="#OPERATIONAL-CAPABILITY_Air_assault">
    <rdfs:label xml:lang="en">air assault</rdfs:label>
    <rdfs:subClassOf rdf:resource="jc3iedm_CAPABILITY.owl#OPERATIONAL-CAPABILITY"/>
    <rdfs:comment xml:lang="en">The capability to perform a mission involving total integration of helicopter assets in their ground or air roles.</rdfs:comment>
    <rdf:type rdf:resource="http://www.w3.org/2002/07/owl#Class"/>
  </rdf:Description>
  <rdf:Description rdf:about="#OPERATIONAL-CAPABILITY_Target_acquisition,_radar">
    <rdfs:label xml:lang="en">target acquisition, radar</rdfs:label>
    <rdfs:subClassOf rdf:resource="jc3iedm_CAPABILITY.owl#OPERATIONAL-CAPABILITY"/>
    <rdfs:comment xml:lang="en">The capability to manage, operate and maintain radar target acquisition assets.</rdfs:comment>
    <rdf:type rdf:resource="http://www.w3.org/2002/07/owl#Class"/>
  </rdf:Description>
  <rdf:Description rdf:about="#OPERATIONAL-CAPABILITY_Airborne">
    <rdfs:label xml:lang="en">airborne</rdfs:label>
    <rdfs:subClassOf rdf:resource="jc3iedm_CAPABILITY.owl#OPERATIONAL-CAPABILITY"/>
    <rdfs:comment xml:lang="en">The capability to carry out operations, either by paradrop or air landing, following an air movement.</rdfs:comment>
    <rdf:type rdf:resource="http://www.w3.org/2002/07/owl#Class"/>
  </rdf:Description>
  <rdf:Description rdf:about="#OPERATIONAL-CAPABILITY_Legal">
    <rdfs:label xml:lang="en">legal</rdfs:label>
    <rdfs:subClassOf rdf:resource="jc3iedm_CAPABILITY.owl#OPERATIONAL-CAPABILITY"/>
    <rdfs:comment xml:lang="en">The capability to provide legal services.</rdfs:comment>
    <rdf:type rdf:resource="http://www.w3.org/2002/07/owl#Class"/>
  </rdf:Description>
  <rdf:Description rdf:about="jc3iedm_CAPABILITY.owl#SURVEILLANCE-CAPABILITY">
    <rdf:type rdf:resource="http://www.w3.org/2002/07/owl#Class"/>
    <rdfs:label xml:lang="en">surveillance capability</rdfs:label>
    <rdfs:comment xml:lang="en">A CAPABILITY, required for planning, of those FACILITYs, MATERIELs, ORGANISATIONs and PERSONs or FACILITY-TYPEs, EQUIPMENT-TYPEs, ORGANISATION-TYPEs and PERSON-TYPEs that are deemed as having the nominal ability to observe aerospace, surface or subsurface areas, places, persons, or things, by visual, aural, electronic, photographic or other means.</rdfs:comment>
    <rdfs:subClassOf rdf:resource="jc3iedm_CAPABILITY.owl#CAPABILITY"/>
  </rdf:Description>
  <rdf:Description rdf:about="#OPERATIONAL-CAPABILITY_Civilian_law_enforcement">
    <rdfs:label xml:lang="en">civilian law enforcement</rdfs:label>
    <rdfs:subClassOf rdf:resource="jc3iedm_CAPABILITY.owl#OPERATIONAL-CAPABILITY"/>
    <rdfs:comment xml:lang="en">The capability to conduct civilian law enforcement operations.</rdfs:comment>
    <rdf:type rdf:resource="http://www.w3.org/2002/07/owl#Class"/>
  </rdf:Description>
  <rdf:Description rdf:about="#MOBILITY-CAPABILITY_Airborne">
    <rdfs:label xml:lang="en">airborne</rdfs:label>
    <rdfs:subClassOf rdf:resource="jc3iedm_CAPABILITY.owl#MOBILITY-CAPABILITY"/>
    <rdfs:comment xml:lang="en">The capability to be employed, following transport by air, in an assault debarkation either by parachuting or touchdown.</rdfs:comment>
    <rdf:type rdf:resource="http://www.w3.org/2002/07/owl#Class"/>
  </rdf:Description>
  <rdf:Description rdf:about="#OPERATIONAL-CAPABILITY_Search_and_rescue">
    <rdfs:label xml:lang="en">search and rescue</rdfs:label>
    <rdfs:subClassOf rdf:resource="jc3iedm_CAPABILITY.owl#OPERATIONAL-CAPABILITY"/>
    <rdfs:comment xml:lang="en">The capability to use aircraft, surface craft, submarines, specialised rescue teams, and equipment to search for and rescue personnel in distress on land or sea.</rdfs:comment>
    <rdf:type rdf:resource="http://www.w3.org/2002/07/owl#Class"/>
  </rdf:Description>
  <rdf:Description rdf:about="#OPERATIONAL-CAPABILITY_Maintenance,_ordnance">
    <rdfs:label xml:lang="en">maintenance, ordnance</rdfs:label>
    <rdfs:subClassOf rdf:resource="jc3iedm_CAPABILITY.owl#OPERATIONAL-CAPABILITY"/>
    <rdfs:comment xml:lang="en">The capability to maintain ordnance (ammunition) in or to restore it to a specified condition.</rdfs:comment>
    <rdf:type rdf:resource="http://www.w3.org/2002/07/owl#Class"/>
  </rdf:Description>
  <rdf:Description rdf:about="#MAINTENANCE-CAPABILITY_Steam">
    <rdfs:label xml:lang="en">steam</rdfs:label>
    <rdfs:subClassOf rdf:resource="jc3iedm_CAPABILITY.owl#MAINTENANCE-CAPABILITY"/>
    <rdfs:comment xml:lang="en">The specific MAINTENANCE-CAPABILITY determines the ability to provide steam repair.</rdfs:comment>
    <rdf:type rdf:resource="http://www.w3.org/2002/07/owl#Class"/>
  </rdf:Description>
  <rdf:Description rdf:about="#FIRE-CAPABILITY_Ground_to_sea">
    <rdfs:label xml:lang="en">ground to sea</rdfs:label>
    <rdfs:subClassOf rdf:resource="jc3iedm_CAPABILITY.owl#FIRE-CAPABILITY"/>
    <rdfs:comment xml:lang="en">The specific value implies that a specific FIRE-CAPABILITY involves firing from the ground to targets at sea.</rdfs:comment>
    <rdf:type rdf:resource="http://www.w3.org/2002/07/owl#Class"/>
  </rdf:Description>
  <rdf:Description rdf:about="#SURVEILLANCE-CAPABILITY_Not_otherwise_specified">
    <rdfs:label xml:lang="en">not otherwise specified</rdfs:label>
    <rdfs:subClassOf rdf:resource="jc3iedm_CAPABILITY.owl#SURVEILLANCE-CAPABILITY"/>
    <rdfs:comment xml:lang="en">The appropriate value is not in the set of specified values.</rdfs:comment>
    <rdf:type rdf:resource="http://www.w3.org/2002/07/owl#Class"/>
  </rdf:Description>
  <rdf:Description rdf:about="#OPERATIONAL-CAPABILITY_Surveillance">
    <rdfs:label xml:lang="en">surveillance</rdfs:label>
    <rdfs:subClassOf rdf:resource="jc3iedm_CAPABILITY.owl#OPERATIONAL-CAPABILITY"/>
    <rdfs:comment xml:lang="en">The capability to perform systematic observation of aerospace, surface or subsurface areas, places, persons, or things by visual, aural, electronic, photographic, or other means.</rdfs:comment>
    <rdf:type rdf:resource="http://www.w3.org/2002/07/owl#Class"/>
  </rdf:Description>
  <rdf:Description rdf:about="#FIRE-CAPABILITY_Air_to_ground">
    <rdfs:label xml:lang="en">air to ground</rdfs:label>
    <rdfs:subClassOf rdf:resource="jc3iedm_CAPABILITY.owl#FIRE-CAPABILITY"/>
    <rdfs:comment xml:lang="en">The specific value implies that a specific FIRE-CAPABILITY involves firing from aircraft at targets on the ground.</rdfs:comment>
    <rdf:type rdf:resource="http://www.w3.org/2002/07/owl#Class"/>
  </rdf:Description>
  <rdf:Description rdf:about="#MOBILITY-CAPABILITY_Military_load_classification">
    <rdfs:label xml:lang="en">military load classification</rdfs:label>
    <rdfs:subClassOf rdf:resource="jc3iedm_CAPABILITY.owl#MOBILITY-CAPABILITY"/>
    <rdfs:comment xml:lang="en">The characteristics, required for planning, of those CONTROL-FEATUREs, FACILITYs and MATERIELs or CONTROL-FEATURE-TYPEs, FACILITY-TYPEs and EQUIPMENT-TYPEs, and ORGANISATION-TYPEs that represents the standard system in which a route, bridge or raft is assigned class number(s) representing the load it can carry. Vehicles are also assigned number(s) indicating the minimum class of route, bridge or raft they are authorized to use.</rdfs:comment>
    <rdf:type rdf:resource="http://www.w3.org/2002/07/owl#Class"/>
  </rdf:Description>
  <rdf:Description rdf:about="#SUPPORT-CAPABILITY_Laundry">
    <rdfs:label xml:lang="en">laundry</rdfs:label>
    <rdfs:subClassOf rdf:resource="jc3iedm_CAPABILITY.owl#SUPPORT-CAPABILITY"/>
    <rdfs:comment xml:lang="en">The capability to provide laundry services.</rdfs:comment>
    <rdf:type rdf:resource="http://www.w3.org/2002/07/owl#Class"/>
  </rdf:Description>
  <rdf:Description rdf:about="#OPERATIONAL-CAPABILITY_Surveillance,_meteorological">
    <rdfs:label xml:lang="en">surveillance, meteorological</rdfs:label>
    <rdfs:subClassOf rdf:resource="jc3iedm_CAPABILITY.owl#OPERATIONAL-CAPABILITY"/>
    <rdfs:comment xml:lang="en">The capability to perform systematic observation of meteorological conditions.</rdfs:comment>
    <rdf:type rdf:resource="http://www.w3.org/2002/07/owl#Class"/>
  </rdf:Description>
  <rdf:Description rdf:about="jc3iedm_CAPABILITY.owl#MAINTENANCE-CAPABILITY">
    <rdf:type rdf:resource="http://www.w3.org/2002/07/owl#Class"/>
    <rdfs:label xml:lang="en">maintenance capability</rdfs:label>
    <rdfs:comment xml:lang="en">A CAPABILITY, required for planning, of those FACILITYs, MATERIELs, ORGANISATIONs and PERSONs or FACILITY-TYPEs, EQUIPMENT-TYPEs, ORGANISATION-TYPEs, and PERSON-TYPEs that are deemed as having the ability to provide a range of activities required to restore or maintain operational usage.</rdfs:comment>
    <rdfs:subClassOf rdf:resource="jc3iedm_CAPABILITY.owl#CAPABILITY"/>
  </rdf:Description>
  <rdf:Description rdf:about="#MOBILITY-CAPABILITY_Water,_lake">
    <rdfs:label xml:lang="en">water, lake</rdfs:label>
    <rdfs:subClassOf rdf:resource="jc3iedm_CAPABILITY.owl#MOBILITY-CAPABILITY"/>
    <rdfs:comment xml:lang="en">The capability of a device to navigate lakes.</rdfs:comment>
    <rdf:type rdf:resource="http://www.w3.org/2002/07/owl#Class"/>
  </rdf:Description>
  <rdf:Description rdf:about="#FIRE-CAPABILITY_Sea_to_sea">
    <rdfs:label xml:lang="en">sea to sea</rdfs:label>
    <rdfs:subClassOf rdf:resource="jc3iedm_CAPABILITY.owl#FIRE-CAPABILITY"/>
    <rdfs:comment xml:lang="en">The specific value implies that a specific FIRE-CAPABILITY involves firing from a vessel to targets at sea.</rdfs:comment>
    <rdf:type rdf:resource="http://www.w3.org/2002/07/owl#Class"/>
  </rdf:Description>
  <rdf:Description rdf:about="#OPERATIONAL-CAPABILITY_NBC,_chemical,_smoke">
    <rdfs:label xml:lang="en">nbc, chemical, smoke</rdfs:label>
    <rdfs:subClassOf rdf:resource="jc3iedm_CAPABILITY.owl#OPERATIONAL-CAPABILITY"/>
    <rdfs:comment xml:lang="en">The capability to employ chemical materiel released as a cloud of smoke or defence against such employment.</rdfs:comment>
    <rdf:type rdf:resource="http://www.w3.org/2002/07/owl#Class"/>
  </rdf:Description>
  <rdf:Description rdf:about="#OPERATIONAL-CAPABILITY_Peace_support">
    <rdfs:label xml:lang="en">peace support</rdfs:label>
    <rdfs:subClassOf rdf:resource="jc3iedm_CAPABILITY.owl#OPERATIONAL-CAPABILITY"/>
    <rdfs:comment xml:lang="en">The capability to conduct multi-functional operations involving military forces and diplomatic and humanitarian agencies. The operations are designed to achieve humanitarian goals or a long term peace settlement.</rdfs:comment>
    <rdf:type rdf:resource="http://www.w3.org/2002/07/owl#Class"/>
  </rdf:Description>
  <rdf:Description rdf:about="#FIRE-CAPABILITY_Air_to_sea">
    <rdfs:label xml:lang="en">air to sea</rdfs:label>
    <rdfs:subClassOf rdf:resource="jc3iedm_CAPABILITY.owl#FIRE-CAPABILITY"/>
    <rdfs:comment xml:lang="en">The specific value implies that a specific FIRE-CAPABILITY involves firing from aircraft at targets at sea.</rdfs:comment>
    <rdf:type rdf:resource="http://www.w3.org/2002/07/owl#Class"/>
  </rdf:Description>
  <rdf:Description rdf:about="#MOBILITY-CAPABILITY_Water,_river">
    <rdfs:label xml:lang="en">water, river</rdfs:label>
    <rdfs:subClassOf rdf:resource="jc3iedm_CAPABILITY.owl#MOBILITY-CAPABILITY"/>
    <rdfs:comment xml:lang="en">The capability of a device to navigate rivers.</rdfs:comment>
    <rdf:type rdf:resource="http://www.w3.org/2002/07/owl#Class"/>
  </rdf:Description>
  <rdf:Description rdf:about="jc3iedm_CAPABILITY.owl#capability-day-night-code">
    <rdf:type rdf:resource="http://www.w3.org/2002/07/owl#DatatypeProperty"/>
    <rdfs:domain rdf:resource="jc3iedm_CAPABILITY.owl#CAPABILITY"/>
    <rdfs:range rdf:resource="http://www.w3.org/2001/XMLSchema#string"/>
  </rdf:Description>
  <rdf:Description rdf:about="#ENGINEERING-CAPABILITY_Demolition">
    <rdfs:label xml:lang="en">demolition</rdfs:label>
    <rdfs:subClassOf rdf:resource="jc3iedm_CAPABILITY.owl#ENGINEERING-CAPABILITY"/>
    <rdfs:comment xml:lang="en">The action or process of demolishing or being demolished.</rdfs:comment>
    <rdf:type rdf:resource="http://www.w3.org/2002/07/owl#Class"/>
  </rdf:Description>
  <rdf:Description rdf:about="#MOBILITY-CAPABILITY_Land,_towed">
    <rdfs:label xml:lang="en">land, towed</rdfs:label>
    <rdfs:subClassOf rdf:resource="jc3iedm_CAPABILITY.owl#MOBILITY-CAPABILITY"/>
    <rdfs:comment xml:lang="en">The capability of a device to move by means of external propulsion (mechanical or animal).</rdfs:comment>
    <rdf:type rdf:resource="http://www.w3.org/2002/07/owl#Class"/>
  </rdf:Description>
  <rdf:Description rdf:about="#MOBILITY-CAPABILITY_Water,_bay">
    <rdfs:label xml:lang="en">water, bay</rdfs:label>
    <rdfs:subClassOf rdf:resource="jc3iedm_CAPABILITY.owl#MOBILITY-CAPABILITY"/>
    <rdfs:comment xml:lang="en">The capability of a device to navigate in bays.</rdfs:comment>
    <rdf:type rdf:resource="http://www.w3.org/2002/07/owl#Class"/>
  </rdf:Description>
  <rdf:Description rdf:about="#OPERATIONAL-CAPABILITY_NBC,_chemical">
    <rdfs:label xml:lang="en">nbc, chemical</rdfs:label>
    <rdfs:subClassOf rdf:resource="jc3iedm_CAPABILITY.owl#OPERATIONAL-CAPABILITY"/>
    <rdfs:comment xml:lang="en">The capability to employ chemical materiel to kill, injure, or incapacitate for a significant period of time, man or animals, and deny or hinder the use of areas, facilities or materiel; or defence against such employment.</rdfs:comment>
    <rdf:type rdf:resource="http://www.w3.org/2002/07/owl#Class"/>
  </rdf:Description>
  <rdf:Description rdf:about="#OPERATIONAL-CAPABILITY_Transportation,_movement_control">
    <rdfs:label xml:lang="en">transportation, movement control</rdfs:label>
    <rdfs:subClassOf rdf:resource="jc3iedm_CAPABILITY.owl#OPERATIONAL-CAPABILITY"/>
    <rdfs:comment xml:lang="en">The capability to provide planning, routing, scheduling and control of personnel and freight movements over lines of communication.</rdfs:comment>
    <rdf:type rdf:resource="http://www.w3.org/2002/07/owl#Class"/>
  </rdf:Description>
  <rdf:Description rdf:about="#OPERATIONAL-CAPABILITY_Supply_(class_IV)">
    <rdfs:label xml:lang="en">supply (class iv)</rdfs:label>
    <rdfs:subClassOf rdf:resource="jc3iedm_CAPABILITY.owl#OPERATIONAL-CAPABILITY"/>
    <rdfs:comment xml:lang="en">The capability to provide construction materials.</rdfs:comment>
    <rdf:type rdf:resource="http://www.w3.org/2002/07/owl#Class"/>
  </rdf:Description>
  <rdf:Description rdf:about="#MAINTENANCE-CAPABILITY_Paint_shop">
    <rdfs:label xml:lang="en">paint shop</rdfs:label>
    <rdfs:subClassOf rdf:resource="jc3iedm_CAPABILITY.owl#MAINTENANCE-CAPABILITY"/>
    <rdfs:comment xml:lang="en">Equipment and resources for painting any part of a docked vessel.</rdfs:comment>
    <rdf:type rdf:resource="http://www.w3.org/2002/07/owl#Class"/>
  </rdf:Description>
  <rdf:Description rdf:about="jc3iedm_CAPABILITY.owl#capability-unit-of-measure-code">
    <rdf:type rdf:resource="http://www.w3.org/2002/07/owl#DatatypeProperty"/>
    <rdfs:domain rdf:resource="jc3iedm_CAPABILITY.owl#CAPABILITY"/>
    <rdfs:range rdf:resource="http://www.w3.org/2001/XMLSchema#string"/>
  </rdf:Description>
  <rdf:Description rdf:about="#MAINTENANCE-CAPABILITY_Navigational_equipment">
    <rdfs:label xml:lang="en">navigational equipment</rdfs:label>
    <rdfs:subClassOf rdf:resource="jc3iedm_CAPABILITY.owl#MAINTENANCE-CAPABILITY"/>
    <rdfs:comment xml:lang="en">The specific MAINTENANCE-CAPABILITY determines the ability to provide navigational equipment repair.</rdfs:comment>
    <rdf:type rdf:resource="http://www.w3.org/2002/07/owl#Class"/>
  </rdf:Description>
  <rdf:Description rdf:about="#MOBILITY-CAPABILITY_Amphibious">
    <rdfs:label xml:lang="en">amphibious</rdfs:label>
    <rdfs:subClassOf rdf:resource="jc3iedm_CAPABILITY.owl#MOBILITY-CAPABILITY"/>
    <rdfs:comment xml:lang="en">The capability of a device to operate both on land and in water.</rdfs:comment>
    <rdf:type rdf:resource="http://www.w3.org/2002/07/owl#Class"/>
  </rdf:Description>
  <rdf:Description rdf:about="#OPERATIONAL-CAPABILITY_Recovery">
    <rdfs:label xml:lang="en">recovery</rdfs:label>
    <rdfs:subClassOf rdf:resource="jc3iedm_CAPABILITY.owl#OPERATIONAL-CAPABILITY"/>
    <rdfs:comment xml:lang="en">The capability to contact, protect and extract personnel, small groups or units, or materiel.</rdfs:comment>
    <rdf:type rdf:resource="http://www.w3.org/2002/07/owl#Class"/>
  </rdf:Description>
  <rdf:Description rdf:about="#SUPPORT-CAPABILITY_Electrical">
    <rdfs:label xml:lang="en">electrical</rdfs:label>
    <rdfs:subClassOf rdf:resource="jc3iedm_CAPABILITY.owl#SUPPORT-CAPABILITY"/>
    <rdfs:comment xml:lang="en">The capability to provide electrical power.</rdfs:comment>
    <rdf:type rdf:resource="http://www.w3.org/2002/07/owl#Class"/>
  </rdf:Description>
  <rdf:Description rdf:about="jc3iedm_CAPABILITY.owl#STORAGE-CAPABILITY">
    <rdf:type rdf:resource="http://www.w3.org/2002/07/owl#Class"/>
    <rdfs:label xml:lang="en">storage capability</rdfs:label>
    <rdfs:comment xml:lang="en">A CAPABILITY, required for planning, of those FACILITYs and MATERIELs or EQUIPMENT-TYPEs and FACILITY-TYPEs that are deemed as having the ability to hold a specific OBJECT-TYPE.</rdfs:comment>
    <rdfs:subClassOf rdf:resource="jc3iedm_CAPABILITY.owl#CAPABILITY"/>
  </rdf:Description>
  <rdf:Description rdf:about="#SUPPORT-CAPABILITY_Supply_(class_IV)">
    <rdfs:label xml:lang="en">supply (class iv)</rdfs:label>
    <rdfs:subClassOf rdf:resource="jc3iedm_CAPABILITY.owl#SUPPORT-CAPABILITY"/>
    <rdfs:comment xml:lang="en">The capability to provide construction materials (supplies for which initial issue allowances are not prescribed by approved issue tables).</rdfs:comment>
    <rdf:type rdf:resource="http://www.w3.org/2002/07/owl#Class"/>
  </rdf:Description>
  <rdf:Description rdf:about="#OPERATIONAL-CAPABILITY_Supply_(class_I)">
    <rdfs:label xml:lang="en">supply (class i)</rdfs:label>
    <rdfs:subClassOf rdf:resource="jc3iedm_CAPABILITY.owl#OPERATIONAL-CAPABILITY"/>
    <rdfs:comment xml:lang="en">The capability to provide combat/fresh rations, water and personal, health and welfare items.</rdfs:comment>
    <rdf:type rdf:resource="http://www.w3.org/2002/07/owl#Class"/>
  </rdf:Description>
  <rdf:Description rdf:about="#OPERATIONAL-CAPABILITY_Command_operations">
    <rdfs:label xml:lang="en">command operations</rdfs:label>
    <rdfs:subClassOf rdf:resource="jc3iedm_CAPABILITY.owl#OPERATIONAL-CAPABILITY"/>
    <rdfs:comment xml:lang="en">No definition provided in APP-6A.</rdfs:comment>
    <rdf:type rdf:resource="http://www.w3.org/2002/07/owl#Class"/>
  </rdf:Description>
  <rdf:Description rdf:about="#OPERATIONAL-CAPABILITY_Maintenance,_electro-optical">
    <rdfs:label xml:lang="en">maintenance, electro optical</rdfs:label>
    <rdfs:subClassOf rdf:resource="jc3iedm_CAPABILITY.owl#OPERATIONAL-CAPABILITY"/>
    <rdfs:comment xml:lang="en">The capability to maintain electro-optical materiel in or to restore it to a specified condition.</rdfs:comment>
    <rdf:type rdf:resource="http://www.w3.org/2002/07/owl#Class"/>
  </rdf:Description>
  <rdf:Description rdf:about="jc3iedm_CAPABILITY.owl#MOBILITY-CAPABILITY">
    <rdf:type rdf:resource="http://www.w3.org/2002/07/owl#Class"/>
    <rdfs:label xml:lang="en">mobility capability</rdfs:label>
    <rdfs:comment xml:lang="en">A CAPABILITY, required for planning, of those FACILITYs, MATERIELs, ORGANISATIONs and PERSONs or FACILITY-TYPEs, EQUIPMENT-TYPEs, ORGANISATION-TYPEs, and PERSON-TYPEs that are deemed as having the nominal ability to move in space, air, on water, under water, or over a specific type of terrain.</rdfs:comment>
    <rdfs:subClassOf rdf:resource="jc3iedm_CAPABILITY.owl#CAPABILITY"/>
  </rdf:Description>
  <rdf:Description rdf:about="#MOBILITY-CAPABILITY_Water,_sea">
    <rdfs:label xml:lang="en">water, sea</rdfs:label>
    <rdfs:subClassOf rdf:resource="jc3iedm_CAPABILITY.owl#MOBILITY-CAPABILITY"/>
    <rdfs:comment xml:lang="en">The capability of a device to navigate seas.</rdfs:comment>
    <rdf:type rdf:resource="http://www.w3.org/2002/07/owl#Class"/>
  </rdf:Description>
  <rdf:Description rdf:about="#MAINTENANCE-CAPABILITY_Tank_cleaning">
    <rdfs:label xml:lang="en">tank cleaning</rdfs:label>
    <rdfs:subClassOf rdf:resource="jc3iedm_CAPABILITY.owl#MAINTENANCE-CAPABILITY"/>
    <rdfs:comment xml:lang="en">Equipment and resources for the removal of any trace of the original contents of any tank belonging to a docked vessel. Removal is often carried out by means of a high-pressure water jet.</rdfs:comment>
    <rdf:type rdf:resource="http://www.w3.org/2002/07/owl#Class"/>
  </rdf:Description>
  <rdf:Description rdf:about="#SUPPORT-CAPABILITY_Medical">
    <rdfs:label xml:lang="en">medical</rdfs:label>
    <rdfs:subClassOf rdf:resource="jc3iedm_CAPABILITY.owl#SUPPORT-CAPABILITY"/>
    <rdfs:comment xml:lang="en">The capability to treat people for illnesses and injuries.</rdfs:comment>
    <rdf:type rdf:resource="http://www.w3.org/2002/07/owl#Class"/>
  </rdf:Description>
  <rdf:Description rdf:about="#OPERATIONAL-CAPABILITY_Signal,_node,_small_extension">
    <rdfs:label xml:lang="en">signal, node, small extension</rdfs:label>
    <rdfs:subClassOf rdf:resource="jc3iedm_CAPABILITY.owl#OPERATIONAL-CAPABILITY"/>
    <rdfs:comment xml:lang="en">The capability in signal services to manage, operate and control a communications small extension node.</rdfs:comment>
    <rdf:type rdf:resource="http://www.w3.org/2002/07/owl#Class"/>
  </rdf:Description>
  <rdf:Description rdf:about="#MOBILITY-CAPABILITY_Road_march">
    <rdfs:label xml:lang="en">road march</rdfs:label>
    <rdfs:subClassOf rdf:resource="jc3iedm_CAPABILITY.owl#MOBILITY-CAPABILITY"/>
    <rdfs:comment xml:lang="en">The capability of a formation moving on a road.</rdfs:comment>
    <rdf:type rdf:resource="http://www.w3.org/2002/07/owl#Class"/>
  </rdf:Description>
  <rdf:Description rdf:about="jc3iedm_CAPABILITY.owl#SUPPORT-CAPABILITY">
    <rdf:type rdf:resource="http://www.w3.org/2002/07/owl#Class"/>
    <rdfs:label xml:lang="en">support capability</rdfs:label>
    <rdfs:comment xml:lang="en">A CAPABILITY, required for planning, of those FACILITYs, MATERIELs and ORGANISATIONs or FACILITY-TYPEs, EQUIPMENT-TYPEs and ORGANISATION-TYPEs that are deemed as having the ability to provide supplies or services.</rdfs:comment>
    <rdfs:subClassOf rdf:resource="jc3iedm_CAPABILITY.owl#CAPABILITY"/>
  </rdf:Description>
  <rdf:Description rdf:about="#OPERATIONAL-CAPABILITY_Water_purification">
    <rdfs:label xml:lang="en">water purification</rdfs:label>
    <rdfs:subClassOf rdf:resource="jc3iedm_CAPABILITY.owl#OPERATIONAL-CAPABILITY"/>
    <rdfs:comment xml:lang="en">The capability to provide clean potable drinking/bathing water.</rdfs:comment>
    <rdf:type rdf:resource="http://www.w3.org/2002/07/owl#Class"/>
  </rdf:Description>
  <rdf:Description rdf:about="#OPERATIONAL-CAPABILITY_Supply_(class_II)">
    <rdfs:label xml:lang="en">supply (class ii)</rdfs:label>
    <rdfs:subClassOf rdf:resource="jc3iedm_CAPABILITY.owl#OPERATIONAL-CAPABILITY"/>
    <rdfs:comment xml:lang="en">The capability to provide materiel.</rdfs:comment>
    <rdf:type rdf:resource="http://www.w3.org/2002/07/owl#Class"/>
  </rdf:Description>
  <rdf:Description rdf:about="#MAINTENANCE-CAPABILITY_Shotblast">
    <rdfs:label xml:lang="en">shotblast</rdfs:label>
    <rdfs:subClassOf rdf:resource="jc3iedm_CAPABILITY.owl#MAINTENANCE-CAPABILITY"/>
    <rdfs:comment xml:lang="en">Equipment and resources for the cleaning of metal, belonging to a docked vessel, by the impact of a stream of shot (lead pellets).</rdfs:comment>
    <rdf:type rdf:resource="http://www.w3.org/2002/07/owl#Class"/>
  </rdf:Description>
  <rdf:Description rdf:about="#OPERATIONAL-CAPABILITY_Public_affairs,_joint_information">
    <rdfs:label xml:lang="en">public affairs, joint information</rdfs:label>
    <rdfs:subClassOf rdf:resource="jc3iedm_CAPABILITY.owl#OPERATIONAL-CAPABILITY"/>
    <rdfs:comment xml:lang="en">The capability to provide those public information, command information, and community relations activities directed towards the general public in a joint services environment.</rdfs:comment>
    <rdf:type rdf:resource="http://www.w3.org/2002/07/owl#Class"/>
  </rdf:Description>
  <rdf:Description rdf:about="#OPERATIONAL-CAPABILITY_Central_intelligence">
    <rdfs:label xml:lang="en">central intelligence</rdfs:label>
    <rdfs:subClassOf rdf:resource="jc3iedm_CAPABILITY.owl#OPERATIONAL-CAPABILITY"/>
    <rdfs:comment xml:lang="en">No definition provided in APP-6A.</rdfs:comment>
    <rdf:type rdf:resource="http://www.w3.org/2002/07/owl#Class"/>
  </rdf:Description>
  <rdf:Description rdf:about="#SUPPORT-CAPABILITY_Bedding">
    <rdfs:label xml:lang="en">bedding</rdfs:label>
    <rdfs:subClassOf rdf:resource="jc3iedm_CAPABILITY.owl#SUPPORT-CAPABILITY"/>
    <rdfs:comment xml:lang="en">The capability to provide bedding.</rdfs:comment>
    <rdf:type rdf:resource="http://www.w3.org/2002/07/owl#Class"/>
  </rdf:Description>
  <rdf:Description rdf:about="#SUPPORT-CAPABILITY_Recreation">
    <rdfs:label xml:lang="en">recreation</rdfs:label>
    <rdfs:subClassOf rdf:resource="jc3iedm_CAPABILITY.owl#SUPPORT-CAPABILITY"/>
    <rdfs:comment xml:lang="en">The capability to provide recreation services.</rdfs:comment>
    <rdf:type rdf:resource="http://www.w3.org/2002/07/owl#Class"/>
  </rdf:Description>
  <rdf:Description rdf:about="#MOBILITY-CAPABILITY_Water,_fjord">
    <rdfs:label xml:lang="en">water, fjord</rdfs:label>
    <rdfs:subClassOf rdf:resource="jc3iedm_CAPABILITY.owl#MOBILITY-CAPABILITY"/>
    <rdfs:comment xml:lang="en">The capability of a device to navigate fjords.</rdfs:comment>
    <rdf:type rdf:resource="http://www.w3.org/2002/07/owl#Class"/>
  </rdf:Description>
  <rdf:Description rdf:about="#OPERATIONAL-CAPABILITY_Morale,_welfare_recreation">
    <rdfs:label xml:lang="en">morale, welfare recreation</rdfs:label>
    <rdfs:subClassOf rdf:resource="jc3iedm_CAPABILITY.owl#OPERATIONAL-CAPABILITY"/>
    <rdfs:comment xml:lang="en">The capability to provide morale, welfare and recreation services in support of military personnel.</rdfs:comment>
    <rdf:type rdf:resource="http://www.w3.org/2002/07/owl#Class"/>
  </rdf:Description>
  <rdf:Description rdf:about="#OPERATIONAL-CAPABILITY_Supply_(class_III_aviation)">
    <rdfs:label xml:lang="en">supply (class iii aviation)</rdfs:label>
    <rdfs:subClassOf rdf:resource="jc3iedm_CAPABILITY.owl#OPERATIONAL-CAPABILITY"/>
    <rdfs:comment xml:lang="en">The capability to provide aviation fuel and lubricants.</rdfs:comment>
    <rdf:type rdf:resource="http://www.w3.org/2002/07/owl#Class"/>
  </rdf:Description>
  <rdf:Description rdf:about="#OPERATIONAL-CAPABILITY_Engineer,_construction_naval">
    <rdfs:label xml:lang="en">engineer, construction naval</rdfs:label>
    <rdfs:subClassOf rdf:resource="jc3iedm_CAPABILITY.owl#OPERATIONAL-CAPABILITY"/>
    <rdfs:comment xml:lang="en">The capability to build various facilities in direct support of naval operations.</rdfs:comment>
    <rdf:type rdf:resource="http://www.w3.org/2002/07/owl#Class"/>
  </rdf:Description>
  <rdf:Description rdf:about="#OPERATIONAL-CAPABILITY_Targeting">
    <rdfs:label xml:lang="en">targeting</rdfs:label>
    <rdfs:subClassOf rdf:resource="jc3iedm_CAPABILITY.owl#OPERATIONAL-CAPABILITY"/>
    <rdfs:comment xml:lang="en">The capability to provide targeting services.</rdfs:comment>
    <rdf:type rdf:resource="http://www.w3.org/2002/07/owl#Class"/>
  </rdf:Description>
  <rdf:Description rdf:about="#OPERATIONAL-CAPABILITY_Reconnaissance">
    <rdfs:label xml:lang="en">reconnaissance</rdfs:label>
    <rdfs:subClassOf rdf:resource="jc3iedm_CAPABILITY.owl#OPERATIONAL-CAPABILITY"/>
    <rdfs:comment xml:lang="en">The capability to obtain, by visual observation or other detection methods, information about the activities and resources of an enemy or potential enemy, or to secure data concerning the meteorological, hydrographical, or geographic characteristics of a particular area.</rdfs:comment>
    <rdf:type rdf:resource="http://www.w3.org/2002/07/owl#Class"/>
  </rdf:Description>
  <rdf:Description rdf:about="jc3iedm_CAPABILITY.owl#ENGINEERING-CAPABILITY">
    <rdf:type rdf:resource="http://www.w3.org/2002/07/owl#Class"/>
    <rdfs:label xml:lang="en">engineering capability</rdfs:label>
    <rdfs:comment xml:lang="en">A CAPABILITY, required for planning, of those ORGANISATIONs and PERSONs or ORGANISATION-TYPEs and PERSON-TYPEs that are deemed as having the ability to perform construction or destruction activities.</rdfs:comment>
    <rdfs:subClassOf rdf:resource="jc3iedm_CAPABILITY.owl#CAPABILITY"/>
  </rdf:Description>
  <rdf:Description rdf:about="#SUPPORT-CAPABILITY_Supply_(class_III_aviation)">
    <rdfs:label xml:lang="en">supply (class iii aviation)</rdfs:label>
    <rdfs:subClassOf rdf:resource="jc3iedm_CAPABILITY.owl#SUPPORT-CAPABILITY"/>
    <rdfs:comment xml:lang="en">The capability to provide aviation fuel and lubricants.</rdfs:comment>
    <rdf:type rdf:resource="http://www.w3.org/2002/07/owl#Class"/>
  </rdf:Description>
  <rdf:Description rdf:about="#OPERATIONAL-CAPABILITY_Anti-submarine_warfare">
    <rdfs:label xml:lang="en">anti submarine warfare</rdfs:label>
    <rdfs:subClassOf rdf:resource="jc3iedm_CAPABILITY.owl#OPERATIONAL-CAPABILITY"/>
    <rdfs:comment xml:lang="en">Operations conducted with the intention of denying the enemy the effective use of his submarines.</rdfs:comment>
    <rdf:type rdf:resource="http://www.w3.org/2002/07/owl#Class"/>
  </rdf:Description>
  <rdf:Description rdf:about="#OPERATIONAL-CAPABILITY_Mine_countermeasure">
    <rdfs:label xml:lang="en">mine countermeasure</rdfs:label>
    <rdfs:subClassOf rdf:resource="jc3iedm_CAPABILITY.owl#OPERATIONAL-CAPABILITY"/>
    <rdfs:comment xml:lang="en">The capability to prevent or reduce damage or danger from mines.</rdfs:comment>
    <rdf:type rdf:resource="http://www.w3.org/2002/07/owl#Class"/>
  </rdf:Description>
  <rdf:Description rdf:about="#MOBILITY-CAPABILITY_Self-deployable">
    <rdfs:label xml:lang="en">self deployable</rdfs:label>
    <rdfs:subClassOf rdf:resource="jc3iedm_CAPABILITY.owl#MOBILITY-CAPABILITY"/>
    <rdfs:comment xml:lang="en">The capability of a device to be brought into effective action by its own means.</rdfs:comment>
    <rdf:type rdf:resource="http://www.w3.org/2002/07/owl#Class"/>
  </rdf:Description>
  <rdf:Description rdf:about="#SUPPORT-CAPABILITY_Supply_(class_III)">
    <rdfs:label xml:lang="en">supply (class iii)</rdfs:label>
    <rdfs:subClassOf rdf:resource="jc3iedm_CAPABILITY.owl#SUPPORT-CAPABILITY"/>
    <rdfs:comment xml:lang="en">The capability to provide fuel and lubricants.</rdfs:comment>
    <rdf:type rdf:resource="http://www.w3.org/2002/07/owl#Class"/>
  </rdf:Description>
  <rdf:Description rdf:about="#OPERATIONAL-CAPABILITY_Air_defence">
    <rdfs:label xml:lang="en">air defence</rdfs:label>
    <rdfs:subClassOf rdf:resource="jc3iedm_CAPABILITY.owl#OPERATIONAL-CAPABILITY"/>
    <rdfs:comment xml:lang="en">The capability to nullify or reduce the effectiveness of hostile air action.</rdfs:comment>
    <rdf:type rdf:resource="http://www.w3.org/2002/07/owl#Class"/>
  </rdf:Description>
  <rdf:Description rdf:about="#TRANSMISSION-CAPABILITY_Transmit">
    <rdfs:label xml:lang="en">transmit</rdfs:label>
    <rdfs:subClassOf rdf:resource="jc3iedm_CAPABILITY.owl#TRANSMISSION-CAPABILITY"/>
    <rdfs:comment xml:lang="en">The ability to broadcast or send out a signal or programme.</rdfs:comment>
    <rdf:type rdf:resource="http://www.w3.org/2002/07/owl#Class"/>
  </rdf:Description>
  <rdf:Description rdf:about="#OPERATIONAL-CAPABILITY_Military_intelligence,_aerial_exploitation">
    <rdfs:label xml:lang="en">military intelligence, aerial exploitation</rdfs:label>
    <rdfs:subClassOf rdf:resource="jc3iedm_CAPABILITY.owl#OPERATIONAL-CAPABILITY"/>
    <rdfs:comment xml:lang="en">No definition provided in APP-6A.</rdfs:comment>
    <rdf:type rdf:resource="http://www.w3.org/2002/07/owl#Class"/>
  </rdf:Description>
  <rdf:Description rdf:about="#OPERATIONAL-CAPABILITY_Public_affairs">
    <rdfs:label xml:lang="en">public affairs</rdfs:label>
    <rdfs:subClassOf rdf:resource="jc3iedm_CAPABILITY.owl#OPERATIONAL-CAPABILITY"/>
    <rdfs:comment xml:lang="en">The capability to provide those public information, command information, and community relations activities directed towards the general public.</rdfs:comment>
    <rdf:type rdf:resource="http://www.w3.org/2002/07/owl#Class"/>
  </rdf:Description>
  <rdf:Description rdf:about="#OPERATIONAL-CAPABILITY_NBC,_biological">
    <rdfs:label xml:lang="en">nbc, biological</rdfs:label>
    <rdfs:subClassOf rdf:resource="jc3iedm_CAPABILITY.owl#OPERATIONAL-CAPABILITY"/>
    <rdfs:comment xml:lang="en">The capability to employ biological materiel to produce casualties in man or animals and damage to plants or materiel; or defence against such employment.</rdfs:comment>
    <rdf:type rdf:resource="http://www.w3.org/2002/07/owl#Class"/>
  </rdf:Description>
  <rdf:Description rdf:about="#OPERATIONAL-CAPABILITY_Surveillance,_long_range">
    <rdfs:label xml:lang="en">surveillance, long range</rdfs:label>
    <rdfs:subClassOf rdf:resource="jc3iedm_CAPABILITY.owl#OPERATIONAL-CAPABILITY"/>
    <rdfs:comment xml:lang="en">The capability to perform, from long range, systematic observation of aerospace, surface or subsurface areas, places, persons, or things by visual, aural, electronic, photographic, or other means from a ground station.</rdfs:comment>
    <rdf:type rdf:resource="http://www.w3.org/2002/07/owl#Class"/>
  </rdf:Description>
  <rdf:Description rdf:about="#OPERATIONAL-CAPABILITY_NBC,_chemical_decontamination">
    <rdfs:label xml:lang="en">nbc, chemical decontamination</rdfs:label>
    <rdfs:subClassOf rdf:resource="jc3iedm_CAPABILITY.owl#OPERATIONAL-CAPABILITY"/>
    <rdfs:comment xml:lang="en">The capability to make any person, object, or area safe by absorbing, destroying, neutralizing, making harmless, or removing, chemical materiel.</rdfs:comment>
    <rdf:type rdf:resource="http://www.w3.org/2002/07/owl#Class"/>
  </rdf:Description>
  <rdf:Description rdf:about="#FIRE-CAPABILITY_Air_to_air">
    <rdfs:label xml:lang="en">air to air</rdfs:label>
    <rdfs:subClassOf rdf:resource="jc3iedm_CAPABILITY.owl#FIRE-CAPABILITY"/>
    <rdfs:comment xml:lang="en">The specific value implies that a specific FIRE-CAPABILITY involves firing from aircraft at targets in the air.</rdfs:comment>
    <rdf:type rdf:resource="http://www.w3.org/2002/07/owl#Class"/>
  </rdf:Description>
  <rdf:Description rdf:about="#MOBILITY-CAPABILITY_Animal,_mounted">
    <rdfs:label xml:lang="en">animal, mounted</rdfs:label>
    <rdfs:subClassOf rdf:resource="jc3iedm_CAPABILITY.owl#MOBILITY-CAPABILITY"/>
    <rdfs:comment xml:lang="en">The capability to move by using an animal as a carrier.</rdfs:comment>
    <rdf:type rdf:resource="http://www.w3.org/2002/07/owl#Class"/>
  </rdf:Description>
  <rdf:Description rdf:about="jc3iedm_CAPABILITY.owl#FIRE-CAPABILITY">
    <rdf:type rdf:resource="http://www.w3.org/2002/07/owl#Class"/>
    <rdfs:label xml:lang="en">fire capability</rdfs:label>
    <rdfs:comment xml:lang="en">A CAPABILITY, required for planning, of those FACILITYs, MATERIELs, ORGANISATIONs and PERSONs, or FACILITY-TYPEs, EQUIPMENT-TYPEs, ORGANISATION-TYPEs and PERSON-TYPEs that are deemed as having the ability to discharge or launch a projectile or missile.</rdfs:comment>
    <rdfs:subClassOf rdf:resource="jc3iedm_CAPABILITY.owl#CAPABILITY"/>
  </rdf:Description>
  <rdf:Description rdf:about="#MOBILITY-CAPABILITY_Dismounted">
    <rdfs:label xml:lang="en">dismounted</rdfs:label>
    <rdfs:subClassOf rdf:resource="jc3iedm_CAPABILITY.owl#MOBILITY-CAPABILITY"/>
    <rdfs:comment xml:lang="en">The capability of moving on foot.</rdfs:comment>
    <rdf:type rdf:resource="http://www.w3.org/2002/07/owl#Class"/>
  </rdf:Description>
  <rdf:Description rdf:about="#OPERATIONAL-CAPABILITY_Transportation,_missile">
    <rdfs:label xml:lang="en">transportation, missile</rdfs:label>
    <rdfs:subClassOf rdf:resource="jc3iedm_CAPABILITY.owl#OPERATIONAL-CAPABILITY"/>
    <rdfs:comment xml:lang="en">The capability to provide equipment for transportation of missiles.</rdfs:comment>
    <rdf:type rdf:resource="http://www.w3.org/2002/07/owl#Class"/>
  </rdf:Description>
  <rdf:Description rdf:about="#OPERATIONAL-CAPABILITY_Maritime">
    <rdfs:label xml:lang="en">maritime</rdfs:label>
    <rdfs:subClassOf rdf:resource="jc3iedm_CAPABILITY.owl#OPERATIONAL-CAPABILITY"/>
    <rdfs:comment xml:lang="en">The capability to perform maritime/deep water operations.</rdfs:comment>
    <rdf:type rdf:resource="http://www.w3.org/2002/07/owl#Class"/>
  </rdf:Description>
  <rdf:Description rdf:about="#SUPPORT-CAPABILITY_Personal_equipment">
    <rdfs:label xml:lang="en">personal equipment</rdfs:label>
    <rdfs:subClassOf rdf:resource="jc3iedm_CAPABILITY.owl#SUPPORT-CAPABILITY"/>
    <rdfs:comment xml:lang="en">The capability to provide clothing.</rdfs:comment>
    <rdf:type rdf:resource="http://www.w3.org/2002/07/owl#Class"/>
  </rdf:Description>
  <rdf:Description rdf:about="#OPERATIONAL-CAPABILITY_Maintenance,_ordnance_missile">
    <rdfs:label xml:lang="en">maintenance, ordnance missile</rdfs:label>
    <rdfs:subClassOf rdf:resource="jc3iedm_CAPABILITY.owl#OPERATIONAL-CAPABILITY"/>
    <rdfs:comment xml:lang="en">The capability to maintain ordnance missile (materiel) in or to restore it to a specified condition.</rdfs:comment>
    <rdf:type rdf:resource="http://www.w3.org/2002/07/owl#Class"/>
  </rdf:Description>
  <rdf:Description rdf:about="#OPERATIONAL-CAPABILITY_Utility">
    <rdfs:label xml:lang="en">utility</rdfs:label>
    <rdfs:subClassOf rdf:resource="jc3iedm_CAPABILITY.owl#OPERATIONAL-CAPABILITY"/>
    <rdfs:comment xml:lang="en">The capability to provide utilities (water, gas, electric, et al).</rdfs:comment>
    <rdf:type rdf:resource="http://www.w3.org/2002/07/owl#Class"/>
  </rdf:Description>
  <rdf:Description rdf:about="#OPERATIONAL-CAPABILITY_NBC,_nuclear">
    <rdfs:label xml:lang="en">nbc, nuclear</rdfs:label>
    <rdfs:subClassOf rdf:resource="jc3iedm_CAPABILITY.owl#OPERATIONAL-CAPABILITY"/>
    <rdfs:comment xml:lang="en">No definition provided in APP-6A.</rdfs:comment>
    <rdf:type rdf:resource="http://www.w3.org/2002/07/owl#Class"/>
  </rdf:Description>
  <rdf:Description rdf:about="#OPERATIONAL-CAPABILITY_Electronic_warfare,_direction_finding">
    <rdfs:label xml:lang="en">electronic warfare, direction finding</rdfs:label>
    <rdfs:subClassOf rdf:resource="jc3iedm_CAPABILITY.owl#OPERATIONAL-CAPABILITY"/>
    <rdfs:comment xml:lang="en">The capability for obtaining bearings of radio frequency emitters by using a directional antenna and a display unit on an intercept receiver or ancillary equipment.</rdfs:comment>
    <rdf:type rdf:resource="http://www.w3.org/2002/07/owl#Class"/>
  </rdf:Description>
  <rdf:Description rdf:about="#SUPPORT-CAPABILITY_Medical_supplies">
    <rdfs:label xml:lang="en">medical supplies</rdfs:label>
    <rdfs:subClassOf rdf:resource="jc3iedm_CAPABILITY.owl#SUPPORT-CAPABILITY"/>
    <rdfs:comment xml:lang="en">The capability to provide medicine.</rdfs:comment>
    <rdf:type rdf:resource="http://www.w3.org/2002/07/owl#Class"/>
  </rdf:Description>
  <rdf:Description rdf:about="#OPERATIONAL-CAPABILITY_Signal,_radio">
    <rdfs:label xml:lang="en">signal, radio</rdfs:label>
    <rdfs:subClassOf rdf:resource="jc3iedm_CAPABILITY.owl#OPERATIONAL-CAPABILITY"/>
    <rdfs:comment xml:lang="en">The capability in signal services to manage, operate and control a radio communications.</rdfs:comment>
    <rdf:type rdf:resource="http://www.w3.org/2002/07/owl#Class"/>
  </rdf:Description>
  <rdf:Description rdf:about="jc3iedm_CAPABILITY.owl#CAPABILITY">
    <rdf:type rdf:resource="http://www.w3.org/2002/07/owl#Class"/>
    <rdfs:label xml:lang="en">capability</rdfs:label>
    <rdfs:comment xml:lang="en">The potential ability to do work, perform a function or mission, achieve an objective, or provide a service.</rdfs:comment>
  </rdf:Description>
  <rdf:Description rdf:about="#OPERATIONAL-CAPABILITY_Maintenance">
    <rdfs:label xml:lang="en">maintenance</rdfs:label>
    <rdfs:subClassOf rdf:resource="jc3iedm_CAPABILITY.owl#OPERATIONAL-CAPABILITY"/>
    <rdfs:comment xml:lang="en">The capability to provide supply and repair services to keep a force in condition to carry out its mission.</rdfs:comment>
    <rdf:type rdf:resource="http://www.w3.org/2002/07/owl#Class"/>
  </rdf:Description>
  <rdf:Description rdf:about="#SURVEILLANCE-CAPABILITY_Human">
    <rdfs:label xml:lang="en">human</rdfs:label>
    <rdfs:subClassOf rdf:resource="jc3iedm_CAPABILITY.owl#SURVEILLANCE-CAPABILITY"/>
    <rdfs:comment xml:lang="en">The ability to gain information by exploiting human senses.</rdfs:comment>
    <rdf:type rdf:resource="http://www.w3.org/2002/07/owl#Class"/>
  </rdf:Description>
  <rdf:Description rdf:about="#OPERATIONAL-CAPABILITY_Target_acquisition,_flash">
    <rdfs:label xml:lang="en">target acquisition, flash</rdfs:label>
    <rdfs:subClassOf rdf:resource="jc3iedm_CAPABILITY.owl#OPERATIONAL-CAPABILITY"/>
    <rdfs:comment xml:lang="en">The capability to manage, operate and maintain flash target acquisition assets.</rdfs:comment>
    <rdf:type rdf:resource="http://www.w3.org/2002/07/owl#Class"/>
  </rdf:Description>
  <rdf:Description rdf:about="#SUPPORT-CAPABILITY_Food/rations">
    <rdfs:label xml:lang="en">food/rations</rdfs:label>
    <rdfs:subClassOf rdf:resource="jc3iedm_CAPABILITY.owl#SUPPORT-CAPABILITY"/>
    <rdfs:comment xml:lang="en">The capability to provide food.</rdfs:comment>
    <rdf:type rdf:resource="http://www.w3.org/2002/07/owl#Class"/>
  </rdf:Description>
  <rdf:Description rdf:about="#MOBILITY-CAPABILITY_Water,_surface">
    <rdfs:label xml:lang="en">water, surface</rdfs:label>
    <rdfs:subClassOf rdf:resource="jc3iedm_CAPABILITY.owl#MOBILITY-CAPABILITY"/>
    <rdfs:comment xml:lang="en">The capability of a device to move on the water surface.</rdfs:comment>
    <rdf:type rdf:resource="http://www.w3.org/2002/07/owl#Class"/>
  </rdf:Description>
  <rdf:Description rdf:about="#MOBILITY-CAPABILITY_Water,_canal">
    <rdfs:label xml:lang="en">water, canal</rdfs:label>
    <rdfs:subClassOf rdf:resource="jc3iedm_CAPABILITY.owl#MOBILITY-CAPABILITY"/>
    <rdfs:comment xml:lang="en">The capability of a device to navigate canals.</rdfs:comment>
    <rdf:type rdf:resource="http://www.w3.org/2002/07/owl#Class"/>
  </rdf:Description>
  <rdf:Description rdf:about="#OPERATIONAL-CAPABILITY_Interrogation">
    <rdfs:label xml:lang="en">interrogation</rdfs:label>
    <rdfs:subClassOf rdf:resource="jc3iedm_CAPABILITY.owl#OPERATIONAL-CAPABILITY"/>
    <rdfs:comment xml:lang="en">The capability to procure information by direct questioning of a person under the control of a questioner.</rdfs:comment>
    <rdf:type rdf:resource="http://www.w3.org/2002/07/owl#Class"/>
  </rdf:Description>
  <rdf:Description rdf:about="#OPERATIONAL-CAPABILITY_Medical_evacuation">
    <rdfs:label xml:lang="en">medical evacuation</rdfs:label>
    <rdfs:subClassOf rdf:resource="jc3iedm_CAPABILITY.owl#OPERATIONAL-CAPABILITY"/>
    <rdfs:comment xml:lang="en">The capability for timely and efficient movement of patients while providing en route medical care to and between medical treatment facilities.</rdfs:comment>
    <rdf:type rdf:resource="http://www.w3.org/2002/07/owl#Class"/>
  </rdf:Description>
  <rdf:Description rdf:about="#OPERATIONAL-CAPABILITY_Signal,_node,_large_extension">
    <rdfs:label xml:lang="en">signal, node, large extension</rdfs:label>
    <rdfs:subClassOf rdf:resource="jc3iedm_CAPABILITY.owl#OPERATIONAL-CAPABILITY"/>
    <rdfs:comment xml:lang="en">The capability in signal services to manage, operate and control a communications large extension node.</rdfs:comment>
    <rdf:type rdf:resource="http://www.w3.org/2002/07/owl#Class"/>
  </rdf:Description>
  <rdf:Description rdf:about="#OPERATIONAL-CAPABILITY_Engineer,_construction">
    <rdfs:label xml:lang="en">engineer, construction</rdfs:label>
    <rdfs:subClassOf rdf:resource="jc3iedm_CAPABILITY.owl#OPERATIONAL-CAPABILITY"/>
    <rdfs:comment xml:lang="en">The capability to build various facilities in direct support of military operations.</rdfs:comment>
    <rdf:type rdf:resource="http://www.w3.org/2002/07/owl#Class"/>
  </rdf:Description>
  <rdf:Description rdf:about="#OPERATIONAL-CAPABILITY_Aerial_refuelling">
    <rdfs:label xml:lang="en">aerial refuelling</rdfs:label>
    <rdfs:subClassOf rdf:resource="jc3iedm_CAPABILITY.owl#OPERATIONAL-CAPABILITY"/>
    <rdfs:comment xml:lang="en">The capability to refuel aircraft in flight, which extends presence, increases range, and serves as a force multiplier.</rdfs:comment>
    <rdf:type rdf:resource="http://www.w3.org/2002/07/owl#Class"/>
  </rdf:Description>
  <rdf:Description rdf:about="#TRANSMISSION-CAPABILITY_Receive">
    <rdfs:label xml:lang="en">receive</rdfs:label>
    <rdfs:subClassOf rdf:resource="jc3iedm_CAPABILITY.owl#TRANSMISSION-CAPABILITY"/>
    <rdfs:comment xml:lang="en">The ability to detect or pick up a broadcast, a signal or programme.</rdfs:comment>
    <rdf:type rdf:resource="http://www.w3.org/2002/07/owl#Class"/>
  </rdf:Description>
  <rdf:Description rdf:about="#OPERATIONAL-CAPABILITY_Signal,_support">
    <rdfs:label xml:lang="en">signal, support</rdfs:label>
    <rdfs:subClassOf rdf:resource="jc3iedm_CAPABILITY.owl#OPERATIONAL-CAPABILITY"/>
    <rdfs:comment xml:lang="en">The capability to provide personnel and equipment from other forces for the establishment of a special or supplementary communications system.</rdfs:comment>
    <rdf:type rdf:resource="http://www.w3.org/2002/07/owl#Class"/>
  </rdf:Description>
  <rdf:Description rdf:about="#MOBILITY-CAPABILITY_Water,_tidal">
    <rdfs:label xml:lang="en">water, tidal</rdfs:label>
    <rdfs:subClassOf rdf:resource="jc3iedm_CAPABILITY.owl#MOBILITY-CAPABILITY"/>
    <rdfs:comment xml:lang="en">The capability of a device to navigate tidal waters.</rdfs:comment>
    <rdf:type rdf:resource="http://www.w3.org/2002/07/owl#Class"/>
  </rdf:Description>
  <rdf:Description rdf:about="#MAINTENANCE-CAPABILITY_Cable">
    <rdfs:label xml:lang="en">cable</rdfs:label>
    <rdfs:subClassOf rdf:resource="jc3iedm_CAPABILITY.owl#MAINTENANCE-CAPABILITY"/>
    <rdfs:comment xml:lang="en">The specific MAINTENANCE-CAPABILITY determines the ability to provide cable repair.</rdfs:comment>
    <rdf:type rdf:resource="http://www.w3.org/2002/07/owl#Class"/>
  </rdf:Description>
  <rdf:Description rdf:about="#MAINTENANCE-CAPABILITY_Electrical">
    <rdfs:label xml:lang="en">electrical</rdfs:label>
    <rdfs:subClassOf rdf:resource="jc3iedm_CAPABILITY.owl#MAINTENANCE-CAPABILITY"/>
    <rdfs:comment xml:lang="en">The specific MAINTENANCE-CAPABILITY determines the ability to provide electrical repair.</rdfs:comment>
    <rdf:type rdf:resource="http://www.w3.org/2002/07/owl#Class"/>
  </rdf:Description>
  <rdf:Description rdf:about="#OPERATIONAL-CAPABILITY_Military_intelligence,_operation">
    <rdfs:label xml:lang="en">military intelligence, operation</rdfs:label>
    <rdfs:subClassOf rdf:resource="jc3iedm_CAPABILITY.owl#OPERATIONAL-CAPABILITY"/>
    <rdfs:comment xml:lang="en">The capability to provide information required for the planning and conducting campaigns and major operations to accomplish strategic objectives within theatres or areas of operations.</rdfs:comment>
    <rdf:type rdf:resource="http://www.w3.org/2002/07/owl#Class"/>
  </rdf:Description>
  <rdf:Description rdf:about="#MOBILITY-CAPABILITY_Air,_rotary_wing">
    <rdfs:label xml:lang="en">air, rotary wing</rdfs:label>
    <rdfs:subClassOf rdf:resource="jc3iedm_CAPABILITY.owl#MOBILITY-CAPABILITY"/>
    <rdfs:comment xml:lang="en">The capability to move through the air by deriving lift from aerofoils that rotate.</rdfs:comment>
    <rdf:type rdf:resource="http://www.w3.org/2002/07/owl#Class"/>
  </rdf:Description>
  <rdf:Description rdf:about="#MOBILITY-CAPABILITY_Air,_lighter_than_air">
    <rdfs:label xml:lang="en">air, lighter than air</rdfs:label>
    <rdfs:subClassOf rdf:resource="jc3iedm_CAPABILITY.owl#MOBILITY-CAPABILITY"/>
    <rdfs:comment xml:lang="en">The capability of an air vehicle to remain airborne and move by displacing a weight of air greater than its own.</rdfs:comment>
    <rdf:type rdf:resource="http://www.w3.org/2002/07/owl#Class"/>
  </rdf:Description>
  <rdf:Description rdf:about="#MOBILITY-CAPABILITY_Air,_fixed_wing">
    <rdfs:label xml:lang="en">air, fixed wing</rdfs:label>
    <rdfs:subClassOf rdf:resource="jc3iedm_CAPABILITY.owl#MOBILITY-CAPABILITY"/>
    <rdfs:comment xml:lang="en">The capability to move through the air by deriving lift from fixed wings.</rdfs:comment>
    <rdf:type rdf:resource="http://www.w3.org/2002/07/owl#Class"/>
  </rdf:Description>
  <rdf:Description rdf:about="#FIRE-CAPABILITY_Ground_to_air">
    <rdfs:label xml:lang="en">ground to air</rdfs:label>
    <rdfs:subClassOf rdf:resource="jc3iedm_CAPABILITY.owl#FIRE-CAPABILITY"/>
    <rdfs:comment xml:lang="en">The specific value implies that a specific FIRE-CAPABILITY involves firing from the ground to an airborne target.</rdfs:comment>
    <rdf:type rdf:resource="http://www.w3.org/2002/07/owl#Class"/>
  </rdf:Description>
  <rdf:Description rdf:about="#OPERATIONAL-CAPABILITY_Joint_intelligence">
    <rdfs:label xml:lang="en">joint intelligence</rdfs:label>
    <rdfs:subClassOf rdf:resource="jc3iedm_CAPABILITY.owl#OPERATIONAL-CAPABILITY"/>
    <rdfs:comment xml:lang="en">The capability to produce intelligence from elements of more than one Service.</rdfs:comment>
    <rdf:type rdf:resource="http://www.w3.org/2002/07/owl#Class"/>
  </rdf:Description>
  <rdf:Description rdf:about="#TRANSMISSION-CAPABILITY_Transceive">
    <rdfs:label xml:lang="en">transceive</rdfs:label>
    <rdfs:subClassOf rdf:resource="jc3iedm_CAPABILITY.owl#TRANSMISSION-CAPABILITY"/>
    <rdfs:comment xml:lang="en">The ability to detect, pick up, broadcast or send out a signal or programme.</rdfs:comment>
    <rdf:type rdf:resource="http://www.w3.org/2002/07/owl#Class"/>
  </rdf:Description>
  <rdf:Description rdf:about="#">
    <owl:imports rdf:resource="jc3iedm_CAPABILITY.owl#"/>
    <rdf:type rdf:resource="http://www.w3.org/2002/07/owl#Ontology"/>
  </rdf:Description>
  <rdf:Description rdf:about="#OPERATIONAL-CAPABILITY_Target_acquisition,_sound">
    <rdfs:label xml:lang="en">target acquisition, sound</rdfs:label>
    <rdfs:subClassOf rdf:resource="jc3iedm_CAPABILITY.owl#OPERATIONAL-CAPABILITY"/>
    <rdfs:comment xml:lang="en">The capability to manage, operate and maintain sound target acquisition assets.</rdfs:comment>
    <rdf:type rdf:resource="http://www.w3.org/2002/07/owl#Class"/>
  </rdf:Description>
  <rdf:Description rdf:about="#OPERATIONAL-CAPABILITY_Signal,_radio_teletype">
    <rdfs:label xml:lang="en">signal, radio teletype</rdfs:label>
    <rdfs:subClassOf rdf:resource="jc3iedm_CAPABILITY.owl#OPERATIONAL-CAPABILITY"/>
    <rdfs:comment xml:lang="en">The capability in signal services to manage, operate and control a radio teletype communications.</rdfs:comment>
    <rdf:type rdf:resource="http://www.w3.org/2002/07/owl#Class"/>
  </rdf:Description>
  <rdf:Description rdf:about="#OPERATIONAL-CAPABILITY_Amphibious">
    <rdfs:label xml:lang="en">amphibious</rdfs:label>
    <rdfs:subClassOf rdf:resource="jc3iedm_CAPABILITY.owl#OPERATIONAL-CAPABILITY"/>
    <rdfs:comment xml:lang="en">The capability to conduct an operation launched from the sea by military forces against a hostile or potentially hostile shore.</rdfs:comment>
    <rdf:type rdf:resource="http://www.w3.org/2002/07/owl#Class"/>
  </rdf:Description>
  <rdf:Description rdf:about="#SUPPORT-CAPABILITY_Supply_(class_V)">
    <rdfs:label xml:lang="en">supply (class v)</rdfs:label>
    <rdfs:subClassOf rdf:resource="jc3iedm_CAPABILITY.owl#SUPPORT-CAPABILITY"/>
    <rdfs:comment xml:lang="en">The capability to provide ammunition, explosives and chemical agents.</rdfs:comment>
    <rdf:type rdf:resource="http://www.w3.org/2002/07/owl#Class"/>
  </rdf:Description>
  <rdf:Description rdf:about="#OPERATIONAL-CAPABILITY_Arctic">
    <rdfs:label xml:lang="en">arctic</rdfs:label>
    <rdfs:subClassOf rdf:resource="jc3iedm_CAPABILITY.owl#OPERATIONAL-CAPABILITY"/>
    <rdfs:comment xml:lang="en">The capability to perform a mission involving an arctic operation.</rdfs:comment>
    <rdf:type rdf:resource="http://www.w3.org/2002/07/owl#Class"/>
  </rdf:Description>
  <rdf:Description rdf:about="#MOBILITY-CAPABILITY_Air,_composite">
    <rdfs:label xml:lang="en">air, composite</rdfs:label>
    <rdfs:subClassOf rdf:resource="jc3iedm_CAPABILITY.owl#MOBILITY-CAPABILITY"/>
    <rdfs:comment xml:lang="en">The capability to move through the air by means that combine deriving lift from fixed wings or from aerofoils that rotate.</rdfs:comment>
    <rdf:type rdf:resource="http://www.w3.org/2002/07/owl#Class"/>
  </rdf:Description>
  <rdf:Description rdf:about="#OPERATIONAL-CAPABILITY_Artillery_survey">
    <rdfs:label xml:lang="en">artillery survey</rdfs:label>
    <rdfs:subClassOf rdf:resource="jc3iedm_CAPABILITY.owl#OPERATIONAL-CAPABILITY"/>
    <rdfs:comment xml:lang="en">The capability to calculate the coordinates and the altitude of an object/point and from which the bearings/azimuths to a number of reference objects are also known.</rdfs:comment>
    <rdf:type rdf:resource="http://www.w3.org/2002/07/owl#Class"/>
  </rdf:Description>
  <rdf:Description rdf:about="#MOBILITY-CAPABILITY_Land,_tracked">
    <rdfs:label xml:lang="en">land, tracked</rdfs:label>
    <rdfs:subClassOf rdf:resource="jc3iedm_CAPABILITY.owl#MOBILITY-CAPABILITY"/>
    <rdfs:comment xml:lang="en">The capability of a device to move on caterpillar treads.</rdfs:comment>
    <rdf:type rdf:resource="http://www.w3.org/2002/07/owl#Class"/>
  </rdf:Description>
  <rdf:Description rdf:about="#SUPPORT-CAPABILITY_Supply_(class_I)">
    <rdfs:label xml:lang="en">supply (class i)</rdfs:label>
    <rdfs:subClassOf rdf:resource="jc3iedm_CAPABILITY.owl#SUPPORT-CAPABILITY"/>
    <rdfs:comment xml:lang="en">The capability to provide combat/fresh rations, water and personal, health and welfare items.</rdfs:comment>
    <rdf:type rdf:resource="http://www.w3.org/2002/07/owl#Class"/>
  </rdf:Description>
  <rdf:Description rdf:about="#MOBILITY-CAPABILITY_Water,_swamp">
    <rdfs:label xml:lang="en">water, swamp</rdfs:label>
    <rdfs:subClassOf rdf:resource="jc3iedm_CAPABILITY.owl#MOBILITY-CAPABILITY"/>
    <rdfs:comment xml:lang="en">The capability of a device to navigate swamps.</rdfs:comment>
    <rdf:type rdf:resource="http://www.w3.org/2002/07/owl#Class"/>
  </rdf:Description>
  <rdf:Description rdf:about="#SUPPORT-CAPABILITY_Engine">
    <rdfs:label xml:lang="en">engine</rdfs:label>
    <rdfs:subClassOf rdf:resource="jc3iedm_CAPABILITY.owl#SUPPORT-CAPABILITY"/>
    <rdfs:comment xml:lang="en">The capability to provide engine supplies.</rdfs:comment>
    <rdf:type rdf:resource="http://www.w3.org/2002/07/owl#Class"/>
  </rdf:Description>
  <rdf:Description rdf:about="#OPERATIONAL-CAPABILITY_Labour">
    <rdfs:label xml:lang="en">labour</rdfs:label>
    <rdfs:subClassOf rdf:resource="jc3iedm_CAPABILITY.owl#OPERATIONAL-CAPABILITY"/>
    <rdfs:comment xml:lang="en">The capability to provide labour services.</rdfs:comment>
    <rdf:type rdf:resource="http://www.w3.org/2002/07/owl#Class"/>
  </rdf:Description>
  <rdf:Description rdf:about="jc3iedm_CAPABILITY.owl#TRANSMISSION-CAPABILITY">
    <rdf:type rdf:resource="http://www.w3.org/2002/07/owl#Class"/>
    <rdfs:label xml:lang="en">transmission capability</rdfs:label>
    <rdfs:comment xml:lang="en">A CAPABILITY, required for planning, of those MATERIELs or MATERIEL-TYPEs that are deemed as having the ability to generate, receive or affect signals in the electromagnetic spectrum.</rdfs:comment>
    <rdfs:subClassOf rdf:resource="jc3iedm_CAPABILITY.owl#CAPABILITY"/>
  </rdf:Description>
  <rdf:Description rdf:about="#OPERATIONAL-CAPABILITY_Signal,_radio_tactical_satellite">
    <rdfs:label xml:lang="en">signal, radio tactical satellite</rdfs:label>
    <rdfs:subClassOf rdf:resource="jc3iedm_CAPABILITY.owl#OPERATIONAL-CAPABILITY"/>
    <rdfs:comment xml:lang="en">The capability in signal services to manage, operate and control a tactical satellite terminal.</rdfs:comment>
    <rdf:type rdf:resource="http://www.w3.org/2002/07/owl#Class"/>
  </rdf:Description>
  <rdf:Description rdf:about="#OPERATIONAL-CAPABILITY_Training">
    <rdfs:label xml:lang="en">training</rdfs:label>
    <rdfs:subClassOf rdf:resource="jc3iedm_CAPABILITY.owl#OPERATIONAL-CAPABILITY"/>
    <rdfs:comment xml:lang="en">A capability that enables an equipment to be used to train personnel.</rdfs:comment>
    <rdf:type rdf:resource="http://www.w3.org/2002/07/owl#Class"/>
  </rdf:Description>
  <rdf:Description rdf:about="#OPERATIONAL-CAPABILITY_Signals_intelligence_(SIGINT)">
    <rdfs:label xml:lang="en">signals intelligence (sigint)</rdfs:label>
    <rdfs:subClassOf rdf:resource="jc3iedm_CAPABILITY.owl#OPERATIONAL-CAPABILITY"/>
    <rdfs:comment xml:lang="en">The capability to provide intelligence derived from communications, electronics, and instrumentation signals.</rdfs:comment>
    <rdf:type rdf:resource="http://www.w3.org/2002/07/owl#Class"/>
  </rdf:Description>
  <rdf:Description rdf:about="jc3iedm_CAPABILITY.owl#physical_model_only">
    <rdf:type rdf:resource="http://www.w3.org/2002/07/owl#DatatypeProperty"/>
    <rdfs:domain rdf:resource="jc3iedm_CAPABILITY.owl#CAPABILITY"/>
  </rdf:Description>
  <rdf:Description rdf:about="#FIRE-CAPABILITY_Sea_to_ground">
    <rdfs:label xml:lang="en">sea to ground</rdfs:label>
    <rdfs:subClassOf rdf:resource="jc3iedm_CAPABILITY.owl#FIRE-CAPABILITY"/>
    <rdfs:comment xml:lang="en">The specific value implies that a specific FIRE-CAPABILITY involves firing from a vessel to targets on the ground.</rdfs:comment>
    <rdf:type rdf:resource="http://www.w3.org/2002/07/owl#Class"/>
  </rdf:Description>
  <rdf:Description rdf:about="#OPERATIONAL-CAPABILITY_Surveillance,_sensor">
    <rdfs:label xml:lang="en">surveillance, sensor</rdfs:label>
    <rdfs:subClassOf rdf:resource="jc3iedm_CAPABILITY.owl#OPERATIONAL-CAPABILITY"/>
    <rdfs:comment xml:lang="en">The capability to manage, operate and maintain sensor surveillance assets.</rdfs:comment>
    <rdf:type rdf:resource="http://www.w3.org/2002/07/owl#Class"/>
  </rdf:Description>
  <rdf:Description rdf:about="#OPERATIONAL-CAPABILITY_NBC,_radiological">
    <rdfs:label xml:lang="en">nbc, radiological</rdfs:label>
    <rdfs:subClassOf rdf:resource="jc3iedm_CAPABILITY.owl#OPERATIONAL-CAPABILITY"/>
    <rdfs:comment xml:lang="en">The capability to employ radiological materiel to produce casualties in man or animals and damage to plants or materiel; or defence against such employment.</rdfs:comment>
    <rdf:type rdf:resource="http://www.w3.org/2002/07/owl#Class"/>
  </rdf:Description>
  <rdf:Description rdf:about="#OPERATIONAL-CAPABILITY_Replacement_holding">
    <rdfs:label xml:lang="en">replacement holding</rdfs:label>
    <rdfs:subClassOf rdf:resource="jc3iedm_CAPABILITY.owl#OPERATIONAL-CAPABILITY"/>
    <rdfs:comment xml:lang="en">The capability to provide personnel to take the place of other personnel who depart a unit.</rdfs:comment>
    <rdf:type rdf:resource="http://www.w3.org/2002/07/owl#Class"/>
  </rdf:Description>
  <rdf:Description rdf:about="#OPERATIONAL-CAPABILITY_Transportation,_APOD/APOE">
    <rdfs:label xml:lang="en">transportation, apod/apoe</rdfs:label>
    <rdfs:subClassOf rdf:resource="jc3iedm_CAPABILITY.owl#OPERATIONAL-CAPABILITY"/>
    <rdfs:comment xml:lang="en">The capability to provide transportation services at aerial ports where cargo or personnel arrive or depart.</rdfs:comment>
    <rdf:type rdf:resource="http://www.w3.org/2002/07/owl#Class"/>
  </rdf:Description>
  <rdf:Description rdf:about="#SUPPORT-CAPABILITY_Messing">
    <rdfs:label xml:lang="en">messing</rdfs:label>
    <rdfs:subClassOf rdf:resource="jc3iedm_CAPABILITY.owl#SUPPORT-CAPABILITY"/>
    <rdfs:comment xml:lang="en">The capability to provide a place providing meals and recreational facilities.</rdfs:comment>
    <rdf:type rdf:resource="http://www.w3.org/2002/07/owl#Class"/>
  </rdf:Description>
  <rdf:Description rdf:about="#MAINTENANCE-CAPABILITY_Steelwork_fabrication">
    <rdfs:label xml:lang="en">steelwork fabrication</rdfs:label>
    <rdfs:subClassOf rdf:resource="jc3iedm_CAPABILITY.owl#MAINTENANCE-CAPABILITY"/>
    <rdfs:comment xml:lang="en">Equipment and resources for the construction or manufacture of any article made of steel required for a docked vessel.</rdfs:comment>
    <rdf:type rdf:resource="http://www.w3.org/2002/07/owl#Class"/>
  </rdf:Description>
  <rdf:Description rdf:about="#OPERATIONAL-CAPABILITY_NBC,_decontamination">
    <rdfs:label xml:lang="en">nbc, decontamination</rdfs:label>
    <rdfs:subClassOf rdf:resource="jc3iedm_CAPABILITY.owl#OPERATIONAL-CAPABILITY"/>
    <rdfs:comment xml:lang="en">The capability to make any person, object, or area safe by absorbing, destroying, neutralizing, making harmless, or removing, chemical or biological materiel, or by removing radioactive material clinging to or around it.</rdfs:comment>
    <rdf:type rdf:resource="http://www.w3.org/2002/07/owl#Class"/>
  </rdf:Description>
  <rdf:Description rdf:about="#OPERATIONAL-CAPABILITY_Supply_(class_V)">
    <rdfs:label xml:lang="en">supply (class v)</rdfs:label>
    <rdfs:subClassOf rdf:resource="jc3iedm_CAPABILITY.owl#OPERATIONAL-CAPABILITY"/>
    <rdfs:comment xml:lang="en">The capability to provide ammunition, explosives and chemical agents.</rdfs:comment>
    <rdf:type rdf:resource="http://www.w3.org/2002/07/owl#Class"/>
  </rdf:Description>
  <rdf:Description rdf:about="#OPERATIONAL-CAPABILITY_Public_affairs,_broadcast">
    <rdfs:label xml:lang="en">public affairs, broadcast</rdfs:label>
    <rdfs:subClassOf rdf:resource="jc3iedm_CAPABILITY.owl#OPERATIONAL-CAPABILITY"/>
    <rdfs:comment xml:lang="en">The capability to provide those public information, command information, and community relation activities over a broadcast medium, such as radio or TV, directed towards the general public.</rdfs:comment>
    <rdf:type rdf:resource="http://www.w3.org/2002/07/owl#Class"/>
  </rdf:Description>
  <rdf:Description rdf:about="#SUPPORT-CAPABILITY_Security">
    <rdfs:label xml:lang="en">security</rdfs:label>
    <rdfs:subClassOf rdf:resource="jc3iedm_CAPABILITY.owl#SUPPORT-CAPABILITY"/>
    <rdfs:comment xml:lang="en">The capability to provide security services.</rdfs:comment>
    <rdf:type rdf:resource="http://www.w3.org/2002/07/owl#Class"/>
  </rdf:Description>
  <rdf:Description rdf:about="#OPERATIONAL-CAPABILITY_Scout">
    <rdfs:label xml:lang="en">scout</rdfs:label>
    <rdfs:subClassOf rdf:resource="jc3iedm_CAPABILITY.owl#OPERATIONAL-CAPABILITY"/>
    <rdfs:comment xml:lang="en">The capability to move out ahead of the main force in order to reconnoitre the position or movements of the enemy.</rdfs:comment>
    <rdf:type rdf:resource="http://www.w3.org/2002/07/owl#Class"/>
  </rdf:Description>
  <rdf:Description rdf:about="jc3iedm_CAPABILITY.owl#HANDLING-CAPABILITY">
    <rdf:type rdf:resource="http://www.w3.org/2002/07/owl#Class"/>
    <rdfs:label xml:lang="en">handling capability</rdfs:label>
    <rdfs:comment xml:lang="en">A CAPABILITY, required for planning, of those FACILITYs and MATERIELs, or FACILITY-TYPEs and EQUIPMENT-TYPEs that are deemed as having the ability to move materiels (raw materials, scrap, semi-finished, and finished) to, through, and from productive processes; in warehouses and storage; and in receiving and shipping areas.</rdfs:comment>
    <rdfs:subClassOf rdf:resource="jc3iedm_CAPABILITY.owl#CAPABILITY"/>
  </rdf:Description>
  <rdf:Description rdf:about="#SUPPORT-CAPABILITY_Helicopter_platform">
    <rdfs:label xml:lang="en">helicopter platform</rdfs:label>
    <rdfs:subClassOf rdf:resource="jc3iedm_CAPABILITY.owl#SUPPORT-CAPABILITY"/>
    <rdfs:comment xml:lang="en">The capability to provide a surface for helicopter take off and landing.</rdfs:comment>
    <rdf:type rdf:resource="http://www.w3.org/2002/07/owl#Class"/>
  </rdf:Description>
  <rdf:Description rdf:about="#OPERATIONAL-CAPABILITY_Signal,_forward_communications">
    <rdfs:label xml:lang="en">signal, forward communications</rdfs:label>
    <rdfs:subClassOf rdf:resource="jc3iedm_CAPABILITY.owl#OPERATIONAL-CAPABILITY"/>
    <rdfs:comment xml:lang="en">The capability to provide tactical communications in the combat zone.</rdfs:comment>
    <rdf:type rdf:resource="http://www.w3.org/2002/07/owl#Class"/>
  </rdf:Description>
  <rdf:Description rdf:about="#MOBILITY-CAPABILITY_Water,_creek">
    <rdfs:label xml:lang="en">water, creek</rdfs:label>
    <rdfs:subClassOf rdf:resource="jc3iedm_CAPABILITY.owl#MOBILITY-CAPABILITY"/>
    <rdfs:comment xml:lang="en">The capability of a device to navigate in creeks.</rdfs:comment>
    <rdf:type rdf:resource="http://www.w3.org/2002/07/owl#Class"/>
  </rdf:Description>
  <rdf:Description rdf:about="#SUPPORT-CAPABILITY_Healthcare">
    <rdfs:label xml:lang="en">healthcare</rdfs:label>
    <rdfs:subClassOf rdf:resource="jc3iedm_CAPABILITY.owl#SUPPORT-CAPABILITY"/>
    <rdfs:comment xml:lang="en">The capability to provide health care services.</rdfs:comment>
    <rdf:type rdf:resource="http://www.w3.org/2002/07/owl#Class"/>
  </rdf:Description>
  <rdf:Description rdf:about="#SURVEILLANCE-CAPABILITY_Imaging">
    <rdfs:label xml:lang="en">imaging</rdfs:label>
    <rdfs:subClassOf rdf:resource="jc3iedm_CAPABILITY.owl#SURVEILLANCE-CAPABILITY"/>
    <rdfs:comment xml:lang="en">The ability to gain information by exploiting imaging systems.</rdfs:comment>
    <rdf:type rdf:resource="http://www.w3.org/2002/07/owl#Class"/>
  </rdf:Description>
  <rdf:Description rdf:about="#OPERATIONAL-CAPABILITY_Tactical_air_reconnaissance">
    <rdfs:label xml:lang="en">tactical air reconnaissance</rdfs:label>
    <rdfs:subClassOf rdf:resource="jc3iedm_CAPABILITY.owl#OPERATIONAL-CAPABILITY"/>
    <rdfs:comment xml:lang="en">The capability to use of air vehicles to obtain information concerning terrain, weather, and the disposition, composition, movement, installations, lines of communications, electronic and communication emissions of enemy forces. Also included are artillery and naval gunfire adjustment, and systematic and random observation of ground battle areas, targets, and/ or sectors of airspace.</rdfs:comment>
    <rdf:type rdf:resource="http://www.w3.org/2002/07/owl#Class"/>
  </rdf:Description>
  <rdf:Description rdf:about="#SUPPORT-CAPABILITY_Fuel,_heating">
    <rdfs:label xml:lang="en">fuel, heating</rdfs:label>
    <rdfs:subClassOf rdf:resource="jc3iedm_CAPABILITY.owl#SUPPORT-CAPABILITY"/>
    <rdfs:comment xml:lang="en">The capability to provide fuel for heating.</rdfs:comment>
    <rdf:type rdf:resource="http://www.w3.org/2002/07/owl#Class"/>
  </rdf:Description>
  <rdf:Description rdf:about="#MAINTENANCE-CAPABILITY_Plumbing">
    <rdfs:label xml:lang="en">plumbing</rdfs:label>
    <rdfs:subClassOf rdf:resource="jc3iedm_CAPABILITY.owl#MAINTENANCE-CAPABILITY"/>
    <rdfs:comment xml:lang="en">Equipment and resources for fitting and repairing pipes, fixtures and other apparatus of a water gas or sewage system belonging to a docked vessel.</rdfs:comment>
    <rdf:type rdf:resource="http://www.w3.org/2002/07/owl#Class"/>
  </rdf:Description>
  <rdf:Description rdf:about="#OPERATIONAL-CAPABILITY_Surveillance,_ground_module">
    <rdfs:label xml:lang="en">surveillance, ground module</rdfs:label>
    <rdfs:subClassOf rdf:resource="jc3iedm_CAPABILITY.owl#OPERATIONAL-CAPABILITY"/>
    <rdfs:comment xml:lang="en">The capability to manage and operate a ground module for a surveillance system.</rdfs:comment>
    <rdf:type rdf:resource="http://www.w3.org/2002/07/owl#Class"/>
  </rdf:Description>
  <rdf:Description rdf:about="#OPERATIONAL-CAPABILITY_Engineer,_combat">
    <rdfs:label xml:lang="en">engineer, combat</rdfs:label>
    <rdfs:subClassOf rdf:resource="jc3iedm_CAPABILITY.owl#OPERATIONAL-CAPABILITY"/>
    <rdfs:comment xml:lang="en">The capability to perform engineer functions in direct support of combat operations.</rdfs:comment>
    <rdf:type rdf:resource="http://www.w3.org/2002/07/owl#Class"/>
  </rdf:Description>
  <rdf:Description rdf:about="#SURVEILLANCE-CAPABILITY_Electronic">
    <rdfs:label xml:lang="en">electronic</rdfs:label>
    <rdfs:subClassOf rdf:resource="jc3iedm_CAPABILITY.owl#SURVEILLANCE-CAPABILITY"/>
    <rdfs:comment xml:lang="en">The ability to gain information by exploiting non-communications electronic systems (generally pulsed).</rdfs:comment>
    <rdf:type rdf:resource="http://www.w3.org/2002/07/owl#Class"/>
  </rdf:Description>
  <rdf:Description rdf:about="#FIRE-CAPABILITY_Ground_to_ground">
    <rdfs:label xml:lang="en">ground to ground</rdfs:label>
    <rdfs:subClassOf rdf:resource="jc3iedm_CAPABILITY.owl#FIRE-CAPABILITY"/>
    <rdfs:comment xml:lang="en">The specific value implies that a specific FIRE-CAPABILITY involves surface firing.</rdfs:comment>
    <rdf:type rdf:resource="http://www.w3.org/2002/07/owl#Class"/>
  </rdf:Description>
  <rdf:Description rdf:about="#MOBILITY-CAPABILITY_Water,_nontidal">
    <rdfs:label xml:lang="en">water, nontidal</rdfs:label>
    <rdfs:subClassOf rdf:resource="jc3iedm_CAPABILITY.owl#MOBILITY-CAPABILITY"/>
    <rdfs:comment xml:lang="en">The capability of a device to navigate non-tidal waters.</rdfs:comment>
    <rdf:type rdf:resource="http://www.w3.org/2002/07/owl#Class"/>
  </rdf:Description>
  <rdf:Description rdf:about="#ENGINEERING-CAPABILITY_Breaching">
    <rdfs:label xml:lang="en">breaching</rdfs:label>
    <rdfs:subClassOf rdf:resource="jc3iedm_CAPABILITY.owl#ENGINEERING-CAPABILITY"/>
    <rdfs:comment xml:lang="en">The action or process of making a gap in a wall or barrier.</rdfs:comment>
    <rdf:type rdf:resource="http://www.w3.org/2002/07/owl#Class"/>
  </rdf:Description>
  <rdf:Description rdf:about="#OPERATIONAL-CAPABILITY_Target_acquisition">
    <rdfs:label xml:lang="en">target acquisition</rdfs:label>
    <rdfs:subClassOf rdf:resource="jc3iedm_CAPABILITY.owl#OPERATIONAL-CAPABILITY"/>
    <rdfs:comment xml:lang="en">The capability to manage, operate and maintain target acquisition assets.</rdfs:comment>
    <rdf:type rdf:resource="http://www.w3.org/2002/07/owl#Class"/>
  </rdf:Description>
  <rdf:Description rdf:about="#SUPPORT-CAPABILITY_Deck">
    <rdfs:label xml:lang="en">deck</rdfs:label>
    <rdfs:subClassOf rdf:resource="jc3iedm_CAPABILITY.owl#SUPPORT-CAPABILITY"/>
    <rdfs:comment xml:lang="en">The capability to provide deck supplies.</rdfs:comment>
    <rdf:type rdf:resource="http://www.w3.org/2002/07/owl#Class"/>
  </rdf:Description>
  <rdf:Description rdf:about="#OPERATIONAL-CAPABILITY_Supply_(class_III)">
    <rdfs:label xml:lang="en">supply (class iii)</rdfs:label>
    <rdfs:subClassOf rdf:resource="jc3iedm_CAPABILITY.owl#OPERATIONAL-CAPABILITY"/>
    <rdfs:comment xml:lang="en">The capability to provide fuel and lubricants.</rdfs:comment>
    <rdf:type rdf:resource="http://www.w3.org/2002/07/owl#Class"/>
  </rdf:Description>
  <rdf:Description rdf:about="#OPERATIONAL-CAPABILITY_Marine">
    <rdfs:label xml:lang="en">marine</rdfs:label>
    <rdfs:subClassOf rdf:resource="jc3iedm_CAPABILITY.owl#OPERATIONAL-CAPABILITY"/>
    <rdfs:comment xml:lang="en">The capability to perform maritime/littoral operations.</rdfs:comment>
    <rdf:type rdf:resource="http://www.w3.org/2002/07/owl#Class"/>
  </rdf:Description>
  <rdf:Description rdf:about="#OPERATIONAL-CAPABILITY_Air_interdiction">
    <rdfs:label xml:lang="en">air interdiction</rdfs:label>
    <rdfs:subClassOf rdf:resource="jc3iedm_CAPABILITY.owl#OPERATIONAL-CAPABILITY"/>
    <rdfs:comment xml:lang="en">Air operations conducted to destroy, neutralize, or delay the enemy's military potential before it can be brought to bear effectively against friendly forces at such distance from friendly forces that detailed integration of each air mission with the fire and movement of friendly forces is not required.</rdfs:comment>
    <rdf:type rdf:resource="http://www.w3.org/2002/07/owl#Class"/>
  </rdf:Description>
  <rdf:Description rdf:about="#OPERATIONAL-CAPABILITY_Signal,_node_centre">
    <rdfs:label xml:lang="en">signal, node centre</rdfs:label>
    <rdfs:subClassOf rdf:resource="jc3iedm_CAPABILITY.owl#OPERATIONAL-CAPABILITY"/>
    <rdfs:comment xml:lang="en">The capability in signal services to manage, operate and control a communications node centre.</rdfs:comment>
    <rdf:type rdf:resource="http://www.w3.org/2002/07/owl#Class"/>
  </rdf:Description>
  <rdf:Description rdf:about="#SUPPORT-CAPABILITY_Shelter">
    <rdfs:label xml:lang="en">shelter</rdfs:label>
    <rdfs:subClassOf rdf:resource="jc3iedm_CAPABILITY.owl#SUPPORT-CAPABILITY"/>
    <rdfs:comment xml:lang="en">The capability to provide shelter.</rdfs:comment>
    <rdf:type rdf:resource="http://www.w3.org/2002/07/owl#Class"/>
  </rdf:Description>
  <rdf:Description rdf:about="#MOBILITY-CAPABILITY_Land,_self-propelled">
    <rdfs:label xml:lang="en">land, self propelled</rdfs:label>
    <rdfs:subClassOf rdf:resource="jc3iedm_CAPABILITY.owl#MOBILITY-CAPABILITY"/>
    <rdfs:comment xml:lang="en">The capability of a device to move over land under its own power.</rdfs:comment>
    <rdf:type rdf:resource="http://www.w3.org/2002/07/owl#Class"/>
  </rdf:Description>
</rdf:RDF>
