<rdf:RDF
    xmlns:rdf="http://www.w3.org/1999/02/22-rdf-syntax-ns#"
    xmlns:owl="http://www.w3.org/2002/07/owl#"
    xmlns:xsd="http://www.w3.org/2001/XMLSchema#"
    xmlns:rdfs="http://www.w3.org/2000/01/rdf-schema#"
    xmlns="http://cbml.googlecode.com/svn/trunk/jc3iedmOnt/rootClassOnt/jc3iedm_OBJECT-TYPEExtended.owl#"
  xml:base="http://cbml.googlecode.com/svn/trunk/jc3iedmOnt/rootClassOnt/jc3iedm_OBJECT-TYPEExtended.owl#" > 
  <rdf:Description rdf:about="#CONTROL-FEATURE-TYPE_Low_altitude_missile_engagement_zone">
    <rdfs:subClassOf rdf:resource="jc3iedm_OBJECT-TYPE.owl#CONTROL-FEATURE-TYPE"/>
    <rdfs:label xml:lang="en">low altitude missile engagement zone</rdfs:label>
    <rdfs:comment xml:lang="en">Airspace within which the responsibility for engagement normally rests with the commander of the low-to-medium altitude GBAD systems.</rdfs:comment>
    <rdf:type rdf:resource="http://www.w3.org/2002/07/owl#Class"/>
  </rdf:Description>
  <rdf:Description rdf:about="#CONTROL-FEATURE-TYPE_Crossing_site">
    <rdfs:subClassOf rdf:resource="jc3iedm_OBJECT-TYPE.owl#CONTROL-FEATURE-TYPE"/>
    <rdfs:label xml:lang="en">crossing site</rdfs:label>
    <rdfs:comment xml:lang="en">The location along a water obstacle where the crossing can be made using amphibious vehicles, assault boats, rafts, bridges, or fording vehicles.</rdfs:comment>
    <rdf:type rdf:resource="http://www.w3.org/2002/07/owl#Class"/>
  </rdf:Description>
  <rdf:Description rdf:about="#TASK-FORMATION-TYPE_Not_otherwise_specified">
    <rdfs:subClassOf rdf:resource="jc3iedm_OBJECT-TYPE.owl#TASK-FORMATION-TYPE"/>
    <rdfs:label xml:lang="en">not otherwise specified</rdfs:label>
    <rdfs:comment xml:lang="en">The appropriate value is not in the set of specified values.</rdfs:comment>
    <rdf:type rdf:resource="http://www.w3.org/2002/07/owl#Class"/>
  </rdf:Description>
  <rdf:Description rdf:about="#SURFACE-VESSEL-TYPE_Barge,_repair,_berthing_and_messing">
    <rdfs:subClassOf rdf:resource="jc3iedm_OBJECT-TYPE.owl#SURFACE-VESSEL-TYPE"/>
    <rdfs:label xml:lang="en">barge, repair, berthing and messing</rdfs:label>
    <rdfs:comment xml:lang="en">Craft which both serves as a floating work ship and has berthing facilities for the assigned personnel. It provides messing facilities.</rdfs:comment>
    <rdf:type rdf:resource="http://www.w3.org/2002/07/owl#Class"/>
  </rdf:Description>
  <rdf:Description rdf:about="#CONTROL-FEATURE-TYPE_Special_operations_forces_airspace">
    <rdfs:subClassOf rdf:resource="jc3iedm_OBJECT-TYPE.owl#CONTROL-FEATURE-TYPE"/>
    <rdfs:label xml:lang="en">special operations forces airspace</rdfs:label>
    <rdfs:comment xml:lang="en">Airspace specifically for special operations forces missions requested by special operations forces airspace planners.</rdfs:comment>
    <rdf:type rdf:resource="http://www.w3.org/2002/07/owl#Class"/>
  </rdf:Description>
  <rdf:Description rdf:about="#SURFACE-VESSEL-TYPE_Destroyer,_helicopter_capable,_guided_missile">
    <rdfs:subClassOf rdf:resource="jc3iedm_OBJECT-TYPE.owl#SURFACE-VESSEL-TYPE"/>
    <rdfs:label xml:lang="en">destroyer, helicopter capable, guided missile</rdfs:label>
    <rdfs:comment xml:lang="en">A destroyer type ship fitted with one more force guided missile systems and with a flight deck with a primary mission of operating and maintaining helicopters. Major surface combatant in range of about 95 to 140 metres whole general mission is to operations with strike, ASW and amphibious forces, and to perform screening and convoy duties. May have helicopters not especially fitted for ASW.</rdfs:comment>
    <rdf:type rdf:resource="http://www.w3.org/2002/07/owl#Class"/>
  </rdf:Description>
  <rdf:Description rdf:about="#CONTROL-FEATURE-TYPE_Special_electronic_mission_area">
    <rdfs:subClassOf rdf:resource="jc3iedm_OBJECT-TYPE.owl#CONTROL-FEATURE-TYPE"/>
    <rdfs:label xml:lang="en">special electronic mission area</rdfs:label>
    <rdfs:comment xml:lang="en">Airspace established specifically for airborne platforms conducting special electronic missions.</rdfs:comment>
    <rdf:type rdf:resource="http://www.w3.org/2002/07/owl#Class"/>
  </rdf:Description>
  <rdf:Description rdf:about="#CONTROL-FEATURE-TYPE_Identification_safety_range">
    <rdfs:subClassOf rdf:resource="jc3iedm_OBJECT-TYPE.owl#CONTROL-FEATURE-TYPE"/>
    <rdfs:label xml:lang="en">identification safety range</rdfs:label>
    <rdfs:comment xml:lang="en">Minimum range to which an aircraft may close to a maritime force without having been positively identified as friendly.</rdfs:comment>
    <rdf:type rdf:resource="http://www.w3.org/2002/07/owl#Class"/>
  </rdf:Description>
  <rdf:Description rdf:about="#VEHICLE-TYPE_Battle_tank,_medium,_recovery">
    <rdfs:subClassOf rdf:resource="jc3iedm_OBJECT-TYPE.owl#VEHICLE-TYPE"/>
    <rdfs:label xml:lang="en">battle tank, medium, recovery</rdfs:label>
    <rdfs:comment xml:lang="en">A vehicle designed to recover medium weight battle tanks.</rdfs:comment>
    <rdf:type rdf:resource="http://www.w3.org/2002/07/owl#Class"/>
  </rdf:Description>
  <rdf:Description rdf:about="#FACILITY-TYPE_Gas_processing_facility">
    <rdfs:subClassOf rdf:resource="jc3iedm_OBJECT-TYPE.owl#FACILITY-TYPE"/>
    <rdfs:label xml:lang="en">gas processing facility</rdfs:label>
    <rdfs:comment xml:lang="en">Installations for processing and purification of natural gas or separating natural gas from crude oil.</rdfs:comment>
    <rdf:type rdf:resource="http://www.w3.org/2002/07/owl#Class"/>
  </rdf:Description>
  <rdf:Description rdf:about="#ROUTE-TYPE_Maritime_minefield_sweep_track">
    <rdfs:subClassOf rdf:resource="jc3iedm_OBJECT-TYPE.owl#ROUTE-TYPE"/>
    <rdfs:label xml:lang="en">maritime minefield sweep track</rdfs:label>
    <rdfs:comment xml:lang="en">The prescribed line over the ground along which the centre of the mine counter measures gear must travel in order that the lane swept can be defined by the width and the depth swept.</rdfs:comment>
    <rdf:type rdf:resource="http://www.w3.org/2002/07/owl#Class"/>
  </rdf:Description>
  <rdf:Description rdf:about="#SURFACE-VESSEL-TYPE_Degaussing_vessel">
    <rdfs:subClassOf rdf:resource="jc3iedm_OBJECT-TYPE.owl#SURFACE-VESSEL-TYPE"/>
    <rdfs:label xml:lang="en">degaussing vessel</rdfs:label>
    <rdfs:comment xml:lang="en">Vessel of any size used for degaussing purposes.</rdfs:comment>
    <rdf:type rdf:resource="http://www.w3.org/2002/07/owl#Class"/>
  </rdf:Description>
  <rdf:Description rdf:about="#CONTROL-FEATURE-TYPE_Standard_surface_to_air_missile_engagement_zone">
    <rdfs:subClassOf rdf:resource="jc3iedm_OBJECT-TYPE.owl#CONTROL-FEATURE-TYPE"/>
    <rdfs:label xml:lang="en">standard surface to air missile engagement zone</rdfs:label>
    <rdfs:comment xml:lang="en">A designated airspace in which, under weapons control status (WCS) Weapons Free, ships are automatically cleared to fire at any target which penetrates the zone, unless known to be friendly, adhering to airspace control (ASC) procedures or unless otherwise directed by the AAWC (anti air warfare commander).</rdfs:comment>
    <rdf:type rdf:resource="http://www.w3.org/2002/07/owl#Class"/>
  </rdf:Description>
  <rdf:Description rdf:about="#ORGANISATION-TYPE_Command_post">
    <rdfs:subClassOf rdf:resource="jc3iedm_OBJECT-TYPE.owl#ORGANISATION-TYPE"/>
    <rdfs:label xml:lang="en">command post</rdfs:label>
    <rdfs:comment xml:lang="en">The ORGANISATION-TYPE is a command post.</rdfs:comment>
    <rdf:type rdf:resource="http://www.w3.org/2002/07/owl#Class"/>
  </rdf:Description>
  <rdf:Description rdf:about="#FACILITY-TYPE_Medical_facility,_unit_medical_station">
    <rdfs:subClassOf rdf:resource="jc3iedm_OBJECT-TYPE.owl#FACILITY-TYPE"/>
    <rdfs:label xml:lang="en">medical facility, unit medical station</rdfs:label>
    <rdfs:comment xml:lang="en">A facility used as a first level care medical facility for a unit.</rdfs:comment>
    <rdf:type rdf:resource="http://www.w3.org/2002/07/owl#Class"/>
  </rdf:Description>
  <rdf:Description rdf:about="jc3iedm_OBJECT-TYPE.owl#government-organisation-type-main-activity-code">
    <rdf:type rdf:resource="http://www.w3.org/2002/07/owl#DatatypeProperty"/>
    <rdfs:domain rdf:resource="jc3iedm_OBJECT-TYPE.owl#GOVERNMENT-ORGANISATION-TYPE"/>
    <rdfs:range rdf:resource="http://www.w3.org/2001/XMLSchema#string"/>
  </rdf:Description>
  <rdf:Description rdf:about="#SURFACE-VESSEL-TYPE_Oceanographic_research_ship,_polar">
    <rdfs:subClassOf rdf:resource="jc3iedm_OBJECT-TYPE.owl#SURFACE-VESSEL-TYPE"/>
    <rdfs:label xml:lang="en">oceanographic research ship, polar</rdfs:label>
    <rdfs:comment xml:lang="en">Ship which conducts multi-discipline research at sea in oceanographic radiomagnetics, meteorology and oceanography, specially fitted for ice operations. Must have icebreaker bow.</rdfs:comment>
    <rdf:type rdf:resource="http://www.w3.org/2002/07/owl#Class"/>
  </rdf:Description>
  <rdf:Description rdf:about="#CONTROL-FEATURE-TYPE_Boundary,_organisation">
    <rdfs:subClassOf rdf:resource="jc3iedm_OBJECT-TYPE.owl#CONTROL-FEATURE-TYPE"/>
    <rdfs:label xml:lang="en">boundary, organisation</rdfs:label>
    <rdfs:comment xml:lang="en">1. A line which delineates surface areas (or airspace) for the purpose of facilitating coordination and deconfliction of operations between adjacent units, formations or areas. 2. A control measure normally drawn along identifiable terrain features and used to delineate areas of tactical responsibility between adjacent units and between higher headquarters to the rear of the subordinate units. Control measures which define the left and right limits of a unit's zone of action or sector. Together with the rear and forward boundary and a coordinating altitude, lateral boundaries define the area of operations for a commander.</rdfs:comment>
    <rdf:type rdf:resource="http://www.w3.org/2002/07/owl#Class"/>
  </rdf:Description>
  <rdf:Description rdf:about="#SURFACE-VESSEL-TYPE_Merchant_ship,_tug,_ocean-going_salvage">
    <rdfs:subClassOf rdf:resource="jc3iedm_OBJECT-TYPE.owl#SURFACE-VESSEL-TYPE"/>
    <rdfs:label xml:lang="en">merchant ship, tug, ocean going salvage</rdfs:label>
    <rdfs:comment xml:lang="en">Non-naval sea-going tug that can provide towing, salvage, repair, diving and rescue services to ships and craft.</rdfs:comment>
    <rdf:type rdf:resource="http://www.w3.org/2002/07/owl#Class"/>
  </rdf:Description>
  <rdf:Description rdf:about="#CONSUMABLE-MATERIEL-TYPE_Drug">
    <rdfs:subClassOf rdf:resource="jc3iedm_OBJECT-TYPE.owl#CONSUMABLE-MATERIEL-TYPE"/>
    <rdfs:label xml:lang="en">drug</rdfs:label>
    <rdfs:comment xml:lang="en">A narcotic, hallucinogen, or stimulant, esp. one causing addiction.</rdfs:comment>
    <rdf:type rdf:resource="http://www.w3.org/2002/07/owl#Class"/>
  </rdf:Description>
  <rdf:Description rdf:about="#FACILITY-TYPE_Water_supply">
    <rdfs:subClassOf rdf:resource="jc3iedm_OBJECT-TYPE.owl#FACILITY-TYPE"/>
    <rdfs:label xml:lang="en">water supply</rdfs:label>
    <rdfs:comment xml:lang="en">A facility containing the equipment used for the storage and/or distribution of water.</rdfs:comment>
    <rdf:type rdf:resource="http://www.w3.org/2002/07/owl#Class"/>
  </rdf:Description>
  <rdf:Description rdf:about="#FACILITY-TYPE_Production_complex,_guided_missile">
    <rdfs:subClassOf rdf:resource="jc3iedm_OBJECT-TYPE.owl#FACILITY-TYPE"/>
    <rdfs:label xml:lang="en">production complex, guided missile</rdfs:label>
    <rdfs:comment xml:lang="en">A facility used for production of guided missiles.</rdfs:comment>
    <rdf:type rdf:resource="http://www.w3.org/2002/07/owl#Class"/>
  </rdf:Description>
  <rdf:Description rdf:about="jc3iedm_OBJECT-TYPE.owl#weapon-type-subcategory-code">
    <rdf:type rdf:resource="http://www.w3.org/2002/07/owl#DatatypeProperty"/>
    <rdfs:domain rdf:resource="jc3iedm_OBJECT-TYPE.owl#WEAPON-TYPE"/>
    <rdfs:range rdf:resource="http://www.w3.org/2001/XMLSchema#string"/>
  </rdf:Description>
  <rdf:Description rdf:about="#AMMUNITION-TYPE_Rocket/missile,_medium">
    <rdfs:subClassOf rdf:resource="jc3iedm_OBJECT-TYPE.owl#AMMUNITION-TYPE"/>
    <rdfs:label xml:lang="en">rocket/missile, medium</rdfs:label>
    <rdfs:comment xml:lang="en">A powered projectile designed for use by medium launchers.</rdfs:comment>
    <rdf:type rdf:resource="http://www.w3.org/2002/07/owl#Class"/>
  </rdf:Description>
  <rdf:Description rdf:about="#UNIT-TYPE_Armoured_anti_armour">
    <rdfs:subClassOf rdf:resource="jc3iedm_OBJECT-TYPE.owl#UNIT-TYPE"/>
    <rdfs:label xml:lang="en">armoured anti armour</rdfs:label>
    <rdfs:comment xml:lang="en">A UNIT-TYPE equipped with armoured vehicles whose principal designation is the employment of direct fire weapon systems against armoured vehicles.</rdfs:comment>
    <rdf:type rdf:resource="http://www.w3.org/2002/07/owl#Class"/>
  </rdf:Description>
  <rdf:Description rdf:about="jc3iedm_OBJECT-TYPE.owl#aircraft-type-model-code">
    <rdf:type rdf:resource="http://www.w3.org/2002/07/owl#DatatypeProperty"/>
    <rdfs:domain rdf:resource="jc3iedm_OBJECT-TYPE.owl#AIRCRAFT-TYPE"/>
    <rdfs:range rdf:resource="http://www.w3.org/2001/XMLSchema#string"/>
  </rdf:Description>
  <rdf:Description rdf:about="#CONTROL-FEATURE-TYPE_Flight_information_region">
    <rdfs:subClassOf rdf:resource="jc3iedm_OBJECT-TYPE.owl#CONTROL-FEATURE-TYPE"/>
    <rdfs:label xml:lang="en">flight information region</rdfs:label>
    <rdfs:comment xml:lang="en">An airspace of defined dimensions within which flight information service and alerting service are provided.</rdfs:comment>
    <rdf:type rdf:resource="http://www.w3.org/2002/07/owl#Class"/>
  </rdf:Description>
  <rdf:Description rdf:about="#CONTROL-FEATURE-TYPE_Weapon_control_area">
    <rdfs:subClassOf rdf:resource="jc3iedm_OBJECT-TYPE.owl#CONTROL-FEATURE-TYPE"/>
    <rdfs:label xml:lang="en">weapon control area</rdfs:label>
    <rdfs:comment xml:lang="en">The area in which a specified weapon control status is imposed.</rdfs:comment>
    <rdf:type rdf:resource="http://www.w3.org/2002/07/owl#Class"/>
  </rdf:Description>
  <rdf:Description rdf:about="#SURFACE-VESSEL-TYPE_Minelayer,_river">
    <rdfs:subClassOf rdf:resource="jc3iedm_OBJECT-TYPE.owl#SURFACE-VESSEL-TYPE"/>
    <rdfs:label xml:lang="en">minelayer, river</rdfs:label>
    <rdfs:comment xml:lang="en">Small minelayer 15 metres or less suitable only for operations on rivers or in protected roadsteads.</rdfs:comment>
    <rdf:type rdf:resource="http://www.w3.org/2002/07/owl#Class"/>
  </rdf:Description>
  <rdf:Description rdf:about="#FACILITY-TYPE_Forward_observer_position">
    <rdfs:subClassOf rdf:resource="jc3iedm_OBJECT-TYPE.owl#FACILITY-TYPE"/>
    <rdfs:label xml:lang="en">forward observer position</rdfs:label>
    <rdfs:comment xml:lang="en">A facility from which military observations are made or fires directed and adjusted by the occupants and which possesses appropriate communications; it may be airborne.</rdfs:comment>
    <rdf:type rdf:resource="http://www.w3.org/2002/07/owl#Class"/>
  </rdf:Description>
  <rdf:Description rdf:about="#SURFACE-VESSEL-TYPE_Training_ship,_small_(naval)">
    <rdfs:subClassOf rdf:resource="jc3iedm_OBJECT-TYPE.owl#SURFACE-VESSEL-TYPE"/>
    <rdfs:label xml:lang="en">training ship, small (naval)</rdfs:label>
    <rdfs:comment xml:lang="en">Large non-ocean-going ship designed to serve as a training ship.</rdfs:comment>
    <rdf:type rdf:resource="http://www.w3.org/2002/07/owl#Class"/>
  </rdf:Description>
  <rdf:Description rdf:about="#SURFACE-VESSEL-TYPE_Houseboat">
    <rdfs:subClassOf rdf:resource="jc3iedm_OBJECT-TYPE.owl#SURFACE-VESSEL-TYPE"/>
    <rdfs:label xml:lang="en">houseboat</rdfs:label>
    <rdfs:comment xml:lang="en">Vessel designed or converted to provide living accommodation.</rdfs:comment>
    <rdf:type rdf:resource="http://www.w3.org/2002/07/owl#Class"/>
  </rdf:Description>
  <rdf:Description rdf:about="#CONTROL-FEATURE-TYPE_Missile_engagement_zone,_general">
    <rdfs:subClassOf rdf:resource="jc3iedm_OBJECT-TYPE.owl#CONTROL-FEATURE-TYPE"/>
    <rdfs:label xml:lang="en">missile engagement zone, general</rdfs:label>
    <rdfs:comment xml:lang="en">In air defence, that airspace of defined dimensions within which the responsibility for engagement of air threats normally rests with short-range air defence weapons. It may be established within a low or high altitude missile engagement.</rdfs:comment>
    <rdf:type rdf:resource="http://www.w3.org/2002/07/owl#Class"/>
  </rdf:Description>
  <rdf:Description rdf:about="jc3iedm_OBJECT-TYPE.owl#consumable-materiel-type-perishability-indicator-code">
    <rdf:type rdf:resource="http://www.w3.org/2002/07/owl#DatatypeProperty"/>
    <rdfs:domain rdf:resource="jc3iedm_OBJECT-TYPE.owl#CONSUMABLE-MATERIEL-TYPE"/>
    <rdfs:range rdf:resource="http://www.w3.org/2001/XMLSchema#string"/>
  </rdf:Description>
  <rdf:Description rdf:about="#CONTROL-FEATURE-TYPE_Biological_concentration_time_contour_line">
    <rdfs:subClassOf rdf:resource="jc3iedm_OBJECT-TYPE.owl#CONTROL-FEATURE-TYPE"/>
    <rdfs:label xml:lang="en">biological concentration time contour line</rdfs:label>
    <rdfs:comment xml:lang="en">A line on a map, diagram or overlay joining all points at which the biological concentration-time (for which a quantified portion of exposed personnel are expected to experience (or not experience) effects of given severity) at a given time is the same. Biological concentration time is the product of the concentration of a biological substance in the atmosphere and the exposure time.</rdfs:comment>
    <rdf:type rdf:resource="http://www.w3.org/2002/07/owl#Class"/>
  </rdf:Description>
  <rdf:Description rdf:about="#FACILITY-TYPE_Supply_dump">
    <rdfs:subClassOf rdf:resource="jc3iedm_OBJECT-TYPE.owl#FACILITY-TYPE"/>
    <rdfs:label xml:lang="en">supply dump</rdfs:label>
    <rdfs:comment xml:lang="en">A temporary storage area, usually in the open, for bombs, ammunition, equipment, or supplies.</rdfs:comment>
    <rdf:type rdf:resource="http://www.w3.org/2002/07/owl#Class"/>
  </rdf:Description>
  <rdf:Description rdf:about="#MISCELLANEOUS-EQUIPMENT-TYPE_Cable">
    <rdfs:subClassOf rdf:resource="jc3iedm_OBJECT-TYPE.owl#MISCELLANEOUS-EQUIPMENT-TYPE"/>
    <rdfs:label xml:lang="en">cable</rdfs:label>
    <rdfs:comment xml:lang="en">A strong thick rope of hemp or wire.</rdfs:comment>
    <rdf:type rdf:resource="http://www.w3.org/2002/07/owl#Class"/>
  </rdf:Description>
  <rdf:Description rdf:about="#CONTROL-FEATURE-TYPE_Ship_control_zone">
    <rdfs:subClassOf rdf:resource="jc3iedm_OBJECT-TYPE.owl#CONTROL-FEATURE-TYPE"/>
    <rdfs:label xml:lang="en">ship control zone</rdfs:label>
    <rdfs:comment xml:lang="en">An area activated around a ship operating aircraft, which is not to be entered by friendly aircraft without permission, in order to prevent friendly interference.</rdfs:comment>
    <rdf:type rdf:resource="http://www.w3.org/2002/07/owl#Class"/>
  </rdf:Description>
  <rdf:Description rdf:about="#ROUTE-TYPE_Polar_route">
    <rdfs:subClassOf rdf:resource="jc3iedm_OBJECT-TYPE.owl#ROUTE-TYPE"/>
    <rdfs:label xml:lang="en">polar route</rdfs:label>
    <rdfs:comment xml:lang="en">Polar route.</rdfs:comment>
    <rdf:type rdf:resource="http://www.w3.org/2002/07/owl#Class"/>
  </rdf:Description>
  <rdf:Description rdf:about="#CONTROL-FEATURE-TYPE_Unexploded_ordnance_area">
    <rdfs:subClassOf rdf:resource="jc3iedm_OBJECT-TYPE.owl#CONTROL-FEATURE-TYPE"/>
    <rdfs:label xml:lang="en">unexploded ordnance area</rdfs:label>
    <rdfs:comment xml:lang="en">An area in which there are unexploded ordnance. Explosive ordnance which has been primed, fused, armed, or otherwise prepared for action, and which has been fired, dropped, launched, or placed in such a manner as to constitute a hazard to operations, installations, personnel, or material, and remains unexploded either by malfunction or for any other cause.</rdfs:comment>
    <rdf:type rdf:resource="http://www.w3.org/2002/07/owl#Class"/>
  </rdf:Description>
  <rdf:Description rdf:about="jc3iedm_OBJECT-TYPE.owl#HARBOUR-TYPE">
    <rdf:type rdf:resource="http://www.w3.org/2002/07/owl#Class"/>
    <rdfs:label xml:lang="en">harbour type</rdfs:label>
    <rdfs:comment xml:lang="en">A FACILITY-TYPE that is a restricted body of water, an anchorage, or other limited coastal water area and its water approaches from which and in which shipping operations are projected or supported.</rdfs:comment>
    <rdfs:subClassOf rdf:resource="jc3iedm_OBJECT-TYPE.owl#FACILITY-TYPE"/>
  </rdf:Description>
  <rdf:Description rdf:about="#SURFACE-VESSEL-TYPE_Dry_dock_floating,_closed,_medium">
    <rdfs:subClassOf rdf:resource="jc3iedm_OBJECT-TYPE.owl#SURFACE-VESSEL-TYPE"/>
    <rdfs:label xml:lang="en">dry dock floating, closed, medium</rdfs:label>
    <rdfs:comment xml:lang="en">Non-self-propelled dry dock, closed bow and stern between 60-200 metres.</rdfs:comment>
    <rdf:type rdf:resource="http://www.w3.org/2002/07/owl#Class"/>
  </rdf:Description>
  <rdf:Description rdf:about="#CONSUMABLE-MATERIEL-TYPE_Personal_equipment">
    <rdfs:subClassOf rdf:resource="jc3iedm_OBJECT-TYPE.owl#CONSUMABLE-MATERIEL-TYPE"/>
    <rdfs:label xml:lang="en">personal equipment</rdfs:label>
    <rdfs:comment xml:lang="en">Equipment issued to or carried by an individual.</rdfs:comment>
    <rdf:type rdf:resource="http://www.w3.org/2002/07/owl#Class"/>
  </rdf:Description>
  <rdf:Description rdf:about="jc3iedm_OBJECT-TYPE.owl#aircraft-type-military-civilian-code">
    <rdf:type rdf:resource="http://www.w3.org/2002/07/owl#DatatypeProperty"/>
    <rdfs:domain rdf:resource="jc3iedm_OBJECT-TYPE.owl#AIRCRAFT-TYPE"/>
    <rdfs:range rdf:resource="http://www.w3.org/2001/XMLSchema#string"/>
  </rdf:Description>
  <rdf:Description rdf:about="#UNIT-TYPE_NBC">
    <rdfs:subClassOf rdf:resource="jc3iedm_OBJECT-TYPE.owl#UNIT-TYPE"/>
    <rdfs:label xml:lang="en">nbc</rdfs:label>
    <rdfs:comment xml:lang="en">A UNIT-TYPE whose principal designation is chemical, biological, radiological, or nuclear materiel defence.</rdfs:comment>
    <rdf:type rdf:resource="http://www.w3.org/2002/07/owl#Class"/>
  </rdf:Description>
  <rdf:Description rdf:about="#FACILITY-TYPE_Radar_post">
    <rdfs:subClassOf rdf:resource="jc3iedm_OBJECT-TYPE.owl#FACILITY-TYPE"/>
    <rdfs:label xml:lang="en">radar post</rdfs:label>
    <rdfs:comment xml:lang="en">No definition provided in ADatP-3 Baseline 13.1 FFIRN/FUD 1874/4.</rdfs:comment>
    <rdf:type rdf:resource="http://www.w3.org/2002/07/owl#Class"/>
  </rdf:Description>
  <rdf:Description rdf:about="#CONTROL-FEATURE-TYPE_Orbit_point">
    <rdfs:subClassOf rdf:resource="jc3iedm_OBJECT-TYPE.owl#CONTROL-FEATURE-TYPE"/>
    <rdfs:label xml:lang="en">orbit point</rdfs:label>
    <rdfs:comment xml:lang="en">A geographically or electronically defined location used in stationing aircraft in flight during tactical operations when a predetermined pattern is not established.</rdfs:comment>
    <rdf:type rdf:resource="http://www.w3.org/2002/07/owl#Class"/>
  </rdf:Description>
  <rdf:Description rdf:about="#FACILITY-TYPE_Military_base/facility,_submarine">
    <rdfs:subClassOf rdf:resource="jc3iedm_OBJECT-TYPE.owl#FACILITY-TYPE"/>
    <rdfs:label xml:lang="en">military base/facility, submarine</rdfs:label>
    <rdfs:comment xml:lang="en">A facility that is used as a naval base and where submarines may receive or discharge their cargoes or receive maintenance.</rdfs:comment>
    <rdf:type rdf:resource="http://www.w3.org/2002/07/owl#Class"/>
  </rdf:Description>
  <rdf:Description rdf:about="#HARBOUR-TYPE_Coastal_(Natural)">
    <rdfs:subClassOf rdf:resource="jc3iedm_OBJECT-TYPE.owl#HARBOUR-TYPE"/>
    <rdfs:label xml:lang="en">coastal (natural)</rdfs:label>
    <rdfs:comment xml:lang="en">A coastal harbour sheltered from the wind and sea by virtue of its location within a natural coastal indentation or in the protective lee of an island, cape, reef or other natural barrier.</rdfs:comment>
    <rdf:type rdf:resource="http://www.w3.org/2002/07/owl#Class"/>
  </rdf:Description>
  <rdf:Description rdf:about="#CONTROL-FEATURE-TYPE_Artillery_area">
    <rdfs:subClassOf rdf:resource="jc3iedm_OBJECT-TYPE.owl#CONTROL-FEATURE-TYPE"/>
    <rdfs:label xml:lang="en">artillery area</rdfs:label>
    <rdfs:comment xml:lang="en">A CONTROL-FEATURE-TYPE with an area location assigned to artillery units for terrain management purposes on which the artillery manoeuvres.</rdfs:comment>
    <rdf:type rdf:resource="http://www.w3.org/2002/07/owl#Class"/>
  </rdf:Description>
  <rdf:Description rdf:about="#SURFACE-VESSEL-TYPE_Command_craft,_miscellaneous">
    <rdfs:subClassOf rdf:resource="jc3iedm_OBJECT-TYPE.owl#SURFACE-VESSEL-TYPE"/>
    <rdfs:label xml:lang="en">command craft, miscellaneous</rdfs:label>
    <rdfs:comment xml:lang="en">Craft 40 metres or less employed as a command ship but not designed for use at sea.</rdfs:comment>
    <rdf:type rdf:resource="http://www.w3.org/2002/07/owl#Class"/>
  </rdf:Description>
  <rdf:Description rdf:about="#FACILITY-TYPE_Service,_research,_utility_facility,_public_water_service">
    <rdfs:subClassOf rdf:resource="jc3iedm_OBJECT-TYPE.owl#FACILITY-TYPE"/>
    <rdfs:label xml:lang="en">service, research, utility facility, public water service</rdfs:label>
    <rdfs:comment xml:lang="en">A facility generally used to support service, research or utility functions in support of public water services.</rdfs:comment>
    <rdf:type rdf:resource="http://www.w3.org/2002/07/owl#Class"/>
  </rdf:Description>
  <rdf:Description rdf:about="#PRIVATE-SECTOR-ORGANISATION-TYPE_Fishing_industry">
    <rdfs:subClassOf rdf:resource="jc3iedm_OBJECT-TYPE.owl#PRIVATE-SECTOR-ORGANISATION-TYPE"/>
    <rdfs:label xml:lang="en">fishing industry</rdfs:label>
    <rdfs:comment xml:lang="en">A PRIVATE-SECTOR-ORGANISATION-TYPE whose predominant business is the production and processing of seafood products.</rdfs:comment>
    <rdf:type rdf:resource="http://www.w3.org/2002/07/owl#Class"/>
  </rdf:Description>
  <rdf:Description rdf:about="jc3iedm_OBJECT-TYPE.owl#RADIOACTIVE-MATERIEL-TYPE">
    <rdf:type rdf:resource="http://www.w3.org/2002/07/owl#Class"/>
    <rdfs:label xml:lang="en">radioactive materiel type</rdfs:label>
    <rdfs:comment xml:lang="en">A CONSUMABLE-MATERIEL-TYPE that is a substance which spontaneously emits radiation, and which may kill, seriously injure, or incapacitate personnel through its physiological effects or causes the deterioration of materiel.</rdfs:comment>
    <rdfs:subClassOf rdf:resource="jc3iedm_OBJECT-TYPE.owl#CONSUMABLE-MATERIEL-TYPE"/>
  </rdf:Description>
  <rdf:Description rdf:about="#SUBSURFACE-VESSEL-TYPE_Submarine,_coastal">
    <rdfs:subClassOf rdf:resource="jc3iedm_OBJECT-TYPE.owl#SUBSURFACE-VESSEL-TYPE"/>
    <rdfs:label xml:lang="en">submarine, coastal</rdfs:label>
    <rdfs:comment xml:lang="en">Submarine designed primarily for operations in coastal and shallow waters.</rdfs:comment>
    <rdf:type rdf:resource="http://www.w3.org/2002/07/owl#Class"/>
  </rdf:Description>
  <rdf:Description rdf:about="#SURFACE-VESSEL-TYPE_Patrol_craft,_torpedo">
    <rdfs:subClassOf rdf:resource="jc3iedm_OBJECT-TYPE.owl#SURFACE-VESSEL-TYPE"/>
    <rdfs:label xml:lang="en">patrol craft, torpedo</rdfs:label>
    <rdfs:comment xml:lang="en">High-speed (35 knots) anti-surface ship patrol craft in size range 20 - 30 metres fitted with torpedoes.</rdfs:comment>
    <rdf:type rdf:resource="http://www.w3.org/2002/07/owl#Class"/>
  </rdf:Description>
  <rdf:Description rdf:about="#CONTROL-FEATURE-TYPE_Unmanned_aerial_vehicle_airspace">
    <rdfs:subClassOf rdf:resource="jc3iedm_OBJECT-TYPE.owl#CONTROL-FEATURE-TYPE"/>
    <rdfs:label xml:lang="en">unmanned aerial vehicle airspace</rdfs:label>
    <rdfs:comment xml:lang="en">Airspace created specifically for unmanned aerial vehicle operations.</rdfs:comment>
    <rdf:type rdf:resource="http://www.w3.org/2002/07/owl#Class"/>
  </rdf:Description>
  <rdf:Description rdf:about="#FACILITY-TYPE_Prisoner_of_war_holding_area">
    <rdfs:subClassOf rdf:resource="jc3iedm_OBJECT-TYPE.owl#FACILITY-TYPE"/>
    <rdfs:label xml:lang="en">prisoner of war holding area</rdfs:label>
    <rdfs:comment xml:lang="en">A facility where Prisoners of war are provided custodial care pending further disposition.</rdfs:comment>
    <rdf:type rdf:resource="http://www.w3.org/2002/07/owl#Class"/>
  </rdf:Description>
  <rdf:Description rdf:about="#FACILITY-TYPE_Personnel_barrier">
    <rdfs:subClassOf rdf:resource="jc3iedm_OBJECT-TYPE.owl#FACILITY-TYPE"/>
    <rdfs:label xml:lang="en">personnel barrier</rdfs:label>
    <rdfs:comment xml:lang="en">A coordinated series of obstacles designed or employed to detect, channel, direct, restrict, delay or stop the movement of personnel.</rdfs:comment>
    <rdf:type rdf:resource="http://www.w3.org/2002/07/owl#Class"/>
  </rdf:Description>
  <rdf:Description rdf:about="#SURFACE-VESSEL-TYPE_Amphibious_transport,_dock">
    <rdfs:subClassOf rdf:resource="jc3iedm_OBJECT-TYPE.owl#SURFACE-VESSEL-TYPE"/>
    <rdfs:label xml:lang="en">amphibious transport, dock</rdfs:label>
    <rdfs:comment xml:lang="en">Ship that carries about 1000 troops. Capable of carrying up to 9 LCM (Landing craft, mechanized). Primarily a troop ship and armoured car carrier, with considerable internal berthing space. Must have permanent helicopter platform.</rdfs:comment>
    <rdf:type rdf:resource="http://www.w3.org/2002/07/owl#Class"/>
  </rdf:Description>
  <rdf:Description rdf:about="#MARITIME-EQUIPMENT-TYPE_Float">
    <rdfs:subClassOf rdf:resource="jc3iedm_OBJECT-TYPE.owl#MARITIME-EQUIPMENT-TYPE"/>
    <rdfs:label xml:lang="en">float</rdfs:label>
    <rdfs:comment xml:lang="en">A cork or other buoyant object that is used to support other equipment, a mine sweep wire for surface minesweepng.</rdfs:comment>
    <rdf:type rdf:resource="http://www.w3.org/2002/07/owl#Class"/>
  </rdf:Description>
  <rdf:Description rdf:about="#FACILITY-TYPE_Ammunition_supply_point">
    <rdfs:subClassOf rdf:resource="jc3iedm_OBJECT-TYPE.owl#FACILITY-TYPE"/>
    <rdfs:label xml:lang="en">ammunition supply point</rdfs:label>
    <rdfs:comment xml:lang="en">A facility at which ammunition, obtained from supporting supply points by a division or other unit, are broken down for distribution to other units.</rdfs:comment>
    <rdf:type rdf:resource="http://www.w3.org/2002/07/owl#Class"/>
  </rdf:Description>
  <rdf:Description rdf:about="#FACILITY-TYPE_Freight_terminal">
    <rdfs:subClassOf rdf:resource="jc3iedm_OBJECT-TYPE.owl#FACILITY-TYPE"/>
    <rdfs:label xml:lang="en">freight terminal</rdfs:label>
    <rdfs:comment xml:lang="en">A facility processing 'goods' in transit or being transferred from one transportation means to another.</rdfs:comment>
    <rdf:type rdf:resource="http://www.w3.org/2002/07/owl#Class"/>
  </rdf:Description>
  <rdf:Description rdf:about="jc3iedm_OBJECT-TYPE.owl#chemical-materiel-type-subcategory-code">
    <rdf:type rdf:resource="http://www.w3.org/2002/07/owl#DatatypeProperty"/>
    <rdfs:domain rdf:resource="jc3iedm_OBJECT-TYPE.owl#CHEMICAL-MATERIEL-TYPE"/>
    <rdfs:range rdf:resource="http://www.w3.org/2001/XMLSchema#string"/>
  </rdf:Description>
  <rdf:Description rdf:about="#CONTROL-FEATURE-TYPE_Ambulance_exchange_point">
    <rdfs:subClassOf rdf:resource="jc3iedm_OBJECT-TYPE.owl#CONTROL-FEATURE-TYPE"/>
    <rdfs:label xml:lang="en">ambulance exchange point</rdfs:label>
    <rdfs:comment xml:lang="en">A location where a patient is transferred from one ambulance to another en-route to a medical treatment facility. This may be an established point in an ambulance shuttle system or it may be designated independently.</rdfs:comment>
    <rdf:type rdf:resource="http://www.w3.org/2002/07/owl#Class"/>
  </rdf:Description>
  <rdf:Description rdf:about="#FACILITY-TYPE_Refugee_holding_area">
    <rdfs:subClassOf rdf:resource="jc3iedm_OBJECT-TYPE.owl#FACILITY-TYPE"/>
    <rdfs:label xml:lang="en">refugee holding area</rdfs:label>
    <rdfs:comment xml:lang="en">A facility where refugees are assembled for classification, sorting or further movement to other facilities or installations.</rdfs:comment>
    <rdf:type rdf:resource="http://www.w3.org/2002/07/owl#Class"/>
  </rdf:Description>
  <rdf:Description rdf:about="#MISCELLANEOUS-EQUIPMENT-TYPE_Container">
    <rdfs:subClassOf rdf:resource="jc3iedm_OBJECT-TYPE.owl#MISCELLANEOUS-EQUIPMENT-TYPE"/>
    <rdfs:label xml:lang="en">container</rdfs:label>
    <rdfs:comment xml:lang="en">A receptacle in which material is held or carried.</rdfs:comment>
    <rdf:type rdf:resource="http://www.w3.org/2002/07/owl#Class"/>
  </rdf:Description>
  <rdf:Description rdf:about="#FACILITY-TYPE_Steeple/spire">
    <rdfs:subClassOf rdf:resource="jc3iedm_OBJECT-TYPE.owl#FACILITY-TYPE"/>
    <rdfs:label xml:lang="en">steeple/spire</rdfs:label>
    <rdfs:comment xml:lang="en">In architecture, a steeply pointed pyramidal or conical structure usually attached to an ecclesiastical or public building.</rdfs:comment>
    <rdf:type rdf:resource="http://www.w3.org/2002/07/owl#Class"/>
  </rdf:Description>
  <rdf:Description rdf:about="#SURFACE-VESSEL-TYPE_Dry_dock,_floating,_workshop">
    <rdfs:subClassOf rdf:resource="jc3iedm_OBJECT-TYPE.owl#SURFACE-VESSEL-TYPE"/>
    <rdfs:label xml:lang="en">dry dock, floating, workshop</rdfs:label>
    <rdfs:comment xml:lang="en">Non-self- propelled dry dock with workshop facilities.</rdfs:comment>
    <rdf:type rdf:resource="http://www.w3.org/2002/07/owl#Class"/>
  </rdf:Description>
  <rdf:Description rdf:about="#SUBSURFACE-VESSEL-TYPE_Submersible,_research,_military">
    <rdfs:subClassOf rdf:resource="jc3iedm_OBJECT-TYPE.owl#SUBSURFACE-VESSEL-TYPE"/>
    <rdfs:label xml:lang="en">submersible, research, military</rdfs:label>
    <rdfs:comment xml:lang="en">Military operated submersible with no combat capability used in research role.</rdfs:comment>
    <rdf:type rdf:resource="http://www.w3.org/2002/07/owl#Class"/>
  </rdf:Description>
  <rdf:Description rdf:about="#AMMUNITION-TYPE_Proximity_fuse">
    <rdfs:subClassOf rdf:resource="jc3iedm_OBJECT-TYPE.owl#AMMUNITION-TYPE"/>
    <rdfs:label xml:lang="en">proximity fuse</rdfs:label>
    <rdfs:comment xml:lang="en">A fuse wherein primary initiation occurs by remotely sensing the presence, distance or direction of a target or its associated environment by means of a signal generated by the fuse or emitted by the target, or by detecting a disturbance of a natural field surrounding the target.</rdfs:comment>
    <rdf:type rdf:resource="http://www.w3.org/2002/07/owl#Class"/>
  </rdf:Description>
  <rdf:Description rdf:about="#FACILITY-TYPE_Bivouac">
    <rdfs:subClassOf rdf:resource="jc3iedm_OBJECT-TYPE.owl#FACILITY-TYPE"/>
    <rdfs:label xml:lang="en">bivouac</rdfs:label>
    <rdfs:comment xml:lang="en">A temporary encampment, under canvas, of troops in the field.</rdfs:comment>
    <rdf:type rdf:resource="http://www.w3.org/2002/07/owl#Class"/>
  </rdf:Description>
  <rdf:Description rdf:about="#EXECUTIVE-MILITARY-ORGANISATION-TYPE_Not_otherwise_specified">
    <rdfs:subClassOf rdf:resource="jc3iedm_OBJECT-TYPE.owl#EXECUTIVE-MILITARY-ORGANISATION-TYPE"/>
    <rdfs:label xml:lang="en">not otherwise specified</rdfs:label>
    <rdfs:comment xml:lang="en">The appropriate value is not in the set of specified values.</rdfs:comment>
    <rdf:type rdf:resource="http://www.w3.org/2002/07/owl#Class"/>
  </rdf:Description>
  <rdf:Description rdf:about="#CONTROL-FEATURE-TYPE_Defensive_position">
    <rdfs:subClassOf rdf:resource="jc3iedm_OBJECT-TYPE.owl#CONTROL-FEATURE-TYPE"/>
    <rdfs:label xml:lang="en">defensive position</rdfs:label>
    <rdfs:comment xml:lang="en">A CONTROL-FEATURE-TYPE that is used in planning to designate a belt of terrain, generally parallel to the front, which includes two or more organised, or partially organised, battle positions.</rdfs:comment>
    <rdf:type rdf:resource="http://www.w3.org/2002/07/owl#Class"/>
  </rdf:Description>
  <rdf:Description rdf:about="#SURFACE-VESSEL-TYPE_Mine_countermeasures_vessel,_hovercraft">
    <rdfs:subClassOf rdf:resource="jc3iedm_OBJECT-TYPE.owl#SURFACE-VESSEL-TYPE"/>
    <rdfs:label xml:lang="en">mine countermeasures vessel, hovercraft</rdfs:label>
    <rdfs:comment xml:lang="en">A mine countermeasures vessel that is air cushion or surface effect design.</rdfs:comment>
    <rdf:type rdf:resource="http://www.w3.org/2002/07/owl#Class"/>
  </rdf:Description>
  <rdf:Description rdf:about="#TASK-FORMATION-TYPE_Naval_task_force">
    <rdfs:subClassOf rdf:resource="jc3iedm_OBJECT-TYPE.owl#TASK-FORMATION-TYPE"/>
    <rdfs:label xml:lang="en">naval task force</rdfs:label>
    <rdfs:comment xml:lang="en">A TASK-FORMATION-TYPE that is a component of a fleet organized by the commander of a task fleet or higher authority for the accomplishment of a specific task or tasks.</rdfs:comment>
    <rdf:type rdf:resource="http://www.w3.org/2002/07/owl#Class"/>
  </rdf:Description>
  <rdf:Description rdf:about="#MISCELLANEOUS-EQUIPMENT-TYPE_Dispenser">
    <rdfs:subClassOf rdf:resource="jc3iedm_OBJECT-TYPE.owl#MISCELLANEOUS-EQUIPMENT-TYPE"/>
    <rdfs:label xml:lang="en">dispenser</rdfs:label>
    <rdfs:comment xml:lang="en">A device that is used to carry and release submunitions.</rdfs:comment>
    <rdf:type rdf:resource="http://www.w3.org/2002/07/owl#Class"/>
  </rdf:Description>
  <rdf:Description rdf:about="#SURFACE-VESSEL-TYPE_Frigate,_small_or_corvette,_guided_missile">
    <rdfs:subClassOf rdf:resource="jc3iedm_OBJECT-TYPE.owl#SURFACE-VESSEL-TYPE"/>
    <rdfs:label xml:lang="en">frigate, small or corvette, guided missile</rdfs:label>
    <rdfs:comment xml:lang="en">General designator for frigate fitted with one or more force guided missile systems. A surface combatant in size range of about 75-150 metres. Fitted primarily to fulfil an ASW role. Generally has lighter surface armament than a Destroyer, general. Classification determined by armament or capability.</rdfs:comment>
    <rdf:type rdf:resource="http://www.w3.org/2002/07/owl#Class"/>
  </rdf:Description>
  <rdf:Description rdf:about="#SURFACE-VESSEL-TYPE_Minehunter/sweeper_w/drone">
    <rdfs:subClassOf rdf:resource="jc3iedm_OBJECT-TYPE.owl#SURFACE-VESSEL-TYPE"/>
    <rdfs:label xml:lang="en">minehunter/sweeper w/drone</rdfs:label>
    <rdfs:comment xml:lang="en">A mine warfare craft equipped for both hunting and sweeping mines by the use of a drone.</rdfs:comment>
    <rdf:type rdf:resource="http://www.w3.org/2002/07/owl#Class"/>
  </rdf:Description>
  <rdf:Description rdf:about="#MILITARY-OBSTACLE-TYPE_Wire_obstacle,_low_wire_fence">
    <rdfs:subClassOf rdf:resource="jc3iedm_OBJECT-TYPE.owl#MILITARY-OBSTACLE-TYPE"/>
    <rdfs:label xml:lang="en">wire obstacle, low wire fence</rdfs:label>
    <rdfs:comment xml:lang="en">No definition provided in APP-6A.</rdfs:comment>
    <rdf:type rdf:resource="http://www.w3.org/2002/07/owl#Class"/>
  </rdf:Description>
  <rdf:Description rdf:about="#CONTROL-FEATURE-TYPE_Air_traffic_control_airspace">
    <rdfs:subClassOf rdf:resource="jc3iedm_OBJECT-TYPE.owl#CONTROL-FEATURE-TYPE"/>
    <rdfs:label xml:lang="en">air traffic control airspace</rdfs:label>
    <rdfs:comment xml:lang="en">Airspace of defined dimensions within which air traffic control service is provided to instrument flight rules (IFR) and visual flight rules (VFR) flights in accordance with civil air traffic control regulations.</rdfs:comment>
    <rdf:type rdf:resource="http://www.w3.org/2002/07/owl#Class"/>
  </rdf:Description>
  <rdf:Description rdf:about="#CONTROL-FEATURE-TYPE_Rocket/missile_area">
    <rdfs:subClassOf rdf:resource="jc3iedm_OBJECT-TYPE.owl#CONTROL-FEATURE-TYPE"/>
    <rdfs:label xml:lang="en">rocket/missile area</rdfs:label>
    <rdfs:comment xml:lang="en">A CONTROL-FEATURE-TYPE with an area location assigned to rocket/missile units for terrain management purposes on which they manoeuvre.</rdfs:comment>
    <rdf:type rdf:resource="http://www.w3.org/2002/07/owl#Class"/>
  </rdf:Description>
  <rdf:Description rdf:about="#ROUTE-TYPE_Variable_track_route">
    <rdfs:subClassOf rdf:resource="jc3iedm_OBJECT-TYPE.owl#ROUTE-TYPE"/>
    <rdfs:label xml:lang="en">variable track route</rdfs:label>
    <rdfs:comment xml:lang="en">Any combination of other than standard routes.</rdfs:comment>
    <rdf:type rdf:resource="http://www.w3.org/2002/07/owl#Class"/>
  </rdf:Description>
  <rdf:Description rdf:about="jc3iedm_OBJECT-TYPE.owl#civilian-post-type-category-code">
    <rdf:type rdf:resource="http://www.w3.org/2002/07/owl#DatatypeProperty"/>
    <rdfs:domain rdf:resource="jc3iedm_OBJECT-TYPE.owl#CIVILIAN-POST-TYPE"/>
    <rdfs:range rdf:resource="http://www.w3.org/2001/XMLSchema#string"/>
  </rdf:Description>
  <rdf:Description rdf:about="#CONTROL-FEATURE-TYPE_Main_axis_of_advance">
    <rdfs:subClassOf rdf:resource="jc3iedm_OBJECT-TYPE.owl#CONTROL-FEATURE-TYPE"/>
    <rdfs:label xml:lang="en">main axis of advance</rdfs:label>
    <rdfs:comment xml:lang="en">A main route of advance, assigned for control, which extends towards the enemy. A main axis of advance symbol graphically portrays a commander’s intention for the main elements of his force, such as avoidance of built-up areas or envelopment of an enemy force. It follows terrain suitable for the size of the force to which the axis was assigned, and is often a road, a group of roads, or a designated series of locations. An axis of advance is not used to direct the control of terrain or the clearance of enemy forces from specific locations. Intermediate objectives are normally assigned for these purposes.</rdfs:comment>
    <rdf:type rdf:resource="http://www.w3.org/2002/07/owl#Class"/>
  </rdf:Description>
  <rdf:Description rdf:about="#AMMUNITION-TYPE_Air-to-air_missile">
    <rdfs:subClassOf rdf:resource="jc3iedm_OBJECT-TYPE.owl#AMMUNITION-TYPE"/>
    <rdfs:label xml:lang="en">air to air missile</rdfs:label>
    <rdfs:comment xml:lang="en">An air-launched guided missile for use against air targets.</rdfs:comment>
    <rdf:type rdf:resource="http://www.w3.org/2002/07/owl#Class"/>
  </rdf:Description>
  <rdf:Description rdf:about="#HARBOUR-TYPE_Inland_water_way">
    <rdfs:subClassOf rdf:resource="jc3iedm_OBJECT-TYPE.owl#HARBOUR-TYPE"/>
    <rdfs:label xml:lang="en">inland water way</rdfs:label>
    <rdfs:comment xml:lang="en">A harbour located in the interior portion of a river, canal or lake that is not connected with the sea by a navigable waterway.</rdfs:comment>
    <rdf:type rdf:resource="http://www.w3.org/2002/07/owl#Class"/>
  </rdf:Description>
  <rdf:Description rdf:about="#MILITARY-POST-TYPE_Airborne_mission_commander">
    <rdfs:subClassOf rdf:resource="jc3iedm_OBJECT-TYPE.owl#MILITARY-POST-TYPE"/>
    <rdfs:label xml:lang="en">airborne mission commander</rdfs:label>
    <rdfs:comment xml:lang="en">A MILITARY-POST-TYPE that executes component’s rescue coordination centre (RCC) and coordinates the combat search and rescue (CSAR) effort between the combat search and rescue task force (CSARTF) and the RCC (or joint search and rescue centre) by monitoring the status of all CSARTF elements, requesting additional assets when needed, and ensuring the recovery and supporting forces arrive at their designated areas to accomplish the CSAR mission.</rdfs:comment>
    <rdf:type rdf:resource="http://www.w3.org/2002/07/owl#Class"/>
  </rdf:Description>
  <rdf:Description rdf:about="#VEHICLE-TYPE_Command_post,_armoured">
    <rdfs:subClassOf rdf:resource="jc3iedm_OBJECT-TYPE.owl#VEHICLE-TYPE"/>
    <rdfs:label xml:lang="en">command post, armoured</rdfs:label>
    <rdfs:comment xml:lang="en">An armoured vehicle designed to be used as a command post or as part of a command post.</rdfs:comment>
    <rdf:type rdf:resource="http://www.w3.org/2002/07/owl#Class"/>
  </rdf:Description>
  <rdf:Description rdf:about="#SURFACE-VESSEL-TYPE_Lighter,_open,_cargo">
    <rdfs:subClassOf rdf:resource="jc3iedm_OBJECT-TYPE.owl#SURFACE-VESSEL-TYPE"/>
    <rdfs:label xml:lang="en">lighter, open, cargo</rdfs:label>
    <rdfs:comment xml:lang="en">Barge-like vessel used in loading and unloading ships or in transporting loads for short distances, but open and used for transporting cargo.</rdfs:comment>
    <rdf:type rdf:resource="http://www.w3.org/2002/07/owl#Class"/>
  </rdf:Description>
  <rdf:Description rdf:about="#AIRCRAFT-TYPE_Light">
    <rdfs:subClassOf rdf:resource="jc3iedm_OBJECT-TYPE.owl#AIRCRAFT-TYPE"/>
    <rdfs:label xml:lang="en">light</rdfs:label>
    <rdfs:comment xml:lang="en">An aircraft is capable of lifting lightweight loads.</rdfs:comment>
    <rdf:type rdf:resource="http://www.w3.org/2002/07/owl#Class"/>
  </rdf:Description>
  <rdf:Description rdf:about="#CONTROL-FEATURE-TYPE_Start_point">
    <rdfs:subClassOf rdf:resource="jc3iedm_OBJECT-TYPE.owl#CONTROL-FEATURE-TYPE"/>
    <rdfs:label xml:lang="en">start point</rdfs:label>
    <rdfs:comment xml:lang="en">A well-defined point on a route at which movement of vehicles begins to be under the control of the commander of this movement. It is at this point that the column is formed by the successive passing, at an appointed time, of each of the elements composing the column. In addition to the principal start point of a column there may be secondary start points for its different elements.</rdfs:comment>
    <rdf:type rdf:resource="http://www.w3.org/2002/07/owl#Class"/>
  </rdf:Description>
  <rdf:Description rdf:about="#SUBSURFACE-VESSEL-TYPE_Submarine,_military_capability_unknown">
    <rdfs:subClassOf rdf:resource="jc3iedm_OBJECT-TYPE.owl#SUBSURFACE-VESSEL-TYPE"/>
    <rdfs:label xml:lang="en">submarine, military capability unknown</rdfs:label>
    <rdfs:comment xml:lang="en">Submarine whose full military capability is unknown or has not been determined.</rdfs:comment>
    <rdf:type rdf:resource="http://www.w3.org/2002/07/owl#Class"/>
  </rdf:Description>
  <rdf:Description rdf:about="#MILITARY-POST-TYPE_Surgical_physician">
    <rdfs:subClassOf rdf:resource="jc3iedm_OBJECT-TYPE.owl#MILITARY-POST-TYPE"/>
    <rdfs:label xml:lang="en">surgical physician</rdfs:label>
    <rdfs:comment xml:lang="en">A MILITARY-POST-TYPE that is identified as a physician specialising in Surgery.</rdfs:comment>
    <rdf:type rdf:resource="http://www.w3.org/2002/07/owl#Class"/>
  </rdf:Description>
  <rdf:Description rdf:about="#VEHICLE-TYPE_Armoured_personnel_carrier,_recovery">
    <rdfs:subClassOf rdf:resource="jc3iedm_OBJECT-TYPE.owl#VEHICLE-TYPE"/>
    <rdfs:label xml:lang="en">armoured personnel carrier, recovery</rdfs:label>
    <rdfs:comment xml:lang="en">A vehicle designed to recover armoured personnel carriers.</rdfs:comment>
    <rdf:type rdf:resource="http://www.w3.org/2002/07/owl#Class"/>
  </rdf:Description>
  <rdf:Description rdf:about="jc3iedm_OBJECT-TYPE.owl#MILITARY-POST-TYPE">
    <rdf:type rdf:resource="http://www.w3.org/2002/07/owl#Class"/>
    <rdfs:label xml:lang="en">military post type</rdfs:label>
    <rdfs:comment xml:lang="en">A MILITARY-ORGANISATION-TYPE with a set of duties that can be fulfilled by one person.</rdfs:comment>
    <rdfs:subClassOf rdf:resource="jc3iedm_OBJECT-TYPE.owl#MILITARY-ORGANISATION-TYPE"/>
  </rdf:Description>
  <rdf:Description rdf:about="#SURFACE-VESSEL-TYPE_Landing_ship,_logistics">
    <rdfs:subClassOf rdf:resource="jc3iedm_OBJECT-TYPE.owl#SURFACE-VESSEL-TYPE"/>
    <rdfs:label xml:lang="en">landing ship, logistics</rdfs:label>
    <rdfs:comment xml:lang="en">Landing ship capable of carrying initial, second and follow-on echelon equipment, vehicles and troops. Normally ramped, not part of initial assault force.</rdfs:comment>
    <rdf:type rdf:resource="http://www.w3.org/2002/07/owl#Class"/>
  </rdf:Description>
  <rdf:Description rdf:about="#FACILITY-TYPE_Shoran_station">
    <rdfs:subClassOf rdf:resource="jc3iedm_OBJECT-TYPE.owl#FACILITY-TYPE"/>
    <rdfs:label xml:lang="en">shoran station</rdfs:label>
    <rdfs:comment xml:lang="en">A facility used in short range navigation.</rdfs:comment>
    <rdf:type rdf:resource="http://www.w3.org/2002/07/owl#Class"/>
  </rdf:Description>
  <rdf:Description rdf:about="#FACILITY-TYPE_Ruins">
    <rdfs:subClassOf rdf:resource="jc3iedm_OBJECT-TYPE.owl#FACILITY-TYPE"/>
    <rdfs:label xml:lang="en">ruins</rdfs:label>
    <rdfs:comment xml:lang="en">A site or location where remains of ancient civilisations or human activity have been discovered.</rdfs:comment>
    <rdf:type rdf:resource="http://www.w3.org/2002/07/owl#Class"/>
  </rdf:Description>
  <rdf:Description rdf:about="#SURFACE-VESSEL-TYPE_Support_barge,_missile">
    <rdfs:subClassOf rdf:resource="jc3iedm_OBJECT-TYPE.owl#SURFACE-VESSEL-TYPE"/>
    <rdfs:label xml:lang="en">support barge, missile</rdfs:label>
    <rdfs:comment xml:lang="en">Any self-propelled craft specially fitted and employed primarily in support of missile R&amp;D, missile testing, associated training and/or space flights in coastal waters, but not at sea.</rdfs:comment>
    <rdf:type rdf:resource="http://www.w3.org/2002/07/owl#Class"/>
  </rdf:Description>
  <rdf:Description rdf:about="#CONTROL-FEATURE-TYPE_Boundary,_political/administrative">
    <rdfs:subClassOf rdf:resource="jc3iedm_OBJECT-TYPE.owl#CONTROL-FEATURE-TYPE"/>
    <rdfs:label xml:lang="en">boundary, political/administrative</rdfs:label>
    <rdfs:comment xml:lang="en">A CONTROL-FEATURE-TYPE with a line location by which political or administrative areas of responsibility are defined.</rdfs:comment>
    <rdf:type rdf:resource="http://www.w3.org/2002/07/owl#Class"/>
  </rdf:Description>
  <rdf:Description rdf:about="jc3iedm_OBJECT-TYPE.owl#ELECTRONIC-EQUIPMENT-TYPE">
    <rdf:type rdf:resource="http://www.w3.org/2002/07/owl#Class"/>
    <rdfs:label xml:lang="en">electronic equipment type</rdfs:label>
    <rdfs:comment xml:lang="en">An EQUIPMENT-TYPE that is designed to use electronic processing to realise its primary function.</rdfs:comment>
    <rdfs:subClassOf rdf:resource="jc3iedm_OBJECT-TYPE.owl#EQUIPMENT-TYPE"/>
  </rdf:Description>
  <rdf:Description rdf:about="#SURFACE-VESSEL-TYPE_Repair_barge,_nuclear_propulsion">
    <rdfs:subClassOf rdf:resource="jc3iedm_OBJECT-TYPE.owl#SURFACE-VESSEL-TYPE"/>
    <rdfs:label xml:lang="en">repair barge, nuclear propulsion</rdfs:label>
    <rdfs:comment xml:lang="en">Barge optimised to repair nuclear propulsion plants.</rdfs:comment>
    <rdf:type rdf:resource="http://www.w3.org/2002/07/owl#Class"/>
  </rdf:Description>
  <rdf:Description rdf:about="#SURFACE-VESSEL-TYPE_Minesweeper,_ocean">
    <rdfs:subClassOf rdf:resource="jc3iedm_OBJECT-TYPE.owl#SURFACE-VESSEL-TYPE"/>
    <rdfs:label xml:lang="en">minesweeper, ocean</rdfs:label>
    <rdfs:comment xml:lang="en">Non-magnetic minesweeper 46 metres or more designed for open ocean operations.</rdfs:comment>
    <rdf:type rdf:resource="http://www.w3.org/2002/07/owl#Class"/>
  </rdf:Description>
  <rdf:Description rdf:about="#MILITARY-POST-TYPE_Psychology_physician">
    <rdfs:subClassOf rdf:resource="jc3iedm_OBJECT-TYPE.owl#MILITARY-POST-TYPE"/>
    <rdfs:label xml:lang="en">psychology physician</rdfs:label>
    <rdfs:comment xml:lang="en">A MILITARY-POST-TYPE that is identified as a physician specialising in Psychology.</rdfs:comment>
    <rdf:type rdf:resource="http://www.w3.org/2002/07/owl#Class"/>
  </rdf:Description>
  <rdf:Description rdf:about="#SURFACE-VESSEL-TYPE_Service_craft,_seaplane">
    <rdfs:subClassOf rdf:resource="jc3iedm_OBJECT-TYPE.owl#SURFACE-VESSEL-TYPE"/>
    <rdfs:label xml:lang="en">service craft, seaplane</rdfs:label>
    <rdfs:comment xml:lang="en">Craft used to rescue, tow, service or support seaplanes.</rdfs:comment>
    <rdf:type rdf:resource="http://www.w3.org/2002/07/owl#Class"/>
  </rdf:Description>
  <rdf:Description rdf:about="#UNIT-TYPE_Aviation">
    <rdfs:subClassOf rdf:resource="jc3iedm_OBJECT-TYPE.owl#UNIT-TYPE"/>
    <rdfs:label xml:lang="en">aviation</rdfs:label>
    <rdfs:comment xml:lang="en">A UNIT-TYPE whose principal designation is the employment of aircraft capable of performing a variety of battlespace functions, including reconnaissance, air operations, and tactical lift.</rdfs:comment>
    <rdf:type rdf:resource="http://www.w3.org/2002/07/owl#Class"/>
  </rdf:Description>
  <rdf:Description rdf:about="#RADIOACTIVE-MATERIEL-TYPE_Not_otherwise_specified">
    <rdfs:subClassOf rdf:resource="jc3iedm_OBJECT-TYPE.owl#RADIOACTIVE-MATERIEL-TYPE"/>
    <rdfs:label xml:lang="en">not otherwise specified</rdfs:label>
    <rdfs:comment xml:lang="en">The appropriate value is not in the set of specified values.</rdfs:comment>
    <rdf:type rdf:resource="http://www.w3.org/2002/07/owl#Class"/>
  </rdf:Description>
  <rdf:Description rdf:about="#SURFACE-VESSEL-TYPE_Minesweeper,_fleet,_hydrofoil">
    <rdfs:subClassOf rdf:resource="jc3iedm_OBJECT-TYPE.owl#SURFACE-VESSEL-TYPE"/>
    <rdfs:label xml:lang="en">minesweeper, fleet, hydrofoil</rdfs:label>
    <rdfs:comment xml:lang="en">Minesweeper in size range 46 metres or more which cannot be regarded as being non-magnetic, fitted with hydrofoils.</rdfs:comment>
    <rdf:type rdf:resource="http://www.w3.org/2002/07/owl#Class"/>
  </rdf:Description>
  <rdf:Description rdf:about="#FACILITY-TYPE_Tower,_television_transmitter">
    <rdfs:subClassOf rdf:resource="jc3iedm_OBJECT-TYPE.owl#FACILITY-TYPE"/>
    <rdfs:label xml:lang="en">tower, television transmitter</rdfs:label>
    <rdfs:comment xml:lang="en">A relatively tall structure mounted with a television transmitter.</rdfs:comment>
    <rdf:type rdf:resource="http://www.w3.org/2002/07/owl#Class"/>
  </rdf:Description>
  <rdf:Description rdf:about="#CHEMICAL-MATERIEL-TYPE_Not_otherwise_specified">
    <rdfs:subClassOf rdf:resource="jc3iedm_OBJECT-TYPE.owl#CHEMICAL-MATERIEL-TYPE"/>
    <rdfs:label xml:lang="en">not otherwise specified</rdfs:label>
    <rdfs:comment xml:lang="en">The appropriate value is not in the set of specified values.</rdfs:comment>
    <rdf:type rdf:resource="http://www.w3.org/2002/07/owl#Class"/>
  </rdf:Description>
  <rdf:Description rdf:about="jc3iedm_OBJECT-TYPE.owl#CBRN-EQUIPMENT-TYPE">
    <rdf:type rdf:resource="http://www.w3.org/2002/07/owl#Class"/>
    <rdfs:label xml:lang="en">cbrn equipment type</rdfs:label>
    <rdfs:comment xml:lang="en">An EQUIPMENT-TYPE that is designed for specialised roles in detecting, decontaminating or reconnoitring CBRN agents.</rdfs:comment>
    <rdfs:subClassOf rdf:resource="jc3iedm_OBJECT-TYPE.owl#EQUIPMENT-TYPE"/>
  </rdf:Description>
  <rdf:Description rdf:about="#SURFACE-VESSEL-TYPE_Salvage_ship">
    <rdfs:subClassOf rdf:resource="jc3iedm_OBJECT-TYPE.owl#SURFACE-VESSEL-TYPE"/>
    <rdfs:label xml:lang="en">salvage ship</rdfs:label>
    <rdfs:comment xml:lang="en">Ship at least 40 metres used to provide mobile salvage, repairs, diving and rescue services.</rdfs:comment>
    <rdf:type rdf:resource="http://www.w3.org/2002/07/owl#Class"/>
  </rdf:Description>
  <rdf:Description rdf:about="#ROUTE-TYPE_Trunk_route">
    <rdfs:subClassOf rdf:resource="jc3iedm_OBJECT-TYPE.owl#ROUTE-TYPE"/>
    <rdfs:label xml:lang="en">trunk route</rdfs:label>
    <rdfs:comment xml:lang="en">Trunk route.</rdfs:comment>
    <rdf:type rdf:resource="http://www.w3.org/2002/07/owl#Class"/>
  </rdf:Description>
  <rdf:Description rdf:about="#CONTROL-FEATURE-TYPE_Operations_zone">
    <rdfs:subClassOf rdf:resource="jc3iedm_OBJECT-TYPE.owl#CONTROL-FEATURE-TYPE"/>
    <rdfs:label xml:lang="en">operations zone</rdfs:label>
    <rdfs:comment xml:lang="en">That portion of an area of war necessary for military operations and for the administration of such operations.</rdfs:comment>
    <rdf:type rdf:resource="http://www.w3.org/2002/07/owl#Class"/>
  </rdf:Description>
  <rdf:Description rdf:about="#MISCELLANEOUS-EQUIPMENT-TYPE_Air_compressor">
    <rdfs:subClassOf rdf:resource="jc3iedm_OBJECT-TYPE.owl#MISCELLANEOUS-EQUIPMENT-TYPE"/>
    <rdfs:label xml:lang="en">air compressor</rdfs:label>
    <rdfs:comment xml:lang="en">A machine for compressing air for use as a motive power.</rdfs:comment>
    <rdf:type rdf:resource="http://www.w3.org/2002/07/owl#Class"/>
  </rdf:Description>
  <rdf:Description rdf:about="#FACILITY-TYPE_Military_materiel_facility,_ammunition_and_explosives_production">
    <rdfs:subClassOf rdf:resource="jc3iedm_OBJECT-TYPE.owl#FACILITY-TYPE"/>
    <rdfs:label xml:lang="en">military materiel facility, ammunition and explosives production</rdfs:label>
    <rdfs:comment xml:lang="en">A facility used as for munitions and explosives production.</rdfs:comment>
    <rdf:type rdf:resource="http://www.w3.org/2002/07/owl#Class"/>
  </rdf:Description>
  <rdf:Description rdf:about="#GROUP-ORGANISATION-TYPE_Writer">
    <rdfs:subClassOf rdf:resource="jc3iedm_OBJECT-TYPE.owl#GROUP-ORGANISATION-TYPE"/>
    <rdfs:label xml:lang="en">writer</rdfs:label>
    <rdfs:comment xml:lang="en">A GROUP-ORGANISATION-TYPE that comprises persons that practice or perform writing.</rdfs:comment>
    <rdf:type rdf:resource="http://www.w3.org/2002/07/owl#Class"/>
  </rdf:Description>
  <rdf:Description rdf:about="#SURFACE-VESSEL-TYPE_Mine_warfare_vessel,_general">
    <rdfs:subClassOf rdf:resource="jc3iedm_OBJECT-TYPE.owl#SURFACE-VESSEL-TYPE"/>
    <rdfs:label xml:lang="en">mine warfare vessel, general</rdfs:label>
    <rdfs:comment xml:lang="en">General designator for mine warfare vessels.</rdfs:comment>
    <rdf:type rdf:resource="http://www.w3.org/2002/07/owl#Class"/>
  </rdf:Description>
  <rdf:Description rdf:about="#SURFACE-VESSEL-TYPE_Corvette">
    <rdfs:subClassOf rdf:resource="jc3iedm_OBJECT-TYPE.owl#SURFACE-VESSEL-TYPE"/>
    <rdfs:label xml:lang="en">corvette</rdfs:label>
    <rdfs:comment xml:lang="en">A speedy, lightly armed warship smaller than a destroyer.</rdfs:comment>
    <rdf:type rdf:resource="http://www.w3.org/2002/07/owl#Class"/>
  </rdf:Description>
  <rdf:Description rdf:about="#CIVILIAN-POST-TYPE_Not_otherwise_specified">
    <rdfs:subClassOf rdf:resource="jc3iedm_OBJECT-TYPE.owl#CIVILIAN-POST-TYPE"/>
    <rdfs:label xml:lang="en">not otherwise specified</rdfs:label>
    <rdfs:comment xml:lang="en">The appropriate value is not in the set of specified values.</rdfs:comment>
    <rdf:type rdf:resource="http://www.w3.org/2002/07/owl#Class"/>
  </rdf:Description>
  <rdf:Description rdf:about="#SURFACE-VESSEL-TYPE_Instrumentation_ship,_hydroacoustic_range">
    <rdfs:subClassOf rdf:resource="jc3iedm_OBJECT-TYPE.owl#SURFACE-VESSEL-TYPE"/>
    <rdfs:label xml:lang="en">instrumentation ship, hydroacoustic range</rdfs:label>
    <rdfs:comment xml:lang="en">Ship specially fitted with instrumentation for hydro acoustic range operations.</rdfs:comment>
    <rdf:type rdf:resource="http://www.w3.org/2002/07/owl#Class"/>
  </rdf:Description>
  <rdf:Description rdf:about="#SURFACE-VESSEL-TYPE_Landing_craft,_fire_support">
    <rdfs:subClassOf rdf:resource="jc3iedm_OBJECT-TYPE.owl#SURFACE-VESSEL-TYPE"/>
    <rdfs:label xml:lang="en">landing craft, fire support</rdfs:label>
    <rdfs:comment xml:lang="en">Landing craft optimised to provide fire support with guns or rockets during amphibious assaults. Probably does not carry troops.</rdfs:comment>
    <rdf:type rdf:resource="http://www.w3.org/2002/07/owl#Class"/>
  </rdf:Description>
  <rdf:Description rdf:about="#FACILITY-TYPE_Traffic_control_post">
    <rdfs:subClassOf rdf:resource="jc3iedm_OBJECT-TYPE.owl#FACILITY-TYPE"/>
    <rdfs:label xml:lang="en">traffic control post</rdfs:label>
    <rdfs:comment xml:lang="en">A facility at which traffic is controlled either by police or by mechanical means.</rdfs:comment>
    <rdf:type rdf:resource="http://www.w3.org/2002/07/owl#Class"/>
  </rdf:Description>
  <rdf:Description rdf:about="#SURFACE-VESSEL-TYPE_Ammunition_ship">
    <rdfs:subClassOf rdf:resource="jc3iedm_OBJECT-TYPE.owl#SURFACE-VESSEL-TYPE"/>
    <rdfs:label xml:lang="en">ammunition ship</rdfs:label>
    <rdfs:comment xml:lang="en">Ship about 120 metres or more capable of transporting 5000 or more tons of ammunition and capable of providing underway replenishment of ammunition.</rdfs:comment>
    <rdf:type rdf:resource="http://www.w3.org/2002/07/owl#Class"/>
  </rdf:Description>
  <rdf:Description rdf:about="#SURFACE-VESSEL-TYPE_Merchant_ship,_car/passenger_ferry">
    <rdfs:subClassOf rdf:resource="jc3iedm_OBJECT-TYPE.owl#SURFACE-VESSEL-TYPE"/>
    <rdfs:label xml:lang="en">merchant ship, car/passenger ferry</rdfs:label>
    <rdfs:comment xml:lang="en">Non-naval ship or craft designed to run a ferry service of both cars and passengers.</rdfs:comment>
    <rdf:type rdf:resource="http://www.w3.org/2002/07/owl#Class"/>
  </rdf:Description>
  <rdf:Description rdf:about="#UNIT-TYPE_Aviation,_VSTOL">
    <rdfs:subClassOf rdf:resource="jc3iedm_OBJECT-TYPE.owl#UNIT-TYPE"/>
    <rdfs:label xml:lang="en">aviation, vstol</rdfs:label>
    <rdfs:comment xml:lang="en">A UNIT-TYPE whose designation indicates employment of vertical/short takeoff and landing assets in the air regime.</rdfs:comment>
    <rdf:type rdf:resource="http://www.w3.org/2002/07/owl#Class"/>
  </rdf:Description>
  <rdf:Description rdf:about="#SURFACE-VESSEL-TYPE_Ice_breaker">
    <rdfs:subClassOf rdf:resource="jc3iedm_OBJECT-TYPE.owl#SURFACE-VESSEL-TYPE"/>
    <rdfs:label xml:lang="en">ice breaker</rdfs:label>
    <rdfs:comment xml:lang="en">Armed ship in size range 70 metres or more used primarily for icebreaking duties.</rdfs:comment>
    <rdf:type rdf:resource="http://www.w3.org/2002/07/owl#Class"/>
  </rdf:Description>
  <rdf:Description rdf:about="#SURFACE-VESSEL-TYPE_Hovercraft_ice_breaker">
    <rdfs:subClassOf rdf:resource="jc3iedm_OBJECT-TYPE.owl#SURFACE-VESSEL-TYPE"/>
    <rdfs:label xml:lang="en">hovercraft ice breaker</rdfs:label>
    <rdfs:comment xml:lang="en">Hovercraft specially fitted to assist in icebreaking.</rdfs:comment>
    <rdf:type rdf:resource="http://www.w3.org/2002/07/owl#Class"/>
  </rdf:Description>
  <rdf:Description rdf:about="jc3iedm_OBJECT-TYPE.owl#MARITIME-EQUIPMENT-TYPE">
    <rdf:type rdf:resource="http://www.w3.org/2002/07/owl#Class"/>
    <rdfs:label xml:lang="en">maritime equipment type</rdfs:label>
    <rdfs:comment xml:lang="en">An EQUIPMENT-TYPE that is designed to be used in a maritime environment.</rdfs:comment>
    <rdfs:subClassOf rdf:resource="jc3iedm_OBJECT-TYPE.owl#EQUIPMENT-TYPE"/>
  </rdf:Description>
  <rdf:Description rdf:about="#FACILITY-TYPE_Military_materiel_facility,_aircraft_production_and_assembly">
    <rdfs:subClassOf rdf:resource="jc3iedm_OBJECT-TYPE.owl#FACILITY-TYPE"/>
    <rdfs:label xml:lang="en">military materiel facility, aircraft production and assembly</rdfs:label>
    <rdfs:comment xml:lang="en">A facility used as for aircraft production and assembly.</rdfs:comment>
    <rdf:type rdf:resource="http://www.w3.org/2002/07/owl#Class"/>
  </rdf:Description>
  <rdf:Description rdf:about="#GEOGRAPHIC-FEATURE-TYPE_Coastal_hydrography">
    <rdfs:subClassOf rdf:resource="jc3iedm_OBJECT-TYPE.owl#GEOGRAPHIC-FEATURE-TYPE"/>
    <rdfs:label xml:lang="en">coastal hydrography</rdfs:label>
    <rdfs:comment xml:lang="en">Natural features representing different aspects of interchange between water and land.</rdfs:comment>
    <rdf:type rdf:resource="http://www.w3.org/2002/07/owl#Class"/>
  </rdf:Description>
  <rdf:Description rdf:about="#CONTROL-FEATURE-TYPE_Safety_sector">
    <rdfs:subClassOf rdf:resource="jc3iedm_OBJECT-TYPE.owl#CONTROL-FEATURE-TYPE"/>
    <rdfs:label xml:lang="en">safety sector</rdfs:label>
    <rdfs:comment xml:lang="en">An airspace established to route friendly aircraft to maritime forces with minimum risk.</rdfs:comment>
    <rdf:type rdf:resource="http://www.w3.org/2002/07/owl#Class"/>
  </rdf:Description>
  <rdf:Description rdf:about="#MISCELLANEOUS-EQUIPMENT-TYPE_Marker">
    <rdfs:subClassOf rdf:resource="jc3iedm_OBJECT-TYPE.owl#MISCELLANEOUS-EQUIPMENT-TYPE"/>
    <rdfs:label xml:lang="en">marker</rdfs:label>
    <rdfs:comment xml:lang="en">A visual or electronic aid used to mark a designated point or area.</rdfs:comment>
    <rdf:type rdf:resource="http://www.w3.org/2002/07/owl#Class"/>
  </rdf:Description>
  <rdf:Description rdf:about="#SURFACE-VESSEL-TYPE_Minehunter/sweeper,_general">
    <rdfs:subClassOf rdf:resource="jc3iedm_OBJECT-TYPE.owl#SURFACE-VESSEL-TYPE"/>
    <rdfs:label xml:lang="en">minehunter/sweeper, general</rdfs:label>
    <rdfs:comment xml:lang="en">A mine warfare craft equipped for both hunting and sweeping mines.</rdfs:comment>
    <rdf:type rdf:resource="http://www.w3.org/2002/07/owl#Class"/>
  </rdf:Description>
  <rdf:Description rdf:about="#PRIVATE-SECTOR-ORGANISATION-TYPE_Multi-national">
    <rdfs:subClassOf rdf:resource="jc3iedm_OBJECT-TYPE.owl#PRIVATE-SECTOR-ORGANISATION-TYPE"/>
    <rdfs:label xml:lang="en">multi national</rdfs:label>
    <rdfs:comment xml:lang="en">A PRIVATE-SECTOR-ORGANISATION-TYPE whose predominant business is multi-national in scope and nature.</rdfs:comment>
    <rdf:type rdf:resource="http://www.w3.org/2002/07/owl#Class"/>
  </rdf:Description>
  <rdf:Description rdf:about="#MILITARY-POST-TYPE_Mickey_net_controller">
    <rdfs:subClassOf rdf:resource="jc3iedm_OBJECT-TYPE.owl#MILITARY-POST-TYPE"/>
    <rdfs:label xml:lang="en">mickey net controller</rdfs:label>
    <rdfs:comment xml:lang="en">A MILITARY-POST-TYPE that is identified as the HAVE QUICK Mickey net controller.</rdfs:comment>
    <rdf:type rdf:resource="http://www.w3.org/2002/07/owl#Class"/>
  </rdf:Description>
  <rdf:Description rdf:about="#SURFACE-VESSEL-TYPE_Fishing_vessel,_refrigerated">
    <rdfs:subClassOf rdf:resource="jc3iedm_OBJECT-TYPE.owl#SURFACE-VESSEL-TYPE"/>
    <rdfs:label xml:lang="en">fishing vessel, refrigerated</rdfs:label>
    <rdfs:comment xml:lang="en">Fishing vessel equipped with refrigerated holds.</rdfs:comment>
    <rdf:type rdf:resource="http://www.w3.org/2002/07/owl#Class"/>
  </rdf:Description>
  <rdf:Description rdf:about="#TASK-FORMATION-TYPE_Marine_air_traffic_control_mobile_team">
    <rdfs:subClassOf rdf:resource="jc3iedm_OBJECT-TYPE.owl#TASK-FORMATION-TYPE"/>
    <rdfs:label xml:lang="en">marine air traffic control mobile team</rdfs:label>
    <rdfs:comment xml:lang="en">A TASK-FORMATION-TYPE, subordinate to the U. S. Marine TACC, that controls local airspace/aircraft in and around Marine Air Ground Task Force (MAGTF) airfields and provides precision approach control for MAGTF aircraft.</rdfs:comment>
    <rdf:type rdf:resource="http://www.w3.org/2002/07/owl#Class"/>
  </rdf:Description>
  <rdf:Description rdf:about="#CONTROL-FEATURE-TYPE_Surface-to-surface_missile_system_area">
    <rdfs:subClassOf rdf:resource="jc3iedm_OBJECT-TYPE.owl#CONTROL-FEATURE-TYPE"/>
    <rdfs:label xml:lang="en">surface to surface missile system area</rdfs:label>
    <rdfs:comment xml:lang="en">Airspace defined specifically for army tactical missile system and tomahawk land attack missile launch and impact points.</rdfs:comment>
    <rdf:type rdf:resource="http://www.w3.org/2002/07/owl#Class"/>
  </rdf:Description>
  <rdf:Description rdf:about="#AIRCRAFT-TYPE_Space_vehicle">
    <rdfs:subClassOf rdf:resource="jc3iedm_OBJECT-TYPE.owl#AIRCRAFT-TYPE"/>
    <rdfs:label xml:lang="en">space vehicle</rdfs:label>
    <rdfs:comment xml:lang="en">An aircraft capable of operating in the region beyond the earth’s atmosphere.</rdfs:comment>
    <rdf:type rdf:resource="http://www.w3.org/2002/07/owl#Class"/>
  </rdf:Description>
  <rdf:Description rdf:about="#MISCELLANEOUS-EQUIPMENT-TYPE_Decoy">
    <rdfs:subClassOf rdf:resource="jc3iedm_OBJECT-TYPE.owl#MISCELLANEOUS-EQUIPMENT-TYPE"/>
    <rdfs:label xml:lang="en">decoy</rdfs:label>
    <rdfs:comment xml:lang="en">An imitation in any sense of a person, object or phenomenon which is intended to deceive enemy surveillance devices or mislead enemy evaluation.</rdfs:comment>
    <rdf:type rdf:resource="http://www.w3.org/2002/07/owl#Class"/>
  </rdf:Description>
  <rdf:Description rdf:about="#UNIT-TYPE_Anti-armour">
    <rdfs:subClassOf rdf:resource="jc3iedm_OBJECT-TYPE.owl#UNIT-TYPE"/>
    <rdfs:label xml:lang="en">anti armour</rdfs:label>
    <rdfs:comment xml:lang="en">A UNIT-TYPE whose principal designation is the employment of direct fire weapon systems against armoured vehicles.</rdfs:comment>
    <rdf:type rdf:resource="http://www.w3.org/2002/07/owl#Class"/>
  </rdf:Description>
  <rdf:Description rdf:about="#FACILITY-TYPE_Fence">
    <rdfs:subClassOf rdf:resource="jc3iedm_OBJECT-TYPE.owl#FACILITY-TYPE"/>
    <rdfs:label xml:lang="en">fence</rdfs:label>
    <rdfs:comment xml:lang="en">A man-made barrier of relatively light structure used as an enclosure or boundary.</rdfs:comment>
    <rdf:type rdf:resource="http://www.w3.org/2002/07/owl#Class"/>
  </rdf:Description>
  <rdf:Description rdf:about="#CONSUMABLE-MATERIEL-TYPE_Not_known">
    <rdfs:subClassOf rdf:resource="jc3iedm_OBJECT-TYPE.owl#CONSUMABLE-MATERIEL-TYPE"/>
    <rdfs:label xml:lang="en">not known</rdfs:label>
    <rdfs:comment xml:lang="en">It is not possible to determine which value is most applicable.</rdfs:comment>
    <rdf:type rdf:resource="http://www.w3.org/2002/07/owl#Class"/>
  </rdf:Description>
  <rdf:Description rdf:about="#FACILITY-TYPE_Bank">
    <rdfs:subClassOf rdf:resource="jc3iedm_OBJECT-TYPE.owl#FACILITY-TYPE"/>
    <rdfs:label xml:lang="en">bank</rdfs:label>
    <rdfs:comment xml:lang="en">An establishment where money is stored for saving or commercial purposes.</rdfs:comment>
    <rdf:type rdf:resource="http://www.w3.org/2002/07/owl#Class"/>
  </rdf:Description>
  <rdf:Description rdf:about="#CONTROL-FEATURE-TYPE_Chemical_concentration_time_contour_line">
    <rdfs:subClassOf rdf:resource="jc3iedm_OBJECT-TYPE.owl#CONTROL-FEATURE-TYPE"/>
    <rdfs:label xml:lang="en">chemical concentration time contour line</rdfs:label>
    <rdfs:comment xml:lang="en">A line on a map, diagram or overlay joining all points at which the chemical concentration-time (for which a quantified portion of exposed personnel are expected to experience (or not experience) effects of given severity) at a given time is the same. Chemical concentration time is the product of the concentration of a chemical substance in the atmosphere and the exposure time.</rdfs:comment>
    <rdf:type rdf:resource="http://www.w3.org/2002/07/owl#Class"/>
  </rdf:Description>
  <rdf:Description rdf:about="#AMMUNITION-TYPE_Rocket/missile,_anti-personnel">
    <rdfs:subClassOf rdf:resource="jc3iedm_OBJECT-TYPE.owl#AMMUNITION-TYPE"/>
    <rdfs:label xml:lang="en">rocket/missile, anti personnel</rdfs:label>
    <rdfs:comment xml:lang="en">A powered projectile designed for use against people.</rdfs:comment>
    <rdf:type rdf:resource="http://www.w3.org/2002/07/owl#Class"/>
  </rdf:Description>
  <rdf:Description rdf:about="jc3iedm_OBJECT-TYPE.owl#TASK-FORMATION-TYPE">
    <rdf:type rdf:resource="http://www.w3.org/2002/07/owl#Class"/>
    <rdfs:label xml:lang="en">task formation type</rdfs:label>
    <rdfs:comment xml:lang="en">A MILITARY-ORGANISATION-TYPE that is constituted on a temporary or semi-permanent basis for the purpose of carrying out a specific operation, mission or task.</rdfs:comment>
    <rdfs:subClassOf rdf:resource="jc3iedm_OBJECT-TYPE.owl#MILITARY-ORGANISATION-TYPE"/>
  </rdf:Description>
  <rdf:Description rdf:about="#SURFACE-VESSEL-TYPE_Merchant_ship,_water_tender">
    <rdfs:subClassOf rdf:resource="jc3iedm_OBJECT-TYPE.owl#SURFACE-VESSEL-TYPE"/>
    <rdfs:label xml:lang="en">merchant ship, water tender</rdfs:label>
    <rdfs:comment xml:lang="en">Non-naval ship designed primarily for transporting potable water.</rdfs:comment>
    <rdf:type rdf:resource="http://www.w3.org/2002/07/owl#Class"/>
  </rdf:Description>
  <rdf:Description rdf:about="jc3iedm_OBJECT-TYPE.owl#bridge-type-design-type-code">
    <rdf:type rdf:resource="http://www.w3.org/2002/07/owl#DatatypeProperty"/>
    <rdfs:domain rdf:resource="jc3iedm_OBJECT-TYPE.owl#BRIDGE-TYPE"/>
    <rdfs:range rdf:resource="http://www.w3.org/2001/XMLSchema#string"/>
  </rdf:Description>
  <rdf:Description rdf:about="jc3iedm_OBJECT-TYPE.owl#ORGANISATION-TYPE">
    <rdf:type rdf:resource="http://www.w3.org/2002/07/owl#Class"/>
    <rdfs:label xml:lang="en">organisation type</rdfs:label>
    <rdfs:comment xml:lang="en">An OBJECT-TYPE that represents administrative or functional structures.</rdfs:comment>
  </rdf:Description>
  <rdf:Description rdf:about="#FACILITY-TYPE_Civilian-military_coordination_centre">
    <rdfs:subClassOf rdf:resource="jc3iedm_OBJECT-TYPE.owl#FACILITY-TYPE"/>
    <rdfs:label xml:lang="en">civilian military coordination centre</rdfs:label>
    <rdfs:comment xml:lang="en">A facility at which civilian-military coordination operations are performed.</rdfs:comment>
    <rdf:type rdf:resource="http://www.w3.org/2002/07/owl#Class"/>
  </rdf:Description>
  <rdf:Description rdf:about="#MILITARY-POST-TYPE_Orthopaedics_physician">
    <rdfs:subClassOf rdf:resource="jc3iedm_OBJECT-TYPE.owl#MILITARY-POST-TYPE"/>
    <rdfs:label xml:lang="en">orthopaedics physician</rdfs:label>
    <rdfs:comment xml:lang="en">A MILITARY-POST-TYPE that is identified as a physician specialising in Orthopaedics.</rdfs:comment>
    <rdf:type rdf:resource="http://www.w3.org/2002/07/owl#Class"/>
  </rdf:Description>
  <rdf:Description rdf:about="#FACILITY-TYPE_Drainage/sewage">
    <rdfs:subClassOf rdf:resource="jc3iedm_OBJECT-TYPE.owl#FACILITY-TYPE"/>
    <rdfs:label xml:lang="en">drainage/sewage</rdfs:label>
    <rdfs:comment xml:lang="en">A facility used for emptying of liquid and channelling sewage to get rid of waste, dirty water and drain water.</rdfs:comment>
    <rdf:type rdf:resource="http://www.w3.org/2002/07/owl#Class"/>
  </rdf:Description>
  <rdf:Description rdf:about="jc3iedm_OBJECT-TYPE.owl#radioactive-materiel-type-category-code">
    <rdf:type rdf:resource="http://www.w3.org/2002/07/owl#DatatypeProperty"/>
    <rdfs:domain rdf:resource="jc3iedm_OBJECT-TYPE.owl#RADIOACTIVE-MATERIEL-TYPE"/>
    <rdfs:range rdf:resource="http://www.w3.org/2001/XMLSchema#string"/>
  </rdf:Description>
  <rdf:Description rdf:about="#ROUTE-TYPE_Temporary_minimum_risk_route">
    <rdfs:subClassOf rdf:resource="jc3iedm_OBJECT-TYPE.owl#ROUTE-TYPE"/>
    <rdfs:label xml:lang="en">temporary minimum risk route</rdfs:label>
    <rdfs:comment xml:lang="en">A temporary route of defined dimension recommended for use by high speed fixed-wing aircraft to route them between TRs and the rear of the forward area and their operations areas.</rdfs:comment>
    <rdf:type rdf:resource="http://www.w3.org/2002/07/owl#Class"/>
  </rdf:Description>
  <rdf:Description rdf:about="#ORGANISATION-TYPE_Marine_tactical_air_command_centre">
    <rdfs:subClassOf rdf:resource="jc3iedm_OBJECT-TYPE.owl#ORGANISATION-TYPE"/>
    <rdfs:label xml:lang="en">marine tactical air command centre</rdfs:label>
    <rdfs:comment xml:lang="en">The ORGANISATION-TYPE that is the senior U.S. Marine command and control agency providing centralized command for Marine Air Ground Task Forces, and serves as the command post for the aviation combat element (ACE) commander.</rdfs:comment>
    <rdf:type rdf:resource="http://www.w3.org/2002/07/owl#Class"/>
  </rdf:Description>
  <rdf:Description rdf:about="#SUBSURFACE-VESSEL-TYPE_Submarine,_midget,_swimmer">
    <rdfs:subClassOf rdf:resource="jc3iedm_OBJECT-TYPE.owl#SUBSURFACE-VESSEL-TYPE"/>
    <rdfs:label xml:lang="en">submarine, midget, swimmer</rdfs:label>
    <rdfs:comment xml:lang="en">Midget submarine or submersible designed primarily for special operations and operated by naval forces.</rdfs:comment>
    <rdf:type rdf:resource="http://www.w3.org/2002/07/owl#Class"/>
  </rdf:Description>
  <rdf:Description rdf:about="#CONTROL-FEATURE-TYPE_CBRN_release_or_attack_area">
    <rdfs:subClassOf rdf:resource="jc3iedm_OBJECT-TYPE.owl#CONTROL-FEATURE-TYPE"/>
    <rdfs:label xml:lang="en">cbrn release or attack area</rdfs:label>
    <rdfs:comment xml:lang="en">A CONTROL-FEATURE-TYPE that identifies the predicted or confirmed area immediately affected by the CBRN-EVENT. If the release is an attack, then the release area is generally called the attack area.</rdfs:comment>
    <rdf:type rdf:resource="http://www.w3.org/2002/07/owl#Class"/>
  </rdf:Description>
  <rdf:Description rdf:about="jc3iedm_OBJECT-TYPE.owl#geographic-feature-type-subcategory-code">
    <rdf:type rdf:resource="http://www.w3.org/2002/07/owl#DatatypeProperty"/>
    <rdfs:domain rdf:resource="jc3iedm_OBJECT-TYPE.owl#GEOGRAPHIC-FEATURE-TYPE"/>
    <rdfs:range rdf:resource="http://www.w3.org/2001/XMLSchema#string"/>
  </rdf:Description>
  <rdf:Description rdf:about="#CONTROL-FEATURE-TYPE_Land_missile_engagement_zone">
    <rdfs:subClassOf rdf:resource="jc3iedm_OBJECT-TYPE.owl#CONTROL-FEATURE-TYPE"/>
    <rdfs:label xml:lang="en">land missile engagement zone</rdfs:label>
    <rdfs:comment xml:lang="en">Airspace of defined dimensions within which the responsibility for engagement of air threats normally rests with the commander of the surface based air defence system.</rdfs:comment>
    <rdf:type rdf:resource="http://www.w3.org/2002/07/owl#Class"/>
  </rdf:Description>
  <rdf:Description rdf:about="#VEHICLE-TYPE_Motorcycle">
    <rdfs:subClassOf rdf:resource="jc3iedm_OBJECT-TYPE.owl#VEHICLE-TYPE"/>
    <rdfs:label xml:lang="en">motorcycle</rdfs:label>
    <rdfs:comment xml:lang="en">A vehicle with two wheels in tandem, self-propelled and sometimes having a sidecar with a third wheel.</rdfs:comment>
    <rdf:type rdf:resource="http://www.w3.org/2002/07/owl#Class"/>
  </rdf:Description>
  <rdf:Description rdf:about="#MARITIME-EQUIPMENT-TYPE_Otter">
    <rdfs:subClassOf rdf:resource="jc3iedm_OBJECT-TYPE.owl#MARITIME-EQUIPMENT-TYPE"/>
    <rdfs:label xml:lang="en">otter</rdfs:label>
    <rdfs:comment xml:lang="en">In naval mine warfare, a device which, when towed, displaces itself sideways to a predetermined distance.</rdfs:comment>
    <rdf:type rdf:resource="http://www.w3.org/2002/07/owl#Class"/>
  </rdf:Description>
  <rdf:Description rdf:about="#ROUTE-TYPE_Flight_path">
    <rdfs:subClassOf rdf:resource="jc3iedm_OBJECT-TYPE.owl#ROUTE-TYPE"/>
    <rdfs:label xml:lang="en">flight path</rdfs:label>
    <rdfs:comment xml:lang="en">The line connecting the successive positions occupied, or to be occupied, by an aircraft, missile or space vehicle as it moves through air or space.</rdfs:comment>
    <rdf:type rdf:resource="http://www.w3.org/2002/07/owl#Class"/>
  </rdf:Description>
  <rdf:Description rdf:about="#MILITARY-POST-TYPE_Head/neck_physician">
    <rdfs:subClassOf rdf:resource="jc3iedm_OBJECT-TYPE.owl#MILITARY-POST-TYPE"/>
    <rdfs:label xml:lang="en">head/neck physician</rdfs:label>
    <rdfs:comment xml:lang="en">A MILITARY-POST-TYPE that is identified as a physician specialising in Head/neck.</rdfs:comment>
    <rdf:type rdf:resource="http://www.w3.org/2002/07/owl#Class"/>
  </rdf:Description>
  <rdf:Description rdf:about="jc3iedm_OBJECT-TYPE.owl#miscellaneous-equipment-type-subcategory-code">
    <rdf:type rdf:resource="http://www.w3.org/2002/07/owl#DatatypeProperty"/>
    <rdfs:domain rdf:resource="jc3iedm_OBJECT-TYPE.owl#MISCELLANEOUS-EQUIPMENT-TYPE"/>
    <rdfs:range rdf:resource="http://www.w3.org/2001/XMLSchema#string"/>
  </rdf:Description>
  <rdf:Description rdf:about="#SURFACE-VESSEL-TYPE_Aircraft_carrier,_helicopter/VSTOL,_guided_missile">
    <rdfs:subClassOf rdf:resource="jc3iedm_OBJECT-TYPE.owl#SURFACE-VESSEL-TYPE"/>
    <rdfs:label xml:lang="en">aircraft carrier, helicopter/vstol, guided missile</rdfs:label>
    <rdfs:comment xml:lang="en">Aircraft carrier without arrest gear/catapult operating VSTOL aircraft and/or helicopters which is not an amphibious or minewarfare ship, fitted with one or more force guided missile systems.</rdfs:comment>
    <rdf:type rdf:resource="http://www.w3.org/2002/07/owl#Class"/>
  </rdf:Description>
  <rdf:Description rdf:about="#CIVILIAN-POST-TYPE_Corporate_executive">
    <rdfs:subClassOf rdf:resource="jc3iedm_OBJECT-TYPE.owl#CIVILIAN-POST-TYPE"/>
    <rdfs:label xml:lang="en">corporate executive</rdfs:label>
    <rdfs:comment xml:lang="en">A CIVILIAN-POST-TYPE whose job entails the leadership in an executive or administrative function in a private sector business.</rdfs:comment>
    <rdf:type rdf:resource="http://www.w3.org/2002/07/owl#Class"/>
  </rdf:Description>
  <rdf:Description rdf:about="#CONTROL-FEATURE-TYPE_Support_by_fire_position">
    <rdfs:subClassOf rdf:resource="jc3iedm_OBJECT-TYPE.owl#CONTROL-FEATURE-TYPE"/>
    <rdfs:label xml:lang="en">support by fire position</rdfs:label>
    <rdfs:comment xml:lang="en">A CONTROL-FEATURE-TYPE that is an area by which a manoeuvre element moves to a position in the battlespace where it can engage the enemy by direct fire. The manoeuvre element does not attempt to manoeuvre to capture enemy forces or terrain.</rdfs:comment>
    <rdf:type rdf:resource="http://www.w3.org/2002/07/owl#Class"/>
  </rdf:Description>
  <rdf:Description rdf:about="jc3iedm_OBJECT-TYPE.owl#aircraft-type-design-role-code">
    <rdf:type rdf:resource="http://www.w3.org/2002/07/owl#DatatypeProperty"/>
    <rdfs:domain rdf:resource="jc3iedm_OBJECT-TYPE.owl#AIRCRAFT-TYPE"/>
    <rdfs:range rdf:resource="http://www.w3.org/2001/XMLSchema#string"/>
  </rdf:Description>
  <rdf:Description rdf:about="#CONTROL-FEATURE-TYPE_Main_threat_axis">
    <rdfs:subClassOf rdf:resource="jc3iedm_OBJECT-TYPE.owl#CONTROL-FEATURE-TYPE"/>
    <rdfs:label xml:lang="en">main threat axis</rdfs:label>
    <rdfs:comment xml:lang="en">A CONTROL-FEATURE-TYPE that represents the line or area along which the enemy forces are assumed to constitute the largest threat.</rdfs:comment>
    <rdf:type rdf:resource="http://www.w3.org/2002/07/owl#Class"/>
  </rdf:Description>
  <rdf:Description rdf:about="#MARITIME-EQUIPMENT-TYPE_Diaphragm">
    <rdfs:subClassOf rdf:resource="jc3iedm_OBJECT-TYPE.owl#MARITIME-EQUIPMENT-TYPE"/>
    <rdfs:label xml:lang="en">diaphragm</rdfs:label>
    <rdfs:comment xml:lang="en">No definition provided in ADatP-3 Baseline 13.1 FFIRN/FUD 1135/55.</rdfs:comment>
    <rdf:type rdf:resource="http://www.w3.org/2002/07/owl#Class"/>
  </rdf:Description>
  <rdf:Description rdf:about="#MISCELLANEOUS-EQUIPMENT-TYPE_Container_delivery_system">
    <rdfs:subClassOf rdf:resource="jc3iedm_OBJECT-TYPE.owl#MISCELLANEOUS-EQUIPMENT-TYPE"/>
    <rdfs:label xml:lang="en">container delivery system</rdfs:label>
    <rdfs:comment xml:lang="en">A system for aerial delivery of supplies and small items of equipment from low or high altitudes into a small area.</rdfs:comment>
    <rdf:type rdf:resource="http://www.w3.org/2002/07/owl#Class"/>
  </rdf:Description>
  <rdf:Description rdf:about="#FACILITY-TYPE_Military_base/facility">
    <rdfs:subClassOf rdf:resource="jc3iedm_OBJECT-TYPE.owl#FACILITY-TYPE"/>
    <rdfs:label xml:lang="en">military base/facility</rdfs:label>
    <rdfs:comment xml:lang="en">A facility that is used as a military base.</rdfs:comment>
    <rdf:type rdf:resource="http://www.w3.org/2002/07/owl#Class"/>
  </rdf:Description>
  <rdf:Description rdf:about="#FACILITY-TYPE_Quay">
    <rdfs:subClassOf rdf:resource="jc3iedm_OBJECT-TYPE.owl#FACILITY-TYPE"/>
    <rdfs:label xml:lang="en">quay</rdfs:label>
    <rdfs:comment xml:lang="en">A FACILITY-TYPE that is a solidly constructed platform, usually parallel to the shoreline of navigable water, alongside which a vessel can be docked or berthed and, on which, the vessel can be accessed and cargo can be loaded or unloaded on one side of the vessel only.</rdfs:comment>
    <rdf:type rdf:resource="http://www.w3.org/2002/07/owl#Class"/>
  </rdf:Description>
  <rdf:Description rdf:about="#MILITARY-POST-TYPE_Scout">
    <rdfs:subClassOf rdf:resource="jc3iedm_OBJECT-TYPE.owl#MILITARY-POST-TYPE"/>
    <rdfs:label xml:lang="en">scout</rdfs:label>
    <rdfs:comment xml:lang="en">A MILITARY-POST-TYPE that is identified as one sent out ahead of the main force in order to reconnoitre the position and movement of the enemy.</rdfs:comment>
    <rdf:type rdf:resource="http://www.w3.org/2002/07/owl#Class"/>
  </rdf:Description>
  <rdf:Description rdf:about="#UNIT-TYPE_Maintenance">
    <rdfs:subClassOf rdf:resource="jc3iedm_OBJECT-TYPE.owl#UNIT-TYPE"/>
    <rdfs:label xml:lang="en">maintenance</rdfs:label>
    <rdfs:comment xml:lang="en">A UNIT-TYPE whose principal designation is the repair and maintenance of equipment.</rdfs:comment>
    <rdf:type rdf:resource="http://www.w3.org/2002/07/owl#Class"/>
  </rdf:Description>
  <rdf:Description rdf:about="#FACILITY-TYPE_Cemetery/graveyard/burial_ground">
    <rdfs:subClassOf rdf:resource="jc3iedm_OBJECT-TYPE.owl#FACILITY-TYPE"/>
    <rdfs:label xml:lang="en">cemetery/graveyard/burial ground</rdfs:label>
    <rdfs:comment xml:lang="en">A facility that is an area of land for burying the dead.</rdfs:comment>
    <rdf:type rdf:resource="http://www.w3.org/2002/07/owl#Class"/>
  </rdf:Description>
  <rdf:Description rdf:about="#ROUTE-TYPE_Supersonic_route">
    <rdfs:subClassOf rdf:resource="jc3iedm_OBJECT-TYPE.owl#ROUTE-TYPE"/>
    <rdfs:label xml:lang="en">supersonic route</rdfs:label>
    <rdfs:comment xml:lang="en">Supersonic route.</rdfs:comment>
    <rdf:type rdf:resource="http://www.w3.org/2002/07/owl#Class"/>
  </rdf:Description>
  <rdf:Description rdf:about="#SURFACE-VESSEL-TYPE_Minehunter,_inshore">
    <rdfs:subClassOf rdf:resource="jc3iedm_OBJECT-TYPE.owl#SURFACE-VESSEL-TYPE"/>
    <rdfs:label xml:lang="en">minehunter, inshore</rdfs:label>
    <rdfs:comment xml:lang="en">Ship equipped with specific equipment to hunt mines and designed for operating in more shallow waters or estuaries.</rdfs:comment>
    <rdf:type rdf:resource="http://www.w3.org/2002/07/owl#Class"/>
  </rdf:Description>
  <rdf:Description rdf:about="#MISCELLANEOUS-EQUIPMENT-TYPE_Demolition_equipment">
    <rdfs:subClassOf rdf:resource="jc3iedm_OBJECT-TYPE.owl#MISCELLANEOUS-EQUIPMENT-TYPE"/>
    <rdfs:label xml:lang="en">demolition equipment</rdfs:label>
    <rdfs:comment xml:lang="en">Equipment specifically designed to be used in executing demolition tasks.</rdfs:comment>
    <rdf:type rdf:resource="http://www.w3.org/2002/07/owl#Class"/>
  </rdf:Description>
  <rdf:Description rdf:about="#CIVILIAN-POST-TYPE_Aid_administrator">
    <rdfs:subClassOf rdf:resource="jc3iedm_OBJECT-TYPE.owl#CIVILIAN-POST-TYPE"/>
    <rdfs:label xml:lang="en">aid administrator</rdfs:label>
    <rdfs:comment xml:lang="en">A CIVILIAN-POST-TYPE whose job is to manage or direct the affairs of an organisation that provides relief services.</rdfs:comment>
    <rdf:type rdf:resource="http://www.w3.org/2002/07/owl#Class"/>
  </rdf:Description>
  <rdf:Description rdf:about="#CONTROL-FEATURE-TYPE_Limited_access_area">
    <rdfs:subClassOf rdf:resource="jc3iedm_OBJECT-TYPE.owl#CONTROL-FEATURE-TYPE"/>
    <rdfs:label xml:lang="en">limited access area</rdfs:label>
    <rdfs:comment xml:lang="en">A CONTROL-FEATURE-TYPE with an area location to indicate to what personnel or equipment the area is impassable. Note - this definition does not identify whether it is a procedural issue, limitation or a trafficability issue.</rdfs:comment>
    <rdf:type rdf:resource="http://www.w3.org/2002/07/owl#Class"/>
  </rdf:Description>
  <rdf:Description rdf:about="#AMMUNITION-TYPE_Mine,_seabed_-_explosive_charge_500kg_or_greater">
    <rdfs:subClassOf rdf:resource="jc3iedm_OBJECT-TYPE.owl#AMMUNITION-TYPE"/>
    <rdfs:label xml:lang="en">mine, seabed   explosive charge 500kg or greater</rdfs:label>
    <rdfs:comment xml:lang="en">A mine with negative buoyancy which remains on the seabed with explosive charge of 500kg or greater.</rdfs:comment>
    <rdf:type rdf:resource="http://www.w3.org/2002/07/owl#Class"/>
  </rdf:Description>
  <rdf:Description rdf:about="#CONTROL-FEATURE-TYPE_Exit_gate">
    <rdfs:subClassOf rdf:resource="jc3iedm_OBJECT-TYPE.owl#CONTROL-FEATURE-TYPE"/>
    <rdfs:label xml:lang="en">exit gate</rdfs:label>
    <rdfs:comment xml:lang="en">The point to which an aircraft will be directed to commence the transit outbound from an airfield or force at sea.</rdfs:comment>
    <rdf:type rdf:resource="http://www.w3.org/2002/07/owl#Class"/>
  </rdf:Description>
  <rdf:Description rdf:about="#CONTROL-FEATURE-TYPE_Rear_combat_zone">
    <rdfs:subClassOf rdf:resource="jc3iedm_OBJECT-TYPE.owl#CONTROL-FEATURE-TYPE"/>
    <rdfs:label xml:lang="en">rear combat zone</rdfs:label>
    <rdfs:comment xml:lang="en">A CONTROL-FEATURE-TYPE with an area location usually compromising the territory between the corps rear boundary and the army group rear boundary.</rdfs:comment>
    <rdf:type rdf:resource="http://www.w3.org/2002/07/owl#Class"/>
  </rdf:Description>
  <rdf:Description rdf:about="#ROUTE-TYPE_Low_level_transit_route">
    <rdfs:subClassOf rdf:resource="jc3iedm_OBJECT-TYPE.owl#ROUTE-TYPE"/>
    <rdfs:label xml:lang="en">low level transit route</rdfs:label>
    <rdfs:comment xml:lang="en">A temporary corridor of defined dimensions established in the forward area to minimise the risk to friendly aircraft from friendly air defences or surface forces.</rdfs:comment>
    <rdf:type rdf:resource="http://www.w3.org/2002/07/owl#Class"/>
  </rdf:Description>
  <rdf:Description rdf:about="#AIRCRAFT-TYPE_Not_otherwise_specified">
    <rdfs:label xml:lang="en">not otherwise specified</rdfs:label>
    <rdfs:subClassOf rdf:resource="jc3iedm_OBJECT-TYPE.owl#AIRCRAFT-TYPE"/>
    <rdfs:comment xml:lang="en">The appropriate value is not in the set of specified values.</rdfs:comment>
    <rdf:type rdf:resource="http://www.w3.org/2002/07/owl#Class"/>
  </rdf:Description>
  <rdf:Description rdf:about="#ORGANISATION-TYPE_Marine_tactical_air_operations_centre">
    <rdfs:subClassOf rdf:resource="jc3iedm_OBJECT-TYPE.owl#ORGANISATION-TYPE"/>
    <rdfs:label xml:lang="en">marine tactical air operations centre</rdfs:label>
    <rdfs:comment xml:lang="en">The ORGANISATION-TYPE that is the principal air control agency of the U.S. Marine air command and control system responsible for airspace control and management. It provides real-time surveillance, direction, positive control, and navigational assistance for friendly aircraft. It performs real-time direction and control of all anti-air warfare operations, to include manned interceptors and surface-to-air weapons. It is subordinate to the tactical air command centre.</rdfs:comment>
    <rdf:type rdf:resource="http://www.w3.org/2002/07/owl#Class"/>
  </rdf:Description>
  <rdf:Description rdf:about="#EXECUTIVE-MILITARY-ORGANISATION-TYPE_Personnel">
    <rdfs:subClassOf rdf:resource="jc3iedm_OBJECT-TYPE.owl#EXECUTIVE-MILITARY-ORGANISATION-TYPE"/>
    <rdfs:label xml:lang="en">personnel</rdfs:label>
    <rdfs:comment xml:lang="en">An EXECUTIVE-MILITARY-ORGANISATION-TYPE that provides management of personnel services.</rdfs:comment>
    <rdf:type rdf:resource="http://www.w3.org/2002/07/owl#Class"/>
  </rdf:Description>
  <rdf:Description rdf:about="#CONTROL-FEATURE-TYPE_Reference_point">
    <rdfs:subClassOf rdf:resource="jc3iedm_OBJECT-TYPE.owl#CONTROL-FEATURE-TYPE"/>
    <rdfs:label xml:lang="en">reference point</rdfs:label>
    <rdfs:comment xml:lang="en">A point or set of coordinates generally used for control purposes or to indicate a reference position.</rdfs:comment>
    <rdf:type rdf:resource="http://www.w3.org/2002/07/owl#Class"/>
  </rdf:Description>
  <rdf:Description rdf:about="jc3iedm_OBJECT-TYPE.owl#CHEMICAL-MATERIEL-TYPE">
    <rdf:type rdf:resource="http://www.w3.org/2002/07/owl#Class"/>
    <rdfs:label xml:lang="en">chemical materiel type</rdfs:label>
    <rdfs:comment xml:lang="en">A CONSUMABLE-MATERIEL-TYPE that is a substance that is not produced by a living organism, and does not emit radiation but may kill, seriously injure, or incapacitate personnel through its physiological effects or cause the deterioration of materiel.</rdfs:comment>
    <rdfs:subClassOf rdf:resource="jc3iedm_OBJECT-TYPE.owl#CONSUMABLE-MATERIEL-TYPE"/>
  </rdf:Description>
  <rdf:Description rdf:about="#TASK-FORMATION-TYPE_Joint_task_force">
    <rdfs:subClassOf rdf:resource="jc3iedm_OBJECT-TYPE.owl#TASK-FORMATION-TYPE"/>
    <rdfs:label xml:lang="en">joint task force</rdfs:label>
    <rdfs:comment xml:lang="en">A temporary grouping of units, under one commander, formed for the purpose of carrying out a specific joint operation or mission.</rdfs:comment>
    <rdf:type rdf:resource="http://www.w3.org/2002/07/owl#Class"/>
  </rdf:Description>
  <rdf:Description rdf:about="#FACILITY-TYPE_Hangar">
    <rdfs:subClassOf rdf:resource="jc3iedm_OBJECT-TYPE.owl#FACILITY-TYPE"/>
    <rdfs:label xml:lang="en">hangar</rdfs:label>
    <rdfs:comment xml:lang="en">A covered space, shed or shelter for the accommodation of aircraft or spacecraft.</rdfs:comment>
    <rdf:type rdf:resource="http://www.w3.org/2002/07/owl#Class"/>
  </rdf:Description>
  <rdf:Description rdf:about="jc3iedm_OBJECT-TYPE.owl#subsurface-vessel-type-dived-displacement-quantity">
    <rdf:type rdf:resource="http://www.w3.org/2002/07/owl#DatatypeProperty"/>
    <rdfs:domain rdf:resource="jc3iedm_OBJECT-TYPE.owl#SUBSURFACE-VESSEL-TYPE"/>
  </rdf:Description>
  <rdf:Description rdf:about="#CONTROL-FEATURE-TYPE_Mine_danger_area,_sea">
    <rdfs:subClassOf rdf:resource="jc3iedm_OBJECT-TYPE.owl#CONTROL-FEATURE-TYPE"/>
    <rdfs:label xml:lang="en">mine danger area, sea</rdfs:label>
    <rdfs:comment xml:lang="en">An area established around the position of a suspected or known mine.</rdfs:comment>
    <rdf:type rdf:resource="http://www.w3.org/2002/07/owl#Class"/>
  </rdf:Description>
  <rdf:Description rdf:about="#SURFACE-VESSEL-TYPE_Merchant_ship,_cable_layer">
    <rdfs:subClassOf rdf:resource="jc3iedm_OBJECT-TYPE.owl#SURFACE-VESSEL-TYPE"/>
    <rdfs:label xml:lang="en">merchant ship, cable layer</rdfs:label>
    <rdfs:comment xml:lang="en">Non-naval ship designed to lay and/or retrieve cables.</rdfs:comment>
    <rdf:type rdf:resource="http://www.w3.org/2002/07/owl#Class"/>
  </rdf:Description>
  <rdf:Description rdf:about="#SURFACE-VESSEL-TYPE_Aircraft_carrier,_helicopter/VSTOL,_nuclear_powered">
    <rdfs:subClassOf rdf:resource="jc3iedm_OBJECT-TYPE.owl#SURFACE-VESSEL-TYPE"/>
    <rdfs:label xml:lang="en">aircraft carrier, helicopter/vstol, nuclear powered</rdfs:label>
    <rdfs:comment xml:lang="en">Aircraft carrier without arrest gear/catapult operating VSTOL aircraft and/or helicopters that is not an amphibious or minewarfare ship, having nuclear power.</rdfs:comment>
    <rdf:type rdf:resource="http://www.w3.org/2002/07/owl#Class"/>
  </rdf:Description>
  <rdf:Description rdf:about="jc3iedm_OBJECT-TYPE.owl#weapon-type-category-code">
    <rdf:type rdf:resource="http://www.w3.org/2002/07/owl#DatatypeProperty"/>
    <rdfs:domain rdf:resource="jc3iedm_OBJECT-TYPE.owl#WEAPON-TYPE"/>
    <rdfs:range rdf:resource="http://www.w3.org/2001/XMLSchema#string"/>
  </rdf:Description>
  <rdf:Description rdf:about="#FACILITY-TYPE_Farm">
    <rdfs:subClassOf rdf:resource="jc3iedm_OBJECT-TYPE.owl#FACILITY-TYPE"/>
    <rdfs:label xml:lang="en">farm</rdfs:label>
    <rdfs:comment xml:lang="en">Land devoted to agricultural production, raising and breeding of animals or an area of water devoted to the raising and breeding of aquatic animals.</rdfs:comment>
    <rdf:type rdf:resource="http://www.w3.org/2002/07/owl#Class"/>
  </rdf:Description>
  <rdf:Description rdf:about="#SURFACE-VESSEL-TYPE_Hovercraft,_ferry">
    <rdfs:subClassOf rdf:resource="jc3iedm_OBJECT-TYPE.owl#SURFACE-VESSEL-TYPE"/>
    <rdfs:label xml:lang="en">hovercraft, ferry</rdfs:label>
    <rdfs:comment xml:lang="en">Hovercraft fitted to carry passengers and/or vehicles.</rdfs:comment>
    <rdf:type rdf:resource="http://www.w3.org/2002/07/owl#Class"/>
  </rdf:Description>
  <rdf:Description rdf:about="#AMMUNITION-TYPE_Moving_mine,_sea">
    <rdfs:subClassOf rdf:resource="jc3iedm_OBJECT-TYPE.owl#AMMUNITION-TYPE"/>
    <rdfs:label xml:lang="en">moving mine, sea</rdfs:label>
    <rdfs:comment xml:lang="en">The collective description of mines, such as drifting, oscillating, creeping, mobile, rising, homing and bouquet mines.</rdfs:comment>
    <rdf:type rdf:resource="http://www.w3.org/2002/07/owl#Class"/>
  </rdf:Description>
  <rdf:Description rdf:about="#SUBSURFACE-VESSEL-TYPE_Submersible,_research_(commercial)">
    <rdfs:subClassOf rdf:resource="jc3iedm_OBJECT-TYPE.owl#SUBSURFACE-VESSEL-TYPE"/>
    <rdfs:label xml:lang="en">submersible, research (commercial)</rdfs:label>
    <rdfs:comment xml:lang="en">Submersible with no combat capability used in research role.</rdfs:comment>
    <rdf:type rdf:resource="http://www.w3.org/2002/07/owl#Class"/>
  </rdf:Description>
  <rdf:Description rdf:about="jc3iedm_OBJECT-TYPE.owl#materiel-type-issuing-width-dimension">
    <rdf:type rdf:resource="http://www.w3.org/2002/07/owl#DatatypeProperty"/>
    <rdfs:domain rdf:resource="jc3iedm_OBJECT-TYPE.owl#MATERIEL-TYPE"/>
  </rdf:Description>
  <rdf:Description rdf:about="#TASK-FORMATION-TYPE_Land_task_force">
    <rdfs:subClassOf rdf:resource="jc3iedm_OBJECT-TYPE.owl#TASK-FORMATION-TYPE"/>
    <rdfs:label xml:lang="en">land task force</rdfs:label>
    <rdfs:comment xml:lang="en">A temporary grouping of units, under one commander, formed for the purpose of carrying out a specific land operation or mission.</rdfs:comment>
    <rdf:type rdf:resource="http://www.w3.org/2002/07/owl#Class"/>
  </rdf:Description>
  <rdf:Description rdf:about="#CONTROL-FEATURE-TYPE_Zone_II">
    <rdfs:subClassOf rdf:resource="jc3iedm_OBJECT-TYPE.owl#CONTROL-FEATURE-TYPE"/>
    <rdfs:label xml:lang="en">zone ii</rdfs:label>
    <rdfs:comment xml:lang="en">A circular area (less Zone I area) of Secondary Hazard where the total dose received by exposed, unprotected personnel is not expected to reach 150 cGy within a period of four hours after the actual arrival of fallout. Within this zone, personnel may receive a total dose of 50 cGy or greater within the first 24 hours after arrival of fallout. The boundaries of Zone II are determined by the Zone 1 downwind distance arc, the Zone 2 distance arc and the 2 radial lines.</rdfs:comment>
    <rdf:type rdf:resource="http://www.w3.org/2002/07/owl#Class"/>
  </rdf:Description>
  <rdf:Description rdf:about="#CONTROL-FEATURE-TYPE_Deep_battle_synchronisation_line">
    <rdfs:subClassOf rdf:resource="jc3iedm_OBJECT-TYPE.owl#CONTROL-FEATURE-TYPE"/>
    <rdfs:label xml:lang="en">deep battle synchronisation line</rdfs:label>
    <rdfs:comment xml:lang="en">The forward boundary of the ground component commander's (GCC) area of operation. The DBSL defines the geographic areas of responsibility of the GCC and air component commander.</rdfs:comment>
    <rdf:type rdf:resource="http://www.w3.org/2002/07/owl#Class"/>
  </rdf:Description>
  <rdf:Description rdf:about="#FACILITY-TYPE_Site,_radar">
    <rdfs:subClassOf rdf:resource="jc3iedm_OBJECT-TYPE.owl#FACILITY-TYPE"/>
    <rdfs:label xml:lang="en">site, radar</rdfs:label>
    <rdfs:comment xml:lang="en">A facility containing radar that may be employed for the tracking and identification of battlespace objects.</rdfs:comment>
    <rdf:type rdf:resource="http://www.w3.org/2002/07/owl#Class"/>
  </rdf:Description>
  <rdf:Description rdf:about="#CONTROL-FEATURE-TYPE_CBRN_reading/sample/detection">
    <rdfs:subClassOf rdf:resource="jc3iedm_OBJECT-TYPE.owl#CONTROL-FEATURE-TYPE"/>
    <rdfs:label xml:lang="en">cbrn reading/sample/detection</rdfs:label>
    <rdfs:comment xml:lang="en">The point at which a reading, sample or detection of an NBC (CBRN) contaminant is performed.</rdfs:comment>
    <rdf:type rdf:resource="http://www.w3.org/2002/07/owl#Class"/>
  </rdf:Description>
  <rdf:Description rdf:about="#CONTROL-FEATURE-TYPE_Way_point">
    <rdfs:subClassOf rdf:resource="jc3iedm_OBJECT-TYPE.owl#CONTROL-FEATURE-TYPE"/>
    <rdfs:label xml:lang="en">way point</rdfs:label>
    <rdfs:comment xml:lang="en">1. In air operations, a point or a series of points in space to which an aircraft, ship, or cruise missile may be vectored. 2. A designated point or series of points loaded and stored in a global positioning system or other electronic navigational aid system to facilitate movement.</rdfs:comment>
    <rdf:type rdf:resource="http://www.w3.org/2002/07/owl#Class"/>
  </rdf:Description>
  <rdf:Description rdf:about="#SURFACE-VESSEL-TYPE_Oiler_replenishment,_(naval)">
    <rdfs:subClassOf rdf:resource="jc3iedm_OBJECT-TYPE.owl#SURFACE-VESSEL-TYPE"/>
    <rdfs:label xml:lang="en">oiler replenishment, (naval)</rdfs:label>
    <rdfs:comment xml:lang="en">Ship of at least 140 metres capable of providing rapid replenishment of POL and solid store products.</rdfs:comment>
    <rdf:type rdf:resource="http://www.w3.org/2002/07/owl#Class"/>
  </rdf:Description>
  <rdf:Description rdf:about="#CONTROL-FEATURE-TYPE_Warning_area">
    <rdfs:subClassOf rdf:resource="jc3iedm_OBJECT-TYPE.owl#CONTROL-FEATURE-TYPE"/>
    <rdfs:label xml:lang="en">warning area</rdfs:label>
    <rdfs:comment xml:lang="en">Airspace extending from 3 nautical miles (5.556 km) outward from the coast of the continental (US) that contains activity that may be hazardous to non-participating aircraft.</rdfs:comment>
    <rdf:type rdf:resource="http://www.w3.org/2002/07/owl#Class"/>
  </rdf:Description>
  <rdf:Description rdf:about="#CBRN-EQUIPMENT-TYPE_Automated_chemical_and_biological_agent_detector">
    <rdfs:subClassOf rdf:resource="jc3iedm_OBJECT-TYPE.owl#CBRN-EQUIPMENT-TYPE"/>
    <rdfs:label xml:lang="en">automated chemical and biological agent detector</rdfs:label>
    <rdfs:comment xml:lang="en">An unattended chemical and biological detection and alarm system.</rdfs:comment>
    <rdf:type rdf:resource="http://www.w3.org/2002/07/owl#Class"/>
  </rdf:Description>
  <rdf:Description rdf:about="jc3iedm_OBJECT-TYPE.owl#route-type-category-code">
    <rdf:type rdf:resource="http://www.w3.org/2002/07/owl#DatatypeProperty"/>
    <rdfs:domain rdf:resource="jc3iedm_OBJECT-TYPE.owl#ROUTE-TYPE"/>
    <rdfs:range rdf:resource="http://www.w3.org/2001/XMLSchema#string"/>
  </rdf:Description>
  <rdf:Description rdf:about="#UNIT-TYPE_Transportation_and_supply">
    <rdfs:subClassOf rdf:resource="jc3iedm_OBJECT-TYPE.owl#UNIT-TYPE"/>
    <rdfs:label xml:lang="en">transportation and supply</rdfs:label>
    <rdfs:comment xml:lang="en">A UNIT-TYPE whose principal designation is the provision of transport for assets and the distribution of supplies.</rdfs:comment>
    <rdf:type rdf:resource="http://www.w3.org/2002/07/owl#Class"/>
  </rdf:Description>
  <rdf:Description rdf:about="#CONTROL-FEATURE-TYPE_High_density_airspace_control_zone">
    <rdfs:subClassOf rdf:resource="jc3iedm_OBJECT-TYPE.owl#CONTROL-FEATURE-TYPE"/>
    <rdfs:label xml:lang="en">high density airspace control zone</rdfs:label>
    <rdfs:comment xml:lang="en">Airspace designated in an airspace control plan or airspace control order in which there is a concentrated employment of numerous and varied weapons and airspace users. A high-density airspace control zone has defined dimensions that usually coincide with geographical features or navigational aids. Access to a high-density airspace control zone is normally controlled by the manoeuvre commander. The manoeuvre commander can also direct a more restrictive weapons status within the high-density airspace control zone.</rdfs:comment>
    <rdf:type rdf:resource="http://www.w3.org/2002/07/owl#Class"/>
  </rdf:Description>
  <rdf:Description rdf:about="jc3iedm_OBJECT-TYPE.owl#equipment-type-maximum-height-dimension">
    <rdf:type rdf:resource="http://www.w3.org/2002/07/owl#DatatypeProperty"/>
    <rdfs:domain rdf:resource="jc3iedm_OBJECT-TYPE.owl#EQUIPMENT-TYPE"/>
  </rdf:Description>
  <rdf:Description rdf:about="#SUBSURFACE-VESSEL-TYPE_Not_known">
    <rdfs:subClassOf rdf:resource="jc3iedm_OBJECT-TYPE.owl#SUBSURFACE-VESSEL-TYPE"/>
    <rdfs:label xml:lang="en">not known</rdfs:label>
    <rdfs:comment xml:lang="en">It is not possible to determine which value is most applicable.</rdfs:comment>
    <rdf:type rdf:resource="http://www.w3.org/2002/07/owl#Class"/>
  </rdf:Description>
  <rdf:Description rdf:about="jc3iedm_OBJECT-TYPE.owl#vessel-type-propeller-count">
    <rdf:type rdf:resource="http://www.w3.org/2002/07/owl#DatatypeProperty"/>
    <rdfs:domain rdf:resource="jc3iedm_OBJECT-TYPE.owl#VESSEL-TYPE"/>
  </rdf:Description>
  <rdf:Description rdf:about="#AIRCRAFT-TYPE_Lighter_than_air">
    <rdfs:subClassOf rdf:resource="jc3iedm_OBJECT-TYPE.owl#AIRCRAFT-TYPE"/>
    <rdfs:label xml:lang="en">lighter than air</rdfs:label>
    <rdfs:comment xml:lang="en">A machine or device capable of atmospheric flight weighing less than the air it displaces.</rdfs:comment>
    <rdf:type rdf:resource="http://www.w3.org/2002/07/owl#Class"/>
  </rdf:Description>
  <rdf:Description rdf:about="#SURFACE-VESSEL-TYPE_Armed_police_gunboat">
    <rdfs:subClassOf rdf:resource="jc3iedm_OBJECT-TYPE.owl#SURFACE-VESSEL-TYPE"/>
    <rdfs:label xml:lang="en">armed police gunboat</rdfs:label>
    <rdfs:comment xml:lang="en">Armed vessel operated by police. Size may vary.</rdfs:comment>
    <rdf:type rdf:resource="http://www.w3.org/2002/07/owl#Class"/>
  </rdf:Description>
  <rdf:Description rdf:about="#SURFACE-VESSEL-TYPE_Landing_craft,_medium,_air_cushion">
    <rdfs:subClassOf rdf:resource="jc3iedm_OBJECT-TYPE.owl#SURFACE-VESSEL-TYPE"/>
    <rdfs:label xml:lang="en">landing craft, medium, air cushion</rdfs:label>
    <rdfs:comment xml:lang="en">Landing craft in size range 15-25 metres capable of carrying 1 tank or 50-200 troops. Must have landing ramp. It is an air cushion or surface effect design.</rdfs:comment>
    <rdf:type rdf:resource="http://www.w3.org/2002/07/owl#Class"/>
  </rdf:Description>
  <rdf:Description rdf:about="#MILITARY-POST-TYPE_Air_liaison_officer">
    <rdfs:subClassOf rdf:resource="jc3iedm_OBJECT-TYPE.owl#MILITARY-POST-TYPE"/>
    <rdfs:label xml:lang="en">air liaison officer</rdfs:label>
    <rdfs:comment xml:lang="en">A tactical air force or naval aviation officer attached to a ground or naval unit or formation as the advisor on tactical air operation matters.</rdfs:comment>
    <rdf:type rdf:resource="http://www.w3.org/2002/07/owl#Class"/>
  </rdf:Description>
  <rdf:Description rdf:about="#MILITARY-POST-TYPE_Anaesthetics_physician">
    <rdfs:subClassOf rdf:resource="jc3iedm_OBJECT-TYPE.owl#MILITARY-POST-TYPE"/>
    <rdfs:label xml:lang="en">anaesthetics physician</rdfs:label>
    <rdfs:comment xml:lang="en">A MILITARY-POST-TYPE that is identified as a physician specialising in Anaesthetics.</rdfs:comment>
    <rdf:type rdf:resource="http://www.w3.org/2002/07/owl#Class"/>
  </rdf:Description>
  <rdf:Description rdf:about="#CONTROL-FEATURE-TYPE_Radiation_dose_contour_line">
    <rdfs:subClassOf rdf:resource="jc3iedm_OBJECT-TYPE.owl#CONTROL-FEATURE-TYPE"/>
    <rdfs:label xml:lang="en">radiation dose contour line</rdfs:label>
    <rdfs:comment xml:lang="en">A line on a map, diagram or overlay joining all points at which the radiation dose at a given time is the same. Radiation dose is the amount of energy from ionizing radiation that would be absorbed.</rdfs:comment>
    <rdf:type rdf:resource="http://www.w3.org/2002/07/owl#Class"/>
  </rdf:Description>
  <rdf:Description rdf:about="#SURFACE-VESSEL-TYPE_Hovercraft,_small">
    <rdfs:subClassOf rdf:resource="jc3iedm_OBJECT-TYPE.owl#SURFACE-VESSEL-TYPE"/>
    <rdfs:label xml:lang="en">hovercraft, small</rdfs:label>
    <rdfs:comment xml:lang="en">Non-military hovercraft under ?? Metres.</rdfs:comment>
    <rdf:type rdf:resource="http://www.w3.org/2002/07/owl#Class"/>
  </rdf:Description>
  <rdf:Description rdf:about="#FACILITY-TYPE_Bath">
    <rdfs:subClassOf rdf:resource="jc3iedm_OBJECT-TYPE.owl#FACILITY-TYPE"/>
    <rdfs:label xml:lang="en">bath</rdfs:label>
    <rdfs:comment xml:lang="en">A facility used for personal cleanliness.</rdfs:comment>
    <rdf:type rdf:resource="http://www.w3.org/2002/07/owl#Class"/>
  </rdf:Description>
  <rdf:Description rdf:about="#ORGANISATION-TYPE_Operations_centre">
    <rdfs:subClassOf rdf:resource="jc3iedm_OBJECT-TYPE.owl#ORGANISATION-TYPE"/>
    <rdfs:label xml:lang="en">operations centre</rdfs:label>
    <rdfs:comment xml:lang="en">The ORGANISATION-TYPE is an operations centre.</rdfs:comment>
    <rdf:type rdf:resource="http://www.w3.org/2002/07/owl#Class"/>
  </rdf:Description>
  <rdf:Description rdf:about="#SUBSURFACE-VESSEL-TYPE_Submarine,_ballistic_missile,_nuclear">
    <rdfs:subClassOf rdf:resource="jc3iedm_OBJECT-TYPE.owl#SUBSURFACE-VESSEL-TYPE"/>
    <rdfs:label xml:lang="en">submarine, ballistic missile, nuclear</rdfs:label>
    <rdfs:comment xml:lang="en">A subsurface vessel designed to deliver ballistic missile attacks against assigned targets from either a submerged or surfaced condition with nuclear power.</rdfs:comment>
    <rdf:type rdf:resource="http://www.w3.org/2002/07/owl#Class"/>
  </rdf:Description>
  <rdf:Description rdf:about="#SURFACE-VESSEL-TYPE_Tug,_harbour,_small">
    <rdfs:subClassOf rdf:resource="jc3iedm_OBJECT-TYPE.owl#SURFACE-VESSEL-TYPE"/>
    <rdfs:label xml:lang="en">tug, harbour, small</rdfs:label>
    <rdfs:comment xml:lang="en">Harbour tug under 20 metres with total horsepower under 500.</rdfs:comment>
    <rdf:type rdf:resource="http://www.w3.org/2002/07/owl#Class"/>
  </rdf:Description>
  <rdf:Description rdf:about="jc3iedm_OBJECT-TYPE.owl#unit-type-qualifier-code">
    <rdf:type rdf:resource="http://www.w3.org/2002/07/owl#DatatypeProperty"/>
    <rdfs:domain rdf:resource="jc3iedm_OBJECT-TYPE.owl#UNIT-TYPE"/>
    <rdfs:range rdf:resource="http://www.w3.org/2001/XMLSchema#string"/>
  </rdf:Description>
  <rdf:Description rdf:about="#AMMUNITION-TYPE_Mine,_off-route">
    <rdfs:subClassOf rdf:resource="jc3iedm_OBJECT-TYPE.owl#AMMUNITION-TYPE"/>
    <rdfs:label xml:lang="en">mine, off route</rdfs:label>
    <rdfs:comment xml:lang="en">A mine or mines designed to attack a target obliquely to the targets direction of travel (i.e. in the targets flank or side).</rdfs:comment>
    <rdf:type rdf:resource="http://www.w3.org/2002/07/owl#Class"/>
  </rdf:Description>
  <rdf:Description rdf:about="#CONTROL-FEATURE-TYPE_Pickup_zone">
    <rdfs:subClassOf rdf:resource="jc3iedm_OBJECT-TYPE.owl#CONTROL-FEATURE-TYPE"/>
    <rdfs:label xml:lang="en">pickup zone</rdfs:label>
    <rdfs:comment xml:lang="en">A geographic area used to pick up troops and/or equipment by helicopter.</rdfs:comment>
    <rdf:type rdf:resource="http://www.w3.org/2002/07/owl#Class"/>
  </rdf:Description>
  <rdf:Description rdf:about="#AMMUNITION-TYPE_Air-to-surface_missile">
    <rdfs:subClassOf rdf:resource="jc3iedm_OBJECT-TYPE.owl#AMMUNITION-TYPE"/>
    <rdfs:label xml:lang="en">air to surface missile</rdfs:label>
    <rdfs:comment xml:lang="en">A self-propelled airborne munition which is guided automatically, or by remote control, fired from an aircraft at an object on the ground or sea.</rdfs:comment>
    <rdf:type rdf:resource="http://www.w3.org/2002/07/owl#Class"/>
  </rdf:Description>
  <rdf:Description rdf:about="#SURFACE-VESSEL-TYPE_Minesweeper,_fleet,_air_cushion">
    <rdfs:subClassOf rdf:resource="jc3iedm_OBJECT-TYPE.owl#SURFACE-VESSEL-TYPE"/>
    <rdfs:label xml:lang="en">minesweeper, fleet, air cushion</rdfs:label>
    <rdfs:comment xml:lang="en">Minesweeper in size range 46 metres or more that cannot be regarded as being non-magnetic, with an air cushion or surface effect design.</rdfs:comment>
    <rdf:type rdf:resource="http://www.w3.org/2002/07/owl#Class"/>
  </rdf:Description>
  <rdf:Description rdf:about="#SURFACE-VESSEL-TYPE_Mine_countermeasures_support_ship,_small">
    <rdfs:subClassOf rdf:resource="jc3iedm_OBJECT-TYPE.owl#SURFACE-VESSEL-TYPE"/>
    <rdfs:label xml:lang="en">mine countermeasures support ship, small</rdfs:label>
    <rdfs:comment xml:lang="en">A smaller armed combatant fitted for the control and diminished support of MCM vessels in combat situations. Has limited facilities for repair of Mine countermeasures vessels and their equipment.</rdfs:comment>
    <rdf:type rdf:resource="http://www.w3.org/2002/07/owl#Class"/>
  </rdf:Description>
  <rdf:Description rdf:about="#SURFACE-VESSEL-TYPE_Patrol_craft,_coastal_escort">
    <rdfs:subClassOf rdf:resource="jc3iedm_OBJECT-TYPE.owl#SURFACE-VESSEL-TYPE"/>
    <rdfs:label xml:lang="en">patrol craft, coastal escort</rdfs:label>
    <rdfs:comment xml:lang="en">Vessel in size range 55-75 metres designed and fitted primarily for ASW role and coastal duty. NOTE: Improved seakeeping, vice mere large size, distinguishes Patrol craft, coastal escort from Patrol craft, submarine chaser/escort, general, and vessels lacking this should be typed as Patrol craft, submarine chaser/escort, general.</rdfs:comment>
    <rdf:type rdf:resource="http://www.w3.org/2002/07/owl#Class"/>
  </rdf:Description>
  <rdf:Description rdf:about="#SURFACE-VESSEL-TYPE_Submarine_chaser">
    <rdfs:subClassOf rdf:resource="jc3iedm_OBJECT-TYPE.owl#SURFACE-VESSEL-TYPE"/>
    <rdfs:label xml:lang="en">submarine chaser</rdfs:label>
    <rdfs:comment xml:lang="en">Patrol craft optimised for the ASW role.</rdfs:comment>
    <rdf:type rdf:resource="http://www.w3.org/2002/07/owl#Class"/>
  </rdf:Description>
  <rdf:Description rdf:about="#CIVILIAN-POST-TYPE_Government_minister">
    <rdfs:subClassOf rdf:resource="jc3iedm_OBJECT-TYPE.owl#CIVILIAN-POST-TYPE"/>
    <rdfs:label xml:lang="en">government minister</rdfs:label>
    <rdfs:comment xml:lang="en">A CIVILIAN-POST-TYPE whose job entails the lower level executive duties of the government.</rdfs:comment>
    <rdf:type rdf:resource="http://www.w3.org/2002/07/owl#Class"/>
  </rdf:Description>
  <rdf:Description rdf:about="#FACILITY-TYPE_Anchorage">
    <rdfs:subClassOf rdf:resource="jc3iedm_OBJECT-TYPE.owl#FACILITY-TYPE"/>
    <rdfs:label xml:lang="en">anchorage</rdfs:label>
    <rdfs:comment xml:lang="en">A FACILITY-TYPE that is a place where vessels anchor.</rdfs:comment>
    <rdf:type rdf:resource="http://www.w3.org/2002/07/owl#Class"/>
  </rdf:Description>
  <rdf:Description rdf:about="#ELECTRONIC-EQUIPMENT-TYPE_Not_otherwise_specified">
    <rdfs:subClassOf rdf:resource="jc3iedm_OBJECT-TYPE.owl#ELECTRONIC-EQUIPMENT-TYPE"/>
    <rdfs:label xml:lang="en">not otherwise specified</rdfs:label>
    <rdfs:comment xml:lang="en">The appropriate value is not in the set of specified values.</rdfs:comment>
    <rdf:type rdf:resource="http://www.w3.org/2002/07/owl#Class"/>
  </rdf:Description>
  <rdf:Description rdf:about="jc3iedm_OBJECT-TYPE.owl#unit-type-general-mobility-code">
    <rdf:type rdf:resource="http://www.w3.org/2002/07/owl#DatatypeProperty"/>
    <rdfs:domain rdf:resource="jc3iedm_OBJECT-TYPE.owl#UNIT-TYPE"/>
    <rdfs:range rdf:resource="http://www.w3.org/2001/XMLSchema#string"/>
  </rdf:Description>
  <rdf:Description rdf:about="#ENGINEERING-EQUIPMENT-TYPE_Pile_driver">
    <rdfs:subClassOf rdf:resource="jc3iedm_OBJECT-TYPE.owl#ENGINEERING-EQUIPMENT-TYPE"/>
    <rdfs:label xml:lang="en">pile driver</rdfs:label>
    <rdfs:comment xml:lang="en">A machine for driving piles into the ground, usually consisting of a heavy block of iron, suspended in a frame between two vertical guide-posts, and alternately let fall upon the pile-head, and raised by steam, manual, or other power; some, working with steam, act on the principle of the steam-hammer.</rdfs:comment>
    <rdf:type rdf:resource="http://www.w3.org/2002/07/owl#Class"/>
  </rdf:Description>
  <rdf:Description rdf:about="#HARBOUR-TYPE_Coastal_(Breakwater)">
    <rdfs:subClassOf rdf:resource="jc3iedm_OBJECT-TYPE.owl#HARBOUR-TYPE"/>
    <rdfs:label xml:lang="en">coastal (breakwater)</rdfs:label>
    <rdfs:comment xml:lang="en">A coastal harbour lying behind a man-made breakwater constructed to provide shelter, or supplement inadequate shelter already provided by natural sources.</rdfs:comment>
    <rdf:type rdf:resource="http://www.w3.org/2002/07/owl#Class"/>
  </rdf:Description>
  <rdf:Description rdf:about="#CONTROL-FEATURE-TYPE_Identification_Friend_Foe_switch_on_line">
    <rdfs:subClassOf rdf:resource="jc3iedm_OBJECT-TYPE.owl#CONTROL-FEATURE-TYPE"/>
    <rdfs:label xml:lang="en">identification friend foe switch on line</rdfs:label>
    <rdfs:comment xml:lang="en">Line demarking where friendly aircraft returning to friendly territory start emitting an Identification-Friend-Foe signal.</rdfs:comment>
    <rdf:type rdf:resource="http://www.w3.org/2002/07/owl#Class"/>
  </rdf:Description>
  <rdf:Description rdf:about="#SURFACE-VESSEL-TYPE_Dry_dock,_auxiliary,_repair,_medium">
    <rdfs:subClassOf rdf:resource="jc3iedm_OBJECT-TYPE.owl#SURFACE-VESSEL-TYPE"/>
    <rdfs:label xml:lang="en">dry dock, auxiliary, repair, medium</rdfs:label>
    <rdfs:comment xml:lang="en">Medium and small ship employed as a mobile repair facility providing limited support to various types of ships. Not a lifting ship. Repair primary function, support secondary.</rdfs:comment>
    <rdf:type rdf:resource="http://www.w3.org/2002/07/owl#Class"/>
  </rdf:Description>
  <rdf:Description rdf:about="#ENGINEERING-EQUIPMENT-TYPE_Power_shovel">
    <rdfs:subClassOf rdf:resource="jc3iedm_OBJECT-TYPE.owl#ENGINEERING-EQUIPMENT-TYPE"/>
    <rdfs:label xml:lang="en">power shovel</rdfs:label>
    <rdfs:comment xml:lang="en">A mechanically powered spade-like implement, consisting of a broad blade of metal or other material, attached to a handle and used for raising and removing quantities of earth, grain, coal or other loose material.</rdfs:comment>
    <rdf:type rdf:resource="http://www.w3.org/2002/07/owl#Class"/>
  </rdf:Description>
  <rdf:Description rdf:about="jc3iedm_OBJECT-TYPE.owl#AIRFIELD-TYPE">
    <rdf:type rdf:resource="http://www.w3.org/2002/07/owl#Class"/>
    <rdfs:label xml:lang="en">airfield type</rdfs:label>
    <rdfs:comment xml:lang="en">A FACILITY-TYPE that is a class of an area prepared for the accommodation (including any buildings, installations, or equipment) of landing and take off of aircraft.</rdfs:comment>
    <rdfs:subClassOf rdf:resource="jc3iedm_OBJECT-TYPE.owl#FACILITY-TYPE"/>
  </rdf:Description>
  <rdf:Description rdf:about="#CONSUMABLE-MATERIEL-TYPE_Water">
    <rdfs:subClassOf rdf:resource="jc3iedm_OBJECT-TYPE.owl#CONSUMABLE-MATERIEL-TYPE"/>
    <rdfs:label xml:lang="en">water</rdfs:label>
    <rdfs:comment xml:lang="en">A clear, colourless, nearly odourless and tasteless liquid.</rdfs:comment>
    <rdf:type rdf:resource="http://www.w3.org/2002/07/owl#Class"/>
  </rdf:Description>
  <rdf:Description rdf:about="#MILITARY-OBSTACLE-TYPE_Wall_obstacle">
    <rdfs:subClassOf rdf:resource="jc3iedm_OBJECT-TYPE.owl#MILITARY-OBSTACLE-TYPE"/>
    <rdfs:label xml:lang="en">wall obstacle</rdfs:label>
    <rdfs:comment xml:lang="en">A continuous, vertical structure, such as a concrete or rock wall created in order to be used as an obstacle.</rdfs:comment>
    <rdf:type rdf:resource="http://www.w3.org/2002/07/owl#Class"/>
  </rdf:Description>
  <rdf:Description rdf:about="#CIVILIAN-POST-TYPE_Release_authority">
    <rdfs:subClassOf rdf:resource="jc3iedm_OBJECT-TYPE.owl#CIVILIAN-POST-TYPE"/>
    <rdfs:label xml:lang="en">release authority</rdfs:label>
    <rdfs:comment xml:lang="en">A CIVILIAN-POST-TYPE whose job is to authorize the release of a product or information.</rdfs:comment>
    <rdf:type rdf:resource="http://www.w3.org/2002/07/owl#Class"/>
  </rdf:Description>
  <rdf:Description rdf:about="#CONTROL-FEATURE-TYPE_Passage_point">
    <rdfs:subClassOf rdf:resource="jc3iedm_OBJECT-TYPE.owl#CONTROL-FEATURE-TYPE"/>
    <rdfs:label xml:lang="en">passage point</rdfs:label>
    <rdfs:comment xml:lang="en">A specifically designated place where units will pass through one another either in an advance or withdrawal. It is located where the commander desires subordinate units to physically execute a passage of lines.</rdfs:comment>
    <rdf:type rdf:resource="http://www.w3.org/2002/07/owl#Class"/>
  </rdf:Description>
  <rdf:Description rdf:about="#VEHICLE-TYPE_Assault_vehicle">
    <rdfs:subClassOf rdf:resource="jc3iedm_OBJECT-TYPE.owl#VEHICLE-TYPE"/>
    <rdfs:label xml:lang="en">assault vehicle</rdfs:label>
    <rdfs:comment xml:lang="en">A vehicle designed to carry assault troops.</rdfs:comment>
    <rdf:type rdf:resource="http://www.w3.org/2002/07/owl#Class"/>
  </rdf:Description>
  <rdf:Description rdf:about="#CONTROL-FEATURE-TYPE_Objective_area">
    <rdfs:subClassOf rdf:resource="jc3iedm_OBJECT-TYPE.owl#CONTROL-FEATURE-TYPE"/>
    <rdfs:label xml:lang="en">objective area</rdfs:label>
    <rdfs:comment xml:lang="en">A defined geographical area within which is located an objective to be captured or reached by the military forces. This area is defined by competent authority for purposes of command and control.</rdfs:comment>
    <rdf:type rdf:resource="http://www.w3.org/2002/07/owl#Class"/>
  </rdf:Description>
  <rdf:Description rdf:about="#AMMUNITION-TYPE_Depth_charge">
    <rdfs:subClassOf rdf:resource="jc3iedm_OBJECT-TYPE.owl#AMMUNITION-TYPE"/>
    <rdfs:label xml:lang="en">depth charge</rdfs:label>
    <rdfs:comment xml:lang="en">Any charge designed for explosion under water, especially such a charge dropped or catapulted from delivery equipment and used against submarines.</rdfs:comment>
    <rdf:type rdf:resource="http://www.w3.org/2002/07/owl#Class"/>
  </rdf:Description>
  <rdf:Description rdf:about="#MARITIME-EQUIPMENT-TYPE_Swell_recorder">
    <rdfs:subClassOf rdf:resource="jc3iedm_OBJECT-TYPE.owl#MARITIME-EQUIPMENT-TYPE"/>
    <rdfs:label xml:lang="en">swell recorder</rdfs:label>
    <rdfs:comment xml:lang="en">A device used to record the pressure fluctuation on the bottom.</rdfs:comment>
    <rdf:type rdf:resource="http://www.w3.org/2002/07/owl#Class"/>
  </rdf:Description>
  <rdf:Description rdf:about="jc3iedm_OBJECT-TYPE.owl#FEATURE-TYPE">
    <rdf:type rdf:resource="http://www.w3.org/2002/07/owl#Class"/>
    <rdfs:label xml:lang="en">feature type</rdfs:label>
    <rdfs:comment xml:lang="en">An OBJECT-TYPE that encompasses meteorological, geographic, and control features of military significance.</rdfs:comment>
  </rdf:Description>
  <rdf:Description rdf:about="#CONTROL-FEATURE-TYPE_Temporary_segregated_area">
    <rdfs:subClassOf rdf:resource="jc3iedm_OBJECT-TYPE.owl#CONTROL-FEATURE-TYPE"/>
    <rdfs:label xml:lang="en">temporary segregated area</rdfs:label>
    <rdfs:comment xml:lang="en">An airspace of defined dimensions within which activities require the reservation of airspace for the exclusive use of specific users during a determined period of time.</rdfs:comment>
    <rdf:type rdf:resource="http://www.w3.org/2002/07/owl#Class"/>
  </rdf:Description>
  <rdf:Description rdf:about="#SURFACE-VESSEL-TYPE_Not_otherwise_specified">
    <rdfs:subClassOf rdf:resource="jc3iedm_OBJECT-TYPE.owl#SURFACE-VESSEL-TYPE"/>
    <rdfs:label xml:lang="en">not otherwise specified</rdfs:label>
    <rdfs:comment xml:lang="en">The appropriate value is not in the set of specified values.</rdfs:comment>
    <rdf:type rdf:resource="http://www.w3.org/2002/07/owl#Class"/>
  </rdf:Description>
  <rdf:Description rdf:about="#CONTROL-FEATURE-TYPE_Area_of_responsibility">
    <rdfs:subClassOf rdf:resource="jc3iedm_OBJECT-TYPE.owl#CONTROL-FEATURE-TYPE"/>
    <rdfs:label xml:lang="en">area of responsibility</rdfs:label>
    <rdfs:comment xml:lang="en">A CONTROL-FEATURE-TYPE with an area location which defines an area of land in which responsibility is specifically assigned to the commander of the area for the development and maintenance of installations, control of movement and the conduct of tactical operations involving troops under his control along with parallel authority to exercise these functions.</rdfs:comment>
    <rdf:type rdf:resource="http://www.w3.org/2002/07/owl#Class"/>
  </rdf:Description>
  <rdf:Description rdf:about="#SURFACE-VESSEL-TYPE_Training_ship_sail_(naval)">
    <rdfs:subClassOf rdf:resource="jc3iedm_OBJECT-TYPE.owl#SURFACE-VESSEL-TYPE"/>
    <rdfs:label xml:lang="en">training ship sail (naval)</rdfs:label>
    <rdfs:comment xml:lang="en">Naval sail training ship.</rdfs:comment>
    <rdf:type rdf:resource="http://www.w3.org/2002/07/owl#Class"/>
  </rdf:Description>
  <rdf:Description rdf:about="#CONTROL-FEATURE-TYPE_Chemically_contaminated_area">
    <rdfs:subClassOf rdf:resource="jc3iedm_OBJECT-TYPE.owl#CONTROL-FEATURE-TYPE"/>
    <rdfs:label xml:lang="en">chemically contaminated area</rdfs:label>
    <rdfs:comment xml:lang="en">A CONTROL-FEATURE-TYPE that identifies the predicted or confirmed contour of an area in which chemical agents may produce casualties in man or animals and damage to plants or materiel.</rdfs:comment>
    <rdf:type rdf:resource="http://www.w3.org/2002/07/owl#Class"/>
  </rdf:Description>
  <rdf:Description rdf:about="#GROUP-ORGANISATION-TYPE_Terrorist">
    <rdfs:subClassOf rdf:resource="jc3iedm_OBJECT-TYPE.owl#GROUP-ORGANISATION-TYPE"/>
    <rdfs:label xml:lang="en">terrorist</rdfs:label>
    <rdfs:comment xml:lang="en">A GROUP-ORGANISATION-TYPE that comprises persons that attempt to further their views by a system of coercive intimidation.</rdfs:comment>
    <rdf:type rdf:resource="http://www.w3.org/2002/07/owl#Class"/>
  </rdf:Description>
  <rdf:Description rdf:about="#SURFACE-VESSEL-TYPE_Floating_dredger">
    <rdfs:subClassOf rdf:resource="jc3iedm_OBJECT-TYPE.owl#SURFACE-VESSEL-TYPE"/>
    <rdfs:label xml:lang="en">floating dredger</rdfs:label>
    <rdfs:comment xml:lang="en">Craft employed as a dredge.</rdfs:comment>
    <rdf:type rdf:resource="http://www.w3.org/2002/07/owl#Class"/>
  </rdf:Description>
  <rdf:Description rdf:about="#SURFACE-VESSEL-TYPE_Patrol_ship,_fast">
    <rdfs:subClassOf rdf:resource="jc3iedm_OBJECT-TYPE.owl#SURFACE-VESSEL-TYPE"/>
    <rdfs:label xml:lang="en">patrol ship, fast</rdfs:label>
    <rdfs:comment xml:lang="en">Patrol, blockade and surveillance ship in range 45-85 metres overall. Designed to operate in other than open ocean areas. Has special mission of attacking hostile ships. Must have at least 76mm main armament and be capable of at least 35 knots - 65 km/hr.</rdfs:comment>
    <rdf:type rdf:resource="http://www.w3.org/2002/07/owl#Class"/>
  </rdf:Description>
  <rdf:Description rdf:about="#MARITIME-EQUIPMENT-TYPE_Anchor">
    <rdfs:subClassOf rdf:resource="jc3iedm_OBJECT-TYPE.owl#MARITIME-EQUIPMENT-TYPE"/>
    <rdfs:label xml:lang="en">anchor</rdfs:label>
    <rdfs:comment xml:lang="en">An equipment for holding a vessel in a fixed position mooring it to the bottom of the sea or river by means of a heavy structure traditionally composed of a long shank with a ring at one end for the cable and at the other end two arms tending upwards with barbs on each side.</rdfs:comment>
    <rdf:type rdf:resource="http://www.w3.org/2002/07/owl#Class"/>
  </rdf:Description>
  <rdf:Description rdf:about="#FACILITY-TYPE_Medical_facility,_hospital,_not_otherwise_specified">
    <rdfs:subClassOf rdf:resource="jc3iedm_OBJECT-TYPE.owl#FACILITY-TYPE"/>
    <rdfs:label xml:lang="en">medical facility, hospital, not otherwise specified</rdfs:label>
    <rdfs:comment xml:lang="en">A facility established for the purpose of furnishing medical and/or dental care to eligible individuals.</rdfs:comment>
    <rdf:type rdf:resource="http://www.w3.org/2002/07/owl#Class"/>
  </rdf:Description>
  <rdf:Description rdf:about="#SURFACE-VESSEL-TYPE_Repair_ship,_small">
    <rdfs:subClassOf rdf:resource="jc3iedm_OBJECT-TYPE.owl#SURFACE-VESSEL-TYPE"/>
    <rdfs:label xml:lang="en">repair ship, small</rdfs:label>
    <rdfs:comment xml:lang="en">Ship 40-120 metres capable of providing mobile repair facilities and possible limited support to smaller boats.</rdfs:comment>
    <rdf:type rdf:resource="http://www.w3.org/2002/07/owl#Class"/>
  </rdf:Description>
  <rdf:Description rdf:about="#CONTROL-FEATURE-TYPE_Blocking_position">
    <rdfs:subClassOf rdf:resource="jc3iedm_OBJECT-TYPE.owl#CONTROL-FEATURE-TYPE"/>
    <rdfs:label xml:lang="en">blocking position</rdfs:label>
    <rdfs:comment xml:lang="en">A defensive position so sited as to deny the enemy access to a given area or to prevent his advance in a given direction.</rdfs:comment>
    <rdf:type rdf:resource="http://www.w3.org/2002/07/owl#Class"/>
  </rdf:Description>
  <rdf:Description rdf:about="#SURFACE-VESSEL-TYPE_Lighter,_covered,_ferry">
    <rdfs:subClassOf rdf:resource="jc3iedm_OBJECT-TYPE.owl#SURFACE-VESSEL-TYPE"/>
    <rdfs:label xml:lang="en">lighter, covered, ferry</rdfs:label>
    <rdfs:comment xml:lang="en">Self-propelled transport craft under 40 metres.</rdfs:comment>
    <rdf:type rdf:resource="http://www.w3.org/2002/07/owl#Class"/>
  </rdf:Description>
  <rdf:Description rdf:about="#ORGANISATION-TYPE_Combined_air_operations_centre">
    <rdfs:subClassOf rdf:resource="jc3iedm_OBJECT-TYPE.owl#ORGANISATION-TYPE"/>
    <rdfs:label xml:lang="en">combined air operations centre</rdfs:label>
    <rdfs:comment xml:lang="en">The ORGANISATION-TYPE that is staffed by members of more than one nation, established for planning, directing, and executing combined air operations in support of the combined force commander's operation or campaign objectives.</rdfs:comment>
    <rdf:type rdf:resource="http://www.w3.org/2002/07/owl#Class"/>
  </rdf:Description>
  <rdf:Description rdf:about="#CONTROL-FEATURE-TYPE_Air_defence_operations_area">
    <rdfs:subClassOf rdf:resource="jc3iedm_OBJECT-TYPE.owl#CONTROL-FEATURE-TYPE"/>
    <rdfs:label xml:lang="en">air defence operations area</rdfs:label>
    <rdfs:comment xml:lang="en">A geographical area within which procedures are established to minimize interference between air defence operations and other types of operations.</rdfs:comment>
    <rdf:type rdf:resource="http://www.w3.org/2002/07/owl#Class"/>
  </rdf:Description>
  <rdf:Description rdf:about="#VEHICLE-TYPE_Trailer">
    <rdfs:subClassOf rdf:resource="jc3iedm_OBJECT-TYPE.owl#VEHICLE-TYPE"/>
    <rdfs:label xml:lang="en">trailer</rdfs:label>
    <rdfs:comment xml:lang="en">A vehicle designed to be towed by another.</rdfs:comment>
    <rdf:type rdf:resource="http://www.w3.org/2002/07/owl#Class"/>
  </rdf:Description>
  <rdf:Description rdf:about="#FACILITY-TYPE_Road,_junction">
    <rdfs:subClassOf rdf:resource="jc3iedm_OBJECT-TYPE.owl#FACILITY-TYPE"/>
    <rdfs:label xml:lang="en">road, junction</rdfs:label>
    <rdfs:comment xml:lang="en">A site where two or more roads join or form a connection.</rdfs:comment>
    <rdf:type rdf:resource="http://www.w3.org/2002/07/owl#Class"/>
  </rdf:Description>
  <rdf:Description rdf:about="#ORGANISATION-TYPE_Not_known">
    <rdfs:subClassOf rdf:resource="jc3iedm_OBJECT-TYPE.owl#ORGANISATION-TYPE"/>
    <rdfs:label xml:lang="en">not known</rdfs:label>
    <rdfs:comment xml:lang="en">It is not possible to determine which value is most applicable.</rdfs:comment>
    <rdf:type rdf:resource="http://www.w3.org/2002/07/owl#Class"/>
  </rdf:Description>
  <rdf:Description rdf:about="jc3iedm_OBJECT-TYPE.owl#aircraft-type-category-code">
    <rdf:type rdf:resource="http://www.w3.org/2002/07/owl#DatatypeProperty"/>
    <rdfs:domain rdf:resource="jc3iedm_OBJECT-TYPE.owl#AIRCRAFT-TYPE"/>
    <rdfs:range rdf:resource="http://www.w3.org/2001/XMLSchema#string"/>
  </rdf:Description>
  <rdf:Description rdf:about="#FACILITY-TYPE_Control_tower">
    <rdfs:subClassOf rdf:resource="jc3iedm_OBJECT-TYPE.owl#FACILITY-TYPE"/>
    <rdfs:label xml:lang="en">control tower</rdfs:label>
    <rdfs:comment xml:lang="en">A tower-like structure that houses the persons and equipment used to control the flow of air, rail, or marine traffic.</rdfs:comment>
    <rdf:type rdf:resource="http://www.w3.org/2002/07/owl#Class"/>
  </rdf:Description>
  <rdf:Description rdf:about="#ENGINEERING-EQUIPMENT-TYPE_Bridge_vehicle">
    <rdfs:subClassOf rdf:resource="jc3iedm_OBJECT-TYPE.owl#ENGINEERING-EQUIPMENT-TYPE"/>
    <rdfs:label xml:lang="en">bridge vehicle</rdfs:label>
    <rdfs:comment xml:lang="en">A vehicle used to deliver a bridge.</rdfs:comment>
    <rdf:type rdf:resource="http://www.w3.org/2002/07/owl#Class"/>
  </rdf:Description>
  <rdf:Description rdf:about="#SURFACE-VESSEL-TYPE_Floating_barracks">
    <rdfs:subClassOf rdf:resource="jc3iedm_OBJECT-TYPE.owl#SURFACE-VESSEL-TYPE"/>
    <rdfs:label xml:lang="en">floating barracks</rdfs:label>
    <rdfs:comment xml:lang="en">Craft used as accommodation for vessels crews.</rdfs:comment>
    <rdf:type rdf:resource="http://www.w3.org/2002/07/owl#Class"/>
  </rdf:Description>
  <rdf:Description rdf:about="#SURFACE-VESSEL-TYPE_Minelayer,_ocean">
    <rdfs:subClassOf rdf:resource="jc3iedm_OBJECT-TYPE.owl#SURFACE-VESSEL-TYPE"/>
    <rdfs:label xml:lang="en">minelayer, ocean</rdfs:label>
    <rdfs:comment xml:lang="en">Large ship over 85 metres used primarily for minelaying.</rdfs:comment>
    <rdf:type rdf:resource="http://www.w3.org/2002/07/owl#Class"/>
  </rdf:Description>
  <rdf:Description rdf:about="#CONTROL-FEATURE-TYPE_Report_line">
    <rdfs:subClassOf rdf:resource="jc3iedm_OBJECT-TYPE.owl#CONTROL-FEATURE-TYPE"/>
    <rdfs:label xml:lang="en">report line</rdfs:label>
    <rdfs:comment xml:lang="en">A line at which troops, after having reached it, must report to their command echelon.</rdfs:comment>
    <rdf:type rdf:resource="http://www.w3.org/2002/07/owl#Class"/>
  </rdf:Description>
  <rdf:Description rdf:about="#SURFACE-VESSEL-TYPE_Amphibious_transport,_personnel">
    <rdfs:subClassOf rdf:resource="jc3iedm_OBJECT-TYPE.owl#SURFACE-VESSEL-TYPE"/>
    <rdfs:label xml:lang="en">amphibious transport, personnel</rdfs:label>
    <rdfs:comment xml:lang="en">A large ship capable of carrying 1300-1500 assault troops and capable of landing them in its own organic landing craft.</rdfs:comment>
    <rdf:type rdf:resource="http://www.w3.org/2002/07/owl#Class"/>
  </rdf:Description>
  <rdf:Description rdf:about="#SURFACE-VESSEL-TYPE_Ice_breaker,_nuclear_powered">
    <rdfs:subClassOf rdf:resource="jc3iedm_OBJECT-TYPE.owl#SURFACE-VESSEL-TYPE"/>
    <rdfs:label xml:lang="en">ice breaker, nuclear powered</rdfs:label>
    <rdfs:comment xml:lang="en">Armed ship in size range 70 metres or more used primarily for icebreaking duties. It has nuclear power.</rdfs:comment>
    <rdf:type rdf:resource="http://www.w3.org/2002/07/owl#Class"/>
  </rdf:Description>
  <rdf:Description rdf:about="jc3iedm_OBJECT-TYPE.owl#BIOLOGICAL-MATERIEL-TYPE">
    <rdf:type rdf:resource="http://www.w3.org/2002/07/owl#Class"/>
    <rdfs:label xml:lang="en">biological materiel type</rdfs:label>
    <rdfs:comment xml:lang="en">A CONSUMABLE-MATERIEL-TYPE that is either a microorganism that causes disease in man, plants, or animals or causes the deterioration of materiel; or a toxin, produced by an animal, plant, or microorganism, which may kill, seriously injure, or incapacitate personnel through its physiological effects.</rdfs:comment>
    <rdfs:subClassOf rdf:resource="jc3iedm_OBJECT-TYPE.owl#CONSUMABLE-MATERIEL-TYPE"/>
  </rdf:Description>
  <rdf:Description rdf:about="#MILITARY-POST-TYPE_Liaison_officer">
    <rdfs:subClassOf rdf:resource="jc3iedm_OBJECT-TYPE.owl#MILITARY-POST-TYPE"/>
    <rdfs:label xml:lang="en">liaison officer</rdfs:label>
    <rdfs:comment xml:lang="en">A MILITARY-POST-TYPE responsible for liaison duties.</rdfs:comment>
    <rdf:type rdf:resource="http://www.w3.org/2002/07/owl#Class"/>
  </rdf:Description>
  <rdf:Description rdf:about="#AMMUNITION-TYPE_Hand_grenade">
    <rdfs:subClassOf rdf:resource="jc3iedm_OBJECT-TYPE.owl#AMMUNITION-TYPE"/>
    <rdfs:label xml:lang="en">hand grenade</rdfs:label>
    <rdfs:comment xml:lang="en">An explosive missile, smaller than a bombshell, thrown by hand.</rdfs:comment>
    <rdf:type rdf:resource="http://www.w3.org/2002/07/owl#Class"/>
  </rdf:Description>
  <rdf:Description rdf:about="#MILITARY-POST-TYPE_Internal_medicine_physician">
    <rdfs:subClassOf rdf:resource="jc3iedm_OBJECT-TYPE.owl#MILITARY-POST-TYPE"/>
    <rdfs:label xml:lang="en">internal medicine physician</rdfs:label>
    <rdfs:comment xml:lang="en">A MILITARY-POST-TYPE that is identified as a physician specialising in Internal medicine.</rdfs:comment>
    <rdf:type rdf:resource="http://www.w3.org/2002/07/owl#Class"/>
  </rdf:Description>
  <rdf:Description rdf:about="#ROUTE-TYPE_Airway">
    <rdfs:subClassOf rdf:resource="jc3iedm_OBJECT-TYPE.owl#ROUTE-TYPE"/>
    <rdfs:label xml:lang="en">airway</rdfs:label>
    <rdfs:comment xml:lang="en">A control area or portion thereof established in the form of a corridor equipped with radio navigational aids.</rdfs:comment>
    <rdf:type rdf:resource="http://www.w3.org/2002/07/owl#Class"/>
  </rdf:Description>
  <rdf:Description rdf:about="#UNIT-TYPE_Artillery">
    <rdfs:subClassOf rdf:resource="jc3iedm_OBJECT-TYPE.owl#UNIT-TYPE"/>
    <rdfs:label xml:lang="en">artillery</rdfs:label>
    <rdfs:comment xml:lang="en">A UNIT-TYPE whose principal designation is the employment of large guns, cannon or ordnance in support of manoeuvre units.</rdfs:comment>
    <rdf:type rdf:resource="http://www.w3.org/2002/07/owl#Class"/>
  </rdf:Description>
  <rdf:Description rdf:about="#SURFACE-VESSEL-TYPE_Aviation_supply_ship">
    <rdfs:subClassOf rdf:resource="jc3iedm_OBJECT-TYPE.owl#SURFACE-VESSEL-TYPE"/>
    <rdfs:label xml:lang="en">aviation supply ship</rdfs:label>
    <rdfs:comment xml:lang="en">Ship equipped to carry and supply aviation stores.</rdfs:comment>
    <rdf:type rdf:resource="http://www.w3.org/2002/07/owl#Class"/>
  </rdf:Description>
  <rdf:Description rdf:about="#CONTROL-FEATURE-TYPE_Military_operations_area">
    <rdfs:subClassOf rdf:resource="jc3iedm_OBJECT-TYPE.owl#CONTROL-FEATURE-TYPE"/>
    <rdfs:label xml:lang="en">military operations area</rdfs:label>
    <rdfs:comment xml:lang="en">Airspace established outside class "A" airspace to separate or segregate certain non-hazardous military activities from instrument flight rule traffic and to identify for visual flight rule traffic where these activities are conducted.</rdfs:comment>
    <rdf:type rdf:resource="http://www.w3.org/2002/07/owl#Class"/>
  </rdf:Description>
  <rdf:Description rdf:about="jc3iedm_OBJECT-TYPE.owl#vessel-type-operational-displacement-quantity">
    <rdf:type rdf:resource="http://www.w3.org/2002/07/owl#DatatypeProperty"/>
    <rdfs:domain rdf:resource="jc3iedm_OBJECT-TYPE.owl#VESSEL-TYPE"/>
  </rdf:Description>
  <rdf:Description rdf:about="#RAILCAR-TYPE_Rolling_stock">
    <rdfs:subClassOf rdf:resource="jc3iedm_OBJECT-TYPE.owl#RAILCAR-TYPE"/>
    <rdfs:label xml:lang="en">rolling stock</rdfs:label>
    <rdfs:comment xml:lang="en">Generic term for wagons, either passenger, freight or specialised that are used to form a train.</rdfs:comment>
    <rdf:type rdf:resource="http://www.w3.org/2002/07/owl#Class"/>
  </rdf:Description>
  <rdf:Description rdf:about="#SURFACE-VESSEL-TYPE_Ammunition_ship,_small">
    <rdfs:subClassOf rdf:resource="jc3iedm_OBJECT-TYPE.owl#SURFACE-VESSEL-TYPE"/>
    <rdfs:label xml:lang="en">ammunition ship, small</rdfs:label>
    <rdfs:comment xml:lang="en">Ship between 40-120 metres handling less than 5000 tons of ammunition and capable of providing underway replenishment of ammunition.</rdfs:comment>
    <rdf:type rdf:resource="http://www.w3.org/2002/07/owl#Class"/>
  </rdf:Description>
  <rdf:Description rdf:about="#AMMUNITION-TYPE_Explosive">
    <rdfs:subClassOf rdf:resource="jc3iedm_OBJECT-TYPE.owl#AMMUNITION-TYPE"/>
    <rdfs:label xml:lang="en">explosive</rdfs:label>
    <rdfs:comment xml:lang="en">An explosive substance.</rdfs:comment>
    <rdf:type rdf:resource="http://www.w3.org/2002/07/owl#Class"/>
  </rdf:Description>
  <rdf:Description rdf:about="#VEHICLE-TYPE_Engineering,_not_otherwise_specified">
    <rdfs:subClassOf rdf:resource="jc3iedm_OBJECT-TYPE.owl#VEHICLE-TYPE"/>
    <rdfs:label xml:lang="en">engineering, not otherwise specified</rdfs:label>
    <rdfs:comment xml:lang="en">A vehicle used by engineers, without any other precision.</rdfs:comment>
    <rdf:type rdf:resource="http://www.w3.org/2002/07/owl#Class"/>
  </rdf:Description>
  <rdf:Description rdf:about="#SURFACE-VESSEL-TYPE_Patrol/torpedo_boat_support_ship_tender">
    <rdfs:subClassOf rdf:resource="jc3iedm_OBJECT-TYPE.owl#SURFACE-VESSEL-TYPE"/>
    <rdfs:label xml:lang="en">patrol/torpedo boat support ship tender</rdfs:label>
    <rdfs:comment xml:lang="en">Ship of any size employed primarily to furnish facilities and services for the support and repair of small patrol craft, the primary function being support.</rdfs:comment>
    <rdf:type rdf:resource="http://www.w3.org/2002/07/owl#Class"/>
  </rdf:Description>
  <rdf:Description rdf:about="#VEHICLE-TYPE_Armoured_C2V/ACV">
    <rdfs:subClassOf rdf:resource="jc3iedm_OBJECT-TYPE.owl#VEHICLE-TYPE"/>
    <rdfs:label xml:lang="en">armoured c2v/acv</rdfs:label>
    <rdfs:comment xml:lang="en">An Armoured Command and Control Vehicle (C2V) or an Armoured Combat Vehicle (ACV).</rdfs:comment>
    <rdf:type rdf:resource="http://www.w3.org/2002/07/owl#Class"/>
  </rdf:Description>
  <rdf:Description rdf:about="#UNIT-TYPE_Missile,_surface-to-air">
    <rdfs:subClassOf rdf:resource="jc3iedm_OBJECT-TYPE.owl#UNIT-TYPE"/>
    <rdfs:label xml:lang="en">missile, surface to air</rdfs:label>
    <rdfs:comment xml:lang="en">A UNIT-TYPE whose principal designation is the employment of surface-based missiles to fire at air targets.</rdfs:comment>
    <rdf:type rdf:resource="http://www.w3.org/2002/07/owl#Class"/>
  </rdf:Description>
  <rdf:Description rdf:about="jc3iedm_OBJECT-TYPE.owl#surface-vessel-type-displacement-quantity">
    <rdf:type rdf:resource="http://www.w3.org/2002/07/owl#DatatypeProperty"/>
    <rdfs:domain rdf:resource="jc3iedm_OBJECT-TYPE.owl#SURFACE-VESSEL-TYPE"/>
  </rdf:Description>
  <rdf:Description rdf:about="#ELECTRONIC-EQUIPMENT-TYPE_Communication">
    <rdfs:subClassOf rdf:resource="jc3iedm_OBJECT-TYPE.owl#ELECTRONIC-EQUIPMENT-TYPE"/>
    <rdfs:label xml:lang="en">communication</rdfs:label>
    <rdfs:comment xml:lang="en">A group of interrelated communications equipment utilising the electromagnetic spectrum for the transmission and/or receiving of speech and data information.</rdfs:comment>
    <rdf:type rdf:resource="http://www.w3.org/2002/07/owl#Class"/>
  </rdf:Description>
  <rdf:Description rdf:about="#SURFACE-VESSEL-TYPE_Patrol_ship,_icebreaker">
    <rdfs:subClassOf rdf:resource="jc3iedm_OBJECT-TYPE.owl#SURFACE-VESSEL-TYPE"/>
    <rdfs:label xml:lang="en">patrol ship, icebreaker</rdfs:label>
    <rdfs:comment xml:lang="en">Any ship designed as an icebreaker but employed primarily in a patrol mission. The icebreaking capability is to facilitate the patrol function through ice, rather than to support the movement of other ships.</rdfs:comment>
    <rdf:type rdf:resource="http://www.w3.org/2002/07/owl#Class"/>
  </rdf:Description>
  <rdf:Description rdf:about="#SURFACE-VESSEL-TYPE_Catboat">
    <rdfs:subClassOf rdf:resource="jc3iedm_OBJECT-TYPE.owl#SURFACE-VESSEL-TYPE"/>
    <rdfs:label xml:lang="en">catboat</rdfs:label>
    <rdfs:comment xml:lang="en">Small fishing vessel of specific design, usually powered by sail.</rdfs:comment>
    <rdf:type rdf:resource="http://www.w3.org/2002/07/owl#Class"/>
  </rdf:Description>
  <rdf:Description rdf:about="#FACILITY-TYPE_Gate">
    <rdfs:subClassOf rdf:resource="jc3iedm_OBJECT-TYPE.owl#FACILITY-TYPE"/>
    <rdfs:label xml:lang="en">gate</rdfs:label>
    <rdfs:comment xml:lang="en">A barrier that controls passage to a road, railway, tunnel or bridge.</rdfs:comment>
    <rdf:type rdf:resource="http://www.w3.org/2002/07/owl#Class"/>
  </rdf:Description>
  <rdf:Description rdf:about="#CONTROL-FEATURE-TYPE_Infiltration_line">
    <rdfs:subClassOf rdf:resource="jc3iedm_OBJECT-TYPE.owl#CONTROL-FEATURE-TYPE"/>
    <rdfs:label xml:lang="en">infiltration line</rdfs:label>
    <rdfs:comment xml:lang="en">An infiltration lane is a control measure that fixes fire planning responsibilities and coordinates forward and lateral movement of infiltrating units.</rdfs:comment>
    <rdf:type rdf:resource="http://www.w3.org/2002/07/owl#Class"/>
  </rdf:Description>
  <rdf:Description rdf:about="#AMMUNITION-TYPE_Mine,_wide_area">
    <rdfs:subClassOf rdf:resource="jc3iedm_OBJECT-TYPE.owl#AMMUNITION-TYPE"/>
    <rdfs:label xml:lang="en">mine, wide area</rdfs:label>
    <rdfs:comment xml:lang="en">A mine designed to disable armoured vehicles and will allow large areas to be sown with smart mines that should be difficult to neutralize.</rdfs:comment>
    <rdf:type rdf:resource="http://www.w3.org/2002/07/owl#Class"/>
  </rdf:Description>
  <rdf:Description rdf:about="#MARITIME-EQUIPMENT-TYPE_Not_known">
    <rdfs:subClassOf rdf:resource="jc3iedm_OBJECT-TYPE.owl#MARITIME-EQUIPMENT-TYPE"/>
    <rdfs:label xml:lang="en">not known</rdfs:label>
    <rdfs:comment xml:lang="en">It is not possible to determine which value is most applicable.</rdfs:comment>
    <rdf:type rdf:resource="http://www.w3.org/2002/07/owl#Class"/>
  </rdf:Description>
  <rdf:Description rdf:about="#SURFACE-VESSEL-TYPE_Landing_craft,_mechanized">
    <rdfs:subClassOf rdf:resource="jc3iedm_OBJECT-TYPE.owl#SURFACE-VESSEL-TYPE"/>
    <rdfs:label xml:lang="en">landing craft, mechanized</rdfs:label>
    <rdfs:comment xml:lang="en">Landing craft in size range 15-25 metres capable of carrying 1 tank or 50-200 troops. Must have landing ramp.</rdfs:comment>
    <rdf:type rdf:resource="http://www.w3.org/2002/07/owl#Class"/>
  </rdf:Description>
  <rdf:Description rdf:about="#RADIOACTIVE-MATERIEL-TYPE_Iodine-133">
    <rdfs:subClassOf rdf:resource="jc3iedm_OBJECT-TYPE.owl#RADIOACTIVE-MATERIEL-TYPE"/>
    <rdfs:label xml:lang="en">iodine 133</rdfs:label>
    <rdfs:comment xml:lang="en">A radioactive isotope of the chemical element of atomic number 53, a halogen forming black crystals and a violet vapour.</rdfs:comment>
    <rdf:type rdf:resource="http://www.w3.org/2002/07/owl#Class"/>
  </rdf:Description>
  <rdf:Description rdf:about="#UNIT-TYPE_Combat">
    <rdfs:subClassOf rdf:resource="jc3iedm_OBJECT-TYPE.owl#UNIT-TYPE"/>
    <rdfs:label xml:lang="en">combat</rdfs:label>
    <rdfs:comment xml:lang="en">A UNIT-TYPE who closes with and destroys enemy forces or provides firepower and destructive capabilities in the battlespace.</rdfs:comment>
    <rdf:type rdf:resource="http://www.w3.org/2002/07/owl#Class"/>
  </rdf:Description>
  <rdf:Description rdf:about="#MILITARY-OBSTACLE-TYPE_Wire_obstacle,_not_otherwise_specified">
    <rdfs:subClassOf rdf:resource="jc3iedm_OBJECT-TYPE.owl#MILITARY-OBSTACLE-TYPE"/>
    <rdfs:label xml:lang="en">wire obstacle, not otherwise specified</rdfs:label>
    <rdfs:comment xml:lang="en">No definition provided in APP-6A.</rdfs:comment>
    <rdf:type rdf:resource="http://www.w3.org/2002/07/owl#Class"/>
  </rdf:Description>
  <rdf:Description rdf:about="#CONTROL-FEATURE-TYPE_Zone_of_fire">
    <rdfs:subClassOf rdf:resource="jc3iedm_OBJECT-TYPE.owl#CONTROL-FEATURE-TYPE"/>
    <rdfs:label xml:lang="en">zone of fire</rdfs:label>
    <rdfs:comment xml:lang="en">An area into which a designated ground unit or fire support asset delivers, or is prepared to deliver, fires.</rdfs:comment>
    <rdf:type rdf:resource="http://www.w3.org/2002/07/owl#Class"/>
  </rdf:Description>
  <rdf:Description rdf:about="#CONTROL-FEATURE-TYPE_Airhead">
    <rdfs:subClassOf rdf:resource="jc3iedm_OBJECT-TYPE.owl#CONTROL-FEATURE-TYPE"/>
    <rdfs:label xml:lang="en">airhead</rdfs:label>
    <rdfs:comment xml:lang="en">A designated area in a hostile or threatened territory which, when seized and held, ensures the continuous air landing of troops and material and provides manoeuvre space for operations. Normally it is the area seized in the assault phase of an airborne or air assault operation. Army--The airhead contains enough drop zones (DZs), landing zones (LZs), and extraction zones (EZs) to ensure mass, interior lines of communication and defence in depth.</rdfs:comment>
    <rdf:type rdf:resource="http://www.w3.org/2002/07/owl#Class"/>
  </rdf:Description>
  <rdf:Description rdf:about="#FACILITY-TYPE_Tunnel">
    <rdfs:subClassOf rdf:resource="jc3iedm_OBJECT-TYPE.owl#FACILITY-TYPE"/>
    <rdfs:label xml:lang="en">tunnel</rdfs:label>
    <rdfs:comment xml:lang="en">An underground or underwater passage, open at both ends, and usually containing a road or railway.</rdfs:comment>
    <rdf:type rdf:resource="http://www.w3.org/2002/07/owl#Class"/>
  </rdf:Description>
  <rdf:Description rdf:about="#SURFACE-VESSEL-TYPE_Cable/netlaying_ship">
    <rdfs:subClassOf rdf:resource="jc3iedm_OBJECT-TYPE.owl#SURFACE-VESSEL-TYPE"/>
    <rdfs:label xml:lang="en">cable/netlaying ship</rdfs:label>
    <rdfs:comment xml:lang="en">Ship equipped for cable or netlaying.</rdfs:comment>
    <rdf:type rdf:resource="http://www.w3.org/2002/07/owl#Class"/>
  </rdf:Description>
  <rdf:Description rdf:about="#PERSON-TYPE_Civilian">
    <rdfs:subClassOf rdf:resource="jc3iedm_OBJECT-TYPE.owl#PERSON-TYPE"/>
    <rdfs:label xml:lang="en">civilian</rdfs:label>
    <rdfs:comment xml:lang="en">A PERSON-TYPE who is not a uniformed member of a regular armed force.</rdfs:comment>
    <rdf:type rdf:resource="http://www.w3.org/2002/07/owl#Class"/>
  </rdf:Description>
  <rdf:Description rdf:about="#SURFACE-VESSEL-TYPE_Merchant_ship,_scientific_research/survey">
    <rdfs:subClassOf rdf:resource="jc3iedm_OBJECT-TYPE.owl#SURFACE-VESSEL-TYPE"/>
    <rdfs:label xml:lang="en">merchant ship, scientific research/survey</rdfs:label>
    <rdfs:comment xml:lang="en">Non-naval ship employed to conduct scientific research.</rdfs:comment>
    <rdf:type rdf:resource="http://www.w3.org/2002/07/owl#Class"/>
  </rdf:Description>
  <rdf:Description rdf:about="#SURFACE-VESSEL-TYPE_Yawl">
    <rdfs:subClassOf rdf:resource="jc3iedm_OBJECT-TYPE.owl#SURFACE-VESSEL-TYPE"/>
    <rdfs:label xml:lang="en">yawl</rdfs:label>
    <rdfs:comment xml:lang="en">Sailing vessel of yawl design.</rdfs:comment>
    <rdf:type rdf:resource="http://www.w3.org/2002/07/owl#Class"/>
  </rdf:Description>
  <rdf:Description rdf:about="#BIOLOGICAL-MATERIEL-TYPE_Not_otherwise_specified">
    <rdfs:subClassOf rdf:resource="jc3iedm_OBJECT-TYPE.owl#BIOLOGICAL-MATERIEL-TYPE"/>
    <rdfs:label xml:lang="en">not otherwise specified</rdfs:label>
    <rdfs:comment xml:lang="en">The appropriate value is not in the set of specified values.</rdfs:comment>
    <rdf:type rdf:resource="http://www.w3.org/2002/07/owl#Class"/>
  </rdf:Description>
  <rdf:Description rdf:about="#CONTROL-FEATURE-TYPE_Named_area_of_interest">
    <rdfs:subClassOf rdf:resource="jc3iedm_OBJECT-TYPE.owl#CONTROL-FEATURE-TYPE"/>
    <rdfs:label xml:lang="en">named area of interest</rdfs:label>
    <rdfs:comment xml:lang="en">A point or area along a particular avenue of approach through which enemy activity is expected to occur. Activity or lack of activity within an NAI will help to confirm or deny a particular enemy course of action.</rdfs:comment>
    <rdf:type rdf:resource="http://www.w3.org/2002/07/owl#Class"/>
  </rdf:Description>
  <rdf:Description rdf:about="#FACILITY-TYPE_Station,_general">
    <rdfs:subClassOf rdf:resource="jc3iedm_OBJECT-TYPE.owl#FACILITY-TYPE"/>
    <rdfs:label xml:lang="en">station, general</rdfs:label>
    <rdfs:comment xml:lang="en">A stopping place for the transfer of passengers and/or freight.</rdfs:comment>
    <rdf:type rdf:resource="http://www.w3.org/2002/07/owl#Class"/>
  </rdf:Description>
  <rdf:Description rdf:about="#SURFACE-VESSEL-TYPE_Aircraft_rescue_vessel">
    <rdfs:subClassOf rdf:resource="jc3iedm_OBJECT-TYPE.owl#SURFACE-VESSEL-TYPE"/>
    <rdfs:label xml:lang="en">aircraft rescue vessel</rdfs:label>
    <rdfs:comment xml:lang="en">Any ship equipped to rescue personnel trapped in a sunken aircraft. May also have facilities to salvage sunken aircraft.</rdfs:comment>
    <rdf:type rdf:resource="http://www.w3.org/2002/07/owl#Class"/>
  </rdf:Description>
  <rdf:Description rdf:about="#EXECUTIVE-MILITARY-ORGANISATION-TYPE_Logistics">
    <rdfs:subClassOf rdf:resource="jc3iedm_OBJECT-TYPE.owl#EXECUTIVE-MILITARY-ORGANISATION-TYPE"/>
    <rdfs:label xml:lang="en">logistics</rdfs:label>
    <rdfs:comment xml:lang="en">An EXECUTIVE-MILITARY-ORGANISATION-TYPE that provides management of logistics services.</rdfs:comment>
    <rdf:type rdf:resource="http://www.w3.org/2002/07/owl#Class"/>
  </rdf:Description>
  <rdf:Description rdf:about="#GROUP-ORGANISATION-TYPE_Displaced_person">
    <rdfs:subClassOf rdf:resource="jc3iedm_OBJECT-TYPE.owl#GROUP-ORGANISATION-TYPE"/>
    <rdfs:label xml:lang="en">displaced person</rdfs:label>
    <rdfs:comment xml:lang="en">A GROUP-ORGANISATION-TYPE that comprises persons removed from their home country by military or political pressure.</rdfs:comment>
    <rdf:type rdf:resource="http://www.w3.org/2002/07/owl#Class"/>
  </rdf:Description>
  <rdf:Description rdf:about="jc3iedm_OBJECT-TYPE.owl#ammunition-type-mine-maritime-firing-code">
    <rdf:type rdf:resource="http://www.w3.org/2002/07/owl#DatatypeProperty"/>
    <rdfs:domain rdf:resource="jc3iedm_OBJECT-TYPE.owl#AMMUNITION-TYPE"/>
    <rdfs:range rdf:resource="http://www.w3.org/2001/XMLSchema#string"/>
  </rdf:Description>
  <rdf:Description rdf:about="#ORGANISATION-TYPE_Headquarters">
    <rdfs:subClassOf rdf:resource="jc3iedm_OBJECT-TYPE.owl#ORGANISATION-TYPE"/>
    <rdfs:label xml:lang="en">headquarters</rdfs:label>
    <rdfs:comment xml:lang="en">The ORGANISATION-TYPE is a headquarters.</rdfs:comment>
    <rdf:type rdf:resource="http://www.w3.org/2002/07/owl#Class"/>
  </rdf:Description>
  <rdf:Description rdf:about="#SURFACE-VESSEL-TYPE_Patrol_boat,_hydrofoil">
    <rdfs:subClassOf rdf:resource="jc3iedm_OBJECT-TYPE.owl#SURFACE-VESSEL-TYPE"/>
    <rdfs:label xml:lang="en">patrol boat, hydrofoil</rdfs:label>
    <rdfs:comment xml:lang="en">Coastal patrol unit intended for a basically coastal guarding function. Includes any coastal patrol ship under 45 metres that cannot qualify as a Patrol ship, gun equipped, general in armament. May be unarmed and fitted with hydrofoils.</rdfs:comment>
    <rdf:type rdf:resource="http://www.w3.org/2002/07/owl#Class"/>
  </rdf:Description>
  <rdf:Description rdf:about="#FACILITY-TYPE_Electronic_installation,_surface_surveillance_jammer">
    <rdfs:subClassOf rdf:resource="jc3iedm_OBJECT-TYPE.owl#FACILITY-TYPE"/>
    <rdfs:label xml:lang="en">electronic installation, surface surveillance jammer</rdfs:label>
    <rdfs:comment xml:lang="en">A facility whose essential function is jamming to prevent or reduce the enemy's effective use of the electromagnetic spectrum for surface surveillance.</rdfs:comment>
    <rdf:type rdf:resource="http://www.w3.org/2002/07/owl#Class"/>
  </rdf:Description>
  <rdf:Description rdf:about="#SURFACE-VESSEL-TYPE_Harbour_utility_craft">
    <rdfs:subClassOf rdf:resource="jc3iedm_OBJECT-TYPE.owl#SURFACE-VESSEL-TYPE"/>
    <rdfs:label xml:lang="en">harbour utility craft</rdfs:label>
    <rdfs:comment xml:lang="en">Former landing craft, utility in size range 25-55 metres and full load of 120-500 tons with landing ramp/other landing facilities employed for general cargo transport purposes.</rdfs:comment>
    <rdf:type rdf:resource="http://www.w3.org/2002/07/owl#Class"/>
  </rdf:Description>
  <rdf:Description rdf:about="#CONTROL-FEATURE-TYPE_Search_area/reconnaissance_area">
    <rdfs:subClassOf rdf:resource="jc3iedm_OBJECT-TYPE.owl#CONTROL-FEATURE-TYPE"/>
    <rdfs:label xml:lang="en">search area/reconnaissance area</rdfs:label>
    <rdfs:comment xml:lang="en">Used to depict the area within which a unit or formation is responsible for reconnaissance. As shown, the points of the arrows indicate the width of that area but not its forward edge.</rdfs:comment>
    <rdf:type rdf:resource="http://www.w3.org/2002/07/owl#Class"/>
  </rdf:Description>
  <rdf:Description rdf:about="#FACILITY-TYPE_Detainee_collection_point">
    <rdfs:subClassOf rdf:resource="jc3iedm_OBJECT-TYPE.owl#FACILITY-TYPE"/>
    <rdfs:label xml:lang="en">detainee collection point</rdfs:label>
    <rdfs:comment xml:lang="en">A facility where detainees are assembled for classification, sorting or further movement to other facilities or installations.</rdfs:comment>
    <rdf:type rdf:resource="http://www.w3.org/2002/07/owl#Class"/>
  </rdf:Description>
  <rdf:Description rdf:about="#SURFACE-VESSEL-TYPE_Battleship,_general">
    <rdfs:subClassOf rdf:resource="jc3iedm_OBJECT-TYPE.owl#SURFACE-VESSEL-TYPE"/>
    <rdfs:label xml:lang="en">battleship, general</rdfs:label>
    <rdfs:comment xml:lang="en">Capital surface ship designed for surface action with a reasonable compromise between speed, protection and armament that may include guided missiles. A very large, heavily armoured vessel.</rdfs:comment>
    <rdf:type rdf:resource="http://www.w3.org/2002/07/owl#Class"/>
  </rdf:Description>
  <rdf:Description rdf:about="#VEHICLE-TYPE_Not_otherwise_specified">
    <rdfs:subClassOf rdf:resource="jc3iedm_OBJECT-TYPE.owl#VEHICLE-TYPE"/>
    <rdfs:label xml:lang="en">not otherwise specified</rdfs:label>
    <rdfs:comment xml:lang="en">The appropriate value is not in the set of specified values.</rdfs:comment>
    <rdf:type rdf:resource="http://www.w3.org/2002/07/owl#Class"/>
  </rdf:Description>
  <rdf:Description rdf:about="jc3iedm_OBJECT-TYPE.owl#vessel-type-height-above-the-waterline-dimension">
    <rdf:type rdf:resource="http://www.w3.org/2002/07/owl#DatatypeProperty"/>
    <rdfs:domain rdf:resource="jc3iedm_OBJECT-TYPE.owl#VESSEL-TYPE"/>
  </rdf:Description>
  <rdf:Description rdf:about="#FACILITY-TYPE_Depot,_ammunition">
    <rdfs:subClassOf rdf:resource="jc3iedm_OBJECT-TYPE.owl#FACILITY-TYPE"/>
    <rdfs:label xml:lang="en">depot, ammunition</rdfs:label>
    <rdfs:comment xml:lang="en">An area used for the storage of ammunition.</rdfs:comment>
    <rdf:type rdf:resource="http://www.w3.org/2002/07/owl#Class"/>
  </rdf:Description>
  <rdf:Description rdf:about="#SURFACE-VESSEL-TYPE_Barracks_craft">
    <rdfs:subClassOf rdf:resource="jc3iedm_OBJECT-TYPE.owl#SURFACE-VESSEL-TYPE"/>
    <rdfs:label xml:lang="en">barracks craft</rdfs:label>
    <rdfs:comment xml:lang="en">Ship of at least 120 metres employed to transport troops, their supplies and equipment but also with capability of providing barrack facilities.</rdfs:comment>
    <rdf:type rdf:resource="http://www.w3.org/2002/07/owl#Class"/>
  </rdf:Description>
  <rdf:Description rdf:about="#SURFACE-VESSEL-TYPE_Patrol_combatant,_guided_missile_(Motor_gunboat)">
    <rdfs:subClassOf rdf:resource="jc3iedm_OBJECT-TYPE.owl#SURFACE-VESSEL-TYPE"/>
    <rdfs:label xml:lang="en">patrol combatant, guided missile (motor gunboat)</rdfs:label>
    <rdfs:comment xml:lang="en">Patrol, blockade and surveillance ship in range 45-85 metres overall. Designed to operate in other than open ocean areas. Has special mission of attacking hostile ships. Must have at least 76mm main armament and is fitted with guns and other than force guided missile systems. Also known as motor gunboat.</rdfs:comment>
    <rdf:type rdf:resource="http://www.w3.org/2002/07/owl#Class"/>
  </rdf:Description>
  <rdf:Description rdf:about="jc3iedm_OBJECT-TYPE.owl#military-obstacle-type-category-code">
    <rdf:type rdf:resource="http://www.w3.org/2002/07/owl#DatatypeProperty"/>
    <rdfs:domain rdf:resource="jc3iedm_OBJECT-TYPE.owl#MILITARY-OBSTACLE-TYPE"/>
    <rdfs:range rdf:resource="http://www.w3.org/2001/XMLSchema#string"/>
  </rdf:Description>
  <rdf:Description rdf:about="#MARITIME-EQUIPMENT-TYPE_Sonar,_maritime">
    <rdfs:subClassOf rdf:resource="jc3iedm_OBJECT-TYPE.owl#MARITIME-EQUIPMENT-TYPE"/>
    <rdfs:label xml:lang="en">sonar, maritime</rdfs:label>
    <rdfs:comment xml:lang="en">An acoustic device used primarily for the detection and location of underwater objects.</rdfs:comment>
    <rdf:type rdf:resource="http://www.w3.org/2002/07/owl#Class"/>
  </rdf:Description>
  <rdf:Description rdf:about="#FACILITY-TYPE_Petrochemical_refinery">
    <rdfs:subClassOf rdf:resource="jc3iedm_OBJECT-TYPE.owl#FACILITY-TYPE"/>
    <rdfs:label xml:lang="en">petrochemical refinery</rdfs:label>
    <rdfs:comment xml:lang="en">Installations for refining crude oil and/or intermediate petroleum products or for refining synthetic petroleum.</rdfs:comment>
    <rdf:type rdf:resource="http://www.w3.org/2002/07/owl#Class"/>
  </rdf:Description>
  <rdf:Description rdf:about="#VEHICLE-TYPE_General_purpose">
    <rdfs:subClassOf rdf:resource="jc3iedm_OBJECT-TYPE.owl#VEHICLE-TYPE"/>
    <rdfs:label xml:lang="en">general purpose</rdfs:label>
    <rdfs:comment xml:lang="en">A vehicle designed for multiple uses.</rdfs:comment>
    <rdf:type rdf:resource="http://www.w3.org/2002/07/owl#Class"/>
  </rdf:Description>
  <rdf:Description rdf:about="#ORGANISATION-TYPE_Wing_operations_centre">
    <rdfs:subClassOf rdf:resource="jc3iedm_OBJECT-TYPE.owl#ORGANISATION-TYPE"/>
    <rdfs:label xml:lang="en">wing operations centre</rdfs:label>
    <rdfs:comment xml:lang="en">No definition provided in ADatP-3 Baseline 13.1 FFIRN/FUD 1874/4.</rdfs:comment>
    <rdf:type rdf:resource="http://www.w3.org/2002/07/owl#Class"/>
  </rdf:Description>
  <rdf:Description rdf:about="#FACILITY-TYPE_Shop">
    <rdfs:subClassOf rdf:resource="jc3iedm_OBJECT-TYPE.owl#FACILITY-TYPE"/>
    <rdfs:label xml:lang="en">shop</rdfs:label>
    <rdfs:comment xml:lang="en">A small retail store or a speciality department in a large store.</rdfs:comment>
    <rdf:type rdf:resource="http://www.w3.org/2002/07/owl#Class"/>
  </rdf:Description>
  <rdf:Description rdf:about="#FACILITY-TYPE_Pier">
    <rdfs:subClassOf rdf:resource="jc3iedm_OBJECT-TYPE.owl#FACILITY-TYPE"/>
    <rdfs:label xml:lang="en">pier</rdfs:label>
    <rdfs:comment xml:lang="en">A solid structure of stone, or of earth faced with piles, extending into the sea or a tidal river to protect or partially enclose a harbour and form a landing place for vessels, or a breakwater.</rdfs:comment>
    <rdf:type rdf:resource="http://www.w3.org/2002/07/owl#Class"/>
  </rdf:Description>
  <rdf:Description rdf:about="#ORGANISATION-TYPE_Direct_air_support_centre,_airborne">
    <rdfs:subClassOf rdf:resource="jc3iedm_OBJECT-TYPE.owl#ORGANISATION-TYPE"/>
    <rdfs:label xml:lang="en">direct air support centre, airborne</rdfs:label>
    <rdfs:comment xml:lang="en">The ORGANISATION-TYPE that is the principal air control agency of the U.S. Marine air command and control system, operating in an airborne platform responsible for the direction and control of air operations directly supporting the ground combat element.</rdfs:comment>
    <rdf:type rdf:resource="http://www.w3.org/2002/07/owl#Class"/>
  </rdf:Description>
  <rdf:Description rdf:about="#RAILCAR-TYPE_Not_known">
    <rdfs:subClassOf rdf:resource="jc3iedm_OBJECT-TYPE.owl#RAILCAR-TYPE"/>
    <rdfs:label xml:lang="en">not known</rdfs:label>
    <rdfs:comment xml:lang="en">It is not possible to determine which value is most applicable.</rdfs:comment>
    <rdf:type rdf:resource="http://www.w3.org/2002/07/owl#Class"/>
  </rdf:Description>
  <rdf:Description rdf:about="#SURFACE-VESSEL-TYPE_Attack_boat,_guided_missile">
    <rdfs:subClassOf rdf:resource="jc3iedm_OBJECT-TYPE.owl#SURFACE-VESSEL-TYPE"/>
    <rdfs:label xml:lang="en">attack boat, guided missile</rdfs:label>
    <rdfs:comment xml:lang="en">High speed (35 knots - 65 km/hr) anti-surface ship patrol craft in size range 20 - 30 metres with torpedoes and with a force guided missile system.</rdfs:comment>
    <rdf:type rdf:resource="http://www.w3.org/2002/07/owl#Class"/>
  </rdf:Description>
  <rdf:Description rdf:about="#SURFACE-VESSEL-TYPE_Junk">
    <rdfs:subClassOf rdf:resource="jc3iedm_OBJECT-TYPE.owl#SURFACE-VESSEL-TYPE"/>
    <rdfs:label xml:lang="en">junk</rdfs:label>
    <rdfs:comment xml:lang="en">Sail/motor powered vessel, usually associated with China, of wooden construction designed with high bow and poop deck area. Usually used for transportation purposes.</rdfs:comment>
    <rdf:type rdf:resource="http://www.w3.org/2002/07/owl#Class"/>
  </rdf:Description>
  <rdf:Description rdf:about="#TASK-FORMATION-TYPE_Patrol">
    <rdfs:subClassOf rdf:resource="jc3iedm_OBJECT-TYPE.owl#TASK-FORMATION-TYPE"/>
    <rdfs:label xml:lang="en">patrol</rdfs:label>
    <rdfs:comment xml:lang="en">A TASK-FORMATION-TYPE that is a detachment of ground, sea, or air forces sent out for the purpose of gathering information or carrying out a destructive, harassing, mopping-up, or security mission.</rdfs:comment>
    <rdf:type rdf:resource="http://www.w3.org/2002/07/owl#Class"/>
  </rdf:Description>
  <rdf:Description rdf:about="#SURFACE-VESSEL-TYPE_Patrol_craft,_air_cushion,_fast">
    <rdfs:subClassOf rdf:resource="jc3iedm_OBJECT-TYPE.owl#SURFACE-VESSEL-TYPE"/>
    <rdfs:label xml:lang="en">patrol craft, air cushion, fast</rdfs:label>
    <rdfs:comment xml:lang="en">Vessel in size range 35-55 metres designed and fitted primarily for escort duties in ASW role capable of at least 35 knots - 65 km/hr and has either an air cushion or surface effect design.</rdfs:comment>
    <rdf:type rdf:resource="http://www.w3.org/2002/07/owl#Class"/>
  </rdf:Description>
  <rdf:Description rdf:about="#AMMUNITION-TYPE_Rocket/missile,_anti-tank">
    <rdfs:subClassOf rdf:resource="jc3iedm_OBJECT-TYPE.owl#AMMUNITION-TYPE"/>
    <rdfs:label xml:lang="en">rocket/missile, anti tank</rdfs:label>
    <rdfs:comment xml:lang="en">A powered projectile designed for use against tanks.</rdfs:comment>
    <rdf:type rdf:resource="http://www.w3.org/2002/07/owl#Class"/>
  </rdf:Description>
  <rdf:Description rdf:about="jc3iedm_OBJECT-TYPE.owl#MISCELLANEOUS-EQUIPMENT-TYPE">
    <rdf:type rdf:resource="http://www.w3.org/2002/07/owl#Class"/>
    <rdfs:label xml:lang="en">miscellaneous equipment type</rdfs:label>
    <rdfs:comment xml:lang="en">An EQUIPMENT-TYPE whose designed function does not fit in any other defined category.</rdfs:comment>
    <rdfs:subClassOf rdf:resource="jc3iedm_OBJECT-TYPE.owl#EQUIPMENT-TYPE"/>
  </rdf:Description>
  <rdf:Description rdf:about="#MARITIME-EQUIPMENT-TYPE_Kite,_depressor">
    <rdfs:subClassOf rdf:resource="jc3iedm_OBJECT-TYPE.owl#MARITIME-EQUIPMENT-TYPE"/>
    <rdfs:label xml:lang="en">kite, depressor</rdfs:label>
    <rdfs:comment xml:lang="en">A device which when towed submerges and planes at a predetermined depth without sideways displacement.</rdfs:comment>
    <rdf:type rdf:resource="http://www.w3.org/2002/07/owl#Class"/>
  </rdf:Description>
  <rdf:Description rdf:about="#SURFACE-VESSEL-TYPE_Assault_ship,_personnel">
    <rdfs:subClassOf rdf:resource="jc3iedm_OBJECT-TYPE.owl#SURFACE-VESSEL-TYPE"/>
    <rdfs:label xml:lang="en">assault ship, personnel</rdfs:label>
    <rdfs:comment xml:lang="en">Amphibious ship designed specifically to carry personnel.</rdfs:comment>
    <rdf:type rdf:resource="http://www.w3.org/2002/07/owl#Class"/>
  </rdf:Description>
  <rdf:Description rdf:about="#AMMUNITION-TYPE_Rocket/missile,_light">
    <rdfs:subClassOf rdf:resource="jc3iedm_OBJECT-TYPE.owl#AMMUNITION-TYPE"/>
    <rdfs:label xml:lang="en">rocket/missile, light</rdfs:label>
    <rdfs:comment xml:lang="en">A powered projectile designed for use by light launchers.</rdfs:comment>
    <rdf:type rdf:resource="http://www.w3.org/2002/07/owl#Class"/>
  </rdf:Description>
  <rdf:Description rdf:about="#SURFACE-VESSEL-TYPE_Missile_support_ship">
    <rdfs:subClassOf rdf:resource="jc3iedm_OBJECT-TYPE.owl#SURFACE-VESSEL-TYPE"/>
    <rdfs:label xml:lang="en">missile support ship</rdfs:label>
    <rdfs:comment xml:lang="en">Ship larger than 40 metres employed primarily to transport missiles.</rdfs:comment>
    <rdf:type rdf:resource="http://www.w3.org/2002/07/owl#Class"/>
  </rdf:Description>
  <rdf:Description rdf:about="#SURFACE-VESSEL-TYPE_Merchant_ship,_container,_self-sustained">
    <rdfs:subClassOf rdf:resource="jc3iedm_OBJECT-TYPE.owl#SURFACE-VESSEL-TYPE"/>
    <rdfs:label xml:lang="en">merchant ship, container, self sustained</rdfs:label>
    <rdfs:comment xml:lang="en">Non-naval ship designed to carry cargo in loadable and unloadable containers and equipped with its own handling equipment.</rdfs:comment>
    <rdf:type rdf:resource="http://www.w3.org/2002/07/owl#Class"/>
  </rdf:Description>
  <rdf:Description rdf:about="jc3iedm_OBJECT-TYPE.owl#unit-type-arm-specialisation-code">
    <rdf:type rdf:resource="http://www.w3.org/2002/07/owl#DatatypeProperty"/>
    <rdfs:domain rdf:resource="jc3iedm_OBJECT-TYPE.owl#UNIT-TYPE"/>
    <rdfs:range rdf:resource="http://www.w3.org/2001/XMLSchema#string"/>
  </rdf:Description>
  <rdf:Description rdf:about="#CONTROL-FEATURE-TYPE_Transit_corridor">
    <rdfs:subClassOf rdf:resource="jc3iedm_OBJECT-TYPE.owl#CONTROL-FEATURE-TYPE"/>
    <rdfs:label xml:lang="en">transit corridor</rdfs:label>
    <rdfs:comment xml:lang="en">Bi-directional corridor in the rear area. Air traffic services not normally provided.</rdfs:comment>
    <rdf:type rdf:resource="http://www.w3.org/2002/07/owl#Class"/>
  </rdf:Description>
  <rdf:Description rdf:about="#SURFACE-VESSEL-TYPE_Minehunter,_auxiliary">
    <rdfs:subClassOf rdf:resource="jc3iedm_OBJECT-TYPE.owl#SURFACE-VESSEL-TYPE"/>
    <rdfs:label xml:lang="en">minehunter, auxiliary</rdfs:label>
    <rdfs:comment xml:lang="en">Any seagoing ship not designed as a mine hunter but converted to such use.</rdfs:comment>
    <rdf:type rdf:resource="http://www.w3.org/2002/07/owl#Class"/>
  </rdf:Description>
  <rdf:Description rdf:about="#SURFACE-VESSEL-TYPE_Cable/netlaying_ship,_small">
    <rdfs:subClassOf rdf:resource="jc3iedm_OBJECT-TYPE.owl#SURFACE-VESSEL-TYPE"/>
    <rdfs:label xml:lang="en">cable/netlaying ship, small</rdfs:label>
    <rdfs:comment xml:lang="en">Smaller ship equipped for cable or netlaying.</rdfs:comment>
    <rdf:type rdf:resource="http://www.w3.org/2002/07/owl#Class"/>
  </rdf:Description>
  <rdf:Description rdf:about="#TASK-FORMATION-TYPE_Amphibious_task_force">
    <rdfs:subClassOf rdf:resource="jc3iedm_OBJECT-TYPE.owl#TASK-FORMATION-TYPE"/>
    <rdfs:label xml:lang="en">amphibious task force</rdfs:label>
    <rdfs:comment xml:lang="en">A temporary grouping of units, under one commander, formed for the purpose of carrying out a specific amphibious operation or mission.</rdfs:comment>
    <rdf:type rdf:resource="http://www.w3.org/2002/07/owl#Class"/>
  </rdf:Description>
  <rdf:Description rdf:about="#MISCELLANEOUS-EQUIPMENT-TYPE_Flag">
    <rdfs:subClassOf rdf:resource="jc3iedm_OBJECT-TYPE.owl#MISCELLANEOUS-EQUIPMENT-TYPE"/>
    <rdfs:label xml:lang="en">flag</rdfs:label>
    <rdfs:comment xml:lang="en">A piece of bunting or other material usually oblong or square attached by one edge to a staff or pole and fixed to a float, mine, buoy in order to mark its location.</rdfs:comment>
    <rdf:type rdf:resource="http://www.w3.org/2002/07/owl#Class"/>
  </rdf:Description>
  <rdf:Description rdf:about="#FACILITY-TYPE_Military_materiel_facility,_ship_construction">
    <rdfs:subClassOf rdf:resource="jc3iedm_OBJECT-TYPE.owl#FACILITY-TYPE"/>
    <rdfs:label xml:lang="en">military materiel facility, ship construction</rdfs:label>
    <rdfs:comment xml:lang="en">A facility used as for ship construction.</rdfs:comment>
    <rdf:type rdf:resource="http://www.w3.org/2002/07/owl#Class"/>
  </rdf:Description>
  <rdf:Description rdf:about="#SURFACE-VESSEL-TYPE_Patrol_combatant,_guided_missile">
    <rdfs:subClassOf rdf:resource="jc3iedm_OBJECT-TYPE.owl#SURFACE-VESSEL-TYPE"/>
    <rdfs:label xml:lang="en">patrol combatant, guided missile</rdfs:label>
    <rdfs:comment xml:lang="en">Patrol, blockade and surveillance ship in range 45-85 metres overall. Designed to operate in other than open ocean areas. Has special mission of attacking hostile ships. Must have at least 76mm main armament and is fitted with one or more force guided missile systems.</rdfs:comment>
    <rdf:type rdf:resource="http://www.w3.org/2002/07/owl#Class"/>
  </rdf:Description>
  <rdf:Description rdf:about="#MARITIME-EQUIPMENT-TYPE_Maritime_mine_disposal_vehicle">
    <rdfs:subClassOf rdf:resource="jc3iedm_OBJECT-TYPE.owl#MARITIME-EQUIPMENT-TYPE"/>
    <rdfs:label xml:lang="en">maritime mine disposal vehicle</rdfs:label>
    <rdfs:comment xml:lang="en">ROV used to destroy mines normally armed with MDC mine disposal charge.</rdfs:comment>
    <rdf:type rdf:resource="http://www.w3.org/2002/07/owl#Class"/>
  </rdf:Description>
  <rdf:Description rdf:about="jc3iedm_OBJECT-TYPE.owl#PRIVATE-SECTOR-ORGANISATION-TYPE">
    <rdf:type rdf:resource="http://www.w3.org/2002/07/owl#Class"/>
    <rdfs:label xml:lang="en">private sector organisation type</rdfs:label>
    <rdfs:comment xml:lang="en">An ORGANISATION-TYPE that is a non-government organisation and is constituted for business, commerce, manufacturing, trade, relief or philanthropy.</rdfs:comment>
    <rdfs:subClassOf rdf:resource="jc3iedm_OBJECT-TYPE.owl#ORGANISATION-TYPE"/>
  </rdf:Description>
  <rdf:Description rdf:about="#CONTROL-FEATURE-TYPE_Safe_area_for_evasion">
    <rdfs:subClassOf rdf:resource="jc3iedm_OBJECT-TYPE.owl#CONTROL-FEATURE-TYPE"/>
    <rdfs:label xml:lang="en">safe area for evasion</rdfs:label>
    <rdfs:comment xml:lang="en">Designated area in hostile territory that offers the evader or escapee a reasonable chance of avoiding capture and of surviving until he can be evacuated.</rdfs:comment>
    <rdf:type rdf:resource="http://www.w3.org/2002/07/owl#Class"/>
  </rdf:Description>
  <rdf:Description rdf:about="#CONTROL-FEATURE-TYPE_Rear_boundary_of_the_forward_area">
    <rdfs:subClassOf rdf:resource="jc3iedm_OBJECT-TYPE.owl#CONTROL-FEATURE-TYPE"/>
    <rdfs:label xml:lang="en">rear boundary of the forward area</rdfs:label>
    <rdfs:comment xml:lang="en">A line delineating the rear of an area in proximity to combat.</rdfs:comment>
    <rdf:type rdf:resource="http://www.w3.org/2002/07/owl#Class"/>
  </rdf:Description>
  <rdf:Description rdf:about="#CONTROL-FEATURE-TYPE_Forward_arming_and_refuelling_point">
    <rdfs:subClassOf rdf:resource="jc3iedm_OBJECT-TYPE.owl#CONTROL-FEATURE-TYPE"/>
    <rdfs:label xml:lang="en">forward arming and refuelling point</rdfs:label>
    <rdfs:comment xml:lang="en">A point designated by a deployed aviation commander that permits combat aircraft to rapidly refuel and rearm simultaneously.</rdfs:comment>
    <rdf:type rdf:resource="http://www.w3.org/2002/07/owl#Class"/>
  </rdf:Description>
  <rdf:Description rdf:about="#SURFACE-VESSEL-TYPE_Stores_ship_(naval)">
    <rdfs:subClassOf rdf:resource="jc3iedm_OBJECT-TYPE.owl#SURFACE-VESSEL-TYPE"/>
    <rdfs:label xml:lang="en">stores ship (naval)</rdfs:label>
    <rdfs:comment xml:lang="en">Ship 60 metres or more capable of underway replenishment of ships with refrigerated and dry provisions. May carry ammunition and POL but main emphasis is on dry provisions.</rdfs:comment>
    <rdf:type rdf:resource="http://www.w3.org/2002/07/owl#Class"/>
  </rdf:Description>
  <rdf:Description rdf:about="#SURFACE-VESSEL-TYPE_Patrol_combatant,_hovercraft,_guided_missile">
    <rdfs:subClassOf rdf:resource="jc3iedm_OBJECT-TYPE.owl#SURFACE-VESSEL-TYPE"/>
    <rdfs:label xml:lang="en">patrol combatant, hovercraft, guided missile</rdfs:label>
    <rdfs:comment xml:lang="en">A high-speed patrol hovercraft, which can conduct surveillance screening and special operations and is operated by naval or marine forces and is fitted with other than force guided missile systems.</rdfs:comment>
    <rdf:type rdf:resource="http://www.w3.org/2002/07/owl#Class"/>
  </rdf:Description>
  <rdf:Description rdf:about="#FACILITY-TYPE_Trail">
    <rdfs:subClassOf rdf:resource="jc3iedm_OBJECT-TYPE.owl#FACILITY-TYPE"/>
    <rdfs:label xml:lang="en">trail</rdfs:label>
    <rdfs:comment xml:lang="en">A beaten path, especially through a wild region.</rdfs:comment>
    <rdf:type rdf:resource="http://www.w3.org/2002/07/owl#Class"/>
  </rdf:Description>
  <rdf:Description rdf:about="#CONTROL-FEATURE-TYPE_Reconnaissance_and_interdiction_planning_line">
    <rdfs:subClassOf rdf:resource="jc3iedm_OBJECT-TYPE.owl#CONTROL-FEATURE-TYPE"/>
    <rdfs:label xml:lang="en">reconnaissance and interdiction planning line</rdfs:label>
    <rdfs:comment xml:lang="en">A CONTROL-FEATURE-TYPE with a line location to divide responsibility for the nomination of ground targets. Short of the RIPL the ground commander has this responsibility for nominating targets that have a direct bearing on the land battle. Beyond this, the targeting authority lies with the Air Commander.</rdfs:comment>
    <rdf:type rdf:resource="http://www.w3.org/2002/07/owl#Class"/>
  </rdf:Description>
  <rdf:Description rdf:about="#SURFACE-VESSEL-TYPE_Aircraft_carrier,_guided_missile">
    <rdfs:subClassOf rdf:resource="jc3iedm_OBJECT-TYPE.owl#SURFACE-VESSEL-TYPE"/>
    <rdfs:label xml:lang="en">aircraft carrier, guided missile</rdfs:label>
    <rdfs:comment xml:lang="en">Designator for multi-role aircraft carriers, fitted with one or more force guided missile systems.</rdfs:comment>
    <rdf:type rdf:resource="http://www.w3.org/2002/07/owl#Class"/>
  </rdf:Description>
  <rdf:Description rdf:about="#SURFACE-VESSEL-TYPE_Dry_dock_floating,_closed,_large">
    <rdfs:subClassOf rdf:resource="jc3iedm_OBJECT-TYPE.owl#SURFACE-VESSEL-TYPE"/>
    <rdfs:label xml:lang="en">dry dock floating, closed, large</rdfs:label>
    <rdfs:comment xml:lang="en">Non-self-propelled dry dock, closed bow and stern over 200 metres.</rdfs:comment>
    <rdf:type rdf:resource="http://www.w3.org/2002/07/owl#Class"/>
  </rdf:Description>
  <rdf:Description rdf:about="#VEHICLE-TYPE_Cross-country_truck">
    <rdfs:subClassOf rdf:resource="jc3iedm_OBJECT-TYPE.owl#VEHICLE-TYPE"/>
    <rdfs:label xml:lang="en">cross country truck</rdfs:label>
    <rdfs:comment xml:lang="en">An automotive vehicle designed to be used off road for transporting loads.</rdfs:comment>
    <rdf:type rdf:resource="http://www.w3.org/2002/07/owl#Class"/>
  </rdf:Description>
  <rdf:Description rdf:about="#CONTROL-FEATURE-TYPE_Limit_of_advance">
    <rdfs:subClassOf rdf:resource="jc3iedm_OBJECT-TYPE.owl#CONTROL-FEATURE-TYPE"/>
    <rdfs:label xml:lang="en">limit of advance</rdfs:label>
    <rdfs:comment xml:lang="en">An easily recognized terrain feature beyond which attacking elements will not advance.</rdfs:comment>
    <rdf:type rdf:resource="http://www.w3.org/2002/07/owl#Class"/>
  </rdf:Description>
  <rdf:Description rdf:about="#MARITIME-EQUIPMENT-TYPE_Obstructors,_mine">
    <rdfs:subClassOf rdf:resource="jc3iedm_OBJECT-TYPE.owl#MARITIME-EQUIPMENT-TYPE"/>
    <rdfs:label xml:lang="en">obstructors, mine</rdfs:label>
    <rdfs:comment xml:lang="en">A device laid with the sole object of obstructing or damaging mechanical minesweeping equipment.</rdfs:comment>
    <rdf:type rdf:resource="http://www.w3.org/2002/07/owl#Class"/>
  </rdf:Description>
  <rdf:Description rdf:about="jc3iedm_OBJECT-TYPE.owl#organisation-type-command-function-indicator-code">
    <rdf:type rdf:resource="http://www.w3.org/2002/07/owl#DatatypeProperty"/>
    <rdfs:domain rdf:resource="jc3iedm_OBJECT-TYPE.owl#ORGANISATION-TYPE"/>
    <rdfs:range rdf:resource="http://www.w3.org/2001/XMLSchema#string"/>
  </rdf:Description>
  <rdf:Description rdf:about="#EXECUTIVE-MILITARY-ORGANISATION-TYPE_Transportation">
    <rdfs:subClassOf rdf:resource="jc3iedm_OBJECT-TYPE.owl#EXECUTIVE-MILITARY-ORGANISATION-TYPE"/>
    <rdfs:label xml:lang="en">transportation</rdfs:label>
    <rdfs:comment xml:lang="en">An EXECUTIVE-MILITARY-ORGANISATION-TYPE that provides management of transportation services.</rdfs:comment>
    <rdf:type rdf:resource="http://www.w3.org/2002/07/owl#Class"/>
  </rdf:Description>
  <rdf:Description rdf:about="jc3iedm_OBJECT-TYPE.owl#surface-vessel-type-category-code">
    <rdf:type rdf:resource="http://www.w3.org/2002/07/owl#DatatypeProperty"/>
    <rdfs:domain rdf:resource="jc3iedm_OBJECT-TYPE.owl#SURFACE-VESSEL-TYPE"/>
    <rdfs:range rdf:resource="http://www.w3.org/2001/XMLSchema#string"/>
  </rdf:Description>
  <rdf:Description rdf:about="#SURFACE-VESSEL-TYPE_Patrol_boat,_river/roadstead">
    <rdfs:subClassOf rdf:resource="jc3iedm_OBJECT-TYPE.owl#SURFACE-VESSEL-TYPE"/>
    <rdfs:label xml:lang="en">patrol boat, river/roadstead</rdfs:label>
    <rdfs:comment xml:lang="en">Lightly armed unit generally suitable by design only for operations in sheltered waters, such as rivers and roadsteads.</rdfs:comment>
    <rdf:type rdf:resource="http://www.w3.org/2002/07/owl#Class"/>
  </rdf:Description>
  <rdf:Description rdf:about="#FACILITY-TYPE_Motorway">
    <rdfs:subClassOf rdf:resource="jc3iedm_OBJECT-TYPE.owl#FACILITY-TYPE"/>
    <rdfs:label xml:lang="en">motorway</rdfs:label>
    <rdfs:comment xml:lang="en">An open, broad way, often with shoulders and barriers, maintained for vehicular use.</rdfs:comment>
    <rdf:type rdf:resource="http://www.w3.org/2002/07/owl#Class"/>
  </rdf:Description>
  <rdf:Description rdf:about="#SURFACE-VESSEL-TYPE_Merchant_ship,_tug,_ocean-going">
    <rdfs:subClassOf rdf:resource="jc3iedm_OBJECT-TYPE.owl#SURFACE-VESSEL-TYPE"/>
    <rdfs:label xml:lang="en">merchant ship, tug, ocean going</rdfs:label>
    <rdfs:comment xml:lang="en">Non-naval sea-going tug with horsepower of 1000 or more, length usually over 60 metres.</rdfs:comment>
    <rdf:type rdf:resource="http://www.w3.org/2002/07/owl#Class"/>
  </rdf:Description>
  <rdf:Description rdf:about="#SURFACE-VESSEL-TYPE_Barge,_pontoon_storage">
    <rdfs:subClassOf rdf:resource="jc3iedm_OBJECT-TYPE.owl#SURFACE-VESSEL-TYPE"/>
    <rdfs:label xml:lang="en">barge, pontoon storage</rdfs:label>
    <rdfs:comment xml:lang="en">Craft used to stow pontoons.</rdfs:comment>
    <rdf:type rdf:resource="http://www.w3.org/2002/07/owl#Class"/>
  </rdf:Description>
  <rdf:Description rdf:about="#SURFACE-VESSEL-TYPE_Dry_dock_floating,_open,_small">
    <rdfs:subClassOf rdf:resource="jc3iedm_OBJECT-TYPE.owl#SURFACE-VESSEL-TYPE"/>
    <rdfs:label xml:lang="en">dry dock floating, open, small</rdfs:label>
    <rdfs:comment xml:lang="en">Non-self-propelled open-ended dry dock less than 60 metres.</rdfs:comment>
    <rdf:type rdf:resource="http://www.w3.org/2002/07/owl#Class"/>
  </rdf:Description>
  <rdf:Description rdf:about="#SURFACE-VESSEL-TYPE_Repair_ship">
    <rdfs:subClassOf rdf:resource="jc3iedm_OBJECT-TYPE.owl#SURFACE-VESSEL-TYPE"/>
    <rdfs:label xml:lang="en">repair ship</rdfs:label>
    <rdfs:comment xml:lang="en">Ship of at least 120 metres or more employed as a mobile repair facility providing limited support to various types of ships. Not a lifting ship. Repair primary function, support secondary.</rdfs:comment>
    <rdf:type rdf:resource="http://www.w3.org/2002/07/owl#Class"/>
  </rdf:Description>
  <rdf:Description rdf:about="#ROUTE-TYPE_Not_otherwise_specified">
    <rdfs:subClassOf rdf:resource="jc3iedm_OBJECT-TYPE.owl#ROUTE-TYPE"/>
    <rdfs:label xml:lang="en">not otherwise specified</rdfs:label>
    <rdfs:comment xml:lang="en">The appropriate value is not in the set of specified values.</rdfs:comment>
    <rdf:type rdf:resource="http://www.w3.org/2002/07/owl#Class"/>
  </rdf:Description>
  <rdf:Description rdf:about="#MISCELLANEOUS-EQUIPMENT-TYPE_Megaphone">
    <rdfs:subClassOf rdf:resource="jc3iedm_OBJECT-TYPE.owl#MISCELLANEOUS-EQUIPMENT-TYPE"/>
    <rdfs:label xml:lang="en">megaphone</rdfs:label>
    <rdfs:comment xml:lang="en">A non-electronic instrument for carrying sound a long distance.</rdfs:comment>
    <rdf:type rdf:resource="http://www.w3.org/2002/07/owl#Class"/>
  </rdf:Description>
  <rdf:Description rdf:about="#CONTROL-FEATURE-TYPE_Fire_umbrella">
    <rdfs:subClassOf rdf:resource="jc3iedm_OBJECT-TYPE.owl#CONTROL-FEATURE-TYPE"/>
    <rdfs:label xml:lang="en">fire umbrella</rdfs:label>
    <rdfs:comment xml:lang="en">The airspace over a naval force at sea within the fire of ships' anti-aircraft weapons can endanger aircraft, and within which special procedures are established for identification and operation of friendly aircraft.</rdfs:comment>
    <rdf:type rdf:resource="http://www.w3.org/2002/07/owl#Class"/>
  </rdf:Description>
  <rdf:Description rdf:about="#CONTROL-FEATURE-TYPE_Hide">
    <rdfs:subClassOf rdf:resource="jc3iedm_OBJECT-TYPE.owl#CONTROL-FEATURE-TYPE"/>
    <rdfs:label xml:lang="en">hide</rdfs:label>
    <rdfs:comment xml:lang="en">An area in which a force conceals itself before operations or before moving into battle position.</rdfs:comment>
    <rdf:type rdf:resource="http://www.w3.org/2002/07/owl#Class"/>
  </rdf:Description>
  <rdf:Description rdf:about="#SURFACE-VESSEL-TYPE_Barge,_non-self_propelled">
    <rdfs:subClassOf rdf:resource="jc3iedm_OBJECT-TYPE.owl#SURFACE-VESSEL-TYPE"/>
    <rdfs:label xml:lang="en">barge, non self propelled</rdfs:label>
    <rdfs:comment xml:lang="en">A vessel that has no power of its own and must be towed.</rdfs:comment>
    <rdf:type rdf:resource="http://www.w3.org/2002/07/owl#Class"/>
  </rdf:Description>
  <rdf:Description rdf:about="#ROUTE-TYPE_Egress_route">
    <rdfs:subClassOf rdf:resource="jc3iedm_OBJECT-TYPE.owl#ROUTE-TYPE"/>
    <rdfs:label xml:lang="en">egress route</rdfs:label>
    <rdfs:comment xml:lang="en">An outbound route from a specific area or target.</rdfs:comment>
    <rdf:type rdf:resource="http://www.w3.org/2002/07/owl#Class"/>
  </rdf:Description>
  <rdf:Description rdf:about="#CONTROL-FEATURE-TYPE_Area_of_coverage">
    <rdfs:subClassOf rdf:resource="jc3iedm_OBJECT-TYPE.owl#CONTROL-FEATURE-TYPE"/>
    <rdfs:label xml:lang="en">area of coverage</rdfs:label>
    <rdfs:comment xml:lang="en">The summation of geographical areas under surveillance or protected by supporting fire.</rdfs:comment>
    <rdf:type rdf:resource="http://www.w3.org/2002/07/owl#Class"/>
  </rdf:Description>
  <rdf:Description rdf:about="#SURFACE-VESSEL-TYPE_Minesweeper,_inshore,_air_cushion">
    <rdfs:subClassOf rdf:resource="jc3iedm_OBJECT-TYPE.owl#SURFACE-VESSEL-TYPE"/>
    <rdfs:label xml:lang="en">minesweeper, inshore, air cushion</rdfs:label>
    <rdfs:comment xml:lang="en">Minesweeper between 20-40 metres. Intended and equipped for inshore minesweeping with an air cushion or surface effect design.</rdfs:comment>
    <rdf:type rdf:resource="http://www.w3.org/2002/07/owl#Class"/>
  </rdf:Description>
  <rdf:Description rdf:about="#SURFACE-VESSEL-TYPE_Assault_ship,_tank">
    <rdfs:subClassOf rdf:resource="jc3iedm_OBJECT-TYPE.owl#SURFACE-VESSEL-TYPE"/>
    <rdfs:label xml:lang="en">assault ship, tank</rdfs:label>
    <rdfs:comment xml:lang="en">Assault ship optimised for carrying tanks.</rdfs:comment>
    <rdf:type rdf:resource="http://www.w3.org/2002/07/owl#Class"/>
  </rdf:Description>
  <rdf:Description rdf:about="#SURFACE-VESSEL-TYPE_Patrol_combatant,_hovercraft,_mine-warfare">
    <rdfs:subClassOf rdf:resource="jc3iedm_OBJECT-TYPE.owl#SURFACE-VESSEL-TYPE"/>
    <rdfs:label xml:lang="en">patrol combatant, hovercraft, mine warfare</rdfs:label>
    <rdfs:comment xml:lang="en">A high-speed patrol hovercraft which is used primarily in minewarfare.</rdfs:comment>
    <rdf:type rdf:resource="http://www.w3.org/2002/07/owl#Class"/>
  </rdf:Description>
  <rdf:Description rdf:about="#FACILITY-TYPE_Camp">
    <rdfs:subClassOf rdf:resource="jc3iedm_OBJECT-TYPE.owl#FACILITY-TYPE"/>
    <rdfs:label xml:lang="en">camp</rdfs:label>
    <rdfs:comment xml:lang="en">An accommodation based upon a number of tents or huts.</rdfs:comment>
    <rdf:type rdf:resource="http://www.w3.org/2002/07/owl#Class"/>
  </rdf:Description>
  <rdf:Description rdf:about="#CONTROL-FEATURE-TYPE_General_area">
    <rdfs:subClassOf rdf:resource="jc3iedm_OBJECT-TYPE.owl#CONTROL-FEATURE-TYPE"/>
    <rdfs:label xml:lang="en">general area</rdfs:label>
    <rdfs:comment xml:lang="en">A CONTROL-FEATURE-TYPE that identifies an area defined by a higher commander within which the subordinate must accomplish his mission and protect his forces. It applies to both land and naval forces.</rdfs:comment>
    <rdf:type rdf:resource="http://www.w3.org/2002/07/owl#Class"/>
  </rdf:Description>
  <rdf:Description rdf:about="#CONTROL-FEATURE-TYPE_Exit_point">
    <rdfs:subClassOf rdf:resource="jc3iedm_OBJECT-TYPE.owl#CONTROL-FEATURE-TYPE"/>
    <rdfs:label xml:lang="en">exit point</rdfs:label>
    <rdfs:comment xml:lang="en">A point designated for use by vehicles or personnel in leaving an area, line or volume.</rdfs:comment>
    <rdf:type rdf:resource="http://www.w3.org/2002/07/owl#Class"/>
  </rdf:Description>
  <rdf:Description rdf:about="#SURFACE-VESSEL-TYPE_Attack_boat,_guided_missile,_hydrofoil">
    <rdfs:subClassOf rdf:resource="jc3iedm_OBJECT-TYPE.owl#SURFACE-VESSEL-TYPE"/>
    <rdfs:label xml:lang="en">attack boat, guided missile, hydrofoil</rdfs:label>
    <rdfs:comment xml:lang="en">High speed (35 knots - 65 km/hr) anti-surface ship patrol craft in size range 20 - 30 metres fitted with torpedoes and with force guided missile system and hydrofoils.</rdfs:comment>
    <rdf:type rdf:resource="http://www.w3.org/2002/07/owl#Class"/>
  </rdf:Description>
  <rdf:Description rdf:about="#CONTROL-FEATURE-TYPE_Main_battle_area">
    <rdfs:subClassOf rdf:resource="jc3iedm_OBJECT-TYPE.owl#CONTROL-FEATURE-TYPE"/>
    <rdfs:label xml:lang="en">main battle area</rdfs:label>
    <rdfs:comment xml:lang="en">That portion of the battlespace in which the decisive battle is fought to defeat the enemy. For any particular command, the main battle area extends rearward from the forward edge of the battle area to the rear boundary of the command's subordinate units.</rdfs:comment>
    <rdf:type rdf:resource="http://www.w3.org/2002/07/owl#Class"/>
  </rdf:Description>
  <rdf:Description rdf:about="#SURFACE-VESSEL-TYPE_Auxiliary,_miscellaneous">
    <rdfs:subClassOf rdf:resource="jc3iedm_OBJECT-TYPE.owl#SURFACE-VESSEL-TYPE"/>
    <rdfs:label xml:lang="en">auxiliary, miscellaneous</rdfs:label>
    <rdfs:comment xml:lang="en">Ship 40 metres or more employed in general or multi-purpose functions of support, training, R&amp;D, or a testing nature.</rdfs:comment>
    <rdf:type rdf:resource="http://www.w3.org/2002/07/owl#Class"/>
  </rdf:Description>
  <rdf:Description rdf:about="jc3iedm_OBJECT-TYPE.owl#weapon-type-calibre-text">
    <rdf:type rdf:resource="http://www.w3.org/2002/07/owl#DatatypeProperty"/>
    <rdfs:domain rdf:resource="jc3iedm_OBJECT-TYPE.owl#WEAPON-TYPE"/>
    <rdfs:range rdf:resource="http://www.w3.org/2001/XMLSchema#string"/>
  </rdf:Description>
  <rdf:Description rdf:about="#FACILITY-TYPE_POL_point">
    <rdfs:subClassOf rdf:resource="jc3iedm_OBJECT-TYPE.owl#FACILITY-TYPE"/>
    <rdfs:label xml:lang="en">pol point</rdfs:label>
    <rdfs:comment xml:lang="en">A facility for the distribution of petroleum and associated products.</rdfs:comment>
    <rdf:type rdf:resource="http://www.w3.org/2002/07/owl#Class"/>
  </rdf:Description>
  <rdf:Description rdf:about="#SURFACE-VESSEL-TYPE_Yacht">
    <rdfs:subClassOf rdf:resource="jc3iedm_OBJECT-TYPE.owl#SURFACE-VESSEL-TYPE"/>
    <rdfs:label xml:lang="en">yacht</rdfs:label>
    <rdfs:comment xml:lang="en">Vessel with one or more sails as primary source of power.</rdfs:comment>
    <rdf:type rdf:resource="http://www.w3.org/2002/07/owl#Class"/>
  </rdf:Description>
  <rdf:Description rdf:about="#MILITARY-OBSTACLE-TYPE_Wire_obstacle,_single_concertina">
    <rdfs:subClassOf rdf:resource="jc3iedm_OBJECT-TYPE.owl#MILITARY-OBSTACLE-TYPE"/>
    <rdfs:label xml:lang="en">wire obstacle, single concertina</rdfs:label>
    <rdfs:comment xml:lang="en">No definition provided in APP-6A.</rdfs:comment>
    <rdf:type rdf:resource="http://www.w3.org/2002/07/owl#Class"/>
  </rdf:Description>
  <rdf:Description rdf:about="#FACILITY-TYPE_Depot,_medical">
    <rdfs:subClassOf rdf:resource="jc3iedm_OBJECT-TYPE.owl#FACILITY-TYPE"/>
    <rdfs:label xml:lang="en">depot, medical</rdfs:label>
    <rdfs:comment xml:lang="en">An area used for the storage of medical supplies.</rdfs:comment>
    <rdf:type rdf:resource="http://www.w3.org/2002/07/owl#Class"/>
  </rdf:Description>
  <rdf:Description rdf:about="#CONSUMABLE-MATERIEL-TYPE_Improvised_explosive_device">
    <rdfs:subClassOf rdf:resource="jc3iedm_OBJECT-TYPE.owl#CONSUMABLE-MATERIEL-TYPE"/>
    <rdfs:label xml:lang="en">improvised explosive device</rdfs:label>
    <rdfs:comment xml:lang="en">A device placed or fabricated in an improvised manner incorporating destructive, lethal, noxious, pyrotechnic or incendiary chemicals and designed to destroy, incapacitate, harass or distract.</rdfs:comment>
    <rdf:type rdf:resource="http://www.w3.org/2002/07/owl#Class"/>
  </rdf:Description>
  <rdf:Description rdf:about="#FACILITY-TYPE_Port">
    <rdfs:subClassOf rdf:resource="jc3iedm_OBJECT-TYPE.owl#FACILITY-TYPE"/>
    <rdfs:label xml:lang="en">port</rdfs:label>
    <rdfs:comment xml:lang="en">A town or place possessing a harbour where vessels load and unload, or begin or end their voyage.</rdfs:comment>
    <rdf:type rdf:resource="http://www.w3.org/2002/07/owl#Class"/>
  </rdf:Description>
  <rdf:Description rdf:about="#CONTROL-FEATURE-TYPE_End_of_route_point">
    <rdfs:subClassOf rdf:resource="jc3iedm_OBJECT-TYPE.owl#CONTROL-FEATURE-TYPE"/>
    <rdfs:label xml:lang="en">end of route point</rdfs:label>
    <rdfs:comment xml:lang="en">Identifies the end point of a route.</rdfs:comment>
    <rdf:type rdf:resource="http://www.w3.org/2002/07/owl#Class"/>
  </rdf:Description>
  <rdf:Description rdf:about="#SURFACE-VESSEL-TYPE_Dry_dock_companion_craft">
    <rdfs:subClassOf rdf:resource="jc3iedm_OBJECT-TYPE.owl#SURFACE-VESSEL-TYPE"/>
    <rdfs:label xml:lang="en">dry dock companion craft</rdfs:label>
    <rdfs:comment xml:lang="en">Craft used to support the operations of a dry dock.</rdfs:comment>
    <rdf:type rdf:resource="http://www.w3.org/2002/07/owl#Class"/>
  </rdf:Description>
  <rdf:Description rdf:about="#MILITARY-POST-TYPE_Gunner">
    <rdfs:subClassOf rdf:resource="jc3iedm_OBJECT-TYPE.owl#MILITARY-POST-TYPE"/>
    <rdfs:label xml:lang="en">gunner</rdfs:label>
    <rdfs:comment xml:lang="en">A MILITARY-POST-TYPE that is identified as one who operates a gun.</rdfs:comment>
    <rdf:type rdf:resource="http://www.w3.org/2002/07/owl#Class"/>
  </rdf:Description>
  <rdf:Description rdf:about="#CONTROL-FEATURE-TYPE_Supply_area">
    <rdfs:subClassOf rdf:resource="jc3iedm_OBJECT-TYPE.owl#CONTROL-FEATURE-TYPE"/>
    <rdfs:label xml:lang="en">supply area</rdfs:label>
    <rdfs:comment xml:lang="en">A CONTROL-FEATURE-TYPE that identifies the contour of an area where supply units, depots, and dumps may be located.</rdfs:comment>
    <rdf:type rdf:resource="http://www.w3.org/2002/07/owl#Class"/>
  </rdf:Description>
  <rdf:Description rdf:about="#SURFACE-VESSEL-TYPE_Torpedo_boat,_small">
    <rdfs:subClassOf rdf:resource="jc3iedm_OBJECT-TYPE.owl#SURFACE-VESSEL-TYPE"/>
    <rdfs:label xml:lang="en">torpedo boat, small</rdfs:label>
    <rdfs:comment xml:lang="en">High-speed (35 knots - 65 km/hr) anti-surface ship patrol craft smaller in size range 20 - 30 metres fitted with torpedoes.</rdfs:comment>
    <rdf:type rdf:resource="http://www.w3.org/2002/07/owl#Class"/>
  </rdf:Description>
  <rdf:Description rdf:about="#FACILITY-TYPE_Supply_point">
    <rdfs:subClassOf rdf:resource="jc3iedm_OBJECT-TYPE.owl#FACILITY-TYPE"/>
    <rdfs:label xml:lang="en">supply point</rdfs:label>
    <rdfs:comment xml:lang="en">A facility where supply services are provided.</rdfs:comment>
    <rdf:type rdf:resource="http://www.w3.org/2002/07/owl#Class"/>
  </rdf:Description>
  <rdf:Description rdf:about="#SURFACE-VESSEL-TYPE_Deperming_ship">
    <rdfs:subClassOf rdf:resource="jc3iedm_OBJECT-TYPE.owl#SURFACE-VESSEL-TYPE"/>
    <rdfs:label xml:lang="en">deperming ship</rdfs:label>
    <rdfs:comment xml:lang="en">Ship designed for deperming operations.</rdfs:comment>
    <rdf:type rdf:resource="http://www.w3.org/2002/07/owl#Class"/>
  </rdf:Description>
  <rdf:Description rdf:about="#GROUP-ORGANISATION-TYPE_Prisoner_of_war">
    <rdfs:subClassOf rdf:resource="jc3iedm_OBJECT-TYPE.owl#GROUP-ORGANISATION-TYPE"/>
    <rdfs:label xml:lang="en">prisoner of war</rdfs:label>
    <rdfs:comment xml:lang="en">A GROUP-ORGANISATION-TYPE that comprises persons that have fallen in the hands of or surrendered to an opponent.</rdfs:comment>
    <rdf:type rdf:resource="http://www.w3.org/2002/07/owl#Class"/>
  </rdf:Description>
  <rdf:Description rdf:about="#SURFACE-VESSEL-TYPE_Merchant_ship,_distilling">
    <rdfs:subClassOf rdf:resource="jc3iedm_OBJECT-TYPE.owl#SURFACE-VESSEL-TYPE"/>
    <rdfs:label xml:lang="en">merchant ship, distilling</rdfs:label>
    <rdfs:comment xml:lang="en">Non-naval ship capable of distilling and transporting potable water.</rdfs:comment>
    <rdf:type rdf:resource="http://www.w3.org/2002/07/owl#Class"/>
  </rdf:Description>
  <rdf:Description rdf:about="jc3iedm_OBJECT-TYPE.owl#chemical-materiel-type-category-code">
    <rdf:type rdf:resource="http://www.w3.org/2002/07/owl#DatatypeProperty"/>
    <rdfs:domain rdf:resource="jc3iedm_OBJECT-TYPE.owl#CHEMICAL-MATERIEL-TYPE"/>
    <rdfs:range rdf:resource="http://www.w3.org/2001/XMLSchema#string"/>
  </rdf:Description>
  <rdf:Description rdf:about="#FACILITY-TYPE_Omnirange_station">
    <rdfs:subClassOf rdf:resource="jc3iedm_OBJECT-TYPE.owl#FACILITY-TYPE"/>
    <rdfs:label xml:lang="en">omnirange station</rdfs:label>
    <rdfs:comment xml:lang="en">A facility used for non-directional radio transmissions.</rdfs:comment>
    <rdf:type rdf:resource="http://www.w3.org/2002/07/owl#Class"/>
  </rdf:Description>
  <rdf:Description rdf:about="#SURFACE-VESSEL-TYPE_Frigate,_small_or_corvette">
    <rdfs:subClassOf rdf:resource="jc3iedm_OBJECT-TYPE.owl#SURFACE-VESSEL-TYPE"/>
    <rdfs:label xml:lang="en">frigate, small or corvette</rdfs:label>
    <rdfs:comment xml:lang="en">General designator for frigate but smaller. A surface combatant in size range of about 75-150 metres. Fitted primarily to fulfil an ASW role. Generally has lighter surface armament than a Destroyer, general. Classification determined by armament or capability.</rdfs:comment>
    <rdf:type rdf:resource="http://www.w3.org/2002/07/owl#Class"/>
  </rdf:Description>
  <rdf:Description rdf:about="#SURFACE-VESSEL-TYPE_Submarine_rescue_ship">
    <rdfs:subClassOf rdf:resource="jc3iedm_OBJECT-TYPE.owl#SURFACE-VESSEL-TYPE"/>
    <rdfs:label xml:lang="en">submarine rescue ship</rdfs:label>
    <rdfs:comment xml:lang="en">Any ship equipped to rescue personnel entrapped in a sunken submarine.</rdfs:comment>
    <rdf:type rdf:resource="http://www.w3.org/2002/07/owl#Class"/>
  </rdf:Description>
  <rdf:Description rdf:about="#SURFACE-VESSEL-TYPE_Barge,_nuclear_ship_support">
    <rdfs:subClassOf rdf:resource="jc3iedm_OBJECT-TYPE.owl#SURFACE-VESSEL-TYPE"/>
    <rdfs:label xml:lang="en">barge, nuclear ship support</rdfs:label>
    <rdfs:comment xml:lang="en">Craft used to transport radioactive materials.</rdfs:comment>
    <rdf:type rdf:resource="http://www.w3.org/2002/07/owl#Class"/>
  </rdf:Description>
  <rdf:Description rdf:about="#FACILITY-TYPE_Canal">
    <rdfs:subClassOf rdf:resource="jc3iedm_OBJECT-TYPE.owl#FACILITY-TYPE"/>
    <rdfs:label xml:lang="en">canal</rdfs:label>
    <rdfs:comment xml:lang="en">A man-made or improved natural waterway used for transportation.</rdfs:comment>
    <rdf:type rdf:resource="http://www.w3.org/2002/07/owl#Class"/>
  </rdf:Description>
  <rdf:Description rdf:about="#SURFACE-VESSEL-TYPE_Merchant,_refrigerated">
    <rdfs:subClassOf rdf:resource="jc3iedm_OBJECT-TYPE.owl#SURFACE-VESSEL-TYPE"/>
    <rdfs:label xml:lang="en">merchant, refrigerated</rdfs:label>
    <rdfs:comment xml:lang="en">Non-naval ship designed primarily to transport cargo in refrigerated spaces.</rdfs:comment>
    <rdf:type rdf:resource="http://www.w3.org/2002/07/owl#Class"/>
  </rdf:Description>
  <rdf:Description rdf:about="#CONTROL-FEATURE-TYPE_Crossover_zone">
    <rdfs:subClassOf rdf:resource="jc3iedm_OBJECT-TYPE.owl#CONTROL-FEATURE-TYPE"/>
    <rdfs:label xml:lang="en">crossover zone</rdfs:label>
    <rdfs:comment xml:lang="en">The airspace beyond the maritime Missile Engagement Zone (MEZ) that may be entered by Combat Air Patrol (CAP) aircraft when in hot pursuit in order to complete an interception.</rdfs:comment>
    <rdf:type rdf:resource="http://www.w3.org/2002/07/owl#Class"/>
  </rdf:Description>
  <rdf:Description rdf:about="#CONTROL-FEATURE-TYPE_Initial_point">
    <rdfs:subClassOf rdf:resource="jc3iedm_OBJECT-TYPE.owl#CONTROL-FEATURE-TYPE"/>
    <rdfs:label xml:lang="en">initial point</rdfs:label>
    <rdfs:comment xml:lang="en">A well-defined point, easily distinguishable visually and/or electronically, used as a starting point for a weapons or reconnaissance run on a target.</rdfs:comment>
    <rdf:type rdf:resource="http://www.w3.org/2002/07/owl#Class"/>
  </rdf:Description>
  <rdf:Description rdf:about="#ELECTRONIC-EQUIPMENT-TYPE_Public_address_system">
    <rdfs:subClassOf rdf:resource="jc3iedm_OBJECT-TYPE.owl#ELECTRONIC-EQUIPMENT-TYPE"/>
    <rdfs:label xml:lang="en">public address system</rdfs:label>
    <rdfs:comment xml:lang="en">A device capable of delivering voice messages.</rdfs:comment>
    <rdf:type rdf:resource="http://www.w3.org/2002/07/owl#Class"/>
  </rdf:Description>
  <rdf:Description rdf:about="#FACILITY-TYPE_Crossing/level_crossing">
    <rdfs:subClassOf rdf:resource="jc3iedm_OBJECT-TYPE.owl#FACILITY-TYPE"/>
    <rdfs:label xml:lang="en">crossing/level crossing</rdfs:label>
    <rdfs:comment xml:lang="en">A facility that is a point where two or more line features intersect or cross at the same level.</rdfs:comment>
    <rdf:type rdf:resource="http://www.w3.org/2002/07/owl#Class"/>
  </rdf:Description>
  <rdf:Description rdf:about="#FACILITY-TYPE_Dressing_station">
    <rdfs:subClassOf rdf:resource="jc3iedm_OBJECT-TYPE.owl#FACILITY-TYPE"/>
    <rdfs:label xml:lang="en">dressing station</rdfs:label>
    <rdfs:comment xml:lang="en">A movable facility for the initial treatment of casualties.</rdfs:comment>
    <rdf:type rdf:resource="http://www.w3.org/2002/07/owl#Class"/>
  </rdf:Description>
  <rdf:Description rdf:about="#SUBSURFACE-VESSEL-TYPE_Submarine,_auxiliary,_nuclear_powered">
    <rdfs:subClassOf rdf:resource="jc3iedm_OBJECT-TYPE.owl#SUBSURFACE-VESSEL-TYPE"/>
    <rdfs:label xml:lang="en">submarine, auxiliary, nuclear powered</rdfs:label>
    <rdfs:comment xml:lang="en">Submarine used mainly in a non-combatant role that has at least a residual combat capability and with nuclear power.</rdfs:comment>
    <rdf:type rdf:resource="http://www.w3.org/2002/07/owl#Class"/>
  </rdf:Description>
  <rdf:Description rdf:about="#CONTROL-FEATURE-TYPE_Release_other_than_attack_(ROTA)_isolation_and_hazard_area">
    <rdfs:subClassOf rdf:resource="jc3iedm_OBJECT-TYPE.owl#CONTROL-FEATURE-TYPE"/>
    <rdfs:label xml:lang="en">release other than attack (rota) isolation and hazard area</rdfs:label>
    <rdfs:comment xml:lang="en">The predicted or confirmed contour of the toxic industrial material isolation and hazard area.</rdfs:comment>
    <rdf:type rdf:resource="http://www.w3.org/2002/07/owl#Class"/>
  </rdf:Description>
  <rdf:Description rdf:about="jc3iedm_OBJECT-TYPE.owl#consumable-materiel-type-subcategory-code">
    <rdf:type rdf:resource="http://www.w3.org/2002/07/owl#DatatypeProperty"/>
    <rdfs:domain rdf:resource="jc3iedm_OBJECT-TYPE.owl#CONSUMABLE-MATERIEL-TYPE"/>
    <rdfs:range rdf:resource="http://www.w3.org/2001/XMLSchema#string"/>
  </rdf:Description>
  <rdf:Description rdf:about="#FACILITY-TYPE_Production_complex,_general_motor_vehicle">
    <rdfs:subClassOf rdf:resource="jc3iedm_OBJECT-TYPE.owl#FACILITY-TYPE"/>
    <rdfs:label xml:lang="en">production complex, general motor vehicle</rdfs:label>
    <rdfs:comment xml:lang="en">A facility used for non-military motor vehicle production and assembly.</rdfs:comment>
    <rdf:type rdf:resource="http://www.w3.org/2002/07/owl#Class"/>
  </rdf:Description>
  <rdf:Description rdf:about="#SURFACE-VESSEL-TYPE_Oiler/tanker,_general">
    <rdfs:subClassOf rdf:resource="jc3iedm_OBJECT-TYPE.owl#SURFACE-VESSEL-TYPE"/>
    <rdfs:label xml:lang="en">oiler/tanker, general</rdfs:label>
    <rdfs:comment xml:lang="en">General designator for oilers.</rdfs:comment>
    <rdf:type rdf:resource="http://www.w3.org/2002/07/owl#Class"/>
  </rdf:Description>
  <rdf:Description rdf:about="jc3iedm_OBJECT-TYPE.owl#subsurface-vessel-type-torpedo-loading-gear-indicator-code">
    <rdf:type rdf:resource="http://www.w3.org/2002/07/owl#DatatypeProperty"/>
    <rdfs:domain rdf:resource="jc3iedm_OBJECT-TYPE.owl#SUBSURFACE-VESSEL-TYPE"/>
    <rdfs:range rdf:resource="http://www.w3.org/2001/XMLSchema#string"/>
  </rdf:Description>
  <rdf:Description rdf:about="#VEHICLE-TYPE_Not_known">
    <rdfs:subClassOf rdf:resource="jc3iedm_OBJECT-TYPE.owl#VEHICLE-TYPE"/>
    <rdfs:label xml:lang="en">not known</rdfs:label>
    <rdfs:comment xml:lang="en">It is not possible to determine which value is most applicable.</rdfs:comment>
    <rdf:type rdf:resource="http://www.w3.org/2002/07/owl#Class"/>
  </rdf:Description>
  <rdf:Description rdf:about="jc3iedm_OBJECT-TYPE.owl#aircraft-type-airframe-design-code">
    <rdf:type rdf:resource="http://www.w3.org/2002/07/owl#DatatypeProperty"/>
    <rdfs:domain rdf:resource="jc3iedm_OBJECT-TYPE.owl#AIRCRAFT-TYPE"/>
    <rdfs:range rdf:resource="http://www.w3.org/2001/XMLSchema#string"/>
  </rdf:Description>
  <rdf:Description rdf:about="#CONTROL-FEATURE-TYPE_Drop_zone">
    <rdfs:subClassOf rdf:resource="jc3iedm_OBJECT-TYPE.owl#CONTROL-FEATURE-TYPE"/>
    <rdfs:label xml:lang="en">drop zone</rdfs:label>
    <rdfs:comment xml:lang="en">A specific area upon which airborne troops, equipment, or supplies are airdropped by parachute. NOTE: This zone can include one or more drop sites.</rdfs:comment>
    <rdf:type rdf:resource="http://www.w3.org/2002/07/owl#Class"/>
  </rdf:Description>
  <rdf:Description rdf:about="#FACILITY-TYPE_Town_hall">
    <rdfs:subClassOf rdf:resource="jc3iedm_OBJECT-TYPE.owl#FACILITY-TYPE"/>
    <rdfs:label xml:lang="en">town hall</rdfs:label>
    <rdfs:comment xml:lang="en">A building for the administration of local government, having public meeting rooms, etc.</rdfs:comment>
    <rdf:type rdf:resource="http://www.w3.org/2002/07/owl#Class"/>
  </rdf:Description>
  <rdf:Description rdf:about="jc3iedm_OBJECT-TYPE.owl#subsurface-vessel-type-category-code">
    <rdf:type rdf:resource="http://www.w3.org/2002/07/owl#DatatypeProperty"/>
    <rdfs:domain rdf:resource="jc3iedm_OBJECT-TYPE.owl#SUBSURFACE-VESSEL-TYPE"/>
    <rdfs:range rdf:resource="http://www.w3.org/2001/XMLSchema#string"/>
  </rdf:Description>
  <rdf:Description rdf:about="#MILITARY-OBSTACLE-TYPE_Dragon_teeth">
    <rdfs:subClassOf rdf:resource="jc3iedm_OBJECT-TYPE.owl#MILITARY-OBSTACLE-TYPE"/>
    <rdfs:label xml:lang="en">dragon teeth</rdfs:label>
    <rdfs:comment xml:lang="en">Regular spaced concrete or metal barriers laid in single or multiple rows to prevent vehicle movement.</rdfs:comment>
    <rdf:type rdf:resource="http://www.w3.org/2002/07/owl#Class"/>
  </rdf:Description>
  <rdf:Description rdf:about="#MILITARY-OBSTACLE-TYPE_Minefield,_maritime">
    <rdfs:subClassOf rdf:resource="jc3iedm_OBJECT-TYPE.owl#MILITARY-OBSTACLE-TYPE"/>
    <rdfs:label xml:lang="en">minefield, maritime</rdfs:label>
    <rdfs:comment xml:lang="en">An obstacle that is made by laying maritime mines in a body of water with or without pattern.</rdfs:comment>
    <rdf:type rdf:resource="http://www.w3.org/2002/07/owl#Class"/>
  </rdf:Description>
  <rdf:Description rdf:about="#GOVERNMENT-ORGANISATION-TYPE_International_civil">
    <rdfs:subClassOf rdf:resource="jc3iedm_OBJECT-TYPE.owl#GOVERNMENT-ORGANISATION-TYPE"/>
    <rdfs:label xml:lang="en">international civil</rdfs:label>
    <rdfs:comment xml:lang="en">A GOVERNMENT-ORGANISATION-TYPE that is officially involved in international civil affairs.</rdfs:comment>
    <rdf:type rdf:resource="http://www.w3.org/2002/07/owl#Class"/>
  </rdf:Description>
  <rdf:Description rdf:about="#SURFACE-VESSEL-TYPE_Net_cargo_craft">
    <rdfs:subClassOf rdf:resource="jc3iedm_OBJECT-TYPE.owl#SURFACE-VESSEL-TYPE"/>
    <rdfs:label xml:lang="en">net cargo craft</rdfs:label>
    <rdfs:comment xml:lang="en">Craft 40 metres or less used to store and transport harbour defence craft.</rdfs:comment>
    <rdf:type rdf:resource="http://www.w3.org/2002/07/owl#Class"/>
  </rdf:Description>
  <rdf:Description rdf:about="#WEAPON-TYPE_Not_otherwise_specified">
    <rdfs:subClassOf rdf:resource="jc3iedm_OBJECT-TYPE.owl#WEAPON-TYPE"/>
    <rdfs:label xml:lang="en">not otherwise specified</rdfs:label>
    <rdfs:comment xml:lang="en">The appropriate value is not in the set of specified values.</rdfs:comment>
    <rdf:type rdf:resource="http://www.w3.org/2002/07/owl#Class"/>
  </rdf:Description>
  <rdf:Description rdf:about="#ORGANISATION-TYPE_Surface-to-air_missile-operations_centre">
    <rdfs:subClassOf rdf:resource="jc3iedm_OBJECT-TYPE.owl#ORGANISATION-TYPE"/>
    <rdfs:label xml:lang="en">surface to air missile operations centre</rdfs:label>
    <rdfs:comment xml:lang="en">No definition provided in ADatP-3 Baseline 13.1 FFIRN/FUD 1874/4.</rdfs:comment>
    <rdf:type rdf:resource="http://www.w3.org/2002/07/owl#Class"/>
  </rdf:Description>
  <rdf:Description rdf:about="#SURFACE-VESSEL-TYPE_Assault_craft,_missile_equipped">
    <rdfs:subClassOf rdf:resource="jc3iedm_OBJECT-TYPE.owl#SURFACE-VESSEL-TYPE"/>
    <rdfs:label xml:lang="en">assault craft, missile equipped</rdfs:label>
    <rdfs:comment xml:lang="en">Landing craft equipped with other than force guided missiles.</rdfs:comment>
    <rdf:type rdf:resource="http://www.w3.org/2002/07/owl#Class"/>
  </rdf:Description>
  <rdf:Description rdf:about="#SURFACE-VESSEL-TYPE_Gate_craft">
    <rdfs:subClassOf rdf:resource="jc3iedm_OBJECT-TYPE.owl#SURFACE-VESSEL-TYPE"/>
    <rdfs:label xml:lang="en">gate craft</rdfs:label>
    <rdfs:comment xml:lang="en">Craft used for control or maintenance of harbour defence equipment.</rdfs:comment>
    <rdf:type rdf:resource="http://www.w3.org/2002/07/owl#Class"/>
  </rdf:Description>
  <rdf:Description rdf:about="#TASK-FORMATION-TYPE_Military-convoy-type">
    <rdfs:subClassOf rdf:resource="jc3iedm_OBJECT-TYPE.owl#TASK-FORMATION-TYPE"/>
    <rdfs:label xml:lang="en">military convoy type</rdfs:label>
    <rdfs:comment xml:lang="en">A TASK-FORMATION-TYPE that is a land or maritime convoy that is controlled and reported as a military unit.</rdfs:comment>
    <rdf:type rdf:resource="http://www.w3.org/2002/07/owl#Class"/>
  </rdf:Description>
  <rdf:Description rdf:about="#CONTROL-FEATURE-TYPE_Bridgehead">
    <rdfs:subClassOf rdf:resource="jc3iedm_OBJECT-TYPE.owl#CONTROL-FEATURE-TYPE"/>
    <rdfs:label xml:lang="en">bridgehead</rdfs:label>
    <rdfs:comment xml:lang="en">An area of ground held or to be gained on the enemy’s side of an obstacle. Army--In river-crossing operations, an area on the enemy’s side of the water obstacle that is large enough to accommodate the majority of the crossing force, has adequate terrain to permit defence of the crossing sites, and provides a base for continuing the attack.</rdfs:comment>
    <rdf:type rdf:resource="http://www.w3.org/2002/07/owl#Class"/>
  </rdf:Description>
  <rdf:Description rdf:about="#CONTROL-FEATURE-TYPE_Attack_by_fire_position">
    <rdfs:subClassOf rdf:resource="jc3iedm_OBJECT-TYPE.owl#CONTROL-FEATURE-TYPE"/>
    <rdfs:label xml:lang="en">attack by fire position</rdfs:label>
    <rdfs:comment xml:lang="en">A CONTROL-FEATURE-TYPE that is an area against which fire is employed to destroy the enemy from a distance, normally used when the mission does not dictate or support occupation of the objective.</rdfs:comment>
    <rdf:type rdf:resource="http://www.w3.org/2002/07/owl#Class"/>
  </rdf:Description>
  <rdf:Description rdf:about="#UNIT-TYPE_Manoeuvre">
    <rdfs:subClassOf rdf:resource="jc3iedm_OBJECT-TYPE.owl#UNIT-TYPE"/>
    <rdfs:label xml:lang="en">manoeuvre</rdfs:label>
    <rdfs:comment xml:lang="en">A UNIT-TYPE whose principal designation is the employment of forces in the battlespace through movement in combination with fire, or fire potential, to achieve a position of advantage in respect to the enemy in order to accomplish the mission.</rdfs:comment>
    <rdf:type rdf:resource="http://www.w3.org/2002/07/owl#Class"/>
  </rdf:Description>
  <rdf:Description rdf:about="#FACILITY-TYPE_Fire-fighters_barracks">
    <rdfs:subClassOf rdf:resource="jc3iedm_OBJECT-TYPE.owl#FACILITY-TYPE"/>
    <rdfs:label xml:lang="en">fire fighters barracks</rdfs:label>
    <rdfs:comment xml:lang="en">A building housing fire-fighters and their equipment.</rdfs:comment>
    <rdf:type rdf:resource="http://www.w3.org/2002/07/owl#Class"/>
  </rdf:Description>
  <rdf:Description rdf:about="jc3iedm_OBJECT-TYPE.owl#BRIDGE-TYPE">
    <rdf:type rdf:resource="http://www.w3.org/2002/07/owl#Class"/>
    <rdfs:label xml:lang="en">bridge type</rdfs:label>
    <rdfs:comment xml:lang="en">A FACILITY-TYPE that is a class of structures (including overpasses and viaducts), fixed or moveable, spanning and/or providing passage over an object.</rdfs:comment>
    <rdfs:subClassOf rdf:resource="jc3iedm_OBJECT-TYPE.owl#FACILITY-TYPE"/>
  </rdf:Description>
  <rdf:Description rdf:about="#FACILITY-TYPE_Radar_head">
    <rdfs:subClassOf rdf:resource="jc3iedm_OBJECT-TYPE.owl#FACILITY-TYPE"/>
    <rdfs:label xml:lang="en">radar head</rdfs:label>
    <rdfs:comment xml:lang="en">No definition provided in ADatP-3 Baseline 13.1 FFIRN/FUD 1874/4.</rdfs:comment>
    <rdf:type rdf:resource="http://www.w3.org/2002/07/owl#Class"/>
  </rdf:Description>
  <rdf:Description rdf:about="#ELECTRONIC-EQUIPMENT-TYPE_C3I">
    <rdfs:subClassOf rdf:resource="jc3iedm_OBJECT-TYPE.owl#ELECTRONIC-EQUIPMENT-TYPE"/>
    <rdfs:label xml:lang="en">c3i</rdfs:label>
    <rdfs:comment xml:lang="en">Equipment specifically designed to be used for Command, Control, Communications and Intelligence (C3I) support.</rdfs:comment>
    <rdf:type rdf:resource="http://www.w3.org/2002/07/owl#Class"/>
  </rdf:Description>
  <rdf:Description rdf:about="#GROUP-ORGANISATION-TYPE_Gang">
    <rdfs:subClassOf rdf:resource="jc3iedm_OBJECT-TYPE.owl#GROUP-ORGANISATION-TYPE"/>
    <rdfs:label xml:lang="en">gang</rdfs:label>
    <rdfs:comment xml:lang="en">A GROUP-ORGANISATION-TYPE that comprises persons that go together or act in concert.</rdfs:comment>
    <rdf:type rdf:resource="http://www.w3.org/2002/07/owl#Class"/>
  </rdf:Description>
  <rdf:Description rdf:about="#SURFACE-VESSEL-TYPE_Patrol_ship,_offshore">
    <rdfs:subClassOf rdf:resource="jc3iedm_OBJECT-TYPE.owl#SURFACE-VESSEL-TYPE"/>
    <rdfs:label xml:lang="en">patrol ship, offshore</rdfs:label>
    <rdfs:comment xml:lang="en">Coastal patrol unit in size over 60 metres designed for use in offshore waters. May or may not be armed with guns.</rdfs:comment>
    <rdf:type rdf:resource="http://www.w3.org/2002/07/owl#Class"/>
  </rdf:Description>
  <rdf:Description rdf:about="#AMMUNITION-TYPE_Mine,_anti-tank">
    <rdfs:subClassOf rdf:resource="jc3iedm_OBJECT-TYPE.owl#AMMUNITION-TYPE"/>
    <rdfs:label xml:lang="en">mine, anti tank</rdfs:label>
    <rdfs:comment xml:lang="en">A mine designed to immobilise or destroy a tank.</rdfs:comment>
    <rdf:type rdf:resource="http://www.w3.org/2002/07/owl#Class"/>
  </rdf:Description>
  <rdf:Description rdf:about="#CONTROL-FEATURE-TYPE_Encirclement">
    <rdfs:subClassOf rdf:resource="jc3iedm_OBJECT-TYPE.owl#CONTROL-FEATURE-TYPE"/>
    <rdfs:label xml:lang="en">encirclement</rdfs:label>
    <rdfs:comment xml:lang="en">The loss of freedom of manoeuvre to one force resulting from an enemy force’s control of all routes of egress and reinforcement.</rdfs:comment>
    <rdf:type rdf:resource="http://www.w3.org/2002/07/owl#Class"/>
  </rdf:Description>
  <rdf:Description rdf:about="#SURFACE-VESSEL-TYPE_Service_craft,_experimental">
    <rdfs:subClassOf rdf:resource="jc3iedm_OBJECT-TYPE.owl#SURFACE-VESSEL-TYPE"/>
    <rdfs:label xml:lang="en">service craft, experimental</rdfs:label>
    <rdfs:comment xml:lang="en">Craft, usually under 40 metres overall employed in general or multi-purpose functions of support, training, R&amp;D or test in nature and used for experimental purposes.</rdfs:comment>
    <rdf:type rdf:resource="http://www.w3.org/2002/07/owl#Class"/>
  </rdf:Description>
  <rdf:Description rdf:about="#SURFACE-VESSEL-TYPE_Merchant_ship,_liquid_gas">
    <rdfs:subClassOf rdf:resource="jc3iedm_OBJECT-TYPE.owl#SURFACE-VESSEL-TYPE"/>
    <rdfs:label xml:lang="en">merchant ship, liquid gas</rdfs:label>
    <rdfs:comment xml:lang="en">Non-naval ship designed to transport liquid gas.</rdfs:comment>
    <rdf:type rdf:resource="http://www.w3.org/2002/07/owl#Class"/>
  </rdf:Description>
  <rdf:Description rdf:about="#MARITIME-EQUIPMENT-TYPE_Buoy">
    <rdfs:subClassOf rdf:resource="jc3iedm_OBJECT-TYPE.owl#MARITIME-EQUIPMENT-TYPE"/>
    <rdfs:label xml:lang="en">buoy</rdfs:label>
    <rdfs:comment xml:lang="en">A floating object fastened in a particular place to mark the position of underwater objects or the course that ships have to navigate.</rdfs:comment>
    <rdf:type rdf:resource="http://www.w3.org/2002/07/owl#Class"/>
  </rdf:Description>
  <rdf:Description rdf:about="#AMMUNITION-TYPE_Bomb">
    <rdfs:subClassOf rdf:resource="jc3iedm_OBJECT-TYPE.owl#AMMUNITION-TYPE"/>
    <rdfs:label xml:lang="en">bomb</rdfs:label>
    <rdfs:comment xml:lang="en">A case filled with explosive, inflammable material, poison gas, or smoke, etc., dropped from aircraft, or thrown or deposited by hand.</rdfs:comment>
    <rdf:type rdf:resource="http://www.w3.org/2002/07/owl#Class"/>
  </rdf:Description>
  <rdf:Description rdf:about="jc3iedm_OBJECT-TYPE.owl#MILITARY-ORGANISATION-TYPE">
    <rdf:type rdf:resource="http://www.w3.org/2002/07/owl#Class"/>
    <rdfs:label xml:lang="en">military organisation type</rdfs:label>
    <rdfs:comment xml:lang="en">A GOVERNMENT-ORGANISATION-TYPE that is officially sanctioned and is trained and equipped to exert force.</rdfs:comment>
    <rdfs:subClassOf rdf:resource="jc3iedm_OBJECT-TYPE.owl#GOVERNMENT-ORGANISATION-TYPE"/>
  </rdf:Description>
  <rdf:Description rdf:about="#VEHICLE-TYPE_Materiel_handling">
    <rdfs:subClassOf rdf:resource="jc3iedm_OBJECT-TYPE.owl#VEHICLE-TYPE"/>
    <rdfs:label xml:lang="en">materiel handling</rdfs:label>
    <rdfs:comment xml:lang="en">A vehicle which, as its primary, is designed to provide materiel handling facilities in or out of the battlespace.</rdfs:comment>
    <rdf:type rdf:resource="http://www.w3.org/2002/07/owl#Class"/>
  </rdf:Description>
  <rdf:Description rdf:about="#SURFACE-VESSEL-TYPE_Range_tender">
    <rdfs:subClassOf rdf:resource="jc3iedm_OBJECT-TYPE.owl#SURFACE-VESSEL-TYPE"/>
    <rdfs:label xml:lang="en">range tender</rdfs:label>
    <rdfs:comment xml:lang="en">Craft used for safety and utility purposes on ranges.</rdfs:comment>
    <rdf:type rdf:resource="http://www.w3.org/2002/07/owl#Class"/>
  </rdf:Description>
  <rdf:Description rdf:about="#SURFACE-VESSEL-TYPE_Lighter,_amphibious,_re-supply,_cargo">
    <rdfs:subClassOf rdf:resource="jc3iedm_OBJECT-TYPE.owl#SURFACE-VESSEL-TYPE"/>
    <rdfs:label xml:lang="en">lighter, amphibious, re supply, cargo</rdfs:label>
    <rdfs:comment xml:lang="en">A lighter designed to carry cargo for the re-supply of landing forces.</rdfs:comment>
    <rdf:type rdf:resource="http://www.w3.org/2002/07/owl#Class"/>
  </rdf:Description>
  <rdf:Description rdf:about="#SURFACE-VESSEL-TYPE_Assault_craft,_gun_equipped">
    <rdfs:subClassOf rdf:resource="jc3iedm_OBJECT-TYPE.owl#SURFACE-VESSEL-TYPE"/>
    <rdfs:label xml:lang="en">assault craft, gun equipped</rdfs:label>
    <rdfs:comment xml:lang="en">Assault landing craft equipped with guns.</rdfs:comment>
    <rdf:type rdf:resource="http://www.w3.org/2002/07/owl#Class"/>
  </rdf:Description>
  <rdf:Description rdf:about="#CONTROL-FEATURE-TYPE_Turning_point">
    <rdfs:subClassOf rdf:resource="jc3iedm_OBJECT-TYPE.owl#CONTROL-FEATURE-TYPE"/>
    <rdfs:label xml:lang="en">turning point</rdfs:label>
    <rdfs:comment xml:lang="en">The aircraft, ship or other vehicle will change direction at this point.</rdfs:comment>
    <rdf:type rdf:resource="http://www.w3.org/2002/07/owl#Class"/>
  </rdf:Description>
  <rdf:Description rdf:about="#MILITARY-ORGANISATION-TYPE_Not_otherwise_specified">
    <rdfs:subClassOf rdf:resource="jc3iedm_OBJECT-TYPE.owl#MILITARY-ORGANISATION-TYPE"/>
    <rdfs:label xml:lang="en">not otherwise specified</rdfs:label>
    <rdfs:comment xml:lang="en">The appropriate value is not in the set of specified values.</rdfs:comment>
    <rdf:type rdf:resource="http://www.w3.org/2002/07/owl#Class"/>
  </rdf:Description>
  <rdf:Description rdf:about="#WEAPON-TYPE_Field_artillery">
    <rdfs:subClassOf rdf:resource="jc3iedm_OBJECT-TYPE.owl#WEAPON-TYPE"/>
    <rdfs:label xml:lang="en">field artillery</rdfs:label>
    <rdfs:comment xml:lang="en">Artillery that is self-propelled or towed for use in the field in support of manoeuvre forces.</rdfs:comment>
    <rdf:type rdf:resource="http://www.w3.org/2002/07/owl#Class"/>
  </rdf:Description>
  <rdf:Description rdf:about="#CONTROL-FEATURE-TYPE_Class-B_airspace">
    <rdfs:subClassOf rdf:resource="jc3iedm_OBJECT-TYPE.owl#CONTROL-FEATURE-TYPE"/>
    <rdfs:label xml:lang="en">class b airspace</rdfs:label>
    <rdfs:comment xml:lang="en">An airspace in which instrument flight rule and visual flight rule flights are permitted; all flights are subject to air traffic control service and are separated from each other.</rdfs:comment>
    <rdf:type rdf:resource="http://www.w3.org/2002/07/owl#Class"/>
  </rdf:Description>
  <rdf:Description rdf:about="#AMMUNITION-TYPE_Gun_shell">
    <rdfs:subClassOf rdf:resource="jc3iedm_OBJECT-TYPE.owl#AMMUNITION-TYPE"/>
    <rdfs:label xml:lang="en">gun shell</rdfs:label>
    <rdfs:comment xml:lang="en">A munition that is propelled from a barrel and thereafter follows a ballistic trajectory.</rdfs:comment>
    <rdf:type rdf:resource="http://www.w3.org/2002/07/owl#Class"/>
  </rdf:Description>
  <rdf:Description rdf:about="#SURFACE-VESSEL-TYPE_Fisheries_patrol_craft">
    <rdfs:subClassOf rdf:resource="jc3iedm_OBJECT-TYPE.owl#SURFACE-VESSEL-TYPE"/>
    <rdfs:label xml:lang="en">fisheries patrol craft</rdfs:label>
    <rdfs:comment xml:lang="en">Fisheries service operated vessel (fisheries patrol craft) in size range 35-55 metres designed and fitted primarily for escort duties in ASW role.</rdfs:comment>
    <rdf:type rdf:resource="http://www.w3.org/2002/07/owl#Class"/>
  </rdf:Description>
  <rdf:Description rdf:about="#CONSUMABLE-MATERIEL-TYPE_Spare_parts">
    <rdfs:subClassOf rdf:resource="jc3iedm_OBJECT-TYPE.owl#CONSUMABLE-MATERIEL-TYPE"/>
    <rdfs:label xml:lang="en">spare parts</rdfs:label>
    <rdfs:comment xml:lang="en">A generic term covering materiel used as replacement parts.</rdfs:comment>
    <rdf:type rdf:resource="http://www.w3.org/2002/07/owl#Class"/>
  </rdf:Description>
  <rdf:Description rdf:about="#GROUP-ORGANISATION-TYPE_Intellectual">
    <rdfs:subClassOf rdf:resource="jc3iedm_OBJECT-TYPE.owl#GROUP-ORGANISATION-TYPE"/>
    <rdfs:label xml:lang="en">intellectual</rdfs:label>
    <rdfs:comment xml:lang="en">A GROUP-ORGANISATION-TYPE that comprises intellectual beings possessing superior powers of intellect.</rdfs:comment>
    <rdf:type rdf:resource="http://www.w3.org/2002/07/owl#Class"/>
  </rdf:Description>
  <rdf:Description rdf:about="#VEHICLE-TYPE_Combat_engineer_vehicle">
    <rdfs:subClassOf rdf:resource="jc3iedm_OBJECT-TYPE.owl#VEHICLE-TYPE"/>
    <rdfs:label xml:lang="en">combat engineer vehicle</rdfs:label>
    <rdfs:comment xml:lang="en">No definition provided in ADatP-3 Baseline 13.1 FFIRN/FUD 1650/6.</rdfs:comment>
    <rdf:type rdf:resource="http://www.w3.org/2002/07/owl#Class"/>
  </rdf:Description>
  <rdf:Description rdf:about="#SURFACE-VESSEL-TYPE_Merchant_ship,_space/missile_associated">
    <rdfs:subClassOf rdf:resource="jc3iedm_OBJECT-TYPE.owl#SURFACE-VESSEL-TYPE"/>
    <rdfs:label xml:lang="en">merchant ship, space/missile associated</rdfs:label>
    <rdfs:comment xml:lang="en">Non-naval ship designed or converted primarily to support space and missile programmes.</rdfs:comment>
    <rdf:type rdf:resource="http://www.w3.org/2002/07/owl#Class"/>
  </rdf:Description>
  <rdf:Description rdf:about="#SURFACE-VESSEL-TYPE_Merchant_ship,_special_liquids">
    <rdfs:subClassOf rdf:resource="jc3iedm_OBJECT-TYPE.owl#SURFACE-VESSEL-TYPE"/>
    <rdfs:label xml:lang="en">merchant ship, special liquids</rdfs:label>
    <rdfs:comment xml:lang="en">Non-naval ship 40 metres or more designed to transport a special kind of propellant or other non-nuclear associated liquid cargo.</rdfs:comment>
    <rdf:type rdf:resource="http://www.w3.org/2002/07/owl#Class"/>
  </rdf:Description>
  <rdf:Description rdf:about="#SURFACE-VESSEL-TYPE_Service_craft,_surface_effect,_experimental">
    <rdfs:subClassOf rdf:resource="jc3iedm_OBJECT-TYPE.owl#SURFACE-VESSEL-TYPE"/>
    <rdfs:label xml:lang="en">service craft, surface effect, experimental</rdfs:label>
    <rdfs:comment xml:lang="en">Craft, usually under 40 metres overall employed in general or multi-purpose functions of support, training, R&amp;D or test in nature. It is used for experimental purposes with a surface effect design.</rdfs:comment>
    <rdf:type rdf:resource="http://www.w3.org/2002/07/owl#Class"/>
  </rdf:Description>
  <rdf:Description rdf:about="#FACILITY-TYPE_Logistics_release_point">
    <rdfs:subClassOf rdf:resource="jc3iedm_OBJECT-TYPE.owl#FACILITY-TYPE"/>
    <rdfs:label xml:lang="en">logistics release point</rdfs:label>
    <rdfs:comment xml:lang="en">The facility along the supply route where the supported unit meets the supporting unit to transfer supplies.</rdfs:comment>
    <rdf:type rdf:resource="http://www.w3.org/2002/07/owl#Class"/>
  </rdf:Description>
  <rdf:Description rdf:about="#MILITARY-OBSTACLE-TYPE_Beam_post_obstacle">
    <rdfs:subClassOf rdf:resource="jc3iedm_OBJECT-TYPE.owl#MILITARY-OBSTACLE-TYPE"/>
    <rdfs:label xml:lang="en">beam post obstacle</rdfs:label>
    <rdfs:comment xml:lang="en">A squared-off log or a large, oblong piece of timber, metal, or stone inserted in the ground to obstruct movement.</rdfs:comment>
    <rdf:type rdf:resource="http://www.w3.org/2002/07/owl#Class"/>
  </rdf:Description>
  <rdf:Description rdf:about="#SURFACE-VESSEL-TYPE_Destroyer,_training">
    <rdfs:subClassOf rdf:resource="jc3iedm_OBJECT-TYPE.owl#SURFACE-VESSEL-TYPE"/>
    <rdfs:label xml:lang="en">destroyer, training</rdfs:label>
    <rdfs:comment xml:lang="en">A destroyer type ship used primarily in a training role. Major surface combatant in range of about 95 to 140 metres whole general mission is to conduct operations with strike, ASW and amphibious forces, and to perform screening and convoy duties. May have helicopters not especially fitted for ASW.</rdfs:comment>
    <rdf:type rdf:resource="http://www.w3.org/2002/07/owl#Class"/>
  </rdf:Description>
  <rdf:Description rdf:about="#MILITARY-POST-TYPE_Forward_air_controller,_airborne">
    <rdfs:subClassOf rdf:resource="jc3iedm_OBJECT-TYPE.owl#MILITARY-POST-TYPE"/>
    <rdfs:label xml:lang="en">forward air controller, airborne</rdfs:label>
    <rdfs:comment xml:lang="en">A MILITARY-POST-TYPE that is a specifically trained and qualified aviation officer who exercises control from the air of aircraft engaged in close air support of ground troops. The forward air controller (airborne) is normally an airborne extension of the tactical air control party.</rdfs:comment>
    <rdf:type rdf:resource="http://www.w3.org/2002/07/owl#Class"/>
  </rdf:Description>
  <rdf:Description rdf:about="#SURFACE-VESSEL-TYPE_Auxiliary_flag_or_command_ship">
    <rdfs:subClassOf rdf:resource="jc3iedm_OBJECT-TYPE.owl#SURFACE-VESSEL-TYPE"/>
    <rdfs:label xml:lang="en">auxiliary flag or command ship</rdfs:label>
    <rdfs:comment xml:lang="en">Ship 55 metres or more used to provide afloat communications facilities and accommodation for a force commander and his operations staff.</rdfs:comment>
    <rdf:type rdf:resource="http://www.w3.org/2002/07/owl#Class"/>
  </rdf:Description>
  <rdf:Description rdf:about="#CONTROL-FEATURE-TYPE_Landing_point">
    <rdfs:subClassOf rdf:resource="jc3iedm_OBJECT-TYPE.owl#CONTROL-FEATURE-TYPE"/>
    <rdfs:label xml:lang="en">landing point</rdfs:label>
    <rdfs:comment xml:lang="en">The aircraft, ship or other vehicle will land at the route point.</rdfs:comment>
    <rdf:type rdf:resource="http://www.w3.org/2002/07/owl#Class"/>
  </rdf:Description>
  <rdf:Description rdf:about="#GEOGRAPHIC-FEATURE-TYPE_Snow/ice">
    <rdfs:subClassOf rdf:resource="jc3iedm_OBJECT-TYPE.owl#GEOGRAPHIC-FEATURE-TYPE"/>
    <rdfs:label xml:lang="en">snow/ice</rdfs:label>
    <rdfs:comment xml:lang="en">Natural features that are characterised by frozen water.</rdfs:comment>
    <rdf:type rdf:resource="http://www.w3.org/2002/07/owl#Class"/>
  </rdf:Description>
  <rdf:Description rdf:about="jc3iedm_OBJECT-TYPE.owl#aircraft-type-training-category-code">
    <rdf:type rdf:resource="http://www.w3.org/2002/07/owl#DatatypeProperty"/>
    <rdfs:domain rdf:resource="jc3iedm_OBJECT-TYPE.owl#AIRCRAFT-TYPE"/>
    <rdfs:range rdf:resource="http://www.w3.org/2001/XMLSchema#string"/>
  </rdf:Description>
  <rdf:Description rdf:about="#FACILITY-TYPE_Rail_facility,_repair">
    <rdfs:subClassOf rdf:resource="jc3iedm_OBJECT-TYPE.owl#FACILITY-TYPE"/>
    <rdfs:label xml:lang="en">rail facility, repair</rdfs:label>
    <rdfs:comment xml:lang="en">An installation on a railway where railway equipment may be repaired.</rdfs:comment>
    <rdf:type rdf:resource="http://www.w3.org/2002/07/owl#Class"/>
  </rdf:Description>
  <rdf:Description rdf:about="#CONTROL-FEATURE-TYPE_No_fire_line">
    <rdfs:subClassOf rdf:resource="jc3iedm_OBJECT-TYPE.owl#CONTROL-FEATURE-TYPE"/>
    <rdfs:label xml:lang="en">no fire line</rdfs:label>
    <rdfs:comment xml:lang="en">A line short of which artillery or ships do not fire except on request or approval of the supported commander, but beyond which they may fire at any time without danger to friendly troops.</rdfs:comment>
    <rdf:type rdf:resource="http://www.w3.org/2002/07/owl#Class"/>
  </rdf:Description>
  <rdf:Description rdf:about="#ORGANISATION-TYPE_Direct_air_support_centre">
    <rdfs:subClassOf rdf:resource="jc3iedm_OBJECT-TYPE.owl#ORGANISATION-TYPE"/>
    <rdfs:label xml:lang="en">direct air support centre</rdfs:label>
    <rdfs:comment xml:lang="en">The ORGANISATION-TYPE that is the principal air control agency of the U.S. Marine air command and control system responsible for the direction and control of air operations directly supporting the ground combat element. It processes and coordinates requests for immediate air support and coordinates air missions requiring integration with ground forces and other supporting arms.</rdfs:comment>
    <rdf:type rdf:resource="http://www.w3.org/2002/07/owl#Class"/>
  </rdf:Description>
  <rdf:Description rdf:about="#SURFACE-VESSEL-TYPE_Oiler_replenishment,_small_(naval)">
    <rdfs:subClassOf rdf:resource="jc3iedm_OBJECT-TYPE.owl#SURFACE-VESSEL-TYPE"/>
    <rdfs:label xml:lang="en">oiler replenishment, small (naval)</rdfs:label>
    <rdfs:comment xml:lang="en">Ship between 40-140 metres capable of providing rapid replenishment of POL and solid store products.</rdfs:comment>
    <rdf:type rdf:resource="http://www.w3.org/2002/07/owl#Class"/>
  </rdf:Description>
  <rdf:Description rdf:about="#VEHICLE-TYPE_Armoured_service_support">
    <rdfs:subClassOf rdf:resource="jc3iedm_OBJECT-TYPE.owl#VEHICLE-TYPE"/>
    <rdfs:label xml:lang="en">armoured service support</rdfs:label>
    <rdfs:comment xml:lang="en">An armoured vehicle mainly used for maintenance, recovery, ambulance functions or resupply.</rdfs:comment>
    <rdf:type rdf:resource="http://www.w3.org/2002/07/owl#Class"/>
  </rdf:Description>
  <rdf:Description rdf:about="#CONTROL-FEATURE-TYPE_Communication_zone">
    <rdfs:subClassOf rdf:resource="jc3iedm_OBJECT-TYPE.owl#CONTROL-FEATURE-TYPE"/>
    <rdfs:label xml:lang="en">communication zone</rdfs:label>
    <rdfs:comment xml:lang="en">A CONTROL-FEATURE-TYPE with an area location which defines the rear part of theatre of operations (behind but contiguous to the combat zone) which contains the lines of communication, establishments for supply and evacuation, and other agencies required for the immediate support and maintenance of the field forces.</rdfs:comment>
    <rdf:type rdf:resource="http://www.w3.org/2002/07/owl#Class"/>
  </rdf:Description>
  <rdf:Description rdf:about="#CONTROL-FEATURE-TYPE_Fire_position_area">
    <rdfs:subClassOf rdf:resource="jc3iedm_OBJECT-TYPE.owl#CONTROL-FEATURE-TYPE"/>
    <rdfs:label xml:lang="en">fire position area</rdfs:label>
    <rdfs:comment xml:lang="en">The specific location within an Artillery area CONTROL-FEATURE-TYPE from which a fire unit delivers fire.</rdfs:comment>
    <rdf:type rdf:resource="http://www.w3.org/2002/07/owl#Class"/>
  </rdf:Description>
  <rdf:Description rdf:about="#UNIT-TYPE_Missile,_surface-to-surface">
    <rdfs:subClassOf rdf:resource="jc3iedm_OBJECT-TYPE.owl#UNIT-TYPE"/>
    <rdfs:label xml:lang="en">missile, surface to surface</rdfs:label>
    <rdfs:comment xml:lang="en">A UNIT-TYPE whose principal designation is the employment of surface-based missiles to fire at surface targets.</rdfs:comment>
    <rdf:type rdf:resource="http://www.w3.org/2002/07/owl#Class"/>
  </rdf:Description>
  <rdf:Description rdf:about="#VEHICLE-TYPE_Bus">
    <rdfs:subClassOf rdf:resource="jc3iedm_OBJECT-TYPE.owl#VEHICLE-TYPE"/>
    <rdfs:label xml:lang="en">bus</rdfs:label>
    <rdfs:comment xml:lang="en">A large passenger road vehicle.</rdfs:comment>
    <rdf:type rdf:resource="http://www.w3.org/2002/07/owl#Class"/>
  </rdf:Description>
  <rdf:Description rdf:about="#VEHICLE-TYPE_Command_post">
    <rdfs:subClassOf rdf:resource="jc3iedm_OBJECT-TYPE.owl#VEHICLE-TYPE"/>
    <rdfs:label xml:lang="en">command post</rdfs:label>
    <rdfs:comment xml:lang="en">A vehicle designed to be used as a command post or as part of a command post.</rdfs:comment>
    <rdf:type rdf:resource="http://www.w3.org/2002/07/owl#Class"/>
  </rdf:Description>
  <rdf:Description rdf:about="#FACILITY-TYPE_Electronic_installation,_warfare">
    <rdfs:subClassOf rdf:resource="jc3iedm_OBJECT-TYPE.owl#FACILITY-TYPE"/>
    <rdfs:label xml:lang="en">electronic installation, warfare</rdfs:label>
    <rdfs:comment xml:lang="en">A facility whose essential function is to exploit the electromagnetic spectrum encompassing: the search for, interception and identification of electromagnetic emissions, the employment of electromagnetic energy, including directed energy, to reduce or prevent hostile use of the electromagnetic spectrum, and actions to ensure its effective use by friendly forces.</rdfs:comment>
    <rdf:type rdf:resource="http://www.w3.org/2002/07/owl#Class"/>
  </rdf:Description>
  <rdf:Description rdf:about="#FACILITY-TYPE_Shelter,_underground">
    <rdfs:subClassOf rdf:resource="jc3iedm_OBJECT-TYPE.owl#FACILITY-TYPE"/>
    <rdfs:label xml:lang="en">shelter, underground</rdfs:label>
    <rdfs:comment xml:lang="en">A fortified structure built underground, used to house personnel and/or equipment.</rdfs:comment>
    <rdf:type rdf:resource="http://www.w3.org/2002/07/owl#Class"/>
  </rdf:Description>
  <rdf:Description rdf:about="#CONTROL-FEATURE-TYPE_Airborne_early_warning_area">
    <rdfs:subClassOf rdf:resource="jc3iedm_OBJECT-TYPE.owl#CONTROL-FEATURE-TYPE"/>
    <rdfs:label xml:lang="en">airborne early warning area</rdfs:label>
    <rdfs:comment xml:lang="en">Airspace established specifically for airborne platforms conducting early warning.</rdfs:comment>
    <rdf:type rdf:resource="http://www.w3.org/2002/07/owl#Class"/>
  </rdf:Description>
  <rdf:Description rdf:about="#FACILITY-TYPE_Site,_electronic_warfare">
    <rdfs:subClassOf rdf:resource="jc3iedm_OBJECT-TYPE.owl#FACILITY-TYPE"/>
    <rdfs:label xml:lang="en">site, electronic warfare</rdfs:label>
    <rdfs:comment xml:lang="en">A facility that carries out Electronic Warfare.</rdfs:comment>
    <rdf:type rdf:resource="http://www.w3.org/2002/07/owl#Class"/>
  </rdf:Description>
  <rdf:Description rdf:about="#FACILITY-TYPE_Missile_site">
    <rdfs:subClassOf rdf:resource="jc3iedm_OBJECT-TYPE.owl#FACILITY-TYPE"/>
    <rdfs:label xml:lang="en">missile site</rdfs:label>
    <rdfs:comment xml:lang="en">An area with related facilities for storing and launching missiles.</rdfs:comment>
    <rdf:type rdf:resource="http://www.w3.org/2002/07/owl#Class"/>
  </rdf:Description>
  <rdf:Description rdf:about="#CONTROL-FEATURE-TYPE_Nuclear_target">
    <rdfs:subClassOf rdf:resource="jc3iedm_OBJECT-TYPE.owl#CONTROL-FEATURE-TYPE"/>
    <rdfs:label xml:lang="en">nuclear target</rdfs:label>
    <rdfs:comment xml:lang="en">No definition provided in APP-6B JUN 08.</rdfs:comment>
    <rdf:type rdf:resource="http://www.w3.org/2002/07/owl#Class"/>
  </rdf:Description>
  <rdf:Description rdf:about="#CBRN-EQUIPMENT-TYPE_Radiological_kit">
    <rdfs:subClassOf rdf:resource="jc3iedm_OBJECT-TYPE.owl#CBRN-EQUIPMENT-TYPE"/>
    <rdfs:label xml:lang="en">radiological kit</rdfs:label>
    <rdfs:comment xml:lang="en">A collection of personal dosimeters or detectors for determination of radiation exposure history and protection against radiation hazards issued to a person.</rdfs:comment>
    <rdf:type rdf:resource="http://www.w3.org/2002/07/owl#Class"/>
  </rdf:Description>
  <rdf:Description rdf:about="#SURFACE-VESSEL-TYPE_Merchant_ship,_passenger">
    <rdfs:subClassOf rdf:resource="jc3iedm_OBJECT-TYPE.owl#SURFACE-VESSEL-TYPE"/>
    <rdfs:label xml:lang="en">merchant ship, passenger</rdfs:label>
    <rdfs:comment xml:lang="en">Non-naval ship designed primarily to transport passengers.</rdfs:comment>
    <rdf:type rdf:resource="http://www.w3.org/2002/07/owl#Class"/>
  </rdf:Description>
  <rdf:Description rdf:about="#SURFACE-VESSEL-TYPE_Barge,_radiological_repair">
    <rdfs:subClassOf rdf:resource="jc3iedm_OBJECT-TYPE.owl#SURFACE-VESSEL-TYPE"/>
    <rdfs:label xml:lang="en">barge, radiological repair</rdfs:label>
    <rdfs:comment xml:lang="en">Barge used to repair and/or service radioactive equipment.</rdfs:comment>
    <rdf:type rdf:resource="http://www.w3.org/2002/07/owl#Class"/>
  </rdf:Description>
  <rdf:Description rdf:about="#SURFACE-VESSEL-TYPE_Merchant_ship,_container,_non-self-sustained">
    <rdfs:subClassOf rdf:resource="jc3iedm_OBJECT-TYPE.owl#SURFACE-VESSEL-TYPE"/>
    <rdfs:label xml:lang="en">merchant ship, container, non self sustained</rdfs:label>
    <rdfs:comment xml:lang="en">Non-naval ship designed to carry cargo in loadable and unloadable containers. Not equipped to handle the containers with own equipment.</rdfs:comment>
    <rdf:type rdf:resource="http://www.w3.org/2002/07/owl#Class"/>
  </rdf:Description>
  <rdf:Description rdf:about="#SURFACE-VESSEL-TYPE_Destroyer_tender">
    <rdfs:subClassOf rdf:resource="jc3iedm_OBJECT-TYPE.owl#SURFACE-VESSEL-TYPE"/>
    <rdfs:label xml:lang="en">destroyer tender</rdfs:label>
    <rdfs:comment xml:lang="en">Ships of any size but usually large, employed primarily to furnish facilities and services for the support and repair of destroyer type ships.</rdfs:comment>
    <rdf:type rdf:resource="http://www.w3.org/2002/07/owl#Class"/>
  </rdf:Description>
  <rdf:Description rdf:about="#FACILITY-TYPE_Maintenance_facility,_aircraft">
    <rdfs:subClassOf rdf:resource="jc3iedm_OBJECT-TYPE.owl#FACILITY-TYPE"/>
    <rdfs:label xml:lang="en">maintenance facility, aircraft</rdfs:label>
    <rdfs:comment xml:lang="en">A facility containing the resources and infrastructure to enable it to be used for the repair and servicing of aircraft.</rdfs:comment>
    <rdf:type rdf:resource="http://www.w3.org/2002/07/owl#Class"/>
  </rdf:Description>
  <rdf:Description rdf:about="#CONSUMABLE-MATERIEL-TYPE_Crops">
    <rdfs:subClassOf rdf:resource="jc3iedm_OBJECT-TYPE.owl#CONSUMABLE-MATERIEL-TYPE"/>
    <rdfs:label xml:lang="en">crops</rdfs:label>
    <rdfs:comment xml:lang="en">Cultivated agricultural plants, as grain, vegetables or fruit.</rdfs:comment>
    <rdf:type rdf:resource="http://www.w3.org/2002/07/owl#Class"/>
  </rdf:Description>
  <rdf:Description rdf:about="#VESSEL-TYPE_Not_known">
    <rdfs:subClassOf rdf:resource="jc3iedm_OBJECT-TYPE.owl#VESSEL-TYPE"/>
    <rdfs:label xml:lang="en">not known</rdfs:label>
    <rdfs:comment xml:lang="en">It is not possible to determine which value is most applicable.</rdfs:comment>
    <rdf:type rdf:resource="http://www.w3.org/2002/07/owl#Class"/>
  </rdf:Description>
  <rdf:Description rdf:about="#ENGINEERING-EQUIPMENT-TYPE_Dozer">
    <rdfs:subClassOf rdf:resource="jc3iedm_OBJECT-TYPE.owl#ENGINEERING-EQUIPMENT-TYPE"/>
    <rdfs:label xml:lang="en">dozer</rdfs:label>
    <rdfs:comment xml:lang="en">A heavy caterpillar tractor fitted with a broad steel blade in front, used for removing obstacles, levelling uneven surfaces, etc.</rdfs:comment>
    <rdf:type rdf:resource="http://www.w3.org/2002/07/owl#Class"/>
  </rdf:Description>
  <rdf:Description rdf:about="#GROUP-ORGANISATION-TYPE_Landowner">
    <rdfs:subClassOf rdf:resource="jc3iedm_OBJECT-TYPE.owl#GROUP-ORGANISATION-TYPE"/>
    <rdfs:label xml:lang="en">landowner</rdfs:label>
    <rdfs:comment xml:lang="en">A GROUP-ORGANISATION-TYPE that comprises persons that are owners or proprietors of land.</rdfs:comment>
    <rdf:type rdf:resource="http://www.w3.org/2002/07/owl#Class"/>
  </rdf:Description>
  <rdf:Description rdf:about="#ENGINEERING-EQUIPMENT-TYPE_Earthmover">
    <rdfs:subClassOf rdf:resource="jc3iedm_OBJECT-TYPE.owl#ENGINEERING-EQUIPMENT-TYPE"/>
    <rdfs:label xml:lang="en">earthmover</rdfs:label>
    <rdfs:comment xml:lang="en">A vehicle designed for the excavation or shifting of large quantities of earth.</rdfs:comment>
    <rdf:type rdf:resource="http://www.w3.org/2002/07/owl#Class"/>
  </rdf:Description>
  <rdf:Description rdf:about="#CONTROL-FEATURE-TYPE_Joint_operations_area">
    <rdfs:subClassOf rdf:resource="jc3iedm_OBJECT-TYPE.owl#CONTROL-FEATURE-TYPE"/>
    <rdfs:label xml:lang="en">joint operations area</rdfs:label>
    <rdfs:comment xml:lang="en">Area of land, sea, and airspace defined by a combat commander or subordinate unified commander, in which joint force commander conducts military operations to accomplish a specific mission.</rdfs:comment>
    <rdf:type rdf:resource="http://www.w3.org/2002/07/owl#Class"/>
  </rdf:Description>
  <rdf:Description rdf:about="#FACILITY-TYPE_Pipeline">
    <rdfs:subClassOf rdf:resource="jc3iedm_OBJECT-TYPE.owl#FACILITY-TYPE"/>
    <rdfs:label xml:lang="en">pipeline</rdfs:label>
    <rdfs:comment xml:lang="en">A system of pipes above or under ground including their supports, which transports liquids or gas over distance.</rdfs:comment>
    <rdf:type rdf:resource="http://www.w3.org/2002/07/owl#Class"/>
  </rdf:Description>
  <rdf:Description rdf:about="#MARITIME-EQUIPMENT-TYPE_Sweep">
    <rdfs:subClassOf rdf:resource="jc3iedm_OBJECT-TYPE.owl#MARITIME-EQUIPMENT-TYPE"/>
    <rdfs:label xml:lang="en">sweep</rdfs:label>
    <rdfs:comment xml:lang="en">Equipment designed to be employed in minesweeping operations.</rdfs:comment>
    <rdf:type rdf:resource="http://www.w3.org/2002/07/owl#Class"/>
  </rdf:Description>
  <rdf:Description rdf:about="#AMMUNITION-TYPE_Small-arms_ammunition">
    <rdfs:subClassOf rdf:resource="jc3iedm_OBJECT-TYPE.owl#AMMUNITION-TYPE"/>
    <rdfs:label xml:lang="en">small arms ammunition</rdfs:label>
    <rdfs:comment xml:lang="en">Ammunition designed for hand held weapons.</rdfs:comment>
    <rdf:type rdf:resource="http://www.w3.org/2002/07/owl#Class"/>
  </rdf:Description>
  <rdf:Description rdf:about="#MILITARY-OBSTACLE-TYPE_Not_otherwise_specified">
    <rdfs:subClassOf rdf:resource="jc3iedm_OBJECT-TYPE.owl#MILITARY-OBSTACLE-TYPE"/>
    <rdfs:label xml:lang="en">not otherwise specified</rdfs:label>
    <rdfs:comment xml:lang="en">The appropriate value is not in the set of specified values.</rdfs:comment>
    <rdf:type rdf:resource="http://www.w3.org/2002/07/owl#Class"/>
  </rdf:Description>
  <rdf:Description rdf:about="jc3iedm_OBJECT-TYPE.owl#materiel-type-reportable-item-text">
    <rdf:type rdf:resource="http://www.w3.org/2002/07/owl#DatatypeProperty"/>
    <rdfs:domain rdf:resource="jc3iedm_OBJECT-TYPE.owl#MATERIEL-TYPE"/>
    <rdfs:range rdf:resource="http://www.w3.org/2001/XMLSchema#string"/>
  </rdf:Description>
  <rdf:Description rdf:about="#CONTROL-FEATURE-TYPE_Targeted_area_of_interest">
    <rdfs:subClassOf rdf:resource="jc3iedm_OBJECT-TYPE.owl#CONTROL-FEATURE-TYPE"/>
    <rdfs:label xml:lang="en">targeted area of interest</rdfs:label>
    <rdfs:comment xml:lang="en">The geographical area or point along a mobility corridor the successful interdiction of which will cause an enemy to either abandon a particular course of action or require him to use specialized engineer support to continue and where he can be acquired and engaged by friendly forces. Not all TAI will form part of the friendly COA; only TAI associated with higher payoff targets (HTP) are of interest to the staff. These are identified during staff planning and wargaming. TAI differ from engagement areas in degree. Engagement areas plan for the use of all available weapons; TAI might be engaged by a single weapon.</rdfs:comment>
    <rdf:type rdf:resource="http://www.w3.org/2002/07/owl#Class"/>
  </rdf:Description>
  <rdf:Description rdf:about="#ENGINEERING-EQUIPMENT-TYPE_Mine-detection">
    <rdfs:subClassOf rdf:resource="jc3iedm_OBJECT-TYPE.owl#ENGINEERING-EQUIPMENT-TYPE"/>
    <rdfs:label xml:lang="en">mine detection</rdfs:label>
    <rdfs:comment xml:lang="en">An equipment whose purpose is to detect the presence of mines.</rdfs:comment>
    <rdf:type rdf:resource="http://www.w3.org/2002/07/owl#Class"/>
  </rdf:Description>
  <rdf:Description rdf:about="#FACILITY-TYPE_Fortification">
    <rdfs:subClassOf rdf:resource="jc3iedm_OBJECT-TYPE.owl#FACILITY-TYPE"/>
    <rdfs:label xml:lang="en">fortification</rdfs:label>
    <rdfs:comment xml:lang="en">An emplacement or shelter of a temporary or permanent nature constructed for defence by forces for protection of forces.</rdfs:comment>
    <rdf:type rdf:resource="http://www.w3.org/2002/07/owl#Class"/>
  </rdf:Description>
  <rdf:Description rdf:about="#AMMUNITION-TYPE_Mine,_moored">
    <rdfs:subClassOf rdf:resource="jc3iedm_OBJECT-TYPE.owl#AMMUNITION-TYPE"/>
    <rdfs:label xml:lang="en">mine, moored</rdfs:label>
    <rdfs:comment xml:lang="en">A contact or influence-operated mine of positive buoyancy held below the surface by a mooring attached to a sinker or anchor on the bottom.</rdfs:comment>
    <rdf:type rdf:resource="http://www.w3.org/2002/07/owl#Class"/>
  </rdf:Description>
  <rdf:Description rdf:about="#VEHICLE-TYPE_Bicycle">
    <rdfs:subClassOf rdf:resource="jc3iedm_OBJECT-TYPE.owl#VEHICLE-TYPE"/>
    <rdfs:label xml:lang="en">bicycle</rdfs:label>
    <rdfs:comment xml:lang="en">A vehicle of two wheels held in a frame one behind the other, propelled by pedals and steered with handlebars attached to the front wheel.</rdfs:comment>
    <rdf:type rdf:resource="http://www.w3.org/2002/07/owl#Class"/>
  </rdf:Description>
  <rdf:Description rdf:about="#SURFACE-VESSEL-TYPE_Hovercraft,_transport_cargo">
    <rdfs:subClassOf rdf:resource="jc3iedm_OBJECT-TYPE.owl#SURFACE-VESSEL-TYPE"/>
    <rdfs:label xml:lang="en">hovercraft, transport cargo</rdfs:label>
    <rdfs:comment xml:lang="en">Hovercraft capable of carrying vehicles and cargo. Not fitted to carry passengers.</rdfs:comment>
    <rdf:type rdf:resource="http://www.w3.org/2002/07/owl#Class"/>
  </rdf:Description>
  <rdf:Description rdf:about="#FACILITY-TYPE_Site,_logistic">
    <rdfs:subClassOf rdf:resource="jc3iedm_OBJECT-TYPE.owl#FACILITY-TYPE"/>
    <rdfs:label xml:lang="en">site, logistic</rdfs:label>
    <rdfs:comment xml:lang="en">A facility for the storage, maintenance, research, or disposal of material.</rdfs:comment>
    <rdf:type rdf:resource="http://www.w3.org/2002/07/owl#Class"/>
  </rdf:Description>
  <rdf:Description rdf:about="#CONTROL-FEATURE-TYPE_Predicted_impact_point">
    <rdfs:subClassOf rdf:resource="jc3iedm_OBJECT-TYPE.owl#CONTROL-FEATURE-TYPE"/>
    <rdfs:label xml:lang="en">predicted impact point</rdfs:label>
    <rdfs:comment xml:lang="en">The point at which a projectile, bomb or re-entry vehicle is expected to strike on earth.</rdfs:comment>
    <rdf:type rdf:resource="http://www.w3.org/2002/07/owl#Class"/>
  </rdf:Description>
  <rdf:Description rdf:about="#CONTROL-FEATURE-TYPE_Line_of_contact">
    <rdfs:subClassOf rdf:resource="jc3iedm_OBJECT-TYPE.owl#CONTROL-FEATURE-TYPE"/>
    <rdfs:label xml:lang="en">line of contact</rdfs:label>
    <rdfs:comment xml:lang="en">The designation of forward friendly positions as the LD when opposing forces are in contact.</rdfs:comment>
    <rdf:type rdf:resource="http://www.w3.org/2002/07/owl#Class"/>
  </rdf:Description>
  <rdf:Description rdf:about="#FACILITY-TYPE_Equipment,_manufacture">
    <rdfs:subClassOf rdf:resource="jc3iedm_OBJECT-TYPE.owl#FACILITY-TYPE"/>
    <rdfs:label xml:lang="en">equipment, manufacture</rdfs:label>
    <rdfs:comment xml:lang="en">A facility generally used specifically to support the manufacture of equipment.</rdfs:comment>
    <rdf:type rdf:resource="http://www.w3.org/2002/07/owl#Class"/>
  </rdf:Description>
  <rdf:Description rdf:about="#SURFACE-VESSEL-TYPE_Stores_ship,_small_(naval)">
    <rdfs:subClassOf rdf:resource="jc3iedm_OBJECT-TYPE.owl#SURFACE-VESSEL-TYPE"/>
    <rdfs:label xml:lang="en">stores ship, small (naval)</rdfs:label>
    <rdfs:comment xml:lang="en">Ship under 60 metres capable of underway replenishment of ships with refrigerated and dry provisions. May carry ammunition and POL but main emphasis is on dry provisions.</rdfs:comment>
    <rdf:type rdf:resource="http://www.w3.org/2002/07/owl#Class"/>
  </rdf:Description>
  <rdf:Description rdf:about="#FACILITY-TYPE_Military_materiel_facility,_missile_and_space_system_production">
    <rdfs:subClassOf rdf:resource="jc3iedm_OBJECT-TYPE.owl#FACILITY-TYPE"/>
    <rdfs:label xml:lang="en">military materiel facility, missile and space system production</rdfs:label>
    <rdfs:comment xml:lang="en">A facility used as for missile and space system production.</rdfs:comment>
    <rdf:type rdf:resource="http://www.w3.org/2002/07/owl#Class"/>
  </rdf:Description>
  <rdf:Description rdf:about="#FACILITY-TYPE_Military_materiel_facility,_atomic_energy_reactor">
    <rdfs:subClassOf rdf:resource="jc3iedm_OBJECT-TYPE.owl#FACILITY-TYPE"/>
    <rdfs:label xml:lang="en">military materiel facility, atomic energy reactor</rdfs:label>
    <rdfs:comment xml:lang="en">A facility used as an atomic energy reactor.</rdfs:comment>
    <rdf:type rdf:resource="http://www.w3.org/2002/07/owl#Class"/>
  </rdf:Description>
  <rdf:Description rdf:about="#SURFACE-VESSEL-TYPE_Patrol_boat,_offshore">
    <rdfs:subClassOf rdf:resource="jc3iedm_OBJECT-TYPE.owl#SURFACE-VESSEL-TYPE"/>
    <rdfs:label xml:lang="en">patrol boat, offshore</rdfs:label>
    <rdfs:comment xml:lang="en">Coastal patrol unit in size 45-60 metres designed for use in offshore waters. May or may not be armed with guns.</rdfs:comment>
    <rdf:type rdf:resource="http://www.w3.org/2002/07/owl#Class"/>
  </rdf:Description>
  <rdf:Description rdf:about="#MILITARY-POST-TYPE_Alternative_JAAT_controller">
    <rdfs:subClassOf rdf:resource="jc3iedm_OBJECT-TYPE.owl#MILITARY-POST-TYPE"/>
    <rdfs:label xml:lang="en">alternative jaat controller</rdfs:label>
    <rdfs:comment xml:lang="en">A MILITARY-POST-TYPE that is identified as the designated alternate controller of a Joint Air Attack Team.</rdfs:comment>
    <rdf:type rdf:resource="http://www.w3.org/2002/07/owl#Class"/>
  </rdf:Description>
  <rdf:Description rdf:about="jc3iedm_OBJECT-TYPE.owl#object-type-category-code">
    <rdf:type rdf:resource="http://www.w3.org/2002/07/owl#DatatypeProperty"/>
    <rdfs:domain rdf:resource="jc3iedm_OBJECT-TYPE.owl#OBJECT-TYPE"/>
    <rdfs:range rdf:resource="http://www.w3.org/2001/XMLSchema#string"/>
  </rdf:Description>
  <rdf:Description rdf:about="jc3iedm_OBJECT-TYPE.owl#person-type-category-code">
    <rdf:type rdf:resource="http://www.w3.org/2002/07/owl#DatatypeProperty"/>
    <rdfs:domain rdf:resource="jc3iedm_OBJECT-TYPE.owl#PERSON-TYPE"/>
    <rdfs:range rdf:resource="http://www.w3.org/2001/XMLSchema#string"/>
  </rdf:Description>
  <rdf:Description rdf:about="#SURFACE-VESSEL-TYPE_Aviation_tender">
    <rdfs:subClassOf rdf:resource="jc3iedm_OBJECT-TYPE.owl#SURFACE-VESSEL-TYPE"/>
    <rdfs:label xml:lang="en">aviation tender</rdfs:label>
    <rdfs:comment xml:lang="en">General designator for vessels that have repair and support facilities for aircraft.</rdfs:comment>
    <rdf:type rdf:resource="http://www.w3.org/2002/07/owl#Class"/>
  </rdf:Description>
  <rdf:Description rdf:about="jc3iedm_OBJECT-TYPE.owl#VESSEL-TYPE">
    <rdf:type rdf:resource="http://www.w3.org/2002/07/owl#Class"/>
    <rdfs:label xml:lang="en">vessel type</rdfs:label>
    <rdfs:comment xml:lang="en">An EQUIPMENT-TYPE that is designed to operate on or under the water surface.</rdfs:comment>
    <rdfs:subClassOf rdf:resource="jc3iedm_OBJECT-TYPE.owl#EQUIPMENT-TYPE"/>
  </rdf:Description>
  <rdf:Description rdf:about="#SURFACE-VESSEL-TYPE_Aviation_logistic_support_ship">
    <rdfs:subClassOf rdf:resource="jc3iedm_OBJECT-TYPE.owl#SURFACE-VESSEL-TYPE"/>
    <rdfs:label xml:lang="en">aviation logistic support ship</rdfs:label>
    <rdfs:comment xml:lang="en">Large ship equipped to provide aviation logistic support.</rdfs:comment>
    <rdf:type rdf:resource="http://www.w3.org/2002/07/owl#Class"/>
  </rdf:Description>
  <rdf:Description rdf:about="#MARITIME-EQUIPMENT-TYPE_Towed_array_surveillance_system,_tactical">
    <rdfs:subClassOf rdf:resource="jc3iedm_OBJECT-TYPE.owl#MARITIME-EQUIPMENT-TYPE"/>
    <rdfs:label xml:lang="en">towed array surveillance system, tactical</rdfs:label>
    <rdfs:comment xml:lang="en">No definition provided in ADatP-3 Baseline 13.1 FFIRN/FUD 1434/1.</rdfs:comment>
    <rdf:type rdf:resource="http://www.w3.org/2002/07/owl#Class"/>
  </rdf:Description>
  <rdf:Description rdf:about="jc3iedm_OBJECT-TYPE.owl#person-type-subcategory-code">
    <rdf:type rdf:resource="http://www.w3.org/2002/07/owl#DatatypeProperty"/>
    <rdfs:domain rdf:resource="jc3iedm_OBJECT-TYPE.owl#PERSON-TYPE"/>
    <rdfs:range rdf:resource="http://www.w3.org/2001/XMLSchema#string"/>
  </rdf:Description>
  <rdf:Description rdf:about="#SURFACE-VESSEL-TYPE_Frigate,_guided_missile">
    <rdfs:subClassOf rdf:resource="jc3iedm_OBJECT-TYPE.owl#SURFACE-VESSEL-TYPE"/>
    <rdfs:label xml:lang="en">frigate, guided missile</rdfs:label>
    <rdfs:comment xml:lang="en">A frigate fitted with one or more force guided missile systems. A surface combatant in size range of about 75-150 metres. Fitted primarily to fulfil an ASW role.</rdfs:comment>
    <rdf:type rdf:resource="http://www.w3.org/2002/07/owl#Class"/>
  </rdf:Description>
  <rdf:Description rdf:about="#ENGINEERING-EQUIPMENT-TYPE_Ditcher">
    <rdfs:subClassOf rdf:resource="jc3iedm_OBJECT-TYPE.owl#ENGINEERING-EQUIPMENT-TYPE"/>
    <rdfs:label xml:lang="en">ditcher</rdfs:label>
    <rdfs:comment xml:lang="en">A machine used to make ditches.</rdfs:comment>
    <rdf:type rdf:resource="http://www.w3.org/2002/07/owl#Class"/>
  </rdf:Description>
  <rdf:Description rdf:about="jc3iedm_OBJECT-TYPE.owl#RAILCAR-TYPE">
    <rdf:type rdf:resource="http://www.w3.org/2002/07/owl#Class"/>
    <rdfs:label xml:lang="en">railcar type</rdfs:label>
    <rdfs:comment xml:lang="en">An EQUIPMENT-TYPE that is designed to operate on rail tracks.</rdfs:comment>
    <rdfs:subClassOf rdf:resource="jc3iedm_OBJECT-TYPE.owl#EQUIPMENT-TYPE"/>
  </rdf:Description>
  <rdf:Description rdf:about="#SURFACE-VESSEL-TYPE_Aircraft_carrier,_training">
    <rdfs:subClassOf rdf:resource="jc3iedm_OBJECT-TYPE.owl#SURFACE-VESSEL-TYPE"/>
    <rdfs:label xml:lang="en">aircraft carrier, training</rdfs:label>
    <rdfs:comment xml:lang="en">Designator for multi-role aircraft carriers used primarily in a training role.</rdfs:comment>
    <rdf:type rdf:resource="http://www.w3.org/2002/07/owl#Class"/>
  </rdf:Description>
  <rdf:Description rdf:about="#FACILITY-TYPE_Military_base/facility,_airport/airbase">
    <rdfs:subClassOf rdf:resource="jc3iedm_OBJECT-TYPE.owl#FACILITY-TYPE"/>
    <rdfs:label xml:lang="en">military base/facility, airport/airbase</rdfs:label>
    <rdfs:comment xml:lang="en">A facility that is used as a military base prepared for the accommodation, landing and takeoff of aircraft.</rdfs:comment>
    <rdf:type rdf:resource="http://www.w3.org/2002/07/owl#Class"/>
  </rdf:Description>
  <rdf:Description rdf:about="#FACILITY-TYPE_Cropland">
    <rdfs:subClassOf rdf:resource="jc3iedm_OBJECT-TYPE.owl#FACILITY-TYPE"/>
    <rdfs:label xml:lang="en">cropland</rdfs:label>
    <rdfs:comment xml:lang="en">An area that has been tilled for the planting of crops.</rdfs:comment>
    <rdf:type rdf:resource="http://www.w3.org/2002/07/owl#Class"/>
  </rdf:Description>
  <rdf:Description rdf:about="jc3iedm_OBJECT-TYPE.owl#object-type-decoy-indicator-code">
    <rdf:type rdf:resource="http://www.w3.org/2002/07/owl#DatatypeProperty"/>
    <rdfs:domain rdf:resource="jc3iedm_OBJECT-TYPE.owl#OBJECT-TYPE"/>
    <rdfs:range rdf:resource="http://www.w3.org/2001/XMLSchema#string"/>
  </rdf:Description>
  <rdf:Description rdf:about="#SURFACE-VESSEL-TYPE_Aircraft_carrier,_light,_guided_missile">
    <rdfs:subClassOf rdf:resource="jc3iedm_OBJECT-TYPE.owl#SURFACE-VESSEL-TYPE"/>
    <rdfs:label xml:lang="en">aircraft carrier, light, guided missile</rdfs:label>
    <rdfs:comment xml:lang="en">Designator for multi-role aircraft carriers, fitted with one or more force guided missile systems under a certain tonnage (tbd).</rdfs:comment>
    <rdf:type rdf:resource="http://www.w3.org/2002/07/owl#Class"/>
  </rdf:Description>
  <rdf:Description rdf:about="#SURFACE-VESSEL-TYPE_Minesweeper,_coastal,_training">
    <rdfs:subClassOf rdf:resource="jc3iedm_OBJECT-TYPE.owl#SURFACE-VESSEL-TYPE"/>
    <rdfs:label xml:lang="en">minesweeper, coastal, training</rdfs:label>
    <rdfs:comment xml:lang="en">Non-magnetic minesweeper between 40-70 metres, used primarily in a training role.</rdfs:comment>
    <rdf:type rdf:resource="http://www.w3.org/2002/07/owl#Class"/>
  </rdf:Description>
  <rdf:Description rdf:about="#MISCELLANEOUS-EQUIPMENT-TYPE_Photographic">
    <rdfs:subClassOf rdf:resource="jc3iedm_OBJECT-TYPE.owl#MISCELLANEOUS-EQUIPMENT-TYPE"/>
    <rdfs:label xml:lang="en">photographic</rdfs:label>
    <rdfs:comment xml:lang="en">Equipment associated with photography.</rdfs:comment>
    <rdf:type rdf:resource="http://www.w3.org/2002/07/owl#Class"/>
  </rdf:Description>
  <rdf:Description rdf:about="#SURFACE-VESSEL-TYPE_Amphibious_assault_ship,_beaching">
    <rdfs:subClassOf rdf:resource="jc3iedm_OBJECT-TYPE.owl#SURFACE-VESSEL-TYPE"/>
    <rdfs:label xml:lang="en">amphibious assault ship, beaching</rdfs:label>
    <rdfs:comment xml:lang="en">Amphibious ship designed for beaching operations.</rdfs:comment>
    <rdf:type rdf:resource="http://www.w3.org/2002/07/owl#Class"/>
  </rdf:Description>
  <rdf:Description rdf:about="#SURFACE-VESSEL-TYPE_Lighter,_ammunition">
    <rdfs:subClassOf rdf:resource="jc3iedm_OBJECT-TYPE.owl#SURFACE-VESSEL-TYPE"/>
    <rdfs:label xml:lang="en">lighter, ammunition</rdfs:label>
    <rdfs:comment xml:lang="en">Craft 40 metres or less used for transporting ammunition.</rdfs:comment>
    <rdf:type rdf:resource="http://www.w3.org/2002/07/owl#Class"/>
  </rdf:Description>
  <rdf:Description rdf:about="#SUBSURFACE-VESSEL-TYPE_Deep_submergence_vehicle">
    <rdfs:subClassOf rdf:resource="jc3iedm_OBJECT-TYPE.owl#SUBSURFACE-VESSEL-TYPE"/>
    <rdfs:label xml:lang="en">deep submergence vehicle</rdfs:label>
    <rdfs:comment xml:lang="en">Submersible designed to operate at great depth (more than 300 metres).</rdfs:comment>
    <rdf:type rdf:resource="http://www.w3.org/2002/07/owl#Class"/>
  </rdf:Description>
  <rdf:Description rdf:about="#ORGANISATION-TYPE_Tactical_air_control_party">
    <rdfs:subClassOf rdf:resource="jc3iedm_OBJECT-TYPE.owl#ORGANISATION-TYPE"/>
    <rdfs:label xml:lang="en">tactical air control party</rdfs:label>
    <rdfs:comment xml:lang="en">The ORGANISATION-TYPE that is an agency that provides assistance in the submission of pre-planned and immediate air support requests, as well as providing terminal control for supporting aircraft. It is an integral part of each combat unit from division down to battalion level and serves as an air advisor to each manoeuvre unit.</rdfs:comment>
    <rdf:type rdf:resource="http://www.w3.org/2002/07/owl#Class"/>
  </rdf:Description>
  <rdf:Description rdf:about="#CONTROL-FEATURE-TYPE_Smoke_target">
    <rdfs:subClassOf rdf:resource="jc3iedm_OBJECT-TYPE.owl#CONTROL-FEATURE-TYPE"/>
    <rdfs:label xml:lang="en">smoke target</rdfs:label>
    <rdfs:comment xml:lang="en">A line along which, or an area in which, fires with smoke bombs or rockets degrades temporarily the capability of enemy forces to see through.</rdfs:comment>
    <rdf:type rdf:resource="http://www.w3.org/2002/07/owl#Class"/>
  </rdf:Description>
  <rdf:Description rdf:about="#VEHICLE-TYPE_Combat_support_vehicle">
    <rdfs:subClassOf rdf:resource="jc3iedm_OBJECT-TYPE.owl#VEHICLE-TYPE"/>
    <rdfs:label xml:lang="en">combat support vehicle</rdfs:label>
    <rdfs:comment xml:lang="en">No definition provided in ADatP-3 Baseline 13.1 FFIRN/FUD 1650/6.</rdfs:comment>
    <rdf:type rdf:resource="http://www.w3.org/2002/07/owl#Class"/>
  </rdf:Description>
  <rdf:Description rdf:about="#CONTROL-FEATURE-TYPE_Missile_arc">
    <rdfs:subClassOf rdf:resource="jc3iedm_OBJECT-TYPE.owl#CONTROL-FEATURE-TYPE"/>
    <rdfs:label xml:lang="en">missile arc</rdfs:label>
    <rdfs:comment xml:lang="en">An area of arc subtending 10 degrees, or as large as ordered by the officer in tactical command (OTC), centred on the bearing of the target with a range that extends to the maximum range of the surface-to-air missile (SAM).</rdfs:comment>
    <rdf:type rdf:resource="http://www.w3.org/2002/07/owl#Class"/>
  </rdf:Description>
  <rdf:Description rdf:about="#FACILITY-TYPE_Production_complex,_petroleum">
    <rdfs:subClassOf rdf:resource="jc3iedm_OBJECT-TYPE.owl#FACILITY-TYPE"/>
    <rdfs:label xml:lang="en">production complex, petroleum</rdfs:label>
    <rdfs:comment xml:lang="en">A facility used for petroleum based products production.</rdfs:comment>
    <rdf:type rdf:resource="http://www.w3.org/2002/07/owl#Class"/>
  </rdf:Description>
  <rdf:Description rdf:about="#SURFACE-VESSEL-TYPE_Mine_countermeasures_vessels_support_ship_(tender)">
    <rdfs:subClassOf rdf:resource="jc3iedm_OBJECT-TYPE.owl#SURFACE-VESSEL-TYPE"/>
    <rdfs:label xml:lang="en">mine countermeasures vessels support ship (tender)</rdfs:label>
    <rdfs:comment xml:lang="en">A ship of any size employed primarily to furnish facilities and services for the support, repair and limited command of mine countermeasures vessels.</rdfs:comment>
    <rdf:type rdf:resource="http://www.w3.org/2002/07/owl#Class"/>
  </rdf:Description>
  <rdf:Description rdf:about="#SURFACE-VESSEL-TYPE_Experimental_weapon_testing_barge">
    <rdfs:subClassOf rdf:resource="jc3iedm_OBJECT-TYPE.owl#SURFACE-VESSEL-TYPE"/>
    <rdfs:label xml:lang="en">experimental weapon testing barge</rdfs:label>
    <rdfs:comment xml:lang="en">Barge used for experimental weapon testing.</rdfs:comment>
    <rdf:type rdf:resource="http://www.w3.org/2002/07/owl#Class"/>
  </rdf:Description>
  <rdf:Description rdf:about="#SURFACE-VESSEL-TYPE_Minehunter,_general">
    <rdfs:subClassOf rdf:resource="jc3iedm_OBJECT-TYPE.owl#SURFACE-VESSEL-TYPE"/>
    <rdfs:label xml:lang="en">minehunter, general</rdfs:label>
    <rdfs:comment xml:lang="en">Ship equipped with specific equipment to hunt mines.</rdfs:comment>
    <rdf:type rdf:resource="http://www.w3.org/2002/07/owl#Class"/>
  </rdf:Description>
  <rdf:Description rdf:about="#VEHICLE-TYPE_Firefighting">
    <rdfs:subClassOf rdf:resource="jc3iedm_OBJECT-TYPE.owl#VEHICLE-TYPE"/>
    <rdfs:label xml:lang="en">firefighting</rdfs:label>
    <rdfs:comment xml:lang="en">A large motor vehicle designed to carry fire-fighters and equipment to a fire and supports extinguishing operations.</rdfs:comment>
    <rdf:type rdf:resource="http://www.w3.org/2002/07/owl#Class"/>
  </rdf:Description>
  <rdf:Description rdf:about="#SURFACE-VESSEL-TYPE_Support_ship,_missile_range">
    <rdfs:subClassOf rdf:resource="jc3iedm_OBJECT-TYPE.owl#SURFACE-VESSEL-TYPE"/>
    <rdfs:label xml:lang="en">support ship, missile range</rdfs:label>
    <rdfs:comment xml:lang="en">Ship employed in missile range support operations.</rdfs:comment>
    <rdf:type rdf:resource="http://www.w3.org/2002/07/owl#Class"/>
  </rdf:Description>
  <rdf:Description rdf:about="jc3iedm_OBJECT-TYPE.owl#equipment-type-fuel-capacity-quantity">
    <rdf:type rdf:resource="http://www.w3.org/2002/07/owl#DatatypeProperty"/>
    <rdfs:domain rdf:resource="jc3iedm_OBJECT-TYPE.owl#EQUIPMENT-TYPE"/>
  </rdf:Description>
  <rdf:Description rdf:about="#UNIT-TYPE_Engineer">
    <rdfs:subClassOf rdf:resource="jc3iedm_OBJECT-TYPE.owl#UNIT-TYPE"/>
    <rdfs:label xml:lang="en">engineer</rdfs:label>
    <rdfs:comment xml:lang="en">A UNIT-TYPE whose principal designation is major construction, demolition, and extensive camouflage projects.</rdfs:comment>
    <rdf:type rdf:resource="http://www.w3.org/2002/07/owl#Class"/>
  </rdf:Description>
  <rdf:Description rdf:about="#WEAPON-TYPE_Not_known">
    <rdfs:subClassOf rdf:resource="jc3iedm_OBJECT-TYPE.owl#WEAPON-TYPE"/>
    <rdfs:label xml:lang="en">not known</rdfs:label>
    <rdfs:comment xml:lang="en">It is not possible to determine which value is most applicable.</rdfs:comment>
    <rdf:type rdf:resource="http://www.w3.org/2002/07/owl#Class"/>
  </rdf:Description>
  <rdf:Description rdf:about="#ORGANISATION-TYPE_Air_operations_coordination_centre">
    <rdfs:subClassOf rdf:resource="jc3iedm_OBJECT-TYPE.owl#ORGANISATION-TYPE"/>
    <rdfs:label xml:lang="en">air operations coordination centre</rdfs:label>
    <rdfs:comment xml:lang="en">The ORGANISATION-TYPE of a tactical air control system collocated with a corps headquarters or an appropriate land force headquarters, which coordinates and directs close air support and other tactical air support.</rdfs:comment>
    <rdf:type rdf:resource="http://www.w3.org/2002/07/owl#Class"/>
  </rdf:Description>
  <rdf:Description rdf:about="#CONTROL-FEATURE-TYPE_Approach_direction">
    <rdfs:subClassOf rdf:resource="jc3iedm_OBJECT-TYPE.owl#CONTROL-FEATURE-TYPE"/>
    <rdfs:label xml:lang="en">approach direction</rdfs:label>
    <rdfs:comment xml:lang="en">A CONTROL-FEATURE-TYPE that specifies approach directional details for takeoff and landing.</rdfs:comment>
    <rdf:type rdf:resource="http://www.w3.org/2002/07/owl#Class"/>
  </rdf:Description>
  <rdf:Description rdf:about="#AMMUNITION-TYPE_Torpedo">
    <rdfs:subClassOf rdf:resource="jc3iedm_OBJECT-TYPE.owl#AMMUNITION-TYPE"/>
    <rdfs:label xml:lang="en">torpedo</rdfs:label>
    <rdfs:comment xml:lang="en">A weapon for destroying ships by rupturing their hulls below the waterline.</rdfs:comment>
    <rdf:type rdf:resource="http://www.w3.org/2002/07/owl#Class"/>
  </rdf:Description>
  <rdf:Description rdf:about="#SURFACE-VESSEL-TYPE_Stores_ship_issue_(naval)">
    <rdfs:subClassOf rdf:resource="jc3iedm_OBJECT-TYPE.owl#SURFACE-VESSEL-TYPE"/>
    <rdfs:label xml:lang="en">stores ship issue (naval)</rdfs:label>
    <rdfs:comment xml:lang="en">Ship 40 metres or more used to provide supplies and services.</rdfs:comment>
    <rdf:type rdf:resource="http://www.w3.org/2002/07/owl#Class"/>
  </rdf:Description>
  <rdf:Description rdf:about="#SURFACE-VESSEL-TYPE_Cruiser,_general">
    <rdfs:subClassOf rdf:resource="jc3iedm_OBJECT-TYPE.owl#SURFACE-VESSEL-TYPE"/>
    <rdfs:label xml:lang="en">cruiser, general</rdfs:label>
    <rdfs:comment xml:lang="en">General designator for all cruiser type ships of 140 metres or more. A fast warship of medium tonnage with a long cruising radius and les firepower and armour than a battleship.</rdfs:comment>
    <rdf:type rdf:resource="http://www.w3.org/2002/07/owl#Class"/>
  </rdf:Description>
  <rdf:Description rdf:about="#ROUTE-TYPE_Rhumb_line_route">
    <rdfs:subClassOf rdf:resource="jc3iedm_OBJECT-TYPE.owl#ROUTE-TYPE"/>
    <rdfs:label xml:lang="en">rhumb line route</rdfs:label>
    <rdfs:comment xml:lang="en">The route that maintains a constant direction, shown on a map as a line crossing all meridians at the same angle.</rdfs:comment>
    <rdf:type rdf:resource="http://www.w3.org/2002/07/owl#Class"/>
  </rdf:Description>
  <rdf:Description rdf:about="#SURFACE-VESSEL-TYPE_Aviation_tender,_guided_missile_support">
    <rdfs:subClassOf rdf:resource="jc3iedm_OBJECT-TYPE.owl#SURFACE-VESSEL-TYPE"/>
    <rdfs:label xml:lang="en">aviation tender, guided missile support</rdfs:label>
    <rdfs:comment xml:lang="en">Ship with supply and support facilities for airborne guided missiles.</rdfs:comment>
    <rdf:type rdf:resource="http://www.w3.org/2002/07/owl#Class"/>
  </rdf:Description>
  <rdf:Description rdf:about="jc3iedm_OBJECT-TYPE.owl#person-type-rank-code">
    <rdf:type rdf:resource="http://www.w3.org/2002/07/owl#DatatypeProperty"/>
    <rdfs:domain rdf:resource="jc3iedm_OBJECT-TYPE.owl#PERSON-TYPE"/>
    <rdfs:range rdf:resource="http://www.w3.org/2001/XMLSchema#string"/>
  </rdf:Description>
  <rdf:Description rdf:about="#CONTROL-FEATURE-TYPE_Buffer_zone">
    <rdfs:subClassOf rdf:resource="jc3iedm_OBJECT-TYPE.owl#CONTROL-FEATURE-TYPE"/>
    <rdfs:label xml:lang="en">buffer zone</rdfs:label>
    <rdfs:comment xml:lang="en">Airspace designed specifically to provide a buffer between various airspace control measures.</rdfs:comment>
    <rdf:type rdf:resource="http://www.w3.org/2002/07/owl#Class"/>
  </rdf:Description>
  <rdf:Description rdf:about="#AMMUNITION-TYPE_Anti-tank_guided_weapon">
    <rdfs:subClassOf rdf:resource="jc3iedm_OBJECT-TYPE.owl#AMMUNITION-TYPE"/>
    <rdfs:label xml:lang="en">anti tank guided weapon</rdfs:label>
    <rdfs:comment xml:lang="en">A guided weapon designed to immobilise or destroy a tank.</rdfs:comment>
    <rdf:type rdf:resource="http://www.w3.org/2002/07/owl#Class"/>
  </rdf:Description>
  <rdf:Description rdf:about="#VESSEL-TYPE_Unclassified_miscellaneous_unit">
    <rdfs:subClassOf rdf:resource="jc3iedm_OBJECT-TYPE.owl#VESSEL-TYPE"/>
    <rdfs:label xml:lang="en">unclassified miscellaneous unit</rdfs:label>
    <rdfs:comment xml:lang="en">Ship, vessel or craft whose designation has not been classified.</rdfs:comment>
    <rdf:type rdf:resource="http://www.w3.org/2002/07/owl#Class"/>
  </rdf:Description>
  <rdf:Description rdf:about="#FACILITY-TYPE_Military_base/facility,_army">
    <rdfs:subClassOf rdf:resource="jc3iedm_OBJECT-TYPE.owl#FACILITY-TYPE"/>
    <rdfs:label xml:lang="en">military base/facility, army</rdfs:label>
    <rdfs:comment xml:lang="en">A facility that is used as a military base by the army.</rdfs:comment>
    <rdf:type rdf:resource="http://www.w3.org/2002/07/owl#Class"/>
  </rdf:Description>
  <rdf:Description rdf:about="#SURFACE-VESSEL-TYPE_Service_craft,_miscellaneous">
    <rdfs:subClassOf rdf:resource="jc3iedm_OBJECT-TYPE.owl#SURFACE-VESSEL-TYPE"/>
    <rdfs:label xml:lang="en">service craft, miscellaneous</rdfs:label>
    <rdfs:comment xml:lang="en">Craft, usually under 40 metres overall employed in general or multi-purpose functions of support, training, R&amp;D or test in nature.</rdfs:comment>
    <rdf:type rdf:resource="http://www.w3.org/2002/07/owl#Class"/>
  </rdf:Description>
  <rdf:Description rdf:about="#GOVERNMENT-ORGANISATION-TYPE_International_civil/military">
    <rdfs:subClassOf rdf:resource="jc3iedm_OBJECT-TYPE.owl#GOVERNMENT-ORGANISATION-TYPE"/>
    <rdfs:label xml:lang="en">international civil/military</rdfs:label>
    <rdfs:comment xml:lang="en">A GOVERNMENT-ORGANISATION-TYPE that is officially involved in international affairs that include both civil and military elements.</rdfs:comment>
    <rdf:type rdf:resource="http://www.w3.org/2002/07/owl#Class"/>
  </rdf:Description>
  <rdf:Description rdf:about="#FACILITY-TYPE_Hut">
    <rdfs:subClassOf rdf:resource="jc3iedm_OBJECT-TYPE.owl#FACILITY-TYPE"/>
    <rdfs:label xml:lang="en">hut</rdfs:label>
    <rdfs:comment xml:lang="en">A small simple or crude house or shelter.</rdfs:comment>
    <rdf:type rdf:resource="http://www.w3.org/2002/07/owl#Class"/>
  </rdf:Description>
  <rdf:Description rdf:about="jc3iedm_OBJECT-TYPE.owl#biological-materiel-type-persistency-code">
    <rdf:type rdf:resource="http://www.w3.org/2002/07/owl#DatatypeProperty"/>
    <rdfs:domain rdf:resource="jc3iedm_OBJECT-TYPE.owl#BIOLOGICAL-MATERIEL-TYPE"/>
    <rdfs:range rdf:resource="http://www.w3.org/2001/XMLSchema#string"/>
  </rdf:Description>
  <rdf:Description rdf:about="#SURFACE-VESSEL-TYPE_Primary_casualty_receiving_ship">
    <rdfs:subClassOf rdf:resource="jc3iedm_OBJECT-TYPE.owl#SURFACE-VESSEL-TYPE"/>
    <rdfs:label xml:lang="en">primary casualty receiving ship</rdfs:label>
    <rdfs:comment xml:lang="en">Ship of at least 40 metres whose primary purpose is to provide 3rd line medical and surgical care. Not declared by ICRC/red crescent (TU ships only). May be armed and carrying secure communications.</rdfs:comment>
    <rdf:type rdf:resource="http://www.w3.org/2002/07/owl#Class"/>
  </rdf:Description>
  <rdf:Description rdf:about="#CONTROL-FEATURE-TYPE_Obstacle_line">
    <rdfs:subClassOf rdf:resource="jc3iedm_OBJECT-TYPE.owl#CONTROL-FEATURE-TYPE"/>
    <rdfs:label xml:lang="en">obstacle line</rdfs:label>
    <rdfs:comment xml:lang="en">A conceptual control measure used at battalion or brigade level to show placement intent without specifying a particular type of linear obstacle.</rdfs:comment>
    <rdf:type rdf:resource="http://www.w3.org/2002/07/owl#Class"/>
  </rdf:Description>
  <rdf:Description rdf:about="#SURFACE-VESSEL-TYPE_Landing_craft,_tank">
    <rdfs:subClassOf rdf:resource="jc3iedm_OBJECT-TYPE.owl#SURFACE-VESSEL-TYPE"/>
    <rdfs:label xml:lang="en">landing craft, tank</rdfs:label>
    <rdfs:comment xml:lang="en">Landing craft in size range 15-25 metres capable of carrying 1 tank or 50-200 troops. Must have landing ramp and is optimised for carrying and landing tanks and vehicles.</rdfs:comment>
    <rdf:type rdf:resource="http://www.w3.org/2002/07/owl#Class"/>
  </rdf:Description>
  <rdf:Description rdf:about="#CONTROL-FEATURE-TYPE_Silent_surface_to_air_missile_engagement_zone">
    <rdfs:subClassOf rdf:resource="jc3iedm_OBJECT-TYPE.owl#CONTROL-FEATURE-TYPE"/>
    <rdfs:label xml:lang="en">silent surface to air missile engagement zone</rdfs:label>
    <rdfs:comment xml:lang="en">Maritime MEZ designated area, promulgated in the OPTASK AAW message, within which the: (a) Ships remain covert, receiving the air picture via data links. (b) Ship Weapon Control Status is automatically "Weapons Free". (c) No friendly aircraft are allowed in the Maritime MEZ SSMEZ, except for airborne early warning (AEW) aircraft, anti-surface warfare (ASuW) aircraft and anti-submarine warfare (ASW) aircraft that are required to operate within this area, provided that the following criteria are met: 1. SAM ships be alerted to the mission. 2. Aircraft are kept under positive control. 3. Aircraft are being continuously tracked and their position transmitted via data link. 4. Gridlock between data link reporting unit and SAM ship is excellent. (d) No safety sectors are established in a Maritime MEZ SSMEZ.</rdfs:comment>
    <rdf:type rdf:resource="http://www.w3.org/2002/07/owl#Class"/>
  </rdf:Description>
  <rdf:Description rdf:about="#ENGINEERING-EQUIPMENT-TYPE_Construction">
    <rdfs:subClassOf rdf:resource="jc3iedm_OBJECT-TYPE.owl#ENGINEERING-EQUIPMENT-TYPE"/>
    <rdfs:label xml:lang="en">construction</rdfs:label>
    <rdfs:comment xml:lang="en">An equipment used to build a facility.</rdfs:comment>
    <rdf:type rdf:resource="http://www.w3.org/2002/07/owl#Class"/>
  </rdf:Description>
  <rdf:Description rdf:about="#UNIT-TYPE_Internal_security_forces">
    <rdfs:subClassOf rdf:resource="jc3iedm_OBJECT-TYPE.owl#UNIT-TYPE"/>
    <rdfs:label xml:lang="en">internal security forces</rdfs:label>
    <rdfs:comment xml:lang="en">A UNIT-TYPE whose principal designation is maintenance of a state of law and order prevailing within a nation.</rdfs:comment>
    <rdf:type rdf:resource="http://www.w3.org/2002/07/owl#Class"/>
  </rdf:Description>
  <rdf:Description rdf:about="#ROUTE-TYPE_Q-route">
    <rdfs:subClassOf rdf:resource="jc3iedm_OBJECT-TYPE.owl#ROUTE-TYPE"/>
    <rdfs:label xml:lang="en">q route</rdfs:label>
    <rdfs:comment xml:lang="en">A system of preplanned shipping lanes in mined or potentially mined waters used to minimize the area the mine countermeasures commander has to keep clear of mines in order to provide safe passage for friendly shipping.</rdfs:comment>
    <rdf:type rdf:resource="http://www.w3.org/2002/07/owl#Class"/>
  </rdf:Description>
  <rdf:Description rdf:about="#SURFACE-VESSEL-TYPE_Survey_ship,_coastal">
    <rdfs:subClassOf rdf:resource="jc3iedm_OBJECT-TYPE.owl#SURFACE-VESSEL-TYPE"/>
    <rdfs:label xml:lang="en">survey ship, coastal</rdfs:label>
    <rdfs:comment xml:lang="en">Ship 40 metres or more employed to conduct hydrographic and limited oceanographic surveys only in coastal and inshore waters.</rdfs:comment>
    <rdf:type rdf:resource="http://www.w3.org/2002/07/owl#Class"/>
  </rdf:Description>
  <rdf:Description rdf:about="#GROUP-ORGANISATION-TYPE_Media,_local">
    <rdfs:subClassOf rdf:resource="jc3iedm_OBJECT-TYPE.owl#GROUP-ORGANISATION-TYPE"/>
    <rdfs:label xml:lang="en">media, local</rdfs:label>
    <rdfs:comment xml:lang="en">A GROUP-ORGANISATION-TYPE that comprises persons that report for local mass communications, but do not take part in the actions.</rdfs:comment>
    <rdf:type rdf:resource="http://www.w3.org/2002/07/owl#Class"/>
  </rdf:Description>
  <rdf:Description rdf:about="#CONTROL-FEATURE-TYPE_Fire_support_coordination_line">
    <rdfs:subClassOf rdf:resource="jc3iedm_OBJECT-TYPE.owl#CONTROL-FEATURE-TYPE"/>
    <rdfs:label xml:lang="en">fire support coordination line</rdfs:label>
    <rdfs:comment xml:lang="en">A CONTROL-FEATURE-TYPE with an area location that is established and adjusted by appropriate land or amphibious force commanders within their boundaries in consultation with superior, subordinate, supporting, and affected commanders. Fire support coordination lines (FSCLs) facilitate the expeditious attack of surface targets of opportunity beyond the coordinating measure.</rdfs:comment>
    <rdf:type rdf:resource="http://www.w3.org/2002/07/owl#Class"/>
  </rdf:Description>
  <rdf:Description rdf:about="#ROUTE-TYPE_Unmanned_aerial_vehicle_route">
    <rdfs:subClassOf rdf:resource="jc3iedm_OBJECT-TYPE.owl#ROUTE-TYPE"/>
    <rdfs:label xml:lang="en">unmanned aerial vehicle route</rdfs:label>
    <rdfs:comment xml:lang="en">The CONTROL-FEATURE-TYPE that specifies a route along which an unmanned aerial vehicle travels.</rdfs:comment>
    <rdf:type rdf:resource="http://www.w3.org/2002/07/owl#Class"/>
  </rdf:Description>
  <rdf:Description rdf:about="#FACILITY-TYPE_NBC_observation_post_(dismounted)">
    <rdfs:subClassOf rdf:resource="jc3iedm_OBJECT-TYPE.owl#FACILITY-TYPE"/>
    <rdfs:label xml:lang="en">nbc observation post (dismounted)</rdfs:label>
    <rdfs:comment xml:lang="en">A facility from which chemical, biological, radiological, or nuclear observations are made and which possesses appropriate communications; it is dismounted.</rdfs:comment>
    <rdf:type rdf:resource="http://www.w3.org/2002/07/owl#Class"/>
  </rdf:Description>
  <rdf:Description rdf:about="#CONTROL-FEATURE-TYPE_Maritime_fighter_engagement_zone">
    <rdfs:subClassOf rdf:resource="jc3iedm_OBJECT-TYPE.owl#CONTROL-FEATURE-TYPE"/>
    <rdfs:label xml:lang="en">maritime fighter engagement zone</rdfs:label>
    <rdfs:comment xml:lang="en">The airspace beyond the crossover zone out to limits defined by the officer in tactical command, in which fighters have freedom of action to identify and engage air targets.</rdfs:comment>
    <rdf:type rdf:resource="http://www.w3.org/2002/07/owl#Class"/>
  </rdf:Description>
  <rdf:Description rdf:about="#SURFACE-VESSEL-TYPE_Patrol_combatant,_guided_missile,_air_cushion">
    <rdfs:subClassOf rdf:resource="jc3iedm_OBJECT-TYPE.owl#SURFACE-VESSEL-TYPE"/>
    <rdfs:label xml:lang="en">patrol combatant, guided missile, air cushion</rdfs:label>
    <rdfs:comment xml:lang="en">Patrol, blockade and surveillance ship in range 45-85 metres overall. Designed to operate in other than open ocean areas. Has special mission of attacking hostile ships. Must have at least 76mm main armament. It is fitted with one or more force guided missile systems and is either an air cushion or surface effect design.</rdfs:comment>
    <rdf:type rdf:resource="http://www.w3.org/2002/07/owl#Class"/>
  </rdf:Description>
  <rdf:Description rdf:about="#SURFACE-VESSEL-TYPE_Dry_dock_floating,_open,_large">
    <rdfs:subClassOf rdf:resource="jc3iedm_OBJECT-TYPE.owl#SURFACE-VESSEL-TYPE"/>
    <rdfs:label xml:lang="en">dry dock floating, open, large</rdfs:label>
    <rdfs:comment xml:lang="en">Non-self-propelled open-ended dry dock 200 metres or more.</rdfs:comment>
    <rdf:type rdf:resource="http://www.w3.org/2002/07/owl#Class"/>
  </rdf:Description>
  <rdf:Description rdf:about="#ROUTE-TYPE_Lateral_route">
    <rdfs:subClassOf rdf:resource="jc3iedm_OBJECT-TYPE.owl#ROUTE-TYPE"/>
    <rdfs:label xml:lang="en">lateral route</rdfs:label>
    <rdfs:comment xml:lang="en">A route generally parallel to the forward edge of the battle area, which crosses, or feeds into, axial routes.</rdfs:comment>
    <rdf:type rdf:resource="http://www.w3.org/2002/07/owl#Class"/>
  </rdf:Description>
  <rdf:Description rdf:about="#SURFACE-VESSEL-TYPE_Fishing_vessel,_general">
    <rdfs:subClassOf rdf:resource="jc3iedm_OBJECT-TYPE.owl#SURFACE-VESSEL-TYPE"/>
    <rdfs:label xml:lang="en">fishing vessel, general</rdfs:label>
    <rdfs:comment xml:lang="en">Fishing vessel over 30 metres.</rdfs:comment>
    <rdf:type rdf:resource="http://www.w3.org/2002/07/owl#Class"/>
  </rdf:Description>
  <rdf:Description rdf:about="#SURFACE-VESSEL-TYPE_Dry_dock_floating,_closed,_small">
    <rdfs:subClassOf rdf:resource="jc3iedm_OBJECT-TYPE.owl#SURFACE-VESSEL-TYPE"/>
    <rdfs:label xml:lang="en">dry dock floating, closed, small</rdfs:label>
    <rdfs:comment xml:lang="en">Non-self-propelled dry dock, closed bow and stern under 60 metres.</rdfs:comment>
    <rdf:type rdf:resource="http://www.w3.org/2002/07/owl#Class"/>
  </rdf:Description>
  <rdf:Description rdf:about="jc3iedm_OBJECT-TYPE.owl#ROUTE-TYPE">
    <rdf:type rdf:resource="http://www.w3.org/2002/07/owl#Class"/>
    <rdfs:label xml:lang="en">route type</rdfs:label>
    <rdfs:comment xml:lang="en">A CONTROL-FEATURE-TYPE that is the prescribed course to be travelled from a point of origin to a destination.</rdfs:comment>
    <rdfs:subClassOf rdf:resource="jc3iedm_OBJECT-TYPE.owl#CONTROL-FEATURE-TYPE"/>
  </rdf:Description>
  <rdf:Description rdf:about="#SURFACE-VESSEL-TYPE_Torpedo_retriever_craft">
    <rdfs:subClassOf rdf:resource="jc3iedm_OBJECT-TYPE.owl#SURFACE-VESSEL-TYPE"/>
    <rdfs:label xml:lang="en">torpedo retriever craft</rdfs:label>
    <rdfs:comment xml:lang="en">Craft used primarily to retrieve spent torpedoes during exercises. However may be armed and used as a harbour patrol craft as an auxiliary duty.</rdfs:comment>
    <rdf:type rdf:resource="http://www.w3.org/2002/07/owl#Class"/>
  </rdf:Description>
  <rdf:Description rdf:about="#CONSUMABLE-MATERIEL-TYPE_Food">
    <rdfs:subClassOf rdf:resource="jc3iedm_OBJECT-TYPE.owl#CONSUMABLE-MATERIEL-TYPE"/>
    <rdfs:label xml:lang="en">food</rdfs:label>
    <rdfs:comment xml:lang="en">Materiel to be used as nourishment in solid or liquid form.</rdfs:comment>
    <rdf:type rdf:resource="http://www.w3.org/2002/07/owl#Class"/>
  </rdf:Description>
  <rdf:Description rdf:about="jc3iedm_OBJECT-TYPE.owl#feature-type-category-code">
    <rdf:type rdf:resource="http://www.w3.org/2002/07/owl#DatatypeProperty"/>
    <rdfs:domain rdf:resource="jc3iedm_OBJECT-TYPE.owl#FEATURE-TYPE"/>
    <rdfs:range rdf:resource="http://www.w3.org/2001/XMLSchema#string"/>
  </rdf:Description>
  <rdf:Description rdf:about="#SURFACE-VESSEL-TYPE_Aircraft_ferry/cargo_ship">
    <rdfs:subClassOf rdf:resource="jc3iedm_OBJECT-TYPE.owl#SURFACE-VESSEL-TYPE"/>
    <rdfs:label xml:lang="en">aircraft ferry/cargo ship</rdfs:label>
    <rdfs:comment xml:lang="en">Ship at least 80 metres employed to transport general cargo and provisions. No underway replenishment facilities, employed to transport aircraft and aircraft spares.</rdfs:comment>
    <rdf:type rdf:resource="http://www.w3.org/2002/07/owl#Class"/>
  </rdf:Description>
  <rdf:Description rdf:about="#CONTROL-FEATURE-TYPE_Search_centre">
    <rdfs:subClassOf rdf:resource="jc3iedm_OBJECT-TYPE.owl#CONTROL-FEATURE-TYPE"/>
    <rdfs:label xml:lang="en">search centre</rdfs:label>
    <rdfs:comment xml:lang="en">A CONTROL-FEATURE-TYPE with a point location that specifies the centre point of a search area.</rdfs:comment>
    <rdf:type rdf:resource="http://www.w3.org/2002/07/owl#Class"/>
  </rdf:Description>
  <rdf:Description rdf:about="#AMMUNITION-TYPE_Maritime_mine_disposal_charge">
    <rdfs:subClassOf rdf:resource="jc3iedm_OBJECT-TYPE.owl#AMMUNITION-TYPE"/>
    <rdfs:label xml:lang="en">maritime mine disposal charge</rdfs:label>
    <rdfs:comment xml:lang="en">An explosive charge that is used to destroy a mine.</rdfs:comment>
    <rdf:type rdf:resource="http://www.w3.org/2002/07/owl#Class"/>
  </rdf:Description>
  <rdf:Description rdf:about="#FACILITY-TYPE_Communications_tower">
    <rdfs:subClassOf rdf:resource="jc3iedm_OBJECT-TYPE.owl#FACILITY-TYPE"/>
    <rdfs:label xml:lang="en">communications tower</rdfs:label>
    <rdfs:comment xml:lang="en">A relatively tall structure used for transmitting and/or receiving electronic communications signals.</rdfs:comment>
    <rdf:type rdf:resource="http://www.w3.org/2002/07/owl#Class"/>
  </rdf:Description>
  <rdf:Description rdf:about="#SURFACE-VESSEL-TYPE_Auxiliary_repair_dock">
    <rdfs:subClassOf rdf:resource="jc3iedm_OBJECT-TYPE.owl#SURFACE-VESSEL-TYPE"/>
    <rdfs:label xml:lang="en">auxiliary repair dock</rdfs:label>
    <rdfs:comment xml:lang="en">Dry dock with repair facilities for all ship sizes.</rdfs:comment>
    <rdf:type rdf:resource="http://www.w3.org/2002/07/owl#Class"/>
  </rdf:Description>
  <rdf:Description rdf:about="#MISCELLANEOUS-EQUIPMENT-TYPE_Aircraft_refuelling">
    <rdfs:subClassOf rdf:resource="jc3iedm_OBJECT-TYPE.owl#MISCELLANEOUS-EQUIPMENT-TYPE"/>
    <rdfs:label xml:lang="en">aircraft refuelling</rdfs:label>
    <rdfs:comment xml:lang="en">Equipment designed to facilitate aerial refuelling.</rdfs:comment>
    <rdf:type rdf:resource="http://www.w3.org/2002/07/owl#Class"/>
  </rdf:Description>
  <rdf:Description rdf:about="#SURFACE-VESSEL-TYPE_Merchant_ship,_roll-on,_roll-off_(ro/ro)">
    <rdfs:subClassOf rdf:resource="jc3iedm_OBJECT-TYPE.owl#SURFACE-VESSEL-TYPE"/>
    <rdfs:label xml:lang="en">merchant ship, roll on, roll off (ro/ro)</rdfs:label>
    <rdfs:comment xml:lang="en">Non-naval ship 40 metres or more, having capability for roll-on/roll-off cargo.</rdfs:comment>
    <rdf:type rdf:resource="http://www.w3.org/2002/07/owl#Class"/>
  </rdf:Description>
  <rdf:Description rdf:about="#FACILITY-TYPE_Depot,_NBC">
    <rdfs:subClassOf rdf:resource="jc3iedm_OBJECT-TYPE.owl#FACILITY-TYPE"/>
    <rdfs:label xml:lang="en">depot, nbc</rdfs:label>
    <rdfs:comment xml:lang="en">An area used for the storage of chemical, biological, radiological, or nuclear materiel.</rdfs:comment>
    <rdf:type rdf:resource="http://www.w3.org/2002/07/owl#Class"/>
  </rdf:Description>
  <rdf:Description rdf:about="#CONTROL-FEATURE-TYPE_Airspace_control_area">
    <rdfs:subClassOf rdf:resource="jc3iedm_OBJECT-TYPE.owl#CONTROL-FEATURE-TYPE"/>
    <rdfs:label xml:lang="en">airspace control area</rdfs:label>
    <rdfs:comment xml:lang="en">Airspace which is laterally defined by boundaries of the area of operations.</rdfs:comment>
    <rdf:type rdf:resource="http://www.w3.org/2002/07/owl#Class"/>
  </rdf:Description>
  <rdf:Description rdf:about="#FACILITY-TYPE_Jetty">
    <rdfs:subClassOf rdf:resource="jc3iedm_OBJECT-TYPE.owl#FACILITY-TYPE"/>
    <rdfs:label xml:lang="en">jetty</rdfs:label>
    <rdfs:comment xml:lang="en">A FACILITY-TYPE that is a platform that may be fixed or floating extending from a shore, normally attached to a wharf or the shore, and which allows access to a vessel lying alongside, used to secure, protect and provide landing and docking for vessels.</rdfs:comment>
    <rdf:type rdf:resource="http://www.w3.org/2002/07/owl#Class"/>
  </rdf:Description>
  <rdf:Description rdf:about="#SURFACE-VESSEL-TYPE_Missile_range_instrumentation_ship">
    <rdfs:subClassOf rdf:resource="jc3iedm_OBJECT-TYPE.owl#SURFACE-VESSEL-TYPE"/>
    <rdfs:label xml:lang="en">missile range instrumentation ship</rdfs:label>
    <rdfs:comment xml:lang="en">Ship employed at sea to provide telemetry and recover missiles.</rdfs:comment>
    <rdf:type rdf:resource="http://www.w3.org/2002/07/owl#Class"/>
  </rdf:Description>
  <rdf:Description rdf:about="#FACILITY-TYPE_Urban_area">
    <rdfs:subClassOf rdf:resource="jc3iedm_OBJECT-TYPE.owl#FACILITY-TYPE"/>
    <rdfs:label xml:lang="en">urban area</rdfs:label>
    <rdfs:comment xml:lang="en">A developed area, constituting, forming, or including a city, town, or burgh, or part of such.</rdfs:comment>
    <rdf:type rdf:resource="http://www.w3.org/2002/07/owl#Class"/>
  </rdf:Description>
  <rdf:Description rdf:about="#AMMUNITION-TYPE_Sea_mine">
    <rdfs:subClassOf rdf:resource="jc3iedm_OBJECT-TYPE.owl#AMMUNITION-TYPE"/>
    <rdfs:label xml:lang="en">sea mine</rdfs:label>
    <rdfs:comment xml:lang="en">An explosive device laid in the water with the intention of damaging or sinking ships or of deterring shipping from entering an area.</rdfs:comment>
    <rdf:type rdf:resource="http://www.w3.org/2002/07/owl#Class"/>
  </rdf:Description>
  <rdf:Description rdf:about="#SURFACE-VESSEL-TYPE_Barge,_gasoline">
    <rdfs:subClassOf rdf:resource="jc3iedm_OBJECT-TYPE.owl#SURFACE-VESSEL-TYPE"/>
    <rdfs:label xml:lang="en">barge, gasoline</rdfs:label>
    <rdfs:comment xml:lang="en">Craft 60 metres or less used to store and transport clean petroleum products.</rdfs:comment>
    <rdf:type rdf:resource="http://www.w3.org/2002/07/owl#Class"/>
  </rdf:Description>
  <rdf:Description rdf:about="#CONTROL-FEATURE-TYPE_Obstacle_free_area">
    <rdfs:subClassOf rdf:resource="jc3iedm_OBJECT-TYPE.owl#CONTROL-FEATURE-TYPE"/>
    <rdfs:label xml:lang="en">obstacle free area</rdfs:label>
    <rdfs:comment xml:lang="en">An area the commander designates as restricted from the emplacement of man-made obstacles, normally to facilitate future operations.</rdfs:comment>
    <rdf:type rdf:resource="http://www.w3.org/2002/07/owl#Class"/>
  </rdf:Description>
  <rdf:Description rdf:about="#SURFACE-VESSEL-TYPE_Lighter,_torpedo_transport">
    <rdfs:subClassOf rdf:resource="jc3iedm_OBJECT-TYPE.owl#SURFACE-VESSEL-TYPE"/>
    <rdfs:label xml:lang="en">lighter, torpedo transport</rdfs:label>
    <rdfs:comment xml:lang="en">Self-propelled craft 40 metres or less employed for transporting torpedoes.</rdfs:comment>
    <rdf:type rdf:resource="http://www.w3.org/2002/07/owl#Class"/>
  </rdf:Description>
  <rdf:Description rdf:about="#CONTROL-FEATURE-TYPE_Engagement_area">
    <rdfs:subClassOf rdf:resource="jc3iedm_OBJECT-TYPE.owl#CONTROL-FEATURE-TYPE"/>
    <rdfs:label xml:lang="en">engagement area</rdfs:label>
    <rdfs:comment xml:lang="en">An area where the commander intends to contain and destroy an enemy force with the massed fires of all available weapons and supporting systems.</rdfs:comment>
    <rdf:type rdf:resource="http://www.w3.org/2002/07/owl#Class"/>
  </rdf:Description>
  <rdf:Description rdf:about="#PRIVATE-SECTOR-ORGANISATION-TYPE_Trade">
    <rdfs:subClassOf rdf:resource="jc3iedm_OBJECT-TYPE.owl#PRIVATE-SECTOR-ORGANISATION-TYPE"/>
    <rdfs:label xml:lang="en">trade</rdfs:label>
    <rdfs:comment xml:lang="en">A PRIVATE-SECTOR-ORGANISATION-TYPE whose predominant business is trade in nature.</rdfs:comment>
    <rdf:type rdf:resource="http://www.w3.org/2002/07/owl#Class"/>
  </rdf:Description>
  <rdf:Description rdf:about="#CONTROL-FEATURE-TYPE_Strong_point">
    <rdfs:subClassOf rdf:resource="jc3iedm_OBJECT-TYPE.owl#CONTROL-FEATURE-TYPE"/>
    <rdfs:label xml:lang="en">strong point</rdfs:label>
    <rdfs:comment xml:lang="en">A defensive position, usually strongly fortified and heavily armed with automatic weapons around which other positions are grouped for its protection. Army--A position requiring extensive engineering effort for obstacles and survivability positions and positioned to control or block an avenue of approach. Normally, command and control, aid stations, and critical supply stockpiles will be dug-in with overhead protection. Trenches and other protective construction will be done to protect soldiers and weapons from damage during assault by mounted and dismounted forces.</rdfs:comment>
    <rdf:type rdf:resource="http://www.w3.org/2002/07/owl#Class"/>
  </rdf:Description>
  <rdf:Description rdf:about="#SUBSURFACE-VESSEL-TYPE_Submarine,_training">
    <rdfs:subClassOf rdf:resource="jc3iedm_OBJECT-TYPE.owl#SUBSURFACE-VESSEL-TYPE"/>
    <rdfs:label xml:lang="en">submarine, training</rdfs:label>
    <rdfs:comment xml:lang="en">Submarine used primarily in a training role but with at least a residual combat capability.</rdfs:comment>
    <rdf:type rdf:resource="http://www.w3.org/2002/07/owl#Class"/>
  </rdf:Description>
  <rdf:Description rdf:about="#SURFACE-VESSEL-TYPE_Patrol_boat,_fast">
    <rdfs:subClassOf rdf:resource="jc3iedm_OBJECT-TYPE.owl#SURFACE-VESSEL-TYPE"/>
    <rdfs:label xml:lang="en">patrol boat, fast</rdfs:label>
    <rdfs:comment xml:lang="en">Coastal patrol unit intended for a basically coastal guarding function. Includes any coastal patrol ship under 45 metres which cannot qualify as a PG in armament. May be unarmed and capable of at least 35 knots - 65 km/hr.</rdfs:comment>
    <rdf:type rdf:resource="http://www.w3.org/2002/07/owl#Class"/>
  </rdf:Description>
  <rdf:Description rdf:about="#FACILITY-TYPE_Medical_facility,_hospital">
    <rdfs:subClassOf rdf:resource="jc3iedm_OBJECT-TYPE.owl#FACILITY-TYPE"/>
    <rdfs:label xml:lang="en">medical facility, hospital</rdfs:label>
    <rdfs:comment xml:lang="en">A fixed medical treatment facility capable of providing inpatient care.</rdfs:comment>
    <rdf:type rdf:resource="http://www.w3.org/2002/07/owl#Class"/>
  </rdf:Description>
  <rdf:Description rdf:about="jc3iedm_OBJECT-TYPE.owl#CONTROL-FEATURE-TYPE">
    <rdf:type rdf:resource="http://www.w3.org/2002/07/owl#Class"/>
    <rdfs:label xml:lang="en">control feature type</rdfs:label>
    <rdfs:comment xml:lang="en">A non-tangible FEATURE-TYPE of military interest that may be represented as a geometric figure and is associated with the conduct of military operations.</rdfs:comment>
    <rdfs:subClassOf rdf:resource="jc3iedm_OBJECT-TYPE.owl#FEATURE-TYPE"/>
  </rdf:Description>
  <rdf:Description rdf:about="#UNIT-TYPE_Combat_service_support">
    <rdfs:subClassOf rdf:resource="jc3iedm_OBJECT-TYPE.owl#UNIT-TYPE"/>
    <rdfs:label xml:lang="en">combat service support</rdfs:label>
    <rdfs:comment xml:lang="en">A UNIT-TYPE tasked to provide support to combat forces, primarily in the fields of administration and logistics.</rdfs:comment>
    <rdf:type rdf:resource="http://www.w3.org/2002/07/owl#Class"/>
  </rdf:Description>
  <rdf:Description rdf:about="#SUBSURFACE-VESSEL-TYPE_Submarine,_attack,_guided_missile">
    <rdfs:subClassOf rdf:resource="jc3iedm_OBJECT-TYPE.owl#SUBSURFACE-VESSEL-TYPE"/>
    <rdfs:label xml:lang="en">submarine, attack, guided missile</rdfs:label>
    <rdfs:comment xml:lang="en">Submarine fitted with underwater to surface or surface-to-surface missiles.</rdfs:comment>
    <rdf:type rdf:resource="http://www.w3.org/2002/07/owl#Class"/>
  </rdf:Description>
  <rdf:Description rdf:about="#SURFACE-VESSEL-TYPE_Destroyer,_helicopter_capable">
    <rdfs:subClassOf rdf:resource="jc3iedm_OBJECT-TYPE.owl#SURFACE-VESSEL-TYPE"/>
    <rdfs:label xml:lang="en">destroyer, helicopter capable</rdfs:label>
    <rdfs:comment xml:lang="en">A destroyer type ship fitted with a flight deck with a primary mission of operating and maintaining helicopters. Major surface combatant in range of about 95 to 140 metres whole general mission is to conduct operations with strike, ASW and amphibious forces, and to perform screening and convoy duties. May have helicopters not especially fitted for ASW.</rdfs:comment>
    <rdf:type rdf:resource="http://www.w3.org/2002/07/owl#Class"/>
  </rdf:Description>
  <rdf:Description rdf:about="#AIRFIELD-TYPE_Military">
    <rdfs:subClassOf rdf:resource="jc3iedm_OBJECT-TYPE.owl#AIRFIELD-TYPE"/>
    <rdfs:label xml:lang="en">military</rdfs:label>
    <rdfs:comment xml:lang="en">Military airports controlled and operated by military authorities primarily used by military aircrafts although civil aircrafts may have landing privileges and/or contract rights.</rdfs:comment>
    <rdf:type rdf:resource="http://www.w3.org/2002/07/owl#Class"/>
  </rdf:Description>
  <rdf:Description rdf:about="#CONSUMABLE-MATERIEL-TYPE_Money">
    <rdfs:subClassOf rdf:resource="jc3iedm_OBJECT-TYPE.owl#CONSUMABLE-MATERIEL-TYPE"/>
    <rdfs:label xml:lang="en">money</rdfs:label>
    <rdfs:comment xml:lang="en">The official currency, coins and negotiable paper notes issued by a government.</rdfs:comment>
    <rdf:type rdf:resource="http://www.w3.org/2002/07/owl#Class"/>
  </rdf:Description>
  <rdf:Description rdf:about="#FACILITY-TYPE_Ammunition_transfer_point">
    <rdfs:subClassOf rdf:resource="jc3iedm_OBJECT-TYPE.owl#FACILITY-TYPE"/>
    <rdfs:label xml:lang="en">ammunition transfer point</rdfs:label>
    <rdfs:comment xml:lang="en">A facility for physical transfer of ammunition from one means of transport to another or to the final receiving unit.</rdfs:comment>
    <rdf:type rdf:resource="http://www.w3.org/2002/07/owl#Class"/>
  </rdf:Description>
  <rdf:Description rdf:about="#CONTROL-FEATURE-TYPE_Not_otherwise_specified">
    <rdfs:subClassOf rdf:resource="jc3iedm_OBJECT-TYPE.owl#CONTROL-FEATURE-TYPE"/>
    <rdfs:label xml:lang="en">not otherwise specified</rdfs:label>
    <rdfs:comment xml:lang="en">The appropriate value is not in the set of specified values.</rdfs:comment>
    <rdf:type rdf:resource="http://www.w3.org/2002/07/owl#Class"/>
  </rdf:Description>
  <rdf:Description rdf:about="#FACILITY-TYPE_Service,_research,_utility_facility">
    <rdfs:subClassOf rdf:resource="jc3iedm_OBJECT-TYPE.owl#FACILITY-TYPE"/>
    <rdfs:label xml:lang="en">service, research, utility facility</rdfs:label>
    <rdfs:comment xml:lang="en">A facility generally used to support service, research or utility functions.</rdfs:comment>
    <rdf:type rdf:resource="http://www.w3.org/2002/07/owl#Class"/>
  </rdf:Description>
  <rdf:Description rdf:about="#SURFACE-VESSEL-TYPE_Landing_craft,_personnel,_large">
    <rdfs:subClassOf rdf:resource="jc3iedm_OBJECT-TYPE.owl#SURFACE-VESSEL-TYPE"/>
    <rdfs:label xml:lang="en">landing craft, personnel, large</rdfs:label>
    <rdfs:comment xml:lang="en">11 metre landing control boat used primarily to control amphibious seaborne assault waves.</rdfs:comment>
    <rdf:type rdf:resource="http://www.w3.org/2002/07/owl#Class"/>
  </rdf:Description>
  <rdf:Description rdf:about="#CONTROL-FEATURE-TYPE_Forward_operating_location">
    <rdfs:subClassOf rdf:resource="jc3iedm_OBJECT-TYPE.owl#CONTROL-FEATURE-TYPE"/>
    <rdfs:label xml:lang="en">forward operating location</rdfs:label>
    <rdfs:comment xml:lang="en">An advanced position, usually of a temporary nature, from which air or ground units operate.</rdfs:comment>
    <rdf:type rdf:resource="http://www.w3.org/2002/07/owl#Class"/>
  </rdf:Description>
  <rdf:Description rdf:about="#SURFACE-VESSEL-TYPE_Service_craft,_target">
    <rdfs:subClassOf rdf:resource="jc3iedm_OBJECT-TYPE.owl#SURFACE-VESSEL-TYPE"/>
    <rdfs:label xml:lang="en">service craft, target</rdfs:label>
    <rdfs:comment xml:lang="en">Craft 45 metres or less employed as a target in support of gunnery or missile firing training.</rdfs:comment>
    <rdf:type rdf:resource="http://www.w3.org/2002/07/owl#Class"/>
  </rdf:Description>
  <rdf:Description rdf:about="#CBRN-EQUIPMENT-TYPE_Not_otherwise_specified">
    <rdfs:subClassOf rdf:resource="jc3iedm_OBJECT-TYPE.owl#CBRN-EQUIPMENT-TYPE"/>
    <rdfs:label xml:lang="en">not otherwise specified</rdfs:label>
    <rdfs:comment xml:lang="en">The appropriate value is not in the set of specified values.</rdfs:comment>
    <rdf:type rdf:resource="http://www.w3.org/2002/07/owl#Class"/>
  </rdf:Description>
  <rdf:Description rdf:about="jc3iedm_OBJECT-TYPE.owl#EXECUTIVE-MILITARY-ORGANISATION-TYPE">
    <rdf:type rdf:resource="http://www.w3.org/2002/07/owl#Class"/>
    <rdfs:label xml:lang="en">executive military organisation type</rdfs:label>
    <rdfs:comment xml:lang="en">A MILITARY-ORGANISATION-TYPE whose function is to manage and direct the military establishment.</rdfs:comment>
    <rdfs:subClassOf rdf:resource="jc3iedm_OBJECT-TYPE.owl#MILITARY-ORGANISATION-TYPE"/>
  </rdf:Description>
  <rdf:Description rdf:about="#SURFACE-VESSEL-TYPE_Catamaran">
    <rdfs:subClassOf rdf:resource="jc3iedm_OBJECT-TYPE.owl#SURFACE-VESSEL-TYPE"/>
    <rdfs:label xml:lang="en">catamaran</rdfs:label>
    <rdfs:comment xml:lang="en">Sail or engine powered vessel with twin hulls.</rdfs:comment>
    <rdf:type rdf:resource="http://www.w3.org/2002/07/owl#Class"/>
  </rdf:Description>
  <rdf:Description rdf:about="#PERSON-TYPE_Paramilitary">
    <rdfs:subClassOf rdf:resource="jc3iedm_OBJECT-TYPE.owl#PERSON-TYPE"/>
    <rdfs:label xml:lang="en">paramilitary</rdfs:label>
    <rdfs:comment xml:lang="en">A PERSON-TYPE who is a member of an irregular armed force.</rdfs:comment>
    <rdf:type rdf:resource="http://www.w3.org/2002/07/owl#Class"/>
  </rdf:Description>
  <rdf:Description rdf:about="jc3iedm_OBJECT-TYPE.owl#engineering-equipment-type-category-code">
    <rdf:type rdf:resource="http://www.w3.org/2002/07/owl#DatatypeProperty"/>
    <rdfs:domain rdf:resource="jc3iedm_OBJECT-TYPE.owl#ENGINEERING-EQUIPMENT-TYPE"/>
    <rdfs:range rdf:resource="http://www.w3.org/2001/XMLSchema#string"/>
  </rdf:Description>
  <rdf:Description rdf:about="#CONTROL-FEATURE-TYPE_High_altitude_missile_engagement_zone">
    <rdfs:subClassOf rdf:resource="jc3iedm_OBJECT-TYPE.owl#CONTROL-FEATURE-TYPE"/>
    <rdfs:label xml:lang="en">high altitude missile engagement zone</rdfs:label>
    <rdfs:comment xml:lang="en">The airspace of defined dimensions within which the responsibility for engagement of air threats normally rests with high-altitude surface-to-air missiles.</rdfs:comment>
    <rdf:type rdf:resource="http://www.w3.org/2002/07/owl#Class"/>
  </rdf:Description>
  <rdf:Description rdf:about="#SURFACE-VESSEL-TYPE_Fire/rescue_boat,_small">
    <rdfs:subClassOf rdf:resource="jc3iedm_OBJECT-TYPE.owl#SURFACE-VESSEL-TYPE"/>
    <rdfs:label xml:lang="en">fire/rescue boat, small</rdfs:label>
    <rdfs:comment xml:lang="en">Harbour craft extensively equipped for firefighting. For this type that capability is more important than horsepower alone. Must have several fire monitors.</rdfs:comment>
    <rdf:type rdf:resource="http://www.w3.org/2002/07/owl#Class"/>
  </rdf:Description>
  <rdf:Description rdf:about="#FACILITY-TYPE_Waste_pile">
    <rdfs:subClassOf rdf:resource="jc3iedm_OBJECT-TYPE.owl#FACILITY-TYPE"/>
    <rdfs:label xml:lang="en">waste pile</rdfs:label>
    <rdfs:comment xml:lang="en">Unusable or unwanted material, which may include hazardous materiel.</rdfs:comment>
    <rdf:type rdf:resource="http://www.w3.org/2002/07/owl#Class"/>
  </rdf:Description>
  <rdf:Description rdf:about="#SURFACE-VESSEL-TYPE_Floating_pile_driver">
    <rdfs:subClassOf rdf:resource="jc3iedm_OBJECT-TYPE.owl#SURFACE-VESSEL-TYPE"/>
    <rdfs:label xml:lang="en">floating pile driver</rdfs:label>
    <rdfs:comment xml:lang="en">Craft used as a pile driver.</rdfs:comment>
    <rdf:type rdf:resource="http://www.w3.org/2002/07/owl#Class"/>
  </rdf:Description>
  <rdf:Description rdf:about="#VEHICLE-TYPE_Special_purpose">
    <rdfs:subClassOf rdf:resource="jc3iedm_OBJECT-TYPE.owl#VEHICLE-TYPE"/>
    <rdfs:label xml:lang="en">special purpose</rdfs:label>
    <rdfs:comment xml:lang="en">A vehicle specifically designed for special use.</rdfs:comment>
    <rdf:type rdf:resource="http://www.w3.org/2002/07/owl#Class"/>
  </rdf:Description>
  <rdf:Description rdf:about="#TASK-FORMATION-TYPE_Naval_task_group">
    <rdfs:subClassOf rdf:resource="jc3iedm_OBJECT-TYPE.owl#TASK-FORMATION-TYPE"/>
    <rdfs:label xml:lang="en">naval task group</rdfs:label>
    <rdfs:comment xml:lang="en">A TASK-FORMATION-TYPE that is a component of a task force organized by the commander of the task force or higher authority for accomplishing specific tasks.</rdfs:comment>
    <rdf:type rdf:resource="http://www.w3.org/2002/07/owl#Class"/>
  </rdf:Description>
  <rdf:Description rdf:about="#FACILITY-TYPE_Vehicle_storage/parking_area">
    <rdfs:subClassOf rdf:resource="jc3iedm_OBJECT-TYPE.owl#FACILITY-TYPE"/>
    <rdfs:label xml:lang="en">vehicle storage/parking area</rdfs:label>
    <rdfs:comment xml:lang="en">An open land area used for storing or parking vehicles or vessels. (Including Recreational Vehicles).</rdfs:comment>
    <rdf:type rdf:resource="http://www.w3.org/2002/07/owl#Class"/>
  </rdf:Description>
  <rdf:Description rdf:about="#FACILITY-TYPE_High-technology_complex">
    <rdfs:subClassOf rdf:resource="jc3iedm_OBJECT-TYPE.owl#FACILITY-TYPE"/>
    <rdfs:label xml:lang="en">high technology complex</rdfs:label>
    <rdfs:comment xml:lang="en">A building or set of integrated buildings that use state-of-the-art-technology designed for a specific purpose such as manufacturing, research and development or other related activity.</rdfs:comment>
    <rdf:type rdf:resource="http://www.w3.org/2002/07/owl#Class"/>
  </rdf:Description>
  <rdf:Description rdf:about="#ORGANISATION-TYPE_Squadron_operations_centre">
    <rdfs:subClassOf rdf:resource="jc3iedm_OBJECT-TYPE.owl#ORGANISATION-TYPE"/>
    <rdfs:label xml:lang="en">squadron operations centre</rdfs:label>
    <rdfs:comment xml:lang="en">No definition provided in ADatP-3 Baseline 13.1 FFIRN/FUD 1874/4.</rdfs:comment>
    <rdf:type rdf:resource="http://www.w3.org/2002/07/owl#Class"/>
  </rdf:Description>
  <rdf:Description rdf:about="#SUBSURFACE-VESSEL-TYPE_Submersible,_rescue,_military">
    <rdfs:subClassOf rdf:resource="jc3iedm_OBJECT-TYPE.owl#SUBSURFACE-VESSEL-TYPE"/>
    <rdfs:label xml:lang="en">submersible, rescue, military</rdfs:label>
    <rdfs:comment xml:lang="en">Military operated submersible designed specifically for underwater rescue operations.</rdfs:comment>
    <rdf:type rdf:resource="http://www.w3.org/2002/07/owl#Class"/>
  </rdf:Description>
  <rdf:Description rdf:about="#SURFACE-VESSEL-TYPE_Craft,_torpedo_trials">
    <rdfs:subClassOf rdf:resource="jc3iedm_OBJECT-TYPE.owl#SURFACE-VESSEL-TYPE"/>
    <rdfs:label xml:lang="en">craft, torpedo trials</rdfs:label>
    <rdfs:comment xml:lang="en">Craft used at sea for torpedo trials.</rdfs:comment>
    <rdf:type rdf:resource="http://www.w3.org/2002/07/owl#Class"/>
  </rdf:Description>
  <rdf:Description rdf:about="#SURFACE-VESSEL-TYPE_Police_diving_tender">
    <rdfs:subClassOf rdf:resource="jc3iedm_OBJECT-TYPE.owl#SURFACE-VESSEL-TYPE"/>
    <rdfs:label xml:lang="en">police diving tender</rdfs:label>
    <rdfs:comment xml:lang="en">Police operated craft usually 40 metres or less equipped to provide support for divers.</rdfs:comment>
    <rdf:type rdf:resource="http://www.w3.org/2002/07/owl#Class"/>
  </rdf:Description>
  <rdf:Description rdf:about="#MISCELLANEOUS-EQUIPMENT-TYPE_Bottle">
    <rdfs:subClassOf rdf:resource="jc3iedm_OBJECT-TYPE.owl#MISCELLANEOUS-EQUIPMENT-TYPE"/>
    <rdfs:label xml:lang="en">bottle</rdfs:label>
    <rdfs:comment xml:lang="en">A container with a narrow neck, used for storing liquids, or a large metal cylinder holding liquefied gas.</rdfs:comment>
    <rdf:type rdf:resource="http://www.w3.org/2002/07/owl#Class"/>
  </rdf:Description>
  <rdf:Description rdf:about="#SURFACE-VESSEL-TYPE_Amphibious_ship,_general">
    <rdfs:subClassOf rdf:resource="jc3iedm_OBJECT-TYPE.owl#SURFACE-VESSEL-TYPE"/>
    <rdfs:label xml:lang="en">amphibious ship, general</rdfs:label>
    <rdfs:comment xml:lang="en">General designator for amphibious vessels.</rdfs:comment>
    <rdf:type rdf:resource="http://www.w3.org/2002/07/owl#Class"/>
  </rdf:Description>
  <rdf:Description rdf:about="#SURFACE-VESSEL-TYPE_Minesweeper,_drone">
    <rdfs:subClassOf rdf:resource="jc3iedm_OBJECT-TYPE.owl#SURFACE-VESSEL-TYPE"/>
    <rdfs:label xml:lang="en">minesweeper, drone</rdfs:label>
    <rdfs:comment xml:lang="en">Unmanned remotely controlled or towed vehicle capable of clearing mines.</rdfs:comment>
    <rdf:type rdf:resource="http://www.w3.org/2002/07/owl#Class"/>
  </rdf:Description>
  <rdf:Description rdf:about="#FACILITY-TYPE_Support_area">
    <rdfs:subClassOf rdf:resource="jc3iedm_OBJECT-TYPE.owl#FACILITY-TYPE"/>
    <rdfs:label xml:lang="en">support area</rdfs:label>
    <rdfs:comment xml:lang="en">A facility in which combat services support (CSS) elements and some staff elements locate to support a unit.</rdfs:comment>
    <rdf:type rdf:resource="http://www.w3.org/2002/07/owl#Class"/>
  </rdf:Description>
  <rdf:Description rdf:about="#CONSUMABLE-MATERIEL-TYPE_Flare">
    <rdfs:subClassOf rdf:resource="jc3iedm_OBJECT-TYPE.owl#CONSUMABLE-MATERIEL-TYPE"/>
    <rdfs:label xml:lang="en">flare</rdfs:label>
    <rdfs:comment xml:lang="en">A pyrotechnic munition producing a bright light for illumination or identification.</rdfs:comment>
    <rdf:type rdf:resource="http://www.w3.org/2002/07/owl#Class"/>
  </rdf:Description>
  <rdf:Description rdf:about="jc3iedm_OBJECT-TYPE.owl#aircraft-type-wing-span-dimension">
    <rdf:type rdf:resource="http://www.w3.org/2002/07/owl#DatatypeProperty"/>
    <rdfs:domain rdf:resource="jc3iedm_OBJECT-TYPE.owl#AIRCRAFT-TYPE"/>
  </rdf:Description>
  <rdf:Description rdf:about="#TASK-FORMATION-TYPE_Air_task_force">
    <rdfs:subClassOf rdf:resource="jc3iedm_OBJECT-TYPE.owl#TASK-FORMATION-TYPE"/>
    <rdfs:label xml:lang="en">air task force</rdfs:label>
    <rdfs:comment xml:lang="en">A temporary grouping of units, under one commander, formed for the purpose of carrying out a specific air operation or mission.</rdfs:comment>
    <rdf:type rdf:resource="http://www.w3.org/2002/07/owl#Class"/>
  </rdf:Description>
  <rdf:Description rdf:about="#FACILITY-TYPE_Worship_place">
    <rdfs:subClassOf rdf:resource="jc3iedm_OBJECT-TYPE.owl#FACILITY-TYPE"/>
    <rdfs:label xml:lang="en">worship place</rdfs:label>
    <rdfs:comment xml:lang="en">A building or open space where people assemble for religious purpose.</rdfs:comment>
    <rdf:type rdf:resource="http://www.w3.org/2002/07/owl#Class"/>
  </rdf:Description>
  <rdf:Description rdf:about="#RAILCAR-TYPE_Not_otherwise_specified">
    <rdfs:subClassOf rdf:resource="jc3iedm_OBJECT-TYPE.owl#RAILCAR-TYPE"/>
    <rdfs:label xml:lang="en">not otherwise specified</rdfs:label>
    <rdfs:comment xml:lang="en">The appropriate value is not in the set of specified values.</rdfs:comment>
    <rdf:type rdf:resource="http://www.w3.org/2002/07/owl#Class"/>
  </rdf:Description>
  <rdf:Description rdf:about="#SURFACE-VESSEL-TYPE_Warping_tug">
    <rdfs:subClassOf rdf:resource="jc3iedm_OBJECT-TYPE.owl#SURFACE-VESSEL-TYPE"/>
    <rdfs:label xml:lang="en">warping tug</rdfs:label>
    <rdfs:comment xml:lang="en">Tug used for warping ships in berths.</rdfs:comment>
    <rdf:type rdf:resource="http://www.w3.org/2002/07/owl#Class"/>
  </rdf:Description>
  <rdf:Description rdf:about="#FACILITY-TYPE_Observation_post">
    <rdfs:subClassOf rdf:resource="jc3iedm_OBJECT-TYPE.owl#FACILITY-TYPE"/>
    <rdfs:label xml:lang="en">observation post</rdfs:label>
    <rdfs:comment xml:lang="en">A facility from which military observations are made or fires directed and adjusted and which possesses appropriate communications; it may be airborne.</rdfs:comment>
    <rdf:type rdf:resource="http://www.w3.org/2002/07/owl#Class"/>
  </rdf:Description>
  <rdf:Description rdf:about="jc3iedm_OBJECT-TYPE.owl#military-post-type-rank-code">
    <rdf:type rdf:resource="http://www.w3.org/2002/07/owl#DatatypeProperty"/>
    <rdfs:domain rdf:resource="jc3iedm_OBJECT-TYPE.owl#MILITARY-POST-TYPE"/>
    <rdfs:range rdf:resource="http://www.w3.org/2001/XMLSchema#string"/>
  </rdf:Description>
  <rdf:Description rdf:about="#UNIT-TYPE_Supply">
    <rdfs:subClassOf rdf:resource="jc3iedm_OBJECT-TYPE.owl#UNIT-TYPE"/>
    <rdfs:label xml:lang="en">supply</rdfs:label>
    <rdfs:comment xml:lang="en">A UNIT-TYPE whose principal designation is the provision of all material and items used in the equipping, supporting and maintaining of military forces.</rdfs:comment>
    <rdf:type rdf:resource="http://www.w3.org/2002/07/owl#Class"/>
  </rdf:Description>
  <rdf:Description rdf:about="#CONTROL-FEATURE-TYPE_Logical_node">
    <rdfs:subClassOf rdf:resource="jc3iedm_OBJECT-TYPE.owl#CONTROL-FEATURE-TYPE"/>
    <rdfs:label xml:lang="en">logical node</rdfs:label>
    <rdfs:comment xml:lang="en">A CONTROL-FEATURE-TYPE that participates as a logical element in a communications network.</rdfs:comment>
    <rdf:type rdf:resource="http://www.w3.org/2002/07/owl#Class"/>
  </rdf:Description>
  <rdf:Description rdf:about="#SURFACE-VESSEL-TYPE_Mine_countermeasures_command_and_support">
    <rdfs:subClassOf rdf:resource="jc3iedm_OBJECT-TYPE.owl#SURFACE-VESSEL-TYPE"/>
    <rdfs:label xml:lang="en">mine countermeasures command and support</rdfs:label>
    <rdfs:comment xml:lang="en">An armed combatant fitted for the command and support of MCM vessels and their equipment.</rdfs:comment>
    <rdf:type rdf:resource="http://www.w3.org/2002/07/owl#Class"/>
  </rdf:Description>
  <rdf:Description rdf:about="#SURFACE-VESSEL-TYPE_Amphibious_assault_vehicle">
    <rdfs:subClassOf rdf:resource="jc3iedm_OBJECT-TYPE.owl#SURFACE-VESSEL-TYPE"/>
    <rdfs:label xml:lang="en">amphibious assault vehicle</rdfs:label>
    <rdfs:comment xml:lang="en">Wheeled vehicle designed to carry assault troops in amphibious operations.</rdfs:comment>
    <rdf:type rdf:resource="http://www.w3.org/2002/07/owl#Class"/>
  </rdf:Description>
  <rdf:Description rdf:about="#FACILITY-TYPE_Munitions_complex">
    <rdfs:subClassOf rdf:resource="jc3iedm_OBJECT-TYPE.owl#FACILITY-TYPE"/>
    <rdfs:label xml:lang="en">munitions complex</rdfs:label>
    <rdfs:comment xml:lang="en">A facility that could be used for munitions and explosives production or storage.</rdfs:comment>
    <rdf:type rdf:resource="http://www.w3.org/2002/07/owl#Class"/>
  </rdf:Description>
  <rdf:Description rdf:about="#CONTROL-FEATURE-TYPE_Area_of_interest">
    <rdfs:subClassOf rdf:resource="jc3iedm_OBJECT-TYPE.owl#CONTROL-FEATURE-TYPE"/>
    <rdfs:label xml:lang="en">area of interest</rdfs:label>
    <rdfs:comment xml:lang="en">A CONTROL-FEATURE-TYPE with an area location which denotes that area of concern to the commander, including the area of influence, and extending into enemy territory to the objectives of current or planned operations. This area also includes areas occupied by enemy forces that could jeopardise the accomplishment of the mission.</rdfs:comment>
    <rdf:type rdf:resource="http://www.w3.org/2002/07/owl#Class"/>
  </rdf:Description>
  <rdf:Description rdf:about="#CONTROL-FEATURE-TYPE_Restricted_operations_zone">
    <rdfs:subClassOf rdf:resource="jc3iedm_OBJECT-TYPE.owl#CONTROL-FEATURE-TYPE"/>
    <rdfs:label xml:lang="en">restricted operations zone</rdfs:label>
    <rdfs:comment xml:lang="en">A volume of airspace of defined dimensions designated for a specific operational mission. Entry into that zone is authorised only by the originating headquarters.</rdfs:comment>
    <rdf:type rdf:resource="http://www.w3.org/2002/07/owl#Class"/>
  </rdf:Description>
  <rdf:Description rdf:about="#SURFACE-VESSEL-TYPE_Barge,_heating">
    <rdfs:subClassOf rdf:resource="jc3iedm_OBJECT-TYPE.owl#SURFACE-VESSEL-TYPE"/>
    <rdfs:label xml:lang="en">barge, heating</rdfs:label>
    <rdfs:comment xml:lang="en">Craft of any size used to provide heat to moored ships or ship facilities.</rdfs:comment>
    <rdf:type rdf:resource="http://www.w3.org/2002/07/owl#Class"/>
  </rdf:Description>
  <rdf:Description rdf:about="#CONTROL-FEATURE-TYPE_Point_of_departure">
    <rdfs:subClassOf rdf:resource="jc3iedm_OBJECT-TYPE.owl#CONTROL-FEATURE-TYPE"/>
    <rdfs:label xml:lang="en">point of departure</rdfs:label>
    <rdfs:comment xml:lang="en">In night or limited visibility attacks, a specific place on the line of departure (LD) where a unit will cross.</rdfs:comment>
    <rdf:type rdf:resource="http://www.w3.org/2002/07/owl#Class"/>
  </rdf:Description>
  <rdf:Description rdf:about="jc3iedm_OBJECT-TYPE.owl#EQUIPMENT-TYPE">
    <rdf:type rdf:resource="http://www.w3.org/2002/07/owl#Class"/>
    <rdfs:label xml:lang="en">equipment type</rdfs:label>
    <rdfs:comment xml:lang="en">A MATERIEL-TYPE that is not intended for consumption.</rdfs:comment>
    <rdfs:subClassOf rdf:resource="jc3iedm_OBJECT-TYPE.owl#MATERIEL-TYPE"/>
  </rdf:Description>
  <rdf:Description rdf:about="#MISCELLANEOUS-EQUIPMENT-TYPE_Electronic_media,_detached_physical_storage">
    <rdfs:subClassOf rdf:resource="jc3iedm_OBJECT-TYPE.owl#MISCELLANEOUS-EQUIPMENT-TYPE"/>
    <rdfs:label xml:lang="en">electronic media, detached physical storage</rdfs:label>
    <rdfs:comment xml:lang="en">A discrete physical storage device (e.g., CD, DVD, USB stick, etc.).</rdfs:comment>
    <rdf:type rdf:resource="http://www.w3.org/2002/07/owl#Class"/>
  </rdf:Description>
  <rdf:Description rdf:about="#SURFACE-VESSEL-TYPE_Landing_craft,_personnel">
    <rdfs:subClassOf rdf:resource="jc3iedm_OBJECT-TYPE.owl#SURFACE-VESSEL-TYPE"/>
    <rdfs:label xml:lang="en">landing craft, personnel</rdfs:label>
    <rdfs:comment xml:lang="en">Landing craft in size range 7.5-30 metres overall suitable only for carrying personnel. May be fast and/or ramped.</rdfs:comment>
    <rdf:type rdf:resource="http://www.w3.org/2002/07/owl#Class"/>
  </rdf:Description>
  <rdf:Description rdf:about="#SURFACE-VESSEL-TYPE_Service_ship,_target">
    <rdfs:subClassOf rdf:resource="jc3iedm_OBJECT-TYPE.owl#SURFACE-VESSEL-TYPE"/>
    <rdfs:label xml:lang="en">service ship, target</rdfs:label>
    <rdfs:comment xml:lang="en">Ship employed in servicing surface targets.</rdfs:comment>
    <rdf:type rdf:resource="http://www.w3.org/2002/07/owl#Class"/>
  </rdf:Description>
  <rdf:Description rdf:about="#FACILITY-TYPE_Mine">
    <rdfs:subClassOf rdf:resource="jc3iedm_OBJECT-TYPE.owl#FACILITY-TYPE"/>
    <rdfs:label xml:lang="en">mine</rdfs:label>
    <rdfs:comment xml:lang="en">A facility where materials are extracted from the ground.</rdfs:comment>
    <rdf:type rdf:resource="http://www.w3.org/2002/07/owl#Class"/>
  </rdf:Description>
  <rdf:Description rdf:about="#ROUTE-TYPE_Usual_coastal_route">
    <rdfs:subClassOf rdf:resource="jc3iedm_OBJECT-TYPE.owl#ROUTE-TYPE"/>
    <rdfs:label xml:lang="en">usual coastal route</rdfs:label>
    <rdfs:comment xml:lang="en">The route that follows the shape or boundary of a coast.</rdfs:comment>
    <rdf:type rdf:resource="http://www.w3.org/2002/07/owl#Class"/>
  </rdf:Description>
  <rdf:Description rdf:about="#CONTROL-FEATURE-TYPE_Chemical_atmospheric_concentration_contour_line">
    <rdfs:subClassOf rdf:resource="jc3iedm_OBJECT-TYPE.owl#CONTROL-FEATURE-TYPE"/>
    <rdfs:label xml:lang="en">chemical atmospheric concentration contour line</rdfs:label>
    <rdfs:comment xml:lang="en">A line on a map, diagram or overlay joining all points at which the chemical atmospheric concentration at a given time is the same. Chemical atmospheric concentration is the mass of a chemical substance distributed in the atmosphere per unit volume.</rdfs:comment>
    <rdf:type rdf:resource="http://www.w3.org/2002/07/owl#Class"/>
  </rdf:Description>
  <rdf:Description rdf:about="#CONTROL-FEATURE-TYPE_Slow_go_area">
    <rdfs:subClassOf rdf:resource="jc3iedm_OBJECT-TYPE.owl#CONTROL-FEATURE-TYPE"/>
    <rdfs:label xml:lang="en">slow go area</rdfs:label>
    <rdfs:comment xml:lang="en">An area that is trafficable with difficulty.</rdfs:comment>
    <rdf:type rdf:resource="http://www.w3.org/2002/07/owl#Class"/>
  </rdf:Description>
  <rdf:Description rdf:about="#CONTROL-FEATURE-TYPE_Airfield_zone">
    <rdfs:subClassOf rdf:resource="jc3iedm_OBJECT-TYPE.owl#CONTROL-FEATURE-TYPE"/>
    <rdfs:label xml:lang="en">airfield zone</rdfs:label>
    <rdfs:comment xml:lang="en">A CONTROL-FEATURE-TYPE that approximates the location of the airspace of an airfield.</rdfs:comment>
    <rdf:type rdf:resource="http://www.w3.org/2002/07/owl#Class"/>
  </rdf:Description>
  <rdf:Description rdf:about="#FACILITY-TYPE_Transloading_facility">
    <rdfs:subClassOf rdf:resource="jc3iedm_OBJECT-TYPE.owl#FACILITY-TYPE"/>
    <rdfs:label xml:lang="en">transloading facility</rdfs:label>
    <rdfs:comment xml:lang="en">Enables transfer of materiel from one mode of transportation to another or between the same modes of transportation.</rdfs:comment>
    <rdf:type rdf:resource="http://www.w3.org/2002/07/owl#Class"/>
  </rdf:Description>
  <rdf:Description rdf:about="#AMMUNITION-TYPE_Mine,_deep_moored">
    <rdfs:subClassOf rdf:resource="jc3iedm_OBJECT-TYPE.owl#AMMUNITION-TYPE"/>
    <rdfs:label xml:lang="en">mine, deep moored</rdfs:label>
    <rdfs:comment xml:lang="en">Any mine case in more than a certain depth of water is deep.</rdfs:comment>
    <rdf:type rdf:resource="http://www.w3.org/2002/07/owl#Class"/>
  </rdf:Description>
  <rdf:Description rdf:about="#AMMUNITION-TYPE_Missile,_guided">
    <rdfs:subClassOf rdf:resource="jc3iedm_OBJECT-TYPE.owl#AMMUNITION-TYPE"/>
    <rdfs:label xml:lang="en">missile, guided</rdfs:label>
    <rdfs:comment xml:lang="en">An unmanned self-propelled vehicle whose trajectory or course, while in flight, is controlled.</rdfs:comment>
    <rdf:type rdf:resource="http://www.w3.org/2002/07/owl#Class"/>
  </rdf:Description>
  <rdf:Description rdf:about="#SURFACE-VESSEL-TYPE_Lighter,_covered,_refrigerated">
    <rdfs:subClassOf rdf:resource="jc3iedm_OBJECT-TYPE.owl#SURFACE-VESSEL-TYPE"/>
    <rdfs:label xml:lang="en">lighter, covered, refrigerated</rdfs:label>
    <rdfs:comment xml:lang="en">Refrigerated cargo transport craft 40 metres or less.</rdfs:comment>
    <rdf:type rdf:resource="http://www.w3.org/2002/07/owl#Class"/>
  </rdf:Description>
  <rdf:Description rdf:about="#SURFACE-VESSEL-TYPE_Merchant,_dredger">
    <rdfs:subClassOf rdf:resource="jc3iedm_OBJECT-TYPE.owl#SURFACE-VESSEL-TYPE"/>
    <rdfs:label xml:lang="en">merchant, dredger</rdfs:label>
    <rdfs:comment xml:lang="en">Non-naval ship designed to dredge channels in open seas.</rdfs:comment>
    <rdf:type rdf:resource="http://www.w3.org/2002/07/owl#Class"/>
  </rdf:Description>
  <rdf:Description rdf:about="#FACILITY-TYPE_Rail_facilities">
    <rdfs:subClassOf rdf:resource="jc3iedm_OBJECT-TYPE.owl#FACILITY-TYPE"/>
    <rdfs:label xml:lang="en">rail facilities</rdfs:label>
    <rdfs:comment xml:lang="en">An installation on a railway where loads may be transferred between trains and other means of transport.</rdfs:comment>
    <rdf:type rdf:resource="http://www.w3.org/2002/07/owl#Class"/>
  </rdf:Description>
  <rdf:Description rdf:about="#FACILITY-TYPE_Water_treatment_facility">
    <rdfs:subClassOf rdf:resource="jc3iedm_OBJECT-TYPE.owl#FACILITY-TYPE"/>
    <rdfs:label xml:lang="en">water treatment facility</rdfs:label>
    <rdfs:comment xml:lang="en">A facility used for the handling and treatment of water.</rdfs:comment>
    <rdf:type rdf:resource="http://www.w3.org/2002/07/owl#Class"/>
  </rdf:Description>
  <rdf:Description rdf:about="jc3iedm_OBJECT-TYPE.owl#consumable-materiel-type-hazard-code">
    <rdf:type rdf:resource="http://www.w3.org/2002/07/owl#DatatypeProperty"/>
    <rdfs:domain rdf:resource="jc3iedm_OBJECT-TYPE.owl#CONSUMABLE-MATERIEL-TYPE"/>
    <rdfs:range rdf:resource="http://www.w3.org/2001/XMLSchema#string"/>
  </rdf:Description>
  <rdf:Description rdf:about="jc3iedm_OBJECT-TYPE.owl#aircraft-type-weather-qualifier-code">
    <rdf:type rdf:resource="http://www.w3.org/2002/07/owl#DatatypeProperty"/>
    <rdfs:domain rdf:resource="jc3iedm_OBJECT-TYPE.owl#AIRCRAFT-TYPE"/>
    <rdfs:range rdf:resource="http://www.w3.org/2001/XMLSchema#string"/>
  </rdf:Description>
  <rdf:Description rdf:about="#SURFACE-VESSEL-TYPE_Cargo_ship,_roll-on_roll-off_(naval)">
    <rdfs:subClassOf rdf:resource="jc3iedm_OBJECT-TYPE.owl#SURFACE-VESSEL-TYPE"/>
    <rdfs:label xml:lang="en">cargo ship, roll on roll off (naval)</rdfs:label>
    <rdfs:comment xml:lang="en">Ship at least 40 metres overall designed to transport vehicles, guns and tanks in a non-combatant situation. Must have roll-on/roll-off capability for vehicles.</rdfs:comment>
    <rdf:type rdf:resource="http://www.w3.org/2002/07/owl#Class"/>
  </rdf:Description>
  <rdf:Description rdf:about="#CONTROL-FEATURE-TYPE_Landing_zone">
    <rdfs:subClassOf rdf:resource="jc3iedm_OBJECT-TYPE.owl#CONTROL-FEATURE-TYPE"/>
    <rdfs:label xml:lang="en">landing zone</rdfs:label>
    <rdfs:comment xml:lang="en">A specified area used for the landing of aircraft.</rdfs:comment>
    <rdf:type rdf:resource="http://www.w3.org/2002/07/owl#Class"/>
  </rdf:Description>
  <rdf:Description rdf:about="jc3iedm_OBJECT-TYPE.owl#unit-type-arm-category-code">
    <rdf:type rdf:resource="http://www.w3.org/2002/07/owl#DatatypeProperty"/>
    <rdfs:domain rdf:resource="jc3iedm_OBJECT-TYPE.owl#UNIT-TYPE"/>
    <rdfs:range rdf:resource="http://www.w3.org/2001/XMLSchema#string"/>
  </rdf:Description>
  <rdf:Description rdf:about="#CONTROL-FEATURE-TYPE_Restricted_operations_area">
    <rdfs:subClassOf rdf:resource="jc3iedm_OBJECT-TYPE.owl#CONTROL-FEATURE-TYPE"/>
    <rdfs:label xml:lang="en">restricted operations area</rdfs:label>
    <rdfs:comment xml:lang="en">Airspace designated by the airspace control authority, in response to specific operational situations/requirements within which the operation of one or more airspace users is restricted.</rdfs:comment>
    <rdf:type rdf:resource="http://www.w3.org/2002/07/owl#Class"/>
  </rdf:Description>
  <rdf:Description rdf:about="#CONTROL-FEATURE-TYPE_Site_of_alleged_kills">
    <rdfs:subClassOf rdf:resource="jc3iedm_OBJECT-TYPE.owl#CONTROL-FEATURE-TYPE"/>
    <rdfs:label xml:lang="en">site of alleged kills</rdfs:label>
    <rdfs:comment xml:lang="en">A CONTROL-FEATURE-TYPE that marks a point or area where alleged kills have occurred.</rdfs:comment>
    <rdf:type rdf:resource="http://www.w3.org/2002/07/owl#Class"/>
  </rdf:Description>
  <rdf:Description rdf:about="#SURFACE-VESSEL-TYPE_Landing_ship,_vehicle">
    <rdfs:subClassOf rdf:resource="jc3iedm_OBJECT-TYPE.owl#SURFACE-VESSEL-TYPE"/>
    <rdfs:label xml:lang="en">landing ship, vehicle</rdfs:label>
    <rdfs:comment xml:lang="en">Ship in size range 45-60 metres overall, intended primarily to carry vehicles. Must have bow doors and/or landing ramp. Not capable of beaching.</rdfs:comment>
    <rdf:type rdf:resource="http://www.w3.org/2002/07/owl#Class"/>
  </rdf:Description>
  <rdf:Description rdf:about="jc3iedm_OBJECT-TYPE.owl#vessel-type-dead-weight-quantity">
    <rdf:type rdf:resource="http://www.w3.org/2002/07/owl#DatatypeProperty"/>
    <rdfs:domain rdf:resource="jc3iedm_OBJECT-TYPE.owl#VESSEL-TYPE"/>
  </rdf:Description>
  <rdf:Description rdf:about="#CONTROL-FEATURE-TYPE_Forward_area_air_defence_zone">
    <rdfs:subClassOf rdf:resource="jc3iedm_OBJECT-TYPE.owl#CONTROL-FEATURE-TYPE"/>
    <rdfs:label xml:lang="en">forward area air defence zone</rdfs:label>
    <rdfs:comment xml:lang="en">An area of forward area air defence (FAAD) deployment that may fall within a missile engagement zone.</rdfs:comment>
    <rdf:type rdf:resource="http://www.w3.org/2002/07/owl#Class"/>
  </rdf:Description>
  <rdf:Description rdf:about="#WEAPON-TYPE_Anti-tank">
    <rdfs:subClassOf rdf:resource="jc3iedm_OBJECT-TYPE.owl#WEAPON-TYPE"/>
    <rdfs:label xml:lang="en">anti tank</rdfs:label>
    <rdfs:comment xml:lang="en">A weapon specifically designed for the engagement of armoured vehicles.</rdfs:comment>
    <rdf:type rdf:resource="http://www.w3.org/2002/07/owl#Class"/>
  </rdf:Description>
  <rdf:Description rdf:about="#ROUTE-TYPE_Advisory_route">
    <rdfs:subClassOf rdf:resource="jc3iedm_OBJECT-TYPE.owl#ROUTE-TYPE"/>
    <rdfs:label xml:lang="en">advisory route</rdfs:label>
    <rdfs:comment xml:lang="en">A designated route along which air traffic advisory service is available.</rdfs:comment>
    <rdf:type rdf:resource="http://www.w3.org/2002/07/owl#Class"/>
  </rdf:Description>
  <rdf:Description rdf:about="#ENGINEERING-EQUIPMENT-TYPE_Mine_clearer">
    <rdfs:subClassOf rdf:resource="jc3iedm_OBJECT-TYPE.owl#ENGINEERING-EQUIPMENT-TYPE"/>
    <rdfs:label xml:lang="en">mine clearer</rdfs:label>
    <rdfs:comment xml:lang="en">A vehicle whose purpose is to remove or destroy mines.</rdfs:comment>
    <rdf:type rdf:resource="http://www.w3.org/2002/07/owl#Class"/>
  </rdf:Description>
  <rdf:Description rdf:about="#CONTROL-FEATURE-TYPE_Air-to-air_refuelling_area">
    <rdfs:subClassOf rdf:resource="jc3iedm_OBJECT-TYPE.owl#CONTROL-FEATURE-TYPE"/>
    <rdfs:label xml:lang="en">air to air refuelling area</rdfs:label>
    <rdfs:comment xml:lang="en">Airspace of defined dimensions set aside for air-to-air refuelling operations, excluding special operation forces air-to-air missions.</rdfs:comment>
    <rdf:type rdf:resource="http://www.w3.org/2002/07/owl#Class"/>
  </rdf:Description>
  <rdf:Description rdf:about="#FACILITY-TYPE_Medical_facility,_hospital_field">
    <rdfs:subClassOf rdf:resource="jc3iedm_OBJECT-TYPE.owl#FACILITY-TYPE"/>
    <rdfs:label xml:lang="en">medical facility, hospital field</rdfs:label>
    <rdfs:comment xml:lang="en">A movable medical treatment facility capable of providing inpatient care.</rdfs:comment>
    <rdf:type rdf:resource="http://www.w3.org/2002/07/owl#Class"/>
  </rdf:Description>
  <rdf:Description rdf:about="#FACILITY-TYPE_Installation">
    <rdfs:subClassOf rdf:resource="jc3iedm_OBJECT-TYPE.owl#FACILITY-TYPE"/>
    <rdfs:label xml:lang="en">installation</rdfs:label>
    <rdfs:comment xml:lang="en">A grouping of facilities, located in the same vicinity, which support particular functions. Installations may be elements of a base.</rdfs:comment>
    <rdf:type rdf:resource="http://www.w3.org/2002/07/owl#Class"/>
  </rdf:Description>
  <rdf:Description rdf:about="#SURFACE-VESSEL-TYPE_Minehunter/sweeper,_coastal">
    <rdfs:subClassOf rdf:resource="jc3iedm_OBJECT-TYPE.owl#SURFACE-VESSEL-TYPE"/>
    <rdfs:label xml:lang="en">minehunter/sweeper, coastal</rdfs:label>
    <rdfs:comment xml:lang="en">A mine warfare craft equipped for both hunting and sweeping mines, limited to coastal waters.</rdfs:comment>
    <rdf:type rdf:resource="http://www.w3.org/2002/07/owl#Class"/>
  </rdf:Description>
  <rdf:Description rdf:about="#CONTROL-FEATURE-TYPE_Terminal_radar_service_area">
    <rdfs:subClassOf rdf:resource="jc3iedm_OBJECT-TYPE.owl#CONTROL-FEATURE-TYPE"/>
    <rdfs:label xml:lang="en">terminal radar service area</rdfs:label>
    <rdfs:comment xml:lang="en">Airspace surrounding designated airports wherein air traffic control provides radar vectoring, sequencing, and separation on a full-time basis for all instrument flight rule and participating visual flight rule aircraft.</rdfs:comment>
    <rdf:type rdf:resource="http://www.w3.org/2002/07/owl#Class"/>
  </rdf:Description>
  <rdf:Description rdf:about="#SURFACE-VESSEL-TYPE_Minesweeper,_boat">
    <rdfs:subClassOf rdf:resource="jc3iedm_OBJECT-TYPE.owl#SURFACE-VESSEL-TYPE"/>
    <rdfs:label xml:lang="en">minesweeper, boat</rdfs:label>
    <rdfs:comment xml:lang="en">Minesweeper less than 12.5 metres.</rdfs:comment>
    <rdf:type rdf:resource="http://www.w3.org/2002/07/owl#Class"/>
  </rdf:Description>
  <rdf:Description rdf:about="#GOVERNMENT-ORGANISATION-TYPE_Not_otherwise_specified">
    <rdfs:subClassOf rdf:resource="jc3iedm_OBJECT-TYPE.owl#GOVERNMENT-ORGANISATION-TYPE"/>
    <rdfs:label xml:lang="en">not otherwise specified</rdfs:label>
    <rdfs:comment xml:lang="en">The appropriate value is not in the set of specified values.</rdfs:comment>
    <rdf:type rdf:resource="http://www.w3.org/2002/07/owl#Class"/>
  </rdf:Description>
  <rdf:Description rdf:about="#ORGANISATION-TYPE_Forward_air_control_party">
    <rdfs:subClassOf rdf:resource="jc3iedm_OBJECT-TYPE.owl#ORGANISATION-TYPE"/>
    <rdfs:label xml:lang="en">forward air control party</rdfs:label>
    <rdfs:comment xml:lang="en">No definition provided in ADatP-3 Baseline 13.1 FFIRN/FUD 1395/5.</rdfs:comment>
    <rdf:type rdf:resource="http://www.w3.org/2002/07/owl#Class"/>
  </rdf:Description>
  <rdf:Description rdf:about="#SURFACE-VESSEL-TYPE_Repair_ship,_battle_damage">
    <rdfs:subClassOf rdf:resource="jc3iedm_OBJECT-TYPE.owl#SURFACE-VESSEL-TYPE"/>
    <rdfs:label xml:lang="en">repair ship, battle damage</rdfs:label>
    <rdfs:comment xml:lang="en">Ship of at least 120 metres or more employed as a mobile repair facility providing limited support to various types of ships. Not a lifting ship. Repair primary function, support secondary and optimised for repair of battle damage.</rdfs:comment>
    <rdf:type rdf:resource="http://www.w3.org/2002/07/owl#Class"/>
  </rdf:Description>
  <rdf:Description rdf:about="#SURFACE-VESSEL-TYPE_Mine_countermeasures_vessel,_diving">
    <rdfs:subClassOf rdf:resource="jc3iedm_OBJECT-TYPE.owl#SURFACE-VESSEL-TYPE"/>
    <rdfs:label xml:lang="en">mine countermeasures vessel, diving</rdfs:label>
    <rdfs:comment xml:lang="en">A mine countermeasures vessel specially equipped to carry out and support diving operations.</rdfs:comment>
    <rdf:type rdf:resource="http://www.w3.org/2002/07/owl#Class"/>
  </rdf:Description>
  <rdf:Description rdf:about="#CBRN-EQUIPMENT-TYPE_Biological_integrated_detector">
    <rdfs:subClassOf rdf:resource="jc3iedm_OBJECT-TYPE.owl#CBRN-EQUIPMENT-TYPE"/>
    <rdfs:label xml:lang="en">biological integrated detector</rdfs:label>
    <rdfs:comment xml:lang="en">An integrated biological detection, alarm, and identification system.</rdfs:comment>
    <rdf:type rdf:resource="http://www.w3.org/2002/07/owl#Class"/>
  </rdf:Description>
  <rdf:Description rdf:about="#CONTROL-FEATURE-TYPE_Biological_surface_deposition_concentration_contour_line">
    <rdfs:subClassOf rdf:resource="jc3iedm_OBJECT-TYPE.owl#CONTROL-FEATURE-TYPE"/>
    <rdfs:label xml:lang="en">biological surface deposition concentration contour line</rdfs:label>
    <rdfs:comment xml:lang="en">A line on a map, diagram or overlay joining all points at which the biological surface deposition concentration at a given time is the same. Biological surface deposition concentration is the mass of a biological substance distributed on a surface per unit area.</rdfs:comment>
    <rdf:type rdf:resource="http://www.w3.org/2002/07/owl#Class"/>
  </rdf:Description>
  <rdf:Description rdf:about="#CONSUMABLE-MATERIEL-TYPE_Construction_materials">
    <rdfs:subClassOf rdf:resource="jc3iedm_OBJECT-TYPE.owl#CONSUMABLE-MATERIEL-TYPE"/>
    <rdfs:label xml:lang="en">construction materials</rdfs:label>
    <rdfs:comment xml:lang="en">Any material that may be used in construction.</rdfs:comment>
    <rdf:type rdf:resource="http://www.w3.org/2002/07/owl#Class"/>
  </rdf:Description>
  <rdf:Description rdf:about="#CONTROL-FEATURE-TYPE_Rally_point">
    <rdfs:subClassOf rdf:resource="jc3iedm_OBJECT-TYPE.owl#CONTROL-FEATURE-TYPE"/>
    <rdfs:label xml:lang="en">rally point</rdfs:label>
    <rdfs:comment xml:lang="en">An easily identifiable point location on the ground at which units can reassemble/reorganise if they become disbursed or aircrews/passengers can assemble and reorganise following an incident requiring a forced landing.</rdfs:comment>
    <rdf:type rdf:resource="http://www.w3.org/2002/07/owl#Class"/>
  </rdf:Description>
  <rdf:Description rdf:about="#MILITARY-OBSTACLE-TYPE_Barrier,_vehicle">
    <rdfs:subClassOf rdf:resource="jc3iedm_OBJECT-TYPE.owl#MILITARY-OBSTACLE-TYPE"/>
    <rdfs:label xml:lang="en">barrier, vehicle</rdfs:label>
    <rdfs:comment xml:lang="en">An obstruction made of vehicles erected to bar the advance of persons or vehicles, or to prevent access to a place.</rdfs:comment>
    <rdf:type rdf:resource="http://www.w3.org/2002/07/owl#Class"/>
  </rdf:Description>
  <rdf:Description rdf:about="jc3iedm_OBJECT-TYPE.owl#executive-military-organisation-type-category-code">
    <rdf:type rdf:resource="http://www.w3.org/2002/07/owl#DatatypeProperty"/>
    <rdfs:domain rdf:resource="jc3iedm_OBJECT-TYPE.owl#EXECUTIVE-MILITARY-ORGANISATION-TYPE"/>
    <rdfs:range rdf:resource="http://www.w3.org/2001/XMLSchema#string"/>
  </rdf:Description>
  <rdf:Description rdf:about="#CONTROL-FEATURE-TYPE_Obstacle_zone">
    <rdfs:subClassOf rdf:resource="jc3iedm_OBJECT-TYPE.owl#CONTROL-FEATURE-TYPE"/>
    <rdfs:label xml:lang="en">obstacle zone</rdfs:label>
    <rdfs:comment xml:lang="en">A division-level command and control measure, normally done graphically, to designate specific land areas where lower echelons are allowed to employ tactical obstacles.</rdfs:comment>
    <rdf:type rdf:resource="http://www.w3.org/2002/07/owl#Class"/>
  </rdf:Description>
  <rdf:Description rdf:about="#AMMUNITION-TYPE_Missile,_anti-radiation">
    <rdfs:subClassOf rdf:resource="jc3iedm_OBJECT-TYPE.owl#AMMUNITION-TYPE"/>
    <rdfs:label xml:lang="en">missile, anti radiation</rdfs:label>
    <rdfs:comment xml:lang="en">A missile that homes passively on a radiation source.</rdfs:comment>
    <rdf:type rdf:resource="http://www.w3.org/2002/07/owl#Class"/>
  </rdf:Description>
  <rdf:Description rdf:about="#CIVILIAN-POST-TYPE_Alderman">
    <rdfs:subClassOf rdf:resource="jc3iedm_OBJECT-TYPE.owl#CIVILIAN-POST-TYPE"/>
    <rdfs:label xml:lang="en">alderman</rdfs:label>
    <rdfs:comment xml:lang="en">A CIVILIAN-POST-TYPE whose job entails the participation in the legislative body of town or city governments.</rdfs:comment>
    <rdf:type rdf:resource="http://www.w3.org/2002/07/owl#Class"/>
  </rdf:Description>
  <rdf:Description rdf:about="#MILITARY-OBSTACLE-TYPE_Tetrahedron">
    <rdfs:subClassOf rdf:resource="jc3iedm_OBJECT-TYPE.owl#MILITARY-OBSTACLE-TYPE"/>
    <rdfs:label xml:lang="en">tetrahedron</rdfs:label>
    <rdfs:comment xml:lang="en">No definition provided in APP-6A.</rdfs:comment>
    <rdf:type rdf:resource="http://www.w3.org/2002/07/owl#Class"/>
  </rdf:Description>
  <rdf:Description rdf:about="#CIVILIAN-POST-TYPE_Police_chief">
    <rdfs:subClassOf rdf:resource="jc3iedm_OBJECT-TYPE.owl#CIVILIAN-POST-TYPE"/>
    <rdfs:label xml:lang="en">police chief</rdfs:label>
    <rdfs:comment xml:lang="en">A CIVILIAN-POST-TYPE whose job is the chief officer of a civil force to which is entrusted the duty of maintaining public order, enforcing regulations and detecting crime.</rdfs:comment>
    <rdf:type rdf:resource="http://www.w3.org/2002/07/owl#Class"/>
  </rdf:Description>
  <rdf:Description rdf:about="#SURFACE-VESSEL-TYPE_Torpedo_boat,_air_cushion">
    <rdfs:subClassOf rdf:resource="jc3iedm_OBJECT-TYPE.owl#SURFACE-VESSEL-TYPE"/>
    <rdfs:label xml:lang="en">torpedo boat, air cushion</rdfs:label>
    <rdfs:comment xml:lang="en">High-speed (35 knots - 65 km/hr) anti-surface ship patrol craft in size range 20 - 30 metres fitted with torpedoes with either an air cushion or surface effect design.</rdfs:comment>
    <rdf:type rdf:resource="http://www.w3.org/2002/07/owl#Class"/>
  </rdf:Description>
  <rdf:Description rdf:about="#CONTROL-FEATURE-TYPE_Restricted_fire_line">
    <rdfs:subClassOf rdf:resource="jc3iedm_OBJECT-TYPE.owl#CONTROL-FEATURE-TYPE"/>
    <rdfs:label xml:lang="en">restricted fire line</rdfs:label>
    <rdfs:comment xml:lang="en">A line established between converging forces that prohibits fires or the effect of fires across the line without prior coordination.</rdfs:comment>
    <rdf:type rdf:resource="http://www.w3.org/2002/07/owl#Class"/>
  </rdf:Description>
  <rdf:Description rdf:about="#ROUTE-TYPE_Alternate_supply_route">
    <rdfs:subClassOf rdf:resource="jc3iedm_OBJECT-TYPE.owl#ROUTE-TYPE"/>
    <rdfs:label xml:lang="en">alternate supply route</rdfs:label>
    <rdfs:comment xml:lang="en">A route or routes designated within an area of operations to provide for the movement of traffic when main supply routes become disabled or congested.</rdfs:comment>
    <rdf:type rdf:resource="http://www.w3.org/2002/07/owl#Class"/>
  </rdf:Description>
  <rdf:Description rdf:about="#CONTROL-FEATURE-TYPE_Forward_combat_zone">
    <rdfs:subClassOf rdf:resource="jc3iedm_OBJECT-TYPE.owl#CONTROL-FEATURE-TYPE"/>
    <rdfs:label xml:lang="en">forward combat zone</rdfs:label>
    <rdfs:comment xml:lang="en">A CONTROL-FEATURE-TYPE with an area location compromising the territory forward of the corps rear boundary.</rdfs:comment>
    <rdf:type rdf:resource="http://www.w3.org/2002/07/owl#Class"/>
  </rdf:Description>
  <rdf:Description rdf:about="#CBRN-EQUIPMENT-TYPE_Automated_biological_detector">
    <rdfs:subClassOf rdf:resource="jc3iedm_OBJECT-TYPE.owl#CBRN-EQUIPMENT-TYPE"/>
    <rdfs:label xml:lang="en">automated biological detector</rdfs:label>
    <rdfs:comment xml:lang="en">An unattended biological detection and alarm system.</rdfs:comment>
    <rdf:type rdf:resource="http://www.w3.org/2002/07/owl#Class"/>
  </rdf:Description>
  <rdf:Description rdf:about="#SUBSURFACE-VESSEL-TYPE_Submarine,_general">
    <rdfs:subClassOf rdf:resource="jc3iedm_OBJECT-TYPE.owl#SUBSURFACE-VESSEL-TYPE"/>
    <rdfs:label xml:lang="en">submarine, general</rdfs:label>
    <rdfs:comment xml:lang="en">General designator for a warship, capable of operating under water and usually equipped with torpedoes, missiles and a periscope.</rdfs:comment>
    <rdf:type rdf:resource="http://www.w3.org/2002/07/owl#Class"/>
  </rdf:Description>
  <rdf:Description rdf:about="#SURFACE-VESSEL-TYPE_Distilling_ship_(naval)">
    <rdfs:subClassOf rdf:resource="jc3iedm_OBJECT-TYPE.owl#SURFACE-VESSEL-TYPE"/>
    <rdfs:label xml:lang="en">distilling ship (naval)</rdfs:label>
    <rdfs:comment xml:lang="en">Ship capable of distilling and transporting potable water.</rdfs:comment>
    <rdf:type rdf:resource="http://www.w3.org/2002/07/owl#Class"/>
  </rdf:Description>
  <rdf:Description rdf:about="#SURFACE-VESSEL-TYPE_Minelayer,_inshore">
    <rdfs:subClassOf rdf:resource="jc3iedm_OBJECT-TYPE.owl#SURFACE-VESSEL-TYPE"/>
    <rdfs:label xml:lang="en">minelayer, inshore</rdfs:label>
    <rdfs:comment xml:lang="en">Minelayer in size range 25 - 50 metres overall.</rdfs:comment>
    <rdf:type rdf:resource="http://www.w3.org/2002/07/owl#Class"/>
  </rdf:Description>
  <rdf:Description rdf:about="#SURFACE-VESSEL-TYPE_Racing_cruiser">
    <rdfs:subClassOf rdf:resource="jc3iedm_OBJECT-TYPE.owl#SURFACE-VESSEL-TYPE"/>
    <rdfs:label xml:lang="en">racing cruiser</rdfs:label>
    <rdfs:comment xml:lang="en">Sailing vessel designed specifically for ocean racing. May have auxiliary inboard engines.</rdfs:comment>
    <rdf:type rdf:resource="http://www.w3.org/2002/07/owl#Class"/>
  </rdf:Description>
  <rdf:Description rdf:about="#CONTROL-FEATURE-TYPE_Final_protective_fire">
    <rdfs:subClassOf rdf:resource="jc3iedm_OBJECT-TYPE.owl#CONTROL-FEATURE-TYPE"/>
    <rdfs:label xml:lang="en">final protective fire</rdfs:label>
    <rdfs:comment xml:lang="en">An immediately available prearranged barrier of fire designed to impede enemy movement across defensive lines or areas.</rdfs:comment>
    <rdf:type rdf:resource="http://www.w3.org/2002/07/owl#Class"/>
  </rdf:Description>
  <rdf:Description rdf:about="#CONTROL-FEATURE-TYPE_Penetration_box">
    <rdfs:subClassOf rdf:resource="jc3iedm_OBJECT-TYPE.owl#CONTROL-FEATURE-TYPE"/>
    <rdfs:label xml:lang="en">penetration box</rdfs:label>
    <rdfs:comment xml:lang="en">A CONTROL-FEATURE-TYPE that defines the area intended for penetration through enemy defences, a form of offensive which seeks to break through the enemy's defence and disrupt the defensive system.</rdfs:comment>
    <rdf:type rdf:resource="http://www.w3.org/2002/07/owl#Class"/>
  </rdf:Description>
  <rdf:Description rdf:about="#MILITARY-OBSTACLE-TYPE_Minefield,_anti-personnel">
    <rdfs:subClassOf rdf:resource="jc3iedm_OBJECT-TYPE.owl#MILITARY-OBSTACLE-TYPE"/>
    <rdfs:label xml:lang="en">minefield, anti personnel</rdfs:label>
    <rdfs:comment xml:lang="en">An obstacle made by laying mines of anti-personnel type laid with or without pattern.</rdfs:comment>
    <rdf:type rdf:resource="http://www.w3.org/2002/07/owl#Class"/>
  </rdf:Description>
  <rdf:Description rdf:about="#TASK-FORMATION-TYPE_Initial_terminal_guidance_team">
    <rdfs:subClassOf rdf:resource="jc3iedm_OBJECT-TYPE.owl#TASK-FORMATION-TYPE"/>
    <rdfs:label xml:lang="en">initial terminal guidance team</rdfs:label>
    <rdfs:comment xml:lang="en">A TASK-FORMATION-TYPE that provides electronic, mechanical, visual, or other assistance given an aircraft pilot to facilitate arrival at, operation within or over, landing upon, or departure from an air landing or airdrop facility.</rdfs:comment>
    <rdf:type rdf:resource="http://www.w3.org/2002/07/owl#Class"/>
  </rdf:Description>
  <rdf:Description rdf:about="#CONTROL-FEATURE-TYPE_CBRN_cloud_radius">
    <rdfs:subClassOf rdf:resource="jc3iedm_OBJECT-TYPE.owl#CONTROL-FEATURE-TYPE"/>
    <rdfs:label xml:lang="en">cbrn cloud radius</rdfs:label>
    <rdfs:comment xml:lang="en">A CONTROL-FEATURE-TYPE that identifies the linear distance from the centre of the CBRN-EVENT to the outer edge of the initial cloud.</rdfs:comment>
    <rdf:type rdf:resource="http://www.w3.org/2002/07/owl#Class"/>
  </rdf:Description>
  <rdf:Description rdf:about="#CHEMICAL-MATERIEL-TYPE_Nerve_agent">
    <rdfs:subClassOf rdf:resource="jc3iedm_OBJECT-TYPE.owl#CHEMICAL-MATERIEL-TYPE"/>
    <rdfs:label xml:lang="en">nerve agent</rdfs:label>
    <rdfs:comment xml:lang="en">A potentially lethal CHEMICAL-MATERIEL-TYPE that interferes with the transmission of nerve impulses.</rdfs:comment>
    <rdf:type rdf:resource="http://www.w3.org/2002/07/owl#Class"/>
  </rdf:Description>
  <rdf:Description rdf:about="#SURFACE-VESSEL-TYPE_Ammunition_ship,_transport">
    <rdfs:subClassOf rdf:resource="jc3iedm_OBJECT-TYPE.owl#SURFACE-VESSEL-TYPE"/>
    <rdfs:label xml:lang="en">ammunition ship, transport</rdfs:label>
    <rdfs:comment xml:lang="en">Ship capable of transporting 5000 or more tons of ammunition but lacking sophisticated underway replenishment capabilities.</rdfs:comment>
    <rdf:type rdf:resource="http://www.w3.org/2002/07/owl#Class"/>
  </rdf:Description>
  <rdf:Description rdf:about="#SURFACE-VESSEL-TYPE_Minelayer,_auxiliary">
    <rdfs:subClassOf rdf:resource="jc3iedm_OBJECT-TYPE.owl#SURFACE-VESSEL-TYPE"/>
    <rdfs:label xml:lang="en">minelayer, auxiliary</rdfs:label>
    <rdfs:comment xml:lang="en">Any fishing or merchant ship having both capability and mission to lay mines.</rdfs:comment>
    <rdf:type rdf:resource="http://www.w3.org/2002/07/owl#Class"/>
  </rdf:Description>
  <rdf:Description rdf:about="#CONTROL-FEATURE-TYPE_Drop_point">
    <rdfs:subClassOf rdf:resource="jc3iedm_OBJECT-TYPE.owl#CONTROL-FEATURE-TYPE"/>
    <rdfs:label xml:lang="en">drop point</rdfs:label>
    <rdfs:comment xml:lang="en">Position of weapon release.</rdfs:comment>
    <rdf:type rdf:resource="http://www.w3.org/2002/07/owl#Class"/>
  </rdf:Description>
  <rdf:Description rdf:about="#FACILITY-TYPE_Police_station">
    <rdfs:subClassOf rdf:resource="jc3iedm_OBJECT-TYPE.owl#FACILITY-TYPE"/>
    <rdfs:label xml:lang="en">police station</rdfs:label>
    <rdfs:comment xml:lang="en">The office of a local police force.</rdfs:comment>
    <rdf:type rdf:resource="http://www.w3.org/2002/07/owl#Class"/>
  </rdf:Description>
  <rdf:Description rdf:about="#CONSUMABLE-MATERIEL-TYPE_Exercise_mine">
    <rdfs:subClassOf rdf:resource="jc3iedm_OBJECT-TYPE.owl#CONSUMABLE-MATERIEL-TYPE"/>
    <rdfs:label xml:lang="en">exercise mine</rdfs:label>
    <rdfs:comment xml:lang="en">In naval mine warfare, a mine suitable for use in mine warfare exercises, fitted with visible or audible indicating devices to show where and when it would normally fire.</rdfs:comment>
    <rdf:type rdf:resource="http://www.w3.org/2002/07/owl#Class"/>
  </rdf:Description>
  <rdf:Description rdf:about="jc3iedm_OBJECT-TYPE.owl#AMMUNITION-TYPE">
    <rdf:type rdf:resource="http://www.w3.org/2002/07/owl#Class"/>
    <rdfs:label xml:lang="en">ammunition type</rdfs:label>
    <rdfs:comment xml:lang="en">A CONSUMABLE-MATERIEL-TYPE that is a complete device charged with explosives, propellants, pyrotechnics, initiating composition, or nuclear, biological, or chemical material for use in military operations.</rdfs:comment>
    <rdfs:subClassOf rdf:resource="jc3iedm_OBJECT-TYPE.owl#CONSUMABLE-MATERIEL-TYPE"/>
  </rdf:Description>
  <rdf:Description rdf:about="jc3iedm_OBJECT-TYPE.owl#physical_model_only">
    <rdf:type rdf:resource="http://www.w3.org/2002/07/owl#DatatypeProperty"/>
    <rdfs:domain rdf:resource="jc3iedm_OBJECT-TYPE.owl#TASK-FORMATION-TYPE"/>
  </rdf:Description>
  <rdf:Description rdf:about="#SURFACE-VESSEL-TYPE_Lighter,_aircraft_transport">
    <rdfs:subClassOf rdf:resource="jc3iedm_OBJECT-TYPE.owl#SURFACE-VESSEL-TYPE"/>
    <rdfs:label xml:lang="en">lighter, aircraft transport</rdfs:label>
    <rdfs:comment xml:lang="en">Barge-like vessel used in loading and unloading ships or in transporting loads for short distances, optimised for transporting aircraft.</rdfs:comment>
    <rdf:type rdf:resource="http://www.w3.org/2002/07/owl#Class"/>
  </rdf:Description>
  <rdf:Description rdf:about="#WEAPON-TYPE_Rocket_artillery">
    <rdfs:subClassOf rdf:resource="jc3iedm_OBJECT-TYPE.owl#WEAPON-TYPE"/>
    <rdfs:label xml:lang="en">rocket artillery</rdfs:label>
    <rdfs:comment xml:lang="en">A system designed to launch one or more powered unguided objects at a target.</rdfs:comment>
    <rdf:type rdf:resource="http://www.w3.org/2002/07/owl#Class"/>
  </rdf:Description>
  <rdf:Description rdf:about="#FACILITY-TYPE_Power_plant,_hydroelectric">
    <rdfs:subClassOf rdf:resource="jc3iedm_OBJECT-TYPE.owl#FACILITY-TYPE"/>
    <rdfs:label xml:lang="en">power plant, hydroelectric</rdfs:label>
    <rdfs:comment xml:lang="en">A facility that provides power produced from hydroelectric processes.</rdfs:comment>
    <rdf:type rdf:resource="http://www.w3.org/2002/07/owl#Class"/>
  </rdf:Description>
  <rdf:Description rdf:about="#CONTROL-FEATURE-TYPE_Assembly_area,_supply">
    <rdfs:subClassOf rdf:resource="jc3iedm_OBJECT-TYPE.owl#CONTROL-FEATURE-TYPE"/>
    <rdfs:label xml:lang="en">assembly area, supply</rdfs:label>
    <rdfs:comment xml:lang="en">In a supply installation, the gross area used for collecting and combining components into complete units, kits, or assemblies.</rdfs:comment>
    <rdf:type rdf:resource="http://www.w3.org/2002/07/owl#Class"/>
  </rdf:Description>
  <rdf:Description rdf:about="#SURFACE-VESSEL-TYPE_Amphibious_fire_support_ship">
    <rdfs:subClassOf rdf:resource="jc3iedm_OBJECT-TYPE.owl#SURFACE-VESSEL-TYPE"/>
    <rdfs:label xml:lang="en">amphibious fire support ship</rdfs:label>
    <rdfs:comment xml:lang="en">Landing ship converted for use in amphibious assaults. Armament is usually rocket launchers, but may also have bombardment guns. May or may not carry troops.</rdfs:comment>
    <rdf:type rdf:resource="http://www.w3.org/2002/07/owl#Class"/>
  </rdf:Description>
  <rdf:Description rdf:about="#SURFACE-VESSEL-TYPE_Ambulance_boat">
    <rdfs:subClassOf rdf:resource="jc3iedm_OBJECT-TYPE.owl#SURFACE-VESSEL-TYPE"/>
    <rdfs:label xml:lang="en">ambulance boat</rdfs:label>
    <rdfs:comment xml:lang="en">Craft 40 metres or less employed to transport sick/wounded and/or medical personnel.</rdfs:comment>
    <rdf:type rdf:resource="http://www.w3.org/2002/07/owl#Class"/>
  </rdf:Description>
  <rdf:Description rdf:about="#SURFACE-VESSEL-TYPE_Drone_aircraft,_catapult_control_craft">
    <rdfs:subClassOf rdf:resource="jc3iedm_OBJECT-TYPE.owl#SURFACE-VESSEL-TYPE"/>
    <rdfs:label xml:lang="en">drone aircraft, catapult control craft</rdfs:label>
    <rdfs:comment xml:lang="en">Craft equipped with catapult for the launching of drone aircraft and after launch capable of serving as the control craft for the drone.</rdfs:comment>
    <rdf:type rdf:resource="http://www.w3.org/2002/07/owl#Class"/>
  </rdf:Description>
  <rdf:Description rdf:about="#MISCELLANEOUS-EQUIPMENT-TYPE_Generator">
    <rdfs:subClassOf rdf:resource="jc3iedm_OBJECT-TYPE.owl#MISCELLANEOUS-EQUIPMENT-TYPE"/>
    <rdfs:label xml:lang="en">generator</rdfs:label>
    <rdfs:comment xml:lang="en">An apparatus for the production of electricity.</rdfs:comment>
    <rdf:type rdf:resource="http://www.w3.org/2002/07/owl#Class"/>
  </rdf:Description>
  <rdf:Description rdf:about="#UNIT-TYPE_Air_defence">
    <rdfs:subClassOf rdf:resource="jc3iedm_OBJECT-TYPE.owl#UNIT-TYPE"/>
    <rdfs:label xml:lang="en">air defence</rdfs:label>
    <rdfs:comment xml:lang="en">A UNIT-TYPE whose principal designation is the employment of weapon systems against hostile air assets.</rdfs:comment>
    <rdf:type rdf:resource="http://www.w3.org/2002/07/owl#Class"/>
  </rdf:Description>
  <rdf:Description rdf:about="#AMMUNITION-TYPE_Submunition">
    <rdfs:subClassOf rdf:resource="jc3iedm_OBJECT-TYPE.owl#AMMUNITION-TYPE"/>
    <rdfs:label xml:lang="en">submunition</rdfs:label>
    <rdfs:comment xml:lang="en">Any munition that, to perform its task, separates from a parent munition.</rdfs:comment>
    <rdf:type rdf:resource="http://www.w3.org/2002/07/owl#Class"/>
  </rdf:Description>
  <rdf:Description rdf:about="#MILITARY-OBSTACLE-TYPE_Crater_obstacle">
    <rdfs:subClassOf rdf:resource="jc3iedm_OBJECT-TYPE.owl#MILITARY-OBSTACLE-TYPE"/>
    <rdfs:label xml:lang="en">crater obstacle</rdfs:label>
    <rdfs:comment xml:lang="en">A pit or hole in the ground created by an explosion or an impact in order to be used as an obstacle.</rdfs:comment>
    <rdf:type rdf:resource="http://www.w3.org/2002/07/owl#Class"/>
  </rdf:Description>
  <rdf:Description rdf:about="#UNIT-TYPE_Landing_support">
    <rdfs:subClassOf rdf:resource="jc3iedm_OBJECT-TYPE.owl#UNIT-TYPE"/>
    <rdfs:label xml:lang="en">landing support</rdfs:label>
    <rdfs:comment xml:lang="en">A UNIT-TYPE whose principal designation is the provision of landing support services.</rdfs:comment>
    <rdf:type rdf:resource="http://www.w3.org/2002/07/owl#Class"/>
  </rdf:Description>
  <rdf:Description rdf:about="#FACILITY-TYPE_Depot,_POL">
    <rdfs:subClassOf rdf:resource="jc3iedm_OBJECT-TYPE.owl#FACILITY-TYPE"/>
    <rdfs:label xml:lang="en">depot, pol</rdfs:label>
    <rdfs:comment xml:lang="en">An area used for the storage of petroleum, oil and/or lubricants.</rdfs:comment>
    <rdf:type rdf:resource="http://www.w3.org/2002/07/owl#Class"/>
  </rdf:Description>
  <rdf:Description rdf:about="#ENGINEERING-EQUIPMENT-TYPE_Mine_layer,_armoured_vehicle_mounted">
    <rdfs:subClassOf rdf:resource="jc3iedm_OBJECT-TYPE.owl#ENGINEERING-EQUIPMENT-TYPE"/>
    <rdfs:label xml:lang="en">mine layer, armoured vehicle mounted</rdfs:label>
    <rdfs:comment xml:lang="en">An armoured vehicle whose purpose is to lay mines.</rdfs:comment>
    <rdf:type rdf:resource="http://www.w3.org/2002/07/owl#Class"/>
  </rdf:Description>
  <rdf:Description rdf:about="#SURFACE-VESSEL-TYPE_Cutter">
    <rdfs:subClassOf rdf:resource="jc3iedm_OBJECT-TYPE.owl#SURFACE-VESSEL-TYPE"/>
    <rdfs:label xml:lang="en">cutter</rdfs:label>
    <rdfs:comment xml:lang="en">Sailing vessel of cutter design.</rdfs:comment>
    <rdf:type rdf:resource="http://www.w3.org/2002/07/owl#Class"/>
  </rdf:Description>
  <rdf:Description rdf:about="#UNIT-TYPE_Special_operations_forces">
    <rdfs:subClassOf rdf:resource="jc3iedm_OBJECT-TYPE.owl#UNIT-TYPE"/>
    <rdfs:label xml:lang="en">special operations forces</rdfs:label>
    <rdfs:comment xml:lang="en">A UNIT-TYPE that provides unique capabilities of special reconnaissance, direct action and military assistance in order to undertake difficult, dangerous and sometimes politically sensitive missions for the theatre commander.</rdfs:comment>
    <rdf:type rdf:resource="http://www.w3.org/2002/07/owl#Class"/>
  </rdf:Description>
  <rdf:Description rdf:about="#TASK-FORMATION-TYPE_Land_formation">
    <rdfs:subClassOf rdf:resource="jc3iedm_OBJECT-TYPE.owl#TASK-FORMATION-TYPE"/>
    <rdfs:label xml:lang="en">land formation</rdfs:label>
    <rdfs:comment xml:lang="en">An ordered arrangement of troops and/or vehicles for a specific purpose.</rdfs:comment>
    <rdf:type rdf:resource="http://www.w3.org/2002/07/owl#Class"/>
  </rdf:Description>
  <rdf:Description rdf:about="#MILITARY-OBSTACLE-TYPE_Minefield,_not_otherwise_specified">
    <rdfs:subClassOf rdf:resource="jc3iedm_OBJECT-TYPE.owl#MILITARY-OBSTACLE-TYPE"/>
    <rdfs:label xml:lang="en">minefield, not otherwise specified</rdfs:label>
    <rdfs:comment xml:lang="en">An obstacle made by laying mines of an unspecified type laid with or without pattern.</rdfs:comment>
    <rdf:type rdf:resource="http://www.w3.org/2002/07/owl#Class"/>
  </rdf:Description>
  <rdf:Description rdf:about="#SURFACE-VESSEL-TYPE_Patrol_craft,_submarine_chaser/escort,_general">
    <rdfs:subClassOf rdf:resource="jc3iedm_OBJECT-TYPE.owl#SURFACE-VESSEL-TYPE"/>
    <rdfs:label xml:lang="en">patrol craft, submarine chaser/escort, general</rdfs:label>
    <rdfs:comment xml:lang="en">Vessel in size range 35-55 metres designed and fitted primarily for escort duties in ASW role.</rdfs:comment>
    <rdf:type rdf:resource="http://www.w3.org/2002/07/owl#Class"/>
  </rdf:Description>
  <rdf:Description rdf:about="#FACILITY-TYPE_Building">
    <rdfs:subClassOf rdf:resource="jc3iedm_OBJECT-TYPE.owl#FACILITY-TYPE"/>
    <rdfs:label xml:lang="en">building</rdfs:label>
    <rdfs:comment xml:lang="en">A relatively permanent structure, roofed and usually walled and designed for some particular use.</rdfs:comment>
    <rdf:type rdf:resource="http://www.w3.org/2002/07/owl#Class"/>
  </rdf:Description>
  <rdf:Description rdf:about="#SURFACE-VESSEL-TYPE_Merchant_ship,_lash">
    <rdfs:subClassOf rdf:resource="jc3iedm_OBJECT-TYPE.owl#SURFACE-VESSEL-TYPE"/>
    <rdfs:label xml:lang="en">merchant ship, lash</rdfs:label>
    <rdfs:comment xml:lang="en">Non-naval ship equipped with gantry crane, capable of embarking and disembarking pre-loaded standard sized barge (lash lighters).</rdfs:comment>
    <rdf:type rdf:resource="http://www.w3.org/2002/07/owl#Class"/>
  </rdf:Description>
  <rdf:Description rdf:about="#WEAPON-TYPE_Cannon">
    <rdfs:subClassOf rdf:resource="jc3iedm_OBJECT-TYPE.owl#WEAPON-TYPE"/>
    <rdfs:label xml:lang="en">cannon</rdfs:label>
    <rdfs:comment xml:lang="en">A weapon for firing projectiles, having a heavy metal tube installed on a carriage or mounting.</rdfs:comment>
    <rdf:type rdf:resource="http://www.w3.org/2002/07/owl#Class"/>
  </rdf:Description>
  <rdf:Description rdf:about="#FACILITY-TYPE_Field_storage_stack-ammunition">
    <rdfs:subClassOf rdf:resource="jc3iedm_OBJECT-TYPE.owl#FACILITY-TYPE"/>
    <rdfs:label xml:lang="en">field storage stack ammunition</rdfs:label>
    <rdfs:comment xml:lang="en">A facility where approximately 1 tonne gross weight of ammunition and explosives stored under tactical field conditions.</rdfs:comment>
    <rdf:type rdf:resource="http://www.w3.org/2002/07/owl#Class"/>
  </rdf:Description>
  <rdf:Description rdf:about="#ROUTE-TYPE_Main_supply_route">
    <rdfs:subClassOf rdf:resource="jc3iedm_OBJECT-TYPE.owl#ROUTE-TYPE"/>
    <rdfs:label xml:lang="en">main supply route</rdfs:label>
    <rdfs:comment xml:lang="en">The route or routes designated with an area of operations on which the bulk of traffic flows in support of military operations.</rdfs:comment>
    <rdf:type rdf:resource="http://www.w3.org/2002/07/owl#Class"/>
  </rdf:Description>
  <rdf:Description rdf:about="#CONTROL-FEATURE-TYPE_Holding_line">
    <rdfs:subClassOf rdf:resource="jc3iedm_OBJECT-TYPE.owl#CONTROL-FEATURE-TYPE"/>
    <rdfs:label xml:lang="en">holding line</rdfs:label>
    <rdfs:comment xml:lang="en">In retrograde river-crossing operations, the outer limit of the area established between the enemy and the water obstacle to preclude direct and observed indirect fires into crossing areas.</rdfs:comment>
    <rdf:type rdf:resource="http://www.w3.org/2002/07/owl#Class"/>
  </rdf:Description>
  <rdf:Description rdf:about="#SURFACE-VESSEL-TYPE_Amphibious_assault_ship,_multi-purpose">
    <rdfs:subClassOf rdf:resource="jc3iedm_OBJECT-TYPE.owl#SURFACE-VESSEL-TYPE"/>
    <rdfs:label xml:lang="en">amphibious assault ship, multi purpose</rdfs:label>
    <rdfs:comment xml:lang="en">A large multi-purpose amphibious ship that embarks and lands elements of a landing force by helicopter, landing craft and amphibious vehicles. Can also conduct sea control and power projection missions with VSTOL aircraft and ASW helicopters.</rdfs:comment>
    <rdf:type rdf:resource="http://www.w3.org/2002/07/owl#Class"/>
  </rdf:Description>
  <rdf:Description rdf:about="jc3iedm_OBJECT-TYPE.owl#vessel-type-prismatic-coefficient-ratio">
    <rdf:type rdf:resource="http://www.w3.org/2002/07/owl#DatatypeProperty"/>
    <rdfs:domain rdf:resource="jc3iedm_OBJECT-TYPE.owl#VESSEL-TYPE"/>
  </rdf:Description>
  <rdf:Description rdf:about="jc3iedm_OBJECT-TYPE.owl#task-formation-type-category-code">
    <rdf:type rdf:resource="http://www.w3.org/2002/07/owl#DatatypeProperty"/>
    <rdfs:domain rdf:resource="jc3iedm_OBJECT-TYPE.owl#TASK-FORMATION-TYPE"/>
    <rdfs:range rdf:resource="http://www.w3.org/2001/XMLSchema#string"/>
  </rdf:Description>
  <rdf:Description rdf:about="jc3iedm_OBJECT-TYPE.owl#CONSUMABLE-MATERIEL-TYPE">
    <rdf:type rdf:resource="http://www.w3.org/2002/07/owl#Class"/>
    <rdfs:label xml:lang="en">consumable materiel type</rdfs:label>
    <rdfs:comment xml:lang="en">A MATERIEL-TYPE that is an expendable class of supply.</rdfs:comment>
    <rdfs:subClassOf rdf:resource="jc3iedm_OBJECT-TYPE.owl#MATERIEL-TYPE"/>
  </rdf:Description>
  <rdf:Description rdf:about="#FACILITY-TYPE_Wall">
    <rdfs:subClassOf rdf:resource="jc3iedm_OBJECT-TYPE.owl#FACILITY-TYPE"/>
    <rdfs:label xml:lang="en">wall</rdfs:label>
    <rdfs:comment xml:lang="en">A continuous, vertical structure, such as a concrete or rock wall serving to enclose, divide, support or protect an area of land. Includes sea walls.</rdfs:comment>
    <rdf:type rdf:resource="http://www.w3.org/2002/07/owl#Class"/>
  </rdf:Description>
  <rdf:Description rdf:about="#CONTROL-FEATURE-TYPE_Q-zone">
    <rdfs:subClassOf rdf:resource="jc3iedm_OBJECT-TYPE.owl#CONTROL-FEATURE-TYPE"/>
    <rdfs:label xml:lang="en">q zone</rdfs:label>
    <rdfs:comment xml:lang="en">A CONTROL-FEATURE-TYPE that represents one of the 18 main geographical sea areas of the world.</rdfs:comment>
    <rdf:type rdf:resource="http://www.w3.org/2002/07/owl#Class"/>
  </rdf:Description>
  <rdf:Description rdf:about="#UNIT-TYPE_Transportation">
    <rdfs:subClassOf rdf:resource="jc3iedm_OBJECT-TYPE.owl#UNIT-TYPE"/>
    <rdfs:label xml:lang="en">transportation</rdfs:label>
    <rdfs:comment xml:lang="en">A UNIT-TYPE whose principal designation is the provision of transport for assets.</rdfs:comment>
    <rdf:type rdf:resource="http://www.w3.org/2002/07/owl#Class"/>
  </rdf:Description>
  <rdf:Description rdf:about="#SURFACE-VESSEL-TYPE_Survey_ship,_polar">
    <rdfs:subClassOf rdf:resource="jc3iedm_OBJECT-TYPE.owl#SURFACE-VESSEL-TYPE"/>
    <rdfs:label xml:lang="en">survey ship, polar</rdfs:label>
    <rdfs:comment xml:lang="en">Ship used for surveying arctic/antarctic areas.</rdfs:comment>
    <rdf:type rdf:resource="http://www.w3.org/2002/07/owl#Class"/>
  </rdf:Description>
  <rdf:Description rdf:about="#CHEMICAL-MATERIEL-TYPE_Irritant">
    <rdfs:subClassOf rdf:resource="jc3iedm_OBJECT-TYPE.owl#CHEMICAL-MATERIEL-TYPE"/>
    <rdfs:label xml:lang="en">irritant</rdfs:label>
    <rdfs:comment xml:lang="en">A CHEMICAL-MATERIEL-TYPE that is designed to irritate the eyes, lungs and skin.</rdfs:comment>
    <rdf:type rdf:resource="http://www.w3.org/2002/07/owl#Class"/>
  </rdf:Description>
  <rdf:Description rdf:about="#FACILITY-TYPE_Foxhole">
    <rdfs:subClassOf rdf:resource="jc3iedm_OBJECT-TYPE.owl#FACILITY-TYPE"/>
    <rdfs:label xml:lang="en">foxhole</rdfs:label>
    <rdfs:comment xml:lang="en">A hole in the ground used by a soldier for protection.</rdfs:comment>
    <rdf:type rdf:resource="http://www.w3.org/2002/07/owl#Class"/>
  </rdf:Description>
  <rdf:Description rdf:about="#SURFACE-VESSEL-TYPE_Fishing_vessel,_factory_ship">
    <rdfs:subClassOf rdf:resource="jc3iedm_OBJECT-TYPE.owl#SURFACE-VESSEL-TYPE"/>
    <rdfs:label xml:lang="en">fishing vessel, factory ship</rdfs:label>
    <rdfs:comment xml:lang="en">Fishing vessel equipped to prepare fish or other seafood into commercial products.</rdfs:comment>
    <rdf:type rdf:resource="http://www.w3.org/2002/07/owl#Class"/>
  </rdf:Description>
  <rdf:Description rdf:about="#CONTROL-FEATURE-TYPE_Kill_box">
    <rdfs:subClassOf rdf:resource="jc3iedm_OBJECT-TYPE.owl#CONTROL-FEATURE-TYPE"/>
    <rdfs:label xml:lang="en">kill box</rdfs:label>
    <rdfs:comment xml:lang="en">A volume of airspace where fighter aircraft operate in a weapons free mode and can use their weapons in beyond line of sight operations.</rdfs:comment>
    <rdf:type rdf:resource="http://www.w3.org/2002/07/owl#Class"/>
  </rdf:Description>
  <rdf:Description rdf:about="#SURFACE-VESSEL-TYPE_Barge,_special_purpose,_non-self_propelled">
    <rdfs:subClassOf rdf:resource="jc3iedm_OBJECT-TYPE.owl#SURFACE-VESSEL-TYPE"/>
    <rdfs:label xml:lang="en">barge, special purpose, non self propelled</rdfs:label>
    <rdfs:comment xml:lang="en">Barge used for various designated special purposes.</rdfs:comment>
    <rdf:type rdf:resource="http://www.w3.org/2002/07/owl#Class"/>
  </rdf:Description>
  <rdf:Description rdf:about="jc3iedm_OBJECT-TYPE.owl#GOVERNMENT-ORGANISATION-TYPE">
    <rdf:type rdf:resource="http://www.w3.org/2002/07/owl#Class"/>
    <rdfs:label xml:lang="en">government organisation type</rdfs:label>
    <rdfs:comment xml:lang="en">An ORGANISATION-TYPE that controls and administers public policy either under a national or international mandate.</rdfs:comment>
    <rdfs:subClassOf rdf:resource="jc3iedm_OBJECT-TYPE.owl#ORGANISATION-TYPE"/>
  </rdf:Description>
  <rdf:Description rdf:about="#SUBSURFACE-VESSEL-TYPE_Deep_submergence_vehicle,_military">
    <rdfs:subClassOf rdf:resource="jc3iedm_OBJECT-TYPE.owl#SUBSURFACE-VESSEL-TYPE"/>
    <rdfs:label xml:lang="en">deep submergence vehicle, military</rdfs:label>
    <rdfs:comment xml:lang="en">Military operated submersible designed to operate at great depth (more than 300 metres).</rdfs:comment>
    <rdf:type rdf:resource="http://www.w3.org/2002/07/owl#Class"/>
  </rdf:Description>
  <rdf:Description rdf:about="jc3iedm_OBJECT-TYPE.owl#control-feature-type-echelon-code">
    <rdf:type rdf:resource="http://www.w3.org/2002/07/owl#DatatypeProperty"/>
    <rdfs:domain rdf:resource="jc3iedm_OBJECT-TYPE.owl#CONTROL-FEATURE-TYPE"/>
    <rdfs:range rdf:resource="http://www.w3.org/2001/XMLSchema#string"/>
  </rdf:Description>
  <rdf:Description rdf:about="#FACILITY-TYPE_Processing_facility">
    <rdfs:subClassOf rdf:resource="jc3iedm_OBJECT-TYPE.owl#FACILITY-TYPE"/>
    <rdfs:label xml:lang="en">processing facility</rdfs:label>
    <rdfs:comment xml:lang="en">A facility generally used to support a particular method of operation in any manufacture or to support a series of actions or events.</rdfs:comment>
    <rdf:type rdf:resource="http://www.w3.org/2002/07/owl#Class"/>
  </rdf:Description>
  <rdf:Description rdf:about="#SURFACE-VESSEL-TYPE_Merchant_ship,_replenishment_oiler_small">
    <rdfs:subClassOf rdf:resource="jc3iedm_OBJECT-TYPE.owl#SURFACE-VESSEL-TYPE"/>
    <rdfs:label xml:lang="en">merchant ship, replenishment oiler small</rdfs:label>
    <rdfs:comment xml:lang="en">Non-naval ship able to provide replenishment to ships at sea of POL and solid store products. Less than 120 metres in size.</rdfs:comment>
    <rdf:type rdf:resource="http://www.w3.org/2002/07/owl#Class"/>
  </rdf:Description>
  <rdf:Description rdf:about="#GEOGRAPHIC-FEATURE-TYPE_Inland_water">
    <rdfs:subClassOf rdf:resource="jc3iedm_OBJECT-TYPE.owl#GEOGRAPHIC-FEATURE-TYPE"/>
    <rdfs:label xml:lang="en">inland water</rdfs:label>
    <rdfs:comment xml:lang="en">A sea, lake, river, etc situated in the interior of a land mass.</rdfs:comment>
    <rdf:type rdf:resource="http://www.w3.org/2002/07/owl#Class"/>
  </rdf:Description>
  <rdf:Description rdf:about="#SURFACE-VESSEL-TYPE_Cruiser,_guided_missile,_helicopter_capable,_nuclear_powered">
    <rdfs:subClassOf rdf:resource="jc3iedm_OBJECT-TYPE.owl#SURFACE-VESSEL-TYPE"/>
    <rdfs:label xml:lang="en">cruiser, guided missile, helicopter capable, nuclear powered</rdfs:label>
    <rdfs:comment xml:lang="en">Cruiser with one or more force guided missile systems as its main armament, fitted with a flight deck with a primary mission of operating and maintaining helicopters but with nuclear power.</rdfs:comment>
    <rdf:type rdf:resource="http://www.w3.org/2002/07/owl#Class"/>
  </rdf:Description>
  <rdf:Description rdf:about="#FACILITY-TYPE_Apron">
    <rdfs:subClassOf rdf:resource="jc3iedm_OBJECT-TYPE.owl#FACILITY-TYPE"/>
    <rdfs:label xml:lang="en">apron</rdfs:label>
    <rdfs:comment xml:lang="en">A FACILITY-TYPE that is an area intended for parking, loading, unloading and/or servicing.</rdfs:comment>
    <rdf:type rdf:resource="http://www.w3.org/2002/07/owl#Class"/>
  </rdf:Description>
  <rdf:Description rdf:about="#ENGINEERING-EQUIPMENT-TYPE_Minefield_marking">
    <rdfs:subClassOf rdf:resource="jc3iedm_OBJECT-TYPE.owl#ENGINEERING-EQUIPMENT-TYPE"/>
    <rdfs:label xml:lang="en">minefield marking</rdfs:label>
    <rdfs:comment xml:lang="en">An equipment used to delimit a minefield.</rdfs:comment>
    <rdf:type rdf:resource="http://www.w3.org/2002/07/owl#Class"/>
  </rdf:Description>
  <rdf:Description rdf:about="#ROUTE-TYPE_Q-route-segment">
    <rdfs:subClassOf rdf:resource="jc3iedm_OBJECT-TYPE.owl#ROUTE-TYPE"/>
    <rdfs:label xml:lang="en">q route segment</rdfs:label>
    <rdfs:comment xml:lang="en">A part of a system of preplanned shipping lanes in mined or potentially mined waters used to minimize the area the mine countermeasures commander has to keep clear of mines in order to provide safe passage for friendly shipping.</rdfs:comment>
    <rdf:type rdf:resource="http://www.w3.org/2002/07/owl#Class"/>
  </rdf:Description>
  <rdf:Description rdf:about="#FACILITY-TYPE_Alternate_decontamination_facility">
    <rdfs:subClassOf rdf:resource="jc3iedm_OBJECT-TYPE.owl#FACILITY-TYPE"/>
    <rdfs:label xml:lang="en">alternate decontamination facility</rdfs:label>
    <rdfs:comment xml:lang="en">A decontamination facility designated as the alternate to the primary decontamination facility that can be used in place of the where personnel and/or materiel (incl. vehicles) can be cleaned after (potential) contamination of radioactive, biological, or chemical material.</rdfs:comment>
    <rdf:type rdf:resource="http://www.w3.org/2002/07/owl#Class"/>
  </rdf:Description>
  <rdf:Description rdf:about="#OBJECT-TYPE_Not_known">
    <rdfs:subClassOf rdf:resource="jc3iedm_OBJECT-TYPE.owl#OBJECT-TYPE"/>
    <rdfs:label xml:lang="en">not known</rdfs:label>
    <rdfs:comment xml:lang="en">It is not possible to determine which value is most applicable.</rdfs:comment>
    <rdf:type rdf:resource="http://www.w3.org/2002/07/owl#Class"/>
  </rdf:Description>
  <rdf:Description rdf:about="#SURFACE-VESSEL-TYPE_Cargo_ship,_light_(naval)">
    <rdfs:subClassOf rdf:resource="jc3iedm_OBJECT-TYPE.owl#SURFACE-VESSEL-TYPE"/>
    <rdfs:label xml:lang="en">cargo ship, light (naval)</rdfs:label>
    <rdfs:comment xml:lang="en">Ship at least 40 - 80 metres employed to transport general cargo and provisions. No underway replenishment facilities.</rdfs:comment>
    <rdf:type rdf:resource="http://www.w3.org/2002/07/owl#Class"/>
  </rdf:Description>
  <rdf:Description rdf:about="#VEHICLE-TYPE_Armoured_personnel_carrier">
    <rdfs:subClassOf rdf:resource="jc3iedm_OBJECT-TYPE.owl#VEHICLE-TYPE"/>
    <rdfs:label xml:lang="en">armoured personnel carrier</rdfs:label>
    <rdfs:comment xml:lang="en">A lightly armoured, highly mobile vehicle, amphibious and air-droppable, used primarily for transporting personnel and their individual equipment during tactical operations.</rdfs:comment>
    <rdf:type rdf:resource="http://www.w3.org/2002/07/owl#Class"/>
  </rdf:Description>
  <rdf:Description rdf:about="#CONTROL-FEATURE-TYPE_Minimum_safe_distance_2">
    <rdfs:subClassOf rdf:resource="jc3iedm_OBJECT-TYPE.owl#CONTROL-FEATURE-TYPE"/>
    <rdfs:label xml:lang="en">minimum safe distance 2</rdfs:label>
    <rdfs:comment xml:lang="en">Minimum Safe Distance 2 identifies the minimum safe distance for warned, exposed personnel measured to the nearest 100 metres from the planned ground zero. Within Minimum Safe Distance 2 and outside of Minimum Safe Distance 1 there is a limit of negligible risk to warned and protected personnel. Maximum protective measures will be required. Minimum Safe Distance 2 is used when there is a single burst.</rdfs:comment>
    <rdf:type rdf:resource="http://www.w3.org/2002/07/owl#Class"/>
  </rdf:Description>
  <rdf:Description rdf:about="jc3iedm_OBJECT-TYPE.owl#AIRCRAFT-TYPE">
    <rdf:type rdf:resource="http://www.w3.org/2002/07/owl#Class"/>
    <rdfs:label xml:lang="en">aircraft type</rdfs:label>
    <rdfs:comment xml:lang="en">An EQUIPMENT-TYPE that is designed to fly.</rdfs:comment>
    <rdfs:subClassOf rdf:resource="jc3iedm_OBJECT-TYPE.owl#EQUIPMENT-TYPE"/>
  </rdf:Description>
  <rdf:Description rdf:about="#FACILITY-TYPE_Site,_military_bridging">
    <rdfs:subClassOf rdf:resource="jc3iedm_OBJECT-TYPE.owl#FACILITY-TYPE"/>
    <rdfs:label xml:lang="en">site, military bridging</rdfs:label>
    <rdfs:comment xml:lang="en">A facility that is used as a basis for military bridging.</rdfs:comment>
    <rdf:type rdf:resource="http://www.w3.org/2002/07/owl#Class"/>
  </rdf:Description>
  <rdf:Description rdf:about="#CONTROL-FEATURE-TYPE_Entry_line">
    <rdfs:subClassOf rdf:resource="jc3iedm_OBJECT-TYPE.owl#CONTROL-FEATURE-TYPE"/>
    <rdfs:label xml:lang="en">entry line</rdfs:label>
    <rdfs:comment xml:lang="en">The line bounding a controlled area (such as crossing area) that controls entry to that area.</rdfs:comment>
    <rdf:type rdf:resource="http://www.w3.org/2002/07/owl#Class"/>
  </rdf:Description>
  <rdf:Description rdf:about="#GEOGRAPHIC-FEATURE-TYPE_Not_known">
    <rdfs:subClassOf rdf:resource="jc3iedm_OBJECT-TYPE.owl#GEOGRAPHIC-FEATURE-TYPE"/>
    <rdfs:label xml:lang="en">not known</rdfs:label>
    <rdfs:comment xml:lang="en">It is not possible to determine which value is most applicable.</rdfs:comment>
    <rdf:type rdf:resource="http://www.w3.org/2002/07/owl#Class"/>
  </rdf:Description>
  <rdf:Description rdf:about="#SURFACE-VESSEL-TYPE_Frigate,_helicopter_capable">
    <rdfs:subClassOf rdf:resource="jc3iedm_OBJECT-TYPE.owl#SURFACE-VESSEL-TYPE"/>
    <rdfs:label xml:lang="en">frigate, helicopter capable</rdfs:label>
    <rdfs:comment xml:lang="en">A frigate fitted with a flight deck with a primary mission of operating and maintaining helicopters. A surface combatant in size range of about 75-150 metres. Fitted primarily to fulfil an ASW role.</rdfs:comment>
    <rdf:type rdf:resource="http://www.w3.org/2002/07/owl#Class"/>
  </rdf:Description>
  <rdf:Description rdf:about="#CONTROL-FEATURE-TYPE_Direction_of_attack">
    <rdfs:subClassOf rdf:resource="jc3iedm_OBJECT-TYPE.owl#CONTROL-FEATURE-TYPE"/>
    <rdfs:label xml:lang="en">direction of attack</rdfs:label>
    <rdfs:comment xml:lang="en">A specific direction or route that the main attack or the centre of mass of the unit main body of the force will follow.</rdfs:comment>
    <rdf:type rdf:resource="http://www.w3.org/2002/07/owl#Class"/>
  </rdf:Description>
  <rdf:Description rdf:about="#VEHICLE-TYPE_Snowplough">
    <rdfs:subClassOf rdf:resource="jc3iedm_OBJECT-TYPE.owl#VEHICLE-TYPE"/>
    <rdfs:label xml:lang="en">snowplough</rdfs:label>
    <rdfs:comment xml:lang="en">A vehicle designed to push snow aside.</rdfs:comment>
    <rdf:type rdf:resource="http://www.w3.org/2002/07/owl#Class"/>
  </rdf:Description>
  <rdf:Description rdf:about="#FACILITY-TYPE_Maintenance_facility,_motor_vehicle">
    <rdfs:subClassOf rdf:resource="jc3iedm_OBJECT-TYPE.owl#FACILITY-TYPE"/>
    <rdfs:label xml:lang="en">maintenance facility, motor vehicle</rdfs:label>
    <rdfs:comment xml:lang="en">A facility containing the resources and infrastructure to enable it to be used for the repair and servicing of motor vehicles.</rdfs:comment>
    <rdf:type rdf:resource="http://www.w3.org/2002/07/owl#Class"/>
  </rdf:Description>
  <rdf:Description rdf:about="#MILITARY-OBSTACLE-TYPE_Ditch_obstacle,_not_otherwise_specified">
    <rdfs:subClassOf rdf:resource="jc3iedm_OBJECT-TYPE.owl#MILITARY-OBSTACLE-TYPE"/>
    <rdfs:label xml:lang="en">ditch obstacle, not otherwise specified</rdfs:label>
    <rdfs:comment xml:lang="en">A channel constructed for the purpose of blocking movement.</rdfs:comment>
    <rdf:type rdf:resource="http://www.w3.org/2002/07/owl#Class"/>
  </rdf:Description>
  <rdf:Description rdf:about="#ELECTRONIC-EQUIPMENT-TYPE_Fire_control">
    <rdfs:subClassOf rdf:resource="jc3iedm_OBJECT-TYPE.owl#ELECTRONIC-EQUIPMENT-TYPE"/>
    <rdfs:label xml:lang="en">fire control</rdfs:label>
    <rdfs:comment xml:lang="en">A group of interrelated fire control equipments and/or instruments designed for use with a weapon or group of weapons.</rdfs:comment>
    <rdf:type rdf:resource="http://www.w3.org/2002/07/owl#Class"/>
  </rdf:Description>
  <rdf:Description rdf:about="#FACILITY-TYPE_Site,_artillery_locating">
    <rdfs:subClassOf rdf:resource="jc3iedm_OBJECT-TYPE.owl#FACILITY-TYPE"/>
    <rdfs:label xml:lang="en">site, artillery locating</rdfs:label>
    <rdfs:comment xml:lang="en">A facility containing equipment employed for locating artillery.</rdfs:comment>
    <rdf:type rdf:resource="http://www.w3.org/2002/07/owl#Class"/>
  </rdf:Description>
  <rdf:Description rdf:about="#SURFACE-VESSEL-TYPE_Seaplane,_coast_guard">
    <rdfs:subClassOf rdf:resource="jc3iedm_OBJECT-TYPE.owl#SURFACE-VESSEL-TYPE"/>
    <rdfs:label xml:lang="en">seaplane, coast guard</rdfs:label>
    <rdfs:comment xml:lang="en">Coast guard aircraft capable of operating from water.</rdfs:comment>
    <rdf:type rdf:resource="http://www.w3.org/2002/07/owl#Class"/>
  </rdf:Description>
  <rdf:Description rdf:about="#SURFACE-VESSEL-TYPE_Ferry_boat">
    <rdfs:subClassOf rdf:resource="jc3iedm_OBJECT-TYPE.owl#SURFACE-VESSEL-TYPE"/>
    <rdfs:label xml:lang="en">ferry boat</rdfs:label>
    <rdfs:comment xml:lang="en">Boat or craft designed to provide ferry service in coastal and protected waters.</rdfs:comment>
    <rdf:type rdf:resource="http://www.w3.org/2002/07/owl#Class"/>
  </rdf:Description>
  <rdf:Description rdf:about="#MILITARY-POST-TYPE_Primary_care_physician">
    <rdfs:subClassOf rdf:resource="jc3iedm_OBJECT-TYPE.owl#MILITARY-POST-TYPE"/>
    <rdfs:label xml:lang="en">primary care physician</rdfs:label>
    <rdfs:comment xml:lang="en">A MILITARY-POST-TYPE that is identified as a physician specialising in Primary care.</rdfs:comment>
    <rdf:type rdf:resource="http://www.w3.org/2002/07/owl#Class"/>
  </rdf:Description>
  <rdf:Description rdf:about="#UNIT-TYPE_Administrative">
    <rdfs:subClassOf rdf:resource="jc3iedm_OBJECT-TYPE.owl#UNIT-TYPE"/>
    <rdfs:label xml:lang="en">administrative</rdfs:label>
    <rdfs:comment xml:lang="en">A UNIT-TYPE whose principal designation the management and execution of all military matters not included in strategy or tactics.</rdfs:comment>
    <rdf:type rdf:resource="http://www.w3.org/2002/07/owl#Class"/>
  </rdf:Description>
  <rdf:Description rdf:about="#CONTROL-FEATURE-TYPE_Minimum_safe_distance_1">
    <rdfs:subClassOf rdf:resource="jc3iedm_OBJECT-TYPE.owl#CONTROL-FEATURE-TYPE"/>
    <rdfs:label xml:lang="en">minimum safe distance 1</rdfs:label>
    <rdfs:comment xml:lang="en">Minimum Safe Distance 1 identifies the minimum safe distance for warned, protected personnel measured to the nearest 100 metres from the expected ground zero. The recommended action within Minimum Safe Distance 1 prior to strike is evacuation of all personnel (if evacuation is not possible or if a commander elects a higher degree of risk, maximum protective measures will be required). Minimum Safe Distance 1 is used when there is a single burst.</rdfs:comment>
    <rdf:type rdf:resource="http://www.w3.org/2002/07/owl#Class"/>
  </rdf:Description>
  <rdf:Description rdf:about="#FACILITY-TYPE_Maintenance_facility,_armour/artillery">
    <rdfs:subClassOf rdf:resource="jc3iedm_OBJECT-TYPE.owl#FACILITY-TYPE"/>
    <rdfs:label xml:lang="en">maintenance facility, armour/artillery</rdfs:label>
    <rdfs:comment xml:lang="en">A facility containing the resources and infrastructure to enable it to be used for the repair and servicing of armour/artillery equipment.</rdfs:comment>
    <rdf:type rdf:resource="http://www.w3.org/2002/07/owl#Class"/>
  </rdf:Description>
  <rdf:Description rdf:about="#CBRN-EQUIPMENT-TYPE_CBRN_reconnaissance_vehicle">
    <rdfs:subClassOf rdf:resource="jc3iedm_OBJECT-TYPE.owl#CBRN-EQUIPMENT-TYPE"/>
    <rdfs:label xml:lang="en">cbrn reconnaissance vehicle</rdfs:label>
    <rdfs:comment xml:lang="en">A vehicle that, as its primary function, is equipped to perform by visual observation or other detection methods, information a particular area potentially contaminated by an NBC (CBRN) event.</rdfs:comment>
    <rdf:type rdf:resource="http://www.w3.org/2002/07/owl#Class"/>
  </rdf:Description>
  <rdf:Description rdf:about="#SURFACE-VESSEL-TYPE_Submarine_tender">
    <rdfs:subClassOf rdf:resource="jc3iedm_OBJECT-TYPE.owl#SURFACE-VESSEL-TYPE"/>
    <rdfs:label xml:lang="en">submarine tender</rdfs:label>
    <rdfs:comment xml:lang="en">Ship of at least 120 metres or more that provides mobile base facilities and support for submarines.</rdfs:comment>
    <rdf:type rdf:resource="http://www.w3.org/2002/07/owl#Class"/>
  </rdf:Description>
  <rdf:Description rdf:about="#CONTROL-FEATURE-TYPE_Biological_atmospheric_concentration_contour_line">
    <rdfs:subClassOf rdf:resource="jc3iedm_OBJECT-TYPE.owl#CONTROL-FEATURE-TYPE"/>
    <rdfs:label xml:lang="en">biological atmospheric concentration contour line</rdfs:label>
    <rdfs:comment xml:lang="en">A line on a map, diagram or overlay joining all points at which the biological atmospheric concentration at a given time is the same. Biological atmospheric concentration is the mass of a biological substance distributed in the atmosphere per unit volume.</rdfs:comment>
    <rdf:type rdf:resource="http://www.w3.org/2002/07/owl#Class"/>
  </rdf:Description>
  <rdf:Description rdf:about="#SURFACE-VESSEL-TYPE_Attack_boat,_guided_missile,_air_cushion">
    <rdfs:subClassOf rdf:resource="jc3iedm_OBJECT-TYPE.owl#SURFACE-VESSEL-TYPE"/>
    <rdfs:label xml:lang="en">attack boat, guided missile, air cushion</rdfs:label>
    <rdfs:comment xml:lang="en">High speed (35 knots - 65 km/hr) anti-surface ship patrol craft in size range 20 - 30 metres fitted with torpedoes and with a force guided missile system and is of an air cushion or surface effect design.</rdfs:comment>
    <rdf:type rdf:resource="http://www.w3.org/2002/07/owl#Class"/>
  </rdf:Description>
  <rdf:Description rdf:about="jc3iedm_OBJECT-TYPE.owl#equipment-type-maximum-width-dimension">
    <rdf:type rdf:resource="http://www.w3.org/2002/07/owl#DatatypeProperty"/>
    <rdfs:domain rdf:resource="jc3iedm_OBJECT-TYPE.owl#EQUIPMENT-TYPE"/>
  </rdf:Description>
  <rdf:Description rdf:about="#FACILITY-TYPE_Maintenance_collection_point">
    <rdfs:subClassOf rdf:resource="jc3iedm_OBJECT-TYPE.owl#FACILITY-TYPE"/>
    <rdfs:label xml:lang="en">maintenance collection point</rdfs:label>
    <rdfs:comment xml:lang="en">A facility established to collect equipment awaiting repair, controlled exchange, cannibalisation or evacuation. May be operated by the user or by intermediate maintenance units.</rdfs:comment>
    <rdf:type rdf:resource="http://www.w3.org/2002/07/owl#Class"/>
  </rdf:Description>
  <rdf:Description rdf:about="jc3iedm_OBJECT-TYPE.owl#vessel-type-draught-dimension">
    <rdf:type rdf:resource="http://www.w3.org/2002/07/owl#DatatypeProperty"/>
    <rdfs:domain rdf:resource="jc3iedm_OBJECT-TYPE.owl#VESSEL-TYPE"/>
  </rdf:Description>
  <rdf:Description rdf:about="#GEOGRAPHIC-FEATURE-TYPE_Landform">
    <rdfs:subClassOf rdf:resource="jc3iedm_OBJECT-TYPE.owl#GEOGRAPHIC-FEATURE-TYPE"/>
    <rdfs:label xml:lang="en">landform</rdfs:label>
    <rdfs:comment xml:lang="en">Natural features of the earth's surface.</rdfs:comment>
    <rdf:type rdf:resource="http://www.w3.org/2002/07/owl#Class"/>
  </rdf:Description>
  <rdf:Description rdf:about="#CONTROL-FEATURE-TYPE_Communication_checkpoint">
    <rdfs:subClassOf rdf:resource="jc3iedm_OBJECT-TYPE.owl#CONTROL-FEATURE-TYPE"/>
    <rdfs:label xml:lang="en">communication checkpoint</rdfs:label>
    <rdfs:comment xml:lang="en">An air control point that requires serial leaders to report either to the aviation mission commander or the terminal control facility.</rdfs:comment>
    <rdf:type rdf:resource="http://www.w3.org/2002/07/owl#Class"/>
  </rdf:Description>
  <rdf:Description rdf:about="#FACILITY-TYPE_Ammunition_cache">
    <rdfs:subClassOf rdf:resource="jc3iedm_OBJECT-TYPE.owl#FACILITY-TYPE"/>
    <rdfs:label xml:lang="en">ammunition cache</rdfs:label>
    <rdfs:comment xml:lang="en">A hiding place for ammunition.</rdfs:comment>
    <rdf:type rdf:resource="http://www.w3.org/2002/07/owl#Class"/>
  </rdf:Description>
  <rdf:Description rdf:about="#FACILITY-TYPE_Channel_pass_lock">
    <rdfs:subClassOf rdf:resource="jc3iedm_OBJECT-TYPE.owl#FACILITY-TYPE"/>
    <rdfs:label xml:lang="en">channel pass lock</rdfs:label>
    <rdfs:comment xml:lang="en">A confined section of a canal or river where the level can be changed for raising and lowering boats between adjacent sections by the use of gates and sluices.</rdfs:comment>
    <rdf:type rdf:resource="http://www.w3.org/2002/07/owl#Class"/>
  </rdf:Description>
  <rdf:Description rdf:about="#SURFACE-VESSEL-TYPE_Minehunter,_coastal">
    <rdfs:subClassOf rdf:resource="jc3iedm_OBJECT-TYPE.owl#SURFACE-VESSEL-TYPE"/>
    <rdfs:label xml:lang="en">minehunter, coastal</rdfs:label>
    <rdfs:comment xml:lang="en">Ship equipped with specific equipment to hunt mines and designed to operate in coastal waters.</rdfs:comment>
    <rdf:type rdf:resource="http://www.w3.org/2002/07/owl#Class"/>
  </rdf:Description>
  <rdf:Description rdf:about="#CONTROL-FEATURE-TYPE_Joint_engagement_zone">
    <rdfs:subClassOf rdf:resource="jc3iedm_OBJECT-TYPE.owl#CONTROL-FEATURE-TYPE"/>
    <rdfs:label xml:lang="en">joint engagement zone</rdfs:label>
    <rdfs:comment xml:lang="en">Airspace in which friendly surface-to-air missiles and fighters are simultaneously employed and operated.</rdfs:comment>
    <rdf:type rdf:resource="http://www.w3.org/2002/07/owl#Class"/>
  </rdf:Description>
  <rdf:Description rdf:about="#CBRN-EQUIPMENT-TYPE_Automated_radiation_detector">
    <rdfs:subClassOf rdf:resource="jc3iedm_OBJECT-TYPE.owl#CBRN-EQUIPMENT-TYPE"/>
    <rdfs:label xml:lang="en">automated radiation detector</rdfs:label>
    <rdfs:comment xml:lang="en">An unattended radiation detector.</rdfs:comment>
    <rdf:type rdf:resource="http://www.w3.org/2002/07/owl#Class"/>
  </rdf:Description>
  <rdf:Description rdf:about="#SURFACE-VESSEL-TYPE_Trimaran">
    <rdfs:subClassOf rdf:resource="jc3iedm_OBJECT-TYPE.owl#SURFACE-VESSEL-TYPE"/>
    <rdfs:label xml:lang="en">trimaran</rdfs:label>
    <rdfs:comment xml:lang="en">Sail or engine powered vessel with three hulls.</rdfs:comment>
    <rdf:type rdf:resource="http://www.w3.org/2002/07/owl#Class"/>
  </rdf:Description>
  <rdf:Description rdf:about="jc3iedm_OBJECT-TYPE.owl#unit-type-category-code">
    <rdf:type rdf:resource="http://www.w3.org/2002/07/owl#DatatypeProperty"/>
    <rdfs:domain rdf:resource="jc3iedm_OBJECT-TYPE.owl#UNIT-TYPE"/>
    <rdfs:range rdf:resource="http://www.w3.org/2001/XMLSchema#string"/>
  </rdf:Description>
  <rdf:Description rdf:about="#ENGINEERING-EQUIPMENT-TYPE_Mine_layer,_trailer_mounted">
    <rdfs:subClassOf rdf:resource="jc3iedm_OBJECT-TYPE.owl#ENGINEERING-EQUIPMENT-TYPE"/>
    <rdfs:label xml:lang="en">mine layer, trailer mounted</rdfs:label>
    <rdfs:comment xml:lang="en">A trailer whose purpose is to lay mines.</rdfs:comment>
    <rdf:type rdf:resource="http://www.w3.org/2002/07/owl#Class"/>
  </rdf:Description>
  <rdf:Description rdf:about="#FACILITY-TYPE_Tower,_flak">
    <rdfs:subClassOf rdf:resource="jc3iedm_OBJECT-TYPE.owl#FACILITY-TYPE"/>
    <rdfs:label xml:lang="en">tower, flak</rdfs:label>
    <rdfs:comment xml:lang="en">A relatively tall structure mounted with an anti-aircraft gun.</rdfs:comment>
    <rdf:type rdf:resource="http://www.w3.org/2002/07/owl#Class"/>
  </rdf:Description>
  <rdf:Description rdf:about="#GROUP-ORGANISATION-TYPE_Criminal">
    <rdfs:subClassOf rdf:resource="jc3iedm_OBJECT-TYPE.owl#GROUP-ORGANISATION-TYPE"/>
    <rdfs:label xml:lang="en">criminal</rdfs:label>
    <rdfs:comment xml:lang="en">A GROUP-ORGANISATION-TYPE that comprises persons who attempt to profit by violating the law.</rdfs:comment>
    <rdf:type rdf:resource="http://www.w3.org/2002/07/owl#Class"/>
  </rdf:Description>
  <rdf:Description rdf:about="#FACILITY-TYPE_Site,_air-defence_radar">
    <rdfs:subClassOf rdf:resource="jc3iedm_OBJECT-TYPE.owl#FACILITY-TYPE"/>
    <rdfs:label xml:lang="en">site, air defence radar</rdfs:label>
    <rdfs:comment xml:lang="en">A facility containing radar employed for air-defence purposes.</rdfs:comment>
    <rdf:type rdf:resource="http://www.w3.org/2002/07/owl#Class"/>
  </rdf:Description>
  <rdf:Description rdf:about="#CHEMICAL-MATERIEL-TYPE_Not_known">
    <rdfs:subClassOf rdf:resource="jc3iedm_OBJECT-TYPE.owl#CHEMICAL-MATERIEL-TYPE"/>
    <rdfs:label xml:lang="en">not known</rdfs:label>
    <rdfs:comment xml:lang="en">It is not possible to determine which value is most applicable.</rdfs:comment>
    <rdf:type rdf:resource="http://www.w3.org/2002/07/owl#Class"/>
  </rdf:Description>
  <rdf:Description rdf:about="jc3iedm_OBJECT-TYPE.owl#SUBSURFACE-VESSEL-TYPE">
    <rdf:type rdf:resource="http://www.w3.org/2002/07/owl#Class"/>
    <rdfs:label xml:lang="en">subsurface vessel type</rdfs:label>
    <rdfs:comment xml:lang="en">A vessel principally designed to operate under the water surface.</rdfs:comment>
    <rdfs:subClassOf rdf:resource="jc3iedm_OBJECT-TYPE.owl#VESSEL-TYPE"/>
  </rdf:Description>
  <rdf:Description rdf:about="jc3iedm_OBJECT-TYPE.owl#organisation-type-category-code">
    <rdf:type rdf:resource="http://www.w3.org/2002/07/owl#DatatypeProperty"/>
    <rdfs:domain rdf:resource="jc3iedm_OBJECT-TYPE.owl#ORGANISATION-TYPE"/>
    <rdfs:range rdf:resource="http://www.w3.org/2001/XMLSchema#string"/>
  </rdf:Description>
  <rdf:Description rdf:about="#CIVILIAN-POST-TYPE_Department_head">
    <rdfs:subClassOf rdf:resource="jc3iedm_OBJECT-TYPE.owl#CIVILIAN-POST-TYPE"/>
    <rdfs:label xml:lang="en">department head</rdfs:label>
    <rdfs:comment xml:lang="en">A CIVILIAN-POST-TYPE whose job entails the leadership of a separate division or branch of an organisation.</rdfs:comment>
    <rdf:type rdf:resource="http://www.w3.org/2002/07/owl#Class"/>
  </rdf:Description>
  <rdf:Description rdf:about="#FACILITY-TYPE_Orchard/plantation">
    <rdfs:subClassOf rdf:resource="jc3iedm_OBJECT-TYPE.owl#FACILITY-TYPE"/>
    <rdfs:label xml:lang="en">orchard/plantation</rdfs:label>
    <rdfs:comment xml:lang="en">An area covered by systematic plantings of trees that yield fruits, nuts or other products.</rdfs:comment>
    <rdf:type rdf:resource="http://www.w3.org/2002/07/owl#Class"/>
  </rdf:Description>
  <rdf:Description rdf:about="#CONTROL-FEATURE-TYPE_Class-D_airspace">
    <rdfs:subClassOf rdf:resource="jc3iedm_OBJECT-TYPE.owl#CONTROL-FEATURE-TYPE"/>
    <rdfs:label xml:lang="en">class d airspace</rdfs:label>
    <rdfs:comment xml:lang="en">An airspace in which instrument flight rule and visual flight rule flights are permitted; all flights are subject to air traffic control service and instrument flight rule flights are separated from other instrument flight rule flights and receive traffic information in respect to visual flight rule flights. Visual flight rule flights receive traffic information in respect to all other flights.</rdfs:comment>
    <rdf:type rdf:resource="http://www.w3.org/2002/07/owl#Class"/>
  </rdf:Description>
  <rdf:Description rdf:about="#SURFACE-VESSEL-TYPE_Diving_tender_2">
    <rdfs:subClassOf rdf:resource="jc3iedm_OBJECT-TYPE.owl#SURFACE-VESSEL-TYPE"/>
    <rdfs:label xml:lang="en">diving tender 2</rdfs:label>
    <rdfs:comment xml:lang="en">Small craft optimised to act as tender for diving operations.</rdfs:comment>
    <rdf:type rdf:resource="http://www.w3.org/2002/07/owl#Class"/>
  </rdf:Description>
  <rdf:Description rdf:about="#GROUP-ORGANISATION-TYPE_Journalist">
    <rdfs:subClassOf rdf:resource="jc3iedm_OBJECT-TYPE.owl#GROUP-ORGANISATION-TYPE"/>
    <rdfs:label xml:lang="en">journalist</rdfs:label>
    <rdfs:comment xml:lang="en">A GROUP-ORGANISATION-TYPE that comprises persons that earn their living by editing or writing for a public journal.</rdfs:comment>
    <rdf:type rdf:resource="http://www.w3.org/2002/07/owl#Class"/>
  </rdf:Description>
  <rdf:Description rdf:about="#MISCELLANEOUS-EQUIPMENT-TYPE_Line">
    <rdfs:subClassOf rdf:resource="jc3iedm_OBJECT-TYPE.owl#MISCELLANEOUS-EQUIPMENT-TYPE"/>
    <rdfs:label xml:lang="en">line</rdfs:label>
    <rdfs:comment xml:lang="en">A piece of rope, cord, wire serving a special purpose.</rdfs:comment>
    <rdf:type rdf:resource="http://www.w3.org/2002/07/owl#Class"/>
  </rdf:Description>
  <rdf:Description rdf:about="#MILITARY-POST-TYPE_Ground_manoeuvre_commander">
    <rdfs:subClassOf rdf:resource="jc3iedm_OBJECT-TYPE.owl#MILITARY-POST-TYPE"/>
    <rdfs:label xml:lang="en">ground manoeuvre commander</rdfs:label>
    <rdfs:comment xml:lang="en">A MILITARY-POST-TYPE that is identified as the designated commander of a ground manoeuvre unit.</rdfs:comment>
    <rdf:type rdf:resource="http://www.w3.org/2002/07/owl#Class"/>
  </rdf:Description>
  <rdf:Description rdf:about="#CONTROL-FEATURE-TYPE_Main_beam_axis">
    <rdfs:subClassOf rdf:resource="jc3iedm_OBJECT-TYPE.owl#CONTROL-FEATURE-TYPE"/>
    <rdfs:label xml:lang="en">main beam axis</rdfs:label>
    <rdfs:comment xml:lang="en">The direction within the beam of an antenna for which the amplitude of the specified field component is a maximum or about which the beam may be considered symmetrical.</rdfs:comment>
    <rdf:type rdf:resource="http://www.w3.org/2002/07/owl#Class"/>
  </rdf:Description>
  <rdf:Description rdf:about="#FACILITY-TYPE_Washing_facility">
    <rdfs:subClassOf rdf:resource="jc3iedm_OBJECT-TYPE.owl#FACILITY-TYPE"/>
    <rdfs:label xml:lang="en">washing facility</rdfs:label>
    <rdfs:comment xml:lang="en">A facility for washing personnel and/or equipment.</rdfs:comment>
    <rdf:type rdf:resource="http://www.w3.org/2002/07/owl#Class"/>
  </rdf:Description>
  <rdf:Description rdf:about="#VEHICLE-TYPE_Battle_tank,_heavy,_recovery">
    <rdfs:subClassOf rdf:resource="jc3iedm_OBJECT-TYPE.owl#VEHICLE-TYPE"/>
    <rdfs:label xml:lang="en">battle tank, heavy, recovery</rdfs:label>
    <rdfs:comment xml:lang="en">A vehicle designed to recover heavy weight battle tanks.</rdfs:comment>
    <rdf:type rdf:resource="http://www.w3.org/2002/07/owl#Class"/>
  </rdf:Description>
  <rdf:Description rdf:about="#FACILITY-TYPE_Built-up_area">
    <rdfs:subClassOf rdf:resource="jc3iedm_OBJECT-TYPE.owl#FACILITY-TYPE"/>
    <rdfs:label xml:lang="en">built up area</rdfs:label>
    <rdfs:comment xml:lang="en">A facility containing a concentration of buildings and other structures.</rdfs:comment>
    <rdf:type rdf:resource="http://www.w3.org/2002/07/owl#Class"/>
  </rdf:Description>
  <rdf:Description rdf:about="#MILITARY-POST-TYPE_Operations_officer">
    <rdfs:subClassOf rdf:resource="jc3iedm_OBJECT-TYPE.owl#MILITARY-POST-TYPE"/>
    <rdfs:label xml:lang="en">operations officer</rdfs:label>
    <rdfs:comment xml:lang="en">A MILITARY-POST-TYPE that is identified as the officer who is responsible for activities relating to planning and directing military operations.</rdfs:comment>
    <rdf:type rdf:resource="http://www.w3.org/2002/07/owl#Class"/>
  </rdf:Description>
  <rdf:Description rdf:about="#SURFACE-VESSEL-TYPE_Auxiliary_rescue_craft">
    <rdfs:subClassOf rdf:resource="jc3iedm_OBJECT-TYPE.owl#SURFACE-VESSEL-TYPE"/>
    <rdfs:label xml:lang="en">auxiliary rescue craft</rdfs:label>
    <rdfs:comment xml:lang="en">Vessel designed for local rescue operations inshore or offshore.</rdfs:comment>
    <rdf:type rdf:resource="http://www.w3.org/2002/07/owl#Class"/>
  </rdf:Description>
  <rdf:Description rdf:about="#CONTROL-FEATURE-TYPE_Coordination_level">
    <rdfs:subClassOf rdf:resource="jc3iedm_OBJECT-TYPE.owl#CONTROL-FEATURE-TYPE"/>
    <rdfs:label xml:lang="en">coordination level</rdfs:label>
    <rdfs:comment xml:lang="en">A procedural method to separate fixed and rotary wing aircraft by determining an altitude below which fixed wing aircraft normally will not fly.</rdfs:comment>
    <rdf:type rdf:resource="http://www.w3.org/2002/07/owl#Class"/>
  </rdf:Description>
  <rdf:Description rdf:about="#CONTROL-FEATURE-TYPE_Navigation_point">
    <rdfs:subClassOf rdf:resource="jc3iedm_OBJECT-TYPE.owl#CONTROL-FEATURE-TYPE"/>
    <rdfs:label xml:lang="en">navigation point</rdfs:label>
    <rdfs:comment xml:lang="en">The aircraft, ship or other vehicle will change course, speed and/or altitude at this point.</rdfs:comment>
    <rdf:type rdf:resource="http://www.w3.org/2002/07/owl#Class"/>
  </rdf:Description>
  <rdf:Description rdf:about="#SURFACE-VESSEL-TYPE_Lighter,_amphibious,_re-supply,_vehicle">
    <rdfs:subClassOf rdf:resource="jc3iedm_OBJECT-TYPE.owl#SURFACE-VESSEL-TYPE"/>
    <rdfs:label xml:lang="en">lighter, amphibious, re supply, vehicle</rdfs:label>
    <rdfs:comment xml:lang="en">A lighter designed to carry cargo and vehicles for the re-supply of landing forces.</rdfs:comment>
    <rdf:type rdf:resource="http://www.w3.org/2002/07/owl#Class"/>
  </rdf:Description>
  <rdf:Description rdf:about="#FACILITY-TYPE_Shelter,_surface">
    <rdfs:subClassOf rdf:resource="jc3iedm_OBJECT-TYPE.owl#FACILITY-TYPE"/>
    <rdfs:label xml:lang="en">shelter, surface</rdfs:label>
    <rdfs:comment xml:lang="en">A fortified structure built on the surface, used to house personnel and/or equipment.</rdfs:comment>
    <rdf:type rdf:resource="http://www.w3.org/2002/07/owl#Class"/>
  </rdf:Description>
  <rdf:Description rdf:about="#SURFACE-VESSEL-TYPE_Net_tender,_boom">
    <rdfs:subClassOf rdf:resource="jc3iedm_OBJECT-TYPE.owl#SURFACE-VESSEL-TYPE"/>
    <rdfs:label xml:lang="en">net tender, boom</rdfs:label>
    <rdfs:comment xml:lang="en">Craft 40 metres or less used to maintain nets, booms and other harbour defence equipment. May/may not be able to lay and recover same.</rdfs:comment>
    <rdf:type rdf:resource="http://www.w3.org/2002/07/owl#Class"/>
  </rdf:Description>
  <rdf:Description rdf:about="#SURFACE-VESSEL-TYPE_Row_boat">
    <rdfs:subClassOf rdf:resource="jc3iedm_OBJECT-TYPE.owl#SURFACE-VESSEL-TYPE"/>
    <rdfs:label xml:lang="en">row boat</rdfs:label>
    <rdfs:comment xml:lang="en">Vessel powered by oars.</rdfs:comment>
    <rdf:type rdf:resource="http://www.w3.org/2002/07/owl#Class"/>
  </rdf:Description>
  <rdf:Description rdf:about="#SUBSURFACE-VESSEL-TYPE_Deep_submersible_rescue_vehicle_(military)">
    <rdfs:subClassOf rdf:resource="jc3iedm_OBJECT-TYPE.owl#SUBSURFACE-VESSEL-TYPE"/>
    <rdfs:label xml:lang="en">deep submersible rescue vehicle (military)</rdfs:label>
    <rdfs:comment xml:lang="en">Military operated submersible designed for submarine rescue operations at great depth (more than 300 metres) and military operated.</rdfs:comment>
    <rdf:type rdf:resource="http://www.w3.org/2002/07/owl#Class"/>
  </rdf:Description>
  <rdf:Description rdf:about="#SURFACE-VESSEL-TYPE_Auxiliary_ship,_general">
    <rdfs:subClassOf rdf:resource="jc3iedm_OBJECT-TYPE.owl#SURFACE-VESSEL-TYPE"/>
    <rdfs:label xml:lang="en">auxiliary ship, general</rdfs:label>
    <rdfs:comment xml:lang="en">General designator for all naval auxiliary ship types.</rdfs:comment>
    <rdf:type rdf:resource="http://www.w3.org/2002/07/owl#Class"/>
  </rdf:Description>
  <rdf:Description rdf:about="#EXECUTIVE-MILITARY-ORGANISATION-TYPE_Supply">
    <rdfs:subClassOf rdf:resource="jc3iedm_OBJECT-TYPE.owl#EXECUTIVE-MILITARY-ORGANISATION-TYPE"/>
    <rdfs:label xml:lang="en">supply</rdfs:label>
    <rdfs:comment xml:lang="en">An EXECUTIVE-MILITARY-ORGANISATION-TYPE that provides management of supply services.</rdfs:comment>
    <rdf:type rdf:resource="http://www.w3.org/2002/07/owl#Class"/>
  </rdf:Description>
  <rdf:Description rdf:about="jc3iedm_OBJECT-TYPE.owl#materiel-type-stock-number-text">
    <rdf:type rdf:resource="http://www.w3.org/2002/07/owl#DatatypeProperty"/>
    <rdfs:domain rdf:resource="jc3iedm_OBJECT-TYPE.owl#MATERIEL-TYPE"/>
    <rdfs:range rdf:resource="http://www.w3.org/2001/XMLSchema#string"/>
  </rdf:Description>
  <rdf:Description rdf:about="#SURFACE-VESSEL-TYPE_Yard_floating_drydock">
    <rdfs:subClassOf rdf:resource="jc3iedm_OBJECT-TYPE.owl#SURFACE-VESSEL-TYPE"/>
    <rdfs:label xml:lang="en">yard floating drydock</rdfs:label>
    <rdfs:comment xml:lang="en">General designator for floating dry docks.</rdfs:comment>
    <rdf:type rdf:resource="http://www.w3.org/2002/07/owl#Class"/>
  </rdf:Description>
  <rdf:Description rdf:about="#CONTROL-FEATURE-TYPE_Combat_air_patrol_area">
    <rdfs:subClassOf rdf:resource="jc3iedm_OBJECT-TYPE.owl#CONTROL-FEATURE-TYPE"/>
    <rdfs:label xml:lang="en">combat air patrol area</rdfs:label>
    <rdfs:comment xml:lang="en">An area established for aircraft to patrol over an objective area, over the force protected, over the critical area of a combat zone, or over an air defence area, for the purpose of interception and destroying hostile aircraft before they reach their target.</rdfs:comment>
    <rdf:type rdf:resource="http://www.w3.org/2002/07/owl#Class"/>
  </rdf:Description>
  <rdf:Description rdf:about="#SURFACE-VESSEL-TYPE_Auxiliary_aircraft_landing_training_ship">
    <rdfs:subClassOf rdf:resource="jc3iedm_OBJECT-TYPE.owl#SURFACE-VESSEL-TYPE"/>
    <rdfs:label xml:lang="en">auxiliary aircraft landing training ship</rdfs:label>
    <rdfs:comment xml:lang="en">Training carrier for command and fleet carrier qualification requirements.</rdfs:comment>
    <rdf:type rdf:resource="http://www.w3.org/2002/07/owl#Class"/>
  </rdf:Description>
  <rdf:Description rdf:about="#CONTROL-FEATURE-TYPE_Identification_Friend_Foe_switch_off_line">
    <rdfs:subClassOf rdf:resource="jc3iedm_OBJECT-TYPE.owl#CONTROL-FEATURE-TYPE"/>
    <rdfs:label xml:lang="en">identification friend foe switch off line</rdfs:label>
    <rdfs:comment xml:lang="en">Line demarking where friendly aircraft enroute to targets stop emitting an Identification-Friend-Foe signal.</rdfs:comment>
    <rdf:type rdf:resource="http://www.w3.org/2002/07/owl#Class"/>
  </rdf:Description>
  <rdf:Description rdf:about="#FACILITY-TYPE_House">
    <rdfs:subClassOf rdf:resource="jc3iedm_OBJECT-TYPE.owl#FACILITY-TYPE"/>
    <rdfs:label xml:lang="en">house</rdfs:label>
    <rdfs:comment xml:lang="en">A detached household used as a dwelling for one or more persons.</rdfs:comment>
    <rdf:type rdf:resource="http://www.w3.org/2002/07/owl#Class"/>
  </rdf:Description>
  <rdf:Description rdf:about="#VEHICLE-TYPE_Transporter,_tank">
    <rdfs:subClassOf rdf:resource="jc3iedm_OBJECT-TYPE.owl#VEHICLE-TYPE"/>
    <rdfs:label xml:lang="en">transporter, tank</rdfs:label>
    <rdfs:comment xml:lang="en">A vehicle whose primary role is the transportation of main battle tanks.</rdfs:comment>
    <rdf:type rdf:resource="http://www.w3.org/2002/07/owl#Class"/>
  </rdf:Description>
  <rdf:Description rdf:about="#ENGINEERING-EQUIPMENT-TYPE_Mine-clearing">
    <rdfs:subClassOf rdf:resource="jc3iedm_OBJECT-TYPE.owl#ENGINEERING-EQUIPMENT-TYPE"/>
    <rdfs:label xml:lang="en">mine clearing</rdfs:label>
    <rdfs:comment xml:lang="en">An equipment whose purpose is to remove or destroy mines.</rdfs:comment>
    <rdf:type rdf:resource="http://www.w3.org/2002/07/owl#Class"/>
  </rdf:Description>
  <rdf:Description rdf:about="#SURFACE-VESSEL-TYPE_Minesweeper,_coastal,_hydrofoil">
    <rdfs:subClassOf rdf:resource="jc3iedm_OBJECT-TYPE.owl#SURFACE-VESSEL-TYPE"/>
    <rdfs:label xml:lang="en">minesweeper, coastal, hydrofoil</rdfs:label>
    <rdfs:comment xml:lang="en">Non-magnetic minesweeper between 40-70 metres, fitted with hydrofoils.</rdfs:comment>
    <rdf:type rdf:resource="http://www.w3.org/2002/07/owl#Class"/>
  </rdf:Description>
  <rdf:Description rdf:about="jc3iedm_OBJECT-TYPE.owl#biological-materiel-type-subcategory-code">
    <rdf:type rdf:resource="http://www.w3.org/2002/07/owl#DatatypeProperty"/>
    <rdfs:domain rdf:resource="jc3iedm_OBJECT-TYPE.owl#BIOLOGICAL-MATERIEL-TYPE"/>
    <rdfs:range rdf:resource="http://www.w3.org/2001/XMLSchema#string"/>
  </rdf:Description>
  <rdf:Description rdf:about="jc3iedm_OBJECT-TYPE.owl#object-type-name-text">
    <rdf:type rdf:resource="http://www.w3.org/2002/07/owl#DatatypeProperty"/>
    <rdfs:domain rdf:resource="jc3iedm_OBJECT-TYPE.owl#OBJECT-TYPE"/>
    <rdfs:range rdf:resource="http://www.w3.org/2001/XMLSchema#string"/>
  </rdf:Description>
  <rdf:Description rdf:about="#PRIVATE-SECTOR-ORGANISATION-TYPE_News_media">
    <rdfs:subClassOf rdf:resource="jc3iedm_OBJECT-TYPE.owl#PRIVATE-SECTOR-ORGANISATION-TYPE"/>
    <rdfs:label xml:lang="en">news media</rdfs:label>
    <rdfs:comment xml:lang="en">A PRIVATE-SECTOR-ORGANISATION-TYPE whose predominant business is the gathering and dissemination of news.</rdfs:comment>
    <rdf:type rdf:resource="http://www.w3.org/2002/07/owl#Class"/>
  </rdf:Description>
  <rdf:Description rdf:about="#FACILITY-TYPE_Basin">
    <rdfs:subClassOf rdf:resource="jc3iedm_OBJECT-TYPE.owl#FACILITY-TYPE"/>
    <rdfs:label xml:lang="en">basin</rdfs:label>
    <rdfs:comment xml:lang="en">A FACILITY-TYPE that is an open area of water, usually artificial and enclosed by dock gates lined with wharves, warehouses and berths to enable vessels to load and unload.</rdfs:comment>
    <rdf:type rdf:resource="http://www.w3.org/2002/07/owl#Class"/>
  </rdf:Description>
  <rdf:Description rdf:about="#FACILITY-TYPE_Tacan_station">
    <rdfs:subClassOf rdf:resource="jc3iedm_OBJECT-TYPE.owl#FACILITY-TYPE"/>
    <rdfs:label xml:lang="en">tacan station</rdfs:label>
    <rdfs:comment xml:lang="en">A facility used in a global tactical air navigation system.</rdfs:comment>
    <rdf:type rdf:resource="http://www.w3.org/2002/07/owl#Class"/>
  </rdf:Description>
  <rdf:Description rdf:about="#CONTROL-FEATURE-TYPE_Fighter_engagement_zone">
    <rdfs:subClassOf rdf:resource="jc3iedm_OBJECT-TYPE.owl#CONTROL-FEATURE-TYPE"/>
    <rdfs:label xml:lang="en">fighter engagement zone</rdfs:label>
    <rdfs:comment xml:lang="en">The airspace beyond the crossover zone out to limits defined by the officer in tactical command, in which fighters have freedom of action to identify and engage air targets.</rdfs:comment>
    <rdf:type rdf:resource="http://www.w3.org/2002/07/owl#Class"/>
  </rdf:Description>
  <rdf:Description rdf:about="#PRIVATE-SECTOR-ORGANISATION-TYPE_Philanthropic">
    <rdfs:subClassOf rdf:resource="jc3iedm_OBJECT-TYPE.owl#PRIVATE-SECTOR-ORGANISATION-TYPE"/>
    <rdfs:label xml:lang="en">philanthropic</rdfs:label>
    <rdfs:comment xml:lang="en">A PRIVATE-SECTOR-ORGANISATION-TYPE whose predominant business is philanthropic in nature.</rdfs:comment>
    <rdf:type rdf:resource="http://www.w3.org/2002/07/owl#Class"/>
  </rdf:Description>
  <rdf:Description rdf:about="#FACILITY-TYPE_Depot,_nuclear_storage">
    <rdfs:subClassOf rdf:resource="jc3iedm_OBJECT-TYPE.owl#FACILITY-TYPE"/>
    <rdfs:label xml:lang="en">depot, nuclear storage</rdfs:label>
    <rdfs:comment xml:lang="en">An area used for the storage of nuclear weapons.</rdfs:comment>
    <rdf:type rdf:resource="http://www.w3.org/2002/07/owl#Class"/>
  </rdf:Description>
  <rdf:Description rdf:about="jc3iedm_OBJECT-TYPE.owl#WEAPON-TYPE">
    <rdf:type rdf:resource="http://www.w3.org/2002/07/owl#Class"/>
    <rdfs:label xml:lang="en">weapon type</rdfs:label>
    <rdfs:comment xml:lang="en">An EQUIPMENT-TYPE of any kind used in warfare or combat to attack and overcome an enemy.</rdfs:comment>
    <rdfs:subClassOf rdf:resource="jc3iedm_OBJECT-TYPE.owl#EQUIPMENT-TYPE"/>
  </rdf:Description>
  <rdf:Description rdf:about="#SURFACE-VESSEL-TYPE_Landing_craft,_utility,_air_cushion">
    <rdfs:subClassOf rdf:resource="jc3iedm_OBJECT-TYPE.owl#SURFACE-VESSEL-TYPE"/>
    <rdfs:label xml:lang="en">landing craft, utility, air cushion</rdfs:label>
    <rdfs:comment xml:lang="en">All-purpose landing craft in size range 25-55 metres and full load of 120-500 tons with landing ramp/other landing facilities used for handling 2-3 tanks or 300-450 troops with an air cushion or surface effect design.</rdfs:comment>
    <rdf:type rdf:resource="http://www.w3.org/2002/07/owl#Class"/>
  </rdf:Description>
  <rdf:Description rdf:about="#SURFACE-VESSEL-TYPE_Whale_factory_ship">
    <rdfs:subClassOf rdf:resource="jc3iedm_OBJECT-TYPE.owl#SURFACE-VESSEL-TYPE"/>
    <rdfs:label xml:lang="en">whale factory ship</rdfs:label>
    <rdfs:comment xml:lang="en">Vessel equipped to prepare whales into commercial products.</rdfs:comment>
    <rdf:type rdf:resource="http://www.w3.org/2002/07/owl#Class"/>
  </rdf:Description>
  <rdf:Description rdf:about="#SURFACE-VESSEL-TYPE_Amphibious_cargo_ship">
    <rdfs:subClassOf rdf:resource="jc3iedm_OBJECT-TYPE.owl#SURFACE-VESSEL-TYPE"/>
    <rdfs:label xml:lang="en">amphibious cargo ship</rdfs:label>
    <rdfs:comment xml:lang="en">Ship which carries supplies for amphibious assaults and can land the same in its own organic landing craft.</rdfs:comment>
    <rdf:type rdf:resource="http://www.w3.org/2002/07/owl#Class"/>
  </rdf:Description>
  <rdf:Description rdf:about="jc3iedm_OBJECT-TYPE.owl#ammunition-type-calibre-text">
    <rdf:type rdf:resource="http://www.w3.org/2002/07/owl#DatatypeProperty"/>
    <rdfs:domain rdf:resource="jc3iedm_OBJECT-TYPE.owl#AMMUNITION-TYPE"/>
    <rdfs:range rdf:resource="http://www.w3.org/2001/XMLSchema#string"/>
  </rdf:Description>
  <rdf:Description rdf:about="#CONTROL-FEATURE-TYPE_Biologically_contaminated_area">
    <rdfs:subClassOf rdf:resource="jc3iedm_OBJECT-TYPE.owl#CONTROL-FEATURE-TYPE"/>
    <rdfs:label xml:lang="en">biologically contaminated area</rdfs:label>
    <rdfs:comment xml:lang="en">A CONTROL-FEATURE-TYPE that identifies the predicted or confirmed contour of an area in which biological agents may produce casualties in man or animals and damage to plants or materiel.</rdfs:comment>
    <rdf:type rdf:resource="http://www.w3.org/2002/07/owl#Class"/>
  </rdf:Description>
  <rdf:Description rdf:about="#SURFACE-VESSEL-TYPE_Runabout">
    <rdfs:subClassOf rdf:resource="jc3iedm_OBJECT-TYPE.owl#SURFACE-VESSEL-TYPE"/>
    <rdfs:label xml:lang="en">runabout</rdfs:label>
    <rdfs:comment xml:lang="en">Vessel of no specific design used for utility purposes.</rdfs:comment>
    <rdf:type rdf:resource="http://www.w3.org/2002/07/owl#Class"/>
  </rdf:Description>
  <rdf:Description rdf:about="#ELECTRONIC-EQUIPMENT-TYPE_Radar">
    <rdfs:subClassOf rdf:resource="jc3iedm_OBJECT-TYPE.owl#ELECTRONIC-EQUIPMENT-TYPE"/>
    <rdfs:label xml:lang="en">radar</rdfs:label>
    <rdfs:comment xml:lang="en">Radio equipment based on emission of radio waves towards an object and analysis of the waves returned by that object or emitted in response to excitation by the received waves.</rdfs:comment>
    <rdf:type rdf:resource="http://www.w3.org/2002/07/owl#Class"/>
  </rdf:Description>
  <rdf:Description rdf:about="#SURFACE-VESSEL-TYPE_Buoy_tender,_heavy_lift">
    <rdfs:subClassOf rdf:resource="jc3iedm_OBJECT-TYPE.owl#SURFACE-VESSEL-TYPE"/>
    <rdfs:label xml:lang="en">buoy tender, heavy lift</rdfs:label>
    <rdfs:comment xml:lang="en">Ship 40 metres or more employed for the placing and tending of buoys and aids to navigation in coastal and adjoining waters with heavy lift capability.</rdfs:comment>
    <rdf:type rdf:resource="http://www.w3.org/2002/07/owl#Class"/>
  </rdf:Description>
  <rdf:Description rdf:about="#SURFACE-VESSEL-TYPE_Launch">
    <rdfs:subClassOf rdf:resource="jc3iedm_OBJECT-TYPE.owl#SURFACE-VESSEL-TYPE"/>
    <rdfs:label xml:lang="en">launch</rdfs:label>
    <rdfs:comment xml:lang="en">Small craft less than 20 metres employed in sheltered waters for transporting personnel.</rdfs:comment>
    <rdf:type rdf:resource="http://www.w3.org/2002/07/owl#Class"/>
  </rdf:Description>
  <rdf:Description rdf:about="jc3iedm_OBJECT-TYPE.owl#geographic-feature-type-category-code">
    <rdf:type rdf:resource="http://www.w3.org/2002/07/owl#DatatypeProperty"/>
    <rdfs:domain rdf:resource="jc3iedm_OBJECT-TYPE.owl#GEOGRAPHIC-FEATURE-TYPE"/>
    <rdfs:range rdf:resource="http://www.w3.org/2001/XMLSchema#string"/>
  </rdf:Description>
  <rdf:Description rdf:about="#CONTROL-FEATURE-TYPE_Control_point">
    <rdfs:subClassOf rdf:resource="jc3iedm_OBJECT-TYPE.owl#CONTROL-FEATURE-TYPE"/>
    <rdfs:label xml:lang="en">control point</rdfs:label>
    <rdfs:comment xml:lang="en">A position along a route of march at which men are stationed to give information and instructions for the regulation of supply or traffic.</rdfs:comment>
    <rdf:type rdf:resource="http://www.w3.org/2002/07/owl#Class"/>
  </rdf:Description>
  <rdf:Description rdf:about="#WEAPON-TYPE_Missile_system">
    <rdfs:subClassOf rdf:resource="jc3iedm_OBJECT-TYPE.owl#WEAPON-TYPE"/>
    <rdfs:label xml:lang="en">missile system</rdfs:label>
    <rdfs:comment xml:lang="en">A system designed to launch one or more powered guided objects at a target.</rdfs:comment>
    <rdf:type rdf:resource="http://www.w3.org/2002/07/owl#Class"/>
  </rdf:Description>
  <rdf:Description rdf:about="#FACILITY-TYPE_Intelligence_centre,_tactical">
    <rdfs:subClassOf rdf:resource="jc3iedm_OBJECT-TYPE.owl#FACILITY-TYPE"/>
    <rdfs:label xml:lang="en">intelligence centre, tactical</rdfs:label>
    <rdfs:comment xml:lang="en">A facility, at the tactical level, used by intelligence personnel for intelligence operations.</rdfs:comment>
    <rdf:type rdf:resource="http://www.w3.org/2002/07/owl#Class"/>
  </rdf:Description>
  <rdf:Description rdf:about="#SURFACE-VESSEL-TYPE_Launch,_covered">
    <rdfs:subClassOf rdf:resource="jc3iedm_OBJECT-TYPE.owl#SURFACE-VESSEL-TYPE"/>
    <rdfs:label xml:lang="en">launch, covered</rdfs:label>
    <rdfs:comment xml:lang="en">Small craft less than 20 metres employed in sheltered waters for transporting personnel but with covered areas.</rdfs:comment>
    <rdf:type rdf:resource="http://www.w3.org/2002/07/owl#Class"/>
  </rdf:Description>
  <rdf:Description rdf:about="#RADIOACTIVE-MATERIEL-TYPE_Cesium-137">
    <rdfs:subClassOf rdf:resource="jc3iedm_OBJECT-TYPE.owl#RADIOACTIVE-MATERIEL-TYPE"/>
    <rdfs:label xml:lang="en">cesium 137</rdfs:label>
    <rdfs:comment xml:lang="en">A radioactive isotope of the chemical element of atomic number 55, a soft, silvery, rare, extremely reactive metal of the alkali metal group.</rdfs:comment>
    <rdf:type rdf:resource="http://www.w3.org/2002/07/owl#Class"/>
  </rdf:Description>
  <rdf:Description rdf:about="#GROUP-ORGANISATION-TYPE_Media,_international">
    <rdfs:subClassOf rdf:resource="jc3iedm_OBJECT-TYPE.owl#GROUP-ORGANISATION-TYPE"/>
    <rdfs:label xml:lang="en">media, international</rdfs:label>
    <rdfs:comment xml:lang="en">A GROUP-ORGANISATION-TYPE that comprises persons that report for international mass communications, but do not take part in the actions.</rdfs:comment>
    <rdf:type rdf:resource="http://www.w3.org/2002/07/owl#Class"/>
  </rdf:Description>
  <rdf:Description rdf:about="#FACILITY-TYPE_Industrial_installation">
    <rdfs:subClassOf rdf:resource="jc3iedm_OBJECT-TYPE.owl#FACILITY-TYPE"/>
    <rdfs:label xml:lang="en">industrial installation</rdfs:label>
    <rdfs:comment xml:lang="en">A facility containing factories and/or productive installations.</rdfs:comment>
    <rdf:type rdf:resource="http://www.w3.org/2002/07/owl#Class"/>
  </rdf:Description>
  <rdf:Description rdf:about="#SURFACE-VESSEL-TYPE_Hospital_ship">
    <rdfs:subClassOf rdf:resource="jc3iedm_OBJECT-TYPE.owl#SURFACE-VESSEL-TYPE"/>
    <rdfs:label xml:lang="en">hospital ship</rdfs:label>
    <rdfs:comment xml:lang="en">Ship of at least 40 metres which provides 3rd line medical and surgical care. Declared to and protected by the ICRC (International Committee of the Red Cross/red crescent (TU ships only)) and marked accordingly.</rdfs:comment>
    <rdf:type rdf:resource="http://www.w3.org/2002/07/owl#Class"/>
  </rdf:Description>
  <rdf:Description rdf:about="#AIRFIELD-TYPE_Civil">
    <rdfs:subClassOf rdf:resource="jc3iedm_OBJECT-TYPE.owl#AIRFIELD-TYPE"/>
    <rdfs:label xml:lang="en">civil</rdfs:label>
    <rdfs:comment xml:lang="en">Civil airports controlled and operated by civil authorities primarily used by civil aircrafts although military aircrafts may have landing privileges and/or contract rights.</rdfs:comment>
    <rdf:type rdf:resource="http://www.w3.org/2002/07/owl#Class"/>
  </rdf:Description>
  <rdf:Description rdf:about="#PRIVATE-SECTOR-ORGANISATION-TYPE_Not_otherwise_specified">
    <rdfs:subClassOf rdf:resource="jc3iedm_OBJECT-TYPE.owl#PRIVATE-SECTOR-ORGANISATION-TYPE"/>
    <rdfs:label xml:lang="en">not otherwise specified</rdfs:label>
    <rdfs:comment xml:lang="en">The appropriate value is not in the set of specified values.</rdfs:comment>
    <rdf:type rdf:resource="http://www.w3.org/2002/07/owl#Class"/>
  </rdf:Description>
  <rdf:Description rdf:about="#SUBSURFACE-VESSEL-TYPE_Submarine,_ballistic_missile">
    <rdfs:subClassOf rdf:resource="jc3iedm_OBJECT-TYPE.owl#SUBSURFACE-VESSEL-TYPE"/>
    <rdfs:label xml:lang="en">submarine, ballistic missile</rdfs:label>
    <rdfs:comment xml:lang="en">A subsurface vessel designed to deliver ballistic missile attacks against assigned targets from either a submerged or surfaced condition.</rdfs:comment>
    <rdf:type rdf:resource="http://www.w3.org/2002/07/owl#Class"/>
  </rdf:Description>
  <rdf:Description rdf:about="#CONTROL-FEATURE-TYPE_Coordinating_point">
    <rdfs:subClassOf rdf:resource="jc3iedm_OBJECT-TYPE.owl#CONTROL-FEATURE-TYPE"/>
    <rdfs:label xml:lang="en">coordinating point</rdfs:label>
    <rdfs:comment xml:lang="en">Designated point at which, in all types of combat, adjacent units/formations must make contact for purposes of control and coordination. Army--A control measure that indicates a specific location for the coordination of fires and manoeuvre between adjacent units. They usually are indicated whenever a boundary crosses the forward battle area (FEBA), and may be indicated when a boundary crosses phase lines (PLs) used to control security forces.</rdfs:comment>
    <rdf:type rdf:resource="http://www.w3.org/2002/07/owl#Class"/>
  </rdf:Description>
  <rdf:Description rdf:about="#VEHICLE-TYPE_Semi">
    <rdfs:subClassOf rdf:resource="jc3iedm_OBJECT-TYPE.owl#VEHICLE-TYPE"/>
    <rdfs:label xml:lang="en">semi</rdfs:label>
    <rdfs:comment xml:lang="en">A road trailer that has a wheel system at the rear only and is coupled to a suitable tractor to form an articulated lorry.</rdfs:comment>
    <rdf:type rdf:resource="http://www.w3.org/2002/07/owl#Class"/>
  </rdf:Description>
  <rdf:Description rdf:about="#SURFACE-VESSEL-TYPE_Attack_boat,_guided_missile,_training">
    <rdfs:subClassOf rdf:resource="jc3iedm_OBJECT-TYPE.owl#SURFACE-VESSEL-TYPE"/>
    <rdfs:label xml:lang="en">attack boat, guided missile, training</rdfs:label>
    <rdfs:comment xml:lang="en">High speed (35 knots - 65 km/hr) anti-surface ship patrol craft in size range 20 - 30 metres fitted with torpedoes and with force guided missile system and used primarily in a training role.</rdfs:comment>
    <rdf:type rdf:resource="http://www.w3.org/2002/07/owl#Class"/>
  </rdf:Description>
  <rdf:Description rdf:about="#SURFACE-VESSEL-TYPE_Personnel_transport">
    <rdfs:subClassOf rdf:resource="jc3iedm_OBJECT-TYPE.owl#SURFACE-VESSEL-TYPE"/>
    <rdfs:label xml:lang="en">personnel transport</rdfs:label>
    <rdfs:comment xml:lang="en">Ship of at least 120 metres employed to transport troops, their supplies and equipment.</rdfs:comment>
    <rdf:type rdf:resource="http://www.w3.org/2002/07/owl#Class"/>
  </rdf:Description>
  <rdf:Description rdf:about="#CONTROL-FEATURE-TYPE_Carrier_control_zone">
    <rdfs:subClassOf rdf:resource="jc3iedm_OBJECT-TYPE.owl#CONTROL-FEATURE-TYPE"/>
    <rdfs:label xml:lang="en">carrier control zone</rdfs:label>
    <rdfs:comment xml:lang="en">Area around a ship operating fixed/rotary wing aircraft.</rdfs:comment>
    <rdf:type rdf:resource="http://www.w3.org/2002/07/owl#Class"/>
  </rdf:Description>
  <rdf:Description rdf:about="#HARBOUR-TYPE_Open_roadstead">
    <rdfs:subClassOf rdf:resource="jc3iedm_OBJECT-TYPE.owl#HARBOUR-TYPE"/>
    <rdfs:label xml:lang="en">open roadstead</rdfs:label>
    <rdfs:comment xml:lang="en">A port, which has no artificial barrier to provide shelter from the wind, sea and swell.</rdfs:comment>
    <rdf:type rdf:resource="http://www.w3.org/2002/07/owl#Class"/>
  </rdf:Description>
  <rdf:Description rdf:about="#CONTROL-FEATURE-TYPE_Release_line">
    <rdfs:subClassOf rdf:resource="jc3iedm_OBJECT-TYPE.owl#CONTROL-FEATURE-TYPE"/>
    <rdfs:label xml:lang="en">release line</rdfs:label>
    <rdfs:comment xml:lang="en">Phase line used in river-crossing operations that delineates a change in the headquarters controlling movement.</rdfs:comment>
    <rdf:type rdf:resource="http://www.w3.org/2002/07/owl#Class"/>
  </rdf:Description>
  <rdf:Description rdf:about="#CONTROL-FEATURE-TYPE_End_of_mission_point">
    <rdfs:subClassOf rdf:resource="jc3iedm_OBJECT-TYPE.owl#CONTROL-FEATURE-TYPE"/>
    <rdfs:label xml:lang="en">end of mission point</rdfs:label>
    <rdfs:comment xml:lang="en">The mission will terminate at the specific point.</rdfs:comment>
    <rdf:type rdf:resource="http://www.w3.org/2002/07/owl#Class"/>
  </rdf:Description>
  <rdf:Description rdf:about="#ROUTE-TYPE_Special_corridor">
    <rdfs:subClassOf rdf:resource="jc3iedm_OBJECT-TYPE.owl#ROUTE-TYPE"/>
    <rdfs:label xml:lang="en">special corridor</rdfs:label>
    <rdfs:comment xml:lang="en">An area established to accommodate the special routing requirements of specific missions.</rdfs:comment>
    <rdf:type rdf:resource="http://www.w3.org/2002/07/owl#Class"/>
  </rdf:Description>
  <rdf:Description rdf:about="#SURFACE-VESSEL-TYPE_Floating_crane">
    <rdfs:subClassOf rdf:resource="jc3iedm_OBJECT-TYPE.owl#SURFACE-VESSEL-TYPE"/>
    <rdfs:label xml:lang="en">floating crane</rdfs:label>
    <rdfs:comment xml:lang="en">Barge-like vessels usually non-self-propelled equipped with a crane.</rdfs:comment>
    <rdf:type rdf:resource="http://www.w3.org/2002/07/owl#Class"/>
  </rdf:Description>
  <rdf:Description rdf:about="jc3iedm_OBJECT-TYPE.owl#electronic-equipment-type-subcategory-code">
    <rdf:type rdf:resource="http://www.w3.org/2002/07/owl#DatatypeProperty"/>
    <rdfs:domain rdf:resource="jc3iedm_OBJECT-TYPE.owl#ELECTRONIC-EQUIPMENT-TYPE"/>
    <rdfs:range rdf:resource="http://www.w3.org/2001/XMLSchema#string"/>
  </rdf:Description>
  <rdf:Description rdf:about="#FACILITY-TYPE_Decontamination_facility">
    <rdfs:subClassOf rdf:resource="jc3iedm_OBJECT-TYPE.owl#FACILITY-TYPE"/>
    <rdfs:label xml:lang="en">decontamination facility</rdfs:label>
    <rdfs:comment xml:lang="en">A facility where personnel and/or materiel (incl. vehicles) can be cleaned after (potential) contamination of radioactive, biological, or chemical material.</rdfs:comment>
    <rdf:type rdf:resource="http://www.w3.org/2002/07/owl#Class"/>
  </rdf:Description>
  <rdf:Description rdf:about="#CONTROL-FEATURE-TYPE_Boundary,_airspace">
    <rdfs:subClassOf rdf:resource="jc3iedm_OBJECT-TYPE.owl#CONTROL-FEATURE-TYPE"/>
    <rdfs:label xml:lang="en">boundary, airspace</rdfs:label>
    <rdfs:comment xml:lang="en">The lateral limits of an airspace control area, airspace control sub-area, high-density airspace control zone or airspace restricted area.</rdfs:comment>
    <rdf:type rdf:resource="http://www.w3.org/2002/07/owl#Class"/>
  </rdf:Description>
  <rdf:Description rdf:about="#FACILITY-TYPE_Ferry_installation">
    <rdfs:subClassOf rdf:resource="jc3iedm_OBJECT-TYPE.owl#FACILITY-TYPE"/>
    <rdfs:label xml:lang="en">ferry installation</rdfs:label>
    <rdfs:comment xml:lang="en">A facility (including the terminals and the water craft) to enable moving equipment and personnel across a body of water.</rdfs:comment>
    <rdf:type rdf:resource="http://www.w3.org/2002/07/owl#Class"/>
  </rdf:Description>
  <rdf:Description rdf:about="#FACILITY-TYPE_Monument">
    <rdfs:subClassOf rdf:resource="jc3iedm_OBJECT-TYPE.owl#FACILITY-TYPE"/>
    <rdfs:label xml:lang="en">monument</rdfs:label>
    <rdfs:comment xml:lang="en">A structure generally created for commemorative purposes.</rdfs:comment>
    <rdf:type rdf:resource="http://www.w3.org/2002/07/owl#Class"/>
  </rdf:Description>
  <rdf:Description rdf:about="#FACILITY-TYPE_Maintenance_facility">
    <rdfs:subClassOf rdf:resource="jc3iedm_OBJECT-TYPE.owl#FACILITY-TYPE"/>
    <rdfs:label xml:lang="en">maintenance facility</rdfs:label>
    <rdfs:comment xml:lang="en">A facility containing the resources and infrastructure to enable it to be used for the repair and servicing of equipment.</rdfs:comment>
    <rdf:type rdf:resource="http://www.w3.org/2002/07/owl#Class"/>
  </rdf:Description>
  <rdf:Description rdf:about="#MILITARY-POST-TYPE_Forward_air_controller">
    <rdfs:subClassOf rdf:resource="jc3iedm_OBJECT-TYPE.owl#MILITARY-POST-TYPE"/>
    <rdfs:label xml:lang="en">forward air controller</rdfs:label>
    <rdfs:comment xml:lang="en">A MILITARY-POST-TYPE that is identified as the member of the tactical air control party who, from a forward ground or airborne position, controls aircraft in close air support of ground troops.</rdfs:comment>
    <rdf:type rdf:resource="http://www.w3.org/2002/07/owl#Class"/>
  </rdf:Description>
  <rdf:Description rdf:about="#MILITARY-OBSTACLE-TYPE_Minefield,_anti-tank">
    <rdfs:subClassOf rdf:resource="jc3iedm_OBJECT-TYPE.owl#MILITARY-OBSTACLE-TYPE"/>
    <rdfs:label xml:lang="en">minefield, anti tank</rdfs:label>
    <rdfs:comment xml:lang="en">An obstacle made by laying mines of anti-tank type laid with or without pattern.</rdfs:comment>
    <rdf:type rdf:resource="http://www.w3.org/2002/07/owl#Class"/>
  </rdf:Description>
  <rdf:Description rdf:about="jc3iedm_OBJECT-TYPE.owl#PERSON-TYPE">
    <rdf:type rdf:resource="http://www.w3.org/2002/07/owl#Class"/>
    <rdfs:label xml:lang="en">person type</rdfs:label>
    <rdfs:comment xml:lang="en">An OBJECT-TYPE that represents human beings about whom information is to be held.</rdfs:comment>
  </rdf:Description>
  <rdf:Description rdf:about="#CONTROL-FEATURE-TYPE_Contact_point,_land">
    <rdfs:subClassOf rdf:resource="jc3iedm_OBJECT-TYPE.owl#CONTROL-FEATURE-TYPE"/>
    <rdfs:label xml:lang="en">contact point, land</rdfs:label>
    <rdfs:comment xml:lang="en">A CONTROL-FEATURE-TYPE with an easily identifiable point location, where two or more units are required to make contact.</rdfs:comment>
    <rdf:type rdf:resource="http://www.w3.org/2002/07/owl#Class"/>
  </rdf:Description>
  <rdf:Description rdf:about="#AIRCRAFT-TYPE_Heavy">
    <rdfs:subClassOf rdf:resource="jc3iedm_OBJECT-TYPE.owl#AIRCRAFT-TYPE"/>
    <rdfs:label xml:lang="en">heavy</rdfs:label>
    <rdfs:comment xml:lang="en">An aircraft is capable of lifting heavy loads.</rdfs:comment>
    <rdf:type rdf:resource="http://www.w3.org/2002/07/owl#Class"/>
  </rdf:Description>
  <rdf:Description rdf:about="#FACILITY-TYPE_Reservoir">
    <rdfs:subClassOf rdf:resource="jc3iedm_OBJECT-TYPE.owl#FACILITY-TYPE"/>
    <rdfs:label xml:lang="en">reservoir</rdfs:label>
    <rdfs:comment xml:lang="en">A man-made open enclosure or area formed for the storage of water.</rdfs:comment>
    <rdf:type rdf:resource="http://www.w3.org/2002/07/owl#Class"/>
  </rdf:Description>
  <rdf:Description rdf:about="#ORGANISATION-TYPE_Airborne_warning_and_control_system">
    <rdfs:subClassOf rdf:resource="jc3iedm_OBJECT-TYPE.owl#ORGANISATION-TYPE"/>
    <rdfs:label xml:lang="en">airborne warning and control system</rdfs:label>
    <rdfs:comment xml:lang="en">The ORGANISATION-TYPE that is an Airborne Warning and Control System (AWACS) aircraft that provides all-weather surveillance, command, control and communications needed by commanders of air defence forces.</rdfs:comment>
    <rdf:type rdf:resource="http://www.w3.org/2002/07/owl#Class"/>
  </rdf:Description>
  <rdf:Description rdf:about="jc3iedm_OBJECT-TYPE.owl#vessel-type-propulsion-type-code">
    <rdf:type rdf:resource="http://www.w3.org/2002/07/owl#DatatypeProperty"/>
    <rdfs:domain rdf:resource="jc3iedm_OBJECT-TYPE.owl#VESSEL-TYPE"/>
    <rdfs:range rdf:resource="http://www.w3.org/2001/XMLSchema#string"/>
  </rdf:Description>
  <rdf:Description rdf:about="#SURFACE-VESSEL-TYPE_Destroyer,_general">
    <rdfs:subClassOf rdf:resource="jc3iedm_OBJECT-TYPE.owl#SURFACE-VESSEL-TYPE"/>
    <rdfs:label xml:lang="en">destroyer, general</rdfs:label>
    <rdfs:comment xml:lang="en">General designator for destroyer type ships. Major surface combatant in range of about 95 to 140 metres whole general mission is to conduct operations with strike, ASW and amphibious forces, and to perform screening and convoy duties. May have helicopters not especially fitted for ASW.</rdfs:comment>
    <rdf:type rdf:resource="http://www.w3.org/2002/07/owl#Class"/>
  </rdf:Description>
  <rdf:Description rdf:about="#FACILITY-TYPE_Electrical_supply">
    <rdfs:subClassOf rdf:resource="jc3iedm_OBJECT-TYPE.owl#FACILITY-TYPE"/>
    <rdfs:label xml:lang="en">electrical supply</rdfs:label>
    <rdfs:comment xml:lang="en">A facility containing the equipment used for the production and/or distribution of electricity.</rdfs:comment>
    <rdf:type rdf:resource="http://www.w3.org/2002/07/owl#Class"/>
  </rdf:Description>
  <rdf:Description rdf:about="#VEHICLE-TYPE_Armoured">
    <rdfs:subClassOf rdf:resource="jc3iedm_OBJECT-TYPE.owl#VEHICLE-TYPE"/>
    <rdfs:label xml:lang="en">armoured</rdfs:label>
    <rdfs:comment xml:lang="en">A vehicle that has some form of ballistic protection (excluding tanks).</rdfs:comment>
    <rdf:type rdf:resource="http://www.w3.org/2002/07/owl#Class"/>
  </rdf:Description>
  <rdf:Description rdf:about="#MILITARY-OBSTACLE-TYPE_Anti-tank_obstacle">
    <rdfs:subClassOf rdf:resource="jc3iedm_OBJECT-TYPE.owl#MILITARY-OBSTACLE-TYPE"/>
    <rdfs:label xml:lang="en">anti tank obstacle</rdfs:label>
    <rdfs:comment xml:lang="en">A facility that is an obstacle that is designed or employed to disrupt, fix, turn or block the movement of tanks.</rdfs:comment>
    <rdf:type rdf:resource="http://www.w3.org/2002/07/owl#Class"/>
  </rdf:Description>
  <rdf:Description rdf:about="#CONTROL-FEATURE-TYPE_Pop-up_point">
    <rdfs:subClassOf rdf:resource="jc3iedm_OBJECT-TYPE.owl#CONTROL-FEATURE-TYPE"/>
    <rdfs:label xml:lang="en">pop up point</rdfs:label>
    <rdfs:comment xml:lang="en">The location at which aircraft quickly gain altitude for target acquisition and engagement.</rdfs:comment>
    <rdf:type rdf:resource="http://www.w3.org/2002/07/owl#Class"/>
  </rdf:Description>
  <rdf:Description rdf:about="#SURFACE-VESSEL-TYPE_Landing_ship,_dock">
    <rdfs:subClassOf rdf:resource="jc3iedm_OBJECT-TYPE.owl#SURFACE-VESSEL-TYPE"/>
    <rdfs:label xml:lang="en">landing ship, dock</rdfs:label>
    <rdfs:comment xml:lang="en">Primarily a tank and vehicle carrier but capable of transporting 150-400 assault troops and launch them embarked in organic landing craft without off-loading in the landing area. Need not have a helicopter platform.</rdfs:comment>
    <rdf:type rdf:resource="http://www.w3.org/2002/07/owl#Class"/>
  </rdf:Description>
  <rdf:Description rdf:about="#SURFACE-VESSEL-TYPE_Minelayer,_coastal">
    <rdfs:subClassOf rdf:resource="jc3iedm_OBJECT-TYPE.owl#SURFACE-VESSEL-TYPE"/>
    <rdfs:label xml:lang="en">minelayer, coastal</rdfs:label>
    <rdfs:comment xml:lang="en">Minelayer in size range 50 - 85 metres overall.</rdfs:comment>
    <rdf:type rdf:resource="http://www.w3.org/2002/07/owl#Class"/>
  </rdf:Description>
  <rdf:Description rdf:about="#CONTROL-FEATURE-TYPE_Axis_of_advance">
    <rdfs:subClassOf rdf:resource="jc3iedm_OBJECT-TYPE.owl#CONTROL-FEATURE-TYPE"/>
    <rdfs:label xml:lang="en">axis of advance</rdfs:label>
    <rdfs:comment xml:lang="en">A general route of advance, assigned for control, which extends towards the enemy. An axis of advance symbol graphically portrays a commander’s intention, such as avoidance of built-up areas or envelopment of an enemy force. It follows terrain suitable for the size of the force to which the axis was assigned, and is often a road, a group of roads, or a designated series of locations. An axis of advance is not used to direct the control of terrain or the clearance of enemy forces from specific locations. Intermediate objectives are normally assigned for these purposes.</rdfs:comment>
    <rdf:type rdf:resource="http://www.w3.org/2002/07/owl#Class"/>
  </rdf:Description>
  <rdf:Description rdf:about="#CONTROL-FEATURE-TYPE_Forward_line_of_troops">
    <rdfs:subClassOf rdf:resource="jc3iedm_OBJECT-TYPE.owl#CONTROL-FEATURE-TYPE"/>
    <rdfs:label xml:lang="en">forward line of troops</rdfs:label>
    <rdfs:comment xml:lang="en">Line indicating the most forward positions of friendly forces in any kind of military operation at a specific time.</rdfs:comment>
    <rdf:type rdf:resource="http://www.w3.org/2002/07/owl#Class"/>
  </rdf:Description>
  <rdf:Description rdf:about="#CONTROL-FEATURE-TYPE_Line_of_departure,_land">
    <rdfs:subClassOf rdf:resource="jc3iedm_OBJECT-TYPE.owl#CONTROL-FEATURE-TYPE"/>
    <rdfs:label xml:lang="en">line of departure, land</rdfs:label>
    <rdfs:comment xml:lang="en">A line designated to coordinate the departure of attack elements (commitment of attacking units or scouting elements at a specific time).</rdfs:comment>
    <rdf:type rdf:resource="http://www.w3.org/2002/07/owl#Class"/>
  </rdf:Description>
  <rdf:Description rdf:about="#CHEMICAL-MATERIEL-TYPE_Vomiting_agent">
    <rdfs:subClassOf rdf:resource="jc3iedm_OBJECT-TYPE.owl#CHEMICAL-MATERIEL-TYPE"/>
    <rdfs:label xml:lang="en">vomiting agent</rdfs:label>
    <rdfs:comment xml:lang="en">A CHEMICAL-MATERIEL-TYPE that is designed to incapacitate by inducing vomiting in humans.</rdfs:comment>
    <rdf:type rdf:resource="http://www.w3.org/2002/07/owl#Class"/>
  </rdf:Description>
  <rdf:Description rdf:about="#ORGANISATION-TYPE_Air_control_centre">
    <rdfs:subClassOf rdf:resource="jc3iedm_OBJECT-TYPE.owl#ORGANISATION-TYPE"/>
    <rdfs:label xml:lang="en">air control centre</rdfs:label>
    <rdfs:comment xml:lang="en">No definition provided in ADatP-3 Baseline 13.1 FFIRN/FUD 1874/4.</rdfs:comment>
    <rdf:type rdf:resource="http://www.w3.org/2002/07/owl#Class"/>
  </rdf:Description>
  <rdf:Description rdf:about="#MILITARY-POST-TYPE_Other_physician">
    <rdfs:subClassOf rdf:resource="jc3iedm_OBJECT-TYPE.owl#MILITARY-POST-TYPE"/>
    <rdfs:label xml:lang="en">other physician</rdfs:label>
    <rdfs:comment xml:lang="en">A MILITARY-POST-TYPE that is identified as a physician with an unidentified speciality.</rdfs:comment>
    <rdf:type rdf:resource="http://www.w3.org/2002/07/owl#Class"/>
  </rdf:Description>
  <rdf:Description rdf:about="#SURFACE-VESSEL-TYPE_Barge,_repair_and_berthing">
    <rdfs:subClassOf rdf:resource="jc3iedm_OBJECT-TYPE.owl#SURFACE-VESSEL-TYPE"/>
    <rdfs:label xml:lang="en">barge, repair and berthing</rdfs:label>
    <rdfs:comment xml:lang="en">Craft which both serves as a floating work ship and has berthing facilities for the assigned personnel. May/may not provide messing facilities as well.</rdfs:comment>
    <rdf:type rdf:resource="http://www.w3.org/2002/07/owl#Class"/>
  </rdf:Description>
  <rdf:Description rdf:about="#SURFACE-VESSEL-TYPE_Launch,_hydrofoil">
    <rdfs:subClassOf rdf:resource="jc3iedm_OBJECT-TYPE.owl#SURFACE-VESSEL-TYPE"/>
    <rdfs:label xml:lang="en">launch, hydrofoil</rdfs:label>
    <rdfs:comment xml:lang="en">Small craft less than 20 metres employed in sheltered waters for transporting personnel, but fitted with hydrofoils.</rdfs:comment>
    <rdf:type rdf:resource="http://www.w3.org/2002/07/owl#Class"/>
  </rdf:Description>
  <rdf:Description rdf:about="#SURFACE-VESSEL-TYPE_Tug,_harbour,_medium">
    <rdfs:subClassOf rdf:resource="jc3iedm_OBJECT-TYPE.owl#SURFACE-VESSEL-TYPE"/>
    <rdfs:label xml:lang="en">tug, harbour, medium</rdfs:label>
    <rdfs:comment xml:lang="en">Harbour tug between 20-40 metres with total horsepower between 500 and 1300.</rdfs:comment>
    <rdf:type rdf:resource="http://www.w3.org/2002/07/owl#Class"/>
  </rdf:Description>
  <rdf:Description rdf:about="#SURFACE-VESSEL-TYPE_Training_craft,_sail">
    <rdfs:subClassOf rdf:resource="jc3iedm_OBJECT-TYPE.owl#SURFACE-VESSEL-TYPE"/>
    <rdfs:label xml:lang="en">training craft, sail</rdfs:label>
    <rdfs:comment xml:lang="en">Sailing craft of any size used for training.</rdfs:comment>
    <rdf:type rdf:resource="http://www.w3.org/2002/07/owl#Class"/>
  </rdf:Description>
  <rdf:Description rdf:about="#FACILITY-TYPE_Improved_bed,_type_unknown">
    <rdfs:subClassOf rdf:resource="jc3iedm_OBJECT-TYPE.owl#FACILITY-TYPE"/>
    <rdfs:label xml:lang="en">improved bed, type unknown</rdfs:label>
    <rdfs:comment xml:lang="en">No definition provided in ADatP-3 Baseline 13.1 FFIRN/FUD 1650/6.</rdfs:comment>
    <rdf:type rdf:resource="http://www.w3.org/2002/07/owl#Class"/>
  </rdf:Description>
  <rdf:Description rdf:about="#ORGANISATION-TYPE_Marine_tactical_air_direction_centre">
    <rdfs:subClassOf rdf:resource="jc3iedm_OBJECT-TYPE.owl#ORGANISATION-TYPE"/>
    <rdfs:label xml:lang="en">marine tactical air direction centre</rdfs:label>
    <rdfs:comment xml:lang="en">The ORGANISATION-TYPE that is under the overall control of the tactical air control centre (afloat) or tactical air command centre, from which aircraft and air warning service functions of tactical air operations in an area of concern are directed.</rdfs:comment>
    <rdf:type rdf:resource="http://www.w3.org/2002/07/owl#Class"/>
  </rdf:Description>
  <rdf:Description rdf:about="#CONTROL-FEATURE-TYPE_Weapons_free_zone">
    <rdfs:subClassOf rdf:resource="jc3iedm_OBJECT-TYPE.owl#CONTROL-FEATURE-TYPE"/>
    <rdfs:label xml:lang="en">weapons free zone</rdfs:label>
    <rdfs:comment xml:lang="en">An air defence zone (ADZ) established around key assets or facilities which merit special protection by ground based air defence assets, other than airbases, where weapons may be fired at any target not positively identified as friendly.</rdfs:comment>
    <rdf:type rdf:resource="http://www.w3.org/2002/07/owl#Class"/>
  </rdf:Description>
  <rdf:Description rdf:about="#FACILITY-TYPE_Trench">
    <rdfs:subClassOf rdf:resource="jc3iedm_OBJECT-TYPE.owl#FACILITY-TYPE"/>
    <rdfs:label xml:lang="en">trench</rdfs:label>
    <rdfs:comment xml:lang="en">A linear excavation dug for defensive purposes.</rdfs:comment>
    <rdf:type rdf:resource="http://www.w3.org/2002/07/owl#Class"/>
  </rdf:Description>
  <rdf:Description rdf:about="#SUBSURFACE-VESSEL-TYPE_Submarine,_attack,_nuclear">
    <rdfs:subClassOf rdf:resource="jc3iedm_OBJECT-TYPE.owl#SUBSURFACE-VESSEL-TYPE"/>
    <rdfs:label xml:lang="en">submarine, attack, nuclear</rdfs:label>
    <rdfs:comment xml:lang="en">Nuclear propelled attack submarine with both anti-submarine and anti-surface capability.</rdfs:comment>
    <rdf:type rdf:resource="http://www.w3.org/2002/07/owl#Class"/>
  </rdf:Description>
  <rdf:Description rdf:about="#VEHICLE-TYPE_Military_utility">
    <rdfs:subClassOf rdf:resource="jc3iedm_OBJECT-TYPE.owl#VEHICLE-TYPE"/>
    <rdfs:label xml:lang="en">military utility</rdfs:label>
    <rdfs:comment xml:lang="en">A small, sturdy, four-wheel-drive army vehicle, used chiefly for reconnaissance; a similar vehicle in non-military use.</rdfs:comment>
    <rdf:type rdf:resource="http://www.w3.org/2002/07/owl#Class"/>
  </rdf:Description>
  <rdf:Description rdf:about="#CHEMICAL-MATERIEL-TYPE_Mustard_agent">
    <rdfs:subClassOf rdf:resource="jc3iedm_OBJECT-TYPE.owl#CHEMICAL-MATERIEL-TYPE"/>
    <rdfs:label xml:lang="en">mustard agent</rdfs:label>
    <rdfs:comment xml:lang="en">A potentially lethal CHEMICAL-MATERIEL-TYPE, which is a colourless oily liquid whose vapour is a powerful irritant and vesicant, used in chemical weapons.</rdfs:comment>
    <rdf:type rdf:resource="http://www.w3.org/2002/07/owl#Class"/>
  </rdf:Description>
  <rdf:Description rdf:about="#">
    <owl:imports rdf:resource="jc3iedm_OBJECT-TYPE.owl#"/>
    <rdf:type rdf:resource="http://www.w3.org/2002/07/owl#Ontology"/>
  </rdf:Description>
  <rdf:Description rdf:about="#CONTROL-FEATURE-TYPE_Maritime_missile_engagement_zone">
    <rdfs:subClassOf rdf:resource="jc3iedm_OBJECT-TYPE.owl#CONTROL-FEATURE-TYPE"/>
    <rdfs:label xml:lang="en">maritime missile engagement zone</rdfs:label>
    <rdfs:comment xml:lang="en">A designated airspace in which, under weapons control status weapons free, ships are automatically cleared to fire at any target which penetrates the zone, unless known to be friendly, adhering to airspace control procedures or unless otherwise directed by the anti-air warfare commander.</rdfs:comment>
    <rdf:type rdf:resource="http://www.w3.org/2002/07/owl#Class"/>
  </rdf:Description>
  <rdf:Description rdf:about="#SURFACE-VESSEL-TYPE_Stores_ship_issue,_small_(naval)">
    <rdfs:subClassOf rdf:resource="jc3iedm_OBJECT-TYPE.owl#SURFACE-VESSEL-TYPE"/>
    <rdfs:label xml:lang="en">stores ship issue, small (naval)</rdfs:label>
    <rdfs:comment xml:lang="en">Ship less than 40 metres or more used to provide supplies and services.</rdfs:comment>
    <rdf:type rdf:resource="http://www.w3.org/2002/07/owl#Class"/>
  </rdf:Description>
  <rdf:Description rdf:about="#SURFACE-VESSEL-TYPE_Repair_ship,_cable">
    <rdfs:subClassOf rdf:resource="jc3iedm_OBJECT-TYPE.owl#SURFACE-VESSEL-TYPE"/>
    <rdfs:label xml:lang="en">repair ship, cable</rdfs:label>
    <rdfs:comment xml:lang="en">Ship 40 metres or more employed to lay, retrieve and maintain submarine cables.</rdfs:comment>
    <rdf:type rdf:resource="http://www.w3.org/2002/07/owl#Class"/>
  </rdf:Description>
  <rdf:Description rdf:about="#FACILITY-TYPE_Detainee_holding_area">
    <rdfs:subClassOf rdf:resource="jc3iedm_OBJECT-TYPE.owl#FACILITY-TYPE"/>
    <rdfs:label xml:lang="en">detainee holding area</rdfs:label>
    <rdfs:comment xml:lang="en">A facility where detainees are provided custodial care pending further disposition.</rdfs:comment>
    <rdf:type rdf:resource="http://www.w3.org/2002/07/owl#Class"/>
  </rdf:Description>
  <rdf:Description rdf:about="#SURFACE-VESSEL-TYPE_Barracks_ship">
    <rdfs:subClassOf rdf:resource="jc3iedm_OBJECT-TYPE.owl#SURFACE-VESSEL-TYPE"/>
    <rdfs:label xml:lang="en">barracks ship</rdfs:label>
    <rdfs:comment xml:lang="en">A self-propelled of any size employed as a mobile base facility and support ship for the crews of other vessels (usually small craft) and has no repair facilities.</rdfs:comment>
    <rdf:type rdf:resource="http://www.w3.org/2002/07/owl#Class"/>
  </rdf:Description>
  <rdf:Description rdf:about="#CONTROL-FEATURE-TYPE_Takeoff_point">
    <rdfs:subClassOf rdf:resource="jc3iedm_OBJECT-TYPE.owl#CONTROL-FEATURE-TYPE"/>
    <rdfs:label xml:lang="en">takeoff point</rdfs:label>
    <rdfs:comment xml:lang="en">The aircraft will take off from the route point.</rdfs:comment>
    <rdf:type rdf:resource="http://www.w3.org/2002/07/owl#Class"/>
  </rdf:Description>
  <rdf:Description rdf:about="#BIOLOGICAL-MATERIEL-TYPE_Viral">
    <rdfs:subClassOf rdf:resource="jc3iedm_OBJECT-TYPE.owl#BIOLOGICAL-MATERIEL-TYPE"/>
    <rdfs:label xml:lang="en">viral</rdfs:label>
    <rdfs:comment xml:lang="en">A generic term for a BIOLOGICAL-MATERIEL-TYPE of the nature of a virus; submicroscopic infective particle, typically consisting of nucleic acid coated in protein, which is able to multiply within the cells of a host organism.</rdfs:comment>
    <rdf:type rdf:resource="http://www.w3.org/2002/07/owl#Class"/>
  </rdf:Description>
  <rdf:Description rdf:about="#CONTROL-FEATURE-TYPE_Air_defence_action_area">
    <rdfs:subClassOf rdf:resource="jc3iedm_OBJECT-TYPE.owl#CONTROL-FEATURE-TYPE"/>
    <rdfs:label xml:lang="en">air defence action area</rdfs:label>
    <rdfs:comment xml:lang="en">An area and the airspace above it within which friendly aircraft or surface-to-air weapons are normally given precedence in operations except under specified conditions.</rdfs:comment>
    <rdf:type rdf:resource="http://www.w3.org/2002/07/owl#Class"/>
  </rdf:Description>
  <rdf:Description rdf:about="#CONTROL-FEATURE-TYPE_Control_zone">
    <rdfs:subClassOf rdf:resource="jc3iedm_OBJECT-TYPE.owl#CONTROL-FEATURE-TYPE"/>
    <rdfs:label xml:lang="en">control zone</rdfs:label>
    <rdfs:comment xml:lang="en">A controlled airspace extending upwards from the surface of the earth to a specified upper limit.</rdfs:comment>
    <rdf:type rdf:resource="http://www.w3.org/2002/07/owl#Class"/>
  </rdf:Description>
  <rdf:Description rdf:about="#SURFACE-VESSEL-TYPE_Fishing_vessel,_inspection">
    <rdfs:subClassOf rdf:resource="jc3iedm_OBJECT-TYPE.owl#SURFACE-VESSEL-TYPE"/>
    <rdfs:label xml:lang="en">fishing vessel, inspection</rdfs:label>
    <rdfs:comment xml:lang="en">Any ship other than naval used for inspection of fishing vessels.</rdfs:comment>
    <rdf:type rdf:resource="http://www.w3.org/2002/07/owl#Class"/>
  </rdf:Description>
  <rdf:Description rdf:about="#RADIOACTIVE-MATERIEL-TYPE_Not_known">
    <rdfs:subClassOf rdf:resource="jc3iedm_OBJECT-TYPE.owl#RADIOACTIVE-MATERIEL-TYPE"/>
    <rdfs:label xml:lang="en">not known</rdfs:label>
    <rdfs:comment xml:lang="en">It is not possible to determine which value is most applicable.</rdfs:comment>
    <rdf:type rdf:resource="http://www.w3.org/2002/07/owl#Class"/>
  </rdf:Description>
  <rdf:Description rdf:about="#GROUP-ORGANISATION-TYPE_Prisoner">
    <rdfs:subClassOf rdf:resource="jc3iedm_OBJECT-TYPE.owl#GROUP-ORGANISATION-TYPE"/>
    <rdfs:label xml:lang="en">prisoner</rdfs:label>
    <rdfs:comment xml:lang="en">A GROUP-ORGANISATION-TYPE in custody on a criminal charge and on trial.</rdfs:comment>
    <rdf:type rdf:resource="http://www.w3.org/2002/07/owl#Class"/>
  </rdf:Description>
  <rdf:Description rdf:about="#FACILITY-TYPE_Site,_surface_to_surface_missile">
    <rdfs:subClassOf rdf:resource="jc3iedm_OBJECT-TYPE.owl#FACILITY-TYPE"/>
    <rdfs:label xml:lang="en">site, surface to surface missile</rdfs:label>
    <rdfs:comment xml:lang="en">An installation dedicated to the storage and launch of surface-to-surface missiles.</rdfs:comment>
    <rdf:type rdf:resource="http://www.w3.org/2002/07/owl#Class"/>
  </rdf:Description>
  <rdf:Description rdf:about="#SURFACE-VESSEL-TYPE_Lighter,_open">
    <rdfs:subClassOf rdf:resource="jc3iedm_OBJECT-TYPE.owl#SURFACE-VESSEL-TYPE"/>
    <rdfs:label xml:lang="en">lighter, open</rdfs:label>
    <rdfs:comment xml:lang="en">Barge-like vessel used in loading and unloading ships or in transporting loads for short distances.</rdfs:comment>
    <rdf:type rdf:resource="http://www.w3.org/2002/07/owl#Class"/>
  </rdf:Description>
  <rdf:Description rdf:about="#CONTROL-FEATURE-TYPE_Attack_position">
    <rdfs:subClassOf rdf:resource="jc3iedm_OBJECT-TYPE.owl#CONTROL-FEATURE-TYPE"/>
    <rdfs:label xml:lang="en">attack position</rdfs:label>
    <rdfs:comment xml:lang="en">The last position occupied or passed through by the assault echelon before crossing the line of departure (LD).</rdfs:comment>
    <rdf:type rdf:resource="http://www.w3.org/2002/07/owl#Class"/>
  </rdf:Description>
  <rdf:Description rdf:about="jc3iedm_OBJECT-TYPE.owl#unit-type-size-code">
    <rdf:type rdf:resource="http://www.w3.org/2002/07/owl#DatatypeProperty"/>
    <rdfs:domain rdf:resource="jc3iedm_OBJECT-TYPE.owl#UNIT-TYPE"/>
    <rdfs:range rdf:resource="http://www.w3.org/2001/XMLSchema#string"/>
  </rdf:Description>
  <rdf:Description rdf:about="#SURFACE-VESSEL-TYPE_Landing_craft,_swimmer_support">
    <rdfs:subClassOf rdf:resource="jc3iedm_OBJECT-TYPE.owl#SURFACE-VESSEL-TYPE"/>
    <rdfs:label xml:lang="en">landing craft, swimmer support</rdfs:label>
    <rdfs:comment xml:lang="en">High-speed craft utilised primarily for underwater demolition and/or special warfare operations.</rdfs:comment>
    <rdf:type rdf:resource="http://www.w3.org/2002/07/owl#Class"/>
  </rdf:Description>
  <rdf:Description rdf:about="#CONTROL-FEATURE-TYPE_Combat_zone">
    <rdfs:subClassOf rdf:resource="jc3iedm_OBJECT-TYPE.owl#CONTROL-FEATURE-TYPE"/>
    <rdfs:label xml:lang="en">combat zone</rdfs:label>
    <rdfs:comment xml:lang="en">A CONTROL-FEATURE-TYPE with an area location that denotes the area required by combat forces for the conduct of operations.</rdfs:comment>
    <rdf:type rdf:resource="http://www.w3.org/2002/07/owl#Class"/>
  </rdf:Description>
  <rdf:Description rdf:about="#SUBSURFACE-VESSEL-TYPE_Not_otherwise_specified">
    <rdfs:subClassOf rdf:resource="jc3iedm_OBJECT-TYPE.owl#SUBSURFACE-VESSEL-TYPE"/>
    <rdfs:label xml:lang="en">not otherwise specified</rdfs:label>
    <rdfs:comment xml:lang="en">The appropriate value is not in the set of specified values.</rdfs:comment>
    <rdf:type rdf:resource="http://www.w3.org/2002/07/owl#Class"/>
  </rdf:Description>
  <rdf:Description rdf:about="#CONTROL-FEATURE-TYPE_Airspace_coordination_area">
    <rdfs:subClassOf rdf:resource="jc3iedm_OBJECT-TYPE.owl#CONTROL-FEATURE-TYPE"/>
    <rdfs:label xml:lang="en">airspace coordination area</rdfs:label>
    <rdfs:comment xml:lang="en">A CONTROL-FEATURE-TYPE that is a three-dimensional block of airspace in a target area, established by the appropriate ground commander, in which friendly aircraft are reasonably safe from friendly surface fire. The ACA may be formal or informal.</rdfs:comment>
    <rdf:type rdf:resource="http://www.w3.org/2002/07/owl#Class"/>
  </rdf:Description>
  <rdf:Description rdf:about="#SURFACE-VESSEL-TYPE_Destroyer,_coast_guard">
    <rdfs:subClassOf rdf:resource="jc3iedm_OBJECT-TYPE.owl#SURFACE-VESSEL-TYPE"/>
    <rdfs:label xml:lang="en">destroyer, coast guard</rdfs:label>
    <rdfs:comment xml:lang="en">A coast guard destroyer type ship. Major surface combatant in range of about 95 to 140 metres whole general mission is to conduct operations with strike, ASW and amphibious forces, and to perform screening and convoy duties. May have helicopters not especially fitted for ASW.</rdfs:comment>
    <rdf:type rdf:resource="http://www.w3.org/2002/07/owl#Class"/>
  </rdf:Description>
  <rdf:Description rdf:about="#SURFACE-VESSEL-TYPE_Patrol_craft,_hydrofoil,_fast">
    <rdfs:subClassOf rdf:resource="jc3iedm_OBJECT-TYPE.owl#SURFACE-VESSEL-TYPE"/>
    <rdfs:label xml:lang="en">patrol craft, hydrofoil, fast</rdfs:label>
    <rdfs:comment xml:lang="en">Vessel in size range 35-55 metres designed and fitted primarily for escort duties in ASW role. It is capable of at least 35 knots and is fitted with hydrofoils.</rdfs:comment>
    <rdf:type rdf:resource="http://www.w3.org/2002/07/owl#Class"/>
  </rdf:Description>
  <rdf:Description rdf:about="#CONTROL-FEATURE-TYPE_Free_fire_area">
    <rdfs:subClassOf rdf:resource="jc3iedm_OBJECT-TYPE.owl#CONTROL-FEATURE-TYPE"/>
    <rdfs:label xml:lang="en">free fire area</rdfs:label>
    <rdfs:comment xml:lang="en">Supplementary permissive fire support coordination measure, established to facilitate the rapid engagement of targets of opportunity, into which any weapon system may fire without additional coordination with the establishing headquarters.</rdfs:comment>
    <rdf:type rdf:resource="http://www.w3.org/2002/07/owl#Class"/>
  </rdf:Description>
  <rdf:Description rdf:about="#FACILITY-TYPE_Meteorological_facility">
    <rdfs:subClassOf rdf:resource="jc3iedm_OBJECT-TYPE.owl#FACILITY-TYPE"/>
    <rdfs:label xml:lang="en">meteorological facility</rdfs:label>
    <rdfs:comment xml:lang="en">A facility that supports the study of or the science of, the motions and phenomena of the atmosphere, with a view to forecasting the weather.</rdfs:comment>
    <rdf:type rdf:resource="http://www.w3.org/2002/07/owl#Class"/>
  </rdf:Description>
  <rdf:Description rdf:about="#TASK-FORMATION-TYPE_Naval_task_unit">
    <rdfs:subClassOf rdf:resource="jc3iedm_OBJECT-TYPE.owl#TASK-FORMATION-TYPE"/>
    <rdfs:label xml:lang="en">naval task unit</rdfs:label>
    <rdfs:comment xml:lang="en">A TASK-FORMATION-TYPE that is a component of a task group organized by the commander of a task group or higher authority for accomplishing specific tasks.</rdfs:comment>
    <rdf:type rdf:resource="http://www.w3.org/2002/07/owl#Class"/>
  </rdf:Description>
  <rdf:Description rdf:about="#TASK-FORMATION-TYPE_Air_formation">
    <rdfs:subClassOf rdf:resource="jc3iedm_OBJECT-TYPE.owl#TASK-FORMATION-TYPE"/>
    <rdfs:label xml:lang="en">air formation</rdfs:label>
    <rdfs:comment xml:lang="en">An ordered arrangement of two or more aircraft proceeding together under a commander.</rdfs:comment>
    <rdf:type rdf:resource="http://www.w3.org/2002/07/owl#Class"/>
  </rdf:Description>
  <rdf:Description rdf:about="#MISCELLANEOUS-EQUIPMENT-TYPE_Lamp">
    <rdfs:subClassOf rdf:resource="jc3iedm_OBJECT-TYPE.owl#MISCELLANEOUS-EQUIPMENT-TYPE"/>
    <rdfs:label xml:lang="en">lamp</rdfs:label>
    <rdfs:comment xml:lang="en">An equipment that is used to provide light to illuminate the location of an equipment, e.g a buoy.</rdfs:comment>
    <rdf:type rdf:resource="http://www.w3.org/2002/07/owl#Class"/>
  </rdf:Description>
  <rdf:Description rdf:about="#FACILITY-TYPE_Road">
    <rdfs:subClassOf rdf:resource="jc3iedm_OBJECT-TYPE.owl#FACILITY-TYPE"/>
    <rdfs:label xml:lang="en">road</rdfs:label>
    <rdfs:comment xml:lang="en">An open way maintained for vehicular use.</rdfs:comment>
    <rdf:type rdf:resource="http://www.w3.org/2002/07/owl#Class"/>
  </rdf:Description>
  <rdf:Description rdf:about="#CONTROL-FEATURE-TYPE_Assembly_area,_general">
    <rdfs:subClassOf rdf:resource="jc3iedm_OBJECT-TYPE.owl#CONTROL-FEATURE-TYPE"/>
    <rdfs:label xml:lang="en">assembly area, general</rdfs:label>
    <rdfs:comment xml:lang="en">An area in which a command is assembled preparatory to further action.</rdfs:comment>
    <rdf:type rdf:resource="http://www.w3.org/2002/07/owl#Class"/>
  </rdf:Description>
  <rdf:Description rdf:about="#MARITIME-EQUIPMENT-TYPE_Cutter">
    <rdfs:subClassOf rdf:resource="jc3iedm_OBJECT-TYPE.owl#MARITIME-EQUIPMENT-TYPE"/>
    <rdfs:label xml:lang="en">cutter</rdfs:label>
    <rdfs:comment xml:lang="en">In naval mine warfare a device fitted to a sweep wire to cut or part the mooring of mines or obstructors. It may also be fitted in, or to, the mooring of a mine or obstructors to part a sweep wire.</rdfs:comment>
    <rdf:type rdf:resource="http://www.w3.org/2002/07/owl#Class"/>
  </rdf:Description>
  <rdf:Description rdf:about="#CONTROL-FEATURE-TYPE_Reduced_coordination_airspace">
    <rdfs:subClassOf rdf:resource="jc3iedm_OBJECT-TYPE.owl#CONTROL-FEATURE-TYPE"/>
    <rdfs:label xml:lang="en">reduced coordination airspace</rdfs:label>
    <rdfs:comment xml:lang="en">A portion of defined dimensions within which general air traffic (GAT) is permitted "off-route" without requiring GAT controllers to initiate coordination with operational air traffic (OAT) controllers.</rdfs:comment>
    <rdf:type rdf:resource="http://www.w3.org/2002/07/owl#Class"/>
  </rdf:Description>
  <rdf:Description rdf:about="jc3iedm_OBJECT-TYPE.owl#CIVILIAN-POST-TYPE">
    <rdf:type rdf:resource="http://www.w3.org/2002/07/owl#Class"/>
    <rdfs:label xml:lang="en">civilian post type</rdfs:label>
    <rdfs:comment xml:lang="en">An ORGANISATION-TYPE with a set of duties that are intended to be fulfilled by one person in private sector and non-military government organisations.</rdfs:comment>
    <rdfs:subClassOf rdf:resource="jc3iedm_OBJECT-TYPE.owl#ORGANISATION-TYPE"/>
  </rdf:Description>
  <rdf:Description rdf:about="#SURFACE-VESSEL-TYPE_Amphibious_force_flagship_or_amphibious_command_ship">
    <rdfs:subClassOf rdf:resource="jc3iedm_OBJECT-TYPE.owl#SURFACE-VESSEL-TYPE"/>
    <rdfs:label xml:lang="en">amphibious force flagship or amphibious command ship</rdfs:label>
    <rdfs:comment xml:lang="en">Command ship for amphibious task force and landing operations. May carry a limited number of troops and supplies for the headquarters element of the landing force.</rdfs:comment>
    <rdf:type rdf:resource="http://www.w3.org/2002/07/owl#Class"/>
  </rdf:Description>
  <rdf:Description rdf:about="#SURFACE-VESSEL-TYPE_Barge,_garbage">
    <rdfs:subClassOf rdf:resource="jc3iedm_OBJECT-TYPE.owl#SURFACE-VESSEL-TYPE"/>
    <rdfs:label xml:lang="en">barge, garbage</rdfs:label>
    <rdfs:comment xml:lang="en">Self-propelled craft used for the collection of garbage.</rdfs:comment>
    <rdf:type rdf:resource="http://www.w3.org/2002/07/owl#Class"/>
  </rdf:Description>
  <rdf:Description rdf:about="#CONTROL-FEATURE-TYPE_Right_radial_line">
    <rdfs:subClassOf rdf:resource="jc3iedm_OBJECT-TYPE.owl#CONTROL-FEATURE-TYPE"/>
    <rdfs:label xml:lang="en">right radial line</rdfs:label>
    <rdfs:comment xml:lang="en">The line extending outward from the area of Secondary Hazard marking the maximum extent to the right (facing in the effective downwind direction) where significant fallout is expected to occur.</rdfs:comment>
    <rdf:type rdf:resource="http://www.w3.org/2002/07/owl#Class"/>
  </rdf:Description>
  <rdf:Description rdf:about="#SURFACE-VESSEL-TYPE_Hovercraft,_scientific_research/survey">
    <rdfs:subClassOf rdf:resource="jc3iedm_OBJECT-TYPE.owl#SURFACE-VESSEL-TYPE"/>
    <rdfs:label xml:lang="en">hovercraft, scientific research/survey</rdfs:label>
    <rdfs:comment xml:lang="en">Non-military hovercraft specially equipped for research or survey duties.</rdfs:comment>
    <rdf:type rdf:resource="http://www.w3.org/2002/07/owl#Class"/>
  </rdf:Description>
  <rdf:Description rdf:about="#CONTROL-FEATURE-TYPE_Staging_area">
    <rdfs:subClassOf rdf:resource="jc3iedm_OBJECT-TYPE.owl#CONTROL-FEATURE-TYPE"/>
    <rdfs:label xml:lang="en">staging area</rdfs:label>
    <rdfs:comment xml:lang="en">A CONTROL-FEATURE-TYPE that is a general locality established for the concentration of organisations and transient persons between movements over the lines of communications.</rdfs:comment>
    <rdf:type rdf:resource="http://www.w3.org/2002/07/owl#Class"/>
  </rdf:Description>
  <rdf:Description rdf:about="#CONTROL-FEATURE-TYPE_Altitude_reservation_area">
    <rdfs:subClassOf rdf:resource="jc3iedm_OBJECT-TYPE.owl#CONTROL-FEATURE-TYPE"/>
    <rdfs:label xml:lang="en">altitude reservation area</rdfs:label>
    <rdfs:comment xml:lang="en">Block of altitude, normally medium to high, reserved for aircraft to transit or loiter within the Force Air Coordination Area (FACA) for mission accomplishment.</rdfs:comment>
    <rdf:type rdf:resource="http://www.w3.org/2002/07/owl#Class"/>
  </rdf:Description>
  <rdf:Description rdf:about="jc3iedm_OBJECT-TYPE.owl#military-obstacle-type-subcategory-code">
    <rdf:type rdf:resource="http://www.w3.org/2002/07/owl#DatatypeProperty"/>
    <rdfs:domain rdf:resource="jc3iedm_OBJECT-TYPE.owl#MILITARY-OBSTACLE-TYPE"/>
    <rdfs:range rdf:resource="http://www.w3.org/2001/XMLSchema#string"/>
  </rdf:Description>
  <rdf:Description rdf:about="#CONTROL-FEATURE-TYPE_Contact_point,_air">
    <rdfs:subClassOf rdf:resource="jc3iedm_OBJECT-TYPE.owl#CONTROL-FEATURE-TYPE"/>
    <rdfs:label xml:lang="en">contact point, air</rdfs:label>
    <rdfs:comment xml:lang="en">A CONTROL-FEATURE-TYPE that identifies the position at which a mission leader makes radio contact with an air control agency. Note: A point used for control purposes in air-to-air refuelling and close air support missions.</rdfs:comment>
    <rdf:type rdf:resource="http://www.w3.org/2002/07/owl#Class"/>
  </rdf:Description>
  <rdf:Description rdf:about="#SUBSURFACE-VESSEL-TYPE_Submarine,_military_capability_unknown,_nuclear_powered">
    <rdfs:subClassOf rdf:resource="jc3iedm_OBJECT-TYPE.owl#SUBSURFACE-VESSEL-TYPE"/>
    <rdfs:label xml:lang="en">submarine, military capability unknown, nuclear powered</rdfs:label>
    <rdfs:comment xml:lang="en">Submarine with nuclear power whose full military capability is unknown or has not been determined.</rdfs:comment>
    <rdf:type rdf:resource="http://www.w3.org/2002/07/owl#Class"/>
  </rdf:Description>
  <rdf:Description rdf:about="#CHEMICAL-MATERIEL-TYPE_Penetrating_agent">
    <rdfs:subClassOf rdf:resource="jc3iedm_OBJECT-TYPE.owl#CHEMICAL-MATERIEL-TYPE"/>
    <rdfs:label xml:lang="en">penetrating agent</rdfs:label>
    <rdfs:comment xml:lang="en">A CHEMICAL-MATERIEL-TYPE that is designed to penetrate the individual and collective equipment, therefore enabling an associated lethal agent to act.</rdfs:comment>
    <rdf:type rdf:resource="http://www.w3.org/2002/07/owl#Class"/>
  </rdf:Description>
  <rdf:Description rdf:about="#SURFACE-VESSEL-TYPE_Launch,_covered,_large">
    <rdfs:subClassOf rdf:resource="jc3iedm_OBJECT-TYPE.owl#SURFACE-VESSEL-TYPE"/>
    <rdfs:label xml:lang="en">launch, covered, large</rdfs:label>
    <rdfs:comment xml:lang="en">Small craft over 20 metres employed in sheltered waters for transporting personnel.</rdfs:comment>
    <rdf:type rdf:resource="http://www.w3.org/2002/07/owl#Class"/>
  </rdf:Description>
  <rdf:Description rdf:about="#FACILITY-TYPE_Electronic_installation,_radar_dome">
    <rdfs:subClassOf rdf:resource="jc3iedm_OBJECT-TYPE.owl#FACILITY-TYPE"/>
    <rdfs:label xml:lang="en">electronic installation, radar dome</rdfs:label>
    <rdfs:comment xml:lang="en">A cover usually intended for protecting radar from the effects of its physical environment without degrading significantly its electrical performance.</rdfs:comment>
    <rdf:type rdf:resource="http://www.w3.org/2002/07/owl#Class"/>
  </rdf:Description>
  <rdf:Description rdf:about="#CONTROL-FEATURE-TYPE_Alert_area">
    <rdfs:subClassOf rdf:resource="jc3iedm_OBJECT-TYPE.owl#CONTROL-FEATURE-TYPE"/>
    <rdfs:label xml:lang="en">alert area</rdfs:label>
    <rdfs:comment xml:lang="en">Airspace which may contain a high volume of pilot training activities or an unusual type of aerial activity, neither of which is hazardous to aircraft.</rdfs:comment>
    <rdf:type rdf:resource="http://www.w3.org/2002/07/owl#Class"/>
  </rdf:Description>
  <rdf:Description rdf:about="#CONTROL-FEATURE-TYPE_Training_area">
    <rdfs:subClassOf rdf:resource="jc3iedm_OBJECT-TYPE.owl#CONTROL-FEATURE-TYPE"/>
    <rdfs:label xml:lang="en">training area</rdfs:label>
    <rdfs:comment xml:lang="en">Battlespace created during a contingency for the purpose of conducting training.</rdfs:comment>
    <rdf:type rdf:resource="http://www.w3.org/2002/07/owl#Class"/>
  </rdf:Description>
  <rdf:Description rdf:about="#SURFACE-VESSEL-TYPE_Ketch">
    <rdfs:subClassOf rdf:resource="jc3iedm_OBJECT-TYPE.owl#SURFACE-VESSEL-TYPE"/>
    <rdfs:label xml:lang="en">ketch</rdfs:label>
    <rdfs:comment xml:lang="en">Vessel of specific design, usually powered by sail.</rdfs:comment>
    <rdf:type rdf:resource="http://www.w3.org/2002/07/owl#Class"/>
  </rdf:Description>
  <rdf:Description rdf:about="#MISCELLANEOUS-EQUIPMENT-TYPE_Paper">
    <rdfs:subClassOf rdf:resource="jc3iedm_OBJECT-TYPE.owl#MISCELLANEOUS-EQUIPMENT-TYPE"/>
    <rdfs:label xml:lang="en">paper</rdfs:label>
    <rdfs:comment xml:lang="en">A substance composed of fibres for writing, printing or drawing on.</rdfs:comment>
    <rdf:type rdf:resource="http://www.w3.org/2002/07/owl#Class"/>
  </rdf:Description>
  <rdf:Description rdf:about="#ENGINEERING-EQUIPMENT-TYPE_Bridge_launching_vehicle,_armoured">
    <rdfs:subClassOf rdf:resource="jc3iedm_OBJECT-TYPE.owl#ENGINEERING-EQUIPMENT-TYPE"/>
    <rdfs:label xml:lang="en">bridge launching vehicle, armoured</rdfs:label>
    <rdfs:comment xml:lang="en">A bridge that is carried on an armoured vehicle and is deployed from the vehicle for immediate use (VBPP, AVLB).</rdfs:comment>
    <rdf:type rdf:resource="http://www.w3.org/2002/07/owl#Class"/>
  </rdf:Description>
  <rdf:Description rdf:about="jc3iedm_OBJECT-TYPE.owl#control-feature-type-category-code">
    <rdf:type rdf:resource="http://www.w3.org/2002/07/owl#DatatypeProperty"/>
    <rdfs:domain rdf:resource="jc3iedm_OBJECT-TYPE.owl#CONTROL-FEATURE-TYPE"/>
    <rdfs:range rdf:resource="http://www.w3.org/2001/XMLSchema#string"/>
  </rdf:Description>
  <rdf:Description rdf:about="#FACILITY-TYPE_Service,_research,_utility_facility,_technological_research_facility">
    <rdfs:subClassOf rdf:resource="jc3iedm_OBJECT-TYPE.owl#FACILITY-TYPE"/>
    <rdfs:label xml:lang="en">service, research, utility facility, technological research facility</rdfs:label>
    <rdfs:comment xml:lang="en">A facility generally used to support service, research or utility functions in support of technological research.</rdfs:comment>
    <rdf:type rdf:resource="http://www.w3.org/2002/07/owl#Class"/>
  </rdf:Description>
  <rdf:Description rdf:about="#MILITARY-OBSTACLE-TYPE_Wire_obstacle,_single_fence">
    <rdfs:subClassOf rdf:resource="jc3iedm_OBJECT-TYPE.owl#MILITARY-OBSTACLE-TYPE"/>
    <rdfs:label xml:lang="en">wire obstacle, single fence</rdfs:label>
    <rdfs:comment xml:lang="en">No definition provided in APP-6A.</rdfs:comment>
    <rdf:type rdf:resource="http://www.w3.org/2002/07/owl#Class"/>
  </rdf:Description>
  <rdf:Description rdf:about="#PERSON-TYPE_Not_otherwise_specified">
    <rdfs:subClassOf rdf:resource="jc3iedm_OBJECT-TYPE.owl#PERSON-TYPE"/>
    <rdfs:label xml:lang="en">not otherwise specified</rdfs:label>
    <rdfs:comment xml:lang="en">The appropriate value is not in the set of specified values.</rdfs:comment>
    <rdf:type rdf:resource="http://www.w3.org/2002/07/owl#Class"/>
  </rdf:Description>
  <rdf:Description rdf:about="#CONTROL-FEATURE-TYPE_Forming_up_place">
    <rdfs:subClassOf rdf:resource="jc3iedm_OBJECT-TYPE.owl#CONTROL-FEATURE-TYPE"/>
    <rdfs:label xml:lang="en">forming up place</rdfs:label>
    <rdfs:comment xml:lang="en">The last position occupied by the assault echelon before crossing the start line/line of departure.</rdfs:comment>
    <rdf:type rdf:resource="http://www.w3.org/2002/07/owl#Class"/>
  </rdf:Description>
  <rdf:Description rdf:about="#AMMUNITION-TYPE_Mine,_not_otherwise_specified">
    <rdfs:subClassOf rdf:resource="jc3iedm_OBJECT-TYPE.owl#AMMUNITION-TYPE"/>
    <rdfs:label xml:lang="en">mine, not otherwise specified</rdfs:label>
    <rdfs:comment xml:lang="en">A mine whose appropriate value is not in the set of specified values.</rdfs:comment>
    <rdf:type rdf:resource="http://www.w3.org/2002/07/owl#Class"/>
  </rdf:Description>
  <rdf:Description rdf:about="#SURFACE-VESSEL-TYPE_Minehunter,_coastal_with_drone">
    <rdfs:subClassOf rdf:resource="jc3iedm_OBJECT-TYPE.owl#SURFACE-VESSEL-TYPE"/>
    <rdfs:label xml:lang="en">minehunter, coastal with drone</rdfs:label>
    <rdfs:comment xml:lang="en">Ship equipped with specific equipment to hunt mines by the use of a drone.</rdfs:comment>
    <rdf:type rdf:resource="http://www.w3.org/2002/07/owl#Class"/>
  </rdf:Description>
  <rdf:Description rdf:about="jc3iedm_OBJECT-TYPE.owl#maritime-equipment-type-subcategory-code">
    <rdf:type rdf:resource="http://www.w3.org/2002/07/owl#DatatypeProperty"/>
    <rdfs:domain rdf:resource="jc3iedm_OBJECT-TYPE.owl#MARITIME-EQUIPMENT-TYPE"/>
    <rdfs:range rdf:resource="http://www.w3.org/2001/XMLSchema#string"/>
  </rdf:Description>
  <rdf:Description rdf:about="jc3iedm_OBJECT-TYPE.owl#aircraft-type-takeoff-and-landing-code">
    <rdf:type rdf:resource="http://www.w3.org/2002/07/owl#DatatypeProperty"/>
    <rdfs:domain rdf:resource="jc3iedm_OBJECT-TYPE.owl#AIRCRAFT-TYPE"/>
    <rdfs:range rdf:resource="http://www.w3.org/2001/XMLSchema#string"/>
  </rdf:Description>
  <rdf:Description rdf:about="#CONTROL-FEATURE-TYPE_End_aerial_refuelling_point">
    <rdfs:subClassOf rdf:resource="jc3iedm_OBJECT-TYPE.owl#CONTROL-FEATURE-TYPE"/>
    <rdfs:label xml:lang="en">end aerial refuelling point</rdfs:label>
    <rdfs:comment xml:lang="en">A CONTROL-FEATURE-TYPE that identifies the point that marks the end of a straight-line segment along which a tanker aircraft offloads fuel to a receiving aircraft.</rdfs:comment>
    <rdf:type rdf:resource="http://www.w3.org/2002/07/owl#Class"/>
  </rdf:Description>
  <rdf:Description rdf:about="#SURFACE-VESSEL-TYPE_Merchant_ship,_seabee">
    <rdfs:subClassOf rdf:resource="jc3iedm_OBJECT-TYPE.owl#SURFACE-VESSEL-TYPE"/>
    <rdfs:label xml:lang="en">merchant ship, seabee</rdfs:label>
    <rdfs:comment xml:lang="en">Non-naval barge carrying ship with a stern elevator, capable of embarking and disembarking barges of non-standard size.</rdfs:comment>
    <rdf:type rdf:resource="http://www.w3.org/2002/07/owl#Class"/>
  </rdf:Description>
  <rdf:Description rdf:about="#SURFACE-VESSEL-TYPE_Aircraft_carrier,_helicopter/VSTOL,_guided_missile,_nuclear_powered">
    <rdfs:subClassOf rdf:resource="jc3iedm_OBJECT-TYPE.owl#SURFACE-VESSEL-TYPE"/>
    <rdfs:label xml:lang="en">aircraft carrier, helicopter/vstol, guided missile, nuclear powered</rdfs:label>
    <rdfs:comment xml:lang="en">Aircraft carrier without arrest gear/catapult operating VSTOL aircraft and/or helicopters which is not an amphibious or minewarfare ship, fitted with one or more force guided missile systems and with nuclear power.</rdfs:comment>
    <rdf:type rdf:resource="http://www.w3.org/2002/07/owl#Class"/>
  </rdf:Description>
  <rdf:Description rdf:about="#CBRN-EQUIPMENT-TYPE_Chemical_agent_monitor">
    <rdfs:subClassOf rdf:resource="jc3iedm_OBJECT-TYPE.owl#CBRN-EQUIPMENT-TYPE"/>
    <rdfs:label xml:lang="en">chemical agent monitor</rdfs:label>
    <rdfs:comment xml:lang="en">A handheld chemical agent detector.</rdfs:comment>
    <rdf:type rdf:resource="http://www.w3.org/2002/07/owl#Class"/>
  </rdf:Description>
  <rdf:Description rdf:about="jc3iedm_OBJECT-TYPE.owl#chemical-materiel-type-persistency-code">
    <rdf:type rdf:resource="http://www.w3.org/2002/07/owl#DatatypeProperty"/>
    <rdfs:domain rdf:resource="jc3iedm_OBJECT-TYPE.owl#CHEMICAL-MATERIEL-TYPE"/>
    <rdfs:range rdf:resource="http://www.w3.org/2001/XMLSchema#string"/>
  </rdf:Description>
  <rdf:Description rdf:about="#CONTROL-FEATURE-TYPE_Bullseye">
    <rdfs:subClassOf rdf:resource="jc3iedm_OBJECT-TYPE.owl#CONTROL-FEATURE-TYPE"/>
    <rdfs:label xml:lang="en">bullseye</rdfs:label>
    <rdfs:comment xml:lang="en">An established reference point from which the position of an object can be references by bearing (Magnetic) and range (in nautical miles NM) from this point.</rdfs:comment>
    <rdf:type rdf:resource="http://www.w3.org/2002/07/owl#Class"/>
  </rdf:Description>
  <rdf:Description rdf:about="#SURFACE-VESSEL-TYPE_Frigate,_coast_guard">
    <rdfs:subClassOf rdf:resource="jc3iedm_OBJECT-TYPE.owl#SURFACE-VESSEL-TYPE"/>
    <rdfs:label xml:lang="en">frigate, coast guard</rdfs:label>
    <rdfs:comment xml:lang="en">A coast guard frigate. A surface combatant in size range of about 75-150 metres. Fitted primarily to fulfil an ASW role. Generally has lighter surface armament than a Destroyer, general.</rdfs:comment>
    <rdf:type rdf:resource="http://www.w3.org/2002/07/owl#Class"/>
  </rdf:Description>
  <rdf:Description rdf:about="#FACILITY-TYPE_Berm">
    <rdfs:subClassOf rdf:resource="jc3iedm_OBJECT-TYPE.owl#FACILITY-TYPE"/>
    <rdfs:label xml:lang="en">berm</rdfs:label>
    <rdfs:comment xml:lang="en">An artificial ridge or embankment.</rdfs:comment>
    <rdf:type rdf:resource="http://www.w3.org/2002/07/owl#Class"/>
  </rdf:Description>
  <rdf:Description rdf:about="#ROUTE-TYPE_Air_traffic_services_route">
    <rdfs:subClassOf rdf:resource="jc3iedm_OBJECT-TYPE.owl#ROUTE-TYPE"/>
    <rdfs:label xml:lang="en">air traffic services route</rdfs:label>
    <rdfs:comment xml:lang="en">A specified route designed for channelling the flow of traffic as necessary for the provision of air traffic services (ATS).</rdfs:comment>
    <rdf:type rdf:resource="http://www.w3.org/2002/07/owl#Class"/>
  </rdf:Description>
  <rdf:Description rdf:about="#SURFACE-VESSEL-TYPE_Landing_ship,_medium">
    <rdfs:subClassOf rdf:resource="jc3iedm_OBJECT-TYPE.owl#SURFACE-VESSEL-TYPE"/>
    <rdfs:label xml:lang="en">landing ship, medium</rdfs:label>
    <rdfs:comment xml:lang="en">Ship in size range 45-85 metres, capable of beaching to land troops and/or tanks. Must have bow doors and/or landing ramp.</rdfs:comment>
    <rdf:type rdf:resource="http://www.w3.org/2002/07/owl#Class"/>
  </rdf:Description>
  <rdf:Description rdf:about="#FACILITY-TYPE_Power_plant,_nuclear">
    <rdfs:subClassOf rdf:resource="jc3iedm_OBJECT-TYPE.owl#FACILITY-TYPE"/>
    <rdfs:label xml:lang="en">power plant, nuclear</rdfs:label>
    <rdfs:comment xml:lang="en">A facility that provides power produced from nuclear energy.</rdfs:comment>
    <rdf:type rdf:resource="http://www.w3.org/2002/07/owl#Class"/>
  </rdf:Description>
  <rdf:Description rdf:about="jc3iedm_OBJECT-TYPE.owl#materiel-type-issuing-height-dimension">
    <rdf:type rdf:resource="http://www.w3.org/2002/07/owl#DatatypeProperty"/>
    <rdfs:domain rdf:resource="jc3iedm_OBJECT-TYPE.owl#MATERIEL-TYPE"/>
  </rdf:Description>
  <rdf:Description rdf:about="#MARITIME-EQUIPMENT-TYPE_Weight">
    <rdfs:subClassOf rdf:resource="jc3iedm_OBJECT-TYPE.owl#MARITIME-EQUIPMENT-TYPE"/>
    <rdfs:label xml:lang="en">weight</rdfs:label>
    <rdfs:comment xml:lang="en">A heavy object used to pull, press or hold something down, e.g. buoy, mine.</rdfs:comment>
    <rdf:type rdf:resource="http://www.w3.org/2002/07/owl#Class"/>
  </rdf:Description>
  <rdf:Description rdf:about="#ROUTE-TYPE_DCT">
    <rdfs:subClassOf rdf:resource="jc3iedm_OBJECT-TYPE.owl#ROUTE-TYPE"/>
    <rdfs:label xml:lang="en">dct</rdfs:label>
    <rdfs:comment xml:lang="en">Direct routing.</rdfs:comment>
    <rdf:type rdf:resource="http://www.w3.org/2002/07/owl#Class"/>
  </rdf:Description>
  <rdf:Description rdf:about="jc3iedm_OBJECT-TYPE.owl#equipment-type-unloaded-weight-quantity">
    <rdf:type rdf:resource="http://www.w3.org/2002/07/owl#DatatypeProperty"/>
    <rdfs:domain rdf:resource="jc3iedm_OBJECT-TYPE.owl#EQUIPMENT-TYPE"/>
  </rdf:Description>
  <rdf:Description rdf:about="#ORGANISATION-TYPE_Control_and_reporting_centre">
    <rdfs:subClassOf rdf:resource="jc3iedm_OBJECT-TYPE.owl#ORGANISATION-TYPE"/>
    <rdfs:label xml:lang="en">control and reporting centre</rdfs:label>
    <rdfs:comment xml:lang="en">The ORGANISATION-TYPE that serves as the senior ground radar element of the theatre air control system (TACS). Mission is to detect, identify, and verify airborne targets in assigned area. CRC also provides decentralized execution of air defence and airspace control, provides early warning to air and ground elements and manages subordinate radar units.</rdfs:comment>
    <rdf:type rdf:resource="http://www.w3.org/2002/07/owl#Class"/>
  </rdf:Description>
  <rdf:Description rdf:about="#BIOLOGICAL-MATERIEL-TYPE_Not_known">
    <rdfs:subClassOf rdf:resource="jc3iedm_OBJECT-TYPE.owl#BIOLOGICAL-MATERIEL-TYPE"/>
    <rdfs:label xml:lang="en">not known</rdfs:label>
    <rdfs:comment xml:lang="en">It is not possible to determine which value is most applicable.</rdfs:comment>
    <rdf:type rdf:resource="http://www.w3.org/2002/07/owl#Class"/>
  </rdf:Description>
  <rdf:Description rdf:about="#ENGINEERING-EQUIPMENT-TYPE_Tactical_floating_bridge">
    <rdfs:subClassOf rdf:resource="jc3iedm_OBJECT-TYPE.owl#ENGINEERING-EQUIPMENT-TYPE"/>
    <rdfs:label xml:lang="en">tactical floating bridge</rdfs:label>
    <rdfs:comment xml:lang="en">A bridge that can be laid on floating structure to permit crossing.</rdfs:comment>
    <rdf:type rdf:resource="http://www.w3.org/2002/07/owl#Class"/>
  </rdf:Description>
  <rdf:Description rdf:about="#FACILITY-TYPE_Pumping_station">
    <rdfs:subClassOf rdf:resource="jc3iedm_OBJECT-TYPE.owl#FACILITY-TYPE"/>
    <rdfs:label xml:lang="en">pumping station</rdfs:label>
    <rdfs:comment xml:lang="en">A facility that supports the movement of gases or liquids.</rdfs:comment>
    <rdf:type rdf:resource="http://www.w3.org/2002/07/owl#Class"/>
  </rdf:Description>
  <rdf:Description rdf:about="#FACILITY-TYPE_Production_complex,_chemical">
    <rdfs:subClassOf rdf:resource="jc3iedm_OBJECT-TYPE.owl#FACILITY-TYPE"/>
    <rdfs:label xml:lang="en">production complex, chemical</rdfs:label>
    <rdfs:comment xml:lang="en">A facility used for production of chemicals.</rdfs:comment>
    <rdf:type rdf:resource="http://www.w3.org/2002/07/owl#Class"/>
  </rdf:Description>
  <rdf:Description rdf:about="#MILITARY-OBSTACLE-TYPE_Minefield,_land">
    <rdfs:subClassOf rdf:resource="jc3iedm_OBJECT-TYPE.owl#MILITARY-OBSTACLE-TYPE"/>
    <rdfs:label xml:lang="en">minefield, land</rdfs:label>
    <rdfs:comment xml:lang="en">An obstacle that is an area of land containing mines.</rdfs:comment>
    <rdf:type rdf:resource="http://www.w3.org/2002/07/owl#Class"/>
  </rdf:Description>
  <rdf:Description rdf:about="#CONTROL-FEATURE-TYPE_Base_defence_zone">
    <rdfs:subClassOf rdf:resource="jc3iedm_OBJECT-TYPE.owl#CONTROL-FEATURE-TYPE"/>
    <rdfs:label xml:lang="en">base defence zone</rdfs:label>
    <rdfs:comment xml:lang="en">A zone established around airbases to enhance the effectiveness of local ground based air defence systems.</rdfs:comment>
    <rdf:type rdf:resource="http://www.w3.org/2002/07/owl#Class"/>
  </rdf:Description>
  <rdf:Description rdf:about="#SURFACE-VESSEL-TYPE_Launching_ship,_satellite">
    <rdfs:subClassOf rdf:resource="jc3iedm_OBJECT-TYPE.owl#SURFACE-VESSEL-TYPE"/>
    <rdfs:label xml:lang="en">launching ship, satellite</rdfs:label>
    <rdfs:comment xml:lang="en">Ship employed in monitoring satellite launching operations.</rdfs:comment>
    <rdf:type rdf:resource="http://www.w3.org/2002/07/owl#Class"/>
  </rdf:Description>
  <rdf:Description rdf:about="#FACILITY-TYPE_Forward_arming_and_refuelling_point">
    <rdfs:subClassOf rdf:resource="jc3iedm_OBJECT-TYPE.owl#FACILITY-TYPE"/>
    <rdfs:label xml:lang="en">forward arming and refuelling point</rdfs:label>
    <rdfs:comment xml:lang="en">A temporary facility that is organised, equipped, and deployed by an aviation commander and normally located in the main battle area closer to the area of operations than the aviation unit's combat service support (CSS) area. It provides fuel and ammunition necessary for the employment of aviation manoeuvre units in combat. It permits combat aircraft to rapidly refuel and rearm simultaneously.</rdfs:comment>
    <rdf:type rdf:resource="http://www.w3.org/2002/07/owl#Class"/>
  </rdf:Description>
  <rdf:Description rdf:about="#FACILITY-TYPE_City">
    <rdfs:subClassOf rdf:resource="jc3iedm_OBJECT-TYPE.owl#FACILITY-TYPE"/>
    <rdfs:label xml:lang="en">city</rdfs:label>
    <rdfs:comment xml:lang="en">A large town. In most cases a town created a city by charter.</rdfs:comment>
    <rdf:type rdf:resource="http://www.w3.org/2002/07/owl#Class"/>
  </rdf:Description>
  <rdf:Description rdf:about="#CONTROL-FEATURE-TYPE_Short_range_air_defence_engagement_zone">
    <rdfs:subClassOf rdf:resource="jc3iedm_OBJECT-TYPE.owl#CONTROL-FEATURE-TYPE"/>
    <rdfs:label xml:lang="en">short range air defence engagement zone</rdfs:label>
    <rdfs:comment xml:lang="en">The airspace of defined dimensions within which the responsibility for engagement of air-threats normally rests with short-range air defence (SHORAD) weapons.</rdfs:comment>
    <rdf:type rdf:resource="http://www.w3.org/2002/07/owl#Class"/>
  </rdf:Description>
  <rdf:Description rdf:about="#FACILITY-TYPE_Government_building">
    <rdfs:subClassOf rdf:resource="jc3iedm_OBJECT-TYPE.owl#FACILITY-TYPE"/>
    <rdfs:label xml:lang="en">government building</rdfs:label>
    <rdfs:comment xml:lang="en">A building for the administration of local, regional, or national government.</rdfs:comment>
    <rdf:type rdf:resource="http://www.w3.org/2002/07/owl#Class"/>
  </rdf:Description>
  <rdf:Description rdf:about="#SURFACE-VESSEL-TYPE_Casualty_transport_ship">
    <rdfs:subClassOf rdf:resource="jc3iedm_OBJECT-TYPE.owl#SURFACE-VESSEL-TYPE"/>
    <rdfs:label xml:lang="en">casualty transport ship</rdfs:label>
    <rdfs:comment xml:lang="en">Ship of at least 40 metres whose primary purpose is sustaining post operative casualties during transport out of theatre. Not declared by ICRC/red crescent (TU ships only). May be armed and carrying secure communications.</rdfs:comment>
    <rdf:type rdf:resource="http://www.w3.org/2002/07/owl#Class"/>
  </rdf:Description>
  <rdf:Description rdf:about="#UNIT-TYPE_Signal">
    <rdfs:subClassOf rdf:resource="jc3iedm_OBJECT-TYPE.owl#UNIT-TYPE"/>
    <rdfs:label xml:lang="en">signal</rdfs:label>
    <rdfs:comment xml:lang="en">A UNIT-TYPE whose principal designation is the provision of communications bearer systems.</rdfs:comment>
    <rdf:type rdf:resource="http://www.w3.org/2002/07/owl#Class"/>
  </rdf:Description>
  <rdf:Description rdf:about="#SURFACE-VESSEL-TYPE_Fishing_vessel,_base_ship">
    <rdfs:subClassOf rdf:resource="jc3iedm_OBJECT-TYPE.owl#SURFACE-VESSEL-TYPE"/>
    <rdfs:label xml:lang="en">fishing vessel, base ship</rdfs:label>
    <rdfs:comment xml:lang="en">Fishing vessel support ship (other than supplying fuel/water only).</rdfs:comment>
    <rdf:type rdf:resource="http://www.w3.org/2002/07/owl#Class"/>
  </rdf:Description>
  <rdf:Description rdf:about="#HARBOUR-TYPE_River_(Basins)">
    <rdfs:subClassOf rdf:resource="jc3iedm_OBJECT-TYPE.owl#HARBOUR-TYPE"/>
    <rdfs:label xml:lang="en">river (basins)</rdfs:label>
    <rdfs:comment xml:lang="en">A river harbour in which slips for vessels have been excavated in the banks, obliquely or at right angles to the axis of the stream.</rdfs:comment>
    <rdf:type rdf:resource="http://www.w3.org/2002/07/owl#Class"/>
  </rdf:Description>
  <rdf:Description rdf:about="#FACILITY-TYPE_Mining_installation,_underground">
    <rdfs:subClassOf rdf:resource="jc3iedm_OBJECT-TYPE.owl#FACILITY-TYPE"/>
    <rdfs:label xml:lang="en">mining installation, underground</rdfs:label>
    <rdfs:comment xml:lang="en">A facility where materials are extracted from the ground using underground tunnels and shafts.</rdfs:comment>
    <rdf:type rdf:resource="http://www.w3.org/2002/07/owl#Class"/>
  </rdf:Description>
  <rdf:Description rdf:about="#MARITIME-EQUIPMENT-TYPE_Diverter">
    <rdfs:subClassOf rdf:resource="jc3iedm_OBJECT-TYPE.owl#MARITIME-EQUIPMENT-TYPE"/>
    <rdfs:label xml:lang="en">diverter</rdfs:label>
    <rdfs:comment xml:lang="en">An object used to carry the magnetic cable in a dispersed form of loop, a specific form of float.</rdfs:comment>
    <rdf:type rdf:resource="http://www.w3.org/2002/07/owl#Class"/>
  </rdf:Description>
  <rdf:Description rdf:about="#CONTROL-FEATURE-TYPE_Point_of_interest">
    <rdfs:subClassOf rdf:resource="jc3iedm_OBJECT-TYPE.owl#CONTROL-FEATURE-TYPE"/>
    <rdfs:label xml:lang="en">point of interest</rdfs:label>
    <rdfs:comment xml:lang="en">A CONTROL-FEATURE-TYPE with a point location that is significant for military planning or activity.</rdfs:comment>
    <rdf:type rdf:resource="http://www.w3.org/2002/07/owl#Class"/>
  </rdf:Description>
  <rdf:Description rdf:about="#RAILCAR-TYPE_Tram">
    <rdfs:subClassOf rdf:resource="jc3iedm_OBJECT-TYPE.owl#RAILCAR-TYPE"/>
    <rdfs:label xml:lang="en">tram</rdfs:label>
    <rdfs:comment xml:lang="en">A passenger carrying vehicle that runs on rails normally along roads, with minimal earthworks, typically powered by electricity from overhead power cables via a pantograph.</rdfs:comment>
    <rdf:type rdf:resource="http://www.w3.org/2002/07/owl#Class"/>
  </rdf:Description>
  <rdf:Description rdf:about="#SURFACE-VESSEL-TYPE_Training_ship_(naval)">
    <rdfs:subClassOf rdf:resource="jc3iedm_OBJECT-TYPE.owl#SURFACE-VESSEL-TYPE"/>
    <rdfs:label xml:lang="en">training ship (naval)</rdfs:label>
    <rdfs:comment xml:lang="en">Large ocean-going ship designed to serve as a training ship.</rdfs:comment>
    <rdf:type rdf:resource="http://www.w3.org/2002/07/owl#Class"/>
  </rdf:Description>
  <rdf:Description rdf:about="#SURFACE-VESSEL-TYPE_Minesweeper,_inshore">
    <rdfs:subClassOf rdf:resource="jc3iedm_OBJECT-TYPE.owl#SURFACE-VESSEL-TYPE"/>
    <rdfs:label xml:lang="en">minesweeper, inshore</rdfs:label>
    <rdfs:comment xml:lang="en">Minesweeper between 20-40 metres. Intended and equipped for inshore minesweeping.</rdfs:comment>
    <rdf:type rdf:resource="http://www.w3.org/2002/07/owl#Class"/>
  </rdf:Description>
  <rdf:Description rdf:about="#SURFACE-VESSEL-TYPE_Mine_countermeasures_support_ship">
    <rdfs:subClassOf rdf:resource="jc3iedm_OBJECT-TYPE.owl#SURFACE-VESSEL-TYPE"/>
    <rdfs:label xml:lang="en">mine countermeasures support ship</rdfs:label>
    <rdfs:comment xml:lang="en">An armed combatant fitted for the control and support of MCM vessels in combat situations. Has limited facilities for repair of Mine countermeasures vessels and their equipment.</rdfs:comment>
    <rdf:type rdf:resource="http://www.w3.org/2002/07/owl#Class"/>
  </rdf:Description>
  <rdf:Description rdf:about="#CONTROL-FEATURE-TYPE_Obstacle_lane">
    <rdfs:subClassOf rdf:resource="jc3iedm_OBJECT-TYPE.owl#CONTROL-FEATURE-TYPE"/>
    <rdfs:label xml:lang="en">obstacle lane</rdfs:label>
    <rdfs:comment xml:lang="en">A route through an enemy or friendly obstacle that provides a passing force safe passage. The route may be reduced and proofed as part of a breach operation, or constructed as part of a friendly obstacle. A clear route through an obstacle.</rdfs:comment>
    <rdf:type rdf:resource="http://www.w3.org/2002/07/owl#Class"/>
  </rdf:Description>
  <rdf:Description rdf:about="#SURFACE-VESSEL-TYPE_Combat_support_ship,_fast_(naval)">
    <rdfs:subClassOf rdf:resource="jc3iedm_OBJECT-TYPE.owl#SURFACE-VESSEL-TYPE"/>
    <rdfs:label xml:lang="en">combat support ship, fast (naval)</rdfs:label>
    <rdfs:comment xml:lang="en">Large ship over 230 metres, capable of speeds of 25 knots - 46.3 km/hr or more and/or providing rapid and simultaneous underway replenishment of ships at sea with POL, ammunition, refrigerated and dry provisions, spare parts and general stores. Primary emphasis is on POL replenishment.</rdfs:comment>
    <rdf:type rdf:resource="http://www.w3.org/2002/07/owl#Class"/>
  </rdf:Description>
  <rdf:Description rdf:about="#MILITARY-POST-TYPE_JAAT_controller">
    <rdfs:subClassOf rdf:resource="jc3iedm_OBJECT-TYPE.owl#MILITARY-POST-TYPE"/>
    <rdfs:label xml:lang="en">jaat controller</rdfs:label>
    <rdfs:comment xml:lang="en">A MILITARY-POST-TYPE that is identified as the designated controller of a Joint Air Attack Team.</rdfs:comment>
    <rdf:type rdf:resource="http://www.w3.org/2002/07/owl#Class"/>
  </rdf:Description>
  <rdf:Description rdf:about="#FACILITY-TYPE_Hamlet">
    <rdfs:subClassOf rdf:resource="jc3iedm_OBJECT-TYPE.owl#FACILITY-TYPE"/>
    <rdfs:label xml:lang="en">hamlet</rdfs:label>
    <rdfs:comment xml:lang="en">A small village, especially one without a church.</rdfs:comment>
    <rdf:type rdf:resource="http://www.w3.org/2002/07/owl#Class"/>
  </rdf:Description>
  <rdf:Description rdf:about="#FACILITY-TYPE_Water_tower">
    <rdfs:subClassOf rdf:resource="jc3iedm_OBJECT-TYPE.owl#FACILITY-TYPE"/>
    <rdfs:label xml:lang="en">water tower</rdfs:label>
    <rdfs:comment xml:lang="en">An elevated container and its supporting structure used to hold water.</rdfs:comment>
    <rdf:type rdf:resource="http://www.w3.org/2002/07/owl#Class"/>
  </rdf:Description>
  <rdf:Description rdf:about="jc3iedm_OBJECT-TYPE.owl#ammunition-type-category-code">
    <rdf:type rdf:resource="http://www.w3.org/2002/07/owl#DatatypeProperty"/>
    <rdfs:domain rdf:resource="jc3iedm_OBJECT-TYPE.owl#AMMUNITION-TYPE"/>
    <rdfs:range rdf:resource="http://www.w3.org/2001/XMLSchema#string"/>
  </rdf:Description>
  <rdf:Description rdf:about="#VEHICLE-TYPE_Tractor">
    <rdfs:subClassOf rdf:resource="jc3iedm_OBJECT-TYPE.owl#VEHICLE-TYPE"/>
    <rdfs:label xml:lang="en">tractor</rdfs:label>
    <rdfs:comment xml:lang="en">A powered vehicle that pulls or draws machinery.</rdfs:comment>
    <rdf:type rdf:resource="http://www.w3.org/2002/07/owl#Class"/>
  </rdf:Description>
  <rdf:Description rdf:about="#SURFACE-VESSEL-TYPE_Surveillance_ship,_ocean">
    <rdfs:subClassOf rdf:resource="jc3iedm_OBJECT-TYPE.owl#SURFACE-VESSEL-TYPE"/>
    <rdfs:label xml:lang="en">surveillance ship, ocean</rdfs:label>
    <rdfs:comment xml:lang="en">No definition provided in STANAG 1166.</rdfs:comment>
    <rdf:type rdf:resource="http://www.w3.org/2002/07/owl#Class"/>
  </rdf:Description>
  <rdf:Description rdf:about="#CIVILIAN-POST-TYPE_Publisher">
    <rdfs:subClassOf rdf:resource="jc3iedm_OBJECT-TYPE.owl#CIVILIAN-POST-TYPE"/>
    <rdfs:label xml:lang="en">publisher</rdfs:label>
    <rdfs:comment xml:lang="en">A CIVILIAN-POST-TYPE whose business is the issuing of books, newspapers, music, engravings, videos or the like, as the agent of the author or owner.</rdfs:comment>
    <rdf:type rdf:resource="http://www.w3.org/2002/07/owl#Class"/>
  </rdf:Description>
  <rdf:Description rdf:about="#CONTROL-FEATURE-TYPE_Class-C_airspace">
    <rdfs:subClassOf rdf:resource="jc3iedm_OBJECT-TYPE.owl#CONTROL-FEATURE-TYPE"/>
    <rdfs:label xml:lang="en">class c airspace</rdfs:label>
    <rdfs:comment xml:lang="en">An airspace in which instrument flight rule and visual flight rule flights are permitted; all flights are subject to air traffic control service and instrument flight rule flights are separated from other instrument flight rule flights and from visual flight rule flights. Visual flight rule flights are separated from instrument flight rule flights and receive traffic information in respect to other visual flight rule flights.</rdfs:comment>
    <rdf:type rdf:resource="http://www.w3.org/2002/07/owl#Class"/>
  </rdf:Description>
  <rdf:Description rdf:about="#CONTROL-FEATURE-TYPE_Battle_position">
    <rdfs:subClassOf rdf:resource="jc3iedm_OBJECT-TYPE.owl#CONTROL-FEATURE-TYPE"/>
    <rdfs:label xml:lang="en">battle position</rdfs:label>
    <rdfs:comment xml:lang="en">1. A defensive location oriented on a likely enemy avenue of approach. (FM 3-90) 2. For attack helicopters, an area designated in which they can manoeuvre and fire into a designated engagement area or engage targets of opportunity. (FM 1-112) (Marine Corps) 1. In ground operations, a defensive location oriented on an enemy avenue of approach from which a unit may defend. 2. In air operations, an airspace coordination area containing fire points for attack helicopters.</rdfs:comment>
    <rdf:type rdf:resource="http://www.w3.org/2002/07/owl#Class"/>
  </rdf:Description>
  <rdf:Description rdf:about="#SURFACE-VESSEL-TYPE_Dredger,_non_self-propelled">
    <rdfs:subClassOf rdf:resource="jc3iedm_OBJECT-TYPE.owl#SURFACE-VESSEL-TYPE"/>
    <rdfs:label xml:lang="en">dredger, non self propelled</rdfs:label>
    <rdfs:comment xml:lang="en">Craft employed as a dredge. It is not self-propelled.</rdfs:comment>
    <rdf:type rdf:resource="http://www.w3.org/2002/07/owl#Class"/>
  </rdf:Description>
  <rdf:Description rdf:about="#FACILITY-TYPE_Depot,_missile_ammunition">
    <rdfs:subClassOf rdf:resource="jc3iedm_OBJECT-TYPE.owl#FACILITY-TYPE"/>
    <rdfs:label xml:lang="en">depot, missile ammunition</rdfs:label>
    <rdfs:comment xml:lang="en">An area used for the storage of missile ammunition.</rdfs:comment>
    <rdf:type rdf:resource="http://www.w3.org/2002/07/owl#Class"/>
  </rdf:Description>
  <rdf:Description rdf:about="#SURFACE-VESSEL-TYPE_Cruiser,_gun">
    <rdfs:subClassOf rdf:resource="jc3iedm_OBJECT-TYPE.owl#SURFACE-VESSEL-TYPE"/>
    <rdfs:label xml:lang="en">cruiser, gun</rdfs:label>
    <rdfs:comment xml:lang="en">Cruiser with guns 15 cm (6 inch) or larger as its main armament and with no missile systems.</rdfs:comment>
    <rdf:type rdf:resource="http://www.w3.org/2002/07/owl#Class"/>
  </rdf:Description>
  <rdf:Description rdf:about="#CHEMICAL-MATERIEL-TYPE_Choking_agent">
    <rdfs:subClassOf rdf:resource="jc3iedm_OBJECT-TYPE.owl#CHEMICAL-MATERIEL-TYPE"/>
    <rdfs:label xml:lang="en">choking agent</rdfs:label>
    <rdfs:comment xml:lang="en">A CHEMICAL-MATERIEL-TYPE that affects the human breathing function.</rdfs:comment>
    <rdf:type rdf:resource="http://www.w3.org/2002/07/owl#Class"/>
  </rdf:Description>
  <rdf:Description rdf:about="#AMMUNITION-TYPE_Mine,_maritime,_moving">
    <rdfs:subClassOf rdf:resource="jc3iedm_OBJECT-TYPE.owl#AMMUNITION-TYPE"/>
    <rdfs:label xml:lang="en">mine, maritime, moving</rdfs:label>
    <rdfs:comment xml:lang="en">A mine designed to be propelled to its proposed laying position by propulsion equipment like a torpedo. It sinks at the end of its run and then operates like a mine.</rdfs:comment>
    <rdf:type rdf:resource="http://www.w3.org/2002/07/owl#Class"/>
  </rdf:Description>
  <rdf:Description rdf:about="#GROUP-ORGANISATION-TYPE_Refugee">
    <rdfs:subClassOf rdf:resource="jc3iedm_OBJECT-TYPE.owl#GROUP-ORGANISATION-TYPE"/>
    <rdfs:label xml:lang="en">refugee</rdfs:label>
    <rdfs:comment xml:lang="en">A GROUP-ORGANISATION-TYPE that comprises persons who, owing to religious persecution or political troubles, seek refuge.</rdfs:comment>
    <rdf:type rdf:resource="http://www.w3.org/2002/07/owl#Class"/>
  </rdf:Description>
  <rdf:Description rdf:about="#CONTROL-FEATURE-TYPE_Traverse_level">
    <rdfs:subClassOf rdf:resource="jc3iedm_OBJECT-TYPE.owl#CONTROL-FEATURE-TYPE"/>
    <rdfs:label xml:lang="en">traverse level</rdfs:label>
    <rdfs:comment xml:lang="en">That vertical displacement above low level air defence systems, expressed both as a height and altitude, at which aircraft can cross that area in order to improve the effectiveness of the air defence systems by providing an extra friendly discriminator.</rdfs:comment>
    <rdf:type rdf:resource="http://www.w3.org/2002/07/owl#Class"/>
  </rdf:Description>
  <rdf:Description rdf:about="#MILITARY-POST-TYPE_Assault_support_coordinator,_airborne">
    <rdfs:subClassOf rdf:resource="jc3iedm_OBJECT-TYPE.owl#MILITARY-POST-TYPE"/>
    <rdfs:label xml:lang="en">assault support coordinator, airborne</rdfs:label>
    <rdfs:comment xml:lang="en">A MILITARY-POST-TYPE that provides air coordination and control during helicopter operations within the Marine Air Command and Control System (MACCS). Serves as an extension of Direct Air Support Centre (DASC) or Helicopter Direction Centre (HDC) in support of the air mission commander.</rdfs:comment>
    <rdf:type rdf:resource="http://www.w3.org/2002/07/owl#Class"/>
  </rdf:Description>
  <rdf:Description rdf:about="#VEHICLE-TYPE_Amphibian">
    <rdfs:subClassOf rdf:resource="jc3iedm_OBJECT-TYPE.owl#VEHICLE-TYPE"/>
    <rdfs:label xml:lang="en">amphibian</rdfs:label>
    <rdfs:comment xml:lang="en">A vehicle designed to travel over land and on water.</rdfs:comment>
    <rdf:type rdf:resource="http://www.w3.org/2002/07/owl#Class"/>
  </rdf:Description>
  <rdf:Description rdf:about="#FACILITY-TYPE_Tower,_non-communications">
    <rdfs:subClassOf rdf:resource="jc3iedm_OBJECT-TYPE.owl#FACILITY-TYPE"/>
    <rdfs:label xml:lang="en">tower, non communications</rdfs:label>
    <rdfs:comment xml:lang="en">A relatively tall structure which may be used for observation, support, or storage etc.</rdfs:comment>
    <rdf:type rdf:resource="http://www.w3.org/2002/07/owl#Class"/>
  </rdf:Description>
  <rdf:Description rdf:about="#SURFACE-VESSEL-TYPE_Mine_countermeasures_craft,_training">
    <rdfs:subClassOf rdf:resource="jc3iedm_OBJECT-TYPE.owl#SURFACE-VESSEL-TYPE"/>
    <rdfs:label xml:lang="en">mine countermeasures craft, training</rdfs:label>
    <rdfs:comment xml:lang="en">A vessel used primarily in a mine countermeasures training role.</rdfs:comment>
    <rdf:type rdf:resource="http://www.w3.org/2002/07/owl#Class"/>
  </rdf:Description>
  <rdf:Description rdf:about="#AIRCRAFT-TYPE_Medium">
    <rdfs:subClassOf rdf:resource="jc3iedm_OBJECT-TYPE.owl#AIRCRAFT-TYPE"/>
    <rdfs:label xml:lang="en">medium</rdfs:label>
    <rdfs:comment xml:lang="en">An aircraft is capable of lifting medium weight loads.</rdfs:comment>
    <rdf:type rdf:resource="http://www.w3.org/2002/07/owl#Class"/>
  </rdf:Description>
  <rdf:Description rdf:about="#SURFACE-VESSEL-TYPE_Fisheries_research_ship">
    <rdfs:subClassOf rdf:resource="jc3iedm_OBJECT-TYPE.owl#SURFACE-VESSEL-TYPE"/>
    <rdfs:label xml:lang="en">fisheries research ship</rdfs:label>
    <rdfs:comment xml:lang="en">Vessel equipped to conduct fisheries research.</rdfs:comment>
    <rdf:type rdf:resource="http://www.w3.org/2002/07/owl#Class"/>
  </rdf:Description>
  <rdf:Description rdf:about="jc3iedm_OBJECT-TYPE.owl#railcar-type-gauge-dimension">
    <rdf:type rdf:resource="http://www.w3.org/2002/07/owl#DatatypeProperty"/>
    <rdfs:domain rdf:resource="jc3iedm_OBJECT-TYPE.owl#RAILCAR-TYPE"/>
  </rdf:Description>
  <rdf:Description rdf:about="#ENGINEERING-EQUIPMENT-TYPE_Grader">
    <rdfs:subClassOf rdf:resource="jc3iedm_OBJECT-TYPE.owl#ENGINEERING-EQUIPMENT-TYPE"/>
    <rdfs:label xml:lang="en">grader</rdfs:label>
    <rdfs:comment xml:lang="en">A wheeled machine for levelling the ground.</rdfs:comment>
    <rdf:type rdf:resource="http://www.w3.org/2002/07/owl#Class"/>
  </rdf:Description>
  <rdf:Description rdf:about="#GOVERNMENT-ORGANISATION-TYPE_National_civil">
    <rdfs:subClassOf rdf:resource="jc3iedm_OBJECT-TYPE.owl#GOVERNMENT-ORGANISATION-TYPE"/>
    <rdfs:label xml:lang="en">national civil</rdfs:label>
    <rdfs:comment xml:lang="en">A GOVERNMENT-ORGANISATION-TYPE that is officially involved in national civil affairs.</rdfs:comment>
    <rdf:type rdf:resource="http://www.w3.org/2002/07/owl#Class"/>
  </rdf:Description>
  <rdf:Description rdf:about="#ROUTE-TYPE_Approach_corridor">
    <rdfs:subClassOf rdf:resource="jc3iedm_OBJECT-TYPE.owl#ROUTE-TYPE"/>
    <rdfs:label xml:lang="en">approach corridor</rdfs:label>
    <rdfs:comment xml:lang="en">Airspace established for the safe passage of land based aircraft joining or departing a maritime force.</rdfs:comment>
    <rdf:type rdf:resource="http://www.w3.org/2002/07/owl#Class"/>
  </rdf:Description>
  <rdf:Description rdf:about="#SURFACE-VESSEL-TYPE_Auxiliary_floating_drydock,_large">
    <rdfs:subClassOf rdf:resource="jc3iedm_OBJECT-TYPE.owl#SURFACE-VESSEL-TYPE"/>
    <rdfs:label xml:lang="en">auxiliary floating drydock, large</rdfs:label>
    <rdfs:comment xml:lang="en">Floating dock capable of docking ships of all sizes.</rdfs:comment>
    <rdf:type rdf:resource="http://www.w3.org/2002/07/owl#Class"/>
  </rdf:Description>
  <rdf:Description rdf:about="#FACILITY-TYPE_Supply_dump,_ammunition">
    <rdfs:subClassOf rdf:resource="jc3iedm_OBJECT-TYPE.owl#FACILITY-TYPE"/>
    <rdfs:label xml:lang="en">supply dump, ammunition</rdfs:label>
    <rdfs:comment xml:lang="en">A temporary storage area, usually in the open, for ammunition.</rdfs:comment>
    <rdf:type rdf:resource="http://www.w3.org/2002/07/owl#Class"/>
  </rdf:Description>
  <rdf:Description rdf:about="#SURFACE-VESSEL-TYPE_Tug,_ocean-going,_auxiliary">
    <rdfs:subClassOf rdf:resource="jc3iedm_OBJECT-TYPE.owl#SURFACE-VESSEL-TYPE"/>
    <rdfs:label xml:lang="en">tug, ocean going, auxiliary</rdfs:label>
    <rdfs:comment xml:lang="en">Seagoing tug employed to tow navy ships and craft. Usually about 40-50 metres.</rdfs:comment>
    <rdf:type rdf:resource="http://www.w3.org/2002/07/owl#Class"/>
  </rdf:Description>
  <rdf:Description rdf:about="#VEHICLE-TYPE_Wrecker">
    <rdfs:subClassOf rdf:resource="jc3iedm_OBJECT-TYPE.owl#VEHICLE-TYPE"/>
    <rdfs:label xml:lang="en">wrecker</rdfs:label>
    <rdfs:comment xml:lang="en">A vehicle used in recovering a damaged one.</rdfs:comment>
    <rdf:type rdf:resource="http://www.w3.org/2002/07/owl#Class"/>
  </rdf:Description>
  <rdf:Description rdf:about="#CONTROL-FEATURE-TYPE_Chemical_surface_deposition_concentration_contour_line">
    <rdfs:subClassOf rdf:resource="jc3iedm_OBJECT-TYPE.owl#CONTROL-FEATURE-TYPE"/>
    <rdfs:label xml:lang="en">chemical surface deposition concentration contour line</rdfs:label>
    <rdfs:comment xml:lang="en">A line on a map, diagram or overlay joining all points at which the chemical surface deposition concentration at a given time is the same. Chemical surface deposition concentration is the mass of a chemical substance distributed on a surface per unit area.</rdfs:comment>
    <rdf:type rdf:resource="http://www.w3.org/2002/07/owl#Class"/>
  </rdf:Description>
  <rdf:Description rdf:about="#MILITARY-POST-TYPE_Tactical_air_controller">
    <rdfs:subClassOf rdf:resource="jc3iedm_OBJECT-TYPE.owl#MILITARY-POST-TYPE"/>
    <rdfs:label xml:lang="en">tactical air controller</rdfs:label>
    <rdfs:comment xml:lang="en">A MILITARY-POST-TYPE that is a subordinate operational component of a tactical air control system designed to provide air liaison to land forces and for the control of aircraft.</rdfs:comment>
    <rdf:type rdf:resource="http://www.w3.org/2002/07/owl#Class"/>
  </rdf:Description>
  <rdf:Description rdf:about="#SURFACE-VESSEL-TYPE_Aircraft_carrier,_general">
    <rdfs:subClassOf rdf:resource="jc3iedm_OBJECT-TYPE.owl#SURFACE-VESSEL-TYPE"/>
    <rdfs:label xml:lang="en">aircraft carrier, general</rdfs:label>
    <rdfs:comment xml:lang="en">General designator for aircraft/multi-role aircraft carrier.</rdfs:comment>
    <rdf:type rdf:resource="http://www.w3.org/2002/07/owl#Class"/>
  </rdf:Description>
  <rdf:Description rdf:about="#FACILITY-TYPE_Military_materiel_facility,_engineering_equipment_production,_bridge">
    <rdfs:subClassOf rdf:resource="jc3iedm_OBJECT-TYPE.owl#FACILITY-TYPE"/>
    <rdfs:label xml:lang="en">military materiel facility, engineering equipment production, bridge</rdfs:label>
    <rdfs:comment xml:lang="en">A facility used as for engineering equipment production, bridge.</rdfs:comment>
    <rdf:type rdf:resource="http://www.w3.org/2002/07/owl#Class"/>
  </rdf:Description>
  <rdf:Description rdf:about="#RADIOACTIVE-MATERIEL-TYPE_Nuclear_release_other_than_attack_(ROTA)">
    <rdfs:subClassOf rdf:resource="jc3iedm_OBJECT-TYPE.owl#RADIOACTIVE-MATERIEL-TYPE"/>
    <rdfs:label xml:lang="en">nuclear release other than attack (rota)</rdfs:label>
    <rdfs:comment xml:lang="en">An intended or non-intended release of nuclear radiation from a non-militarily significant source or weapon.</rdfs:comment>
    <rdf:type rdf:resource="http://www.w3.org/2002/07/owl#Class"/>
  </rdf:Description>
  <rdf:Description rdf:about="#FACILITY-TYPE_Loading_platform,_military">
    <rdfs:subClassOf rdf:resource="jc3iedm_OBJECT-TYPE.owl#FACILITY-TYPE"/>
    <rdfs:label xml:lang="en">loading platform, military</rdfs:label>
    <rdfs:comment xml:lang="en">A facility constructed for loading military goods/equipment.</rdfs:comment>
    <rdf:type rdf:resource="http://www.w3.org/2002/07/owl#Class"/>
  </rdf:Description>
  <rdf:Description rdf:about="jc3iedm_OBJECT-TYPE.owl#VEHICLE-TYPE">
    <rdf:type rdf:resource="http://www.w3.org/2002/07/owl#Class"/>
    <rdfs:label xml:lang="en">vehicle type</rdfs:label>
    <rdfs:comment xml:lang="en">An EQUIPMENT-TYPE that is designed to operate on land routes (other than rail) with a primary role of transporting personnel, equipment or supplies.</rdfs:comment>
    <rdfs:subClassOf rdf:resource="jc3iedm_OBJECT-TYPE.owl#EQUIPMENT-TYPE"/>
  </rdf:Description>
  <rdf:Description rdf:about="#CONTROL-FEATURE-TYPE_Hand_over_gate">
    <rdfs:subClassOf rdf:resource="jc3iedm_OBJECT-TYPE.owl#CONTROL-FEATURE-TYPE"/>
    <rdfs:label xml:lang="en">hand over gate</rdfs:label>
    <rdfs:comment xml:lang="en">A point at which the control of the aircraft, if radar hand over is used, changes from one controller to another.</rdfs:comment>
    <rdf:type rdf:resource="http://www.w3.org/2002/07/owl#Class"/>
  </rdf:Description>
  <rdf:Description rdf:about="#HARBOUR-TYPE_Coastal_(Tide_Gates)">
    <rdfs:subClassOf rdf:resource="jc3iedm_OBJECT-TYPE.owl#HARBOUR-TYPE"/>
    <rdfs:label xml:lang="en">coastal (tide gates)</rdfs:label>
    <rdfs:comment xml:lang="en">A coastal harbour, the waters of which are constrained by locks or other mechanical devices in order to provide sufficient water to float vessels at all stages of the tide.</rdfs:comment>
    <rdf:type rdf:resource="http://www.w3.org/2002/07/owl#Class"/>
  </rdf:Description>
  <rdf:Description rdf:about="#WEAPON-TYPE_Anti-submarine">
    <rdfs:subClassOf rdf:resource="jc3iedm_OBJECT-TYPE.owl#WEAPON-TYPE"/>
    <rdfs:label xml:lang="en">anti submarine</rdfs:label>
    <rdfs:comment xml:lang="en">A weapon specifically designed for the engagement of submarines.</rdfs:comment>
    <rdf:type rdf:resource="http://www.w3.org/2002/07/owl#Class"/>
  </rdf:Description>
  <rdf:Description rdf:about="#SURFACE-VESSEL-TYPE_Tug,_ocean-going">
    <rdfs:subClassOf rdf:resource="jc3iedm_OBJECT-TYPE.owl#SURFACE-VESSEL-TYPE"/>
    <rdfs:label xml:lang="en">tug, ocean going</rdfs:label>
    <rdfs:comment xml:lang="en">General designator for tugs capable of operating in open ocean waters.</rdfs:comment>
    <rdf:type rdf:resource="http://www.w3.org/2002/07/owl#Class"/>
  </rdf:Description>
  <rdf:Description rdf:about="#CONTROL-FEATURE-TYPE_Radioactive_area">
    <rdfs:subClassOf rdf:resource="jc3iedm_OBJECT-TYPE.owl#CONTROL-FEATURE-TYPE"/>
    <rdfs:label xml:lang="en">radioactive area</rdfs:label>
    <rdfs:comment xml:lang="en">A CONTROL-FEATURE-TYPE that identifies the predicted or confirmed contour of an area in which radiological materials may produce casualties in man or animals and damage to plants or materiel.</rdfs:comment>
    <rdf:type rdf:resource="http://www.w3.org/2002/07/owl#Class"/>
  </rdf:Description>
  <rdf:Description rdf:about="#ROUTE-TYPE_Conventional_route">
    <rdfs:subClassOf rdf:resource="jc3iedm_OBJECT-TYPE.owl#ROUTE-TYPE"/>
    <rdfs:label xml:lang="en">conventional route</rdfs:label>
    <rdfs:comment xml:lang="en">Conventional route.</rdfs:comment>
    <rdf:type rdf:resource="http://www.w3.org/2002/07/owl#Class"/>
  </rdf:Description>
  <rdf:Description rdf:about="#FACILITY-TYPE_Demolition_debris">
    <rdfs:subClassOf rdf:resource="jc3iedm_OBJECT-TYPE.owl#FACILITY-TYPE"/>
    <rdfs:label xml:lang="en">demolition debris</rdfs:label>
    <rdfs:comment xml:lang="en">The debris left over from the demolition of an object.</rdfs:comment>
    <rdf:type rdf:resource="http://www.w3.org/2002/07/owl#Class"/>
  </rdf:Description>
  <rdf:Description rdf:about="#ROUTE-TYPE_Area_navigation_route">
    <rdfs:subClassOf rdf:resource="jc3iedm_OBJECT-TYPE.owl#ROUTE-TYPE"/>
    <rdfs:label xml:lang="en">area navigation route</rdfs:label>
    <rdfs:comment xml:lang="en">An air traffic services route established for the use of aircraft capable of employing area navigation.</rdfs:comment>
    <rdf:type rdf:resource="http://www.w3.org/2002/07/owl#Class"/>
  </rdf:Description>
  <rdf:Description rdf:about="#CONTROL-FEATURE-TYPE_Class-G_airspace">
    <rdfs:subClassOf rdf:resource="jc3iedm_OBJECT-TYPE.owl#CONTROL-FEATURE-TYPE"/>
    <rdfs:label xml:lang="en">class g airspace</rdfs:label>
    <rdfs:comment xml:lang="en">An airspace in which instrument flight rule and visual flights are permitted; all flights receive flight information service if requested.</rdfs:comment>
    <rdf:type rdf:resource="http://www.w3.org/2002/07/owl#Class"/>
  </rdf:Description>
  <rdf:Description rdf:about="jc3iedm_OBJECT-TYPE.owl#military-post-type-category-code">
    <rdf:type rdf:resource="http://www.w3.org/2002/07/owl#DatatypeProperty"/>
    <rdfs:domain rdf:resource="jc3iedm_OBJECT-TYPE.owl#MILITARY-POST-TYPE"/>
    <rdfs:range rdf:resource="http://www.w3.org/2001/XMLSchema#string"/>
  </rdf:Description>
  <rdf:Description rdf:about="#FACILITY-TYPE_Office">
    <rdfs:subClassOf rdf:resource="jc3iedm_OBJECT-TYPE.owl#FACILITY-TYPE"/>
    <rdfs:label xml:lang="en">office</rdfs:label>
    <rdfs:comment xml:lang="en">A place in which business, professional or clerical activities are conducted.</rdfs:comment>
    <rdf:type rdf:resource="http://www.w3.org/2002/07/owl#Class"/>
  </rdf:Description>
  <rdf:Description rdf:about="#SURFACE-VESSEL-TYPE_Repair_ship,_radiological">
    <rdfs:subClassOf rdf:resource="jc3iedm_OBJECT-TYPE.owl#SURFACE-VESSEL-TYPE"/>
    <rdfs:label xml:lang="en">repair ship, radiological</rdfs:label>
    <rdfs:comment xml:lang="en">Ship optimised to provide mobile repairs to radiological installations and facilities.</rdfs:comment>
    <rdf:type rdf:resource="http://www.w3.org/2002/07/owl#Class"/>
  </rdf:Description>
  <rdf:Description rdf:about="#SURFACE-VESSEL-TYPE_Sloop">
    <rdfs:subClassOf rdf:resource="jc3iedm_OBJECT-TYPE.owl#SURFACE-VESSEL-TYPE"/>
    <rdfs:label xml:lang="en">sloop</rdfs:label>
    <rdfs:comment xml:lang="en">Sailing vessel of sloop design.</rdfs:comment>
    <rdf:type rdf:resource="http://www.w3.org/2002/07/owl#Class"/>
  </rdf:Description>
  <rdf:Description rdf:about="jc3iedm_OBJECT-TYPE.owl#vessel-type-maximum-speed-rate">
    <rdf:type rdf:resource="http://www.w3.org/2002/07/owl#DatatypeProperty"/>
    <rdfs:domain rdf:resource="jc3iedm_OBJECT-TYPE.owl#VESSEL-TYPE"/>
  </rdf:Description>
  <rdf:Description rdf:about="#SURFACE-VESSEL-TYPE_Dry_dock_floating,_open,_medium">
    <rdfs:subClassOf rdf:resource="jc3iedm_OBJECT-TYPE.owl#SURFACE-VESSEL-TYPE"/>
    <rdfs:label xml:lang="en">dry dock floating, open, medium</rdfs:label>
    <rdfs:comment xml:lang="en">Non-self-propelled open ended dry dock between 60-200 metres.</rdfs:comment>
    <rdf:type rdf:resource="http://www.w3.org/2002/07/owl#Class"/>
  </rdf:Description>
  <rdf:Description rdf:about="#MILITARY-POST-TYPE_Maintenance_technician">
    <rdfs:subClassOf rdf:resource="jc3iedm_OBJECT-TYPE.owl#MILITARY-POST-TYPE"/>
    <rdfs:label xml:lang="en">maintenance technician</rdfs:label>
    <rdfs:comment xml:lang="en">A MILITARY-POST-TYPE that is identified as the person specialised to take all actions to retain materiel in or to restore it to a specified condition.</rdfs:comment>
    <rdf:type rdf:resource="http://www.w3.org/2002/07/owl#Class"/>
  </rdf:Description>
  <rdf:Description rdf:about="#SURFACE-VESSEL-TYPE_Floating_workshop,_repair">
    <rdfs:subClassOf rdf:resource="jc3iedm_OBJECT-TYPE.owl#SURFACE-VESSEL-TYPE"/>
    <rdfs:label xml:lang="en">floating workshop, repair</rdfs:label>
    <rdfs:comment xml:lang="en">Craft about 30 metres fitted out as a general or special purpose mobile workshop.</rdfs:comment>
    <rdf:type rdf:resource="http://www.w3.org/2002/07/owl#Class"/>
  </rdf:Description>
  <rdf:Description rdf:about="#FACILITY-TYPE_Field_storage_area-ammunition">
    <rdfs:subClassOf rdf:resource="jc3iedm_OBJECT-TYPE.owl#FACILITY-TYPE"/>
    <rdfs:label xml:lang="en">field storage area ammunition</rdfs:label>
    <rdfs:comment xml:lang="en">A facility with a group of field storage sites containing a max of 5000 tonnes gross weight of ammunition and explosives.</rdfs:comment>
    <rdf:type rdf:resource="http://www.w3.org/2002/07/owl#Class"/>
  </rdf:Description>
  <rdf:Description rdf:about="#VEHICLE-TYPE_Maintenance">
    <rdfs:subClassOf rdf:resource="jc3iedm_OBJECT-TYPE.owl#VEHICLE-TYPE"/>
    <rdfs:label xml:lang="en">maintenance</rdfs:label>
    <rdfs:comment xml:lang="en">A vehicle which, as its primary function, is designed to provide equipment support facilities in or out of the battlespace.</rdfs:comment>
    <rdf:type rdf:resource="http://www.w3.org/2002/07/owl#Class"/>
  </rdf:Description>
  <rdf:Description rdf:about="#CONTROL-FEATURE-TYPE_Bomb_area">
    <rdfs:subClassOf rdf:resource="jc3iedm_OBJECT-TYPE.owl#CONTROL-FEATURE-TYPE"/>
    <rdfs:label xml:lang="en">bomb area</rdfs:label>
    <rdfs:comment xml:lang="en">An area or a group of targets constituting an area designated for bombing.</rdfs:comment>
    <rdf:type rdf:resource="http://www.w3.org/2002/07/owl#Class"/>
  </rdf:Description>
  <rdf:Description rdf:about="#MISCELLANEOUS-EQUIPMENT-TYPE_Machinery">
    <rdfs:subClassOf rdf:resource="jc3iedm_OBJECT-TYPE.owl#MISCELLANEOUS-EQUIPMENT-TYPE"/>
    <rdfs:label xml:lang="en">machinery</rdfs:label>
    <rdfs:comment xml:lang="en">Machines or machine parts in general.</rdfs:comment>
    <rdf:type rdf:resource="http://www.w3.org/2002/07/owl#Class"/>
  </rdf:Description>
  <rdf:Description rdf:about="#AMMUNITION-TYPE_Cruise_missile">
    <rdfs:subClassOf rdf:resource="jc3iedm_OBJECT-TYPE.owl#AMMUNITION-TYPE"/>
    <rdfs:label xml:lang="en">cruise missile</rdfs:label>
    <rdfs:comment xml:lang="en">A weapon in the form of a pilotless jet aircraft carrying a warhead and capable of flying at low altitudes.</rdfs:comment>
    <rdf:type rdf:resource="http://www.w3.org/2002/07/owl#Class"/>
  </rdf:Description>
  <rdf:Description rdf:about="#FEATURE-TYPE_Not_otherwise_specified">
    <rdfs:subClassOf rdf:resource="jc3iedm_OBJECT-TYPE.owl#FEATURE-TYPE"/>
    <rdfs:label xml:lang="en">not otherwise specified</rdfs:label>
    <rdfs:comment xml:lang="en">The appropriate value is not in the set of specified values.</rdfs:comment>
    <rdf:type rdf:resource="http://www.w3.org/2002/07/owl#Class"/>
  </rdf:Description>
  <rdf:Description rdf:about="#UNIT-TYPE_Fire_support">
    <rdfs:subClassOf rdf:resource="jc3iedm_OBJECT-TYPE.owl#UNIT-TYPE"/>
    <rdfs:label xml:lang="en">fire support</rdfs:label>
    <rdfs:comment xml:lang="en">A UNIT-TYPE whose principal designation is the employment of fire, coordinated with the manoeuvre of forces, to destroy neutralize or suppress the enemy.</rdfs:comment>
    <rdf:type rdf:resource="http://www.w3.org/2002/07/owl#Class"/>
  </rdf:Description>
  <rdf:Description rdf:about="#SURFACE-VESSEL-TYPE_Tug,_ocean-going_or_ship_salvage/rescue">
    <rdfs:subClassOf rdf:resource="jc3iedm_OBJECT-TYPE.owl#SURFACE-VESSEL-TYPE"/>
    <rdfs:label xml:lang="en">tug, ocean going or ship salvage/rescue</rdfs:label>
    <rdfs:comment xml:lang="en">Ship that can provide salvage, repair, diving and rescue services, and tow ships and craft.</rdfs:comment>
    <rdf:type rdf:resource="http://www.w3.org/2002/07/owl#Class"/>
  </rdf:Description>
  <rdf:Description rdf:about="#SURFACE-VESSEL-TYPE_Depot_ship/tender">
    <rdfs:subClassOf rdf:resource="jc3iedm_OBJECT-TYPE.owl#SURFACE-VESSEL-TYPE"/>
    <rdfs:label xml:lang="en">depot ship/tender</rdfs:label>
    <rdfs:comment xml:lang="en">Usually a large ship designed to provide support and depot facilities to other vessels of a specific type.</rdfs:comment>
    <rdf:type rdf:resource="http://www.w3.org/2002/07/owl#Class"/>
  </rdf:Description>
  <rdf:Description rdf:about="#MISCELLANEOUS-EQUIPMENT-TYPE_Searchlight">
    <rdfs:subClassOf rdf:resource="jc3iedm_OBJECT-TYPE.owl#MISCELLANEOUS-EQUIPMENT-TYPE"/>
    <rdfs:label xml:lang="en">searchlight</rdfs:label>
    <rdfs:comment xml:lang="en">An electric arc-lamp fitted with a reflector and suspended in a frame so that it may throw a beam of light in any desired direction; used in naval defence and for signalling purposes, etc.</rdfs:comment>
    <rdf:type rdf:resource="http://www.w3.org/2002/07/owl#Class"/>
  </rdf:Description>
  <rdf:Description rdf:about="#SURFACE-VESSEL-TYPE_Minesweeper,_coastal">
    <rdfs:subClassOf rdf:resource="jc3iedm_OBJECT-TYPE.owl#SURFACE-VESSEL-TYPE"/>
    <rdfs:label xml:lang="en">minesweeper, coastal</rdfs:label>
    <rdfs:comment xml:lang="en">Non-magnetic minesweeper between 40-70 metres.</rdfs:comment>
    <rdf:type rdf:resource="http://www.w3.org/2002/07/owl#Class"/>
  </rdf:Description>
  <rdf:Description rdf:about="#SURFACE-VESSEL-TYPE_Cruiser,_guided_missile">
    <rdfs:subClassOf rdf:resource="jc3iedm_OBJECT-TYPE.owl#SURFACE-VESSEL-TYPE"/>
    <rdfs:label xml:lang="en">cruiser, guided missile</rdfs:label>
    <rdfs:comment xml:lang="en">Cruiser with one or more force guided missile systems as its main armament.</rdfs:comment>
    <rdf:type rdf:resource="http://www.w3.org/2002/07/owl#Class"/>
  </rdf:Description>
  <rdf:Description rdf:about="#BIOLOGICAL-MATERIEL-TYPE_Bacterial">
    <rdfs:subClassOf rdf:resource="jc3iedm_OBJECT-TYPE.owl#BIOLOGICAL-MATERIEL-TYPE"/>
    <rdfs:label xml:lang="en">bacterial</rdfs:label>
    <rdfs:comment xml:lang="en">A generic term for a BIOLOGICAL-MATERIEL-TYPE, member of a large group of unicellular micro-organisms (prokaryotes) that have cell walls but lack an organised nucleus and other structures, and include numerous disease causing forms.</rdfs:comment>
    <rdf:type rdf:resource="http://www.w3.org/2002/07/owl#Class"/>
  </rdf:Description>
  <rdf:Description rdf:about="#MISCELLANEOUS-EQUIPMENT-TYPE_Not_otherwise_specified">
    <rdfs:subClassOf rdf:resource="jc3iedm_OBJECT-TYPE.owl#MISCELLANEOUS-EQUIPMENT-TYPE"/>
    <rdfs:label xml:lang="en">not otherwise specified</rdfs:label>
    <rdfs:comment xml:lang="en">The appropriate value is not in the set of specified values.</rdfs:comment>
    <rdf:type rdf:resource="http://www.w3.org/2002/07/owl#Class"/>
  </rdf:Description>
  <rdf:Description rdf:about="#MILITARY-OBSTACLE-TYPE_Wire_obstacle,_double_strand_concertina">
    <rdfs:subClassOf rdf:resource="jc3iedm_OBJECT-TYPE.owl#MILITARY-OBSTACLE-TYPE"/>
    <rdfs:label xml:lang="en">wire obstacle, double strand concertina</rdfs:label>
    <rdfs:comment xml:lang="en">No definition provided in APP-6A.</rdfs:comment>
    <rdf:type rdf:resource="http://www.w3.org/2002/07/owl#Class"/>
  </rdf:Description>
  <rdf:Description rdf:about="#FACILITY-TYPE_Railway">
    <rdfs:subClassOf rdf:resource="jc3iedm_OBJECT-TYPE.owl#FACILITY-TYPE"/>
    <rdfs:label xml:lang="en">railway</rdfs:label>
    <rdfs:comment xml:lang="en">A rail or set of parallel rails on which a train or tram runs.</rdfs:comment>
    <rdf:type rdf:resource="http://www.w3.org/2002/07/owl#Class"/>
  </rdf:Description>
  <rdf:Description rdf:about="jc3iedm_OBJECT-TYPE.owl#harbour-type-category-code">
    <rdf:type rdf:resource="http://www.w3.org/2002/07/owl#DatatypeProperty"/>
    <rdfs:domain rdf:resource="jc3iedm_OBJECT-TYPE.owl#HARBOUR-TYPE"/>
    <rdfs:range rdf:resource="http://www.w3.org/2001/XMLSchema#string"/>
  </rdf:Description>
  <rdf:Description rdf:about="#CONTROL-FEATURE-TYPE_Air_defence_identification_zone">
    <rdfs:subClassOf rdf:resource="jc3iedm_OBJECT-TYPE.owl#CONTROL-FEATURE-TYPE"/>
    <rdfs:label xml:lang="en">air defence identification zone</rdfs:label>
    <rdfs:comment xml:lang="en">Airspace within which ready identification, location, and control of airborne vehicles are required.</rdfs:comment>
    <rdf:type rdf:resource="http://www.w3.org/2002/07/owl#Class"/>
  </rdf:Description>
  <rdf:Description rdf:about="#SUBSURFACE-VESSEL-TYPE_Submarine,_patrol">
    <rdfs:subClassOf rdf:resource="jc3iedm_OBJECT-TYPE.owl#SUBSURFACE-VESSEL-TYPE"/>
    <rdfs:label xml:lang="en">submarine, patrol</rdfs:label>
    <rdfs:comment xml:lang="en">Long-range patrol submarine. May have primary anti- surface or anti-submarine role.</rdfs:comment>
    <rdf:type rdf:resource="http://www.w3.org/2002/07/owl#Class"/>
  </rdf:Description>
  <rdf:Description rdf:about="#CONSUMABLE-MATERIEL-TYPE_Fuel">
    <rdfs:subClassOf rdf:resource="jc3iedm_OBJECT-TYPE.owl#CONSUMABLE-MATERIEL-TYPE"/>
    <rdfs:label xml:lang="en">fuel</rdfs:label>
    <rdfs:comment xml:lang="en">A substance burned to create energy.</rdfs:comment>
    <rdf:type rdf:resource="http://www.w3.org/2002/07/owl#Class"/>
  </rdf:Description>
  <rdf:Description rdf:about="#CONTROL-FEATURE-TYPE_Safety_zone">
    <rdfs:subClassOf rdf:resource="jc3iedm_OBJECT-TYPE.owl#CONTROL-FEATURE-TYPE"/>
    <rdfs:label xml:lang="en">safety zone</rdfs:label>
    <rdfs:comment xml:lang="en">An area (land, sea or air) reserved for non-combat operations of friendly aircraft, surface ships, submarines or ground forces.</rdfs:comment>
    <rdf:type rdf:resource="http://www.w3.org/2002/07/owl#Class"/>
  </rdf:Description>
  <rdf:Description rdf:about="#CONTROL-FEATURE-TYPE_Force_air_coordination_area">
    <rdfs:subClassOf rdf:resource="jc3iedm_OBJECT-TYPE.owl#CONTROL-FEATURE-TYPE"/>
    <rdfs:label xml:lang="en">force air coordination area</rdfs:label>
    <rdfs:comment xml:lang="en">An area surrounding a force within which air coordination measures are required to prevent mutual interference between all friendly surface and air units and their weapon systems.</rdfs:comment>
    <rdf:type rdf:resource="http://www.w3.org/2002/07/owl#Class"/>
  </rdf:Description>
  <rdf:Description rdf:about="#GROUP-ORGANISATION-TYPE_Village_elder">
    <rdfs:subClassOf rdf:resource="jc3iedm_OBJECT-TYPE.owl#GROUP-ORGANISATION-TYPE"/>
    <rdfs:label xml:lang="en">village elder</rdfs:label>
    <rdfs:comment xml:lang="en">A GROUP-ORGANISATION-TYPE that comprises persons that are of ripe years and experience whose counsel is therefore sought and valued.</rdfs:comment>
    <rdf:type rdf:resource="http://www.w3.org/2002/07/owl#Class"/>
  </rdf:Description>
  <rdf:Description rdf:about="#CONTROL-FEATURE-TYPE_Coordinated_air_defence_area">
    <rdfs:subClassOf rdf:resource="jc3iedm_OBJECT-TYPE.owl#CONTROL-FEATURE-TYPE"/>
    <rdfs:label xml:lang="en">coordinated air defence area</rdfs:label>
    <rdfs:comment xml:lang="en">A mutually defined block of airspace between land-based air commander and a naval commander when their forces are operating in close proximity to one another.</rdfs:comment>
    <rdf:type rdf:resource="http://www.w3.org/2002/07/owl#Class"/>
  </rdf:Description>
  <rdf:Description rdf:about="#FACILITY-TYPE_School">
    <rdfs:subClassOf rdf:resource="jc3iedm_OBJECT-TYPE.owl#FACILITY-TYPE"/>
    <rdfs:label xml:lang="en">school</rdfs:label>
    <rdfs:comment xml:lang="en">A facility whose essential function is instruction and education.</rdfs:comment>
    <rdf:type rdf:resource="http://www.w3.org/2002/07/owl#Class"/>
  </rdf:Description>
  <rdf:Description rdf:about="#WEAPON-TYPE_Tank">
    <rdfs:subClassOf rdf:resource="jc3iedm_OBJECT-TYPE.owl#WEAPON-TYPE"/>
    <rdfs:label xml:lang="en">tank</rdfs:label>
    <rdfs:comment xml:lang="en">An armoured vehicle whose principal weapon is a direct fire gun optimised for the destruction of armoured vehicles.</rdfs:comment>
    <rdf:type rdf:resource="http://www.w3.org/2002/07/owl#Class"/>
  </rdf:Description>
  <rdf:Description rdf:about="#SURFACE-VESSEL-TYPE_Minesweeper,_coastal_w/drone(s)">
    <rdfs:subClassOf rdf:resource="jc3iedm_OBJECT-TYPE.owl#SURFACE-VESSEL-TYPE"/>
    <rdfs:label xml:lang="en">minesweeper, coastal w/drone(s)</rdfs:label>
    <rdfs:comment xml:lang="en">Coastal minesweeper capable of deploying and/or controlling unmanned remote controlled or towed vehicle(s) used for clearing mines.</rdfs:comment>
    <rdf:type rdf:resource="http://www.w3.org/2002/07/owl#Class"/>
  </rdf:Description>
  <rdf:Description rdf:about="#UNIT-TYPE_Aviation,_composite">
    <rdfs:subClassOf rdf:resource="jc3iedm_OBJECT-TYPE.owl#UNIT-TYPE"/>
    <rdfs:label xml:lang="en">aviation, composite</rdfs:label>
    <rdfs:comment xml:lang="en">A UNIT-TYPE whose designation indicates employment of a mix of fixed wing, rotary wing and/or VSTOL aircraft.</rdfs:comment>
    <rdf:type rdf:resource="http://www.w3.org/2002/07/owl#Class"/>
  </rdf:Description>
  <rdf:Description rdf:about="#SURFACE-VESSEL-TYPE_Landing_craft">
    <rdfs:subClassOf rdf:resource="jc3iedm_OBJECT-TYPE.owl#SURFACE-VESSEL-TYPE"/>
    <rdfs:label xml:lang="en">landing craft</rdfs:label>
    <rdfs:comment xml:lang="en">General designation for amphibious landing craft.</rdfs:comment>
    <rdf:type rdf:resource="http://www.w3.org/2002/07/owl#Class"/>
  </rdf:Description>
  <rdf:Description rdf:about="#SURFACE-VESSEL-TYPE_Patrol_craft,_training">
    <rdfs:subClassOf rdf:resource="jc3iedm_OBJECT-TYPE.owl#SURFACE-VESSEL-TYPE"/>
    <rdfs:label xml:lang="en">patrol craft, training</rdfs:label>
    <rdfs:comment xml:lang="en">Vessel in size range 35-55 metres designed and fitted primarily for escort duties in ASW role and used primarily in a training role.</rdfs:comment>
    <rdf:type rdf:resource="http://www.w3.org/2002/07/owl#Class"/>
  </rdf:Description>
  <rdf:Description rdf:about="#FACILITY-TYPE_Interchange/complex_junction">
    <rdfs:subClassOf rdf:resource="jc3iedm_OBJECT-TYPE.owl#FACILITY-TYPE"/>
    <rdfs:label xml:lang="en">interchange/complex junction</rdfs:label>
    <rdfs:comment xml:lang="en">A connection designed to provide traffic access from one road to another.</rdfs:comment>
    <rdf:type rdf:resource="http://www.w3.org/2002/07/owl#Class"/>
  </rdf:Description>
  <rdf:Description rdf:about="#CONTROL-FEATURE-TYPE_Surface_to_air_weapon_control_position">
    <rdfs:subClassOf rdf:resource="jc3iedm_OBJECT-TYPE.owl#CONTROL-FEATURE-TYPE"/>
    <rdfs:label xml:lang="en">surface to air weapon control position</rdfs:label>
    <rdfs:comment xml:lang="en">No definition provided in ADatP-3 Baseline 11.</rdfs:comment>
    <rdf:type rdf:resource="http://www.w3.org/2002/07/owl#Class"/>
  </rdf:Description>
  <rdf:Description rdf:about="jc3iedm_OBJECT-TYPE.owl#GROUP-ORGANISATION-TYPE">
    <rdf:type rdf:resource="http://www.w3.org/2002/07/owl#Class"/>
    <rdfs:label xml:lang="en">group organisation type</rdfs:label>
    <rdfs:comment xml:lang="en">An ORGANISATION-TYPE that is non-formal in nature and classes together its members due to mutual or common circumstances.</rdfs:comment>
    <rdfs:subClassOf rdf:resource="jc3iedm_OBJECT-TYPE.owl#ORGANISATION-TYPE"/>
  </rdf:Description>
  <rdf:Description rdf:about="#MILITARY-OBSTACLE-TYPE_Anti-tank_ditch">
    <rdfs:subClassOf rdf:resource="jc3iedm_OBJECT-TYPE.owl#MILITARY-OBSTACLE-TYPE"/>
    <rdfs:label xml:lang="en">anti tank ditch</rdfs:label>
    <rdfs:comment xml:lang="en">A facility that is a ditch obstacle designed to stop tanks.</rdfs:comment>
    <rdf:type rdf:resource="http://www.w3.org/2002/07/owl#Class"/>
  </rdf:Description>
  <rdf:Description rdf:about="#MILITARY-POST-TYPE_Attack_helicopter_commander">
    <rdfs:subClassOf rdf:resource="jc3iedm_OBJECT-TYPE.owl#MILITARY-POST-TYPE"/>
    <rdfs:label xml:lang="en">attack helicopter commander</rdfs:label>
    <rdfs:comment xml:lang="en">A MILITARY-POST-TYPE that is identified as the designated commander of an attack helicopter unit.</rdfs:comment>
    <rdf:type rdf:resource="http://www.w3.org/2002/07/owl#Class"/>
  </rdf:Description>
  <rdf:Description rdf:about="#SURFACE-VESSEL-TYPE_Armed_customs_gunboat">
    <rdfs:subClassOf rdf:resource="jc3iedm_OBJECT-TYPE.owl#SURFACE-VESSEL-TYPE"/>
    <rdfs:label xml:lang="en">armed customs gunboat</rdfs:label>
    <rdfs:comment xml:lang="en">Armed vessel operated by customs. Size may vary.</rdfs:comment>
    <rdf:type rdf:resource="http://www.w3.org/2002/07/owl#Class"/>
  </rdf:Description>
  <rdf:Description rdf:about="#CONTROL-FEATURE-TYPE_Falcon_radials_area">
    <rdfs:subClassOf rdf:resource="jc3iedm_OBJECT-TYPE.owl#CONTROL-FEATURE-TYPE"/>
    <rdfs:label xml:lang="en">falcon radials area</rdfs:label>
    <rdfs:comment xml:lang="en">Planned magnetic bearings along which aircraft depart and return to ships.</rdfs:comment>
    <rdf:type rdf:resource="http://www.w3.org/2002/07/owl#Class"/>
  </rdf:Description>
  <rdf:Description rdf:about="#FACILITY-TYPE_Power_plant,_fossil_fuel">
    <rdfs:subClassOf rdf:resource="jc3iedm_OBJECT-TYPE.owl#FACILITY-TYPE"/>
    <rdfs:label xml:lang="en">power plant, fossil fuel</rdfs:label>
    <rdfs:comment xml:lang="en">A facility that provides power produced from fossil fuels.</rdfs:comment>
    <rdf:type rdf:resource="http://www.w3.org/2002/07/owl#Class"/>
  </rdf:Description>
  <rdf:Description rdf:about="#FACILITY-TYPE_Crossing,_railway/river">
    <rdfs:subClassOf rdf:resource="jc3iedm_OBJECT-TYPE.owl#FACILITY-TYPE"/>
    <rdfs:label xml:lang="en">crossing, railway/river</rdfs:label>
    <rdfs:comment xml:lang="en">A facility where railway track crosses a highway or street, or where a river can be crossed.</rdfs:comment>
    <rdf:type rdf:resource="http://www.w3.org/2002/07/owl#Class"/>
  </rdf:Description>
  <rdf:Description rdf:about="#MILITARY-POST-TYPE_Dentistry_physician">
    <rdfs:subClassOf rdf:resource="jc3iedm_OBJECT-TYPE.owl#MILITARY-POST-TYPE"/>
    <rdfs:label xml:lang="en">dentistry physician</rdfs:label>
    <rdfs:comment xml:lang="en">A MILITARY-POST-TYPE that is identified as a physician specialising in Dentistry.</rdfs:comment>
    <rdf:type rdf:resource="http://www.w3.org/2002/07/owl#Class"/>
  </rdf:Description>
  <rdf:Description rdf:about="#SURFACE-VESSEL-TYPE_Aircraft_carrier,_guided_missile,_nuclear_power">
    <rdfs:subClassOf rdf:resource="jc3iedm_OBJECT-TYPE.owl#SURFACE-VESSEL-TYPE"/>
    <rdfs:label xml:lang="en">aircraft carrier, guided missile, nuclear power</rdfs:label>
    <rdfs:comment xml:lang="en">Designator for multi-role aircraft carriers, fitted with one or more force guided missile systems, nuclear powered.</rdfs:comment>
    <rdf:type rdf:resource="http://www.w3.org/2002/07/owl#Class"/>
  </rdf:Description>
  <rdf:Description rdf:about="#AMMUNITION-TYPE_Air_launched_missile">
    <rdfs:subClassOf rdf:resource="jc3iedm_OBJECT-TYPE.owl#AMMUNITION-TYPE"/>
    <rdfs:label xml:lang="en">air launched missile</rdfs:label>
    <rdfs:comment xml:lang="en">A self-propelled airborne munition that is guided automatically, or by remote control, fired from an aircraft.</rdfs:comment>
    <rdf:type rdf:resource="http://www.w3.org/2002/07/owl#Class"/>
  </rdf:Description>
  <rdf:Description rdf:about="#FACILITY-TYPE_Helicopter_landing_pad">
    <rdfs:subClassOf rdf:resource="jc3iedm_OBJECT-TYPE.owl#FACILITY-TYPE"/>
    <rdfs:label xml:lang="en">helicopter landing pad</rdfs:label>
    <rdfs:comment xml:lang="en">An improved area used for takeoff, and landing, by helicopters and other vertical takeoff and landing aircraft.</rdfs:comment>
    <rdf:type rdf:resource="http://www.w3.org/2002/07/owl#Class"/>
  </rdf:Description>
  <rdf:Description rdf:about="#CONTROL-FEATURE-TYPE_Danger_area">
    <rdfs:subClassOf rdf:resource="jc3iedm_OBJECT-TYPE.owl#CONTROL-FEATURE-TYPE"/>
    <rdfs:label xml:lang="en">danger area</rdfs:label>
    <rdfs:comment xml:lang="en">An airspace of defined dimensions within which activities dangerous to the flight of aircraft may exist at specified times.</rdfs:comment>
    <rdf:type rdf:resource="http://www.w3.org/2002/07/owl#Class"/>
  </rdf:Description>
  <rdf:Description rdf:about="#FACILITY-TYPE_Not_otherwise_specified">
    <rdfs:subClassOf rdf:resource="jc3iedm_OBJECT-TYPE.owl#FACILITY-TYPE"/>
    <rdfs:label xml:lang="en">not otherwise specified</rdfs:label>
    <rdfs:comment xml:lang="en">The appropriate value is not in the set of specified values.</rdfs:comment>
    <rdf:type rdf:resource="http://www.w3.org/2002/07/owl#Class"/>
  </rdf:Description>
  <rdf:Description rdf:about="#SURFACE-VESSEL-TYPE_Merchant_ship,_tanker">
    <rdfs:subClassOf rdf:resource="jc3iedm_OBJECT-TYPE.owl#SURFACE-VESSEL-TYPE"/>
    <rdfs:label xml:lang="en">merchant ship, tanker</rdfs:label>
    <rdfs:comment xml:lang="en">Non-naval ship designed to transport liquids (or gases).</rdfs:comment>
    <rdf:type rdf:resource="http://www.w3.org/2002/07/owl#Class"/>
  </rdf:Description>
  <rdf:Description rdf:about="#CONTROL-FEATURE-TYPE_Aircraft_control_position">
    <rdfs:subClassOf rdf:resource="jc3iedm_OBJECT-TYPE.owl#CONTROL-FEATURE-TYPE"/>
    <rdfs:label xml:lang="en">aircraft control position</rdfs:label>
    <rdfs:comment xml:lang="en">No definition provided in ADatP-3 Baseline 13.1 FFIRN/FUD 1044/66.</rdfs:comment>
    <rdf:type rdf:resource="http://www.w3.org/2002/07/owl#Class"/>
  </rdf:Description>
  <rdf:Description rdf:about="#ROUTE-TYPE_Minimum_risk_route">
    <rdfs:subClassOf rdf:resource="jc3iedm_OBJECT-TYPE.owl#ROUTE-TYPE"/>
    <rdfs:label xml:lang="en">minimum risk route</rdfs:label>
    <rdfs:comment xml:lang="en">A temporary corridor of defined dimensions recommended for use by high-speed, fixed-wing aircraft that presents the minimum known hazards to low-flying aircraft transiting the combat zone. Army--An MRR is a temporary flight route recommended for USAF use. It presents the minimum known hazards to low-flying aircraft in the control zone (CZ). The MRR must be approved by the airspace control authority and avoids fire support targets such as air defence weapons, landing zones, pick-up zones, FARPs, and Army airfields.</rdfs:comment>
    <rdf:type rdf:resource="http://www.w3.org/2002/07/owl#Class"/>
  </rdf:Description>
  <rdf:Description rdf:about="#SURFACE-VESSEL-TYPE_Oiler,_small_(naval)">
    <rdfs:subClassOf rdf:resource="jc3iedm_OBJECT-TYPE.owl#SURFACE-VESSEL-TYPE"/>
    <rdfs:label xml:lang="en">oiler, small (naval)</rdfs:label>
    <rdfs:comment xml:lang="en">Ship in size range 60-100 metres capable of furnishing underway replenishment of POL products.</rdfs:comment>
    <rdf:type rdf:resource="http://www.w3.org/2002/07/owl#Class"/>
  </rdf:Description>
  <rdf:Description rdf:about="#MILITARY-OBSTACLE-TYPE_Wire_obstacle,_double_fence">
    <rdfs:subClassOf rdf:resource="jc3iedm_OBJECT-TYPE.owl#MILITARY-OBSTACLE-TYPE"/>
    <rdfs:label xml:lang="en">wire obstacle, double fence</rdfs:label>
    <rdfs:comment xml:lang="en">No definition provided in APP-6A.</rdfs:comment>
    <rdf:type rdf:resource="http://www.w3.org/2002/07/owl#Class"/>
  </rdf:Description>
  <rdf:Description rdf:about="#FACILITY-TYPE_Military_materiel_facility,_engineering_equipment_production">
    <rdfs:subClassOf rdf:resource="jc3iedm_OBJECT-TYPE.owl#FACILITY-TYPE"/>
    <rdfs:label xml:lang="en">military materiel facility, engineering equipment production</rdfs:label>
    <rdfs:comment xml:lang="en">A facility used as for engineering equipment production.</rdfs:comment>
    <rdf:type rdf:resource="http://www.w3.org/2002/07/owl#Class"/>
  </rdf:Description>
  <rdf:Description rdf:about="#VEHICLE-TYPE_Automobile">
    <rdfs:subClassOf rdf:resource="jc3iedm_OBJECT-TYPE.owl#VEHICLE-TYPE"/>
    <rdfs:label xml:lang="en">automobile</rdfs:label>
    <rdfs:comment xml:lang="en">A self-propelled passenger vehicle.</rdfs:comment>
    <rdf:type rdf:resource="http://www.w3.org/2002/07/owl#Class"/>
  </rdf:Description>
  <rdf:Description rdf:about="#FACILITY-TYPE_Chimney/smokestack">
    <rdfs:subClassOf rdf:resource="jc3iedm_OBJECT-TYPE.owl#FACILITY-TYPE"/>
    <rdfs:label xml:lang="en">chimney/smokestack</rdfs:label>
    <rdfs:comment xml:lang="en">A vertical structure containing a passage or flue for discharging smoke and gases of combustion.</rdfs:comment>
    <rdf:type rdf:resource="http://www.w3.org/2002/07/owl#Class"/>
  </rdf:Description>
  <rdf:Description rdf:about="#PERSON-TYPE_Military">
    <rdfs:subClassOf rdf:resource="jc3iedm_OBJECT-TYPE.owl#PERSON-TYPE"/>
    <rdfs:label xml:lang="en">military</rdfs:label>
    <rdfs:comment xml:lang="en">A PERSON-TYPE who is a uniformed member of a regular armed force.</rdfs:comment>
    <rdf:type rdf:resource="http://www.w3.org/2002/07/owl#Class"/>
  </rdf:Description>
  <rdf:Description rdf:about="#CONTROL-FEATURE-TYPE_Desired_mean_point_of_impact">
    <rdfs:subClassOf rdf:resource="jc3iedm_OBJECT-TYPE.owl#CONTROL-FEATURE-TYPE"/>
    <rdfs:label xml:lang="en">desired mean point of impact</rdfs:label>
    <rdfs:comment xml:lang="en">The point at which a projectile, bomb, or re-entry vehicle is expected to impact.</rdfs:comment>
    <rdf:type rdf:resource="http://www.w3.org/2002/07/owl#Class"/>
  </rdf:Description>
  <rdf:Description rdf:about="#SURFACE-VESSEL-TYPE_Patrol_boat,_police">
    <rdfs:subClassOf rdf:resource="jc3iedm_OBJECT-TYPE.owl#SURFACE-VESSEL-TYPE"/>
    <rdfs:label xml:lang="en">patrol boat, police</rdfs:label>
    <rdfs:comment xml:lang="en">Police operated coastal patrol unit intended for a basically coastal guarding function. Includes any coastal patrol ship under 45 metres that cannot qualify as a Patrol ship, gun equipped, general in armament. May be unarmed.</rdfs:comment>
    <rdf:type rdf:resource="http://www.w3.org/2002/07/owl#Class"/>
  </rdf:Description>
  <rdf:Description rdf:about="#UNIT-TYPE_Not_otherwise_specified">
    <rdfs:subClassOf rdf:resource="jc3iedm_OBJECT-TYPE.owl#UNIT-TYPE"/>
    <rdfs:label xml:lang="en">not otherwise specified</rdfs:label>
    <rdfs:comment xml:lang="en">The appropriate value is not in the set of specified values.</rdfs:comment>
    <rdf:type rdf:resource="http://www.w3.org/2002/07/owl#Class"/>
  </rdf:Description>
  <rdf:Description rdf:about="#FACILITY-TYPE_Ford,_stone_lined_bed">
    <rdfs:subClassOf rdf:resource="jc3iedm_OBJECT-TYPE.owl#FACILITY-TYPE"/>
    <rdfs:label xml:lang="en">ford, stone lined bed</rdfs:label>
    <rdfs:comment xml:lang="en">A shallow place in a river or other water marked with a stone-lined bed that can be crossed without bridging, boats, or rafts.</rdfs:comment>
    <rdf:type rdf:resource="http://www.w3.org/2002/07/owl#Class"/>
  </rdf:Description>
  <rdf:Description rdf:about="#CONTROL-FEATURE-TYPE_No_go_area,_civil">
    <rdfs:subClassOf rdf:resource="jc3iedm_OBJECT-TYPE.owl#CONTROL-FEATURE-TYPE"/>
    <rdfs:label xml:lang="en">no go area, civil</rdfs:label>
    <rdfs:comment xml:lang="en">An area to which access is denied by civil authority or group of people (e.g. faction, gang, militia).</rdfs:comment>
    <rdf:type rdf:resource="http://www.w3.org/2002/07/owl#Class"/>
  </rdf:Description>
  <rdf:Description rdf:about="#CBRN-EQUIPMENT-TYPE_CBRN_decontamination_vehicle">
    <rdfs:subClassOf rdf:resource="jc3iedm_OBJECT-TYPE.owl#CBRN-EQUIPMENT-TYPE"/>
    <rdfs:label xml:lang="en">cbrn decontamination vehicle</rdfs:label>
    <rdfs:comment xml:lang="en">A vehicle that, as its primary function, is equipped to decontaminate persons or equipment contaminated by an NBC (CBRN) exposure.</rdfs:comment>
    <rdf:type rdf:resource="http://www.w3.org/2002/07/owl#Class"/>
  </rdf:Description>
  <rdf:Description rdf:about="#AMMUNITION-TYPE_Seabed_mine">
    <rdfs:subClassOf rdf:resource="jc3iedm_OBJECT-TYPE.owl#AMMUNITION-TYPE"/>
    <rdfs:label xml:lang="en">seabed mine</rdfs:label>
    <rdfs:comment xml:lang="en">A mine with negative buoyancy, which remains on the seabed. (bottom mine)</rdfs:comment>
    <rdf:type rdf:resource="http://www.w3.org/2002/07/owl#Class"/>
  </rdf:Description>
  <rdf:Description rdf:about="#SURFACE-VESSEL-TYPE_Speedboat">
    <rdfs:subClassOf rdf:resource="jc3iedm_OBJECT-TYPE.owl#SURFACE-VESSEL-TYPE"/>
    <rdfs:label xml:lang="en">speedboat</rdfs:label>
    <rdfs:comment xml:lang="en">Small, sleek boat capable of high speeds with or without outboard engines.</rdfs:comment>
    <rdf:type rdf:resource="http://www.w3.org/2002/07/owl#Class"/>
  </rdf:Description>
  <rdf:Description rdf:about="#FACILITY-TYPE_Apartment_building">
    <rdfs:subClassOf rdf:resource="jc3iedm_OBJECT-TYPE.owl#FACILITY-TYPE"/>
    <rdfs:label xml:lang="en">apartment building</rdfs:label>
    <rdfs:comment xml:lang="en">A residential unit consisting of a block of flats.</rdfs:comment>
    <rdf:type rdf:resource="http://www.w3.org/2002/07/owl#Class"/>
  </rdf:Description>
  <rdf:Description rdf:about="jc3iedm_OBJECT-TYPE.owl#organisation-type-description-text">
    <rdf:type rdf:resource="http://www.w3.org/2002/07/owl#DatatypeProperty"/>
    <rdfs:domain rdf:resource="jc3iedm_OBJECT-TYPE.owl#ORGANISATION-TYPE"/>
    <rdfs:range rdf:resource="http://www.w3.org/2001/XMLSchema#string"/>
  </rdf:Description>
  <rdf:Description rdf:about="#SURFACE-VESSEL-TYPE_Deep_submergence_support_ship">
    <rdfs:subClassOf rdf:resource="jc3iedm_OBJECT-TYPE.owl#SURFACE-VESSEL-TYPE"/>
    <rdfs:label xml:lang="en">deep submergence support ship</rdfs:label>
    <rdfs:comment xml:lang="en">A ship with special facilities to support deep submergence diving operations.</rdfs:comment>
    <rdf:type rdf:resource="http://www.w3.org/2002/07/owl#Class"/>
  </rdf:Description>
  <rdf:Description rdf:about="#FACILITY-TYPE_Depot,_not_otherwise_specified">
    <rdfs:subClassOf rdf:resource="jc3iedm_OBJECT-TYPE.owl#FACILITY-TYPE"/>
    <rdfs:label xml:lang="en">depot, not otherwise specified</rdfs:label>
    <rdfs:comment xml:lang="en">An area used for the storage of products or supplies. A facility for the receipt, classification, storage, accounting, issue, maintenance, procurement, manufacture, assembly, research, salvage or disposal of material.</rdfs:comment>
    <rdf:type rdf:resource="http://www.w3.org/2002/07/owl#Class"/>
  </rdf:Description>
  <rdf:Description rdf:about="#SURFACE-VESSEL-TYPE_Minesweeper,_general">
    <rdfs:subClassOf rdf:resource="jc3iedm_OBJECT-TYPE.owl#SURFACE-VESSEL-TYPE"/>
    <rdfs:label xml:lang="en">minesweeper, general</rdfs:label>
    <rdfs:comment xml:lang="en">Ship designed to sweep mines.</rdfs:comment>
    <rdf:type rdf:resource="http://www.w3.org/2002/07/owl#Class"/>
  </rdf:Description>
  <rdf:Description rdf:about="#FACILITY-TYPE_Network">
    <rdfs:subClassOf rdf:resource="jc3iedm_OBJECT-TYPE.owl#FACILITY-TYPE"/>
    <rdfs:label xml:lang="en">network</rdfs:label>
    <rdfs:comment xml:lang="en">A FACILITY-TYPE that provides communication and information services.</rdfs:comment>
    <rdf:type rdf:resource="http://www.w3.org/2002/07/owl#Class"/>
  </rdf:Description>
  <rdf:Description rdf:about="#VEHICLE-TYPE_Half-track">
    <rdfs:subClassOf rdf:resource="jc3iedm_OBJECT-TYPE.owl#VEHICLE-TYPE"/>
    <rdfs:label xml:lang="en">half track</rdfs:label>
    <rdfs:comment xml:lang="en">A vehicle, usually military, with wheels in front and tracks in the rear.</rdfs:comment>
    <rdf:type rdf:resource="http://www.w3.org/2002/07/owl#Class"/>
  </rdf:Description>
  <rdf:Description rdf:about="#CHEMICAL-MATERIEL-TYPE_Blister_agent">
    <rdfs:subClassOf rdf:resource="jc3iedm_OBJECT-TYPE.owl#CHEMICAL-MATERIEL-TYPE"/>
    <rdfs:label xml:lang="en">blister agent</rdfs:label>
    <rdfs:comment xml:lang="en">A CHEMICAL-MATERIEL-TYPE that injures the eyes and lungs, and burns or blisters the skin. Also called "vesicant agent".</rdfs:comment>
    <rdf:type rdf:resource="http://www.w3.org/2002/07/owl#Class"/>
  </rdf:Description>
  <rdf:Description rdf:about="#SURFACE-VESSEL-TYPE_Floating_dry_dock_workshop_(hull)">
    <rdfs:subClassOf rdf:resource="jc3iedm_OBJECT-TYPE.owl#SURFACE-VESSEL-TYPE"/>
    <rdfs:label xml:lang="en">floating dry dock workshop (hull)</rdfs:label>
    <rdfs:comment xml:lang="en">Non-self- propelled dry dock with workshop facilities optimised for hull repairs.</rdfs:comment>
    <rdf:type rdf:resource="http://www.w3.org/2002/07/owl#Class"/>
  </rdf:Description>
  <rdf:Description rdf:about="#CIVILIAN-POST-TYPE_Mayor">
    <rdfs:subClassOf rdf:resource="jc3iedm_OBJECT-TYPE.owl#CIVILIAN-POST-TYPE"/>
    <rdfs:label xml:lang="en">mayor</rdfs:label>
    <rdfs:comment xml:lang="en">A CIVILIAN-POST-TYPE whose job is the chief officer of the municipal corporation of a city or borough.</rdfs:comment>
    <rdf:type rdf:resource="http://www.w3.org/2002/07/owl#Class"/>
  </rdf:Description>
  <rdf:Description rdf:about="#CONTROL-FEATURE-TYPE_Electronic_combat_area">
    <rdfs:subClassOf rdf:resource="jc3iedm_OBJECT-TYPE.owl#CONTROL-FEATURE-TYPE"/>
    <rdfs:label xml:lang="en">electronic combat area</rdfs:label>
    <rdfs:comment xml:lang="en">Airspace established specifically for airborne platforms engaging in electronic combat.</rdfs:comment>
    <rdf:type rdf:resource="http://www.w3.org/2002/07/owl#Class"/>
  </rdf:Description>
  <rdf:Description rdf:about="#GROUP-ORGANISATION-TYPE_Merchant">
    <rdfs:subClassOf rdf:resource="jc3iedm_OBJECT-TYPE.owl#GROUP-ORGANISATION-TYPE"/>
    <rdfs:label xml:lang="en">merchant</rdfs:label>
    <rdfs:comment xml:lang="en">A GROUP-ORGANISATION-TYPE that comprises persons whose occupation is the purchase and sale of marketable commodities for profit.</rdfs:comment>
    <rdf:type rdf:resource="http://www.w3.org/2002/07/owl#Class"/>
  </rdf:Description>
  <rdf:Description rdf:about="#RADIOACTIVE-MATERIEL-TYPE_Plutonium-239">
    <rdfs:subClassOf rdf:resource="jc3iedm_OBJECT-TYPE.owl#RADIOACTIVE-MATERIEL-TYPE"/>
    <rdfs:label xml:lang="en">plutonium 239</rdfs:label>
    <rdfs:comment xml:lang="en">A radioactive isotope of the chemical element of atomic number 94, a dense silvery radioactive metal of the actinide series, used as a fuel in nuclear reactors and as an explosive in nuclear fission weapons.</rdfs:comment>
    <rdf:type rdf:resource="http://www.w3.org/2002/07/owl#Class"/>
  </rdf:Description>
  <rdf:Description rdf:about="#MILITARY-OBSTACLE-TYPE_Abatis">
    <rdfs:subClassOf rdf:resource="jc3iedm_OBJECT-TYPE.owl#MILITARY-OBSTACLE-TYPE"/>
    <rdfs:label xml:lang="en">abatis</rdfs:label>
    <rdfs:comment xml:lang="en">A vehicular obstacle constructed by felling trees (leaving a 1-2 meter stump above the ground on both sides of a road, trail, gap, or defile) so that they fall, interlocking, toward the expected direction of enemy approach. The trees should remain attached to the stumps, be at a 45 degree angle to the roadway, and the obstacle itself should be at least 75 meters in depth to be most effective.</rdfs:comment>
    <rdf:type rdf:resource="http://www.w3.org/2002/07/owl#Class"/>
  </rdf:Description>
  <rdf:Description rdf:about="#SURFACE-VESSEL-TYPE_Auxiliary_floating_drydock,_medium">
    <rdfs:subClassOf rdf:resource="jc3iedm_OBJECT-TYPE.owl#SURFACE-VESSEL-TYPE"/>
    <rdfs:label xml:lang="en">auxiliary floating drydock, medium</rdfs:label>
    <rdfs:comment xml:lang="en">Floating dock capable of docking medium and small ships.</rdfs:comment>
    <rdf:type rdf:resource="http://www.w3.org/2002/07/owl#Class"/>
  </rdf:Description>
  <rdf:Description rdf:about="#TASK-FORMATION-TYPE_Naval_task_element">
    <rdfs:subClassOf rdf:resource="jc3iedm_OBJECT-TYPE.owl#TASK-FORMATION-TYPE"/>
    <rdfs:label xml:lang="en">naval task element</rdfs:label>
    <rdfs:comment xml:lang="en">A TASK-FORMATION-TYPE that is a component of a task unit organized by the commander of the task unit or higher authority for accomplishing a specific task.</rdfs:comment>
    <rdf:type rdf:resource="http://www.w3.org/2002/07/owl#Class"/>
  </rdf:Description>
  <rdf:Description rdf:about="#SURFACE-VESSEL-TYPE_Merchant_ship,_tug,_ocean-going_rescue">
    <rdfs:subClassOf rdf:resource="jc3iedm_OBJECT-TYPE.owl#SURFACE-VESSEL-TYPE"/>
    <rdfs:label xml:lang="en">merchant ship, tug, ocean going rescue</rdfs:label>
    <rdfs:comment xml:lang="en">Non-naval sea-going tug with horsepower of 1000 or more, length usually over 60 metres and extensively equipped for fire fighting and rescue operations.</rdfs:comment>
    <rdf:type rdf:resource="http://www.w3.org/2002/07/owl#Class"/>
  </rdf:Description>
  <rdf:Description rdf:about="#VEHICLE-TYPE_Landing_vehicle">
    <rdfs:subClassOf rdf:resource="jc3iedm_OBJECT-TYPE.owl#VEHICLE-TYPE"/>
    <rdfs:label xml:lang="en">landing vehicle</rdfs:label>
    <rdfs:comment xml:lang="en">No definition provided in ADatP-3 Baseline 13.1 FFIRN/FUD 1650/6.</rdfs:comment>
    <rdf:type rdf:resource="http://www.w3.org/2002/07/owl#Class"/>
  </rdf:Description>
  <rdf:Description rdf:about="#FACILITY-TYPE_Revetment">
    <rdfs:subClassOf rdf:resource="jc3iedm_OBJECT-TYPE.owl#FACILITY-TYPE"/>
    <rdfs:label xml:lang="en">revetment</rdfs:label>
    <rdfs:comment xml:lang="en">An embankment to provide shelter (as against bomb splinters or strafing).</rdfs:comment>
    <rdf:type rdf:resource="http://www.w3.org/2002/07/owl#Class"/>
  </rdf:Description>
  <rdf:Description rdf:about="#SURFACE-VESSEL-TYPE_Minesweeper,_special_device">
    <rdfs:subClassOf rdf:resource="jc3iedm_OBJECT-TYPE.owl#SURFACE-VESSEL-TYPE"/>
    <rdfs:label xml:lang="en">minesweeper, special device</rdfs:label>
    <rdfs:comment xml:lang="en">A minesweeper fitted with special to type minesweeping devices.</rdfs:comment>
    <rdf:type rdf:resource="http://www.w3.org/2002/07/owl#Class"/>
  </rdf:Description>
  <rdf:Description rdf:about="jc3iedm_OBJECT-TYPE.owl#materiel-type-issuing-length-dimension">
    <rdf:type rdf:resource="http://www.w3.org/2002/07/owl#DatatypeProperty"/>
    <rdfs:domain rdf:resource="jc3iedm_OBJECT-TYPE.owl#MATERIEL-TYPE"/>
  </rdf:Description>
  <rdf:Description rdf:about="#CONSUMABLE-MATERIEL-TYPE_Medical_supply">
    <rdfs:subClassOf rdf:resource="jc3iedm_OBJECT-TYPE.owl#CONSUMABLE-MATERIEL-TYPE"/>
    <rdfs:label xml:lang="en">medical supply</rdfs:label>
    <rdfs:comment xml:lang="en">Supplies for the treatment of injuries, illness and disease, including drugs.</rdfs:comment>
    <rdf:type rdf:resource="http://www.w3.org/2002/07/owl#Class"/>
  </rdf:Description>
  <rdf:Description rdf:about="#RADIOACTIVE-MATERIEL-TYPE_Nuclear_weapon_fallout">
    <rdfs:subClassOf rdf:resource="jc3iedm_OBJECT-TYPE.owl#RADIOACTIVE-MATERIEL-TYPE"/>
    <rdfs:label xml:lang="en">nuclear weapon fallout</rdfs:label>
    <rdfs:comment xml:lang="en">Radioactive residues originating in a nuclear explosion.</rdfs:comment>
    <rdf:type rdf:resource="http://www.w3.org/2002/07/owl#Class"/>
  </rdf:Description>
  <rdf:Description rdf:about="#SURFACE-VESSEL-TYPE_Patrol_ship,_gun_equipped,_general">
    <rdfs:subClassOf rdf:resource="jc3iedm_OBJECT-TYPE.owl#SURFACE-VESSEL-TYPE"/>
    <rdfs:label xml:lang="en">patrol ship, gun equipped, general</rdfs:label>
    <rdfs:comment xml:lang="en">Patrol, blockade and surveillance ship in range 45-85 metres overall. Designed to operate in other than open ocean areas. Has special mission of attacking hostile ships. Must have at least 76mm main armament.</rdfs:comment>
    <rdf:type rdf:resource="http://www.w3.org/2002/07/owl#Class"/>
  </rdf:Description>
  <rdf:Description rdf:about="#AMMUNITION-TYPE_Bomblet">
    <rdfs:subClassOf rdf:resource="jc3iedm_OBJECT-TYPE.owl#AMMUNITION-TYPE"/>
    <rdfs:label xml:lang="en">bomblet</rdfs:label>
    <rdfs:comment xml:lang="en">One of a number of small bombs usually contained in a cluster bomb and released in mid-air.</rdfs:comment>
    <rdf:type rdf:resource="http://www.w3.org/2002/07/owl#Class"/>
  </rdf:Description>
  <rdf:Description rdf:about="#FACILITY-TYPE_Medical_support">
    <rdfs:subClassOf rdf:resource="jc3iedm_OBJECT-TYPE.owl#FACILITY-TYPE"/>
    <rdfs:label xml:lang="en">medical support</rdfs:label>
    <rdfs:comment xml:lang="en">A facility that hosts medical personnel who carry out treatment of sick or wounded persons.</rdfs:comment>
    <rdf:type rdf:resource="http://www.w3.org/2002/07/owl#Class"/>
  </rdf:Description>
  <rdf:Description rdf:about="#CONTROL-FEATURE-TYPE_Identification_safety_point">
    <rdfs:subClassOf rdf:resource="jc3iedm_OBJECT-TYPE.owl#CONTROL-FEATURE-TYPE"/>
    <rdfs:label xml:lang="en">identification safety point</rdfs:label>
    <rdfs:comment xml:lang="en">A point at which aircraft, on joining a maritime force, will attempt to establish two-way communications with the surface force and commence identification procedures.</rdfs:comment>
    <rdf:type rdf:resource="http://www.w3.org/2002/07/owl#Class"/>
  </rdf:Description>
  <rdf:Description rdf:about="jc3iedm_OBJECT-TYPE.owl#ENGINEERING-EQUIPMENT-TYPE">
    <rdf:type rdf:resource="http://www.w3.org/2002/07/owl#Class"/>
    <rdfs:label xml:lang="en">engineering equipment type</rdfs:label>
    <rdfs:comment xml:lang="en">An EQUIPMENT-TYPE that is designed to accomplish engineering functions.</rdfs:comment>
    <rdfs:subClassOf rdf:resource="jc3iedm_OBJECT-TYPE.owl#EQUIPMENT-TYPE"/>
  </rdf:Description>
  <rdf:Description rdf:about="#SURFACE-VESSEL-TYPE_Patrol_combatant,_hovercraft">
    <rdfs:subClassOf rdf:resource="jc3iedm_OBJECT-TYPE.owl#SURFACE-VESSEL-TYPE"/>
    <rdfs:label xml:lang="en">patrol combatant, hovercraft</rdfs:label>
    <rdfs:comment xml:lang="en">A high-speed patrol hovercraft that can conduct surveillance screening and special operations and is operated by naval or marine forces.</rdfs:comment>
    <rdf:type rdf:resource="http://www.w3.org/2002/07/owl#Class"/>
  </rdf:Description>
  <rdf:Description rdf:about="#WEAPON-TYPE_Mortar">
    <rdfs:subClassOf rdf:resource="jc3iedm_OBJECT-TYPE.owl#WEAPON-TYPE"/>
    <rdfs:label xml:lang="en">mortar</rdfs:label>
    <rdfs:comment xml:lang="en">A portable, muzzle-loading cannon used to fire shells at low velocities, short ranges, and high trajectories.</rdfs:comment>
    <rdf:type rdf:resource="http://www.w3.org/2002/07/owl#Class"/>
  </rdf:Description>
  <rdf:Description rdf:about="#VEHICLE-TYPE_Armoured_reconnaissance_carrier">
    <rdfs:subClassOf rdf:resource="jc3iedm_OBJECT-TYPE.owl#VEHICLE-TYPE"/>
    <rdfs:label xml:lang="en">armoured reconnaissance carrier</rdfs:label>
    <rdfs:comment xml:lang="en">An armoured vehicle used to carry persons for reconnaissance activities.</rdfs:comment>
    <rdf:type rdf:resource="http://www.w3.org/2002/07/owl#Class"/>
  </rdf:Description>
  <rdf:Description rdf:about="#SURFACE-VESSEL-TYPE_Oiler_transport_(naval)">
    <rdfs:subClassOf rdf:resource="jc3iedm_OBJECT-TYPE.owl#SURFACE-VESSEL-TYPE"/>
    <rdfs:label xml:lang="en">oiler transport (naval)</rdfs:label>
    <rdfs:comment xml:lang="en">Ship usually exceeding 120 metres capable of transporting POL products but not specially fitted to provide underway replenishment.</rdfs:comment>
    <rdf:type rdf:resource="http://www.w3.org/2002/07/owl#Class"/>
  </rdf:Description>
  <rdf:Description rdf:about="#TASK-FORMATION-TYPE_Combat_control_team">
    <rdfs:subClassOf rdf:resource="jc3iedm_OBJECT-TYPE.owl#TASK-FORMATION-TYPE"/>
    <rdfs:label xml:lang="en">combat control team</rdfs:label>
    <rdfs:comment xml:lang="en">A TASK-FORMATION-TYPE that consists of parachute and combat diver qualified personnel trained and equipped to rapidly establish and control drop, landing, and extraction zone air traffic in austere or hostile conditions. They survey and establish terminal airheads as well as provide guidance to aircraft for airlift operations. They provide command and control, and conduct reconnaissance, surveillance, and survey assessments of potential objective airfields or assault zones.</rdfs:comment>
    <rdf:type rdf:resource="http://www.w3.org/2002/07/owl#Class"/>
  </rdf:Description>
  <rdf:Description rdf:about="#SURFACE-VESSEL-TYPE_Patrol_combatant,_hydrofoil">
    <rdfs:subClassOf rdf:resource="jc3iedm_OBJECT-TYPE.owl#SURFACE-VESSEL-TYPE"/>
    <rdfs:label xml:lang="en">patrol combatant, hydrofoil</rdfs:label>
    <rdfs:comment xml:lang="en">Patrol, blockade and surveillance ship in range 45-85 metres overall. Designed to operate in other than open ocean areas. Has special mission of attacking hostile ships. Must have at least 76mm main armament and is fitted with hydrofoils.</rdfs:comment>
    <rdf:type rdf:resource="http://www.w3.org/2002/07/owl#Class"/>
  </rdf:Description>
  <rdf:Description rdf:about="#VEHICLE-TYPE_Trolley_bus">
    <rdfs:subClassOf rdf:resource="jc3iedm_OBJECT-TYPE.owl#VEHICLE-TYPE"/>
    <rdfs:label xml:lang="en">trolley bus</rdfs:label>
    <rdfs:comment xml:lang="en">A bus powered by electricity obtained from an overhead cable by means of a trolley-wheel.</rdfs:comment>
    <rdf:type rdf:resource="http://www.w3.org/2002/07/owl#Class"/>
  </rdf:Description>
  <rdf:Description rdf:about="#FACILITY-TYPE_Mass_grave">
    <rdfs:subClassOf rdf:resource="jc3iedm_OBJECT-TYPE.owl#FACILITY-TYPE"/>
    <rdfs:label xml:lang="en">mass grave</rdfs:label>
    <rdfs:comment xml:lang="en">A FACILITY-TYPE used for the burial of multiple bodies.</rdfs:comment>
    <rdf:type rdf:resource="http://www.w3.org/2002/07/owl#Class"/>
  </rdf:Description>
  <rdf:Description rdf:about="#AMMUNITION-TYPE_Mine,_anti-tank_with_anti-handling_device">
    <rdfs:subClassOf rdf:resource="jc3iedm_OBJECT-TYPE.owl#AMMUNITION-TYPE"/>
    <rdfs:label xml:lang="en">mine, anti tank with anti handling device</rdfs:label>
    <rdfs:comment xml:lang="en">A mine designed to immobilize or destroy a tank. The mine includes an internal or external device arranged to actuate it in case of attempts to deactivate the mine.</rdfs:comment>
    <rdf:type rdf:resource="http://www.w3.org/2002/07/owl#Class"/>
  </rdf:Description>
  <rdf:Description rdf:about="#SURFACE-VESSEL-TYPE_Oiler_transport,_small_(naval)">
    <rdfs:subClassOf rdf:resource="jc3iedm_OBJECT-TYPE.owl#SURFACE-VESSEL-TYPE"/>
    <rdfs:label xml:lang="en">oiler transport, small (naval)</rdfs:label>
    <rdfs:comment xml:lang="en">Ship between 40-120 metres capable of transporting POL products but not specially fitted to provide underway replenishment.</rdfs:comment>
    <rdf:type rdf:resource="http://www.w3.org/2002/07/owl#Class"/>
  </rdf:Description>
  <rdf:Description rdf:about="#CONTROL-FEATURE-TYPE_No_go_area">
    <rdfs:subClassOf rdf:resource="jc3iedm_OBJECT-TYPE.owl#CONTROL-FEATURE-TYPE"/>
    <rdfs:label xml:lang="en">no go area</rdfs:label>
    <rdfs:comment xml:lang="en">An area that is not trafficable.</rdfs:comment>
    <rdf:type rdf:resource="http://www.w3.org/2002/07/owl#Class"/>
  </rdf:Description>
  <rdf:Description rdf:about="#FACILITY-TYPE_Unit_of_accommodation">
    <rdfs:subClassOf rdf:resource="jc3iedm_OBJECT-TYPE.owl#FACILITY-TYPE"/>
    <rdfs:label xml:lang="en">unit of accommodation</rdfs:label>
    <rdfs:comment xml:lang="en">An amount of living space distinct and separate. (Intended for humanitarian aid scenario to enable general indication of accommodation requirements).</rdfs:comment>
    <rdf:type rdf:resource="http://www.w3.org/2002/07/owl#Class"/>
  </rdf:Description>
  <rdf:Description rdf:about="#FACILITY-TYPE_Civilian_collection_point">
    <rdfs:subClassOf rdf:resource="jc3iedm_OBJECT-TYPE.owl#FACILITY-TYPE"/>
    <rdfs:label xml:lang="en">civilian collection point</rdfs:label>
    <rdfs:comment xml:lang="en">A facility where civilians are assembled for classification, sorting or further movement to other facilities or installations.</rdfs:comment>
    <rdf:type rdf:resource="http://www.w3.org/2002/07/owl#Class"/>
  </rdf:Description>
  <rdf:Description rdf:about="#PRIVATE-SECTOR-ORGANISATION-TYPE_Defence_industry">
    <rdfs:subClassOf rdf:resource="jc3iedm_OBJECT-TYPE.owl#PRIVATE-SECTOR-ORGANISATION-TYPE"/>
    <rdfs:label xml:lang="en">defence industry</rdfs:label>
    <rdfs:comment xml:lang="en">A PRIVATE-SECTOR-ORGANISATION-TYPE whose predominant business is defence in nature.</rdfs:comment>
    <rdf:type rdf:resource="http://www.w3.org/2002/07/owl#Class"/>
  </rdf:Description>
  <rdf:Description rdf:about="#CONTROL-FEATURE-TYPE_Radiation_dose_rate_contour_line">
    <rdfs:subClassOf rdf:resource="jc3iedm_OBJECT-TYPE.owl#CONTROL-FEATURE-TYPE"/>
    <rdfs:label xml:lang="en">radiation dose rate contour line</rdfs:label>
    <rdfs:comment xml:lang="en">A line on a map, diagram or overlay joining all points at which the radiation dose rate at a given time is the same. Radiation dose rate is the rate at which energy from ionizing radiation is absorbed.</rdfs:comment>
    <rdf:type rdf:resource="http://www.w3.org/2002/07/owl#Class"/>
  </rdf:Description>
  <rdf:Description rdf:about="#SURFACE-VESSEL-TYPE_Barge,_salvage">
    <rdfs:subClassOf rdf:resource="jc3iedm_OBJECT-TYPE.owl#SURFACE-VESSEL-TYPE"/>
    <rdfs:label xml:lang="en">barge, salvage</rdfs:label>
    <rdfs:comment xml:lang="en">Any utility barge used for salvage.</rdfs:comment>
    <rdf:type rdf:resource="http://www.w3.org/2002/07/owl#Class"/>
  </rdf:Description>
  <rdf:Description rdf:about="#PRIVATE-SECTOR-ORGANISATION-TYPE_Manufacturing">
    <rdfs:subClassOf rdf:resource="jc3iedm_OBJECT-TYPE.owl#PRIVATE-SECTOR-ORGANISATION-TYPE"/>
    <rdfs:label xml:lang="en">manufacturing</rdfs:label>
    <rdfs:comment xml:lang="en">A PRIVATE-SECTOR-ORGANISATION-TYPE whose predominant business is manufacturing in nature.</rdfs:comment>
    <rdf:type rdf:resource="http://www.w3.org/2002/07/owl#Class"/>
  </rdf:Description>
  <rdf:Description rdf:about="#AMMUNITION-TYPE_Mine,_shallow_moored">
    <rdfs:subClassOf rdf:resource="jc3iedm_OBJECT-TYPE.owl#AMMUNITION-TYPE"/>
    <rdfs:label xml:lang="en">mine, shallow moored</rdfs:label>
    <rdfs:comment xml:lang="en">Any mine case in less than a certain depth of water is shallow.</rdfs:comment>
    <rdf:type rdf:resource="http://www.w3.org/2002/07/owl#Class"/>
  </rdf:Description>
  <rdf:Description rdf:about="#FACILITY-TYPE_Town">
    <rdfs:subClassOf rdf:resource="jc3iedm_OBJECT-TYPE.owl#FACILITY-TYPE"/>
    <rdfs:label xml:lang="en">town</rdfs:label>
    <rdfs:comment xml:lang="en">An urban area with a name, defined boundaries and local government, being larger than a village and usually not created a city.</rdfs:comment>
    <rdf:type rdf:resource="http://www.w3.org/2002/07/owl#Class"/>
  </rdf:Description>
  <rdf:Description rdf:about="#SURFACE-VESSEL-TYPE_Ammunition_ship,_transport,_small">
    <rdfs:subClassOf rdf:resource="jc3iedm_OBJECT-TYPE.owl#SURFACE-VESSEL-TYPE"/>
    <rdfs:label xml:lang="en">ammunition ship, transport, small</rdfs:label>
    <rdfs:comment xml:lang="en">Ship capable of handling less than 5000 tons of ammunition but lacking sophisticated underway replenishment capabilities.</rdfs:comment>
    <rdf:type rdf:resource="http://www.w3.org/2002/07/owl#Class"/>
  </rdf:Description>
  <rdf:Description rdf:about="#UNIT-TYPE_Armour">
    <rdfs:subClassOf rdf:resource="jc3iedm_OBJECT-TYPE.owl#UNIT-TYPE"/>
    <rdfs:label xml:lang="en">armour</rdfs:label>
    <rdfs:comment xml:lang="en">A UNIT-TYPE whose principal designation is the employment of tanks or other armoured direct fire weapon systems.</rdfs:comment>
    <rdf:type rdf:resource="http://www.w3.org/2002/07/owl#Class"/>
  </rdf:Description>
  <rdf:Description rdf:about="#CBRN-EQUIPMENT-TYPE_Not_known">
    <rdfs:subClassOf rdf:resource="jc3iedm_OBJECT-TYPE.owl#CBRN-EQUIPMENT-TYPE"/>
    <rdfs:label xml:lang="en">not known</rdfs:label>
    <rdfs:comment xml:lang="en">It is not possible to determine which value is most applicable.</rdfs:comment>
    <rdf:type rdf:resource="http://www.w3.org/2002/07/owl#Class"/>
  </rdf:Description>
  <rdf:Description rdf:about="#SURFACE-VESSEL-TYPE_Merchant_ship,_meteorological">
    <rdfs:subClassOf rdf:resource="jc3iedm_OBJECT-TYPE.owl#SURFACE-VESSEL-TYPE"/>
    <rdfs:label xml:lang="en">merchant ship, meteorological</rdfs:label>
    <rdfs:comment xml:lang="en">Non-naval ship designed primarily to monitor meteorological conditions.</rdfs:comment>
    <rdf:type rdf:resource="http://www.w3.org/2002/07/owl#Class"/>
  </rdf:Description>
  <rdf:Description rdf:about="#VEHICLE-TYPE_Transporter,_general">
    <rdfs:subClassOf rdf:resource="jc3iedm_OBJECT-TYPE.owl#VEHICLE-TYPE"/>
    <rdfs:label xml:lang="en">transporter, general</rdfs:label>
    <rdfs:comment xml:lang="en">A vehicle whose primary role is the transportation of heavy equipment.</rdfs:comment>
    <rdf:type rdf:resource="http://www.w3.org/2002/07/owl#Class"/>
  </rdf:Description>
  <rdf:Description rdf:about="#RADIOACTIVE-MATERIEL-TYPE_Cobalt-60">
    <rdfs:subClassOf rdf:resource="jc3iedm_OBJECT-TYPE.owl#RADIOACTIVE-MATERIEL-TYPE"/>
    <rdfs:label xml:lang="en">cobalt 60</rdfs:label>
    <rdfs:comment xml:lang="en">A radioactive isotope of the chemical element of atomic number 27, a hard silvery-white magnetic metal.</rdfs:comment>
    <rdf:type rdf:resource="http://www.w3.org/2002/07/owl#Class"/>
  </rdf:Description>
  <rdf:Description rdf:about="#SURFACE-VESSEL-TYPE_Mine_countermeasures_vessel,_unspecified">
    <rdfs:subClassOf rdf:resource="jc3iedm_OBJECT-TYPE.owl#SURFACE-VESSEL-TYPE"/>
    <rdfs:label xml:lang="en">mine countermeasures vessel, unspecified</rdfs:label>
    <rdfs:comment xml:lang="en">General designator for mine countermeasures vessel with no specification.</rdfs:comment>
    <rdf:type rdf:resource="http://www.w3.org/2002/07/owl#Class"/>
  </rdf:Description>
  <rdf:Description rdf:about="#AMMUNITION-TYPE_Projectile,_not_otherwise_specified">
    <rdfs:subClassOf rdf:resource="jc3iedm_OBJECT-TYPE.owl#AMMUNITION-TYPE"/>
    <rdfs:label xml:lang="en">projectile, not otherwise specified</rdfs:label>
    <rdfs:comment xml:lang="en">An object capable of being propelled by a force normally from a gun, and continuing in motion by virtue of its kinetic energy.</rdfs:comment>
    <rdf:type rdf:resource="http://www.w3.org/2002/07/owl#Class"/>
  </rdf:Description>
  <rdf:Description rdf:about="jc3iedm_OBJECT-TYPE.owl#GEOGRAPHIC-FEATURE-TYPE">
    <rdf:type rdf:resource="http://www.w3.org/2002/07/owl#Class"/>
    <rdfs:label xml:lang="en">geographic feature type</rdfs:label>
    <rdfs:comment xml:lang="en">A FEATURE-TYPE that describes terrain characteristics to which military significance is attached.</rdfs:comment>
    <rdfs:subClassOf rdf:resource="jc3iedm_OBJECT-TYPE.owl#FEATURE-TYPE"/>
  </rdf:Description>
  <rdf:Description rdf:about="#SURFACE-VESSEL-TYPE_Fishing_vessel,_whale_catcher">
    <rdfs:subClassOf rdf:resource="jc3iedm_OBJECT-TYPE.owl#SURFACE-VESSEL-TYPE"/>
    <rdfs:label xml:lang="en">fishing vessel, whale catcher</rdfs:label>
    <rdfs:comment xml:lang="en">Fishing vessel equipped to engage in whale hunting.</rdfs:comment>
    <rdf:type rdf:resource="http://www.w3.org/2002/07/owl#Class"/>
  </rdf:Description>
  <rdf:Description rdf:about="#BIOLOGICAL-MATERIEL-TYPE_Toxic_industrial_material">
    <rdfs:subClassOf rdf:resource="jc3iedm_OBJECT-TYPE.owl#BIOLOGICAL-MATERIEL-TYPE"/>
    <rdfs:label xml:lang="en">toxic industrial material</rdfs:label>
    <rdfs:comment xml:lang="en">A generic term for a BIOLOGICAL-MATERIEL-TYPE compound in solid, liquid, aerosolised or gaseous form. It may be used, or stored for use, for industrial, commercial, medical, military or domestic purposes.</rdfs:comment>
    <rdf:type rdf:resource="http://www.w3.org/2002/07/owl#Class"/>
  </rdf:Description>
  <rdf:Description rdf:about="jc3iedm_OBJECT-TYPE.owl#equipment-type-category-code">
    <rdf:type rdf:resource="http://www.w3.org/2002/07/owl#DatatypeProperty"/>
    <rdfs:domain rdf:resource="jc3iedm_OBJECT-TYPE.owl#EQUIPMENT-TYPE"/>
    <rdfs:range rdf:resource="http://www.w3.org/2001/XMLSchema#string"/>
  </rdf:Description>
  <rdf:Description rdf:about="#CONTROL-FEATURE-TYPE_Key_terrain">
    <rdfs:subClassOf rdf:resource="jc3iedm_OBJECT-TYPE.owl#CONTROL-FEATURE-TYPE"/>
    <rdfs:label xml:lang="en">key terrain</rdfs:label>
    <rdfs:comment xml:lang="en">Any locality, or area, the seizure of which affords a marked advantage to either combatant.</rdfs:comment>
    <rdf:type rdf:resource="http://www.w3.org/2002/07/owl#Class"/>
  </rdf:Description>
  <rdf:Description rdf:about="#SURFACE-VESSEL-TYPE_Hovercraft,_general">
    <rdfs:subClassOf rdf:resource="jc3iedm_OBJECT-TYPE.owl#SURFACE-VESSEL-TYPE"/>
    <rdfs:label xml:lang="en">hovercraft, general</rdfs:label>
    <rdfs:comment xml:lang="en">A vehicle or craft that can be supported by a cushion of air ejected downwards against a surface close below it, and can in principle travel over any relatively smooth surface (as a body of water, marshland, gently sloping land) while having no significant contact with it.</rdfs:comment>
    <rdf:type rdf:resource="http://www.w3.org/2002/07/owl#Class"/>
  </rdf:Description>
  <rdf:Description rdf:about="#SURFACE-VESSEL-TYPE_Service_craft,_yard,_general">
    <rdfs:subClassOf rdf:resource="jc3iedm_OBJECT-TYPE.owl#SURFACE-VESSEL-TYPE"/>
    <rdfs:label xml:lang="en">service craft, yard, general</rdfs:label>
    <rdfs:comment xml:lang="en">General designator for yard service craft.</rdfs:comment>
    <rdf:type rdf:resource="http://www.w3.org/2002/07/owl#Class"/>
  </rdf:Description>
  <rdf:Description rdf:about="#FACILITY-TYPE_Military_base/facility,_seaport/naval_base">
    <rdfs:subClassOf rdf:resource="jc3iedm_OBJECT-TYPE.owl#FACILITY-TYPE"/>
    <rdfs:label xml:lang="en">military base/facility, seaport/naval base</rdfs:label>
    <rdfs:comment xml:lang="en">A facility that is used as a naval base and where ships may receive or discharge their cargoes.</rdfs:comment>
    <rdf:type rdf:resource="http://www.w3.org/2002/07/owl#Class"/>
  </rdf:Description>
  <rdf:Description rdf:about="#CONSUMABLE-MATERIEL-TYPE_Not_otherwise_specified">
    <rdfs:subClassOf rdf:resource="jc3iedm_OBJECT-TYPE.owl#CONSUMABLE-MATERIEL-TYPE"/>
    <rdfs:label xml:lang="en">not otherwise specified</rdfs:label>
    <rdfs:comment xml:lang="en">The appropriate value is not in the set of specified values.</rdfs:comment>
    <rdf:type rdf:resource="http://www.w3.org/2002/07/owl#Class"/>
  </rdf:Description>
  <rdf:Description rdf:about="#CONTROL-FEATURE-TYPE_Target_reference_point">
    <rdfs:subClassOf rdf:resource="jc3iedm_OBJECT-TYPE.owl#CONTROL-FEATURE-TYPE"/>
    <rdfs:label xml:lang="en">target reference point</rdfs:label>
    <rdfs:comment xml:lang="en">An easily recognisable point location on the ground (either natural or man-made) used to initiate, distribute, and control fires. TRPs can also designate the centre of an area where the commander plans to distribute or converge the fires of all his weapons rapidly. They are used by task force and below, and can further delineate sectors of fire within an engagement area. TRPs are designated using the standard target symbol and numbers issued by the fire support officer. Once designated, TRPs also constitute indirect fire targets.</rdfs:comment>
    <rdf:type rdf:resource="http://www.w3.org/2002/07/owl#Class"/>
  </rdf:Description>
  <rdf:Description rdf:about="#SURFACE-VESSEL-TYPE_Tank_cleaning_craft">
    <rdfs:subClassOf rdf:resource="jc3iedm_OBJECT-TYPE.owl#SURFACE-VESSEL-TYPE"/>
    <rdfs:label xml:lang="en">tank cleaning craft</rdfs:label>
    <rdfs:comment xml:lang="en">Craft equipped for steam cleaning liquid storage tanks or ships.</rdfs:comment>
    <rdf:type rdf:resource="http://www.w3.org/2002/07/owl#Class"/>
  </rdf:Description>
  <rdf:Description rdf:about="#CONTROL-FEATURE-TYPE_Air_defence_area">
    <rdfs:subClassOf rdf:resource="jc3iedm_OBJECT-TYPE.owl#CONTROL-FEATURE-TYPE"/>
    <rdfs:label xml:lang="en">air defence area</rdfs:label>
    <rdfs:comment xml:lang="en">A specifically defined airspace for which air defence must be planned and provided.</rdfs:comment>
    <rdf:type rdf:resource="http://www.w3.org/2002/07/owl#Class"/>
  </rdf:Description>
  <rdf:Description rdf:about="#CONTROL-FEATURE-TYPE_Close_air_support_holding_area">
    <rdfs:subClassOf rdf:resource="jc3iedm_OBJECT-TYPE.owl#CONTROL-FEATURE-TYPE"/>
    <rdfs:label xml:lang="en">close air support holding area</rdfs:label>
    <rdfs:comment xml:lang="en">Airspace designed for holding orbit and used by rotary and fixed-winged aircraft in close proximity to friendly forces.</rdfs:comment>
    <rdf:type rdf:resource="http://www.w3.org/2002/07/owl#Class"/>
  </rdf:Description>
  <rdf:Description rdf:about="#FACILITY-TYPE_Railway,_junction">
    <rdfs:subClassOf rdf:resource="jc3iedm_OBJECT-TYPE.owl#FACILITY-TYPE"/>
    <rdfs:label xml:lang="en">railway, junction</rdfs:label>
    <rdfs:comment xml:lang="en">A site where two or more railway tracks join or form a connection.</rdfs:comment>
    <rdf:type rdf:resource="http://www.w3.org/2002/07/owl#Class"/>
  </rdf:Description>
  <rdf:Description rdf:about="#CONTROL-FEATURE-TYPE_Land_fighter_engagement_zone">
    <rdfs:subClassOf rdf:resource="jc3iedm_OBJECT-TYPE.owl#CONTROL-FEATURE-TYPE"/>
    <rdfs:label xml:lang="en">land fighter engagement zone</rdfs:label>
    <rdfs:comment xml:lang="en">Airspace of defined dimensions within which the responsibility for engagement of air threats normally rests with the commander of the AD fighter package.</rdfs:comment>
    <rdf:type rdf:resource="http://www.w3.org/2002/07/owl#Class"/>
  </rdf:Description>
  <rdf:Description rdf:about="#FACILITY-TYPE_Berth">
    <rdfs:subClassOf rdf:resource="jc3iedm_OBJECT-TYPE.owl#FACILITY-TYPE"/>
    <rdfs:label xml:lang="en">berth</rdfs:label>
    <rdfs:comment xml:lang="en">A FACILITY-TYPE that is a space or length in the water at a harbour allocated to or reserved for a vessel to dock and moor for loading or unloading.</rdfs:comment>
    <rdf:type rdf:resource="http://www.w3.org/2002/07/owl#Class"/>
  </rdf:Description>
  <rdf:Description rdf:about="#CONTROL-FEATURE-TYPE_Safe_lane">
    <rdfs:subClassOf rdf:resource="jc3iedm_OBJECT-TYPE.owl#CONTROL-FEATURE-TYPE"/>
    <rdfs:label xml:lang="en">safe lane</rdfs:label>
    <rdfs:comment xml:lang="en">A bi-directional lane connecting an airbase, landing site and/or base defence zone to adjacent routes/corridors. Safe lanes may also be used to connect adjacent activated routes/corridors.</rdfs:comment>
    <rdf:type rdf:resource="http://www.w3.org/2002/07/owl#Class"/>
  </rdf:Description>
  <rdf:Description rdf:about="#CONTROL-FEATURE-TYPE_Downed_aircrew_pickup_point">
    <rdfs:subClassOf rdf:resource="jc3iedm_OBJECT-TYPE.owl#CONTROL-FEATURE-TYPE"/>
    <rdfs:label xml:lang="en">downed aircrew pickup point</rdfs:label>
    <rdfs:comment xml:lang="en">A point to where aviators will attempt to evade and escape to be recovered by friendly forces.</rdfs:comment>
    <rdf:type rdf:resource="http://www.w3.org/2002/07/owl#Class"/>
  </rdf:Description>
  <rdf:Description rdf:about="#FACILITY-TYPE_Slipway">
    <rdfs:subClassOf rdf:resource="jc3iedm_OBJECT-TYPE.owl#FACILITY-TYPE"/>
    <rdfs:label xml:lang="en">slipway</rdfs:label>
    <rdfs:comment xml:lang="en">A FACILITY-TYPE that provides a sloping surface or inclined structure leading down to the water.</rdfs:comment>
    <rdf:type rdf:resource="http://www.w3.org/2002/07/owl#Class"/>
  </rdf:Description>
  <rdf:Description rdf:about="#ELECTRONIC-EQUIPMENT-TYPE_Not_known">
    <rdfs:subClassOf rdf:resource="jc3iedm_OBJECT-TYPE.owl#ELECTRONIC-EQUIPMENT-TYPE"/>
    <rdfs:label xml:lang="en">not known</rdfs:label>
    <rdfs:comment xml:lang="en">It is not possible to determine which value is most applicable.</rdfs:comment>
    <rdf:type rdf:resource="http://www.w3.org/2002/07/owl#Class"/>
  </rdf:Description>
  <rdf:Description rdf:about="#SURFACE-VESSEL-TYPE_Minesweeper,_light">
    <rdfs:subClassOf rdf:resource="jc3iedm_OBJECT-TYPE.owl#SURFACE-VESSEL-TYPE"/>
    <rdfs:label xml:lang="en">minesweeper, light</rdfs:label>
    <rdfs:comment xml:lang="en">A small vessel designed to sweep mines.</rdfs:comment>
    <rdf:type rdf:resource="http://www.w3.org/2002/07/owl#Class"/>
  </rdf:Description>
  <rdf:Description rdf:about="#MISCELLANEOUS-EQUIPMENT-TYPE_Hazard_light">
    <rdfs:subClassOf rdf:resource="jc3iedm_OBJECT-TYPE.owl#MISCELLANEOUS-EQUIPMENT-TYPE"/>
    <rdfs:label xml:lang="en">hazard light</rdfs:label>
    <rdfs:comment xml:lang="en">A light source that is designed to identify the source or location of a hazard.</rdfs:comment>
    <rdf:type rdf:resource="http://www.w3.org/2002/07/owl#Class"/>
  </rdf:Description>
  <rdf:Description rdf:about="#ELECTRONIC-EQUIPMENT-TYPE_Data-processing">
    <rdfs:subClassOf rdf:resource="jc3iedm_OBJECT-TYPE.owl#ELECTRONIC-EQUIPMENT-TYPE"/>
    <rdfs:label xml:lang="en">data processing</rdfs:label>
    <rdfs:comment xml:lang="en">Equipment for storing, sharing and manipulation of data.</rdfs:comment>
    <rdf:type rdf:resource="http://www.w3.org/2002/07/owl#Class"/>
  </rdf:Description>
  <rdf:Description rdf:about="#CONSUMABLE-MATERIEL-TYPE_POL">
    <rdfs:subClassOf rdf:resource="jc3iedm_OBJECT-TYPE.owl#CONSUMABLE-MATERIEL-TYPE"/>
    <rdfs:label xml:lang="en">pol</rdfs:label>
    <rdfs:comment xml:lang="en">Petroleum, Oil, and Lubricant - A broad term that includes all petroleum and associated products used by the armed forces.</rdfs:comment>
    <rdf:type rdf:resource="http://www.w3.org/2002/07/owl#Class"/>
  </rdf:Description>
  <rdf:Description rdf:about="#SURFACE-VESSEL-TYPE_Submarine_tender,_small">
    <rdfs:subClassOf rdf:resource="jc3iedm_OBJECT-TYPE.owl#SURFACE-VESSEL-TYPE"/>
    <rdfs:label xml:lang="en">submarine tender, small</rdfs:label>
    <rdfs:comment xml:lang="en">Ship between 40-120 metres, which provide mobile base facilities and support for submarines.</rdfs:comment>
    <rdf:type rdf:resource="http://www.w3.org/2002/07/owl#Class"/>
  </rdf:Description>
  <rdf:Description rdf:about="#SURFACE-VESSEL-TYPE_Floating_target">
    <rdfs:subClassOf rdf:resource="jc3iedm_OBJECT-TYPE.owl#SURFACE-VESSEL-TYPE"/>
    <rdfs:label xml:lang="en">floating target</rdfs:label>
    <rdfs:comment xml:lang="en">Craft built to simulate a target.</rdfs:comment>
    <rdf:type rdf:resource="http://www.w3.org/2002/07/owl#Class"/>
  </rdf:Description>
  <rdf:Description rdf:about="#MARITIME-EQUIPMENT-TYPE_Electrode">
    <rdfs:subClassOf rdf:resource="jc3iedm_OBJECT-TYPE.owl#MARITIME-EQUIPMENT-TYPE"/>
    <rdfs:label xml:lang="en">electrode</rdfs:label>
    <rdfs:comment xml:lang="en">In naval mine warfare, a magnetic cable sweep in which salt water and the seabed form part of the electric circuit.</rdfs:comment>
    <rdf:type rdf:resource="http://www.w3.org/2002/07/owl#Class"/>
  </rdf:Description>
  <rdf:Description rdf:about="#SURFACE-VESSEL-TYPE_Light_ship">
    <rdfs:subClassOf rdf:resource="jc3iedm_OBJECT-TYPE.owl#SURFACE-VESSEL-TYPE"/>
    <rdfs:label xml:lang="en">light ship</rdfs:label>
    <rdfs:comment xml:lang="en">Ship actually moored or anchored in a fixed position showing navigational aiding light(s).</rdfs:comment>
    <rdf:type rdf:resource="http://www.w3.org/2002/07/owl#Class"/>
  </rdf:Description>
  <rdf:Description rdf:about="#SURFACE-VESSEL-TYPE_Tug,_ocean-going,_rescue">
    <rdfs:subClassOf rdf:resource="jc3iedm_OBJECT-TYPE.owl#SURFACE-VESSEL-TYPE"/>
    <rdfs:label xml:lang="en">tug, ocean going, rescue</rdfs:label>
    <rdfs:comment xml:lang="en">Seagoing tug employed to tow navy ships and craft. Usually about 40-50 metres, but equipped to operate with fleets and extensively equipped for fire fighting and rescue operations.</rdfs:comment>
    <rdf:type rdf:resource="http://www.w3.org/2002/07/owl#Class"/>
  </rdf:Description>
  <rdf:Description rdf:about="#CONTROL-FEATURE-TYPE_Obstacle_belt">
    <rdfs:subClassOf rdf:resource="jc3iedm_OBJECT-TYPE.owl#CONTROL-FEATURE-TYPE"/>
    <rdfs:label xml:lang="en">obstacle belt</rdfs:label>
    <rdfs:comment xml:lang="en">Normally, a brigade-level obstacle control measure that specifies the intent and location of subordinate obstacles. It also supports the intent of the higher headquarters obstacle zone.</rdfs:comment>
    <rdf:type rdf:resource="http://www.w3.org/2002/07/owl#Class"/>
  </rdf:Description>
  <rdf:Description rdf:about="#FACILITY-TYPE_Headquarters_facility">
    <rdfs:subClassOf rdf:resource="jc3iedm_OBJECT-TYPE.owl#FACILITY-TYPE"/>
    <rdfs:label xml:lang="en">headquarters facility</rdfs:label>
    <rdfs:comment xml:lang="en">A facility from which administrative and/or command functions are performed.</rdfs:comment>
    <rdf:type rdf:resource="http://www.w3.org/2002/07/owl#Class"/>
  </rdf:Description>
  <rdf:Description rdf:about="#CONTROL-FEATURE-TYPE_Incident_point">
    <rdfs:subClassOf rdf:resource="jc3iedm_OBJECT-TYPE.owl#CONTROL-FEATURE-TYPE"/>
    <rdfs:label xml:lang="en">incident point</rdfs:label>
    <rdfs:comment xml:lang="en">A CONTROL-FEATURE-TYPE that identifies a point where an incident has occurred.</rdfs:comment>
    <rdf:type rdf:resource="http://www.w3.org/2002/07/owl#Class"/>
  </rdf:Description>
  <rdf:Description rdf:about="#SURFACE-VESSEL-TYPE_Barge,_cable">
    <rdfs:subClassOf rdf:resource="jc3iedm_OBJECT-TYPE.owl#SURFACE-VESSEL-TYPE"/>
    <rdfs:label xml:lang="en">barge, cable</rdfs:label>
    <rdfs:comment xml:lang="en">Craft used to carry cables for laying.</rdfs:comment>
    <rdf:type rdf:resource="http://www.w3.org/2002/07/owl#Class"/>
  </rdf:Description>
  <rdf:Description rdf:about="#MILITARY-POST-TYPE_Authorised_commander">
    <rdfs:subClassOf rdf:resource="jc3iedm_OBJECT-TYPE.owl#MILITARY-POST-TYPE"/>
    <rdfs:label xml:lang="en">authorised commander</rdfs:label>
    <rdfs:comment xml:lang="en">A MILITARY-POST-TYPE that is identified as the duly appointed officer in charge of a unit, post, camp, or operation.</rdfs:comment>
    <rdf:type rdf:resource="http://www.w3.org/2002/07/owl#Class"/>
  </rdf:Description>
  <rdf:Description rdf:about="#SURFACE-VESSEL-TYPE_Torpedo_boat,_training">
    <rdfs:subClassOf rdf:resource="jc3iedm_OBJECT-TYPE.owl#SURFACE-VESSEL-TYPE"/>
    <rdfs:label xml:lang="en">torpedo boat, training</rdfs:label>
    <rdfs:comment xml:lang="en">High-speed (35 knots - 65 km/hr) anti-surface ship patrol craft in size range 20 - 30 metres fitted with torpedoes and used primarily in a training role.</rdfs:comment>
    <rdf:type rdf:resource="http://www.w3.org/2002/07/owl#Class"/>
  </rdf:Description>
  <rdf:Description rdf:about="#MILITARY-POST-TYPE_Rifleman">
    <rdfs:subClassOf rdf:resource="jc3iedm_OBJECT-TYPE.owl#MILITARY-POST-TYPE"/>
    <rdfs:label xml:lang="en">rifleman</rdfs:label>
    <rdfs:comment xml:lang="en">A MILITARY-POST-TYPE that is identified as a soldier armed with a rifle.</rdfs:comment>
    <rdf:type rdf:resource="http://www.w3.org/2002/07/owl#Class"/>
  </rdf:Description>
  <rdf:Description rdf:about="#SURFACE-VESSEL-TYPE_Radiological_liquid_ship">
    <rdfs:subClassOf rdf:resource="jc3iedm_OBJECT-TYPE.owl#SURFACE-VESSEL-TYPE"/>
    <rdfs:label xml:lang="en">radiological liquid ship</rdfs:label>
    <rdfs:comment xml:lang="en">Ship 40 metres or more designed to transport radioactive liquids.</rdfs:comment>
    <rdf:type rdf:resource="http://www.w3.org/2002/07/owl#Class"/>
  </rdf:Description>
  <rdf:Description rdf:about="#CONTROL-FEATURE-TYPE_Amphibious_defence_zone">
    <rdfs:subClassOf rdf:resource="jc3iedm_OBJECT-TYPE.owl#CONTROL-FEATURE-TYPE"/>
    <rdfs:label xml:lang="en">amphibious defence zone</rdfs:label>
    <rdfs:comment xml:lang="en">Area encompassing the amphibious objective area and adjoining airspace as required for the accompanying naval force.</rdfs:comment>
    <rdf:type rdf:resource="http://www.w3.org/2002/07/owl#Class"/>
  </rdf:Description>
  <rdf:Description rdf:about="#FACILITY-TYPE_Railway_crossing">
    <rdfs:subClassOf rdf:resource="jc3iedm_OBJECT-TYPE.owl#FACILITY-TYPE"/>
    <rdfs:label xml:lang="en">railway crossing</rdfs:label>
    <rdfs:comment xml:lang="en">A predefined place at which a railway may be crossed at the same level by a road.</rdfs:comment>
    <rdf:type rdf:resource="http://www.w3.org/2002/07/owl#Class"/>
  </rdf:Description>
  <rdf:Description rdf:about="jc3iedm_OBJECT-TYPE.owl#subsurface-vessel-type-speed-cavitation-quantity">
    <rdf:type rdf:resource="http://www.w3.org/2002/07/owl#DatatypeProperty"/>
    <rdfs:domain rdf:resource="jc3iedm_OBJECT-TYPE.owl#SUBSURFACE-VESSEL-TYPE"/>
  </rdf:Description>
  <rdf:Description rdf:about="#MARITIME-EQUIPMENT-TYPE_Paravane">
    <rdfs:subClassOf rdf:resource="jc3iedm_OBJECT-TYPE.owl#MARITIME-EQUIPMENT-TYPE"/>
    <rdfs:label xml:lang="en">paravane</rdfs:label>
    <rdfs:comment xml:lang="en">A towed body with planes and a cutter with a means of depth keeping, which displaces itself sideways and can be used as a ship protection measure against certain moored mines.</rdfs:comment>
    <rdf:type rdf:resource="http://www.w3.org/2002/07/owl#Class"/>
  </rdf:Description>
  <rdf:Description rdf:about="#ORGANISATION-TYPE_Air_support_operations_centre">
    <rdfs:subClassOf rdf:resource="jc3iedm_OBJECT-TYPE.owl#ORGANISATION-TYPE"/>
    <rdfs:label xml:lang="en">air support operations centre</rdfs:label>
    <rdfs:comment xml:lang="en">The ORGANISATION-TYPE of a tactical air control system collocated with a corps headquarters or an appropriate land force headquarters, which coordinates and directs close air support and other tactical air support.</rdfs:comment>
    <rdf:type rdf:resource="http://www.w3.org/2002/07/owl#Class"/>
  </rdf:Description>
  <rdf:Description rdf:about="#FACILITY-TYPE_Prisoner_of_war_collection_point">
    <rdfs:subClassOf rdf:resource="jc3iedm_OBJECT-TYPE.owl#FACILITY-TYPE"/>
    <rdfs:label xml:lang="en">prisoner of war collection point</rdfs:label>
    <rdfs:comment xml:lang="en">A facility where Prisoners of war are assembled for classification, sorting or further movement to other facilities or installations.</rdfs:comment>
    <rdf:type rdf:resource="http://www.w3.org/2002/07/owl#Class"/>
  </rdf:Description>
  <rdf:Description rdf:about="jc3iedm_OBJECT-TYPE.owl#consumable-materiel-type-issuing-count">
    <rdf:type rdf:resource="http://www.w3.org/2002/07/owl#DatatypeProperty"/>
    <rdfs:domain rdf:resource="jc3iedm_OBJECT-TYPE.owl#CONSUMABLE-MATERIEL-TYPE"/>
  </rdf:Description>
  <rdf:Description rdf:about="jc3iedm_OBJECT-TYPE.owl#aircraft-type-load-category-code">
    <rdf:type rdf:resource="http://www.w3.org/2002/07/owl#DatatypeProperty"/>
    <rdfs:domain rdf:resource="jc3iedm_OBJECT-TYPE.owl#AIRCRAFT-TYPE"/>
    <rdfs:range rdf:resource="http://www.w3.org/2001/XMLSchema#string"/>
  </rdf:Description>
  <rdf:Description rdf:about="#ORGANISATION-TYPE_Coordination_centre">
    <rdfs:subClassOf rdf:resource="jc3iedm_OBJECT-TYPE.owl#ORGANISATION-TYPE"/>
    <rdfs:label xml:lang="en">coordination centre</rdfs:label>
    <rdfs:comment xml:lang="en">The ORGANISATION-TYPE is a coordination centre.</rdfs:comment>
    <rdf:type rdf:resource="http://www.w3.org/2002/07/owl#Class"/>
  </rdf:Description>
  <rdf:Description rdf:about="#CONSUMABLE-MATERIEL-TYPE_Fuse">
    <rdfs:subClassOf rdf:resource="jc3iedm_OBJECT-TYPE.owl#CONSUMABLE-MATERIEL-TYPE"/>
    <rdfs:label xml:lang="en">fuse</rdfs:label>
    <rdfs:comment xml:lang="en">A device that initiates an explosive train.</rdfs:comment>
    <rdf:type rdf:resource="http://www.w3.org/2002/07/owl#Class"/>
  </rdf:Description>
  <rdf:Description rdf:about="#SURFACE-VESSEL-TYPE_Water_tender_(naval)">
    <rdfs:subClassOf rdf:resource="jc3iedm_OBJECT-TYPE.owl#SURFACE-VESSEL-TYPE"/>
    <rdfs:label xml:lang="en">water tender (naval)</rdfs:label>
    <rdfs:comment xml:lang="en">Ship used primarily for transporting potable water.</rdfs:comment>
    <rdf:type rdf:resource="http://www.w3.org/2002/07/owl#Class"/>
  </rdf:Description>
  <rdf:Description rdf:about="jc3iedm_OBJECT-TYPE.owl#railcar-type-category-code">
    <rdf:type rdf:resource="http://www.w3.org/2002/07/owl#DatatypeProperty"/>
    <rdfs:domain rdf:resource="jc3iedm_OBJECT-TYPE.owl#RAILCAR-TYPE"/>
    <rdfs:range rdf:resource="http://www.w3.org/2001/XMLSchema#string"/>
  </rdf:Description>
  <rdf:Description rdf:about="#CONTROL-FEATURE-TYPE_Coordination_fire_line">
    <rdfs:subClassOf rdf:resource="jc3iedm_OBJECT-TYPE.owl#CONTROL-FEATURE-TYPE"/>
    <rdfs:label xml:lang="en">coordination fire line</rdfs:label>
    <rdfs:comment xml:lang="en">A line beyond which conventional surface fire support may fire at any time within the area of operations of the establishing headquarters without additional coordination. NOTE Also known as Coordinated fire line.</rdfs:comment>
    <rdf:type rdf:resource="http://www.w3.org/2002/07/owl#Class"/>
  </rdf:Description>
  <rdf:Description rdf:about="#FACILITY-TYPE_Shed">
    <rdfs:subClassOf rdf:resource="jc3iedm_OBJECT-TYPE.owl#FACILITY-TYPE"/>
    <rdfs:label xml:lang="en">shed</rdfs:label>
    <rdfs:comment xml:lang="en">A storage facility usually characterised by one or more open sides, support pillars and a roof.</rdfs:comment>
    <rdf:type rdf:resource="http://www.w3.org/2002/07/owl#Class"/>
  </rdf:Description>
  <rdf:Description rdf:about="#SURFACE-VESSEL-TYPE_Merchant_ship,_general">
    <rdfs:subClassOf rdf:resource="jc3iedm_OBJECT-TYPE.owl#SURFACE-VESSEL-TYPE"/>
    <rdfs:label xml:lang="en">merchant ship, general</rdfs:label>
    <rdfs:comment xml:lang="en">General designator for non-naval ship designed to transport cargo or passengers.</rdfs:comment>
    <rdf:type rdf:resource="http://www.w3.org/2002/07/owl#Class"/>
  </rdf:Description>
  <rdf:Description rdf:about="#SURFACE-VESSEL-TYPE_Special_warfare_craft,_light">
    <rdfs:subClassOf rdf:resource="jc3iedm_OBJECT-TYPE.owl#SURFACE-VESSEL-TYPE"/>
    <rdfs:label xml:lang="en">special warfare craft, light</rdfs:label>
    <rdfs:comment xml:lang="en">A light craft specifically designed for special warfare operations.</rdfs:comment>
    <rdf:type rdf:resource="http://www.w3.org/2002/07/owl#Class"/>
  </rdf:Description>
  <rdf:Description rdf:about="#CONTROL-FEATURE-TYPE_Engineer_regulating_point">
    <rdfs:subClassOf rdf:resource="jc3iedm_OBJECT-TYPE.owl#CONTROL-FEATURE-TYPE"/>
    <rdfs:label xml:lang="en">engineer regulating point</rdfs:label>
    <rdfs:comment xml:lang="en">Checkpoint to ensure that vehicles do not exceed the capacity of the crossing means and to give drivers final instructions on site-specific procedures and information, such as speed and vehicle interval.</rdfs:comment>
    <rdf:type rdf:resource="http://www.w3.org/2002/07/owl#Class"/>
  </rdf:Description>
  <rdf:Description rdf:about="#WEAPON-TYPE_Air-defence">
    <rdfs:subClassOf rdf:resource="jc3iedm_OBJECT-TYPE.owl#WEAPON-TYPE"/>
    <rdfs:label xml:lang="en">air defence</rdfs:label>
    <rdfs:comment xml:lang="en">A weapon specifically designed for the engagement of aircraft.</rdfs:comment>
    <rdf:type rdf:resource="http://www.w3.org/2002/07/owl#Class"/>
  </rdf:Description>
  <rdf:Description rdf:about="#RADIOACTIVE-MATERIEL-TYPE_Spent_reactor_fuel">
    <rdfs:subClassOf rdf:resource="jc3iedm_OBJECT-TYPE.owl#RADIOACTIVE-MATERIEL-TYPE"/>
    <rdfs:label xml:lang="en">spent reactor fuel</rdfs:label>
    <rdfs:comment xml:lang="en">Nuclear reactor fuel that has been used in a live nuclear reactor.</rdfs:comment>
    <rdf:type rdf:resource="http://www.w3.org/2002/07/owl#Class"/>
  </rdf:Description>
  <rdf:Description rdf:about="#SURFACE-VESSEL-TYPE_Destroyer,_escort">
    <rdfs:subClassOf rdf:resource="jc3iedm_OBJECT-TYPE.owl#SURFACE-VESSEL-TYPE"/>
    <rdfs:label xml:lang="en">destroyer, escort</rdfs:label>
    <rdfs:comment xml:lang="en">A destroyer type ship optimised for escort duties. Major surface combatant in range of about 95 to 140 metres whole general mission is to conduct operations with strike, ASW and amphibious forces, and to perform screening and convoy duties. May have helicopters not especially fitted for ASW.</rdfs:comment>
    <rdf:type rdf:resource="http://www.w3.org/2002/07/owl#Class"/>
  </rdf:Description>
  <rdf:Description rdf:about="jc3iedm_OBJECT-TYPE.owl#aircraft-type-design-range-code">
    <rdf:type rdf:resource="http://www.w3.org/2002/07/owl#DatatypeProperty"/>
    <rdfs:domain rdf:resource="jc3iedm_OBJECT-TYPE.owl#AIRCRAFT-TYPE"/>
    <rdfs:range rdf:resource="http://www.w3.org/2001/XMLSchema#string"/>
  </rdf:Description>
  <rdf:Description rdf:about="#GROUP-ORGANISATION-TYPE_Not_otherwise_specified">
    <rdfs:subClassOf rdf:resource="jc3iedm_OBJECT-TYPE.owl#GROUP-ORGANISATION-TYPE"/>
    <rdfs:label xml:lang="en">not otherwise specified</rdfs:label>
    <rdfs:comment xml:lang="en">The appropriate value is not in the set of specified values.</rdfs:comment>
    <rdf:type rdf:resource="http://www.w3.org/2002/07/owl#Class"/>
  </rdf:Description>
  <rdf:Description rdf:about="#CONTROL-FEATURE-TYPE_Entry_gate">
    <rdfs:subClassOf rdf:resource="jc3iedm_OBJECT-TYPE.owl#CONTROL-FEATURE-TYPE"/>
    <rdfs:label xml:lang="en">entry gate</rdfs:label>
    <rdfs:comment xml:lang="en">The point to which an aircraft will be directed to commence the transit inbound from an airfield or force at sea.</rdfs:comment>
    <rdf:type rdf:resource="http://www.w3.org/2002/07/owl#Class"/>
  </rdf:Description>
  <rdf:Description rdf:about="#SURFACE-VESSEL-TYPE_Landing_craft,_vehicle_personnel">
    <rdfs:subClassOf rdf:resource="jc3iedm_OBJECT-TYPE.owl#SURFACE-VESSEL-TYPE"/>
    <rdfs:label xml:lang="en">landing craft, vehicle personnel</rdfs:label>
    <rdfs:comment xml:lang="en">Landing craft in size range 7.5-30 metres capable of carrying a light vehicle in place of troops. Must have bow ramp.</rdfs:comment>
    <rdf:type rdf:resource="http://www.w3.org/2002/07/owl#Class"/>
  </rdf:Description>
  <rdf:Description rdf:about="#ENGINEERING-EQUIPMENT-TYPE_Mine-laying">
    <rdfs:subClassOf rdf:resource="jc3iedm_OBJECT-TYPE.owl#ENGINEERING-EQUIPMENT-TYPE"/>
    <rdfs:label xml:lang="en">mine laying</rdfs:label>
    <rdfs:comment xml:lang="en">An equipment whose purpose is to lay mines.</rdfs:comment>
    <rdf:type rdf:resource="http://www.w3.org/2002/07/owl#Class"/>
  </rdf:Description>
  <rdf:Description rdf:about="#CONTROL-FEATURE-TYPE_Check_point,_general">
    <rdfs:subClassOf rdf:resource="jc3iedm_OBJECT-TYPE.owl#CONTROL-FEATURE-TYPE"/>
    <rdfs:label xml:lang="en">check point, general</rdfs:label>
    <rdfs:comment xml:lang="en">A CONTROL-FEATURE-TYPE used as a means of controlling movement, a registration target for fire adjustment, or reference for location.</rdfs:comment>
    <rdf:type rdf:resource="http://www.w3.org/2002/07/owl#Class"/>
  </rdf:Description>
  <rdf:Description rdf:about="#FACILITY-TYPE_Mining_installation,_open_sky">
    <rdfs:subClassOf rdf:resource="jc3iedm_OBJECT-TYPE.owl#FACILITY-TYPE"/>
    <rdfs:label xml:lang="en">mining installation, open sky</rdfs:label>
    <rdfs:comment xml:lang="en">A facility where materials are extracted from the ground directly, without using tunnels.</rdfs:comment>
    <rdf:type rdf:resource="http://www.w3.org/2002/07/owl#Class"/>
  </rdf:Description>
  <rdf:Description rdf:about="#ENGINEERING-EQUIPMENT-TYPE_Not_otherwise_specified">
    <rdfs:subClassOf rdf:resource="jc3iedm_OBJECT-TYPE.owl#ENGINEERING-EQUIPMENT-TYPE"/>
    <rdfs:label xml:lang="en">not otherwise specified</rdfs:label>
    <rdfs:comment xml:lang="en">The appropriate value is not in the set of specified values.</rdfs:comment>
    <rdf:type rdf:resource="http://www.w3.org/2002/07/owl#Class"/>
  </rdf:Description>
  <rdf:Description rdf:about="#RAILCAR-TYPE_Locomotive">
    <rdfs:subClassOf rdf:resource="jc3iedm_OBJECT-TYPE.owl#RAILCAR-TYPE"/>
    <rdfs:label xml:lang="en">locomotive</rdfs:label>
    <rdfs:comment xml:lang="en">A detachable, wheeled engine used for pulling trains.</rdfs:comment>
    <rdf:type rdf:resource="http://www.w3.org/2002/07/owl#Class"/>
  </rdf:Description>
  <rdf:Description rdf:about="#CIVILIAN-POST-TYPE_Governor">
    <rdfs:subClassOf rdf:resource="jc3iedm_OBJECT-TYPE.owl#CIVILIAN-POST-TYPE"/>
    <rdfs:label xml:lang="en">governor</rdfs:label>
    <rdfs:comment xml:lang="en">A CIVILIAN-POST-TYPE whose job is the executive leadership and administrative control over a group of people.</rdfs:comment>
    <rdf:type rdf:resource="http://www.w3.org/2002/07/owl#Class"/>
  </rdf:Description>
  <rdf:Description rdf:about="#MILITARY-POST-TYPE_Sniper">
    <rdfs:subClassOf rdf:resource="jc3iedm_OBJECT-TYPE.owl#MILITARY-POST-TYPE"/>
    <rdfs:label xml:lang="en">sniper</rdfs:label>
    <rdfs:comment xml:lang="en">A MILITARY-POST-TYPE that is identified as one who snipes, or shoots from concealment.</rdfs:comment>
    <rdf:type rdf:resource="http://www.w3.org/2002/07/owl#Class"/>
  </rdf:Description>
  <rdf:Description rdf:about="#SURFACE-VESSEL-TYPE_Fire_service_rescue_tender">
    <rdfs:subClassOf rdf:resource="jc3iedm_OBJECT-TYPE.owl#SURFACE-VESSEL-TYPE"/>
    <rdfs:label xml:lang="en">fire service rescue tender</rdfs:label>
    <rdfs:comment xml:lang="en">Harbour craft operated by customs fire service extensively equipped for firefighting. For this type that capability is more important than horsepower alone. Must have several fire monitors.</rdfs:comment>
    <rdf:type rdf:resource="http://www.w3.org/2002/07/owl#Class"/>
  </rdf:Description>
  <rdf:Description rdf:about="#FACILITY-TYPE_Check_point,_police">
    <rdfs:subClassOf rdf:resource="jc3iedm_OBJECT-TYPE.owl#FACILITY-TYPE"/>
    <rdfs:label xml:lang="en">check point, police</rdfs:label>
    <rdfs:comment xml:lang="en">A facility where police check vehicular or pedestrian traffic in order to enforce circulation control measures and other laws, orders, and regulations.</rdfs:comment>
    <rdf:type rdf:resource="http://www.w3.org/2002/07/owl#Class"/>
  </rdf:Description>
  <rdf:Description rdf:about="#CONTROL-FEATURE-TYPE_Amphibious_objective_area">
    <rdfs:subClassOf rdf:resource="jc3iedm_OBJECT-TYPE.owl#CONTROL-FEATURE-TYPE"/>
    <rdfs:label xml:lang="en">amphibious objective area</rdfs:label>
    <rdfs:comment xml:lang="en">Geographic area delineated for the purpose of command and control within which is located the objective(s) to be secured by the amphibious task force.</rdfs:comment>
    <rdf:type rdf:resource="http://www.w3.org/2002/07/owl#Class"/>
  </rdf:Description>
  <rdf:Description rdf:about="#FACILITY-TYPE_Site,_navigation_radar">
    <rdfs:subClassOf rdf:resource="jc3iedm_OBJECT-TYPE.owl#FACILITY-TYPE"/>
    <rdfs:label xml:lang="en">site, navigation radar</rdfs:label>
    <rdfs:comment xml:lang="en">A facility containing radar employed for navigation purposes.</rdfs:comment>
    <rdf:type rdf:resource="http://www.w3.org/2002/07/owl#Class"/>
  </rdf:Description>
  <rdf:Description rdf:about="#AIRCRAFT-TYPE_Yes">
    <rdfs:subClassOf rdf:resource="jc3iedm_OBJECT-TYPE.owl#AIRCRAFT-TYPE"/>
    <rdfs:label xml:lang="en">yes</rdfs:label>
    <rdfs:comment xml:lang="en">The AIRCRAFT-TYPE is designed to be used as a trainer.</rdfs:comment>
    <rdf:type rdf:resource="http://www.w3.org/2002/07/owl#Class"/>
  </rdf:Description>
  <rdf:Description rdf:about="#UNIT-TYPE_Military_intelligence">
    <rdfs:subClassOf rdf:resource="jc3iedm_OBJECT-TYPE.owl#UNIT-TYPE"/>
    <rdfs:label xml:lang="en">military intelligence</rdfs:label>
    <rdfs:comment xml:lang="en">A UNIT-TYPE whose principal designation is the processing of information concerning foreign nations, hostile or potentially hostile forces or elements, or areas of actual or potential operations.</rdfs:comment>
    <rdf:type rdf:resource="http://www.w3.org/2002/07/owl#Class"/>
  </rdf:Description>
  <rdf:Description rdf:about="#CONTROL-FEATURE-TYPE_Left_radial_line">
    <rdfs:subClassOf rdf:resource="jc3iedm_OBJECT-TYPE.owl#CONTROL-FEATURE-TYPE"/>
    <rdfs:label xml:lang="en">left radial line</rdfs:label>
    <rdfs:comment xml:lang="en">The line extending outward from the area of Secondary Hazard marking the maximum extent to the left (facing in the effective downwind direction) where significant fallout is expected to occur.</rdfs:comment>
    <rdf:type rdf:resource="http://www.w3.org/2002/07/owl#Class"/>
  </rdf:Description>
  <rdf:Description rdf:about="jc3iedm_OBJECT-TYPE.owl#consumable-materiel-type-united-nations-number-code">
    <rdf:type rdf:resource="http://www.w3.org/2002/07/owl#DatatypeProperty"/>
    <rdfs:domain rdf:resource="jc3iedm_OBJECT-TYPE.owl#CONSUMABLE-MATERIEL-TYPE"/>
    <rdfs:range rdf:resource="http://www.w3.org/2001/XMLSchema#string"/>
  </rdf:Description>
  <rdf:Description rdf:about="#ROUTE-TYPE_Return_to_force_route">
    <rdfs:subClassOf rdf:resource="jc3iedm_OBJECT-TYPE.owl#ROUTE-TYPE"/>
    <rdfs:label xml:lang="en">return to force route</rdfs:label>
    <rdfs:comment xml:lang="en">Planned route profiles for use by friendly aircraft returning to an aircraft-capable ship.</rdfs:comment>
    <rdf:type rdf:resource="http://www.w3.org/2002/07/owl#Class"/>
  </rdf:Description>
  <rdf:Description rdf:about="#RADIOACTIVE-MATERIEL-TYPE_Toxic_industrial_material">
    <rdfs:subClassOf rdf:resource="jc3iedm_OBJECT-TYPE.owl#RADIOACTIVE-MATERIEL-TYPE"/>
    <rdfs:label xml:lang="en">toxic industrial material</rdfs:label>
    <rdfs:comment xml:lang="en">A generic term for radioactive compounds in solid, liquid, aerosolised or gaseous form. These may be used, or stored for use, for industrial, commercial, medical, military or domestic purposes.</rdfs:comment>
    <rdf:type rdf:resource="http://www.w3.org/2002/07/owl#Class"/>
  </rdf:Description>
  <rdf:Description rdf:about="#TASK-FORMATION-TYPE_Group_(navy)">
    <rdfs:subClassOf rdf:resource="jc3iedm_OBJECT-TYPE.owl#TASK-FORMATION-TYPE"/>
    <rdfs:label xml:lang="en">group (navy)</rdfs:label>
    <rdfs:comment xml:lang="en">A TASK-FORMATION-TYPE that consists of a number of ships and/or aircraft, normally a subdivision of a force, assigned for a specific purpose.</rdfs:comment>
    <rdf:type rdf:resource="http://www.w3.org/2002/07/owl#Class"/>
  </rdf:Description>
  <rdf:Description rdf:about="#SURFACE-VESSEL-TYPE_Survey_ship">
    <rdfs:subClassOf rdf:resource="jc3iedm_OBJECT-TYPE.owl#SURFACE-VESSEL-TYPE"/>
    <rdfs:label xml:lang="en">survey ship</rdfs:label>
    <rdfs:comment xml:lang="en">Ship 40 metres or more employed to conduct hydrographic and limited oceanographic surveys.</rdfs:comment>
    <rdf:type rdf:resource="http://www.w3.org/2002/07/owl#Class"/>
  </rdf:Description>
  <rdf:Description rdf:about="#CONTROL-FEATURE-TYPE_Class-E_airspace">
    <rdfs:subClassOf rdf:resource="jc3iedm_OBJECT-TYPE.owl#CONTROL-FEATURE-TYPE"/>
    <rdfs:label xml:lang="en">class e airspace</rdfs:label>
    <rdfs:comment xml:lang="en">An airspace in which instrument flight rule flights and visual flight rule flights are permitted; all flights are subject to air traffic control service and are separated from other instrument flight rule flights. All flights receive traffic information as far as practical.</rdfs:comment>
    <rdf:type rdf:resource="http://www.w3.org/2002/07/owl#Class"/>
  </rdf:Description>
  <rdf:Description rdf:about="jc3iedm_OBJECT-TYPE.owl#ammunition-type-exercise-mine-flare-colour-code">
    <rdf:type rdf:resource="http://www.w3.org/2002/07/owl#DatatypeProperty"/>
    <rdfs:domain rdf:resource="jc3iedm_OBJECT-TYPE.owl#AMMUNITION-TYPE"/>
    <rdfs:range rdf:resource="http://www.w3.org/2001/XMLSchema#string"/>
  </rdf:Description>
  <rdf:Description rdf:about="#FACILITY-TYPE_Depot,_engineer">
    <rdfs:subClassOf rdf:resource="jc3iedm_OBJECT-TYPE.owl#FACILITY-TYPE"/>
    <rdfs:label xml:lang="en">depot, engineer</rdfs:label>
    <rdfs:comment xml:lang="en">An area used for the storage of engineer equipment.</rdfs:comment>
    <rdf:type rdf:resource="http://www.w3.org/2002/07/owl#Class"/>
  </rdf:Description>
  <rdf:Description rdf:about="#CONTROL-FEATURE-TYPE_Special_use_airspace">
    <rdfs:subClassOf rdf:resource="jc3iedm_OBJECT-TYPE.owl#CONTROL-FEATURE-TYPE"/>
    <rdfs:label xml:lang="en">special use airspace</rdfs:label>
    <rdfs:comment xml:lang="en">Airspace defined for a specific purpose; or to designate airspace in which no flight activity is organized.</rdfs:comment>
    <rdf:type rdf:resource="http://www.w3.org/2002/07/owl#Class"/>
  </rdf:Description>
  <rdf:Description rdf:about="#CONTROL-FEATURE-TYPE_Beachhead">
    <rdfs:subClassOf rdf:resource="jc3iedm_OBJECT-TYPE.owl#CONTROL-FEATURE-TYPE"/>
    <rdfs:label xml:lang="en">beachhead</rdfs:label>
    <rdfs:comment xml:lang="en">A designated area on a hostile or potentially hostile shore that, when seized and held, ensures the continuous landing of troops and materiel, and provides manoeuvre space requisite for subsequent projected operations ashore.</rdfs:comment>
    <rdf:type rdf:resource="http://www.w3.org/2002/07/owl#Class"/>
  </rdf:Description>
  <rdf:Description rdf:about="#CONTROL-FEATURE-TYPE_Waiting_area">
    <rdfs:subClassOf rdf:resource="jc3iedm_OBJECT-TYPE.owl#CONTROL-FEATURE-TYPE"/>
    <rdfs:label xml:lang="en">waiting area</rdfs:label>
    <rdfs:comment xml:lang="en">A location adjacent to the route or axis that may be used for the concealment of vehicles, troops, and equipment while an element is waiting to resume movement. Waiting areas are normally located on both banks close to crossing areas.</rdfs:comment>
    <rdf:type rdf:resource="http://www.w3.org/2002/07/owl#Class"/>
  </rdf:Description>
  <rdf:Description rdf:about="#SURFACE-VESSEL-TYPE_Patrol_craft,_hydrofoil">
    <rdfs:subClassOf rdf:resource="jc3iedm_OBJECT-TYPE.owl#SURFACE-VESSEL-TYPE"/>
    <rdfs:label xml:lang="en">patrol craft, hydrofoil</rdfs:label>
    <rdfs:comment xml:lang="en">Vessel in size range 35-55 metres designed and fitted primarily for escort duties in ASW role and is fitted with hydrofoils.</rdfs:comment>
    <rdf:type rdf:resource="http://www.w3.org/2002/07/owl#Class"/>
  </rdf:Description>
  <rdf:Description rdf:about="#CONTROL-FEATURE-TYPE_Airspace_control_subarea/sector">
    <rdfs:subClassOf rdf:resource="jc3iedm_OBJECT-TYPE.owl#CONTROL-FEATURE-TYPE"/>
    <rdfs:label xml:lang="en">airspace control subarea/sector</rdfs:label>
    <rdfs:comment xml:lang="en">Sub-element of an airspace control area, established to facilitate the control of the overall area.</rdfs:comment>
    <rdf:type rdf:resource="http://www.w3.org/2002/07/owl#Class"/>
  </rdf:Description>
  <rdf:Description rdf:about="#UNIT-TYPE_Combat_support">
    <rdfs:subClassOf rdf:resource="jc3iedm_OBJECT-TYPE.owl#UNIT-TYPE"/>
    <rdfs:label xml:lang="en">combat support</rdfs:label>
    <rdfs:comment xml:lang="en">A UNIT-TYPE that provides critical combat functions in conjunction with combat arms units and soldiers.</rdfs:comment>
    <rdf:type rdf:resource="http://www.w3.org/2002/07/owl#Class"/>
  </rdf:Description>
  <rdf:Description rdf:about="#MARITIME-EQUIPMENT-TYPE_Not_otherwise_specified">
    <rdfs:subClassOf rdf:resource="jc3iedm_OBJECT-TYPE.owl#MARITIME-EQUIPMENT-TYPE"/>
    <rdfs:label xml:lang="en">not otherwise specified</rdfs:label>
    <rdfs:comment xml:lang="en">The appropriate value is not in the set of specified values.</rdfs:comment>
    <rdf:type rdf:resource="http://www.w3.org/2002/07/owl#Class"/>
  </rdf:Description>
  <rdf:Description rdf:about="#CONTROL-FEATURE-TYPE_Concentration_area">
    <rdfs:subClassOf rdf:resource="jc3iedm_OBJECT-TYPE.owl#CONTROL-FEATURE-TYPE"/>
    <rdfs:label xml:lang="en">concentration area</rdfs:label>
    <rdfs:comment xml:lang="en">An area, usually in the theatre of operations, where troops are assembled before beginning active operations.</rdfs:comment>
    <rdf:type rdf:resource="http://www.w3.org/2002/07/owl#Class"/>
  </rdf:Description>
  <rdf:Description rdf:about="jc3iedm_OBJECT-TYPE.owl#group-organisation-type-category-code">
    <rdf:type rdf:resource="http://www.w3.org/2002/07/owl#DatatypeProperty"/>
    <rdfs:domain rdf:resource="jc3iedm_OBJECT-TYPE.owl#GROUP-ORGANISATION-TYPE"/>
    <rdfs:range rdf:resource="http://www.w3.org/2001/XMLSchema#string"/>
  </rdf:Description>
  <rdf:Description rdf:about="#ELECTRONIC-EQUIPMENT-TYPE_Navigational_aid">
    <rdfs:subClassOf rdf:resource="jc3iedm_OBJECT-TYPE.owl#ELECTRONIC-EQUIPMENT-TYPE"/>
    <rdfs:label xml:lang="en">navigational aid</rdfs:label>
    <rdfs:comment xml:lang="en">Any electronic device which provides point-to-point guidance information or position data.</rdfs:comment>
    <rdf:type rdf:resource="http://www.w3.org/2002/07/owl#Class"/>
  </rdf:Description>
  <rdf:Description rdf:about="#FACILITY-TYPE_Sensor_fusion_post">
    <rdfs:subClassOf rdf:resource="jc3iedm_OBJECT-TYPE.owl#FACILITY-TYPE"/>
    <rdfs:label xml:lang="en">sensor fusion post</rdfs:label>
    <rdfs:comment xml:lang="en">No definition provided in ADatP-3 Baseline 13.1 FFIRN/FUD 1874/4.</rdfs:comment>
    <rdf:type rdf:resource="http://www.w3.org/2002/07/owl#Class"/>
  </rdf:Description>
  <rdf:Description rdf:about="#CONTROL-FEATURE-TYPE_Class-A_airspace">
    <rdfs:subClassOf rdf:resource="jc3iedm_OBJECT-TYPE.owl#CONTROL-FEATURE-TYPE"/>
    <rdfs:label xml:lang="en">class a airspace</rdfs:label>
    <rdfs:comment xml:lang="en">An airspace in which only instrument flight rule flights are permitted; all flights are subject to air traffic control service and are separated from each other.</rdfs:comment>
    <rdf:type rdf:resource="http://www.w3.org/2002/07/owl#Class"/>
  </rdf:Description>
  <rdf:Description rdf:about="#AIRCRAFT-TYPE_Fixed_wing">
    <rdfs:subClassOf rdf:resource="jc3iedm_OBJECT-TYPE.owl#AIRCRAFT-TYPE"/>
    <rdfs:label xml:lang="en">fixed wing</rdfs:label>
    <rdfs:comment xml:lang="en">A machine or device capable of atmospheric flight and dependent on wings for lift.</rdfs:comment>
    <rdf:type rdf:resource="http://www.w3.org/2002/07/owl#Class"/>
  </rdf:Description>
  <rdf:Description rdf:about="#MILITARY-POST-TYPE_Intelligence_officer">
    <rdfs:subClassOf rdf:resource="jc3iedm_OBJECT-TYPE.owl#MILITARY-POST-TYPE"/>
    <rdfs:label xml:lang="en">intelligence officer</rdfs:label>
    <rdfs:comment xml:lang="en">A MILITARY-POST-TYPE that is identified as the officer who is responsible for activities relating to gathering and analysing information about an actual or potential foe.</rdfs:comment>
    <rdf:type rdf:resource="http://www.w3.org/2002/07/owl#Class"/>
  </rdf:Description>
  <rdf:Description rdf:about="#SURFACE-VESSEL-TYPE_Combat_stores_ship_(naval)">
    <rdfs:subClassOf rdf:resource="jc3iedm_OBJECT-TYPE.owl#SURFACE-VESSEL-TYPE"/>
    <rdfs:label xml:lang="en">combat stores ship (naval)</rdfs:label>
    <rdfs:comment xml:lang="en">Large ship, usually over 165 metres capable of underway alongside replenishment of ships with refrigerated and dry provisions, technical spares, ammunition, and general stores. May carry POL but main emphasis is on mixed replenishment.</rdfs:comment>
    <rdf:type rdf:resource="http://www.w3.org/2002/07/owl#Class"/>
  </rdf:Description>
  <rdf:Description rdf:about="#HARBOUR-TYPE_Canal_or_lake">
    <rdfs:subClassOf rdf:resource="jc3iedm_OBJECT-TYPE.owl#HARBOUR-TYPE"/>
    <rdfs:label xml:lang="en">canal or lake</rdfs:label>
    <rdfs:comment xml:lang="en">A harbour located in the interior portion of a canal or lake that is connected with the sea by a navigable waterway.</rdfs:comment>
    <rdf:type rdf:resource="http://www.w3.org/2002/07/owl#Class"/>
  </rdf:Description>
  <rdf:Description rdf:about="#RAILCAR-TYPE_Train">
    <rdfs:subClassOf rdf:resource="jc3iedm_OBJECT-TYPE.owl#RAILCAR-TYPE"/>
    <rdfs:label xml:lang="en">train</rdfs:label>
    <rdfs:comment xml:lang="en">A self-propelled passenger carrying vehicle that runs on rails.</rdfs:comment>
    <rdf:type rdf:resource="http://www.w3.org/2002/07/owl#Class"/>
  </rdf:Description>
  <rdf:Description rdf:about="#VEHICLE-TYPE_Heavy_equipment_transport">
    <rdfs:subClassOf rdf:resource="jc3iedm_OBJECT-TYPE.owl#VEHICLE-TYPE"/>
    <rdfs:label xml:lang="en">heavy equipment transport</rdfs:label>
    <rdfs:comment xml:lang="en">A vehicle designed to carry cumbersome or heavy items.</rdfs:comment>
    <rdf:type rdf:resource="http://www.w3.org/2002/07/owl#Class"/>
  </rdf:Description>
  <rdf:Description rdf:about="#CONTROL-FEATURE-TYPE_No_fly_zone">
    <rdfs:subClassOf rdf:resource="jc3iedm_OBJECT-TYPE.owl#CONTROL-FEATURE-TYPE"/>
    <rdfs:label xml:lang="en">no fly zone</rdfs:label>
    <rdfs:comment xml:lang="en">Airspace of specific dimensions set aside for a specific purpose in which no aircraft operations are permitted, except as authorized by the appropriate commander and controlling agency.</rdfs:comment>
    <rdf:type rdf:resource="http://www.w3.org/2002/07/owl#Class"/>
  </rdf:Description>
  <rdf:Description rdf:about="#MISCELLANEOUS-EQUIPMENT-TYPE_Printing_machine">
    <rdfs:subClassOf rdf:resource="jc3iedm_OBJECT-TYPE.owl#MISCELLANEOUS-EQUIPMENT-TYPE"/>
    <rdfs:label xml:lang="en">printing machine</rdfs:label>
    <rdfs:comment xml:lang="en">A machine capable of printing documents</rdfs:comment>
    <rdf:type rdf:resource="http://www.w3.org/2002/07/owl#Class"/>
  </rdf:Description>
  <rdf:Description rdf:about="#FACILITY-TYPE_Electronic_installation">
    <rdfs:subClassOf rdf:resource="jc3iedm_OBJECT-TYPE.owl#FACILITY-TYPE"/>
    <rdfs:label xml:lang="en">electronic installation</rdfs:label>
    <rdfs:comment xml:lang="en">A facility whose essential function is based on the use of electronic equipment.</rdfs:comment>
    <rdf:type rdf:resource="http://www.w3.org/2002/07/owl#Class"/>
  </rdf:Description>
  <rdf:Description rdf:about="jc3iedm_OBJECT-TYPE.owl#consumable-materiel-type-issuing-element-code">
    <rdf:type rdf:resource="http://www.w3.org/2002/07/owl#DatatypeProperty"/>
    <rdfs:domain rdf:resource="jc3iedm_OBJECT-TYPE.owl#CONSUMABLE-MATERIEL-TYPE"/>
    <rdfs:range rdf:resource="http://www.w3.org/2001/XMLSchema#string"/>
  </rdf:Description>
  <rdf:Description rdf:about="#GROUP-ORGANISATION-TYPE_Civilian-convoy-type">
    <rdfs:subClassOf rdf:resource="jc3iedm_OBJECT-TYPE.owl#GROUP-ORGANISATION-TYPE"/>
    <rdfs:label xml:lang="en">civilian convoy type</rdfs:label>
    <rdfs:comment xml:lang="en">A class of civilian convoys.</rdfs:comment>
    <rdf:type rdf:resource="http://www.w3.org/2002/07/owl#Class"/>
  </rdf:Description>
  <rdf:Description rdf:about="#BIOLOGICAL-MATERIEL-TYPE_Toxin">
    <rdfs:subClassOf rdf:resource="jc3iedm_OBJECT-TYPE.owl#BIOLOGICAL-MATERIEL-TYPE"/>
    <rdfs:label xml:lang="en">toxin</rdfs:label>
    <rdfs:comment xml:lang="en">A generic term for a BIOLOGICAL-MATERIEL-TYPE that is a micro-organism product that causes disease in man, plants or animals or causes the deterioration of materiel.</rdfs:comment>
    <rdf:type rdf:resource="http://www.w3.org/2002/07/owl#Class"/>
  </rdf:Description>
  <rdf:Description rdf:about="#CONTROL-FEATURE-TYPE_Control_area">
    <rdfs:subClassOf rdf:resource="jc3iedm_OBJECT-TYPE.owl#CONTROL-FEATURE-TYPE"/>
    <rdfs:label xml:lang="en">control area</rdfs:label>
    <rdfs:comment xml:lang="en">A controlled airspace extending upwards from a specified limit above the earth.</rdfs:comment>
    <rdf:type rdf:resource="http://www.w3.org/2002/07/owl#Class"/>
  </rdf:Description>
  <rdf:Description rdf:about="#CONTROL-FEATURE-TYPE_Intermediate_objective">
    <rdfs:subClassOf rdf:resource="jc3iedm_OBJECT-TYPE.owl#CONTROL-FEATURE-TYPE"/>
    <rdfs:label xml:lang="en">intermediate objective</rdfs:label>
    <rdfs:comment xml:lang="en">An area or feature between the line of departure and an objective that must be seized and/or held.</rdfs:comment>
    <rdf:type rdf:resource="http://www.w3.org/2002/07/owl#Class"/>
  </rdf:Description>
  <rdf:Description rdf:about="#SURFACE-VESSEL-TYPE_Tug,_harbour">
    <rdfs:subClassOf rdf:resource="jc3iedm_OBJECT-TYPE.owl#SURFACE-VESSEL-TYPE"/>
    <rdfs:label xml:lang="en">tug, harbour</rdfs:label>
    <rdfs:comment xml:lang="en">General designator for craft capable of towing naval ships in sheltered or protected seas.</rdfs:comment>
    <rdf:type rdf:resource="http://www.w3.org/2002/07/owl#Class"/>
  </rdf:Description>
  <rdf:Description rdf:about="#ORGANISATION-TYPE_Air_operations_centre">
    <rdfs:subClassOf rdf:resource="jc3iedm_OBJECT-TYPE.owl#ORGANISATION-TYPE"/>
    <rdfs:label xml:lang="en">air operations centre</rdfs:label>
    <rdfs:comment xml:lang="en">The ORGANISATION-TYPE from which aircraft and air warning functions of combat air operations are directed, controlled, and executed. It is the senior agency of the air force component commander from which command and control of air operations are coordinated with other components and services.</rdfs:comment>
    <rdf:type rdf:resource="http://www.w3.org/2002/07/owl#Class"/>
  </rdf:Description>
  <rdf:Description rdf:about="#SURFACE-VESSEL-TYPE_Floating_power_barge">
    <rdfs:subClassOf rdf:resource="jc3iedm_OBJECT-TYPE.owl#SURFACE-VESSEL-TYPE"/>
    <rdfs:label xml:lang="en">floating power barge</rdfs:label>
    <rdfs:comment xml:lang="en">Craft capable of providing auxiliary power.</rdfs:comment>
    <rdf:type rdf:resource="http://www.w3.org/2002/07/owl#Class"/>
  </rdf:Description>
  <rdf:Description rdf:about="#HARBOUR-TYPE_River_(Tide_Gates)">
    <rdfs:subClassOf rdf:resource="jc3iedm_OBJECT-TYPE.owl#HARBOUR-TYPE"/>
    <rdfs:label xml:lang="en">river (tide gates)</rdfs:label>
    <rdfs:comment xml:lang="en">A river harbour, the waters of which are constrained by locks or other mechanical devices in order to provide sufficient water to float vessels at all stages of the tide.</rdfs:comment>
    <rdf:type rdf:resource="http://www.w3.org/2002/07/owl#Class"/>
  </rdf:Description>
  <rdf:Description rdf:about="#FACILITY-TYPE_Bunker">
    <rdfs:subClassOf rdf:resource="jc3iedm_OBJECT-TYPE.owl#FACILITY-TYPE"/>
    <rdfs:label xml:lang="en">bunker</rdfs:label>
    <rdfs:comment xml:lang="en">A fortified chamber, mostly below ground, often built with reinforced concrete and provided with embrasures.</rdfs:comment>
    <rdf:type rdf:resource="http://www.w3.org/2002/07/owl#Class"/>
  </rdf:Description>
  <rdf:Description rdf:about="jc3iedm_OBJECT-TYPE.owl#aircraft-type-main-purpose-code">
    <rdf:type rdf:resource="http://www.w3.org/2002/07/owl#DatatypeProperty"/>
    <rdfs:domain rdf:resource="jc3iedm_OBJECT-TYPE.owl#AIRCRAFT-TYPE"/>
    <rdfs:range rdf:resource="http://www.w3.org/2001/XMLSchema#string"/>
  </rdf:Description>
  <rdf:Description rdf:about="#SURFACE-VESSEL-TYPE_Space_vehicle_recovery_ship">
    <rdfs:subClassOf rdf:resource="jc3iedm_OBJECT-TYPE.owl#SURFACE-VESSEL-TYPE"/>
    <rdfs:label xml:lang="en">space vehicle recovery ship</rdfs:label>
    <rdfs:comment xml:lang="en">Any ship equipped to recover space capsules following space flights.</rdfs:comment>
    <rdf:type rdf:resource="http://www.w3.org/2002/07/owl#Class"/>
  </rdf:Description>
  <rdf:Description rdf:about="jc3iedm_OBJECT-TYPE.owl#military-organisation-type-category-code">
    <rdf:type rdf:resource="http://www.w3.org/2002/07/owl#DatatypeProperty"/>
    <rdfs:domain rdf:resource="jc3iedm_OBJECT-TYPE.owl#MILITARY-ORGANISATION-TYPE"/>
    <rdfs:range rdf:resource="http://www.w3.org/2001/XMLSchema#string"/>
  </rdf:Description>
  <rdf:Description rdf:about="#SURFACE-VESSEL-TYPE_Minesweeper,_coastal,_air_cushion">
    <rdfs:subClassOf rdf:resource="jc3iedm_OBJECT-TYPE.owl#SURFACE-VESSEL-TYPE"/>
    <rdfs:label xml:lang="en">minesweeper, coastal, air cushion</rdfs:label>
    <rdfs:comment xml:lang="en">Non-magnetic minesweeper between 40-70 metres with an air cushion or surface effect design.</rdfs:comment>
    <rdf:type rdf:resource="http://www.w3.org/2002/07/owl#Class"/>
  </rdf:Description>
  <rdf:Description rdf:about="#VEHICLE-TYPE_Ambulance">
    <rdfs:subClassOf rdf:resource="jc3iedm_OBJECT-TYPE.owl#VEHICLE-TYPE"/>
    <rdfs:label xml:lang="en">ambulance</rdfs:label>
    <rdfs:comment xml:lang="en">A vehicle for conveying sick, wounded, incapacitated, or injured persons.</rdfs:comment>
    <rdf:type rdf:resource="http://www.w3.org/2002/07/owl#Class"/>
  </rdf:Description>
  <rdf:Description rdf:about="jc3iedm_OBJECT-TYPE.owl#railcar-type-subcategory-code">
    <rdf:type rdf:resource="http://www.w3.org/2002/07/owl#DatatypeProperty"/>
    <rdfs:domain rdf:resource="jc3iedm_OBJECT-TYPE.owl#RAILCAR-TYPE"/>
    <rdfs:range rdf:resource="http://www.w3.org/2001/XMLSchema#string"/>
  </rdf:Description>
  <rdf:Description rdf:about="#CONTROL-FEATURE-TYPE_Bearing_line">
    <rdfs:subClassOf rdf:resource="jc3iedm_OBJECT-TYPE.owl#CONTROL-FEATURE-TYPE"/>
    <rdfs:label xml:lang="en">bearing line</rdfs:label>
    <rdfs:comment xml:lang="en">A CONTROL-FEATURE-TYPE that is the angle and direction from which electronic, acoustic, or optical contact is made.</rdfs:comment>
    <rdf:type rdf:resource="http://www.w3.org/2002/07/owl#Class"/>
  </rdf:Description>
  <rdf:Description rdf:about="#ROUTE-TYPE_Ingress_route">
    <rdfs:subClassOf rdf:resource="jc3iedm_OBJECT-TYPE.owl#ROUTE-TYPE"/>
    <rdfs:label xml:lang="en">ingress route</rdfs:label>
    <rdfs:comment xml:lang="en">An inbound route to a specific area or target.</rdfs:comment>
    <rdf:type rdf:resource="http://www.w3.org/2002/07/owl#Class"/>
  </rdf:Description>
  <rdf:Description rdf:about="#CONTROL-FEATURE-TYPE_Forward_edge_of_the_battle_area">
    <rdfs:subClassOf rdf:resource="jc3iedm_OBJECT-TYPE.owl#CONTROL-FEATURE-TYPE"/>
    <rdfs:label xml:lang="en">forward edge of the battle area</rdfs:label>
    <rdfs:comment xml:lang="en">The foremost limits of a series of areas in which ground combat units are deployed, excluding the areas in which the covering or screening forces are operating, designated to coordinate fire support, the positioning of forces, or the manoeuvre of units.</rdfs:comment>
    <rdf:type rdf:resource="http://www.w3.org/2002/07/owl#Class"/>
  </rdf:Description>
  <rdf:Description rdf:about="jc3iedm_OBJECT-TYPE.owl#government-organisation-type-category-code">
    <rdf:type rdf:resource="http://www.w3.org/2002/07/owl#DatatypeProperty"/>
    <rdfs:domain rdf:resource="jc3iedm_OBJECT-TYPE.owl#GOVERNMENT-ORGANISATION-TYPE"/>
    <rdfs:range rdf:resource="http://www.w3.org/2001/XMLSchema#string"/>
  </rdf:Description>
  <rdf:Description rdf:about="#SURFACE-VESSEL-TYPE_Merchant_ship,_training">
    <rdfs:subClassOf rdf:resource="jc3iedm_OBJECT-TYPE.owl#SURFACE-VESSEL-TYPE"/>
    <rdfs:label xml:lang="en">merchant ship, training</rdfs:label>
    <rdfs:comment xml:lang="en">Non-naval ship used primarily for training purposes.</rdfs:comment>
    <rdf:type rdf:resource="http://www.w3.org/2002/07/owl#Class"/>
  </rdf:Description>
  <rdf:Description rdf:about="#CONTROL-FEATURE-TYPE_CBRN_hazard_area">
    <rdfs:subClassOf rdf:resource="jc3iedm_OBJECT-TYPE.owl#CONTROL-FEATURE-TYPE"/>
    <rdfs:label xml:lang="en">cbrn hazard area</rdfs:label>
    <rdfs:comment xml:lang="en">A CONTROL-FEATURE-TYPE that identifies the predicted or confirmed contour of the NBC (CBRN) hazard area.</rdfs:comment>
    <rdf:type rdf:resource="http://www.w3.org/2002/07/owl#Class"/>
  </rdf:Description>
  <rdf:Description rdf:about="#FACILITY-TYPE_Refuel_on_the_move_point">
    <rdfs:subClassOf rdf:resource="jc3iedm_OBJECT-TYPE.owl#FACILITY-TYPE"/>
    <rdfs:label xml:lang="en">refuel on the move point</rdfs:label>
    <rdfs:comment xml:lang="en">A facility where vehicles receive a prescribed (timed) amount of fuel and then continue their movement.</rdfs:comment>
    <rdf:type rdf:resource="http://www.w3.org/2002/07/owl#Class"/>
  </rdf:Description>
  <rdf:Description rdf:about="#FACILITY-TYPE_Fuel_handling_point">
    <rdfs:subClassOf rdf:resource="jc3iedm_OBJECT-TYPE.owl#FACILITY-TYPE"/>
    <rdfs:label xml:lang="en">fuel handling point</rdfs:label>
    <rdfs:comment xml:lang="en">A facility for refuelling of POL products.</rdfs:comment>
    <rdf:type rdf:resource="http://www.w3.org/2002/07/owl#Class"/>
  </rdf:Description>
  <rdf:Description rdf:about="#VEHICLE-TYPE_Truck,_dump">
    <rdfs:subClassOf rdf:resource="jc3iedm_OBJECT-TYPE.owl#VEHICLE-TYPE"/>
    <rdfs:label xml:lang="en">truck, dump</rdfs:label>
    <rdfs:comment xml:lang="en">A truck having a body that tilts and opens for unloading materials</rdfs:comment>
    <rdf:type rdf:resource="http://www.w3.org/2002/07/owl#Class"/>
  </rdf:Description>
  <rdf:Description rdf:about="#TASK-FORMATION-TYPE_Flotilla">
    <rdfs:subClassOf rdf:resource="jc3iedm_OBJECT-TYPE.owl#TASK-FORMATION-TYPE"/>
    <rdfs:label xml:lang="en">flotilla</rdfs:label>
    <rdfs:comment xml:lang="en">A small fleet; a fleet of boats or small vessels.</rdfs:comment>
    <rdf:type rdf:resource="http://www.w3.org/2002/07/owl#Class"/>
  </rdf:Description>
  <rdf:Description rdf:about="#SURFACE-VESSEL-TYPE_Patrol_vessel,_general">
    <rdfs:subClassOf rdf:resource="jc3iedm_OBJECT-TYPE.owl#SURFACE-VESSEL-TYPE"/>
    <rdfs:label xml:lang="en">patrol vessel, general</rdfs:label>
    <rdfs:comment xml:lang="en">General designator for patrol vessels.</rdfs:comment>
    <rdf:type rdf:resource="http://www.w3.org/2002/07/owl#Class"/>
  </rdf:Description>
  <rdf:Description rdf:about="#SURFACE-VESSEL-TYPE_Auxiliary_floating_drydock,_small">
    <rdfs:subClassOf rdf:resource="jc3iedm_OBJECT-TYPE.owl#SURFACE-VESSEL-TYPE"/>
    <rdfs:label xml:lang="en">auxiliary floating drydock, small</rdfs:label>
    <rdfs:comment xml:lang="en">Floating dock capable of docking small ships.</rdfs:comment>
    <rdf:type rdf:resource="http://www.w3.org/2002/07/owl#Class"/>
  </rdf:Description>
  <rdf:Description rdf:about="#CONTROL-FEATURE-TYPE_Class-F_airspace">
    <rdfs:subClassOf rdf:resource="jc3iedm_OBJECT-TYPE.owl#CONTROL-FEATURE-TYPE"/>
    <rdfs:label xml:lang="en">class f airspace</rdfs:label>
    <rdfs:comment xml:lang="en">An airspace in which instrument flight rule and visual flight rule flights are permitted; all participating instrument flight rule flights receive an air traffic advisory service and all flights receive flight information service if requested.</rdfs:comment>
    <rdf:type rdf:resource="http://www.w3.org/2002/07/owl#Class"/>
  </rdf:Description>
  <rdf:Description rdf:about="#SURFACE-VESSEL-TYPE_Minehunter/sweeper,_ocean">
    <rdfs:subClassOf rdf:resource="jc3iedm_OBJECT-TYPE.owl#SURFACE-VESSEL-TYPE"/>
    <rdfs:label xml:lang="en">minehunter/sweeper, ocean</rdfs:label>
    <rdfs:comment xml:lang="en">A mine warfare craft equipped for both hunting and sweeping mines and capable of operating in open ocean waters.</rdfs:comment>
    <rdf:type rdf:resource="http://www.w3.org/2002/07/owl#Class"/>
  </rdf:Description>
  <rdf:Description rdf:about="#ROUTE-TYPE_Standard_route">
    <rdfs:subClassOf rdf:resource="jc3iedm_OBJECT-TYPE.owl#ROUTE-TYPE"/>
    <rdfs:label xml:lang="en">standard route</rdfs:label>
    <rdfs:comment xml:lang="en">In naval cooperation and guidance for shipping, a preplanned single track connecting positions within the main shipping route.</rdfs:comment>
    <rdf:type rdf:resource="http://www.w3.org/2002/07/owl#Class"/>
  </rdf:Description>
  <rdf:Description rdf:about="jc3iedm_OBJECT-TYPE.owl#organisation-type-command-and-control-category-code">
    <rdf:type rdf:resource="http://www.w3.org/2002/07/owl#DatatypeProperty"/>
    <rdfs:domain rdf:resource="jc3iedm_OBJECT-TYPE.owl#ORGANISATION-TYPE"/>
    <rdfs:range rdf:resource="http://www.w3.org/2001/XMLSchema#string"/>
  </rdf:Description>
  <rdf:Description rdf:about="#ELECTRONIC-EQUIPMENT-TYPE_Sensor">
    <rdfs:subClassOf rdf:resource="jc3iedm_OBJECT-TYPE.owl#ELECTRONIC-EQUIPMENT-TYPE"/>
    <rdfs:label xml:lang="en">sensor</rdfs:label>
    <rdfs:comment xml:lang="en">A device that detects or measures a physical property and records, indicates, or otherwise responds to it.</rdfs:comment>
    <rdf:type rdf:resource="http://www.w3.org/2002/07/owl#Class"/>
  </rdf:Description>
  <rdf:Description rdf:about="#SURFACE-VESSEL-TYPE_Landing_ship,_tank">
    <rdfs:subClassOf rdf:resource="jc3iedm_OBJECT-TYPE.owl#SURFACE-VESSEL-TYPE"/>
    <rdfs:label xml:lang="en">landing ship, tank</rdfs:label>
    <rdfs:comment xml:lang="en">Ship in size range 85-100 metres employed to transport troops, vehicles and tanks for amphibious assault. Must have bow doors and/or landing ramp.</rdfs:comment>
    <rdf:type rdf:resource="http://www.w3.org/2002/07/owl#Class"/>
  </rdf:Description>
  <rdf:Description rdf:about="#SUBSURFACE-VESSEL-TYPE_Submersible,_rescue_(commercial)">
    <rdfs:subClassOf rdf:resource="jc3iedm_OBJECT-TYPE.owl#SUBSURFACE-VESSEL-TYPE"/>
    <rdfs:label xml:lang="en">submersible, rescue (commercial)</rdfs:label>
    <rdfs:comment xml:lang="en">Submersible designed specifically for underwater rescue operations.</rdfs:comment>
    <rdf:type rdf:resource="http://www.w3.org/2002/07/owl#Class"/>
  </rdf:Description>
  <rdf:Description rdf:about="jc3iedm_OBJECT-TYPE.owl#biological-materiel-type-category-code">
    <rdf:type rdf:resource="http://www.w3.org/2002/07/owl#DatatypeProperty"/>
    <rdfs:domain rdf:resource="jc3iedm_OBJECT-TYPE.owl#BIOLOGICAL-MATERIEL-TYPE"/>
    <rdfs:range rdf:resource="http://www.w3.org/2001/XMLSchema#string"/>
  </rdf:Description>
  <rdf:Description rdf:about="#FACILITY-TYPE_Row_house">
    <rdfs:subClassOf rdf:resource="jc3iedm_OBJECT-TYPE.owl#FACILITY-TYPE"/>
    <rdfs:label xml:lang="en">row house</rdfs:label>
    <rdfs:comment xml:lang="en">Facilities of a type that represent individual houses sharing at least one wall.</rdfs:comment>
    <rdf:type rdf:resource="http://www.w3.org/2002/07/owl#Class"/>
  </rdf:Description>
  <rdf:Description rdf:about="#GROUP-ORGANISATION-TYPE_Media,_national">
    <rdfs:subClassOf rdf:resource="jc3iedm_OBJECT-TYPE.owl#GROUP-ORGANISATION-TYPE"/>
    <rdfs:label xml:lang="en">media, national</rdfs:label>
    <rdfs:comment xml:lang="en">A GROUP-ORGANISATION-TYPE that comprises persons that report for national mass communications, but do not take part in the actions.</rdfs:comment>
    <rdf:type rdf:resource="http://www.w3.org/2002/07/owl#Class"/>
  </rdf:Description>
  <rdf:Description rdf:about="#SURFACE-VESSEL-TYPE_Patrol_craft,_submarine_chaser_fast">
    <rdfs:subClassOf rdf:resource="jc3iedm_OBJECT-TYPE.owl#SURFACE-VESSEL-TYPE"/>
    <rdfs:label xml:lang="en">patrol craft, submarine chaser fast</rdfs:label>
    <rdfs:comment xml:lang="en">Vessel in size range 35-55 metres designed and fitted primarily for escort duties in the anti submarine warfare role capable of at least 35 knots - 65 km/hr.</rdfs:comment>
    <rdf:type rdf:resource="http://www.w3.org/2002/07/owl#Class"/>
  </rdf:Description>
  <rdf:Description rdf:about="#CONTROL-FEATURE-TYPE_Reform_point">
    <rdfs:subClassOf rdf:resource="jc3iedm_OBJECT-TYPE.owl#CONTROL-FEATURE-TYPE"/>
    <rdfs:label xml:lang="en">reform point</rdfs:label>
    <rdfs:comment xml:lang="en">A CONTROL-FEATURE-TYPE that identifies a point where aircraft join again during a mission.</rdfs:comment>
    <rdf:type rdf:resource="http://www.w3.org/2002/07/owl#Class"/>
  </rdf:Description>
  <rdf:Description rdf:about="#FACILITY-TYPE_Passenger_terminal">
    <rdfs:subClassOf rdf:resource="jc3iedm_OBJECT-TYPE.owl#FACILITY-TYPE"/>
    <rdfs:label xml:lang="en">passenger terminal</rdfs:label>
    <rdfs:comment xml:lang="en">A facility that provides transportation services for passengers.</rdfs:comment>
    <rdf:type rdf:resource="http://www.w3.org/2002/07/owl#Class"/>
  </rdf:Description>
  <rdf:Description rdf:about="#SURFACE-VESSEL-TYPE_Customs_launch">
    <rdfs:subClassOf rdf:resource="jc3iedm_OBJECT-TYPE.owl#SURFACE-VESSEL-TYPE"/>
    <rdfs:label xml:lang="en">customs launch</rdfs:label>
    <rdfs:comment xml:lang="en">Customs operated small craft less than 20 metres employed in sheltered waters for transporting personnel.</rdfs:comment>
    <rdf:type rdf:resource="http://www.w3.org/2002/07/owl#Class"/>
  </rdf:Description>
  <rdf:Description rdf:about="#UNIT-TYPE_Information_warfare">
    <rdfs:subClassOf rdf:resource="jc3iedm_OBJECT-TYPE.owl#UNIT-TYPE"/>
    <rdfs:label xml:lang="en">information warfare</rdfs:label>
    <rdfs:comment xml:lang="en">A UNIT-TYPE whose principal designation is to achieve information superiority by affecting a hostile’s information, information-based processes and information systems, while defending one’s own information, information-based processes and information systems.</rdfs:comment>
    <rdf:type rdf:resource="http://www.w3.org/2002/07/owl#Class"/>
  </rdf:Description>
  <rdf:Description rdf:about="#SURFACE-VESSEL-TYPE_Torpedo_boat,_small,_hydrofoil">
    <rdfs:subClassOf rdf:resource="jc3iedm_OBJECT-TYPE.owl#SURFACE-VESSEL-TYPE"/>
    <rdfs:label xml:lang="en">torpedo boat, small, hydrofoil</rdfs:label>
    <rdfs:comment xml:lang="en">High-speed (35 knots - 65 km/hr) anti-surface ship patrol craft smaller in size range 20 - 30 metres fitted with torpedoes and hydrofoils.</rdfs:comment>
    <rdf:type rdf:resource="http://www.w3.org/2002/07/owl#Class"/>
  </rdf:Description>
  <rdf:Description rdf:about="#SURFACE-VESSEL-TYPE_Patrol_boat,_customs">
    <rdfs:subClassOf rdf:resource="jc3iedm_OBJECT-TYPE.owl#SURFACE-VESSEL-TYPE"/>
    <rdfs:label xml:lang="en">patrol boat, customs</rdfs:label>
    <rdfs:comment xml:lang="en">Customs operated coastal patrol unit intended for a basically coastal guarding function. Includes any coastal patrol ship under 45 metres which cannot qualify as a PG in armament. May be unarmed.</rdfs:comment>
    <rdf:type rdf:resource="http://www.w3.org/2002/07/owl#Class"/>
  </rdf:Description>
  <rdf:Description rdf:about="#FACILITY-TYPE_Observation_tower">
    <rdfs:subClassOf rdf:resource="jc3iedm_OBJECT-TYPE.owl#FACILITY-TYPE"/>
    <rdfs:label xml:lang="en">observation tower</rdfs:label>
    <rdfs:comment xml:lang="en">A position from which military observations are made, or fire directed and adjusted, and which possesses appropriate communications.</rdfs:comment>
    <rdf:type rdf:resource="http://www.w3.org/2002/07/owl#Class"/>
  </rdf:Description>
  <rdf:Description rdf:about="#SURFACE-VESSEL-TYPE_Destroyer,_guided_missile">
    <rdfs:subClassOf rdf:resource="jc3iedm_OBJECT-TYPE.owl#SURFACE-VESSEL-TYPE"/>
    <rdfs:label xml:lang="en">destroyer, guided missile</rdfs:label>
    <rdfs:comment xml:lang="en">A destroyer type ship fitted with one more force guided missile systems. Major surface combatant in range of about 95 to 140 metres whole general mission is to conduct operations with strike, ASW and amphibious forces, and to perform screening and convoy duties. May have helicopters not especially fitted for ASW.</rdfs:comment>
    <rdf:type rdf:resource="http://www.w3.org/2002/07/owl#Class"/>
  </rdf:Description>
  <rdf:Description rdf:about="#UNIT-TYPE_Field_artillery">
    <rdfs:subClassOf rdf:resource="jc3iedm_OBJECT-TYPE.owl#UNIT-TYPE"/>
    <rdfs:label xml:lang="en">field artillery</rdfs:label>
    <rdfs:comment xml:lang="en">A UNIT-TYPE whose principal designation is the employment of tube artillery in support of manoeuvre units.</rdfs:comment>
    <rdf:type rdf:resource="http://www.w3.org/2002/07/owl#Class"/>
  </rdf:Description>
  <rdf:Description rdf:about="#RAILCAR-TYPE_Railed_equipment">
    <rdfs:subClassOf rdf:resource="jc3iedm_OBJECT-TYPE.owl#RAILCAR-TYPE"/>
    <rdfs:label xml:lang="en">railed equipment</rdfs:label>
    <rdfs:comment xml:lang="en">Mobile equipment that uses rails to move on, for example, dockyard cranes.</rdfs:comment>
    <rdf:type rdf:resource="http://www.w3.org/2002/07/owl#Class"/>
  </rdf:Description>
  <rdf:Description rdf:about="#SURFACE-VESSEL-TYPE_Lighter,_covered,_dry_dock_companion">
    <rdfs:subClassOf rdf:resource="jc3iedm_OBJECT-TYPE.owl#SURFACE-VESSEL-TYPE"/>
    <rdfs:label xml:lang="en">lighter, covered, dry dock companion</rdfs:label>
    <rdfs:comment xml:lang="en">Craft used to support the operations of a dry dock other than workshops.</rdfs:comment>
    <rdf:type rdf:resource="http://www.w3.org/2002/07/owl#Class"/>
  </rdf:Description>
  <rdf:Description rdf:about="#FACILITY-TYPE_Classification_facility">
    <rdfs:subClassOf rdf:resource="jc3iedm_OBJECT-TYPE.owl#FACILITY-TYPE"/>
    <rdfs:label xml:lang="en">classification facility</rdfs:label>
    <rdfs:comment xml:lang="en">No definition provided in ADatP-3 Baseline 13.1 FFIRN/FUD 1650/6.</rdfs:comment>
    <rdf:type rdf:resource="http://www.w3.org/2002/07/owl#Class"/>
  </rdf:Description>
  <rdf:Description rdf:about="#SURFACE-VESSEL-TYPE_Barge,_oil_storage,_submersible">
    <rdfs:subClassOf rdf:resource="jc3iedm_OBJECT-TYPE.owl#SURFACE-VESSEL-TYPE"/>
    <rdfs:label xml:lang="en">barge, oil storage, submersible</rdfs:label>
    <rdfs:comment xml:lang="en">POL (Petroleum oil and lubricants) storage barge that cannot be towed around the harbour but does sink below the water surface when filled.</rdfs:comment>
    <rdf:type rdf:resource="http://www.w3.org/2002/07/owl#Class"/>
  </rdf:Description>
  <rdf:Description rdf:about="#SURFACE-VESSEL-TYPE_Repair_ship,_aircraft">
    <rdfs:subClassOf rdf:resource="jc3iedm_OBJECT-TYPE.owl#SURFACE-VESSEL-TYPE"/>
    <rdfs:label xml:lang="en">repair ship, aircraft</rdfs:label>
    <rdfs:comment xml:lang="en">Ship of any size used to repair helicopters, aircraft and aircraft engines.</rdfs:comment>
    <rdf:type rdf:resource="http://www.w3.org/2002/07/owl#Class"/>
  </rdf:Description>
  <rdf:Description rdf:about="#AIRFIELD-TYPE_Limited">
    <rdfs:subClassOf rdf:resource="jc3iedm_OBJECT-TYPE.owl#AIRFIELD-TYPE"/>
    <rdfs:label xml:lang="en">limited</rdfs:label>
    <rdfs:comment xml:lang="en">Airfields having permanent type surface runways with less than the minimum facilities required for civil, joint or military airports.</rdfs:comment>
    <rdf:type rdf:resource="http://www.w3.org/2002/07/owl#Class"/>
  </rdf:Description>
  <rdf:Description rdf:about="#SURFACE-VESSEL-TYPE_Merchant_ship,_replenishment_oiler">
    <rdfs:subClassOf rdf:resource="jc3iedm_OBJECT-TYPE.owl#SURFACE-VESSEL-TYPE"/>
    <rdfs:label xml:lang="en">merchant ship, replenishment oiler</rdfs:label>
    <rdfs:comment xml:lang="en">Non-naval ship able to provide replenishment to ships at sea of POL and solid store products. Over 120 metres in size.</rdfs:comment>
    <rdf:type rdf:resource="http://www.w3.org/2002/07/owl#Class"/>
  </rdf:Description>
  <rdf:Description rdf:about="#MISCELLANEOUS-EQUIPMENT-TYPE_Tank">
    <rdfs:subClassOf rdf:resource="jc3iedm_OBJECT-TYPE.owl#MISCELLANEOUS-EQUIPMENT-TYPE"/>
    <rdfs:label xml:lang="en">tank</rdfs:label>
    <rdfs:comment xml:lang="en">A large receptacle or storage chamber, especially for liquid or gas.</rdfs:comment>
    <rdf:type rdf:resource="http://www.w3.org/2002/07/owl#Class"/>
  </rdf:Description>
  <rdf:Description rdf:about="#ROUTE-TYPE_Not_known">
    <rdfs:subClassOf rdf:resource="jc3iedm_OBJECT-TYPE.owl#ROUTE-TYPE"/>
    <rdfs:label xml:lang="en">not known</rdfs:label>
    <rdfs:comment xml:lang="en">It is not possible to determine which value is most applicable.</rdfs:comment>
    <rdf:type rdf:resource="http://www.w3.org/2002/07/owl#Class"/>
  </rdf:Description>
  <rdf:Description rdf:about="#SURFACE-VESSEL-TYPE_Minesweeper,_coastal,_special">
    <rdfs:subClassOf rdf:resource="jc3iedm_OBJECT-TYPE.owl#SURFACE-VESSEL-TYPE"/>
    <rdfs:label xml:lang="en">minesweeper, coastal, special</rdfs:label>
    <rdfs:comment xml:lang="en">A minesweeper fitted with special to type mine-sweeping devices, for use within coastal waters.</rdfs:comment>
    <rdf:type rdf:resource="http://www.w3.org/2002/07/owl#Class"/>
  </rdf:Description>
  <rdf:Description rdf:about="#WEAPON-TYPE_Small_arms">
    <rdfs:subClassOf rdf:resource="jc3iedm_OBJECT-TYPE.owl#WEAPON-TYPE"/>
    <rdfs:label xml:lang="en">small arms</rdfs:label>
    <rdfs:comment xml:lang="en">Individual portable weapon for defensive purposes.</rdfs:comment>
    <rdf:type rdf:resource="http://www.w3.org/2002/07/owl#Class"/>
  </rdf:Description>
  <rdf:Description rdf:about="#CONTROL-FEATURE-TYPE_Entry_point">
    <rdfs:subClassOf rdf:resource="jc3iedm_OBJECT-TYPE.owl#CONTROL-FEATURE-TYPE"/>
    <rdfs:label xml:lang="en">entry point</rdfs:label>
    <rdfs:comment xml:lang="en">A point designated for use by vehicles or personnel in entering an area, line or volume.</rdfs:comment>
    <rdf:type rdf:resource="http://www.w3.org/2002/07/owl#Class"/>
  </rdf:Description>
  <rdf:Description rdf:about="#FACILITY-TYPE_Fort">
    <rdfs:subClassOf rdf:resource="jc3iedm_OBJECT-TYPE.owl#FACILITY-TYPE"/>
    <rdfs:label xml:lang="en">fort</rdfs:label>
    <rdfs:comment xml:lang="en">A fortified place garrisoned with troops.</rdfs:comment>
    <rdf:type rdf:resource="http://www.w3.org/2002/07/owl#Class"/>
  </rdf:Description>
  <rdf:Description rdf:about="#FACILITY-TYPE_Military_materiel_facility,_armament_production">
    <rdfs:subClassOf rdf:resource="jc3iedm_OBJECT-TYPE.owl#FACILITY-TYPE"/>
    <rdfs:label xml:lang="en">military materiel facility, armament production</rdfs:label>
    <rdfs:comment xml:lang="en">A facility used as for armament production.</rdfs:comment>
    <rdf:type rdf:resource="http://www.w3.org/2002/07/owl#Class"/>
  </rdf:Description>
  <rdf:Description rdf:about="#FACILITY-TYPE_Service,_research,_utility_facility,_telecommunications_facility">
    <rdfs:subClassOf rdf:resource="jc3iedm_OBJECT-TYPE.owl#FACILITY-TYPE"/>
    <rdfs:label xml:lang="en">service, research, utility facility, telecommunications facility</rdfs:label>
    <rdfs:comment xml:lang="en">A facility generally used to support service, research or utility functions in support of telecommunications.</rdfs:comment>
    <rdf:type rdf:resource="http://www.w3.org/2002/07/owl#Class"/>
  </rdf:Description>
  <rdf:Description rdf:about="#CBRN-EQUIPMENT-TYPE_Biological_stand-off_detection_system">
    <rdfs:subClassOf rdf:resource="jc3iedm_OBJECT-TYPE.owl#CBRN-EQUIPMENT-TYPE"/>
    <rdfs:label xml:lang="en">biological stand off detection system</rdfs:label>
    <rdfs:comment xml:lang="en">A detector capable of remotely detecting biological contamination.</rdfs:comment>
    <rdf:type rdf:resource="http://www.w3.org/2002/07/owl#Class"/>
  </rdf:Description>
  <rdf:Description rdf:about="#EXECUTIVE-MILITARY-ORGANISATION-TYPE_Headquarters">
    <rdfs:subClassOf rdf:resource="jc3iedm_OBJECT-TYPE.owl#EXECUTIVE-MILITARY-ORGANISATION-TYPE"/>
    <rdfs:label xml:lang="en">headquarters</rdfs:label>
    <rdfs:comment xml:lang="en">An EXECUTIVE-MILITARY-ORGANISATION-TYPE that performs the management functions of an international, national, strategic or service headquarters.</rdfs:comment>
    <rdf:type rdf:resource="http://www.w3.org/2002/07/owl#Class"/>
  </rdf:Description>
  <rdf:Description rdf:about="#SURFACE-VESSEL-TYPE_Patrol_ship,_anti-submarine_warfare">
    <rdfs:subClassOf rdf:resource="jc3iedm_OBJECT-TYPE.owl#SURFACE-VESSEL-TYPE"/>
    <rdfs:label xml:lang="en">patrol ship, anti submarine warfare</rdfs:label>
    <rdfs:comment xml:lang="en">ASW (anti-submarine warfare) patrol ship in size range 45 - 85 metres fitted with medium range sonar and ASW weapons.</rdfs:comment>
    <rdf:type rdf:resource="http://www.w3.org/2002/07/owl#Class"/>
  </rdf:Description>
  <rdf:Description rdf:about="#MILITARY-POST-TYPE_Point_of_contact">
    <rdfs:subClassOf rdf:resource="jc3iedm_OBJECT-TYPE.owl#MILITARY-POST-TYPE"/>
    <rdfs:label xml:lang="en">point of contact</rdfs:label>
    <rdfs:comment xml:lang="en">A MILITARY-POST-TYPE responsible to coordinate details for each element of support required.</rdfs:comment>
    <rdf:type rdf:resource="http://www.w3.org/2002/07/owl#Class"/>
  </rdf:Description>
  <rdf:Description rdf:about="#SURFACE-VESSEL-TYPE_Oceanographic_research_ship">
    <rdfs:subClassOf rdf:resource="jc3iedm_OBJECT-TYPE.owl#SURFACE-VESSEL-TYPE"/>
    <rdfs:label xml:lang="en">oceanographic research ship</rdfs:label>
    <rdfs:comment xml:lang="en">Ship which conducts multi-discipline research at sea in oceanographic radiomagnetics, meteorology and oceanography.</rdfs:comment>
    <rdf:type rdf:resource="http://www.w3.org/2002/07/owl#Class"/>
  </rdf:Description>
  <rdf:Description rdf:about="#ELECTRONIC-EQUIPMENT-TYPE_Instrument_landing_system">
    <rdfs:subClassOf rdf:resource="jc3iedm_OBJECT-TYPE.owl#ELECTRONIC-EQUIPMENT-TYPE"/>
    <rdfs:label xml:lang="en">instrument landing system</rdfs:label>
    <rdfs:comment xml:lang="en">An ELECTRONIC-EQUIPMENT-TYPE that provides aircraft with horizontal and vertical guidance just before landing and during landing, and at certain fixed points, indicates the distance to the reference point of landing.</rdfs:comment>
    <rdf:type rdf:resource="http://www.w3.org/2002/07/owl#Class"/>
  </rdf:Description>
  <rdf:Description rdf:about="#CONTROL-FEATURE-TYPE_Air_control_point">
    <rdfs:subClassOf rdf:resource="jc3iedm_OBJECT-TYPE.owl#CONTROL-FEATURE-TYPE"/>
    <rdfs:label xml:lang="en">air control point</rdfs:label>
    <rdfs:comment xml:lang="en">An easily identifiable point on the terrain or an electronic navigational aid used to provide necessary control during air movement. Air control points are generally designated at each point where the flight route or air corridor makes a definite change in any direction and at any other point deemed necessary for timing or control of the operation.</rdfs:comment>
    <rdf:type rdf:resource="http://www.w3.org/2002/07/owl#Class"/>
  </rdf:Description>
  <rdf:Description rdf:about="#MARITIME-EQUIPMENT-TYPE_Depth-charge_launcher">
    <rdfs:subClassOf rdf:resource="jc3iedm_OBJECT-TYPE.owl#MARITIME-EQUIPMENT-TYPE"/>
    <rdfs:label xml:lang="en">depth charge launcher</rdfs:label>
    <rdfs:comment xml:lang="en">A structural device designed to support and hold a depth-charge in position for firing.</rdfs:comment>
    <rdf:type rdf:resource="http://www.w3.org/2002/07/owl#Class"/>
  </rdf:Description>
  <rdf:Description rdf:about="#MILITARY-OBSTACLE-TYPE_Roadblock">
    <rdfs:subClassOf rdf:resource="jc3iedm_OBJECT-TYPE.owl#MILITARY-OBSTACLE-TYPE"/>
    <rdfs:label xml:lang="en">roadblock</rdfs:label>
    <rdfs:comment xml:lang="en">A barrier or obstacle (usually covered by fire) used to block, or limit the movement of, hostile vehicles along a route.</rdfs:comment>
    <rdf:type rdf:resource="http://www.w3.org/2002/07/owl#Class"/>
  </rdf:Description>
  <rdf:Description rdf:about="jc3iedm_OBJECT-TYPE.owl#surface-vessel-type-maximum-deck-load-quantity">
    <rdf:type rdf:resource="http://www.w3.org/2002/07/owl#DatatypeProperty"/>
    <rdfs:domain rdf:resource="jc3iedm_OBJECT-TYPE.owl#SURFACE-VESSEL-TYPE"/>
  </rdf:Description>
  <rdf:Description rdf:about="#SURFACE-VESSEL-TYPE_Patrol_boat,_general">
    <rdfs:subClassOf rdf:resource="jc3iedm_OBJECT-TYPE.owl#SURFACE-VESSEL-TYPE"/>
    <rdfs:label xml:lang="en">patrol boat, general</rdfs:label>
    <rdfs:comment xml:lang="en">Coastal patrol unit intended for a basically coastal guarding function. Includes any coastal patrol ship under 45 metres which cannot qualify as a PG in armament. May be unarmed.</rdfs:comment>
    <rdf:type rdf:resource="http://www.w3.org/2002/07/owl#Class"/>
  </rdf:Description>
  <rdf:Description rdf:about="jc3iedm_OBJECT-TYPE.owl#vehicle-type-category-code">
    <rdf:type rdf:resource="http://www.w3.org/2002/07/owl#DatatypeProperty"/>
    <rdfs:domain rdf:resource="jc3iedm_OBJECT-TYPE.owl#VEHICLE-TYPE"/>
    <rdfs:range rdf:resource="http://www.w3.org/2001/XMLSchema#string"/>
  </rdf:Description>
  <rdf:Description rdf:about="#FACILITY-TYPE_Rearm,_refuel_and_resupply_point">
    <rdfs:subClassOf rdf:resource="jc3iedm_OBJECT-TYPE.owl#FACILITY-TYPE"/>
    <rdfs:label xml:lang="en">rearm, refuel and resupply point</rdfs:label>
    <rdfs:comment xml:lang="en">A designated facility through which a unit passes where it receives fuel, ammunition, and other necessary supplies to continue combat operations.</rdfs:comment>
    <rdf:type rdf:resource="http://www.w3.org/2002/07/owl#Class"/>
  </rdf:Description>
  <rdf:Description rdf:about="#FACILITY-TYPE_Depot,_chemicals">
    <rdfs:subClassOf rdf:resource="jc3iedm_OBJECT-TYPE.owl#FACILITY-TYPE"/>
    <rdfs:label xml:lang="en">depot, chemicals</rdfs:label>
    <rdfs:comment xml:lang="en">An area used for the storage of chemicals.</rdfs:comment>
    <rdf:type rdf:resource="http://www.w3.org/2002/07/owl#Class"/>
  </rdf:Description>
  <rdf:Description rdf:about="#CONTROL-FEATURE-TYPE_Crossing_area">
    <rdfs:subClassOf rdf:resource="jc3iedm_OBJECT-TYPE.owl#CONTROL-FEATURE-TYPE"/>
    <rdfs:label xml:lang="en">crossing area</rdfs:label>
    <rdfs:comment xml:lang="en">A number of adjacent crossing sites under the control of one commander.</rdfs:comment>
    <rdf:type rdf:resource="http://www.w3.org/2002/07/owl#Class"/>
  </rdf:Description>
  <rdf:Description rdf:about="#FACILITY-TYPE_Governmental_leadership">
    <rdfs:subClassOf rdf:resource="jc3iedm_OBJECT-TYPE.owl#FACILITY-TYPE"/>
    <rdfs:label xml:lang="en">governmental leadership</rdfs:label>
    <rdfs:comment xml:lang="en">A facility used to support governmental leadership functions.</rdfs:comment>
    <rdf:type rdf:resource="http://www.w3.org/2002/07/owl#Class"/>
  </rdf:Description>
  <rdf:Description rdf:about="#CONTROL-FEATURE-TYPE_Decision_point">
    <rdfs:subClassOf rdf:resource="jc3iedm_OBJECT-TYPE.owl#CONTROL-FEATURE-TYPE"/>
    <rdfs:label xml:lang="en">decision point</rdfs:label>
    <rdfs:comment xml:lang="en">An event, area, line, or point in the battlespace where tactical decisions are required resulting from the wargaming process or the operations order. Decision points do not dictate commander's decisions, they only indicate that a decision is required, and they indicate when/where the decision should be made to have the maximum effect on friendly or enemy courses of action.</rdfs:comment>
    <rdf:type rdf:resource="http://www.w3.org/2002/07/owl#Class"/>
  </rdf:Description>
  <rdf:Description rdf:about="#CHEMICAL-MATERIEL-TYPE_Blood_agent">
    <rdfs:subClassOf rdf:resource="jc3iedm_OBJECT-TYPE.owl#CHEMICAL-MATERIEL-TYPE"/>
    <rdfs:label xml:lang="en">blood agent</rdfs:label>
    <rdfs:comment xml:lang="en">A CHEMICAL-MATERIEL-TYPE, including the cyanide group, that affects bodily functions by preventing the normal transfer of oxygen from the blood to body tissues. Also called "cyanogen agent".</rdfs:comment>
    <rdf:type rdf:resource="http://www.w3.org/2002/07/owl#Class"/>
  </rdf:Description>
  <rdf:Description rdf:about="#SUBSURFACE-VESSEL-TYPE_Submersible,_general_(commercial)">
    <rdfs:subClassOf rdf:resource="jc3iedm_OBJECT-TYPE.owl#SUBSURFACE-VESSEL-TYPE"/>
    <rdfs:label xml:lang="en">submersible, general (commercial)</rdfs:label>
    <rdfs:comment xml:lang="en">General designator for non-combatant submersible.</rdfs:comment>
    <rdf:type rdf:resource="http://www.w3.org/2002/07/owl#Class"/>
  </rdf:Description>
  <rdf:Description rdf:about="#ENGINEERING-EQUIPMENT-TYPE_Rock_crusher">
    <rdfs:subClassOf rdf:resource="jc3iedm_OBJECT-TYPE.owl#ENGINEERING-EQUIPMENT-TYPE"/>
    <rdfs:label xml:lang="en">rock crusher</rdfs:label>
    <rdfs:comment xml:lang="en">A machine used to break down rocks.</rdfs:comment>
    <rdf:type rdf:resource="http://www.w3.org/2002/07/owl#Class"/>
  </rdf:Description>
  <rdf:Description rdf:about="#MILITARY-POST-TYPE_Tactical_air_coordinator,_airborne">
    <rdfs:subClassOf rdf:resource="jc3iedm_OBJECT-TYPE.owl#MILITARY-POST-TYPE"/>
    <rdfs:label xml:lang="en">tactical air coordinator, airborne</rdfs:label>
    <rdfs:comment xml:lang="en">A MILITARY-POST-TYPE that is an officer who coordinates, from an aircraft, the action of combat aircraft engaged in close support of ground or sea forces.</rdfs:comment>
    <rdf:type rdf:resource="http://www.w3.org/2002/07/owl#Class"/>
  </rdf:Description>
  <rdf:Description rdf:about="#SURFACE-VESSEL-TYPE_Schooner">
    <rdfs:subClassOf rdf:resource="jc3iedm_OBJECT-TYPE.owl#SURFACE-VESSEL-TYPE"/>
    <rdfs:label xml:lang="en">schooner</rdfs:label>
    <rdfs:comment xml:lang="en">Sailing vessel of schooner design.</rdfs:comment>
    <rdf:type rdf:resource="http://www.w3.org/2002/07/owl#Class"/>
  </rdf:Description>
  <rdf:Description rdf:about="#AIRCRAFT-TYPE_Not_known">
    <rdfs:label xml:lang="en">not known</rdfs:label>
    <rdfs:subClassOf rdf:resource="jc3iedm_OBJECT-TYPE.owl#AIRCRAFT-TYPE"/>
    <rdfs:comment xml:lang="en">It is not possible to determine which value is most applicable.</rdfs:comment>
    <rdf:type rdf:resource="http://www.w3.org/2002/07/owl#Class"/>
  </rdf:Description>
  <rdf:Description rdf:about="#MISCELLANEOUS-EQUIPMENT-TYPE_Smoke_generator">
    <rdfs:subClassOf rdf:resource="jc3iedm_OBJECT-TYPE.owl#MISCELLANEOUS-EQUIPMENT-TYPE"/>
    <rdfs:label xml:lang="en">smoke generator</rdfs:label>
    <rdfs:comment xml:lang="en">A system used to generate smoke in the battlespace.</rdfs:comment>
    <rdf:type rdf:resource="http://www.w3.org/2002/07/owl#Class"/>
  </rdf:Description>
  <rdf:Description rdf:about="#MILITARY-OBSTACLE-TYPE_Barbed_wire_entanglement">
    <rdfs:subClassOf rdf:resource="jc3iedm_OBJECT-TYPE.owl#MILITARY-OBSTACLE-TYPE"/>
    <rdfs:label xml:lang="en">barbed wire entanglement</rdfs:label>
    <rdfs:comment xml:lang="en">An obstacle, consisting of twisted wires armed with barbs or sharp points.</rdfs:comment>
    <rdf:type rdf:resource="http://www.w3.org/2002/07/owl#Class"/>
  </rdf:Description>
  <rdf:Description rdf:about="#ROUTE-TYPE_Maritime_minelaying_track">
    <rdfs:subClassOf rdf:resource="jc3iedm_OBJECT-TYPE.owl#ROUTE-TYPE"/>
    <rdfs:label xml:lang="en">maritime minelaying track</rdfs:label>
    <rdfs:comment xml:lang="en">The prescribed line over the ground along which the centre of the minelaying gear must travel.</rdfs:comment>
    <rdf:type rdf:resource="http://www.w3.org/2002/07/owl#Class"/>
  </rdf:Description>
  <rdf:Description rdf:about="jc3iedm_OBJECT-TYPE.owl#maritime-equipment-type-category-code">
    <rdf:type rdf:resource="http://www.w3.org/2002/07/owl#DatatypeProperty"/>
    <rdfs:domain rdf:resource="jc3iedm_OBJECT-TYPE.owl#MARITIME-EQUIPMENT-TYPE"/>
    <rdfs:range rdf:resource="http://www.w3.org/2001/XMLSchema#string"/>
  </rdf:Description>
  <rdf:Description rdf:about="#FACILITY-TYPE_Sewage_treatment_facility">
    <rdfs:subClassOf rdf:resource="jc3iedm_OBJECT-TYPE.owl#FACILITY-TYPE"/>
    <rdfs:label xml:lang="en">sewage treatment facility</rdfs:label>
    <rdfs:comment xml:lang="en">A facility used for the handling and treatment of sewage.</rdfs:comment>
    <rdf:type rdf:resource="http://www.w3.org/2002/07/owl#Class"/>
  </rdf:Description>
  <rdf:Description rdf:about="#FACILITY-TYPE_POW_camp">
    <rdfs:subClassOf rdf:resource="jc3iedm_OBJECT-TYPE.owl#FACILITY-TYPE"/>
    <rdfs:label xml:lang="en">pow camp</rdfs:label>
    <rdfs:comment xml:lang="en">A camp of semi-permanent nature established for the internment of prisoners of war (POW).</rdfs:comment>
    <rdf:type rdf:resource="http://www.w3.org/2002/07/owl#Class"/>
  </rdf:Description>
  <rdf:Description rdf:about="#CONTROL-FEATURE-TYPE_Killing_area">
    <rdfs:subClassOf rdf:resource="jc3iedm_OBJECT-TYPE.owl#CONTROL-FEATURE-TYPE"/>
    <rdfs:label xml:lang="en">killing area</rdfs:label>
    <rdfs:comment xml:lang="en">A zone in which a commander plans to force the enemy to concentrate so as to destroy him.</rdfs:comment>
    <rdf:type rdf:resource="http://www.w3.org/2002/07/owl#Class"/>
  </rdf:Description>
  <rdf:Description rdf:about="#UNIT-TYPE_Medical">
    <rdfs:subClassOf rdf:resource="jc3iedm_OBJECT-TYPE.owl#UNIT-TYPE"/>
    <rdfs:label xml:lang="en">medical</rdfs:label>
    <rdfs:comment xml:lang="en">A UNIT-TYPE whose principal designation is the provision of medical and dental services and the evacuation of casualties.</rdfs:comment>
    <rdf:type rdf:resource="http://www.w3.org/2002/07/owl#Class"/>
  </rdf:Description>
  <rdf:Description rdf:about="#MILITARY-POST-TYPE_Gynaecology_physician">
    <rdfs:subClassOf rdf:resource="jc3iedm_OBJECT-TYPE.owl#MILITARY-POST-TYPE"/>
    <rdfs:label xml:lang="en">gynaecology physician</rdfs:label>
    <rdfs:comment xml:lang="en">A MILITARY-POST-TYPE that is identified as a physician specialising in Gynaecology.</rdfs:comment>
    <rdf:type rdf:resource="http://www.w3.org/2002/07/owl#Class"/>
  </rdf:Description>
  <rdf:Description rdf:about="#CONTROL-FEATURE-TYPE_Initial_approach_fix">
    <rdfs:subClassOf rdf:resource="jc3iedm_OBJECT-TYPE.owl#CONTROL-FEATURE-TYPE"/>
    <rdfs:label xml:lang="en">initial approach fix</rdfs:label>
    <rdfs:comment xml:lang="en">The point in an instrument approach that the aircraft has departed and is manoeuvring to enter the intermediate or final approach.</rdfs:comment>
    <rdf:type rdf:resource="http://www.w3.org/2002/07/owl#Class"/>
  </rdf:Description>
  <rdf:Description rdf:about="#VEHICLE-TYPE_Truck">
    <rdfs:subClassOf rdf:resource="jc3iedm_OBJECT-TYPE.owl#VEHICLE-TYPE"/>
    <rdfs:label xml:lang="en">truck</rdfs:label>
    <rdfs:comment xml:lang="en">An automotive vehicle used for transporting loads.</rdfs:comment>
    <rdf:type rdf:resource="http://www.w3.org/2002/07/owl#Class"/>
  </rdf:Description>
  <rdf:Description rdf:about="#CONTROL-FEATURE-TYPE_Break-up_point">
    <rdfs:subClassOf rdf:resource="jc3iedm_OBJECT-TYPE.owl#CONTROL-FEATURE-TYPE"/>
    <rdfs:label xml:lang="en">break up point</rdfs:label>
    <rdfs:comment xml:lang="en">A CONTROL-FEATURE-TYPE that identifies a point where aircraft split up during a mission.</rdfs:comment>
    <rdf:type rdf:resource="http://www.w3.org/2002/07/owl#Class"/>
  </rdf:Description>
  <rdf:Description rdf:about="jc3iedm_OBJECT-TYPE.owl#radioactive-materiel-type-primary-radiation-code">
    <rdf:type rdf:resource="http://www.w3.org/2002/07/owl#DatatypeProperty"/>
    <rdfs:domain rdf:resource="jc3iedm_OBJECT-TYPE.owl#RADIOACTIVE-MATERIEL-TYPE"/>
    <rdfs:range rdf:resource="http://www.w3.org/2001/XMLSchema#string"/>
  </rdf:Description>
  <rdf:Description rdf:about="#ROUTE-TYPE_Air_corridor">
    <rdfs:subClassOf rdf:resource="jc3iedm_OBJECT-TYPE.owl#ROUTE-TYPE"/>
    <rdfs:label xml:lang="en">air corridor</rdfs:label>
    <rdfs:comment xml:lang="en">A restricted air route of travel specified for use by friendly aircraft and established for the purpose of preventing friendly aircraft from being fired on by friendly forces.</rdfs:comment>
    <rdf:type rdf:resource="http://www.w3.org/2002/07/owl#Class"/>
  </rdf:Description>
  <rdf:Description rdf:about="#AMMUNITION-TYPE_Pyrotechnic_device">
    <rdfs:subClassOf rdf:resource="jc3iedm_OBJECT-TYPE.owl#AMMUNITION-TYPE"/>
    <rdfs:label xml:lang="en">pyrotechnic device</rdfs:label>
    <rdfs:comment xml:lang="en">A mixture of chemicals which when ignited is capable of reacting exothermically to produce light, heat, smoke, sound or gas, and may also be used to introduce a delay into an explosive train because of its known burning time.</rdfs:comment>
    <rdf:type rdf:resource="http://www.w3.org/2002/07/owl#Class"/>
  </rdf:Description>
  <rdf:Description rdf:about="#ROUTE-TYPE_TACAN_route">
    <rdfs:subClassOf rdf:resource="jc3iedm_OBJECT-TYPE.owl#ROUTE-TYPE"/>
    <rdfs:label xml:lang="en">tacan route</rdfs:label>
    <rdfs:comment xml:lang="en">Tactical air navigation route.</rdfs:comment>
    <rdf:type rdf:resource="http://www.w3.org/2002/07/owl#Class"/>
  </rdf:Description>
  <rdf:Description rdf:about="#MARITIME-EQUIPMENT-TYPE_Radar_reflector">
    <rdfs:subClassOf rdf:resource="jc3iedm_OBJECT-TYPE.owl#MARITIME-EQUIPMENT-TYPE"/>
    <rdfs:label xml:lang="en">radar reflector</rdfs:label>
    <rdfs:comment xml:lang="en">An object designed to increase the radio reflectivity of a vessel so that it is more visible on radar.</rdfs:comment>
    <rdf:type rdf:resource="http://www.w3.org/2002/07/owl#Class"/>
  </rdf:Description>
  <rdf:Description rdf:about="#CONTROL-FEATURE-TYPE_Marshalling_gate">
    <rdfs:subClassOf rdf:resource="jc3iedm_OBJECT-TYPE.owl#CONTROL-FEATURE-TYPE"/>
    <rdfs:label xml:lang="en">marshalling gate</rdfs:label>
    <rdfs:comment xml:lang="en">A point to which aircraft fly for air traffic purposes prior to commencing an outbound transit after takeoff or prior to landing.</rdfs:comment>
    <rdf:type rdf:resource="http://www.w3.org/2002/07/owl#Class"/>
  </rdf:Description>
  <rdf:Description rdf:about="#CONTROL-FEATURE-TYPE_Phase_line">
    <rdfs:subClassOf rdf:resource="jc3iedm_OBJECT-TYPE.owl#CONTROL-FEATURE-TYPE"/>
    <rdfs:label xml:lang="en">phase line</rdfs:label>
    <rdfs:comment xml:lang="en">A line used for control and coordination of military operations, usually a terrain feature extending across the zone of action. Army-- A line used for control and coordination of military operations. It is usually along a recognisable terrain feature extending across the sector or zone of action. Units normally report crossing PLs, but do not halt unless specifically directed.</rdfs:comment>
    <rdf:type rdf:resource="http://www.w3.org/2002/07/owl#Class"/>
  </rdf:Description>
  <rdf:Description rdf:about="#CONTROL-FEATURE-TYPE_Obstacle_restricted_area">
    <rdfs:subClassOf rdf:resource="jc3iedm_OBJECT-TYPE.owl#CONTROL-FEATURE-TYPE"/>
    <rdfs:label xml:lang="en">obstacle restricted area</rdfs:label>
    <rdfs:comment xml:lang="en">A command and control measure used to limit the type or number of obstacles within an area.</rdfs:comment>
    <rdf:type rdf:resource="http://www.w3.org/2002/07/owl#Class"/>
  </rdf:Description>
  <rdf:Description rdf:about="#MILITARY-OBSTACLE-TYPE_Minefield,_mixed">
    <rdfs:subClassOf rdf:resource="jc3iedm_OBJECT-TYPE.owl#MILITARY-OBSTACLE-TYPE"/>
    <rdfs:label xml:lang="en">minefield, mixed</rdfs:label>
    <rdfs:comment xml:lang="en">A minefield made by laying mines of both anti-personnel and anti-tank type laid with or without pattern.</rdfs:comment>
    <rdf:type rdf:resource="http://www.w3.org/2002/07/owl#Class"/>
  </rdf:Description>
  <rdf:Description rdf:about="#SURFACE-VESSEL-TYPE_Barge,_oil_storage">
    <rdfs:subClassOf rdf:resource="jc3iedm_OBJECT-TYPE.owl#SURFACE-VESSEL-TYPE"/>
    <rdfs:label xml:lang="en">barge, oil storage</rdfs:label>
    <rdfs:comment xml:lang="en">POL (petroleum oil and lubricant) storage barge that cannot be towed around the harbour.</rdfs:comment>
    <rdf:type rdf:resource="http://www.w3.org/2002/07/owl#Class"/>
  </rdf:Description>
  <rdf:Description rdf:about="#CONTROL-FEATURE-TYPE_Radar_determined_contour_of_radioactive_cloud">
    <rdfs:subClassOf rdf:resource="jc3iedm_OBJECT-TYPE.owl#CONTROL-FEATURE-TYPE"/>
    <rdfs:label xml:lang="en">radar determined contour of radioactive cloud</rdfs:label>
    <rdfs:comment xml:lang="en">The boundary of the region of the atmosphere where radar measurements indicate the presence of suspended radioactive material.</rdfs:comment>
    <rdf:type rdf:resource="http://www.w3.org/2002/07/owl#Class"/>
  </rdf:Description>
  <rdf:Description rdf:about="#AMMUNITION-TYPE_Rocket">
    <rdfs:subClassOf rdf:resource="jc3iedm_OBJECT-TYPE.owl#AMMUNITION-TYPE"/>
    <rdfs:label xml:lang="en">rocket</rdfs:label>
    <rdfs:comment xml:lang="en">A munition that is self-propelled in flight whose trajectory or course whilst in flight cannot be controlled.</rdfs:comment>
    <rdf:type rdf:resource="http://www.w3.org/2002/07/owl#Class"/>
  </rdf:Description>
  <rdf:Description rdf:about="#SURFACE-VESSEL-TYPE_Cable_tender_yard_craft">
    <rdfs:subClassOf rdf:resource="jc3iedm_OBJECT-TYPE.owl#SURFACE-VESSEL-TYPE"/>
    <rdfs:label xml:lang="en">cable tender yard craft</rdfs:label>
    <rdfs:comment xml:lang="en">Craft under 30 metres used to lay, retrieve and maintain submarine cables.</rdfs:comment>
    <rdf:type rdf:resource="http://www.w3.org/2002/07/owl#Class"/>
  </rdf:Description>
  <rdf:Description rdf:about="jc3iedm_OBJECT-TYPE.owl#vessel-type-magnetic-degaussing-code-number-quantity">
    <rdf:type rdf:resource="http://www.w3.org/2002/07/owl#DatatypeProperty"/>
    <rdfs:domain rdf:resource="jc3iedm_OBJECT-TYPE.owl#VESSEL-TYPE"/>
  </rdf:Description>
  <rdf:Description rdf:about="#MISCELLANEOUS-EQUIPMENT-TYPE_Cable,_reel">
    <rdfs:subClassOf rdf:resource="jc3iedm_OBJECT-TYPE.owl#MISCELLANEOUS-EQUIPMENT-TYPE"/>
    <rdfs:label xml:lang="en">cable, reel</rdfs:label>
    <rdfs:comment xml:lang="en">A large roll of strong thick rope of hemp or wire wound onto a drum or spindle.</rdfs:comment>
    <rdf:type rdf:resource="http://www.w3.org/2002/07/owl#Class"/>
  </rdf:Description>
  <rdf:Description rdf:about="#CBRN-EQUIPMENT-TYPE_Radiation_spectrometer">
    <rdfs:subClassOf rdf:resource="jc3iedm_OBJECT-TYPE.owl#CBRN-EQUIPMENT-TYPE"/>
    <rdfs:label xml:lang="en">radiation spectrometer</rdfs:label>
    <rdfs:comment xml:lang="en">An apparatus used for recording and measuring a radiation energy spectra, especially as a method of analysis.</rdfs:comment>
    <rdf:type rdf:resource="http://www.w3.org/2002/07/owl#Class"/>
  </rdf:Description>
  <rdf:Description rdf:about="#ROUTE-TYPE_Air_route">
    <rdfs:subClassOf rdf:resource="jc3iedm_OBJECT-TYPE.owl#ROUTE-TYPE"/>
    <rdfs:label xml:lang="en">air route</rdfs:label>
    <rdfs:comment xml:lang="en">The navigable airspace between two points identified to the extent necessary for the application of flight.</rdfs:comment>
    <rdf:type rdf:resource="http://www.w3.org/2002/07/owl#Class"/>
  </rdf:Description>
  <rdf:Description rdf:about="#GEOGRAPHIC-FEATURE-TYPE_Wetland">
    <rdfs:subClassOf rdf:resource="jc3iedm_OBJECT-TYPE.owl#GEOGRAPHIC-FEATURE-TYPE"/>
    <rdfs:label xml:lang="en">wetland</rdfs:label>
    <rdfs:comment xml:lang="en">A saturated area, at times covered with water.</rdfs:comment>
    <rdf:type rdf:resource="http://www.w3.org/2002/07/owl#Class"/>
  </rdf:Description>
  <rdf:Description rdf:about="#EXECUTIVE-MILITARY-ORGANISATION-TYPE_Military_service">
    <rdfs:subClassOf rdf:resource="jc3iedm_OBJECT-TYPE.owl#EXECUTIVE-MILITARY-ORGANISATION-TYPE"/>
    <rdfs:label xml:lang="en">military service</rdfs:label>
    <rdfs:comment xml:lang="en">An EXECUTIVE-MILITARY-ORGANISATION-TYPE, other than police, that manages the training, equipping, manning, and operating of an armed uniformed force.</rdfs:comment>
    <rdf:type rdf:resource="http://www.w3.org/2002/07/owl#Class"/>
  </rdf:Description>
  <rdf:Description rdf:about="#AMMUNITION-TYPE_Surface-to-air_missile">
    <rdfs:subClassOf rdf:resource="jc3iedm_OBJECT-TYPE.owl#AMMUNITION-TYPE"/>
    <rdfs:label xml:lang="en">surface to air missile</rdfs:label>
    <rdfs:comment xml:lang="en">A self-propelled airborne munition which is guided automatically, or by remote control, fired from the ground or vessel at an aircraft or other airborne target.</rdfs:comment>
    <rdf:type rdf:resource="http://www.w3.org/2002/07/owl#Class"/>
  </rdf:Description>
  <rdf:Description rdf:about="#UNIT-TYPE_Rocket">
    <rdfs:subClassOf rdf:resource="jc3iedm_OBJECT-TYPE.owl#UNIT-TYPE"/>
    <rdfs:label xml:lang="en">rocket</rdfs:label>
    <rdfs:comment xml:lang="en">A UNIT-TYPE whose principal designation is the employment of rockets in support of manoeuvre units.</rdfs:comment>
    <rdf:type rdf:resource="http://www.w3.org/2002/07/owl#Class"/>
  </rdf:Description>
  <rdf:Description rdf:about="#CONSUMABLE-MATERIEL-TYPE_General_supplies">
    <rdfs:subClassOf rdf:resource="jc3iedm_OBJECT-TYPE.owl#CONSUMABLE-MATERIEL-TYPE"/>
    <rdfs:label xml:lang="en">general supplies</rdfs:label>
    <rdfs:comment xml:lang="en">All disposable materiel and items used in the equipment, support and maintenance of military forces or civilians.</rdfs:comment>
    <rdf:type rdf:resource="http://www.w3.org/2002/07/owl#Class"/>
  </rdf:Description>
  <rdf:Description rdf:about="#CONTROL-FEATURE-TYPE_Cross-border_area">
    <rdfs:subClassOf rdf:resource="jc3iedm_OBJECT-TYPE.owl#CONTROL-FEATURE-TYPE"/>
    <rdfs:label xml:lang="en">cross border area</rdfs:label>
    <rdfs:comment xml:lang="en">A temporary segregated area established over international boundaries for specific operational requirements.</rdfs:comment>
    <rdf:type rdf:resource="http://www.w3.org/2002/07/owl#Class"/>
  </rdf:Description>
  <rdf:Description rdf:about="#FACILITY-TYPE_Nuclear_facility">
    <rdfs:subClassOf rdf:resource="jc3iedm_OBJECT-TYPE.owl#FACILITY-TYPE"/>
    <rdfs:label xml:lang="en">nuclear facility</rdfs:label>
    <rdfs:comment xml:lang="en">An installation with associated buildings capable of handling civilian or military nuclear material.</rdfs:comment>
    <rdf:type rdf:resource="http://www.w3.org/2002/07/owl#Class"/>
  </rdf:Description>
  <rdf:Description rdf:about="#SURFACE-VESSEL-TYPE_Tug,_harbour,_large">
    <rdfs:subClassOf rdf:resource="jc3iedm_OBJECT-TYPE.owl#SURFACE-VESSEL-TYPE"/>
    <rdfs:label xml:lang="en">tug, harbour, large</rdfs:label>
    <rdfs:comment xml:lang="en">Coastal/harbour tug between 30-40 metres with total horsepower of 1300 or more.</rdfs:comment>
    <rdf:type rdf:resource="http://www.w3.org/2002/07/owl#Class"/>
  </rdf:Description>
  <rdf:Description rdf:about="jc3iedm_OBJECT-TYPE.owl#military-organisation-type-service-code">
    <rdf:type rdf:resource="http://www.w3.org/2002/07/owl#DatatypeProperty"/>
    <rdfs:domain rdf:resource="jc3iedm_OBJECT-TYPE.owl#MILITARY-ORGANISATION-TYPE"/>
    <rdfs:range rdf:resource="http://www.w3.org/2001/XMLSchema#string"/>
  </rdf:Description>
  <rdf:Description rdf:about="#SURFACE-VESSEL-TYPE_Hulk_or_relic">
    <rdfs:subClassOf rdf:resource="jc3iedm_OBJECT-TYPE.owl#SURFACE-VESSEL-TYPE"/>
    <rdfs:label xml:lang="en">hulk or relic</rdfs:label>
    <rdfs:comment xml:lang="en">Any unused/historic ship.</rdfs:comment>
    <rdf:type rdf:resource="http://www.w3.org/2002/07/owl#Class"/>
  </rdf:Description>
  <rdf:Description rdf:about="#MILITARY-OBSTACLE-TYPE_Falling_block_obstacle">
    <rdfs:subClassOf rdf:resource="jc3iedm_OBJECT-TYPE.owl#MILITARY-OBSTACLE-TYPE"/>
    <rdfs:label xml:lang="en">falling block obstacle</rdfs:label>
    <rdfs:comment xml:lang="en">A structure that is maintained in an elevated position and can be dropped to form an obstacle.</rdfs:comment>
    <rdf:type rdf:resource="http://www.w3.org/2002/07/owl#Class"/>
  </rdf:Description>
  <rdf:Description rdf:about="#MILITARY-OBSTACLE-TYPE_Wire_obstacle,_triple_strand_concertina">
    <rdfs:subClassOf rdf:resource="jc3iedm_OBJECT-TYPE.owl#MILITARY-OBSTACLE-TYPE"/>
    <rdfs:label xml:lang="en">wire obstacle, triple strand concertina</rdfs:label>
    <rdfs:comment xml:lang="en">No definition provided in APP-6A.</rdfs:comment>
    <rdf:type rdf:resource="http://www.w3.org/2002/07/owl#Class"/>
  </rdf:Description>
  <rdf:Description rdf:about="#ROUTE-TYPE_Standard-use_army_aircraft_flight_route">
    <rdfs:subClassOf rdf:resource="jc3iedm_OBJECT-TYPE.owl#ROUTE-TYPE"/>
    <rdfs:label xml:lang="en">standard use army aircraft flight route</rdfs:label>
    <rdfs:comment xml:lang="en">Route established below the coordination altitude to facilitate movement of army aviation assets in the forward area in direct support of ground operations.</rdfs:comment>
    <rdf:type rdf:resource="http://www.w3.org/2002/07/owl#Class"/>
  </rdf:Description>
  <rdf:Description rdf:about="#FACILITY-TYPE_Mining_installation,_underwater">
    <rdfs:subClassOf rdf:resource="jc3iedm_OBJECT-TYPE.owl#FACILITY-TYPE"/>
    <rdfs:label xml:lang="en">mining installation, underwater</rdfs:label>
    <rdfs:comment xml:lang="en">A facility where materials are extracted from the bottom of a lake, river or sea.</rdfs:comment>
    <rdf:type rdf:resource="http://www.w3.org/2002/07/owl#Class"/>
  </rdf:Description>
  <rdf:Description rdf:about="#CONTROL-FEATURE-TYPE_Positive_identification_radar_advisory_zone">
    <rdfs:subClassOf rdf:resource="jc3iedm_OBJECT-TYPE.owl#CONTROL-FEATURE-TYPE"/>
    <rdfs:label xml:lang="en">positive identification radar advisory zone</rdfs:label>
    <rdfs:comment xml:lang="en">An area within which navy ships separate friendly from hostile aircraft.</rdfs:comment>
    <rdf:type rdf:resource="http://www.w3.org/2002/07/owl#Class"/>
  </rdf:Description>
  <rdf:Description rdf:about="#SURFACE-VESSEL-TYPE_Cruiser,_helicopter_capable">
    <rdfs:subClassOf rdf:resource="jc3iedm_OBJECT-TYPE.owl#SURFACE-VESSEL-TYPE"/>
    <rdfs:label xml:lang="en">cruiser, helicopter capable</rdfs:label>
    <rdfs:comment xml:lang="en">General designator for all cruiser type ships of 140 metres or more, fitted with a flight deck with a primary mission of operating and maintaining helicopters.</rdfs:comment>
    <rdf:type rdf:resource="http://www.w3.org/2002/07/owl#Class"/>
  </rdf:Description>
  <rdf:Description rdf:about="#UNIT-TYPE_Law_enforcement">
    <rdfs:subClassOf rdf:resource="jc3iedm_OBJECT-TYPE.owl#UNIT-TYPE"/>
    <rdfs:label xml:lang="en">law enforcement</rdfs:label>
    <rdfs:comment xml:lang="en">A UNIT-TYPE whose principal designation is the provision of law enforcement services.</rdfs:comment>
    <rdf:type rdf:resource="http://www.w3.org/2002/07/owl#Class"/>
  </rdf:Description>
  <rdf:Description rdf:about="#FACILITY-TYPE_Production_complex,_aircraft">
    <rdfs:subClassOf rdf:resource="jc3iedm_OBJECT-TYPE.owl#FACILITY-TYPE"/>
    <rdfs:label xml:lang="en">production complex, aircraft</rdfs:label>
    <rdfs:comment xml:lang="en">A facility used for aircraft production.</rdfs:comment>
    <rdf:type rdf:resource="http://www.w3.org/2002/07/owl#Class"/>
  </rdf:Description>
  <rdf:Description rdf:about="#MILITARY-OBSTACLE-TYPE_Wire_obstacle,_double_apron_fence">
    <rdfs:subClassOf rdf:resource="jc3iedm_OBJECT-TYPE.owl#MILITARY-OBSTACLE-TYPE"/>
    <rdfs:label xml:lang="en">wire obstacle, double apron fence</rdfs:label>
    <rdfs:comment xml:lang="en">No definition provided in APP-6A.</rdfs:comment>
    <rdf:type rdf:resource="http://www.w3.org/2002/07/owl#Class"/>
  </rdf:Description>
  <rdf:Description rdf:about="#FACILITY-TYPE_Power_transmission_line">
    <rdfs:subClassOf rdf:resource="jc3iedm_OBJECT-TYPE.owl#FACILITY-TYPE"/>
    <rdfs:label xml:lang="en">power transmission line</rdfs:label>
    <rdfs:comment xml:lang="en">A system of above ground wires including their supports, which transmit electricity over distance.</rdfs:comment>
    <rdf:type rdf:resource="http://www.w3.org/2002/07/owl#Class"/>
  </rdf:Description>
  <rdf:Description rdf:about="#ROUTE-TYPE_Great_circle_route">
    <rdfs:subClassOf rdf:resource="jc3iedm_OBJECT-TYPE.owl#ROUTE-TYPE"/>
    <rdfs:label xml:lang="en">great circle route</rdfs:label>
    <rdfs:comment xml:lang="en">The route that follows the shortest arc between two points on the earth's surface.</rdfs:comment>
    <rdf:type rdf:resource="http://www.w3.org/2002/07/owl#Class"/>
  </rdf:Description>
  <rdf:Description rdf:about="#CONTROL-FEATURE-TYPE_Release_point">
    <rdfs:subClassOf rdf:resource="jc3iedm_OBJECT-TYPE.owl#CONTROL-FEATURE-TYPE"/>
    <rdfs:label xml:lang="en">release point</rdfs:label>
    <rdfs:comment xml:lang="en">A well-defined point on a route at which the elements composing a column return under the authority of their respective commanders, each one of these elements continuing its movement toward its own appropriate destination.</rdfs:comment>
    <rdf:type rdf:resource="http://www.w3.org/2002/07/owl#Class"/>
  </rdf:Description>
  <rdf:Description rdf:about="#UNIT-TYPE_Infantry">
    <rdfs:subClassOf rdf:resource="jc3iedm_OBJECT-TYPE.owl#UNIT-TYPE"/>
    <rdfs:label xml:lang="en">infantry</rdfs:label>
    <rdfs:comment xml:lang="en">A UNIT-TYPE whose principal designation is the employment of non-mechanised or lorry-(truck-)borne infantry.</rdfs:comment>
    <rdf:type rdf:resource="http://www.w3.org/2002/07/owl#Class"/>
  </rdf:Description>
  <rdf:Description rdf:about="#ROUTE-TYPE_Transit_route">
    <rdfs:subClassOf rdf:resource="jc3iedm_OBJECT-TYPE.owl#ROUTE-TYPE"/>
    <rdfs:label xml:lang="en">transit route</rdfs:label>
    <rdfs:comment xml:lang="en">A temporary corridor of defined dimensions established in the forward area to minimise the risk to friendly aircraft from friendly air defences or surface forces.</rdfs:comment>
    <rdf:type rdf:resource="http://www.w3.org/2002/07/owl#Class"/>
  </rdf:Description>
  <rdf:Description rdf:about="#SURFACE-VESSEL-TYPE_Merchant_ship,_railroad_car_ferry">
    <rdfs:subClassOf rdf:resource="jc3iedm_OBJECT-TYPE.owl#SURFACE-VESSEL-TYPE"/>
    <rdfs:label xml:lang="en">merchant ship, railroad car ferry</rdfs:label>
    <rdfs:comment xml:lang="en">Non-naval ship or craft designed to ferry railroad cars.</rdfs:comment>
    <rdf:type rdf:resource="http://www.w3.org/2002/07/owl#Class"/>
  </rdf:Description>
  <rdf:Description rdf:about="#MILITARY-POST-TYPE_Approving_authority">
    <rdfs:subClassOf rdf:resource="jc3iedm_OBJECT-TYPE.owl#MILITARY-POST-TYPE"/>
    <rdfs:label xml:lang="en">approving authority</rdfs:label>
    <rdfs:comment xml:lang="en">A MILITARY-POST-TYPE that is identified as the authority with the right and power to approve plans, orders or other official documents.</rdfs:comment>
    <rdf:type rdf:resource="http://www.w3.org/2002/07/owl#Class"/>
  </rdf:Description>
  <rdf:Description rdf:about="#SURFACE-VESSEL-TYPE_Aircraft_carrier,_light">
    <rdfs:subClassOf rdf:resource="jc3iedm_OBJECT-TYPE.owl#SURFACE-VESSEL-TYPE"/>
    <rdfs:label xml:lang="en">aircraft carrier, light</rdfs:label>
    <rdfs:comment xml:lang="en">Designator for multi-role aircraft carriers under a certain tonnage (tbd).</rdfs:comment>
    <rdf:type rdf:resource="http://www.w3.org/2002/07/owl#Class"/>
  </rdf:Description>
  <rdf:Description rdf:about="jc3iedm_OBJECT-TYPE.owl#electronic-equipment-type-category-code">
    <rdf:type rdf:resource="http://www.w3.org/2002/07/owl#DatatypeProperty"/>
    <rdfs:domain rdf:resource="jc3iedm_OBJECT-TYPE.owl#ELECTRONIC-EQUIPMENT-TYPE"/>
    <rdfs:range rdf:resource="http://www.w3.org/2001/XMLSchema#string"/>
  </rdf:Description>
  <rdf:Description rdf:about="jc3iedm_OBJECT-TYPE.owl#cbrn-equipment-type-category-code">
    <rdf:type rdf:resource="http://www.w3.org/2002/07/owl#DatatypeProperty"/>
    <rdfs:domain rdf:resource="jc3iedm_OBJECT-TYPE.owl#CBRN-EQUIPMENT-TYPE"/>
    <rdfs:range rdf:resource="http://www.w3.org/2001/XMLSchema#string"/>
  </rdf:Description>
  <rdf:Description rdf:about="#MILITARY-POST-TYPE_Radiology_physician">
    <rdfs:subClassOf rdf:resource="jc3iedm_OBJECT-TYPE.owl#MILITARY-POST-TYPE"/>
    <rdfs:label xml:lang="en">radiology physician</rdfs:label>
    <rdfs:comment xml:lang="en">A MILITARY-POST-TYPE that is identified as a physician specialising in Radiology.</rdfs:comment>
    <rdf:type rdf:resource="http://www.w3.org/2002/07/owl#Class"/>
  </rdf:Description>
  <rdf:Description rdf:about="#SURFACE-VESSEL-TYPE_Radar_picket_ship,_unarmed">
    <rdfs:subClassOf rdf:resource="jc3iedm_OBJECT-TYPE.owl#SURFACE-VESSEL-TYPE"/>
    <rdfs:label xml:lang="en">radar picket ship, unarmed</rdfs:label>
    <rdfs:comment xml:lang="en">Unarmed surface ship employed for radar picket duty.</rdfs:comment>
    <rdf:type rdf:resource="http://www.w3.org/2002/07/owl#Class"/>
  </rdf:Description>
  <rdf:Description rdf:about="#AIRCRAFT-TYPE_Rotary_wing">
    <rdfs:subClassOf rdf:resource="jc3iedm_OBJECT-TYPE.owl#AIRCRAFT-TYPE"/>
    <rdfs:label xml:lang="en">rotary wing</rdfs:label>
    <rdfs:comment xml:lang="en">A machine or device capable of atmospheric flight and dependent on rotating blades for lift.</rdfs:comment>
    <rdf:type rdf:resource="http://www.w3.org/2002/07/owl#Class"/>
  </rdf:Description>
  <rdf:Description rdf:about="#CHEMICAL-MATERIEL-TYPE_V-agent">
    <rdfs:subClassOf rdf:resource="jc3iedm_OBJECT-TYPE.owl#CHEMICAL-MATERIEL-TYPE"/>
    <rdfs:label xml:lang="en">v agent</rdfs:label>
    <rdfs:comment xml:lang="en">A generic term for a CHEMICAL-MATERIEL-TYPE for a class of nerve agents.</rdfs:comment>
    <rdf:type rdf:resource="http://www.w3.org/2002/07/owl#Class"/>
  </rdf:Description>
  <rdf:Description rdf:about="#CONTROL-FEATURE-TYPE_Coordinating_altitude">
    <rdfs:subClassOf rdf:resource="jc3iedm_OBJECT-TYPE.owl#CONTROL-FEATURE-TYPE"/>
    <rdfs:label xml:lang="en">coordinating altitude</rdfs:label>
    <rdfs:comment xml:lang="en">A procedural airspace control method to separate fixed-and rotary-wing aircraft by determining an altitude below which fixed-wing aircraft will normally not fly and above which rotary-wing aircraft normally will not fly. The coordinating altitude is normally specified in the airspace control plan and may include a buffer zone for small altitude deviations.</rdfs:comment>
    <rdf:type rdf:resource="http://www.w3.org/2002/07/owl#Class"/>
  </rdf:Description>
  <rdf:Description rdf:about="jc3iedm_OBJECT-TYPE.owl#miscellaneous-equipment-type-category-code">
    <rdf:type rdf:resource="http://www.w3.org/2002/07/owl#DatatypeProperty"/>
    <rdfs:domain rdf:resource="jc3iedm_OBJECT-TYPE.owl#MISCELLANEOUS-EQUIPMENT-TYPE"/>
    <rdfs:range rdf:resource="http://www.w3.org/2001/XMLSchema#string"/>
  </rdf:Description>
  <rdf:Description rdf:about="#CONTROL-FEATURE-TYPE_Timing_reference_point">
    <rdfs:subClassOf rdf:resource="jc3iedm_OBJECT-TYPE.owl#CONTROL-FEATURE-TYPE"/>
    <rdfs:label xml:lang="en">timing reference point</rdfs:label>
    <rdfs:comment xml:lang="en">A point used to adjust or control time relative to a known geographical position.</rdfs:comment>
    <rdf:type rdf:resource="http://www.w3.org/2002/07/owl#Class"/>
  </rdf:Description>
  <rdf:Description rdf:about="#SURFACE-VESSEL-TYPE_Fishing_vessel,_training">
    <rdfs:subClassOf rdf:resource="jc3iedm_OBJECT-TYPE.owl#SURFACE-VESSEL-TYPE"/>
    <rdfs:label xml:lang="en">fishing vessel, training</rdfs:label>
    <rdfs:comment xml:lang="en">Vessel used to train personnel in fisheries techniques.</rdfs:comment>
    <rdf:type rdf:resource="http://www.w3.org/2002/07/owl#Class"/>
  </rdf:Description>
  <rdf:Description rdf:about="#SURFACE-VESSEL-TYPE_Frigate,_guided_missile,_helicopter_capable">
    <rdfs:subClassOf rdf:resource="jc3iedm_OBJECT-TYPE.owl#SURFACE-VESSEL-TYPE"/>
    <rdfs:label xml:lang="en">frigate, guided missile, helicopter capable</rdfs:label>
    <rdfs:comment xml:lang="en">A frigate fitted with one or more force guided missile systems and a flight deck with a primary mission of operating and maintaining helicopters. A surface combatant in size range of about 75-150 metres. Fitted primarily to fulfil an ASW role.</rdfs:comment>
    <rdf:type rdf:resource="http://www.w3.org/2002/07/owl#Class"/>
  </rdf:Description>
  <rdf:Description rdf:about="#SURFACE-VESSEL-TYPE_Minelayer,_general">
    <rdfs:subClassOf rdf:resource="jc3iedm_OBJECT-TYPE.owl#SURFACE-VESSEL-TYPE"/>
    <rdfs:label xml:lang="en">minelayer, general</rdfs:label>
    <rdfs:comment xml:lang="en">A ship with a primary mission of laying mines.</rdfs:comment>
    <rdf:type rdf:resource="http://www.w3.org/2002/07/owl#Class"/>
  </rdf:Description>
  <rdf:Description rdf:about="jc3iedm_OBJECT-TYPE.owl#MATERIEL-TYPE">
    <rdf:type rdf:resource="http://www.w3.org/2002/07/owl#Class"/>
    <rdfs:label xml:lang="en">materiel type</rdfs:label>
    <rdfs:comment xml:lang="en">An OBJECT-TYPE that represents equipment, apparatus or supplies of military interest without distinction to its application for administrative or combat purposes.</rdfs:comment>
  </rdf:Description>
  <rdf:Description rdf:about="#MISCELLANEOUS-EQUIPMENT-TYPE_Air-obstruction_lighting">
    <rdfs:subClassOf rdf:resource="jc3iedm_OBJECT-TYPE.owl#MISCELLANEOUS-EQUIPMENT-TYPE"/>
    <rdfs:label xml:lang="en">air obstruction lighting</rdfs:label>
    <rdfs:comment xml:lang="en">A lighting system put on top of a vertical obstacle to air navigation.</rdfs:comment>
    <rdf:type rdf:resource="http://www.w3.org/2002/07/owl#Class"/>
  </rdf:Description>
  <rdf:Description rdf:about="#MISCELLANEOUS-EQUIPMENT-TYPE_Rope">
    <rdfs:subClassOf rdf:resource="jc3iedm_OBJECT-TYPE.owl#MISCELLANEOUS-EQUIPMENT-TYPE"/>
    <rdfs:label xml:lang="en">rope</rdfs:label>
    <rdfs:comment xml:lang="en">A piece of stout cord made of twisted strands of hemp, sisal, cotton, nylon, wire or other similar material.</rdfs:comment>
    <rdf:type rdf:resource="http://www.w3.org/2002/07/owl#Class"/>
  </rdf:Description>
  <rdf:Description rdf:about="#MILITARY-POST-TYPE_Not_otherwise_specified">
    <rdfs:subClassOf rdf:resource="jc3iedm_OBJECT-TYPE.owl#MILITARY-POST-TYPE"/>
    <rdfs:label xml:lang="en">not otherwise specified</rdfs:label>
    <rdfs:comment xml:lang="en">The appropriate value is not in the set of specified values.</rdfs:comment>
    <rdf:type rdf:resource="http://www.w3.org/2002/07/owl#Class"/>
  </rdf:Description>
  <rdf:Description rdf:about="#SURFACE-VESSEL-TYPE_Barge,_water">
    <rdfs:subClassOf rdf:resource="jc3iedm_OBJECT-TYPE.owl#SURFACE-VESSEL-TYPE"/>
    <rdfs:label xml:lang="en">barge, water</rdfs:label>
    <rdfs:comment xml:lang="en">Craft used to transport and store potable water.</rdfs:comment>
    <rdf:type rdf:resource="http://www.w3.org/2002/07/owl#Class"/>
  </rdf:Description>
  <rdf:Description rdf:about="#FACILITY-TYPE_Religious_facility">
    <rdfs:subClassOf rdf:resource="jc3iedm_OBJECT-TYPE.owl#FACILITY-TYPE"/>
    <rdfs:label xml:lang="en">religious facility</rdfs:label>
    <rdfs:comment xml:lang="en">An ecclesiastical facility established for the purpose of worship and prayer.</rdfs:comment>
    <rdf:type rdf:resource="http://www.w3.org/2002/07/owl#Class"/>
  </rdf:Description>
  <rdf:Description rdf:about="#SURFACE-VESSEL-TYPE_Diving_tender">
    <rdfs:subClassOf rdf:resource="jc3iedm_OBJECT-TYPE.owl#SURFACE-VESSEL-TYPE"/>
    <rdfs:label xml:lang="en">diving tender</rdfs:label>
    <rdfs:comment xml:lang="en">Craft usually 40 metres or less equipped to provide support for divers.</rdfs:comment>
    <rdf:type rdf:resource="http://www.w3.org/2002/07/owl#Class"/>
  </rdf:Description>
  <rdf:Description rdf:about="#SURFACE-VESSEL-TYPE_Landing_ship,_general">
    <rdfs:subClassOf rdf:resource="jc3iedm_OBJECT-TYPE.owl#SURFACE-VESSEL-TYPE"/>
    <rdfs:label xml:lang="en">landing ship, general</rdfs:label>
    <rdfs:comment xml:lang="en">General designator for an amphibious landing ship.</rdfs:comment>
    <rdf:type rdf:resource="http://www.w3.org/2002/07/owl#Class"/>
  </rdf:Description>
  <rdf:Description rdf:about="jc3iedm_OBJECT-TYPE.owl#consumable-materiel-type-category-code">
    <rdf:type rdf:resource="http://www.w3.org/2002/07/owl#DatatypeProperty"/>
    <rdfs:domain rdf:resource="jc3iedm_OBJECT-TYPE.owl#CONSUMABLE-MATERIEL-TYPE"/>
    <rdfs:range rdf:resource="http://www.w3.org/2001/XMLSchema#string"/>
  </rdf:Description>
  <rdf:Description rdf:about="#FACILITY-TYPE_Depot,_biological">
    <rdfs:subClassOf rdf:resource="jc3iedm_OBJECT-TYPE.owl#FACILITY-TYPE"/>
    <rdfs:label xml:lang="en">depot, biological</rdfs:label>
    <rdfs:comment xml:lang="en">An area used for the storage of biological agents.</rdfs:comment>
    <rdf:type rdf:resource="http://www.w3.org/2002/07/owl#Class"/>
  </rdf:Description>
  <rdf:Description rdf:about="#SUBSURFACE-VESSEL-TYPE_Submarine,_auxiliary">
    <rdfs:subClassOf rdf:resource="jc3iedm_OBJECT-TYPE.owl#SUBSURFACE-VESSEL-TYPE"/>
    <rdfs:label xml:lang="en">submarine, auxiliary</rdfs:label>
    <rdfs:comment xml:lang="en">Submarine used mainly in a non-combatant role which has at least a residual combat capability.</rdfs:comment>
    <rdf:type rdf:resource="http://www.w3.org/2002/07/owl#Class"/>
  </rdf:Description>
  <rdf:Description rdf:about="#VEHICLE-TYPE_Battle_tank,_light_recovery">
    <rdfs:subClassOf rdf:resource="jc3iedm_OBJECT-TYPE.owl#VEHICLE-TYPE"/>
    <rdfs:label xml:lang="en">battle tank, light recovery</rdfs:label>
    <rdfs:comment xml:lang="en">A vehicle designed to recover light weight battle tanks.</rdfs:comment>
    <rdf:type rdf:resource="http://www.w3.org/2002/07/owl#Class"/>
  </rdf:Description>
  <rdf:Description rdf:about="#CONTROL-FEATURE-TYPE_Impact_point">
    <rdfs:subClassOf rdf:resource="jc3iedm_OBJECT-TYPE.owl#CONTROL-FEATURE-TYPE"/>
    <rdfs:label xml:lang="en">impact point</rdfs:label>
    <rdfs:comment xml:lang="en">1. The point on the drop zone where the first parachutist or air dropped cargo item lands or is expected to land. See FM 90-26. 2. The point at which a projectile, bomb, or re-entry vehicle impacts or is expected to impact.</rdfs:comment>
    <rdf:type rdf:resource="http://www.w3.org/2002/07/owl#Class"/>
  </rdf:Description>
  <rdf:Description rdf:about="#MARITIME-EQUIPMENT-TYPE_Mechanical_influence">
    <rdfs:subClassOf rdf:resource="jc3iedm_OBJECT-TYPE.owl#MARITIME-EQUIPMENT-TYPE"/>
    <rdfs:label xml:lang="en">mechanical influence</rdfs:label>
    <rdfs:comment xml:lang="en">Equipment designed to locate the mine by operating the magnetic firing system of a mine.</rdfs:comment>
    <rdf:type rdf:resource="http://www.w3.org/2002/07/owl#Class"/>
  </rdf:Description>
  <rdf:Description rdf:about="#ORGANISATION-TYPE_Control_and_reporting_post">
    <rdfs:subClassOf rdf:resource="jc3iedm_OBJECT-TYPE.owl#ORGANISATION-TYPE"/>
    <rdfs:label xml:lang="en">control and reporting post</rdfs:label>
    <rdfs:comment xml:lang="en">No definition provided in ADatP-3 Baseline 13.1 FFIRN/FUD 1874/4.</rdfs:comment>
    <rdf:type rdf:resource="http://www.w3.org/2002/07/owl#Class"/>
  </rdf:Description>
  <rdf:Description rdf:about="#AMMUNITION-TYPE_Mine,_seabed_-_explosive_charge_less_than_500kg">
    <rdfs:subClassOf rdf:resource="jc3iedm_OBJECT-TYPE.owl#AMMUNITION-TYPE"/>
    <rdfs:label xml:lang="en">mine, seabed   explosive charge less than 500kg</rdfs:label>
    <rdfs:comment xml:lang="en">A mine with negative buoyancy which remains on the seabed with explosive charge less than 500kg.</rdfs:comment>
    <rdf:type rdf:resource="http://www.w3.org/2002/07/owl#Class"/>
  </rdf:Description>
  <rdf:Description rdf:about="#ORGANISATION-TYPE_Tactical_operations_centre">
    <rdfs:subClassOf rdf:resource="jc3iedm_OBJECT-TYPE.owl#ORGANISATION-TYPE"/>
    <rdfs:label xml:lang="en">tactical operations centre</rdfs:label>
    <rdfs:comment xml:lang="en">A physical grouping of those elements of general and special staff concerned with the current tactical operations and the tactical support thereof.</rdfs:comment>
    <rdf:type rdf:resource="http://www.w3.org/2002/07/owl#Class"/>
  </rdf:Description>
  <rdf:Description rdf:about="#MISCELLANEOUS-EQUIPMENT-TYPE_Beacon,_light">
    <rdfs:subClassOf rdf:resource="jc3iedm_OBJECT-TYPE.owl#MISCELLANEOUS-EQUIPMENT-TYPE"/>
    <rdfs:label xml:lang="en">beacon, light</rdfs:label>
    <rdfs:comment xml:lang="en">A light that is used for the determination of bearings, courses, or locations.</rdfs:comment>
    <rdf:type rdf:resource="http://www.w3.org/2002/07/owl#Class"/>
  </rdf:Description>
  <rdf:Description rdf:about="jc3iedm_OBJECT-TYPE.owl#FACILITY-TYPE">
    <rdf:type rdf:resource="http://www.w3.org/2002/07/owl#Class"/>
    <rdfs:label xml:lang="en">facility type</rdfs:label>
    <rdfs:comment xml:lang="en">An OBJECT-TYPE that is intended to be built, installed or established to serve some particular purpose and is identified by the service it is intended to provide rather than by its content.</rdfs:comment>
  </rdf:Description>
  <rdf:Description rdf:about="#SURFACE-VESSEL-TYPE_Oil_recovery_vessel">
    <rdfs:subClassOf rdf:resource="jc3iedm_OBJECT-TYPE.owl#SURFACE-VESSEL-TYPE"/>
    <rdfs:label xml:lang="en">oil recovery vessel</rdfs:label>
    <rdfs:comment xml:lang="en">A vessel specifically designed for pollution control/oil recovery operations.</rdfs:comment>
    <rdf:type rdf:resource="http://www.w3.org/2002/07/owl#Class"/>
  </rdf:Description>
  <rdf:Description rdf:about="jc3iedm_OBJECT-TYPE.owl#facility-type-category-code">
    <rdf:type rdf:resource="http://www.w3.org/2002/07/owl#DatatypeProperty"/>
    <rdfs:domain rdf:resource="jc3iedm_OBJECT-TYPE.owl#FACILITY-TYPE"/>
    <rdfs:range rdf:resource="http://www.w3.org/2001/XMLSchema#string"/>
  </rdf:Description>
  <rdf:Description rdf:about="#ENGINEERING-EQUIPMENT-TYPE_Mechanised_bridge_layer">
    <rdfs:subClassOf rdf:resource="jc3iedm_OBJECT-TYPE.owl#ENGINEERING-EQUIPMENT-TYPE"/>
    <rdfs:label xml:lang="en">mechanised bridge layer</rdfs:label>
    <rdfs:comment xml:lang="en">A tracked vehicle designed to carry and lay a removable bridge.</rdfs:comment>
    <rdf:type rdf:resource="http://www.w3.org/2002/07/owl#Class"/>
  </rdf:Description>
  <rdf:Description rdf:about="jc3iedm_OBJECT-TYPE.owl#private-sector-organisation-type-category-code">
    <rdf:type rdf:resource="http://www.w3.org/2002/07/owl#DatatypeProperty"/>
    <rdfs:domain rdf:resource="jc3iedm_OBJECT-TYPE.owl#PRIVATE-SECTOR-ORGANISATION-TYPE"/>
    <rdfs:range rdf:resource="http://www.w3.org/2001/XMLSchema#string"/>
  </rdf:Description>
  <rdf:Description rdf:about="#SURFACE-VESSEL-TYPE_Merchant_ship,_icebreaker">
    <rdfs:subClassOf rdf:resource="jc3iedm_OBJECT-TYPE.owl#SURFACE-VESSEL-TYPE"/>
    <rdfs:label xml:lang="en">merchant ship, icebreaker</rdfs:label>
    <rdfs:comment xml:lang="en">Non-naval ship used primarily for icebreaking.</rdfs:comment>
    <rdf:type rdf:resource="http://www.w3.org/2002/07/owl#Class"/>
  </rdf:Description>
  <rdf:Description rdf:about="#CONTROL-FEATURE-TYPE_Boundary_point">
    <rdfs:subClassOf rdf:resource="jc3iedm_OBJECT-TYPE.owl#CONTROL-FEATURE-TYPE"/>
    <rdfs:label xml:lang="en">boundary point</rdfs:label>
    <rdfs:comment xml:lang="en">A point on a boundary.</rdfs:comment>
    <rdf:type rdf:resource="http://www.w3.org/2002/07/owl#Class"/>
  </rdf:Description>
  <rdf:Description rdf:about="#SURFACE-VESSEL-TYPE_Fire_tug">
    <rdfs:subClassOf rdf:resource="jc3iedm_OBJECT-TYPE.owl#SURFACE-VESSEL-TYPE"/>
    <rdfs:label xml:lang="en">fire tug</rdfs:label>
    <rdfs:comment xml:lang="en">Coastal/harbour tug operated by customs fire service, between 30-40 metres with total horsepower of 1300 or more.</rdfs:comment>
    <rdf:type rdf:resource="http://www.w3.org/2002/07/owl#Class"/>
  </rdf:Description>
  <rdf:Description rdf:about="#CONTROL-FEATURE-TYPE_Assault_position">
    <rdfs:subClassOf rdf:resource="jc3iedm_OBJECT-TYPE.owl#CONTROL-FEATURE-TYPE"/>
    <rdfs:label xml:lang="en">assault position</rdfs:label>
    <rdfs:comment xml:lang="en">That position between the line of departure (LD) and the objective in an attack from which forces assault the objective. Ideally, it is the last covered and concealed position before reaching the objective.</rdfs:comment>
    <rdf:type rdf:resource="http://www.w3.org/2002/07/owl#Class"/>
  </rdf:Description>
  <rdf:Description rdf:about="#VEHICLE-TYPE_Forklift">
    <rdfs:subClassOf rdf:resource="jc3iedm_OBJECT-TYPE.owl#VEHICLE-TYPE"/>
    <rdfs:label xml:lang="en">forklift</rdfs:label>
    <rdfs:comment xml:lang="en">A vehicle with a horizontal fork in front for lifting and carrying loads.</rdfs:comment>
    <rdf:type rdf:resource="http://www.w3.org/2002/07/owl#Class"/>
  </rdf:Description>
  <rdf:Description rdf:about="#AMMUNITION-TYPE_Rocket/missile,_heavy">
    <rdfs:subClassOf rdf:resource="jc3iedm_OBJECT-TYPE.owl#AMMUNITION-TYPE"/>
    <rdfs:label xml:lang="en">rocket/missile, heavy</rdfs:label>
    <rdfs:comment xml:lang="en">A powered projectile designed for use by heavy launchers.</rdfs:comment>
    <rdf:type rdf:resource="http://www.w3.org/2002/07/owl#Class"/>
  </rdf:Description>
  <rdf:Description rdf:about="#FACILITY-TYPE_Field_storage_module-ammunition">
    <rdfs:subClassOf rdf:resource="jc3iedm_OBJECT-TYPE.owl#FACILITY-TYPE"/>
    <rdfs:label xml:lang="en">field storage module ammunition</rdfs:label>
    <rdfs:comment xml:lang="en">A facility that is a site containing approximately 10 tonnes gross weight of ammunition and explosives.</rdfs:comment>
    <rdf:type rdf:resource="http://www.w3.org/2002/07/owl#Class"/>
  </rdf:Description>
  <rdf:Description rdf:about="#CONTROL-FEATURE-TYPE_Air_axis_of_advance">
    <rdfs:subClassOf rdf:resource="jc3iedm_OBJECT-TYPE.owl#CONTROL-FEATURE-TYPE"/>
    <rdfs:label xml:lang="en">air axis of advance</rdfs:label>
    <rdfs:comment xml:lang="en">A general air corridor of advance, which extends towards the enemy. An air axis of advance symbol graphically portrays a commander’s air manoeuvre intention, such as avoidance air defence coverage or envelopment of an enemy force. It follows an axis suitable for the airmobile force to which the axis was assigned. An air axis of advance does not directly control or use terrain.</rdfs:comment>
    <rdf:type rdf:resource="http://www.w3.org/2002/07/owl#Class"/>
  </rdf:Description>
  <rdf:Description rdf:about="#FACILITY-TYPE_Railhead">
    <rdfs:subClassOf rdf:resource="jc3iedm_OBJECT-TYPE.owl#FACILITY-TYPE"/>
    <rdfs:label xml:lang="en">railhead</rdfs:label>
    <rdfs:comment xml:lang="en">The point on a railway from which branch-line or road transport of supplies begins.</rdfs:comment>
    <rdf:type rdf:resource="http://www.w3.org/2002/07/owl#Class"/>
  </rdf:Description>
  <rdf:Description rdf:about="#SURFACE-VESSEL-TYPE_Merchant_ship,_heavy_lift">
    <rdfs:subClassOf rdf:resource="jc3iedm_OBJECT-TYPE.owl#SURFACE-VESSEL-TYPE"/>
    <rdfs:label xml:lang="en">merchant ship, heavy lift</rdfs:label>
    <rdfs:comment xml:lang="en">Non-naval ship fitted with heavy duty crane or derrick for heavy lift.</rdfs:comment>
    <rdf:type rdf:resource="http://www.w3.org/2002/07/owl#Class"/>
  </rdf:Description>
  <rdf:Description rdf:about="#SURFACE-VESSEL-TYPE_Salvage_ship,_lifting">
    <rdfs:subClassOf rdf:resource="jc3iedm_OBJECT-TYPE.owl#SURFACE-VESSEL-TYPE"/>
    <rdfs:label xml:lang="en">salvage ship, lifting</rdfs:label>
    <rdfs:comment xml:lang="en">Ship at least 40 metres used to provide mobile salvage, repairs, diving and rescue services, must have heavy lifting capability.</rdfs:comment>
    <rdf:type rdf:resource="http://www.w3.org/2002/07/owl#Class"/>
  </rdf:Description>
  <rdf:Description rdf:about="#FACILITY-TYPE_Dry-dock">
    <rdfs:subClassOf rdf:resource="jc3iedm_OBJECT-TYPE.owl#FACILITY-TYPE"/>
    <rdfs:label xml:lang="en">dry dock</rdfs:label>
    <rdfs:comment xml:lang="en">A FACILITY-TYPE that provides an enclosure for maintenance, building or repairing ships, from which water can be pumped out.</rdfs:comment>
    <rdf:type rdf:resource="http://www.w3.org/2002/07/owl#Class"/>
  </rdf:Description>
  <rdf:Description rdf:about="#SURFACE-VESSEL-TYPE_Buoy_tender">
    <rdfs:subClassOf rdf:resource="jc3iedm_OBJECT-TYPE.owl#SURFACE-VESSEL-TYPE"/>
    <rdfs:label xml:lang="en">buoy tender</rdfs:label>
    <rdfs:comment xml:lang="en">Ship 40 metres or more employed for the placing and tending of buoys and aids to navigation in coastal and adjoining waters.</rdfs:comment>
    <rdf:type rdf:resource="http://www.w3.org/2002/07/owl#Class"/>
  </rdf:Description>
  <rdf:Description rdf:about="#SURFACE-VESSEL-TYPE_Barge,_fuel_oil">
    <rdfs:subClassOf rdf:resource="jc3iedm_OBJECT-TYPE.owl#SURFACE-VESSEL-TYPE"/>
    <rdfs:label xml:lang="en">barge, fuel oil</rdfs:label>
    <rdfs:comment xml:lang="en">Craft of any design 60 metres or less used to store and transport POL products.</rdfs:comment>
    <rdf:type rdf:resource="http://www.w3.org/2002/07/owl#Class"/>
  </rdf:Description>
  <rdf:Description rdf:about="#AMMUNITION-TYPE_Mortar_bomb">
    <rdfs:subClassOf rdf:resource="jc3iedm_OBJECT-TYPE.owl#AMMUNITION-TYPE"/>
    <rdfs:label xml:lang="en">mortar bomb</rdfs:label>
    <rdfs:comment xml:lang="en">A round fired from a mortar weapon.</rdfs:comment>
    <rdf:type rdf:resource="http://www.w3.org/2002/07/owl#Class"/>
  </rdf:Description>
  <rdf:Description rdf:about="#AMMUNITION-TYPE_Not_otherwise_specified">
    <rdfs:subClassOf rdf:resource="jc3iedm_OBJECT-TYPE.owl#AMMUNITION-TYPE"/>
    <rdfs:label xml:lang="en">not otherwise specified</rdfs:label>
    <rdfs:comment xml:lang="en">The appropriate value is not in the set of specified values.</rdfs:comment>
    <rdf:type rdf:resource="http://www.w3.org/2002/07/owl#Class"/>
  </rdf:Description>
  <rdf:Description rdf:about="#SURFACE-VESSEL-TYPE_Minesweeper,_fleet">
    <rdfs:subClassOf rdf:resource="jc3iedm_OBJECT-TYPE.owl#SURFACE-VESSEL-TYPE"/>
    <rdfs:label xml:lang="en">minesweeper, fleet</rdfs:label>
    <rdfs:comment xml:lang="en">Minesweeper in size range 46 metres or more that cannot be regarded as being non-magnetic.</rdfs:comment>
    <rdf:type rdf:resource="http://www.w3.org/2002/07/owl#Class"/>
  </rdf:Description>
  <rdf:Description rdf:about="#FACILITY-TYPE_Ford,_concrete_lined_bed">
    <rdfs:subClassOf rdf:resource="jc3iedm_OBJECT-TYPE.owl#FACILITY-TYPE"/>
    <rdfs:label xml:lang="en">ford, concrete lined bed</rdfs:label>
    <rdfs:comment xml:lang="en">A shallow place in a river or other water marked with a concrete-lined bed that can be crossed without bridging, boats, or rafts.</rdfs:comment>
    <rdf:type rdf:resource="http://www.w3.org/2002/07/owl#Class"/>
  </rdf:Description>
  <rdf:Description rdf:about="#UNIT-TYPE_Logistics">
    <rdfs:subClassOf rdf:resource="jc3iedm_OBJECT-TYPE.owl#UNIT-TYPE"/>
    <rdfs:label xml:lang="en">logistics</rdfs:label>
    <rdfs:comment xml:lang="en">A UNIT-TYPE whose principal designation is the planning and support of the movement and maintenance of forces.</rdfs:comment>
    <rdf:type rdf:resource="http://www.w3.org/2002/07/owl#Class"/>
  </rdf:Description>
  <rdf:Description rdf:about="jc3iedm_OBJECT-TYPE.owl#equipment-type-maximum-length-dimension">
    <rdf:type rdf:resource="http://www.w3.org/2002/07/owl#DatatypeProperty"/>
    <rdfs:domain rdf:resource="jc3iedm_OBJECT-TYPE.owl#EQUIPMENT-TYPE"/>
  </rdf:Description>
  <rdf:Description rdf:about="#FACILITY-TYPE_Shipyard">
    <rdfs:subClassOf rdf:resource="jc3iedm_OBJECT-TYPE.owl#FACILITY-TYPE"/>
    <rdfs:label xml:lang="en">shipyard</rdfs:label>
    <rdfs:comment xml:lang="en">A large enclosure, adjoining the sea or a river, in which ships are built, repaired or maintained.</rdfs:comment>
    <rdf:type rdf:resource="http://www.w3.org/2002/07/owl#Class"/>
  </rdf:Description>
  <rdf:Description rdf:about="#SURFACE-VESSEL-TYPE_Landing_craft,_personnel,_armoured">
    <rdfs:subClassOf rdf:resource="jc3iedm_OBJECT-TYPE.owl#SURFACE-VESSEL-TYPE"/>
    <rdfs:label xml:lang="en">landing craft, personnel, armoured</rdfs:label>
    <rdfs:comment xml:lang="en">Landing craft in size range 7.5-30 metres overall suitable only for carrying personnel. May be fast and/or ramped and armoured for protection.</rdfs:comment>
    <rdf:type rdf:resource="http://www.w3.org/2002/07/owl#Class"/>
  </rdf:Description>
  <rdf:Description rdf:about="#CONTROL-FEATURE-TYPE_Target_location">
    <rdfs:subClassOf rdf:resource="jc3iedm_OBJECT-TYPE.owl#CONTROL-FEATURE-TYPE"/>
    <rdfs:label xml:lang="en">target location</rdfs:label>
    <rdfs:comment xml:lang="en">A designated location that is expected to contain a target or targets.</rdfs:comment>
    <rdf:type rdf:resource="http://www.w3.org/2002/07/owl#Class"/>
  </rdf:Description>
  <rdf:Description rdf:about="#FACILITY-TYPE_Village">
    <rdfs:subClassOf rdf:resource="jc3iedm_OBJECT-TYPE.owl#FACILITY-TYPE"/>
    <rdfs:label xml:lang="en">village</rdfs:label>
    <rdfs:comment xml:lang="en">A group of houses and associated buildings, larger than a hamlet and smaller than a town, especially in a rural area.</rdfs:comment>
    <rdf:type rdf:resource="http://www.w3.org/2002/07/owl#Class"/>
  </rdf:Description>
  <rdf:Description rdf:about="#CONTROL-FEATURE-TYPE_Final_coordination_line">
    <rdfs:subClassOf rdf:resource="jc3iedm_OBJECT-TYPE.owl#CONTROL-FEATURE-TYPE"/>
    <rdfs:label xml:lang="en">final coordination line</rdfs:label>
    <rdfs:comment xml:lang="en">A line close to the enemy position used to coordinate the lifting and/or shifting of supporting fires with the final deployment of manoeuvre elements. It should be recognisable on the ground. It is not a fire support coordination measure.</rdfs:comment>
    <rdf:type rdf:resource="http://www.w3.org/2002/07/owl#Class"/>
  </rdf:Description>
  <rdf:Description rdf:about="jc3iedm_OBJECT-TYPE.owl#consumable-materiel-type-issuing-weight-quantity">
    <rdf:type rdf:resource="http://www.w3.org/2002/07/owl#DatatypeProperty"/>
    <rdfs:domain rdf:resource="jc3iedm_OBJECT-TYPE.owl#CONSUMABLE-MATERIEL-TYPE"/>
  </rdf:Description>
  <rdf:Description rdf:about="#GROUP-ORGANISATION-TYPE_Police_chief">
    <rdfs:subClassOf rdf:resource="jc3iedm_OBJECT-TYPE.owl#GROUP-ORGANISATION-TYPE"/>
    <rdfs:label xml:lang="en">police chief</rdfs:label>
    <rdfs:comment xml:lang="en">A GROUP-ORGANISATION-TYPE that comprises persons that have the responsibility for the regulation, discipline, and control of a community for the enforcement of law and public order.</rdfs:comment>
    <rdf:type rdf:resource="http://www.w3.org/2002/07/owl#Class"/>
  </rdf:Description>
  <rdf:Description rdf:about="jc3iedm_OBJECT-TYPE.owl#weapon-type-fire-guidance-indicator-code">
    <rdf:type rdf:resource="http://www.w3.org/2002/07/owl#DatatypeProperty"/>
    <rdfs:domain rdf:resource="jc3iedm_OBJECT-TYPE.owl#WEAPON-TYPE"/>
    <rdfs:range rdf:resource="http://www.w3.org/2001/XMLSchema#string"/>
  </rdf:Description>
  <rdf:Description rdf:about="#FACILITY-TYPE_Medical_facility">
    <rdfs:subClassOf rdf:resource="jc3iedm_OBJECT-TYPE.owl#FACILITY-TYPE"/>
    <rdfs:label xml:lang="en">medical facility</rdfs:label>
    <rdfs:comment xml:lang="en">A facility used as a medical facility.</rdfs:comment>
    <rdf:type rdf:resource="http://www.w3.org/2002/07/owl#Class"/>
  </rdf:Description>
  <rdf:Description rdf:about="#MISCELLANEOUS-EQUIPMENT-TYPE_Signal_light">
    <rdfs:subClassOf rdf:resource="jc3iedm_OBJECT-TYPE.owl#MISCELLANEOUS-EQUIPMENT-TYPE"/>
    <rdfs:label xml:lang="en">signal light</rdfs:label>
    <rdfs:comment xml:lang="en">A light source designed to be used for communication using a predefined code system of on and off flashes.</rdfs:comment>
    <rdf:type rdf:resource="http://www.w3.org/2002/07/owl#Class"/>
  </rdf:Description>
  <rdf:Description rdf:about="#SURFACE-VESSEL-TYPE_Special_liquid_ship">
    <rdfs:subClassOf rdf:resource="jc3iedm_OBJECT-TYPE.owl#SURFACE-VESSEL-TYPE"/>
    <rdfs:label xml:lang="en">special liquid ship</rdfs:label>
    <rdfs:comment xml:lang="en">Ship 40 metres or more designed to transport a special kind of propellant or other non-nuclear associated liquid cargo.</rdfs:comment>
    <rdf:type rdf:resource="http://www.w3.org/2002/07/owl#Class"/>
  </rdf:Description>
  <rdf:Description rdf:about="#RADIOACTIVE-MATERIEL-TYPE_Fresh_reactor_fuel">
    <rdfs:subClassOf rdf:resource="jc3iedm_OBJECT-TYPE.owl#RADIOACTIVE-MATERIEL-TYPE"/>
    <rdfs:label xml:lang="en">fresh reactor fuel</rdfs:label>
    <rdfs:comment xml:lang="en">Nuclear reactor fuel that has not yet been used in a live nuclear reactor.</rdfs:comment>
    <rdf:type rdf:resource="http://www.w3.org/2002/07/owl#Class"/>
  </rdf:Description>
  <rdf:Description rdf:about="#FACILITY-TYPE_Combat_outpost">
    <rdfs:subClassOf rdf:resource="jc3iedm_OBJECT-TYPE.owl#FACILITY-TYPE"/>
    <rdfs:label xml:lang="en">combat outpost</rdfs:label>
    <rdfs:comment xml:lang="en">A reinforced observation post capable of conducting limited combat operations.</rdfs:comment>
    <rdf:type rdf:resource="http://www.w3.org/2002/07/owl#Class"/>
  </rdf:Description>
  <rdf:Description rdf:about="jc3iedm_OBJECT-TYPE.owl#materiel-type-category-code">
    <rdf:type rdf:resource="http://www.w3.org/2002/07/owl#DatatypeProperty"/>
    <rdfs:domain rdf:resource="jc3iedm_OBJECT-TYPE.owl#MATERIEL-TYPE"/>
    <rdfs:range rdf:resource="http://www.w3.org/2001/XMLSchema#string"/>
  </rdf:Description>
  <rdf:Description rdf:about="#FEATURE-TYPE_Meteorologic_feature_type">
    <rdfs:subClassOf rdf:resource="jc3iedm_OBJECT-TYPE.owl#FEATURE-TYPE"/>
    <rdfs:label xml:lang="en">meteorologic feature type</rdfs:label>
    <rdfs:comment xml:lang="en">A FEATURE-TYPE that describes reported or forecast weather and light conditions.</rdfs:comment>
    <rdf:type rdf:resource="http://www.w3.org/2002/07/owl#Class"/>
  </rdf:Description>
  <rdf:Description rdf:about="#ENGINEERING-EQUIPMENT-TYPE_Construction_vehicle">
    <rdfs:subClassOf rdf:resource="jc3iedm_OBJECT-TYPE.owl#ENGINEERING-EQUIPMENT-TYPE"/>
    <rdfs:label xml:lang="en">construction vehicle</rdfs:label>
    <rdfs:comment xml:lang="en">A vehicle generally used in the construction trade.</rdfs:comment>
    <rdf:type rdf:resource="http://www.w3.org/2002/07/owl#Class"/>
  </rdf:Description>
  <rdf:Description rdf:about="#HARBOUR-TYPE_River_(Natural)">
    <rdfs:subClassOf rdf:resource="jc3iedm_OBJECT-TYPE.owl#HARBOUR-TYPE"/>
    <rdfs:label xml:lang="en">river (natural)</rdfs:label>
    <rdfs:comment xml:lang="en">A harbour located on a river, the waters of which are not retained by any artificial means. The facilities may consist of quays or wharves parallel to the banks of the stream, or piers or jetties, which extend into the stream.</rdfs:comment>
    <rdf:type rdf:resource="http://www.w3.org/2002/07/owl#Class"/>
  </rdf:Description>
  <rdf:Description rdf:about="#MILITARY-POST-TYPE_Sapper">
    <rdfs:subClassOf rdf:resource="jc3iedm_OBJECT-TYPE.owl#MILITARY-POST-TYPE"/>
    <rdfs:label xml:lang="en">sapper</rdfs:label>
    <rdfs:comment xml:lang="en">A MILITARY-POST-TYPE that is identified as one who designs and constructs military works for attack or defence.</rdfs:comment>
    <rdf:type rdf:resource="http://www.w3.org/2002/07/owl#Class"/>
  </rdf:Description>
  <rdf:Description rdf:about="#GROUP-ORGANISATION-TYPE_Local_inhabitant">
    <rdfs:subClassOf rdf:resource="jc3iedm_OBJECT-TYPE.owl#GROUP-ORGANISATION-TYPE"/>
    <rdfs:label xml:lang="en">local inhabitant</rdfs:label>
    <rdfs:comment xml:lang="en">A GROUP-ORGANISATION-TYPE of a particular place regarded with reference to that place.</rdfs:comment>
    <rdf:type rdf:resource="http://www.w3.org/2002/07/owl#Class"/>
  </rdf:Description>
  <rdf:Description rdf:about="#FACILITY-TYPE_Transport_facility">
    <rdfs:subClassOf rdf:resource="jc3iedm_OBJECT-TYPE.owl#FACILITY-TYPE"/>
    <rdfs:label xml:lang="en">transport facility</rdfs:label>
    <rdfs:comment xml:lang="en">A facility that is used to support transport functions.</rdfs:comment>
    <rdf:type rdf:resource="http://www.w3.org/2002/07/owl#Class"/>
  </rdf:Description>
  <rdf:Description rdf:about="#SURFACE-VESSEL-TYPE_Service_ship,_torpedo/target">
    <rdfs:subClassOf rdf:resource="jc3iedm_OBJECT-TYPE.owl#SURFACE-VESSEL-TYPE"/>
    <rdfs:label xml:lang="en">service ship, torpedo/target</rdfs:label>
    <rdfs:comment xml:lang="en">Ship employed in servicing torpedoes and sub-surface targets.</rdfs:comment>
    <rdf:type rdf:resource="http://www.w3.org/2002/07/owl#Class"/>
  </rdf:Description>
  <rdf:Description rdf:about="#FACILITY-TYPE_Naval_air_station">
    <rdfs:subClassOf rdf:resource="jc3iedm_OBJECT-TYPE.owl#FACILITY-TYPE"/>
    <rdfs:label xml:lang="en">naval air station</rdfs:label>
    <rdfs:comment xml:lang="en">A Naval facility that is used by and provides services for naval or other aviation units or organisations.</rdfs:comment>
    <rdf:type rdf:resource="http://www.w3.org/2002/07/owl#Class"/>
  </rdf:Description>
  <rdf:Description rdf:about="#UNIT-TYPE_Aviation,_fixed_wing">
    <rdfs:subClassOf rdf:resource="jc3iedm_OBJECT-TYPE.owl#UNIT-TYPE"/>
    <rdfs:label xml:lang="en">aviation, fixed wing</rdfs:label>
    <rdfs:comment xml:lang="en">A UNIT-TYPE whose designation indicates employment of fixed-wing assets in the air regime.</rdfs:comment>
    <rdf:type rdf:resource="http://www.w3.org/2002/07/owl#Class"/>
  </rdf:Description>
  <rdf:Description rdf:about="#CONTROL-FEATURE-TYPE_Obstacle_gap">
    <rdfs:subClassOf rdf:resource="jc3iedm_OBJECT-TYPE.owl#CONTROL-FEATURE-TYPE"/>
    <rdfs:label xml:lang="en">obstacle gap</rdfs:label>
    <rdfs:comment xml:lang="en">An area within a minefield or obstacle belt, free of live mines or obstacles, whose width and direction will allow a friendly force to pass through in tactical formation.</rdfs:comment>
    <rdf:type rdf:resource="http://www.w3.org/2002/07/owl#Class"/>
  </rdf:Description>
  <rdf:Description rdf:about="#FACILITY-TYPE_Military_materiel_facility,_chemical_and_biological_warfare_production">
    <rdfs:subClassOf rdf:resource="jc3iedm_OBJECT-TYPE.owl#FACILITY-TYPE"/>
    <rdfs:label xml:lang="en">military materiel facility, chemical and biological warfare production</rdfs:label>
    <rdfs:comment xml:lang="en">A facility used as for chemical and biological warfare production.</rdfs:comment>
    <rdf:type rdf:resource="http://www.w3.org/2002/07/owl#Class"/>
  </rdf:Description>
  <rdf:Description rdf:about="#CONTROL-FEATURE-TYPE_Prohibited_area">
    <rdfs:subClassOf rdf:resource="jc3iedm_OBJECT-TYPE.owl#CONTROL-FEATURE-TYPE"/>
    <rdfs:label xml:lang="en">prohibited area</rdfs:label>
    <rdfs:comment xml:lang="en">An airspace of defined dimensions, above the land areas or territorial waters of a state within which the flight of aircraft is prohibited.</rdfs:comment>
    <rdf:type rdf:resource="http://www.w3.org/2002/07/owl#Class"/>
  </rdf:Description>
  <rdf:Description rdf:about="jc3iedm_OBJECT-TYPE.owl#vessel-type-category-code">
    <rdf:type rdf:resource="http://www.w3.org/2002/07/owl#DatatypeProperty"/>
    <rdfs:domain rdf:resource="jc3iedm_OBJECT-TYPE.owl#VESSEL-TYPE"/>
    <rdfs:range rdf:resource="http://www.w3.org/2001/XMLSchema#string"/>
  </rdf:Description>
  <rdf:Description rdf:about="#ENGINEERING-EQUIPMENT-TYPE_Mine_layer">
    <rdfs:subClassOf rdf:resource="jc3iedm_OBJECT-TYPE.owl#ENGINEERING-EQUIPMENT-TYPE"/>
    <rdfs:label xml:lang="en">mine layer</rdfs:label>
    <rdfs:comment xml:lang="en">A vehicle whose purpose is to lay mines.</rdfs:comment>
    <rdf:type rdf:resource="http://www.w3.org/2002/07/owl#Class"/>
  </rdf:Description>
  <rdf:Description rdf:about="#AMMUNITION-TYPE_Not_known">
    <rdfs:subClassOf rdf:resource="jc3iedm_OBJECT-TYPE.owl#AMMUNITION-TYPE"/>
    <rdfs:label xml:lang="en">not known</rdfs:label>
    <rdfs:comment xml:lang="en">It is not possible to determine which value is most applicable.</rdfs:comment>
    <rdf:type rdf:resource="http://www.w3.org/2002/07/owl#Class"/>
  </rdf:Description>
  <rdf:Description rdf:about="#SURFACE-VESSEL-TYPE_Corvette,_coast_guard">
    <rdfs:subClassOf rdf:resource="jc3iedm_OBJECT-TYPE.owl#SURFACE-VESSEL-TYPE"/>
    <rdfs:label xml:lang="en">corvette, coast guard</rdfs:label>
    <rdfs:comment xml:lang="en">General designator for frigate. A coast guard surface combatant in size range of about 75-150 metres, fitted primarily to fulfil an ASW role.</rdfs:comment>
    <rdf:type rdf:resource="http://www.w3.org/2002/07/owl#Class"/>
  </rdf:Description>
  <rdf:Description rdf:about="#CONTROL-FEATURE-TYPE_Linkup_point">
    <rdfs:subClassOf rdf:resource="jc3iedm_OBJECT-TYPE.owl#CONTROL-FEATURE-TYPE"/>
    <rdfs:label xml:lang="en">linkup point</rdfs:label>
    <rdfs:comment xml:lang="en">An easily recognisable point location on the ground where two forces conducting a linkup meet. When one force is stationary, linkup points normally are established where the moving force's routes of advance intersect the stationary force's security elements. Linkup points for two moving forces are established on boundaries where the two forces are expected to converge.</rdfs:comment>
    <rdf:type rdf:resource="http://www.w3.org/2002/07/owl#Class"/>
  </rdf:Description>
  <rdf:Description rdf:about="#SURFACE-VESSEL-TYPE_Barge,_target">
    <rdfs:subClassOf rdf:resource="jc3iedm_OBJECT-TYPE.owl#SURFACE-VESSEL-TYPE"/>
    <rdfs:label xml:lang="en">barge, target</rdfs:label>
    <rdfs:comment xml:lang="en">Self-propelled craft used to simulate a target.</rdfs:comment>
    <rdf:type rdf:resource="http://www.w3.org/2002/07/owl#Class"/>
  </rdf:Description>
  <rdf:Description rdf:about="#FACILITY-TYPE_Ditch">
    <rdfs:subClassOf rdf:resource="jc3iedm_OBJECT-TYPE.owl#FACILITY-TYPE"/>
    <rdfs:label xml:lang="en">ditch</rdfs:label>
    <rdfs:comment xml:lang="en">A channel constructed for the purpose of irrigation or drainage.</rdfs:comment>
    <rdf:type rdf:resource="http://www.w3.org/2002/07/owl#Class"/>
  </rdf:Description>
  <rdf:Description rdf:about="#SURFACE-VESSEL-TYPE_Barge,_garbage_2">
    <rdfs:subClassOf rdf:resource="jc3iedm_OBJECT-TYPE.owl#SURFACE-VESSEL-TYPE"/>
    <rdfs:label xml:lang="en">barge, garbage 2</rdfs:label>
    <rdfs:comment xml:lang="en">Craft, probably self-propelled, used for collecting garbage from ships.</rdfs:comment>
    <rdf:type rdf:resource="http://www.w3.org/2002/07/owl#Class"/>
  </rdf:Description>
  <rdf:Description rdf:about="#CONTROL-FEATURE-TYPE_Radioactive_atmospheric_concentration_contour_line">
    <rdfs:subClassOf rdf:resource="jc3iedm_OBJECT-TYPE.owl#CONTROL-FEATURE-TYPE"/>
    <rdfs:label xml:lang="en">radioactive atmospheric concentration contour line</rdfs:label>
    <rdfs:comment xml:lang="en">A line on a map, diagram or overlay joining all points at which the radiation atmospheric concentration at a given time is the same. Radiation atmospheric concentration is the quantity of radioactive material distributed in the atmosphere per unit volume.</rdfs:comment>
    <rdf:type rdf:resource="http://www.w3.org/2002/07/owl#Class"/>
  </rdf:Description>
  <rdf:Description rdf:about="#FACILITY-TYPE_Emplacement">
    <rdfs:subClassOf rdf:resource="jc3iedm_OBJECT-TYPE.owl#FACILITY-TYPE"/>
    <rdfs:label xml:lang="en">emplacement</rdfs:label>
    <rdfs:comment xml:lang="en">A prepared position for one or more weapons or pieces of equipment for protection against hostile fire or bombardment, and from which they can execute their tasks.</rdfs:comment>
    <rdf:type rdf:resource="http://www.w3.org/2002/07/owl#Class"/>
  </rdf:Description>
  <rdf:Description rdf:about="#CONTROL-FEATURE-TYPE_Radioactive_surface_deposition_concentration_contour_line">
    <rdfs:subClassOf rdf:resource="jc3iedm_OBJECT-TYPE.owl#CONTROL-FEATURE-TYPE"/>
    <rdfs:label xml:lang="en">radioactive surface deposition concentration contour line</rdfs:label>
    <rdfs:comment xml:lang="en">A line on a map, diagram or overlay joining all points at which the radiation surface deposition concentration at a given time is the same. Radiation surface deposition concentration is the quantity of radioactive material distributed on a surface per unit area.</rdfs:comment>
    <rdf:type rdf:resource="http://www.w3.org/2002/07/owl#Class"/>
  </rdf:Description>
  <rdf:Description rdf:about="jc3iedm_OBJECT-TYPE.owl#SURFACE-VESSEL-TYPE">
    <rdf:type rdf:resource="http://www.w3.org/2002/07/owl#Class"/>
    <rdfs:label xml:lang="en">surface vessel type</rdfs:label>
    <rdfs:comment xml:lang="en">A vessel principally designed to operate on the water surface.</rdfs:comment>
    <rdfs:subClassOf rdf:resource="jc3iedm_OBJECT-TYPE.owl#VESSEL-TYPE"/>
  </rdf:Description>
  <rdf:Description rdf:about="#UNIT-TYPE_Explosive_ordnance_disposal">
    <rdfs:subClassOf rdf:resource="jc3iedm_OBJECT-TYPE.owl#UNIT-TYPE"/>
    <rdfs:label xml:lang="en">explosive ordnance disposal</rdfs:label>
    <rdfs:comment xml:lang="en">A UNIT-TYPE whose principal designation is the detection, identification, field evaluation, rendering-safe, recovery and final disposal of unexploded explosive ordnance.</rdfs:comment>
    <rdf:type rdf:resource="http://www.w3.org/2002/07/owl#Class"/>
  </rdf:Description>
  <rdf:Description rdf:about="#SURFACE-VESSEL-TYPE_Tug,_ocean-going,_fleet">
    <rdfs:subClassOf rdf:resource="jc3iedm_OBJECT-TYPE.owl#SURFACE-VESSEL-TYPE"/>
    <rdfs:label xml:lang="en">tug, ocean going, fleet</rdfs:label>
    <rdfs:comment xml:lang="en">Seagoing tug employed to tow navy ships and craft. Usually about 40-50 metres, but equipped to operate with fleets.</rdfs:comment>
    <rdf:type rdf:resource="http://www.w3.org/2002/07/owl#Class"/>
  </rdf:Description>
  <rdf:Description rdf:about="jc3iedm_OBJECT-TYPE.owl#unit-type-supplementary-specialisation-code">
    <rdf:type rdf:resource="http://www.w3.org/2002/07/owl#DatatypeProperty"/>
    <rdfs:domain rdf:resource="jc3iedm_OBJECT-TYPE.owl#UNIT-TYPE"/>
    <rdfs:range rdf:resource="http://www.w3.org/2001/XMLSchema#string"/>
  </rdf:Description>
  <rdf:Description rdf:about="jc3iedm_OBJECT-TYPE.owl#UNIT-TYPE">
    <rdf:type rdf:resource="http://www.w3.org/2002/07/owl#Class"/>
    <rdfs:label xml:lang="en">unit type</rdfs:label>
    <rdfs:comment xml:lang="en">A MILITARY-ORGANISATION-TYPE whose structure is prescribed by competent authority.</rdfs:comment>
    <rdfs:subClassOf rdf:resource="jc3iedm_OBJECT-TYPE.owl#MILITARY-ORGANISATION-TYPE"/>
  </rdf:Description>
  <rdf:Description rdf:about="#CONTROL-FEATURE-TYPE_Reconnaissance_area">
    <rdfs:subClassOf rdf:resource="jc3iedm_OBJECT-TYPE.owl#CONTROL-FEATURE-TYPE"/>
    <rdfs:label xml:lang="en">reconnaissance area</rdfs:label>
    <rdfs:comment xml:lang="en">Airspace established specifically for airborne platforms conducting reconnaissance.</rdfs:comment>
    <rdf:type rdf:resource="http://www.w3.org/2002/07/owl#Class"/>
  </rdf:Description>
  <rdf:Description rdf:about="#FACILITY-TYPE_Cut">
    <rdfs:subClassOf rdf:resource="jc3iedm_OBJECT-TYPE.owl#FACILITY-TYPE"/>
    <rdfs:label xml:lang="en">cut</rdfs:label>
    <rdfs:comment xml:lang="en">An excavation of the earth's surface to provide passage for a road, railway, canal, etc.</rdfs:comment>
    <rdf:type rdf:resource="http://www.w3.org/2002/07/owl#Class"/>
  </rdf:Description>
  <rdf:Description rdf:about="#FACILITY-TYPE_Lighthouse">
    <rdfs:subClassOf rdf:resource="jc3iedm_OBJECT-TYPE.owl#FACILITY-TYPE"/>
    <rdfs:label xml:lang="en">lighthouse</rdfs:label>
    <rdfs:comment xml:lang="en">A tower or other structure, with a powerful light or lights at the top, erected at some important or dangerous point on or near the seacoast for the guidance of mariners.</rdfs:comment>
    <rdf:type rdf:resource="http://www.w3.org/2002/07/owl#Class"/>
  </rdf:Description>
  <rdf:Description rdf:about="#CONTROL-FEATURE-TYPE_Line_of_departure,_sea">
    <rdfs:subClassOf rdf:resource="jc3iedm_OBJECT-TYPE.owl#CONTROL-FEATURE-TYPE"/>
    <rdfs:label xml:lang="en">line of departure, sea</rdfs:label>
    <rdfs:comment xml:lang="en">A suitably marked offshore coordinating line to assist assault craft to land on designated beaches at scheduled times.</rdfs:comment>
    <rdf:type rdf:resource="http://www.w3.org/2002/07/owl#Class"/>
  </rdf:Description>
  <rdf:Description rdf:about="#SURFACE-VESSEL-TYPE_Cargo_ship_(naval)">
    <rdfs:subClassOf rdf:resource="jc3iedm_OBJECT-TYPE.owl#SURFACE-VESSEL-TYPE"/>
    <rdfs:label xml:lang="en">cargo ship (naval)</rdfs:label>
    <rdfs:comment xml:lang="en">Ship at least 80 metres employed to transport general cargo and provisions. No underway replenishment facilities.</rdfs:comment>
    <rdf:type rdf:resource="http://www.w3.org/2002/07/owl#Class"/>
  </rdf:Description>
  <rdf:Description rdf:about="#SURFACE-VESSEL-TYPE_Barge,_special_liquid">
    <rdfs:subClassOf rdf:resource="jc3iedm_OBJECT-TYPE.owl#SURFACE-VESSEL-TYPE"/>
    <rdfs:label xml:lang="en">barge, special liquid</rdfs:label>
    <rdfs:comment xml:lang="en">Craft 60 metres or less designed to transport fluids other than POL products or water in harbour areas.</rdfs:comment>
    <rdf:type rdf:resource="http://www.w3.org/2002/07/owl#Class"/>
  </rdf:Description>
  <rdf:Description rdf:about="#SURFACE-VESSEL-TYPE_Seaplane">
    <rdfs:subClassOf rdf:resource="jc3iedm_OBJECT-TYPE.owl#SURFACE-VESSEL-TYPE"/>
    <rdfs:label xml:lang="en">seaplane</rdfs:label>
    <rdfs:comment xml:lang="en">Aircraft designed to take-off/land on water.</rdfs:comment>
    <rdf:type rdf:resource="http://www.w3.org/2002/07/owl#Class"/>
  </rdf:Description>
  <rdf:Description rdf:about="#FACILITY-TYPE_Barracks">
    <rdfs:subClassOf rdf:resource="jc3iedm_OBJECT-TYPE.owl#FACILITY-TYPE"/>
    <rdfs:label xml:lang="en">barracks</rdfs:label>
    <rdfs:comment xml:lang="en">A building or group of buildings used to house soldiers.</rdfs:comment>
    <rdf:type rdf:resource="http://www.w3.org/2002/07/owl#Class"/>
  </rdf:Description>
  <rdf:Description rdf:about="#CONTROL-FEATURE-TYPE_Missile_detect_point">
    <rdfs:subClassOf rdf:resource="jc3iedm_OBJECT-TYPE.owl#CONTROL-FEATURE-TYPE"/>
    <rdfs:label xml:lang="en">missile detect point</rdfs:label>
    <rdfs:comment xml:lang="en">No definition provided in APP-6B JUN 08.</rdfs:comment>
    <rdf:type rdf:resource="http://www.w3.org/2002/07/owl#Class"/>
  </rdf:Description>
  <rdf:Description rdf:about="#VEHICLE-TYPE_Command_post,_wheeled">
    <rdfs:subClassOf rdf:resource="jc3iedm_OBJECT-TYPE.owl#VEHICLE-TYPE"/>
    <rdfs:label xml:lang="en">command post, wheeled</rdfs:label>
    <rdfs:comment xml:lang="en">A wheeled, non-armoured vehicle, designed to be used as a command post or as part of a command post.</rdfs:comment>
    <rdf:type rdf:resource="http://www.w3.org/2002/07/owl#Class"/>
  </rdf:Description>
  <rdf:Description rdf:about="#FACILITY-TYPE_Command_post_facility">
    <rdfs:subClassOf rdf:resource="jc3iedm_OBJECT-TYPE.owl#FACILITY-TYPE"/>
    <rdfs:label xml:lang="en">command post facility</rdfs:label>
    <rdfs:comment xml:lang="en">A facility from which a commander directs operations or controls forces.</rdfs:comment>
    <rdf:type rdf:resource="http://www.w3.org/2002/07/owl#Class"/>
  </rdf:Description>
  <rdf:Description rdf:about="#GROUP-ORGANISATION-TYPE_Media,_not_otherwise_specified">
    <rdfs:subClassOf rdf:resource="jc3iedm_OBJECT-TYPE.owl#GROUP-ORGANISATION-TYPE"/>
    <rdfs:label xml:lang="en">media, not otherwise specified</rdfs:label>
    <rdfs:comment xml:lang="en">A GROUP-ORGANISATION-TYPE that comprises persons that report for mass communications (especially television, radio, and newspapers) of an origin not specified.</rdfs:comment>
    <rdf:type rdf:resource="http://www.w3.org/2002/07/owl#Class"/>
  </rdf:Description>
  <rdf:Description rdf:about="#ENGINEERING-EQUIPMENT-TYPE_Not_known">
    <rdfs:subClassOf rdf:resource="jc3iedm_OBJECT-TYPE.owl#ENGINEERING-EQUIPMENT-TYPE"/>
    <rdfs:label xml:lang="en">not known</rdfs:label>
    <rdfs:comment xml:lang="en">It is not possible to determine which value is most applicable.</rdfs:comment>
    <rdf:type rdf:resource="http://www.w3.org/2002/07/owl#Class"/>
  </rdf:Description>
  <rdf:Description rdf:about="#MILITARY-OBSTACLE-TYPE_Anti-tank_wall">
    <rdfs:subClassOf rdf:resource="jc3iedm_OBJECT-TYPE.owl#MILITARY-OBSTACLE-TYPE"/>
    <rdfs:label xml:lang="en">anti tank wall</rdfs:label>
    <rdfs:comment xml:lang="en">A wall-like obstacle capable of stopping tanks.</rdfs:comment>
    <rdf:type rdf:resource="http://www.w3.org/2002/07/owl#Class"/>
  </rdf:Description>
  <rdf:Description rdf:about="#TASK-FORMATION-TYPE_Naval_formation">
    <rdfs:subClassOf rdf:resource="jc3iedm_OBJECT-TYPE.owl#TASK-FORMATION-TYPE"/>
    <rdfs:label xml:lang="en">naval formation</rdfs:label>
    <rdfs:comment xml:lang="en">An ordered arrangement of two or more ships, units or aircraft proceeding together under a commander.</rdfs:comment>
    <rdf:type rdf:resource="http://www.w3.org/2002/07/owl#Class"/>
  </rdf:Description>
  <rdf:Description rdf:about="#SURFACE-VESSEL-TYPE_Repair_ship,_heavy,_hull">
    <rdfs:subClassOf rdf:resource="jc3iedm_OBJECT-TYPE.owl#SURFACE-VESSEL-TYPE"/>
    <rdfs:label xml:lang="en">repair ship, heavy, hull</rdfs:label>
    <rdfs:comment xml:lang="en">Ship of at least 120 metres or more employed as a mobile repair facility providing limited support to various types of ships. Not a lifting ship. Repair primary function, support secondary and optimised for extensive repairs to ships hulls.</rdfs:comment>
    <rdf:type rdf:resource="http://www.w3.org/2002/07/owl#Class"/>
  </rdf:Description>
  <rdf:Description rdf:about="#SURFACE-VESSEL-TYPE_Barge,_self-propelled">
    <rdfs:subClassOf rdf:resource="jc3iedm_OBJECT-TYPE.owl#SURFACE-VESSEL-TYPE"/>
    <rdfs:label xml:lang="en">barge, self propelled</rdfs:label>
    <rdfs:comment xml:lang="en">General designator for self-propelled barges.</rdfs:comment>
    <rdf:type rdf:resource="http://www.w3.org/2002/07/owl#Class"/>
  </rdf:Description>
  <rdf:Description rdf:about="#AMMUNITION-TYPE_Mine,_anti-helicopter">
    <rdfs:subClassOf rdf:resource="jc3iedm_OBJECT-TYPE.owl#AMMUNITION-TYPE"/>
    <rdfs:label xml:lang="en">mine, anti helicopter</rdfs:label>
    <rdfs:comment xml:lang="en">A mine designed to cause damage to helicopters.</rdfs:comment>
    <rdf:type rdf:resource="http://www.w3.org/2002/07/owl#Class"/>
  </rdf:Description>
  <rdf:Description rdf:about="#PRIVATE-SECTOR-ORGANISATION-TYPE_Agricultural">
    <rdfs:subClassOf rdf:resource="jc3iedm_OBJECT-TYPE.owl#PRIVATE-SECTOR-ORGANISATION-TYPE"/>
    <rdfs:label xml:lang="en">agricultural</rdfs:label>
    <rdfs:comment xml:lang="en">A PRIVATE-SECTOR-ORGANISATION-TYPE whose predominant business is the production and processing of agricultural products.</rdfs:comment>
    <rdf:type rdf:resource="http://www.w3.org/2002/07/owl#Class"/>
  </rdf:Description>
  <rdf:Description rdf:about="#SURFACE-VESSEL-TYPE_Merchant_ship,_bulk_carrier">
    <rdfs:subClassOf rdf:resource="jc3iedm_OBJECT-TYPE.owl#SURFACE-VESSEL-TYPE"/>
    <rdfs:label xml:lang="en">merchant ship, bulk carrier</rdfs:label>
    <rdfs:comment xml:lang="en">Non-naval ship designed to carry dry cargo in bulk form.</rdfs:comment>
    <rdf:type rdf:resource="http://www.w3.org/2002/07/owl#Class"/>
  </rdf:Description>
  <rdf:Description rdf:about="#SURFACE-VESSEL-TYPE_Aircraft_carrier,_ASW">
    <rdfs:subClassOf rdf:resource="jc3iedm_OBJECT-TYPE.owl#SURFACE-VESSEL-TYPE"/>
    <rdfs:label xml:lang="en">aircraft carrier, asw</rdfs:label>
    <rdfs:comment xml:lang="en">Carrier capable of operating VSTOL and/or helicopters in sustained anti-submarine warfare (ASW) area operations and escort duties.</rdfs:comment>
    <rdf:type rdf:resource="http://www.w3.org/2002/07/owl#Class"/>
  </rdf:Description>
  <rdf:Description rdf:about="#SURFACE-VESSEL-TYPE_Amphibious_assault_ship,_general">
    <rdfs:subClassOf rdf:resource="jc3iedm_OBJECT-TYPE.owl#SURFACE-VESSEL-TYPE"/>
    <rdfs:label xml:lang="en">amphibious assault ship, general</rdfs:label>
    <rdfs:comment xml:lang="en">A large general purpose ship which embarks and lands elements of an assault force in both organic helicopters and organic landing craft. Capable of carrying about 1800 assault troops. Must have internal stowage and ramp, and flooded well capability for vehicles or craft.</rdfs:comment>
    <rdf:type rdf:resource="http://www.w3.org/2002/07/owl#Class"/>
  </rdf:Description>
  <rdf:Description rdf:about="#SURFACE-VESSEL-TYPE_Minehunter,_ocean">
    <rdfs:subClassOf rdf:resource="jc3iedm_OBJECT-TYPE.owl#SURFACE-VESSEL-TYPE"/>
    <rdfs:label xml:lang="en">minehunter, ocean</rdfs:label>
    <rdfs:comment xml:lang="en">Ship equipped with specific equipment to hunt mines and designed for operating in ocean waters.</rdfs:comment>
    <rdf:type rdf:resource="http://www.w3.org/2002/07/owl#Class"/>
  </rdf:Description>
  <rdf:Description rdf:about="#SURFACE-VESSEL-TYPE_Landing_craft,_air_cushion">
    <rdfs:subClassOf rdf:resource="jc3iedm_OBJECT-TYPE.owl#SURFACE-VESSEL-TYPE"/>
    <rdfs:label xml:lang="en">landing craft, air cushion</rdfs:label>
    <rdfs:comment xml:lang="en">High speed (40 knots - 74 km/hr) assault landing craft capable of travelling over land and water from over-the-horizon distances 12-200nm - 22-370 km using air cushion/gas turbine propulsion.</rdfs:comment>
    <rdf:type rdf:resource="http://www.w3.org/2002/07/owl#Class"/>
  </rdf:Description>
  <rdf:Description rdf:about="#CONTROL-FEATURE-TYPE_Landing_area">
    <rdfs:subClassOf rdf:resource="jc3iedm_OBJECT-TYPE.owl#CONTROL-FEATURE-TYPE"/>
    <rdfs:label xml:lang="en">landing area</rdfs:label>
    <rdfs:comment xml:lang="en">The part of the objective area within which the landing operations of an amphibious force are conducted.</rdfs:comment>
    <rdf:type rdf:resource="http://www.w3.org/2002/07/owl#Class"/>
  </rdf:Description>
  <rdf:Description rdf:about="#CIVILIAN-POST-TYPE_Head_of_state">
    <rdfs:subClassOf rdf:resource="jc3iedm_OBJECT-TYPE.owl#CIVILIAN-POST-TYPE"/>
    <rdfs:label xml:lang="en">head of state</rdfs:label>
    <rdfs:comment xml:lang="en">A CIVILIAN-POST-TYPE whose job is the supreme executive magistracy of a country.</rdfs:comment>
    <rdf:type rdf:resource="http://www.w3.org/2002/07/owl#Class"/>
  </rdf:Description>
  <rdf:Description rdf:about="#FACILITY-TYPE_Sensor_outpost/listening_post">
    <rdfs:subClassOf rdf:resource="jc3iedm_OBJECT-TYPE.owl#FACILITY-TYPE"/>
    <rdfs:label xml:lang="en">sensor outpost/listening post</rdfs:label>
    <rdfs:comment xml:lang="en">A facility from which military observations are made or fires directed and adjusted and which possesses appropriate communications; it may be airborne. This is an unmanned Observation Post with electronic or other devices to detect activity within the sensors’ range.</rdfs:comment>
    <rdf:type rdf:resource="http://www.w3.org/2002/07/owl#Class"/>
  </rdf:Description>
  <rdf:Description rdf:about="#SURFACE-VESSEL-TYPE_Mine_countermeasures_vessel,_general">
    <rdfs:subClassOf rdf:resource="jc3iedm_OBJECT-TYPE.owl#SURFACE-VESSEL-TYPE"/>
    <rdfs:label xml:lang="en">mine countermeasures vessel, general</rdfs:label>
    <rdfs:comment xml:lang="en">General designator for mine countermeasures vessels.</rdfs:comment>
    <rdf:type rdf:resource="http://www.w3.org/2002/07/owl#Class"/>
  </rdf:Description>
  <rdf:Description rdf:about="#UNIT-TYPE_Headquarters_staff">
    <rdfs:subClassOf rdf:resource="jc3iedm_OBJECT-TYPE.owl#UNIT-TYPE"/>
    <rdfs:label xml:lang="en">headquarters staff</rdfs:label>
    <rdfs:comment xml:lang="en">A UNIT-TYPE whose principal designation is to provide staff to man a command and control element.</rdfs:comment>
    <rdf:type rdf:resource="http://www.w3.org/2002/07/owl#Class"/>
  </rdf:Description>
  <rdf:Description rdf:about="#SURFACE-VESSEL-TYPE_Frigate,_general">
    <rdfs:subClassOf rdf:resource="jc3iedm_OBJECT-TYPE.owl#SURFACE-VESSEL-TYPE"/>
    <rdfs:label xml:lang="en">frigate, general</rdfs:label>
    <rdfs:comment xml:lang="en">General designator for frigate. A surface combatant in size range of about 75-150 metres. Fitted primarily to fulfil an ASW role. Generally has lighter surface armament than a Destroyer, general.</rdfs:comment>
    <rdf:type rdf:resource="http://www.w3.org/2002/07/owl#Class"/>
  </rdf:Description>
  <rdf:Description rdf:about="#TASK-FORMATION-TYPE_Work_party">
    <rdfs:subClassOf rdf:resource="jc3iedm_OBJECT-TYPE.owl#TASK-FORMATION-TYPE"/>
    <rdfs:label xml:lang="en">work party</rdfs:label>
    <rdfs:comment xml:lang="en">A group of people who come together to carry out a piece of work.</rdfs:comment>
    <rdf:type rdf:resource="http://www.w3.org/2002/07/owl#Class"/>
  </rdf:Description>
  <rdf:Description rdf:about="#SURFACE-VESSEL-TYPE_Frigate,_training">
    <rdfs:subClassOf rdf:resource="jc3iedm_OBJECT-TYPE.owl#SURFACE-VESSEL-TYPE"/>
    <rdfs:label xml:lang="en">frigate, training</rdfs:label>
    <rdfs:comment xml:lang="en">General designator for frigate used primarily in a training role. A surface combatant in size range of about 75-150 metres. Fitted primarily to fulfil an ASW role. Generally has lighter surface armament than a Destroyer, general. Classification determined by armament or capability.</rdfs:comment>
    <rdf:type rdf:resource="http://www.w3.org/2002/07/owl#Class"/>
  </rdf:Description>
  <rdf:Description rdf:about="#SURFACE-VESSEL-TYPE_Merchant_ship,_dry_cargo,_break_bulk">
    <rdfs:subClassOf rdf:resource="jc3iedm_OBJECT-TYPE.owl#SURFACE-VESSEL-TYPE"/>
    <rdfs:label xml:lang="en">merchant ship, dry cargo, break bulk</rdfs:label>
    <rdfs:comment xml:lang="en">Non-naval dry cargo carrying ship capable of handling break bulk cargo.</rdfs:comment>
    <rdf:type rdf:resource="http://www.w3.org/2002/07/owl#Class"/>
  </rdf:Description>
  <rdf:Description rdf:about="#SURFACE-VESSEL-TYPE_Lighter">
    <rdfs:subClassOf rdf:resource="jc3iedm_OBJECT-TYPE.owl#SURFACE-VESSEL-TYPE"/>
    <rdfs:label xml:lang="en">lighter</rdfs:label>
    <rdfs:comment xml:lang="en">General designator for lighters.</rdfs:comment>
    <rdf:type rdf:resource="http://www.w3.org/2002/07/owl#Class"/>
  </rdf:Description>
  <rdf:Description rdf:about="#ENGINEERING-EQUIPMENT-TYPE_Bridging">
    <rdfs:subClassOf rdf:resource="jc3iedm_OBJECT-TYPE.owl#ENGINEERING-EQUIPMENT-TYPE"/>
    <rdfs:label xml:lang="en">bridging</rdfs:label>
    <rdfs:comment xml:lang="en">Equipment designed for the crossing of gaps and other obstacles.</rdfs:comment>
    <rdf:type rdf:resource="http://www.w3.org/2002/07/owl#Class"/>
  </rdf:Description>
  <rdf:Description rdf:about="#AIRCRAFT-TYPE_No">
    <rdfs:subClassOf rdf:resource="jc3iedm_OBJECT-TYPE.owl#AIRCRAFT-TYPE"/>
    <rdfs:label xml:lang="en">no</rdfs:label>
    <rdfs:comment xml:lang="en">The AIRCRAFT-TYPE is not designed to be used as a trainer.</rdfs:comment>
    <rdf:type rdf:resource="http://www.w3.org/2002/07/owl#Class"/>
  </rdf:Description>
  <rdf:Description rdf:about="#ORGANISATION-TYPE_Recognised_air_picture_production_centre">
    <rdfs:subClassOf rdf:resource="jc3iedm_OBJECT-TYPE.owl#ORGANISATION-TYPE"/>
    <rdfs:label xml:lang="en">recognised air picture production centre</rdfs:label>
    <rdfs:comment xml:lang="en">No definition provided in ADatP-3 Baseline 13.1 FFIRN/FUD 1874/4.</rdfs:comment>
    <rdf:type rdf:resource="http://www.w3.org/2002/07/owl#Class"/>
  </rdf:Description>
  <rdf:Description rdf:about="#SURFACE-VESSEL-TYPE_Dhow">
    <rdfs:subClassOf rdf:resource="jc3iedm_OBJECT-TYPE.owl#SURFACE-VESSEL-TYPE"/>
    <rdfs:label xml:lang="en">dhow</rdfs:label>
    <rdfs:comment xml:lang="en">Sailing vessel, usually associated with middle eastern countries of specific design. May be powered by engine or sails, usually used for transportation purposes.</rdfs:comment>
    <rdf:type rdf:resource="http://www.w3.org/2002/07/owl#Class"/>
  </rdf:Description>
  <rdf:Description rdf:about="jc3iedm_OBJECT-TYPE.owl#vessel-type-gross-registered-tonnage-quantity">
    <rdf:type rdf:resource="http://www.w3.org/2002/07/owl#DatatypeProperty"/>
    <rdfs:domain rdf:resource="jc3iedm_OBJECT-TYPE.owl#VESSEL-TYPE"/>
  </rdf:Description>
  <rdf:Description rdf:about="#SUBSURFACE-VESSEL-TYPE_Submarine,_attack,_guided_missile,_nuclear">
    <rdfs:subClassOf rdf:resource="jc3iedm_OBJECT-TYPE.owl#SUBSURFACE-VESSEL-TYPE"/>
    <rdfs:label xml:lang="en">submarine, attack, guided missile, nuclear</rdfs:label>
    <rdfs:comment xml:lang="en">Submarine fitted with underwater to surface or surface-to-surface missiles with nuclear power.</rdfs:comment>
    <rdf:type rdf:resource="http://www.w3.org/2002/07/owl#Class"/>
  </rdf:Description>
  <rdf:Description rdf:about="#CONTROL-FEATURE-TYPE_Extraction_zone">
    <rdfs:subClassOf rdf:resource="jc3iedm_OBJECT-TYPE.owl#CONTROL-FEATURE-TYPE"/>
    <rdfs:label xml:lang="en">extraction zone</rdfs:label>
    <rdfs:comment xml:lang="en">A specified drop zone used for the delivery of equipment and/or supplies by means of an extraction technique from an aircraft flying very close to the ground.</rdfs:comment>
    <rdf:type rdf:resource="http://www.w3.org/2002/07/owl#Class"/>
  </rdf:Description>
  <rdf:Description rdf:about="#PRIVATE-SECTOR-ORGANISATION-TYPE_Retail">
    <rdfs:subClassOf rdf:resource="jc3iedm_OBJECT-TYPE.owl#PRIVATE-SECTOR-ORGANISATION-TYPE"/>
    <rdfs:label xml:lang="en">retail</rdfs:label>
    <rdfs:comment xml:lang="en">A PRIVATE-SECTOR-ORGANISATION-TYPE whose predominant business is retail in nature.</rdfs:comment>
    <rdf:type rdf:resource="http://www.w3.org/2002/07/owl#Class"/>
  </rdf:Description>
  <rdf:Description rdf:about="#AMMUNITION-TYPE_Mine,_not_known">
    <rdfs:subClassOf rdf:resource="jc3iedm_OBJECT-TYPE.owl#AMMUNITION-TYPE"/>
    <rdfs:label xml:lang="en">mine, not known</rdfs:label>
    <rdfs:comment xml:lang="en">It is not possible to determine the type of mine.</rdfs:comment>
    <rdf:type rdf:resource="http://www.w3.org/2002/07/owl#Class"/>
  </rdf:Description>
  <rdf:Description rdf:about="#FACILITY-TYPE_Service,_research,_utility_facility,_electric_power_facility">
    <rdfs:subClassOf rdf:resource="jc3iedm_OBJECT-TYPE.owl#FACILITY-TYPE"/>
    <rdfs:label xml:lang="en">service, research, utility facility, electric power facility</rdfs:label>
    <rdfs:comment xml:lang="en">A facility generally used to support service, research or utility functions in support of electric power.</rdfs:comment>
    <rdf:type rdf:resource="http://www.w3.org/2002/07/owl#Class"/>
  </rdf:Description>
  <rdf:Description rdf:about="#FACILITY-TYPE_Site,_raft">
    <rdfs:subClassOf rdf:resource="jc3iedm_OBJECT-TYPE.owl#FACILITY-TYPE"/>
    <rdfs:label xml:lang="en">site, raft</rdfs:label>
    <rdfs:comment xml:lang="en">No definition provided in APP-6A.</rdfs:comment>
    <rdf:type rdf:resource="http://www.w3.org/2002/07/owl#Class"/>
  </rdf:Description>
  <rdf:Description rdf:about="#MILITARY-POST-TYPE_Forward_observation_officer/air_observation_post">
    <rdfs:subClassOf rdf:resource="jc3iedm_OBJECT-TYPE.owl#MILITARY-POST-TYPE"/>
    <rdfs:label xml:lang="en">forward observation officer/air observation post</rdfs:label>
    <rdfs:comment xml:lang="en">A MILITARY-POST-TYPE that is identified as the observer operating with front line troops on the ground or in the air and trained to adjust ground or naval gunfire and pass back battlespace information.</rdfs:comment>
    <rdf:type rdf:resource="http://www.w3.org/2002/07/owl#Class"/>
  </rdf:Description>
  <rdf:Description rdf:about="#GEOGRAPHIC-FEATURE-TYPE_Continent">
    <rdfs:subClassOf rdf:resource="jc3iedm_OBJECT-TYPE.owl#GEOGRAPHIC-FEATURE-TYPE"/>
    <rdfs:label xml:lang="en">continent</rdfs:label>
    <rdfs:comment xml:lang="en">Any of the world's main continuous expanses of land.</rdfs:comment>
    <rdf:type rdf:resource="http://www.w3.org/2002/07/owl#Class"/>
  </rdf:Description>
  <rdf:Description rdf:about="#ELECTRONIC-EQUIPMENT-TYPE_Electronic_warfare">
    <rdfs:subClassOf rdf:resource="jc3iedm_OBJECT-TYPE.owl#ELECTRONIC-EQUIPMENT-TYPE"/>
    <rdfs:label xml:lang="en">electronic warfare</rdfs:label>
    <rdfs:comment xml:lang="en">An equipment used for military action involving the use of electromagnetic energy to determine, exploit, reduce, or prevent hostile use of the electromagnetic spectrum and action to retain its effective use by friendly forces.</rdfs:comment>
    <rdf:type rdf:resource="http://www.w3.org/2002/07/owl#Class"/>
  </rdf:Description>
  <rdf:Description rdf:about="#FACILITY-TYPE_Military_materiel_facility,_vehicle_production">
    <rdfs:subClassOf rdf:resource="jc3iedm_OBJECT-TYPE.owl#FACILITY-TYPE"/>
    <rdfs:label xml:lang="en">military materiel facility, vehicle production</rdfs:label>
    <rdfs:comment xml:lang="en">A facility used as for vehicle production.</rdfs:comment>
    <rdf:type rdf:resource="http://www.w3.org/2002/07/owl#Class"/>
  </rdf:Description>
  <rdf:Description rdf:about="#SURFACE-VESSEL-TYPE_Special_warfare_craft,_medium">
    <rdfs:subClassOf rdf:resource="jc3iedm_OBJECT-TYPE.owl#SURFACE-VESSEL-TYPE"/>
    <rdfs:label xml:lang="en">special warfare craft, medium</rdfs:label>
    <rdfs:comment xml:lang="en">A medium craft specifically designed for special warfare operations.</rdfs:comment>
    <rdf:type rdf:resource="http://www.w3.org/2002/07/owl#Class"/>
  </rdf:Description>
  <rdf:Description rdf:about="#FACILITY-TYPE_Dam/weir">
    <rdfs:subClassOf rdf:resource="jc3iedm_OBJECT-TYPE.owl#FACILITY-TYPE"/>
    <rdfs:label xml:lang="en">dam/weir</rdfs:label>
    <rdfs:comment xml:lang="en">A permanent barrier across a watercourse used to impound water or to control its flow.</rdfs:comment>
    <rdf:type rdf:resource="http://www.w3.org/2002/07/owl#Class"/>
  </rdf:Description>
  <rdf:Description rdf:about="#SURFACE-VESSEL-TYPE_Training_craft">
    <rdfs:subClassOf rdf:resource="jc3iedm_OBJECT-TYPE.owl#SURFACE-VESSEL-TYPE"/>
    <rdfs:label xml:lang="en">training craft</rdfs:label>
    <rdfs:comment xml:lang="en">General designator for any craft used for training purposes.</rdfs:comment>
    <rdf:type rdf:resource="http://www.w3.org/2002/07/owl#Class"/>
  </rdf:Description>
  <rdf:Description rdf:about="jc3iedm_OBJECT-TYPE.owl#equipment-type-loaded-weight-quantity">
    <rdf:type rdf:resource="http://www.w3.org/2002/07/owl#DatatypeProperty"/>
    <rdfs:domain rdf:resource="jc3iedm_OBJECT-TYPE.owl#EQUIPMENT-TYPE"/>
  </rdf:Description>
  <rdf:Description rdf:about="#MARITIME-EQUIPMENT-TYPE_Rubber_mooring">
    <rdfs:subClassOf rdf:resource="jc3iedm_OBJECT-TYPE.owl#MARITIME-EQUIPMENT-TYPE"/>
    <rdfs:label xml:lang="en">rubber mooring</rdfs:label>
    <rdfs:comment xml:lang="en">Part of the mooring equipment used with a short scope buoy.</rdfs:comment>
    <rdf:type rdf:resource="http://www.w3.org/2002/07/owl#Class"/>
  </rdf:Description>
  <rdf:Description rdf:about="#FACILITY-TYPE_Power_plant,_thermal">
    <rdfs:subClassOf rdf:resource="jc3iedm_OBJECT-TYPE.owl#FACILITY-TYPE"/>
    <rdfs:label xml:lang="en">power plant, thermal</rdfs:label>
    <rdfs:comment xml:lang="en">A facility that provides power produced from thermal processes.</rdfs:comment>
    <rdf:type rdf:resource="http://www.w3.org/2002/07/owl#Class"/>
  </rdf:Description>
  <rdf:Description rdf:about="#CONTROL-FEATURE-TYPE_No_fire_area">
    <rdfs:subClassOf rdf:resource="jc3iedm_OBJECT-TYPE.owl#CONTROL-FEATURE-TYPE"/>
    <rdfs:label xml:lang="en">no fire area</rdfs:label>
    <rdfs:comment xml:lang="en">An area/airspace in which fires or the effects of fires are not allowed without prior clearance from the establishing headquarters, except when a force must defend itself against an engaging enemy force within the no fire area.</rdfs:comment>
    <rdf:type rdf:resource="http://www.w3.org/2002/07/owl#Class"/>
  </rdf:Description>
  <rdf:Description rdf:about="#SURFACE-VESSEL-TYPE_Cruiser,_guided_missile,_helicopter_capable">
    <rdfs:subClassOf rdf:resource="jc3iedm_OBJECT-TYPE.owl#SURFACE-VESSEL-TYPE"/>
    <rdfs:label xml:lang="en">cruiser, guided missile, helicopter capable</rdfs:label>
    <rdfs:comment xml:lang="en">Cruiser with one or more force guided missile systems as its main armament, fitted with a flight deck with a primary mission of operating and maintaining helicopters.</rdfs:comment>
    <rdf:type rdf:resource="http://www.w3.org/2002/07/owl#Class"/>
  </rdf:Description>
  <rdf:Description rdf:about="#SURFACE-VESSEL-TYPE_Police_launch">
    <rdfs:subClassOf rdf:resource="jc3iedm_OBJECT-TYPE.owl#SURFACE-VESSEL-TYPE"/>
    <rdfs:label xml:lang="en">police launch</rdfs:label>
    <rdfs:comment xml:lang="en">Police operated small craft less than 20 metres employed in sheltered waters for transporting personnel.</rdfs:comment>
    <rdf:type rdf:resource="http://www.w3.org/2002/07/owl#Class"/>
  </rdf:Description>
  <rdf:Description rdf:about="#CONTROL-FEATURE-TYPE_Rendezvous_point">
    <rdfs:subClassOf rdf:resource="jc3iedm_OBJECT-TYPE.owl#CONTROL-FEATURE-TYPE"/>
    <rdfs:label xml:lang="en">rendezvous point</rdfs:label>
    <rdfs:comment xml:lang="en">A given location at which to regroup before, during or after an operation at a specified time or in a specified situation.</rdfs:comment>
    <rdf:type rdf:resource="http://www.w3.org/2002/07/owl#Class"/>
  </rdf:Description>
  <rdf:Description rdf:about="#UNIT-TYPE_Headquarters_and_signals">
    <rdfs:subClassOf rdf:resource="jc3iedm_OBJECT-TYPE.owl#UNIT-TYPE"/>
    <rdfs:label xml:lang="en">headquarters and signals</rdfs:label>
    <rdfs:comment xml:lang="en">A UNIT-TYPE whose principal designation is to provide staff and communication equipment to set up a command and control element.</rdfs:comment>
    <rdf:type rdf:resource="http://www.w3.org/2002/07/owl#Class"/>
  </rdf:Description>
  <rdf:Description rdf:about="#CONTROL-FEATURE-TYPE_Terminal_control_area">
    <rdfs:subClassOf rdf:resource="jc3iedm_OBJECT-TYPE.owl#CONTROL-FEATURE-TYPE"/>
    <rdfs:label xml:lang="en">terminal control area</rdfs:label>
    <rdfs:comment xml:lang="en">A control area normally established at the confluence of air traffic services routes in the vicinity of one or more major aerodromes.</rdfs:comment>
    <rdf:type rdf:resource="http://www.w3.org/2002/07/owl#Class"/>
  </rdf:Description>
  <rdf:Description rdf:about="#SURFACE-VESSEL-TYPE_Cruiser,_guided_missile,_nuclear_powered">
    <rdfs:subClassOf rdf:resource="jc3iedm_OBJECT-TYPE.owl#SURFACE-VESSEL-TYPE"/>
    <rdfs:label xml:lang="en">cruiser, guided missile, nuclear powered</rdfs:label>
    <rdfs:comment xml:lang="en">Cruiser with one or more force guided missile systems as its main armament and having nuclear power.</rdfs:comment>
    <rdf:type rdf:resource="http://www.w3.org/2002/07/owl#Class"/>
  </rdf:Description>
  <rdf:Description rdf:about="#SURFACE-VESSEL-TYPE_Ice_breaker,_small">
    <rdfs:subClassOf rdf:resource="jc3iedm_OBJECT-TYPE.owl#SURFACE-VESSEL-TYPE"/>
    <rdfs:label xml:lang="en">ice breaker, small</rdfs:label>
    <rdfs:comment xml:lang="en">Armed ship in size range under 70 metres used primarily for icebreaking duties.</rdfs:comment>
    <rdf:type rdf:resource="http://www.w3.org/2002/07/owl#Class"/>
  </rdf:Description>
  <rdf:Description rdf:about="#CIVILIAN-POST-TYPE_Regional_administrator">
    <rdfs:subClassOf rdf:resource="jc3iedm_OBJECT-TYPE.owl#CIVILIAN-POST-TYPE"/>
    <rdfs:label xml:lang="en">regional administrator</rdfs:label>
    <rdfs:comment xml:lang="en">A CIVILIAN-POST-TYPE whose job is to manage or direct the affairs of a regional organisation.</rdfs:comment>
    <rdf:type rdf:resource="http://www.w3.org/2002/07/owl#Class"/>
  </rdf:Description>
  <rdf:Description rdf:about="#SURFACE-VESSEL-TYPE_Survey_craft">
    <rdfs:subClassOf rdf:resource="jc3iedm_OBJECT-TYPE.owl#SURFACE-VESSEL-TYPE"/>
    <rdfs:label xml:lang="en">survey craft</rdfs:label>
    <rdfs:comment xml:lang="en">Small craft used for survey purposes in sheltered waters.</rdfs:comment>
    <rdf:type rdf:resource="http://www.w3.org/2002/07/owl#Class"/>
  </rdf:Description>
  <rdf:Description rdf:about="#MISCELLANEOUS-EQUIPMENT-TYPE_Not_known">
    <rdfs:subClassOf rdf:resource="jc3iedm_OBJECT-TYPE.owl#MISCELLANEOUS-EQUIPMENT-TYPE"/>
    <rdfs:label xml:lang="en">not known</rdfs:label>
    <rdfs:comment xml:lang="en">It is not possible to determine which value is most applicable.</rdfs:comment>
    <rdf:type rdf:resource="http://www.w3.org/2002/07/owl#Class"/>
  </rdf:Description>
  <rdf:Description rdf:about="#MISCELLANEOUS-EQUIPMENT-TYPE_Guidance">
    <rdfs:subClassOf rdf:resource="jc3iedm_OBJECT-TYPE.owl#MISCELLANEOUS-EQUIPMENT-TYPE"/>
    <rdfs:label xml:lang="en">guidance</rdfs:label>
    <rdfs:comment xml:lang="en">Equipment used to show the way or direct movement.</rdfs:comment>
    <rdf:type rdf:resource="http://www.w3.org/2002/07/owl#Class"/>
  </rdf:Description>
  <rdf:Description rdf:about="#UNIT-TYPE_Reconnaissance">
    <rdfs:subClassOf rdf:resource="jc3iedm_OBJECT-TYPE.owl#UNIT-TYPE"/>
    <rdfs:label xml:lang="en">reconnaissance</rdfs:label>
    <rdfs:comment xml:lang="en">A UNIT-TYPE whose principal designation is to obtain, by visual observation or other detection methods, information about the activities and resources of an enemy or potential enemy; or to secure data concerning the meteorological, hydrographic, or geographic characteristics of a particular area.</rdfs:comment>
    <rdf:type rdf:resource="http://www.w3.org/2002/07/owl#Class"/>
  </rdf:Description>
  <rdf:Description rdf:about="#VEHICLE-TYPE_Armoured_vehicle,_light">
    <rdfs:subClassOf rdf:resource="jc3iedm_OBJECT-TYPE.owl#VEHICLE-TYPE"/>
    <rdfs:label xml:lang="en">armoured vehicle, light</rdfs:label>
    <rdfs:comment xml:lang="en">An armoured vehicle with less armour that uses its increased mobility and possibly more lethal armaments for survivability.</rdfs:comment>
    <rdf:type rdf:resource="http://www.w3.org/2002/07/owl#Class"/>
  </rdf:Description>
  <rdf:Description rdf:about="#CONTROL-FEATURE-TYPE_Restricted_fire_area">
    <rdfs:subClassOf rdf:resource="jc3iedm_OBJECT-TYPE.owl#CONTROL-FEATURE-TYPE"/>
    <rdfs:label xml:lang="en">restricted fire area</rdfs:label>
    <rdfs:comment xml:lang="en">An area/airspace into which specific restrictions are imposed and into which fires that exceed those restrictions are prohibited without prior coordination.</rdfs:comment>
    <rdf:type rdf:resource="http://www.w3.org/2002/07/owl#Class"/>
  </rdf:Description>
  <rdf:Description rdf:about="#SURFACE-VESSEL-TYPE_Landing_craft,_utility">
    <rdfs:subClassOf rdf:resource="jc3iedm_OBJECT-TYPE.owl#SURFACE-VESSEL-TYPE"/>
    <rdfs:label xml:lang="en">landing craft, utility</rdfs:label>
    <rdfs:comment xml:lang="en">All-purpose landing craft in size range 25-55 metres and full load of 120-500 tons with landing ramp/other landing facilities used for handling 2-3 tanks or 300-450 troops.</rdfs:comment>
    <rdf:type rdf:resource="http://www.w3.org/2002/07/owl#Class"/>
  </rdf:Description>
  <rdf:Description rdf:about="#UNIT-TYPE_Aviation,_rotary_wing">
    <rdfs:subClassOf rdf:resource="jc3iedm_OBJECT-TYPE.owl#UNIT-TYPE"/>
    <rdfs:label xml:lang="en">aviation, rotary wing</rdfs:label>
    <rdfs:comment xml:lang="en">A UNIT-TYPE whose designation indicates employment of rotary-wing assets in the air regime.</rdfs:comment>
    <rdf:type rdf:resource="http://www.w3.org/2002/07/owl#Class"/>
  </rdf:Description>
  <rdf:Description rdf:about="#SURFACE-VESSEL-TYPE_Swimmer_delivery_vehicle">
    <rdfs:subClassOf rdf:resource="jc3iedm_OBJECT-TYPE.owl#SURFACE-VESSEL-TYPE"/>
    <rdfs:label xml:lang="en">swimmer delivery vehicle</rdfs:label>
    <rdfs:comment xml:lang="en">Amphibious ship designed to operate swimmers.</rdfs:comment>
    <rdf:type rdf:resource="http://www.w3.org/2002/07/owl#Class"/>
  </rdf:Description>
  <rdf:Description rdf:about="#CONTROL-FEATURE-TYPE_Defence_zone">
    <rdfs:subClassOf rdf:resource="jc3iedm_OBJECT-TYPE.owl#CONTROL-FEATURE-TYPE"/>
    <rdfs:label xml:lang="en">defence zone</rdfs:label>
    <rdfs:comment xml:lang="en">The area extending from the forward edge of the battle area to its rear boundary.</rdfs:comment>
    <rdf:type rdf:resource="http://www.w3.org/2002/07/owl#Class"/>
  </rdf:Description>
  <rdf:Description rdf:about="#TASK-FORMATION-TYPE_Marine_air_traffic_control_detachment">
    <rdfs:subClassOf rdf:resource="jc3iedm_OBJECT-TYPE.owl#TASK-FORMATION-TYPE"/>
    <rdfs:label xml:lang="en">marine air traffic control detachment</rdfs:label>
    <rdfs:comment xml:lang="en">A TASK-FORMATION-TYPE, subordinate to the U.S. Marine TACC, that controls local airspace/aircraft in and around a Marine Air Ground Task Force (MAGTF) airfields and provides precision approach control for MAGTF aircraft.</rdfs:comment>
    <rdf:type rdf:resource="http://www.w3.org/2002/07/owl#Class"/>
  </rdf:Description>
  <rdf:Description rdf:about="#SURFACE-VESSEL-TYPE_Intelligence_collector">
    <rdfs:subClassOf rdf:resource="jc3iedm_OBJECT-TYPE.owl#SURFACE-VESSEL-TYPE"/>
    <rdfs:label xml:lang="en">intelligence collector</rdfs:label>
    <rdfs:comment xml:lang="en">Ship specially fitted for and primarily employed in the collection of electronic intelligence.</rdfs:comment>
    <rdf:type rdf:resource="http://www.w3.org/2002/07/owl#Class"/>
  </rdf:Description>
  <rdf:Description rdf:about="#GEOGRAPHIC-FEATURE-TYPE_Not_otherwise_specified">
    <rdfs:subClassOf rdf:resource="jc3iedm_OBJECT-TYPE.owl#GEOGRAPHIC-FEATURE-TYPE"/>
    <rdfs:label xml:lang="en">not otherwise specified</rdfs:label>
    <rdfs:comment xml:lang="en">The appropriate value is not in the set of specified values.</rdfs:comment>
    <rdf:type rdf:resource="http://www.w3.org/2002/07/owl#Class"/>
  </rdf:Description>
  <rdf:Description rdf:about="#SURFACE-VESSEL-TYPE_Amphibious_assault_ship,_helicopter">
    <rdfs:subClassOf rdf:resource="jc3iedm_OBJECT-TYPE.owl#SURFACE-VESSEL-TYPE"/>
    <rdfs:label xml:lang="en">amphibious assault ship, helicopter</rdfs:label>
    <rdfs:comment xml:lang="en">A large helicopter carrier with the mission of transporting and landing about 1800 assault troops with its organic aircraft. Employment of organic landing craft is not a principle function.</rdfs:comment>
    <rdf:type rdf:resource="http://www.w3.org/2002/07/owl#Class"/>
  </rdf:Description>
  <rdf:Description rdf:about="#SURFACE-VESSEL-TYPE_Aircraft_carrier,_helicopter/VSTOL">
    <rdfs:subClassOf rdf:resource="jc3iedm_OBJECT-TYPE.owl#SURFACE-VESSEL-TYPE"/>
    <rdfs:label xml:lang="en">aircraft carrier, helicopter/vstol</rdfs:label>
    <rdfs:comment xml:lang="en">Aircraft carrier without arrest gear/catapult operating VSTOL aircraft and/or helicopters that is not an amphibious or minewarfare ship.</rdfs:comment>
    <rdf:type rdf:resource="http://www.w3.org/2002/07/owl#Class"/>
  </rdf:Description>
  <rdf:Description rdf:about="jc3iedm_OBJECT-TYPE.owl#aircraft-type-manning-code">
    <rdf:type rdf:resource="http://www.w3.org/2002/07/owl#DatatypeProperty"/>
    <rdfs:domain rdf:resource="jc3iedm_OBJECT-TYPE.owl#AIRCRAFT-TYPE"/>
    <rdfs:range rdf:resource="http://www.w3.org/2001/XMLSchema#string"/>
  </rdf:Description>
  <rdf:Description rdf:about="#ENGINEERING-EQUIPMENT-TYPE_Crane">
    <rdfs:subClassOf rdf:resource="jc3iedm_OBJECT-TYPE.owl#ENGINEERING-EQUIPMENT-TYPE"/>
    <rdfs:label xml:lang="en">crane</rdfs:label>
    <rdfs:comment xml:lang="en">A machine for raising and lowering heavy weights; in its usual form it consists of a vertical post capable of rotation on its axis, a projecting arm or 'jib' over which passes the chain or rope from which the weight is suspended, and a barrel round which the chain or rope is wound.</rdfs:comment>
    <rdf:type rdf:resource="http://www.w3.org/2002/07/owl#Class"/>
  </rdf:Description>
  <rdf:Description rdf:about="#ROUTE-TYPE_Conditional_route">
    <rdfs:subClassOf rdf:resource="jc3iedm_OBJECT-TYPE.owl#ROUTE-TYPE"/>
    <rdfs:label xml:lang="en">conditional route</rdfs:label>
    <rdfs:comment xml:lang="en">A non-permanent air traffic service route or portion thereof which can be planned and used only under certain conditions.</rdfs:comment>
    <rdf:type rdf:resource="http://www.w3.org/2002/07/owl#Class"/>
  </rdf:Description>
  <rdf:Description rdf:about="#MARITIME-EQUIPMENT-TYPE_Pellets">
    <rdfs:subClassOf rdf:resource="jc3iedm_OBJECT-TYPE.owl#MARITIME-EQUIPMENT-TYPE"/>
    <rdfs:label xml:lang="en">pellets</rdfs:label>
    <rdfs:comment xml:lang="en">Orange floats used to support a length of line to aid recovery.</rdfs:comment>
    <rdf:type rdf:resource="http://www.w3.org/2002/07/owl#Class"/>
  </rdf:Description>
  <rdf:Description rdf:about="#CONTROL-FEATURE-TYPE_Light_line">
    <rdfs:subClassOf rdf:resource="jc3iedm_OBJECT-TYPE.owl#CONTROL-FEATURE-TYPE"/>
    <rdfs:label xml:lang="en">light line</rdfs:label>
    <rdfs:comment xml:lang="en">A designated phase line forward of which vehicles are required to use blackout lights at night.</rdfs:comment>
    <rdf:type rdf:resource="http://www.w3.org/2002/07/owl#Class"/>
  </rdf:Description>
  <rdf:Description rdf:about="#SURFACE-VESSEL-TYPE_Stores_ship,_transport">
    <rdfs:subClassOf rdf:resource="jc3iedm_OBJECT-TYPE.owl#SURFACE-VESSEL-TYPE"/>
    <rdfs:label xml:lang="en">stores ship, transport</rdfs:label>
    <rdfs:comment xml:lang="en">Ship capable of transporting 5000 or more tons of refrigerated and dry provisions, technical spares and general stores but lacking sophisticated underway replenishment capabilities.</rdfs:comment>
    <rdf:type rdf:resource="http://www.w3.org/2002/07/owl#Class"/>
  </rdf:Description>
  <rdf:Description rdf:about="#SURFACE-VESSEL-TYPE_Salvage_lift_craft">
    <rdfs:subClassOf rdf:resource="jc3iedm_OBJECT-TYPE.owl#SURFACE-VESSEL-TYPE"/>
    <rdfs:label xml:lang="en">salvage lift craft</rdfs:label>
    <rdfs:comment xml:lang="en">Craft of 40 metres or less employed to raise sunken ships. Lift capacity about 60 tons.</rdfs:comment>
    <rdf:type rdf:resource="http://www.w3.org/2002/07/owl#Class"/>
  </rdf:Description>
  <rdf:Description rdf:about="#CONTROL-FEATURE-TYPE_Search_and_rescue_point">
    <rdfs:subClassOf rdf:resource="jc3iedm_OBJECT-TYPE.owl#CONTROL-FEATURE-TYPE"/>
    <rdfs:label xml:lang="en">search and rescue point</rdfs:label>
    <rdfs:comment xml:lang="en">A reference point used during SAR operations.</rdfs:comment>
    <rdf:type rdf:resource="http://www.w3.org/2002/07/owl#Class"/>
  </rdf:Description>
  <rdf:Description rdf:about="#CBRN-EQUIPMENT-TYPE_Mass_spectrometer">
    <rdfs:subClassOf rdf:resource="jc3iedm_OBJECT-TYPE.owl#CBRN-EQUIPMENT-TYPE"/>
    <rdfs:label xml:lang="en">mass spectrometer</rdfs:label>
    <rdfs:comment xml:lang="en">An apparatus used for recording and measuring the mass spectra of particles, especially as a method of analysis.</rdfs:comment>
    <rdf:type rdf:resource="http://www.w3.org/2002/07/owl#Class"/>
  </rdf:Description>
  <rdf:Description rdf:about="#AMMUNITION-TYPE_Mine,_anti-personnel">
    <rdfs:subClassOf rdf:resource="jc3iedm_OBJECT-TYPE.owl#AMMUNITION-TYPE"/>
    <rdfs:label xml:lang="en">mine, anti personnel</rdfs:label>
    <rdfs:comment xml:lang="en">A mine designed to cause casualties to personnel.</rdfs:comment>
    <rdf:type rdf:resource="http://www.w3.org/2002/07/owl#Class"/>
  </rdf:Description>
  <rdf:Description rdf:about="jc3iedm_OBJECT-TYPE.owl#MILITARY-OBSTACLE-TYPE">
    <rdf:type rdf:resource="http://www.w3.org/2002/07/owl#Class"/>
    <rdfs:label xml:lang="en">military obstacle type</rdfs:label>
    <rdfs:comment xml:lang="en">A FACILITY-TYPE that is a class of man-made devices or passive defence works that are designed to stop, impede, or divert movement of amphibious or ground forces.</rdfs:comment>
    <rdfs:subClassOf rdf:resource="jc3iedm_OBJECT-TYPE.owl#FACILITY-TYPE"/>
  </rdf:Description>
  <rdf:Description rdf:about="jc3iedm_OBJECT-TYPE.owl#materiel-type-supply-class-code">
    <rdf:type rdf:resource="http://www.w3.org/2002/07/owl#DatatypeProperty"/>
    <rdfs:domain rdf:resource="jc3iedm_OBJECT-TYPE.owl#MATERIEL-TYPE"/>
    <rdfs:range rdf:resource="http://www.w3.org/2001/XMLSchema#string"/>
  </rdf:Description>
  <rdf:Description rdf:about="jc3iedm_OBJECT-TYPE.owl#vessel-type-acoustic-merit-index-quantity">
    <rdf:type rdf:resource="http://www.w3.org/2002/07/owl#DatatypeProperty"/>
    <rdfs:domain rdf:resource="jc3iedm_OBJECT-TYPE.owl#VESSEL-TYPE"/>
  </rdf:Description>
  <rdf:Description rdf:about="#FACILITY-TYPE_Cleared_way/firebreak">
    <rdfs:subClassOf rdf:resource="jc3iedm_OBJECT-TYPE.owl#FACILITY-TYPE"/>
    <rdfs:label xml:lang="en">cleared way/firebreak</rdfs:label>
    <rdfs:comment xml:lang="en">A man-made clearing in a cultural area or through a stand of trees, designed to provide access for a road, railroad, pipeline or power transmission line, or to impede the progress of forest fires.</rdfs:comment>
    <rdf:type rdf:resource="http://www.w3.org/2002/07/owl#Class"/>
  </rdf:Description>
  <rdf:Description rdf:about="#CONTROL-FEATURE-TYPE_Final_approach_fix">
    <rdfs:subClassOf rdf:resource="jc3iedm_OBJECT-TYPE.owl#CONTROL-FEATURE-TYPE"/>
    <rdfs:label xml:lang="en">final approach fix</rdfs:label>
    <rdfs:comment xml:lang="en">The point in a non-precision approach where the final approach normally begins.</rdfs:comment>
    <rdf:type rdf:resource="http://www.w3.org/2002/07/owl#Class"/>
  </rdf:Description>
  <rdf:Description rdf:about="jc3iedm_OBJECT-TYPE.owl#OBJECT-TYPE">
    <rdf:type rdf:resource="http://www.w3.org/2002/07/owl#Class"/>
    <rdfs:label xml:lang="en">object type</rdfs:label>
    <rdfs:comment xml:lang="en">An individually identified class of objects that has military or civilian significance.</rdfs:comment>
  </rdf:Description>
  <rdf:Description rdf:about="jc3iedm_OBJECT-TYPE.owl#private-sector-organisation-type-main-activity-code">
    <rdf:type rdf:resource="http://www.w3.org/2002/07/owl#DatatypeProperty"/>
    <rdfs:domain rdf:resource="jc3iedm_OBJECT-TYPE.owl#PRIVATE-SECTOR-ORGANISATION-TYPE"/>
    <rdfs:range rdf:resource="http://www.w3.org/2001/XMLSchema#string"/>
  </rdf:Description>
  <rdf:Description rdf:about="#CHEMICAL-MATERIEL-TYPE_Incapacitating_agent">
    <rdfs:subClassOf rdf:resource="jc3iedm_OBJECT-TYPE.owl#CHEMICAL-MATERIEL-TYPE"/>
    <rdfs:label xml:lang="en">incapacitating agent</rdfs:label>
    <rdfs:comment xml:lang="en">A CHEMICAL-MATERIEL-TYPE that prevents a human from functioning in a normal way.</rdfs:comment>
    <rdf:type rdf:resource="http://www.w3.org/2002/07/owl#Class"/>
  </rdf:Description>
  <rdf:Description rdf:about="#CONTROL-FEATURE-TYPE_Report_point">
    <rdfs:subClassOf rdf:resource="jc3iedm_OBJECT-TYPE.owl#CONTROL-FEATURE-TYPE"/>
    <rdfs:label xml:lang="en">report point</rdfs:label>
    <rdfs:comment xml:lang="en">A CONTROL-FEATURE-TYPE that identifies a point at which troops, after having reached it, must report to their command.</rdfs:comment>
    <rdf:type rdf:resource="http://www.w3.org/2002/07/owl#Class"/>
  </rdf:Description>
  <rdf:Description rdf:about="#CONTROL-FEATURE-TYPE_Spread_point">
    <rdfs:subClassOf rdf:resource="jc3iedm_OBJECT-TYPE.owl#CONTROL-FEATURE-TYPE"/>
    <rdfs:label xml:lang="en">spread point</rdfs:label>
    <rdfs:comment xml:lang="en">A CONTROL-FEATURE-TYPE that identifies a point where aircraft separate during a mission.</rdfs:comment>
    <rdf:type rdf:resource="http://www.w3.org/2002/07/owl#Class"/>
  </rdf:Description>
  <rdf:Description rdf:about="#SURFACE-VESSEL-TYPE_Communications_ship,_small">
    <rdfs:subClassOf rdf:resource="jc3iedm_OBJECT-TYPE.owl#SURFACE-VESSEL-TYPE"/>
    <rdfs:label xml:lang="en">communications ship, small</rdfs:label>
    <rdfs:comment xml:lang="en">Small auxiliary optimised for communications duties.</rdfs:comment>
    <rdf:type rdf:resource="http://www.w3.org/2002/07/owl#Class"/>
  </rdf:Description>
  <rdf:Description rdf:about="#SURFACE-VESSEL-TYPE_Minelayer,_support_ship">
    <rdfs:subClassOf rdf:resource="jc3iedm_OBJECT-TYPE.owl#SURFACE-VESSEL-TYPE"/>
    <rdfs:label xml:lang="en">minelayer, support ship</rdfs:label>
    <rdfs:comment xml:lang="en">A large armed ship (over 90 metres) capable of extensive minelaying, but not capable of speeds over 30 knots - 55 km/hr, with the facilities for command and control of mine warfare ships and boats in combat environment. Has limited support capability.</rdfs:comment>
    <rdf:type rdf:resource="http://www.w3.org/2002/07/owl#Class"/>
  </rdf:Description>
  <rdf:Description rdf:about="#FACILITY-TYPE_Warehouse">
    <rdfs:subClassOf rdf:resource="jc3iedm_OBJECT-TYPE.owl#FACILITY-TYPE"/>
    <rdfs:label xml:lang="en">warehouse</rdfs:label>
    <rdfs:comment xml:lang="en">A facility for the receipt, classification, storage, accounting, issue, maintenance, procurement, manufacture, assembly, research, salvage or disposal of material.</rdfs:comment>
    <rdf:type rdf:resource="http://www.w3.org/2002/07/owl#Class"/>
  </rdf:Description>
  <rdf:Description rdf:about="#FACILITY-TYPE_Relay_facility">
    <rdfs:subClassOf rdf:resource="jc3iedm_OBJECT-TYPE.owl#FACILITY-TYPE"/>
    <rdfs:label xml:lang="en">relay facility</rdfs:label>
    <rdfs:comment xml:lang="en">An installation organised, equipped, and located for the purpose of extending the coverage of electronic communications and detection.</rdfs:comment>
    <rdf:type rdf:resource="http://www.w3.org/2002/07/owl#Class"/>
  </rdf:Description>
  <rdf:Description rdf:about="jc3iedm_OBJECT-TYPE.owl#consumable-materiel-type-issuing-unit-of-measure-code">
    <rdf:type rdf:resource="http://www.w3.org/2002/07/owl#DatatypeProperty"/>
    <rdfs:domain rdf:resource="jc3iedm_OBJECT-TYPE.owl#CONSUMABLE-MATERIEL-TYPE"/>
    <rdfs:range rdf:resource="http://www.w3.org/2001/XMLSchema#string"/>
  </rdf:Description>
  <rdf:Description rdf:about="#PERSON-TYPE_Not_known">
    <rdfs:subClassOf rdf:resource="jc3iedm_OBJECT-TYPE.owl#PERSON-TYPE"/>
    <rdfs:label xml:lang="en">not known</rdfs:label>
    <rdfs:comment xml:lang="en">It is not possible to determine which value is most applicable.</rdfs:comment>
    <rdf:type rdf:resource="http://www.w3.org/2002/07/owl#Class"/>
  </rdf:Description>
  <rdf:Description rdf:about="#SURFACE-VESSEL-TYPE_Aircraft_carrier,_nuclear_powered">
    <rdfs:subClassOf rdf:resource="jc3iedm_OBJECT-TYPE.owl#SURFACE-VESSEL-TYPE"/>
    <rdfs:label xml:lang="en">aircraft carrier, nuclear powered</rdfs:label>
    <rdfs:comment xml:lang="en">Designator for multi-role aircraft carriers with nuclear power.</rdfs:comment>
    <rdf:type rdf:resource="http://www.w3.org/2002/07/owl#Class"/>
  </rdf:Description>
  <rdf:Description rdf:about="#ORGANISATION-TYPE_Not_otherwise_specified">
    <rdfs:label xml:lang="en">not otherwise specified</rdfs:label>
    <rdfs:subClassOf rdf:resource="jc3iedm_OBJECT-TYPE.owl#ORGANISATION-TYPE"/>
    <rdfs:comment xml:lang="en">The appropriate value is not in the set of specified values.</rdfs:comment>
    <rdf:type rdf:resource="http://www.w3.org/2002/07/owl#Class"/>
  </rdf:Description>
  <rdf:Description rdf:about="#CONTROL-FEATURE-TYPE_Zone_I">
    <rdfs:subClassOf rdf:resource="jc3iedm_OBJECT-TYPE.owl#CONTROL-FEATURE-TYPE"/>
    <rdfs:label xml:lang="en">zone i</rdfs:label>
    <rdfs:comment xml:lang="en">A circular area of Immediate Operational Concern where exposed, unprotected personnel may receive doses of 150 cGy or greater in relatively short periods of time (less than 4 hours after actual arrival of fallout). Major disruptions to unit operations and casualties may occur in some parts of this zone. However, radiation risk category for emergency risk is changing from 150 cGy to 125 cGy. Zone I is calculated on the basis of the weapon size and downwind speed. The boundary for Zone 1 is determined by drawing 2 lines tangent to the cloud radius circle and intersecting the points on the radial lines where the Zone 1 downwind distance arc intersects these lines.</rdfs:comment>
    <rdf:type rdf:resource="http://www.w3.org/2002/07/owl#Class"/>
  </rdf:Description>
  <rdf:Description rdf:about="#SURFACE-VESSEL-TYPE_Patrol_craft,_police">
    <rdfs:subClassOf rdf:resource="jc3iedm_OBJECT-TYPE.owl#SURFACE-VESSEL-TYPE"/>
    <rdfs:label xml:lang="en">patrol craft, police</rdfs:label>
    <rdfs:comment xml:lang="en">Police operated vessel in size range 35-55 metres designed and fitted primarily for escort duties in ASW role.</rdfs:comment>
    <rdf:type rdf:resource="http://www.w3.org/2002/07/owl#Class"/>
  </rdf:Description>
  <rdf:Description rdf:about="#FACILITY-TYPE_Heliport">
    <rdfs:subClassOf rdf:resource="jc3iedm_OBJECT-TYPE.owl#FACILITY-TYPE"/>
    <rdfs:label xml:lang="en">heliport</rdfs:label>
    <rdfs:comment xml:lang="en">A place designated for the landing and takeoff of helicopters, including its buildings and facilities.</rdfs:comment>
    <rdf:type rdf:resource="http://www.w3.org/2002/07/owl#Class"/>
  </rdf:Description>
  <rdf:Description rdf:about="#FACILITY-TYPE_Site,_ground_surveillance_radar">
    <rdfs:subClassOf rdf:resource="jc3iedm_OBJECT-TYPE.owl#FACILITY-TYPE"/>
    <rdfs:label xml:lang="en">site, ground surveillance radar</rdfs:label>
    <rdfs:comment xml:lang="en">A facility containing radar employed for ground surveillance purposes.</rdfs:comment>
    <rdf:type rdf:resource="http://www.w3.org/2002/07/owl#Class"/>
  </rdf:Description>
  <rdf:Description rdf:about="#VEHICLE-TYPE_Cart">
    <rdfs:subClassOf rdf:resource="jc3iedm_OBJECT-TYPE.owl#VEHICLE-TYPE"/>
    <rdfs:label xml:lang="en">cart</rdfs:label>
    <rdfs:comment xml:lang="en">A non self-propelled vehicle with two or four wheels for carrying loads.</rdfs:comment>
    <rdf:type rdf:resource="http://www.w3.org/2002/07/owl#Class"/>
  </rdf:Description>
  <rdf:Description rdf:about="#SURFACE-VESSEL-TYPE_Minesweeper,_auxiliary">
    <rdfs:subClassOf rdf:resource="jc3iedm_OBJECT-TYPE.owl#SURFACE-VESSEL-TYPE"/>
    <rdfs:label xml:lang="en">minesweeper, auxiliary</rdfs:label>
    <rdfs:comment xml:lang="en">Any seagoing ship not designed as a minesweeper but converted to such use.</rdfs:comment>
    <rdf:type rdf:resource="http://www.w3.org/2002/07/owl#Class"/>
  </rdf:Description>
  <rdf:Description rdf:about="#CONTROL-FEATURE-TYPE_Restricted_area">
    <rdfs:subClassOf rdf:resource="jc3iedm_OBJECT-TYPE.owl#CONTROL-FEATURE-TYPE"/>
    <rdfs:label xml:lang="en">restricted area</rdfs:label>
    <rdfs:comment xml:lang="en">An airspace of defined dimensions, above the land areas or territorial waters of a state, within which the flight of aircraft is restricted in accordance with certain specified conditions.</rdfs:comment>
    <rdf:type rdf:resource="http://www.w3.org/2002/07/owl#Class"/>
  </rdf:Description>
  <rdf:Description rdf:about="#SURFACE-VESSEL-TYPE_Motor_yacht">
    <rdfs:subClassOf rdf:resource="jc3iedm_OBJECT-TYPE.owl#SURFACE-VESSEL-TYPE"/>
    <rdfs:label xml:lang="en">motor yacht</rdfs:label>
    <rdfs:comment xml:lang="en">Vessel, usually associated with luxury living accommodation, powered by inboard engines.</rdfs:comment>
    <rdf:type rdf:resource="http://www.w3.org/2002/07/owl#Class"/>
  </rdf:Description>
  <rdf:Description rdf:about="#MISCELLANEOUS-EQUIPMENT-TYPE_Magnetic_tape">
    <rdfs:subClassOf rdf:resource="jc3iedm_OBJECT-TYPE.owl#MISCELLANEOUS-EQUIPMENT-TYPE"/>
    <rdfs:label xml:lang="en">magnetic tape</rdfs:label>
    <rdfs:comment xml:lang="en">A tape coated or impregnated with a magnetic material or made of magnetic material intended for data recording.</rdfs:comment>
    <rdf:type rdf:resource="http://www.w3.org/2002/07/owl#Class"/>
  </rdf:Description>
  <rdf:Description rdf:about="#MISCELLANEOUS-EQUIPMENT-TYPE_Film">
    <rdfs:subClassOf rdf:resource="jc3iedm_OBJECT-TYPE.owl#MISCELLANEOUS-EQUIPMENT-TYPE"/>
    <rdfs:label xml:lang="en">film</rdfs:label>
    <rdfs:comment xml:lang="en">A thin flexible transparent material for recording imagery.</rdfs:comment>
    <rdf:type rdf:resource="http://www.w3.org/2002/07/owl#Class"/>
  </rdf:Description>
  <rdf:Description rdf:about="#CHEMICAL-MATERIEL-TYPE_G-agent">
    <rdfs:subClassOf rdf:resource="jc3iedm_OBJECT-TYPE.owl#CHEMICAL-MATERIEL-TYPE"/>
    <rdfs:label xml:lang="en">g agent</rdfs:label>
    <rdfs:comment xml:lang="en">The types of organophosphorus nerve gases.</rdfs:comment>
    <rdf:type rdf:resource="http://www.w3.org/2002/07/owl#Class"/>
  </rdf:Description>
  <rdf:Description rdf:about="#MILITARY-OBSTACLE-TYPE_Trip_wire">
    <rdfs:subClassOf rdf:resource="jc3iedm_OBJECT-TYPE.owl#MILITARY-OBSTACLE-TYPE"/>
    <rdfs:label xml:lang="en">trip wire</rdfs:label>
    <rdfs:comment xml:lang="en">No definition provided in APP-6A.</rdfs:comment>
    <rdf:type rdf:resource="http://www.w3.org/2002/07/owl#Class"/>
  </rdf:Description>
  <rdf:Description rdf:about="#CBRN-EQUIPMENT-TYPE_Automated_chemical_detector">
    <rdfs:subClassOf rdf:resource="jc3iedm_OBJECT-TYPE.owl#CBRN-EQUIPMENT-TYPE"/>
    <rdfs:label xml:lang="en">automated chemical detector</rdfs:label>
    <rdfs:comment xml:lang="en">An unattended chemical detection and alarm system.</rdfs:comment>
    <rdf:type rdf:resource="http://www.w3.org/2002/07/owl#Class"/>
  </rdf:Description>
  <rdf:Description rdf:about="#FACILITY-TYPE_Airborne_early_warning_ground_facility">
    <rdfs:subClassOf rdf:resource="jc3iedm_OBJECT-TYPE.owl#FACILITY-TYPE"/>
    <rdfs:label xml:lang="en">airborne early warning ground facility</rdfs:label>
    <rdfs:comment xml:lang="en">A facility on the ground that has an electromagnetic link to an airborne early warning system.</rdfs:comment>
    <rdf:type rdf:resource="http://www.w3.org/2002/07/owl#Class"/>
  </rdf:Description>
  <rdf:Description rdf:about="#CONTROL-FEATURE-TYPE_Area_of_operations">
    <rdfs:subClassOf rdf:resource="jc3iedm_OBJECT-TYPE.owl#CONTROL-FEATURE-TYPE"/>
    <rdfs:label xml:lang="en">area of operations</rdfs:label>
    <rdfs:comment xml:lang="en">That portion of an area necessary for military operations and for the administration of such operations. Army--A geographical area, usually defined by lateral, forward, and rear boundaries assigned to a commander, by a higher commander, in which he has responsibility and the authority to conduct military operations.</rdfs:comment>
    <rdf:type rdf:resource="http://www.w3.org/2002/07/owl#Class"/>
  </rdf:Description>
  <rdf:Description rdf:about="#MARITIME-EQUIPMENT-TYPE_Towed_array_surveillance_system">
    <rdfs:subClassOf rdf:resource="jc3iedm_OBJECT-TYPE.owl#MARITIME-EQUIPMENT-TYPE"/>
    <rdfs:label xml:lang="en">towed array surveillance system</rdfs:label>
    <rdfs:comment xml:lang="en">No definition provided in ADatP-3 Baseline 13.1 FFIRN/FUD 1434/1.</rdfs:comment>
    <rdf:type rdf:resource="http://www.w3.org/2002/07/owl#Class"/>
  </rdf:Description>
  <rdf:Description rdf:about="#VEHICLE-TYPE_Utility">
    <rdfs:subClassOf rdf:resource="jc3iedm_OBJECT-TYPE.owl#VEHICLE-TYPE"/>
    <rdfs:label xml:lang="en">utility</rdfs:label>
    <rdfs:comment xml:lang="en">A small, sturdy, four-wheel-drive vehicle, used chiefly for reconnaissance; a similar vehicle in non-military use.</rdfs:comment>
    <rdf:type rdf:resource="http://www.w3.org/2002/07/owl#Class"/>
  </rdf:Description>
  <rdf:Description rdf:about="#FACILITY-TYPE_Casualty_collection_point">
    <rdfs:subClassOf rdf:resource="jc3iedm_OBJECT-TYPE.owl#FACILITY-TYPE"/>
    <rdfs:label xml:lang="en">casualty collection point</rdfs:label>
    <rdfs:comment xml:lang="en">A facility where casualties are assembled to be transported to a medical treatment facility for example a company aid post.</rdfs:comment>
    <rdf:type rdf:resource="http://www.w3.org/2002/07/owl#Class"/>
  </rdf:Description>
  <rdf:Description rdf:about="#MILITARY-OBSTACLE-TYPE_Wire_obstacle,_high_wire_fence">
    <rdfs:subClassOf rdf:resource="jc3iedm_OBJECT-TYPE.owl#MILITARY-OBSTACLE-TYPE"/>
    <rdfs:label xml:lang="en">wire obstacle, high wire fence</rdfs:label>
    <rdfs:comment xml:lang="en">No definition provided in APP-6A.</rdfs:comment>
    <rdf:type rdf:resource="http://www.w3.org/2002/07/owl#Class"/>
  </rdf:Description>
  <rdf:Description rdf:about="#SURFACE-VESSEL-TYPE_Merchant_ship,_inland_waterway">
    <rdfs:subClassOf rdf:resource="jc3iedm_OBJECT-TYPE.owl#SURFACE-VESSEL-TYPE"/>
    <rdfs:label xml:lang="en">merchant ship, inland waterway</rdfs:label>
    <rdfs:comment xml:lang="en">Non-naval ship primarily used to transport cargo via inland waterways.</rdfs:comment>
    <rdf:type rdf:resource="http://www.w3.org/2002/07/owl#Class"/>
  </rdf:Description>
  <rdf:Description rdf:about="#FACILITY-TYPE_Not_known">
    <rdfs:subClassOf rdf:resource="jc3iedm_OBJECT-TYPE.owl#FACILITY-TYPE"/>
    <rdfs:label xml:lang="en">not known</rdfs:label>
    <rdfs:comment xml:lang="en">It is not possible to determine which value is most applicable.</rdfs:comment>
    <rdf:type rdf:resource="http://www.w3.org/2002/07/owl#Class"/>
  </rdf:Description>
  <rdf:Description rdf:about="#ORGANISATION-TYPE_Ground_based_air_defence_operations_centre">
    <rdfs:subClassOf rdf:resource="jc3iedm_OBJECT-TYPE.owl#ORGANISATION-TYPE"/>
    <rdfs:label xml:lang="en">ground based air defence operations centre</rdfs:label>
    <rdfs:comment xml:lang="en">No definition provided in ADatP-3 Baseline 13.1 FFIRN/FUD 1874/4.</rdfs:comment>
    <rdf:type rdf:resource="http://www.w3.org/2002/07/owl#Class"/>
  </rdf:Description>
  <rdf:Description rdf:about="#FACILITY-TYPE_Bulk_fuel_installation,_field">
    <rdfs:subClassOf rdf:resource="jc3iedm_OBJECT-TYPE.owl#FACILITY-TYPE"/>
    <rdfs:label xml:lang="en">bulk fuel installation, field</rdfs:label>
    <rdfs:comment xml:lang="en">A facility containing fuel containers, pipe work and dispensing equipment connected together to form a temporary fuel installation within a tactical field location.</rdfs:comment>
    <rdf:type rdf:resource="http://www.w3.org/2002/07/owl#Class"/>
  </rdf:Description>
  <rdf:Description rdf:about="#CONTROL-FEATURE-TYPE_Refuelling_point">
    <rdfs:subClassOf rdf:resource="jc3iedm_OBJECT-TYPE.owl#CONTROL-FEATURE-TYPE"/>
    <rdfs:label xml:lang="en">refuelling point</rdfs:label>
    <rdfs:comment xml:lang="en">The aircraft, ship or other vehicle will refuel at this point.</rdfs:comment>
    <rdf:type rdf:resource="http://www.w3.org/2002/07/owl#Class"/>
  </rdf:Description>
  <rdf:Description rdf:about="#AIRFIELD-TYPE_Joint">
    <rdfs:subClassOf rdf:resource="jc3iedm_OBJECT-TYPE.owl#AIRFIELD-TYPE"/>
    <rdfs:label xml:lang="en">joint</rdfs:label>
    <rdfs:comment xml:lang="en">Joint (civil and military) airports jointly controlled, used or operated by both civil and military agencies.</rdfs:comment>
    <rdf:type rdf:resource="http://www.w3.org/2002/07/owl#Class"/>
  </rdf:Description>
  <rdf:Description rdf:about="#CONTROL-FEATURE-TYPE_Aim_point">
    <rdfs:subClassOf rdf:resource="jc3iedm_OBJECT-TYPE.owl#CONTROL-FEATURE-TYPE"/>
    <rdfs:label xml:lang="en">aim point</rdfs:label>
    <rdfs:comment xml:lang="en">A point associated with a target and assigned for a specific weapon impact.</rdfs:comment>
    <rdf:type rdf:resource="http://www.w3.org/2002/07/owl#Class"/>
  </rdf:Description>
  <rdf:Description rdf:about="#CONTROL-FEATURE-TYPE_Termination_point">
    <rdfs:subClassOf rdf:resource="jc3iedm_OBJECT-TYPE.owl#CONTROL-FEATURE-TYPE"/>
    <rdfs:label xml:lang="en">termination point</rdfs:label>
    <rdfs:comment xml:lang="en">The aircraft, ship or other vehicle will terminate its mission at this route point.</rdfs:comment>
    <rdf:type rdf:resource="http://www.w3.org/2002/07/owl#Class"/>
  </rdf:Description>
  <rdf:Description rdf:about="#CONTROL-FEATURE-TYPE_Amphibious_operation_area">
    <rdfs:subClassOf rdf:resource="jc3iedm_OBJECT-TYPE.owl#CONTROL-FEATURE-TYPE"/>
    <rdfs:label xml:lang="en">amphibious operation area</rdfs:label>
    <rdfs:comment xml:lang="en">A CONTROL-FEATURE-TYPE with an area location, delineated in the initiating directive, for purposes of command and control within which is located the objective(s) to be secured by the amphibious task force.</rdfs:comment>
    <rdf:type rdf:resource="http://www.w3.org/2002/07/owl#Class"/>
  </rdf:Description>
  <rdf:Description rdf:about="#FACILITY-TYPE_Windmill">
    <rdfs:subClassOf rdf:resource="jc3iedm_OBJECT-TYPE.owl#FACILITY-TYPE"/>
    <rdfs:label xml:lang="en">windmill</rdfs:label>
    <rdfs:comment xml:lang="en">A wind-driven system of vanes attached to a tower-like structure (excluding wind-generated power plants).</rdfs:comment>
    <rdf:type rdf:resource="http://www.w3.org/2002/07/owl#Class"/>
  </rdf:Description>
  <rdf:Description rdf:about="#SURFACE-VESSEL-TYPE_Research_ship">
    <rdfs:subClassOf rdf:resource="jc3iedm_OBJECT-TYPE.owl#SURFACE-VESSEL-TYPE"/>
    <rdfs:label xml:lang="en">research ship</rdfs:label>
    <rdfs:comment xml:lang="en">Ship 49 metres or more used to conduct tests, experiments and/or research.</rdfs:comment>
    <rdf:type rdf:resource="http://www.w3.org/2002/07/owl#Class"/>
  </rdf:Description>
  <rdf:Description rdf:about="#SURFACE-VESSEL-TYPE_Patrol_craft,_harbor">
    <rdfs:subClassOf rdf:resource="jc3iedm_OBJECT-TYPE.owl#SURFACE-VESSEL-TYPE"/>
    <rdfs:label xml:lang="en">patrol craft, harbor</rdfs:label>
    <rdfs:comment xml:lang="en">Craft used primarily for training personnel for service aboard patrol types. However, may be armed and used as a Patrol boat, general.</rdfs:comment>
    <rdf:type rdf:resource="http://www.w3.org/2002/07/owl#Class"/>
  </rdf:Description>
  <rdf:Description rdf:about="#MILITARY-POST-TYPE_Pathology_physician">
    <rdfs:subClassOf rdf:resource="jc3iedm_OBJECT-TYPE.owl#MILITARY-POST-TYPE"/>
    <rdfs:label xml:lang="en">pathology physician</rdfs:label>
    <rdfs:comment xml:lang="en">A MILITARY-POST-TYPE that is identified as a physician specialising in Pathology.</rdfs:comment>
    <rdf:type rdf:resource="http://www.w3.org/2002/07/owl#Class"/>
  </rdf:Description>
  <rdf:Description rdf:about="#MATERIEL-TYPE_Not_otherwise_specified">
    <rdfs:subClassOf rdf:resource="jc3iedm_OBJECT-TYPE.owl#MATERIEL-TYPE"/>
    <rdfs:label xml:lang="en">not otherwise specified</rdfs:label>
    <rdfs:comment xml:lang="en">The appropriate value is not in the set of specified values.</rdfs:comment>
    <rdf:type rdf:resource="http://www.w3.org/2002/07/owl#Class"/>
  </rdf:Description>
  <rdf:Description rdf:about="#SURFACE-VESSEL-TYPE_Barge,_disposal,_nuclear_waste">
    <rdfs:subClassOf rdf:resource="jc3iedm_OBJECT-TYPE.owl#SURFACE-VESSEL-TYPE"/>
    <rdfs:label xml:lang="en">barge, disposal, nuclear waste</rdfs:label>
    <rdfs:comment xml:lang="en">Barge specifically designed for the disposal of nuclear waste.</rdfs:comment>
    <rdf:type rdf:resource="http://www.w3.org/2002/07/owl#Class"/>
  </rdf:Description>
  <rdf:Description rdf:about="#ROUTE-TYPE_Reference_track">
    <rdfs:subClassOf rdf:resource="jc3iedm_OBJECT-TYPE.owl#ROUTE-TYPE"/>
    <rdfs:label xml:lang="en">reference track</rdfs:label>
    <rdfs:comment xml:lang="en">The prescribed reference line over the ground along which the centre of the mine counter measures gear must travel.</rdfs:comment>
    <rdf:type rdf:resource="http://www.w3.org/2002/07/owl#Class"/>
  </rdf:Description>
  <rdf:Description rdf:about="#FACILITY-TYPE_Communications_building">
    <rdfs:subClassOf rdf:resource="jc3iedm_OBJECT-TYPE.owl#FACILITY-TYPE"/>
    <rdfs:label xml:lang="en">communications building</rdfs:label>
    <rdfs:comment xml:lang="en">A building in which communications signals are processed or controlled.</rdfs:comment>
    <rdf:type rdf:resource="http://www.w3.org/2002/07/owl#Class"/>
  </rdf:Description>
  <rdf:Description rdf:about="#MILITARY-OBSTACLE-TYPE_Demolition_debris_obstacle">
    <rdfs:subClassOf rdf:resource="jc3iedm_OBJECT-TYPE.owl#MILITARY-OBSTACLE-TYPE"/>
    <rdfs:label xml:lang="en">demolition debris obstacle</rdfs:label>
    <rdfs:comment xml:lang="en">Debris obtained from the demolition of an object in order to be used as an obstacle.</rdfs:comment>
    <rdf:type rdf:resource="http://www.w3.org/2002/07/owl#Class"/>
  </rdf:Description>
  <rdf:Description rdf:about="#SURFACE-VESSEL-TYPE_Minesweeper,_river">
    <rdfs:subClassOf rdf:resource="jc3iedm_OBJECT-TYPE.owl#SURFACE-VESSEL-TYPE"/>
    <rdfs:label xml:lang="en">minesweeper, river</rdfs:label>
    <rdfs:comment xml:lang="en">Shallow water minesweeper in size range 12.5 - 25 metres which has been armoured to provide protection for crew in close combat situations. In the USN a converted lCM-6 known as MSM.</rdfs:comment>
    <rdf:type rdf:resource="http://www.w3.org/2002/07/owl#Class"/>
  </rdf:Description>
  <rdf:Description rdf:about="#FACILITY-TYPE_Field_storage_site-ammunition">
    <rdfs:subClassOf rdf:resource="jc3iedm_OBJECT-TYPE.owl#FACILITY-TYPE"/>
    <rdfs:label xml:lang="en">field storage site ammunition</rdfs:label>
    <rdfs:comment xml:lang="en">A facility with a group of field storage modules containing a max of 200 tonnes gross weight of ammunition and explosives.</rdfs:comment>
    <rdf:type rdf:resource="http://www.w3.org/2002/07/owl#Class"/>
  </rdf:Description>
  <rdf:Description rdf:about="#CONSUMABLE-MATERIEL-TYPE_Map">
    <rdfs:subClassOf rdf:resource="jc3iedm_OBJECT-TYPE.owl#CONSUMABLE-MATERIEL-TYPE"/>
    <rdfs:label xml:lang="en">map</rdfs:label>
    <rdfs:comment xml:lang="en">A piece of paper that is a graphic representation of a part or the whole of the earth.</rdfs:comment>
    <rdf:type rdf:resource="http://www.w3.org/2002/07/owl#Class"/>
  </rdf:Description>
  <rdf:Description rdf:about="#UNIT-TYPE_Not_known">
    <rdfs:label xml:lang="en">not known</rdfs:label>
    <rdfs:subClassOf rdf:resource="jc3iedm_OBJECT-TYPE.owl#UNIT-TYPE"/>
    <rdfs:comment xml:lang="en">It is not possible to determine which value is most applicable.</rdfs:comment>
    <rdf:type rdf:resource="http://www.w3.org/2002/07/owl#Class"/>
  </rdf:Description>
  <rdf:Description rdf:about="#CHEMICAL-MATERIEL-TYPE_Toxic_industrial_material">
    <rdfs:subClassOf rdf:resource="jc3iedm_OBJECT-TYPE.owl#CHEMICAL-MATERIEL-TYPE"/>
    <rdfs:label xml:lang="en">toxic industrial material</rdfs:label>
    <rdfs:comment xml:lang="en">A generic term for a CHEMICAL-MATERIEL-TYPE compound found in solid, liquid, aerosolised or gaseous form. It may be used, or stored for use, for industrial, commercial, medical, military or domestic purposes.</rdfs:comment>
    <rdf:type rdf:resource="http://www.w3.org/2002/07/owl#Class"/>
  </rdf:Description>
  <rdf:Description rdf:about="#SURFACE-VESSEL-TYPE_Patrol_combatant,_guided_missile,_hydrofoil">
    <rdfs:subClassOf rdf:resource="jc3iedm_OBJECT-TYPE.owl#SURFACE-VESSEL-TYPE"/>
    <rdfs:label xml:lang="en">patrol combatant, guided missile, hydrofoil</rdfs:label>
    <rdfs:comment xml:lang="en">Patrol, blockade and surveillance ship in range 45-85 metres overall. Designed to operate in other than open ocean areas. Has special mission of attacking hostile ships. Must have at least 76mm main armament. It is fitted with one or more force guided missile systems and is fitted with hydrofoils.</rdfs:comment>
    <rdf:type rdf:resource="http://www.w3.org/2002/07/owl#Class"/>
  </rdf:Description>
  <rdf:Description rdf:about="#AMMUNITION-TYPE_Surface-to-surface_missile">
    <rdfs:subClassOf rdf:resource="jc3iedm_OBJECT-TYPE.owl#AMMUNITION-TYPE"/>
    <rdfs:label xml:lang="en">surface to surface missile</rdfs:label>
    <rdfs:comment xml:lang="en">A self-propelled airborne munition which is guided automatically, or by remote control, fired from the ground or vessel at an object on the ground or sea.</rdfs:comment>
    <rdf:type rdf:resource="http://www.w3.org/2002/07/owl#Class"/>
  </rdf:Description>
  <rdf:Description rdf:about="#FACILITY-TYPE_Loading_platform">
    <rdfs:subClassOf rdf:resource="jc3iedm_OBJECT-TYPE.owl#FACILITY-TYPE"/>
    <rdfs:label xml:lang="en">loading platform</rdfs:label>
    <rdfs:comment xml:lang="en">A facility constructed for loading goods/equipment.</rdfs:comment>
    <rdf:type rdf:resource="http://www.w3.org/2002/07/owl#Class"/>
  </rdf:Description>
  <rdf:Description rdf:about="#SURFACE-VESSEL-TYPE_Torpedo_boat,_hydrofoil">
    <rdfs:subClassOf rdf:resource="jc3iedm_OBJECT-TYPE.owl#SURFACE-VESSEL-TYPE"/>
    <rdfs:label xml:lang="en">torpedo boat, hydrofoil</rdfs:label>
    <rdfs:comment xml:lang="en">High-speed (35 knots - 65 km/hr) anti-surface ship patrol craft in size range 20 - 30 metres fitted with torpedoes, fitted with hydrofoils.</rdfs:comment>
    <rdf:type rdf:resource="http://www.w3.org/2002/07/owl#Class"/>
  </rdf:Description>
  <rdf:Description rdf:about="#SURFACE-VESSEL-TYPE_Not_known">
    <rdfs:subClassOf rdf:resource="jc3iedm_OBJECT-TYPE.owl#SURFACE-VESSEL-TYPE"/>
    <rdfs:label xml:lang="en">not known</rdfs:label>
    <rdfs:comment xml:lang="en">It is not possible to determine which value is most applicable.</rdfs:comment>
    <rdf:type rdf:resource="http://www.w3.org/2002/07/owl#Class"/>
  </rdf:Description>
  <rdf:Description rdf:about="jc3iedm_OBJECT-TYPE.owl#airfield-type-use-category-code">
    <rdf:type rdf:resource="http://www.w3.org/2002/07/owl#DatatypeProperty"/>
    <rdfs:domain rdf:resource="jc3iedm_OBJECT-TYPE.owl#AIRFIELD-TYPE"/>
    <rdfs:range rdf:resource="http://www.w3.org/2001/XMLSchema#string"/>
  </rdf:Description>
  <rdf:Description rdf:about="#MISCELLANEOUS-EQUIPMENT-TYPE_Low_altitude_parachute_extraction_system">
    <rdfs:subClassOf rdf:resource="jc3iedm_OBJECT-TYPE.owl#MISCELLANEOUS-EQUIPMENT-TYPE"/>
    <rdfs:label xml:lang="en">low altitude parachute extraction system</rdfs:label>
    <rdfs:comment xml:lang="en">A low-level, self-contained system capable of delivering heavy loads into an area where air landing is not feasible from an optimum aircraft wheel altitude of 5 to 10 feet above ground level.</rdfs:comment>
    <rdf:type rdf:resource="http://www.w3.org/2002/07/owl#Class"/>
  </rdf:Description>
</rdf:RDF>
