<rdf:RDF
    xmlns="http://cbml.googlecode.com/svn/trunk/jc3iedmOnt/rootClassOnt/jc3iedm_ACTIONExtended.owl#"
    xmlns:rdf="http://www.w3.org/1999/02/22-rdf-syntax-ns#"
    xmlns:owl="http://www.w3.org/2002/07/owl#"
    xmlns:xsd="http://www.w3.org/2001/XMLSchema#"
    xmlns:rdfs="http://www.w3.org/2000/01/rdf-schema#"
  xml:base="http://cbml.googlecode.com/svn/trunk/jc3iedmOnt/rootClassOnt/">
  <owl:Ontology rdf:about="jc3iedm_ACTIONExtended.owl#">
    <owl:imports rdf:resource="jc3iedm_ACTION.owl#"/>
  </owl:Ontology>
  <owl:Class rdf:about="jc3iedm_ACTIONExtended.owl#ACTION-EVENT_Providing_agricultural_support">
    <rdfs:subClassOf rdf:resource="jc3iedm_ACTION.owl#ACTION-EVENT"/>
    <rdfs:subClassOf>
      <owl:Restriction>
        <owl:hasValue xml:lang="en">PRVAGR</owl:hasValue>
        <owl:onProperty rdf:resource="jc3iedm_ACTION.owl#action-event-category-code"/>
      </owl:Restriction>
    </rdfs:subClassOf>
    <rdfs:label xml:lang="en">providing agricultural support</rdfs:label>
    <rdfs:comment xml:lang="en">Providing advice or supplies for cultivating the soil and rearing animals.</rdfs:comment>
  </owl:Class>
  <owl:Class rdf:about="jc3iedm_ACTIONExtended.owl#ACTION-EVENT_Communications_disruption">
    <rdfs:subClassOf rdf:resource="jc3iedm_ACTION.owl#ACTION-EVENT"/>
    <rdfs:subClassOf>
      <owl:Restriction>
        <owl:hasValue xml:lang="en">COMDIS</owl:hasValue>
        <owl:onProperty rdf:resource="jc3iedm_ACTION.owl#action-event-category-code"/>
      </owl:Restriction>
    </rdfs:subClassOf>
    <rdfs:label xml:lang="en">communications disruption</rdfs:label>
    <rdfs:comment xml:lang="en">Interruption of the passage of communications by natural or man-made phenomena.</rdfs:comment>
  </owl:Class>
  <owl:Class rdf:about="jc3iedm_ACTIONExtended.owl#ACTION-EVENT_Seizing">
    <rdfs:subClassOf rdf:resource="jc3iedm_ACTION.owl#ACTION-EVENT"/>
    <rdfs:subClassOf>
      <owl:Restriction>
        <owl:hasValue xml:lang="en">SEIZNG</owl:hasValue>
        <owl:onProperty rdf:resource="jc3iedm_ACTION.owl#action-event-category-code"/>
      </owl:Restriction>
    </rdfs:subClassOf>
    <rdfs:label xml:lang="en">seizing</rdfs:label>
    <rdfs:comment xml:lang="en">Clearing a designated area and obtaining control of it.</rdfs:comment>
  </owl:Class>
  <owl:Class rdf:about="jc3iedm_ACTIONExtended.owl#ACTION-EVENT_Moving">
    <rdfs:subClassOf rdf:resource="jc3iedm_ACTION.owl#ACTION-EVENT"/>
    <rdfs:subClassOf>
      <owl:Restriction>
        <owl:hasValue xml:lang="en">MOVING</owl:hasValue>
        <owl:onProperty rdf:resource="jc3iedm_ACTION.owl#action-event-category-code"/>
      </owl:Restriction>
    </rdfs:subClassOf>
    <rdfs:label xml:lang="en">moving</rdfs:label>
    <rdfs:comment xml:lang="en">Changing position.</rdfs:comment>
  </owl:Class>
  <owl:Class rdf:about="jc3iedm_ACTIONExtended.owl#ACTION-EVENT_Fix">
    <rdfs:subClassOf rdf:resource="jc3iedm_ACTION.owl#ACTION-EVENT"/>
    <rdfs:subClassOf>
      <owl:Restriction>
        <owl:hasValue xml:lang="en">FIX</owl:hasValue>
        <owl:onProperty rdf:resource="jc3iedm_ACTION.owl#action-event-category-code"/>
      </owl:Restriction>
    </rdfs:subClassOf>
    <rdfs:label xml:lang="en">fix</rdfs:label>
    <rdfs:comment xml:lang="en">Preventing the enemy from moving any part of his force from a specific location for a specific period of time.</rdfs:comment>
  </owl:Class>
  <owl:Class rdf:about="jc3iedm_ACTIONExtended.owl#ACTION-EVENT_Surrender">
    <rdfs:subClassOf rdf:resource="jc3iedm_ACTION.owl#ACTION-EVENT"/>
    <rdfs:subClassOf>
      <owl:Restriction>
        <owl:hasValue xml:lang="en">SURREN</owl:hasValue>
        <owl:onProperty rdf:resource="jc3iedm_ACTION.owl#action-event-category-code"/>
      </owl:Restriction>
    </rdfs:subClassOf>
    <rdfs:label xml:lang="en">surrender</rdfs:label>
    <rdfs:comment xml:lang="en">Yielding to the control or power of the enemy.</rdfs:comment>
  </owl:Class>
  <owl:Class rdf:about="jc3iedm_ACTIONExtended.owl#ACTION-EVENT_POW_return">
    <rdfs:subClassOf rdf:resource="jc3iedm_ACTION.owl#ACTION-EVENT"/>
    <rdfs:subClassOf>
      <owl:Restriction>
        <owl:hasValue xml:lang="en">POWRET</owl:hasValue>
        <owl:onProperty rdf:resource="jc3iedm_ACTION.owl#action-event-category-code"/>
      </owl:Restriction>
    </rdfs:subClassOf>
    <rdfs:label xml:lang="en">pow return</rdfs:label>
    <rdfs:comment xml:lang="en">The arrival of a POW or a group of POWs to their own forces or country.</rdfs:comment>
  </owl:Class>
  <owl:Class rdf:about="jc3iedm_ACTIONExtended.owl#ACTION-EVENT_Attempted_murder">
    <rdfs:subClassOf rdf:resource="jc3iedm_ACTION.owl#ACTION-EVENT"/>
    <rdfs:subClassOf>
      <owl:Restriction>
        <owl:hasValue xml:lang="en">ATMRDR</owl:hasValue>
        <owl:onProperty rdf:resource="jc3iedm_ACTION.owl#action-event-category-code"/>
      </owl:Restriction>
    </rdfs:subClassOf>
    <rdfs:label xml:lang="en">attempted murder</rdfs:label>
    <rdfs:comment xml:lang="en">The attempted act of unlawfully killing of one human being by another, especially with premeditated malice.</rdfs:comment>
  </owl:Class>
  <owl:Class rdf:about="jc3iedm_ACTIONExtended.owl#CHEMICAL-BIOLOGICAL-EVENT_Chemical_alarm">
    <rdfs:subClassOf rdf:resource="jc3iedm_ACTION.owl#CHEMICAL-BIOLOGICAL-EVENT"/>
    <rdfs:subClassOf>
      <owl:Restriction>
        <owl:hasValue xml:lang="en">CHMALM</owl:hasValue>
        <owl:onProperty rdf:resource="jc3iedm_ACTION.owl#chemical-biological-event-category-code"/>
      </owl:Restriction>
    </rdfs:subClassOf>
    <rdfs:label xml:lang="en">chemical alarm</rdfs:label>
    <rdfs:comment xml:lang="en">An action by which a chemical detector is triggered or a group is warned.</rdfs:comment>
  </owl:Class>
  <owl:Class rdf:about="jc3iedm_ACTIONExtended.owl#ACTION-EVENT_Providing_decontamination_services">
    <rdfs:subClassOf rdf:resource="jc3iedm_ACTION.owl#ACTION-EVENT"/>
    <rdfs:subClassOf>
      <owl:Restriction>
        <owl:hasValue xml:lang="en">PRVDCN</owl:hasValue>
        <owl:onProperty rdf:resource="jc3iedm_ACTION.owl#action-event-category-code"/>
      </owl:Restriction>
    </rdfs:subClassOf>
    <rdfs:label xml:lang="en">providing decontamination services</rdfs:label>
    <rdfs:comment xml:lang="en">Providing purification of different items from contamination.</rdfs:comment>
  </owl:Class>
  <owl:Class rdf:about="jc3iedm_ACTIONExtended.owl#ACTION-EVENT_Treaty_violation">
    <rdfs:subClassOf rdf:resource="jc3iedm_ACTION.owl#ACTION-EVENT"/>
    <rdfs:subClassOf>
      <owl:Restriction>
        <owl:hasValue xml:lang="en">TREVIO</owl:hasValue>
        <owl:onProperty rdf:resource="jc3iedm_ACTION.owl#action-event-category-code"/>
      </owl:Restriction>
    </rdfs:subClassOf>
    <rdfs:label xml:lang="en">treaty violation</rdfs:label>
    <rdfs:comment xml:lang="en">An infringement or breaking of the provisions of a formal agreement.</rdfs:comment>
  </owl:Class>
  <owl:Class rdf:about="jc3iedm_ACTIONExtended.owl#ACTION-EVENT_Securing">
    <rdfs:subClassOf rdf:resource="jc3iedm_ACTION.owl#ACTION-EVENT"/>
    <rdfs:subClassOf>
      <owl:Restriction>
        <owl:hasValue xml:lang="en">SECRNG</owl:hasValue>
        <owl:onProperty rdf:resource="jc3iedm_ACTION.owl#action-event-category-code"/>
      </owl:Restriction>
    </rdfs:subClassOf>
    <rdfs:label xml:lang="en">securing</rdfs:label>
    <rdfs:comment xml:lang="en">Gaining possession of a position or terrain feature, with or without force, and making such disposition to prevent, as far as possible, its destruction or loss by enemy action.</rdfs:comment>
  </owl:Class>
  <owl:Class rdf:about="jc3iedm_ACTIONExtended.owl#ACTION-EVENT_Aircraft_launch_activity">
    <rdfs:subClassOf rdf:resource="jc3iedm_ACTION.owl#ACTION-EVENT"/>
    <rdfs:subClassOf>
      <owl:Restriction>
        <owl:hasValue xml:lang="en">AIRLAU</owl:hasValue>
        <owl:onProperty rdf:resource="jc3iedm_ACTION.owl#action-event-category-code"/>
      </owl:Restriction>
    </rdfs:subClassOf>
    <rdfs:label xml:lang="en">aircraft launch activity</rdfs:label>
    <rdfs:comment xml:lang="en">The occurrence of one or more aircraft taking off.</rdfs:comment>
  </owl:Class>
  <owl:Class rdf:about="jc3iedm_ACTIONExtended.owl#ACTION-EVENT_Suppressing">
    <rdfs:subClassOf rdf:resource="jc3iedm_ACTION.owl#ACTION-EVENT"/>
    <rdfs:subClassOf>
      <owl:Restriction>
        <owl:hasValue xml:lang="en">SUPRSN</owl:hasValue>
        <owl:onProperty rdf:resource="jc3iedm_ACTION.owl#action-event-category-code"/>
      </owl:Restriction>
    </rdfs:subClassOf>
    <rdfs:label xml:lang="en">suppressing</rdfs:label>
    <rdfs:comment xml:lang="en">Providing fires that neutralizes or temporarily degrades the capabilities of enemy forces within a specific area. This makes no assumptions as to enemy casualties; it may be a transitory effect.</rdfs:comment>
  </owl:Class>
  <owl:Class rdf:about="jc3iedm_ACTIONExtended.owl#ACTION-EVENT_Recovering">
    <rdfs:subClassOf rdf:resource="jc3iedm_ACTION.owl#ACTION-EVENT"/>
    <rdfs:subClassOf>
      <owl:Restriction>
        <owl:hasValue xml:lang="en">RECVRN</owl:hasValue>
        <owl:onProperty rdf:resource="jc3iedm_ACTION.owl#action-event-category-code"/>
      </owl:Restriction>
    </rdfs:subClassOf>
    <rdfs:label xml:lang="en">recovering</rdfs:label>
    <rdfs:comment xml:lang="en">Retrieving any lost, incapacitated or captured object.</rdfs:comment>
  </owl:Class>
  <owl:Class rdf:about="jc3iedm_ACTIONExtended.owl#ACTION-EVENT_Atmospheric_pollution">
    <rdfs:subClassOf rdf:resource="jc3iedm_ACTION.owl#ACTION-EVENT"/>
    <rdfs:subClassOf>
      <owl:Restriction>
        <owl:hasValue xml:lang="en">ATMPOL</owl:hasValue>
        <owl:onProperty rdf:resource="jc3iedm_ACTION.owl#action-event-category-code"/>
      </owl:Restriction>
    </rdfs:subClassOf>
    <rdfs:label xml:lang="en">atmospheric pollution</rdfs:label>
    <rdfs:comment xml:lang="en">Contamination of the atmosphere caused by a poison or toxin.</rdfs:comment>
  </owl:Class>
  <owl:Class rdf:about="jc3iedm_ACTIONExtended.owl#ACTION-EVENT_Mortar_fire">
    <rdfs:subClassOf rdf:resource="jc3iedm_ACTION.owl#ACTION-EVENT"/>
    <rdfs:subClassOf>
      <owl:Restriction>
        <owl:hasValue xml:lang="en">MRTFIR</owl:hasValue>
        <owl:onProperty rdf:resource="jc3iedm_ACTION.owl#action-event-category-code"/>
      </owl:Restriction>
    </rdfs:subClassOf>
    <rdfs:label xml:lang="en">mortar fire</rdfs:label>
    <rdfs:comment xml:lang="en">The discharge of a projectile from a mortar weapon.</rdfs:comment>
  </owl:Class>
  <owl:Class rdf:about="jc3iedm_ACTIONExtended.owl#ACTION-EVENT_Attack__main">
    <rdfs:subClassOf rdf:resource="jc3iedm_ACTION.owl#ACTION-EVENT"/>
    <rdfs:subClassOf>
      <owl:Restriction>
        <owl:hasValue xml:lang="en">ATTMN</owl:hasValue>
        <owl:onProperty rdf:resource="jc3iedm_ACTION.owl#action-event-category-code"/>
      </owl:Restriction>
    </rdfs:subClassOf>
    <rdfs:label xml:lang="en">attack, main</rdfs:label>
    <rdfs:comment xml:lang="en">Conducting the principal attack or effort into which the commander throws the full weight of the offensive power at his disposal. An attack directed against the chief objective of the campaign or battle.</rdfs:comment>
  </owl:Class>
  <owl:Class rdf:about="jc3iedm_ACTIONExtended.owl#ACTION-EVENT_Accident__mine">
    <rdfs:subClassOf rdf:resource="jc3iedm_ACTION.owl#ACTION-EVENT"/>
    <rdfs:subClassOf>
      <owl:Restriction>
        <owl:hasValue xml:lang="en">ACCMNE</owl:hasValue>
        <owl:onProperty rdf:resource="jc3iedm_ACTION.owl#action-event-category-code"/>
      </owl:Restriction>
    </rdfs:subClassOf>
    <rdfs:label xml:lang="en">accident, mine</rdfs:label>
    <rdfs:comment xml:lang="en">An accident involving unexploded ordnance.</rdfs:comment>
  </owl:Class>
  <owl:Class rdf:about="jc3iedm_ACTIONExtended.owl#ACTION-EVENT_Political_demonstration">
    <rdfs:subClassOf rdf:resource="jc3iedm_ACTION.owl#ACTION-EVENT"/>
    <rdfs:subClassOf>
      <owl:Restriction>
        <owl:hasValue xml:lang="en">POLDEM</owl:hasValue>
        <owl:onProperty rdf:resource="jc3iedm_ACTION.owl#action-event-category-code"/>
      </owl:Restriction>
    </rdfs:subClassOf>
    <rdfs:label xml:lang="en">political demonstration</rdfs:label>
    <rdfs:comment xml:lang="en">A public display of group feelings towards a political idea, person or cause.</rdfs:comment>
  </owl:Class>
  <owl:Class rdf:about="jc3iedm_ACTIONExtended.owl#ACTION-EVENT_Dazzle">
    <rdfs:subClassOf rdf:resource="jc3iedm_ACTION.owl#ACTION-EVENT"/>
    <rdfs:subClassOf>
      <owl:Restriction>
        <owl:hasValue xml:lang="en">DAZZLE</owl:hasValue>
        <owl:onProperty rdf:resource="jc3iedm_ACTION.owl#action-event-category-code"/>
      </owl:Restriction>
    </rdfs:subClassOf>
    <rdfs:label xml:lang="en">dazzle</rdfs:label>
    <rdfs:comment xml:lang="en">Causing a temporary loss of vision or a temporary reduction in visual acuity; may also be applied to effects on optics.</rdfs:comment>
  </owl:Class>
  <owl:Class rdf:about="jc3iedm_ACTIONExtended.owl#REQUEST_Presence">
    <rdfs:subClassOf rdf:resource="jc3iedm_ACTION.owl#REQUEST"/>
    <rdfs:subClassOf>
      <owl:Restriction>
        <owl:hasValue xml:lang="en">PRESNC</owl:hasValue>
        <owl:onProperty rdf:resource="jc3iedm_ACTION.owl#request-category-code"/>
      </owl:Restriction>
    </rdfs:subClassOf>
    <rdfs:label xml:lang="en">presence</rdfs:label>
    <rdfs:comment xml:lang="en">To discover the manifestation of an ACTION-OBJECTIVE in the area of operational interest specified through another ACTION-OBJECTIVE (OBJECT-ITEM: FACILITY, FEATURE).</rdfs:comment>
  </owl:Class>
  <owl:Class rdf:about="jc3iedm_ACTIONExtended.owl#ACTION-EVENT_Build-up">
    <rdfs:subClassOf rdf:resource="jc3iedm_ACTION.owl#ACTION-EVENT"/>
    <rdfs:subClassOf>
      <owl:Restriction>
        <owl:hasValue xml:lang="en">BLDUP</owl:hasValue>
        <owl:onProperty rdf:resource="jc3iedm_ACTION.owl#action-event-category-code"/>
      </owl:Restriction>
    </rdfs:subClassOf>
    <rdfs:label xml:lang="en">build up</rdfs:label>
    <rdfs:comment xml:lang="en">Attaining prescribed strength of units and prescribed levels of vehicles, equipment, stores and supplies.</rdfs:comment>
  </owl:Class>
  <owl:Class rdf:about="jc3iedm_ACTIONExtended.owl#ACTION-EVENT_Accident">
    <rdfs:subClassOf rdf:resource="jc3iedm_ACTION.owl#ACTION-EVENT"/>
    <rdfs:subClassOf>
      <owl:Restriction>
        <owl:hasValue xml:lang="en">ACCDNT</owl:hasValue>
        <owl:onProperty rdf:resource="jc3iedm_ACTION.owl#action-event-category-code"/>
      </owl:Restriction>
    </rdfs:subClassOf>
    <rdfs:label xml:lang="en">accident</rdfs:label>
    <rdfs:comment xml:lang="en">An unfortunate event, esp. one causing physical harm or damage, brought about unintentionally.</rdfs:comment>
  </owl:Class>
  <owl:Class rdf:about="jc3iedm_ACTIONExtended.owl#ACTION-EVENT_Hiding">
    <rdfs:subClassOf rdf:resource="jc3iedm_ACTION.owl#ACTION-EVENT"/>
    <rdfs:subClassOf>
      <owl:Restriction>
        <owl:hasValue xml:lang="en">HIDING</owl:hasValue>
        <owl:onProperty rdf:resource="jc3iedm_ACTION.owl#action-event-category-code"/>
      </owl:Restriction>
    </rdfs:subClassOf>
    <rdfs:label xml:lang="en">hiding</rdfs:label>
    <rdfs:comment xml:lang="en">Concealing an object.</rdfs:comment>
  </owl:Class>
  <owl:Class rdf:about="jc3iedm_ACTIONExtended.owl#ACTION-EVENT_Retain">
    <rdfs:subClassOf rdf:resource="jc3iedm_ACTION.owl#ACTION-EVENT"/>
    <rdfs:subClassOf>
      <owl:Restriction>
        <owl:hasValue xml:lang="en">RETAIN</owl:hasValue>
        <owl:onProperty rdf:resource="jc3iedm_ACTION.owl#action-event-category-code"/>
      </owl:Restriction>
    </rdfs:subClassOf>
    <rdfs:label xml:lang="en">retain</rdfs:label>
    <rdfs:comment xml:lang="en">Occupying and holding a terrain feature to ensure it is free of enemy occupation or use.</rdfs:comment>
  </owl:Class>
  <owl:Class rdf:about="jc3iedm_ACTIONExtended.owl#ACTION-EVENT_Issuing_media_article">
    <rdfs:subClassOf rdf:resource="jc3iedm_ACTION.owl#ACTION-EVENT"/>
    <rdfs:subClassOf>
      <owl:Restriction>
        <owl:hasValue xml:lang="en">ISSMDA</owl:hasValue>
        <owl:onProperty rdf:resource="jc3iedm_ACTION.owl#action-event-category-code"/>
      </owl:Restriction>
    </rdfs:subClassOf>
    <rdfs:label xml:lang="en">issuing media article</rdfs:label>
    <rdfs:comment xml:lang="en">Sending forth or putting into circulation a non-fictional essay, especially one included with others in a newspaper, magazine, or journal.</rdfs:comment>
  </owl:Class>
  <owl:Class rdf:about="jc3iedm_ACTIONExtended.owl#ACTION-EVENT_Border_crossing__illegal">
    <rdfs:subClassOf rdf:resource="jc3iedm_ACTION.owl#ACTION-EVENT"/>
    <rdfs:subClassOf>
      <owl:Restriction>
        <owl:hasValue xml:lang="en">BCILGL</owl:hasValue>
        <owl:onProperty rdf:resource="jc3iedm_ACTION.owl#action-event-category-code"/>
      </owl:Restriction>
    </rdfs:subClassOf>
    <rdfs:label xml:lang="en">border crossing, illegal</rdfs:label>
    <rdfs:comment xml:lang="en">A border crossing that is forbidden by law.</rdfs:comment>
  </owl:Class>
  <owl:Class rdf:about="jc3iedm_ACTIONExtended.owl#ACTION-EVENT_UXO_discovery">
    <rdfs:subClassOf rdf:resource="jc3iedm_ACTION.owl#ACTION-EVENT"/>
    <rdfs:subClassOf>
      <owl:Restriction>
        <owl:hasValue xml:lang="en">UXODSC</owl:hasValue>
        <owl:onProperty rdf:resource="jc3iedm_ACTION.owl#action-event-category-code"/>
      </owl:Restriction>
    </rdfs:subClassOf>
    <rdfs:label xml:lang="en">uxo discovery</rdfs:label>
    <rdfs:comment xml:lang="en">The detection of the presence of unexploded explosive ordnance.</rdfs:comment>
  </owl:Class>
  <owl:Class rdf:about="jc3iedm_ACTIONExtended.owl#ACTION-EVENT_Famine">
    <rdfs:subClassOf rdf:resource="jc3iedm_ACTION.owl#ACTION-EVENT"/>
    <rdfs:subClassOf>
      <owl:Restriction>
        <owl:hasValue xml:lang="en">FAMINE</owl:hasValue>
        <owl:onProperty rdf:resource="jc3iedm_ACTION.owl#action-event-category-code"/>
      </owl:Restriction>
    </rdfs:subClassOf>
    <rdfs:label xml:lang="en">famine</rdfs:label>
    <rdfs:comment xml:lang="en">An extreme scarcity of food.</rdfs:comment>
  </owl:Class>
  <owl:Class rdf:about="jc3iedm_ACTIONExtended.owl#ACTION-EVENT_Redeployment">
    <rdfs:subClassOf rdf:resource="jc3iedm_ACTION.owl#ACTION-EVENT"/>
    <rdfs:subClassOf>
      <owl:Restriction>
        <owl:hasValue xml:lang="en">REDPLN</owl:hasValue>
        <owl:onProperty rdf:resource="jc3iedm_ACTION.owl#action-event-category-code"/>
      </owl:Restriction>
    </rdfs:subClassOf>
    <rdfs:label xml:lang="en">redeployment</rdfs:label>
    <rdfs:comment xml:lang="en">Transferring a unit, an individual, or supplies deployed in one area to another area, or to another location within the area, for the purpose of further employment.</rdfs:comment>
  </owl:Class>
  <owl:Class rdf:about="jc3iedm_ACTIONExtended.owl#CBRN-EVENT_Unidentified_release_other_than_attack_(ROTA)">
    <rdfs:subClassOf rdf:resource="jc3iedm_ACTION.owl#CBRN-EVENT"/>
    <rdfs:subClassOf>
      <owl:Restriction>
        <owl:hasValue xml:lang="en">UNROTA</owl:hasValue>
        <owl:onProperty rdf:resource="jc3iedm_ACTION.owl#cbrn-event-category-code"/>
      </owl:Restriction>
    </rdfs:subClassOf>
    <rdfs:label xml:lang="en">unidentified release other than attack (rota)</rdfs:label>
    <rdfs:comment xml:lang="en">The release of an unknown chemical, biological, nuclear, radiological materiel(s) [agent(s)] into the environment intentionally or accidentally but not for the intended purpose of conducting an attack.</rdfs:comment>
  </owl:Class>
  <owl:Class rdf:about="jc3iedm_ACTIONExtended.owl#NUCLEAR-EVENT_Nuclear_release_other_than_attack_(ROTA)">
    <rdfs:subClassOf rdf:resource="jc3iedm_ACTION.owl#NUCLEAR-EVENT"/>
    <rdfs:subClassOf>
      <owl:Restriction>
        <owl:hasValue xml:lang="en">NROTA</owl:hasValue>
        <owl:onProperty rdf:resource="jc3iedm_ACTION.owl#nuclear-event-category-code"/>
      </owl:Restriction>
    </rdfs:subClassOf>
    <rdfs:label xml:lang="en">nuclear release other than attack (rota)</rdfs:label>
    <rdfs:comment xml:lang="en">The release of nuclear material into the environment intentionally or accidentally but not for the intended purpose of conducting an attack.</rdfs:comment>
  </owl:Class>
  <owl:Class rdf:about="jc3iedm_ACTIONExtended.owl#ACTION-EVENT_Vessel_sinking">
    <rdfs:subClassOf rdf:resource="jc3iedm_ACTION.owl#ACTION-EVENT"/>
    <rdfs:subClassOf>
      <owl:Restriction>
        <owl:hasValue xml:lang="en">SINKIN</owl:hasValue>
        <owl:onProperty rdf:resource="jc3iedm_ACTION.owl#action-event-category-code"/>
      </owl:Restriction>
    </rdfs:subClassOf>
    <rdfs:label xml:lang="en">vessel sinking</rdfs:label>
    <rdfs:comment xml:lang="en">The unforeseen loss, damage or destruction of a vessel by submersion.</rdfs:comment>
  </owl:Class>
  <owl:Class rdf:about="jc3iedm_ACTIONExtended.owl#ACTION-EVENT_Burned_out_object">
    <rdfs:subClassOf rdf:resource="jc3iedm_ACTION.owl#ACTION-EVENT"/>
    <rdfs:subClassOf>
      <owl:Restriction>
        <owl:hasValue xml:lang="en">BRNOBJ</owl:hasValue>
        <owl:onProperty rdf:resource="jc3iedm_ACTION.owl#action-event-category-code"/>
      </owl:Restriction>
    </rdfs:subClassOf>
    <rdfs:label xml:lang="en">burned out object</rdfs:label>
    <rdfs:comment xml:lang="en">Complete destruction of an object by flames.</rdfs:comment>
  </owl:Class>
  <owl:Class rdf:about="jc3iedm_ACTIONExtended.owl#ACTION-EVENT_Penetrating">
    <rdfs:subClassOf rdf:resource="jc3iedm_ACTION.owl#ACTION-EVENT"/>
    <rdfs:subClassOf>
      <owl:Restriction>
        <owl:hasValue xml:lang="en">PENTRT</owl:hasValue>
        <owl:onProperty rdf:resource="jc3iedm_ACTION.owl#action-event-category-code"/>
      </owl:Restriction>
    </rdfs:subClassOf>
    <rdfs:label xml:lang="en">penetrating</rdfs:label>
    <rdfs:comment xml:lang="en">Breaking through the enemy’s defence or disrupting the enemy’s defensive systems.</rdfs:comment>
  </owl:Class>
  <owl:Class rdf:about="jc3iedm_ACTIONExtended.owl#ACTION-EVENT_Labour_strike">
    <rdfs:subClassOf rdf:resource="jc3iedm_ACTION.owl#ACTION-EVENT"/>
    <rdfs:subClassOf>
      <owl:Restriction>
        <owl:hasValue xml:lang="en">LABSTR</owl:hasValue>
        <owl:onProperty rdf:resource="jc3iedm_ACTION.owl#action-event-category-code"/>
      </owl:Restriction>
    </rdfs:subClassOf>
    <rdfs:label xml:lang="en">labour strike</rdfs:label>
    <rdfs:comment xml:lang="en">The organised refusal by employees to work until some grievance is remedied.</rdfs:comment>
  </owl:Class>
  <owl:Class rdf:about="jc3iedm_ACTIONExtended.owl#ACTION-EVENT_Epidemic">
    <rdfs:subClassOf rdf:resource="jc3iedm_ACTION.owl#ACTION-EVENT"/>
    <rdfs:subClassOf>
      <owl:Restriction>
        <owl:hasValue xml:lang="en">EPEDEM</owl:hasValue>
        <owl:onProperty rdf:resource="jc3iedm_ACTION.owl#action-event-category-code"/>
      </owl:Restriction>
    </rdfs:subClassOf>
    <rdfs:label xml:lang="en">epidemic</rdfs:label>
    <rdfs:comment xml:lang="en">A widespread occurrence of a disease in a community at a particular time.</rdfs:comment>
  </owl:Class>
  <owl:Class rdf:about="jc3iedm_ACTIONExtended.owl#ACTION-EVENT_Bombing__accidental">
    <rdfs:subClassOf rdf:resource="jc3iedm_ACTION.owl#ACTION-EVENT"/>
    <rdfs:subClassOf>
      <owl:Restriction>
        <owl:hasValue xml:lang="en">BMBACC</owl:hasValue>
        <owl:onProperty rdf:resource="jc3iedm_ACTION.owl#action-event-category-code"/>
      </owl:Restriction>
    </rdfs:subClassOf>
    <rdfs:label xml:lang="en">bombing, accidental</rdfs:label>
    <rdfs:comment xml:lang="en">An unfortunate bombing incident that happens unexpectedly and unintentionally.</rdfs:comment>
  </owl:Class>
  <owl:Class rdf:about="jc3iedm_ACTIONExtended.owl#ACTION-EVENT_Political_execution">
    <rdfs:subClassOf rdf:resource="jc3iedm_ACTION.owl#ACTION-EVENT"/>
    <rdfs:subClassOf>
      <owl:Restriction>
        <owl:hasValue xml:lang="en">POLEXE</owl:hasValue>
        <owl:onProperty rdf:resource="jc3iedm_ACTION.owl#action-event-category-code"/>
      </owl:Restriction>
    </rdfs:subClassOf>
    <rdfs:label xml:lang="en">political execution</rdfs:label>
    <rdfs:comment xml:lang="en">A putting to death of a person or group of persons for political reasons.</rdfs:comment>
  </owl:Class>
  <owl:Class rdf:about="jc3iedm_ACTIONExtended.owl#ACTION-EVENT_Natural_disaster">
    <rdfs:subClassOf rdf:resource="jc3iedm_ACTION.owl#ACTION-EVENT"/>
    <rdfs:subClassOf>
      <owl:Restriction>
        <owl:hasValue xml:lang="en">NATDIS</owl:hasValue>
        <owl:onProperty rdf:resource="jc3iedm_ACTION.owl#action-event-category-code"/>
      </owl:Restriction>
    </rdfs:subClassOf>
    <rdfs:label xml:lang="en">natural disaster</rdfs:label>
    <rdfs:comment xml:lang="en">The damage caused by force of nature, such as a hurricane, cyclone, tornado or tidal wave.</rdfs:comment>
  </owl:Class>
  <owl:Class rdf:about="jc3iedm_ACTIONExtended.owl#ACTION-EVENT_Strafing__aerial">
    <rdfs:subClassOf rdf:resource="jc3iedm_ACTION.owl#ACTION-EVENT"/>
    <rdfs:subClassOf>
      <owl:Restriction>
        <owl:hasValue xml:lang="en">STRFAR</owl:hasValue>
        <owl:onProperty rdf:resource="jc3iedm_ACTION.owl#action-event-category-code"/>
      </owl:Restriction>
    </rdfs:subClassOf>
    <rdfs:label xml:lang="en">strafing, aerial</rdfs:label>
    <rdfs:comment xml:lang="en">Attack by enemy aircraft against ground targets using forward firing ordnance (bullets, shells, or rockets).</rdfs:comment>
  </owl:Class>
  <owl:Class rdf:about="jc3iedm_ACTIONExtended.owl#ACTION-EVENT_Security_violation">
    <rdfs:subClassOf rdf:resource="jc3iedm_ACTION.owl#ACTION-EVENT"/>
    <rdfs:subClassOf>
      <owl:Restriction>
        <owl:hasValue xml:lang="en">SECVIO</owl:hasValue>
        <owl:onProperty rdf:resource="jc3iedm_ACTION.owl#action-event-category-code"/>
      </owl:Restriction>
    </rdfs:subClassOf>
    <rdfs:label xml:lang="en">security violation</rdfs:label>
    <rdfs:comment xml:lang="en">An infringement of a security protocol.</rdfs:comment>
  </owl:Class>
  <owl:Class rdf:about="jc3iedm_ACTIONExtended.owl#ACTION-EVENT_Robbery">
    <rdfs:subClassOf rdf:resource="jc3iedm_ACTION.owl#ACTION-EVENT"/>
    <rdfs:subClassOf>
      <owl:Restriction>
        <owl:hasValue xml:lang="en">ROBERY</owl:hasValue>
        <owl:onProperty rdf:resource="jc3iedm_ACTION.owl#action-event-category-code"/>
      </owl:Restriction>
    </rdfs:subClassOf>
    <rdfs:label xml:lang="en">robbery</rdfs:label>
    <rdfs:comment xml:lang="en">Unlawfully taking property, valuables or money from a person or place.</rdfs:comment>
  </owl:Class>
  <owl:Class rdf:about="jc3iedm_ACTIONExtended.owl#ACTION-EVENT_Civil_demonstration__legal">
    <rdfs:subClassOf rdf:resource="jc3iedm_ACTION.owl#ACTION-EVENT"/>
    <rdfs:subClassOf>
      <owl:Restriction>
        <owl:hasValue xml:lang="en">CIVDML</owl:hasValue>
        <owl:onProperty rdf:resource="jc3iedm_ACTION.owl#action-event-category-code"/>
      </owl:Restriction>
    </rdfs:subClassOf>
    <rdfs:label xml:lang="en">civil demonstration, legal</rdfs:label>
    <rdfs:comment xml:lang="en">A public meeting or march legally expressing protest or other opinion on an issue.</rdfs:comment>
  </owl:Class>
  <owl:Class rdf:about="jc3iedm_ACTIONExtended.owl#ACTION-EVENT_Canalise">
    <rdfs:subClassOf rdf:resource="jc3iedm_ACTION.owl#ACTION-EVENT"/>
    <rdfs:subClassOf>
      <owl:Restriction>
        <owl:hasValue xml:lang="en">CANLSE</owl:hasValue>
        <owl:onProperty rdf:resource="jc3iedm_ACTION.owl#action-event-category-code"/>
      </owl:Restriction>
    </rdfs:subClassOf>
    <rdfs:label xml:lang="en">canalise</rdfs:label>
    <rdfs:comment xml:lang="en">Restricting operations to a narrow zone by use of existing or reinforcing obstacles or by fire or bombing.</rdfs:comment>
  </owl:Class>
  <owl:Class rdf:about="jc3iedm_ACTIONExtended.owl#ACTION-EVENT_Death__natural_causes">
    <rdfs:subClassOf rdf:resource="jc3iedm_ACTION.owl#ACTION-EVENT"/>
    <rdfs:subClassOf>
      <owl:Restriction>
        <owl:hasValue xml:lang="en">DTHNAT</owl:hasValue>
        <owl:onProperty rdf:resource="jc3iedm_ACTION.owl#action-event-category-code"/>
      </owl:Restriction>
    </rdfs:subClassOf>
    <rdfs:label xml:lang="en">death, natural causes</rdfs:label>
    <rdfs:comment xml:lang="en">Normal termination of life.</rdfs:comment>
  </owl:Class>
  <owl:Class rdf:about="jc3iedm_ACTIONExtended.owl#ACTION-EVENT_Transporting">
    <rdfs:subClassOf rdf:resource="jc3iedm_ACTION.owl#ACTION-EVENT"/>
    <rdfs:subClassOf>
      <owl:Restriction>
        <owl:hasValue xml:lang="en">TRNSPN</owl:hasValue>
        <owl:onProperty rdf:resource="jc3iedm_ACTION.owl#action-event-category-code"/>
      </owl:Restriction>
    </rdfs:subClassOf>
    <rdfs:label xml:lang="en">transporting</rdfs:label>
    <rdfs:comment xml:lang="en">Moving assets to a specified objective by sea, land or air.</rdfs:comment>
  </owl:Class>
  <owl:Class rdf:about="jc3iedm_ACTIONExtended.owl#ACTION-EVENT_Letter_bomb_incident">
    <rdfs:subClassOf rdf:resource="jc3iedm_ACTION.owl#ACTION-EVENT"/>
    <rdfs:subClassOf>
      <owl:Restriction>
        <owl:hasValue xml:lang="en">LTRBMI</owl:hasValue>
        <owl:onProperty rdf:resource="jc3iedm_ACTION.owl#action-event-category-code"/>
      </owl:Restriction>
    </rdfs:subClassOf>
    <rdfs:label xml:lang="en">letter bomb incident</rdfs:label>
    <rdfs:comment xml:lang="en">The detection of a seemingly harmless letter or parcel.</rdfs:comment>
  </owl:Class>
  <owl:Class rdf:about="jc3iedm_ACTIONExtended.owl#ACTION-EVENT_Defeat">
    <rdfs:subClassOf rdf:resource="jc3iedm_ACTION.owl#ACTION-EVENT"/>
    <rdfs:subClassOf>
      <owl:Restriction>
        <owl:hasValue xml:lang="en">DEFEAT</owl:hasValue>
        <owl:onProperty rdf:resource="jc3iedm_ACTION.owl#action-event-category-code"/>
      </owl:Restriction>
    </rdfs:subClassOf>
    <rdfs:label xml:lang="en">defeat</rdfs:label>
    <rdfs:comment xml:lang="en">Diminution of the effectiveness of the enemy to the extent that he is unable to participate further in the battle or at least cannot fulfil his intention.</rdfs:comment>
  </owl:Class>
  <owl:Class rdf:about="jc3iedm_ACTIONExtended.owl#ACTION-EVENT_Following_and_supporting">
    <rdfs:subClassOf rdf:resource="jc3iedm_ACTION.owl#ACTION-EVENT"/>
    <rdfs:subClassOf>
      <owl:Restriction>
        <owl:hasValue xml:lang="en">FOLSPT</owl:hasValue>
        <owl:onProperty rdf:resource="jc3iedm_ACTION.owl#action-event-category-code"/>
      </owl:Restriction>
    </rdfs:subClassOf>
    <rdfs:label xml:lang="en">following and supporting</rdfs:label>
    <rdfs:comment xml:lang="en">Operating as a committed force that follows and supports the mission accomplishment of a force conducting an offensive operation.</rdfs:comment>
  </owl:Class>
  <owl:Class rdf:about="jc3iedm_ACTIONExtended.owl#ACTION-EVENT_Advancing">
    <rdfs:subClassOf rdf:resource="jc3iedm_ACTION.owl#ACTION-EVENT"/>
    <rdfs:subClassOf>
      <owl:Restriction>
        <owl:hasValue xml:lang="en">ADVANC</owl:hasValue>
        <owl:onProperty rdf:resource="jc3iedm_ACTION.owl#action-event-category-code"/>
      </owl:Restriction>
    </rdfs:subClassOf>
    <rdfs:label xml:lang="en">advancing</rdfs:label>
    <rdfs:comment xml:lang="en">Moving towards an objective in some form of tactical formation. This is a transitional phase between operations that may or may not result in contact with the enemy.</rdfs:comment>
  </owl:Class>
  <owl:Class rdf:about="jc3iedm_ACTIONExtended.owl#ACTION-EVENT_Accident__aircraft_ground">
    <rdfs:subClassOf rdf:resource="jc3iedm_ACTION.owl#ACTION-EVENT"/>
    <rdfs:subClassOf>
      <owl:Restriction>
        <owl:hasValue xml:lang="en">ACCAIR</owl:hasValue>
        <owl:onProperty rdf:resource="jc3iedm_ACTION.owl#action-event-category-code"/>
      </owl:Restriction>
    </rdfs:subClassOf>
    <rdfs:label xml:lang="en">accident, aircraft ground</rdfs:label>
    <rdfs:comment xml:lang="en">An accident involving an aircraft during ground operations or maintenance.</rdfs:comment>
  </owl:Class>
  <owl:Class rdf:about="jc3iedm_ACTIONExtended.owl#ACTION-EVENT_Amphibious_operation">
    <rdfs:subClassOf rdf:resource="jc3iedm_ACTION.owl#ACTION-EVENT"/>
    <rdfs:subClassOf>
      <owl:Restriction>
        <owl:hasValue xml:lang="en">AMPH</owl:hasValue>
        <owl:onProperty rdf:resource="jc3iedm_ACTION.owl#action-event-category-code"/>
      </owl:Restriction>
    </rdfs:subClassOf>
    <rdfs:label xml:lang="en">amphibious operation</rdfs:label>
    <rdfs:comment xml:lang="en">Mounting an operation launched from the sea by naval and land forces against a hostile, or potentially hostile shore.</rdfs:comment>
  </owl:Class>
  <owl:Class rdf:about="jc3iedm_ACTIONExtended.owl#ACTION-EVENT_War_military_conference">
    <rdfs:subClassOf rdf:resource="jc3iedm_ACTION.owl#ACTION-EVENT"/>
    <rdfs:subClassOf>
      <owl:Restriction>
        <owl:hasValue xml:lang="en">WARCON</owl:hasValue>
        <owl:onProperty rdf:resource="jc3iedm_ACTION.owl#action-event-category-code"/>
      </owl:Restriction>
    </rdfs:subClassOf>
    <rdfs:label xml:lang="en">war/military conference</rdfs:label>
    <rdfs:comment xml:lang="en">A meeting of a group of persons to discuss war/military process.</rdfs:comment>
  </owl:Class>
  <owl:Class rdf:about="jc3iedm_ACTIONExtended.owl#ACTION-EVENT_Spying">
    <rdfs:subClassOf rdf:resource="jc3iedm_ACTION.owl#ACTION-EVENT"/>
    <rdfs:subClassOf>
      <owl:Restriction>
        <owl:hasValue xml:lang="en">SPYING</owl:hasValue>
        <owl:onProperty rdf:resource="jc3iedm_ACTION.owl#action-event-category-code"/>
      </owl:Restriction>
    </rdfs:subClassOf>
    <rdfs:label xml:lang="en">spying</rdfs:label>
    <rdfs:comment xml:lang="en">Obtaining intelligence information furtively as an agent of a foreign power or competition.</rdfs:comment>
  </owl:Class>
  <owl:Class rdf:about="jc3iedm_ACTIONExtended.owl#ACTION-EVENT_Religious_warfare">
    <rdfs:subClassOf rdf:resource="jc3iedm_ACTION.owl#ACTION-EVENT"/>
    <rdfs:subClassOf>
      <owl:Restriction>
        <owl:hasValue xml:lang="en">RELWAR</owl:hasValue>
        <owl:onProperty rdf:resource="jc3iedm_ACTION.owl#action-event-category-code"/>
      </owl:Restriction>
    </rdfs:subClassOf>
    <rdfs:label xml:lang="en">religious warfare</rdfs:label>
    <rdfs:comment xml:lang="en">An act of open armed conflict due to a difference of religious belief between two separate groups.</rdfs:comment>
  </owl:Class>
  <owl:Class rdf:about="jc3iedm_ACTIONExtended.owl#ACTION-EVENT_Conducting_media_interview">
    <rdfs:subClassOf rdf:resource="jc3iedm_ACTION.owl#ACTION-EVENT"/>
    <rdfs:subClassOf>
      <owl:Restriction>
        <owl:hasValue xml:lang="en">CNDMED</owl:hasValue>
        <owl:onProperty rdf:resource="jc3iedm_ACTION.owl#action-event-category-code"/>
      </owl:Restriction>
    </rdfs:subClassOf>
    <rdfs:label xml:lang="en">conducting media interview</rdfs:label>
    <rdfs:comment xml:lang="en">Conducting a conversation between a reporter etc. and a person of public interest, used as a basis of a broadcast or publication.</rdfs:comment>
  </owl:Class>
  <owl:Class rdf:about="jc3iedm_ACTIONExtended.owl#ACTION-EVENT_Consolidating_of_a_position">
    <rdfs:subClassOf rdf:resource="jc3iedm_ACTION.owl#ACTION-EVENT"/>
    <rdfs:subClassOf>
      <owl:Restriction>
        <owl:hasValue xml:lang="en">CNSLDT</owl:hasValue>
        <owl:onProperty rdf:resource="jc3iedm_ACTION.owl#action-event-category-code"/>
      </owl:Restriction>
    </rdfs:subClassOf>
    <rdfs:label xml:lang="en">consolidating of a position</rdfs:label>
    <rdfs:comment xml:lang="en">Re-organising and strengthening of a newly captured position so that it can be used against the enemy.</rdfs:comment>
  </owl:Class>
  <owl:Class rdf:about="jc3iedm_ACTIONExtended.owl#ACTION-EVENT_Evacuating">
    <rdfs:subClassOf rdf:resource="jc3iedm_ACTION.owl#ACTION-EVENT"/>
    <rdfs:subClassOf>
      <owl:Restriction>
        <owl:hasValue xml:lang="en">EVACTN</owl:hasValue>
        <owl:onProperty rdf:resource="jc3iedm_ACTION.owl#action-event-category-code"/>
      </owl:Restriction>
    </rdfs:subClassOf>
    <rdfs:label xml:lang="en">evacuating</rdfs:label>
    <rdfs:comment xml:lang="en">Clearing or removing materiel and personnel from a given locality.</rdfs:comment>
  </owl:Class>
  <owl:Class rdf:about="jc3iedm_ACTIONExtended.owl#ACTION-EVENT_Crime_against_humanity">
    <rdfs:subClassOf rdf:resource="jc3iedm_ACTION.owl#ACTION-EVENT"/>
    <rdfs:subClassOf>
      <owl:Restriction>
        <owl:hasValue xml:lang="en">CRMHMN</owl:hasValue>
        <owl:onProperty rdf:resource="jc3iedm_ACTION.owl#action-event-category-code"/>
      </owl:Restriction>
    </rdfs:subClassOf>
    <rdfs:label xml:lang="en">crime against humanity</rdfs:label>
    <rdfs:comment xml:lang="en">Violation of the laws so gross in numbers affected that it is considered to affect all humans and not only individuals.</rdfs:comment>
  </owl:Class>
  <owl:Class rdf:about="jc3iedm_ACTIONExtended.owl#ACTION-EVENT_Deception">
    <rdfs:subClassOf rdf:resource="jc3iedm_ACTION.owl#ACTION-EVENT"/>
    <rdfs:subClassOf>
      <owl:Restriction>
        <owl:hasValue xml:lang="en">DCPTIN</owl:hasValue>
        <owl:onProperty rdf:resource="jc3iedm_ACTION.owl#action-event-category-code"/>
      </owl:Restriction>
    </rdfs:subClassOf>
    <rdfs:label xml:lang="en">deception</rdfs:label>
    <rdfs:comment xml:lang="en">Employing measures designed to mislead the enemy by manipulation, distortion, or falsification of evidence to induce him to react in a manner prejudicial to his interests.</rdfs:comment>
  </owl:Class>
  <owl:Class rdf:about="jc3iedm_ACTIONExtended.owl#ACTION-EVENT_Defending">
    <rdfs:subClassOf rdf:resource="jc3iedm_ACTION.owl#ACTION-EVENT"/>
    <rdfs:subClassOf>
      <owl:Restriction>
        <owl:hasValue xml:lang="en">DEFEND</owl:hasValue>
        <owl:onProperty rdf:resource="jc3iedm_ACTION.owl#action-event-category-code"/>
      </owl:Restriction>
    </rdfs:subClassOf>
    <rdfs:label xml:lang="en">defending</rdfs:label>
    <rdfs:comment xml:lang="en">Protecting a defined object against an enemy attack.</rdfs:comment>
  </owl:Class>
  <owl:Class rdf:about="jc3iedm_ACTIONExtended.owl#ACTION-EVENT_Publishing_media_article">
    <rdfs:subClassOf rdf:resource="jc3iedm_ACTION.owl#ACTION-EVENT"/>
    <rdfs:subClassOf>
      <owl:Restriction>
        <owl:hasValue xml:lang="en">PUBMDA</owl:hasValue>
        <owl:onProperty rdf:resource="jc3iedm_ACTION.owl#action-event-category-code"/>
      </owl:Restriction>
    </rdfs:subClassOf>
    <rdfs:label xml:lang="en">publishing media article</rdfs:label>
    <rdfs:comment xml:lang="en">Making generally known a non-fictional essay, especially one included with others in a newspaper, magazine, journal, etc.</rdfs:comment>
  </owl:Class>
  <owl:Class rdf:about="jc3iedm_ACTIONExtended.owl#ACTION-EVENT_Providing_accommodation">
    <rdfs:subClassOf rdf:resource="jc3iedm_ACTION.owl#ACTION-EVENT"/>
    <rdfs:subClassOf>
      <owl:Restriction>
        <owl:hasValue xml:lang="en">PRVACC</owl:hasValue>
        <owl:onProperty rdf:resource="jc3iedm_ACTION.owl#action-event-category-code"/>
      </owl:Restriction>
    </rdfs:subClassOf>
    <rdfs:label xml:lang="en">providing accommodation</rdfs:label>
    <rdfs:comment xml:lang="en">Providing room for receiving people, esp. a place to live or lodgings.</rdfs:comment>
  </owl:Class>
  <owl:Class rdf:about="jc3iedm_ACTIONExtended.owl#ACTION-EVENT_Drug_storage">
    <rdfs:subClassOf rdf:resource="jc3iedm_ACTION.owl#ACTION-EVENT"/>
    <rdfs:subClassOf>
      <owl:Restriction>
        <owl:hasValue xml:lang="en">DRGSTR</owl:hasValue>
        <owl:onProperty rdf:resource="jc3iedm_ACTION.owl#action-event-category-code"/>
      </owl:Restriction>
    </rdfs:subClassOf>
    <rdfs:label xml:lang="en">drug storage</rdfs:label>
    <rdfs:comment xml:lang="en">An action to store drugs.</rdfs:comment>
  </owl:Class>
  <owl:Class rdf:about="jc3iedm_ACTIONExtended.owl#ACTION-EVENT_Alert_cancellation">
    <rdfs:subClassOf rdf:resource="jc3iedm_ACTION.owl#ACTION-EVENT"/>
    <rdfs:subClassOf>
      <owl:Restriction>
        <owl:hasValue xml:lang="en">ALRCAN</owl:hasValue>
        <owl:onProperty rdf:resource="jc3iedm_ACTION.owl#action-event-category-code"/>
      </owl:Restriction>
    </rdfs:subClassOf>
    <rdfs:label xml:lang="en">alert cancellation</rdfs:label>
    <rdfs:comment xml:lang="en">The end of a state of readiness.</rdfs:comment>
  </owl:Class>
  <owl:Class rdf:about="jc3iedm_ACTIONExtended.owl#ACTION-EVENT_Serving_as_an_in-place_force">
    <rdfs:subClassOf rdf:resource="jc3iedm_ACTION.owl#ACTION-EVENT"/>
    <rdfs:subClassOf>
      <owl:Restriction>
        <owl:hasValue xml:lang="en">SRVINP</owl:hasValue>
        <owl:onProperty rdf:resource="jc3iedm_ACTION.owl#action-event-category-code"/>
      </owl:Restriction>
    </rdfs:subClassOf>
    <rdfs:label xml:lang="en">serving as an in place force</rdfs:label>
    <rdfs:comment xml:lang="en">Operating as a force that provides fire and other support to the bridgehead force during an obstacle crossing.</rdfs:comment>
  </owl:Class>
  <owl:Class rdf:about="jc3iedm_ACTIONExtended.owl#ACTION-EVENT_Communications_deactivation">
    <rdfs:subClassOf rdf:resource="jc3iedm_ACTION.owl#ACTION-EVENT"/>
    <rdfs:subClassOf>
      <owl:Restriction>
        <owl:hasValue xml:lang="en">COMDEA</owl:hasValue>
        <owl:onProperty rdf:resource="jc3iedm_ACTION.owl#action-event-category-code"/>
      </owl:Restriction>
    </rdfs:subClassOf>
    <rdfs:label xml:lang="en">communications deactivation</rdfs:label>
    <rdfs:comment xml:lang="en">The disabling of transmission of information.</rdfs:comment>
  </owl:Class>
  <owl:Class rdf:about="jc3iedm_ACTIONExtended.owl#ACTION-EVENT_Hold__defensive">
    <rdfs:subClassOf rdf:resource="jc3iedm_ACTION.owl#ACTION-EVENT"/>
    <rdfs:subClassOf>
      <owl:Restriction>
        <owl:hasValue xml:lang="en">HLDDEF</owl:hasValue>
        <owl:onProperty rdf:resource="jc3iedm_ACTION.owl#action-event-category-code"/>
      </owl:Restriction>
    </rdfs:subClassOf>
    <rdfs:label xml:lang="en">hold, defensive</rdfs:label>
    <rdfs:comment xml:lang="en">Maintaining or retaining possession by force a position or area in defensive operations.</rdfs:comment>
  </owl:Class>
  <owl:Class rdf:about="jc3iedm_ACTIONExtended.owl#NUCLEAR-EVENT_Nuclear_attack">
    <rdfs:subClassOf rdf:resource="jc3iedm_ACTION.owl#NUCLEAR-EVENT"/>
    <rdfs:subClassOf>
      <owl:Restriction>
        <owl:hasValue xml:lang="en">NUCATT</owl:hasValue>
        <owl:onProperty rdf:resource="jc3iedm_ACTION.owl#nuclear-event-category-code"/>
      </owl:Restriction>
    </rdfs:subClassOf>
    <rdfs:label xml:lang="en">nuclear attack</rdfs:label>
    <rdfs:comment xml:lang="en">The delivery of a nuclear weapon against a target.</rdfs:comment>
  </owl:Class>
  <owl:Class rdf:about="jc3iedm_ACTIONExtended.owl#ACTION-EVENT_Fix__electro-optical">
    <rdfs:subClassOf rdf:resource="jc3iedm_ACTION.owl#ACTION-EVENT"/>
    <rdfs:subClassOf>
      <owl:Restriction>
        <owl:hasValue xml:lang="en">FIXELO</owl:hasValue>
        <owl:onProperty rdf:resource="jc3iedm_ACTION.owl#action-event-category-code"/>
      </owl:Restriction>
    </rdfs:subClassOf>
    <rdfs:label xml:lang="en">fix, electro optical</rdfs:label>
    <rdfs:comment xml:lang="en">Determining a position using electro-optical data.</rdfs:comment>
  </owl:Class>
  <owl:Class rdf:about="jc3iedm_ACTIONExtended.owl#CHEMICAL-BIOLOGICAL-EVENT_Biological_release_other_than_attack_(ROTA)">
    <rdfs:subClassOf rdf:resource="jc3iedm_ACTION.owl#CHEMICAL-BIOLOGICAL-EVENT"/>
    <rdfs:subClassOf>
      <owl:Restriction>
        <owl:hasValue xml:lang="en">BIROTA</owl:hasValue>
        <owl:onProperty rdf:resource="jc3iedm_ACTION.owl#chemical-biological-event-category-code"/>
      </owl:Restriction>
    </rdfs:subClassOf>
    <rdfs:label xml:lang="en">biological release other than attack (rota)</rdfs:label>
    <rdfs:comment xml:lang="en">The release of a biological agent or toxin into the environment intentionally or accidentally but not for the intended purpose of conducting an attack.</rdfs:comment>
  </owl:Class>
  <owl:Class rdf:about="jc3iedm_ACTIONExtended.owl#REQUEST_Holding">
    <rdfs:subClassOf rdf:resource="jc3iedm_ACTION.owl#REQUEST"/>
    <rdfs:subClassOf>
      <owl:Restriction>
        <owl:hasValue xml:lang="en">HOLDNG</owl:hasValue>
        <owl:onProperty rdf:resource="jc3iedm_ACTION.owl#request-category-code"/>
      </owl:Restriction>
    </rdfs:subClassOf>
    <rdfs:label xml:lang="en">holding</rdfs:label>
    <rdfs:comment xml:lang="en">To discover the holding of an ACTION-OBJECTIVE (OBJECT-ITEM) by any means.</rdfs:comment>
  </owl:Class>
  <owl:Class rdf:about="jc3iedm_ACTIONExtended.owl#ACTION-EVENT_Attack__deliberate">
    <rdfs:subClassOf rdf:resource="jc3iedm_ACTION.owl#ACTION-EVENT"/>
    <rdfs:subClassOf>
      <owl:Restriction>
        <owl:hasValue xml:lang="en">DLBATK</owl:hasValue>
        <owl:onProperty rdf:resource="jc3iedm_ACTION.owl#action-event-category-code"/>
      </owl:Restriction>
    </rdfs:subClassOf>
    <rdfs:label xml:lang="en">attack, deliberate</rdfs:label>
    <rdfs:comment xml:lang="en">Conducting an offensive operation characterised by pre-planned coordinated employment of firepower and manoeuvre to close with and destroy or capture the enemy.</rdfs:comment>
  </owl:Class>
  <owl:Class rdf:about="jc3iedm_ACTIONExtended.owl#ACTION-EVENT_Bombing__deliberate">
    <rdfs:subClassOf rdf:resource="jc3iedm_ACTION.owl#ACTION-EVENT"/>
    <rdfs:subClassOf>
      <owl:Restriction>
        <owl:hasValue xml:lang="en">BMBDLB</owl:hasValue>
        <owl:onProperty rdf:resource="jc3iedm_ACTION.owl#action-event-category-code"/>
      </owl:Restriction>
    </rdfs:subClassOf>
    <rdfs:label xml:lang="en">bombing, deliberate</rdfs:label>
    <rdfs:comment xml:lang="en">A deliberate and intentional bombing incident.</rdfs:comment>
  </owl:Class>
  <owl:Class rdf:about="jc3iedm_ACTIONExtended.owl#ACTION-EVENT_Missing_individual">
    <rdfs:subClassOf rdf:resource="jc3iedm_ACTION.owl#ACTION-EVENT"/>
    <rdfs:subClassOf>
      <owl:Restriction>
        <owl:hasValue xml:lang="en">MISSIG</owl:hasValue>
        <owl:onProperty rdf:resource="jc3iedm_ACTION.owl#action-event-category-code"/>
      </owl:Restriction>
    </rdfs:subClassOf>
    <rdfs:label xml:lang="en">missing individual</rdfs:label>
    <rdfs:comment xml:lang="en">The absence of a PERSON from an expected or anticipated location.</rdfs:comment>
  </owl:Class>
  <owl:Class rdf:about="jc3iedm_ACTIONExtended.owl#ACTION-EVENT_Riot">
    <rdfs:subClassOf rdf:resource="jc3iedm_ACTION.owl#ACTION-EVENT"/>
    <rdfs:subClassOf>
      <owl:Restriction>
        <owl:hasValue xml:lang="en">RIOT</owl:hasValue>
        <owl:onProperty rdf:resource="jc3iedm_ACTION.owl#action-event-category-code"/>
      </owl:Restriction>
    </rdfs:subClassOf>
    <rdfs:label xml:lang="en">riot</rdfs:label>
    <rdfs:comment xml:lang="en">A disturbance of the peace by a crowd; an occurrence of public disorder.</rdfs:comment>
  </owl:Class>
  <owl:Class rdf:about="jc3iedm_ACTIONExtended.owl#ACTION-EVENT_Providing_host_nation_support">
    <rdfs:subClassOf rdf:resource="jc3iedm_ACTION.owl#ACTION-EVENT"/>
    <rdfs:subClassOf>
      <owl:Restriction>
        <owl:hasValue xml:lang="en">PRVHSN</owl:hasValue>
        <owl:onProperty rdf:resource="jc3iedm_ACTION.owl#action-event-category-code"/>
      </owl:Restriction>
    </rdfs:subClassOf>
    <rdfs:label xml:lang="en">providing host nation support</rdfs:label>
    <rdfs:comment xml:lang="en">Providing civil and/or military assistance rendered by a nation to foreign forces within its territory during peacetime, crises or emergencies, or war based on agreements mutually concluded between nations.</rdfs:comment>
  </owl:Class>
  <owl:Class rdf:about="jc3iedm_ACTIONExtended.owl#ACTION-EVENT_Bombing">
    <rdfs:subClassOf rdf:resource="jc3iedm_ACTION.owl#ACTION-EVENT"/>
    <rdfs:subClassOf>
      <owl:Restriction>
        <owl:hasValue xml:lang="en">BOMBNG</owl:hasValue>
        <owl:onProperty rdf:resource="jc3iedm_ACTION.owl#action-event-category-code"/>
      </owl:Restriction>
    </rdfs:subClassOf>
    <rdfs:label xml:lang="en">bombing</rdfs:label>
    <rdfs:comment xml:lang="en">Attacking, damaging or destroying through the use of bombs.</rdfs:comment>
  </owl:Class>
  <owl:Class rdf:about="jc3iedm_ACTIONExtended.owl#ACTION-EVENT_Aerial_shoot_down">
    <rdfs:subClassOf rdf:resource="jc3iedm_ACTION.owl#ACTION-EVENT"/>
    <rdfs:subClassOf>
      <owl:Restriction>
        <owl:hasValue xml:lang="en">AERSHO</owl:hasValue>
        <owl:onProperty rdf:resource="jc3iedm_ACTION.owl#action-event-category-code"/>
      </owl:Restriction>
    </rdfs:subClassOf>
    <rdfs:label xml:lang="en">aerial shoot down</rdfs:label>
    <rdfs:comment xml:lang="en">The deliberate destruction of an aircraft.</rdfs:comment>
  </owl:Class>
  <owl:Class rdf:about="jc3iedm_ACTIONExtended.owl#ACTION-EVENT_Religious_violence">
    <rdfs:subClassOf rdf:resource="jc3iedm_ACTION.owl#ACTION-EVENT"/>
    <rdfs:subClassOf>
      <owl:Restriction>
        <owl:hasValue xml:lang="en">RELVIO</owl:hasValue>
        <owl:onProperty rdf:resource="jc3iedm_ACTION.owl#action-event-category-code"/>
      </owl:Restriction>
    </rdfs:subClassOf>
    <rdfs:label xml:lang="en">religious violence</rdfs:label>
    <rdfs:comment xml:lang="en">Individual or organised act directed against groups or individuals because of their religious beliefs.</rdfs:comment>
  </owl:Class>
  <owl:Class rdf:about="jc3iedm_ACTIONExtended.owl#ACTION-EVENT_Isolation">
    <rdfs:subClassOf rdf:resource="jc3iedm_ACTION.owl#ACTION-EVENT"/>
    <rdfs:subClassOf>
      <owl:Restriction>
        <owl:hasValue xml:lang="en">ISOLTN</owl:hasValue>
        <owl:onProperty rdf:resource="jc3iedm_ACTION.owl#action-event-category-code"/>
      </owl:Restriction>
    </rdfs:subClassOf>
    <rdfs:label xml:lang="en">isolation</rdfs:label>
    <rdfs:comment xml:lang="en">Sealing off (both physically and psychologically) an enemy from its sources of support, denying an enemy freedom of movement, and preventing an enemy unit from having contact with other enemy forces.</rdfs:comment>
  </owl:Class>
  <owl:Class rdf:about="jc3iedm_ACTIONExtended.owl#ACTION-EVENT_Carrier_launch">
    <rdfs:subClassOf rdf:resource="jc3iedm_ACTION.owl#ACTION-EVENT"/>
    <rdfs:subClassOf>
      <owl:Restriction>
        <owl:hasValue xml:lang="en">CARLNC</owl:hasValue>
        <owl:onProperty rdf:resource="jc3iedm_ACTION.owl#action-event-category-code"/>
      </owl:Restriction>
    </rdfs:subClassOf>
    <rdfs:label xml:lang="en">carrier launch</rdfs:label>
    <rdfs:comment xml:lang="en">Launching of aircraft by a naval platform.</rdfs:comment>
  </owl:Class>
  <owl:Class rdf:about="jc3iedm_ACTIONExtended.owl#ACTION-EVENT_Providing_shelter">
    <rdfs:subClassOf rdf:resource="jc3iedm_ACTION.owl#ACTION-EVENT"/>
    <rdfs:subClassOf>
      <owl:Restriction>
        <owl:hasValue xml:lang="en">PRVSHL</owl:hasValue>
        <owl:onProperty rdf:resource="jc3iedm_ACTION.owl#action-event-category-code"/>
      </owl:Restriction>
    </rdfs:subClassOf>
    <rdfs:label xml:lang="en">providing shelter</rdfs:label>
    <rdfs:comment xml:lang="en">Providing housing.</rdfs:comment>
  </owl:Class>
  <owl:Class rdf:about="jc3iedm_ACTIONExtended.owl#CHEMICAL-BIOLOGICAL-EVENT_Chemical_release_other_than_attack_(ROTA)">
    <rdfs:subClassOf rdf:resource="jc3iedm_ACTION.owl#CHEMICAL-BIOLOGICAL-EVENT"/>
    <rdfs:subClassOf>
      <owl:Restriction>
        <owl:hasValue xml:lang="en">CHROTA</owl:hasValue>
        <owl:onProperty rdf:resource="jc3iedm_ACTION.owl#chemical-biological-event-category-code"/>
      </owl:Restriction>
    </rdfs:subClassOf>
    <rdfs:label xml:lang="en">chemical release other than attack (rota)</rdfs:label>
    <rdfs:comment xml:lang="en">The release of chemicals or chemical agents into the environment intentionally or accidentally but not for the intended purpose of conducting an attack.</rdfs:comment>
  </owl:Class>
  <owl:Class rdf:about="jc3iedm_ACTIONExtended.owl#ACTION-EVENT_Providing_security_services">
    <rdfs:subClassOf rdf:resource="jc3iedm_ACTION.owl#ACTION-EVENT"/>
    <rdfs:subClassOf>
      <owl:Restriction>
        <owl:hasValue xml:lang="en">PRVSCY</owl:hasValue>
        <owl:onProperty rdf:resource="jc3iedm_ACTION.owl#action-event-category-code"/>
      </owl:Restriction>
    </rdfs:subClassOf>
    <rdfs:label xml:lang="en">providing security services</rdfs:label>
    <rdfs:comment xml:lang="en">Providing labour and materiel to assure safety of personnel and facilities.</rdfs:comment>
  </owl:Class>
  <owl:Class rdf:about="jc3iedm_ACTIONExtended.owl#ACTION-EVENT_Accident__workplace">
    <rdfs:subClassOf rdf:resource="jc3iedm_ACTION.owl#ACTION-EVENT"/>
    <rdfs:subClassOf>
      <owl:Restriction>
        <owl:hasValue xml:lang="en">ACCWRK</owl:hasValue>
        <owl:onProperty rdf:resource="jc3iedm_ACTION.owl#action-event-category-code"/>
      </owl:Restriction>
    </rdfs:subClassOf>
    <rdfs:label xml:lang="en">accident, workplace</rdfs:label>
    <rdfs:comment xml:lang="en">An accident occurring at the workplace.</rdfs:comment>
  </owl:Class>
  <owl:Class rdf:about="jc3iedm_ACTIONExtended.owl#ACTION-EVENT_Criminal_incident">
    <rdfs:subClassOf rdf:resource="jc3iedm_ACTION.owl#ACTION-EVENT"/>
    <rdfs:subClassOf>
      <owl:Restriction>
        <owl:hasValue xml:lang="en">CRIMIN</owl:hasValue>
        <owl:onProperty rdf:resource="jc3iedm_ACTION.owl#action-event-category-code"/>
      </owl:Restriction>
    </rdfs:subClassOf>
    <rdfs:label xml:lang="en">criminal incident</rdfs:label>
    <rdfs:comment xml:lang="en">A violation of law.</rdfs:comment>
  </owl:Class>
  <owl:Class rdf:about="jc3iedm_ACTIONExtended.owl#ACTION-EVENT_War_crime">
    <rdfs:subClassOf rdf:resource="jc3iedm_ACTION.owl#ACTION-EVENT"/>
    <rdfs:subClassOf>
      <owl:Restriction>
        <owl:hasValue xml:lang="en">WARCRM</owl:hasValue>
        <owl:onProperty rdf:resource="jc3iedm_ACTION.owl#action-event-category-code"/>
      </owl:Restriction>
    </rdfs:subClassOf>
    <rdfs:label xml:lang="en">war crime</rdfs:label>
    <rdfs:comment xml:lang="en">Violation of the laws and customs of war, i.e. the principles and norms of international law that enshrine the rights and duties of warring parties and neutral states.</rdfs:comment>
  </owl:Class>
  <owl:Class rdf:about="jc3iedm_ACTIONExtended.owl#ACTION-EVENT_Military_mobilisation">
    <rdfs:subClassOf rdf:resource="jc3iedm_ACTION.owl#ACTION-EVENT"/>
    <rdfs:subClassOf>
      <owl:Restriction>
        <owl:hasValue xml:lang="en">MILMOB</owl:hasValue>
        <owl:onProperty rdf:resource="jc3iedm_ACTION.owl#action-event-category-code"/>
      </owl:Restriction>
    </rdfs:subClassOf>
    <rdfs:label xml:lang="en">military mobilisation</rdfs:label>
    <rdfs:comment xml:lang="en">The act of assembling and making ready for active military service.</rdfs:comment>
  </owl:Class>
  <owl:Class rdf:about="jc3iedm_ACTIONExtended.owl#ACTION-EVENT_Refugee_movement">
    <rdfs:subClassOf rdf:resource="jc3iedm_ACTION.owl#ACTION-EVENT"/>
    <rdfs:subClassOf>
      <owl:Restriction>
        <owl:hasValue xml:lang="en">REFMVM</owl:hasValue>
        <owl:onProperty rdf:resource="jc3iedm_ACTION.owl#action-event-category-code"/>
      </owl:Restriction>
    </rdfs:subClassOf>
    <rdfs:label xml:lang="en">refugee movement</rdfs:label>
    <rdfs:comment xml:lang="en">The movement of people who has been forced to leave their country in order to escape war, persecution, or natural disaster.</rdfs:comment>
  </owl:Class>
  <owl:Class rdf:about="jc3iedm_ACTIONExtended.owl#ACTION-EVENT_Cooperating">
    <rdfs:subClassOf rdf:resource="jc3iedm_ACTION.owl#ACTION-EVENT"/>
    <rdfs:subClassOf>
      <owl:Restriction>
        <owl:hasValue xml:lang="en">COOPER</owl:hasValue>
        <owl:onProperty rdf:resource="jc3iedm_ACTION.owl#action-event-category-code"/>
      </owl:Restriction>
    </rdfs:subClassOf>
    <rdfs:label xml:lang="en">cooperating</rdfs:label>
    <rdfs:comment xml:lang="en">Working or acting together.</rdfs:comment>
  </owl:Class>
  <owl:Class rdf:about="jc3iedm_ACTIONExtended.owl#ACTION-EVENT_Conducting_recreational_activities">
    <rdfs:subClassOf rdf:resource="jc3iedm_ACTION.owl#ACTION-EVENT"/>
    <rdfs:subClassOf>
      <owl:Restriction>
        <owl:hasValue xml:lang="en">CNDRCR</owl:hasValue>
        <owl:onProperty rdf:resource="jc3iedm_ACTION.owl#action-event-category-code"/>
      </owl:Restriction>
    </rdfs:subClassOf>
    <rdfs:label xml:lang="en">conducting recreational activities</rdfs:label>
    <rdfs:comment xml:lang="en">Conducting a refreshing or entertaining activity.</rdfs:comment>
  </owl:Class>
  <owl:Class rdf:about="jc3iedm_ACTIONExtended.owl#ACTION-EVENT_Disengaging">
    <rdfs:subClassOf rdf:resource="jc3iedm_ACTION.owl#ACTION-EVENT"/>
    <rdfs:subClassOf>
      <owl:Restriction>
        <owl:hasValue xml:lang="en">DISENG</owl:hasValue>
        <owl:onProperty rdf:resource="jc3iedm_ACTION.owl#action-event-category-code"/>
      </owl:Restriction>
    </rdfs:subClassOf>
    <rdfs:label xml:lang="en">disengaging</rdfs:label>
    <rdfs:comment xml:lang="en">Breaking off an action.</rdfs:comment>
  </owl:Class>
  <owl:Class rdf:about="jc3iedm_ACTIONExtended.owl#ACTION-EVENT_Issuing_press_release">
    <rdfs:subClassOf rdf:resource="jc3iedm_ACTION.owl#ACTION-EVENT"/>
    <rdfs:subClassOf>
      <owl:Restriction>
        <owl:hasValue xml:lang="en">ISSPRS</owl:hasValue>
        <owl:onProperty rdf:resource="jc3iedm_ACTION.owl#action-event-category-code"/>
      </owl:Restriction>
    </rdfs:subClassOf>
    <rdfs:label xml:lang="en">issuing press release</rdfs:label>
    <rdfs:comment xml:lang="en">Sending forth or putting into circulation an official statement issued to media for information.</rdfs:comment>
  </owl:Class>
  <owl:Class rdf:about="jc3iedm_ACTIONExtended.owl#ACTION-EVENT_Border_incursion">
    <rdfs:subClassOf rdf:resource="jc3iedm_ACTION.owl#ACTION-EVENT"/>
    <rdfs:subClassOf>
      <owl:Restriction>
        <owl:hasValue xml:lang="en">BORINC</owl:hasValue>
        <owl:onProperty rdf:resource="jc3iedm_ACTION.owl#action-event-category-code"/>
      </owl:Restriction>
    </rdfs:subClassOf>
    <rdfs:label xml:lang="en">border incursion</rdfs:label>
    <rdfs:comment xml:lang="en">Moving a force or a group of people across a national or territorial border.</rdfs:comment>
  </owl:Class>
  <owl:Class rdf:about="jc3iedm_ACTIONExtended.owl#ACTION-EVENT_Escaping">
    <rdfs:subClassOf rdf:resource="jc3iedm_ACTION.owl#ACTION-EVENT"/>
    <rdfs:subClassOf>
      <owl:Restriction>
        <owl:hasValue xml:lang="en">ESCPNG</owl:hasValue>
        <owl:onProperty rdf:resource="jc3iedm_ACTION.owl#action-event-category-code"/>
      </owl:Restriction>
    </rdfs:subClassOf>
    <rdfs:label xml:lang="en">escaping</rdfs:label>
    <rdfs:comment xml:lang="en">Breaking free from a restriction or control of a place, person, or organisation.</rdfs:comment>
  </owl:Class>
  <owl:Class rdf:about="jc3iedm_ACTIONExtended.owl#ACTION-EVENT_Prisoner_exchange">
    <rdfs:subClassOf rdf:resource="jc3iedm_ACTION.owl#ACTION-EVENT"/>
    <rdfs:subClassOf>
      <owl:Restriction>
        <owl:hasValue xml:lang="en">POWEXC</owl:hasValue>
        <owl:onProperty rdf:resource="jc3iedm_ACTION.owl#action-event-category-code"/>
      </owl:Restriction>
    </rdfs:subClassOf>
    <rdfs:label xml:lang="en">prisoner exchange</rdfs:label>
    <rdfs:comment xml:lang="en">The act of giving or taking POWs in return for others.</rdfs:comment>
  </owl:Class>
  <owl:Class rdf:about="jc3iedm_ACTIONExtended.owl#ACTION-EVENT_Avoiding">
    <rdfs:subClassOf rdf:resource="jc3iedm_ACTION.owl#ACTION-EVENT"/>
    <rdfs:subClassOf>
      <owl:Restriction>
        <owl:hasValue xml:lang="en">AVOIDN</owl:hasValue>
        <owl:onProperty rdf:resource="jc3iedm_ACTION.owl#action-event-category-code"/>
      </owl:Restriction>
    </rdfs:subClassOf>
    <rdfs:label xml:lang="en">avoiding</rdfs:label>
    <rdfs:comment xml:lang="en">Staying clear of a specified object.</rdfs:comment>
  </owl:Class>
  <owl:Class rdf:about="jc3iedm_ACTIONExtended.owl#ACTION-EVENT_Indirect_fire">
    <rdfs:subClassOf rdf:resource="jc3iedm_ACTION.owl#ACTION-EVENT"/>
    <rdfs:subClassOf>
      <owl:Restriction>
        <owl:hasValue xml:lang="en">INDFIR</owl:hasValue>
        <owl:onProperty rdf:resource="jc3iedm_ACTION.owl#action-event-category-code"/>
      </owl:Restriction>
    </rdfs:subClassOf>
    <rdfs:label xml:lang="en">indirect fire</rdfs:label>
    <rdfs:comment xml:lang="en">Fire delivered on a target that is not itself used as a point of aim for the weapons or the director.</rdfs:comment>
  </owl:Class>
  <owl:Class rdf:about="jc3iedm_ACTIONExtended.owl#ACTION-EVENT_Conducting_forward_passage_of_lines">
    <rdfs:subClassOf rdf:resource="jc3iedm_ACTION.owl#ACTION-EVENT"/>
    <rdfs:subClassOf>
      <owl:Restriction>
        <owl:hasValue xml:lang="en">CNFWPS</owl:hasValue>
        <owl:onProperty rdf:resource="jc3iedm_ACTION.owl#action-event-category-code"/>
      </owl:Restriction>
    </rdfs:subClassOf>
    <rdfs:label xml:lang="en">conducting forward passage of lines</rdfs:label>
    <rdfs:comment xml:lang="en">Moving an incoming force through another force that is currently in contact with the enemy in order for the incoming force to come into contact with the enemy.</rdfs:comment>
  </owl:Class>
  <owl:Class rdf:about="jc3iedm_ACTIONExtended.owl#ACTION-EVENT_Containing">
    <rdfs:subClassOf rdf:resource="jc3iedm_ACTION.owl#ACTION-EVENT"/>
    <rdfs:subClassOf>
      <owl:Restriction>
        <owl:hasValue xml:lang="en">CONTAN</owl:hasValue>
        <owl:onProperty rdf:resource="jc3iedm_ACTION.owl#action-event-category-code"/>
      </owl:Restriction>
    </rdfs:subClassOf>
    <rdfs:label xml:lang="en">containing</rdfs:label>
    <rdfs:comment xml:lang="en">Restricting enemy forces by stopping, holding or surrounding them or compelling the enemy forces to centre activity on a given front and to prevent his withdrawing any part of his forces for use elsewhere.</rdfs:comment>
  </owl:Class>
  <owl:Class rdf:about="jc3iedm_ACTIONExtended.owl#ACTION-EVENT_Death_of_spiritual_leader">
    <rdfs:subClassOf rdf:resource="jc3iedm_ACTION.owl#ACTION-EVENT"/>
    <rdfs:subClassOf>
      <owl:Restriction>
        <owl:hasValue xml:lang="en">DEASPL</owl:hasValue>
        <owl:onProperty rdf:resource="jc3iedm_ACTION.owl#action-event-category-code"/>
      </owl:Restriction>
    </rdfs:subClassOf>
    <rdfs:label xml:lang="en">death of spiritual leader</rdfs:label>
    <rdfs:comment xml:lang="en">Self-defined.</rdfs:comment>
  </owl:Class>
  <owl:Class rdf:about="jc3iedm_ACTIONExtended.owl#ACTION-EVENT_Providing_education_services">
    <rdfs:subClassOf rdf:resource="jc3iedm_ACTION.owl#ACTION-EVENT"/>
    <rdfs:subClassOf>
      <owl:Restriction>
        <owl:hasValue xml:lang="en">PRVEDU</owl:hasValue>
        <owl:onProperty rdf:resource="jc3iedm_ACTION.owl#action-event-category-code"/>
      </owl:Restriction>
    </rdfs:subClassOf>
    <rdfs:label xml:lang="en">providing education services</rdfs:label>
    <rdfs:comment xml:lang="en">Providing labour and materiel for the educational process.</rdfs:comment>
  </owl:Class>
  <owl:Class rdf:about="jc3iedm_ACTIONExtended.owl#ACTION-EVENT_Fire">
    <rdfs:subClassOf rdf:resource="jc3iedm_ACTION.owl#ACTION-EVENT"/>
    <rdfs:subClassOf>
      <owl:Restriction>
        <owl:hasValue xml:lang="en">FIRE</owl:hasValue>
        <owl:onProperty rdf:resource="jc3iedm_ACTION.owl#action-event-category-code"/>
      </owl:Restriction>
    </rdfs:subClassOf>
    <rdfs:label xml:lang="en">fire</rdfs:label>
    <rdfs:comment xml:lang="en">A rapid, persistent chemical reaction that releases heat and light, especially the exothermic combination of a combustible substance with oxygen.</rdfs:comment>
  </owl:Class>
  <owl:Class rdf:about="jc3iedm_ACTIONExtended.owl#ACTION-EVENT_Infiltration">
    <rdfs:subClassOf rdf:resource="jc3iedm_ACTION.owl#ACTION-EVENT"/>
    <rdfs:subClassOf>
      <owl:Restriction>
        <owl:hasValue xml:lang="en">INFLTN</owl:hasValue>
        <owl:onProperty rdf:resource="jc3iedm_ACTION.owl#action-event-category-code"/>
      </owl:Restriction>
    </rdfs:subClassOf>
    <rdfs:label xml:lang="en">infiltration</rdfs:label>
    <rdfs:comment xml:lang="en">Moving a force, broken down as individuals or small groups, over, through or around enemy positions with the aim of avoiding detection.</rdfs:comment>
  </owl:Class>
  <owl:Class rdf:about="jc3iedm_ACTIONExtended.owl#ACTION-EVENT_Death_of_chief_of_state">
    <rdfs:subClassOf rdf:resource="jc3iedm_ACTION.owl#ACTION-EVENT"/>
    <rdfs:subClassOf>
      <owl:Restriction>
        <owl:hasValue xml:lang="en">DEACST</owl:hasValue>
        <owl:onProperty rdf:resource="jc3iedm_ACTION.owl#action-event-category-code"/>
      </owl:Restriction>
    </rdfs:subClassOf>
    <rdfs:label xml:lang="en">death of chief of state</rdfs:label>
    <rdfs:comment xml:lang="en">Self-defined.</rdfs:comment>
  </owl:Class>
  <owl:Class rdf:about="jc3iedm_ACTIONExtended.owl#ACTION-EVENT_Serving_as_a_main_body">
    <rdfs:subClassOf rdf:resource="jc3iedm_ACTION.owl#ACTION-EVENT"/>
    <rdfs:subClassOf>
      <owl:Restriction>
        <owl:hasValue xml:lang="en">SRVMNB</owl:hasValue>
        <owl:onProperty rdf:resource="jc3iedm_ACTION.owl#action-event-category-code"/>
      </owl:Restriction>
    </rdfs:subClassOf>
    <rdfs:label xml:lang="en">serving as a main body</rdfs:label>
    <rdfs:comment xml:lang="en">Operating as the main force for a specific operation.</rdfs:comment>
  </owl:Class>
  <owl:Class rdf:about="jc3iedm_ACTIONExtended.owl#ACTION-EVENT_Torture">
    <rdfs:subClassOf rdf:resource="jc3iedm_ACTION.owl#ACTION-EVENT"/>
    <rdfs:subClassOf>
      <owl:Restriction>
        <owl:hasValue xml:lang="en">TORTUR</owl:hasValue>
        <owl:onProperty rdf:resource="jc3iedm_ACTION.owl#action-event-category-code"/>
      </owl:Restriction>
    </rdfs:subClassOf>
    <rdfs:label xml:lang="en">torture</rdfs:label>
    <rdfs:comment xml:lang="en">An action or practice of inflicting severe pain as a punishment or a forcible means of persuasion.</rdfs:comment>
  </owl:Class>
  <owl:Class rdf:about="jc3iedm_ACTIONExtended.owl#ACTION-EVENT_Civil_unrest">
    <rdfs:subClassOf rdf:resource="jc3iedm_ACTION.owl#ACTION-EVENT"/>
    <rdfs:subClassOf>
      <owl:Restriction>
        <owl:hasValue xml:lang="en">CIVUNR</owl:hasValue>
        <owl:onProperty rdf:resource="jc3iedm_ACTION.owl#action-event-category-code"/>
      </owl:Restriction>
    </rdfs:subClassOf>
    <rdfs:label xml:lang="en">civil unrest</rdfs:label>
    <rdfs:comment xml:lang="en">A behaviour that results in the disturbance of the normal order of society that generally falls short of riots and/or property destruction in the civil population.</rdfs:comment>
  </owl:Class>
  <owl:Class rdf:about="jc3iedm_ACTIONExtended.owl#ACTION-EVENT_Accident__weapon">
    <rdfs:subClassOf rdf:resource="jc3iedm_ACTION.owl#ACTION-EVENT"/>
    <rdfs:subClassOf>
      <owl:Restriction>
        <owl:hasValue xml:lang="en">ACCWPN</owl:hasValue>
        <owl:onProperty rdf:resource="jc3iedm_ACTION.owl#action-event-category-code"/>
      </owl:Restriction>
    </rdfs:subClassOf>
    <rdfs:label xml:lang="en">accident, weapon</rdfs:label>
    <rdfs:comment xml:lang="en">An accident involving a weapon.</rdfs:comment>
  </owl:Class>
  <owl:Class rdf:about="jc3iedm_ACTIONExtended.owl#ACTION-EVENT_Early_warning_alert">
    <rdfs:subClassOf rdf:resource="jc3iedm_ACTION.owl#ACTION-EVENT"/>
    <rdfs:subClassOf>
      <owl:Restriction>
        <owl:hasValue xml:lang="en">EARWAR</owl:hasValue>
        <owl:onProperty rdf:resource="jc3iedm_ACTION.owl#action-event-category-code"/>
      </owl:Restriction>
    </rdfs:subClassOf>
    <rdfs:label xml:lang="en">early warning alert</rdfs:label>
    <rdfs:comment xml:lang="en">Early notification of the launch or approach of weapons or weapons carriers.</rdfs:comment>
  </owl:Class>
  <owl:Class rdf:about="jc3iedm_ACTIONExtended.owl#ACTION-EVENT_Providing_transhipment_services">
    <rdfs:subClassOf rdf:resource="jc3iedm_ACTION.owl#ACTION-EVENT"/>
    <rdfs:subClassOf>
      <owl:Restriction>
        <owl:hasValue xml:lang="en">PRVTRS</owl:hasValue>
        <owl:onProperty rdf:resource="jc3iedm_ACTION.owl#action-event-category-code"/>
      </owl:Restriction>
    </rdfs:subClassOf>
    <rdfs:label xml:lang="en">providing transhipment services</rdfs:label>
    <rdfs:comment xml:lang="en">Providing movement of cargo from one ship or train or container to another for further shipment.</rdfs:comment>
  </owl:Class>
  <owl:Class rdf:about="jc3iedm_ACTIONExtended.owl#ACTION-EVENT_Offensive_counteroffensive">
    <rdfs:subClassOf rdf:resource="jc3iedm_ACTION.owl#ACTION-EVENT"/>
    <rdfs:subClassOf>
      <owl:Restriction>
        <owl:hasValue xml:lang="en">OFFCOF</owl:hasValue>
        <owl:onProperty rdf:resource="jc3iedm_ACTION.owl#action-event-category-code"/>
      </owl:Restriction>
    </rdfs:subClassOf>
    <rdfs:label xml:lang="en">offensive/counteroffensive</rdfs:label>
    <rdfs:comment xml:lang="en">Conducting an operation by an attack force.</rdfs:comment>
  </owl:Class>
  <owl:Class rdf:about="jc3iedm_ACTIONExtended.owl#ACTION-EVENT_Psychological_operation">
    <rdfs:subClassOf rdf:resource="jc3iedm_ACTION.owl#ACTION-EVENT"/>
    <rdfs:subClassOf>
      <owl:Restriction>
        <owl:hasValue xml:lang="en">PSYOP</owl:hasValue>
        <owl:onProperty rdf:resource="jc3iedm_ACTION.owl#action-event-category-code"/>
      </owl:Restriction>
    </rdfs:subClassOf>
    <rdfs:label xml:lang="en">psychological operation</rdfs:label>
    <rdfs:comment xml:lang="en">Planned operations to convey selected information and indicators to foreign audiences to influence their emotions, motives, objective reasoning, and ultimately the behaviour of foreign governments, organisations, groups, and individuals. The purpose of psychological operations is to induce or reinforce foreign attitudes and behaviour favourable to the originator's objectives.</rdfs:comment>
  </owl:Class>
  <owl:Class rdf:about="jc3iedm_ACTIONExtended.owl#ACTION-EVENT_Providing_healthcare_services">
    <rdfs:subClassOf rdf:resource="jc3iedm_ACTION.owl#ACTION-EVENT"/>
    <rdfs:subClassOf>
      <owl:Restriction>
        <owl:hasValue xml:lang="en">PRVHLT</owl:hasValue>
        <owl:onProperty rdf:resource="jc3iedm_ACTION.owl#action-event-category-code"/>
      </owl:Restriction>
    </rdfs:subClassOf>
    <rdfs:label xml:lang="en">providing healthcare services</rdfs:label>
    <rdfs:comment xml:lang="en">Providing labour and materiel for maintaining the general health and welfare.</rdfs:comment>
  </owl:Class>
  <owl:Class rdf:about="jc3iedm_ACTIONExtended.owl#ACTION-EVENT_Peace_treaty_agreement">
    <rdfs:subClassOf rdf:resource="jc3iedm_ACTION.owl#ACTION-EVENT"/>
    <rdfs:subClassOf>
      <owl:Restriction>
        <owl:hasValue xml:lang="en">PEAAGR</owl:hasValue>
        <owl:onProperty rdf:resource="jc3iedm_ACTION.owl#action-event-category-code"/>
      </owl:Restriction>
    </rdfs:subClassOf>
    <rdfs:label xml:lang="en">peace treaty agreement</rdfs:label>
    <rdfs:comment xml:lang="en">An arrangement or contract among involved nations or factions to end a conflict.</rdfs:comment>
  </owl:Class>
  <owl:Class rdf:about="jc3iedm_ACTIONExtended.owl#ACTION-EVENT_Terrorism">
    <rdfs:subClassOf rdf:resource="jc3iedm_ACTION.owl#ACTION-EVENT"/>
    <rdfs:subClassOf>
      <owl:Restriction>
        <owl:hasValue xml:lang="en">TERR</owl:hasValue>
        <owl:onProperty rdf:resource="jc3iedm_ACTION.owl#action-event-category-code"/>
      </owl:Restriction>
    </rdfs:subClassOf>
    <rdfs:label xml:lang="en">terrorism</rdfs:label>
    <rdfs:comment xml:lang="en">Using or threatening force or violence against individuals or property in an attempt to coerce or intimidate governments or societies to achieve political, religious or ideological objectives.</rdfs:comment>
  </owl:Class>
  <owl:Class rdf:about="jc3iedm_ACTIONExtended.owl#ACTION-EVENT_Rendezvous">
    <rdfs:subClassOf rdf:resource="jc3iedm_ACTION.owl#ACTION-EVENT"/>
    <rdfs:subClassOf>
      <owl:Restriction>
        <owl:hasValue xml:lang="en">RNDZVS</owl:hasValue>
        <owl:onProperty rdf:resource="jc3iedm_ACTION.owl#action-event-category-code"/>
      </owl:Restriction>
    </rdfs:subClassOf>
    <rdfs:label xml:lang="en">rendezvous</rdfs:label>
    <rdfs:comment xml:lang="en">Achieving a pre-arranged meeting at a given time and place.</rdfs:comment>
  </owl:Class>
  <owl:Class rdf:about="jc3iedm_ACTIONExtended.owl#ACTION-EVENT_Massing_of_forces">
    <rdfs:subClassOf rdf:resource="jc3iedm_ACTION.owl#ACTION-EVENT"/>
    <rdfs:subClassOf>
      <owl:Restriction>
        <owl:hasValue xml:lang="en">MASFOR</owl:hasValue>
        <owl:onProperty rdf:resource="jc3iedm_ACTION.owl#action-event-category-code"/>
      </owl:Restriction>
    </rdfs:subClassOf>
    <rdfs:label xml:lang="en">massing of forces</rdfs:label>
    <rdfs:comment xml:lang="en">The concentration of large quantities of military equipment and personnel.</rdfs:comment>
  </owl:Class>
  <owl:Class rdf:about="jc3iedm_ACTIONExtended.owl#ACTION-EVENT_Obscure">
    <rdfs:subClassOf rdf:resource="jc3iedm_ACTION.owl#ACTION-EVENT"/>
    <rdfs:subClassOf>
      <owl:Restriction>
        <owl:hasValue xml:lang="en">OBSCUR</owl:hasValue>
        <owl:onProperty rdf:resource="jc3iedm_ACTION.owl#action-event-category-code"/>
      </owl:Restriction>
    </rdfs:subClassOf>
    <rdfs:label xml:lang="en">obscure</rdfs:label>
    <rdfs:comment xml:lang="en">Covering something by a smoke screen.</rdfs:comment>
  </owl:Class>
  <owl:Class rdf:about="jc3iedm_ACTIONExtended.owl#ACTION-EVENT_Marking">
    <rdfs:subClassOf rdf:resource="jc3iedm_ACTION.owl#ACTION-EVENT"/>
    <rdfs:subClassOf>
      <owl:Restriction>
        <owl:hasValue xml:lang="en">MARKNG</owl:hasValue>
        <owl:onProperty rdf:resource="jc3iedm_ACTION.owl#action-event-category-code"/>
      </owl:Restriction>
    </rdfs:subClassOf>
    <rdfs:label xml:lang="en">marking</rdfs:label>
    <rdfs:comment xml:lang="en">Making visible (by the use of light/IR/laser/arty) an object in order to allow its identification by another object (usually as a precursor to the use of direct fire weapons).</rdfs:comment>
  </owl:Class>
  <owl:Class rdf:about="jc3iedm_ACTIONExtended.owl#ACTION-EVENT_Delaying">
    <rdfs:subClassOf rdf:resource="jc3iedm_ACTION.owl#ACTION-EVENT"/>
    <rdfs:subClassOf>
      <owl:Restriction>
        <owl:hasValue xml:lang="en">DELAYN</owl:hasValue>
        <owl:onProperty rdf:resource="jc3iedm_ACTION.owl#action-event-category-code"/>
      </owl:Restriction>
    </rdfs:subClassOf>
    <rdfs:label xml:lang="en">delaying</rdfs:label>
    <rdfs:comment xml:lang="en">Slowing the momentum of the enemy by conducting an operation in which the force under pressure trades time for space; the aim is to inflict the maximum damage on the enemy without becoming decisively engaged.</rdfs:comment>
  </owl:Class>
  <owl:Class rdf:about="jc3iedm_ACTIONExtended.owl#ACTION-EVENT_Attack__diversion">
    <rdfs:subClassOf rdf:resource="jc3iedm_ACTION.owl#ACTION-EVENT"/>
    <rdfs:subClassOf>
      <owl:Restriction>
        <owl:hasValue xml:lang="en">ATTDVR</owl:hasValue>
        <owl:onProperty rdf:resource="jc3iedm_ACTION.owl#action-event-category-code"/>
      </owl:Restriction>
    </rdfs:subClassOf>
    <rdfs:label xml:lang="en">attack, diversion</rdfs:label>
    <rdfs:comment xml:lang="en">Conducting an attack wherein a force attacks, or threatens to attack, a target other than the main target for the purpose of drawing enemy defences away from the main effort.</rdfs:comment>
  </owl:Class>
  <owl:Class rdf:about="jc3iedm_ACTIONExtended.owl#ACTION-EVENT_Troublemaking__agitating">
    <rdfs:subClassOf rdf:resource="jc3iedm_ACTION.owl#ACTION-EVENT"/>
    <rdfs:subClassOf>
      <owl:Restriction>
        <owl:hasValue xml:lang="en">TRBAGT</owl:hasValue>
        <owl:onProperty rdf:resource="jc3iedm_ACTION.owl#action-event-category-code"/>
      </owl:Restriction>
    </rdfs:subClassOf>
    <rdfs:label xml:lang="en">troublemaking, agitating</rdfs:label>
    <rdfs:comment xml:lang="en">Stirring up of public interest on a matter of controversy, such as a political or social issue.</rdfs:comment>
  </owl:Class>
  <owl:Class rdf:about="jc3iedm_ACTIONExtended.owl#ACTION-EVENT_Providing_camps">
    <rdfs:subClassOf rdf:resource="jc3iedm_ACTION.owl#ACTION-EVENT"/>
    <rdfs:subClassOf>
      <owl:Restriction>
        <owl:hasValue xml:lang="en">PRVCMP</owl:hasValue>
        <owl:onProperty rdf:resource="jc3iedm_ACTION.owl#action-event-category-code"/>
      </owl:Restriction>
    </rdfs:subClassOf>
    <rdfs:label xml:lang="en">providing camps</rdfs:label>
    <rdfs:comment xml:lang="en">Providing temporary accommodation of various kinds, usually consisting of huts or tents, for detainees, homeless persons, and other emergency use.</rdfs:comment>
  </owl:Class>
  <owl:Class rdf:about="jc3iedm_ACTIONExtended.owl#ACTION-EVENT_Hostage_taking">
    <rdfs:subClassOf rdf:resource="jc3iedm_ACTION.owl#ACTION-EVENT"/>
    <rdfs:subClassOf>
      <owl:Restriction>
        <owl:hasValue xml:lang="en">HSTTKN</owl:hasValue>
        <owl:onProperty rdf:resource="jc3iedm_ACTION.owl#action-event-category-code"/>
      </owl:Restriction>
    </rdfs:subClassOf>
    <rdfs:label xml:lang="en">hostage taking</rdfs:label>
    <rdfs:comment xml:lang="en">Action to seize or hold a person as security for the fulfilment of a condition.</rdfs:comment>
  </owl:Class>
  <owl:Class rdf:about="jc3iedm_ACTIONExtended.owl#ACTION-EVENT_Governmental_collapse">
    <rdfs:subClassOf rdf:resource="jc3iedm_ACTION.owl#ACTION-EVENT"/>
    <rdfs:subClassOf>
      <owl:Restriction>
        <owl:hasValue xml:lang="en">GOVCOL</owl:hasValue>
        <owl:onProperty rdf:resource="jc3iedm_ACTION.owl#action-event-category-code"/>
      </owl:Restriction>
    </rdfs:subClassOf>
    <rdfs:label xml:lang="en">governmental collapse</rdfs:label>
    <rdfs:comment xml:lang="en">The sudden loss of force, effectiveness or authority of the governing organisation.</rdfs:comment>
  </owl:Class>
  <owl:Class rdf:about="jc3iedm_ACTIONExtended.owl#ACTION-EVENT_Serving_as_a_flank_guard">
    <rdfs:subClassOf rdf:resource="jc3iedm_ACTION.owl#ACTION-EVENT"/>
    <rdfs:subClassOf>
      <owl:Restriction>
        <owl:hasValue xml:lang="en">SRVFLK</owl:hasValue>
        <owl:onProperty rdf:resource="jc3iedm_ACTION.owl#action-event-category-code"/>
      </owl:Restriction>
    </rdfs:subClassOf>
    <rdfs:label xml:lang="en">serving as a flank guard</rdfs:label>
    <rdfs:comment xml:lang="en">Operating as a security element whose primary task is to protect the main force by fighting on the designated flank to gain time, whilst also observing and reporting information.</rdfs:comment>
  </owl:Class>
  <owl:Class rdf:about="jc3iedm_ACTIONExtended.owl#ACTION-EVENT_Blocking">
    <rdfs:subClassOf rdf:resource="jc3iedm_ACTION.owl#ACTION-EVENT"/>
    <rdfs:subClassOf>
      <owl:Restriction>
        <owl:hasValue xml:lang="en">BLOCKN</owl:hasValue>
        <owl:onProperty rdf:resource="jc3iedm_ACTION.owl#action-event-category-code"/>
      </owl:Restriction>
    </rdfs:subClassOf>
    <rdfs:label xml:lang="en">blocking</rdfs:label>
    <rdfs:comment xml:lang="en">Denying of enemy access to an area or preventing his advance in a direction or along an avenue of approach.</rdfs:comment>
  </owl:Class>
  <owl:Class rdf:about="jc3iedm_ACTIONExtended.owl#ACTION-EVENT_Outbreak_of_racial_tribal_ethnic_warfare">
    <rdfs:subClassOf rdf:resource="jc3iedm_ACTION.owl#ACTION-EVENT"/>
    <rdfs:subClassOf>
      <owl:Restriction>
        <owl:hasValue xml:lang="en">RACIAL</owl:hasValue>
        <owl:onProperty rdf:resource="jc3iedm_ACTION.owl#action-event-category-code"/>
      </owl:Restriction>
    </rdfs:subClassOf>
    <rdfs:label xml:lang="en">outbreak of racial/tribal/ethnic warfare</rdfs:label>
    <rdfs:comment xml:lang="en">The use of force or violence by or against racial or tribal groups.</rdfs:comment>
  </owl:Class>
  <owl:Class rdf:about="jc3iedm_ACTIONExtended.owl#CHEMICAL-BIOLOGICAL-EVENT_Chemical_attack">
    <rdfs:subClassOf rdf:resource="jc3iedm_ACTION.owl#CHEMICAL-BIOLOGICAL-EVENT"/>
    <rdfs:subClassOf>
      <owl:Restriction>
        <owl:hasValue xml:lang="en">CHMATT</owl:hasValue>
        <owl:onProperty rdf:resource="jc3iedm_ACTION.owl#chemical-biological-event-category-code"/>
      </owl:Restriction>
    </rdfs:subClassOf>
    <rdfs:label xml:lang="en">chemical attack</rdfs:label>
    <rdfs:comment xml:lang="en">Employing the use of chemical materiel(s) [agent(s)] to produce casualties in man or animals and damage to plants or materiel; or defence against such employment.</rdfs:comment>
  </owl:Class>
  <owl:Class rdf:about="jc3iedm_ACTIONExtended.owl#ACTION-EVENT_Naval_gun_fire">
    <rdfs:subClassOf rdf:resource="jc3iedm_ACTION.owl#ACTION-EVENT"/>
    <rdfs:subClassOf>
      <owl:Restriction>
        <owl:hasValue xml:lang="en">NAVGUN</owl:hasValue>
        <owl:onProperty rdf:resource="jc3iedm_ACTION.owl#action-event-category-code"/>
      </owl:Restriction>
    </rdfs:subClassOf>
    <rdfs:label xml:lang="en">naval gun fire</rdfs:label>
    <rdfs:comment xml:lang="en">The act of firing a naval surface-to-surface weapon.</rdfs:comment>
  </owl:Class>
  <owl:Class rdf:about="jc3iedm_ACTIONExtended.owl#ACTION-EVENT_Providing_construction_services">
    <rdfs:subClassOf rdf:resource="jc3iedm_ACTION.owl#ACTION-EVENT"/>
    <rdfs:subClassOf>
      <owl:Restriction>
        <owl:hasValue xml:lang="en">PRVCNS</owl:hasValue>
        <owl:onProperty rdf:resource="jc3iedm_ACTION.owl#action-event-category-code"/>
      </owl:Restriction>
    </rdfs:subClassOf>
    <rdfs:label xml:lang="en">providing construction services</rdfs:label>
    <rdfs:comment xml:lang="en">Providing labour and materiel for construction of facilities.</rdfs:comment>
  </owl:Class>
  <owl:Class rdf:about="jc3iedm_ACTIONExtended.owl#ACTION-EVENT_Petroleum_product_spills">
    <rdfs:subClassOf rdf:resource="jc3iedm_ACTION.owl#ACTION-EVENT"/>
    <rdfs:subClassOf>
      <owl:Restriction>
        <owl:hasValue xml:lang="en">PETSPL</owl:hasValue>
        <owl:onProperty rdf:resource="jc3iedm_ACTION.owl#action-event-category-code"/>
      </owl:Restriction>
    </rdfs:subClassOf>
    <rdfs:label xml:lang="en">petroleum product spills</rdfs:label>
    <rdfs:comment xml:lang="en">The accidental or delivered release of any petroleum product into the environment.</rdfs:comment>
  </owl:Class>
  <owl:Class rdf:about="jc3iedm_ACTIONExtended.owl#ACTION-EVENT_Reconnaissance_in_force">
    <rdfs:subClassOf rdf:resource="jc3iedm_ACTION.owl#ACTION-EVENT"/>
    <rdfs:subClassOf>
      <owl:Restriction>
        <owl:hasValue xml:lang="en">RECCEF</owl:hasValue>
        <owl:onProperty rdf:resource="jc3iedm_ACTION.owl#action-event-category-code"/>
      </owl:Restriction>
    </rdfs:subClassOf>
    <rdfs:label xml:lang="en">reconnaissance in force</rdfs:label>
    <rdfs:comment xml:lang="en">Conducting an offensive operation designed to discover and/or test the enemy’s strength, or to obtain other information.</rdfs:comment>
  </owl:Class>
  <owl:Class rdf:about="jc3iedm_ACTIONExtended.owl#ACTION-EVENT_Issuing_media_documentary">
    <rdfs:subClassOf rdf:resource="jc3iedm_ACTION.owl#ACTION-EVENT"/>
    <rdfs:subClassOf>
      <owl:Restriction>
        <owl:hasValue xml:lang="en">ISSMDD</owl:hasValue>
        <owl:onProperty rdf:resource="jc3iedm_ACTION.owl#action-event-category-code"/>
      </owl:Restriction>
    </rdfs:subClassOf>
    <rdfs:label xml:lang="en">issuing media documentary</rdfs:label>
    <rdfs:comment xml:lang="en">Sending forth or putting into circulation any document published on a media that provides a factual record or report.</rdfs:comment>
  </owl:Class>
  <owl:Class rdf:about="jc3iedm_ACTIONExtended.owl#ACTION-EVENT_Medical_evacuation">
    <rdfs:subClassOf rdf:resource="jc3iedm_ACTION.owl#ACTION-EVENT"/>
    <rdfs:subClassOf>
      <owl:Restriction>
        <owl:hasValue xml:lang="en">MEDEVC</owl:hasValue>
        <owl:onProperty rdf:resource="jc3iedm_ACTION.owl#action-event-category-code"/>
      </owl:Restriction>
    </rdfs:subClassOf>
    <rdfs:label xml:lang="en">medical evacuation</rdfs:label>
    <rdfs:comment xml:lang="en">The process of moving any person who is wounded, injured or ill to/between medical treatment FACILITYs.</rdfs:comment>
  </owl:Class>
  <owl:Class rdf:about="jc3iedm_ACTIONExtended.owl#ACTION-EVENT_Locating">
    <rdfs:subClassOf rdf:resource="jc3iedm_ACTION.owl#ACTION-EVENT"/>
    <rdfs:subClassOf>
      <owl:Restriction>
        <owl:hasValue xml:lang="en">LOCTNG</owl:hasValue>
        <owl:onProperty rdf:resource="jc3iedm_ACTION.owl#action-event-category-code"/>
      </owl:Restriction>
    </rdfs:subClassOf>
    <rdfs:label xml:lang="en">locating</rdfs:label>
    <rdfs:comment xml:lang="en">Establishing the position of an object.</rdfs:comment>
  </owl:Class>
  <owl:Class rdf:about="jc3iedm_ACTIONExtended.owl#ACTION-EVENT_Conducting_conference">
    <rdfs:subClassOf rdf:resource="jc3iedm_ACTION.owl#ACTION-EVENT"/>
    <rdfs:subClassOf>
      <owl:Restriction>
        <owl:hasValue xml:lang="en">CNDCNF</owl:hasValue>
        <owl:onProperty rdf:resource="jc3iedm_ACTION.owl#action-event-category-code"/>
      </owl:Restriction>
    </rdfs:subClassOf>
    <rdfs:label xml:lang="en">conducting conference</rdfs:label>
    <rdfs:comment xml:lang="en">Conducting a meeting for discussion, esp. a regular one held by an association or organisation.</rdfs:comment>
  </owl:Class>
  <owl:Class rdf:about="jc3iedm_ACTIONExtended.owl#ACTION-EVENT_Peace_conference">
    <rdfs:subClassOf rdf:resource="jc3iedm_ACTION.owl#ACTION-EVENT"/>
    <rdfs:subClassOf>
      <owl:Restriction>
        <owl:hasValue xml:lang="en">PEACON</owl:hasValue>
        <owl:onProperty rdf:resource="jc3iedm_ACTION.owl#action-event-category-code"/>
      </owl:Restriction>
    </rdfs:subClassOf>
    <rdfs:label xml:lang="en">peace conference</rdfs:label>
    <rdfs:comment xml:lang="en">A meeting of a group of persons to discuss a peace process.</rdfs:comment>
  </owl:Class>
  <owl:Class rdf:about="jc3iedm_ACTIONExtended.owl#ACTION-EVENT_Following_and_assuming">
    <rdfs:subClassOf rdf:resource="jc3iedm_ACTION.owl#ACTION-EVENT"/>
    <rdfs:subClassOf>
      <owl:Restriction>
        <owl:hasValue xml:lang="en">FOLASS</owl:hasValue>
        <owl:onProperty rdf:resource="jc3iedm_ACTION.owl#action-event-category-code"/>
      </owl:Restriction>
    </rdfs:subClassOf>
    <rdfs:label xml:lang="en">following and assuming</rdfs:label>
    <rdfs:comment xml:lang="en">Operating as a committed force that is following a force conducting an offensive operation and is prepared to continue the mission of the force it is following when that force is fixed, attrited, or otherwise unable to continue.</rdfs:comment>
  </owl:Class>
  <owl:Class rdf:about="jc3iedm_ACTIONExtended.owl#ACTION-EVENT_Border_crossing__planned">
    <rdfs:subClassOf rdf:resource="jc3iedm_ACTION.owl#ACTION-EVENT"/>
    <rdfs:subClassOf>
      <owl:Restriction>
        <owl:hasValue xml:lang="en">BCPLND</owl:hasValue>
        <owl:onProperty rdf:resource="jc3iedm_ACTION.owl#action-event-category-code"/>
      </owl:Restriction>
    </rdfs:subClassOf>
    <rdfs:label xml:lang="en">border crossing, planned</rdfs:label>
    <rdfs:comment xml:lang="en">A border crossing that is known to have been planned ahead of time.</rdfs:comment>
  </owl:Class>
  <owl:Class rdf:about="jc3iedm_ACTIONExtended.owl#ACTION-EVENT_Electronic_warfare">
    <rdfs:subClassOf rdf:resource="jc3iedm_ACTION.owl#ACTION-EVENT"/>
    <rdfs:subClassOf>
      <owl:Restriction>
        <owl:hasValue xml:lang="en">ELCWAR</owl:hasValue>
        <owl:onProperty rdf:resource="jc3iedm_ACTION.owl#action-event-category-code"/>
      </owl:Restriction>
    </rdfs:subClassOf>
    <rdfs:label xml:lang="en">electronic warfare</rdfs:label>
    <rdfs:comment xml:lang="en">Military action to exploit the electro-magnetic spectrum encompassing the search for, interception and identification of electro-magnetic emissions, the employment of electro-magnetic energy, including directed energy, to reduce or prevent hostile use of the electro-magnetic spectrum, and actions to ensure its effective use by friendly forces.</rdfs:comment>
  </owl:Class>
  <owl:Class rdf:about="jc3iedm_ACTIONExtended.owl#ACTION-EVENT_Shooting">
    <rdfs:subClassOf rdf:resource="jc3iedm_ACTION.owl#ACTION-EVENT"/>
    <rdfs:subClassOf>
      <owl:Restriction>
        <owl:hasValue xml:lang="en">SHOTNG</owl:hasValue>
        <owl:onProperty rdf:resource="jc3iedm_ACTION.owl#action-event-category-code"/>
      </owl:Restriction>
    </rdfs:subClassOf>
    <rdfs:label xml:lang="en">shooting</rdfs:label>
    <rdfs:comment xml:lang="en">The act of firing of a weapon, usually at a person.</rdfs:comment>
  </owl:Class>
  <owl:Class rdf:about="jc3iedm_ACTIONExtended.owl#ACTION-EVENT_Religious_demonstration">
    <rdfs:subClassOf rdf:resource="jc3iedm_ACTION.owl#ACTION-EVENT"/>
    <rdfs:subClassOf>
      <owl:Restriction>
        <owl:hasValue xml:lang="en">RELDEM</owl:hasValue>
        <owl:onProperty rdf:resource="jc3iedm_ACTION.owl#action-event-category-code"/>
      </owl:Restriction>
    </rdfs:subClassOf>
    <rdfs:label xml:lang="en">religious demonstration</rdfs:label>
    <rdfs:comment xml:lang="en">A public display of group feelings towards a religious idea, person or cause.</rdfs:comment>
  </owl:Class>
  <owl:Class rdf:about="jc3iedm_ACTIONExtended.owl#ACTION-EVENT_Drug_consumption__illegal">
    <rdfs:subClassOf rdf:resource="jc3iedm_ACTION.owl#ACTION-EVENT"/>
    <rdfs:subClassOf>
      <owl:Restriction>
        <owl:hasValue xml:lang="en">DRGCNS</owl:hasValue>
        <owl:onProperty rdf:resource="jc3iedm_ACTION.owl#action-event-category-code"/>
      </owl:Restriction>
    </rdfs:subClassOf>
    <rdfs:label xml:lang="en">drug consumption, illegal</rdfs:label>
    <rdfs:comment xml:lang="en">An action of consuming illegal drugs.</rdfs:comment>
  </owl:Class>
  <owl:Class rdf:about="jc3iedm_ACTIONExtended.owl#ACTION-EVENT_Arresting_obstructing">
    <rdfs:subClassOf rdf:resource="jc3iedm_ACTION.owl#ACTION-EVENT"/>
    <rdfs:subClassOf>
      <owl:Restriction>
        <owl:hasValue xml:lang="en">ARROBS</owl:hasValue>
        <owl:onProperty rdf:resource="jc3iedm_ACTION.owl#action-event-category-code"/>
      </owl:Restriction>
    </rdfs:subClassOf>
    <rdfs:label xml:lang="en">arresting/obstructing</rdfs:label>
    <rdfs:comment xml:lang="en">Stopping or checking of the motion, progress, growth, or spread of something.</rdfs:comment>
  </owl:Class>
  <owl:Class rdf:about="jc3iedm_ACTIONExtended.owl#ACTION-EVENT_Air_assault">
    <rdfs:subClassOf rdf:resource="jc3iedm_ACTION.owl#ACTION-EVENT"/>
    <rdfs:subClassOf>
      <owl:Restriction>
        <owl:hasValue xml:lang="en">ARASLT</owl:hasValue>
        <owl:onProperty rdf:resource="jc3iedm_ACTION.owl#action-event-category-code"/>
      </owl:Restriction>
    </rdfs:subClassOf>
    <rdfs:label xml:lang="en">air assault</rdfs:label>
    <rdfs:comment xml:lang="en">Mounting an assault utilising a mixture of aviation and ground transport, the principal feature of which is the insertion of combat power.</rdfs:comment>
  </owl:Class>
  <owl:Class rdf:about="jc3iedm_ACTIONExtended.owl#ACTION-EVENT_Traversing">
    <rdfs:subClassOf rdf:resource="jc3iedm_ACTION.owl#ACTION-EVENT"/>
    <rdfs:subClassOf>
      <owl:Restriction>
        <owl:hasValue xml:lang="en">TRVRSN</owl:hasValue>
        <owl:onProperty rdf:resource="jc3iedm_ACTION.owl#action-event-category-code"/>
      </owl:Restriction>
    </rdfs:subClassOf>
    <rdfs:label xml:lang="en">traversing</rdfs:label>
    <rdfs:comment xml:lang="en">Travelling over a designated route.</rdfs:comment>
  </owl:Class>
  <owl:Class rdf:about="jc3iedm_ACTIONExtended.owl#ACTION-EVENT_Providing_storage_services">
    <rdfs:subClassOf rdf:resource="jc3iedm_ACTION.owl#ACTION-EVENT"/>
    <rdfs:subClassOf>
      <owl:Restriction>
        <owl:hasValue xml:lang="en">PRVSTG</owl:hasValue>
        <owl:onProperty rdf:resource="jc3iedm_ACTION.owl#action-event-category-code"/>
      </owl:Restriction>
    </rdfs:subClassOf>
    <rdfs:label xml:lang="en">providing storage services</rdfs:label>
    <rdfs:comment xml:lang="en">Providing services for storage.</rdfs:comment>
  </owl:Class>
  <owl:Class rdf:about="jc3iedm_ACTIONExtended.owl#ACTION-EVENT_Witnessing">
    <rdfs:subClassOf rdf:resource="jc3iedm_ACTION.owl#ACTION-EVENT"/>
    <rdfs:subClassOf>
      <owl:Restriction>
        <owl:hasValue xml:lang="en">WITNSN</owl:hasValue>
        <owl:onProperty rdf:resource="jc3iedm_ACTION.owl#action-event-category-code"/>
      </owl:Restriction>
    </rdfs:subClassOf>
    <rdfs:label xml:lang="en">witnessing</rdfs:label>
    <rdfs:comment xml:lang="en">Observing an activity that may result in the need to provide evidence.</rdfs:comment>
  </owl:Class>
  <owl:Class rdf:about="jc3iedm_ACTIONExtended.owl#ACTION-EVENT_Pestilence">
    <rdfs:subClassOf rdf:resource="jc3iedm_ACTION.owl#ACTION-EVENT"/>
    <rdfs:subClassOf>
      <owl:Restriction>
        <owl:hasValue xml:lang="en">PSTLNC</owl:hasValue>
        <owl:onProperty rdf:resource="jc3iedm_ACTION.owl#action-event-category-code"/>
      </owl:Restriction>
    </rdfs:subClassOf>
    <rdfs:label xml:lang="en">pestilence</rdfs:label>
    <rdfs:comment xml:lang="en">A fatal epidemic disease, especially bubonic plague.</rdfs:comment>
  </owl:Class>
  <owl:Class rdf:about="jc3iedm_ACTIONExtended.owl#ACTION-EVENT_Resting">
    <rdfs:subClassOf rdf:resource="jc3iedm_ACTION.owl#ACTION-EVENT"/>
    <rdfs:subClassOf>
      <owl:Restriction>
        <owl:hasValue xml:lang="en">RESTNG</owl:hasValue>
        <owl:onProperty rdf:resource="jc3iedm_ACTION.owl#action-event-category-code"/>
      </owl:Restriction>
    </rdfs:subClassOf>
    <rdfs:label xml:lang="en">resting</rdfs:label>
    <rdfs:comment xml:lang="en">Observing a specified period of inactivity by an organisation that is out of contact with the enemy.</rdfs:comment>
  </owl:Class>
  <owl:Class rdf:about="jc3iedm_ACTIONExtended.owl#ACTION-EVENT_Conducting_road_service">
    <rdfs:subClassOf rdf:resource="jc3iedm_ACTION.owl#ACTION-EVENT"/>
    <rdfs:subClassOf>
      <owl:Restriction>
        <owl:hasValue xml:lang="en">CNRDSV</owl:hasValue>
        <owl:onProperty rdf:resource="jc3iedm_ACTION.owl#action-event-category-code"/>
      </owl:Restriction>
    </rdfs:subClassOf>
    <rdfs:label xml:lang="en">conducting road service</rdfs:label>
    <rdfs:comment xml:lang="en">Enabling the movement of a number of specific units.</rdfs:comment>
  </owl:Class>
  <owl:Class rdf:about="jc3iedm_ACTIONExtended.owl#ACTION-EVENT_Drive-by_shooting">
    <rdfs:subClassOf rdf:resource="jc3iedm_ACTION.owl#ACTION-EVENT"/>
    <rdfs:subClassOf>
      <owl:Restriction>
        <owl:hasValue xml:lang="en">DRVSHT</owl:hasValue>
        <owl:onProperty rdf:resource="jc3iedm_ACTION.owl#action-event-category-code"/>
      </owl:Restriction>
    </rdfs:subClassOf>
    <rdfs:label xml:lang="en">drive by shooting</rdfs:label>
    <rdfs:comment xml:lang="en">The act of firing a weapon, usually at a person, from a passing vehicle.</rdfs:comment>
  </owl:Class>
  <owl:Class rdf:about="jc3iedm_ACTIONExtended.owl#ACTION-EVENT_Diversion">
    <rdfs:subClassOf rdf:resource="jc3iedm_ACTION.owl#ACTION-EVENT"/>
    <rdfs:subClassOf>
      <owl:Restriction>
        <owl:hasValue xml:lang="en">DIVRSN</owl:hasValue>
        <owl:onProperty rdf:resource="jc3iedm_ACTION.owl#action-event-category-code"/>
      </owl:Restriction>
    </rdfs:subClassOf>
    <rdfs:label xml:lang="en">diversion</rdfs:label>
    <rdfs:comment xml:lang="en">Drawing the attention and forces of an enemy from the point of the principal operation; an attack, alarm, or feint that diverts attention.</rdfs:comment>
  </owl:Class>
  <owl:Class rdf:about="jc3iedm_ACTIONExtended.owl#ACTION-EVENT_Harassing">
    <rdfs:subClassOf rdf:resource="jc3iedm_ACTION.owl#ACTION-EVENT"/>
    <rdfs:subClassOf>
      <owl:Restriction>
        <owl:hasValue xml:lang="en">HARASS</owl:hasValue>
        <owl:onProperty rdf:resource="jc3iedm_ACTION.owl#action-event-category-code"/>
      </owl:Restriction>
    </rdfs:subClassOf>
    <rdfs:label xml:lang="en">harassing</rdfs:label>
    <rdfs:comment xml:lang="en">Conducting an operation or executing a fire plan designed to curtail movement and, by threat of losses, to lower the morale of enemy troops.</rdfs:comment>
  </owl:Class>
  <owl:Class rdf:about="jc3iedm_ACTIONExtended.owl#ACTION-EVENT_Arms_trade">
    <rdfs:subClassOf rdf:resource="jc3iedm_ACTION.owl#ACTION-EVENT"/>
    <rdfs:subClassOf>
      <owl:Restriction>
        <owl:hasValue xml:lang="en">ARMTRD</owl:hasValue>
        <owl:onProperty rdf:resource="jc3iedm_ACTION.owl#action-event-category-code"/>
      </owl:Restriction>
    </rdfs:subClassOf>
    <rdfs:label xml:lang="en">arms trade</rdfs:label>
    <rdfs:comment xml:lang="en">A happening of selling or buying of arms.</rdfs:comment>
  </owl:Class>
  <owl:Class rdf:about="jc3iedm_ACTIONExtended.owl#ACTION-EVENT_Attack__electronic">
    <rdfs:subClassOf rdf:resource="jc3iedm_ACTION.owl#ACTION-EVENT"/>
    <rdfs:subClassOf>
      <owl:Restriction>
        <owl:hasValue xml:lang="en">ATTEL</owl:hasValue>
        <owl:onProperty rdf:resource="jc3iedm_ACTION.owl#action-event-category-code"/>
      </owl:Restriction>
    </rdfs:subClassOf>
    <rdfs:label xml:lang="en">attack, electronic</rdfs:label>
    <rdfs:comment xml:lang="en">Conducting electronic warfare involving the use of electromagnetic energy, directed energy or anti-radiation weapons to attack personnel, facilities, or equipment with the intent of degrading, neutralizing, or destroying enemy combat capability and is considered a form of fires.</rdfs:comment>
  </owl:Class>
  <owl:Class rdf:about="jc3iedm_ACTIONExtended.owl#ACTION-EVENT_Clearing__obstacle">
    <rdfs:subClassOf rdf:resource="jc3iedm_ACTION.owl#ACTION-EVENT"/>
    <rdfs:subClassOf>
      <owl:Restriction>
        <owl:hasValue xml:lang="en">CLROBS</owl:hasValue>
        <owl:onProperty rdf:resource="jc3iedm_ACTION.owl#action-event-category-code"/>
      </owl:Restriction>
    </rdfs:subClassOf>
    <rdfs:label xml:lang="en">clearing, obstacle</rdfs:label>
    <rdfs:comment xml:lang="en">Eliminating or neutralizing an obstacle.</rdfs:comment>
  </owl:Class>
  <owl:Class rdf:about="jc3iedm_ACTIONExtended.owl#ACTION-EVENT_Naval_platform_flight_operations">
    <rdfs:subClassOf rdf:resource="jc3iedm_ACTION.owl#ACTION-EVENT"/>
    <rdfs:subClassOf>
      <owl:Restriction>
        <owl:hasValue xml:lang="en">NAVPLF</owl:hasValue>
        <owl:onProperty rdf:resource="jc3iedm_ACTION.owl#action-event-category-code"/>
      </owl:Restriction>
    </rdfs:subClassOf>
    <rdfs:label xml:lang="en">naval platform flight operations</rdfs:label>
    <rdfs:comment xml:lang="en">Aircraft launch or recovery by a naval platform.</rdfs:comment>
  </owl:Class>
  <owl:Class rdf:about="jc3iedm_ACTIONExtended.owl#ACTION-EVENT_Border_crossing__not-planned">
    <rdfs:subClassOf rdf:resource="jc3iedm_ACTION.owl#ACTION-EVENT"/>
    <rdfs:subClassOf>
      <owl:Restriction>
        <owl:hasValue xml:lang="en">BCNTPL</owl:hasValue>
        <owl:onProperty rdf:resource="jc3iedm_ACTION.owl#action-event-category-code"/>
      </owl:Restriction>
    </rdfs:subClassOf>
    <rdfs:label xml:lang="en">border crossing, not planned</rdfs:label>
    <rdfs:comment xml:lang="en">A border crossing that is unplanned.</rdfs:comment>
  </owl:Class>
  <owl:Class rdf:about="jc3iedm_ACTIONExtended.owl#ACTION-EVENT_Arson">
    <rdfs:subClassOf rdf:resource="jc3iedm_ACTION.owl#ACTION-EVENT"/>
    <rdfs:subClassOf>
      <owl:Restriction>
        <owl:hasValue xml:lang="en">ARSON</owl:hasValue>
        <owl:onProperty rdf:resource="jc3iedm_ACTION.owl#action-event-category-code"/>
      </owl:Restriction>
    </rdfs:subClassOf>
    <rdfs:label xml:lang="en">arson</rdfs:label>
    <rdfs:comment xml:lang="en">The crime of maliciously setting fire to the property of another or of burning one’s own property for an improper purpose, as to collect insurance.</rdfs:comment>
  </owl:Class>
  <owl:Class rdf:about="jc3iedm_ACTIONExtended.owl#ACTION-EVENT_Threaten">
    <rdfs:subClassOf rdf:resource="jc3iedm_ACTION.owl#ACTION-EVENT"/>
    <rdfs:subClassOf>
      <owl:Restriction>
        <owl:hasValue xml:lang="en">THREAT</owl:hasValue>
        <owl:onProperty rdf:resource="jc3iedm_ACTION.owl#action-event-category-code"/>
      </owl:Restriction>
    </rdfs:subClassOf>
    <rdfs:label xml:lang="en">threaten</rdfs:label>
    <rdfs:comment xml:lang="en">Menacing an armed force by manoeuvre or action.</rdfs:comment>
  </owl:Class>
  <owl:Class rdf:about="jc3iedm_ACTIONExtended.owl#REQUEST_Association">
    <rdfs:subClassOf rdf:resource="jc3iedm_ACTION.owl#REQUEST"/>
    <rdfs:subClassOf>
      <owl:Restriction>
        <owl:hasValue xml:lang="en">ASSOC</owl:hasValue>
        <owl:onProperty rdf:resource="jc3iedm_ACTION.owl#request-category-code"/>
      </owl:Restriction>
    </rdfs:subClassOf>
    <rdfs:label xml:lang="en">association</rdfs:label>
    <rdfs:comment xml:lang="en">To discover the relation between two ACTION-OBJECTIVEs (OBJECT-ITEMs) by any means.</rdfs:comment>
  </owl:Class>
  <owl:Class rdf:about="jc3iedm_ACTIONExtended.owl#ACTION-EVENT_Conducting_rearward_passage_of_lines">
    <rdfs:subClassOf rdf:resource="jc3iedm_ACTION.owl#ACTION-EVENT"/>
    <rdfs:subClassOf>
      <owl:Restriction>
        <owl:hasValue xml:lang="en">CNRWPS</owl:hasValue>
        <owl:onProperty rdf:resource="jc3iedm_ACTION.owl#action-event-category-code"/>
      </owl:Restriction>
    </rdfs:subClassOf>
    <rdfs:label xml:lang="en">conducting rearward passage of lines</rdfs:label>
    <rdfs:comment xml:lang="en">Moving a force through the defensive positions of another force behind it in order to break contact with the enemy.</rdfs:comment>
  </owl:Class>
  <owl:Class rdf:about="jc3iedm_ACTIONExtended.owl#CHEMICAL-BIOLOGICAL-EVENT_Chemical_biological_facility_event">
    <rdfs:subClassOf rdf:resource="jc3iedm_ACTION.owl#CHEMICAL-BIOLOGICAL-EVENT"/>
    <rdfs:subClassOf>
      <owl:Restriction>
        <owl:hasValue xml:lang="en">CBFAC</owl:hasValue>
        <owl:onProperty rdf:resource="jc3iedm_ACTION.owl#chemical-biological-event-category-code"/>
      </owl:Restriction>
    </rdfs:subClassOf>
    <rdfs:label xml:lang="en">chemical/biological facility event</rdfs:label>
    <rdfs:comment xml:lang="en">An event that involves viable agent released to the atmosphere following a strike against a facility containing chemical warfare agent(s) and/or biological warfare agent(s).</rdfs:comment>
  </owl:Class>
  <owl:Class rdf:about="jc3iedm_ACTIONExtended.owl#ACTION-EVENT_Assassination">
    <rdfs:subClassOf rdf:resource="jc3iedm_ACTION.owl#ACTION-EVENT"/>
    <rdfs:subClassOf>
      <owl:Restriction>
        <owl:hasValue xml:lang="en">ASSNTN</owl:hasValue>
        <owl:onProperty rdf:resource="jc3iedm_ACTION.owl#action-event-category-code"/>
      </owl:Restriction>
    </rdfs:subClassOf>
    <rdfs:label xml:lang="en">assassination</rdfs:label>
    <rdfs:comment xml:lang="en">Murder of a prominent person.</rdfs:comment>
  </owl:Class>
  <owl:Class rdf:about="jc3iedm_ACTIONExtended.owl#ACTION-EVENT_Hijacking__boat">
    <rdfs:subClassOf rdf:resource="jc3iedm_ACTION.owl#ACTION-EVENT"/>
    <rdfs:subClassOf>
      <owl:Restriction>
        <owl:hasValue xml:lang="en">HJCKBT</owl:hasValue>
        <owl:onProperty rdf:resource="jc3iedm_ACTION.owl#action-event-category-code"/>
      </owl:Restriction>
    </rdfs:subClassOf>
    <rdfs:label xml:lang="en">hijacking, boat</rdfs:label>
    <rdfs:comment xml:lang="en">Seizure of a boat or ship in order to go somewhere other than the scheduled destination.</rdfs:comment>
  </owl:Class>
  <owl:Class rdf:about="jc3iedm_ACTIONExtended.owl#ACTION-EVENT_Retire">
    <rdfs:subClassOf rdf:resource="jc3iedm_ACTION.owl#ACTION-EVENT"/>
    <rdfs:subClassOf>
      <owl:Restriction>
        <owl:hasValue xml:lang="en">RETIRE</owl:hasValue>
        <owl:onProperty rdf:resource="jc3iedm_ACTION.owl#action-event-category-code"/>
      </owl:Restriction>
    </rdfs:subClassOf>
    <rdfs:label xml:lang="en">retire</rdfs:label>
    <rdfs:comment xml:lang="en">Moving a force out of contact with the enemy with the expectation of no further significant contact.</rdfs:comment>
  </owl:Class>
  <owl:Class rdf:about="jc3iedm_ACTIONExtended.owl#ACTION-EVENT_Ambush">
    <rdfs:subClassOf rdf:resource="jc3iedm_ACTION.owl#ACTION-EVENT"/>
    <rdfs:subClassOf>
      <owl:Restriction>
        <owl:hasValue xml:lang="en">AMBUSH</owl:hasValue>
        <owl:onProperty rdf:resource="jc3iedm_ACTION.owl#action-event-category-code"/>
      </owl:Restriction>
    </rdfs:subClassOf>
    <rdfs:label xml:lang="en">ambush</rdfs:label>
    <rdfs:comment xml:lang="en">A surprise attack by fire or other destructive means from concealed positions on a moving or temporarily halted force or group of personnel.</rdfs:comment>
  </owl:Class>
  <owl:Class rdf:about="jc3iedm_ACTIONExtended.owl#ACTION-EVENT_Aircraft_landing">
    <rdfs:subClassOf rdf:resource="jc3iedm_ACTION.owl#ACTION-EVENT"/>
    <rdfs:subClassOf>
      <owl:Restriction>
        <owl:hasValue xml:lang="en">AIRLND</owl:hasValue>
        <owl:onProperty rdf:resource="jc3iedm_ACTION.owl#action-event-category-code"/>
      </owl:Restriction>
    </rdfs:subClassOf>
    <rdfs:label xml:lang="en">aircraft landing</rdfs:label>
    <rdfs:comment xml:lang="en">The action of approaching and alighting on the ground or some other surface after a flight.</rdfs:comment>
  </owl:Class>
  <owl:Class rdf:about="jc3iedm_ACTIONExtended.owl#ACTION-EVENT_Security_compromise">
    <rdfs:subClassOf rdf:resource="jc3iedm_ACTION.owl#ACTION-EVENT"/>
    <rdfs:subClassOf>
      <owl:Restriction>
        <owl:hasValue xml:lang="en">SECCMP</owl:hasValue>
        <owl:onProperty rdf:resource="jc3iedm_ACTION.owl#action-event-category-code"/>
      </owl:Restriction>
    </rdfs:subClassOf>
    <rdfs:label xml:lang="en">security compromise</rdfs:label>
    <rdfs:comment xml:lang="en">A release of information to someone unauthorised.</rdfs:comment>
  </owl:Class>
  <owl:Class rdf:about="jc3iedm_ACTIONExtended.owl#ACTION-EVENT_Providing_infrastructure">
    <rdfs:subClassOf rdf:resource="jc3iedm_ACTION.owl#ACTION-EVENT"/>
    <rdfs:subClassOf>
      <owl:Restriction>
        <owl:hasValue xml:lang="en">PRVINF</owl:hasValue>
        <owl:onProperty rdf:resource="jc3iedm_ACTION.owl#action-event-category-code"/>
      </owl:Restriction>
    </rdfs:subClassOf>
    <rdfs:label xml:lang="en">providing infrastructure</rdfs:label>
    <rdfs:comment xml:lang="en">Providing basic facilities such as roads, bridges, and sewers.</rdfs:comment>
  </owl:Class>
  <owl:Class rdf:about="jc3iedm_ACTIONExtended.owl#ACTION-EVENT_Airspace_violation">
    <rdfs:subClassOf rdf:resource="jc3iedm_ACTION.owl#ACTION-EVENT"/>
    <rdfs:subClassOf>
      <owl:Restriction>
        <owl:hasValue xml:lang="en">AIRVIO</owl:hasValue>
        <owl:onProperty rdf:resource="jc3iedm_ACTION.owl#action-event-category-code"/>
      </owl:Restriction>
    </rdfs:subClassOf>
    <rdfs:label xml:lang="en">airspace violation</rdfs:label>
    <rdfs:comment xml:lang="en">The invasion of the declared own airspace by an aircraft.</rdfs:comment>
  </owl:Class>
  <owl:Class rdf:about="jc3iedm_ACTIONExtended.owl#ACTION-EVENT_Coup_d’état">
    <rdfs:subClassOf rdf:resource="jc3iedm_ACTION.owl#ACTION-EVENT"/>
    <rdfs:subClassOf>
      <owl:Restriction>
        <owl:hasValue xml:lang="en">COUPDE</owl:hasValue>
        <owl:onProperty rdf:resource="jc3iedm_ACTION.owl#action-event-category-code"/>
      </owl:Restriction>
    </rdfs:subClassOf>
    <rdfs:label xml:lang="en">coup d’état</rdfs:label>
    <rdfs:comment xml:lang="en">A violent or illegal seizure of power.</rdfs:comment>
  </owl:Class>
  <owl:Class rdf:about="jc3iedm_ACTIONExtended.owl#ACTION-EVENT_Demonstration">
    <rdfs:subClassOf rdf:resource="jc3iedm_ACTION.owl#ACTION-EVENT"/>
    <rdfs:subClassOf>
      <owl:Restriction>
        <owl:hasValue xml:lang="en">DMNSTR</owl:hasValue>
        <owl:onProperty rdf:resource="jc3iedm_ACTION.owl#action-event-category-code"/>
      </owl:Restriction>
    </rdfs:subClassOf>
    <rdfs:label xml:lang="en">demonstration</rdfs:label>
    <rdfs:comment xml:lang="en">Conducting an offensive operation that is either an attack or a show of force on a front where a decision is not sought, made with the aim of deceiving the enemy. It is similar to a feint with the exception that no contact with the enemy is sought. In OOTW, an operation by military forces in sight of an actual or potential enemy to show military capabilities.</rdfs:comment>
  </owl:Class>
  <owl:Class rdf:about="jc3iedm_ACTIONExtended.owl#ACTION-EVENT_Drug_transportation">
    <rdfs:subClassOf rdf:resource="jc3iedm_ACTION.owl#ACTION-EVENT"/>
    <rdfs:subClassOf>
      <owl:Restriction>
        <owl:hasValue xml:lang="en">DRGTRN</owl:hasValue>
        <owl:onProperty rdf:resource="jc3iedm_ACTION.owl#action-event-category-code"/>
      </owl:Restriction>
    </rdfs:subClassOf>
    <rdfs:label xml:lang="en">drug transportation</rdfs:label>
    <rdfs:comment xml:lang="en">An action to transport drugs.</rdfs:comment>
  </owl:Class>
  <owl:Class rdf:about="jc3iedm_ACTIONExtended.owl#ACTION-EVENT_Communications_interception">
    <rdfs:subClassOf rdf:resource="jc3iedm_ACTION.owl#ACTION-EVENT"/>
    <rdfs:subClassOf>
      <owl:Restriction>
        <owl:hasValue xml:lang="en">COMINT</owl:hasValue>
        <owl:onProperty rdf:resource="jc3iedm_ACTION.owl#action-event-category-code"/>
      </owl:Restriction>
    </rdfs:subClassOf>
    <rdfs:label xml:lang="en">communications interception</rdfs:label>
    <rdfs:comment xml:lang="en">Capturing electromagnetic communications signals.</rdfs:comment>
  </owl:Class>
  <owl:Class rdf:about="jc3iedm_ACTIONExtended.owl#ACTION-EVENT_Attempted_rape">
    <rdfs:subClassOf rdf:resource="jc3iedm_ACTION.owl#ACTION-EVENT"/>
    <rdfs:subClassOf>
      <owl:Restriction>
        <owl:hasValue xml:lang="en">ATRAPE</owl:hasValue>
        <owl:onProperty rdf:resource="jc3iedm_ACTION.owl#action-event-category-code"/>
      </owl:Restriction>
    </rdfs:subClassOf>
    <rdfs:label xml:lang="en">attempted rape</rdfs:label>
    <rdfs:comment xml:lang="en">The attempted act of forcing another person to submit to sexual intercourse.</rdfs:comment>
  </owl:Class>
  <owl:Class rdf:about="jc3iedm_ACTIONExtended.owl#ACTION-EVENT_Volcanic_eruption">
    <rdfs:subClassOf rdf:resource="jc3iedm_ACTION.owl#ACTION-EVENT"/>
    <rdfs:subClassOf>
      <owl:Restriction>
        <owl:hasValue xml:lang="en">VOLCAN</owl:hasValue>
        <owl:onProperty rdf:resource="jc3iedm_ACTION.owl#action-event-category-code"/>
      </owl:Restriction>
    </rdfs:subClassOf>
    <rdfs:label xml:lang="en">volcanic eruption</rdfs:label>
    <rdfs:comment xml:lang="en">The release of lava or steam by a volcano.</rdfs:comment>
  </owl:Class>
  <owl:Class rdf:about="jc3iedm_ACTIONExtended.owl#ACTION-EVENT_Publishing_media_documentary">
    <rdfs:subClassOf rdf:resource="jc3iedm_ACTION.owl#ACTION-EVENT"/>
    <rdfs:subClassOf>
      <owl:Restriction>
        <owl:hasValue xml:lang="en">PUBMDD</owl:hasValue>
        <owl:onProperty rdf:resource="jc3iedm_ACTION.owl#action-event-category-code"/>
      </owl:Restriction>
    </rdfs:subClassOf>
    <rdfs:label xml:lang="en">publishing media documentary</rdfs:label>
    <rdfs:comment xml:lang="en">Making generally known any document published on a media that provides a factual record or report.</rdfs:comment>
  </owl:Class>
  <owl:Class rdf:about="jc3iedm_ACTIONExtended.owl#ACTION-EVENT_Counter_attack">
    <rdfs:subClassOf rdf:resource="jc3iedm_ACTION.owl#ACTION-EVENT"/>
    <rdfs:subClassOf>
      <owl:Restriction>
        <owl:hasValue xml:lang="en">CTRATK</owl:hasValue>
        <owl:onProperty rdf:resource="jc3iedm_ACTION.owl#action-event-category-code"/>
      </owl:Restriction>
    </rdfs:subClassOf>
    <rdfs:label xml:lang="en">counter attack</rdfs:label>
    <rdfs:comment xml:lang="en">Mounting an offensive operation in which an attack by a part or all of a defending force is made against an enemy attacking force, for such specific purposes as regaining ground lost, cutting off or destroying lead enemy units, and with the general objective of regaining the initiative and denying the enemy the attainment of his goal or purpose in attacking.</rdfs:comment>
  </owl:Class>
  <owl:Class rdf:about="jc3iedm_ACTIONExtended.owl#ACTION-TASK_Template">
    <rdfs:subClassOf rdf:resource="jc3iedm_ACTION.owl#ACTION-TASK"/>
    <rdfs:subClassOf>
      <owl:Restriction>
        <owl:hasValue xml:lang="en">TEM</owl:hasValue>
        <owl:onProperty rdf:resource="jc3iedm_ACTION.owl#action-task-category-code"/>
      </owl:Restriction>
    </rdfs:subClassOf>
    <rdfs:label xml:lang="en">template</rdfs:label>
    <rdfs:comment xml:lang="en">An ACTION-TASK that serves as a reference in planning.</rdfs:comment>
  </owl:Class>
  <owl:Class rdf:about="jc3iedm_ACTIONExtended.owl#ACTION-EVENT_Serving_as_a_reserve">
    <rdfs:subClassOf rdf:resource="jc3iedm_ACTION.owl#ACTION-EVENT"/>
    <rdfs:subClassOf>
      <owl:Restriction>
        <owl:hasValue xml:lang="en">SRVRSF</owl:hasValue>
        <owl:onProperty rdf:resource="jc3iedm_ACTION.owl#action-event-category-code"/>
      </owl:Restriction>
    </rdfs:subClassOf>
    <rdfs:label xml:lang="en">serving as a reserve</rdfs:label>
    <rdfs:comment xml:lang="en">Operating as a force that may be committed into combat only on the order of the commander of the organisation who so designated the reserve force.</rdfs:comment>
  </owl:Class>
  <owl:Class rdf:about="jc3iedm_ACTIONExtended.owl#ACTION-EVENT_Indiscriminate_shooting">
    <rdfs:subClassOf rdf:resource="jc3iedm_ACTION.owl#ACTION-EVENT"/>
    <rdfs:subClassOf>
      <owl:Restriction>
        <owl:hasValue xml:lang="en">INDSHO</owl:hasValue>
        <owl:onProperty rdf:resource="jc3iedm_ACTION.owl#action-event-category-code"/>
      </owl:Restriction>
    </rdfs:subClassOf>
    <rdfs:label xml:lang="en">indiscriminate shooting</rdfs:label>
    <rdfs:comment xml:lang="en">Firing without a specific objective and without making distinction.</rdfs:comment>
  </owl:Class>
  <owl:Class rdf:about="jc3iedm_ACTIONExtended.owl#ACTION-EVENT_Attack__supporting">
    <rdfs:subClassOf rdf:resource="jc3iedm_ACTION.owl#ACTION-EVENT"/>
    <rdfs:subClassOf>
      <owl:Restriction>
        <owl:hasValue xml:lang="en">ATTSPT</owl:hasValue>
        <owl:onProperty rdf:resource="jc3iedm_ACTION.owl#action-event-category-code"/>
      </owl:Restriction>
    </rdfs:subClassOf>
    <rdfs:label xml:lang="en">attack, supporting</rdfs:label>
    <rdfs:comment xml:lang="en">Conducting an offensive operation carried out in conjunction with a main attack and designed to achieve one or more of the following: a. deceive the enemy; b. destroy or pin down enemy forces which could interfere with the main attack; c. control ground whose occupation by the enemy will hinder the main attack; or d. force the enemy to commit reserves prematurely or in an indecisive area.</rdfs:comment>
  </owl:Class>
  <owl:Class rdf:about="jc3iedm_ACTIONExtended.owl#ACTION-EVENT_Aerial_engagement">
    <rdfs:subClassOf rdf:resource="jc3iedm_ACTION.owl#ACTION-EVENT"/>
    <rdfs:subClassOf>
      <owl:Restriction>
        <owl:hasValue xml:lang="en">AERENG</owl:hasValue>
        <owl:onProperty rdf:resource="jc3iedm_ACTION.owl#action-event-category-code"/>
      </owl:Restriction>
    </rdfs:subClassOf>
    <rdfs:label xml:lang="en">aerial engagement</rdfs:label>
    <rdfs:comment xml:lang="en">The occurrence of a hostile encounter between military aircraft.</rdfs:comment>
  </owl:Class>
  <owl:Class rdf:about="jc3iedm_ACTIONExtended.owl#ACTION-EVENT_Interdiction">
    <rdfs:subClassOf rdf:resource="jc3iedm_ACTION.owl#ACTION-EVENT"/>
    <rdfs:subClassOf>
      <owl:Restriction>
        <owl:hasValue xml:lang="en">INTDCT</owl:hasValue>
        <owl:onProperty rdf:resource="jc3iedm_ACTION.owl#action-event-category-code"/>
      </owl:Restriction>
    </rdfs:subClassOf>
    <rdfs:label xml:lang="en">interdiction</rdfs:label>
    <rdfs:comment xml:lang="en">Diverting, disrupting, delaying, or destroying the enemy’s surface military potential before it can be used effectively against friendly forces.</rdfs:comment>
  </owl:Class>
  <owl:Class rdf:about="jc3iedm_ACTIONExtended.owl#REQUEST_Location">
    <rdfs:subClassOf rdf:resource="jc3iedm_ACTION.owl#REQUEST"/>
    <rdfs:subClassOf>
      <owl:Restriction>
        <owl:hasValue xml:lang="en">LOCATN</owl:hasValue>
        <owl:onProperty rdf:resource="jc3iedm_ACTION.owl#request-category-code"/>
      </owl:Restriction>
    </rdfs:subClassOf>
    <rdfs:label xml:lang="en">location</rdfs:label>
    <rdfs:comment xml:lang="en">To discover the location of an ACTION-OBJECTIVE (OBJECT-ITEM) by any means.</rdfs:comment>
  </owl:Class>
  <owl:Class rdf:about="jc3iedm_ACTIONExtended.owl#ACTION-EVENT_Carrier_recovery">
    <rdfs:subClassOf rdf:resource="jc3iedm_ACTION.owl#ACTION-EVENT"/>
    <rdfs:subClassOf>
      <owl:Restriction>
        <owl:hasValue xml:lang="en">CARREC</owl:hasValue>
        <owl:onProperty rdf:resource="jc3iedm_ACTION.owl#action-event-category-code"/>
      </owl:Restriction>
    </rdfs:subClassOf>
    <rdfs:label xml:lang="en">carrier recovery</rdfs:label>
    <rdfs:comment xml:lang="en">Aircraft recovery by a naval platform.</rdfs:comment>
  </owl:Class>
  <owl:Class rdf:about="jc3iedm_ACTIONExtended.owl#ACTION-EVENT_Engaging">
    <rdfs:subClassOf rdf:resource="jc3iedm_ACTION.owl#ACTION-EVENT"/>
    <rdfs:subClassOf>
      <owl:Restriction>
        <owl:hasValue xml:lang="en">ENGAGE</owl:hasValue>
        <owl:onProperty rdf:resource="jc3iedm_ACTION.owl#action-event-category-code"/>
      </owl:Restriction>
    </rdfs:subClassOf>
    <rdfs:label xml:lang="en">engaging</rdfs:label>
    <rdfs:comment xml:lang="en">Bringing the enemy under fire.</rdfs:comment>
  </owl:Class>
  <owl:Class rdf:about="jc3iedm_ACTIONExtended.owl#ACTION-EVENT_Serving_as_an_advance_guard">
    <rdfs:subClassOf rdf:resource="jc3iedm_ACTION.owl#ACTION-EVENT"/>
    <rdfs:subClassOf>
      <owl:Restriction>
        <owl:hasValue xml:lang="en">SRVADV</owl:hasValue>
        <owl:onProperty rdf:resource="jc3iedm_ACTION.owl#action-event-category-code"/>
      </owl:Restriction>
    </rdfs:subClassOf>
    <rdfs:label xml:lang="en">serving as an advance guard</rdfs:label>
    <rdfs:comment xml:lang="en">Operating as a security element whose primary task is to move ahead of the main body and protect the main force by fighting to gain time, whilst also observing and reporting information.</rdfs:comment>
  </owl:Class>
  <owl:Class rdf:about="jc3iedm_ACTIONExtended.owl#ACTION-EVENT_Abdication">
    <rdfs:subClassOf rdf:resource="jc3iedm_ACTION.owl#ACTION-EVENT"/>
    <rdfs:subClassOf>
      <owl:Restriction>
        <owl:hasValue xml:lang="en">ABDICA</owl:hasValue>
        <owl:onProperty rdf:resource="jc3iedm_ACTION.owl#action-event-category-code"/>
      </owl:Restriction>
    </rdfs:subClassOf>
    <rdfs:label xml:lang="en">abdication</rdfs:label>
    <rdfs:comment xml:lang="en">The renouncement by a person of his official functions.</rdfs:comment>
  </owl:Class>
  <owl:Class rdf:about="jc3iedm_ACTIONExtended.owl#ACTION-EVENT_Vandalism_Rape_Loot_Ransack_Plunder_Sack">
    <rdfs:subClassOf rdf:resource="jc3iedm_ACTION.owl#ACTION-EVENT"/>
    <rdfs:subClassOf>
      <owl:Restriction>
        <owl:hasValue xml:lang="en">VANDAL</owl:hasValue>
        <owl:onProperty rdf:resource="jc3iedm_ACTION.owl#action-event-category-code"/>
      </owl:Restriction>
    </rdfs:subClassOf>
    <rdfs:label xml:lang="en">vandalism/rape/loot/ransack/plunder/sack</rdfs:label>
    <rdfs:comment xml:lang="en">An act of vandalism, raping, looting, ransacking or plundering against an individual or property.</rdfs:comment>
  </owl:Class>
  <owl:Class rdf:about="jc3iedm_ACTIONExtended.owl#ACTION-EVENT_Suicide">
    <rdfs:subClassOf rdf:resource="jc3iedm_ACTION.owl#ACTION-EVENT"/>
    <rdfs:subClassOf>
      <owl:Restriction>
        <owl:hasValue xml:lang="en">SUICDE</owl:hasValue>
        <owl:onProperty rdf:resource="jc3iedm_ACTION.owl#action-event-category-code"/>
      </owl:Restriction>
    </rdfs:subClassOf>
    <rdfs:label xml:lang="en">suicide</rdfs:label>
    <rdfs:comment xml:lang="en">The action of killing oneself intentionally.</rdfs:comment>
  </owl:Class>
  <owl:Class rdf:about="jc3iedm_ACTIONExtended.owl#ACTION-EVENT_Attack__hasty">
    <rdfs:subClassOf rdf:resource="jc3iedm_ACTION.owl#ACTION-EVENT"/>
    <rdfs:subClassOf>
      <owl:Restriction>
        <owl:hasValue xml:lang="en">HASTY</owl:hasValue>
        <owl:onProperty rdf:resource="jc3iedm_ACTION.owl#action-event-category-code"/>
      </owl:Restriction>
    </rdfs:subClassOf>
    <rdfs:label xml:lang="en">attack, hasty</rdfs:label>
    <rdfs:comment xml:lang="en">In land operations, an attack in which preparation time is traded for speed in order to exploit an opportunity.</rdfs:comment>
  </owl:Class>
  <owl:Class rdf:about="jc3iedm_ACTIONExtended.owl#ACTION-EVENT_Aircraft_loss">
    <rdfs:subClassOf rdf:resource="jc3iedm_ACTION.owl#ACTION-EVENT"/>
    <rdfs:subClassOf>
      <owl:Restriction>
        <owl:hasValue xml:lang="en">ACRLOS</owl:hasValue>
        <owl:onProperty rdf:resource="jc3iedm_ACTION.owl#action-event-category-code"/>
      </owl:Restriction>
    </rdfs:subClassOf>
    <rdfs:label xml:lang="en">aircraft loss</rdfs:label>
    <rdfs:comment xml:lang="en">The unforeseen loss of an aircraft (and personnel), other than crash.</rdfs:comment>
  </owl:Class>
  <owl:Class rdf:about="jc3iedm_ACTIONExtended.owl#REQUEST_Status">
    <rdfs:subClassOf rdf:resource="jc3iedm_ACTION.owl#REQUEST"/>
    <rdfs:subClassOf>
      <owl:Restriction>
        <owl:hasValue xml:lang="en">STATUS</owl:hasValue>
        <owl:onProperty rdf:resource="jc3iedm_ACTION.owl#request-category-code"/>
      </owl:Restriction>
    </rdfs:subClassOf>
    <rdfs:label xml:lang="en">status</rdfs:label>
    <rdfs:comment xml:lang="en">To recognise the status of an ACTION-OBJECTIVE (OBJECT-ITEM) by any means.</rdfs:comment>
  </owl:Class>
  <owl:Class rdf:about="jc3iedm_ACTIONExtended.owl#ACTION-EVENT_Border_crossing__forced">
    <rdfs:subClassOf rdf:resource="jc3iedm_ACTION.owl#ACTION-EVENT"/>
    <rdfs:subClassOf>
      <owl:Restriction>
        <owl:hasValue xml:lang="en">BCFRCD</owl:hasValue>
        <owl:onProperty rdf:resource="jc3iedm_ACTION.owl#action-event-category-code"/>
      </owl:Restriction>
    </rdfs:subClassOf>
    <rdfs:label xml:lang="en">border crossing, forced</rdfs:label>
    <rdfs:comment xml:lang="en">A border crossing that is conducted under pressure.</rdfs:comment>
  </owl:Class>
  <owl:Class rdf:about="jc3iedm_ACTIONExtended.owl#ACTION-EVENT_Providing_repair_services">
    <rdfs:subClassOf rdf:resource="jc3iedm_ACTION.owl#ACTION-EVENT"/>
    <rdfs:subClassOf>
      <owl:Restriction>
        <owl:hasValue xml:lang="en">PRVRPR</owl:hasValue>
        <owl:onProperty rdf:resource="jc3iedm_ACTION.owl#action-event-category-code"/>
      </owl:Restriction>
    </rdfs:subClassOf>
    <rdfs:label xml:lang="en">providing repair services</rdfs:label>
    <rdfs:comment xml:lang="en">Providing labour and materiel to restore objects to sound condition.</rdfs:comment>
  </owl:Class>
  <owl:Class rdf:about="jc3iedm_ACTIONExtended.owl#ACTION-EVENT_Enveloping">
    <rdfs:subClassOf rdf:resource="jc3iedm_ACTION.owl#ACTION-EVENT"/>
    <rdfs:subClassOf>
      <owl:Restriction>
        <owl:hasValue xml:lang="en">ENVLPN</owl:hasValue>
        <owl:onProperty rdf:resource="jc3iedm_ACTION.owl#action-event-category-code"/>
      </owl:Restriction>
    </rdfs:subClassOf>
    <rdfs:label xml:lang="en">enveloping</rdfs:label>
    <rdfs:comment xml:lang="en">Manoeuvring by the main attacking force to pass around or over the enemy’s principal defensive positions with the aim of securing objectives to the enemy’s rear.</rdfs:comment>
  </owl:Class>
  <owl:Class rdf:about="jc3iedm_ACTIONExtended.owl#ACTION-EVENT_Hijacking__not_otherwise_specified">
    <rdfs:subClassOf rdf:resource="jc3iedm_ACTION.owl#ACTION-EVENT"/>
    <rdfs:subClassOf>
      <owl:Restriction>
        <owl:hasValue xml:lang="en">HIJACK</owl:hasValue>
        <owl:onProperty rdf:resource="jc3iedm_ACTION.owl#action-event-category-code"/>
      </owl:Restriction>
    </rdfs:subClassOf>
    <rdfs:label xml:lang="en">hijacking, not otherwise specified</rdfs:label>
    <rdfs:comment xml:lang="en">Seizure of a vehicle in order to go somewhere other than the scheduled destination.</rdfs:comment>
  </owl:Class>
  <owl:Class rdf:about="jc3iedm_ACTIONExtended.owl#ACTION-EVENT_Communications_restoration">
    <rdfs:subClassOf rdf:resource="jc3iedm_ACTION.owl#ACTION-EVENT"/>
    <rdfs:subClassOf>
      <owl:Restriction>
        <owl:hasValue xml:lang="en">COMRES</owl:hasValue>
        <owl:onProperty rdf:resource="jc3iedm_ACTION.owl#action-event-category-code"/>
      </owl:Restriction>
    </rdfs:subClassOf>
    <rdfs:label xml:lang="en">communications restoration</rdfs:label>
    <rdfs:comment xml:lang="en">The reestablishment of the ability to communicate.</rdfs:comment>
  </owl:Class>
  <owl:Class rdf:about="jc3iedm_ACTIONExtended.owl#ACTION-EVENT_Serving_as_a_bridgehead_force">
    <rdfs:subClassOf rdf:resource="jc3iedm_ACTION.owl#ACTION-EVENT"/>
    <rdfs:subClassOf>
      <owl:Restriction>
        <owl:hasValue xml:lang="en">SRVBRD</owl:hasValue>
        <owl:onProperty rdf:resource="jc3iedm_ACTION.owl#action-event-category-code"/>
      </owl:Restriction>
    </rdfs:subClassOf>
    <rdfs:label xml:lang="en">serving as a bridgehead force</rdfs:label>
    <rdfs:comment xml:lang="en">Operating as a force that seizes or controls ground in order to permit the continuous embarkation, landing or crossing of troops or materiel and to provide manoeuvre space during a water obstacle crossing.</rdfs:comment>
  </owl:Class>
  <owl:Class rdf:about="jc3iedm_ACTIONExtended.owl#ACTION-TASK_Order">
    <rdfs:subClassOf rdf:resource="jc3iedm_ACTION.owl#ACTION-TASK"/>
    <rdfs:subClassOf>
      <owl:Restriction>
        <owl:hasValue xml:lang="en">ORD</owl:hasValue>
        <owl:onProperty rdf:resource="jc3iedm_ACTION.owl#action-task-category-code"/>
      </owl:Restriction>
    </rdfs:subClassOf>
    <rdfs:label xml:lang="en">order</rdfs:label>
    <rdfs:comment xml:lang="en">An ACTION-TASK that is directed to be executed.</rdfs:comment>
  </owl:Class>
  <owl:Class rdf:about="jc3iedm_ACTIONExtended.owl#ACTION-EVENT_Flood">
    <rdfs:subClassOf rdf:resource="jc3iedm_ACTION.owl#ACTION-EVENT"/>
    <rdfs:subClassOf>
      <owl:Restriction>
        <owl:hasValue xml:lang="en">FLOOD</owl:hasValue>
        <owl:onProperty rdf:resource="jc3iedm_ACTION.owl#action-event-category-code"/>
      </owl:Restriction>
    </rdfs:subClassOf>
    <rdfs:label xml:lang="en">flood</rdfs:label>
    <rdfs:comment xml:lang="en">The overflowing of a body of water onto dry land.</rdfs:comment>
  </owl:Class>
  <owl:Class rdf:about="jc3iedm_ACTIONExtended.owl#ACTION-EVENT_Publishing_press_release">
    <rdfs:subClassOf rdf:resource="jc3iedm_ACTION.owl#ACTION-EVENT"/>
    <rdfs:subClassOf>
      <owl:Restriction>
        <owl:hasValue xml:lang="en">PUBPRS</owl:hasValue>
        <owl:onProperty rdf:resource="jc3iedm_ACTION.owl#action-event-category-code"/>
      </owl:Restriction>
    </rdfs:subClassOf>
    <rdfs:label xml:lang="en">publishing press release</rdfs:label>
    <rdfs:comment xml:lang="en">Making generally known an official statement issued to media for information.</rdfs:comment>
  </owl:Class>
  <owl:Class rdf:about="jc3iedm_ACTIONExtended.owl#ACTION-EVENT_Looting">
    <rdfs:subClassOf rdf:resource="jc3iedm_ACTION.owl#ACTION-EVENT"/>
    <rdfs:subClassOf>
      <owl:Restriction>
        <owl:hasValue xml:lang="en">LOOTNG</owl:hasValue>
        <owl:onProperty rdf:resource="jc3iedm_ACTION.owl#action-event-category-code"/>
      </owl:Restriction>
    </rdfs:subClassOf>
    <rdfs:label xml:lang="en">looting</rdfs:label>
    <rdfs:comment xml:lang="en">Act to take private property from an enemy in war or stolen by thieves.</rdfs:comment>
  </owl:Class>
  <owl:Class rdf:about="jc3iedm_ACTIONExtended.owl#ACTION-EVENT_Protection__electronic">
    <rdfs:subClassOf rdf:resource="jc3iedm_ACTION.owl#ACTION-EVENT"/>
    <rdfs:subClassOf>
      <owl:Restriction>
        <owl:hasValue xml:lang="en">PROTEL</owl:hasValue>
        <owl:onProperty rdf:resource="jc3iedm_ACTION.owl#action-event-category-code"/>
      </owl:Restriction>
    </rdfs:subClassOf>
    <rdfs:label xml:lang="en">protection, electronic</rdfs:label>
    <rdfs:comment xml:lang="en">That division of electronic warfare involving actions taken to ensure effective friendly use of the electromagnetic spectrum despite the enemy's use of electromagnetic energy.</rdfs:comment>
  </owl:Class>
  <owl:Class rdf:about="jc3iedm_ACTIONExtended.owl#ACTION-EVENT_Providing_laundry_services">
    <rdfs:subClassOf rdf:resource="jc3iedm_ACTION.owl#ACTION-EVENT"/>
    <rdfs:subClassOf>
      <owl:Restriction>
        <owl:hasValue xml:lang="en">PRVLND</owl:hasValue>
        <owl:onProperty rdf:resource="jc3iedm_ACTION.owl#action-event-category-code"/>
      </owl:Restriction>
    </rdfs:subClassOf>
    <rdfs:label xml:lang="en">providing laundry services</rdfs:label>
    <rdfs:comment xml:lang="en">Providing labour and materiel for laundering of clothes or linens.</rdfs:comment>
  </owl:Class>
  <owl:Class rdf:about="jc3iedm_ACTIONExtended.owl#ACTION-EVENT_Disease">
    <rdfs:subClassOf rdf:resource="jc3iedm_ACTION.owl#ACTION-EVENT"/>
    <rdfs:subClassOf>
      <owl:Restriction>
        <owl:hasValue xml:lang="en">DISEAS</owl:hasValue>
        <owl:onProperty rdf:resource="jc3iedm_ACTION.owl#action-event-category-code"/>
      </owl:Restriction>
    </rdfs:subClassOf>
    <rdfs:label xml:lang="en">disease</rdfs:label>
    <rdfs:comment xml:lang="en">A disorder of structure or function in a human, animal, or plant, especially one that produces specific symptoms or that affects a specific part.</rdfs:comment>
  </owl:Class>
  <owl:Class rdf:about="jc3iedm_ACTIONExtended.owl#ACTION-EVENT_Capture">
    <rdfs:subClassOf rdf:resource="jc3iedm_ACTION.owl#ACTION-EVENT"/>
    <rdfs:subClassOf>
      <owl:Restriction>
        <owl:hasValue xml:lang="en">CAPTUR</owl:hasValue>
        <owl:onProperty rdf:resource="jc3iedm_ACTION.owl#action-event-category-code"/>
      </owl:Restriction>
    </rdfs:subClassOf>
    <rdfs:label xml:lang="en">capture</rdfs:label>
    <rdfs:comment xml:lang="en">Taking possession of an object, normally by force; it frequently involves movement as a preliminary phase.</rdfs:comment>
  </owl:Class>
  <owl:Class rdf:about="jc3iedm_ACTIONExtended.owl#ACTION-EVENT_Bypass">
    <rdfs:subClassOf rdf:resource="jc3iedm_ACTION.owl#ACTION-EVENT"/>
    <rdfs:subClassOf>
      <owl:Restriction>
        <owl:hasValue xml:lang="en">BYPASS</owl:hasValue>
        <owl:onProperty rdf:resource="jc3iedm_ACTION.owl#action-event-category-code"/>
      </owl:Restriction>
    </rdfs:subClassOf>
    <rdfs:label xml:lang="en">bypass</rdfs:label>
    <rdfs:comment xml:lang="en">Manoeuvring around an obstacle, position, or enemy force to maintain the momentum of advance.</rdfs:comment>
  </owl:Class>
  <owl:Class rdf:about="jc3iedm_ACTIONExtended.owl#ACTION-EVENT_Crossing">
    <rdfs:subClassOf rdf:resource="jc3iedm_ACTION.owl#ACTION-EVENT"/>
    <rdfs:subClassOf>
      <owl:Restriction>
        <owl:hasValue xml:lang="en">CROSSN</owl:hasValue>
        <owl:onProperty rdf:resource="jc3iedm_ACTION.owl#action-event-category-code"/>
      </owl:Restriction>
    </rdfs:subClassOf>
    <rdfs:label xml:lang="en">crossing</rdfs:label>
    <rdfs:comment xml:lang="en">Traversing a FEATURE or FACILITY.</rdfs:comment>
  </owl:Class>
  <owl:Class rdf:about="jc3iedm_ACTIONExtended.owl#ACTION-EVENT_Firefighting">
    <rdfs:subClassOf rdf:resource="jc3iedm_ACTION.owl#ACTION-EVENT"/>
    <rdfs:subClassOf>
      <owl:Restriction>
        <owl:hasValue xml:lang="en">FRFGTN</owl:hasValue>
        <owl:onProperty rdf:resource="jc3iedm_ACTION.owl#action-event-category-code"/>
      </owl:Restriction>
    </rdfs:subClassOf>
    <rdfs:label xml:lang="en">firefighting</rdfs:label>
    <rdfs:comment xml:lang="en">The activity of extinguishing fires.</rdfs:comment>
  </owl:Class>
  <owl:Class rdf:about="jc3iedm_ACTIONExtended.owl#ACTION-EVENT_Patrolling">
    <rdfs:subClassOf rdf:resource="jc3iedm_ACTION.owl#ACTION-EVENT"/>
    <rdfs:subClassOf>
      <owl:Restriction>
        <owl:hasValue xml:lang="en">PTRLNG</owl:hasValue>
        <owl:onProperty rdf:resource="jc3iedm_ACTION.owl#action-event-category-code"/>
      </owl:Restriction>
    </rdfs:subClassOf>
    <rdfs:label xml:lang="en">patrolling</rdfs:label>
    <rdfs:comment xml:lang="en">Gathering information or carrying out a destructive, harassing, mopping-up, or security mission.</rdfs:comment>
  </owl:Class>
  <owl:Class rdf:about="jc3iedm_ACTIONExtended.owl#ACTION-EVENT_Massive_deportation_banishment">
    <rdfs:subClassOf rdf:resource="jc3iedm_ACTION.owl#ACTION-EVENT"/>
    <rdfs:subClassOf>
      <owl:Restriction>
        <owl:hasValue xml:lang="en">DEPORT</owl:hasValue>
        <owl:onProperty rdf:resource="jc3iedm_ACTION.owl#action-event-category-code"/>
      </owl:Restriction>
    </rdfs:subClassOf>
    <rdfs:label xml:lang="en">massive deportation/banishment</rdfs:label>
    <rdfs:comment xml:lang="en">The driving out or removing from a home or place of usual resort or continuance of a large number of people.</rdfs:comment>
  </owl:Class>
  <owl:Class rdf:about="jc3iedm_ACTIONExtended.owl#ACTION-EVENT_Neutralize__chemical">
    <rdfs:subClassOf rdf:resource="jc3iedm_ACTION.owl#ACTION-EVENT"/>
    <rdfs:subClassOf>
      <owl:Restriction>
        <owl:hasValue xml:lang="en">NTRCHM</owl:hasValue>
        <owl:onProperty rdf:resource="jc3iedm_ACTION.owl#action-event-category-code"/>
      </owl:Restriction>
    </rdfs:subClassOf>
    <rdfs:label xml:lang="en">neutralize, chemical</rdfs:label>
    <rdfs:comment xml:lang="en">Making safe or non-toxic an object contaminated with a chemical agent.</rdfs:comment>
  </owl:Class>
  <owl:Class rdf:about="jc3iedm_ACTIONExtended.owl#REQUEST_Capability">
    <rdfs:subClassOf rdf:resource="jc3iedm_ACTION.owl#REQUEST"/>
    <rdfs:subClassOf>
      <owl:Restriction>
        <owl:hasValue xml:lang="en">CAPAB</owl:hasValue>
        <owl:onProperty rdf:resource="jc3iedm_ACTION.owl#request-category-code"/>
      </owl:Restriction>
    </rdfs:subClassOf>
    <rdfs:label xml:lang="en">capability</rdfs:label>
    <rdfs:comment xml:lang="en">To discover the capability of an ACTION-OBJECTIVE (OBJECT-ITEM) by any means.</rdfs:comment>
  </owl:Class>
  <owl:Class rdf:about="jc3iedm_ACTIONExtended.owl#ACTION-EVENT_National_holiday">
    <rdfs:subClassOf rdf:resource="jc3iedm_ACTION.owl#ACTION-EVENT"/>
    <rdfs:subClassOf>
      <owl:Restriction>
        <owl:hasValue xml:lang="en">HOLIDY</owl:hasValue>
        <owl:onProperty rdf:resource="jc3iedm_ACTION.owl#action-event-category-code"/>
      </owl:Restriction>
    </rdfs:subClassOf>
    <rdfs:label xml:lang="en">national holiday</rdfs:label>
    <rdfs:comment xml:lang="en">A day designated by a national authority as a day when work is not compulsory.</rdfs:comment>
  </owl:Class>
  <owl:Class rdf:about="jc3iedm_ACTIONExtended.owl#ACTION-EVENT_Observing">
    <rdfs:subClassOf rdf:resource="jc3iedm_ACTION.owl#ACTION-EVENT"/>
    <rdfs:subClassOf>
      <owl:Restriction>
        <owl:hasValue xml:lang="en">OBSRNG</owl:hasValue>
        <owl:onProperty rdf:resource="jc3iedm_ACTION.owl#action-event-category-code"/>
      </owl:Restriction>
    </rdfs:subClassOf>
    <rdfs:label xml:lang="en">observing</rdfs:label>
    <rdfs:comment xml:lang="en">Providing continuous view and the potential for reports on the activity of an object.</rdfs:comment>
  </owl:Class>
  <owl:Class rdf:about="jc3iedm_ACTIONExtended.owl#ACTION-EVENT_Electronic_emission">
    <rdfs:subClassOf rdf:resource="jc3iedm_ACTION.owl#ACTION-EVENT"/>
    <rdfs:subClassOf>
      <owl:Restriction>
        <owl:hasValue xml:lang="en">ELCEMS</owl:hasValue>
        <owl:onProperty rdf:resource="jc3iedm_ACTION.owl#action-event-category-code"/>
      </owl:Restriction>
    </rdfs:subClassOf>
    <rdfs:label xml:lang="en">electronic emission</rdfs:label>
    <rdfs:comment xml:lang="en">The radiation of electromagnetic energy.</rdfs:comment>
  </owl:Class>
  <owl:Class rdf:about="jc3iedm_ACTIONExtended.owl#ACTION-EVENT_Collision__mid-air">
    <rdfs:subClassOf rdf:resource="jc3iedm_ACTION.owl#ACTION-EVENT"/>
    <rdfs:subClassOf>
      <owl:Restriction>
        <owl:hasValue xml:lang="en">COLMID</owl:hasValue>
        <owl:onProperty rdf:resource="jc3iedm_ACTION.owl#action-event-category-code"/>
      </owl:Restriction>
    </rdfs:subClassOf>
    <rdfs:label xml:lang="en">collision, mid air</rdfs:label>
    <rdfs:comment xml:lang="en">In-flight collision of an aircraft with another aircraft.</rdfs:comment>
  </owl:Class>
  <owl:Class rdf:about="jc3iedm_ACTIONExtended.owl#ACTION-EVENT_Assisting_a_criminal">
    <rdfs:subClassOf rdf:resource="jc3iedm_ACTION.owl#ACTION-EVENT"/>
    <rdfs:subClassOf>
      <owl:Restriction>
        <owl:hasValue xml:lang="en">ASTCRM</owl:hasValue>
        <owl:onProperty rdf:resource="jc3iedm_ACTION.owl#action-event-category-code"/>
      </owl:Restriction>
    </rdfs:subClassOf>
    <rdfs:label xml:lang="en">assisting a criminal</rdfs:label>
    <rdfs:comment xml:lang="en">Assisting or abetting a known criminal or terrorist.</rdfs:comment>
  </owl:Class>
  <owl:Class rdf:about="jc3iedm_ACTIONExtended.owl#ACTION-EVENT_Serving_as_a_breakout_force">
    <rdfs:subClassOf rdf:resource="jc3iedm_ACTION.owl#ACTION-EVENT"/>
    <rdfs:subClassOf>
      <owl:Restriction>
        <owl:hasValue xml:lang="en">SRVBRK</owl:hasValue>
        <owl:onProperty rdf:resource="jc3iedm_ACTION.owl#action-event-category-code"/>
      </owl:Restriction>
    </rdfs:subClassOf>
    <rdfs:label xml:lang="en">serving as a breakout force</rdfs:label>
    <rdfs:comment xml:lang="en">Operating as a force that is tasked with the continuation of the operation during an obstacle crossing.</rdfs:comment>
  </owl:Class>
  <owl:Class rdf:about="jc3iedm_ACTIONExtended.owl#ACTION-EVENT_Weapon_firing">
    <rdfs:subClassOf rdf:resource="jc3iedm_ACTION.owl#ACTION-EVENT"/>
    <rdfs:subClassOf>
      <owl:Restriction>
        <owl:hasValue xml:lang="en">WPNFIR</owl:hasValue>
        <owl:onProperty rdf:resource="jc3iedm_ACTION.owl#action-event-category-code"/>
      </owl:Restriction>
    </rdfs:subClassOf>
    <rdfs:label xml:lang="en">weapon firing</rdfs:label>
    <rdfs:comment xml:lang="en">The firing of weapons.</rdfs:comment>
  </owl:Class>
  <owl:Class rdf:about="jc3iedm_ACTIONExtended.owl#ACTION-EVENT_Human_rights_violation">
    <rdfs:subClassOf rdf:resource="jc3iedm_ACTION.owl#ACTION-EVENT"/>
    <rdfs:subClassOf>
      <owl:Restriction>
        <owl:hasValue xml:lang="en">HRVIOL</owl:hasValue>
        <owl:onProperty rdf:resource="jc3iedm_ACTION.owl#action-event-category-code"/>
      </owl:Restriction>
    </rdfs:subClassOf>
    <rdfs:label xml:lang="en">human rights violation</rdfs:label>
    <rdfs:comment xml:lang="en">The commitment of an act against human rights.</rdfs:comment>
  </owl:Class>
  <owl:Class rdf:about="jc3iedm_ACTIONExtended.owl#ACTION-EVENT_National_election">
    <rdfs:subClassOf rdf:resource="jc3iedm_ACTION.owl#ACTION-EVENT"/>
    <rdfs:subClassOf>
      <owl:Restriction>
        <owl:hasValue xml:lang="en">NATELC</owl:hasValue>
        <owl:onProperty rdf:resource="jc3iedm_ACTION.owl#action-event-category-code"/>
      </owl:Restriction>
    </rdfs:subClassOf>
    <rdfs:label xml:lang="en">national election</rdfs:label>
    <rdfs:comment xml:lang="en">An ACTION-EVENT in which national officials are selected by vote.</rdfs:comment>
  </owl:Class>
  <owl:Class rdf:about="jc3iedm_ACTIONExtended.owl#ACTION-EVENT_Procuring">
    <rdfs:subClassOf rdf:resource="jc3iedm_ACTION.owl#ACTION-EVENT"/>
    <rdfs:subClassOf>
      <owl:Restriction>
        <owl:hasValue xml:lang="en">PROCUR</owl:hasValue>
        <owl:onProperty rdf:resource="jc3iedm_ACTION.owl#action-event-category-code"/>
      </owl:Restriction>
    </rdfs:subClassOf>
    <rdfs:label xml:lang="en">procuring</rdfs:label>
    <rdfs:comment xml:lang="en">Buying whatever is needed to fulfil a certain action.</rdfs:comment>
  </owl:Class>
  <owl:Class rdf:about="jc3iedm_ACTIONExtended.owl#ACTION-EVENT_Reinforcing">
    <rdfs:subClassOf rdf:resource="jc3iedm_ACTION.owl#ACTION-EVENT"/>
    <rdfs:subClassOf>
      <owl:Restriction>
        <owl:hasValue xml:lang="en">REINFN</owl:hasValue>
        <owl:onProperty rdf:resource="jc3iedm_ACTION.owl#action-event-category-code"/>
      </owl:Restriction>
    </rdfs:subClassOf>
    <rdfs:label xml:lang="en">reinforcing</rdfs:label>
    <rdfs:comment xml:lang="en">Making a force available for the purpose of supplementing an in-place force.</rdfs:comment>
  </owl:Class>
  <owl:Class rdf:about="jc3iedm_ACTIONExtended.owl#ACTION-EVENT_Neutralize__explosive">
    <rdfs:subClassOf rdf:resource="jc3iedm_ACTION.owl#ACTION-EVENT"/>
    <rdfs:subClassOf>
      <owl:Restriction>
        <owl:hasValue xml:lang="en">NTREXP</owl:hasValue>
        <owl:onProperty rdf:resource="jc3iedm_ACTION.owl#action-event-category-code"/>
      </owl:Restriction>
    </rdfs:subClassOf>
    <rdfs:label xml:lang="en">neutralize, explosive</rdfs:label>
    <rdfs:comment xml:lang="en">Rendering bombs, mines, missiles, and booby traps into a safe state.</rdfs:comment>
  </owl:Class>
  <owl:Class rdf:about="jc3iedm_ACTIONExtended.owl#ACTION-EVENT_Attempted_robbery">
    <rdfs:subClassOf rdf:resource="jc3iedm_ACTION.owl#ACTION-EVENT"/>
    <rdfs:subClassOf>
      <owl:Restriction>
        <owl:hasValue xml:lang="en">ATRBRY</owl:hasValue>
        <owl:onProperty rdf:resource="jc3iedm_ACTION.owl#action-event-category-code"/>
      </owl:Restriction>
    </rdfs:subClassOf>
    <rdfs:label xml:lang="en">attempted robbery</rdfs:label>
    <rdfs:comment xml:lang="en">The attempted act of robbing a person or place.</rdfs:comment>
  </owl:Class>
  <owl:Class rdf:about="jc3iedm_ACTIONExtended.owl#ACTION-EVENT_Sabotage">
    <rdfs:subClassOf rdf:resource="jc3iedm_ACTION.owl#ACTION-EVENT"/>
    <rdfs:subClassOf>
      <owl:Restriction>
        <owl:hasValue xml:lang="en">SABOTG</owl:hasValue>
        <owl:onProperty rdf:resource="jc3iedm_ACTION.owl#action-event-category-code"/>
      </owl:Restriction>
    </rdfs:subClassOf>
    <rdfs:label xml:lang="en">sabotage</rdfs:label>
    <rdfs:comment xml:lang="en">An act or acts with intent to injure, interfere with, or obstruct the national defence of a country by wilfully injuring or destroying, or attempting to injure or destroy, any national defence or war material, premises or utilities, to include human and natural resources.</rdfs:comment>
  </owl:Class>
  <owl:Class rdf:about="jc3iedm_ACTIONExtended.owl#ACTION-EVENT_War_crisis_alert">
    <rdfs:subClassOf rdf:resource="jc3iedm_ACTION.owl#ACTION-EVENT"/>
    <rdfs:subClassOf>
      <owl:Restriction>
        <owl:hasValue xml:lang="en">WARALE</owl:hasValue>
        <owl:onProperty rdf:resource="jc3iedm_ACTION.owl#action-event-category-code"/>
      </owl:Restriction>
    </rdfs:subClassOf>
    <rdfs:label xml:lang="en">war/crisis alert</rdfs:label>
    <rdfs:comment xml:lang="en">The state of readiness caused by the possibility of a war.</rdfs:comment>
  </owl:Class>
  <owl:Class rdf:about="jc3iedm_ACTIONExtended.owl#ACTION-EVENT_Organised_crime">
    <rdfs:subClassOf rdf:resource="jc3iedm_ACTION.owl#ACTION-EVENT"/>
    <rdfs:subClassOf>
      <owl:Restriction>
        <owl:hasValue xml:lang="en">ORGCRM</owl:hasValue>
        <owl:onProperty rdf:resource="jc3iedm_ACTION.owl#action-event-category-code"/>
      </owl:Restriction>
    </rdfs:subClassOf>
    <rdfs:label xml:lang="en">organised crime</rdfs:label>
    <rdfs:comment xml:lang="en">Violation of the laws of a civil society performed by a group of persons established for that reason.</rdfs:comment>
  </owl:Class>
  <owl:Class rdf:about="jc3iedm_ACTIONExtended.owl#NUCLEAR-EVENT_Nuclear_waste_disposal">
    <rdfs:subClassOf rdf:resource="jc3iedm_ACTION.owl#NUCLEAR-EVENT"/>
    <rdfs:subClassOf>
      <owl:Restriction>
        <owl:hasValue xml:lang="en">NUCWST</owl:hasValue>
        <owl:onProperty rdf:resource="jc3iedm_ACTION.owl#nuclear-event-category-code"/>
      </owl:Restriction>
    </rdfs:subClassOf>
    <rdfs:label xml:lang="en">nuclear waste disposal</rdfs:label>
    <rdfs:comment xml:lang="en">Removing nuclear polluted substances to a designated storage area.</rdfs:comment>
  </owl:Class>
  <owl:Class rdf:about="jc3iedm_ACTIONExtended.owl#ACTION-EVENT_Jamming">
    <rdfs:subClassOf rdf:resource="jc3iedm_ACTION.owl#ACTION-EVENT"/>
    <rdfs:subClassOf>
      <owl:Restriction>
        <owl:hasValue xml:lang="en">JAMMNG</owl:hasValue>
        <owl:onProperty rdf:resource="jc3iedm_ACTION.owl#action-event-category-code"/>
      </owl:Restriction>
    </rdfs:subClassOf>
    <rdfs:label xml:lang="en">jamming</rdfs:label>
    <rdfs:comment xml:lang="en">Deliberately radiating, re-radiating or reflecting electromagnetic energy with the object of impairing the use of electronic devices, equipment or systems being used by the enemy.</rdfs:comment>
  </owl:Class>
  <owl:Class rdf:about="jc3iedm_ACTIONExtended.owl#ACTION-EVENT_Fix__acoustic">
    <rdfs:subClassOf rdf:resource="jc3iedm_ACTION.owl#ACTION-EVENT"/>
    <rdfs:subClassOf>
      <owl:Restriction>
        <owl:hasValue xml:lang="en">FIXACO</owl:hasValue>
        <owl:onProperty rdf:resource="jc3iedm_ACTION.owl#action-event-category-code"/>
      </owl:Restriction>
    </rdfs:subClassOf>
    <rdfs:label xml:lang="en">fix, acoustic</rdfs:label>
    <rdfs:comment xml:lang="en">Determining a position using acoustic data.</rdfs:comment>
  </owl:Class>
  <owl:Class rdf:about="jc3iedm_ACTIONExtended.owl#ACTION-EVENT_Airborne_assault">
    <rdfs:subClassOf rdf:resource="jc3iedm_ACTION.owl#ACTION-EVENT"/>
    <rdfs:subClassOf>
      <owl:Restriction>
        <owl:hasValue xml:lang="en">ARBNAS</owl:hasValue>
        <owl:onProperty rdf:resource="jc3iedm_ACTION.owl#action-event-category-code"/>
      </owl:Restriction>
    </rdfs:subClassOf>
    <rdfs:label xml:lang="en">airborne assault</rdfs:label>
    <rdfs:comment xml:lang="en">Mounting an airborne operation, a phase beginning with delivery by air of the assault echelon of the force into the objective area and extending through attack of assault objectives and consolidation of the initial airhead.</rdfs:comment>
  </owl:Class>
  <owl:Class rdf:about="jc3iedm_ACTIONExtended.owl#ACTION-EVENT_Guarding">
    <rdfs:subClassOf rdf:resource="jc3iedm_ACTION.owl#ACTION-EVENT"/>
    <rdfs:subClassOf>
      <owl:Restriction>
        <owl:hasValue xml:lang="en">GUARDN</owl:hasValue>
        <owl:onProperty rdf:resource="jc3iedm_ACTION.owl#action-event-category-code"/>
      </owl:Restriction>
    </rdfs:subClassOf>
    <rdfs:label xml:lang="en">guarding</rdfs:label>
    <rdfs:comment xml:lang="en">Operating as a security element to protect the main body by fighting to gain time while also observing and reporting information.</rdfs:comment>
  </owl:Class>
  <owl:Class rdf:about="jc3iedm_ACTIONExtended.owl#ACTION-EVENT_Leaguer">
    <rdfs:subClassOf rdf:resource="jc3iedm_ACTION.owl#ACTION-EVENT"/>
    <rdfs:subClassOf>
      <owl:Restriction>
        <owl:hasValue xml:lang="en">LEAGR</owl:hasValue>
        <owl:onProperty rdf:resource="jc3iedm_ACTION.owl#action-event-category-code"/>
      </owl:Restriction>
    </rdfs:subClassOf>
    <rdfs:label xml:lang="en">leaguer</rdfs:label>
    <rdfs:comment xml:lang="en">Adopting a defended formation as a temporary defensive measure in areas of low or moderate risk of combat.</rdfs:comment>
  </owl:Class>
  <owl:Class rdf:about="jc3iedm_ACTIONExtended.owl#ACTION-EVENT_Conducting_preparatory_fire">
    <rdfs:subClassOf rdf:resource="jc3iedm_ACTION.owl#ACTION-EVENT"/>
    <rdfs:subClassOf>
      <owl:Restriction>
        <owl:hasValue xml:lang="en">CNPRFR</owl:hasValue>
        <owl:onProperty rdf:resource="jc3iedm_ACTION.owl#action-event-category-code"/>
      </owl:Restriction>
    </rdfs:subClassOf>
    <rdfs:label xml:lang="en">conducting preparatory fire</rdfs:label>
    <rdfs:comment xml:lang="en">Delivering fire on a target preparatory to an assault.</rdfs:comment>
  </owl:Class>
  <owl:Class rdf:about="jc3iedm_ACTIONExtended.owl#ACTION-EVENT_Poisoning">
    <rdfs:subClassOf rdf:resource="jc3iedm_ACTION.owl#ACTION-EVENT"/>
    <rdfs:subClassOf>
      <owl:Restriction>
        <owl:hasValue xml:lang="en">POISON</owl:hasValue>
        <owl:onProperty rdf:resource="jc3iedm_ACTION.owl#action-event-category-code"/>
      </owl:Restriction>
    </rdfs:subClassOf>
    <rdfs:label xml:lang="en">poisoning</rdfs:label>
    <rdfs:comment xml:lang="en">Injuring or killing with toxic agents.</rdfs:comment>
  </owl:Class>
  <owl:Class rdf:about="jc3iedm_ACTIONExtended.owl#ACTION-EVENT_Hunting">
    <rdfs:subClassOf rdf:resource="jc3iedm_ACTION.owl#ACTION-EVENT"/>
    <rdfs:subClassOf>
      <owl:Restriction>
        <owl:hasValue xml:lang="en">HUNTNG</owl:hasValue>
        <owl:onProperty rdf:resource="jc3iedm_ACTION.owl#action-event-category-code"/>
      </owl:Restriction>
    </rdfs:subClassOf>
    <rdfs:label xml:lang="en">hunting</rdfs:label>
    <rdfs:comment xml:lang="en">The activity of hunting wild animals or game, especially for food or sport.</rdfs:comment>
  </owl:Class>
  <owl:Class rdf:about="jc3iedm_ACTIONExtended.owl#ACTION-EVENT_Counter-battery_fire">
    <rdfs:subClassOf rdf:resource="jc3iedm_ACTION.owl#ACTION-EVENT"/>
    <rdfs:subClassOf>
      <owl:Restriction>
        <owl:hasValue xml:lang="en">CTRBYF</owl:hasValue>
        <owl:onProperty rdf:resource="jc3iedm_ACTION.owl#action-event-category-code"/>
      </owl:Restriction>
    </rdfs:subClassOf>
    <rdfs:label xml:lang="en">counter battery fire</rdfs:label>
    <rdfs:comment xml:lang="en">Fire delivered for the purpose of destroying or neutralizing indirect fire weapons systems.</rdfs:comment>
  </owl:Class>
  <owl:Class rdf:about="jc3iedm_ACTIONExtended.owl#ACTION-EVENT_Attack__not_otherwise_specified">
    <rdfs:subClassOf rdf:resource="jc3iedm_ACTION.owl#ACTION-EVENT"/>
    <rdfs:subClassOf>
      <owl:Restriction>
        <owl:hasValue xml:lang="en">ATTACK</owl:hasValue>
        <owl:onProperty rdf:resource="jc3iedm_ACTION.owl#action-event-category-code"/>
      </owl:Restriction>
    </rdfs:subClassOf>
    <rdfs:label xml:lang="en">attack, not otherwise specified</rdfs:label>
    <rdfs:comment xml:lang="en">Conducting an offensive operation characterised by coordinated employment of firepower and manoeuvre to close with and destroy or capture the enemy.</rdfs:comment>
  </owl:Class>
  <owl:Class rdf:about="jc3iedm_ACTIONExtended.owl#ACTION-EVENT_Picketing">
    <rdfs:subClassOf rdf:resource="jc3iedm_ACTION.owl#ACTION-EVENT"/>
    <rdfs:subClassOf>
      <owl:Restriction>
        <owl:hasValue xml:lang="en">PCKTNG</owl:hasValue>
        <owl:onProperty rdf:resource="jc3iedm_ACTION.owl#action-event-category-code"/>
      </owl:Restriction>
    </rdfs:subClassOf>
    <rdfs:label xml:lang="en">picketing</rdfs:label>
    <rdfs:comment xml:lang="en">An act by a person or persons outside a place of work, intending to persuade esp. workers not to enter during a strike.</rdfs:comment>
  </owl:Class>
  <owl:Class rdf:about="jc3iedm_ACTIONExtended.owl#ACTION-EVENT_Intimidation">
    <rdfs:subClassOf rdf:resource="jc3iedm_ACTION.owl#ACTION-EVENT"/>
    <rdfs:subClassOf>
      <owl:Restriction>
        <owl:hasValue xml:lang="en">INTMDN</owl:hasValue>
        <owl:onProperty rdf:resource="jc3iedm_ACTION.owl#action-event-category-code"/>
      </owl:Restriction>
    </rdfs:subClassOf>
    <rdfs:label xml:lang="en">intimidation</rdfs:label>
    <rdfs:comment xml:lang="en">Act to frighten or overawe.</rdfs:comment>
  </owl:Class>
  <owl:Class rdf:about="jc3iedm_ACTIONExtended.owl#ACTION-EVENT_Explosion">
    <rdfs:subClassOf rdf:resource="jc3iedm_ACTION.owl#ACTION-EVENT"/>
    <rdfs:subClassOf>
      <owl:Restriction>
        <owl:hasValue xml:lang="en">EXPLOS</owl:hasValue>
        <owl:onProperty rdf:resource="jc3iedm_ACTION.owl#action-event-category-code"/>
      </owl:Restriction>
    </rdfs:subClassOf>
    <rdfs:label xml:lang="en">explosion</rdfs:label>
    <rdfs:comment xml:lang="en">A sudden release of any kind of energy.</rdfs:comment>
  </owl:Class>
  <owl:Class rdf:about="jc3iedm_ACTIONExtended.owl#ACTION-EVENT_Ceremony_or_parade">
    <rdfs:subClassOf rdf:resource="jc3iedm_ACTION.owl#ACTION-EVENT"/>
    <rdfs:subClassOf>
      <owl:Restriction>
        <owl:hasValue xml:lang="en">CEREMN</owl:hasValue>
        <owl:onProperty rdf:resource="jc3iedm_ACTION.owl#action-event-category-code"/>
      </owl:Restriction>
    </rdfs:subClassOf>
    <rdfs:label xml:lang="en">ceremony or parade</rdfs:label>
    <rdfs:comment xml:lang="en">The formal gathering of a group of people in order to carry out an act or series of acts prescribed by ritual protocol or convention.</rdfs:comment>
  </owl:Class>
  <owl:Class rdf:about="jc3iedm_ACTIONExtended.owl#ACTION-EVENT_Deflecting">
    <rdfs:subClassOf rdf:resource="jc3iedm_ACTION.owl#ACTION-EVENT"/>
    <rdfs:subClassOf>
      <owl:Restriction>
        <owl:hasValue xml:lang="en">DEFLCT</owl:hasValue>
        <owl:onProperty rdf:resource="jc3iedm_ACTION.owl#action-event-category-code"/>
      </owl:Restriction>
    </rdfs:subClassOf>
    <rdfs:label xml:lang="en">deflecting</rdfs:label>
    <rdfs:comment xml:lang="en">Preventing an enemy force from following the intended course.</rdfs:comment>
  </owl:Class>
  <owl:Class rdf:about="jc3iedm_ACTIONExtended.owl#ACTION-EVENT_Confiscation">
    <rdfs:subClassOf rdf:resource="jc3iedm_ACTION.owl#ACTION-EVENT"/>
    <rdfs:subClassOf>
      <owl:Restriction>
        <owl:hasValue xml:lang="en">CNFSTN</owl:hasValue>
        <owl:onProperty rdf:resource="jc3iedm_ACTION.owl#action-event-category-code"/>
      </owl:Restriction>
    </rdfs:subClassOf>
    <rdfs:label xml:lang="en">confiscation</rdfs:label>
    <rdfs:comment xml:lang="en">The seizure of property under public authority.</rdfs:comment>
  </owl:Class>
  <owl:Class rdf:about="jc3iedm_ACTIONExtended.owl#ACTION-EVENT_Disrupting">
    <rdfs:subClassOf rdf:resource="jc3iedm_ACTION.owl#ACTION-EVENT"/>
    <rdfs:subClassOf>
      <owl:Restriction>
        <owl:hasValue xml:lang="en">DSRPTN</owl:hasValue>
        <owl:onProperty rdf:resource="jc3iedm_ACTION.owl#action-event-category-code"/>
      </owl:Restriction>
    </rdfs:subClassOf>
    <rdfs:label xml:lang="en">disrupting</rdfs:label>
    <rdfs:comment xml:lang="en">Breaking apart an enemy’s formation and tempo, interrupting the enemy’s time table, causing premature commitment of forces, and/or splintering their attack using integrated fire planning and obstacle effect.</rdfs:comment>
  </owl:Class>
  <owl:Class rdf:about="jc3iedm_ACTIONExtended.owl#ACTION-EVENT_Border_crossing__surveilled">
    <rdfs:subClassOf rdf:resource="jc3iedm_ACTION.owl#ACTION-EVENT"/>
    <rdfs:subClassOf>
      <owl:Restriction>
        <owl:hasValue xml:lang="en">BCSRVL</owl:hasValue>
        <owl:onProperty rdf:resource="jc3iedm_ACTION.owl#action-event-category-code"/>
      </owl:Restriction>
    </rdfs:subClassOf>
    <rdfs:label xml:lang="en">border crossing, surveilled</rdfs:label>
    <rdfs:comment xml:lang="en">A border crossing that is conducted under surveillance.</rdfs:comment>
  </owl:Class>
  <owl:Class rdf:about="jc3iedm_ACTIONExtended.owl#ACTION-EVENT_Equipment_failure">
    <rdfs:subClassOf rdf:resource="jc3iedm_ACTION.owl#ACTION-EVENT"/>
    <rdfs:subClassOf>
      <owl:Restriction>
        <owl:hasValue xml:lang="en">EQPFAI</owl:hasValue>
        <owl:onProperty rdf:resource="jc3iedm_ACTION.owl#action-event-category-code"/>
      </owl:Restriction>
    </rdfs:subClassOf>
    <rdfs:label xml:lang="en">equipment failure</rdfs:label>
    <rdfs:comment xml:lang="en">A cessation of proper functioning or performance of a piece of equipment.</rdfs:comment>
  </owl:Class>
  <owl:Class rdf:about="jc3iedm_ACTIONExtended.owl#ACTION-EVENT_Hold__offensive">
    <rdfs:subClassOf rdf:resource="jc3iedm_ACTION.owl#ACTION-EVENT"/>
    <rdfs:subClassOf>
      <owl:Restriction>
        <owl:hasValue xml:lang="en">HLDOFF</owl:hasValue>
        <owl:onProperty rdf:resource="jc3iedm_ACTION.owl#action-event-category-code"/>
      </owl:Restriction>
    </rdfs:subClassOf>
    <rdfs:label xml:lang="en">hold, offensive</rdfs:label>
    <rdfs:comment xml:lang="en">Exerting sufficient pressure by means of combat power in an attack to prevent the movement or redeployment of enemy forces.</rdfs:comment>
  </owl:Class>
  <owl:Class rdf:about="jc3iedm_ACTIONExtended.owl#ACTION-EVENT_Turning">
    <rdfs:subClassOf rdf:resource="jc3iedm_ACTION.owl#ACTION-EVENT"/>
    <rdfs:subClassOf>
      <owl:Restriction>
        <owl:hasValue xml:lang="en">TURNNG</owl:hasValue>
        <owl:onProperty rdf:resource="jc3iedm_ACTION.owl#action-event-category-code"/>
      </owl:Restriction>
    </rdfs:subClassOf>
    <rdfs:label xml:lang="en">turning</rdfs:label>
    <rdfs:comment xml:lang="en">Compelling an enemy force to move from one avenue of approach or movement corridor to another.</rdfs:comment>
  </owl:Class>
  <owl:Class rdf:about="jc3iedm_ACTIONExtended.owl#REQUEST_Hostility">
    <rdfs:subClassOf rdf:resource="jc3iedm_ACTION.owl#REQUEST"/>
    <rdfs:subClassOf>
      <owl:Restriction>
        <owl:hasValue xml:lang="en">HOSTIL</owl:hasValue>
        <owl:onProperty rdf:resource="jc3iedm_ACTION.owl#request-category-code"/>
      </owl:Restriction>
    </rdfs:subClassOf>
    <rdfs:label xml:lang="en">hostility</rdfs:label>
    <rdfs:comment xml:lang="en">To recognise the friendly or enemy character of an ACTION-OBJECTIVE (OBJECT-ITEM) by any means.</rdfs:comment>
  </owl:Class>
  <owl:Class rdf:about="jc3iedm_ACTIONExtended.owl#ACTION-EVENT_Space_accident">
    <rdfs:subClassOf rdf:resource="jc3iedm_ACTION.owl#ACTION-EVENT"/>
    <rdfs:subClassOf>
      <owl:Restriction>
        <owl:hasValue xml:lang="en">SPACAC</owl:hasValue>
        <owl:onProperty rdf:resource="jc3iedm_ACTION.owl#action-event-category-code"/>
      </owl:Restriction>
    </rdfs:subClassOf>
    <rdfs:label xml:lang="en">space accident</rdfs:label>
    <rdfs:comment xml:lang="en">The unforeseen loss, destruction or damage of a spacecraft.</rdfs:comment>
  </owl:Class>
  <owl:Class rdf:about="jc3iedm_ACTIONExtended.owl#ACTION-EVENT_Attempted_suicide">
    <rdfs:subClassOf rdf:resource="jc3iedm_ACTION.owl#ACTION-EVENT"/>
    <rdfs:subClassOf>
      <owl:Restriction>
        <owl:hasValue xml:lang="en">ATSCDE</owl:hasValue>
        <owl:onProperty rdf:resource="jc3iedm_ACTION.owl#action-event-category-code"/>
      </owl:Restriction>
    </rdfs:subClassOf>
    <rdfs:label xml:lang="en">attempted suicide</rdfs:label>
    <rdfs:comment xml:lang="en">The attempted act of killing oneself intentionally.</rdfs:comment>
  </owl:Class>
  <owl:Class rdf:about="jc3iedm_ACTIONExtended.owl#ACTION-EVENT_Secession_of_portion_of_country">
    <rdfs:subClassOf rdf:resource="jc3iedm_ACTION.owl#ACTION-EVENT"/>
    <rdfs:subClassOf>
      <owl:Restriction>
        <owl:hasValue xml:lang="en">SECCOU</owl:hasValue>
        <owl:onProperty rdf:resource="jc3iedm_ACTION.owl#action-event-category-code"/>
      </owl:Restriction>
    </rdfs:subClassOf>
    <rdfs:label xml:lang="en">secession of portion of country</rdfs:label>
    <rdfs:comment xml:lang="en">The formal withdrawal of a portion of a country.</rdfs:comment>
  </owl:Class>
  <owl:Class rdf:about="jc3iedm_ACTIONExtended.owl#ACTION-EVENT_Identifying">
    <rdfs:subClassOf rdf:resource="jc3iedm_ACTION.owl#ACTION-EVENT"/>
    <rdfs:subClassOf>
      <owl:Restriction>
        <owl:hasValue xml:lang="en">IDENT</owl:hasValue>
        <owl:onProperty rdf:resource="jc3iedm_ACTION.owl#action-event-category-code"/>
      </owl:Restriction>
    </rdfs:subClassOf>
    <rdfs:label xml:lang="en">identifying</rdfs:label>
    <rdfs:comment xml:lang="en">Determining the identification of a particular class of object, recognising the friendly or enemy character of an object, or detecting the presence of an object.</rdfs:comment>
  </owl:Class>
  <owl:Class rdf:about="jc3iedm_ACTIONExtended.owl#ACTION-EVENT_Reconnaissance">
    <rdfs:subClassOf rdf:resource="jc3iedm_ACTION.owl#ACTION-EVENT"/>
    <rdfs:subClassOf>
      <owl:Restriction>
        <owl:hasValue xml:lang="en">RECCE</owl:hasValue>
        <owl:onProperty rdf:resource="jc3iedm_ACTION.owl#action-event-category-code"/>
      </owl:Restriction>
    </rdfs:subClassOf>
    <rdfs:label xml:lang="en">reconnaissance</rdfs:label>
    <rdfs:comment xml:lang="en">Conducting a mission to obtain by visual operations or other detection methods information about the activities and resources of an enemy or potential enemy, or to secure data concerning the meteorological, hydrographic or geographic characteristics of a particular area.</rdfs:comment>
  </owl:Class>
  <owl:Class rdf:about="jc3iedm_ACTIONExtended.owl#ACTION-EVENT_Clearing__air">
    <rdfs:subClassOf rdf:resource="jc3iedm_ACTION.owl#ACTION-EVENT"/>
    <rdfs:subClassOf>
      <owl:Restriction>
        <owl:hasValue xml:lang="en">CLRAIR</owl:hasValue>
        <owl:onProperty rdf:resource="jc3iedm_ACTION.owl#action-event-category-code"/>
      </owl:Restriction>
    </rdfs:subClassOf>
    <rdfs:label xml:lang="en">clearing, air</rdfs:label>
    <rdfs:comment xml:lang="en">Clearing of the air to gain either temporary or permanent air superiority or control in a given sector.</rdfs:comment>
  </owl:Class>
  <owl:Class rdf:about="jc3iedm_ACTIONExtended.owl#ACTION-EVENT_Repairing">
    <rdfs:subClassOf rdf:resource="jc3iedm_ACTION.owl#ACTION-EVENT"/>
    <rdfs:subClassOf>
      <owl:Restriction>
        <owl:hasValue xml:lang="en">REPAIR</owl:hasValue>
        <owl:onProperty rdf:resource="jc3iedm_ACTION.owl#action-event-category-code"/>
      </owl:Restriction>
    </rdfs:subClassOf>
    <rdfs:label xml:lang="en">repairing</rdfs:label>
    <rdfs:comment xml:lang="en">Restoring an item to serviceable condition through correction of a specific failure or unserviceable condition.</rdfs:comment>
  </owl:Class>
  <owl:Class rdf:about="jc3iedm_ACTIONExtended.owl#ACTION-EVENT_Drug_distribution__illegal">
    <rdfs:subClassOf rdf:resource="jc3iedm_ACTION.owl#ACTION-EVENT"/>
    <rdfs:subClassOf>
      <owl:Restriction>
        <owl:hasValue xml:lang="en">DRGDST</owl:hasValue>
        <owl:onProperty rdf:resource="jc3iedm_ACTION.owl#action-event-category-code"/>
      </owl:Restriction>
    </rdfs:subClassOf>
    <rdfs:label xml:lang="en">drug distribution, illegal</rdfs:label>
    <rdfs:comment xml:lang="en">An action to distribute illegal drugs or to illegally distribute legal drugs.</rdfs:comment>
  </owl:Class>
  <owl:Class rdf:about="jc3iedm_ACTIONExtended.owl#ACTION-EVENT_State_of_war">
    <rdfs:subClassOf rdf:resource="jc3iedm_ACTION.owl#ACTION-EVENT"/>
    <rdfs:subClassOf>
      <owl:Restriction>
        <owl:hasValue xml:lang="en">STAWAR</owl:hasValue>
        <owl:onProperty rdf:resource="jc3iedm_ACTION.owl#action-event-category-code"/>
      </owl:Restriction>
    </rdfs:subClassOf>
    <rdfs:label xml:lang="en">state of war</rdfs:label>
    <rdfs:comment xml:lang="en">A state characterised by hostile military activity between the parts.</rdfs:comment>
  </owl:Class>
  <owl:Class rdf:about="jc3iedm_ACTIONExtended.owl#CHEMICAL-BIOLOGICAL-EVENT_Biological_alarm">
    <rdfs:subClassOf rdf:resource="jc3iedm_ACTION.owl#CHEMICAL-BIOLOGICAL-EVENT"/>
    <rdfs:subClassOf>
      <owl:Restriction>
        <owl:hasValue xml:lang="en">BIOALM</owl:hasValue>
        <owl:onProperty rdf:resource="jc3iedm_ACTION.owl#chemical-biological-event-category-code"/>
      </owl:Restriction>
    </rdfs:subClassOf>
    <rdfs:label xml:lang="en">biological alarm</rdfs:label>
    <rdfs:comment xml:lang="en">An action by which a biological detector is triggered or a group is warned.</rdfs:comment>
  </owl:Class>
  <owl:Class rdf:about="jc3iedm_ACTIONExtended.owl#ACTION-EVENT_Demolition">
    <rdfs:subClassOf rdf:resource="jc3iedm_ACTION.owl#ACTION-EVENT"/>
    <rdfs:subClassOf>
      <owl:Restriction>
        <owl:hasValue xml:lang="en">DEMO</owl:hasValue>
        <owl:onProperty rdf:resource="jc3iedm_ACTION.owl#action-event-category-code"/>
      </owl:Restriction>
    </rdfs:subClassOf>
    <rdfs:label xml:lang="en">demolition</rdfs:label>
    <rdfs:comment xml:lang="en">The destruction of structures, facilities, or materiel by use of fire, water, explosives, mechanical, or other means.</rdfs:comment>
  </owl:Class>
  <owl:Class rdf:about="jc3iedm_ACTIONExtended.owl#ACTION-EVENT_Troublemaking__intimidating">
    <rdfs:subClassOf rdf:resource="jc3iedm_ACTION.owl#ACTION-EVENT"/>
    <rdfs:subClassOf>
      <owl:Restriction>
        <owl:hasValue xml:lang="en">TRBINT</owl:hasValue>
        <owl:onProperty rdf:resource="jc3iedm_ACTION.owl#action-event-category-code"/>
      </owl:Restriction>
    </rdfs:subClassOf>
    <rdfs:label xml:lang="en">troublemaking, intimidating</rdfs:label>
    <rdfs:comment xml:lang="en">Discouraging or inhibiting by or as if by threats.</rdfs:comment>
  </owl:Class>
  <owl:Class rdf:about="jc3iedm_ACTIONExtended.owl#ACTION-EVENT_Screening">
    <rdfs:subClassOf rdf:resource="jc3iedm_ACTION.owl#ACTION-EVENT"/>
    <rdfs:subClassOf>
      <owl:Restriction>
        <owl:hasValue xml:lang="en">SCRNNG</owl:hasValue>
        <owl:onProperty rdf:resource="jc3iedm_ACTION.owl#action-event-category-code"/>
      </owl:Restriction>
    </rdfs:subClassOf>
    <rdfs:label xml:lang="en">screening</rdfs:label>
    <rdfs:comment xml:lang="en">Operating as a security element whose primary task is to observe, identify and report information, and which only fights in self-protection.</rdfs:comment>
  </owl:Class>
  <owl:Class rdf:about="jc3iedm_ACTIONExtended.owl#RADIOACTIVE-EVENT_Radiation_alarm">
    <rdfs:subClassOf rdf:resource="jc3iedm_ACTION.owl#RADIOACTIVE-EVENT"/>
    <rdfs:subClassOf>
      <owl:Restriction>
        <owl:hasValue xml:lang="en">RADALM</owl:hasValue>
        <owl:onProperty rdf:resource="jc3iedm_ACTION.owl#radioactive-event-category-code"/>
      </owl:Restriction>
    </rdfs:subClassOf>
    <rdfs:label xml:lang="en">radiation alarm</rdfs:label>
    <rdfs:comment xml:lang="en">An action by which a radiological detector is triggered or a group is warned.</rdfs:comment>
  </owl:Class>
  <owl:Class rdf:about="jc3iedm_ACTIONExtended.owl#ACTION-EVENT_Fix__electromagnetic">
    <rdfs:subClassOf rdf:resource="jc3iedm_ACTION.owl#ACTION-EVENT"/>
    <rdfs:subClassOf>
      <owl:Restriction>
        <owl:hasValue xml:lang="en">FIXELM</owl:hasValue>
        <owl:onProperty rdf:resource="jc3iedm_ACTION.owl#action-event-category-code"/>
      </owl:Restriction>
    </rdfs:subClassOf>
    <rdfs:label xml:lang="en">fix, electromagnetic</rdfs:label>
    <rdfs:comment xml:lang="en">Determining a position using electromagnetic data.</rdfs:comment>
  </owl:Class>
  <owl:Class rdf:about="jc3iedm_ACTIONExtended.owl#ACTION-EVENT_Enemy_contact">
    <rdfs:subClassOf rdf:resource="jc3iedm_ACTION.owl#ACTION-EVENT"/>
    <rdfs:subClassOf>
      <owl:Restriction>
        <owl:hasValue xml:lang="en">ENMCON</owl:hasValue>
        <owl:onProperty rdf:resource="jc3iedm_ACTION.owl#action-event-category-code"/>
      </owl:Restriction>
    </rdfs:subClassOf>
    <rdfs:label xml:lang="en">enemy contact</rdfs:label>
    <rdfs:comment xml:lang="en">The situation when opposing forces are in sight of or in range of direct fire of each other's weapons.</rdfs:comment>
  </owl:Class>
  <owl:Class rdf:about="jc3iedm_ACTIONExtended.owl#ACTION-EVENT_Withdrawal_under_pressure">
    <rdfs:subClassOf rdf:resource="jc3iedm_ACTION.owl#ACTION-EVENT"/>
    <rdfs:subClassOf>
      <owl:Restriction>
        <owl:hasValue xml:lang="en">WDRPRS</owl:hasValue>
        <owl:onProperty rdf:resource="jc3iedm_ACTION.owl#action-event-category-code"/>
      </owl:Restriction>
    </rdfs:subClassOf>
    <rdfs:label xml:lang="en">withdrawal under pressure</rdfs:label>
    <rdfs:comment xml:lang="en">Disengaging from the enemy when the enemy has sufficient contact with friendly forces to interfere with the withdrawal.</rdfs:comment>
  </owl:Class>
  <owl:Class rdf:about="jc3iedm_ACTIONExtended.owl#ACTION-EVENT_Artillery_fire">
    <rdfs:subClassOf rdf:resource="jc3iedm_ACTION.owl#ACTION-EVENT"/>
    <rdfs:subClassOf>
      <owl:Restriction>
        <owl:hasValue xml:lang="en">ARTFIR</owl:hasValue>
        <owl:onProperty rdf:resource="jc3iedm_ACTION.owl#action-event-category-code"/>
      </owl:Restriction>
    </rdfs:subClassOf>
    <rdfs:label xml:lang="en">artillery fire</rdfs:label>
    <rdfs:comment xml:lang="en">The use of artillery fire.</rdfs:comment>
  </owl:Class>
  <owl:Class rdf:about="jc3iedm_ACTIONExtended.owl#CHEMICAL-BIOLOGICAL-EVENT_Biological_sampling">
    <rdfs:subClassOf rdf:resource="jc3iedm_ACTION.owl#CHEMICAL-BIOLOGICAL-EVENT"/>
    <rdfs:subClassOf>
      <owl:Restriction>
        <owl:hasValue xml:lang="en">BIOSMP</owl:hasValue>
        <owl:onProperty rdf:resource="jc3iedm_ACTION.owl#chemical-biological-event-category-code"/>
      </owl:Restriction>
    </rdfs:subClassOf>
    <rdfs:label xml:lang="en">biological sampling</rdfs:label>
    <rdfs:comment xml:lang="en">The action of detecting a biological contaminant.</rdfs:comment>
  </owl:Class>
  <owl:Class rdf:about="jc3iedm_ACTIONExtended.owl#ACTION-EVENT_Strike">
    <rdfs:subClassOf rdf:resource="jc3iedm_ACTION.owl#ACTION-EVENT"/>
    <rdfs:subClassOf>
      <owl:Restriction>
        <owl:hasValue xml:lang="en">STRIKE</owl:hasValue>
        <owl:onProperty rdf:resource="jc3iedm_ACTION.owl#action-event-category-code"/>
      </owl:Restriction>
    </rdfs:subClassOf>
    <rdfs:label xml:lang="en">strike</rdfs:label>
    <rdfs:comment xml:lang="en">The organised refusal by employees to work until some grievance is remedied.</rdfs:comment>
  </owl:Class>
  <owl:Class rdf:about="jc3iedm_ACTIONExtended.owl#ACTION-EVENT_Industrial_espionage_incident">
    <rdfs:subClassOf rdf:resource="jc3iedm_ACTION.owl#ACTION-EVENT"/>
    <rdfs:subClassOf>
      <owl:Restriction>
        <owl:hasValue xml:lang="en">INDESP</owl:hasValue>
        <owl:onProperty rdf:resource="jc3iedm_ACTION.owl#action-event-category-code"/>
      </owl:Restriction>
    </rdfs:subClassOf>
    <rdfs:label xml:lang="en">industrial espionage incident</rdfs:label>
    <rdfs:comment xml:lang="en">The practice of spying or the use of spies to obtain information about the plans and activities of competitors.</rdfs:comment>
  </owl:Class>
  <owl:Class rdf:about="jc3iedm_ACTIONExtended.owl#ACTION-EVENT_Occupying">
    <rdfs:subClassOf rdf:resource="jc3iedm_ACTION.owl#ACTION-EVENT"/>
    <rdfs:subClassOf>
      <owl:Restriction>
        <owl:hasValue xml:lang="en">OCCPNG</owl:hasValue>
        <owl:onProperty rdf:resource="jc3iedm_ACTION.owl#action-event-category-code"/>
      </owl:Restriction>
    </rdfs:subClassOf>
    <rdfs:label xml:lang="en">occupying</rdfs:label>
    <rdfs:comment xml:lang="en">Moving onto an objective, key terrain, or other manmade or natural terrain area without opposition and controlling that entire area.</rdfs:comment>
  </owl:Class>
  <owl:Class rdf:about="jc3iedm_ACTIONExtended.owl#REQUEST_Action">
    <rdfs:subClassOf rdf:resource="jc3iedm_ACTION.owl#REQUEST"/>
    <rdfs:subClassOf>
      <owl:Restriction>
        <owl:hasValue xml:lang="en">ACTION</owl:hasValue>
        <owl:onProperty rdf:resource="jc3iedm_ACTION.owl#request-category-code"/>
      </owl:Restriction>
    </rdfs:subClassOf>
    <rdfs:label xml:lang="en">action</rdfs:label>
    <rdfs:comment xml:lang="en">To discover the actions of an ACTION-OBJECTIVE (OBJECT-ITEM) by any means.</rdfs:comment>
  </owl:Class>
  <owl:Class rdf:about="jc3iedm_ACTIONExtended.owl#CHEMICAL-BIOLOGICAL-EVENT_Chemical_sampling">
    <rdfs:subClassOf rdf:resource="jc3iedm_ACTION.owl#CHEMICAL-BIOLOGICAL-EVENT"/>
    <rdfs:subClassOf>
      <owl:Restriction>
        <owl:hasValue xml:lang="en">CHMSMP</owl:hasValue>
        <owl:onProperty rdf:resource="jc3iedm_ACTION.owl#chemical-biological-event-category-code"/>
      </owl:Restriction>
    </rdfs:subClassOf>
    <rdfs:label xml:lang="en">chemical sampling</rdfs:label>
    <rdfs:comment xml:lang="en">The action of detecting a chemical contaminant.</rdfs:comment>
  </owl:Class>
  <owl:Class rdf:about="jc3iedm_ACTIONExtended.owl#NUCLEAR-EVENT_Nuclear_test">
    <rdfs:subClassOf rdf:resource="jc3iedm_ACTION.owl#NUCLEAR-EVENT"/>
    <rdfs:subClassOf>
      <owl:Restriction>
        <owl:hasValue xml:lang="en">NUCTST</owl:hasValue>
        <owl:onProperty rdf:resource="jc3iedm_ACTION.owl#nuclear-event-category-code"/>
      </owl:Restriction>
    </rdfs:subClassOf>
    <rdfs:label xml:lang="en">nuclear test</rdfs:label>
    <rdfs:comment xml:lang="en">The explosion of a nuclear device for test purpose.</rdfs:comment>
  </owl:Class>
  <owl:Class rdf:about="jc3iedm_ACTIONExtended.owl#ACTION-EVENT_Pursuing">
    <rdfs:subClassOf rdf:resource="jc3iedm_ACTION.owl#ACTION-EVENT"/>
    <rdfs:subClassOf>
      <owl:Restriction>
        <owl:hasValue xml:lang="en">PURSNG</owl:hasValue>
        <owl:onProperty rdf:resource="jc3iedm_ACTION.owl#action-event-category-code"/>
      </owl:Restriction>
    </rdfs:subClassOf>
    <rdfs:label xml:lang="en">pursuing</rdfs:label>
    <rdfs:comment xml:lang="en">Continuing an offensive operation in order to catch or cut off a hostile force attempting to escape, with the aim of destroying it. Typically, contact is maintained and risk taken to harass relentlessly, thereby turning the pursuit into a rout.</rdfs:comment>
  </owl:Class>
  <owl:Class rdf:about="jc3iedm_ACTIONExtended.owl#ACTION-EVENT_Aircraft_crash">
    <rdfs:subClassOf rdf:resource="jc3iedm_ACTION.owl#ACTION-EVENT"/>
    <rdfs:subClassOf>
      <owl:Restriction>
        <owl:hasValue xml:lang="en">AIRCRS</owl:hasValue>
        <owl:onProperty rdf:resource="jc3iedm_ACTION.owl#action-event-category-code"/>
      </owl:Restriction>
    </rdfs:subClassOf>
    <rdfs:label xml:lang="en">aircraft crash</rdfs:label>
    <rdfs:comment xml:lang="en">The unforeseen destruction or damage of an aircraft (and personnel).</rdfs:comment>
  </owl:Class>
  <owl:Class rdf:about="jc3iedm_ACTIONExtended.owl#ACTION-EVENT_Covering">
    <rdfs:subClassOf rdf:resource="jc3iedm_ACTION.owl#ACTION-EVENT"/>
    <rdfs:subClassOf>
      <owl:Restriction>
        <owl:hasValue xml:lang="en">COVERN</owl:hasValue>
        <owl:onProperty rdf:resource="jc3iedm_ACTION.owl#action-event-category-code"/>
      </owl:Restriction>
    </rdfs:subClassOf>
    <rdfs:label xml:lang="en">covering</rdfs:label>
    <rdfs:comment xml:lang="en">Operating as a force apart from the main body to protect the main body by fighting to gain time while also observing and reporting information and preventing enemy ground observation of an direct fire against the main body.</rdfs:comment>
  </owl:Class>
  <owl:Class rdf:about="jc3iedm_ACTIONExtended.owl#ACTION-EVENT_Arresting__legal">
    <rdfs:subClassOf rdf:resource="jc3iedm_ACTION.owl#ACTION-EVENT"/>
    <rdfs:subClassOf>
      <owl:Restriction>
        <owl:hasValue xml:lang="en">ARRLGL</owl:hasValue>
        <owl:onProperty rdf:resource="jc3iedm_ACTION.owl#action-event-category-code"/>
      </owl:Restriction>
    </rdfs:subClassOf>
    <rdfs:label xml:lang="en">arresting, legal</rdfs:label>
    <rdfs:comment xml:lang="en">Seizing and detaining of a person under authority of the law.</rdfs:comment>
  </owl:Class>
  <owl:Class rdf:about="jc3iedm_ACTIONExtended.owl#ACTION-EVENT_Border_raid">
    <rdfs:subClassOf rdf:resource="jc3iedm_ACTION.owl#ACTION-EVENT"/>
    <rdfs:subClassOf>
      <owl:Restriction>
        <owl:hasValue xml:lang="en">BORRAI</owl:hasValue>
        <owl:onProperty rdf:resource="jc3iedm_ACTION.owl#action-event-category-code"/>
      </owl:Restriction>
    </rdfs:subClassOf>
    <rdfs:label xml:lang="en">border raid</rdfs:label>
    <rdfs:comment xml:lang="en">A surprise attack by a force or a group of people across a national or territorial border (restricted to 25 km from the border).</rdfs:comment>
  </owl:Class>
  <owl:Class rdf:about="jc3iedm_ACTIONExtended.owl#ACTION-EVENT_Interception">
    <rdfs:subClassOf rdf:resource="jc3iedm_ACTION.owl#ACTION-EVENT"/>
    <rdfs:subClassOf>
      <owl:Restriction>
        <owl:hasValue xml:lang="en">INTCPN</owl:hasValue>
        <owl:onProperty rdf:resource="jc3iedm_ACTION.owl#action-event-category-code"/>
      </owl:Restriction>
    </rdfs:subClassOf>
    <rdfs:label xml:lang="en">interception</rdfs:label>
    <rdfs:comment xml:lang="en">Conducting electronic warfare support operations with a view to searching, locating and recording radiated electromagnetic energy.</rdfs:comment>
  </owl:Class>
  <owl:Class rdf:about="jc3iedm_ACTIONExtended.owl#ACTION-EVENT_Supporting">
    <rdfs:subClassOf rdf:resource="jc3iedm_ACTION.owl#ACTION-EVENT"/>
    <rdfs:subClassOf>
      <owl:Restriction>
        <owl:hasValue xml:lang="en">SUPRTN</owl:hasValue>
        <owl:onProperty rdf:resource="jc3iedm_ACTION.owl#action-event-category-code"/>
      </owl:Restriction>
    </rdfs:subClassOf>
    <rdfs:label xml:lang="en">supporting</rdfs:label>
    <rdfs:comment xml:lang="en">Aiding, protecting, complementing or sustaining an object.</rdfs:comment>
  </owl:Class>
  <owl:Class rdf:about="jc3iedm_ACTIONExtended.owl#ACTION-EVENT_Oceans__seas_or_water_pollution">
    <rdfs:subClassOf rdf:resource="jc3iedm_ACTION.owl#ACTION-EVENT"/>
    <rdfs:subClassOf>
      <owl:Restriction>
        <owl:hasValue xml:lang="en">WATPOL</owl:hasValue>
        <owl:onProperty rdf:resource="jc3iedm_ACTION.owl#action-event-category-code"/>
      </owl:Restriction>
    </rdfs:subClassOf>
    <rdfs:label xml:lang="en">oceans, seas or water pollution</rdfs:label>
    <rdfs:comment xml:lang="en">Contamination of a body of water caused by a poison or toxin.</rdfs:comment>
  </owl:Class>
  <owl:Class rdf:about="jc3iedm_ACTIONExtended.owl#ACTION-EVENT_Drug_manufacturing__illegal">
    <rdfs:subClassOf rdf:resource="jc3iedm_ACTION.owl#ACTION-EVENT"/>
    <rdfs:subClassOf>
      <owl:Restriction>
        <owl:hasValue xml:lang="en">DRGMNF</owl:hasValue>
        <owl:onProperty rdf:resource="jc3iedm_ACTION.owl#action-event-category-code"/>
      </owl:Restriction>
    </rdfs:subClassOf>
    <rdfs:label xml:lang="en">drug manufacturing, illegal</rdfs:label>
    <rdfs:comment xml:lang="en">An action to manufacture illegal drugs or to illegally manufacture legal drugs.</rdfs:comment>
  </owl:Class>
  <owl:Class rdf:about="jc3iedm_ACTIONExtended.owl#ACTION-EVENT_Accident__traffic">
    <rdfs:subClassOf rdf:resource="jc3iedm_ACTION.owl#ACTION-EVENT"/>
    <rdfs:subClassOf>
      <owl:Restriction>
        <owl:hasValue xml:lang="en">ACCTRF</owl:hasValue>
        <owl:onProperty rdf:resource="jc3iedm_ACTION.owl#action-event-category-code"/>
      </owl:Restriction>
    </rdfs:subClassOf>
    <rdfs:label xml:lang="en">accident, traffic</rdfs:label>
    <rdfs:comment xml:lang="en">An accident involving at least one motor vehicle.</rdfs:comment>
  </owl:Class>
  <owl:Class rdf:about="jc3iedm_ACTIONExtended.owl#ACTION-EVENT_Relief_in_place">
    <rdfs:subClassOf rdf:resource="jc3iedm_ACTION.owl#ACTION-EVENT"/>
    <rdfs:subClassOf>
      <owl:Restriction>
        <owl:hasValue xml:lang="en">RLFPLC</owl:hasValue>
        <owl:onProperty rdf:resource="jc3iedm_ACTION.owl#action-event-category-code"/>
      </owl:Restriction>
    </rdfs:subClassOf>
    <rdfs:label xml:lang="en">relief in place</rdfs:label>
    <rdfs:comment xml:lang="en">An operation in which, by direction of higher authority, all or part of a unit is replaced in an area by the incoming unit. The responsibilities of the replaced elements for the mission and the assigned zone of operations are transferred to the incoming unit. The incoming unit continues the operation as ordered.</rdfs:comment>
  </owl:Class>
  <owl:Class rdf:about="jc3iedm_ACTIONExtended.owl#ACTION-EVENT_Assembling">
    <rdfs:subClassOf rdf:resource="jc3iedm_ACTION.owl#ACTION-EVENT"/>
    <rdfs:subClassOf>
      <owl:Restriction>
        <owl:hasValue xml:lang="en">ASSMBL</owl:hasValue>
        <owl:onProperty rdf:resource="jc3iedm_ACTION.owl#action-event-category-code"/>
      </owl:Restriction>
    </rdfs:subClassOf>
    <rdfs:label xml:lang="en">assembling</rdfs:label>
    <rdfs:comment xml:lang="en">Joining together of multiple objects in the same area.</rdfs:comment>
  </owl:Class>
  <owl:Class rdf:about="jc3iedm_ACTIONExtended.owl#ACTION-EVENT_Civil_war">
    <rdfs:subClassOf rdf:resource="jc3iedm_ACTION.owl#ACTION-EVENT"/>
    <rdfs:subClassOf>
      <owl:Restriction>
        <owl:hasValue xml:lang="en">CIVWAR</owl:hasValue>
        <owl:onProperty rdf:resource="jc3iedm_ACTION.owl#action-event-category-code"/>
      </owl:Restriction>
    </rdfs:subClassOf>
    <rdfs:label xml:lang="en">civil war</rdfs:label>
    <rdfs:comment xml:lang="en">A war among fellow-citizens or within the limits of one community.</rdfs:comment>
  </owl:Class>
  <owl:Class rdf:about="jc3iedm_ACTIONExtended.owl#ACTION-EVENT_Withdrawal">
    <rdfs:subClassOf rdf:resource="jc3iedm_ACTION.owl#ACTION-EVENT"/>
    <rdfs:subClassOf>
      <owl:Restriction>
        <owl:hasValue xml:lang="en">WITDRL</owl:hasValue>
        <owl:onProperty rdf:resource="jc3iedm_ACTION.owl#action-event-category-code"/>
      </owl:Restriction>
    </rdfs:subClassOf>
    <rdfs:label xml:lang="en">withdrawal</rdfs:label>
    <rdfs:comment xml:lang="en">Disengaging a force in contact from an enemy force.</rdfs:comment>
  </owl:Class>
  <owl:Class rdf:about="jc3iedm_ACTIONExtended.owl#ACTION-EVENT_Rape">
    <rdfs:subClassOf rdf:resource="jc3iedm_ACTION.owl#ACTION-EVENT"/>
    <rdfs:subClassOf>
      <owl:Restriction>
        <owl:hasValue xml:lang="en">RAPE</owl:hasValue>
        <owl:onProperty rdf:resource="jc3iedm_ACTION.owl#action-event-category-code"/>
      </owl:Restriction>
    </rdfs:subClassOf>
    <rdfs:label xml:lang="en">rape</rdfs:label>
    <rdfs:comment xml:lang="en">The act of forcing another person to submit to sexual intercourse.</rdfs:comment>
  </owl:Class>
  <owl:Class rdf:about="jc3iedm_ACTIONExtended.owl#CHEMICAL-BIOLOGICAL-EVENT_Biological_attack">
    <rdfs:subClassOf rdf:resource="jc3iedm_ACTION.owl#CHEMICAL-BIOLOGICAL-EVENT"/>
    <rdfs:subClassOf>
      <owl:Restriction>
        <owl:hasValue xml:lang="en">BIOATT</owl:hasValue>
        <owl:onProperty rdf:resource="jc3iedm_ACTION.owl#chemical-biological-event-category-code"/>
      </owl:Restriction>
    </rdfs:subClassOf>
    <rdfs:label xml:lang="en">biological attack</rdfs:label>
    <rdfs:comment xml:lang="en">Employing the use of biological materiel(s) [agent(s)] to kill, injure, or incapacitate, for a significant period of time, man or animals, and deny or hinder the use of areas, facilities or materiel, or defence against such employment.</rdfs:comment>
  </owl:Class>
  <owl:Class rdf:about="jc3iedm_ACTIONExtended.owl#ACTION-EVENT_Illumination">
    <rdfs:subClassOf rdf:resource="jc3iedm_ACTION.owl#ACTION-EVENT"/>
    <rdfs:subClassOf>
      <owl:Restriction>
        <owl:hasValue xml:lang="en">ILLUMN</owl:hasValue>
        <owl:onProperty rdf:resource="jc3iedm_ACTION.owl#action-event-category-code"/>
      </owl:Restriction>
    </rdfs:subClassOf>
    <rdfs:label xml:lang="en">illumination</rdfs:label>
    <rdfs:comment xml:lang="en">Providing battlespace lighting by employing searchlight or pyrotechnic illuminants using diffusion or reflection.</rdfs:comment>
  </owl:Class>
  <owl:Class rdf:about="jc3iedm_ACTIONExtended.owl#ACTION-EVENT_Friendly_fire">
    <rdfs:subClassOf rdf:resource="jc3iedm_ACTION.owl#ACTION-EVENT"/>
    <rdfs:subClassOf>
      <owl:Restriction>
        <owl:hasValue xml:lang="en">FRNDFR</owl:hasValue>
        <owl:onProperty rdf:resource="jc3iedm_ACTION.owl#action-event-category-code"/>
      </owl:Restriction>
    </rdfs:subClassOf>
    <rdfs:label xml:lang="en">friendly fire</rdfs:label>
    <rdfs:comment xml:lang="en">Accidental damage by Allied troops to one's own installations, aircraft or personnel.</rdfs:comment>
  </owl:Class>
  <owl:Class rdf:about="jc3iedm_ACTIONExtended.owl#ACTION-EVENT_Martial_law_implementation">
    <rdfs:subClassOf rdf:resource="jc3iedm_ACTION.owl#ACTION-EVENT"/>
    <rdfs:subClassOf>
      <owl:Restriction>
        <owl:hasValue xml:lang="en">MARLAW</owl:hasValue>
        <owl:onProperty rdf:resource="jc3iedm_ACTION.owl#action-event-category-code"/>
      </owl:Restriction>
    </rdfs:subClassOf>
    <rdfs:label xml:lang="en">martial law implementation</rdfs:label>
    <rdfs:comment xml:lang="en">Giving practical effect to military law, usually by restricting the rights of citizens for security reasons.</rdfs:comment>
  </owl:Class>
  <owl:Class rdf:about="jc3iedm_ACTIONExtended.owl#ACTION-EVENT_Verifying">
    <rdfs:subClassOf rdf:resource="jc3iedm_ACTION.owl#ACTION-EVENT"/>
    <rdfs:subClassOf>
      <owl:Restriction>
        <owl:hasValue xml:lang="en">VERFYN</owl:hasValue>
        <owl:onProperty rdf:resource="jc3iedm_ACTION.owl#action-event-category-code"/>
      </owl:Restriction>
    </rdfs:subClassOf>
    <rdfs:label xml:lang="en">verifying</rdfs:label>
    <rdfs:comment xml:lang="en">Testifying to, asserting, affirming or confirming, as true or certain.</rdfs:comment>
  </owl:Class>
  <owl:Class rdf:about="jc3iedm_ACTIONExtended.owl#ACTION-EVENT_Constructing">
    <rdfs:subClassOf rdf:resource="jc3iedm_ACTION.owl#ACTION-EVENT"/>
    <rdfs:subClassOf>
      <owl:Restriction>
        <owl:hasValue xml:lang="en">CONSTN</owl:hasValue>
        <owl:onProperty rdf:resource="jc3iedm_ACTION.owl#action-event-category-code"/>
      </owl:Restriction>
    </rdfs:subClassOf>
    <rdfs:label xml:lang="en">constructing</rdfs:label>
    <rdfs:comment xml:lang="en">Building, digging or creating an object.</rdfs:comment>
  </owl:Class>
  <owl:Class rdf:about="jc3iedm_ACTIONExtended.owl#ACTION-EVENT_Setting_up">
    <rdfs:subClassOf rdf:resource="jc3iedm_ACTION.owl#ACTION-EVENT"/>
    <rdfs:subClassOf>
      <owl:Restriction>
        <owl:hasValue xml:lang="en">STNGUP</owl:hasValue>
        <owl:onProperty rdf:resource="jc3iedm_ACTION.owl#action-event-category-code"/>
      </owl:Restriction>
    </rdfs:subClassOf>
    <rdfs:label xml:lang="en">setting up</rdfs:label>
    <rdfs:comment xml:lang="en">Establishing a FACILITY, ORGANISATION or FEATURE.</rdfs:comment>
  </owl:Class>
  <owl:Class rdf:about="jc3iedm_ACTIONExtended.owl#ACTION-EVENT_Collision__obstacle">
    <rdfs:subClassOf rdf:resource="jc3iedm_ACTION.owl#ACTION-EVENT"/>
    <rdfs:subClassOf>
      <owl:Restriction>
        <owl:hasValue xml:lang="en">COLOBS</owl:hasValue>
        <owl:onProperty rdf:resource="jc3iedm_ACTION.owl#action-event-category-code"/>
      </owl:Restriction>
    </rdfs:subClassOf>
    <rdfs:label xml:lang="en">collision, obstacle</rdfs:label>
    <rdfs:comment xml:lang="en">In-flight collision of an aircraft with natural or man-made object (fixed or mobile) located on the ground.</rdfs:comment>
  </owl:Class>
  <owl:Class rdf:about="jc3iedm_ACTIONExtended.owl#ACTION-EVENT_Border_crossing__escorted">
    <rdfs:subClassOf rdf:resource="jc3iedm_ACTION.owl#ACTION-EVENT"/>
    <rdfs:subClassOf>
      <owl:Restriction>
        <owl:hasValue xml:lang="en">BCESC</owl:hasValue>
        <owl:onProperty rdf:resource="jc3iedm_ACTION.owl#action-event-category-code"/>
      </owl:Restriction>
    </rdfs:subClassOf>
    <rdfs:label xml:lang="en">border crossing, escorted</rdfs:label>
    <rdfs:comment xml:lang="en">A border crossing that is conducted under escort.</rdfs:comment>
  </owl:Class>
  <owl:Class rdf:about="jc3iedm_ACTIONExtended.owl#ACTION-EVENT_Troublemaking__harassing">
    <rdfs:subClassOf rdf:resource="jc3iedm_ACTION.owl#ACTION-EVENT"/>
    <rdfs:subClassOf>
      <owl:Restriction>
        <owl:hasValue xml:lang="en">TRBHAR</owl:hasValue>
        <owl:onProperty rdf:resource="jc3iedm_ACTION.owl#action-event-category-code"/>
      </owl:Restriction>
    </rdfs:subClassOf>
    <rdfs:label xml:lang="en">troublemaking, harassing</rdfs:label>
    <rdfs:comment xml:lang="en">Persecuting systematically by besetting with annoyances, threats or demands.</rdfs:comment>
  </owl:Class>
  <owl:Class rdf:about="jc3iedm_ACTIONExtended.owl#ACTION-EVENT_Rocket_fire">
    <rdfs:subClassOf rdf:resource="jc3iedm_ACTION.owl#ACTION-EVENT"/>
    <rdfs:subClassOf>
      <owl:Restriction>
        <owl:hasValue xml:lang="en">RKTFIR</owl:hasValue>
        <owl:onProperty rdf:resource="jc3iedm_ACTION.owl#action-event-category-code"/>
      </owl:Restriction>
    </rdfs:subClassOf>
    <rdfs:label xml:lang="en">rocket fire</rdfs:label>
    <rdfs:comment xml:lang="en">The employment of a rocket powered weapon.</rdfs:comment>
  </owl:Class>
  <owl:Class rdf:about="jc3iedm_ACTIONExtended.owl#ACTION-EVENT_Reconstituting">
    <rdfs:subClassOf rdf:resource="jc3iedm_ACTION.owl#ACTION-EVENT"/>
    <rdfs:subClassOf>
      <owl:Restriction>
        <owl:hasValue xml:lang="en">RECNSN</owl:hasValue>
        <owl:onProperty rdf:resource="jc3iedm_ACTION.owl#action-event-category-code"/>
      </owl:Restriction>
    </rdfs:subClassOf>
    <rdfs:label xml:lang="en">reconstituting</rdfs:label>
    <rdfs:comment xml:lang="en">Attaining prescribed strength of units and prescribed levels of vehicles, equipment, stores and supplies. The process will only take place after a unit/formation combat effectiveness has been reduced.</rdfs:comment>
  </owl:Class>
  <owl:Class rdf:about="jc3iedm_ACTIONExtended.owl#ACTION-EVENT_Belly_landing">
    <rdfs:subClassOf rdf:resource="jc3iedm_ACTION.owl#ACTION-EVENT"/>
    <rdfs:subClassOf>
      <owl:Restriction>
        <owl:hasValue xml:lang="en">BLYLND</owl:hasValue>
        <owl:onProperty rdf:resource="jc3iedm_ACTION.owl#action-event-category-code"/>
      </owl:Restriction>
    </rdfs:subClassOf>
    <rdfs:label xml:lang="en">belly landing</rdfs:label>
    <rdfs:comment xml:lang="en">An aircraft has landed without using the landing gear.</rdfs:comment>
  </owl:Class>
  <owl:Class rdf:about="jc3iedm_ACTIONExtended.owl#ACTION-EVENT_Revolution">
    <rdfs:subClassOf rdf:resource="jc3iedm_ACTION.owl#ACTION-EVENT"/>
    <rdfs:subClassOf>
      <owl:Restriction>
        <owl:hasValue xml:lang="en">REVOLU</owl:hasValue>
        <owl:onProperty rdf:resource="jc3iedm_ACTION.owl#action-event-category-code"/>
      </owl:Restriction>
    </rdfs:subClassOf>
    <rdfs:label xml:lang="en">revolution</rdfs:label>
    <rdfs:comment xml:lang="en">The overthrow or renunciation of one government or ruler and the substitution of another by the governed.</rdfs:comment>
  </owl:Class>
  <owl:Class rdf:about="jc3iedm_ACTIONExtended.owl#ACTION-EVENT_Letter_bomb_explosion">
    <rdfs:subClassOf rdf:resource="jc3iedm_ACTION.owl#ACTION-EVENT"/>
    <rdfs:subClassOf>
      <owl:Restriction>
        <owl:hasValue xml:lang="en">LTRBME</owl:hasValue>
        <owl:onProperty rdf:resource="jc3iedm_ACTION.owl#action-event-category-code"/>
      </owl:Restriction>
    </rdfs:subClassOf>
    <rdfs:label xml:lang="en">letter bomb explosion</rdfs:label>
    <rdfs:comment xml:lang="en">The explosion of a seemingly harmless letter or parcel.</rdfs:comment>
  </owl:Class>
  <owl:Class rdf:about="jc3iedm_ACTIONExtended.owl#ACTION-EVENT_Deploying">
    <rdfs:subClassOf rdf:resource="jc3iedm_ACTION.owl#ACTION-EVENT"/>
    <rdfs:subClassOf>
      <owl:Restriction>
        <owl:hasValue xml:lang="en">DEPLOY</owl:hasValue>
        <owl:onProperty rdf:resource="jc3iedm_ACTION.owl#action-event-category-code"/>
      </owl:Restriction>
    </rdfs:subClassOf>
    <rdfs:label xml:lang="en">deploying</rdfs:label>
    <rdfs:comment xml:lang="en">Moving to and adopting a tactical formation or dispersal at a specific location.</rdfs:comment>
  </owl:Class>
  <owl:Class rdf:about="jc3iedm_ACTIONExtended.owl#ACTION-EVENT_Mutual_assistance_pact_agreement">
    <rdfs:subClassOf rdf:resource="jc3iedm_ACTION.owl#ACTION-EVENT"/>
    <rdfs:subClassOf>
      <owl:Restriction>
        <owl:hasValue xml:lang="en">MUTASS</owl:hasValue>
        <owl:onProperty rdf:resource="jc3iedm_ACTION.owl#action-event-category-code"/>
      </owl:Restriction>
    </rdfs:subClassOf>
    <rdfs:label xml:lang="en">mutual assistance pact agreement</rdfs:label>
    <rdfs:comment xml:lang="en">An arrangement or contract between a number of organisations to provide mutual support.</rdfs:comment>
  </owl:Class>
  <owl:Class rdf:about="jc3iedm_ACTIONExtended.owl#ACTION-EVENT_Conducting_sporting_events">
    <rdfs:subClassOf rdf:resource="jc3iedm_ACTION.owl#ACTION-EVENT"/>
    <rdfs:subClassOf>
      <owl:Restriction>
        <owl:hasValue xml:lang="en">CNDSPT</owl:hasValue>
        <owl:onProperty rdf:resource="jc3iedm_ACTION.owl#action-event-category-code"/>
      </owl:Restriction>
    </rdfs:subClassOf>
    <rdfs:label xml:lang="en">conducting sporting events</rdfs:label>
    <rdfs:comment xml:lang="en">Conducting any game or competitive activity, especially an outdoor one involving physical exertion, e.g. cricket, football, racing, hunting.</rdfs:comment>
  </owl:Class>
  <owl:Class rdf:about="jc3iedm_ACTIONExtended.owl#ACTION-EVENT_Kidnapping">
    <rdfs:subClassOf rdf:resource="jc3iedm_ACTION.owl#ACTION-EVENT"/>
    <rdfs:subClassOf>
      <owl:Restriction>
        <owl:hasValue xml:lang="en">KIDNAP</owl:hasValue>
        <owl:onProperty rdf:resource="jc3iedm_ACTION.owl#action-event-category-code"/>
      </owl:Restriction>
    </rdfs:subClassOf>
    <rdfs:label xml:lang="en">kidnapping</rdfs:label>
    <rdfs:comment xml:lang="en">Seizing and holding a person unlawfully, usually for ransom or political gain.</rdfs:comment>
  </owl:Class>
  <owl:Class rdf:about="jc3iedm_ACTIONExtended.owl#NUCLEAR-EVENT_Nuclear_sampling">
    <rdfs:subClassOf rdf:resource="jc3iedm_ACTION.owl#NUCLEAR-EVENT"/>
    <rdfs:subClassOf>
      <owl:Restriction>
        <owl:hasValue xml:lang="en">NUCSMP</owl:hasValue>
        <owl:onProperty rdf:resource="jc3iedm_ACTION.owl#nuclear-event-category-code"/>
      </owl:Restriction>
    </rdfs:subClassOf>
    <rdfs:label xml:lang="en">nuclear sampling</rdfs:label>
    <rdfs:comment xml:lang="en">The action of detecting a radiological contaminant.</rdfs:comment>
  </owl:Class>
  <owl:Class rdf:about="jc3iedm_ACTIONExtended.owl#ACTION-TASK_Plan">
    <rdfs:subClassOf rdf:resource="jc3iedm_ACTION.owl#ACTION-TASK"/>
    <rdfs:subClassOf>
      <owl:Restriction>
        <owl:hasValue xml:lang="en">PLAN</owl:hasValue>
        <owl:onProperty rdf:resource="jc3iedm_ACTION.owl#action-task-category-code"/>
      </owl:Restriction>
    </rdfs:subClassOf>
    <rdfs:label xml:lang="en">plan</rdfs:label>
    <rdfs:comment xml:lang="en">An ACTION-TASK that represents a course of action that is foreseen or anticipated.</rdfs:comment>
  </owl:Class>
  <owl:Class rdf:about="jc3iedm_ACTIONExtended.owl#ACTION-EVENT_Drought">
    <rdfs:subClassOf rdf:resource="jc3iedm_ACTION.owl#ACTION-EVENT"/>
    <rdfs:subClassOf>
      <owl:Restriction>
        <owl:hasValue xml:lang="en">DROUGH</owl:hasValue>
        <owl:onProperty rdf:resource="jc3iedm_ACTION.owl#action-event-category-code"/>
      </owl:Restriction>
    </rdfs:subClassOf>
    <rdfs:label xml:lang="en">drought</rdfs:label>
    <rdfs:comment xml:lang="en">A prolonged or chronic shortage of water.</rdfs:comment>
  </owl:Class>
  <owl:Class rdf:about="jc3iedm_ACTIONExtended.owl#ACTION-EVENT_Clearing__land_combat">
    <rdfs:subClassOf rdf:resource="jc3iedm_ACTION.owl#ACTION-EVENT"/>
    <rdfs:subClassOf>
      <owl:Restriction>
        <owl:hasValue xml:lang="en">CLRLND</owl:hasValue>
        <owl:onProperty rdf:resource="jc3iedm_ACTION.owl#action-event-category-code"/>
      </owl:Restriction>
    </rdfs:subClassOf>
    <rdfs:label xml:lang="en">clearing, land combat</rdfs:label>
    <rdfs:comment xml:lang="en">Removing all enemy forces from a specific location, area, or zone.</rdfs:comment>
  </owl:Class>
  <owl:Class rdf:about="jc3iedm_ACTIONExtended.owl#NUCLEAR-EVENT_Nuclear_war_alert">
    <rdfs:subClassOf rdf:resource="jc3iedm_ACTION.owl#NUCLEAR-EVENT"/>
    <rdfs:subClassOf>
      <owl:Restriction>
        <owl:hasValue xml:lang="en">NUCWAR</owl:hasValue>
        <owl:onProperty rdf:resource="jc3iedm_ACTION.owl#nuclear-event-category-code"/>
      </owl:Restriction>
    </rdfs:subClassOf>
    <rdfs:label xml:lang="en">nuclear war alert</rdfs:label>
    <rdfs:comment xml:lang="en">The state of readiness caused by the possibility of atomic bombings.</rdfs:comment>
  </owl:Class>
  <owl:Class rdf:about="jc3iedm_ACTIONExtended.owl#ACTION-EVENT_Mission_staging">
    <rdfs:subClassOf rdf:resource="jc3iedm_ACTION.owl#ACTION-EVENT"/>
    <rdfs:subClassOf>
      <owl:Restriction>
        <owl:hasValue xml:lang="en">MISSTG</owl:hasValue>
        <owl:onProperty rdf:resource="jc3iedm_ACTION.owl#action-event-category-code"/>
      </owl:Restriction>
    </rdfs:subClassOf>
    <rdfs:label xml:lang="en">mission staging</rdfs:label>
    <rdfs:comment xml:lang="en">The assembly of aircraft for the completion of a mission or other activity.</rdfs:comment>
  </owl:Class>
  <owl:Class rdf:about="jc3iedm_ACTIONExtended.owl#ACTION-EVENT_Serving_as_a_rear_guard">
    <rdfs:subClassOf rdf:resource="jc3iedm_ACTION.owl#ACTION-EVENT"/>
    <rdfs:subClassOf>
      <owl:Restriction>
        <owl:hasValue xml:lang="en">SRVRGD</owl:hasValue>
        <owl:onProperty rdf:resource="jc3iedm_ACTION.owl#action-event-category-code"/>
      </owl:Restriction>
    </rdfs:subClassOf>
    <rdfs:label xml:lang="en">serving as a rear guard</rdfs:label>
    <rdfs:comment xml:lang="en">Operating as a security element whose primary task is to move (or remain) at the rear of the main body and protect the main force by fighting to gain time, whilst also observing and reporting information.</rdfs:comment>
  </owl:Class>
  <owl:Class rdf:about="jc3iedm_ACTIONExtended.owl#ACTION-EVENT_Troublemaking__hooliganism">
    <rdfs:subClassOf rdf:resource="jc3iedm_ACTION.owl#ACTION-EVENT"/>
    <rdfs:subClassOf>
      <owl:Restriction>
        <owl:hasValue xml:lang="en">TRBHLG</owl:hasValue>
        <owl:onProperty rdf:resource="jc3iedm_ACTION.owl#action-event-category-code"/>
      </owl:Restriction>
    </rdfs:subClassOf>
    <rdfs:label xml:lang="en">troublemaking, hooliganism</rdfs:label>
    <rdfs:comment xml:lang="en">Causing difficulties by the actions of hoodlums, especially young ruffians.</rdfs:comment>
  </owl:Class>
  <owl:Class rdf:about="jc3iedm_ACTIONExtended.owl#ACTION-EVENT_Escorting">
    <rdfs:subClassOf rdf:resource="jc3iedm_ACTION.owl#ACTION-EVENT"/>
    <rdfs:subClassOf>
      <owl:Restriction>
        <owl:hasValue xml:lang="en">ESCRTN</owl:hasValue>
        <owl:onProperty rdf:resource="jc3iedm_ACTION.owl#action-event-category-code"/>
      </owl:Restriction>
    </rdfs:subClassOf>
    <rdfs:label xml:lang="en">escorting</rdfs:label>
    <rdfs:comment xml:lang="en">Accompanying and protecting another force or convoy.</rdfs:comment>
  </owl:Class>
  <owl:Class rdf:about="jc3iedm_ACTIONExtended.owl#ACTION-EVENT_Counter_attack_by_fire">
    <rdfs:subClassOf rdf:resource="jc3iedm_ACTION.owl#ACTION-EVENT"/>
    <rdfs:subClassOf>
      <owl:Restriction>
        <owl:hasValue xml:lang="en">CTRFIR</owl:hasValue>
        <owl:onProperty rdf:resource="jc3iedm_ACTION.owl#action-event-category-code"/>
      </owl:Restriction>
    </rdfs:subClassOf>
    <rdfs:label xml:lang="en">counter attack by fire</rdfs:label>
    <rdfs:comment xml:lang="en">Denying the enemy his goal by using fire against an engagement area to defeat or destroy an enemy force.</rdfs:comment>
  </owl:Class>
  <owl:Class rdf:about="jc3iedm_ACTIONExtended.owl#ACTION-EVENT_Execution">
    <rdfs:subClassOf rdf:resource="jc3iedm_ACTION.owl#ACTION-EVENT"/>
    <rdfs:subClassOf>
      <owl:Restriction>
        <owl:hasValue xml:lang="en">EXECTN</owl:hasValue>
        <owl:onProperty rdf:resource="jc3iedm_ACTION.owl#action-event-category-code"/>
      </owl:Restriction>
    </rdfs:subClassOf>
    <rdfs:label xml:lang="en">execution</rdfs:label>
    <rdfs:comment xml:lang="en">Putting a person to death, especially as a legal penalty.</rdfs:comment>
  </owl:Class>
  <owl:Class rdf:about="jc3iedm_ACTIONExtended.owl#ACTION-EVENT_Hijacking__land_vehicle">
    <rdfs:subClassOf rdf:resource="jc3iedm_ACTION.owl#ACTION-EVENT"/>
    <rdfs:subClassOf>
      <owl:Restriction>
        <owl:hasValue xml:lang="en">HJCKLV</owl:hasValue>
        <owl:onProperty rdf:resource="jc3iedm_ACTION.owl#action-event-category-code"/>
      </owl:Restriction>
    </rdfs:subClassOf>
    <rdfs:label xml:lang="en">hijacking, land vehicle</rdfs:label>
    <rdfs:comment xml:lang="en">Seizure of a land vehicle in order to go somewhere other than the scheduled destination.</rdfs:comment>
  </owl:Class>
  <owl:Class rdf:about="jc3iedm_ACTIONExtended.owl#ACTION-EVENT_Gunnery__air-to-air">
    <rdfs:subClassOf rdf:resource="jc3iedm_ACTION.owl#ACTION-EVENT"/>
    <rdfs:subClassOf>
      <owl:Restriction>
        <owl:hasValue xml:lang="en">GUNATA</owl:hasValue>
        <owl:onProperty rdf:resource="jc3iedm_ACTION.owl#action-event-category-code"/>
      </owl:Restriction>
    </rdfs:subClassOf>
    <rdfs:label xml:lang="en">gunnery, air to air</rdfs:label>
    <rdfs:comment xml:lang="en">The act of firing an air-to-air weapon, usually at an aircraft.</rdfs:comment>
  </owl:Class>
  <owl:Class rdf:about="jc3iedm_ACTIONExtended.owl#ACTION-EVENT_Providing_bedding">
    <rdfs:subClassOf rdf:resource="jc3iedm_ACTION.owl#ACTION-EVENT"/>
    <rdfs:subClassOf>
      <owl:Restriction>
        <owl:hasValue xml:lang="en">PRVBDD</owl:hasValue>
        <owl:onProperty rdf:resource="jc3iedm_ACTION.owl#action-event-category-code"/>
      </owl:Restriction>
    </rdfs:subClassOf>
    <rdfs:label xml:lang="en">providing bedding</rdfs:label>
    <rdfs:comment xml:lang="en">Providing (1) sleeping accommodation or (2) mattress and bedclothes.</rdfs:comment>
  </owl:Class>
  <owl:Class rdf:about="jc3iedm_ACTIONExtended.owl#ACTION-EVENT_Recuperating">
    <rdfs:subClassOf rdf:resource="jc3iedm_ACTION.owl#ACTION-EVENT"/>
    <rdfs:subClassOf>
      <owl:Restriction>
        <owl:hasValue xml:lang="en">RECPRN</owl:hasValue>
        <owl:onProperty rdf:resource="jc3iedm_ACTION.owl#action-event-category-code"/>
      </owl:Restriction>
    </rdfs:subClassOf>
    <rdfs:label xml:lang="en">recuperating</rdfs:label>
    <rdfs:comment xml:lang="en">Resting a unit after it has been in action. Some reconstitution may take place as well.</rdfs:comment>
  </owl:Class>
  <owl:Class rdf:about="jc3iedm_ACTIONExtended.owl#ACTION-EVENT_Troublemaking__inciting">
    <rdfs:subClassOf rdf:resource="jc3iedm_ACTION.owl#ACTION-EVENT"/>
    <rdfs:subClassOf>
      <owl:Restriction>
        <owl:hasValue xml:lang="en">TRBINC</owl:hasValue>
        <owl:onProperty rdf:resource="jc3iedm_ACTION.owl#action-event-category-code"/>
      </owl:Restriction>
    </rdfs:subClassOf>
    <rdfs:label xml:lang="en">troublemaking, inciting</rdfs:label>
    <rdfs:comment xml:lang="en">Provoking to action, stirring up or urging on.</rdfs:comment>
  </owl:Class>
  <owl:Class rdf:about="jc3iedm_ACTIONExtended.owl#ACTION-EVENT_Denying">
    <rdfs:subClassOf rdf:resource="jc3iedm_ACTION.owl#ACTION-EVENT"/>
    <rdfs:subClassOf>
      <owl:Restriction>
        <owl:hasValue xml:lang="en">DENYNG</owl:hasValue>
        <owl:onProperty rdf:resource="jc3iedm_ACTION.owl#action-event-category-code"/>
      </owl:Restriction>
    </rdfs:subClassOf>
    <rdfs:label xml:lang="en">denying</rdfs:label>
    <rdfs:comment xml:lang="en">Preventing access by blocking, disrupting, dislocating and/or bringing fire to bear.</rdfs:comment>
  </owl:Class>
  <owl:Class rdf:about="jc3iedm_ACTIONExtended.owl#ACTION-EVENT_Generating_chemical_smoke">
    <rdfs:subClassOf rdf:resource="jc3iedm_ACTION.owl#ACTION-EVENT"/>
    <rdfs:subClassOf>
      <owl:Restriction>
        <owl:hasValue xml:lang="en">GENCHS</owl:hasValue>
        <owl:onProperty rdf:resource="jc3iedm_ACTION.owl#action-event-category-code"/>
      </owl:Restriction>
    </rdfs:subClassOf>
    <rdfs:label xml:lang="en">generating chemical smoke</rdfs:label>
    <rdfs:comment xml:lang="en">Producing chemical smoke to act as a form of cover to protect ongoing operations.</rdfs:comment>
  </owl:Class>
  <owl:Class rdf:about="jc3iedm_ACTIONExtended.owl#ACTION-EVENT_Earthquake">
    <rdfs:subClassOf rdf:resource="jc3iedm_ACTION.owl#ACTION-EVENT"/>
    <rdfs:subClassOf>
      <owl:Restriction>
        <owl:hasValue xml:lang="en">EARTHQ</owl:hasValue>
        <owl:onProperty rdf:resource="jc3iedm_ACTION.owl#action-event-category-code"/>
      </owl:Restriction>
    </rdfs:subClassOf>
    <rdfs:label xml:lang="en">earthquake</rdfs:label>
    <rdfs:comment xml:lang="en">A convulsion of the earth's crust due to the release of accumulated stress as a result of faults in strata or volcanic action.</rdfs:comment>
  </owl:Class>
  <owl:Class rdf:about="jc3iedm_ACTIONExtended.owl#ACTION-EVENT_Election_associated_violence">
    <rdfs:subClassOf rdf:resource="jc3iedm_ACTION.owl#ACTION-EVENT"/>
    <rdfs:subClassOf>
      <owl:Restriction>
        <owl:hasValue xml:lang="en">ELCVIO</owl:hasValue>
        <owl:onProperty rdf:resource="jc3iedm_ACTION.owl#action-event-category-code"/>
      </owl:Restriction>
    </rdfs:subClassOf>
    <rdfs:label xml:lang="en">election associated violence</rdfs:label>
    <rdfs:comment xml:lang="en">The occurrence of violent acts due to an election process.</rdfs:comment>
  </owl:Class>
  <owl:Class rdf:about="jc3iedm_ACTIONExtended.owl#ACTION-EVENT_Troublemaking__bullying">
    <rdfs:subClassOf rdf:resource="jc3iedm_ACTION.owl#ACTION-EVENT"/>
    <rdfs:subClassOf>
      <owl:Restriction>
        <owl:hasValue xml:lang="en">TRBBLL</owl:hasValue>
        <owl:onProperty rdf:resource="jc3iedm_ACTION.owl#action-event-category-code"/>
      </owl:Restriction>
    </rdfs:subClassOf>
    <rdfs:label xml:lang="en">troublemaking, bullying</rdfs:label>
    <rdfs:comment xml:lang="en">Intimidating by the use of superior size or strength.</rdfs:comment>
  </owl:Class>
  <owl:Class rdf:about="jc3iedm_ACTIONExtended.owl#ACTION-EVENT_Suspension_of_hostilities">
    <rdfs:subClassOf rdf:resource="jc3iedm_ACTION.owl#ACTION-EVENT"/>
    <rdfs:subClassOf>
      <owl:Restriction>
        <owl:hasValue xml:lang="en">SUSHOS</owl:hasValue>
        <owl:onProperty rdf:resource="jc3iedm_ACTION.owl#action-event-category-code"/>
      </owl:Restriction>
    </rdfs:subClassOf>
    <rdfs:label xml:lang="en">suspension of hostilities</rdfs:label>
    <rdfs:comment xml:lang="en">The cessation of war activities.</rdfs:comment>
  </owl:Class>
  <owl:Class rdf:about="jc3iedm_ACTIONExtended.owl#ACTION-EVENT_Maintaining">
    <rdfs:subClassOf rdf:resource="jc3iedm_ACTION.owl#ACTION-EVENT"/>
    <rdfs:subClassOf>
      <owl:Restriction>
        <owl:hasValue xml:lang="en">MAINTN</owl:hasValue>
        <owl:onProperty rdf:resource="jc3iedm_ACTION.owl#action-event-category-code"/>
      </owl:Restriction>
    </rdfs:subClassOf>
    <rdfs:label xml:lang="en">maintaining</rdfs:label>
    <rdfs:comment xml:lang="en">Providing services to keep equipment in condition to carry out its function.</rdfs:comment>
  </owl:Class>
  <owl:Class rdf:about="jc3iedm_ACTIONExtended.owl#ACTION-EVENT_Murder">
    <rdfs:subClassOf rdf:resource="jc3iedm_ACTION.owl#ACTION-EVENT"/>
    <rdfs:subClassOf>
      <owl:Restriction>
        <owl:hasValue xml:lang="en">MURDER</owl:hasValue>
        <owl:onProperty rdf:resource="jc3iedm_ACTION.owl#action-event-category-code"/>
      </owl:Restriction>
    </rdfs:subClassOf>
    <rdfs:label xml:lang="en">murder</rdfs:label>
    <rdfs:comment xml:lang="en">The unlawful killing of one human being by another, especially with premeditated malice.</rdfs:comment>
  </owl:Class>
  <owl:Class rdf:about="jc3iedm_ACTIONExtended.owl#ACTION-EVENT_Communications_activation">
    <rdfs:subClassOf rdf:resource="jc3iedm_ACTION.owl#ACTION-EVENT"/>
    <rdfs:subClassOf>
      <owl:Restriction>
        <owl:hasValue xml:lang="en">COMACT</owl:hasValue>
        <owl:onProperty rdf:resource="jc3iedm_ACTION.owl#action-event-category-code"/>
      </owl:Restriction>
    </rdfs:subClassOf>
    <rdfs:label xml:lang="en">communications activation</rdfs:label>
    <rdfs:comment xml:lang="en">The enabling of transmission of information.</rdfs:comment>
  </owl:Class>
  <owl:Class rdf:about="jc3iedm_ACTIONExtended.owl#ACTION-EVENT_Surveillance__electronic">
    <rdfs:subClassOf rdf:resource="jc3iedm_ACTION.owl#ACTION-EVENT"/>
    <rdfs:subClassOf>
      <owl:Restriction>
        <owl:hasValue xml:lang="en">SURVEL</owl:hasValue>
        <owl:onProperty rdf:resource="jc3iedm_ACTION.owl#action-event-category-code"/>
      </owl:Restriction>
    </rdfs:subClassOf>
    <rdfs:label xml:lang="en">surveillance, electronic</rdfs:label>
    <rdfs:comment xml:lang="en">The systematic observation of aerospace, surface or subsurface areas, places, persons, or things, by electronic means.</rdfs:comment>
  </owl:Class>
  <owl:Class rdf:about="jc3iedm_ACTIONExtended.owl#ACTION-EVENT_Civil_demonstration__illegal">
    <rdfs:subClassOf rdf:resource="jc3iedm_ACTION.owl#ACTION-EVENT"/>
    <rdfs:subClassOf>
      <owl:Restriction>
        <owl:hasValue xml:lang="en">CIVDMI</owl:hasValue>
        <owl:onProperty rdf:resource="jc3iedm_ACTION.owl#action-event-category-code"/>
      </owl:Restriction>
    </rdfs:subClassOf>
    <rdfs:label xml:lang="en">civil demonstration, illegal</rdfs:label>
    <rdfs:comment xml:lang="en">A public meeting or march illegally expressing protest or other opinion on an issue.</rdfs:comment>
  </owl:Class>
  <owl:Class rdf:about="jc3iedm_ACTIONExtended.owl#ACTION-EVENT_Breaching">
    <rdfs:subClassOf rdf:resource="jc3iedm_ACTION.owl#ACTION-EVENT"/>
    <rdfs:subClassOf>
      <owl:Restriction>
        <owl:hasValue xml:lang="en">BREACH</owl:hasValue>
        <owl:onProperty rdf:resource="jc3iedm_ACTION.owl#action-event-category-code"/>
      </owl:Restriction>
    </rdfs:subClassOf>
    <rdfs:label xml:lang="en">breaching</rdfs:label>
    <rdfs:comment xml:lang="en">Breaking through or securing a passage through an enemy defence, obstacle, minefield, or fortification.</rdfs:comment>
  </owl:Class>
  <owl:Class rdf:about="jc3iedm_ACTIONExtended.owl#ACTION-EVENT_Genocide">
    <rdfs:subClassOf rdf:resource="jc3iedm_ACTION.owl#ACTION-EVENT"/>
    <rdfs:subClassOf>
      <owl:Restriction>
        <owl:hasValue xml:lang="en">GENOCD</owl:hasValue>
        <owl:onProperty rdf:resource="jc3iedm_ACTION.owl#action-event-category-code"/>
      </owl:Restriction>
    </rdfs:subClassOf>
    <rdfs:label xml:lang="en">genocide</rdfs:label>
    <rdfs:comment xml:lang="en">The deliberated and systematic destruction of a racial, political or cultural group.</rdfs:comment>
  </owl:Class>
  <owl:Class rdf:about="jc3iedm_ACTIONExtended.owl#ACTION-EVENT_Network_seizure">
    <rdfs:subClassOf rdf:resource="jc3iedm_ACTION.owl#ACTION-EVENT"/>
    <rdfs:subClassOf>
      <owl:Restriction>
        <owl:hasValue xml:lang="en">NETSEI</owl:hasValue>
        <owl:onProperty rdf:resource="jc3iedm_ACTION.owl#action-event-category-code"/>
      </owl:Restriction>
    </rdfs:subClassOf>
    <rdfs:label xml:lang="en">network seizure</rdfs:label>
    <rdfs:comment xml:lang="en">Taking electronic control of a communications network.</rdfs:comment>
  </owl:Class>
  <owl:Class rdf:about="jc3iedm_ACTIONExtended.owl#ACTION-EVENT_Neutralize__combat">
    <rdfs:subClassOf rdf:resource="jc3iedm_ACTION.owl#ACTION-EVENT"/>
    <rdfs:subClassOf>
      <owl:Restriction>
        <owl:hasValue xml:lang="en">NTRCOM</owl:hasValue>
        <owl:onProperty rdf:resource="jc3iedm_ACTION.owl#action-event-category-code"/>
      </owl:Restriction>
    </rdfs:subClassOf>
    <rdfs:label xml:lang="en">neutralize, combat</rdfs:label>
    <rdfs:comment xml:lang="en">Rendering ineffective or unusable in military operations.</rdfs:comment>
  </owl:Class>
  <owl:Class rdf:about="jc3iedm_ACTIONExtended.owl#ACTION-EVENT_Hijacking__plane">
    <rdfs:subClassOf rdf:resource="jc3iedm_ACTION.owl#ACTION-EVENT"/>
    <rdfs:subClassOf>
      <owl:Restriction>
        <owl:hasValue xml:lang="en">HJCKPL</owl:hasValue>
        <owl:onProperty rdf:resource="jc3iedm_ACTION.owl#action-event-category-code"/>
      </owl:Restriction>
    </rdfs:subClassOf>
    <rdfs:label xml:lang="en">hijacking, plane</rdfs:label>
    <rdfs:comment xml:lang="en">Seizure of an aircraft in order to go somewhere other than the scheduled destination.</rdfs:comment>
  </owl:Class>
  <owl:Class rdf:about="jc3iedm_ACTIONExtended.owl#ACTION-EVENT_National_state_of_emergency">
    <rdfs:subClassOf rdf:resource="jc3iedm_ACTION.owl#ACTION-EVENT"/>
    <rdfs:subClassOf>
      <owl:Restriction>
        <owl:hasValue xml:lang="en">NATEMG</owl:hasValue>
        <owl:onProperty rdf:resource="jc3iedm_ACTION.owl#action-event-category-code"/>
      </owl:Restriction>
    </rdfs:subClassOf>
    <rdfs:label xml:lang="en">national state of emergency</rdfs:label>
    <rdfs:comment xml:lang="en">A political term, to describe a condition approximating to that of war, wherein the normal constitution is suspended.</rdfs:comment>
  </owl:Class>
  <owl:Class rdf:about="jc3iedm_ACTIONExtended.owl#ACTION-EVENT_Destroying">
    <rdfs:subClassOf rdf:resource="jc3iedm_ACTION.owl#ACTION-EVENT"/>
    <rdfs:subClassOf>
      <owl:Restriction>
        <owl:hasValue xml:lang="en">DSTRYN</owl:hasValue>
        <owl:onProperty rdf:resource="jc3iedm_ACTION.owl#action-event-category-code"/>
      </owl:Restriction>
    </rdfs:subClassOf>
    <rdfs:label xml:lang="en">destroying</rdfs:label>
    <rdfs:comment xml:lang="en">Physically rendering an enemy force combat-ineffective or damaging a target so that it cannot function as intended, nor be restored to a usable condition without being entirely rebuilt.</rdfs:comment>
  </owl:Class>
  <owl:Class rdf:about="jc3iedm_ACTIONExtended.owl#ACTION-EVENT_Reorganising">
    <rdfs:subClassOf rdf:resource="jc3iedm_ACTION.owl#ACTION-EVENT"/>
    <rdfs:subClassOf>
      <owl:Restriction>
        <owl:hasValue xml:lang="en">REORGN</owl:hasValue>
        <owl:onProperty rdf:resource="jc3iedm_ACTION.owl#action-event-category-code"/>
      </owl:Restriction>
    </rdfs:subClassOf>
    <rdfs:label xml:lang="en">reorganising</rdfs:label>
    <rdfs:comment xml:lang="en">Changing a task organisation for a particular operation. (Normally takes place before an operation). This includes the transfer of authority.</rdfs:comment>
  </owl:Class>
  <owl:Class rdf:about="jc3iedm_ACTIONExtended.owl#ACTION-EVENT_Codeword_execution">
    <rdfs:subClassOf rdf:resource="jc3iedm_ACTION.owl#ACTION-EVENT"/>
    <rdfs:subClassOf>
      <owl:Restriction>
        <owl:hasValue xml:lang="en">CDWDEX</owl:hasValue>
        <owl:onProperty rdf:resource="jc3iedm_ACTION.owl#action-event-category-code"/>
      </owl:Restriction>
    </rdfs:subClassOf>
    <rdfs:label xml:lang="en">codeword execution</rdfs:label>
    <rdfs:comment xml:lang="en">Initiating the codeword activity.</rdfs:comment>
  </owl:Class>
  <owl:Class rdf:about="jc3iedm_ACTIONExtended.owl#ACTION-EVENT_Arms_production">
    <rdfs:subClassOf rdf:resource="jc3iedm_ACTION.owl#ACTION-EVENT"/>
    <rdfs:subClassOf>
      <owl:Restriction>
        <owl:hasValue xml:lang="en">ARMPRD</owl:hasValue>
        <owl:onProperty rdf:resource="jc3iedm_ACTION.owl#action-event-category-code"/>
      </owl:Restriction>
    </rdfs:subClassOf>
    <rdfs:label xml:lang="en">arms production</rdfs:label>
    <rdfs:comment xml:lang="en">An activity of, relating to or based on the production of arms.</rdfs:comment>
  </owl:Class>
  <owl:Class rdf:about="jc3iedm_ACTIONExtended.owl#ACTION-EVENT_Sniper_attack">
    <rdfs:subClassOf rdf:resource="jc3iedm_ACTION.owl#ACTION-EVENT"/>
    <rdfs:subClassOf>
      <owl:Restriction>
        <owl:hasValue xml:lang="en">SNPATK</owl:hasValue>
        <owl:onProperty rdf:resource="jc3iedm_ACTION.owl#action-event-category-code"/>
      </owl:Restriction>
    </rdfs:subClassOf>
    <rdfs:label xml:lang="en">sniper attack</rdfs:label>
    <rdfs:comment xml:lang="en">An attack by one who shoots at others from a concealed place.</rdfs:comment>
  </owl:Class>
  <owl:Class rdf:about="jc3iedm_ACTIONExtended.owl#ACTION-EVENT_Exploitation">
    <rdfs:subClassOf rdf:resource="jc3iedm_ACTION.owl#ACTION-EVENT"/>
    <rdfs:subClassOf>
      <owl:Restriction>
        <owl:hasValue xml:lang="en">EXPLTN</owl:hasValue>
        <owl:onProperty rdf:resource="jc3iedm_ACTION.owl#action-event-category-code"/>
      </owl:Restriction>
    </rdfs:subClassOf>
    <rdfs:label xml:lang="en">exploitation</rdfs:label>
    <rdfs:comment xml:lang="en">Taking advantage of a successful attack by mounting an offensive operation to follow-up and harass a dislocated enemy with the aim of further disorganising him in depth. This may provide the opportunity to capture ground that was not part of the objective of the original attack.</rdfs:comment>
  </owl:Class>
  <owl:Class rdf:about="jc3iedm_ACTIONExtended.owl#REQUEST_Type">
    <rdfs:subClassOf rdf:resource="jc3iedm_ACTION.owl#REQUEST"/>
    <rdfs:subClassOf>
      <owl:Restriction>
        <owl:hasValue xml:lang="en">TYPE</owl:hasValue>
        <owl:onProperty rdf:resource="jc3iedm_ACTION.owl#request-category-code"/>
      </owl:Restriction>
    </rdfs:subClassOf>
    <rdfs:label xml:lang="en">type</rdfs:label>
    <rdfs:comment xml:lang="en">To recognise the type of an ACTION-OBJECTIVE (OBJECT-ITEM) by any means.</rdfs:comment>
  </owl:Class>
  <owl:Class rdf:about="jc3iedm_ACTIONExtended.owl#ACTION-EVENT_Booby_trap_discovery">
    <rdfs:subClassOf rdf:resource="jc3iedm_ACTION.owl#ACTION-EVENT"/>
    <rdfs:subClassOf>
      <owl:Restriction>
        <owl:hasValue xml:lang="en">BBYTRD</owl:hasValue>
        <owl:onProperty rdf:resource="jc3iedm_ACTION.owl#action-event-category-code"/>
      </owl:Restriction>
    </rdfs:subClassOf>
    <rdfs:label xml:lang="en">booby trap discovery</rdfs:label>
    <rdfs:comment xml:lang="en">The detection of a device intended to cause damage to unsuspecting people.</rdfs:comment>
  </owl:Class>
  <owl:Class rdf:about="jc3iedm_ACTIONExtended.owl#ACTION-EVENT_Civil_disobedience">
    <rdfs:subClassOf rdf:resource="jc3iedm_ACTION.owl#ACTION-EVENT"/>
    <rdfs:subClassOf>
      <owl:Restriction>
        <owl:hasValue xml:lang="en">CIVDIS</owl:hasValue>
        <owl:onProperty rdf:resource="jc3iedm_ACTION.owl#action-event-category-code"/>
      </owl:Restriction>
    </rdfs:subClassOf>
    <rdfs:label xml:lang="en">civil disobedience</rdfs:label>
    <rdfs:comment xml:lang="en">The refusal to comply with certain laws or to pay taxes etc. as a peaceful form of political protest.</rdfs:comment>
  </owl:Class>
  <owl:Class rdf:about="jc3iedm_ACTIONExtended.owl#ACTION-EVENT_Proxy-bombing">
    <rdfs:subClassOf rdf:resource="jc3iedm_ACTION.owl#ACTION-EVENT"/>
    <rdfs:subClassOf>
      <owl:Restriction>
        <owl:hasValue xml:lang="en">PRXBMB</owl:hasValue>
        <owl:onProperty rdf:resource="jc3iedm_ACTION.owl#action-event-category-code"/>
      </owl:Restriction>
    </rdfs:subClassOf>
    <rdfs:label xml:lang="en">proxy bombing</rdfs:label>
    <rdfs:comment xml:lang="en">A deliberate and intentional bombing incident that happens unexpectedly where the perpetrator acts through a representative.</rdfs:comment>
  </owl:Class>
  <owl:Class rdf:about="jc3iedm_ACTIONExtended.owl#ACTION-EVENT_Mine-laying">
    <rdfs:subClassOf rdf:resource="jc3iedm_ACTION.owl#ACTION-EVENT"/>
    <rdfs:subClassOf>
      <owl:Restriction>
        <owl:hasValue xml:lang="en">MINLAY</owl:hasValue>
        <owl:onProperty rdf:resource="jc3iedm_ACTION.owl#action-event-category-code"/>
      </owl:Restriction>
    </rdfs:subClassOf>
    <rdfs:label xml:lang="en">mine laying</rdfs:label>
    <rdfs:comment xml:lang="en">Emplacement or deployment of one or more mines.</rdfs:comment>
  </owl:Class>
  <owl:Class rdf:about="jc3iedm_ACTIONExtended.owl#ACTION-EVENT_Invasion">
    <rdfs:subClassOf rdf:resource="jc3iedm_ACTION.owl#ACTION-EVENT"/>
    <rdfs:subClassOf>
      <owl:Restriction>
        <owl:hasValue xml:lang="en">INVASI</owl:hasValue>
        <owl:onProperty rdf:resource="jc3iedm_ACTION.owl#action-event-category-code"/>
      </owl:Restriction>
    </rdfs:subClassOf>
    <rdfs:label xml:lang="en">invasion</rdfs:label>
    <rdfs:comment xml:lang="en">The act of taking possession of another land.</rdfs:comment>
  </owl:Class>
  <owl:Class rdf:about="jc3iedm_ACTIONExtended.owl#ACTION-EVENT_Forced_landing">
    <rdfs:subClassOf rdf:resource="jc3iedm_ACTION.owl#ACTION-EVENT"/>
    <rdfs:subClassOf>
      <owl:Restriction>
        <owl:hasValue xml:lang="en">FRCLND</owl:hasValue>
        <owl:onProperty rdf:resource="jc3iedm_ACTION.owl#action-event-category-code"/>
      </owl:Restriction>
    </rdfs:subClassOf>
    <rdfs:label xml:lang="en">forced landing</rdfs:label>
    <rdfs:comment xml:lang="en">An aircraft that by hostile act, or lack of vital resources is compelled to land.</rdfs:comment>
  </owl:Class>
  <owl:Class rdf:about="jc3iedm_ACTIONExtended.owl#ACTION-EVENT_Clearing__radio_net">
    <rdfs:subClassOf rdf:resource="jc3iedm_ACTION.owl#ACTION-EVENT"/>
    <rdfs:subClassOf>
      <owl:Restriction>
        <owl:hasValue xml:lang="en">CLRRAD</owl:hasValue>
        <owl:onProperty rdf:resource="jc3iedm_ACTION.owl#action-event-category-code"/>
      </owl:Restriction>
    </rdfs:subClassOf>
    <rdfs:label xml:lang="en">clearing, radio net</rdfs:label>
    <rdfs:comment xml:lang="en">Eliminating transmissions on a tactical radio net in order to allow a higher precedence transmission to occur.</rdfs:comment>
  </owl:Class>
  <owl:Class rdf:about="jc3iedm_ACTIONExtended.owl#ACTION-EVENT_Drug_operation">
    <rdfs:subClassOf rdf:resource="jc3iedm_ACTION.owl#ACTION-EVENT"/>
    <rdfs:subClassOf>
      <owl:Restriction>
        <owl:hasValue xml:lang="en">DRGOPR</owl:hasValue>
        <owl:onProperty rdf:resource="jc3iedm_ACTION.owl#action-event-category-code"/>
      </owl:Restriction>
    </rdfs:subClassOf>
    <rdfs:label xml:lang="en">drug operation</rdfs:label>
    <rdfs:comment xml:lang="en">Illegal trafficking in drugs by a group or an organisation.</rdfs:comment>
  </owl:Class>
  <owl:Class rdf:about="jc3iedm_ACTIONExtended.owl#ACTION-EVENT_Local_election">
    <rdfs:subClassOf rdf:resource="jc3iedm_ACTION.owl#ACTION-EVENT"/>
    <rdfs:subClassOf>
      <owl:Restriction>
        <owl:hasValue xml:lang="en">LOCELC</owl:hasValue>
        <owl:onProperty rdf:resource="jc3iedm_ACTION.owl#action-event-category-code"/>
      </owl:Restriction>
    </rdfs:subClassOf>
    <rdfs:label xml:lang="en">local election</rdfs:label>
    <rdfs:comment xml:lang="en">An ACTION-EVENT in which local officials are selected by vote.</rdfs:comment>
  </owl:Class>
  <owl:Class rdf:about="jc3iedm_ACTIONExtended.owl#ACTION-EVENT_Resupplying">
    <rdfs:subClassOf rdf:resource="jc3iedm_ACTION.owl#ACTION-EVENT"/>
    <rdfs:subClassOf>
      <owl:Restriction>
        <owl:hasValue xml:lang="en">RESPLN</owl:hasValue>
        <owl:onProperty rdf:resource="jc3iedm_ACTION.owl#action-event-category-code"/>
      </owl:Restriction>
    </rdfs:subClassOf>
    <rdfs:label xml:lang="en">resupplying</rdfs:label>
    <rdfs:comment xml:lang="en">Replenishing stocks in order to maintain the required levels of supply.</rdfs:comment>
  </owl:Class>
  <owl:Class rdf:about="jc3iedm_ACTIONExtended.owl#ACTION-EVENT_Conducting_social_events">
    <rdfs:subClassOf rdf:resource="jc3iedm_ACTION.owl#ACTION-EVENT"/>
    <rdfs:subClassOf>
      <owl:Restriction>
        <owl:hasValue xml:lang="en">CNDSCL</owl:hasValue>
        <owl:onProperty rdf:resource="jc3iedm_ACTION.owl#action-event-category-code"/>
      </owl:Restriction>
    </rdfs:subClassOf>
    <rdfs:label xml:lang="en">conducting social events</rdfs:label>
    <rdfs:comment xml:lang="en">Conducting any social gathering, esp. one organised by a club or congregation.</rdfs:comment>
  </owl:Class>
  <owl:Class rdf:about="jc3iedm_ACTIONExtended.owl#ACTION-EVENT_Distributing">
    <rdfs:subClassOf rdf:resource="jc3iedm_ACTION.owl#ACTION-EVENT"/>
    <rdfs:subClassOf>
      <owl:Restriction>
        <owl:hasValue xml:lang="en">DSTRBT</owl:hasValue>
        <owl:onProperty rdf:resource="jc3iedm_ACTION.owl#action-event-category-code"/>
      </owl:Restriction>
    </rdfs:subClassOf>
    <rdfs:label xml:lang="en">distributing</rdfs:label>
    <rdfs:comment xml:lang="en">Dividing or dispensing in portions.</rdfs:comment>
  </owl:Class>
  <owl:Class rdf:about="jc3iedm_ACTIONExtended.owl#ACTION-EVENT_Deception__electronic">
    <rdfs:subClassOf rdf:resource="jc3iedm_ACTION.owl#ACTION-EVENT"/>
    <rdfs:subClassOf>
      <owl:Restriction>
        <owl:hasValue xml:lang="en">DCPTEL</owl:hasValue>
        <owl:onProperty rdf:resource="jc3iedm_ACTION.owl#action-event-category-code"/>
      </owl:Restriction>
    </rdfs:subClassOf>
    <rdfs:label xml:lang="en">deception, electronic</rdfs:label>
    <rdfs:comment xml:lang="en">In electronic countermeasures, the deliberate radiation, re-radiation, alteration, absorption or reflection of electromagnetic energy in a manner intended to confuse, distract or seduce an enemy or his electronic systems.</rdfs:comment>
  </owl:Class>
  <owl:Class rdf:about="jc3iedm_ACTIONExtended.owl#ACTION-EVENT_Communications_outage">
    <rdfs:subClassOf rdf:resource="jc3iedm_ACTION.owl#ACTION-EVENT"/>
    <rdfs:subClassOf>
      <owl:Restriction>
        <owl:hasValue xml:lang="en">COMOUT</owl:hasValue>
        <owl:onProperty rdf:resource="jc3iedm_ACTION.owl#action-event-category-code"/>
      </owl:Restriction>
    </rdfs:subClassOf>
    <rdfs:label xml:lang="en">communications outage</rdfs:label>
    <rdfs:comment xml:lang="en">The failure of communications equipment due to a mechanical malfunction.</rdfs:comment>
  </owl:Class>
  <owl:Restriction>
    <owl:hasValue xml:lang="en">CHMBIO</owl:hasValue>
    <owl:onProperty rdf:resource="jc3iedm_ACTION.owl#cbrn-event-category-code"/>
  </owl:Restriction>
  <owl:Restriction>
    <owl:hasValue xml:lang="en">RADCTV</owl:hasValue>
    <owl:onProperty rdf:resource="jc3iedm_ACTION.owl#cbrn-event-category-code"/>
  </owl:Restriction>
  <owl:Restriction>
    <owl:hasValue xml:lang="en">RADEVT</owl:hasValue>
    <owl:onProperty rdf:resource="jc3iedm_ACTION.owl#radioactive-event-category-code"/>
  </owl:Restriction>
  <owl:Restriction>
    <owl:hasValue xml:lang="en">RQT</owl:hasValue>
    <owl:onProperty rdf:resource="jc3iedm_ACTION.owl#action-task-category-code"/>
  </owl:Restriction>
  <owl:Restriction>
    <owl:hasValue xml:lang="en">NUCWEP</owl:hasValue>
    <owl:onProperty rdf:resource="jc3iedm_ACTION.owl#nuclear-event-category-code"/>
  </owl:Restriction>
  <owl:Restriction>
    <owl:hasValue xml:lang="en">CBRN</owl:hasValue>
    <owl:onProperty rdf:resource="jc3iedm_ACTION.owl#action-event-category-code"/>
  </owl:Restriction>
  <owl:Restriction>
    <owl:hasValue xml:lang="en">ACTTA</owl:hasValue>
    <owl:onProperty rdf:resource="jc3iedm_ACTION.owl#action-category-code"/>
  </owl:Restriction>
  <owl:Restriction>
    <owl:hasValue xml:lang="en">NUCEVT</owl:hasValue>
    <owl:onProperty rdf:resource="jc3iedm_ACTION.owl#radioactive-event-category-code"/>
  </owl:Restriction>
  <owl:Restriction>
    <owl:hasValue xml:lang="en">ACTEV</owl:hasValue>
    <owl:onProperty rdf:resource="jc3iedm_ACTION.owl#action-category-code"/>
  </owl:Restriction>
</rdf:RDF>
