<rdf:RDF
    xmlns:rdf="http://www.w3.org/1999/02/22-rdf-syntax-ns#"
    xmlns="http://cbml.googlecode.com/svn/trunk/jc3iedmOnt/rootClassOnt/jc3iedm_CAPABILITYSuperExtended.owl#"
    xmlns:owl="http://www.w3.org/2002/07/owl#"
    xmlns:xsd="http://www.w3.org/2001/XMLSchema#"
    xmlns:rdfs="http://www.w3.org/2000/01/rdf-schema#"
  xml:base="http://cbml.googlecode.com/svn/trunk/jc3iedmOnt/rootClassOnt/jc3iedm_CAPABILITYSuperExtended.owl#" > 
  <rdf:Description rdf:about="jc3iedm_CAPABILITYExtended.owl#OPERATIONAL-CAPABILITY_Mountain">
    <rdf:type rdf:resource="http://www.w3.org/2002/07/owl#Class"/>
    <rdfs:comment xml:lang="en">The capability to conduct military operations in mountainous areas.</rdfs:comment>
    <rdfs:label xml:lang="en">mountain</rdfs:label>
    <rdfs:subClassOf rdf:nodeID="A0"/>
    <rdfs:subClassOf rdf:resource="jc3iedm_CAPABILITY.owl#OPERATIONAL-CAPABILITY"/>
  </rdf:Description>
  <rdf:Description rdf:nodeID="A1">
    <rdf:type rdf:resource="http://www.w3.org/2002/07/owl#Restriction"/>
    <owl:onProperty rdf:resource="jc3iedm_CAPABILITY.owl#maintenance-capability-category-code"/>
    <owl:hasValue xml:lang="en">Steelwork fabrication</owl:hasValue>
  </rdf:Description>
  <rdf:Description rdf:nodeID="A2">
    <rdf:type rdf:resource="http://www.w3.org/2002/07/owl#Restriction"/>
    <owl:onProperty rdf:resource="jc3iedm_CAPABILITY.owl#operational-capability-category-code"/>
    <owl:hasValue xml:lang="en">Air interdiction</owl:hasValue>
  </rdf:Description>
  <rdf:Description rdf:nodeID="A3">
    <rdf:type rdf:resource="http://www.w3.org/2002/07/owl#Restriction"/>
    <owl:onProperty rdf:resource="jc3iedm_CAPABILITY.owl#operational-capability-category-code"/>
    <owl:hasValue xml:lang="en">Electronic warfare</owl:hasValue>
  </rdf:Description>
  <rdf:Description rdf:nodeID="A4">
    <rdf:type rdf:resource="http://www.w3.org/2002/07/owl#Restriction"/>
    <owl:onProperty rdf:resource="jc3iedm_CAPABILITY.owl#operational-capability-category-code"/>
    <owl:hasValue xml:lang="en">Medical evacuation</owl:hasValue>
  </rdf:Description>
  <rdf:Description rdf:nodeID="A5">
    <rdf:type rdf:resource="http://www.w3.org/2002/07/owl#Restriction"/>
    <owl:onProperty rdf:resource="jc3iedm_CAPABILITY.owl#support-capability-category-code"/>
    <owl:hasValue xml:lang="en">Supply (class IV)</owl:hasValue>
  </rdf:Description>
  <rdf:Description rdf:nodeID="A6">
    <rdf:type rdf:resource="http://www.w3.org/2002/07/owl#Restriction"/>
    <owl:onProperty rdf:resource="jc3iedm_CAPABILITY.owl#mobility-capability-category-code"/>
    <owl:hasValue xml:lang="en">Water, fjord</owl:hasValue>
  </rdf:Description>
  <rdf:Description rdf:about="jc3iedm_CAPABILITYExtended.owl#MAINTENANCE-CAPABILITY_Shipwright">
    <rdf:type rdf:resource="http://www.w3.org/2002/07/owl#Class"/>
    <rdfs:comment xml:lang="en">Equipment and resources for the construction, fitting and repairing the wooden parts of a docked vessel.</rdfs:comment>
    <rdfs:label xml:lang="en">shipwright</rdfs:label>
    <rdfs:subClassOf rdf:nodeID="A7"/>
    <rdfs:subClassOf rdf:resource="jc3iedm_CAPABILITY.owl#MAINTENANCE-CAPABILITY"/>
  </rdf:Description>
  <rdf:Description rdf:about="jc3iedm_CAPABILITY.owl#storage-capability-cargo-category-code">
    <rdfs:range rdf:resource="http://www.w3.org/2001/XMLSchema#string"/>
    <rdfs:domain rdf:resource="jc3iedm_CAPABILITY.owl#STORAGE-CAPABILITY"/>
    <rdf:type rdf:resource="http://www.w3.org/2002/07/owl#DatatypeProperty"/>
  </rdf:Description>
  <rdf:Description rdf:nodeID="A8">
    <rdf:type rdf:resource="http://www.w3.org/2002/07/owl#Restriction"/>
    <owl:onProperty rdf:resource="jc3iedm_CAPABILITY.owl#maintenance-capability-category-code"/>
    <owl:hasValue xml:lang="en">Steam</owl:hasValue>
  </rdf:Description>
  <rdf:Description rdf:about="jc3iedm_CAPABILITY.owl#storage-capability-descriptor-code">
    <rdfs:range rdf:resource="http://www.w3.org/2001/XMLSchema#string"/>
    <rdfs:domain rdf:resource="jc3iedm_CAPABILITY.owl#STORAGE-CAPABILITY"/>
    <rdf:type rdf:resource="http://www.w3.org/2002/07/owl#DatatypeProperty"/>
  </rdf:Description>
  <rdf:Description rdf:nodeID="A9">
    <rdf:type rdf:resource="http://www.w3.org/2002/07/owl#Restriction"/>
    <owl:onProperty rdf:resource="jc3iedm_CAPABILITY.owl#surveillance-capability-category-code"/>
    <owl:hasValue xml:lang="en">Imaging</owl:hasValue>
  </rdf:Description>
  <rdf:Description rdf:nodeID="A10">
    <rdf:type rdf:resource="http://www.w3.org/2002/07/owl#Restriction"/>
    <owl:onProperty rdf:resource="jc3iedm_CAPABILITY.owl#support-capability-category-code"/>
    <owl:hasValue xml:lang="en">Education</owl:hasValue>
  </rdf:Description>
  <rdf:Description rdf:nodeID="A11">
    <rdf:type rdf:resource="http://www.w3.org/2002/07/owl#Restriction"/>
    <owl:onProperty rdf:resource="jc3iedm_CAPABILITY.owl#support-capability-category-code"/>
    <owl:hasValue xml:lang="en">Healthcare</owl:hasValue>
  </rdf:Description>
  <rdf:Description rdf:nodeID="A12">
    <rdf:type rdf:resource="http://www.w3.org/2002/07/owl#Restriction"/>
    <owl:onProperty rdf:resource="jc3iedm_CAPABILITY.owl#transmission-capability-category-code"/>
    <owl:hasValue xml:lang="en">Transceive</owl:hasValue>
  </rdf:Description>
  <rdf:Description rdf:about="jc3iedm_CAPABILITYExtended.owl#SURVEILLANCE-CAPABILITY_Not_known">
    <rdf:type rdf:resource="http://www.w3.org/2002/07/owl#Class"/>
    <rdfs:comment xml:lang="en">It is not possible to determine which value is most applicable.</rdfs:comment>
    <rdfs:label xml:lang="en">not known</rdfs:label>
    <rdfs:subClassOf rdf:nodeID="A13"/>
    <rdfs:subClassOf rdf:resource="jc3iedm_CAPABILITY.owl#SURVEILLANCE-CAPABILITY"/>
  </rdf:Description>
  <rdf:Description rdf:about="jc3iedm_CAPABILITYExtended.owl#OPERATIONAL-CAPABILITY_Mortuary/graves_registry">
    <rdf:type rdf:resource="http://www.w3.org/2002/07/owl#Class"/>
    <rdfs:comment xml:lang="en">The capability to provide care and disposition of deceased personnel.</rdfs:comment>
    <rdfs:label xml:lang="en">mortuary/graves registry</rdfs:label>
    <rdfs:subClassOf rdf:nodeID="A14"/>
    <rdfs:subClassOf rdf:resource="jc3iedm_CAPABILITY.owl#OPERATIONAL-CAPABILITY"/>
  </rdf:Description>
  <rdf:Description rdf:about="jc3iedm_CAPABILITYExtended.owl#OPERATIONAL-CAPABILITY_Electronic_warfare,_intercept">
    <rdf:type rdf:resource="http://www.w3.org/2002/07/owl#Class"/>
    <rdfs:comment xml:lang="en">The capability to intercept intentional or unintentional radiated electromagnetic energy for the purpose of immediate threat recognition.</rdfs:comment>
    <rdfs:label xml:lang="en">electronic warfare, intercept</rdfs:label>
    <rdfs:subClassOf rdf:nodeID="A15"/>
    <rdfs:subClassOf rdf:resource="jc3iedm_CAPABILITY.owl#OPERATIONAL-CAPABILITY"/>
  </rdf:Description>
  <rdf:Description rdf:nodeID="A16">
    <rdf:type rdf:resource="http://www.w3.org/2002/07/owl#Restriction"/>
    <owl:onProperty rdf:resource="jc3iedm_CAPABILITY.owl#support-capability-category-code"/>
    <owl:hasValue xml:lang="en">Compressed air</owl:hasValue>
  </rdf:Description>
  <rdf:Description rdf:nodeID="A17">
    <rdf:type rdf:resource="http://www.w3.org/2002/07/owl#Restriction"/>
    <owl:onProperty rdf:resource="jc3iedm_CAPABILITY.owl#operational-capability-category-code"/>
    <owl:hasValue xml:lang="en">Labour</owl:hasValue>
  </rdf:Description>
  <rdf:Description rdf:nodeID="A18">
    <rdf:type rdf:resource="http://www.w3.org/2002/07/owl#Restriction"/>
    <owl:onProperty rdf:resource="jc3iedm_CAPABILITY.owl#support-capability-category-code"/>
    <owl:hasValue xml:lang="en">Electrical</owl:hasValue>
  </rdf:Description>
  <rdf:Description rdf:nodeID="A19">
    <rdf:type rdf:resource="http://www.w3.org/2002/07/owl#Restriction"/>
    <owl:onProperty rdf:resource="jc3iedm_CAPABILITY.owl#operational-capability-category-code"/>
    <owl:hasValue xml:lang="en">Supply (water)</owl:hasValue>
  </rdf:Description>
  <rdf:Description rdf:nodeID="A20">
    <rdf:type rdf:resource="http://www.w3.org/2002/07/owl#Restriction"/>
    <owl:onProperty rdf:resource="jc3iedm_CAPABILITY.owl#operational-capability-category-code"/>
    <owl:hasValue xml:lang="en">Reconnaissance</owl:hasValue>
  </rdf:Description>
  <rdf:Description rdf:about="jc3iedm_CAPABILITYExtended.owl#OPERATIONAL-CAPABILITY_Personnel_services">
    <rdf:type rdf:resource="http://www.w3.org/2002/07/owl#Class"/>
    <rdfs:comment xml:lang="en">The capability to provide the support services needed by military and civilian personnel.</rdfs:comment>
    <rdfs:label xml:lang="en">personnel services</rdfs:label>
    <rdfs:subClassOf rdf:nodeID="A21"/>
    <rdfs:subClassOf rdf:resource="jc3iedm_CAPABILITY.owl#OPERATIONAL-CAPABILITY"/>
  </rdf:Description>
  <rdf:Description rdf:nodeID="A22">
    <rdf:type rdf:resource="http://www.w3.org/2002/07/owl#Restriction"/>
    <owl:onProperty rdf:resource="jc3iedm_CAPABILITY.owl#fire-capability-category-code"/>
    <owl:hasValue xml:lang="en">Ground to sea</owl:hasValue>
  </rdf:Description>
  <rdf:Description rdf:about="jc3iedm_CAPABILITYExtended.owl#MOBILITY-CAPABILITY_Arctic">
    <rdf:type rdf:resource="http://www.w3.org/2002/07/owl#Class"/>
    <rdfs:comment xml:lang="en">The capability to move on or through ice.</rdfs:comment>
    <rdfs:label xml:lang="en">arctic</rdfs:label>
    <rdfs:subClassOf rdf:nodeID="A23"/>
    <rdfs:subClassOf rdf:resource="jc3iedm_CAPABILITY.owl#MOBILITY-CAPABILITY"/>
  </rdf:Description>
  <rdf:Description rdf:nodeID="A24">
    <owl:hasValue xml:lang="en">MAINTENANCE-CAPABILITY</owl:hasValue>
    <owl:onProperty rdf:resource="jc3iedm_CAPABILITY.owl#capability-category-code"/>
    <rdf:type rdf:resource="http://www.w3.org/2002/07/owl#Restriction"/>
  </rdf:Description>
  <rdf:Description rdf:about="jc3iedm_CAPABILITYExtended.owl#OPERATIONAL-CAPABILITY_Transportation,_SPOD/SPOE">
    <rdf:type rdf:resource="http://www.w3.org/2002/07/owl#Class"/>
    <rdfs:comment xml:lang="en">The capability to provide transportation services at seaports where cargo or personnel arrive or depart.</rdfs:comment>
    <rdfs:label xml:lang="en">transportation, spod/spoe</rdfs:label>
    <rdfs:subClassOf rdf:nodeID="A25"/>
    <rdfs:subClassOf rdf:resource="jc3iedm_CAPABILITY.owl#OPERATIONAL-CAPABILITY"/>
  </rdf:Description>
  <rdf:Description rdf:nodeID="A26">
    <rdf:type rdf:resource="http://www.w3.org/2002/07/owl#Restriction"/>
    <owl:onProperty rdf:resource="jc3iedm_CAPABILITY.owl#capability-category-code"/>
    <owl:hasValue xml:lang="en">TRANSMISSION-CAPABILITY</owl:hasValue>
  </rdf:Description>
  <rdf:Description rdf:nodeID="A27">
    <rdf:type rdf:resource="http://www.w3.org/2002/07/owl#Restriction"/>
    <owl:onProperty rdf:resource="jc3iedm_CAPABILITY.owl#operational-capability-category-code"/>
    <owl:hasValue xml:lang="en">Recovery</owl:hasValue>
  </rdf:Description>
  <rdf:Description rdf:nodeID="A28">
    <rdf:type rdf:resource="http://www.w3.org/2002/07/owl#Restriction"/>
    <owl:onProperty rdf:resource="jc3iedm_CAPABILITY.owl#fire-capability-category-code"/>
    <owl:hasValue xml:lang="en">Air to air</owl:hasValue>
  </rdf:Description>
  <rdf:Description rdf:nodeID="A29">
    <rdf:type rdf:resource="http://www.w3.org/2002/07/owl#Restriction"/>
    <owl:onProperty rdf:resource="jc3iedm_CAPABILITY.owl#support-capability-category-code"/>
    <owl:hasValue xml:lang="en">Supply (class I)</owl:hasValue>
  </rdf:Description>
  <rdf:Description rdf:nodeID="A30">
    <rdf:type rdf:resource="http://www.w3.org/2002/07/owl#Restriction"/>
    <owl:onProperty rdf:resource="jc3iedm_CAPABILITY.owl#support-capability-category-code"/>
    <owl:hasValue xml:lang="en">Helicopter platform</owl:hasValue>
  </rdf:Description>
  <rdf:Description rdf:nodeID="A31">
    <rdf:type rdf:resource="http://www.w3.org/2002/07/owl#Restriction"/>
    <owl:onProperty rdf:resource="jc3iedm_CAPABILITY.owl#mobility-capability-category-code"/>
    <owl:hasValue xml:lang="en">Land, self-propelled</owl:hasValue>
  </rdf:Description>
  <rdf:Description rdf:nodeID="A32">
    <rdf:type rdf:resource="http://www.w3.org/2002/07/owl#Restriction"/>
    <owl:onProperty rdf:resource="jc3iedm_CAPABILITY.owl#operational-capability-category-code"/>
    <owl:hasValue xml:lang="en">Public affairs</owl:hasValue>
  </rdf:Description>
  <rdf:Description rdf:about="jc3iedm_CAPABILITY.owl#engineering-capability-facility-length-dimension">
    <rdfs:domain rdf:resource="jc3iedm_CAPABILITY.owl#ENGINEERING-CAPABILITY"/>
    <rdf:type rdf:resource="http://www.w3.org/2002/07/owl#DatatypeProperty"/>
  </rdf:Description>
  <rdf:Description rdf:about="jc3iedm_CAPABILITYExtended.owl#OPERATIONAL-CAPABILITY_Railway">
    <rdf:type rdf:resource="http://www.w3.org/2002/07/owl#Class"/>
    <rdfs:comment xml:lang="en">The capability to provide rail services.</rdfs:comment>
    <rdfs:label xml:lang="en">railway</rdfs:label>
    <rdfs:subClassOf rdf:nodeID="A33"/>
    <rdfs:subClassOf rdf:resource="jc3iedm_CAPABILITY.owl#OPERATIONAL-CAPABILITY"/>
  </rdf:Description>
  <rdf:Description rdf:about="jc3iedm_CAPABILITYExtended.owl#MOBILITY-CAPABILITY_Land,_wheeled">
    <rdf:type rdf:resource="http://www.w3.org/2002/07/owl#Class"/>
    <rdfs:comment xml:lang="en">The capability of a device to move on wheels.</rdfs:comment>
    <rdfs:label xml:lang="en">land, wheeled</rdfs:label>
    <rdfs:subClassOf rdf:nodeID="A34"/>
    <rdfs:subClassOf rdf:resource="jc3iedm_CAPABILITY.owl#MOBILITY-CAPABILITY"/>
  </rdf:Description>
  <rdf:Description rdf:nodeID="A23">
    <rdf:type rdf:resource="http://www.w3.org/2002/07/owl#Restriction"/>
    <owl:onProperty rdf:resource="jc3iedm_CAPABILITY.owl#mobility-capability-category-code"/>
    <owl:hasValue xml:lang="en">Arctic</owl:hasValue>
  </rdf:Description>
  <rdf:Description rdf:about="jc3iedm_CAPABILITYExtended.owl#SUPPORT-CAPABILITY_Supply_(class_II)">
    <rdf:type rdf:resource="http://www.w3.org/2002/07/owl#Class"/>
    <rdfs:comment xml:lang="en">The capability to provide materiel (supplies for which allowances are established by tables of organisation and equipment).</rdfs:comment>
    <rdfs:label xml:lang="en">supply (class ii)</rdfs:label>
    <rdfs:subClassOf rdf:nodeID="A35"/>
    <rdfs:subClassOf rdf:resource="jc3iedm_CAPABILITY.owl#SUPPORT-CAPABILITY"/>
  </rdf:Description>
  <rdf:Description rdf:about="jc3iedm_CAPABILITYExtended.owl#SUPPORT-CAPABILITY_Infrastructure_support">
    <rdf:type rdf:resource="http://www.w3.org/2002/07/owl#Class"/>
    <rdfs:comment xml:lang="en">The capability to provide infrastructure support.</rdfs:comment>
    <rdfs:label xml:lang="en">infrastructure support</rdfs:label>
    <rdfs:subClassOf rdf:nodeID="A36"/>
    <rdfs:subClassOf rdf:resource="jc3iedm_CAPABILITY.owl#SUPPORT-CAPABILITY"/>
  </rdf:Description>
  <rdf:Description rdf:nodeID="A37">
    <rdf:type rdf:resource="http://www.w3.org/2002/07/owl#Restriction"/>
    <owl:onProperty rdf:resource="jc3iedm_CAPABILITY.owl#operational-capability-category-code"/>
    <owl:hasValue xml:lang="en">Target acquisition, sound</owl:hasValue>
  </rdf:Description>
  <rdf:Description rdf:about="jc3iedm_CAPABILITYExtended.owl#SUPPORT-CAPABILITY_Compressed_air">
    <rdf:type rdf:resource="http://www.w3.org/2002/07/owl#Class"/>
    <rdfs:comment xml:lang="en">The capability to provide air at more than atmospheric pressure - often used to power mechanical devices or to provide a portable supply of oxygen.</rdfs:comment>
    <rdfs:label xml:lang="en">compressed air</rdfs:label>
    <rdfs:subClassOf rdf:nodeID="A16"/>
    <rdfs:subClassOf rdf:resource="jc3iedm_CAPABILITY.owl#SUPPORT-CAPABILITY"/>
  </rdf:Description>
  <rdf:Description rdf:about="jc3iedm_CAPABILITYExtended.owl#OPERATIONAL-CAPABILITY_Electronic_warfare">
    <rdf:type rdf:resource="http://www.w3.org/2002/07/owl#Class"/>
    <rdfs:comment xml:lang="en">The capability involving the use of electromagnetic energy to determine, exploit, reduce, or prevent hostile use of the electromagnetic spectrum and action to retain its effective use by friendly forces.</rdfs:comment>
    <rdfs:label xml:lang="en">electronic warfare</rdfs:label>
    <rdfs:subClassOf rdf:nodeID="A3"/>
    <rdfs:subClassOf rdf:resource="jc3iedm_CAPABILITY.owl#OPERATIONAL-CAPABILITY"/>
  </rdf:Description>
  <rdf:Description rdf:nodeID="A38">
    <rdf:type rdf:resource="http://www.w3.org/2002/07/owl#Restriction"/>
    <owl:onProperty rdf:resource="jc3iedm_CAPABILITY.owl#capability-category-code"/>
    <owl:hasValue xml:lang="en">SURVEILLANCE-CAPABILITY</owl:hasValue>
  </rdf:Description>
  <rdf:Description rdf:about="jc3iedm_CAPABILITYExtended.owl#OPERATIONAL-CAPABILITY_Counter_intelligence">
    <rdf:type rdf:resource="http://www.w3.org/2002/07/owl#Class"/>
    <rdfs:comment xml:lang="en">The capability to conduct activities that are concerned with identifying and counteracting the threat to security posed by hostile intelligence services or organisations, or by individuals engaged in espionage, sabotage, subversion or terrorism.</rdfs:comment>
    <rdfs:label xml:lang="en">counter intelligence</rdfs:label>
    <rdfs:subClassOf rdf:nodeID="A39"/>
    <rdfs:subClassOf rdf:resource="jc3iedm_CAPABILITY.owl#OPERATIONAL-CAPABILITY"/>
  </rdf:Description>
  <rdf:Description rdf:about="jc3iedm_CAPABILITYExtended.owl#SURVEILLANCE-CAPABILITY_Signal">
    <rdf:type rdf:resource="http://www.w3.org/2002/07/owl#Class"/>
    <rdfs:comment xml:lang="en">The ability to gain information from exploiting EMS (not imagery) systems.</rdfs:comment>
    <rdfs:label xml:lang="en">signal</rdfs:label>
    <rdfs:subClassOf rdf:nodeID="A40"/>
    <rdfs:subClassOf rdf:resource="jc3iedm_CAPABILITY.owl#SURVEILLANCE-CAPABILITY"/>
  </rdf:Description>
  <rdf:Description rdf:about="jc3iedm_CAPABILITYExtended.owl#OPERATIONAL-CAPABILITY_Air_assault">
    <rdf:type rdf:resource="http://www.w3.org/2002/07/owl#Class"/>
    <rdfs:comment xml:lang="en">The capability to perform a mission involving total integration of helicopter assets in their ground or air roles.</rdfs:comment>
    <rdfs:label xml:lang="en">air assault</rdfs:label>
    <rdfs:subClassOf rdf:nodeID="A41"/>
    <rdfs:subClassOf rdf:resource="jc3iedm_CAPABILITY.owl#OPERATIONAL-CAPABILITY"/>
  </rdf:Description>
  <rdf:Description rdf:nodeID="A42">
    <rdf:type rdf:resource="http://www.w3.org/2002/07/owl#Restriction"/>
    <owl:onProperty rdf:resource="jc3iedm_CAPABILITY.owl#operational-capability-category-code"/>
    <owl:hasValue xml:lang="en">NBC, chemical decontamination</owl:hasValue>
  </rdf:Description>
  <rdf:Description rdf:nodeID="A43">
    <rdf:type rdf:resource="http://www.w3.org/2002/07/owl#Restriction"/>
    <owl:onProperty rdf:resource="jc3iedm_CAPABILITY.owl#surveillance-capability-category-code"/>
    <owl:hasValue xml:lang="en">Human</owl:hasValue>
  </rdf:Description>
  <rdf:Description rdf:nodeID="A44">
    <rdf:type rdf:resource="http://www.w3.org/2002/07/owl#Restriction"/>
    <owl:onProperty rdf:resource="jc3iedm_CAPABILITY.owl#maintenance-capability-category-code"/>
    <owl:hasValue xml:lang="en">Navigational equipment</owl:hasValue>
  </rdf:Description>
  <rdf:Description rdf:nodeID="A45">
    <rdf:type rdf:resource="http://www.w3.org/2002/07/owl#Restriction"/>
    <owl:onProperty rdf:resource="jc3iedm_CAPABILITY.owl#operational-capability-category-code"/>
    <owl:hasValue xml:lang="en">NBC, biological</owl:hasValue>
  </rdf:Description>
  <rdf:Description rdf:nodeID="A46">
    <rdf:type rdf:resource="http://www.w3.org/2002/07/owl#Restriction"/>
    <owl:onProperty rdf:resource="jc3iedm_CAPABILITY.owl#surveillance-capability-category-code"/>
    <owl:hasValue xml:lang="en">Not otherwise specified</owl:hasValue>
  </rdf:Description>
  <rdf:Description rdf:about="jc3iedm_CAPABILITYExtended.owl#OPERATIONAL-CAPABILITY_Legal">
    <rdf:type rdf:resource="http://www.w3.org/2002/07/owl#Class"/>
    <rdfs:comment xml:lang="en">The capability to provide legal services.</rdfs:comment>
    <rdfs:label xml:lang="en">legal</rdfs:label>
    <rdfs:subClassOf rdf:nodeID="A47"/>
    <rdfs:subClassOf rdf:resource="jc3iedm_CAPABILITY.owl#OPERATIONAL-CAPABILITY"/>
  </rdf:Description>
  <rdf:Description rdf:nodeID="A48">
    <rdf:type rdf:resource="http://www.w3.org/2002/07/owl#Restriction"/>
    <owl:onProperty rdf:resource="jc3iedm_CAPABILITY.owl#support-capability-category-code"/>
    <owl:hasValue xml:lang="en">Laundry</owl:hasValue>
  </rdf:Description>
  <rdf:Description rdf:about="jc3iedm_CAPABILITY.owl#maintenance-capability-category-code">
    <rdfs:range rdf:resource="http://www.w3.org/2001/XMLSchema#string"/>
    <rdfs:domain rdf:resource="jc3iedm_CAPABILITY.owl#MAINTENANCE-CAPABILITY"/>
    <rdf:type rdf:resource="http://www.w3.org/2002/07/owl#DatatypeProperty"/>
  </rdf:Description>
  <rdf:Description rdf:about="jc3iedm_CAPABILITYExtended.owl#MOBILITY-CAPABILITY_Airborne">
    <rdf:type rdf:resource="http://www.w3.org/2002/07/owl#Class"/>
    <rdfs:comment xml:lang="en">The capability to be employed, following transport by air, in an assault debarkation either by parachuting or touchdown.</rdfs:comment>
    <rdfs:label xml:lang="en">airborne</rdfs:label>
    <rdfs:subClassOf rdf:nodeID="A49"/>
    <rdfs:subClassOf rdf:resource="jc3iedm_CAPABILITY.owl#MOBILITY-CAPABILITY"/>
  </rdf:Description>
  <rdf:Description rdf:nodeID="A36">
    <rdf:type rdf:resource="http://www.w3.org/2002/07/owl#Restriction"/>
    <owl:onProperty rdf:resource="jc3iedm_CAPABILITY.owl#support-capability-category-code"/>
    <owl:hasValue xml:lang="en">Infrastructure support</owl:hasValue>
  </rdf:Description>
  <rdf:Description rdf:about="jc3iedm_CAPABILITYExtended.owl#OPERATIONAL-CAPABILITY_Civilian_law_enforcement">
    <rdf:type rdf:resource="http://www.w3.org/2002/07/owl#Class"/>
    <rdfs:comment xml:lang="en">The capability to conduct civilian law enforcement operations.</rdfs:comment>
    <rdfs:label xml:lang="en">civilian law enforcement</rdfs:label>
    <rdfs:subClassOf rdf:nodeID="A50"/>
    <rdfs:subClassOf rdf:resource="jc3iedm_CAPABILITY.owl#OPERATIONAL-CAPABILITY"/>
  </rdf:Description>
  <rdf:Description rdf:nodeID="A51">
    <rdf:type rdf:resource="http://www.w3.org/2002/07/owl#Restriction"/>
    <owl:onProperty rdf:resource="jc3iedm_CAPABILITY.owl#support-capability-category-code"/>
    <owl:hasValue xml:lang="en">Shelter</owl:hasValue>
  </rdf:Description>
  <rdf:Description rdf:about="jc3iedm_CAPABILITYExtended.owl#OPERATIONAL-CAPABILITY_Maintenance,_ordnance">
    <rdf:type rdf:resource="http://www.w3.org/2002/07/owl#Class"/>
    <rdfs:comment xml:lang="en">The capability to maintain ordnance (ammunition) in or to restore it to a specified condition.</rdfs:comment>
    <rdfs:label xml:lang="en">maintenance, ordnance</rdfs:label>
    <rdfs:subClassOf rdf:nodeID="A52"/>
    <rdfs:subClassOf rdf:resource="jc3iedm_CAPABILITY.owl#OPERATIONAL-CAPABILITY"/>
  </rdf:Description>
  <rdf:Description rdf:about="jc3iedm_CAPABILITYExtended.owl#MAINTENANCE-CAPABILITY_Steam">
    <rdf:type rdf:resource="http://www.w3.org/2002/07/owl#Class"/>
    <rdfs:comment xml:lang="en">The specific MAINTENANCE-CAPABILITY determines the ability to provide steam repair.</rdfs:comment>
    <rdfs:label xml:lang="en">steam</rdfs:label>
    <rdfs:subClassOf rdf:nodeID="A8"/>
    <rdfs:subClassOf rdf:resource="jc3iedm_CAPABILITY.owl#MAINTENANCE-CAPABILITY"/>
  </rdf:Description>
  <rdf:Description rdf:about="jc3iedm_CAPABILITYExtended.owl#FIRE-CAPABILITY_Ground_to_sea">
    <rdf:type rdf:resource="http://www.w3.org/2002/07/owl#Class"/>
    <rdfs:comment xml:lang="en">The specific value implies that a specific FIRE-CAPABILITY involves firing from the ground to targets at sea.</rdfs:comment>
    <rdfs:label xml:lang="en">ground to sea</rdfs:label>
    <rdfs:subClassOf rdf:nodeID="A22"/>
    <rdfs:subClassOf rdf:resource="jc3iedm_CAPABILITY.owl#FIRE-CAPABILITY"/>
  </rdf:Description>
  <rdf:Description rdf:about="jc3iedm_CAPABILITY.owl#engineering-capability-category-code">
    <rdfs:range rdf:resource="http://www.w3.org/2001/XMLSchema#string"/>
    <rdfs:domain rdf:resource="jc3iedm_CAPABILITY.owl#ENGINEERING-CAPABILITY"/>
    <rdf:type rdf:resource="http://www.w3.org/2002/07/owl#DatatypeProperty"/>
  </rdf:Description>
  <rdf:Description rdf:nodeID="A53">
    <rdf:type rdf:resource="http://www.w3.org/2002/07/owl#Restriction"/>
    <owl:onProperty rdf:resource="jc3iedm_CAPABILITY.owl#operational-capability-category-code"/>
    <owl:hasValue xml:lang="en">Transportation, APOD/APOE</owl:hasValue>
  </rdf:Description>
  <rdf:Description rdf:about="jc3iedm_CAPABILITYExtended.owl#SURVEILLANCE-CAPABILITY_Not_otherwise_specified">
    <rdf:type rdf:resource="http://www.w3.org/2002/07/owl#Class"/>
    <rdfs:comment xml:lang="en">The appropriate value is not in the set of specified values.</rdfs:comment>
    <rdfs:label xml:lang="en">not otherwise specified</rdfs:label>
    <rdfs:subClassOf rdf:nodeID="A46"/>
    <rdfs:subClassOf rdf:resource="jc3iedm_CAPABILITY.owl#SURVEILLANCE-CAPABILITY"/>
  </rdf:Description>
  <rdf:Description rdf:nodeID="A54">
    <rdf:type rdf:resource="http://www.w3.org/2002/07/owl#Restriction"/>
    <owl:onProperty rdf:resource="jc3iedm_CAPABILITY.owl#support-capability-category-code"/>
    <owl:hasValue xml:lang="en">Sewage</owl:hasValue>
  </rdf:Description>
  <rdf:Description rdf:about="jc3iedm_CAPABILITYExtended.owl#OPERATIONAL-CAPABILITY_Surveillance">
    <rdf:type rdf:resource="http://www.w3.org/2002/07/owl#Class"/>
    <rdfs:comment xml:lang="en">The capability to perform systematic observation of aerospace, surface or subsurface areas, places, persons, or things by visual, aural, electronic, photographic, or other means.</rdfs:comment>
    <rdfs:label xml:lang="en">surveillance</rdfs:label>
    <rdfs:subClassOf rdf:nodeID="A55"/>
    <rdfs:subClassOf rdf:resource="jc3iedm_CAPABILITY.owl#OPERATIONAL-CAPABILITY"/>
  </rdf:Description>
  <rdf:Description rdf:about="jc3iedm_CAPABILITYExtended.owl#FIRE-CAPABILITY_Air_to_ground">
    <rdf:type rdf:resource="http://www.w3.org/2002/07/owl#Class"/>
    <rdfs:comment xml:lang="en">The specific value implies that a specific FIRE-CAPABILITY involves firing from aircraft at targets on the ground.</rdfs:comment>
    <rdfs:label xml:lang="en">air to ground</rdfs:label>
    <rdfs:subClassOf rdf:nodeID="A56"/>
    <rdfs:subClassOf rdf:resource="jc3iedm_CAPABILITY.owl#FIRE-CAPABILITY"/>
  </rdf:Description>
  <rdf:Description rdf:about="jc3iedm_CAPABILITYExtended.owl#MOBILITY-CAPABILITY_Military_load_classification">
    <rdf:type rdf:resource="http://www.w3.org/2002/07/owl#Class"/>
    <rdfs:comment xml:lang="en">The characteristics, required for planning, of those CONTROL-FEATUREs, FACILITYs and MATERIELs or CONTROL-FEATURE-TYPEs, FACILITY-TYPEs and EQUIPMENT-TYPEs, and ORGANISATION-TYPEs that represents the standard system in which a route, bridge or raft is assigned class number(s) representing the load it can carry. Vehicles are also assigned number(s) indicating the minimum class of route, bridge or raft they are authorized to use.</rdfs:comment>
    <rdfs:label xml:lang="en">military load classification</rdfs:label>
    <rdfs:subClassOf rdf:nodeID="A57"/>
    <rdfs:subClassOf rdf:resource="jc3iedm_CAPABILITY.owl#MOBILITY-CAPABILITY"/>
  </rdf:Description>
  <rdf:Description rdf:nodeID="A58">
    <rdf:type rdf:resource="http://www.w3.org/2002/07/owl#Restriction"/>
    <owl:onProperty rdf:resource="jc3iedm_CAPABILITY.owl#operational-capability-category-code"/>
    <owl:hasValue xml:lang="en">Maritime</owl:hasValue>
  </rdf:Description>
  <rdf:Description rdf:nodeID="A59">
    <rdf:type rdf:resource="http://www.w3.org/2002/07/owl#Restriction"/>
    <owl:onProperty rdf:resource="jc3iedm_CAPABILITY.owl#operational-capability-category-code"/>
    <owl:hasValue xml:lang="en">Interrogation</owl:hasValue>
  </rdf:Description>
  <rdf:Description rdf:about="jc3iedm_CAPABILITYExtended.owl#MOBILITY-CAPABILITY_Water,_lake">
    <rdf:type rdf:resource="http://www.w3.org/2002/07/owl#Class"/>
    <rdfs:comment xml:lang="en">The capability of a device to navigate lakes.</rdfs:comment>
    <rdfs:label xml:lang="en">water, lake</rdfs:label>
    <rdfs:subClassOf rdf:nodeID="A60"/>
    <rdfs:subClassOf rdf:resource="jc3iedm_CAPABILITY.owl#MOBILITY-CAPABILITY"/>
  </rdf:Description>
  <rdf:Description rdf:about="jc3iedm_CAPABILITYExtended.owl#FIRE-CAPABILITY_Sea_to_sea">
    <rdf:type rdf:resource="http://www.w3.org/2002/07/owl#Class"/>
    <rdfs:comment xml:lang="en">The specific value implies that a specific FIRE-CAPABILITY involves firing from a vessel to targets at sea.</rdfs:comment>
    <rdfs:label xml:lang="en">sea to sea</rdfs:label>
    <rdfs:subClassOf rdf:nodeID="A61"/>
    <rdfs:subClassOf rdf:resource="jc3iedm_CAPABILITY.owl#FIRE-CAPABILITY"/>
  </rdf:Description>
  <rdf:Description rdf:nodeID="A62">
    <rdf:type rdf:resource="http://www.w3.org/2002/07/owl#Restriction"/>
    <owl:onProperty rdf:resource="jc3iedm_CAPABILITY.owl#mobility-capability-category-code"/>
    <owl:hasValue xml:lang="en">Air, composite</owl:hasValue>
  </rdf:Description>
  <rdf:Description rdf:about="jc3iedm_CAPABILITYExtended.owl#OPERATIONAL-CAPABILITY_NBC,_chemical,_smoke">
    <rdf:type rdf:resource="http://www.w3.org/2002/07/owl#Class"/>
    <rdfs:comment xml:lang="en">The capability to employ chemical materiel released as a cloud of smoke or defence against such employment.</rdfs:comment>
    <rdfs:label xml:lang="en">nbc, chemical, smoke</rdfs:label>
    <rdfs:subClassOf rdf:nodeID="A63"/>
    <rdfs:subClassOf rdf:resource="jc3iedm_CAPABILITY.owl#OPERATIONAL-CAPABILITY"/>
  </rdf:Description>
  <rdf:Description rdf:nodeID="A64">
    <rdf:type rdf:resource="http://www.w3.org/2002/07/owl#Restriction"/>
    <owl:onProperty rdf:resource="jc3iedm_CAPABILITY.owl#support-capability-category-code"/>
    <owl:hasValue xml:lang="en">Personal equipment</owl:hasValue>
  </rdf:Description>
  <rdf:Description rdf:about="jc3iedm_CAPABILITYExtended.owl#FIRE-CAPABILITY_Air_to_sea">
    <rdf:type rdf:resource="http://www.w3.org/2002/07/owl#Class"/>
    <rdfs:comment xml:lang="en">The specific value implies that a specific FIRE-CAPABILITY involves firing from aircraft at targets at sea.</rdfs:comment>
    <rdfs:label xml:lang="en">air to sea</rdfs:label>
    <rdfs:subClassOf rdf:nodeID="A65"/>
    <rdfs:subClassOf rdf:resource="jc3iedm_CAPABILITY.owl#FIRE-CAPABILITY"/>
  </rdf:Description>
  <rdf:Description rdf:about="jc3iedm_CAPABILITYExtended.owl#OPERATIONAL-CAPABILITY_Peace_support">
    <rdf:type rdf:resource="http://www.w3.org/2002/07/owl#Class"/>
    <rdfs:comment xml:lang="en">The capability to conduct multi-functional operations involving military forces and diplomatic and humanitarian agencies. The operations are designed to achieve humanitarian goals or a long term peace settlement.</rdfs:comment>
    <rdfs:label xml:lang="en">peace support</rdfs:label>
    <rdfs:subClassOf rdf:nodeID="A66"/>
    <rdfs:subClassOf rdf:resource="jc3iedm_CAPABILITY.owl#OPERATIONAL-CAPABILITY"/>
  </rdf:Description>
  <rdf:Description rdf:nodeID="A67">
    <rdf:type rdf:resource="http://www.w3.org/2002/07/owl#Restriction"/>
    <owl:onProperty rdf:resource="jc3iedm_CAPABILITY.owl#operational-capability-category-code"/>
    <owl:hasValue xml:lang="en">Signal, node, small extension</owl:hasValue>
  </rdf:Description>
  <rdf:Description rdf:about="jc3iedm_CAPABILITYExtended.owl#ENGINEERING-CAPABILITY_Demolition">
    <rdf:type rdf:resource="http://www.w3.org/2002/07/owl#Class"/>
    <rdfs:comment xml:lang="en">The action or process of demolishing or being demolished.</rdfs:comment>
    <rdfs:label xml:lang="en">demolition</rdfs:label>
    <rdfs:subClassOf rdf:nodeID="A68"/>
    <rdfs:subClassOf rdf:resource="jc3iedm_CAPABILITY.owl#ENGINEERING-CAPABILITY"/>
  </rdf:Description>
  <rdf:Description rdf:about="jc3iedm_CAPABILITYExtended.owl#MOBILITY-CAPABILITY_Land,_towed">
    <rdf:type rdf:resource="http://www.w3.org/2002/07/owl#Class"/>
    <rdfs:comment xml:lang="en">The capability of a device to move by means of external propulsion (mechanical or animal).</rdfs:comment>
    <rdfs:label xml:lang="en">land, towed</rdfs:label>
    <rdfs:subClassOf rdf:nodeID="A69"/>
    <rdfs:subClassOf rdf:resource="jc3iedm_CAPABILITY.owl#MOBILITY-CAPABILITY"/>
  </rdf:Description>
  <rdf:Description rdf:nodeID="A35">
    <rdf:type rdf:resource="http://www.w3.org/2002/07/owl#Restriction"/>
    <owl:onProperty rdf:resource="jc3iedm_CAPABILITY.owl#support-capability-category-code"/>
    <owl:hasValue xml:lang="en">Supply (class II)</owl:hasValue>
  </rdf:Description>
  <rdf:Description rdf:nodeID="A70">
    <rdf:type rdf:resource="http://www.w3.org/2002/07/owl#Restriction"/>
    <owl:onProperty rdf:resource="jc3iedm_CAPABILITY.owl#operational-capability-category-code"/>
    <owl:hasValue xml:lang="en">Signal, support</owl:hasValue>
  </rdf:Description>
  <rdf:Description rdf:about="jc3iedm_CAPABILITYExtended.owl#OPERATIONAL-CAPABILITY_Transportation,_movement_control">
    <rdf:type rdf:resource="http://www.w3.org/2002/07/owl#Class"/>
    <rdfs:comment xml:lang="en">The capability to provide planning, routing, scheduling and control of personnel and freight movements over lines of communication.</rdfs:comment>
    <rdfs:label xml:lang="en">transportation, movement control</rdfs:label>
    <rdfs:subClassOf rdf:nodeID="A71"/>
    <rdfs:subClassOf rdf:resource="jc3iedm_CAPABILITY.owl#OPERATIONAL-CAPABILITY"/>
  </rdf:Description>
  <rdf:Description rdf:nodeID="A72">
    <rdf:type rdf:resource="http://www.w3.org/2002/07/owl#Restriction"/>
    <owl:onProperty rdf:resource="jc3iedm_CAPABILITY.owl#operational-capability-category-code"/>
    <owl:hasValue xml:lang="en">Targeting</owl:hasValue>
  </rdf:Description>
  <rdf:Description rdf:about="jc3iedm_CAPABILITY.owl#capability-unit-of-measure-code">
    <rdfs:range rdf:resource="http://www.w3.org/2001/XMLSchema#string"/>
    <rdfs:domain rdf:resource="jc3iedm_CAPABILITY.owl#CAPABILITY"/>
    <rdf:type rdf:resource="http://www.w3.org/2002/07/owl#DatatypeProperty"/>
  </rdf:Description>
  <rdf:Description rdf:nodeID="A55">
    <rdf:type rdf:resource="http://www.w3.org/2002/07/owl#Restriction"/>
    <owl:onProperty rdf:resource="jc3iedm_CAPABILITY.owl#operational-capability-category-code"/>
    <owl:hasValue xml:lang="en">Surveillance</owl:hasValue>
  </rdf:Description>
  <rdf:Description rdf:about="jc3iedm_CAPABILITYExtended.owl#MAINTENANCE-CAPABILITY_Navigational_equipment">
    <rdf:type rdf:resource="http://www.w3.org/2002/07/owl#Class"/>
    <rdfs:comment xml:lang="en">The specific MAINTENANCE-CAPABILITY determines the ability to provide navigational equipment repair.</rdfs:comment>
    <rdfs:label xml:lang="en">navigational equipment</rdfs:label>
    <rdfs:subClassOf rdf:nodeID="A44"/>
    <rdfs:subClassOf rdf:resource="jc3iedm_CAPABILITY.owl#MAINTENANCE-CAPABILITY"/>
  </rdf:Description>
  <rdf:Description rdf:about="jc3iedm_CAPABILITYExtended.owl#OPERATIONAL-CAPABILITY_Recovery">
    <rdf:type rdf:resource="http://www.w3.org/2002/07/owl#Class"/>
    <rdfs:comment xml:lang="en">The capability to contact, protect and extract personnel, small groups or units, or materiel.</rdfs:comment>
    <rdfs:label xml:lang="en">recovery</rdfs:label>
    <rdfs:subClassOf rdf:nodeID="A27"/>
    <rdfs:subClassOf rdf:resource="jc3iedm_CAPABILITY.owl#OPERATIONAL-CAPABILITY"/>
  </rdf:Description>
  <rdf:Description rdf:about="jc3iedm_CAPABILITYExtended.owl#SUPPORT-CAPABILITY_Electrical">
    <rdf:type rdf:resource="http://www.w3.org/2002/07/owl#Class"/>
    <rdfs:comment xml:lang="en">The capability to provide electrical power.</rdfs:comment>
    <rdfs:label xml:lang="en">electrical</rdfs:label>
    <rdfs:subClassOf rdf:nodeID="A18"/>
    <rdfs:subClassOf rdf:resource="jc3iedm_CAPABILITY.owl#SUPPORT-CAPABILITY"/>
  </rdf:Description>
  <rdf:Description rdf:about="jc3iedm_CAPABILITYExtended.owl#SUPPORT-CAPABILITY_Supply_(class_IV)">
    <rdf:type rdf:resource="http://www.w3.org/2002/07/owl#Class"/>
    <rdfs:comment xml:lang="en">The capability to provide construction materials (supplies for which initial issue allowances are not prescribed by approved issue tables).</rdfs:comment>
    <rdfs:label xml:lang="en">supply (class iv)</rdfs:label>
    <rdfs:subClassOf rdf:nodeID="A5"/>
    <rdfs:subClassOf rdf:resource="jc3iedm_CAPABILITY.owl#SUPPORT-CAPABILITY"/>
  </rdf:Description>
  <rdf:Description rdf:nodeID="A73">
    <rdf:type rdf:resource="http://www.w3.org/2002/07/owl#Restriction"/>
    <owl:onProperty rdf:resource="jc3iedm_CAPABILITY.owl#operational-capability-category-code"/>
    <owl:hasValue xml:lang="en">NBC, chemical</owl:hasValue>
  </rdf:Description>
  <rdf:Description rdf:about="jc3iedm_CAPABILITYExtended.owl#OPERATIONAL-CAPABILITY_Command_operations">
    <rdf:type rdf:resource="http://www.w3.org/2002/07/owl#Class"/>
    <rdfs:comment xml:lang="en">No definition provided in APP-6A.</rdfs:comment>
    <rdfs:label xml:lang="en">command operations</rdfs:label>
    <rdfs:subClassOf rdf:nodeID="A74"/>
    <rdfs:subClassOf rdf:resource="jc3iedm_CAPABILITY.owl#OPERATIONAL-CAPABILITY"/>
  </rdf:Description>
  <rdf:Description rdf:nodeID="A75">
    <rdf:type rdf:resource="http://www.w3.org/2002/07/owl#Restriction"/>
    <owl:onProperty rdf:resource="jc3iedm_CAPABILITY.owl#mobility-capability-category-code"/>
    <owl:hasValue xml:lang="en">Water, sea</owl:hasValue>
  </rdf:Description>
  <rdf:Description rdf:about="jc3iedm_CAPABILITYExtended.owl#OPERATIONAL-CAPABILITY_Maintenance,_electro-optical">
    <rdf:type rdf:resource="http://www.w3.org/2002/07/owl#Class"/>
    <rdfs:comment xml:lang="en">The capability to maintain electro-optical materiel in or to restore it to a specified condition.</rdfs:comment>
    <rdfs:label xml:lang="en">maintenance, electro optical</rdfs:label>
    <rdfs:subClassOf rdf:nodeID="A76"/>
    <rdfs:subClassOf rdf:resource="jc3iedm_CAPABILITY.owl#OPERATIONAL-CAPABILITY"/>
  </rdf:Description>
  <rdf:Description rdf:nodeID="A77">
    <rdf:type rdf:resource="http://www.w3.org/2002/07/owl#Restriction"/>
    <owl:onProperty rdf:resource="jc3iedm_CAPABILITY.owl#transmission-capability-category-code"/>
    <owl:hasValue xml:lang="en">Receive</owl:hasValue>
  </rdf:Description>
  <rdf:Description rdf:about="jc3iedm_CAPABILITY.owl#MOBILITY-CAPABILITY">
    <rdfs:subClassOf rdf:resource="jc3iedm_CAPABILITY.owl#CAPABILITY"/>
    <rdfs:subClassOf rdf:nodeID="A78"/>
    <rdfs:label xml:lang="en">mobility capability</rdfs:label>
    <rdfs:comment xml:lang="en">A CAPABILITY, required for planning, of those FACILITYs, MATERIELs, ORGANISATIONs and PERSONs or FACILITY-TYPEs, EQUIPMENT-TYPEs, ORGANISATION-TYPEs, and PERSON-TYPEs that are deemed as having the nominal ability to move in space, air, on water, under water, or over a specific type of terrain.</rdfs:comment>
    <rdf:type rdf:resource="http://www.w3.org/2002/07/owl#Class"/>
    <rdfs:subClassOf rdf:nodeID="A79"/>
  </rdf:Description>
  <rdf:Description rdf:about="jc3iedm_CAPABILITYExtended.owl#MOBILITY-CAPABILITY_Water,_sea">
    <rdf:type rdf:resource="http://www.w3.org/2002/07/owl#Class"/>
    <rdfs:comment xml:lang="en">The capability of a device to navigate seas.</rdfs:comment>
    <rdfs:label xml:lang="en">water, sea</rdfs:label>
    <rdfs:subClassOf rdf:nodeID="A75"/>
    <rdfs:subClassOf rdf:resource="jc3iedm_CAPABILITY.owl#MOBILITY-CAPABILITY"/>
  </rdf:Description>
  <rdf:Description rdf:nodeID="A57">
    <rdf:type rdf:resource="http://www.w3.org/2002/07/owl#Restriction"/>
    <owl:onProperty rdf:resource="jc3iedm_CAPABILITY.owl#mobility-capability-category-code"/>
    <owl:hasValue xml:lang="en">Military load classification</owl:hasValue>
  </rdf:Description>
  <rdf:Description rdf:about="jc3iedm_CAPABILITYExtended.owl#OPERATIONAL-CAPABILITY_Signal,_node,_small_extension">
    <rdf:type rdf:resource="http://www.w3.org/2002/07/owl#Class"/>
    <rdfs:comment xml:lang="en">The capability in signal services to manage, operate and control a communications small extension node.</rdfs:comment>
    <rdfs:label xml:lang="en">signal, node, small extension</rdfs:label>
    <rdfs:subClassOf rdf:nodeID="A67"/>
    <rdfs:subClassOf rdf:resource="jc3iedm_CAPABILITY.owl#OPERATIONAL-CAPABILITY"/>
  </rdf:Description>
  <rdf:Description rdf:nodeID="A41">
    <rdf:type rdf:resource="http://www.w3.org/2002/07/owl#Restriction"/>
    <owl:onProperty rdf:resource="jc3iedm_CAPABILITY.owl#operational-capability-category-code"/>
    <owl:hasValue xml:lang="en">Air assault</owl:hasValue>
  </rdf:Description>
  <rdf:Description rdf:about="jc3iedm_CAPABILITYExtended.owl#MOBILITY-CAPABILITY_Road_march">
    <rdf:type rdf:resource="http://www.w3.org/2002/07/owl#Class"/>
    <rdfs:comment xml:lang="en">The capability of a formation moving on a road.</rdfs:comment>
    <rdfs:label xml:lang="en">road march</rdfs:label>
    <rdfs:subClassOf rdf:nodeID="A80"/>
    <rdfs:subClassOf rdf:resource="jc3iedm_CAPABILITY.owl#MOBILITY-CAPABILITY"/>
  </rdf:Description>
  <rdf:Description rdf:about="jc3iedm_CAPABILITY.owl#SUPPORT-CAPABILITY">
    <rdfs:subClassOf rdf:resource="jc3iedm_CAPABILITY.owl#CAPABILITY"/>
    <rdfs:subClassOf rdf:nodeID="A81"/>
    <rdfs:label xml:lang="en">support capability</rdfs:label>
    <rdfs:comment xml:lang="en">A CAPABILITY, required for planning, of those FACILITYs, MATERIELs and ORGANISATIONs or FACILITY-TYPEs, EQUIPMENT-TYPEs and ORGANISATION-TYPEs that are deemed as having the ability to provide supplies or services.</rdfs:comment>
    <rdf:type rdf:resource="http://www.w3.org/2002/07/owl#Class"/>
    <rdfs:subClassOf rdf:nodeID="A82"/>
  </rdf:Description>
  <rdf:Description rdf:about="jc3iedm_CAPABILITYExtended.owl#OPERATIONAL-CAPABILITY_Water_purification">
    <rdf:type rdf:resource="http://www.w3.org/2002/07/owl#Class"/>
    <rdfs:comment xml:lang="en">The capability to provide clean potable drinking/bathing water.</rdfs:comment>
    <rdfs:label xml:lang="en">water purification</rdfs:label>
    <rdfs:subClassOf rdf:nodeID="A83"/>
    <rdfs:subClassOf rdf:resource="jc3iedm_CAPABILITY.owl#OPERATIONAL-CAPABILITY"/>
  </rdf:Description>
  <rdf:Description rdf:nodeID="A84">
    <rdf:type rdf:resource="http://www.w3.org/2002/07/owl#Restriction"/>
    <owl:onProperty rdf:resource="jc3iedm_CAPABILITY.owl#operational-capability-category-code"/>
    <owl:hasValue xml:lang="en">Airborne</owl:hasValue>
  </rdf:Description>
  <rdf:Description rdf:nodeID="A85">
    <rdf:type rdf:resource="http://www.w3.org/2002/07/owl#Restriction"/>
    <owl:onProperty rdf:resource="jc3iedm_CAPABILITY.owl#operational-capability-category-code"/>
    <owl:hasValue xml:lang="en">Supply (class V)</owl:hasValue>
  </rdf:Description>
  <rdf:Description rdf:about="jc3iedm_CAPABILITYExtended.owl#MAINTENANCE-CAPABILITY_Shotblast">
    <rdf:type rdf:resource="http://www.w3.org/2002/07/owl#Class"/>
    <rdfs:comment xml:lang="en">Equipment and resources for the cleaning of metal, belonging to a docked vessel, by the impact of a stream of shot (lead pellets).</rdfs:comment>
    <rdfs:label xml:lang="en">shotblast</rdfs:label>
    <rdfs:subClassOf rdf:nodeID="A86"/>
    <rdfs:subClassOf rdf:resource="jc3iedm_CAPABILITY.owl#MAINTENANCE-CAPABILITY"/>
  </rdf:Description>
  <rdf:Description rdf:nodeID="A87">
    <rdf:type rdf:resource="http://www.w3.org/2002/07/owl#Restriction"/>
    <owl:onProperty rdf:resource="jc3iedm_CAPABILITY.owl#support-capability-category-code"/>
    <owl:hasValue xml:lang="en">Medical</owl:hasValue>
  </rdf:Description>
  <rdf:Description rdf:about="jc3iedm_CAPABILITYExtended.owl#SUPPORT-CAPABILITY_Recreation">
    <rdf:type rdf:resource="http://www.w3.org/2002/07/owl#Class"/>
    <rdfs:comment xml:lang="en">The capability to provide recreation services.</rdfs:comment>
    <rdfs:label xml:lang="en">recreation</rdfs:label>
    <rdfs:subClassOf rdf:nodeID="A88"/>
    <rdfs:subClassOf rdf:resource="jc3iedm_CAPABILITY.owl#SUPPORT-CAPABILITY"/>
  </rdf:Description>
  <rdf:Description rdf:about="jc3iedm_CAPABILITYExtended.owl#MOBILITY-CAPABILITY_Water,_fjord">
    <rdf:type rdf:resource="http://www.w3.org/2002/07/owl#Class"/>
    <rdfs:comment xml:lang="en">The capability of a device to navigate fjords.</rdfs:comment>
    <rdfs:label xml:lang="en">water, fjord</rdfs:label>
    <rdfs:subClassOf rdf:nodeID="A6"/>
    <rdfs:subClassOf rdf:resource="jc3iedm_CAPABILITY.owl#MOBILITY-CAPABILITY"/>
  </rdf:Description>
  <rdf:Description rdf:about="jc3iedm_CAPABILITYExtended.owl#OPERATIONAL-CAPABILITY_Supply_(class_III_aviation)">
    <rdf:type rdf:resource="http://www.w3.org/2002/07/owl#Class"/>
    <rdfs:comment xml:lang="en">The capability to provide aviation fuel and lubricants.</rdfs:comment>
    <rdfs:label xml:lang="en">supply (class iii aviation)</rdfs:label>
    <rdfs:subClassOf rdf:nodeID="A89"/>
    <rdfs:subClassOf rdf:resource="jc3iedm_CAPABILITY.owl#OPERATIONAL-CAPABILITY"/>
  </rdf:Description>
  <rdf:Description rdf:nodeID="A74">
    <rdf:type rdf:resource="http://www.w3.org/2002/07/owl#Restriction"/>
    <owl:onProperty rdf:resource="jc3iedm_CAPABILITY.owl#operational-capability-category-code"/>
    <owl:hasValue xml:lang="en">Command operations</owl:hasValue>
  </rdf:Description>
  <rdf:Description rdf:about="jc3iedm_CAPABILITYExtended.owl#OPERATIONAL-CAPABILITY_Targeting">
    <rdf:type rdf:resource="http://www.w3.org/2002/07/owl#Class"/>
    <rdfs:comment xml:lang="en">The capability to provide targeting services.</rdfs:comment>
    <rdfs:label xml:lang="en">targeting</rdfs:label>
    <rdfs:subClassOf rdf:nodeID="A72"/>
    <rdfs:subClassOf rdf:resource="jc3iedm_CAPABILITY.owl#OPERATIONAL-CAPABILITY"/>
  </rdf:Description>
  <rdf:Description rdf:nodeID="A90">
    <rdf:type rdf:resource="http://www.w3.org/2002/07/owl#Restriction"/>
    <owl:onProperty rdf:resource="jc3iedm_CAPABILITY.owl#operational-capability-category-code"/>
    <owl:hasValue xml:lang="en">Air to ground</owl:hasValue>
  </rdf:Description>
  <rdf:Description rdf:nodeID="A56">
    <rdf:type rdf:resource="http://www.w3.org/2002/07/owl#Restriction"/>
    <owl:onProperty rdf:resource="jc3iedm_CAPABILITY.owl#fire-capability-category-code"/>
    <owl:hasValue xml:lang="en">Air to ground</owl:hasValue>
  </rdf:Description>
  <rdf:Description rdf:about="jc3iedm_CAPABILITYExtended.owl#OPERATIONAL-CAPABILITY_Anti-submarine_warfare">
    <rdf:type rdf:resource="http://www.w3.org/2002/07/owl#Class"/>
    <rdfs:comment xml:lang="en">Operations conducted with the intention of denying the enemy the effective use of his submarines.</rdfs:comment>
    <rdfs:label xml:lang="en">anti submarine warfare</rdfs:label>
    <rdfs:subClassOf rdf:nodeID="A91"/>
    <rdfs:subClassOf rdf:resource="jc3iedm_CAPABILITY.owl#OPERATIONAL-CAPABILITY"/>
  </rdf:Description>
  <rdf:Description rdf:about="jc3iedm_CAPABILITY.owl#support-capability-descriptor-code">
    <rdfs:range rdf:resource="http://www.w3.org/2001/XMLSchema#string"/>
    <rdfs:domain rdf:resource="jc3iedm_CAPABILITY.owl#SUPPORT-CAPABILITY"/>
    <rdf:type rdf:resource="http://www.w3.org/2002/07/owl#DatatypeProperty"/>
  </rdf:Description>
  <rdf:Description rdf:about="jc3iedm_CAPABILITY.owl#handling-capability-descriptor-code">
    <rdfs:range rdf:resource="http://www.w3.org/2001/XMLSchema#string"/>
    <rdfs:domain rdf:resource="jc3iedm_CAPABILITY.owl#HANDLING-CAPABILITY"/>
    <rdf:type rdf:resource="http://www.w3.org/2002/07/owl#DatatypeProperty"/>
  </rdf:Description>
  <rdf:Description rdf:nodeID="A92">
    <rdf:type rdf:resource="http://www.w3.org/2002/07/owl#Restriction"/>
    <owl:onProperty rdf:resource="jc3iedm_CAPABILITY.owl#mobility-capability-category-code"/>
    <owl:hasValue xml:lang="en">Water, creek</owl:hasValue>
  </rdf:Description>
  <rdf:Description rdf:nodeID="A89">
    <rdf:type rdf:resource="http://www.w3.org/2002/07/owl#Restriction"/>
    <owl:onProperty rdf:resource="jc3iedm_CAPABILITY.owl#operational-capability-category-code"/>
    <owl:hasValue xml:lang="en">Supply (class III aviation)</owl:hasValue>
  </rdf:Description>
  <rdf:Description rdf:about="jc3iedm_CAPABILITY.owl#handling-capability-cargo-category-code">
    <rdfs:range rdf:resource="http://www.w3.org/2001/XMLSchema#string"/>
    <rdfs:domain rdf:resource="jc3iedm_CAPABILITY.owl#HANDLING-CAPABILITY"/>
    <rdf:type rdf:resource="http://www.w3.org/2002/07/owl#DatatypeProperty"/>
  </rdf:Description>
  <rdf:Description rdf:about="jc3iedm_CAPABILITYExtended.owl#SUPPORT-CAPABILITY_Supply_(class_III)">
    <rdf:type rdf:resource="http://www.w3.org/2002/07/owl#Class"/>
    <rdfs:comment xml:lang="en">The capability to provide fuel and lubricants.</rdfs:comment>
    <rdfs:label xml:lang="en">supply (class iii)</rdfs:label>
    <rdfs:subClassOf rdf:nodeID="A93"/>
    <rdfs:subClassOf rdf:resource="jc3iedm_CAPABILITY.owl#SUPPORT-CAPABILITY"/>
  </rdf:Description>
  <rdf:Description rdf:about="jc3iedm_CAPABILITYExtended.owl#OPERATIONAL-CAPABILITY_Air_defence">
    <rdf:type rdf:resource="http://www.w3.org/2002/07/owl#Class"/>
    <rdfs:comment xml:lang="en">The capability to nullify or reduce the effectiveness of hostile air action.</rdfs:comment>
    <rdfs:label xml:lang="en">air defence</rdfs:label>
    <rdfs:subClassOf rdf:nodeID="A94"/>
    <rdfs:subClassOf rdf:resource="jc3iedm_CAPABILITY.owl#OPERATIONAL-CAPABILITY"/>
  </rdf:Description>
  <rdf:Description rdf:about="jc3iedm_CAPABILITYExtended.owl#TRANSMISSION-CAPABILITY_Transmit">
    <rdf:type rdf:resource="http://www.w3.org/2002/07/owl#Class"/>
    <rdfs:comment xml:lang="en">The ability to broadcast or send out a signal or programme.</rdfs:comment>
    <rdfs:label xml:lang="en">transmit</rdfs:label>
    <rdfs:subClassOf rdf:nodeID="A95"/>
    <rdfs:subClassOf rdf:resource="jc3iedm_CAPABILITY.owl#TRANSMISSION-CAPABILITY"/>
  </rdf:Description>
  <rdf:Description rdf:about="jc3iedm_CAPABILITYExtended.owl#OPERATIONAL-CAPABILITY_Military_intelligence,_aerial_exploitation">
    <rdf:type rdf:resource="http://www.w3.org/2002/07/owl#Class"/>
    <rdfs:comment xml:lang="en">No definition provided in APP-6A.</rdfs:comment>
    <rdfs:label xml:lang="en">military intelligence, aerial exploitation</rdfs:label>
    <rdfs:subClassOf rdf:nodeID="A96"/>
    <rdfs:subClassOf rdf:resource="jc3iedm_CAPABILITY.owl#OPERATIONAL-CAPABILITY"/>
  </rdf:Description>
  <rdf:Description rdf:nodeID="A97">
    <rdf:type rdf:resource="http://www.w3.org/2002/07/owl#Restriction"/>
    <owl:onProperty rdf:resource="jc3iedm_CAPABILITY.owl#operational-capability-category-code"/>
    <owl:hasValue xml:lang="en">Utility</owl:hasValue>
  </rdf:Description>
  <rdf:Description rdf:nodeID="A98">
    <rdf:type rdf:resource="http://www.w3.org/2002/07/owl#Restriction"/>
    <owl:onProperty rdf:resource="jc3iedm_CAPABILITY.owl#support-capability-category-code"/>
    <owl:hasValue xml:lang="en">Deck</owl:hasValue>
  </rdf:Description>
  <rdf:Description rdf:nodeID="A99">
    <rdf:type rdf:resource="http://www.w3.org/2002/07/owl#Restriction"/>
    <owl:onProperty rdf:resource="jc3iedm_CAPABILITY.owl#fire-capability-category-code"/>
    <owl:hasValue xml:lang="en">Ground to air</owl:hasValue>
  </rdf:Description>
  <rdf:Description rdf:about="jc3iedm_CAPABILITYExtended.owl#OPERATIONAL-CAPABILITY_Surveillance,_long_range">
    <rdf:type rdf:resource="http://www.w3.org/2002/07/owl#Class"/>
    <rdfs:comment xml:lang="en">The capability to perform, from long range, systematic observation of aerospace, surface or subsurface areas, places, persons, or things by visual, aural, electronic, photographic, or other means from a ground station.</rdfs:comment>
    <rdfs:label xml:lang="en">surveillance, long range</rdfs:label>
    <rdfs:subClassOf rdf:nodeID="A100"/>
    <rdfs:subClassOf rdf:resource="jc3iedm_CAPABILITY.owl#OPERATIONAL-CAPABILITY"/>
  </rdf:Description>
  <rdf:Description rdf:about="jc3iedm_CAPABILITYExtended.owl#OPERATIONAL-CAPABILITY_NBC,_chemical_decontamination">
    <rdf:type rdf:resource="http://www.w3.org/2002/07/owl#Class"/>
    <rdfs:comment xml:lang="en">The capability to make any person, object, or area safe by absorbing, destroying, neutralizing, making harmless, or removing, chemical materiel.</rdfs:comment>
    <rdfs:label xml:lang="en">nbc, chemical decontamination</rdfs:label>
    <rdfs:subClassOf rdf:nodeID="A42"/>
    <rdfs:subClassOf rdf:resource="jc3iedm_CAPABILITY.owl#OPERATIONAL-CAPABILITY"/>
  </rdf:Description>
  <rdf:Description rdf:about="jc3iedm_CAPABILITYExtended.owl#FIRE-CAPABILITY_Air_to_air">
    <rdf:type rdf:resource="http://www.w3.org/2002/07/owl#Class"/>
    <rdfs:comment xml:lang="en">The specific value implies that a specific FIRE-CAPABILITY involves firing from aircraft at targets in the air.</rdfs:comment>
    <rdfs:label xml:lang="en">air to air</rdfs:label>
    <rdfs:subClassOf rdf:nodeID="A28"/>
    <rdfs:subClassOf rdf:resource="jc3iedm_CAPABILITY.owl#FIRE-CAPABILITY"/>
  </rdf:Description>
  <rdf:Description rdf:nodeID="A101">
    <owl:hasValue xml:lang="en">HANDLING-CAPABILITY</owl:hasValue>
    <owl:onProperty rdf:resource="jc3iedm_CAPABILITY.owl#capability-category-code"/>
    <rdf:type rdf:resource="http://www.w3.org/2002/07/owl#Restriction"/>
  </rdf:Description>
  <rdf:Description rdf:nodeID="A102">
    <rdf:type rdf:resource="http://www.w3.org/2002/07/owl#Restriction"/>
    <owl:onProperty rdf:resource="jc3iedm_CAPABILITY.owl#mobility-capability-category-code"/>
    <owl:hasValue xml:lang="en">Animal, mounted</owl:hasValue>
  </rdf:Description>
  <rdf:Description rdf:nodeID="A100">
    <rdf:type rdf:resource="http://www.w3.org/2002/07/owl#Restriction"/>
    <owl:onProperty rdf:resource="jc3iedm_CAPABILITY.owl#operational-capability-category-code"/>
    <owl:hasValue xml:lang="en">Surveillance, long range</owl:hasValue>
  </rdf:Description>
  <rdf:Description rdf:nodeID="A103">
    <rdf:type rdf:resource="http://www.w3.org/2002/07/owl#Restriction"/>
    <owl:onProperty rdf:resource="jc3iedm_CAPABILITY.owl#operational-capability-category-code"/>
    <owl:hasValue xml:lang="en">Military intelligence, operation</owl:hasValue>
  </rdf:Description>
  <rdf:Description rdf:about="jc3iedm_CAPABILITYExtended.owl#SUPPORT-CAPABILITY_Personal_equipment">
    <rdf:type rdf:resource="http://www.w3.org/2002/07/owl#Class"/>
    <rdfs:comment xml:lang="en">The capability to provide clothing.</rdfs:comment>
    <rdfs:label xml:lang="en">personal equipment</rdfs:label>
    <rdfs:subClassOf rdf:nodeID="A64"/>
    <rdfs:subClassOf rdf:resource="jc3iedm_CAPABILITY.owl#SUPPORT-CAPABILITY"/>
  </rdf:Description>
  <rdf:Description rdf:about="jc3iedm_CAPABILITYExtended.owl#OPERATIONAL-CAPABILITY_Maintenance,_ordnance_missile">
    <rdf:type rdf:resource="http://www.w3.org/2002/07/owl#Class"/>
    <rdfs:comment xml:lang="en">The capability to maintain ordnance missile (materiel) in or to restore it to a specified condition.</rdfs:comment>
    <rdfs:label xml:lang="en">maintenance, ordnance missile</rdfs:label>
    <rdfs:subClassOf rdf:nodeID="A104"/>
    <rdfs:subClassOf rdf:resource="jc3iedm_CAPABILITY.owl#OPERATIONAL-CAPABILITY"/>
  </rdf:Description>
  <rdf:Description rdf:about="jc3iedm_CAPABILITYExtended.owl#OPERATIONAL-CAPABILITY_Utility">
    <rdf:type rdf:resource="http://www.w3.org/2002/07/owl#Class"/>
    <rdfs:comment xml:lang="en">The capability to provide utilities (water, gas, electric, et al).</rdfs:comment>
    <rdfs:label xml:lang="en">utility</rdfs:label>
    <rdfs:subClassOf rdf:nodeID="A97"/>
    <rdfs:subClassOf rdf:resource="jc3iedm_CAPABILITY.owl#OPERATIONAL-CAPABILITY"/>
  </rdf:Description>
  <rdf:Description rdf:nodeID="A60">
    <rdf:type rdf:resource="http://www.w3.org/2002/07/owl#Restriction"/>
    <owl:onProperty rdf:resource="jc3iedm_CAPABILITY.owl#mobility-capability-category-code"/>
    <owl:hasValue xml:lang="en">Water, lake</owl:hasValue>
  </rdf:Description>
  <rdf:Description rdf:nodeID="A7">
    <rdf:type rdf:resource="http://www.w3.org/2002/07/owl#Restriction"/>
    <owl:onProperty rdf:resource="jc3iedm_CAPABILITY.owl#maintenance-capability-category-code"/>
    <owl:hasValue xml:lang="en">Shipwright</owl:hasValue>
  </rdf:Description>
  <rdf:Description rdf:nodeID="A105">
    <rdf:type rdf:resource="http://www.w3.org/2002/07/owl#Restriction"/>
    <owl:onProperty rdf:resource="jc3iedm_CAPABILITY.owl#operational-capability-category-code"/>
    <owl:hasValue xml:lang="en">Morale, welfare recreation</owl:hasValue>
  </rdf:Description>
  <rdf:Description rdf:about="jc3iedm_CAPABILITYExtended.owl#OPERATIONAL-CAPABILITY_Maintenance">
    <rdf:type rdf:resource="http://www.w3.org/2002/07/owl#Class"/>
    <rdfs:comment xml:lang="en">The capability to provide supply and repair services to keep a force in condition to carry out its mission.</rdfs:comment>
    <rdfs:label xml:lang="en">maintenance</rdfs:label>
    <rdfs:subClassOf rdf:nodeID="A106"/>
    <rdfs:subClassOf rdf:resource="jc3iedm_CAPABILITY.owl#OPERATIONAL-CAPABILITY"/>
  </rdf:Description>
  <rdf:Description rdf:about="jc3iedm_CAPABILITY.owl#surveillance-capability-category-code">
    <rdfs:range rdf:resource="http://www.w3.org/2001/XMLSchema#string"/>
    <rdfs:domain rdf:resource="jc3iedm_CAPABILITY.owl#SURVEILLANCE-CAPABILITY"/>
    <rdf:type rdf:resource="http://www.w3.org/2002/07/owl#DatatypeProperty"/>
  </rdf:Description>
  <rdf:Description rdf:nodeID="A61">
    <rdf:type rdf:resource="http://www.w3.org/2002/07/owl#Restriction"/>
    <owl:onProperty rdf:resource="jc3iedm_CAPABILITY.owl#fire-capability-category-code"/>
    <owl:hasValue xml:lang="en">Sea to sea</owl:hasValue>
  </rdf:Description>
  <rdf:Description rdf:about="jc3iedm_CAPABILITYExtended.owl#SUPPORT-CAPABILITY_Food/rations">
    <rdf:type rdf:resource="http://www.w3.org/2002/07/owl#Class"/>
    <rdfs:comment xml:lang="en">The capability to provide food.</rdfs:comment>
    <rdfs:label xml:lang="en">food/rations</rdfs:label>
    <rdfs:subClassOf rdf:nodeID="A107"/>
    <rdfs:subClassOf rdf:resource="jc3iedm_CAPABILITY.owl#SUPPORT-CAPABILITY"/>
  </rdf:Description>
  <rdf:Description rdf:nodeID="A108">
    <rdf:type rdf:resource="http://www.w3.org/2002/07/owl#Restriction"/>
    <owl:onProperty rdf:resource="jc3iedm_CAPABILITY.owl#operational-capability-category-code"/>
    <owl:hasValue xml:lang="en">NBC, decontamination</owl:hasValue>
  </rdf:Description>
  <rdf:Description rdf:about="jc3iedm_CAPABILITYExtended.owl#OPERATIONAL-CAPABILITY_Engineer,_construction">
    <rdf:type rdf:resource="http://www.w3.org/2002/07/owl#Class"/>
    <rdfs:comment xml:lang="en">The capability to build various facilities in direct support of military operations.</rdfs:comment>
    <rdfs:label xml:lang="en">engineer, construction</rdfs:label>
    <rdfs:subClassOf rdf:nodeID="A109"/>
    <rdfs:subClassOf rdf:resource="jc3iedm_CAPABILITY.owl#OPERATIONAL-CAPABILITY"/>
  </rdf:Description>
  <rdf:Description rdf:nodeID="A110">
    <rdf:type rdf:resource="http://www.w3.org/2002/07/owl#Restriction"/>
    <owl:onProperty rdf:resource="jc3iedm_CAPABILITY.owl#operational-capability-category-code"/>
    <owl:hasValue xml:lang="en">Amphibious</owl:hasValue>
  </rdf:Description>
  <rdf:Description rdf:about="jc3iedm_CAPABILITY.owl#engineering-capability-facility-width-dimension">
    <rdfs:domain rdf:resource="jc3iedm_CAPABILITY.owl#ENGINEERING-CAPABILITY"/>
    <rdf:type rdf:resource="http://www.w3.org/2002/07/owl#DatatypeProperty"/>
  </rdf:Description>
  <rdf:Description rdf:about="jc3iedm_CAPABILITYExtended.owl#MOBILITY-CAPABILITY_Water,_tidal">
    <rdf:type rdf:resource="http://www.w3.org/2002/07/owl#Class"/>
    <rdfs:comment xml:lang="en">The capability of a device to navigate tidal waters.</rdfs:comment>
    <rdfs:label xml:lang="en">water, tidal</rdfs:label>
    <rdfs:subClassOf rdf:nodeID="A111"/>
    <rdfs:subClassOf rdf:resource="jc3iedm_CAPABILITY.owl#MOBILITY-CAPABILITY"/>
  </rdf:Description>
  <rdf:Description rdf:nodeID="A52">
    <rdf:type rdf:resource="http://www.w3.org/2002/07/owl#Restriction"/>
    <owl:onProperty rdf:resource="jc3iedm_CAPABILITY.owl#operational-capability-category-code"/>
    <owl:hasValue xml:lang="en">Maintenance, ordnance</owl:hasValue>
  </rdf:Description>
  <rdf:Description rdf:nodeID="A112">
    <rdf:type rdf:resource="http://www.w3.org/2002/07/owl#Restriction"/>
    <owl:onProperty rdf:resource="jc3iedm_CAPABILITY.owl#maintenance-capability-category-code"/>
    <owl:hasValue xml:lang="en">Tank cleaning</owl:hasValue>
  </rdf:Description>
  <rdf:Description rdf:about="jc3iedm_CAPABILITYExtended.owl#OPERATIONAL-CAPABILITY_Military_intelligence,_operation">
    <rdf:type rdf:resource="http://www.w3.org/2002/07/owl#Class"/>
    <rdfs:comment xml:lang="en">The capability to provide information required for the planning and conducting campaigns and major operations to accomplish strategic objectives within theatres or areas of operations.</rdfs:comment>
    <rdfs:label xml:lang="en">military intelligence, operation</rdfs:label>
    <rdfs:subClassOf rdf:nodeID="A103"/>
    <rdfs:subClassOf rdf:resource="jc3iedm_CAPABILITY.owl#OPERATIONAL-CAPABILITY"/>
  </rdf:Description>
  <rdf:Description rdf:nodeID="A113">
    <rdf:type rdf:resource="http://www.w3.org/2002/07/owl#Restriction"/>
    <owl:onProperty rdf:resource="jc3iedm_CAPABILITY.owl#operational-capability-category-code"/>
    <owl:hasValue xml:lang="en">Mine countermeasure</owl:hasValue>
  </rdf:Description>
  <rdf:Description rdf:about="jc3iedm_CAPABILITYExtended.owl#MOBILITY-CAPABILITY_Air,_lighter_than_air">
    <rdf:type rdf:resource="http://www.w3.org/2002/07/owl#Class"/>
    <rdfs:comment xml:lang="en">The capability of an air vehicle to remain airborne and move by displacing a weight of air greater than its own.</rdfs:comment>
    <rdfs:label xml:lang="en">air, lighter than air</rdfs:label>
    <rdfs:subClassOf rdf:nodeID="A114"/>
    <rdfs:subClassOf rdf:resource="jc3iedm_CAPABILITY.owl#MOBILITY-CAPABILITY"/>
  </rdf:Description>
  <rdf:Description rdf:nodeID="A115">
    <rdf:type rdf:resource="http://www.w3.org/2002/07/owl#Restriction"/>
    <owl:onProperty rdf:resource="jc3iedm_CAPABILITY.owl#operational-capability-category-code"/>
    <owl:hasValue xml:lang="en">Supply (class I)</owl:hasValue>
  </rdf:Description>
  <rdf:Description rdf:nodeID="A116">
    <rdf:type rdf:resource="http://www.w3.org/2002/07/owl#Restriction"/>
    <owl:onProperty rdf:resource="jc3iedm_CAPABILITY.owl#operational-capability-category-code"/>
    <owl:hasValue xml:lang="en">Signal, radio teletype</owl:hasValue>
  </rdf:Description>
  <rdf:Description rdf:about="jc3iedm_CAPABILITYExtended.owl#FIRE-CAPABILITY_Ground_to_air">
    <rdf:type rdf:resource="http://www.w3.org/2002/07/owl#Class"/>
    <rdfs:comment xml:lang="en">The specific value implies that a specific FIRE-CAPABILITY involves firing from the ground to an airborne target.</rdfs:comment>
    <rdfs:label xml:lang="en">ground to air</rdfs:label>
    <rdfs:subClassOf rdf:nodeID="A99"/>
    <rdfs:subClassOf rdf:resource="jc3iedm_CAPABILITY.owl#FIRE-CAPABILITY"/>
  </rdf:Description>
  <rdf:Description rdf:about="jc3iedm_CAPABILITYExtended.owl#">
    <rdf:type rdf:resource="http://www.w3.org/2002/07/owl#Ontology"/>
    <owl:imports rdf:resource="jc3iedm_CAPABILITY.owl#"/>
  </rdf:Description>
  <rdf:Description rdf:nodeID="A117">
    <rdf:type rdf:resource="http://www.w3.org/2002/07/owl#Restriction"/>
    <owl:onProperty rdf:resource="jc3iedm_CAPABILITY.owl#maintenance-capability-category-code"/>
    <owl:hasValue xml:lang="en">Paint shop</owl:hasValue>
  </rdf:Description>
  <rdf:Description rdf:about="jc3iedm_CAPABILITYExtended.owl#OPERATIONAL-CAPABILITY_Signal,_radio_teletype">
    <rdf:type rdf:resource="http://www.w3.org/2002/07/owl#Class"/>
    <rdfs:comment xml:lang="en">The capability in signal services to manage, operate and control a radio teletype communications.</rdfs:comment>
    <rdfs:label xml:lang="en">signal, radio teletype</rdfs:label>
    <rdfs:subClassOf rdf:nodeID="A116"/>
    <rdfs:subClassOf rdf:resource="jc3iedm_CAPABILITY.owl#OPERATIONAL-CAPABILITY"/>
  </rdf:Description>
  <rdf:Description rdf:about="jc3iedm_CAPABILITYExtended.owl#OPERATIONAL-CAPABILITY_Amphibious">
    <rdf:type rdf:resource="http://www.w3.org/2002/07/owl#Class"/>
    <rdfs:comment xml:lang="en">The capability to conduct an operation launched from the sea by military forces against a hostile or potentially hostile shore.</rdfs:comment>
    <rdfs:label xml:lang="en">amphibious</rdfs:label>
    <rdfs:subClassOf rdf:nodeID="A110"/>
    <rdfs:subClassOf rdf:resource="jc3iedm_CAPABILITY.owl#OPERATIONAL-CAPABILITY"/>
  </rdf:Description>
  <rdf:Description rdf:about="jc3iedm_CAPABILITYExtended.owl#SUPPORT-CAPABILITY_Supply_(class_V)">
    <rdf:type rdf:resource="http://www.w3.org/2002/07/owl#Class"/>
    <rdfs:comment xml:lang="en">The capability to provide ammunition, explosives and chemical agents.</rdfs:comment>
    <rdfs:label xml:lang="en">supply (class v)</rdfs:label>
    <rdfs:subClassOf rdf:nodeID="A118"/>
    <rdfs:subClassOf rdf:resource="jc3iedm_CAPABILITY.owl#SUPPORT-CAPABILITY"/>
  </rdf:Description>
  <rdf:Description rdf:nodeID="A50">
    <rdf:type rdf:resource="http://www.w3.org/2002/07/owl#Restriction"/>
    <owl:onProperty rdf:resource="jc3iedm_CAPABILITY.owl#operational-capability-category-code"/>
    <owl:hasValue xml:lang="en">Civilian law enforcement</owl:hasValue>
  </rdf:Description>
  <rdf:Description rdf:about="jc3iedm_CAPABILITY.owl#engineering-capability-descriptor-code">
    <rdfs:range rdf:resource="http://www.w3.org/2001/XMLSchema#string"/>
    <rdfs:domain rdf:resource="jc3iedm_CAPABILITY.owl#ENGINEERING-CAPABILITY"/>
    <rdf:type rdf:resource="http://www.w3.org/2002/07/owl#DatatypeProperty"/>
  </rdf:Description>
  <rdf:Description rdf:nodeID="A119">
    <rdf:type rdf:resource="http://www.w3.org/2002/07/owl#Restriction"/>
    <owl:onProperty rdf:resource="jc3iedm_CAPABILITY.owl#fire-capability-category-code"/>
    <owl:hasValue xml:lang="en">Sea to air</owl:hasValue>
  </rdf:Description>
  <rdf:Description rdf:nodeID="A96">
    <rdf:type rdf:resource="http://www.w3.org/2002/07/owl#Restriction"/>
    <owl:onProperty rdf:resource="jc3iedm_CAPABILITY.owl#operational-capability-category-code"/>
    <owl:hasValue xml:lang="en">Military intelligence, aerial exploitation</owl:hasValue>
  </rdf:Description>
  <rdf:Description rdf:about="jc3iedm_CAPABILITYExtended.owl#MOBILITY-CAPABILITY_Air,_composite">
    <rdf:type rdf:resource="http://www.w3.org/2002/07/owl#Class"/>
    <rdfs:comment xml:lang="en">The capability to move through the air by means that combine deriving lift from fixed wings or from aerofoils that rotate.</rdfs:comment>
    <rdfs:label xml:lang="en">air, composite</rdfs:label>
    <rdfs:subClassOf rdf:nodeID="A62"/>
    <rdfs:subClassOf rdf:resource="jc3iedm_CAPABILITY.owl#MOBILITY-CAPABILITY"/>
  </rdf:Description>
  <rdf:Description rdf:nodeID="A106">
    <rdf:type rdf:resource="http://www.w3.org/2002/07/owl#Restriction"/>
    <owl:onProperty rdf:resource="jc3iedm_CAPABILITY.owl#operational-capability-category-code"/>
    <owl:hasValue xml:lang="en">Maintenance</owl:hasValue>
  </rdf:Description>
  <rdf:Description rdf:nodeID="A120">
    <rdf:type rdf:resource="http://www.w3.org/2002/07/owl#Restriction"/>
    <owl:onProperty rdf:resource="jc3iedm_CAPABILITY.owl#operational-capability-category-code"/>
    <owl:hasValue xml:lang="en">Scout</owl:hasValue>
  </rdf:Description>
  <rdf:Description rdf:about="jc3iedm_CAPABILITYExtended.owl#OPERATIONAL-CAPABILITY_Artillery_survey">
    <rdf:type rdf:resource="http://www.w3.org/2002/07/owl#Class"/>
    <rdfs:comment xml:lang="en">The capability to calculate the coordinates and the altitude of an object/point and from which the bearings/azimuths to a number of reference objects are also known.</rdfs:comment>
    <rdfs:label xml:lang="en">artillery survey</rdfs:label>
    <rdfs:subClassOf rdf:nodeID="A121"/>
    <rdfs:subClassOf rdf:resource="jc3iedm_CAPABILITY.owl#OPERATIONAL-CAPABILITY"/>
  </rdf:Description>
  <rdf:Description rdf:about="jc3iedm_CAPABILITYExtended.owl#SUPPORT-CAPABILITY_Supply_(class_I)">
    <rdf:type rdf:resource="http://www.w3.org/2002/07/owl#Class"/>
    <rdfs:comment xml:lang="en">The capability to provide combat/fresh rations, water and personal, health and welfare items.</rdfs:comment>
    <rdfs:label xml:lang="en">supply (class i)</rdfs:label>
    <rdfs:subClassOf rdf:nodeID="A29"/>
    <rdfs:subClassOf rdf:resource="jc3iedm_CAPABILITY.owl#SUPPORT-CAPABILITY"/>
  </rdf:Description>
  <rdf:Description rdf:about="jc3iedm_CAPABILITYExtended.owl#SUPPORT-CAPABILITY_Engine">
    <rdf:type rdf:resource="http://www.w3.org/2002/07/owl#Class"/>
    <rdfs:comment xml:lang="en">The capability to provide engine supplies.</rdfs:comment>
    <rdfs:label xml:lang="en">engine</rdfs:label>
    <rdfs:subClassOf rdf:nodeID="A122"/>
    <rdfs:subClassOf rdf:resource="jc3iedm_CAPABILITY.owl#SUPPORT-CAPABILITY"/>
  </rdf:Description>
  <rdf:Description rdf:about="jc3iedm_CAPABILITYExtended.owl#OPERATIONAL-CAPABILITY_Labour">
    <rdf:type rdf:resource="http://www.w3.org/2002/07/owl#Class"/>
    <rdfs:comment xml:lang="en">The capability to provide labour services.</rdfs:comment>
    <rdfs:label xml:lang="en">labour</rdfs:label>
    <rdfs:subClassOf rdf:nodeID="A17"/>
    <rdfs:subClassOf rdf:resource="jc3iedm_CAPABILITY.owl#OPERATIONAL-CAPABILITY"/>
  </rdf:Description>
  <rdf:Description rdf:nodeID="A123">
    <rdf:type rdf:resource="http://www.w3.org/2002/07/owl#Restriction"/>
    <owl:onProperty rdf:resource="jc3iedm_CAPABILITY.owl#capability-category-code"/>
    <owl:hasValue xml:lang="en">FIRE-CAPABILITY</owl:hasValue>
  </rdf:Description>
  <rdf:Description rdf:about="jc3iedm_CAPABILITYExtended.owl#OPERATIONAL-CAPABILITY_Training">
    <rdf:type rdf:resource="http://www.w3.org/2002/07/owl#Class"/>
    <rdfs:comment xml:lang="en">A capability that enables an equipment to be used to train personnel.</rdfs:comment>
    <rdfs:label xml:lang="en">training</rdfs:label>
    <rdfs:subClassOf rdf:nodeID="A124"/>
    <rdfs:subClassOf rdf:resource="jc3iedm_CAPABILITY.owl#OPERATIONAL-CAPABILITY"/>
  </rdf:Description>
  <rdf:Description rdf:about="jc3iedm_CAPABILITY.owl#TRANSMISSION-CAPABILITY">
    <rdfs:subClassOf rdf:resource="jc3iedm_CAPABILITY.owl#CAPABILITY"/>
    <rdfs:subClassOf rdf:nodeID="A125"/>
    <rdfs:label xml:lang="en">transmission capability</rdfs:label>
    <rdfs:comment xml:lang="en">A CAPABILITY, required for planning, of those MATERIELs or MATERIEL-TYPEs that are deemed as having the ability to generate, receive or affect signals in the electromagnetic spectrum.</rdfs:comment>
    <rdf:type rdf:resource="http://www.w3.org/2002/07/owl#Class"/>
    <rdfs:subClassOf rdf:nodeID="A26"/>
  </rdf:Description>
  <rdf:Description rdf:about="jc3iedm_CAPABILITYExtended.owl#OPERATIONAL-CAPABILITY_Signal,_radio_tactical_satellite">
    <rdf:type rdf:resource="http://www.w3.org/2002/07/owl#Class"/>
    <rdfs:comment xml:lang="en">The capability in signal services to manage, operate and control a tactical satellite terminal.</rdfs:comment>
    <rdfs:label xml:lang="en">signal, radio tactical satellite</rdfs:label>
    <rdfs:subClassOf rdf:nodeID="A126"/>
    <rdfs:subClassOf rdf:resource="jc3iedm_CAPABILITY.owl#OPERATIONAL-CAPABILITY"/>
  </rdf:Description>
  <rdf:Description rdf:about="jc3iedm_CAPABILITYExtended.owl#OPERATIONAL-CAPABILITY_Signals_intelligence_(SIGINT)">
    <rdf:type rdf:resource="http://www.w3.org/2002/07/owl#Class"/>
    <rdfs:comment xml:lang="en">The capability to provide intelligence derived from communications, electronics, and instrumentation signals.</rdfs:comment>
    <rdfs:label xml:lang="en">signals intelligence (sigint)</rdfs:label>
    <rdfs:subClassOf rdf:nodeID="A127"/>
    <rdfs:subClassOf rdf:resource="jc3iedm_CAPABILITY.owl#OPERATIONAL-CAPABILITY"/>
  </rdf:Description>
  <rdf:Description rdf:nodeID="A128">
    <rdf:type rdf:resource="http://www.w3.org/2002/07/owl#Restriction"/>
    <owl:onProperty rdf:resource="jc3iedm_CAPABILITY.owl#mobility-capability-category-code"/>
    <owl:hasValue xml:lang="en">Water, bay</owl:hasValue>
  </rdf:Description>
  <rdf:Description rdf:nodeID="A95">
    <rdf:type rdf:resource="http://www.w3.org/2002/07/owl#Restriction"/>
    <owl:onProperty rdf:resource="jc3iedm_CAPABILITY.owl#transmission-capability-category-code"/>
    <owl:hasValue xml:lang="en">Transmit</owl:hasValue>
  </rdf:Description>
  <rdf:Description rdf:about="jc3iedm_CAPABILITYExtended.owl#OPERATIONAL-CAPABILITY_Surveillance,_sensor">
    <rdf:type rdf:resource="http://www.w3.org/2002/07/owl#Class"/>
    <rdfs:comment xml:lang="en">The capability to manage, operate and maintain sensor surveillance assets.</rdfs:comment>
    <rdfs:label xml:lang="en">surveillance, sensor</rdfs:label>
    <rdfs:subClassOf rdf:nodeID="A129"/>
    <rdfs:subClassOf rdf:resource="jc3iedm_CAPABILITY.owl#OPERATIONAL-CAPABILITY"/>
  </rdf:Description>
  <rdf:Description rdf:nodeID="A130">
    <rdf:type rdf:resource="http://www.w3.org/2002/07/owl#Restriction"/>
    <owl:onProperty rdf:resource="jc3iedm_CAPABILITY.owl#operational-capability-category-code"/>
    <owl:hasValue xml:lang="en">Surveillance, meteorological</owl:hasValue>
  </rdf:Description>
  <rdf:Description rdf:nodeID="A78">
    <owl:hasValue xml:lang="en">MOBILITY-CAPABILITY</owl:hasValue>
    <owl:onProperty rdf:resource="jc3iedm_CAPABILITY.owl#capability-category-code"/>
    <rdf:type rdf:resource="http://www.w3.org/2002/07/owl#Restriction"/>
  </rdf:Description>
  <rdf:Description rdf:nodeID="A131">
    <rdf:type rdf:resource="http://www.w3.org/2002/07/owl#Restriction"/>
    <owl:onProperty rdf:resource="jc3iedm_CAPABILITY.owl#capability-category-code"/>
    <owl:hasValue xml:lang="en">OPERATIONAL-CAPABILITY</owl:hasValue>
  </rdf:Description>
  <rdf:Description rdf:nodeID="A39">
    <rdf:type rdf:resource="http://www.w3.org/2002/07/owl#Restriction"/>
    <owl:onProperty rdf:resource="jc3iedm_CAPABILITY.owl#operational-capability-category-code"/>
    <owl:hasValue xml:lang="en">Counter intelligence</owl:hasValue>
  </rdf:Description>
  <rdf:Description rdf:nodeID="A132">
    <rdf:type rdf:resource="http://www.w3.org/2002/07/owl#Restriction"/>
    <owl:onProperty rdf:resource="jc3iedm_CAPABILITY.owl#mobility-capability-category-code"/>
    <owl:hasValue xml:lang="en">Water, surface</owl:hasValue>
  </rdf:Description>
  <rdf:Description rdf:nodeID="A133">
    <rdf:type rdf:resource="http://www.w3.org/2002/07/owl#Restriction"/>
    <owl:onProperty rdf:resource="jc3iedm_CAPABILITY.owl#operational-capability-category-code"/>
    <owl:hasValue xml:lang="en">Central intelligence</owl:hasValue>
  </rdf:Description>
  <rdf:Description rdf:about="jc3iedm_CAPABILITYExtended.owl#OPERATIONAL-CAPABILITY_NBC,_decontamination">
    <rdf:type rdf:resource="http://www.w3.org/2002/07/owl#Class"/>
    <rdfs:comment xml:lang="en">The capability to make any person, object, or area safe by absorbing, destroying, neutralizing, making harmless, or removing, chemical or biological materiel, or by removing radioactive material clinging to or around it.</rdfs:comment>
    <rdfs:label xml:lang="en">nbc, decontamination</rdfs:label>
    <rdfs:subClassOf rdf:nodeID="A108"/>
    <rdfs:subClassOf rdf:resource="jc3iedm_CAPABILITY.owl#OPERATIONAL-CAPABILITY"/>
  </rdf:Description>
  <rdf:Description rdf:nodeID="A134">
    <rdf:type rdf:resource="http://www.w3.org/2002/07/owl#Restriction"/>
    <owl:onProperty rdf:resource="jc3iedm_CAPABILITY.owl#operational-capability-category-code"/>
    <owl:hasValue xml:lang="en">NBC, nuclear</owl:hasValue>
  </rdf:Description>
  <rdf:Description rdf:nodeID="A94">
    <rdf:type rdf:resource="http://www.w3.org/2002/07/owl#Restriction"/>
    <owl:onProperty rdf:resource="jc3iedm_CAPABILITY.owl#operational-capability-category-code"/>
    <owl:hasValue xml:lang="en">Air defence</owl:hasValue>
  </rdf:Description>
  <rdf:Description rdf:nodeID="A135">
    <rdf:type rdf:resource="http://www.w3.org/2002/07/owl#Restriction"/>
    <owl:onProperty rdf:resource="jc3iedm_CAPABILITY.owl#operational-capability-category-code"/>
    <owl:hasValue xml:lang="en">Target acquisition, radar</owl:hasValue>
  </rdf:Description>
  <rdf:Description rdf:about="jc3iedm_CAPABILITY.owl#fire-capability-descriptor-code">
    <rdfs:range rdf:resource="http://www.w3.org/2001/XMLSchema#string"/>
    <rdfs:domain rdf:resource="jc3iedm_CAPABILITY.owl#FIRE-CAPABILITY"/>
    <rdf:type rdf:resource="http://www.w3.org/2002/07/owl#DatatypeProperty"/>
  </rdf:Description>
  <rdf:Description rdf:nodeID="A126">
    <rdf:type rdf:resource="http://www.w3.org/2002/07/owl#Restriction"/>
    <owl:onProperty rdf:resource="jc3iedm_CAPABILITY.owl#operational-capability-category-code"/>
    <owl:hasValue xml:lang="en">Signal, radio tactical satellite</owl:hasValue>
  </rdf:Description>
  <rdf:Description rdf:about="jc3iedm_CAPABILITY.owl#fire-capability-category-code">
    <rdfs:range rdf:resource="http://www.w3.org/2001/XMLSchema#string"/>
    <rdfs:domain rdf:resource="jc3iedm_CAPABILITY.owl#FIRE-CAPABILITY"/>
    <rdf:type rdf:resource="http://www.w3.org/2002/07/owl#DatatypeProperty"/>
  </rdf:Description>
  <rdf:Description rdf:about="jc3iedm_CAPABILITYExtended.owl#MOBILITY-CAPABILITY_Water,_creek">
    <rdf:type rdf:resource="http://www.w3.org/2002/07/owl#Class"/>
    <rdfs:comment xml:lang="en">The capability of a device to navigate in creeks.</rdfs:comment>
    <rdfs:label xml:lang="en">water, creek</rdfs:label>
    <rdfs:subClassOf rdf:nodeID="A92"/>
    <rdfs:subClassOf rdf:resource="jc3iedm_CAPABILITY.owl#MOBILITY-CAPABILITY"/>
  </rdf:Description>
  <rdf:Description rdf:nodeID="A136">
    <rdf:type rdf:resource="http://www.w3.org/2002/07/owl#Restriction"/>
    <owl:onProperty rdf:resource="jc3iedm_CAPABILITY.owl#operational-capability-category-code"/>
    <owl:hasValue xml:lang="en">Surveillance, ground module</owl:hasValue>
  </rdf:Description>
  <rdf:Description rdf:about="jc3iedm_CAPABILITYExtended.owl#SUPPORT-CAPABILITY_Healthcare">
    <rdf:type rdf:resource="http://www.w3.org/2002/07/owl#Class"/>
    <rdfs:comment xml:lang="en">The capability to provide health care services.</rdfs:comment>
    <rdfs:label xml:lang="en">healthcare</rdfs:label>
    <rdfs:subClassOf rdf:nodeID="A11"/>
    <rdfs:subClassOf rdf:resource="jc3iedm_CAPABILITY.owl#SUPPORT-CAPABILITY"/>
  </rdf:Description>
  <rdf:Description rdf:about="jc3iedm_CAPABILITYExtended.owl#SURVEILLANCE-CAPABILITY_Imaging">
    <rdf:type rdf:resource="http://www.w3.org/2002/07/owl#Class"/>
    <rdfs:comment xml:lang="en">The ability to gain information by exploiting imaging systems.</rdfs:comment>
    <rdfs:label xml:lang="en">imaging</rdfs:label>
    <rdfs:subClassOf rdf:nodeID="A9"/>
    <rdfs:subClassOf rdf:resource="jc3iedm_CAPABILITY.owl#SURVEILLANCE-CAPABILITY"/>
  </rdf:Description>
  <rdf:Description rdf:about="jc3iedm_CAPABILITYExtended.owl#SUPPORT-CAPABILITY_Fuel,_heating">
    <rdf:type rdf:resource="http://www.w3.org/2002/07/owl#Class"/>
    <rdfs:comment xml:lang="en">The capability to provide fuel for heating.</rdfs:comment>
    <rdfs:label xml:lang="en">fuel, heating</rdfs:label>
    <rdfs:subClassOf rdf:nodeID="A137"/>
    <rdfs:subClassOf rdf:resource="jc3iedm_CAPABILITY.owl#SUPPORT-CAPABILITY"/>
  </rdf:Description>
  <rdf:Description rdf:nodeID="A138">
    <rdf:type rdf:resource="http://www.w3.org/2002/07/owl#Restriction"/>
    <owl:onProperty rdf:resource="jc3iedm_CAPABILITY.owl#mobility-capability-category-code"/>
    <owl:hasValue xml:lang="en">Air, rotary wing</owl:hasValue>
  </rdf:Description>
  <rdf:Description rdf:about="jc3iedm_CAPABILITYExtended.owl#MAINTENANCE-CAPABILITY_Plumbing">
    <rdf:type rdf:resource="http://www.w3.org/2002/07/owl#Class"/>
    <rdfs:comment xml:lang="en">Equipment and resources for fitting and repairing pipes, fixtures and other apparatus of a water gas or sewage system belonging to a docked vessel.</rdfs:comment>
    <rdfs:label xml:lang="en">plumbing</rdfs:label>
    <rdfs:subClassOf rdf:nodeID="A139"/>
    <rdfs:subClassOf rdf:resource="jc3iedm_CAPABILITY.owl#MAINTENANCE-CAPABILITY"/>
  </rdf:Description>
  <rdf:Description rdf:nodeID="A25">
    <rdf:type rdf:resource="http://www.w3.org/2002/07/owl#Restriction"/>
    <owl:onProperty rdf:resource="jc3iedm_CAPABILITY.owl#operational-capability-category-code"/>
    <owl:hasValue xml:lang="en">Transportation, SPOD/SPOE</owl:hasValue>
  </rdf:Description>
  <rdf:Description rdf:about="jc3iedm_CAPABILITY.owl#handling-capability-action-code">
    <rdfs:range rdf:resource="http://www.w3.org/2001/XMLSchema#string"/>
    <rdfs:domain rdf:resource="jc3iedm_CAPABILITY.owl#HANDLING-CAPABILITY"/>
    <rdf:type rdf:resource="http://www.w3.org/2002/07/owl#DatatypeProperty"/>
  </rdf:Description>
  <rdf:Description rdf:nodeID="A140">
    <rdf:type rdf:resource="http://www.w3.org/2002/07/owl#Restriction"/>
    <owl:onProperty rdf:resource="jc3iedm_CAPABILITY.owl#capability-category-code"/>
    <owl:hasValue xml:lang="en">MAINTENANCE-CAPABILITY</owl:hasValue>
  </rdf:Description>
  <rdf:Description rdf:about="jc3iedm_CAPABILITYExtended.owl#FIRE-CAPABILITY_Ground_to_ground">
    <rdf:type rdf:resource="http://www.w3.org/2002/07/owl#Class"/>
    <rdfs:comment xml:lang="en">The specific value implies that a specific FIRE-CAPABILITY involves surface firing.</rdfs:comment>
    <rdfs:label xml:lang="en">ground to ground</rdfs:label>
    <rdfs:subClassOf rdf:nodeID="A141"/>
    <rdfs:subClassOf rdf:resource="jc3iedm_CAPABILITY.owl#FIRE-CAPABILITY"/>
  </rdf:Description>
  <rdf:Description rdf:about="jc3iedm_CAPABILITYExtended.owl#SURVEILLANCE-CAPABILITY_Electronic">
    <rdf:type rdf:resource="http://www.w3.org/2002/07/owl#Class"/>
    <rdfs:comment xml:lang="en">The ability to gain information by exploiting non-communications electronic systems (generally pulsed).</rdfs:comment>
    <rdfs:label xml:lang="en">electronic</rdfs:label>
    <rdfs:subClassOf rdf:nodeID="A142"/>
    <rdfs:subClassOf rdf:resource="jc3iedm_CAPABILITY.owl#SURVEILLANCE-CAPABILITY"/>
  </rdf:Description>
  <rdf:Description rdf:nodeID="A143">
    <rdf:type rdf:resource="http://www.w3.org/2002/07/owl#Restriction"/>
    <owl:onProperty rdf:resource="jc3iedm_CAPABILITY.owl#maintenance-capability-category-code"/>
    <owl:hasValue xml:lang="en">Cable</owl:hasValue>
  </rdf:Description>
  <rdf:Description rdf:about="jc3iedm_CAPABILITYExtended.owl#ENGINEERING-CAPABILITY_Breaching">
    <rdf:type rdf:resource="http://www.w3.org/2002/07/owl#Class"/>
    <rdfs:comment xml:lang="en">The action or process of making a gap in a wall or barrier.</rdfs:comment>
    <rdfs:label xml:lang="en">breaching</rdfs:label>
    <rdfs:subClassOf rdf:nodeID="A144"/>
    <rdfs:subClassOf rdf:resource="jc3iedm_CAPABILITY.owl#ENGINEERING-CAPABILITY"/>
  </rdf:Description>
  <rdf:Description rdf:nodeID="A145">
    <rdf:type rdf:resource="http://www.w3.org/2002/07/owl#Restriction"/>
    <owl:onProperty rdf:resource="jc3iedm_CAPABILITY.owl#support-capability-category-code"/>
    <owl:hasValue xml:lang="en">Water</owl:hasValue>
  </rdf:Description>
  <rdf:Description rdf:about="jc3iedm_CAPABILITYExtended.owl#OPERATIONAL-CAPABILITY_Supply_(class_III)">
    <rdf:type rdf:resource="http://www.w3.org/2002/07/owl#Class"/>
    <rdfs:comment xml:lang="en">The capability to provide fuel and lubricants.</rdfs:comment>
    <rdfs:label xml:lang="en">supply (class iii)</rdfs:label>
    <rdfs:subClassOf rdf:nodeID="A146"/>
    <rdfs:subClassOf rdf:resource="jc3iedm_CAPABILITY.owl#OPERATIONAL-CAPABILITY"/>
  </rdf:Description>
  <rdf:Description rdf:about="jc3iedm_CAPABILITYExtended.owl#OPERATIONAL-CAPABILITY_Marine">
    <rdf:type rdf:resource="http://www.w3.org/2002/07/owl#Class"/>
    <rdfs:comment xml:lang="en">The capability to perform maritime/littoral operations.</rdfs:comment>
    <rdfs:label xml:lang="en">marine</rdfs:label>
    <rdfs:subClassOf rdf:nodeID="A147"/>
    <rdfs:subClassOf rdf:resource="jc3iedm_CAPABILITY.owl#OPERATIONAL-CAPABILITY"/>
  </rdf:Description>
  <rdf:Description rdf:about="jc3iedm_CAPABILITYExtended.owl#OPERATIONAL-CAPABILITY_Signal,_node_centre">
    <rdf:type rdf:resource="http://www.w3.org/2002/07/owl#Class"/>
    <rdfs:comment xml:lang="en">The capability in signal services to manage, operate and control a communications node centre.</rdfs:comment>
    <rdfs:label xml:lang="en">signal, node centre</rdfs:label>
    <rdfs:subClassOf rdf:nodeID="A148"/>
    <rdfs:subClassOf rdf:resource="jc3iedm_CAPABILITY.owl#OPERATIONAL-CAPABILITY"/>
  </rdf:Description>
  <rdf:Description rdf:nodeID="A149">
    <rdf:type rdf:resource="http://www.w3.org/2002/07/owl#Restriction"/>
    <owl:onProperty rdf:resource="jc3iedm_CAPABILITY.owl#operational-capability-category-code"/>
    <owl:hasValue xml:lang="en">Joint intelligence</owl:hasValue>
  </rdf:Description>
  <rdf:Description rdf:nodeID="A150">
    <rdf:type rdf:resource="http://www.w3.org/2002/07/owl#Restriction"/>
    <owl:onProperty rdf:resource="jc3iedm_CAPABILITY.owl#operational-capability-category-code"/>
    <owl:hasValue xml:lang="en">Engineer, combat</owl:hasValue>
  </rdf:Description>
  <rdf:Description rdf:nodeID="A137">
    <rdf:type rdf:resource="http://www.w3.org/2002/07/owl#Restriction"/>
    <owl:onProperty rdf:resource="jc3iedm_CAPABILITY.owl#support-capability-category-code"/>
    <owl:hasValue xml:lang="en">Fuel, heating</owl:hasValue>
  </rdf:Description>
  <rdf:Description rdf:nodeID="A151">
    <rdf:type rdf:resource="http://www.w3.org/2002/07/owl#Restriction"/>
    <owl:onProperty rdf:resource="jc3iedm_CAPABILITY.owl#operational-capability-category-code"/>
    <owl:hasValue xml:lang="en">Tactical air reconnaissance</owl:hasValue>
  </rdf:Description>
  <rdf:Description rdf:nodeID="A152">
    <rdf:type rdf:resource="http://www.w3.org/2002/07/owl#Restriction"/>
    <owl:onProperty rdf:resource="jc3iedm_CAPABILITY.owl#operational-capability-category-code"/>
    <owl:hasValue xml:lang="en">Electronic warfare, direction finding</owl:hasValue>
  </rdf:Description>
  <rdf:Description rdf:about="jc3iedm_CAPABILITYExtended.owl#ENGINEERING-CAPABILITY_Construction">
    <rdf:type rdf:resource="http://www.w3.org/2002/07/owl#Class"/>
    <rdfs:comment xml:lang="en">The action or process of constructing.</rdfs:comment>
    <rdfs:label xml:lang="en">construction</rdfs:label>
    <rdfs:subClassOf rdf:nodeID="A153"/>
    <rdfs:subClassOf rdf:resource="jc3iedm_CAPABILITY.owl#ENGINEERING-CAPABILITY"/>
  </rdf:Description>
  <rdf:Description rdf:about="jc3iedm_CAPABILITYExtended.owl#SUPPORT-CAPABILITY_Education">
    <rdf:type rdf:resource="http://www.w3.org/2002/07/owl#Class"/>
    <rdfs:comment xml:lang="en">The capability to provide education services.</rdfs:comment>
    <rdfs:label xml:lang="en">education</rdfs:label>
    <rdfs:subClassOf rdf:nodeID="A10"/>
    <rdfs:subClassOf rdf:resource="jc3iedm_CAPABILITY.owl#SUPPORT-CAPABILITY"/>
  </rdf:Description>
  <rdf:Description rdf:nodeID="A154">
    <rdf:type rdf:resource="http://www.w3.org/2002/07/owl#Restriction"/>
    <owl:onProperty rdf:resource="jc3iedm_CAPABILITY.owl#operational-capability-category-code"/>
    <owl:hasValue xml:lang="en">Supply, laundry/bath</owl:hasValue>
  </rdf:Description>
  <rdf:Description rdf:nodeID="A155">
    <rdf:type rdf:resource="http://www.w3.org/2002/07/owl#Restriction"/>
    <owl:onProperty rdf:resource="jc3iedm_CAPABILITY.owl#mobility-capability-category-code"/>
    <owl:hasValue xml:lang="en">Dismounted</owl:hasValue>
  </rdf:Description>
  <rdf:Description rdf:about="jc3iedm_CAPABILITY.owl#OPERATIONAL-CAPABILITY">
    <rdfs:subClassOf rdf:resource="jc3iedm_CAPABILITY.owl#CAPABILITY"/>
    <rdfs:subClassOf rdf:nodeID="A156"/>
    <rdfs:label xml:lang="en">operational capability</rdfs:label>
    <rdfs:comment xml:lang="en">A CAPABILITY, required for planning, of those objects and types of objects that are deemed as having the ability, the training and the equipment to perform an operation.</rdfs:comment>
    <rdf:type rdf:resource="http://www.w3.org/2002/07/owl#Class"/>
    <rdfs:subClassOf rdf:nodeID="A131"/>
  </rdf:Description>
  <rdf:Description rdf:about="jc3iedm_CAPABILITYExtended.owl#OPERATIONAL-CAPABILITY_Electronic_warfare,_jamming">
    <rdf:type rdf:resource="http://www.w3.org/2002/07/owl#Class"/>
    <rdfs:comment xml:lang="en">The capability to deliver radiation, re-radiation or reflection of electromagnetic energy with the object of impairing the use of electronic devices, equipment or systems being used by an enemy.</rdfs:comment>
    <rdfs:label xml:lang="en">electronic warfare, jamming</rdfs:label>
    <rdfs:subClassOf rdf:nodeID="A157"/>
    <rdfs:subClassOf rdf:resource="jc3iedm_CAPABILITY.owl#OPERATIONAL-CAPABILITY"/>
  </rdf:Description>
  <rdf:Description rdf:about="jc3iedm_CAPABILITYExtended.owl#OPERATIONAL-CAPABILITY_Signal,_radio_relay">
    <rdf:type rdf:resource="http://www.w3.org/2002/07/owl#Class"/>
    <rdfs:comment xml:lang="en">The capability in signal services to manage, operate and control a communications radio relay.</rdfs:comment>
    <rdfs:label xml:lang="en">signal, radio relay</rdfs:label>
    <rdfs:subClassOf rdf:nodeID="A158"/>
    <rdfs:subClassOf rdf:resource="jc3iedm_CAPABILITY.owl#OPERATIONAL-CAPABILITY"/>
  </rdf:Description>
  <rdf:Description rdf:about="jc3iedm_CAPABILITYExtended.owl#OPERATIONAL-CAPABILITY_Close_air_support">
    <rdf:type rdf:resource="http://www.w3.org/2002/07/owl#Class"/>
    <rdfs:comment xml:lang="en">The capability to perform an air action against hostile targets which are in close proximity to friendly forces and which require detailed integration of each air mission with the fire and movement of those forces.</rdfs:comment>
    <rdfs:label xml:lang="en">close air support</rdfs:label>
    <rdfs:subClassOf rdf:nodeID="A159"/>
    <rdfs:subClassOf rdf:resource="jc3iedm_CAPABILITY.owl#OPERATIONAL-CAPABILITY"/>
  </rdf:Description>
  <rdf:Description rdf:nodeID="A81">
    <owl:hasValue xml:lang="en">SUPPORT-CAPABILITY</owl:hasValue>
    <owl:onProperty rdf:resource="jc3iedm_CAPABILITY.owl#capability-category-code"/>
    <rdf:type rdf:resource="http://www.w3.org/2002/07/owl#Restriction"/>
  </rdf:Description>
  <rdf:Description rdf:about="jc3iedm_CAPABILITY.owl#capability-category-code">
    <rdfs:range rdf:resource="http://www.w3.org/2001/XMLSchema#string"/>
    <rdfs:domain rdf:resource="jc3iedm_CAPABILITY.owl#CAPABILITY"/>
    <rdf:type rdf:resource="http://www.w3.org/2002/07/owl#DatatypeProperty"/>
  </rdf:Description>
  <rdf:Description rdf:about="jc3iedm_CAPABILITYExtended.owl#SUPPORT-CAPABILITY_Sewage">
    <rdf:type rdf:resource="http://www.w3.org/2002/07/owl#Class"/>
    <rdfs:comment xml:lang="en">The capability to provide sewage and refuse disposal.</rdfs:comment>
    <rdfs:label xml:lang="en">sewage</rdfs:label>
    <rdfs:subClassOf rdf:nodeID="A54"/>
    <rdfs:subClassOf rdf:resource="jc3iedm_CAPABILITY.owl#SUPPORT-CAPABILITY"/>
  </rdf:Description>
  <rdf:Description rdf:nodeID="A160">
    <rdf:type rdf:resource="http://www.w3.org/2002/07/owl#Restriction"/>
    <owl:onProperty rdf:resource="jc3iedm_CAPABILITY.owl#operational-capability-category-code"/>
    <owl:hasValue xml:lang="en">Transportation, missile</owl:hasValue>
  </rdf:Description>
  <rdf:Description rdf:nodeID="A121">
    <rdf:type rdf:resource="http://www.w3.org/2002/07/owl#Restriction"/>
    <owl:onProperty rdf:resource="jc3iedm_CAPABILITY.owl#operational-capability-category-code"/>
    <owl:hasValue xml:lang="en">Artillery survey</owl:hasValue>
  </rdf:Description>
  <rdf:Description rdf:nodeID="A142">
    <rdf:type rdf:resource="http://www.w3.org/2002/07/owl#Restriction"/>
    <owl:onProperty rdf:resource="jc3iedm_CAPABILITY.owl#surveillance-capability-category-code"/>
    <owl:hasValue xml:lang="en">Electronic</owl:hasValue>
  </rdf:Description>
  <rdf:Description rdf:nodeID="A47">
    <rdf:type rdf:resource="http://www.w3.org/2002/07/owl#Restriction"/>
    <owl:onProperty rdf:resource="jc3iedm_CAPABILITY.owl#operational-capability-category-code"/>
    <owl:hasValue xml:lang="en">Legal</owl:hasValue>
  </rdf:Description>
  <rdf:Description rdf:about="jc3iedm_CAPABILITYExtended.owl#OPERATIONAL-CAPABILITY_Finance">
    <rdf:type rdf:resource="http://www.w3.org/2002/07/owl#Class"/>
    <rdfs:comment xml:lang="en">The capability to provide financial advice and guidance, support for the procurement process, providing pay and disbursing support.</rdfs:comment>
    <rdfs:label xml:lang="en">finance</rdfs:label>
    <rdfs:subClassOf rdf:nodeID="A161"/>
    <rdfs:subClassOf rdf:resource="jc3iedm_CAPABILITY.owl#OPERATIONAL-CAPABILITY"/>
  </rdf:Description>
  <rdf:Description rdf:nodeID="A158">
    <rdf:type rdf:resource="http://www.w3.org/2002/07/owl#Restriction"/>
    <owl:onProperty rdf:resource="jc3iedm_CAPABILITY.owl#operational-capability-category-code"/>
    <owl:hasValue xml:lang="en">Signal, radio relay</owl:hasValue>
  </rdf:Description>
  <rdf:Description rdf:nodeID="A162">
    <rdf:type rdf:resource="http://www.w3.org/2002/07/owl#Restriction"/>
    <owl:onProperty rdf:resource="jc3iedm_CAPABILITY.owl#support-capability-category-code"/>
    <owl:hasValue xml:lang="en">Bedding</owl:hasValue>
  </rdf:Description>
  <rdf:Description rdf:about="jc3iedm_CAPABILITYExtended.owl#OPERATIONAL-CAPABILITY_Supply_(water)">
    <rdf:type rdf:resource="http://www.w3.org/2002/07/owl#Class"/>
    <rdfs:comment xml:lang="en">The capability to provide drinking water.</rdfs:comment>
    <rdfs:label xml:lang="en">supply (water)</rdfs:label>
    <rdfs:subClassOf rdf:nodeID="A19"/>
    <rdfs:subClassOf rdf:resource="jc3iedm_CAPABILITY.owl#OPERATIONAL-CAPABILITY"/>
  </rdf:Description>
  <rdf:Description rdf:about="jc3iedm_CAPABILITYExtended.owl#MOBILITY-CAPABILITY_Water,_subsurface">
    <rdf:type rdf:resource="http://www.w3.org/2002/07/owl#Class"/>
    <rdfs:comment xml:lang="en">The capability of a device to move on or under the water surface.</rdfs:comment>
    <rdfs:label xml:lang="en">water, subsurface</rdfs:label>
    <rdfs:subClassOf rdf:nodeID="A163"/>
    <rdfs:subClassOf rdf:resource="jc3iedm_CAPABILITY.owl#MOBILITY-CAPABILITY"/>
  </rdf:Description>
  <rdf:Description rdf:about="jc3iedm_CAPABILITYExtended.owl#FIRE-CAPABILITY_Sea_to_air">
    <rdf:type rdf:resource="http://www.w3.org/2002/07/owl#Class"/>
    <rdfs:comment xml:lang="en">The specific value implies that a specific FIRE-CAPABILITY involves firing from a vessel to airborne targets.</rdfs:comment>
    <rdfs:label xml:lang="en">sea to air</rdfs:label>
    <rdfs:subClassOf rdf:nodeID="A119"/>
    <rdfs:subClassOf rdf:resource="jc3iedm_CAPABILITY.owl#FIRE-CAPABILITY"/>
  </rdf:Description>
  <rdf:Description rdf:nodeID="A164">
    <rdf:type rdf:resource="http://www.w3.org/2002/07/owl#Restriction"/>
    <owl:onProperty rdf:resource="jc3iedm_CAPABILITY.owl#mobility-capability-category-code"/>
    <owl:hasValue xml:lang="en">Water, canal</owl:hasValue>
  </rdf:Description>
  <rdf:Description rdf:nodeID="A80">
    <rdf:type rdf:resource="http://www.w3.org/2002/07/owl#Restriction"/>
    <owl:onProperty rdf:resource="jc3iedm_CAPABILITY.owl#mobility-capability-category-code"/>
    <owl:hasValue xml:lang="en">Road march</owl:hasValue>
  </rdf:Description>
  <rdf:Description rdf:about="jc3iedm_CAPABILITYExtended.owl#SUPPORT-CAPABILITY_Water">
    <rdf:type rdf:resource="http://www.w3.org/2002/07/owl#Class"/>
    <rdfs:comment xml:lang="en">The capability to provide potable water.</rdfs:comment>
    <rdfs:label xml:lang="en">water</rdfs:label>
    <rdfs:subClassOf rdf:nodeID="A145"/>
    <rdfs:subClassOf rdf:resource="jc3iedm_CAPABILITY.owl#SUPPORT-CAPABILITY"/>
  </rdf:Description>
  <rdf:Description rdf:about="jc3iedm_CAPABILITYExtended.owl#MOBILITY-CAPABILITY_Land,_railed">
    <rdf:type rdf:resource="http://www.w3.org/2002/07/owl#Class"/>
    <rdfs:comment xml:lang="en">The capability of a device to move along rails.</rdfs:comment>
    <rdfs:label xml:lang="en">land, railed</rdfs:label>
    <rdfs:subClassOf rdf:nodeID="A165"/>
    <rdfs:subClassOf rdf:resource="jc3iedm_CAPABILITY.owl#MOBILITY-CAPABILITY"/>
  </rdf:Description>
  <rdf:Description rdf:nodeID="A166">
    <rdf:type rdf:resource="http://www.w3.org/2002/07/owl#Restriction"/>
    <owl:onProperty rdf:resource="jc3iedm_CAPABILITY.owl#operational-capability-category-code"/>
    <owl:hasValue xml:lang="en">Supply (class II)</owl:hasValue>
  </rdf:Description>
  <rdf:Description rdf:about="jc3iedm_CAPABILITY.owl#storage-capability-condition-code">
    <rdfs:range rdf:resource="http://www.w3.org/2001/XMLSchema#string"/>
    <rdfs:domain rdf:resource="jc3iedm_CAPABILITY.owl#STORAGE-CAPABILITY"/>
    <rdf:type rdf:resource="http://www.w3.org/2002/07/owl#DatatypeProperty"/>
  </rdf:Description>
  <rdf:Description rdf:nodeID="A63">
    <rdf:type rdf:resource="http://www.w3.org/2002/07/owl#Restriction"/>
    <owl:onProperty rdf:resource="jc3iedm_CAPABILITY.owl#operational-capability-category-code"/>
    <owl:hasValue xml:lang="en">NBC, chemical, smoke</owl:hasValue>
  </rdf:Description>
  <rdf:Description rdf:nodeID="A21">
    <rdf:type rdf:resource="http://www.w3.org/2002/07/owl#Restriction"/>
    <owl:onProperty rdf:resource="jc3iedm_CAPABILITY.owl#operational-capability-category-code"/>
    <owl:hasValue xml:lang="en">Personnel services</owl:hasValue>
  </rdf:Description>
  <rdf:Description rdf:about="jc3iedm_CAPABILITYExtended.owl#SURVEILLANCE-CAPABILITY_Communication">
    <rdf:type rdf:resource="http://www.w3.org/2002/07/owl#Class"/>
    <rdfs:comment xml:lang="en">The ability to gain information by exploiting communications systems.</rdfs:comment>
    <rdfs:label xml:lang="en">communication</rdfs:label>
    <rdfs:subClassOf rdf:nodeID="A167"/>
    <rdfs:subClassOf rdf:resource="jc3iedm_CAPABILITY.owl#SURVEILLANCE-CAPABILITY"/>
  </rdf:Description>
  <rdf:Description rdf:nodeID="A168">
    <owl:hasValue xml:lang="en">STORAGE-CAPABILITY</owl:hasValue>
    <owl:onProperty rdf:resource="jc3iedm_CAPABILITY.owl#capability-category-code"/>
    <rdf:type rdf:resource="http://www.w3.org/2002/07/owl#Restriction"/>
  </rdf:Description>
  <rdf:Description rdf:nodeID="A169">
    <rdf:type rdf:resource="http://www.w3.org/2002/07/owl#Restriction"/>
    <owl:onProperty rdf:resource="jc3iedm_CAPABILITY.owl#capability-category-code"/>
    <owl:hasValue xml:lang="en">HANDLING-CAPABILITY</owl:hasValue>
  </rdf:Description>
  <rdf:Description rdf:about="jc3iedm_CAPABILITY.owl#support-capability-category-code">
    <rdfs:range rdf:resource="http://www.w3.org/2001/XMLSchema#string"/>
    <rdfs:domain rdf:resource="jc3iedm_CAPABILITY.owl#SUPPORT-CAPABILITY"/>
    <rdf:type rdf:resource="http://www.w3.org/2002/07/owl#DatatypeProperty"/>
  </rdf:Description>
  <rdf:Description rdf:nodeID="A170">
    <rdf:type rdf:resource="http://www.w3.org/2002/07/owl#Restriction"/>
    <owl:onProperty rdf:resource="jc3iedm_CAPABILITY.owl#mobility-capability-category-code"/>
    <owl:hasValue xml:lang="en">Water, nontidal</owl:hasValue>
  </rdf:Description>
  <rdf:Description rdf:about="jc3iedm_CAPABILITYExtended.owl#OPERATIONAL-CAPABILITY_Supply,_laundry/bath">
    <rdf:type rdf:resource="http://www.w3.org/2002/07/owl#Class"/>
    <rdfs:comment xml:lang="en">The capability to provide laundry and/or bath services.</rdfs:comment>
    <rdfs:label xml:lang="en">supply, laundry/bath</rdfs:label>
    <rdfs:subClassOf rdf:nodeID="A154"/>
    <rdfs:subClassOf rdf:resource="jc3iedm_CAPABILITY.owl#OPERATIONAL-CAPABILITY"/>
  </rdf:Description>
  <rdf:Description rdf:about="jc3iedm_CAPABILITYExtended.owl#OPERATIONAL-CAPABILITY_Attack">
    <rdf:type rdf:resource="http://www.w3.org/2002/07/owl#Class"/>
    <rdfs:comment xml:lang="en">The capability to perform an offensive mission.</rdfs:comment>
    <rdfs:label xml:lang="en">attack</rdfs:label>
    <rdfs:subClassOf rdf:nodeID="A171"/>
    <rdfs:subClassOf rdf:resource="jc3iedm_CAPABILITY.owl#OPERATIONAL-CAPABILITY"/>
  </rdf:Description>
  <rdf:Description rdf:about="jc3iedm_CAPABILITYExtended.owl#OPERATIONAL-CAPABILITY_Military_intelligence,_tactical_exploitation">
    <rdf:type rdf:resource="http://www.w3.org/2002/07/owl#Class"/>
    <rdfs:comment xml:lang="en">The capability to use information required for the planning and conducting tactical operations.</rdfs:comment>
    <rdfs:label xml:lang="en">military intelligence, tactical exploitation</rdfs:label>
    <rdfs:subClassOf rdf:nodeID="A172"/>
    <rdfs:subClassOf rdf:resource="jc3iedm_CAPABILITY.owl#OPERATIONAL-CAPABILITY"/>
  </rdf:Description>
  <rdf:Description rdf:about="jc3iedm_CAPABILITYExtended.owl#OPERATIONAL-CAPABILITY_Air_to_ground">
    <rdf:type rdf:resource="http://www.w3.org/2002/07/owl#Class"/>
    <rdfs:comment xml:lang="en">The capability to perform air to ground operations.</rdfs:comment>
    <rdfs:label xml:lang="en">air to ground</rdfs:label>
    <rdfs:subClassOf rdf:nodeID="A90"/>
    <rdfs:subClassOf rdf:resource="jc3iedm_CAPABILITY.owl#OPERATIONAL-CAPABILITY"/>
  </rdf:Description>
  <rdf:Description rdf:nodeID="A40">
    <rdf:type rdf:resource="http://www.w3.org/2002/07/owl#Restriction"/>
    <owl:onProperty rdf:resource="jc3iedm_CAPABILITY.owl#surveillance-capability-category-code"/>
    <owl:hasValue xml:lang="en">Signal</owl:hasValue>
  </rdf:Description>
  <rdf:Description rdf:about="jc3iedm_CAPABILITYExtended.owl#OPERATIONAL-CAPABILITY_Theatre_missile_defence">
    <rdf:type rdf:resource="http://www.w3.org/2002/07/owl#Class"/>
    <rdfs:comment xml:lang="en">The capability to manage, operate and maintain theatre missile defence assets.</rdfs:comment>
    <rdfs:label xml:lang="en">theatre missile defence</rdfs:label>
    <rdfs:subClassOf rdf:nodeID="A173"/>
    <rdfs:subClassOf rdf:resource="jc3iedm_CAPABILITY.owl#OPERATIONAL-CAPABILITY"/>
  </rdf:Description>
  <rdf:Description rdf:nodeID="A107">
    <rdf:type rdf:resource="http://www.w3.org/2002/07/owl#Restriction"/>
    <owl:onProperty rdf:resource="jc3iedm_CAPABILITY.owl#support-capability-category-code"/>
    <owl:hasValue xml:lang="en">Food/rations</owl:hasValue>
  </rdf:Description>
  <rdf:Description rdf:nodeID="A174">
    <rdf:type rdf:resource="http://www.w3.org/2002/07/owl#Restriction"/>
    <owl:onProperty rdf:resource="jc3iedm_CAPABILITY.owl#operational-capability-category-code"/>
    <owl:hasValue xml:lang="en">Aerial refuelling</owl:hasValue>
  </rdf:Description>
  <rdf:Description rdf:nodeID="A175">
    <rdf:type rdf:resource="http://www.w3.org/2002/07/owl#Restriction"/>
    <owl:onProperty rdf:resource="jc3iedm_CAPABILITY.owl#operational-capability-category-code"/>
    <owl:hasValue xml:lang="en">Public affairs, joint information</owl:hasValue>
  </rdf:Description>
  <rdf:Description rdf:nodeID="A157">
    <rdf:type rdf:resource="http://www.w3.org/2002/07/owl#Restriction"/>
    <owl:onProperty rdf:resource="jc3iedm_CAPABILITY.owl#operational-capability-category-code"/>
    <owl:hasValue xml:lang="en">Electronic warfare, jamming</owl:hasValue>
  </rdf:Description>
  <rdf:Description rdf:nodeID="A83">
    <rdf:type rdf:resource="http://www.w3.org/2002/07/owl#Restriction"/>
    <owl:onProperty rdf:resource="jc3iedm_CAPABILITY.owl#operational-capability-category-code"/>
    <owl:hasValue xml:lang="en">Water purification</owl:hasValue>
  </rdf:Description>
  <rdf:Description rdf:about="jc3iedm_CAPABILITYExtended.owl#OPERATIONAL-CAPABILITY_C2">
    <rdf:type rdf:resource="http://www.w3.org/2002/07/owl#Class"/>
    <rdfs:comment xml:lang="en">The capability to exercise the authority, responsibilities and activities of military commanders in direction and co-ordination or military forces and the implementation of orders related to the execution of operations.</rdfs:comment>
    <rdfs:label xml:lang="en">c2</rdfs:label>
    <rdfs:subClassOf rdf:nodeID="A176"/>
    <rdfs:subClassOf rdf:resource="jc3iedm_CAPABILITY.owl#OPERATIONAL-CAPABILITY"/>
  </rdf:Description>
  <rdf:Description rdf:nodeID="A141">
    <rdf:type rdf:resource="http://www.w3.org/2002/07/owl#Restriction"/>
    <owl:onProperty rdf:resource="jc3iedm_CAPABILITY.owl#fire-capability-category-code"/>
    <owl:hasValue xml:lang="en">Ground to ground</owl:hasValue>
  </rdf:Description>
  <rdf:Description rdf:nodeID="A122">
    <rdf:type rdf:resource="http://www.w3.org/2002/07/owl#Restriction"/>
    <owl:onProperty rdf:resource="jc3iedm_CAPABILITY.owl#support-capability-category-code"/>
    <owl:hasValue xml:lang="en">Engine</owl:hasValue>
  </rdf:Description>
  <rdf:Description rdf:about="jc3iedm_CAPABILITYExtended.owl#OPERATIONAL-CAPABILITY_Electronic_ranging">
    <rdf:type rdf:resource="http://www.w3.org/2002/07/owl#Class"/>
    <rdfs:comment xml:lang="en">The capability to establish target distance electronically.</rdfs:comment>
    <rdfs:label xml:lang="en">electronic ranging</rdfs:label>
    <rdfs:subClassOf rdf:nodeID="A177"/>
    <rdfs:subClassOf rdf:resource="jc3iedm_CAPABILITY.owl#OPERATIONAL-CAPABILITY"/>
  </rdf:Description>
  <rdf:Description rdf:nodeID="A178">
    <rdf:type rdf:resource="http://www.w3.org/2002/07/owl#Restriction"/>
    <owl:onProperty rdf:resource="jc3iedm_CAPABILITY.owl#operational-capability-category-code"/>
    <owl:hasValue xml:lang="en">Search and rescue</owl:hasValue>
  </rdf:Description>
  <rdf:Description rdf:about="jc3iedm_CAPABILITYExtended.owl#OPERATIONAL-CAPABILITY_Target_acquisition,_radar">
    <rdf:type rdf:resource="http://www.w3.org/2002/07/owl#Class"/>
    <rdfs:comment xml:lang="en">The capability to manage, operate and maintain radar target acquisition assets.</rdfs:comment>
    <rdfs:label xml:lang="en">target acquisition, radar</rdfs:label>
    <rdfs:subClassOf rdf:nodeID="A135"/>
    <rdfs:subClassOf rdf:resource="jc3iedm_CAPABILITY.owl#OPERATIONAL-CAPABILITY"/>
  </rdf:Description>
  <rdf:Description rdf:nodeID="A179">
    <owl:hasValue xml:lang="en">ENGINEERING-CAPABILITY</owl:hasValue>
    <owl:onProperty rdf:resource="jc3iedm_CAPABILITY.owl#capability-category-code"/>
    <rdf:type rdf:resource="http://www.w3.org/2002/07/owl#Restriction"/>
  </rdf:Description>
  <rdf:Description rdf:nodeID="A180">
    <rdf:type rdf:resource="http://www.w3.org/2002/07/owl#Restriction"/>
    <owl:onProperty rdf:resource="jc3iedm_CAPABILITY.owl#capability-category-code"/>
    <owl:hasValue xml:lang="en">ENGINEERING-CAPABILITY</owl:hasValue>
  </rdf:Description>
  <rdf:Description rdf:nodeID="A181">
    <rdf:type rdf:resource="http://www.w3.org/2002/07/owl#Restriction"/>
    <owl:onProperty rdf:resource="jc3iedm_CAPABILITY.owl#operational-capability-category-code"/>
    <owl:hasValue xml:lang="en">Signal, node, large extension</owl:hasValue>
  </rdf:Description>
  <rdf:Description rdf:nodeID="A182">
    <rdf:type rdf:resource="http://www.w3.org/2002/07/owl#Restriction"/>
    <owl:onProperty rdf:resource="jc3iedm_CAPABILITY.owl#operational-capability-category-code"/>
    <owl:hasValue xml:lang="en">Target acquisition</owl:hasValue>
  </rdf:Description>
  <rdf:Description rdf:about="jc3iedm_CAPABILITYExtended.owl#OPERATIONAL-CAPABILITY_Airborne">
    <rdf:type rdf:resource="http://www.w3.org/2002/07/owl#Class"/>
    <rdfs:comment xml:lang="en">The capability to carry out operations, either by paradrop or air landing, following an air movement.</rdfs:comment>
    <rdfs:label xml:lang="en">airborne</rdfs:label>
    <rdfs:subClassOf rdf:nodeID="A84"/>
    <rdfs:subClassOf rdf:resource="jc3iedm_CAPABILITY.owl#OPERATIONAL-CAPABILITY"/>
  </rdf:Description>
  <rdf:Description rdf:nodeID="A167">
    <rdf:type rdf:resource="http://www.w3.org/2002/07/owl#Restriction"/>
    <owl:onProperty rdf:resource="jc3iedm_CAPABILITY.owl#surveillance-capability-category-code"/>
    <owl:hasValue xml:lang="en">Communication</owl:hasValue>
  </rdf:Description>
  <rdf:Description rdf:about="jc3iedm_CAPABILITY.owl#SURVEILLANCE-CAPABILITY">
    <rdfs:subClassOf rdf:resource="jc3iedm_CAPABILITY.owl#CAPABILITY"/>
    <rdfs:subClassOf rdf:nodeID="A183"/>
    <rdfs:label xml:lang="en">surveillance capability</rdfs:label>
    <rdfs:comment xml:lang="en">A CAPABILITY, required for planning, of those FACILITYs, MATERIELs, ORGANISATIONs and PERSONs or FACILITY-TYPEs, EQUIPMENT-TYPEs, ORGANISATION-TYPEs and PERSON-TYPEs that are deemed as having the nominal ability to observe aerospace, surface or subsurface areas, places, persons, or things, by visual, aural, electronic, photographic or other means.</rdfs:comment>
    <rdf:type rdf:resource="http://www.w3.org/2002/07/owl#Class"/>
    <rdfs:subClassOf rdf:nodeID="A38"/>
  </rdf:Description>
  <rdf:Description rdf:nodeID="A66">
    <rdf:type rdf:resource="http://www.w3.org/2002/07/owl#Restriction"/>
    <owl:onProperty rdf:resource="jc3iedm_CAPABILITY.owl#operational-capability-category-code"/>
    <owl:hasValue xml:lang="en">Peace support</owl:hasValue>
  </rdf:Description>
  <rdf:Description rdf:about="jc3iedm_CAPABILITYExtended.owl#OPERATIONAL-CAPABILITY_Search_and_rescue">
    <rdf:type rdf:resource="http://www.w3.org/2002/07/owl#Class"/>
    <rdfs:comment xml:lang="en">The capability to use aircraft, surface craft, submarines, specialised rescue teams, and equipment to search for and rescue personnel in distress on land or sea.</rdfs:comment>
    <rdfs:label xml:lang="en">search and rescue</rdfs:label>
    <rdfs:subClassOf rdf:nodeID="A178"/>
    <rdfs:subClassOf rdf:resource="jc3iedm_CAPABILITY.owl#OPERATIONAL-CAPABILITY"/>
  </rdf:Description>
  <rdf:Description rdf:about="jc3iedm_CAPABILITY.owl#mobility-capability-descriptor-code">
    <rdfs:range rdf:resource="http://www.w3.org/2001/XMLSchema#string"/>
    <rdfs:domain rdf:resource="jc3iedm_CAPABILITY.owl#MOBILITY-CAPABILITY"/>
    <rdf:type rdf:resource="http://www.w3.org/2002/07/owl#DatatypeProperty"/>
  </rdf:Description>
  <rdf:Description rdf:nodeID="A184">
    <rdf:type rdf:resource="http://www.w3.org/2002/07/owl#Restriction"/>
    <owl:onProperty rdf:resource="jc3iedm_CAPABILITY.owl#support-capability-category-code"/>
    <owl:hasValue xml:lang="en">Medical supplies</owl:hasValue>
  </rdf:Description>
  <rdf:Description rdf:about="jc3iedm_CAPABILITYExtended.owl#SUPPORT-CAPABILITY_Laundry">
    <rdf:type rdf:resource="http://www.w3.org/2002/07/owl#Class"/>
    <rdfs:comment xml:lang="en">The capability to provide laundry services.</rdfs:comment>
    <rdfs:label xml:lang="en">laundry</rdfs:label>
    <rdfs:subClassOf rdf:nodeID="A48"/>
    <rdfs:subClassOf rdf:resource="jc3iedm_CAPABILITY.owl#SUPPORT-CAPABILITY"/>
  </rdf:Description>
  <rdf:Description rdf:about="jc3iedm_CAPABILITYExtended.owl#OPERATIONAL-CAPABILITY_Surveillance,_meteorological">
    <rdf:type rdf:resource="http://www.w3.org/2002/07/owl#Class"/>
    <rdfs:comment xml:lang="en">The capability to perform systematic observation of meteorological conditions.</rdfs:comment>
    <rdfs:label xml:lang="en">surveillance, meteorological</rdfs:label>
    <rdfs:subClassOf rdf:nodeID="A130"/>
    <rdfs:subClassOf rdf:resource="jc3iedm_CAPABILITY.owl#OPERATIONAL-CAPABILITY"/>
  </rdf:Description>
  <rdf:Description rdf:about="jc3iedm_CAPABILITY.owl#MAINTENANCE-CAPABILITY">
    <rdfs:subClassOf rdf:resource="jc3iedm_CAPABILITY.owl#CAPABILITY"/>
    <rdfs:subClassOf rdf:nodeID="A24"/>
    <rdfs:label xml:lang="en">maintenance capability</rdfs:label>
    <rdfs:comment xml:lang="en">A CAPABILITY, required for planning, of those FACILITYs, MATERIELs, ORGANISATIONs and PERSONs or FACILITY-TYPEs, EQUIPMENT-TYPEs, ORGANISATION-TYPEs, and PERSON-TYPEs that are deemed as having the ability to provide a range of activities required to restore or maintain operational usage.</rdfs:comment>
    <rdf:type rdf:resource="http://www.w3.org/2002/07/owl#Class"/>
    <rdfs:subClassOf rdf:nodeID="A140"/>
  </rdf:Description>
  <rdf:Description rdf:nodeID="A185">
    <rdf:type rdf:resource="http://www.w3.org/2002/07/owl#Restriction"/>
    <owl:onProperty rdf:resource="jc3iedm_CAPABILITY.owl#capability-category-code"/>
    <owl:hasValue xml:lang="en">STORAGE-CAPABILITY</owl:hasValue>
  </rdf:Description>
  <rdf:Description rdf:about="jc3iedm_CAPABILITY.owl#fire-capability-weapon-type-code">
    <rdfs:range rdf:resource="http://www.w3.org/2001/XMLSchema#string"/>
    <rdfs:domain rdf:resource="jc3iedm_CAPABILITY.owl#FIRE-CAPABILITY"/>
    <rdf:type rdf:resource="http://www.w3.org/2002/07/owl#DatatypeProperty"/>
  </rdf:Description>
  <rdf:Description rdf:about="jc3iedm_CAPABILITYExtended.owl#MOBILITY-CAPABILITY_Water,_river">
    <rdf:type rdf:resource="http://www.w3.org/2002/07/owl#Class"/>
    <rdfs:comment xml:lang="en">The capability of a device to navigate rivers.</rdfs:comment>
    <rdfs:label xml:lang="en">water, river</rdfs:label>
    <rdfs:subClassOf rdf:nodeID="A186"/>
    <rdfs:subClassOf rdf:resource="jc3iedm_CAPABILITY.owl#MOBILITY-CAPABILITY"/>
  </rdf:Description>
  <rdf:Description rdf:about="jc3iedm_CAPABILITY.owl#capability-day-night-code">
    <rdfs:range rdf:resource="http://www.w3.org/2001/XMLSchema#string"/>
    <rdfs:domain rdf:resource="jc3iedm_CAPABILITY.owl#CAPABILITY"/>
    <rdf:type rdf:resource="http://www.w3.org/2002/07/owl#DatatypeProperty"/>
  </rdf:Description>
  <rdf:Description rdf:nodeID="A171">
    <rdf:type rdf:resource="http://www.w3.org/2002/07/owl#Restriction"/>
    <owl:onProperty rdf:resource="jc3iedm_CAPABILITY.owl#operational-capability-category-code"/>
    <owl:hasValue xml:lang="en">Attack</owl:hasValue>
  </rdf:Description>
  <rdf:Description rdf:about="jc3iedm_CAPABILITY.owl#engineering-capability-facility-height-dimension">
    <rdfs:domain rdf:resource="jc3iedm_CAPABILITY.owl#ENGINEERING-CAPABILITY"/>
    <rdf:type rdf:resource="http://www.w3.org/2002/07/owl#DatatypeProperty"/>
  </rdf:Description>
  <rdf:Description rdf:about="jc3iedm_CAPABILITYExtended.owl#MOBILITY-CAPABILITY_Water,_bay">
    <rdf:type rdf:resource="http://www.w3.org/2002/07/owl#Class"/>
    <rdfs:comment xml:lang="en">The capability of a device to navigate in bays.</rdfs:comment>
    <rdfs:label xml:lang="en">water, bay</rdfs:label>
    <rdfs:subClassOf rdf:nodeID="A128"/>
    <rdfs:subClassOf rdf:resource="jc3iedm_CAPABILITY.owl#MOBILITY-CAPABILITY"/>
  </rdf:Description>
  <rdf:Description rdf:nodeID="A65">
    <rdf:type rdf:resource="http://www.w3.org/2002/07/owl#Restriction"/>
    <owl:onProperty rdf:resource="jc3iedm_CAPABILITY.owl#fire-capability-category-code"/>
    <owl:hasValue xml:lang="en">Air to sea</owl:hasValue>
  </rdf:Description>
  <rdf:Description rdf:about="jc3iedm_CAPABILITYExtended.owl#OPERATIONAL-CAPABILITY_NBC,_chemical">
    <rdf:type rdf:resource="http://www.w3.org/2002/07/owl#Class"/>
    <rdfs:comment xml:lang="en">The capability to employ chemical materiel to kill, injure, or incapacitate for a significant period of time, man or animals, and deny or hinder the use of areas, facilities or materiel; or defence against such employment.</rdfs:comment>
    <rdfs:label xml:lang="en">nbc, chemical</rdfs:label>
    <rdfs:subClassOf rdf:nodeID="A73"/>
    <rdfs:subClassOf rdf:resource="jc3iedm_CAPABILITY.owl#OPERATIONAL-CAPABILITY"/>
  </rdf:Description>
  <rdf:Description rdf:about="jc3iedm_CAPABILITYExtended.owl#OPERATIONAL-CAPABILITY_Supply_(class_IV)">
    <rdf:type rdf:resource="http://www.w3.org/2002/07/owl#Class"/>
    <rdfs:comment xml:lang="en">The capability to provide construction materials.</rdfs:comment>
    <rdfs:label xml:lang="en">supply (class iv)</rdfs:label>
    <rdfs:subClassOf rdf:nodeID="A187"/>
    <rdfs:subClassOf rdf:resource="jc3iedm_CAPABILITY.owl#OPERATIONAL-CAPABILITY"/>
  </rdf:Description>
  <rdf:Description rdf:about="jc3iedm_CAPABILITYExtended.owl#MAINTENANCE-CAPABILITY_Paint_shop">
    <rdf:type rdf:resource="http://www.w3.org/2002/07/owl#Class"/>
    <rdfs:comment xml:lang="en">Equipment and resources for painting any part of a docked vessel.</rdfs:comment>
    <rdfs:label xml:lang="en">paint shop</rdfs:label>
    <rdfs:subClassOf rdf:nodeID="A117"/>
    <rdfs:subClassOf rdf:resource="jc3iedm_CAPABILITY.owl#MAINTENANCE-CAPABILITY"/>
  </rdf:Description>
  <rdf:Description rdf:nodeID="A147">
    <rdf:type rdf:resource="http://www.w3.org/2002/07/owl#Restriction"/>
    <owl:onProperty rdf:resource="jc3iedm_CAPABILITY.owl#operational-capability-category-code"/>
    <owl:hasValue xml:lang="en">Marine</owl:hasValue>
  </rdf:Description>
  <rdf:Description rdf:about="jc3iedm_CAPABILITYExtended.owl#MOBILITY-CAPABILITY_Amphibious">
    <rdf:type rdf:resource="http://www.w3.org/2002/07/owl#Class"/>
    <rdfs:comment xml:lang="en">The capability of a device to operate both on land and in water.</rdfs:comment>
    <rdfs:label xml:lang="en">amphibious</rdfs:label>
    <rdfs:subClassOf rdf:nodeID="A188"/>
    <rdfs:subClassOf rdf:resource="jc3iedm_CAPABILITY.owl#MOBILITY-CAPABILITY"/>
  </rdf:Description>
  <rdf:Description rdf:nodeID="A82">
    <rdf:type rdf:resource="http://www.w3.org/2002/07/owl#Restriction"/>
    <owl:onProperty rdf:resource="jc3iedm_CAPABILITY.owl#capability-category-code"/>
    <owl:hasValue xml:lang="en">SUPPORT-CAPABILITY</owl:hasValue>
  </rdf:Description>
  <rdf:Description rdf:about="jc3iedm_CAPABILITY.owl#STORAGE-CAPABILITY">
    <rdfs:subClassOf rdf:resource="jc3iedm_CAPABILITY.owl#CAPABILITY"/>
    <rdfs:subClassOf rdf:nodeID="A168"/>
    <rdfs:label xml:lang="en">storage capability</rdfs:label>
    <rdfs:comment xml:lang="en">A CAPABILITY, required for planning, of those FACILITYs and MATERIELs or EQUIPMENT-TYPEs and FACILITY-TYPEs that are deemed as having the ability to hold a specific OBJECT-TYPE.</rdfs:comment>
    <rdf:type rdf:resource="http://www.w3.org/2002/07/owl#Class"/>
    <rdfs:subClassOf rdf:nodeID="A185"/>
  </rdf:Description>
  <rdf:Description rdf:nodeID="A68">
    <rdf:type rdf:resource="http://www.w3.org/2002/07/owl#Restriction"/>
    <owl:onProperty rdf:resource="jc3iedm_CAPABILITY.owl#engineering-capability-category-code"/>
    <owl:hasValue xml:lang="en">Demolition</owl:hasValue>
  </rdf:Description>
  <rdf:Description rdf:about="jc3iedm_CAPABILITYExtended.owl#OPERATIONAL-CAPABILITY_Supply_(class_I)">
    <rdf:type rdf:resource="http://www.w3.org/2002/07/owl#Class"/>
    <rdfs:comment xml:lang="en">The capability to provide combat/fresh rations, water and personal, health and welfare items.</rdfs:comment>
    <rdfs:label xml:lang="en">supply (class i)</rdfs:label>
    <rdfs:subClassOf rdf:nodeID="A115"/>
    <rdfs:subClassOf rdf:resource="jc3iedm_CAPABILITY.owl#OPERATIONAL-CAPABILITY"/>
  </rdf:Description>
  <rdf:Description rdf:about="jc3iedm_CAPABILITYExtended.owl#SUPPORT-CAPABILITY_Medical">
    <rdf:type rdf:resource="http://www.w3.org/2002/07/owl#Class"/>
    <rdfs:comment xml:lang="en">The capability to treat people for illnesses and injuries.</rdfs:comment>
    <rdfs:label xml:lang="en">medical</rdfs:label>
    <rdfs:subClassOf rdf:nodeID="A87"/>
    <rdfs:subClassOf rdf:resource="jc3iedm_CAPABILITY.owl#SUPPORT-CAPABILITY"/>
  </rdf:Description>
  <rdf:Description rdf:about="jc3iedm_CAPABILITYExtended.owl#MAINTENANCE-CAPABILITY_Tank_cleaning">
    <rdf:type rdf:resource="http://www.w3.org/2002/07/owl#Class"/>
    <rdfs:comment xml:lang="en">Equipment and resources for the removal of any trace of the original contents of any tank belonging to a docked vessel. Removal is often carried out by means of a high-pressure water jet.</rdfs:comment>
    <rdfs:label xml:lang="en">tank cleaning</rdfs:label>
    <rdfs:subClassOf rdf:nodeID="A112"/>
    <rdfs:subClassOf rdf:resource="jc3iedm_CAPABILITY.owl#MAINTENANCE-CAPABILITY"/>
  </rdf:Description>
  <rdf:Description rdf:nodeID="A86">
    <rdf:type rdf:resource="http://www.w3.org/2002/07/owl#Restriction"/>
    <owl:onProperty rdf:resource="jc3iedm_CAPABILITY.owl#maintenance-capability-category-code"/>
    <owl:hasValue xml:lang="en">Shotblast</owl:hasValue>
  </rdf:Description>
  <rdf:Description rdf:nodeID="A88">
    <rdf:type rdf:resource="http://www.w3.org/2002/07/owl#Restriction"/>
    <owl:onProperty rdf:resource="jc3iedm_CAPABILITY.owl#support-capability-category-code"/>
    <owl:hasValue xml:lang="en">Recreation</owl:hasValue>
  </rdf:Description>
  <rdf:Description rdf:about="jc3iedm_CAPABILITYExtended.owl#OPERATIONAL-CAPABILITY_Supply_(class_II)">
    <rdf:type rdf:resource="http://www.w3.org/2002/07/owl#Class"/>
    <rdfs:comment xml:lang="en">The capability to provide materiel.</rdfs:comment>
    <rdfs:label xml:lang="en">supply (class ii)</rdfs:label>
    <rdfs:subClassOf rdf:nodeID="A166"/>
    <rdfs:subClassOf rdf:resource="jc3iedm_CAPABILITY.owl#OPERATIONAL-CAPABILITY"/>
  </rdf:Description>
  <rdf:Description rdf:about="jc3iedm_CAPABILITYExtended.owl#OPERATIONAL-CAPABILITY_Public_affairs,_joint_information">
    <rdf:type rdf:resource="http://www.w3.org/2002/07/owl#Class"/>
    <rdfs:comment xml:lang="en">The capability to provide those public information, command information, and community relations activities directed towards the general public in a joint services environment.</rdfs:comment>
    <rdfs:label xml:lang="en">public affairs, joint information</rdfs:label>
    <rdfs:subClassOf rdf:nodeID="A175"/>
    <rdfs:subClassOf rdf:resource="jc3iedm_CAPABILITY.owl#OPERATIONAL-CAPABILITY"/>
  </rdf:Description>
  <rdf:Description rdf:about="jc3iedm_CAPABILITYExtended.owl#OPERATIONAL-CAPABILITY_Central_intelligence">
    <rdf:type rdf:resource="http://www.w3.org/2002/07/owl#Class"/>
    <rdfs:comment xml:lang="en">No definition provided in APP-6A.</rdfs:comment>
    <rdfs:label xml:lang="en">central intelligence</rdfs:label>
    <rdfs:subClassOf rdf:nodeID="A133"/>
    <rdfs:subClassOf rdf:resource="jc3iedm_CAPABILITY.owl#OPERATIONAL-CAPABILITY"/>
  </rdf:Description>
  <rdf:Description rdf:nodeID="A69">
    <rdf:type rdf:resource="http://www.w3.org/2002/07/owl#Restriction"/>
    <owl:onProperty rdf:resource="jc3iedm_CAPABILITY.owl#mobility-capability-category-code"/>
    <owl:hasValue xml:lang="en">Land, towed</owl:hasValue>
  </rdf:Description>
  <rdf:Description rdf:about="jc3iedm_CAPABILITYExtended.owl#SUPPORT-CAPABILITY_Bedding">
    <rdf:type rdf:resource="http://www.w3.org/2002/07/owl#Class"/>
    <rdfs:comment xml:lang="en">The capability to provide bedding.</rdfs:comment>
    <rdfs:label xml:lang="en">bedding</rdfs:label>
    <rdfs:subClassOf rdf:nodeID="A162"/>
    <rdfs:subClassOf rdf:resource="jc3iedm_CAPABILITY.owl#SUPPORT-CAPABILITY"/>
  </rdf:Description>
  <rdf:Description rdf:nodeID="A139">
    <rdf:type rdf:resource="http://www.w3.org/2002/07/owl#Restriction"/>
    <owl:onProperty rdf:resource="jc3iedm_CAPABILITY.owl#maintenance-capability-category-code"/>
    <owl:hasValue xml:lang="en">Plumbing</owl:hasValue>
  </rdf:Description>
  <rdf:Description rdf:about="jc3iedm_CAPABILITYExtended.owl#OPERATIONAL-CAPABILITY_Morale,_welfare_recreation">
    <rdf:type rdf:resource="http://www.w3.org/2002/07/owl#Class"/>
    <rdfs:comment xml:lang="en">The capability to provide morale, welfare and recreation services in support of military personnel.</rdfs:comment>
    <rdfs:label xml:lang="en">morale, welfare recreation</rdfs:label>
    <rdfs:subClassOf rdf:nodeID="A105"/>
    <rdfs:subClassOf rdf:resource="jc3iedm_CAPABILITY.owl#OPERATIONAL-CAPABILITY"/>
  </rdf:Description>
  <rdf:Description rdf:nodeID="A176">
    <rdf:type rdf:resource="http://www.w3.org/2002/07/owl#Restriction"/>
    <owl:onProperty rdf:resource="jc3iedm_CAPABILITY.owl#operational-capability-category-code"/>
    <owl:hasValue xml:lang="en">C2</owl:hasValue>
  </rdf:Description>
  <rdf:Description rdf:nodeID="A165">
    <rdf:type rdf:resource="http://www.w3.org/2002/07/owl#Restriction"/>
    <owl:onProperty rdf:resource="jc3iedm_CAPABILITY.owl#mobility-capability-category-code"/>
    <owl:hasValue xml:lang="en">Land, railed</owl:hasValue>
  </rdf:Description>
  <rdf:Description rdf:about="jc3iedm_CAPABILITYExtended.owl#OPERATIONAL-CAPABILITY_Engineer,_construction_naval">
    <rdf:type rdf:resource="http://www.w3.org/2002/07/owl#Class"/>
    <rdfs:comment xml:lang="en">The capability to build various facilities in direct support of naval operations.</rdfs:comment>
    <rdfs:label xml:lang="en">engineer, construction naval</rdfs:label>
    <rdfs:subClassOf rdf:nodeID="A189"/>
    <rdfs:subClassOf rdf:resource="jc3iedm_CAPABILITY.owl#OPERATIONAL-CAPABILITY"/>
  </rdf:Description>
  <rdf:Description rdf:about="jc3iedm_CAPABILITYExtended.owl#OPERATIONAL-CAPABILITY_Reconnaissance">
    <rdf:type rdf:resource="http://www.w3.org/2002/07/owl#Class"/>
    <rdfs:comment xml:lang="en">The capability to obtain, by visual observation or other detection methods, information about the activities and resources of an enemy or potential enemy, or to secure data concerning the meteorological, hydrographical, or geographic characteristics of a particular area.</rdfs:comment>
    <rdfs:label xml:lang="en">reconnaissance</rdfs:label>
    <rdfs:subClassOf rdf:nodeID="A20"/>
    <rdfs:subClassOf rdf:resource="jc3iedm_CAPABILITY.owl#OPERATIONAL-CAPABILITY"/>
  </rdf:Description>
  <rdf:Description rdf:nodeID="A190">
    <rdf:type rdf:resource="http://www.w3.org/2002/07/owl#Restriction"/>
    <owl:onProperty rdf:resource="jc3iedm_CAPABILITY.owl#mobility-capability-category-code"/>
    <owl:hasValue xml:lang="en">Self-deployable</owl:hasValue>
  </rdf:Description>
  <rdf:Description rdf:about="jc3iedm_CAPABILITY.owl#ENGINEERING-CAPABILITY">
    <rdfs:subClassOf rdf:resource="jc3iedm_CAPABILITY.owl#CAPABILITY"/>
    <rdfs:subClassOf rdf:nodeID="A179"/>
    <rdfs:label xml:lang="en">engineering capability</rdfs:label>
    <rdfs:comment xml:lang="en">A CAPABILITY, required for planning, of those ORGANISATIONs and PERSONs or ORGANISATION-TYPEs and PERSON-TYPEs that are deemed as having the ability to perform construction or destruction activities.</rdfs:comment>
    <rdf:type rdf:resource="http://www.w3.org/2002/07/owl#Class"/>
    <rdfs:subClassOf rdf:nodeID="A180"/>
  </rdf:Description>
  <rdf:Description rdf:about="jc3iedm_CAPABILITYExtended.owl#SUPPORT-CAPABILITY_Supply_(class_III_aviation)">
    <rdf:type rdf:resource="http://www.w3.org/2002/07/owl#Class"/>
    <rdfs:comment xml:lang="en">The capability to provide aviation fuel and lubricants.</rdfs:comment>
    <rdfs:label xml:lang="en">supply (class iii aviation)</rdfs:label>
    <rdfs:subClassOf rdf:nodeID="A191"/>
    <rdfs:subClassOf rdf:resource="jc3iedm_CAPABILITY.owl#SUPPORT-CAPABILITY"/>
  </rdf:Description>
  <rdf:Description rdf:about="jc3iedm_CAPABILITY.owl#transmission-capability-category-code">
    <rdfs:range rdf:resource="http://www.w3.org/2001/XMLSchema#string"/>
    <rdfs:domain rdf:resource="jc3iedm_CAPABILITY.owl#TRANSMISSION-CAPABILITY"/>
    <rdf:type rdf:resource="http://www.w3.org/2002/07/owl#DatatypeProperty"/>
  </rdf:Description>
  <rdf:Description rdf:about="jc3iedm_CAPABILITYExtended.owl#OPERATIONAL-CAPABILITY_Mine_countermeasure">
    <rdf:type rdf:resource="http://www.w3.org/2002/07/owl#Class"/>
    <rdfs:comment xml:lang="en">The capability to prevent or reduce damage or danger from mines.</rdfs:comment>
    <rdfs:label xml:lang="en">mine countermeasure</rdfs:label>
    <rdfs:subClassOf rdf:nodeID="A113"/>
    <rdfs:subClassOf rdf:resource="jc3iedm_CAPABILITY.owl#OPERATIONAL-CAPABILITY"/>
  </rdf:Description>
  <rdf:Description rdf:about="jc3iedm_CAPABILITYExtended.owl#MOBILITY-CAPABILITY_Self-deployable">
    <rdf:type rdf:resource="http://www.w3.org/2002/07/owl#Class"/>
    <rdfs:comment xml:lang="en">The capability of a device to be brought into effective action by its own means.</rdfs:comment>
    <rdfs:label xml:lang="en">self deployable</rdfs:label>
    <rdfs:subClassOf rdf:nodeID="A190"/>
    <rdfs:subClassOf rdf:resource="jc3iedm_CAPABILITY.owl#MOBILITY-CAPABILITY"/>
  </rdf:Description>
  <rdf:Description rdf:nodeID="A192">
    <rdf:type rdf:resource="http://www.w3.org/2002/07/owl#Restriction"/>
    <owl:onProperty rdf:resource="jc3iedm_CAPABILITY.owl#fire-capability-category-code"/>
    <owl:hasValue xml:lang="en">Sea to ground</owl:hasValue>
  </rdf:Description>
  <rdf:Description rdf:nodeID="A79">
    <rdf:type rdf:resource="http://www.w3.org/2002/07/owl#Restriction"/>
    <owl:onProperty rdf:resource="jc3iedm_CAPABILITY.owl#capability-category-code"/>
    <owl:hasValue xml:lang="en">MOBILITY-CAPABILITY</owl:hasValue>
  </rdf:Description>
  <rdf:Description rdf:nodeID="A114">
    <rdf:type rdf:resource="http://www.w3.org/2002/07/owl#Restriction"/>
    <owl:onProperty rdf:resource="jc3iedm_CAPABILITY.owl#mobility-capability-category-code"/>
    <owl:hasValue xml:lang="en">Air, lighter than air</owl:hasValue>
  </rdf:Description>
  <rdf:Description rdf:about="jc3iedm_CAPABILITYExtended.owl#OPERATIONAL-CAPABILITY_Public_affairs">
    <rdf:type rdf:resource="http://www.w3.org/2002/07/owl#Class"/>
    <rdfs:comment xml:lang="en">The capability to provide those public information, command information, and community relations activities directed towards the general public.</rdfs:comment>
    <rdfs:label xml:lang="en">public affairs</rdfs:label>
    <rdfs:subClassOf rdf:nodeID="A32"/>
    <rdfs:subClassOf rdf:resource="jc3iedm_CAPABILITY.owl#OPERATIONAL-CAPABILITY"/>
  </rdf:Description>
  <rdf:Description rdf:nodeID="A109">
    <rdf:type rdf:resource="http://www.w3.org/2002/07/owl#Restriction"/>
    <owl:onProperty rdf:resource="jc3iedm_CAPABILITY.owl#operational-capability-category-code"/>
    <owl:hasValue xml:lang="en">Engineer, construction</owl:hasValue>
  </rdf:Description>
  <rdf:Description rdf:nodeID="A14">
    <rdf:type rdf:resource="http://www.w3.org/2002/07/owl#Restriction"/>
    <owl:onProperty rdf:resource="jc3iedm_CAPABILITY.owl#operational-capability-category-code"/>
    <owl:hasValue xml:lang="en">Mortuary/graves registry</owl:hasValue>
  </rdf:Description>
  <rdf:Description rdf:nodeID="A193">
    <rdf:type rdf:resource="http://www.w3.org/2002/07/owl#Restriction"/>
    <owl:onProperty rdf:resource="jc3iedm_CAPABILITY.owl#operational-capability-category-code"/>
    <owl:hasValue xml:lang="en">Arctic</owl:hasValue>
  </rdf:Description>
  <rdf:Description rdf:about="jc3iedm_CAPABILITYExtended.owl#OPERATIONAL-CAPABILITY_NBC,_biological">
    <rdf:type rdf:resource="http://www.w3.org/2002/07/owl#Class"/>
    <rdfs:comment xml:lang="en">The capability to employ biological materiel to produce casualties in man or animals and damage to plants or materiel; or defence against such employment.</rdfs:comment>
    <rdfs:label xml:lang="en">nbc, biological</rdfs:label>
    <rdfs:subClassOf rdf:nodeID="A45"/>
    <rdfs:subClassOf rdf:resource="jc3iedm_CAPABILITY.owl#OPERATIONAL-CAPABILITY"/>
  </rdf:Description>
  <rdf:Description rdf:nodeID="A118">
    <rdf:type rdf:resource="http://www.w3.org/2002/07/owl#Restriction"/>
    <owl:onProperty rdf:resource="jc3iedm_CAPABILITY.owl#support-capability-category-code"/>
    <owl:hasValue xml:lang="en">Supply (class V)</owl:hasValue>
  </rdf:Description>
  <rdf:Description rdf:about="jc3iedm_CAPABILITYExtended.owl#MOBILITY-CAPABILITY_Animal,_mounted">
    <rdf:type rdf:resource="http://www.w3.org/2002/07/owl#Class"/>
    <rdfs:comment xml:lang="en">The capability to move by using an animal as a carrier.</rdfs:comment>
    <rdfs:label xml:lang="en">animal, mounted</rdfs:label>
    <rdfs:subClassOf rdf:nodeID="A102"/>
    <rdfs:subClassOf rdf:resource="jc3iedm_CAPABILITY.owl#MOBILITY-CAPABILITY"/>
  </rdf:Description>
  <rdf:Description rdf:about="jc3iedm_CAPABILITY.owl#operational-capability-qualifier-code">
    <rdfs:range rdf:resource="http://www.w3.org/2001/XMLSchema#string"/>
    <rdfs:domain rdf:resource="jc3iedm_CAPABILITY.owl#OPERATIONAL-CAPABILITY"/>
    <rdf:type rdf:resource="http://www.w3.org/2002/07/owl#DatatypeProperty"/>
  </rdf:Description>
  <rdf:Description rdf:about="#">
    <owl:imports rdf:resource="jc3iedm_CAPABILITYExtended.owl#"/>
    <rdf:type rdf:resource="http://www.w3.org/2002/07/owl#Ontology"/>
  </rdf:Description>
  <rdf:Description rdf:about="jc3iedm_CAPABILITY.owl#FIRE-CAPABILITY">
    <rdfs:subClassOf rdf:resource="jc3iedm_CAPABILITY.owl#CAPABILITY"/>
    <rdfs:subClassOf rdf:nodeID="A194"/>
    <rdfs:label xml:lang="en">fire capability</rdfs:label>
    <rdfs:comment xml:lang="en">A CAPABILITY, required for planning, of those FACILITYs, MATERIELs, ORGANISATIONs and PERSONs, or FACILITY-TYPEs, EQUIPMENT-TYPEs, ORGANISATION-TYPEs and PERSON-TYPEs that are deemed as having the ability to discharge or launch a projectile or missile.</rdfs:comment>
    <rdf:type rdf:resource="http://www.w3.org/2002/07/owl#Class"/>
    <rdfs:subClassOf rdf:nodeID="A123"/>
  </rdf:Description>
  <rdf:Description rdf:nodeID="A144">
    <rdf:type rdf:resource="http://www.w3.org/2002/07/owl#Restriction"/>
    <owl:onProperty rdf:resource="jc3iedm_CAPABILITY.owl#engineering-capability-category-code"/>
    <owl:hasValue xml:lang="en">Breaching</owl:hasValue>
  </rdf:Description>
  <rdf:Description rdf:about="jc3iedm_CAPABILITYExtended.owl#MOBILITY-CAPABILITY_Dismounted">
    <rdf:type rdf:resource="http://www.w3.org/2002/07/owl#Class"/>
    <rdfs:comment xml:lang="en">The capability of moving on foot.</rdfs:comment>
    <rdfs:label xml:lang="en">dismounted</rdfs:label>
    <rdfs:subClassOf rdf:nodeID="A155"/>
    <rdfs:subClassOf rdf:resource="jc3iedm_CAPABILITY.owl#MOBILITY-CAPABILITY"/>
  </rdf:Description>
  <rdf:Description rdf:about="jc3iedm_CAPABILITYExtended.owl#OPERATIONAL-CAPABILITY_Transportation,_missile">
    <rdf:type rdf:resource="http://www.w3.org/2002/07/owl#Class"/>
    <rdfs:comment xml:lang="en">The capability to provide equipment for transportation of missiles.</rdfs:comment>
    <rdfs:label xml:lang="en">transportation, missile</rdfs:label>
    <rdfs:subClassOf rdf:nodeID="A160"/>
    <rdfs:subClassOf rdf:resource="jc3iedm_CAPABILITY.owl#OPERATIONAL-CAPABILITY"/>
  </rdf:Description>
  <rdf:Description rdf:nodeID="A188">
    <rdf:type rdf:resource="http://www.w3.org/2002/07/owl#Restriction"/>
    <owl:onProperty rdf:resource="jc3iedm_CAPABILITY.owl#mobility-capability-category-code"/>
    <owl:hasValue xml:lang="en">Amphibious</owl:hasValue>
  </rdf:Description>
  <rdf:Description rdf:about="jc3iedm_CAPABILITY.owl#mobility-capability-terrain-type-code">
    <rdfs:range rdf:resource="http://www.w3.org/2001/XMLSchema#string"/>
    <rdfs:domain rdf:resource="jc3iedm_CAPABILITY.owl#MOBILITY-CAPABILITY"/>
    <rdf:type rdf:resource="http://www.w3.org/2002/07/owl#DatatypeProperty"/>
  </rdf:Description>
  <rdf:Description rdf:about="jc3iedm_CAPABILITYExtended.owl#OPERATIONAL-CAPABILITY_Maritime">
    <rdf:type rdf:resource="http://www.w3.org/2002/07/owl#Class"/>
    <rdfs:comment xml:lang="en">The capability to perform maritime/deep water operations.</rdfs:comment>
    <rdfs:label xml:lang="en">maritime</rdfs:label>
    <rdfs:subClassOf rdf:nodeID="A58"/>
    <rdfs:subClassOf rdf:resource="jc3iedm_CAPABILITY.owl#OPERATIONAL-CAPABILITY"/>
  </rdf:Description>
  <rdf:Description rdf:nodeID="A195">
    <rdf:type rdf:resource="http://www.w3.org/2002/07/owl#Restriction"/>
    <owl:onProperty rdf:resource="jc3iedm_CAPABILITY.owl#operational-capability-category-code"/>
    <owl:hasValue xml:lang="en">Replacement holding</owl:hasValue>
  </rdf:Description>
  <rdf:Description rdf:nodeID="A13">
    <rdf:type rdf:resource="http://www.w3.org/2002/07/owl#Restriction"/>
    <owl:onProperty rdf:resource="jc3iedm_CAPABILITY.owl#surveillance-capability-category-code"/>
    <owl:hasValue xml:lang="en">Not known</owl:hasValue>
  </rdf:Description>
  <rdf:Description rdf:about="jc3iedm_CAPABILITYExtended.owl#OPERATIONAL-CAPABILITY_NBC,_nuclear">
    <rdf:type rdf:resource="http://www.w3.org/2002/07/owl#Class"/>
    <rdfs:comment xml:lang="en">No definition provided in APP-6A.</rdfs:comment>
    <rdfs:label xml:lang="en">nbc, nuclear</rdfs:label>
    <rdfs:subClassOf rdf:nodeID="A134"/>
    <rdfs:subClassOf rdf:resource="jc3iedm_CAPABILITY.owl#OPERATIONAL-CAPABILITY"/>
  </rdf:Description>
  <rdf:Description rdf:nodeID="A191">
    <rdf:type rdf:resource="http://www.w3.org/2002/07/owl#Restriction"/>
    <owl:onProperty rdf:resource="jc3iedm_CAPABILITY.owl#support-capability-category-code"/>
    <owl:hasValue xml:lang="en">Supply (class III aviation)</owl:hasValue>
  </rdf:Description>
  <rdf:Description rdf:about="jc3iedm_CAPABILITYExtended.owl#OPERATIONAL-CAPABILITY_Electronic_warfare,_direction_finding">
    <rdf:type rdf:resource="http://www.w3.org/2002/07/owl#Class"/>
    <rdfs:comment xml:lang="en">The capability for obtaining bearings of radio frequency emitters by using a directional antenna and a display unit on an intercept receiver or ancillary equipment.</rdfs:comment>
    <rdfs:label xml:lang="en">electronic warfare, direction finding</rdfs:label>
    <rdfs:subClassOf rdf:nodeID="A152"/>
    <rdfs:subClassOf rdf:resource="jc3iedm_CAPABILITY.owl#OPERATIONAL-CAPABILITY"/>
  </rdf:Description>
  <rdf:Description rdf:about="jc3iedm_CAPABILITYExtended.owl#SUPPORT-CAPABILITY_Medical_supplies">
    <rdf:type rdf:resource="http://www.w3.org/2002/07/owl#Class"/>
    <rdfs:comment xml:lang="en">The capability to provide medicine.</rdfs:comment>
    <rdfs:label xml:lang="en">medical supplies</rdfs:label>
    <rdfs:subClassOf rdf:nodeID="A184"/>
    <rdfs:subClassOf rdf:resource="jc3iedm_CAPABILITY.owl#SUPPORT-CAPABILITY"/>
  </rdf:Description>
  <rdf:Description rdf:about="jc3iedm_CAPABILITYExtended.owl#OPERATIONAL-CAPABILITY_Signal,_radio">
    <rdf:type rdf:resource="http://www.w3.org/2002/07/owl#Class"/>
    <rdfs:comment xml:lang="en">The capability in signal services to manage, operate and control a radio communications.</rdfs:comment>
    <rdfs:label xml:lang="en">signal, radio</rdfs:label>
    <rdfs:subClassOf rdf:nodeID="A196"/>
    <rdfs:subClassOf rdf:resource="jc3iedm_CAPABILITY.owl#OPERATIONAL-CAPABILITY"/>
  </rdf:Description>
  <rdf:Description rdf:about="jc3iedm_CAPABILITY.owl#CAPABILITY">
    <rdfs:label xml:lang="en">capability</rdfs:label>
    <rdfs:comment xml:lang="en">The potential ability to do work, perform a function or mission, achieve an objective, or provide a service.</rdfs:comment>
    <rdf:type rdf:resource="http://www.w3.org/2002/07/owl#Class"/>
  </rdf:Description>
  <rdf:Description rdf:about="jc3iedm_CAPABILITYExtended.owl#SURVEILLANCE-CAPABILITY_Human">
    <rdf:type rdf:resource="http://www.w3.org/2002/07/owl#Class"/>
    <rdfs:comment xml:lang="en">The ability to gain information by exploiting human senses.</rdfs:comment>
    <rdfs:label xml:lang="en">human</rdfs:label>
    <rdfs:subClassOf rdf:nodeID="A43"/>
    <rdfs:subClassOf rdf:resource="jc3iedm_CAPABILITY.owl#SURVEILLANCE-CAPABILITY"/>
  </rdf:Description>
  <rdf:Description rdf:about="jc3iedm_CAPABILITY.owl#operational-capability-category-code">
    <rdfs:range rdf:resource="http://www.w3.org/2001/XMLSchema#string"/>
    <rdfs:domain rdf:resource="jc3iedm_CAPABILITY.owl#OPERATIONAL-CAPABILITY"/>
    <rdf:type rdf:resource="http://www.w3.org/2002/07/owl#DatatypeProperty"/>
  </rdf:Description>
  <rdf:Description rdf:nodeID="A146">
    <rdf:type rdf:resource="http://www.w3.org/2002/07/owl#Restriction"/>
    <owl:onProperty rdf:resource="jc3iedm_CAPABILITY.owl#operational-capability-category-code"/>
    <owl:hasValue xml:lang="en">Supply (class III)</owl:hasValue>
  </rdf:Description>
  <rdf:Description rdf:nodeID="A93">
    <rdf:type rdf:resource="http://www.w3.org/2002/07/owl#Restriction"/>
    <owl:onProperty rdf:resource="jc3iedm_CAPABILITY.owl#support-capability-category-code"/>
    <owl:hasValue xml:lang="en">Supply (class III)</owl:hasValue>
  </rdf:Description>
  <rdf:Description rdf:about="jc3iedm_CAPABILITYExtended.owl#OPERATIONAL-CAPABILITY_Target_acquisition,_flash">
    <rdf:type rdf:resource="http://www.w3.org/2002/07/owl#Class"/>
    <rdfs:comment xml:lang="en">The capability to manage, operate and maintain flash target acquisition assets.</rdfs:comment>
    <rdfs:label xml:lang="en">target acquisition, flash</rdfs:label>
    <rdfs:subClassOf rdf:nodeID="A197"/>
    <rdfs:subClassOf rdf:resource="jc3iedm_CAPABILITY.owl#OPERATIONAL-CAPABILITY"/>
  </rdf:Description>
  <rdf:Description rdf:about="jc3iedm_CAPABILITYExtended.owl#MOBILITY-CAPABILITY_Water,_surface">
    <rdf:type rdf:resource="http://www.w3.org/2002/07/owl#Class"/>
    <rdfs:comment xml:lang="en">The capability of a device to move on the water surface.</rdfs:comment>
    <rdfs:label xml:lang="en">water, surface</rdfs:label>
    <rdfs:subClassOf rdf:nodeID="A132"/>
    <rdfs:subClassOf rdf:resource="jc3iedm_CAPABILITY.owl#MOBILITY-CAPABILITY"/>
  </rdf:Description>
  <rdf:Description rdf:about="jc3iedm_CAPABILITYExtended.owl#OPERATIONAL-CAPABILITY_Interrogation">
    <rdf:type rdf:resource="http://www.w3.org/2002/07/owl#Class"/>
    <rdfs:comment xml:lang="en">The capability to procure information by direct questioning of a person under the control of a questioner.</rdfs:comment>
    <rdfs:label xml:lang="en">interrogation</rdfs:label>
    <rdfs:subClassOf rdf:nodeID="A59"/>
    <rdfs:subClassOf rdf:resource="jc3iedm_CAPABILITY.owl#OPERATIONAL-CAPABILITY"/>
  </rdf:Description>
  <rdf:Description rdf:about="jc3iedm_CAPABILITYExtended.owl#MOBILITY-CAPABILITY_Water,_canal">
    <rdf:type rdf:resource="http://www.w3.org/2002/07/owl#Class"/>
    <rdfs:comment xml:lang="en">The capability of a device to navigate canals.</rdfs:comment>
    <rdfs:label xml:lang="en">water, canal</rdfs:label>
    <rdfs:subClassOf rdf:nodeID="A164"/>
    <rdfs:subClassOf rdf:resource="jc3iedm_CAPABILITY.owl#MOBILITY-CAPABILITY"/>
  </rdf:Description>
  <rdf:Description rdf:about="jc3iedm_CAPABILITYExtended.owl#OPERATIONAL-CAPABILITY_Medical_evacuation">
    <rdf:type rdf:resource="http://www.w3.org/2002/07/owl#Class"/>
    <rdfs:comment xml:lang="en">The capability for timely and efficient movement of patients while providing en route medical care to and between medical treatment facilities.</rdfs:comment>
    <rdfs:label xml:lang="en">medical evacuation</rdfs:label>
    <rdfs:subClassOf rdf:nodeID="A4"/>
    <rdfs:subClassOf rdf:resource="jc3iedm_CAPABILITY.owl#OPERATIONAL-CAPABILITY"/>
  </rdf:Description>
  <rdf:Description rdf:nodeID="A198">
    <rdf:type rdf:resource="http://www.w3.org/2002/07/owl#Restriction"/>
    <owl:onProperty rdf:resource="jc3iedm_CAPABILITY.owl#operational-capability-category-code"/>
    <owl:hasValue xml:lang="en">Signal, forward communications</owl:hasValue>
  </rdf:Description>
  <rdf:Description rdf:about="jc3iedm_CAPABILITYExtended.owl#OPERATIONAL-CAPABILITY_Signal,_node,_large_extension">
    <rdf:type rdf:resource="http://www.w3.org/2002/07/owl#Class"/>
    <rdfs:comment xml:lang="en">The capability in signal services to manage, operate and control a communications large extension node.</rdfs:comment>
    <rdfs:label xml:lang="en">signal, node, large extension</rdfs:label>
    <rdfs:subClassOf rdf:nodeID="A181"/>
    <rdfs:subClassOf rdf:resource="jc3iedm_CAPABILITY.owl#OPERATIONAL-CAPABILITY"/>
  </rdf:Description>
  <rdf:Description rdf:about="jc3iedm_CAPABILITYExtended.owl#OPERATIONAL-CAPABILITY_Aerial_refuelling">
    <rdf:type rdf:resource="http://www.w3.org/2002/07/owl#Class"/>
    <rdfs:comment xml:lang="en">The capability to refuel aircraft in flight, which extends presence, increases range, and serves as a force multiplier.</rdfs:comment>
    <rdfs:label xml:lang="en">aerial refuelling</rdfs:label>
    <rdfs:subClassOf rdf:nodeID="A174"/>
    <rdfs:subClassOf rdf:resource="jc3iedm_CAPABILITY.owl#OPERATIONAL-CAPABILITY"/>
  </rdf:Description>
  <rdf:Description rdf:nodeID="A173">
    <rdf:type rdf:resource="http://www.w3.org/2002/07/owl#Restriction"/>
    <owl:onProperty rdf:resource="jc3iedm_CAPABILITY.owl#operational-capability-category-code"/>
    <owl:hasValue xml:lang="en">Theatre missile defence</owl:hasValue>
  </rdf:Description>
  <rdf:Description rdf:about="jc3iedm_CAPABILITYExtended.owl#TRANSMISSION-CAPABILITY_Receive">
    <rdf:type rdf:resource="http://www.w3.org/2002/07/owl#Class"/>
    <rdfs:comment xml:lang="en">The ability to detect or pick up a broadcast, a signal or programme.</rdfs:comment>
    <rdfs:label xml:lang="en">receive</rdfs:label>
    <rdfs:subClassOf rdf:nodeID="A77"/>
    <rdfs:subClassOf rdf:resource="jc3iedm_CAPABILITY.owl#TRANSMISSION-CAPABILITY"/>
  </rdf:Description>
  <rdf:Description rdf:about="jc3iedm_CAPABILITYExtended.owl#OPERATIONAL-CAPABILITY_Signal,_support">
    <rdf:type rdf:resource="http://www.w3.org/2002/07/owl#Class"/>
    <rdfs:comment xml:lang="en">The capability to provide personnel and equipment from other forces for the establishment of a special or supplementary communications system.</rdfs:comment>
    <rdfs:label xml:lang="en">signal, support</rdfs:label>
    <rdfs:subClassOf rdf:nodeID="A70"/>
    <rdfs:subClassOf rdf:resource="jc3iedm_CAPABILITY.owl#OPERATIONAL-CAPABILITY"/>
  </rdf:Description>
  <rdf:Description rdf:nodeID="A153">
    <rdf:type rdf:resource="http://www.w3.org/2002/07/owl#Restriction"/>
    <owl:onProperty rdf:resource="jc3iedm_CAPABILITY.owl#engineering-capability-category-code"/>
    <owl:hasValue xml:lang="en">Construction</owl:hasValue>
  </rdf:Description>
  <rdf:Description rdf:about="jc3iedm_CAPABILITYExtended.owl#MAINTENANCE-CAPABILITY_Cable">
    <rdf:type rdf:resource="http://www.w3.org/2002/07/owl#Class"/>
    <rdfs:comment xml:lang="en">The specific MAINTENANCE-CAPABILITY determines the ability to provide cable repair.</rdfs:comment>
    <rdfs:label xml:lang="en">cable</rdfs:label>
    <rdfs:subClassOf rdf:nodeID="A143"/>
    <rdfs:subClassOf rdf:resource="jc3iedm_CAPABILITY.owl#MAINTENANCE-CAPABILITY"/>
  </rdf:Description>
  <rdf:Description rdf:nodeID="A91">
    <rdf:type rdf:resource="http://www.w3.org/2002/07/owl#Restriction"/>
    <owl:onProperty rdf:resource="jc3iedm_CAPABILITY.owl#operational-capability-category-code"/>
    <owl:hasValue xml:lang="en">Anti-submarine warfare</owl:hasValue>
  </rdf:Description>
  <rdf:Description rdf:nodeID="A0">
    <rdf:type rdf:resource="http://www.w3.org/2002/07/owl#Restriction"/>
    <owl:onProperty rdf:resource="jc3iedm_CAPABILITY.owl#operational-capability-category-code"/>
    <owl:hasValue xml:lang="en">Mountain</owl:hasValue>
  </rdf:Description>
  <rdf:Description rdf:about="jc3iedm_CAPABILITY.owl#surveillance-capability-descriptor-code">
    <rdfs:range rdf:resource="http://www.w3.org/2001/XMLSchema#string"/>
    <rdfs:domain rdf:resource="jc3iedm_CAPABILITY.owl#SURVEILLANCE-CAPABILITY"/>
    <rdf:type rdf:resource="http://www.w3.org/2002/07/owl#DatatypeProperty"/>
  </rdf:Description>
  <rdf:Description rdf:about="jc3iedm_CAPABILITYExtended.owl#MAINTENANCE-CAPABILITY_Electrical">
    <rdf:type rdf:resource="http://www.w3.org/2002/07/owl#Class"/>
    <rdfs:comment xml:lang="en">The specific MAINTENANCE-CAPABILITY determines the ability to provide electrical repair.</rdfs:comment>
    <rdfs:label xml:lang="en">electrical</rdfs:label>
    <rdfs:subClassOf rdf:nodeID="A199"/>
    <rdfs:subClassOf rdf:resource="jc3iedm_CAPABILITY.owl#MAINTENANCE-CAPABILITY"/>
  </rdf:Description>
  <rdf:Description rdf:about="jc3iedm_CAPABILITYExtended.owl#MOBILITY-CAPABILITY_Air,_rotary_wing">
    <rdf:type rdf:resource="http://www.w3.org/2002/07/owl#Class"/>
    <rdfs:comment xml:lang="en">The capability to move through the air by deriving lift from aerofoils that rotate.</rdfs:comment>
    <rdfs:label xml:lang="en">air, rotary wing</rdfs:label>
    <rdfs:subClassOf rdf:nodeID="A138"/>
    <rdfs:subClassOf rdf:resource="jc3iedm_CAPABILITY.owl#MOBILITY-CAPABILITY"/>
  </rdf:Description>
  <rdf:Description rdf:nodeID="A111">
    <rdf:type rdf:resource="http://www.w3.org/2002/07/owl#Restriction"/>
    <owl:onProperty rdf:resource="jc3iedm_CAPABILITY.owl#mobility-capability-category-code"/>
    <owl:hasValue xml:lang="en">Water, tidal</owl:hasValue>
  </rdf:Description>
  <rdf:Description rdf:nodeID="A200">
    <rdf:type rdf:resource="http://www.w3.org/2002/07/owl#Restriction"/>
    <owl:onProperty rdf:resource="jc3iedm_CAPABILITY.owl#operational-capability-category-code"/>
    <owl:hasValue xml:lang="en">Public affairs, broadcast</owl:hasValue>
  </rdf:Description>
  <rdf:Description rdf:nodeID="A177">
    <rdf:type rdf:resource="http://www.w3.org/2002/07/owl#Restriction"/>
    <owl:onProperty rdf:resource="jc3iedm_CAPABILITY.owl#operational-capability-category-code"/>
    <owl:hasValue xml:lang="en">Electronic ranging</owl:hasValue>
  </rdf:Description>
  <rdf:Description rdf:about="jc3iedm_CAPABILITYExtended.owl#MOBILITY-CAPABILITY_Air,_fixed_wing">
    <rdf:type rdf:resource="http://www.w3.org/2002/07/owl#Class"/>
    <rdfs:comment xml:lang="en">The capability to move through the air by deriving lift from fixed wings.</rdfs:comment>
    <rdfs:label xml:lang="en">air, fixed wing</rdfs:label>
    <rdfs:subClassOf rdf:nodeID="A201"/>
    <rdfs:subClassOf rdf:resource="jc3iedm_CAPABILITY.owl#MOBILITY-CAPABILITY"/>
  </rdf:Description>
  <rdf:Description rdf:about="jc3iedm_CAPABILITYExtended.owl#OPERATIONAL-CAPABILITY_Joint_intelligence">
    <rdf:type rdf:resource="http://www.w3.org/2002/07/owl#Class"/>
    <rdfs:comment xml:lang="en">The capability to produce intelligence from elements of more than one Service.</rdfs:comment>
    <rdfs:label xml:lang="en">joint intelligence</rdfs:label>
    <rdfs:subClassOf rdf:nodeID="A149"/>
    <rdfs:subClassOf rdf:resource="jc3iedm_CAPABILITY.owl#OPERATIONAL-CAPABILITY"/>
  </rdf:Description>
  <rdf:Description rdf:about="jc3iedm_CAPABILITYExtended.owl#TRANSMISSION-CAPABILITY_Transceive">
    <rdf:type rdf:resource="http://www.w3.org/2002/07/owl#Class"/>
    <rdfs:comment xml:lang="en">The ability to detect, pick up, broadcast or send out a signal or programme.</rdfs:comment>
    <rdfs:label xml:lang="en">transceive</rdfs:label>
    <rdfs:subClassOf rdf:nodeID="A12"/>
    <rdfs:subClassOf rdf:resource="jc3iedm_CAPABILITY.owl#TRANSMISSION-CAPABILITY"/>
  </rdf:Description>
  <rdf:Description rdf:about="jc3iedm_CAPABILITYExtended.owl#OPERATIONAL-CAPABILITY_Target_acquisition,_sound">
    <rdf:type rdf:resource="http://www.w3.org/2002/07/owl#Class"/>
    <rdfs:comment xml:lang="en">The capability to manage, operate and maintain sound target acquisition assets.</rdfs:comment>
    <rdfs:label xml:lang="en">target acquisition, sound</rdfs:label>
    <rdfs:subClassOf rdf:nodeID="A37"/>
    <rdfs:subClassOf rdf:resource="jc3iedm_CAPABILITY.owl#OPERATIONAL-CAPABILITY"/>
  </rdf:Description>
  <rdf:Description rdf:nodeID="A197">
    <rdf:type rdf:resource="http://www.w3.org/2002/07/owl#Restriction"/>
    <owl:onProperty rdf:resource="jc3iedm_CAPABILITY.owl#operational-capability-category-code"/>
    <owl:hasValue xml:lang="en">Target acquisition, flash</owl:hasValue>
  </rdf:Description>
  <rdf:Description rdf:nodeID="A172">
    <rdf:type rdf:resource="http://www.w3.org/2002/07/owl#Restriction"/>
    <owl:onProperty rdf:resource="jc3iedm_CAPABILITY.owl#operational-capability-category-code"/>
    <owl:hasValue xml:lang="en">Military intelligence, tactical exploitation</owl:hasValue>
  </rdf:Description>
  <rdf:Description rdf:nodeID="A156">
    <owl:hasValue xml:lang="en">OPERATIONAL-CAPABILITY</owl:hasValue>
    <owl:onProperty rdf:resource="jc3iedm_CAPABILITY.owl#capability-category-code"/>
    <rdf:type rdf:resource="http://www.w3.org/2002/07/owl#Restriction"/>
  </rdf:Description>
  <rdf:Description rdf:nodeID="A194">
    <owl:hasValue xml:lang="en">FIRE-CAPABILITY</owl:hasValue>
    <owl:onProperty rdf:resource="jc3iedm_CAPABILITY.owl#capability-category-code"/>
    <rdf:type rdf:resource="http://www.w3.org/2002/07/owl#Restriction"/>
  </rdf:Description>
  <rdf:Description rdf:about="jc3iedm_CAPABILITYExtended.owl#OPERATIONAL-CAPABILITY_Arctic">
    <rdf:type rdf:resource="http://www.w3.org/2002/07/owl#Class"/>
    <rdfs:comment xml:lang="en">The capability to perform a mission involving an arctic operation.</rdfs:comment>
    <rdfs:label xml:lang="en">arctic</rdfs:label>
    <rdfs:subClassOf rdf:nodeID="A193"/>
    <rdfs:subClassOf rdf:resource="jc3iedm_CAPABILITY.owl#OPERATIONAL-CAPABILITY"/>
  </rdf:Description>
  <rdf:Description rdf:nodeID="A125">
    <owl:hasValue xml:lang="en">TRANSMISSION-CAPABILITY</owl:hasValue>
    <owl:onProperty rdf:resource="jc3iedm_CAPABILITY.owl#capability-category-code"/>
    <rdf:type rdf:resource="http://www.w3.org/2002/07/owl#Restriction"/>
  </rdf:Description>
  <rdf:Description rdf:nodeID="A159">
    <rdf:type rdf:resource="http://www.w3.org/2002/07/owl#Restriction"/>
    <owl:onProperty rdf:resource="jc3iedm_CAPABILITY.owl#operational-capability-category-code"/>
    <owl:hasValue xml:lang="en">Close air support</owl:hasValue>
  </rdf:Description>
  <rdf:Description rdf:about="jc3iedm_CAPABILITYExtended.owl#MOBILITY-CAPABILITY_Land,_tracked">
    <rdf:type rdf:resource="http://www.w3.org/2002/07/owl#Class"/>
    <rdfs:comment xml:lang="en">The capability of a device to move on caterpillar treads.</rdfs:comment>
    <rdfs:label xml:lang="en">land, tracked</rdfs:label>
    <rdfs:subClassOf rdf:nodeID="A202"/>
    <rdfs:subClassOf rdf:resource="jc3iedm_CAPABILITY.owl#MOBILITY-CAPABILITY"/>
  </rdf:Description>
  <rdf:Description rdf:about="jc3iedm_CAPABILITYExtended.owl#MOBILITY-CAPABILITY_Water,_swamp">
    <rdf:type rdf:resource="http://www.w3.org/2002/07/owl#Class"/>
    <rdfs:comment xml:lang="en">The capability of a device to navigate swamps.</rdfs:comment>
    <rdfs:label xml:lang="en">water, swamp</rdfs:label>
    <rdfs:subClassOf rdf:nodeID="A203"/>
    <rdfs:subClassOf rdf:resource="jc3iedm_CAPABILITY.owl#MOBILITY-CAPABILITY"/>
  </rdf:Description>
  <rdf:Description rdf:nodeID="A187">
    <rdf:type rdf:resource="http://www.w3.org/2002/07/owl#Restriction"/>
    <owl:onProperty rdf:resource="jc3iedm_CAPABILITY.owl#operational-capability-category-code"/>
    <owl:hasValue xml:lang="en">Supply (class IV)</owl:hasValue>
  </rdf:Description>
  <rdf:Description rdf:nodeID="A76">
    <rdf:type rdf:resource="http://www.w3.org/2002/07/owl#Restriction"/>
    <owl:onProperty rdf:resource="jc3iedm_CAPABILITY.owl#operational-capability-category-code"/>
    <owl:hasValue xml:lang="en">Maintenance, electro-optical</owl:hasValue>
  </rdf:Description>
  <rdf:Description rdf:nodeID="A34">
    <rdf:type rdf:resource="http://www.w3.org/2002/07/owl#Restriction"/>
    <owl:onProperty rdf:resource="jc3iedm_CAPABILITY.owl#mobility-capability-category-code"/>
    <owl:hasValue xml:lang="en">Land, wheeled</owl:hasValue>
  </rdf:Description>
  <rdf:Description rdf:about="jc3iedm_CAPABILITY.owl#operational-capability-level-code">
    <rdfs:range rdf:resource="http://www.w3.org/2001/XMLSchema#string"/>
    <rdfs:domain rdf:resource="jc3iedm_CAPABILITY.owl#OPERATIONAL-CAPABILITY"/>
    <rdf:type rdf:resource="http://www.w3.org/2002/07/owl#DatatypeProperty"/>
  </rdf:Description>
  <rdf:Description rdf:nodeID="A199">
    <rdf:type rdf:resource="http://www.w3.org/2002/07/owl#Restriction"/>
    <owl:onProperty rdf:resource="jc3iedm_CAPABILITY.owl#maintenance-capability-category-code"/>
    <owl:hasValue xml:lang="en">Electrical</owl:hasValue>
  </rdf:Description>
  <rdf:Description rdf:about="jc3iedm_CAPABILITY.owl#maintenance-capability-station-count">
    <rdfs:domain rdf:resource="jc3iedm_CAPABILITY.owl#MAINTENANCE-CAPABILITY"/>
    <rdf:type rdf:resource="http://www.w3.org/2002/07/owl#DatatypeProperty"/>
  </rdf:Description>
  <rdf:Description rdf:about="jc3iedm_CAPABILITYExtended.owl#FIRE-CAPABILITY_Sea_to_ground">
    <rdf:type rdf:resource="http://www.w3.org/2002/07/owl#Class"/>
    <rdfs:comment xml:lang="en">The specific value implies that a specific FIRE-CAPABILITY involves firing from a vessel to targets on the ground.</rdfs:comment>
    <rdfs:label xml:lang="en">sea to ground</rdfs:label>
    <rdfs:subClassOf rdf:nodeID="A192"/>
    <rdfs:subClassOf rdf:resource="jc3iedm_CAPABILITY.owl#FIRE-CAPABILITY"/>
  </rdf:Description>
  <rdf:Description rdf:nodeID="A127">
    <rdf:type rdf:resource="http://www.w3.org/2002/07/owl#Restriction"/>
    <owl:onProperty rdf:resource="jc3iedm_CAPABILITY.owl#operational-capability-category-code"/>
    <owl:hasValue xml:lang="en">Signals intelligence (SIGINT)</owl:hasValue>
  </rdf:Description>
  <rdf:Description rdf:about="jc3iedm_CAPABILITYExtended.owl#OPERATIONAL-CAPABILITY_NBC,_radiological">
    <rdf:type rdf:resource="http://www.w3.org/2002/07/owl#Class"/>
    <rdfs:comment xml:lang="en">The capability to employ radiological materiel to produce casualties in man or animals and damage to plants or materiel; or defence against such employment.</rdfs:comment>
    <rdfs:label xml:lang="en">nbc, radiological</rdfs:label>
    <rdfs:subClassOf rdf:nodeID="A204"/>
    <rdfs:subClassOf rdf:resource="jc3iedm_CAPABILITY.owl#OPERATIONAL-CAPABILITY"/>
  </rdf:Description>
  <rdf:Description rdf:about="jc3iedm_CAPABILITY.owl#transmission-capability-descriptor-code">
    <rdfs:range rdf:resource="http://www.w3.org/2001/XMLSchema#string"/>
    <rdfs:domain rdf:resource="jc3iedm_CAPABILITY.owl#TRANSMISSION-CAPABILITY"/>
    <rdf:type rdf:resource="http://www.w3.org/2002/07/owl#DatatypeProperty"/>
  </rdf:Description>
  <rdf:Description rdf:about="jc3iedm_CAPABILITYExtended.owl#OPERATIONAL-CAPABILITY_Replacement_holding">
    <rdf:type rdf:resource="http://www.w3.org/2002/07/owl#Class"/>
    <rdfs:comment xml:lang="en">The capability to provide personnel to take the place of other personnel who depart a unit.</rdfs:comment>
    <rdfs:label xml:lang="en">replacement holding</rdfs:label>
    <rdfs:subClassOf rdf:nodeID="A195"/>
    <rdfs:subClassOf rdf:resource="jc3iedm_CAPABILITY.owl#OPERATIONAL-CAPABILITY"/>
  </rdf:Description>
  <rdf:Description rdf:nodeID="A183">
    <owl:hasValue xml:lang="en">SURVEILLANCE-CAPABILITY</owl:hasValue>
    <owl:onProperty rdf:resource="jc3iedm_CAPABILITY.owl#capability-category-code"/>
    <rdf:type rdf:resource="http://www.w3.org/2002/07/owl#Restriction"/>
  </rdf:Description>
  <rdf:Description rdf:nodeID="A15">
    <rdf:type rdf:resource="http://www.w3.org/2002/07/owl#Restriction"/>
    <owl:onProperty rdf:resource="jc3iedm_CAPABILITY.owl#operational-capability-category-code"/>
    <owl:hasValue xml:lang="en">Electronic warfare, intercept</owl:hasValue>
  </rdf:Description>
  <rdf:Description rdf:nodeID="A196">
    <rdf:type rdf:resource="http://www.w3.org/2002/07/owl#Restriction"/>
    <owl:onProperty rdf:resource="jc3iedm_CAPABILITY.owl#operational-capability-category-code"/>
    <owl:hasValue xml:lang="en">Signal, radio</owl:hasValue>
  </rdf:Description>
  <rdf:Description rdf:about="jc3iedm_CAPABILITYExtended.owl#OPERATIONAL-CAPABILITY_Transportation,_APOD/APOE">
    <rdf:type rdf:resource="http://www.w3.org/2002/07/owl#Class"/>
    <rdfs:comment xml:lang="en">The capability to provide transportation services at aerial ports where cargo or personnel arrive or depart.</rdfs:comment>
    <rdfs:label xml:lang="en">transportation, apod/apoe</rdfs:label>
    <rdfs:subClassOf rdf:nodeID="A53"/>
    <rdfs:subClassOf rdf:resource="jc3iedm_CAPABILITY.owl#OPERATIONAL-CAPABILITY"/>
  </rdf:Description>
  <rdf:Description rdf:about="jc3iedm_CAPABILITYExtended.owl#SUPPORT-CAPABILITY_Messing">
    <rdf:type rdf:resource="http://www.w3.org/2002/07/owl#Class"/>
    <rdfs:comment xml:lang="en">The capability to provide a place providing meals and recreational facilities.</rdfs:comment>
    <rdfs:label xml:lang="en">messing</rdfs:label>
    <rdfs:subClassOf rdf:nodeID="A205"/>
    <rdfs:subClassOf rdf:resource="jc3iedm_CAPABILITY.owl#SUPPORT-CAPABILITY"/>
  </rdf:Description>
  <rdf:Description rdf:nodeID="A33">
    <rdf:type rdf:resource="http://www.w3.org/2002/07/owl#Restriction"/>
    <owl:onProperty rdf:resource="jc3iedm_CAPABILITY.owl#operational-capability-category-code"/>
    <owl:hasValue xml:lang="en">Railway</owl:hasValue>
  </rdf:Description>
  <rdf:Description rdf:about="jc3iedm_CAPABILITYExtended.owl#MAINTENANCE-CAPABILITY_Steelwork_fabrication">
    <rdf:type rdf:resource="http://www.w3.org/2002/07/owl#Class"/>
    <rdfs:comment xml:lang="en">Equipment and resources for the construction or manufacture of any article made of steel required for a docked vessel.</rdfs:comment>
    <rdfs:label xml:lang="en">steelwork fabrication</rdfs:label>
    <rdfs:subClassOf rdf:nodeID="A1"/>
    <rdfs:subClassOf rdf:resource="jc3iedm_CAPABILITY.owl#MAINTENANCE-CAPABILITY"/>
  </rdf:Description>
  <rdf:Description rdf:nodeID="A203">
    <rdf:type rdf:resource="http://www.w3.org/2002/07/owl#Restriction"/>
    <owl:onProperty rdf:resource="jc3iedm_CAPABILITY.owl#mobility-capability-category-code"/>
    <owl:hasValue xml:lang="en">Water, swamp</owl:hasValue>
  </rdf:Description>
  <rdf:Description rdf:about="jc3iedm_CAPABILITYExtended.owl#OPERATIONAL-CAPABILITY_Supply_(class_V)">
    <rdf:type rdf:resource="http://www.w3.org/2002/07/owl#Class"/>
    <rdfs:comment xml:lang="en">The capability to provide ammunition, explosives and chemical agents.</rdfs:comment>
    <rdfs:label xml:lang="en">supply (class v)</rdfs:label>
    <rdfs:subClassOf rdf:nodeID="A85"/>
    <rdfs:subClassOf rdf:resource="jc3iedm_CAPABILITY.owl#OPERATIONAL-CAPABILITY"/>
  </rdf:Description>
  <rdf:Description rdf:about="jc3iedm_CAPABILITYExtended.owl#OPERATIONAL-CAPABILITY_Public_affairs,_broadcast">
    <rdf:type rdf:resource="http://www.w3.org/2002/07/owl#Class"/>
    <rdfs:comment xml:lang="en">The capability to provide those public information, command information, and community relation activities over a broadcast medium, such as radio or TV, directed towards the general public.</rdfs:comment>
    <rdfs:label xml:lang="en">public affairs, broadcast</rdfs:label>
    <rdfs:subClassOf rdf:nodeID="A200"/>
    <rdfs:subClassOf rdf:resource="jc3iedm_CAPABILITY.owl#OPERATIONAL-CAPABILITY"/>
  </rdf:Description>
  <rdf:Description rdf:about="jc3iedm_CAPABILITYExtended.owl#SUPPORT-CAPABILITY_Security">
    <rdf:type rdf:resource="http://www.w3.org/2002/07/owl#Class"/>
    <rdfs:comment xml:lang="en">The capability to provide security services.</rdfs:comment>
    <rdfs:label xml:lang="en">security</rdfs:label>
    <rdfs:subClassOf rdf:nodeID="A206"/>
    <rdfs:subClassOf rdf:resource="jc3iedm_CAPABILITY.owl#SUPPORT-CAPABILITY"/>
  </rdf:Description>
  <rdf:Description rdf:nodeID="A186">
    <rdf:type rdf:resource="http://www.w3.org/2002/07/owl#Restriction"/>
    <owl:onProperty rdf:resource="jc3iedm_CAPABILITY.owl#mobility-capability-category-code"/>
    <owl:hasValue xml:lang="en">Water, river</owl:hasValue>
  </rdf:Description>
  <rdf:Description rdf:about="jc3iedm_CAPABILITYExtended.owl#OPERATIONAL-CAPABILITY_Scout">
    <rdf:type rdf:resource="http://www.w3.org/2002/07/owl#Class"/>
    <rdfs:comment xml:lang="en">The capability to move out ahead of the main force in order to reconnoitre the position or movements of the enemy.</rdfs:comment>
    <rdfs:label xml:lang="en">scout</rdfs:label>
    <rdfs:subClassOf rdf:nodeID="A120"/>
    <rdfs:subClassOf rdf:resource="jc3iedm_CAPABILITY.owl#OPERATIONAL-CAPABILITY"/>
  </rdf:Description>
  <rdf:Description rdf:about="jc3iedm_CAPABILITY.owl#HANDLING-CAPABILITY">
    <rdfs:subClassOf rdf:resource="jc3iedm_CAPABILITY.owl#CAPABILITY"/>
    <rdfs:subClassOf rdf:nodeID="A101"/>
    <rdfs:label xml:lang="en">handling capability</rdfs:label>
    <rdfs:comment xml:lang="en">A CAPABILITY, required for planning, of those FACILITYs and MATERIELs, or FACILITY-TYPEs and EQUIPMENT-TYPEs that are deemed as having the ability to move materiels (raw materials, scrap, semi-finished, and finished) to, through, and from productive processes; in warehouses and storage; and in receiving and shipping areas.</rdfs:comment>
    <rdf:type rdf:resource="http://www.w3.org/2002/07/owl#Class"/>
    <rdfs:subClassOf rdf:nodeID="A169"/>
  </rdf:Description>
  <rdf:Description rdf:about="jc3iedm_CAPABILITYExtended.owl#SUPPORT-CAPABILITY_Helicopter_platform">
    <rdf:type rdf:resource="http://www.w3.org/2002/07/owl#Class"/>
    <rdfs:comment xml:lang="en">The capability to provide a surface for helicopter take off and landing.</rdfs:comment>
    <rdfs:label xml:lang="en">helicopter platform</rdfs:label>
    <rdfs:subClassOf rdf:nodeID="A30"/>
    <rdfs:subClassOf rdf:resource="jc3iedm_CAPABILITY.owl#SUPPORT-CAPABILITY"/>
  </rdf:Description>
  <rdf:Description rdf:about="jc3iedm_CAPABILITYExtended.owl#OPERATIONAL-CAPABILITY_Signal,_forward_communications">
    <rdf:type rdf:resource="http://www.w3.org/2002/07/owl#Class"/>
    <rdfs:comment xml:lang="en">The capability to provide tactical communications in the combat zone.</rdfs:comment>
    <rdfs:label xml:lang="en">signal, forward communications</rdfs:label>
    <rdfs:subClassOf rdf:nodeID="A198"/>
    <rdfs:subClassOf rdf:resource="jc3iedm_CAPABILITY.owl#OPERATIONAL-CAPABILITY"/>
  </rdf:Description>
  <rdf:Description rdf:nodeID="A201">
    <rdf:type rdf:resource="http://www.w3.org/2002/07/owl#Restriction"/>
    <owl:onProperty rdf:resource="jc3iedm_CAPABILITY.owl#mobility-capability-category-code"/>
    <owl:hasValue xml:lang="en">Air, fixed wing</owl:hasValue>
  </rdf:Description>
  <rdf:Description rdf:nodeID="A206">
    <rdf:type rdf:resource="http://www.w3.org/2002/07/owl#Restriction"/>
    <owl:onProperty rdf:resource="jc3iedm_CAPABILITY.owl#support-capability-category-code"/>
    <owl:hasValue xml:lang="en">Security</owl:hasValue>
  </rdf:Description>
  <rdf:Description rdf:nodeID="A124">
    <rdf:type rdf:resource="http://www.w3.org/2002/07/owl#Restriction"/>
    <owl:onProperty rdf:resource="jc3iedm_CAPABILITY.owl#operational-capability-category-code"/>
    <owl:hasValue xml:lang="en">Training</owl:hasValue>
  </rdf:Description>
  <rdf:Description rdf:about="jc3iedm_CAPABILITY.owl#mobility-capability-category-code">
    <rdfs:range rdf:resource="http://www.w3.org/2001/XMLSchema#string"/>
    <rdfs:domain rdf:resource="jc3iedm_CAPABILITY.owl#MOBILITY-CAPABILITY"/>
    <rdf:type rdf:resource="http://www.w3.org/2002/07/owl#DatatypeProperty"/>
  </rdf:Description>
  <rdf:Description rdf:nodeID="A129">
    <rdf:type rdf:resource="http://www.w3.org/2002/07/owl#Restriction"/>
    <owl:onProperty rdf:resource="jc3iedm_CAPABILITY.owl#operational-capability-category-code"/>
    <owl:hasValue xml:lang="en">Surveillance, sensor</owl:hasValue>
  </rdf:Description>
  <rdf:Description rdf:about="jc3iedm_CAPABILITYExtended.owl#OPERATIONAL-CAPABILITY_Tactical_air_reconnaissance">
    <rdf:type rdf:resource="http://www.w3.org/2002/07/owl#Class"/>
    <rdfs:comment xml:lang="en">The capability to use of air vehicles to obtain information concerning terrain, weather, and the disposition, composition, movement, installations, lines of communications, electronic and communication emissions of enemy forces. Also included are artillery and naval gunfire adjustment, and systematic and random observation of ground battle areas, targets, and/ or sectors of airspace.</rdfs:comment>
    <rdfs:label xml:lang="en">tactical air reconnaissance</rdfs:label>
    <rdfs:subClassOf rdf:nodeID="A151"/>
    <rdfs:subClassOf rdf:resource="jc3iedm_CAPABILITY.owl#OPERATIONAL-CAPABILITY"/>
  </rdf:Description>
  <rdf:Description rdf:nodeID="A104">
    <rdf:type rdf:resource="http://www.w3.org/2002/07/owl#Restriction"/>
    <owl:onProperty rdf:resource="jc3iedm_CAPABILITY.owl#operational-capability-category-code"/>
    <owl:hasValue xml:lang="en">Maintenance, ordnance missile</owl:hasValue>
  </rdf:Description>
  <rdf:Description rdf:nodeID="A148">
    <rdf:type rdf:resource="http://www.w3.org/2002/07/owl#Restriction"/>
    <owl:onProperty rdf:resource="jc3iedm_CAPABILITY.owl#operational-capability-category-code"/>
    <owl:hasValue xml:lang="en">Signal, node centre</owl:hasValue>
  </rdf:Description>
  <rdf:Description rdf:nodeID="A202">
    <rdf:type rdf:resource="http://www.w3.org/2002/07/owl#Restriction"/>
    <owl:onProperty rdf:resource="jc3iedm_CAPABILITY.owl#mobility-capability-category-code"/>
    <owl:hasValue xml:lang="en">Land, tracked</owl:hasValue>
  </rdf:Description>
  <rdf:Description rdf:nodeID="A163">
    <rdf:type rdf:resource="http://www.w3.org/2002/07/owl#Restriction"/>
    <owl:onProperty rdf:resource="jc3iedm_CAPABILITY.owl#mobility-capability-category-code"/>
    <owl:hasValue xml:lang="en">Water, subsurface</owl:hasValue>
  </rdf:Description>
  <rdf:Description rdf:about="jc3iedm_CAPABILITYExtended.owl#OPERATIONAL-CAPABILITY_Surveillance,_ground_module">
    <rdf:type rdf:resource="http://www.w3.org/2002/07/owl#Class"/>
    <rdfs:comment xml:lang="en">The capability to manage and operate a ground module for a surveillance system.</rdfs:comment>
    <rdfs:label xml:lang="en">surveillance, ground module</rdfs:label>
    <rdfs:subClassOf rdf:nodeID="A136"/>
    <rdfs:subClassOf rdf:resource="jc3iedm_CAPABILITY.owl#OPERATIONAL-CAPABILITY"/>
  </rdf:Description>
  <rdf:Description rdf:about="jc3iedm_CAPABILITY.owl#maintenance-capability-level-code">
    <rdfs:range rdf:resource="http://www.w3.org/2001/XMLSchema#string"/>
    <rdfs:domain rdf:resource="jc3iedm_CAPABILITY.owl#MAINTENANCE-CAPABILITY"/>
    <rdf:type rdf:resource="http://www.w3.org/2002/07/owl#DatatypeProperty"/>
  </rdf:Description>
  <rdf:Description rdf:about="jc3iedm_CAPABILITYExtended.owl#OPERATIONAL-CAPABILITY_Engineer,_combat">
    <rdf:type rdf:resource="http://www.w3.org/2002/07/owl#Class"/>
    <rdfs:comment xml:lang="en">The capability to perform engineer functions in direct support of combat operations.</rdfs:comment>
    <rdfs:label xml:lang="en">engineer, combat</rdfs:label>
    <rdfs:subClassOf rdf:nodeID="A150"/>
    <rdfs:subClassOf rdf:resource="jc3iedm_CAPABILITY.owl#OPERATIONAL-CAPABILITY"/>
  </rdf:Description>
  <rdf:Description rdf:nodeID="A49">
    <rdf:type rdf:resource="http://www.w3.org/2002/07/owl#Restriction"/>
    <owl:onProperty rdf:resource="jc3iedm_CAPABILITY.owl#mobility-capability-category-code"/>
    <owl:hasValue xml:lang="en">Airborne</owl:hasValue>
  </rdf:Description>
  <rdf:Description rdf:nodeID="A161">
    <rdf:type rdf:resource="http://www.w3.org/2002/07/owl#Restriction"/>
    <owl:onProperty rdf:resource="jc3iedm_CAPABILITY.owl#operational-capability-category-code"/>
    <owl:hasValue xml:lang="en">Finance</owl:hasValue>
  </rdf:Description>
  <rdf:Description rdf:nodeID="A204">
    <rdf:type rdf:resource="http://www.w3.org/2002/07/owl#Restriction"/>
    <owl:onProperty rdf:resource="jc3iedm_CAPABILITY.owl#operational-capability-category-code"/>
    <owl:hasValue xml:lang="en">NBC, radiological</owl:hasValue>
  </rdf:Description>
  <rdf:Description rdf:nodeID="A71">
    <rdf:type rdf:resource="http://www.w3.org/2002/07/owl#Restriction"/>
    <owl:onProperty rdf:resource="jc3iedm_CAPABILITY.owl#operational-capability-category-code"/>
    <owl:hasValue xml:lang="en">Transportation, movement control</owl:hasValue>
  </rdf:Description>
  <rdf:Description rdf:about="jc3iedm_CAPABILITYExtended.owl#MOBILITY-CAPABILITY_Water,_nontidal">
    <rdf:type rdf:resource="http://www.w3.org/2002/07/owl#Class"/>
    <rdfs:comment xml:lang="en">The capability of a device to navigate non-tidal waters.</rdfs:comment>
    <rdfs:label xml:lang="en">water, nontidal</rdfs:label>
    <rdfs:subClassOf rdf:nodeID="A170"/>
    <rdfs:subClassOf rdf:resource="jc3iedm_CAPABILITY.owl#MOBILITY-CAPABILITY"/>
  </rdf:Description>
  <rdf:Description rdf:nodeID="A189">
    <rdf:type rdf:resource="http://www.w3.org/2002/07/owl#Restriction"/>
    <owl:onProperty rdf:resource="jc3iedm_CAPABILITY.owl#operational-capability-category-code"/>
    <owl:hasValue xml:lang="en">Engineer, construction naval</owl:hasValue>
  </rdf:Description>
  <rdf:Description rdf:about="jc3iedm_CAPABILITYExtended.owl#OPERATIONAL-CAPABILITY_Target_acquisition">
    <rdf:type rdf:resource="http://www.w3.org/2002/07/owl#Class"/>
    <rdfs:comment xml:lang="en">The capability to manage, operate and maintain target acquisition assets.</rdfs:comment>
    <rdfs:label xml:lang="en">target acquisition</rdfs:label>
    <rdfs:subClassOf rdf:nodeID="A182"/>
    <rdfs:subClassOf rdf:resource="jc3iedm_CAPABILITY.owl#OPERATIONAL-CAPABILITY"/>
  </rdf:Description>
  <rdf:Description rdf:about="jc3iedm_CAPABILITYExtended.owl#SUPPORT-CAPABILITY_Deck">
    <rdf:type rdf:resource="http://www.w3.org/2002/07/owl#Class"/>
    <rdfs:comment xml:lang="en">The capability to provide deck supplies.</rdfs:comment>
    <rdfs:label xml:lang="en">deck</rdfs:label>
    <rdfs:subClassOf rdf:nodeID="A98"/>
    <rdfs:subClassOf rdf:resource="jc3iedm_CAPABILITY.owl#SUPPORT-CAPABILITY"/>
  </rdf:Description>
  <rdf:Description rdf:nodeID="A205">
    <rdf:type rdf:resource="http://www.w3.org/2002/07/owl#Restriction"/>
    <owl:onProperty rdf:resource="jc3iedm_CAPABILITY.owl#support-capability-category-code"/>
    <owl:hasValue xml:lang="en">Messing</owl:hasValue>
  </rdf:Description>
  <rdf:Description rdf:about="jc3iedm_CAPABILITYExtended.owl#OPERATIONAL-CAPABILITY_Air_interdiction">
    <rdf:type rdf:resource="http://www.w3.org/2002/07/owl#Class"/>
    <rdfs:comment xml:lang="en">Air operations conducted to destroy, neutralize, or delay the enemy's military potential before it can be brought to bear effectively against friendly forces at such distance from friendly forces that detailed integration of each air mission with the fire and movement of friendly forces is not required.</rdfs:comment>
    <rdfs:label xml:lang="en">air interdiction</rdfs:label>
    <rdfs:subClassOf rdf:nodeID="A2"/>
    <rdfs:subClassOf rdf:resource="jc3iedm_CAPABILITY.owl#OPERATIONAL-CAPABILITY"/>
  </rdf:Description>
  <rdf:Description rdf:about="jc3iedm_CAPABILITYExtended.owl#SUPPORT-CAPABILITY_Shelter">
    <rdf:type rdf:resource="http://www.w3.org/2002/07/owl#Class"/>
    <rdfs:comment xml:lang="en">The capability to provide shelter.</rdfs:comment>
    <rdfs:label xml:lang="en">shelter</rdfs:label>
    <rdfs:subClassOf rdf:nodeID="A51"/>
    <rdfs:subClassOf rdf:resource="jc3iedm_CAPABILITY.owl#SUPPORT-CAPABILITY"/>
  </rdf:Description>
  <rdf:Description rdf:about="jc3iedm_CAPABILITYExtended.owl#MOBILITY-CAPABILITY_Land,_self-propelled">
    <rdf:type rdf:resource="http://www.w3.org/2002/07/owl#Class"/>
    <rdfs:comment xml:lang="en">The capability of a device to move over land under its own power.</rdfs:comment>
    <rdfs:label xml:lang="en">land, self propelled</rdfs:label>
    <rdfs:subClassOf rdf:nodeID="A31"/>
    <rdfs:subClassOf rdf:resource="jc3iedm_CAPABILITY.owl#MOBILITY-CAPABILITY"/>
  </rdf:Description>
</rdf:RDF>
